<http://purl.org/ASN/schema/core/StatusScheme> <http://www.w3.org/2000/01/rdf-schema#isDefinedBy> <http://purl.org/ASN/schema/core/> .
<http://purl.org/ASN/schema/core/prerequisiteCompetency> <http://www.w3.org/2000/01/rdf-schema#subPropertyOf> <http://purl.org/dc/terms/conformsTo> .
<http://purl.org/ASN/schema/core/source> <http://www.w3.org/2000/01/rdf-schema#comment> "The original resource which this resource is based on or derived from."@en-us .
<http://purl.org/ASN/schema/core/minorCorrelation> <http://www.w3.org/2000/01/rdf-schema#subPropertyOf> <http://purl.org/dc/terms/conformsTo> .
<http://purl.org/ASN/schema/core/statementLabel> <http://www.w3.org/2000/01/rdf-schema#comment> "The textual label designating the class of statement in the structure of statements in the Standard Document--e.g., Standard, Benchmark, Strand, Topic, etc." .
<http://purl.org/ASN/schema/core/CriterionCategory> <http://www.w3.org/1999/02/22-rdf-syntax-ns#type> <http://www.w3.org/2000/01/rdf-schema#Class> .
<http://purl.org/ASN/schema/core/alignFrom> <http://www.w3.org/1999/02/22-rdf-syntax-ns#type> <http://www.w3.org/1999/02/22-rdf-syntax-ns#Property> .
<http://purl.org/ASN/schema/core/assessmentRubric> <http://www.w3.org/2000/01/rdf-schema#range> <http://purl.org/ASN/schema/core/RubricCriterion> .
<http://purl.org/ASN/schema/core/levelFor> <http://www.w3.org/2000/01/rdf-schema#comment> "Reference to the asn:RubricCriterian to which the asn:CriterionLevel being described belongs."@en-us .
<http://purl.org/ASN/schema/core/crossSubjectReference> <http://www.w3.org/2000/01/rdf-schema#subPropertyOf> <http://purl.org/dc/elements/1.1/references> .
<http://purl.org/ASN/schema/core/listID> <http://www.w3.org/2000/01/rdf-schema#subPropertyOf> <http://purl.org/dc/terms/identifer> .
<http://purl.org/ASN/schema/core/DerivedStandardDocument> <http://www.w3.org/2000/01/rdf-schema#comment> "A collection of statements representing an expectation of what students should know, value, and be able to do at a target age or age range that are substantially defined by a different jurisdiction."@en-us .
<http://purl.org/ASN/schema/core/alignFrom> <http://www.w3.org/2000/01/rdf-schema#isDefinedBy> <http://purl.org/ASN/schema/core/> .
<http://purl.org/ASN/schema/core/StatusScheme> <http://www.w3.org/2000/01/rdf-schema#label> "Status Encoding Schemes"@en-us .
<http://purl.org/ASN/schema/core/prerequisiteAlignment> <http://www.w3.org/2000/01/rdf-schema#domain> <http://purl.org/ASN/schema/core/Statement> .
<http://purl.org/ASN/schema/core/qualityLabel> <http://www.w3.org/2000/01/rdf-schema#description> "Qualitative description of this degree of achievement used for column headers in tabular rubrics."@en-us .
<http://purl.org/ASN/schema/core/teachesCompetency> <http://www.w3.org/2000/01/rdf-schema#comment> "The competency that the learning resource being described teaches." .
<http://purl.org/ASN/schema/core/benchmark> <http://www.w3.org/1999/02/22-rdf-syntax-ns#type> <http://www.w3.org/2000/01/rdf-schema#Property> .
<http://purl.org/ASN/schema/core/CriterionCategory> <http://www.w3.org/2000/01/rdf-schema#comment> "Resource identifying a category by which Rubric Criterion may be grouped."@en-us .
<http://purl.org/ASN/schema/core/listID> <http://www.w3.org/1999/02/22-rdf-syntax-ns#type> <http://www.w3.org/1999/02/22-rdf-syntax-ns#Property> .
<http://purl.org/ASN/schema/core/DerivedStandardDocument> <http://www.w3.org/1999/02/22-rdf-syntax-ns#type> <http://www.w3.org/2000/01/rdf-schema#Class> .
<http://purl.org/ASN/schema/core/listID> <http://www.w3.org/2000/01/rdf-schema#isDefinedBy> <http://purl.org/ASN/schema/core/> .
<http://purl.org/ASN/schema/core/criterionFor> <http://www.w3.org/2000/01/rdf-schema#domain> <http://purl.org/ASN/schema/core/RubricCriterion> .
<http://purl.org/ASN/schema/core/narrowAlignment> <http://www.w3.org/2000/01/rdf-schema#comment> "The competency being described covers all of the relevant concepts in the target competency as well as relevant concepts not found in the target competency." .
<http://purl.org/ASN/schema/core/levelFor> <http://www.w3.org/2000/01/rdf-schema#label> "Level For"@en-us .
<http://purl.org/ASN/schema/core/> <http://purl.org/dc/elements/1.1/publisher> "University of Washington"@en-us .
<http://purl.org/ASN/schema/core/teachesCompetency> <http://www.w3.org/1999/02/22-rdf-syntax-ns#type> <http://www.w3.org/1999/02/22-rdf-syntax-ns#Property> .
<http://purl.org/ASN/schema/core/repositoryDate> <http://www.w3.org/1999/02/22-rdf-syntax-ns#type> <http://www.w3.org/1999/02/22-rdf-syntax-ns#Property> .
<http://purl.org/ASN/schema/core/hasScope> <http://www.w3.org/2000/01/rdf-schema#isDefinedBy> <http://purl.org/ASN/schema/core/> .
<http://purl.org/ASN/schema/core/teachesCompetency> <http://www.w3.org/2000/01/rdf-schema#isDefinedBy> <http://purl.org/ASN/schema/core/> .
<http://purl.org/ASN/schema/core/repositoryDate> <http://www.w3.org/2000/01/rdf-schema#isDefinedBy> <http://purl.org/ASN/schema/core/> .
<http://purl.org/ASN/schema/core/majorCorrelation> <http://www.w3.org/1999/02/22-rdf-syntax-ns#type> <http://www.w3.org/1999/02/22-rdf-syntax-ns#Property> .
<http://purl.org/ASN/schema/core/criterionFor> <http://www.w3.org/2000/01/rdf-schema#range> <http://purl.org/ASN/schema/core/Rubric> .
<http://purl.org/ASN/schema/core/repositoryDate> <http://www.w3.org/2000/01/rdf-schema#label> "Repository Date" .
<http://purl.org/ASN/schema/core/conceptTerm> <http://www.w3.org/2000/01/rdf-schema#comment> "A term from a controlled vocabulary used by the promulgating agency to refine and differentiate individual statements contextually." .
<http://purl.org/ASN/schema/core/majorCorrelation> <http://www.w3.org/2000/01/rdf-schema#isDefinedBy> <http://purl.org/ASN/schema/core/> .
<http://purl.org/ASN/schema/core/skillEmbodied> <http://www.w3.org/2000/01/rdf-schema#comment> "Cognitive, affective, psychomotor or other skill directly or indirectly embodied in the statement." .
<http://purl.org/ASN/schema/core/levelFor> <http://www.w3.org/2000/01/rdf-schema#isDefinedBy> <http://purl.org/ASN/schema/core/> .
<http://purl.org/ASN/schema/core/sequence> <http://www.w3.org/2000/01/rdf-schema#domain> <http://purl.org/ASN/schema/core/RubricCriterion> .
<http://purl.org/ASN/schema/core/benchmark> <http://www.w3.org/2000/01/rdf-schema#domain> <http://purl.org/ASN/schema/core/CriterionLevel> .
<http://purl.org/ASN/schema/core/prerequisiteAlignment> <http://www.w3.org/1999/02/22-rdf-syntax-ns#type> <http://www.w3.org/1999/02/22-rdf-syntax-ns#Property> .
<http://purl.org/ASN/schema/core/prerequisiteAlignment> <http://www.w3.org/2000/01/rdf-schema#isDefinedBy> <http://purl.org/ASN/schema/core/> .
<http://purl.org/ASN/schema/core/sequence> <http://www.w3.org/2000/01/rdf-schema#label> "Sequence"@en-us .
<http://purl.org/ASN/schema/core/broadCorrelation> <http://www.w3.org/2000/01/rdf-schema#subPropertyOf> <http://purl.org/dc/terms/conformsTo> .
<http://purl.org/ASN/schema/core/majorCorrelation> <http://www.w3.org/2000/01/rdf-schema#label> "Major Correlation" .
<http://purl.org/ASN/schema/core/assessesCompetency> <http://www.w3.org/2000/01/rdf-schema#range> <http://purl.org/ASN/schema/core/Statement> .
<http://purl.org/ASN/schema/core/crossSubjectReference> <http://www.w3.org/2000/01/rdf-schema#label> "Cross-subject Reference" .
<http://purl.org/ASN/schema/core/hasCriterionCategory> <http://www.w3.org/2000/01/rdf-schema#range> <http://purl.org/ASN/schema/core/CriterionCategory> .
<http://purl.org/ASN/schema/core/majorAlignment> <http://www.w3.org/2000/01/rdf-schema#comment> "Major overlap of relevant concepts between the two competencies." .
<http://purl.org/ASN/schema/core/indexingStatus> <http://www.w3.org/2000/01/rdf-schema#label> "Indexing Status" .
<http://purl.org/ASN/schema/core/altStatementNotation> <http://www.w3.org/1999/02/22-rdf-syntax-ns#type> <http://www.w3.org/1999/02/22-rdf-syntax-ns#Property> .
<http://purl.org/ASN/schema/core/hasCriterionCategory> <http://purl.org/vocab/vann/usageNote> "Large rubrics are occasionally divided into logical sections or categories that need to be identified and described."@en-us .
<http://purl.org/ASN/schema/core/comment> <http://www.w3.org/2000/01/rdf-schema#comment> "Supplemental text provided by the promulgating body that clarifies the nature, scope or use of the statement being described." .
<http://purl.org/ASN/schema/core/complexityLevel> <http://www.w3.org/2000/01/rdf-schema#subPropertyOf> <http://purl.org/ASN/schema/core/proficiencyLevel> .
<http://purl.org/ASN/schema/core/derivedFrom> <http://www.w3.org/2000/01/rdf-schema#comment> "The URI of a statement from which the derived statement being described has been derived." .
<http://purl.org/ASN/schema/core/hasCriterion> <http://purl.org/vocab/vann/usageNote> "Both asn:RubricCriterion and CriterionCategory have an asn:sequence property to identify node order; however, json-ld encodings should use @list on the asn:hasCriterion and asn:hasLevel properties to maintain sequencing of RubricCriterion."@en-us .
<http://purl.org/ASN/schema/core/altStatementNotation> <http://www.w3.org/2000/01/rdf-schema#isDefinedBy> <http://purl.org/ASN/schema/core/> .
<http://purl.org/ASN/schema/core/identifier> <http://www.w3.org/2000/01/rdf-schema#label> "Alternative Identifier" .
<http://purl.org/ASN/schema/core/CorrelationResource> <http://www.w3.org/2000/01/rdf-schema#isDefinedBy> <http://purl.org/ASN/schema/core/> .
<http://purl.org/ASN/schema/core/EducationalFramework> <http://www.w3.org/1999/02/22-rdf-syntax-ns#type> <http://www.w3.org/2000/01/rdf-schema#Class> .
<http://purl.org/ASN/schema/core/assessmentRubric> <http://www.w3.org/2000/01/rdf-schema#comment> "Explicit set of criteria used for assessing an articulated competency or set of competencies."@en-us .
<http://purl.org/ASN/schema/core/teachesCompetency> <http://www.w3.org/2000/01/rdf-schema#domain> <http://purl.org/ASN/schema/core/LearningResource> .
<http://purl.org/ASN/schema/core/assessesCompetency> <http://www.w3.org/2000/01/rdf-schema#comment> "The competency that the learning resource being described assesses." .
<http://purl.org/ASN/schema/core/exactCorrelation> <http://www.w3.org/2000/01/rdf-schema#range> <http://purl.org/ASN/schema/core/Statement> .
<http://purl.org/ASN/schema/core/CriterionLevel> <http://www.w3.org/2000/01/rdf-schema#comment> "Resource identifying one or more benchmarks that must be met to achieve a performance task."@en-us .
<http://purl.org/ASN/schema/core/skillEmbodied> <http://www.w3.org/2000/01/rdf-schema#label> "Skill Embodied" .
<http://purl.org/ASN/schema/core/source> <http://www.w3.org/2000/01/rdf-schema#range> <http://www.w3.org/2001/XMLSchema#anyURI> .
<http://purl.org/ASN/schema/core/RubricCriterion> <http://www.w3.org/1999/02/22-rdf-syntax-ns#type> <http://www.w3.org/2000/01/rdf-schema#Class> .
<http://purl.org/ASN/schema/core/altStatementNotation> <http://www.w3.org/2000/01/rdf-schema#subPropertyOf> <http://purl.org/dc/terms/identifer> .
<http://purl.org/ASN/schema/core/benchmark> <http://www.w3.org/2000/01/rdf-schema#comment> "Description of a level of achievement on a performance task defined by the RubricCriterion."@en-us .
<http://purl.org/ASN/schema/core/sequence> <http://www.w3.org/2000/01/rdf-schema#range> <http://www.w3.org/2001/XMLSchema#integer> .
<http://purl.org/ASN/schema/core/CorrelationResource> <http://purl.org/dc/elements/1.1/description> "The CorrelationResource is an entity intended to provide a rich description of a mapping (correlation) between a LearningResource and a Statement when a binary assertion of a relationship is insufficient." .
<http://purl.org/ASN/schema/core/exactAlignment> <http://www.w3.org/2000/01/rdf-schema#range> <http://purl.org/ASN/schema/core/Statement> .
<http://purl.org/ASN/schema/core/exactCorrelation> <http://www.w3.org/2000/01/rdf-schema#label> "Exact Correlation" .
<http://purl.org/ASN/schema/core/hasCriterion> <http://www.w3.org/1999/02/22-rdf-syntax-ns#type> <http://www.w3.org/2000/01/rdf-schema#Property> .
<http://purl.org/ASN/schema/core/EducationalFramework> <http://www.w3.org/2000/01/rdf-schema#comment> "The class of all structured sets of conceptual resources intentionally designed for use as value vocabulary terms in education and training contexts."@en-us .
<http://purl.org/ASN/schema/core/alignTo> <http://www.w3.org/1999/02/22-rdf-syntax-ns#type> <http://www.w3.org/1999/02/22-rdf-syntax-ns#Property> .
<http://purl.org/ASN/schema/core/Rubric> <http://www.w3.org/2000/01/rdf-schema#isDefinedBy> <http://purl.org/ASN/schema/core/> .
<http://purl.org/ASN/schema/core/localSubject> <http://www.w3.org/2000/01/rdf-schema#label> "Local Subject" .
<http://purl.org/ASN/schema/core/alignTo> <http://www.w3.org/2000/01/rdf-schema#isDefinedBy> <http://purl.org/ASN/schema/core/> .
<http://purl.org/ASN/schema/core/assessmentRubric> <http://www.w3.org/2000/01/rdf-schema#domain> <http://purl.org/ASN/schema/core/StandardDocument> .
<http://purl.org/ASN/schema/core/localSubject> <http://www.w3.org/2000/01/rdf-schema#subPropertyOf> <http://purl.org/dc/terms/subject> .
<http://purl.org/ASN/schema/core/conceptKeyword> <http://www.w3.org/2000/01/rdf-schema#subPropertyOf> <http://purl.org/dc/elements/1.1/subject> .
<http://purl.org/ASN/schema/core/majorCorrelation> <http://www.w3.org/2000/01/rdf-schema#domain> <http://purl.org/ASN/schema/core/LearningResource> .
<http://purl.org/ASN/schema/core/source> <http://www.w3.org/1999/02/22-rdf-syntax-ns#type> <http://www.w3.org/2000/01/rdf-schema#Property> .
<http://purl.org/ASN/schema/core/localSubject> <http://www.w3.org/2000/01/rdf-schema#comment> "The text string denoting the subject of the statement as designated by the promulgating agency. This subject may be different from the asn:subject used for subject classification within the ASN." .
<http://purl.org/ASN/schema/core/CorrelationResource> <http://www.w3.org/2000/01/rdf-schema#comment> "A resource that describes the mapping between a learning resource and a node in a learning outcomes framework."@en-us .
<http://purl.org/ASN/schema/core/hasCriterion> <http://www.w3.org/2000/01/rdf-schema#range> <http://purl.org/ASN/schema/core/RubricCriterion> .
<http://purl.org/ASN/schema/core/> <http://purl.org/dc/elements/1.1/title> "The Achievement Standards Network Core Properties"@en-us .
<http://purl.org/ASN/schema/core/alignTo> <http://www.w3.org/2000/01/rdf-schema#label> "align to" .
<http://purl.org/ASN/schema/core/jurisdiction> <http://purl.org/dc/elements/1.1/description> "The URI of the jurisdiction from the ASNJurisdiction controlled vocabulary."@en-us .
<http://purl.org/ASN/schema/core/LearningResource> <http://www.w3.org/2000/01/rdf-schema#isDefinedBy> <http://purl.org/ASN/schema/core/> .
<http://purl.org/ASN/schema/core/alignFrom> <http://www.w3.org/2000/01/rdf-schema#comment> "A standards document or statement from which the statement or document being described is aligned." .
<http://purl.org/ASN/schema/core/exactAlignment> <http://www.w3.org/2000/01/rdf-schema#comment> "The relevant concepts in both competencies are coextensive." .
<http://purl.org/ASN/schema/core/proficiencyLevel> <http://purl.org/dc/elements/1.1/description> "The value of asn:proficiencyLevel should be a concept IRI of a member of the class asn:ProficiencyScale."@en .
<http://purl.org/ASN/schema/core/identifier> <http://www.w3.org/2000/01/rdf-schema#comment> "An alternative URI by which the resource is identified." .
<http://purl.org/ASN/schema/core/narrowCorrelation> <http://www.w3.org/2000/01/rdf-schema#domain> <http://purl.org/ASN/schema/core/LearningResource> .
<http://purl.org/ASN/schema/core/DerivedStandardDocument> <http://www.w3.org/2000/01/rdf-schema#label> "Derived Standard Document"@en-us .
<http://purl.org/ASN/schema/core/crossSubjectReference> <http://www.w3.org/2000/01/rdf-schema#comment> "An explicit reference by the promulgating agency establishing a relationship between the statement being described and statement in a separate subject standards document (interdisciplinary statement references)." .
<http://purl.org/ASN/schema/core/proficiencyLevel> <http://www.w3.org/2000/01/rdf-schema#range> <http://purl.org/ASN/schema/core/ProficiencyScale> .
<http://purl.org/ASN/schema/core/hasScope> <http://www.w3.org/2000/01/rdf-schema#range> <http://www.w3.org/1999/02/22-rdf-syntax-ns#langString> .
<http://purl.org/ASN/schema/core/minorAlignment> <http://www.w3.org/2000/01/rdf-schema#isDefinedBy> <http://purl.org/ASN/schema/core/> .
<http://purl.org/ASN/schema/core/JurisdictionScheme> <http://www.w3.org/1999/02/22-rdf-syntax-ns#type> <http://www.w3.org/2000/01/rdf-schema#Class> .
<http://purl.org/ASN/schema/core/conceptTerm> <http://www.w3.org/2000/01/rdf-schema#subPropertyOf> <http://purl.org/dc/elements/1.1/subject> .
<http://purl.org/ASN/schema/core/minorAlignment> <http://www.w3.org/1999/02/22-rdf-syntax-ns#type> <http://www.w3.org/1999/02/22-rdf-syntax-ns#Property> .
<http://purl.org/ASN/schema/core/DerivedStatement> <http://www.w3.org/1999/02/22-rdf-syntax-ns#type> <http://www.w3.org/2000/01/rdf-schema#Class> .
<http://purl.org/ASN/schema/core/benchmark> <http://purl.org/vocab/vann/usageNote> "Can have one or more per CriterionLevel."@en-us .
<http://purl.org/ASN/schema/core/minorAlignment> <http://www.w3.org/2000/01/rdf-schema#domain> <http://purl.org/ASN/schema/core/Statement> .
<http://purl.org/ASN/schema/core/CriterionLevel> <http://www.w3.org/2000/01/rdf-schema#label> "Criterion Level"@en-us .
<http://purl.org/ASN/schema/core/exactCorrelation> <http://www.w3.org/2000/01/rdf-schema#subPropertyOf> <http://purl.org/dc/terms/conformsTo> .
<http://purl.org/ASN/schema/core/source> <http://www.w3.org/2000/01/rdf-schema#domain> <http://purl.org/ASN/schema/core/Rubric> .
<http://purl.org/ASN/schema/core/statementNotation> <http://www.w3.org/1999/02/22-rdf-syntax-ns#type> <http://www.w3.org/1999/02/22-rdf-syntax-ns#Property> .
<http://purl.org/ASN/schema/core/narrowCorrelation> <http://www.w3.org/2000/01/rdf-schema#comment> "The learning resource being described covers all of the relevant concepts in the competency statement as well as relevant concepts not found in the competency." .
<http://purl.org/ASN/schema/core/CorrelationResource> <http://www.w3.org/2000/01/rdf-schema#label> "Correlation Resource"@en-us .
<http://purl.org/ASN/schema/core/weight> <http://www.w3.org/2000/01/rdf-schema#comment> "A textually asserted measurement of the weight, degree, percent, or strength of a recommendation, requirement, or comparison; e.g., \"15%\", \".5\"." .
<http://purl.org/ASN/schema/core/statementNotation> <http://www.w3.org/2000/01/rdf-schema#isDefinedBy> <http://purl.org/ASN/schema/core/> .
<http://purl.org/ASN/schema/core/broadAlignment> <http://www.w3.org/2000/01/rdf-schema#comment> "The target competency covers all of the relevant concepts in the competency being described as well as relevant concepts not found in the competency being described." .
<http://purl.org/ASN/schema/core/sequence> <http://www.w3.org/2002/07/owl#equivalentProperty> <https://ceds.ed.gov/CEDSElementDetails.aspx?TermId=14445> .
<http://purl.org/ASN/schema/core/publicationStatus> <http://www.w3.org/2000/01/rdf-schema#label> "Publication Status" .
<http://purl.org/ASN/schema/core/statementNotation> <http://www.w3.org/2000/01/rdf-schema#subPropertyOf> <http://purl.org/dc/terms/identifer> .
<http://purl.org/ASN/schema/core/hasCriterion> <http://www.w3.org/2000/01/rdf-schema#domain> <http://purl.org/ASN/schema/core/Rubric> .
<http://purl.org/ASN/schema/core/statementLabel> <http://www.w3.org/2000/01/rdf-schema#isDefinedBy> <http://purl.org/ASN/schema/core/> .
<http://purl.org/ASN/schema/core/prerequisiteAlignment> <http://www.w3.org/2000/01/rdf-schema#label> "Prerequisite Alignment" .
<http://purl.org/ASN/schema/core/jurisdiction> <http://www.w3.org/2000/01/rdf-schema#isDefinedBy> <http://purl.org/ASN/schema/core/> .
<http://purl.org/ASN/schema/core/proficiencyLevel> <http://schema.org/domainIncludes> <http://purl.org/ASN/schema/core/Statement> .
<http://purl.org/ASN/schema/core/statementLabel> <http://www.w3.org/1999/02/22-rdf-syntax-ns#type> <http://www.w3.org/1999/02/22-rdf-syntax-ns#Property> .
<http://purl.org/ASN/schema/core/jurisdiction> <http://www.w3.org/1999/02/22-rdf-syntax-ns#type> <http://www.w3.org/1999/02/22-rdf-syntax-ns#Property> .
<http://purl.org/ASN/schema/core/proficiencyLevel> <http://www.w3.org/1999/02/22-rdf-syntax-ns#type> <http://www.w3.org/1999/02/22-rdf-syntax-ns#Property> .
<http://purl.org/ASN/schema/core/narrowCorrelation> <http://www.w3.org/2000/01/rdf-schema#label> "Narrow Correlation" .
<http://purl.org/ASN/schema/core/narrowCorrelation> <http://www.w3.org/2000/01/rdf-schema#isDefinedBy> <http://purl.org/ASN/schema/core/> .
<http://purl.org/ASN/schema/core/score> <http://www.w3.org/2000/01/rdf-schema#domain> <http://purl.org/ASN/schema/core/CriterionLevel> .
<http://purl.org/ASN/schema/core/EducationalFramework> <http://purl.org/dc/elements/1.1/description> "Similar to the class skos:ConceptScheme with an intended focus on education and training. Examples of educational frameworks include, but are not limited to, frameworks enumerating competencies, text complexity, proficiency scales, assessment rubrics of various forms, and specialized subject vocabularies."@en-us .
<http://purl.org/ASN/schema/core/proficiencyLevel> <http://www.w3.org/2000/01/rdf-schema#isDefinedBy> <http://purl.org/ASN/schema/core/> .
<http://purl.org/ASN/schema/core/ProficiencyScale> <http://www.w3.org/2000/01/rdf-schema#isDefinedBy> <http://purl.org/ASN/schema/core/> .
<http://purl.org/ASN/schema/core/narrowCorrelation> <http://www.w3.org/1999/02/22-rdf-syntax-ns#type> <http://www.w3.org/1999/02/22-rdf-syntax-ns#Property> .
<http://purl.org/ASN/schema/core/CriterionCategory> <http://www.w3.org/2000/01/rdf-schema#label> "Criterion Category"@en-us .
<http://purl.org/ASN/schema/core/jurisdiction> <http://www.w3.org/2000/01/rdf-schema#comment> "The jurisdiction or domain of the standard's application--e.g., California, Nebraska, etc." .
<http://purl.org/ASN/schema/core/statementNotation> <http://www.w3.org/2000/01/rdf-schema#label> "Statement Notation" .
<http://purl.org/ASN/schema/core/assessesCompetency> <http://www.w3.org/2000/01/rdf-schema#subPropertyOf> <http://purl.org/dc/terms/conformsTo> .
<http://purl.org/ASN/schema/core/authorityStatus> <http://www.w3.org/2000/01/rdf-schema#comment> "The status of a standards statement denoting whether the statement owes its origin to the promulgating agency of the standards document of which the statement is a member (i.e., value \"Original\") or to some 3rd party (i.e., \"Derived\")." .
<http://purl.org/ASN/schema/core/qualityLabel> <http://www.w3.org/2000/01/rdf-schema#domain> <http://purl.org/ASN/schema/core/CriterionLevel> .
<http://purl.org/ASN/schema/core/criterionFor> <http://www.w3.org/2000/01/rdf-schema#isDefinedBy> <http://purl.org/ASN/schema/core/> .
<http://purl.org/ASN/schema/core/exportVersion> <http://www.w3.org/2000/01/rdf-schema#label> "Export Version" .
<http://purl.org/ASN/schema/core/minorCorrelation> <http://www.w3.org/2000/01/rdf-schema#comment> "Minor overlap of relevant concepts between the learning resource being described and the competency statement." .
<http://purl.org/ASN/schema/core/broadCorrelation> <http://www.w3.org/2000/01/rdf-schema#range> <http://purl.org/ASN/schema/core/Statement> .
<http://purl.org/ASN/schema/core/majorAlignment> <http://www.w3.org/2000/01/rdf-schema#label> "Major Alignment" .
<http://purl.org/ASN/schema/core/exportVersion> <http://www.w3.org/2000/01/rdf-schema#isDefinedBy> <http://purl.org/ASN/schema/core/> .
<http://purl.org/ASN/schema/core/hasCriterion> <http://www.w3.org/2000/01/rdf-schema#label> "Has Criterion"@en-us .
<http://purl.org/ASN/schema/core/hasCriterionCategory> <http://www.w3.org/2000/01/rdf-schema#isDefinedBy> <http://purl.org/ASN/schema/core/> .
<http://purl.org/ASN/schema/core/hasScope> <http://www.w3.org/2000/01/rdf-schema#comment> "Description of what the rubric's creator intended to assess or evaluate."@en-us .
<http://purl.org/ASN/schema/core/exportVersion> <http://www.w3.org/1999/02/22-rdf-syntax-ns#type> <http://www.w3.org/1999/02/22-rdf-syntax-ns#Property> .
<http://purl.org/ASN/schema/core/proficiencyLevel> <http://schema.org/domainIncludes> <http://purl.org/ASN/schema/core/LearningResource> .
<http://purl.org/ASN/schema/core/narrowAlignment> <http://www.w3.org/2000/01/rdf-schema#range> <http://purl.org/ASN/schema/core/Statement> .
<http://purl.org/ASN/schema/core/CriterionLevel> <http://www.w3.org/2000/01/rdf-schema#isDefinedBy> <http://purl.org/ASN/schema/core/> .
<http://purl.org/ASN/schema/core/alignTo> <http://purl.org/dc/elements/1.1/description> "An alignment is an assertion of some degree of eqiuvalency\n            between the subject and the object of the assertion."@en-us .
<http://purl.org/ASN/schema/core/altStatementNotation> <http://www.w3.org/2000/01/rdf-schema#label> "Alternative Statement Notation" .
<http://purl.org/ASN/schema/core/sequence> <http://www.w3.org/2000/01/rdf-schema#comment> "Numeric value representing the resource's position in the list (array) of resources."@en-us .
<http://purl.org/ASN/schema/core/DerivedStatement> <http://www.w3.org/2000/01/rdf-schema#subClassOf> <http://purl.org/ASN/schema/core/Statement> .
<http://purl.org/ASN/schema/core/publicationStatus> <http://www.w3.org/2000/01/rdf-schema#comment> "The publication status of the of the standards document--e.g., Draft, Published, Deprecated." .
<http://purl.org/ASN/schema/core/broadAlignment> <http://www.w3.org/2000/01/rdf-schema#label> "Broad Alignment" .
<http://purl.org/ASN/schema/core/score> <http://www.w3.org/1999/02/22-rdf-syntax-ns#type> <http://www.w3.org/2000/01/rdf-schema#Property> .
<http://purl.org/ASN/schema/core/majorCorrelation> <http://www.w3.org/2000/01/rdf-schema#comment> "Major overlap of relevant concepts between the learning resource being described and the competency statement." .
<http://purl.org/ASN/schema/core/assessmentRubric> <http://www.w3.org/2000/01/rdf-schema#label> "Assessment Rubric"@en-us .
<http://purl.org/ASN/schema/core/qualityLabel> <http://www.w3.org/1999/02/22-rdf-syntax-ns#type> <http://www.w3.org/2000/01/rdf-schema#Property> .
<http://purl.org/ASN/schema/core/statementLabel> <http://www.w3.org/2000/01/rdf-schema#label> "Statement Label" .
<http://purl.org/ASN/schema/core/Statement> <http://www.w3.org/1999/02/22-rdf-syntax-ns#type> <http://www.w3.org/2000/01/rdf-schema#Class> .
<http://purl.org/ASN/schema/core/assessmentRubric> <http://www.w3.org/1999/02/22-rdf-syntax-ns#type> <http://www.w3.org/2000/01/rdf-schema#Property> .
<http://purl.org/ASN/schema/core/minorCorrelation> <http://www.w3.org/2000/01/rdf-schema#range> <http://purl.org/ASN/schema/core/Statement> .
<http://purl.org/ASN/schema/core/sequence> <http://www.w3.org/2000/01/rdf-schema#isDefinedBy> <http://purl.org/ASN/schema/core/> .
<http://purl.org/ASN/schema/core/JurisdictionScheme> <http://www.w3.org/2000/01/rdf-schema#comment> "Controlled vocabularies of terms denoting the juristiction or domain of the standards document."@en-us .
<http://purl.org/ASN/schema/core/score> <http://www.w3.org/2000/01/rdf-schema#comment> "Points to be awarded for achieving this level for a RubricCriterion."@en-us .
<http://purl.org/ASN/schema/core/prerequisiteCompetency> <http://www.w3.org/2000/01/rdf-schema#range> <http://purl.org/ASN/schema/core/Statement> .
<http://purl.org/ASN/schema/core/DerivedStatement> <http://www.w3.org/2000/01/rdf-schema#comment> "An assertion representing an expectation of what students should know, value, and be able to do at a target age or age range that is derived from a statement defined by a different jurisdiction."@en-us .
<http://purl.org/ASN/schema/core/derivedFrom> <http://www.w3.org/2000/01/rdf-schema#label> "Derived From" .
<http://purl.org/ASN/schema/core/ProficiencyScale> <http://www.w3.org/2000/01/rdf-schema#label> "Proficiency Scale"@en-us .
<http://purl.org/ASN/schema/core/majorAlignment> <http://www.w3.org/2000/01/rdf-schema#range> <http://purl.org/ASN/schema/core/Statement> .
<http://purl.org/ASN/schema/core/hasLevel> <http://www.w3.org/1999/02/22-rdf-syntax-ns#type> <http://www.w3.org/2000/01/rdf-schema#Property> .
<http://purl.org/ASN/schema/core/broadAlignment> <http://www.w3.org/2000/01/rdf-schema#range> <http://purl.org/ASN/schema/core/Statement> .
<http://purl.org/ASN/schema/core/StandardDocument> <http://www.w3.org/2000/01/rdf-schema#isDefinedBy> <http://purl.org/ASN/schema/core/> .
<http://purl.org/ASN/schema/core/minorAlignment> <http://www.w3.org/2000/01/rdf-schema#comment> "Minor overlap of relevant concepts between the two competencies." .
<http://purl.org/ASN/schema/core/assessesCompetency> <http://www.w3.org/2000/01/rdf-schema#isDefinedBy> <http://purl.org/ASN/schema/core/> .
<http://purl.org/ASN/schema/core/comment> <http://purl.org/dc/elements/1.1/description> "Use comment when the text provides useful context for the statement."@en-us .
<http://purl.org/ASN/schema/core/> <http://purl.org/dc/elements/1.1/description> "The Achievement Standards Network Core namespace provides URIs for many of the terms used in ASN metadata instances. Custom ASN application profiles can be achieved through use of properties and classes from other RDF schemas and ontologies. Vocabulary terms are declared using RDF Schema language to support RDF applications."@en-us .
<http://purl.org/ASN/schema/core/weight> <http://www.w3.org/2000/01/rdf-schema#label> "Weight" .
<http://purl.org/ASN/schema/core/assessesCompetency> <http://www.w3.org/1999/02/22-rdf-syntax-ns#type> <http://www.w3.org/1999/02/22-rdf-syntax-ns#Property> .
<http://purl.org/ASN/schema/core/narrowCorrelation> <http://www.w3.org/2000/01/rdf-schema#subPropertyOf> <http://purl.org/dc/terms/conformsTo> .
<http://purl.org/ASN/schema/core/weight> <http://www.w3.org/2000/01/rdf-schema#domain> <http://purl.org/ASN/schema/core/Statement> .
<http://purl.org/ASN/schema/core/assessesCompetency> <http://www.w3.org/2000/01/rdf-schema#label> "Assesses Competency" .
<http://purl.org/ASN/schema/core/prerequisiteAlignment> <http://www.w3.org/2000/01/rdf-schema#range> <http://purl.org/ASN/schema/core/Statement> .
<http://purl.org/ASN/schema/core/conceptKeyword> <http://www.w3.org/1999/02/22-rdf-syntax-ns#type> <http://www.w3.org/1999/02/22-rdf-syntax-ns#Property> .
<http://purl.org/ASN/schema/core/crossSubjectReference> <http://www.w3.org/1999/02/22-rdf-syntax-ns#type> <http://www.w3.org/1999/02/22-rdf-syntax-ns#Property> .
<http://purl.org/ASN/schema/core/conceptKeyword> <http://www.w3.org/2000/01/rdf-schema#isDefinedBy> <http://purl.org/ASN/schema/core/> .
<http://purl.org/ASN/schema/core/crossSubjectReference> <http://www.w3.org/2000/01/rdf-schema#isDefinedBy> <http://purl.org/ASN/schema/core/> .
<http://purl.org/ASN/schema/core/criterionFor> <http://www.w3.org/2000/01/rdf-schema#comment> "Reference to the asn:Rubric to which the asn:RubricCriteria being described belongs."@en-us .
<http://purl.org/ASN/schema/core/majorCorrelation> <http://www.w3.org/2000/01/rdf-schema#range> <http://purl.org/ASN/schema/core/Statement> .
<http://purl.org/ASN/schema/core/hasLevel> <http://www.w3.org/2000/01/rdf-schema#domain> <http://purl.org/ASN/schema/core/RubricCriterion> .
<http://purl.org/ASN/schema/core/Rubric> <http://www.w3.org/1999/02/22-rdf-syntax-ns#type> <http://www.w3.org/2000/01/rdf-schema#Class> .
<http://purl.org/ASN/schema/core/hasScope> <http://www.w3.org/2000/01/rdf-schema#label> "Has Scope"@en-us .
<http://purl.org/ASN/schema/core/levelFor> <http://www.w3.org/1999/02/22-rdf-syntax-ns#type> <http://www.w3.org/2000/01/rdf-schema#Property> .
<http://purl.org/ASN/schema/core/teachesCompetency> <http://www.w3.org/2000/01/rdf-schema#range> <http://purl.org/ASN/schema/core/Statement> .
<http://purl.org/ASN/schema/core/hasScope> <http://www.w3.org/1999/02/22-rdf-syntax-ns#type> <http://www.w3.org/2000/01/rdf-schema#Property> .
<http://purl.org/ASN/schema/core/indexingStatus> <http://www.w3.org/2000/01/rdf-schema#comment> "The status of the statement denoting whether correlators should or should not assign the statement during correlation--Values=\"Yes\"/\"No\"." .
<http://purl.org/ASN/schema/core/exportVersion> <http://www.w3.org/2000/01/rdf-schema#comment> "The URI of the export version of the standards file." .
<http://purl.org/ASN/schema/core/hasLevel> <http://www.w3.org/2000/01/rdf-schema#label> "Has Level"@en-us .
<http://purl.org/ASN/schema/core/hasLevel> <http://purl.org/vocab/vann/usageNote> "Both asn:RubricCriterion and CriterionCategory have an asn:sequence property to identify node order; however, json-ld encodings should use @list on the asn:hasCriterion and asn:hasLevel properties to maintain such sequencing."@en-us .
<http://purl.org/ASN/schema/core/RubricCriterion> <http://www.w3.org/2000/01/rdf-schema#isDefinedBy> <http://purl.org/ASN/schema/core/> .
<http://purl.org/ASN/schema/core/derivedFrom> <http://www.w3.org/2000/01/rdf-schema#isDefinedBy> <http://purl.org/ASN/schema/core/> .
<http://purl.org/ASN/schema/core/prerequisiteAlignment> <http://www.w3.org/2000/01/rdf-schema#comment> "The competency being described is a prerequisite to the target competency." .
<http://purl.org/ASN/schema/core/benchmark> <http://www.w3.org/2000/01/rdf-schema#isDefinedBy> <http://purl.org/ASN/schema/core/> .
<http://purl.org/ASN/schema/core/derivedFrom> <http://www.w3.org/1999/02/22-rdf-syntax-ns#type> <http://www.w3.org/1999/02/22-rdf-syntax-ns#Property> .
<http://purl.org/ASN/schema/core/LearningResource> <http://www.w3.org/2000/01/rdf-schema#comment> "A resource that is used as part of an Educational Activity(e.g. a textbook) or that describes (e.g. a lesson plan) or records the Educational Activity (e.g. an audio- or video-recording of a lesson)."@en-us .
<http://purl.org/ASN/schema/core/Rubric> <http://www.w3.org/2000/01/rdf-schema#comment> "Resource providing guidance in evaluating the quality and level of person's responses or actions based on an explicit set of criteria."@en-us .
<http://purl.org/ASN/schema/core/weight> <http://www.w3.org/2000/01/rdf-schema#isDefinedBy> <http://purl.org/ASN/schema/core/> .
<http://purl.org/ASN/schema/core/teachesCompetency> <http://www.w3.org/2000/01/rdf-schema#label> "Teaches Competency" .
<http://purl.org/ASN/schema/core/listID> <http://www.w3.org/2000/01/rdf-schema#comment> "A set of one or more alphanumeric characters and/or symbols denoting the positioning of the statement being described in a sequential listing of statements." .
<http://purl.org/ASN/schema/core/weight> <http://www.w3.org/1999/02/22-rdf-syntax-ns#type> <http://www.w3.org/1999/02/22-rdf-syntax-ns#Property> .
<http://purl.org/ASN/schema/core/hasCriterion> <http://www.w3.org/2000/01/rdf-schema#comment> "RubricCriterian referenced by the Rubric that defining criterion to be met to demonstrate quality in execution in performance of a task or obtaining an objectivetask."@en-us .
<http://purl.org/ASN/schema/core/qualityLabel> <http://www.w3.org/2000/01/rdf-schema#range> <http://www.w3.org/2001/XMLSchema#string> .
<http://purl.org/ASN/schema/core/> <http://purl.org/dc/terms/modified> "2019-02-26"^^<dcterms:W3CDTF> .
<http://purl.org/ASN/schema/core/assessmentRubric> <http://www.w3.org/2000/01/rdf-schema#range> <http://purl.org/ASN/schema/core/Rubric> .
<http://purl.org/ASN/schema/core/authorityStatus> <http://www.w3.org/2000/01/rdf-schema#isDefinedBy> <http://purl.org/ASN/schema/core/> .
<http://purl.org/ASN/schema/core/CorrelationResource> <http://www.w3.org/1999/02/22-rdf-syntax-ns#type> <http://www.w3.org/2000/01/rdf-schema#Class> .
<http://purl.org/ASN/schema/core/Statement> <http://www.w3.org/2000/01/rdf-schema#comment> "An assertion representing an expectation of what students should know, value, and be able to do at a target age or age range."@en-us .
<http://purl.org/ASN/schema/core/comment> <http://www.w3.org/2000/01/rdf-schema#label> "comment" .
<http://purl.org/ASN/schema/core/EducationalFramework> <http://www.w3.org/2000/01/rdf-schema#isDefinedBy> <http://purl.org/ASN/schema/core/> .
<http://purl.org/ASN/schema/core/levelFor> <http://www.w3.org/2000/01/rdf-schema#domain> <http://purl.org/ASN/schema/core/CriterionLevel> .
<http://purl.org/ASN/schema/core/authorityStatus> <http://www.w3.org/1999/02/22-rdf-syntax-ns#type> <http://www.w3.org/1999/02/22-rdf-syntax-ns#Property> .
<http://purl.org/ASN/schema/core/exactCorrelation> <http://www.w3.org/2000/01/rdf-schema#domain> <http://purl.org/ASN/schema/core/LearningResource> .
<http://purl.org/ASN/schema/core/hasCriterionCategory> <http://www.w3.org/2000/01/rdf-schema#domain> <http://purl.org/ASN/schema/core/Rubric> .
<http://purl.org/ASN/schema/core/source> <http://www.w3.org/2000/01/rdf-schema#isDefinedBy> <http://purl.org/ASN/schema/core/> .
<http://purl.org/ASN/schema/core/StandardDocument> <http://www.w3.org/2000/01/rdf-schema#comment> "A collection of statements representing an expectation of what students should know, value, and be able to do at a target age or age range."@en-us .
<http://purl.org/ASN/schema/core/comprisedOf> <http://purl.org/dc/elements/1.1/description> "Deliberately not defining domains and ranges for the property at this time." .
<http://purl.org/ASN/schema/core/listID> <http://www.w3.org/2000/01/rdf-schema#label> "List ID" .
<http://purl.org/ASN/schema/core/criterionFor> <http://www.w3.org/2000/01/rdf-schema#label> "Criterian For"@en-us .
<http://purl.org/ASN/schema/core/hasLevel> <http://www.w3.org/2000/01/rdf-schema#comment> "Resource description of a level of performance based on a RubricCriterion."@en-us .
<http://purl.org/ASN/schema/core/repositoryDate> <http://www.w3.org/2000/01/rdf-schema#comment> "The date the standards document was added to the repository." .
<http://purl.org/ASN/schema/core/indexingStatus> <http://www.w3.org/1999/02/22-rdf-syntax-ns#type> <http://www.w3.org/1999/02/22-rdf-syntax-ns#Property> .
<http://purl.org/ASN/schema/core/assessesCompetency> <http://www.w3.org/2000/01/rdf-schema#domain> <http://purl.org/ASN/schema/core/LearningResource> .
<http://purl.org/ASN/schema/core/benchmark> <http://www.w3.org/2002/07/owl#equivalentProperty> <https://ceds.ed.gov/CEDSElementDetails.aspx?TermId=14443> .
<http://purl.org/ASN/schema/core/indexingStatus> <http://www.w3.org/2000/01/rdf-schema#isDefinedBy> <http://purl.org/ASN/schema/core/> .
<http://purl.org/ASN/schema/core/LearningResource> <http://www.w3.org/2000/01/rdf-schema#label> "Learning Resource"@en-us .
<http://purl.org/ASN/schema/core/JurisdictionScheme> <http://www.w3.org/2000/01/rdf-schema#label> "Jurisdiction Encoding Schemes"@en-us .
<http://purl.org/ASN/schema/core/exactCorrelation> <http://www.w3.org/2000/01/rdf-schema#comment> "The relevant concepts in the educational resource and the standard statement are coextensive." .
<http://purl.org/ASN/schema/core/exactAlignment> <http://www.w3.org/1999/02/22-rdf-syntax-ns#type> <http://www.w3.org/1999/02/22-rdf-syntax-ns#Property> .
<http://purl.org/ASN/schema/core/comprisedOf> <http://www.w3.org/2000/01/rdf-schema#comment> "The resource being described includes, comprehends or encompass, in whole or in part, the meaning, nature or importance of the resource being referenced."@en-us .
<http://purl.org/ASN/schema/core/hasCriterion> <http://www.w3.org/2000/01/rdf-schema#isDefinedBy> <http://purl.org/ASN/schema/core/> .
<http://purl.org/ASN/schema/core/exactAlignment> <http://www.w3.org/2000/01/rdf-schema#isDefinedBy> <http://purl.org/ASN/schema/core/> .
<http://purl.org/ASN/schema/core/exactAlignment> <http://www.w3.org/2000/01/rdf-schema#domain> <http://purl.org/ASN/schema/core/Statement> .
<http://purl.org/ASN/schema/core/DerivedStandardDocument> <http://www.w3.org/2000/01/rdf-schema#isDefinedBy> <http://purl.org/ASN/schema/core/> .
<http://purl.org/ASN/schema/core/prerequisiteCompetency> <http://www.w3.org/2000/01/rdf-schema#label> "Prerequisite Competency" .
<http://purl.org/ASN/schema/core/exactCorrelation> <http://www.w3.org/1999/02/22-rdf-syntax-ns#type> <http://www.w3.org/1999/02/22-rdf-syntax-ns#Property> .
<http://purl.org/ASN/schema/core/> <http://purl.org/dc/terms/issued> "2004-04-29"^^<dcterms:W3CDTF> .
<http://purl.org/ASN/schema/core/exactCorrelation> <http://www.w3.org/2000/01/rdf-schema#isDefinedBy> <http://purl.org/ASN/schema/core/> .
<http://purl.org/ASN/schema/core/StatusScheme> <http://www.w3.org/2000/01/rdf-schema#comment> "Controlled vocabularies of terms denoting the publication status of the standards document."@en-us .
<http://purl.org/ASN/schema/core/RubricCriterion> <http://www.w3.org/2000/01/rdf-schema#label> "Rubric Criterion"@en-us .
<http://purl.org/ASN/schema/core/complexityLevel> <http://www.w3.org/2000/01/rdf-schema#comment> "The expected performance level of a learner or professional as defined by a competency." .
<http://purl.org/ASN/schema/core/conceptKeyword> <http://www.w3.org/2000/01/rdf-schema#label> "Concept Keyword" .
<http://purl.org/ASN/schema/core/publicationStatus> <http://www.w3.org/1999/02/22-rdf-syntax-ns#type> <http://www.w3.org/1999/02/22-rdf-syntax-ns#Property> .
<http://purl.org/ASN/schema/core/authorityStatus> <http://www.w3.org/2000/01/rdf-schema#label> "Authority Status" .
<http://purl.org/ASN/schema/core/StatusScheme> <http://www.w3.org/1999/02/22-rdf-syntax-ns#type> <http://www.w3.org/2000/01/rdf-schema#Class> .
<http://purl.org/ASN/schema/core/RubricCriterion> <http://www.w3.org/2000/01/rdf-schema#comment> "Resource identifying a criterion that must be met to demonstrate quality performance of a objective or task."@en-us .
<http://purl.org/ASN/schema/core/publicationStatus> <http://www.w3.org/2000/01/rdf-schema#isDefinedBy> <http://purl.org/ASN/schema/core/> .
<http://purl.org/ASN/schema/core/CriterionCategory> <http://www.w3.org/2000/01/rdf-schema#isDefinedBy> <http://purl.org/ASN/schema/core/> .
<http://purl.org/ASN/schema/core/skillEmbodied> <http://www.w3.org/2000/01/rdf-schema#isDefinedBy> <http://purl.org/ASN/schema/core/> .
<http://purl.org/ASN/schema/core/broadCorrelation> <http://www.w3.org/2000/01/rdf-schema#comment> "The competency covers all of the relevant concepts in the learning resource being described as well as relevant concepts not found in the learning resource." .
<http://purl.org/ASN/schema/core/Rubric> <http://www.w3.org/2000/01/rdf-schema#label> "Rubric"@en-us .
<http://purl.org/ASN/schema/core/altStatementNotation> <http://www.w3.org/2000/01/rdf-schema#comment> "An alphanumeric notation or ID code identifying the statement in common use among end-users." .
<http://purl.org/ASN/schema/core/skillEmbodied> <http://www.w3.org/1999/02/22-rdf-syntax-ns#type> <http://www.w3.org/1999/02/22-rdf-syntax-ns#Property> .
<http://purl.org/ASN/schema/core/score> <http://www.w3.org/2000/01/rdf-schema#label> "Criterion Level Score"@en-us .
<http://purl.org/ASN/schema/core/minorAlignment> <http://www.w3.org/2000/01/rdf-schema#label> "Minor Alignment" .
<http://purl.org/ASN/schema/core/repositoryDate> <http://www.w3.org/2000/01/rdf-schema#subPropertyOf> <http://purl.org/dc/terms/date> .
<http://purl.org/ASN/schema/core/proficiencyLevel> <http://www.w3.org/2000/01/rdf-schema#comment> "The expected performance level of a learner or professional in relationship to a competency."@en .
<http://purl.org/ASN/schema/core/StandardDocument> <http://www.w3.org/1999/02/22-rdf-syntax-ns#type> <http://www.w3.org/2000/01/rdf-schema#Class> .
<http://purl.org/ASN/schema/core/EducationalFramework> <http://www.w3.org/2000/01/rdf-schema#label> "Educational Framework"@en-us .
<http://purl.org/ASN/schema/core/alignFrom> <http://www.w3.org/2000/01/rdf-schema#label> "align from" .
<http://purl.org/ASN/schema/core/comprisedOf> <http://www.w3.org/1999/02/22-rdf-syntax-ns#type> <http://www.w3.org/1999/02/22-rdf-syntax-ns#Property> .
<http://purl.org/ASN/schema/core/DerivedStatement> <http://www.w3.org/2000/01/rdf-schema#label> "Derived Statement"@en-us .
<http://purl.org/ASN/schema/core/qualityLabel> <http://www.w3.org/2000/01/rdf-schema#label> "Quality Label"@en-us .
<http://purl.org/ASN/schema/core/comprisedOf> <http://www.w3.org/2000/01/rdf-schema#isDefinedBy> <http://purl.org/ASN/schema/core/> .
<http://purl.org/ASN/schema/core/prerequisiteCompetency> <http://www.w3.org/2000/01/rdf-schema#comment> "A prerequisite competency for the learning resource being described." .
<http://purl.org/ASN/schema/core/prerequisiteCompetency> <http://www.w3.org/2000/01/rdf-schema#domain> <http://purl.org/ASN/schema/core/LearningResource> .
<http://purl.org/ASN/schema/core/> <http://purl.org/dc/elements/1.1/language> "English"@en-us .
<http://purl.org/ASN/schema/core/minorCorrelation> <http://www.w3.org/2000/01/rdf-schema#domain> <http://purl.org/ASN/schema/core/LearningResource> .
<http://purl.org/ASN/schema/core/score> <http://www.w3.org/2002/07/owl#equivalentProperty> <https://ceds.ed.gov/CEDSElementDetails.aspx?TermId=14447> .
<http://purl.org/ASN/schema/core/Statement> <http://www.w3.org/2000/01/rdf-schema#isDefinedBy> <http://purl.org/ASN/schema/core/> .
<http://purl.org/ASN/schema/core/broadCorrelation> <http://www.w3.org/2000/01/rdf-schema#domain> <http://purl.org/ASN/schema/core/LearningResource> .
<http://purl.org/ASN/schema/core/minorAlignment> <http://www.w3.org/2000/01/rdf-schema#range> <http://purl.org/ASN/schema/core/Statement> .
<http://purl.org/ASN/schema/core/source> <http://www.w3.org/2000/01/rdf-schema#label> "Source"@en-us .
<http://purl.org/ASN/schema/core/CriterionLevel> <http://www.w3.org/1999/02/22-rdf-syntax-ns#type> <http://www.w3.org/2000/01/rdf-schema#Class> .
<http://purl.org/ASN/schema/core/benchmark> <http://www.w3.org/2000/01/rdf-schema#range> <http://www.w3.org/1999/02/22-rdf-syntax-ns#langString> .
<http://purl.org/ASN/schema/core/derivedFrom> <http://purl.org/dc/elements/1.1/description> "The derivedFrom property is used by 3rd parties only in derived statements and must appear in conjunction with a value of \"Derived\" in the statement's authorityStatus property."@en-us .
<http://purl.org/ASN/schema/core/ProficiencyScale> <http://www.w3.org/2000/01/rdf-schema#comment> "The class of all structured concept schemes identifying discrete levels of expertise and performance mastery required either by a competency or to be achieved by a learner."@en-us .
<http://purl.org/ASN/schema/core/conceptKeyword> <http://www.w3.org/2000/01/rdf-schema#comment> "A word or phrase used by the promulgating agency to refine and differentiate individual statements contextually." .
<http://purl.org/ASN/schema/core/alignTo> <http://www.w3.org/2000/01/rdf-schema#comment> "A standards document or statement to which the statement or document being described is aligned." .
<http://purl.org/ASN/schema/core/ProficiencyScale> <http://www.w3.org/1999/02/22-rdf-syntax-ns#type> <http://www.w3.org/2000/01/rdf-schema#Class> .
<http://purl.org/ASN/schema/core/complexityLevel> <http://www.w3.org/2000/01/rdf-schema#range> <http://purl.org/ASN/schema/core/ProficiencyScale> .
<http://purl.org/ASN/schema/core/hasLevel> <http://www.w3.org/2002/07/owl#equivalentProperty> <https://ceds.ed.gov/CEDSElementDetails.aspx?TermId=14443> .
<http://purl.org/ASN/schema/core/broadAlignment> <http://www.w3.org/2000/01/rdf-schema#isDefinedBy> <http://purl.org/ASN/schema/core/> .
<http://purl.org/ASN/schema/core/majorAlignment> <http://www.w3.org/1999/02/22-rdf-syntax-ns#type> <http://www.w3.org/1999/02/22-rdf-syntax-ns#Property> .
<http://purl.org/ASN/schema/core/hasLevel> <http://www.w3.org/2000/01/rdf-schema#isDefinedBy> <http://purl.org/ASN/schema/core/> .
<http://purl.org/ASN/schema/core/broadAlignment> <http://www.w3.org/1999/02/22-rdf-syntax-ns#type> <http://www.w3.org/1999/02/22-rdf-syntax-ns#Property> .
<http://purl.org/ASN/schema/core/majorAlignment> <http://www.w3.org/2000/01/rdf-schema#isDefinedBy> <http://purl.org/ASN/schema/core/> .
<http://purl.org/ASN/schema/core/minorCorrelation> <http://www.w3.org/2000/01/rdf-schema#label> "Minor Correlation" .
<http://purl.org/ASN/schema/core/minorCorrelation> <http://www.w3.org/1999/02/22-rdf-syntax-ns#type> <http://www.w3.org/1999/02/22-rdf-syntax-ns#Property> .
<http://purl.org/ASN/schema/core/sequence> <http://www.w3.org/1999/02/22-rdf-syntax-ns#type> <http://www.w3.org/2000/01/rdf-schema#Property> .
<http://purl.org/ASN/schema/core/prerequisiteCompetency> <http://www.w3.org/2000/01/rdf-schema#isDefinedBy> <http://purl.org/ASN/schema/core/> .
<http://purl.org/ASN/schema/core/minorCorrelation> <http://www.w3.org/2000/01/rdf-schema#isDefinedBy> <http://purl.org/ASN/schema/core/> .
<http://purl.org/ASN/schema/core/> <http://purl.org/dc/elements/1.1/contributor> "D2L"@en-us .
<http://purl.org/ASN/schema/core/ProficiencyScale> <http://purl.org/dc/elements/1.1/description> "Proficiency scales define levels of performance (what a person does) as distinct from knowledge of specific information (what a person knows) and outline tasks a person can manage and the skills necessary to progressively accomplish explicit competencies at increasing levels of complexity. Proficiency scales: (1) assist in making judgments about the kinds of tasks related to a competency that a person is able to perform; and (2) to compare the abilities of different persons with regard to achievement of those competencies at different levels."@en-us .
<http://purl.org/ASN/schema/core/proficiencyLevel> <http://www.w3.org/2000/01/rdf-schema#label> "Proficiency Level" .
<http://purl.org/ASN/schema/core/prerequisiteCompetency> <http://www.w3.org/1999/02/22-rdf-syntax-ns#type> <http://www.w3.org/1999/02/22-rdf-syntax-ns#Property> .
<http://purl.org/ASN/schema/core/complexityLevel> <http://www.w3.org/2000/01/rdf-schema#domain> <http://purl.org/ASN/schema/core/Statement> .
<http://purl.org/ASN/schema/core/narrowAlignment> <http://www.w3.org/2000/01/rdf-schema#domain> <http://purl.org/ASN/schema/core/Statement> .
<http://purl.org/ASN/schema/core/qualityLabel> <http://www.w3.org/2000/01/rdf-schema#isDefinedBy> <http://purl.org/ASN/schema/core/> .
<http://purl.org/ASN/schema/core/jurisdiction> <http://www.w3.org/2000/01/rdf-schema#label> "Jurisdiction" .
<http://purl.org/ASN/schema/core/teachesCompetency> <http://www.w3.org/2000/01/rdf-schema#subPropertyOf> <http://purl.org/dc/terms/conformsTo> .
<http://purl.org/ASN/schema/core/DerivedStandardDocument> <http://www.w3.org/2000/01/rdf-schema#subClassOf> <http://purl.org/ASN/schema/core/StandardDocument> .
<http://purl.org/ASN/schema/core/assessmentRubric> <http://www.w3.org/2000/01/rdf-schema#isDefinedBy> <http://purl.org/ASN/schema/core/> .
<http://purl.org/ASN/schema/core/identifier> <http://www.w3.org/2000/01/rdf-schema#subPropertyOf> <http://purl.org/dc/terms/identifier> .
<http://purl.org/ASN/schema/core/hasCriterionCategory> <http://www.w3.org/2000/01/rdf-schema#label> "Has Criterion Category"@en-us .
<http://purl.org/ASN/schema/core/hasCriterionCategory> <http://www.w3.org/2000/01/rdf-schema#comment> "Resource referenced by the Rubric that defines categories for clustering logical sets of RubricCriterion."@en-us .
<http://purl.org/ASN/schema/core/broadCorrelation> <http://www.w3.org/2000/01/rdf-schema#label> "Broad Correlation" .
<http://purl.org/ASN/schema/core/score> <http://www.w3.org/2000/01/rdf-schema#range> <http://www.w3.org/2001/XMLSchema#float> .
<http://purl.org/ASN/schema/core/score> <http://www.w3.org/2000/01/rdf-schema#isDefinedBy> <http://purl.org/ASN/schema/core/> .
<http://purl.org/ASN/schema/core/localSubject> <http://www.w3.org/1999/02/22-rdf-syntax-ns#type> <http://www.w3.org/1999/02/22-rdf-syntax-ns#Property> .
<http://purl.org/ASN/schema/core/localSubject> <http://www.w3.org/2000/01/rdf-schema#isDefinedBy> <http://purl.org/ASN/schema/core/> .
<http://purl.org/ASN/schema/core/hasLevel> <http://www.w3.org/2000/01/rdf-schema#range> <http://purl.org/ASN/schema/core/CriterionLevel> .
<http://purl.org/ASN/schema/core/narrowAlignment> <http://www.w3.org/2000/01/rdf-schema#label> "Narrow Alignment" .
<http://purl.org/ASN/schema/core/comprisedOf> <http://www.w3.org/2000/01/rdf-schema#label> "Comprised Of" .
<http://purl.org/ASN/schema/core/sequence> <http://www.w3.org/2000/01/rdf-schema#domain> <http://purl.org/ASN/schema/core/CriterionLevel> .
<http://purl.org/ASN/schema/core/identifier> <http://www.w3.org/1999/02/22-rdf-syntax-ns#type> <http://www.w3.org/1999/02/22-rdf-syntax-ns#Property> .
<http://purl.org/ASN/schema/core/JurisdictionScheme> <http://www.w3.org/2000/01/rdf-schema#isDefinedBy> <http://purl.org/ASN/schema/core/> .
<http://purl.org/ASN/schema/core/narrowAlignment> <http://www.w3.org/2000/01/rdf-schema#isDefinedBy> <http://purl.org/ASN/schema/core/> .
<http://purl.org/ASN/schema/core/benchmark> <http://www.w3.org/2000/01/rdf-schema#label> "Benchmark"@en-us .
<http://purl.org/ASN/schema/core/complexityLevel> <http://www.w3.org/2000/01/rdf-schema#isDefinedBy> <http://purl.org/ASN/schema/core/> .
<http://purl.org/ASN/schema/core/identifier> <http://www.w3.org/2000/01/rdf-schema#isDefinedBy> <http://purl.org/ASN/schema/core/> .
<http://purl.org/ASN/schema/core/majorCorrelation> <http://www.w3.org/2000/01/rdf-schema#subPropertyOf> <http://purl.org/dc/terms/conformsTo> .
<http://purl.org/ASN/schema/core/narrowAlignment> <http://www.w3.org/1999/02/22-rdf-syntax-ns#type> <http://www.w3.org/1999/02/22-rdf-syntax-ns#Property> .
<http://purl.org/ASN/schema/core/complexityLevel> <http://www.w3.org/1999/02/22-rdf-syntax-ns#type> <http://www.w3.org/1999/02/22-rdf-syntax-ns#Property> .
<http://purl.org/ASN/schema/core/hasCriterionCategory> <http://www.w3.org/1999/02/22-rdf-syntax-ns#type> <http://www.w3.org/2000/01/rdf-schema#Property> .
<http://purl.org/ASN/schema/core/DerivedStatement> <http://www.w3.org/2000/01/rdf-schema#isDefinedBy> <http://purl.org/ASN/schema/core/> .
<http://purl.org/ASN/schema/core/exactAlignment> <http://www.w3.org/2000/01/rdf-schema#label> "Exact Alignment" .
<http://purl.org/ASN/schema/core/hasScope> <http://www.w3.org/2000/01/rdf-schema#domain> <http://purl.org/ASN/schema/core/Rubric> .
<http://purl.org/ASN/schema/core/broadCorrelation> <http://www.w3.org/2000/01/rdf-schema#isDefinedBy> <http://purl.org/ASN/schema/core/> .
<http://purl.org/ASN/schema/core/StandardDocument> <http://www.w3.org/2000/01/rdf-schema#label> "Standard Document"@en-us .
<http://purl.org/ASN/schema/core/broadCorrelation> <http://www.w3.org/1999/02/22-rdf-syntax-ns#type> <http://www.w3.org/1999/02/22-rdf-syntax-ns#Property> .
<http://purl.org/ASN/schema/core/criterionFor> <http://www.w3.org/1999/02/22-rdf-syntax-ns#type> <http://www.w3.org/2000/01/rdf-schema#Property> .
<http://purl.org/ASN/schema/core/LearningResource> <http://www.w3.org/1999/02/22-rdf-syntax-ns#type> <http://www.w3.org/2000/01/rdf-schema#Class> .
<http://purl.org/ASN/schema/core/comment> <http://www.w3.org/1999/02/22-rdf-syntax-ns#type> <http://www.w3.org/1999/02/22-rdf-syntax-ns#Property> .
<http://purl.org/ASN/schema/core/complexityLevel> <http://purl.org/dc/elements/1.1/description> "The value of asn:complexityLevel should be a concept IRI of a member of the class asn:ProficiencyScale."@en-us .
<http://purl.org/ASN/schema/core/conceptTerm> <http://www.w3.org/2000/01/rdf-schema#label> "Concept Term" .
<http://purl.org/ASN/schema/core/levelFor> <http://www.w3.org/2000/01/rdf-schema#range> <http://purl.org/ASN/schema/core/RubricCriterion> .
<http://purl.org/ASN/schema/core/Statement> <http://www.w3.org/2000/01/rdf-schema#label> "Statement"@en-us .
<http://purl.org/ASN/schema/core/conceptTerm> <http://www.w3.org/1999/02/22-rdf-syntax-ns#type> <http://www.w3.org/1999/02/22-rdf-syntax-ns#Property> .
<http://purl.org/ASN/schema/core/broadAlignment> <http://www.w3.org/2000/01/rdf-schema#domain> <http://purl.org/ASN/schema/core/Statement> .
<http://purl.org/ASN/schema/core/narrowCorrelation> <http://www.w3.org/2000/01/rdf-schema#range> <http://purl.org/ASN/schema/core/Statement> .
<http://purl.org/ASN/schema/core/alignFrom> <http://purl.org/dc/elements/1.1/description> "An alignment is an assertion of some degree of eqiuvalency between the subject and the object of the assertion."@en-us .
<http://purl.org/ASN/schema/core/comment> <http://www.w3.org/2000/01/rdf-schema#isDefinedBy> <http://purl.org/ASN/schema/core/> .
<http://purl.org/ASN/schema/core/complexityLevel> <http://www.w3.org/2000/01/rdf-schema#label> "Complexity Level" .
<http://purl.org/ASN/schema/core/conceptTerm> <http://www.w3.org/2000/01/rdf-schema#isDefinedBy> <http://purl.org/ASN/schema/core/> .
<http://purl.org/ASN/schema/core/statementNotation> <http://www.w3.org/2000/01/rdf-schema#comment> "An alphanumeric identifier of a Statement as defined by the promulgating agency. Statement notation must be unique within the defining organization's namespace." .
<http://purl.org/ASN/schema/core/majorAlignment> <http://www.w3.org/2000/01/rdf-schema#domain> <http://purl.org/ASN/schema/core/Statement> .
