<https://data.nasa.gov/ontologies/atmonto/data#etmsDepartures> <http://www.w3.org/2000/01/rdf-schema#comment> "Count of departures at airport based on ETMS (Enhanced Traffic Management System) data." .
<https://data.nasa.gov/ontologies/atmonto/NAS#Airport> <http://www.w3.org/2000/01/rdf-schema#subClassOf> <https://data.nasa.gov/ontologies/atmonto/data#METARreportingStation> .
_:B0969422aX2D6d5dX2D4265X2D83a8X2D066412c1e4df <http://www.w3.org/1999/02/22-rdf-syntax-ns#rest> _:Bf27add84X2D9124X2D4875X2Da3aeX2Dae2ca2ff433f .
<https://data.nasa.gov/ontologies/atmonto/data#seaLevelPressure> <http://www.w3.org/1999/02/22-rdf-syntax-ns#type> <http://www.w3.org/2002/07/owl#DatatypeProperty> .
<https://data.nasa.gov/ontologies/atmonto/data#scheduledArrivals> <http://www.w3.org/2000/01/rdf-schema#range> <http://www.w3.org/2001/XMLSchema#integer> .
<https://data.nasa.gov/ontologies/atmonto/data#VisibilityCondition> <http://www.w3.org/2000/01/rdf-schema#subClassOf> <https://data.nasa.gov/ontologies/atmonto/data#MetCondition> .
<https://data.nasa.gov/ontologies/atmonto/data#oagGateDepartureDelay> <http://www.w3.org/2000/01/rdf-schema#comment> "Minutes of OAG (Official Airline Guide) based gate departure delay in excess of 15 minutes." .
<https://data.nasa.gov/ontologies/atmonto/data#hasASPMmetCondition> <http://www.w3.org/1999/02/22-rdf-syntax-ns#type> <http://www.w3.org/2002/07/owl#ObjectProperty> .
<https://data.nasa.gov/ontologies/atmonto/data#runwayVisibleRange> <http://www.w3.org/2000/01/rdf-schema#range> <https://data.nasa.gov/ontologies/atmonto/NAS#RunwayVisibleRangeMeasurement> .
_:B70dd1fefX2D2850X2D4663X2Db3f0X2Da291ae44a230 <http://www.w3.org/1999/02/22-rdf-syntax-ns#rest> <http://www.w3.org/1999/02/22-rdf-syntax-ns#nil> .
<https://data.nasa.gov/ontologies/atmonto/data#oagGateDepartureDelay> <http://www.w3.org/2000/01/rdf-schema#range> <http://www.w3.org/2001/XMLSchema#integer> .
<https://data.nasa.gov/ontologies/atmonto/data#FixFlow> <http://www.w3.org/2000/01/rdf-schema#label> "Fix flow" .
<https://data.nasa.gov/ontologies/atmonto/data#associatedMETARreportingStation> <http://www.w3.org/2000/01/rdf-schema#comment> "Links a METAR report to the reporting station where the data were collected." .
<https://data.nasa.gov/ontologies/atmonto/data#cloudCover> <http://www.w3.org/2000/01/rdf-schema#label> "cloud cover" .
<https://data.nasa.gov/ontologies/atmonto/data#hasAirportData> <http://www.w3.org/2000/01/rdf-schema#label> "has airport data" .
_:Bfae980e0X2De811X2D47caX2Da09bX2D9125d95d22d5 <http://www.w3.org/2002/07/owl#allValuesFrom> _:B37b4539cX2Defd3X2D4968X2D8828X2D0816c74be323 .
<https://data.nasa.gov/ontologies/atmonto/data#aspmFlightRules> <http://www.w3.org/2000/01/rdf-schema#domain> <https://data.nasa.gov/ontologies/atmonto/data#AirportData> .
_:Bc93945cdX2Dbbb5X2D4eacX2Da84cX2D697ea4b10cb0 <http://www.w3.org/1999/02/22-rdf-syntax-ns#type> <http://www.w3.org/2002/07/owl#Restriction> .
<https://data.nasa.gov/ontologies/atmonto/data#runwayReportedOn> <http://www.w3.org/1999/02/22-rdf-syntax-ns#type> <http://www.w3.org/2002/07/owl#ObjectProperty> .
_:B2b621779X2D2b0eX2D4b01X2D8daaX2D4ca45b169260 <http://www.w3.org/1999/02/22-rdf-syntax-ns#rest> <http://www.w3.org/1999/02/22-rdf-syntax-ns#nil> .
_:Be07d6f98X2D2f29X2D4301X2Db3a4X2D6815000d445d <http://www.w3.org/1999/02/22-rdf-syntax-ns#type> <http://www.w3.org/2002/07/owl#Restriction> .
<https://data.nasa.gov/ontologies/atmonto/data#dataIntervalStartDay> <http://www.w3.org/2000/01/rdf-schema#range> <https://data.nasa.gov/ontologies/atmonto/NAS#NASday> .
<https://data.nasa.gov/ontologies/atmonto/data#runwaySurfaceFriction> <http://www.w3.org/1999/02/22-rdf-syntax-ns#type> <http://www.w3.org/2002/07/owl#DatatypeProperty> .
_:B250d7406X2D0509X2D47c9X2Dac7aX2Daee37a2553ab <http://www.w3.org/2002/07/owl#oneOf> _:B4463fd56X2D8ffbX2D4550X2D8bc2X2Dbae635adbf25 .
<https://data.nasa.gov/ontologies/atmonto/data#surfaceWindSpeed> <http://www.w3.org/2000/01/rdf-schema#domain> <https://data.nasa.gov/ontologies/atmonto/data#SurfaceWindCondition> .
<https://data.nasa.gov/ontologies/atmonto/data#forecastIssueTime> <http://www.w3.org/2000/01/rdf-schema#domain> <https://data.nasa.gov/ontologies/atmonto/data#TAFreport> .
<https://data.nasa.gov/ontologies/atmonto/data#associatedMETARreportingStation> <http://www.w3.org/2000/01/rdf-schema#domain> <https://data.nasa.gov/ontologies/atmonto/data#METARreport> .
<https://data.nasa.gov/ontologies/atmonto/data#WITIproperty> <http://www.w3.org/1999/02/22-rdf-syntax-ns#type> <http://www.w3.org/2002/07/owl#Class> .
_:Bfac1032cX2Dd316X2D4b77X2Da395X2D41ef2744759a <http://www.w3.org/1999/02/22-rdf-syntax-ns#first> "gradual" .
<https://data.nasa.gov/ontologies/atmonto/data#metarReportModifier> <http://www.w3.org/2000/01/rdf-schema#domain> <https://data.nasa.gov/ontologies/atmonto/data#METARreport> .
<https://data.nasa.gov/ontologies/atmonto/data#hasTAFreport> <http://www.w3.org/2000/01/rdf-schema#label> "has TAFreport" .
<https://data.nasa.gov/ontologies/atmonto/data#etmsDepartures> <http://www.w3.org/1999/02/22-rdf-syntax-ns#type> <http://www.w3.org/2002/07/owl#DatatypeProperty> .
<https://data.nasa.gov/ontologies/atmonto/data#hasSkyCondition> <http://www.w3.org/2000/01/rdf-schema#label> "has sky condition" .
<https://data.nasa.gov/ontologies/atmonto/data#hasAirportData> <http://www.w3.org/1999/02/22-rdf-syntax-ns#type> <http://www.w3.org/2002/07/owl#ObjectProperty> .
<https://data.nasa.gov/ontologies/atmonto/data#oagArrivalDelay> <http://www.w3.org/2000/01/rdf-schema#domain> <https://data.nasa.gov/ontologies/atmonto/data#AirportData> .
<https://data.nasa.gov/ontologies/atmonto/data#surfaceTemperature> <http://www.w3.org/2000/01/rdf-schema#label> "surface temperature" .
_:Bd6384cdeX2Dd08aX2D4cf2X2D882fX2Dd0745776d655 <http://www.w3.org/1999/02/22-rdf-syntax-ns#type> <http://www.w3.org/2002/07/owl#Restriction> .
<https://data.nasa.gov/ontologies/atmonto/data#CloudLayer> <http://www.w3.org/2000/01/rdf-schema#subClassOf> _:B1af074b8X2D5962X2D4fcbX2Daca3X2Da844f3426735 .
<https://data.nasa.gov/ontologies/atmonto/data#TAFreport> <http://www.w3.org/2000/01/rdf-schema#subClassOf> _:B8e425b69X2D6e28X2D45ceX2Dbe5aX2D37148e4c513b .
<https://data.nasa.gov/ontologies/atmonto/data#highWindWITIdaily> <http://www.w3.org/2000/01/rdf-schema#range> <http://www.w3.org/2001/XMLSchema#float> .
<https://data.nasa.gov/ontologies/atmonto/data#dataIntervalStartDay> <http://www.w3.org/1999/02/22-rdf-syntax-ns#type> <http://www.w3.org/2002/07/owl#ObjectProperty> .
<https://data.nasa.gov/ontologies/atmonto/NAS#StandAloneWeatherStation> <http://www.w3.org/2000/01/rdf-schema#subClassOf> <https://data.nasa.gov/ontologies/atmonto/data#METARreportingStation> .
<https://data.nasa.gov/ontologies/atmonto/data#hasSkyCondition> <http://www.w3.org/2000/01/rdf-schema#domain> <https://data.nasa.gov/ontologies/atmonto/data#MeteorologicalCondition> .
<https://data.nasa.gov/ontologies/atmonto/data#etmsArrivals> <http://www.w3.org/2000/01/rdf-schema#domain> <https://data.nasa.gov/ontologies/atmonto/data#AirportData> .
<https://data.nasa.gov/ontologies/atmonto/data#limitedVisibilityDistance> <http://www.w3.org/2000/01/rdf-schema#comment> "The visibility distance (in miles) at the reporting station. Only applicable if data:unlimitedVisibility is False." .
_:Bfae980e0X2De811X2D47caX2Da09bX2D9125d95d22d5 <http://www.w3.org/2002/07/owl#onProperty> <https://data.nasa.gov/ontologies/atmonto/data#cloudCover> .
_:B6401bc46X2D5951X2D460fX2D8449X2D8cac8d53dacc <http://www.w3.org/1999/02/22-rdf-syntax-ns#type> <http://www.w3.org/2002/07/owl#Restriction> .
<https://data.nasa.gov/ontologies/atmonto/data#IntervalData> <http://www.w3.org/2000/01/rdf-schema#label> "Interval data" .
<https://data.nasa.gov/ontologies/atmonto/data#TAFmeteorologicalCondition> <http://www.w3.org/2000/01/rdf-schema#comment> "Meteorological conditions reported as part of a TAF forecast. Includes sky, wind, visibility and weather components for current and future time periods." .
<https://data.nasa.gov/ontologies/atmonto/data#weatherIntensity> <http://www.w3.org/2000/01/rdf-schema#comment> "An indicator of the intensity of the weather: light, moderate, heavy." .
<https://data.nasa.gov/ontologies/atmonto/data#CloudLayerProfile> <http://www.w3.org/2000/01/rdf-schema#comment> "A sequence of cloud layers, ordered from the ground upward. Represents cloud conditions." .
<https://data.nasa.gov/ontologies/atmonto/data#windDirectionLower> <http://www.w3.org/2000/01/rdf-schema#comment> "Lower bound (in degrees) of two bounding values describing a variable wind direction." .
_:Be0657408X2Dc1a6X2D446aX2D8e38X2D6dc3b0f5ac14 <http://www.w3.org/1999/02/22-rdf-syntax-ns#rest> _:B7b5530c5X2D489cX2D4cc0X2Da132X2Dccd6bb298bac .
<https://data.nasa.gov/ontologies/atmonto/data#runwayVisibleRange> <http://www.w3.org/1999/02/22-rdf-syntax-ns#type> <http://www.w3.org/2002/07/owl#FunctionalProperty> .
_:B8c48c716X2D963cX2D4959X2Db42cX2Dbd4a96019db6 <http://www.w3.org/2002/07/owl#onProperty> <https://data.nasa.gov/ontologies/atmonto/data#cloudCover> .
<https://data.nasa.gov/ontologies/atmonto/data#meteorologicalConditionStatus> <http://www.w3.org/2000/01/rdf-schema#range> <http://www.w3.org/2001/XMLSchema#string> .
<https://data.nasa.gov/ontologies/atmonto/data#ASPMmeteorologicalCondition> <http://www.w3.org/2000/01/rdf-schema#subClassOf> <https://data.nasa.gov/ontologies/atmonto/data#MeteorologicalCondition> .
<http://spinrdf.org/arg#class> <http://www.w3.org/2000/01/rdf-schema#subPropertyOf> <http://spinrdf.org/sp#arg> .
<https://data.nasa.gov/ontologies/atmonto/data#rapidityOfWeatherChange> <http://www.w3.org/2000/01/rdf-schema#comment> "Indicates how fast change is expected from the prior state to the forecast meteorological conditions: \"rapid\" , \"gradual\" , \"transient\"." .
<https://data.nasa.gov/ontologies/atmonto/data#lowCeilingWITIhourly> <http://www.w3.org/2000/01/rdf-schema#range> <http://www.w3.org/2001/XMLSchema#float> .
<https://data.nasa.gov/ontologies/atmonto/data#limitedVisibilityDistance> <http://www.w3.org/2000/01/rdf-schema#domain> <https://data.nasa.gov/ontologies/atmonto/data#VisibilityCondition> .
_:B6f05af65X2D3ac3X2D4eabX2D8ba2X2D79da922e7fed <http://www.w3.org/1999/02/22-rdf-syntax-ns#type> <http://www.w3.org/2002/07/owl#Restriction> .
<https://data.nasa.gov/ontologies/atmonto/data#unlimitedVisibility> <http://www.w3.org/1999/02/22-rdf-syntax-ns#type> <http://www.w3.org/2002/07/owl#DatatypeProperty> .
<https://data.nasa.gov/ontologies/atmonto/data#lowVisibilityWITIdaily> <http://www.w3.org/2000/01/rdf-schema#domain> <https://data.nasa.gov/ontologies/atmonto/data#AirportData> .
<https://data.nasa.gov/ontologies/atmonto/data#tafReportString> <http://www.w3.org/2000/01/rdf-schema#comment> "The full text of the entire TAF report." .
<https://data.nasa.gov/ontologies/atmonto/data#edctDepartureHold> <http://www.w3.org/2000/01/rdf-schema#domain> <https://data.nasa.gov/ontologies/atmonto/data#AirportData> .
<https://data.nasa.gov/ontologies/atmonto/data#associatedMETARreportingStation> <http://www.w3.org/2000/01/rdf-schema#label> "METAR reporting station" .
<https://data.nasa.gov/ontologies/atmonto/data#totalAirborneDelay> <http://www.w3.org/1999/02/22-rdf-syntax-ns#type> <http://www.w3.org/2002/07/owl#DatatypeProperty> .
_:B8ebf7271X2Db1a5X2D4b4aX2Daa9cX2D74891abd525a <http://www.w3.org/1999/02/22-rdf-syntax-ns#first> "immediate proximity" .
_:B5f8fce50X2Dc5d8X2D48daX2Db7c6X2D7c1b6f6af3c4 <http://www.w3.org/1999/02/22-rdf-syntax-ns#rest> _:B32708683X2D2838X2D496bX2Db4d3X2Da7511750f66b .
<https://data.nasa.gov/ontologies/atmonto/data#scheduledDepartures> <http://www.w3.org/2000/01/rdf-schema#domain> <https://data.nasa.gov/ontologies/atmonto/data#AirportData> .
_:Bb855cbbbX2De2e6X2D4090X2D875cX2D7250d013f1b5 <http://www.w3.org/1999/02/22-rdf-syntax-ns#type> <http://www.w3.org/2002/07/owl#Restriction> .
<https://data.nasa.gov/ontologies/atmonto/data#meteorologicalConditionStatus> <http://www.w3.org/2000/01/rdf-schema#label> "meteorological condition status" .
<https://data.nasa.gov/ontologies/atmonto/data#metarReportString> <http://www.w3.org/2000/01/rdf-schema#range> <http://www.w3.org/2001/XMLSchema#string> .
_:B41ecb1f3X2D60e9X2D435eX2Dad0eX2D1d88e2ff9118 <http://www.w3.org/1999/02/22-rdf-syntax-ns#first> "freezing" .
<https://data.nasa.gov/ontologies/atmonto/data#windShearHeight> <http://www.w3.org/2000/01/rdf-schema#range> <http://www.w3.org/2001/XMLSchema#float> .
_:Bdb55bab6X2Db468X2D44cfX2Da5b8X2D694e6526dfe0 <http://www.w3.org/1999/02/22-rdf-syntax-ns#rest> _:B795569e6X2D13d8X2D47e9X2Dbf2aX2D18d54d334b74 .
<https://data.nasa.gov/ontologies/atmonto/data#runwayReportedOn> <http://www.w3.org/2000/01/rdf-schema#domain> <https://data.nasa.gov/ontologies/atmonto/data#RunwayStatusData> .
<https://data.nasa.gov/ontologies/atmonto/data#weatherProximity> <http://www.w3.org/2000/01/rdf-schema#label> "weather proximity" .
<https://data.nasa.gov/ontologies/atmonto/data#surfaceWindDirectionStatus> <http://www.w3.org/1999/02/22-rdf-syntax-ns#type> <http://www.w3.org/2002/07/owl#DatatypeProperty> .
<https://data.nasa.gov/ontologies/atmonto/data#SectorFlow> <http://www.w3.org/2000/01/rdf-schema#subClassOf> _:Bebd0d737X2D5b76X2D489dX2D8cb9X2D2aad44a9506d .
_:B37b4539cX2Defd3X2D4968X2D8828X2D0816c74be323 <http://www.w3.org/2002/07/owl#oneOf> _:Bdb55bab6X2Db468X2D44cfX2Da5b8X2D694e6526dfe0 .
_:B707feedbX2Dbc93X2D4d7aX2D9954X2D1fff0050275c <http://www.w3.org/1999/02/22-rdf-syntax-ns#rest> _:B2635a848X2Dce68X2D4e2bX2Db928X2Dd7161a537f11 .
<https://data.nasa.gov/ontologies/atmonto/data#windShearHeight> <http://www.w3.org/2000/01/rdf-schema#label> "wind shear height" .
_:B035d8c87X2D8e8bX2D4c64X2D80c1X2Dc15f119e4b26 <http://www.w3.org/2002/07/owl#allValuesFrom> _:B872639bbX2D4805X2D484bX2Db538X2D2f7feb5abf7c .
<https://data.nasa.gov/ontologies/atmonto/data#METARreport> <http://www.w3.org/2000/01/rdf-schema#subClassOf> _:Bf20a1683X2D7158X2D4ef2X2Da159X2D2674318ddcfd .
_:B46fafbb9X2D8a44X2D44f2X2Da251X2D9afc5da3912e <http://www.w3.org/1999/02/22-rdf-syntax-ns#first> "SPECI" .
_:Bebd0d737X2D5b76X2D489dX2D8cb9X2D2aad44a9506d <http://www.w3.org/2002/07/owl#allValuesFrom> <https://data.nasa.gov/ontologies/atmonto/NAS#Sector> .
<https://data.nasa.gov/ontologies/atmonto/data#runwayVisibleRange> <http://www.w3.org/2000/01/rdf-schema#comment> "Links a visibility condition to a runway visible range measurement class instance." .
<https://data.nasa.gov/ontologies/atmonto/data#metarReportString> <http://www.w3.org/2000/01/rdf-schema#label> "METAR report string" .
_:Bd270744aX2D8b58X2D4e82X2D84aeX2Dbec1f8e37e13 <http://www.w3.org/2002/07/owl#allValuesFrom> <https://data.nasa.gov/ontologies/atmonto/data#TAFmeteorologicalCondition> .
<https://data.nasa.gov/ontologies/atmonto/data#CloudLayer> <http://www.w3.org/2000/01/rdf-schema#label> "Cloud layer" .
_:Bb2447386X2D2e28X2D4c69X2Dba49X2De5dfe47e13ba <http://www.w3.org/1999/02/22-rdf-syntax-ns#type> <http://www.w3.org/2002/07/owl#Restriction> .
_:B4463fd56X2D8ffbX2D4550X2D8bc2X2Dbae635adbf25 <http://www.w3.org/1999/02/22-rdf-syntax-ns#rest> _:B72137fc5X2D81ccX2D4df0X2D8a6fX2D197abe2a15e1 .
<https://data.nasa.gov/ontologies/atmonto/data#ceiling> <http://www.w3.org/2000/01/rdf-schema#range> <http://www.w3.org/2001/XMLSchema#integer> .
<https://data.nasa.gov/ontologies/atmonto/data#AirportData> <http://www.w3.org/2000/01/rdf-schema#comment> "Represents a collection of airport data for a given time period, as reported by the FAA's ASPM system." .
<https://data.nasa.gov/ontologies/atmonto/data#METARreport> <http://www.w3.org/2000/01/rdf-schema#subClassOf> _:B6401bc46X2D5951X2D460fX2D8449X2D8cac8d53dacc .
<https://data.nasa.gov/ontologies/atmonto/data#metarReportType> <http://www.w3.org/1999/02/22-rdf-syntax-ns#type> <http://www.w3.org/2002/07/owl#DatatypeProperty> .
<http://spinrdf.org/arg#class> <http://www.w3.org/1999/02/22-rdf-syntax-ns#type> <http://www.w3.org/1999/02/22-rdf-syntax-ns#Property> .
_:B1af074b8X2D5962X2D4fcbX2Daca3X2Da844f3426735 <http://www.w3.org/1999/02/22-rdf-syntax-ns#type> <http://www.w3.org/2002/07/owl#Restriction> .
<https://data.nasa.gov/ontologies/atmonto/data#dataIntervalEndTime> <http://www.w3.org/2000/01/rdf-schema#range> <http://www.w3.org/2001/XMLSchema#dateTime> .
_:B70d3bda9X2D6639X2D4f0eX2D8d65X2D7c412969f5f8 <http://www.w3.org/2002/07/owl#onProperty> <https://data.nasa.gov/ontologies/atmonto/data#weatherProximity> .
<https://data.nasa.gov/ontologies/atmonto/data#CloudLayer> <http://www.w3.org/1999/02/22-rdf-syntax-ns#type> <http://www.w3.org/2002/07/owl#Class> .
<https://data.nasa.gov/ontologies/atmonto/data#hasSurfaceWindCondition> <http://www.w3.org/2000/01/rdf-schema#domain> <https://data.nasa.gov/ontologies/atmonto/data#MeteorologicalCondition> .
_:Bf20a1683X2D7158X2D4ef2X2Da159X2D2674318ddcfd <http://www.w3.org/2002/07/owl#cardinality> "1"^^<http://www.w3.org/2001/XMLSchema#nonNegativeInteger> .
<https://data.nasa.gov/ontologies/atmonto/data#lowCeilingWITIdaily> <http://www.w3.org/1999/02/22-rdf-syntax-ns#type> <http://www.w3.org/2002/07/owl#FunctionalProperty> .
<https://data.nasa.gov/ontologies/atmonto/data#dataIntervalEndTime> <http://www.w3.org/2000/01/rdf-schema#comment> "For temporally-dependent data, the ending time of the data's period of validity." .
_:Bb4bc8a40X2Db4beX2D4bcdX2D812eX2D895e29907502 <http://www.w3.org/1999/02/22-rdf-syntax-ns#rest> <http://www.w3.org/1999/02/22-rdf-syntax-ns#nil> .
<https://data.nasa.gov/ontologies/atmonto/data#weatherIntensity> <http://www.w3.org/2000/01/rdf-schema#range> <http://www.w3.org/2001/XMLSchema#string> .
<https://data.nasa.gov/ontologies/atmonto/data#FixFlow> <http://www.w3.org/1999/02/22-rdf-syntax-ns#type> <http://www.w3.org/2002/07/owl#Class> .
<https://data.nasa.gov/ontologies/atmonto/data#etmsArrivals> <http://www.w3.org/2000/01/rdf-schema#range> <http://www.w3.org/2001/XMLSchema#integer> .
<https://data.nasa.gov/ontologies/atmonto/data#seaLevelPressure> <http://www.w3.org/2000/01/rdf-schema#domain> <https://data.nasa.gov/ontologies/atmonto/data#MeteorologicalCondition> .
<https://data.nasa.gov/ontologies/atmonto/data#hasCloudLayerProfile> <http://www.w3.org/2000/01/rdf-schema#domain> <https://data.nasa.gov/ontologies/atmonto/data#SkyCondition> .
<https://data.nasa.gov/ontologies/atmonto/data#edctDepartureHold> <http://www.w3.org/2000/01/rdf-schema#range> <http://www.w3.org/2001/XMLSchema#float> .
<https://data.nasa.gov/ontologies/atmonto/data#CloudLayerProfile> <http://www.w3.org/2000/01/rdf-schema#subClassOf> <https://data.nasa.gov/ontologies/atmonto/general#Sequence> .
<https://data.nasa.gov/ontologies/atmonto/data#departureDemand> <http://www.w3.org/2000/01/rdf-schema#label> "departure demand" .
<https://data.nasa.gov/ontologies/atmonto/data#oagArrivalDelay> <http://www.w3.org/2000/01/rdf-schema#range> <http://www.w3.org/2001/XMLSchema#integer> .
<https://data.nasa.gov/ontologies/atmonto/data#departureDemand> <http://www.w3.org/1999/02/22-rdf-syntax-ns#type> <http://www.w3.org/2002/07/owl#DatatypeProperty> .
_:B1b277598X2Dd23fX2D4f2aX2Db4caX2D14883857655f <http://www.w3.org/1999/02/22-rdf-syntax-ns#rest> _:Bf3a1516bX2D1813X2D48e1X2DaaabX2D215f13285700 .
_:Bc93945cdX2Dbbb5X2D4eacX2Da84cX2D697ea4b10cb0 <http://www.w3.org/2002/07/owl#maxCardinality> "1"^^<http://www.w3.org/2001/XMLSchema#int> .
_:B8e425b69X2D6e28X2D45ceX2Dbe5aX2D37148e4c513b <http://www.w3.org/2002/07/owl#allValuesFrom> <https://data.nasa.gov/ontologies/atmonto/data#TAFmeteorologicalCondition> .
<https://data.nasa.gov/ontologies/atmonto/data#oagGateDepartureDelay> <http://www.w3.org/2000/01/rdf-schema#domain> <https://data.nasa.gov/ontologies/atmonto/data#AirportData> .
<https://data.nasa.gov/ontologies/atmonto/data#airportArrivalRate> <http://www.w3.org/2000/01/rdf-schema#label> "airport arrival rate" .
_:B805beb7dX2De0a6X2D4d92X2Dbc13X2Dff6a40662f87 <http://www.w3.org/2002/07/owl#onProperty> <https://data.nasa.gov/ontologies/atmonto/data#aspmFlightRules> .
<https://data.nasa.gov/ontologies/atmonto/data#MeteorologicalCondition> <http://www.w3.org/2000/01/rdf-schema#subClassOf> _:B4c7117e3X2Df7ceX2D41b2X2D9a3eX2Deb7cb89d18ff .
<https://data.nasa.gov/ontologies/atmonto/data#lowVisibilityWITIdaily> <http://www.w3.org/2000/01/rdf-schema#range> <http://www.w3.org/2001/XMLSchema#float> .
<https://data.nasa.gov/ontologies/atmonto/data#baseAltitude> <http://www.w3.org/2000/01/rdf-schema#range> <http://www.w3.org/2001/XMLSchema#integer> .
<https://data.nasa.gov/ontologies/atmonto/data#lowVisibilityWITIhourly> <http://www.w3.org/2000/01/rdf-schema#label> "low visibility WITI hourly" .
<https://data.nasa.gov/ontologies/atmonto/data#hasASPMmetCondition> <http://www.w3.org/2000/01/rdf-schema#comment> "Links meteorological information to the collection of temporally-dependent data associated with an airport." .
<https://data.nasa.gov/ontologies/atmonto/data#scheduledArrivals> <http://www.w3.org/2000/01/rdf-schema#domain> <https://data.nasa.gov/ontologies/atmonto/data#AirportData> .
<https://data.nasa.gov/ontologies/atmonto/data#tafReportType> <http://www.w3.org/2000/01/rdf-schema#domain> <https://data.nasa.gov/ontologies/atmonto/data#TAFreport> .
<https://data.nasa.gov/ontologies/atmonto/data#lowCeilingWITIhourly> <http://www.w3.org/2000/01/rdf-schema#domain> <https://data.nasa.gov/ontologies/atmonto/data#AirportData> .
<https://data.nasa.gov/ontologies/atmonto/data#hourlyPrecipitation> <http://www.w3.org/2000/01/rdf-schema#range> <http://www.w3.org/2001/XMLSchema#float> .
<https://data.nasa.gov/ontologies/atmonto/data#TAFreport> <http://www.w3.org/2000/01/rdf-schema#subClassOf> _:Bd270744aX2D8b58X2D4e82X2D84aeX2Dbec1f8e37e13 .
<https://data.nasa.gov/ontologies/atmonto/data#weatherQualifier> <http://www.w3.org/2000/01/rdf-schema#comment> "An additional qualifier describing the reported weather phenomenon: shallow, partial, patchy, low drifting, blowing, shower, thunderstorm, freezing." .
_:B99eb8123X2D4b4cX2D4ea1X2Da30cX2D98f3275b841f <http://www.w3.org/2002/07/owl#maxCardinality> "1"^^<http://www.w3.org/2001/XMLSchema#nonNegativeInteger> .
_:B8914685fX2D58a2X2D466cX2Daf8bX2D76835b10c083 <http://www.w3.org/2002/07/owl#onProperty> <https://data.nasa.gov/ontologies/atmonto/ATM#flowMeasurementRegion> .
<https://data.nasa.gov/ontologies/atmonto/data#dataIntervalEndTime> <http://www.w3.org/1999/02/22-rdf-syntax-ns#type> <http://www.w3.org/2002/07/owl#DatatypeProperty> .
_:B0c83ab22X2Dd668X2D47a1X2D9e72X2Dc5f247057922 <http://www.w3.org/1999/02/22-rdf-syntax-ns#first> "sand" .
_:B1c6feb5eX2Ded53X2D4a66X2D8040X2D8209c323332e <http://www.w3.org/2002/07/owl#onProperty> <https://data.nasa.gov/ontologies/atmonto/general#hasFirstItem> .
<https://data.nasa.gov/ontologies/atmonto/data#WeatherCondition> <http://www.w3.org/2000/01/rdf-schema#subClassOf> _:Bb855cbbbX2De2e6X2D4090X2D875cX2D7250d013f1b5 .
<https://data.nasa.gov/ontologies/atmonto/data#hasASPMmetCondition> <http://www.w3.org/2000/01/rdf-schema#domain> <https://data.nasa.gov/ontologies/atmonto/data#AirportData> .
_:B9c90bf4aX2D2609X2D4c54X2Db976X2D6348225f7b0f <http://www.w3.org/1999/02/22-rdf-syntax-ns#rest> <http://www.w3.org/1999/02/22-rdf-syntax-ns#nil> .
<https://data.nasa.gov/ontologies/atmonto/data#FixCapacity> <http://www.w3.org/2000/01/rdf-schema#comment> "A subclass of interval-based data representing the maximum controllable number of aircraft flowing through a fix per some interval of time, given weather and other air traffic control constraints." .
<https://data.nasa.gov/ontologies/atmonto/data#weatherProximity> <http://www.w3.org/2000/01/rdf-schema#domain> <https://data.nasa.gov/ontologies/atmonto/data#WeatherCondition> .
<https://data.nasa.gov/ontologies/atmonto/data#AirportData> <http://www.w3.org/2000/01/rdf-schema#subClassOf> _:B805beb7dX2De0a6X2D4d92X2Dbc13X2Dff6a40662f87 .
<https://data.nasa.gov/ontologies/atmonto/data#METARreportingStation> <http://www.w3.org/2000/01/rdf-schema#label> "METARreporting station" .
<https://data.nasa.gov/ontologies/atmonto/data#WITIproperty> <http://www.w3.org/2000/01/rdf-schema#comment> "A class of different properties relating to WITI (Weather-Impacted Traffic Index)" .
<https://data.nasa.gov/ontologies/atmonto/data#highWindWITIdaily> <http://www.w3.org/2000/01/rdf-schema#domain> <https://data.nasa.gov/ontologies/atmonto/data#AirportData> .
_:B3720f7beX2Dc05dX2D4ad7X2D9f53X2D0bf28577eadf <http://www.w3.org/1999/02/22-rdf-syntax-ns#first> "snow grains" .
_:B72137fc5X2D81ccX2D4df0X2D8a6fX2D197abe2a15e1 <http://www.w3.org/1999/02/22-rdf-syntax-ns#rest> _:Bc5ce5750X2Dcef0X2D4485X2Da53cX2D15c509fcbb76 .
<https://data.nasa.gov/ontologies/atmonto/data#surfaceTemperature> <http://www.w3.org/2000/01/rdf-schema#range> <http://www.w3.org/2001/XMLSchema#float> .
<https://data.nasa.gov/ontologies/atmonto/data#ceiling> <http://www.w3.org/2000/01/rdf-schema#label> "ceiling" .
_:B161b837fX2D3e40X2D4812X2Da32eX2D985cebe5c814 <http://www.w3.org/2002/07/owl#oneOf> _:B85efb7d4X2D33b4X2D42f9X2D9c19X2Dbb7c072ea364 .
<https://data.nasa.gov/ontologies/atmonto/data#scheduledDepartures> <http://www.w3.org/2000/01/rdf-schema#range> <http://www.w3.org/2001/XMLSchema#integer> .
_:B049b6b81X2Dfb65X2D461cX2Da676X2D8c02cc81e607 <http://www.w3.org/1999/02/22-rdf-syntax-ns#type> <http://www.w3.org/2002/07/owl#Restriction> .
<https://data.nasa.gov/ontologies/atmonto/data#dataIntervalStartDay> <http://www.w3.org/2000/01/rdf-schema#comment> "Links temporally-dependent data to the starting day of its period of validity." .
_:B85efb7d4X2D33b4X2D42f9X2D9c19X2Dbb7c072ea364 <http://www.w3.org/1999/02/22-rdf-syntax-ns#first> "open" .
<https://data.nasa.gov/ontologies/atmonto/data#weatherProximity> <http://www.w3.org/1999/02/22-rdf-syntax-ns#type> <http://www.w3.org/2002/07/owl#DatatypeProperty> .
<https://data.nasa.gov/ontologies/atmonto/data#metarReportModifier> <http://www.w3.org/1999/02/22-rdf-syntax-ns#type> <http://www.w3.org/2002/07/owl#FunctionalProperty> .
_:B72bab791X2D0b7cX2D4affX2Dafe5X2Dfdcf7d4a9f3c <http://www.w3.org/1999/02/22-rdf-syntax-ns#rest> _:B3e86c2f0X2Dd810X2D42a7X2D9fceX2D5d86be533d87 .
<https://data.nasa.gov/ontologies/atmonto/data#hasSkyCondition> <http://www.w3.org/2000/01/rdf-schema#range> <https://data.nasa.gov/ontologies/atmonto/data#SkyCondition> .
_:B2b069507X2Dcd7aX2D4102X2DaedbX2Dc5cf54058891 <http://www.w3.org/1999/02/22-rdf-syntax-ns#first> "small hail and/or snow pellets" .
_:Bf568bd21X2Df8efX2D464fX2D83abX2D64c80580b5a6 <http://www.w3.org/1999/02/22-rdf-syntax-ns#rest> _:B964063e1X2D598aX2D4833X2Da717X2D006b0ad56c4f .
<https://data.nasa.gov/ontologies/atmonto/data#hasMETARreport> <http://www.w3.org/2000/01/rdf-schema#range> <https://data.nasa.gov/ontologies/atmonto/data#METARreport> .
<https://data.nasa.gov/ontologies/atmonto/data#WeatherCondition> <http://www.w3.org/2000/01/rdf-schema#subClassOf> _:B99eb8123X2D4b4cX2D4ea1X2Da30cX2D98f3275b841f .
<https://data.nasa.gov/ontologies/atmonto/data#hasWeatherCondition> <http://www.w3.org/2000/01/rdf-schema#label> "has weather condition" .
_:B4463fd56X2D8ffbX2D4550X2D8bc2X2Dbae635adbf25 <http://www.w3.org/1999/02/22-rdf-syntax-ns#first> "drizzle" .
<https://data.nasa.gov/ontologies/atmonto/data#edctArrivalHold> <http://www.w3.org/1999/02/22-rdf-syntax-ns#type> <http://www.w3.org/2002/07/owl#DatatypeProperty> .
_:B3e86c2f0X2Dd810X2D42a7X2D9fceX2D5d86be533d87 <http://www.w3.org/1999/02/22-rdf-syntax-ns#first> "spray" .
_:B0fea9690X2Da2d4X2D4976X2Daa0cX2D1f5129c61150 <http://www.w3.org/2002/07/owl#onProperty> <https://data.nasa.gov/ontologies/atmonto/data#surfaceWindDirectionStatus> .
<https://data.nasa.gov/ontologies/atmonto/data#dewpoint> <http://www.w3.org/2000/01/rdf-schema#comment> "The dewpoint recorded as part of a meteorological condition report." .
_:Bdb55bab6X2Db468X2D44cfX2Da5b8X2D694e6526dfe0 <http://www.w3.org/1999/02/22-rdf-syntax-ns#first> "clear" .
_:Bf3a1516bX2D1813X2D48e1X2DaaabX2D215f13285700 <http://www.w3.org/1999/02/22-rdf-syntax-ns#first> "altocumulus castellanus" .
<https://data.nasa.gov/ontologies/atmonto/data#weatherProximity> <http://www.w3.org/2000/01/rdf-schema#comment> "Describes the location of the weather phenomena in relation to the reporting station: immediate proximity or in vicinity." .
<https://data.nasa.gov/ontologies/atmonto/data#runwayStatus> <http://www.w3.org/2000/01/rdf-schema#domain> <https://data.nasa.gov/ontologies/atmonto/data#RunwayStatusData> .
<https://data.nasa.gov/ontologies/atmonto/data#rapidityOfWeatherChange> <http://www.w3.org/2000/01/rdf-schema#range> <http://www.w3.org/2001/XMLSchema#string> .
<https://data.nasa.gov/ontologies/atmonto/data#lowVisibilityWITIhourly> <http://www.w3.org/1999/02/22-rdf-syntax-ns#type> <https://data.nasa.gov/ontologies/atmonto/data#WITIproperty> .
_:Bf20a1683X2D7158X2D4ef2X2Da159X2D2674318ddcfd <http://www.w3.org/2002/07/owl#onProperty> <https://data.nasa.gov/ontologies/atmonto/data#metarReportModifier> .
_:Bebd0d737X2D5b76X2D489dX2D8cb9X2D2aad44a9506d <http://www.w3.org/1999/02/22-rdf-syntax-ns#type> <http://www.w3.org/2002/07/owl#Restriction> .
<https://data.nasa.gov/ontologies/atmonto/data#meteorologicalConditionStatus> <http://www.w3.org/2000/01/rdf-schema#comment> "An indicator of whether the meteorological condition is based on actual observations (observed) or on future projections (forecast)." .
<https://data.nasa.gov/ontologies/atmonto/data#unlimitedVisibility> <http://www.w3.org/2000/01/rdf-schema#domain> <https://data.nasa.gov/ontologies/atmonto/data#VisibilityCondition> .
_:B1eed5083X2D3b8dX2D4c08X2Dadf1X2D1eea74c97d5c <http://www.w3.org/1999/02/22-rdf-syntax-ns#type> <http://www.w3.org/2002/07/owl#Restriction> .
<https://data.nasa.gov/ontologies/atmonto/data#AirportData> <http://www.w3.org/2000/01/rdf-schema#label> "Airport Data" .
<https://data.nasa.gov/ontologies/atmonto/data#limitedVisibilityDistance> <http://www.w3.org/1999/02/22-rdf-syntax-ns#type> <http://www.w3.org/2002/07/owl#DatatypeProperty> .
<https://data.nasa.gov/ontologies/atmonto/data#weatherQualifier> <http://www.w3.org/2000/01/rdf-schema#range> <http://www.w3.org/2001/XMLSchema#string> .
_:Bf20a1683X2D7158X2D4ef2X2Da159X2D2674318ddcfd <http://www.w3.org/1999/02/22-rdf-syntax-ns#type> <http://www.w3.org/2002/07/owl#Restriction> .
_:Bc0b04394X2D0f2aX2D495aX2Db48aX2D3909da332a75 <http://www.w3.org/1999/02/22-rdf-syntax-ns#rest> _:B5f8fce50X2Dc5d8X2D48daX2Db7c6X2D7c1b6f6af3c4 .
<https://data.nasa.gov/ontologies/atmonto/data#arrivalDemand> <http://www.w3.org/2000/01/rdf-schema#range> <http://www.w3.org/2001/XMLSchema#integer> .
<https://data.nasa.gov/ontologies/atmonto/data#dataIntervalStartTime> <http://www.w3.org/1999/02/22-rdf-syntax-ns#type> <http://www.w3.org/2002/07/owl#DatatypeProperty> .
<https://data.nasa.gov/ontologies/atmonto/data#hasAirportData> <http://www.w3.org/2000/01/rdf-schema#range> <https://data.nasa.gov/ontologies/atmonto/data#AirportData> .
_:Bc5ce5750X2Dcef0X2D4485X2Da53cX2D15c509fcbb76 <http://www.w3.org/1999/02/22-rdf-syntax-ns#first> "snow" .
<https://data.nasa.gov/ontologies/atmonto/data#departureDemand> <http://www.w3.org/1999/02/22-rdf-syntax-ns#type> <http://www.w3.org/2002/07/owl#FunctionalProperty> .
_:B85efb7d4X2D33b4X2D42f9X2D9c19X2Dbb7c072ea364 <http://www.w3.org/1999/02/22-rdf-syntax-ns#rest> _:B25e3a789X2Da464X2D4768X2Db69fX2D2b31e7ea7980 .
_:Bb2447386X2D2e28X2D4c69X2Dba49X2De5dfe47e13ba <http://www.w3.org/2002/07/owl#cardinality> "1"^^<http://www.w3.org/2001/XMLSchema#nonNegativeInteger> .
<https://data.nasa.gov/ontologies/atmonto/data#windDirectionLower> <http://www.w3.org/1999/02/22-rdf-syntax-ns#type> <http://www.w3.org/2002/07/owl#DatatypeProperty> .
_:B1c6feb5eX2Ded53X2D4a66X2D8040X2D8209c323332e <http://www.w3.org/1999/02/22-rdf-syntax-ns#type> <http://www.w3.org/2002/07/owl#Restriction> .
_:Bf3a1516bX2D1813X2D48e1X2DaaabX2D215f13285700 <http://www.w3.org/1999/02/22-rdf-syntax-ns#rest> <http://www.w3.org/1999/02/22-rdf-syntax-ns#nil> .
_:B31730194X2Da2aeX2D4755X2D9b1eX2D53849b794653 <http://www.w3.org/1999/02/22-rdf-syntax-ns#first> "transient" .
<https://data.nasa.gov/ontologies/atmonto/data#metarReportType> <http://www.w3.org/1999/02/22-rdf-syntax-ns#type> <http://www.w3.org/2002/07/owl#FunctionalProperty> .
<https://data.nasa.gov/ontologies/atmonto/data#lowVisibilityWITIdaily> <http://www.w3.org/2000/01/rdf-schema#label> "low visibility WITI daily" .
<https://data.nasa.gov/ontologies/atmonto/data#SectorCapacity> <http://www.w3.org/2000/01/rdf-schema#subClassOf> <https://data.nasa.gov/ontologies/atmonto/ATM#AircraftCapacity> .
_:B14b9247fX2D1e6fX2D4a13X2Da9a1X2D0429fef1984c <http://www.w3.org/1999/02/22-rdf-syntax-ns#first> "hail" .
<https://data.nasa.gov/ontologies/atmonto/data#metConditionProbability> <http://www.w3.org/1999/02/22-rdf-syntax-ns#type> <http://www.w3.org/2002/07/owl#DatatypeProperty> .
_:B41ecb1f3X2D60e9X2D435eX2Dad0eX2D1d88e2ff9118 <http://www.w3.org/1999/02/22-rdf-syntax-ns#rest> <http://www.w3.org/1999/02/22-rdf-syntax-ns#nil> .
<https://data.nasa.gov/ontologies/atmonto/data#TAFreport> <http://www.w3.org/2000/01/rdf-schema#comment> "Meteorological conditions provided in a periodic TAF forecast. Includes sky, wind, visibility and weather components." .
_:Bcffad628X2Dfcf7X2D4d00X2Dbaa1X2De1d98d14a19d <http://www.w3.org/1999/02/22-rdf-syntax-ns#rest> _:Bc6eac04aX2D276dX2D4b24X2Dbb5fX2Ddaf57af65002 .
_:B1bfa9b51X2Dccd1X2D46e9X2Db402X2D287ac5521893 <http://www.w3.org/1999/02/22-rdf-syntax-ns#first> "widespread dust" .
<https://data.nasa.gov/ontologies/atmonto/data#lowVisibilityWITIdaily> <http://www.w3.org/1999/02/22-rdf-syntax-ns#type> <https://data.nasa.gov/ontologies/atmonto/data#WITIproperty> .
<https://data.nasa.gov/ontologies/atmonto/data#departureDemand> <http://www.w3.org/2000/01/rdf-schema#comment> "The number of aircraft intending to depart during the specified time period." .
<https://data.nasa.gov/ontologies/atmonto/data#dewpoint> <http://www.w3.org/2000/01/rdf-schema#range> <http://www.w3.org/2001/XMLSchema#float> .
<https://data.nasa.gov/ontologies/atmonto/data#hasASPMmetCondition> <http://www.w3.org/2000/01/rdf-schema#range> <https://data.nasa.gov/ontologies/atmonto/data#ASPMmeteorologicalCondition> .
<https://data.nasa.gov/ontologies/atmonto/data#SectorFlow> <http://www.w3.org/1999/02/22-rdf-syntax-ns#type> <http://www.w3.org/2002/07/owl#Class> .
_:Bed0be29bX2D57deX2D4f76X2Db3c4X2Dc697a028d67d <http://www.w3.org/1999/02/22-rdf-syntax-ns#type> <http://www.w3.org/2002/07/owl#Restriction> .
<https://data.nasa.gov/ontologies/atmonto/data#SectorCapacity> <http://www.w3.org/2000/01/rdf-schema#label> "Sector capacity" .
<https://data.nasa.gov/ontologies/atmonto/data#airportDepartureRate> <http://www.w3.org/2000/01/rdf-schema#range> <http://www.w3.org/2001/XMLSchema#integer> .
<https://data.nasa.gov/ontologies/atmonto/data#TAFmeteorologicalCondition> <http://www.w3.org/2000/01/rdf-schema#subClassOf> _:B035d8c87X2D8e8bX2D4c64X2D80c1X2Dc15f119e4b26 .
<https://data.nasa.gov/ontologies/atmonto/data#tafReportString> <http://www.w3.org/1999/02/22-rdf-syntax-ns#type> <http://www.w3.org/2002/07/owl#DatatypeProperty> .
<https://data.nasa.gov/ontologies/atmonto/data#dataIntervalStartTime> <http://www.w3.org/2000/01/rdf-schema#range> <http://www.w3.org/2001/XMLSchema#dateTime> .
<https://data.nasa.gov/ontologies/atmonto/data#dataIntervalEndDay> <http://www.w3.org/2000/01/rdf-schema#comment> "Links temporally-dependent data to the ending day of its period of validity." .
<https://data.nasa.gov/ontologies/atmonto/data#metarReportModifier> <http://www.w3.org/2000/01/rdf-schema#label> "metar report modifier" .
<https://data.nasa.gov/ontologies/atmonto/data#unlimitedVisibility> <http://www.w3.org/2000/01/rdf-schema#label> "unlimited visibility" .
<https://data.nasa.gov/ontologies/atmonto/data#AirportData> <http://www.w3.org/2000/01/rdf-schema#subClassOf> _:Bed0be29bX2D57deX2D4f76X2Db3c4X2Dc697a028d67d .
<https://data.nasa.gov/ontologies/atmonto/data#ceiling> <http://www.w3.org/2000/01/rdf-schema#comment> "The vertical visibility (in feet) measured from the ground to the lowest cloud layer reported as broken or overcast." .
_:Bcffad628X2Dfcf7X2D4d00X2Dbaa1X2De1d98d14a19d <http://www.w3.org/1999/02/22-rdf-syntax-ns#first> "moderate" .
_:B049b6b81X2Dfb65X2D461cX2Da676X2D8c02cc81e607 <http://www.w3.org/2002/07/owl#cardinality> "1"^^<http://www.w3.org/2001/XMLSchema#nonNegativeInteger> .
<https://data.nasa.gov/ontologies/atmonto/data#metarReportModifier> <http://www.w3.org/1999/02/22-rdf-syntax-ns#type> <http://www.w3.org/2002/07/owl#DatatypeProperty> .
_:B8ebf7271X2Db1a5X2D4b4aX2Daa9cX2D74891abd525a <http://www.w3.org/1999/02/22-rdf-syntax-ns#rest> _:B2b621779X2D2b0eX2D4b01X2D8daaX2D4ca45b169260 .
<https://data.nasa.gov/ontologies/atmonto/data#hasWeatherCondition> <http://www.w3.org/1999/02/22-rdf-syntax-ns#type> <http://www.w3.org/2002/07/owl#ObjectProperty> .
<https://data.nasa.gov/ontologies/atmonto/data#edctArrivalHold> <http://www.w3.org/1999/02/22-rdf-syntax-ns#type> <http://www.w3.org/2002/07/owl#FunctionalProperty> .
_:B035d8c87X2D8e8bX2D4c64X2D80c1X2Dc15f119e4b26 <http://www.w3.org/2002/07/owl#onProperty> <https://data.nasa.gov/ontologies/atmonto/data#rapidityOfWeatherChange> .
_:B7b5530c5X2D489cX2D4cc0X2Da132X2Dccd6bb298bac <http://www.w3.org/1999/02/22-rdf-syntax-ns#first> "V" .
_:Bebcc5a6dX2D4c71X2D4c01X2Dbb24X2D303e16cf078c <http://www.w3.org/1999/02/22-rdf-syntax-ns#first> "scattered clouds" .
<https://data.nasa.gov/ontologies/atmonto/data#TAFmeteorologicalCondition> <http://www.w3.org/2000/01/rdf-schema#subClassOf> <https://data.nasa.gov/ontologies/atmonto/data#MeteorologicalCondition> .
<https://data.nasa.gov/ontologies/atmonto/data#tafReportString> <http://www.w3.org/2000/01/rdf-schema#label> "taf report string" .
_:B31ecb3a2X2D633bX2D4b66X2D8d6eX2De894ef9060a9 <http://www.w3.org/2002/07/owl#oneOf> _:B32e8d549X2D4b04X2D4ec9X2Daca6X2De401856abf2a .
_:Bc416aebdX2D893bX2D40e2X2Dbbe6X2D9efbb3d57b65 <http://www.w3.org/1999/02/22-rdf-syntax-ns#first> "observed" .
<https://data.nasa.gov/ontologies/atmonto/data#FixFlow> <http://www.w3.org/2000/01/rdf-schema#subClassOf> _:B8914685fX2D58a2X2D466cX2Daf8bX2D76835b10c083 .
<https://data.nasa.gov/ontologies/atmonto/data#edctArrivalHold> <http://www.w3.org/2000/01/rdf-schema#comment> "EDCT (Estimated Departure Clearance Time) hold minutes at other airports arriving this airport." .
<https://data.nasa.gov/ontologies/atmonto/data#IntervalData> <http://www.w3.org/1999/02/22-rdf-syntax-ns#type> <http://www.w3.org/2002/07/owl#Class> .
<https://data.nasa.gov/ontologies/atmonto/data#highWindWITIhourly> <http://www.w3.org/2000/01/rdf-schema#label> "high wind WITI hourly" .
<https://data.nasa.gov/ontologies/atmonto/data#FixFlow> <http://www.w3.org/2000/01/rdf-schema#domain> <https://data.nasa.gov/ontologies/atmonto/data#FixFlow> .
<https://data.nasa.gov/ontologies/atmonto/data#hasAirportData> <http://www.w3.org/2000/01/rdf-schema#domain> <https://data.nasa.gov/ontologies/atmonto/NAS#Airport> .
<https://data.nasa.gov/ontologies/atmonto/data#tafReportType> <http://www.w3.org/2000/01/rdf-schema#range> <http://www.w3.org/2001/XMLSchema#string> .
<https://data.nasa.gov/ontologies/atmonto/data#WeatherCondition> <http://www.w3.org/2000/01/rdf-schema#comment> "The current or forecast weather conditions at a given airport or other reporting station." .
<https://data.nasa.gov/ontologies/atmonto/data#cloudType> <http://www.w3.org/2000/01/rdf-schema#domain> <https://data.nasa.gov/ontologies/atmonto/data#CloudLayer> .
<https://data.nasa.gov/ontologies/atmonto/data> <http://www.w3.org/2002/07/owl#imports> <https://data.nasa.gov/ontologies/atmonto/ATM> .
<https://data.nasa.gov/ontologies/atmonto/data#runwayStatus> <http://www.w3.org/2000/01/rdf-schema#comment> "An indicator of whether the runway is open or closed during the specified period." .
_:Bc9c398a1X2Dd4dcX2D4f15X2D8c3bX2D3e579a6ee161 <http://www.w3.org/2002/07/owl#onProperty> <https://data.nasa.gov/ontologies/atmonto/data#cloudType> .
<https://data.nasa.gov/ontologies/atmonto/data#cloudCover> <http://www.w3.org/2000/01/rdf-schema#comment> "For a given homogenous cloud layer, the type of cloud cover present: clear, few clouds, scattered clouds, broken clouds, overcast, vertical visibility layer." .
<https://data.nasa.gov/ontologies/atmonto/data#airportArrivalRate> <http://www.w3.org/2000/01/rdf-schema#domain> <https://data.nasa.gov/ontologies/atmonto/data#AirportData> .
<https://data.nasa.gov/ontologies/atmonto/data#associatedMETARreportingStation> <http://www.w3.org/2000/01/rdf-schema#range> <https://data.nasa.gov/ontologies/atmonto/data#METARreportingStation> .
<https://data.nasa.gov/ontologies/atmonto/data#topAltitude> <http://www.w3.org/2000/01/rdf-schema#domain> <https://data.nasa.gov/ontologies/atmonto/data#CloudLayer> .
<https://data.nasa.gov/ontologies/atmonto/data#forecastingAirport> <http://www.w3.org/1999/02/22-rdf-syntax-ns#type> <http://www.w3.org/2002/07/owl#ObjectProperty> .
<https://data.nasa.gov/ontologies/atmonto/data#rapidityOfWeatherChange> <http://www.w3.org/2000/01/rdf-schema#domain> <https://data.nasa.gov/ontologies/atmonto/data#TAFmeteorologicalCondition> .
<https://data.nasa.gov/ontologies/atmonto/data#hasASPMmetCondition> <http://www.w3.org/2000/01/rdf-schema#label> "has ASPMmet condition" .
<https://data.nasa.gov/ontologies/atmonto/data#FixCapacity> <http://www.w3.org/1999/02/22-rdf-syntax-ns#type> <http://www.w3.org/2002/07/owl#Class> .
_:Bb855cbbbX2De2e6X2D4090X2D875cX2D7250d013f1b5 <http://www.w3.org/2002/07/owl#onProperty> <https://data.nasa.gov/ontologies/atmonto/data#weatherPhenomenon> .
<https://data.nasa.gov/ontologies/atmonto/data#weatherPhenomenon> <http://www.w3.org/2000/01/rdf-schema#range> <http://www.w3.org/2001/XMLSchema#string> .
_:B32e8d549X2D4b04X2D4ec9X2Daca6X2De401856abf2a <http://www.w3.org/1999/02/22-rdf-syntax-ns#rest> _:B46fafbb9X2D8a44X2D44f2X2Da251X2D9afc5da3912e .
_:B964063e1X2D598aX2D4833X2Da717X2D006b0ad56c4f <http://www.w3.org/1999/02/22-rdf-syntax-ns#rest> _:B0969422aX2D6d5dX2D4265X2D83a8X2D066412c1e4df .
<https://data.nasa.gov/ontologies/atmonto/data#WeatherCondition> <http://www.w3.org/2000/01/rdf-schema#subClassOf> _:Bc93945cdX2Dbbb5X2D4eacX2Da84cX2D697ea4b10cb0 .
<https://data.nasa.gov/ontologies/atmonto/data#surfaceGustSpeed> <http://www.w3.org/1999/02/22-rdf-syntax-ns#type> <http://www.w3.org/2002/07/owl#DatatypeProperty> .
_:B70dd1fefX2D2850X2D4663X2Db3f0X2Da291ae44a230 <http://www.w3.org/1999/02/22-rdf-syntax-ns#first> "duststorm" .
<https://data.nasa.gov/ontologies/atmonto/data#lowVisibilityWITIhourly> <http://www.w3.org/2000/01/rdf-schema#range> <http://www.w3.org/2001/XMLSchema#float> .
<https://data.nasa.gov/ontologies/atmonto/data#weatherPhenomenon> <http://www.w3.org/2000/01/rdf-schema#label> "weather phenomenon" .
_:B8f07340fX2D4b3fX2D42f7X2Da7a2X2Da835853aa3d2 <http://www.w3.org/1999/02/22-rdf-syntax-ns#first> "COR" .
_:B909dd746X2D45deX2D42daX2D9cc2X2D69a07074a11a <http://www.w3.org/1999/02/22-rdf-syntax-ns#type> <http://www.w3.org/2000/01/rdf-schema#Datatype> .
_:B1eed5083X2D3b8dX2D4c08X2Dadf1X2D1eea74c97d5c <http://www.w3.org/2002/07/owl#cardinality> "1"^^<http://www.w3.org/2001/XMLSchema#nonNegativeInteger> .
<https://data.nasa.gov/ontologies/atmonto/data#highWindWITIdaily> <http://www.w3.org/2000/01/rdf-schema#comment> "The high wind weather impacted traffic index (WITI) computed for the airport during the specified timeframe (daily). WITI is an estimate of the number of flights potentially impacted due to inclement weather based on the scheduled traffic demand for a defined geographic region of the air traffic system (in this case, an airport). If the winds at the airport are above a set threshold, then the high wind WITI is set to the number of scheduled arrivals for that timeframe." .
<https://data.nasa.gov/ontologies/atmonto/data#highWindWITIhourly> <http://www.w3.org/1999/02/22-rdf-syntax-ns#type> <http://www.w3.org/2002/07/owl#FunctionalProperty> .
_:Bd6384cdeX2Dd08aX2D4cf2X2D882fX2Dd0745776d655 <http://www.w3.org/2002/07/owl#allValuesFrom> _:B161b837fX2D3e40X2D4812X2Da32eX2D985cebe5c814 .
_:B1af074b8X2D5962X2D4fcbX2Daca3X2Da844f3426735 <http://www.w3.org/2002/07/owl#allValuesFrom> _:Bfa09714cX2DdcfbX2D4b9eX2D9927X2Dad5d6499080b .
_:Bc5ce5750X2Dcef0X2D4485X2Da53cX2D15c509fcbb76 <http://www.w3.org/1999/02/22-rdf-syntax-ns#rest> _:B3720f7beX2Dc05dX2D4ad7X2D9f53X2D0bf28577eadf .
<https://data.nasa.gov/ontologies/atmonto/data#surfaceWindSpeed> <http://www.w3.org/2000/01/rdf-schema#comment> "The speed in knots of the surface wind." .
<https://data.nasa.gov/ontologies/atmonto/data#runwayVisibleRange> <http://www.w3.org/2000/01/rdf-schema#domain> <https://data.nasa.gov/ontologies/atmonto/data#VisibilityCondition> .
<https://data.nasa.gov/ontologies/atmonto/data#RunwayStatusData> <http://www.w3.org/2000/01/rdf-schema#subClassOf> _:Bd6384cdeX2Dd08aX2D4cf2X2D882fX2Dd0745776d655 .
<https://data.nasa.gov/ontologies/atmonto/data#hourlyPrecipitation> <http://www.w3.org/2000/01/rdf-schema#label> "hourly precipitation" .
<https://data.nasa.gov/ontologies/atmonto/data#metConditionProbability> <http://www.w3.org/2000/01/rdf-schema#domain> <https://data.nasa.gov/ontologies/atmonto/data#MeteorologicalCondition> .
<https://data.nasa.gov/ontologies/atmonto/data#hasVisibilityCondition> <http://www.w3.org/1999/02/22-rdf-syntax-ns#type> <http://www.w3.org/2002/07/owl#ObjectProperty> .
_:Bf9bf06dbX2D3d8bX2D49ddX2Da012X2Dc9846897439f <http://www.w3.org/1999/02/22-rdf-syntax-ns#first> "volcanic ash" .
_:Bbf6eefb7X2D4f53X2D441dX2D97a5X2D04b495a23c9c <http://www.w3.org/1999/02/22-rdf-syntax-ns#first> "tornado/waterspout" .
_:B70d3bda9X2D6639X2D4f0eX2D8d65X2D7c412969f5f8 <http://www.w3.org/2002/07/owl#allValuesFrom> _:B909dd746X2D45deX2D42daX2D9cc2X2D69a07074a11a .
<https://data.nasa.gov/ontologies/atmonto/data#lowCeilingWITIdaily> <http://www.w3.org/2000/01/rdf-schema#comment> "The low ceiling weather impacted traffic index (WITI) computed for the airport during the specified timeframe (daily). WITI is an estimate of the number of flights potentially impacted due to inclement weather based on the scheduled traffic demand for a defined geographic region of the air traffic system (in this case, an airport). If the ceiling at the airport is below a set threshold, then the low ceiling WITI is set to the number of scheduled arrivals for that timeframe." .
_:B0969422aX2D6d5dX2D4265X2D83a8X2D066412c1e4df <http://www.w3.org/1999/02/22-rdf-syntax-ns#first> "corrected" .
<https://data.nasa.gov/ontologies/atmonto/data#WeatherCondition> <http://www.w3.org/2000/01/rdf-schema#subClassOf> _:B70d3bda9X2D6639X2D4f0eX2D8d65X2D7c412969f5f8 .
<https://data.nasa.gov/ontologies/atmonto/data#totalAirborneDelay> <http://www.w3.org/2000/01/rdf-schema#comment> "Total airborne flight delay in minutes for this airport during the specified period." .
<https://data.nasa.gov/ontologies/atmonto/data#topAltitude> <http://www.w3.org/1999/02/22-rdf-syntax-ns#type> <http://www.w3.org/2002/07/owl#DatatypeProperty> .
<https://data.nasa.gov/ontologies/atmonto/data#windDirectionFixed> <http://www.w3.org/1999/02/22-rdf-syntax-ns#type> <http://www.w3.org/2002/07/owl#DatatypeProperty> .
<https://data.nasa.gov/ontologies/atmonto/data#hasVisibilityCondition> <http://www.w3.org/2000/01/rdf-schema#comment> "Associates a meteorological condition with the details of the surface visibility conditions at the reporting location.." .
<https://data.nasa.gov/ontologies/atmonto/data#seaLevelPressure> <http://www.w3.org/2000/01/rdf-schema#label> "sea level pressure" .
_:B161b837fX2D3e40X2D4812X2Da32eX2D985cebe5c814 <http://www.w3.org/1999/02/22-rdf-syntax-ns#type> <http://www.w3.org/2000/01/rdf-schema#Datatype> .
<https://data.nasa.gov/ontologies/atmonto/data#runwaySurfaceFriction> <http://www.w3.org/1999/02/22-rdf-syntax-ns#type> <http://www.w3.org/2002/07/owl#FunctionalProperty> .
<https://data.nasa.gov/ontologies/atmonto/data#highWindWITIdaily> <http://www.w3.org/2000/01/rdf-schema#label> "high wind WITI daily" .
<https://data.nasa.gov/ontologies/atmonto/data#windDirectionUpper> <http://www.w3.org/1999/02/22-rdf-syntax-ns#type> <http://www.w3.org/2002/07/owl#DatatypeProperty> .
_:B8f07340fX2D4b3fX2D42f7X2Da7a2X2Da835853aa3d2 <http://www.w3.org/1999/02/22-rdf-syntax-ns#rest> <http://www.w3.org/1999/02/22-rdf-syntax-ns#nil> .
<https://data.nasa.gov/ontologies/atmonto/data#METARreport> <http://www.w3.org/2000/01/rdf-schema#comment> "Meteorological conditions provided in a periodic METAR report. Includes sky, wind, visibility and weather components." .
<https://data.nasa.gov/ontologies/atmonto/data#lowVisibilityWITIhourly> <http://www.w3.org/2000/01/rdf-schema#domain> <https://data.nasa.gov/ontologies/atmonto/data#AirportData> .
_:Bc9c398a1X2Dd4dcX2D4f15X2D8c3bX2D3e579a6ee161 <http://www.w3.org/2002/07/owl#maxCardinality> "1"^^<http://www.w3.org/2001/XMLSchema#nonNegativeInteger> .
<https://data.nasa.gov/ontologies/atmonto/data#hasMETARreport> <http://www.w3.org/2000/01/rdf-schema#domain> <https://data.nasa.gov/ontologies/atmonto/data#METARreportingStation> .
<https://data.nasa.gov/ontologies/atmonto/data#aspmFlightRules> <http://www.w3.org/2000/01/rdf-schema#range> <http://www.w3.org/2001/XMLSchema#string> .
<https://data.nasa.gov/ontologies/atmonto/data#airportDepartureRate> <http://www.w3.org/2000/01/rdf-schema#domain> <https://data.nasa.gov/ontologies/atmonto/data#AirportData> .
_:Be07d6f98X2D2f29X2D4301X2Db3a4X2D6815000d445d <http://www.w3.org/2002/07/owl#allValuesFrom> <https://data.nasa.gov/ontologies/atmonto/ATM#NavigationFix> .
<https://data.nasa.gov/ontologies/atmonto/NAS#RunwayVisibleRangeMeasurement> <http://www.w3.org/2000/01/rdf-schema#subClassOf> <https://data.nasa.gov/ontologies/atmonto/data#IntervalData> .
<https://data.nasa.gov/ontologies/atmonto/ATM#AircraftFlowCapacity> <http://www.w3.org/2000/01/rdf-schema#subClassOf> <https://data.nasa.gov/ontologies/atmonto/data#IntervalData> .
<https://data.nasa.gov/ontologies/atmonto/data#forecastingAirport> <http://www.w3.org/2000/01/rdf-schema#range> <https://data.nasa.gov/ontologies/atmonto/NAS#Airport> .
_:Bebcc5a6dX2D4c71X2D4c01X2Dbb24X2D303e16cf078c <http://www.w3.org/1999/02/22-rdf-syntax-ns#rest> _:Bd2d0bf49X2D78c9X2D45fdX2D868bX2D977560253335 .
<https://data.nasa.gov/ontologies/atmonto/data#VisibilityCondition> <http://www.w3.org/1999/02/22-rdf-syntax-ns#type> <http://www.w3.org/2002/07/owl#Class> .
<https://data.nasa.gov/ontologies/atmonto/data#oagArrivalDelay> <http://www.w3.org/2000/01/rdf-schema#comment> "Minutes of OAG (Official Airline Guide) based arrival delay in excess of 15 minutes." .
_:Bd4a3a582X2D9a9fX2D415aX2D9694X2Dc01bdb73db07 <http://www.w3.org/1999/02/22-rdf-syntax-ns#rest> _:B69d15ecaX2D4fa3X2D45edX2Da7d1X2D16ba12529690 .
<https://data.nasa.gov/ontologies/atmonto/data#hourlyPrecipitation> <http://www.w3.org/2000/01/rdf-schema#comment> "Recorded hourly precipitation rate at the measurement station in inches." .
_:Bfa09714cX2DdcfbX2D4b9eX2D9927X2Dad5d6499080b <http://www.w3.org/1999/02/22-rdf-syntax-ns#type> <http://www.w3.org/2000/01/rdf-schema#Datatype> .
<https://data.nasa.gov/ontologies/atmonto/data#windShearHeight> <http://www.w3.org/2000/01/rdf-schema#domain> <https://data.nasa.gov/ontologies/atmonto/data#SurfaceWindCondition> .
<https://data.nasa.gov/ontologies/atmonto/data#hasSkyCondition> <http://www.w3.org/2000/01/rdf-schema#comment> "Associates a meteorological condition with the details of the sky and cloud conditions at the reporting location.." .
_:Bcfbdc0bdX2Daa20X2D44ffX2D9949X2De9daeac6a1bf <http://www.w3.org/1999/02/22-rdf-syntax-ns#rest> <http://www.w3.org/1999/02/22-rdf-syntax-ns#nil> .
<https://data.nasa.gov/ontologies/atmonto/data#tafReportType> <http://www.w3.org/2000/01/rdf-schema#label> "taf report type" .
_:Bf568bd21X2Df8efX2D464fX2D83abX2D64c80580b5a6 <http://www.w3.org/1999/02/22-rdf-syntax-ns#first> "routine" .
<https://data.nasa.gov/ontologies/atmonto/data#runwayStatus> <http://www.w3.org/2000/01/rdf-schema#range> <http://www.w3.org/2001/XMLSchema#string> .
_:B7c0bd641X2Dd3c5X2D4dfbX2Db8faX2D67cf310a0048 <http://www.w3.org/1999/02/22-rdf-syntax-ns#rest> _:B4e280221X2Db9eaX2D4d95X2Db31cX2D56635ce48129 .
<https://data.nasa.gov/ontologies/atmonto/data#IntervalData> <http://www.w3.org/2000/01/rdf-schema#comment> "State data that has a temporal lifetime: a start and end time." .
<https://data.nasa.gov/ontologies/atmonto/data#TAFmeteorologicalCondition> <http://www.w3.org/2000/01/rdf-schema#subClassOf> <https://data.nasa.gov/ontologies/atmonto/general#SequencedItem> .
<https://data.nasa.gov/ontologies/atmonto/data#arrivalDemand> <http://www.w3.org/2000/01/rdf-schema#domain> <https://data.nasa.gov/ontologies/atmonto/data#AirportData> .
_:B9381954aX2Dcd8eX2D4902X2DbddbX2D1acd0d5d9150 <http://www.w3.org/1999/02/22-rdf-syntax-ns#type> <http://www.w3.org/2002/07/owl#Restriction> .
<https://data.nasa.gov/ontologies/atmonto/data#runwayReportedOn> <http://www.w3.org/2000/01/rdf-schema#range> <https://data.nasa.gov/ontologies/atmonto/NAS#PhysicalRunway> .
<https://data.nasa.gov/ontologies/atmonto/data#windDirectionFixed> <http://www.w3.org/2000/01/rdf-schema#label> "fixed wind direction" .
_:B5ba85c47X2D6e17X2D4e4bX2Dba3eX2D2d76ff83a78e <http://www.w3.org/1999/02/22-rdf-syntax-ns#rest> _:B70dd1fefX2D2850X2D4663X2Db3f0X2Da291ae44a230 .
<https://data.nasa.gov/ontologies/atmonto/data#runwayReportedOn> <http://www.w3.org/2000/01/rdf-schema#comment> "Associates a runway status report with the physical runway being measured." .
<https://data.nasa.gov/ontologies/atmonto/data#METARreport> <http://www.w3.org/2000/01/rdf-schema#subClassOf> <https://data.nasa.gov/ontologies/atmonto/data#MeteorologicalCondition> .
<https://data.nasa.gov/ontologies/atmonto/data#cloudType> <http://www.w3.org/1999/02/22-rdf-syntax-ns#type> <http://www.w3.org/2002/07/owl#DatatypeProperty> .
<https://data.nasa.gov/ontologies/atmonto/data#etmsDepartures> <http://www.w3.org/1999/02/22-rdf-syntax-ns#type> <http://www.w3.org/2002/07/owl#FunctionalProperty> .
<https://data.nasa.gov/ontologies/atmonto/data#highWindWITIdaily> <http://www.w3.org/1999/02/22-rdf-syntax-ns#type> <https://data.nasa.gov/ontologies/atmonto/data#WITIproperty> .
<https://data.nasa.gov/ontologies/atmonto/data#forecastingAirport> <http://www.w3.org/2000/01/rdf-schema#domain> <https://data.nasa.gov/ontologies/atmonto/data#TAFreport> .
_:B0fea9690X2Da2d4X2D4976X2Daa0cX2D1f5129c61150 <http://www.w3.org/1999/02/22-rdf-syntax-ns#type> <http://www.w3.org/2002/07/owl#Restriction> .
<https://data.nasa.gov/ontologies/atmonto/data#surfaceWindDirectionStatus> <http://www.w3.org/2000/01/rdf-schema#comment> "Information about the direction of the wind, either fixed, varyingWithinRange, or variable." .
<https://data.nasa.gov/ontologies/atmonto/data#etmsArrivals> <http://www.w3.org/2000/01/rdf-schema#label> "etms arrivals" .
_:Bd616d3c5X2D5a5aX2D4e0bX2D8540X2D04e9934f4846 <http://www.w3.org/1999/02/22-rdf-syntax-ns#first> "AUTO" .
_:Bf9bf06dbX2D3d8bX2D49ddX2Da012X2Dc9846897439f <http://www.w3.org/1999/02/22-rdf-syntax-ns#rest> _:B1bfa9b51X2Dccd1X2D46e9X2Db402X2D287ac5521893 .
<https://data.nasa.gov/ontologies/atmonto/data#scheduledArrivals> <http://www.w3.org/2000/01/rdf-schema#comment> "Count of scheduled arrivals. (Most probably from OAG (Official Airline Guide))" .
_:B8cf977bcX2D2117X2D4e12X2D8f80X2Da16200b800f9 <http://www.w3.org/1999/02/22-rdf-syntax-ns#rest> _:Bfac1032cX2Dd316X2D4b77X2Da395X2D41ef2744759a .
<https://data.nasa.gov/ontologies/atmonto/data#MeteorologicalCondition> <http://www.w3.org/2000/01/rdf-schema#subClassOf> _:Bdaeec009X2D8f1bX2D49e4X2D9273X2De4481e737d48 .
_:Bbf6eefb7X2D4f53X2D441dX2D97a5X2D04b495a23c9c <http://www.w3.org/1999/02/22-rdf-syntax-ns#rest> _:B5ba85c47X2D6e17X2D4e4bX2Dba3eX2D2d76ff83a78e .
<https://data.nasa.gov/ontologies/atmonto/data#CloudLayerProfile> <http://www.w3.org/2000/01/rdf-schema#subClassOf> _:B1c6feb5eX2Ded53X2D4a66X2D8040X2D8209c323332e .
_:B4455496dX2Db59fX2D4b8eX2D85b7X2D501844a10d5d <http://www.w3.org/1999/02/22-rdf-syntax-ns#type> <http://www.w3.org/2000/01/rdf-schema#Datatype> .
<https://data.nasa.gov/ontologies/atmonto/data#WITIproperty> <http://www.w3.org/2000/01/rdf-schema#label> "WITIproperty" .
_:B97306119X2D6454X2D46caX2Da1d6X2Dee39ce88006f <http://www.w3.org/2002/07/owl#allValuesFrom> _:B2c6b6bcfX2Dea96X2D4171X2D8b43X2D9ee49ed8f0a1 .
<https://data.nasa.gov/ontologies/atmonto/data#metarStationHasPrecipitationSensor> <http://www.w3.org/2000/01/rdf-schema#range> <http://www.w3.org/2001/XMLSchema#boolean> .
_:B5d4f6142X2Da1f0X2D4072X2Da809X2D852ce5e44b4d <http://www.w3.org/1999/02/22-rdf-syntax-ns#type> <http://www.w3.org/2000/01/rdf-schema#Datatype> .
<https://data.nasa.gov/ontologies/atmonto/data#lowCeilingWITIhourly> <http://www.w3.org/1999/02/22-rdf-syntax-ns#type> <https://data.nasa.gov/ontologies/atmonto/data#WITIproperty> .
<https://data.nasa.gov/ontologies/atmonto/data#surfaceWindSpeed> <http://www.w3.org/2000/01/rdf-schema#range> <http://www.w3.org/2001/XMLSchema#float> .
_:B230cdf26X2D6a04X2D4dceX2Daf60X2D2c2e2894276a <http://www.w3.org/1999/02/22-rdf-syntax-ns#first> "overcast" .
<https://data.nasa.gov/ontologies/atmonto/data#dewpoint> <http://www.w3.org/2000/01/rdf-schema#label> "dewpoint" .
_:B1eed5083X2D3b8dX2D4c08X2Dadf1X2D1eea74c97d5c <http://www.w3.org/2002/07/owl#onProperty> <https://data.nasa.gov/ontologies/atmonto/data#surfaceWindDirectionStatus> .
_:B99eb8123X2D4b4cX2D4ea1X2Da30cX2D98f3275b841f <http://www.w3.org/2002/07/owl#onProperty> <https://data.nasa.gov/ontologies/atmonto/data#weatherProximity> .
_:B9381954aX2Dcd8eX2D4902X2DbddbX2D1acd0d5d9150 <http://www.w3.org/2002/07/owl#allValuesFrom> <https://data.nasa.gov/ontologies/atmonto/NAS#Sector> .
<https://data.nasa.gov/ontologies/atmonto/data#METARreportingStation> <http://www.w3.org/1999/02/22-rdf-syntax-ns#type> <http://www.w3.org/2002/07/owl#Class> .
<https://data.nasa.gov/ontologies/atmonto/data#WeatherCondition> <http://www.w3.org/2000/01/rdf-schema#subClassOf> _:Bb0924366X2Da055X2D481bX2Dac3aX2D179dc523f9ab .
<https://data.nasa.gov/ontologies/atmonto/data#surfaceGustSpeed> <http://www.w3.org/2000/01/rdf-schema#label> "surface gust speed" .
_:Bb0924366X2Da055X2D481bX2Dac3aX2D179dc523f9ab <http://www.w3.org/2002/07/owl#onProperty> <https://data.nasa.gov/ontologies/atmonto/data#weatherIntensity> .
<https://data.nasa.gov/ontologies/atmonto/data#TAFreport> <http://www.w3.org/2000/01/rdf-schema#subClassOf> <https://data.nasa.gov/ontologies/atmonto/general#Sequence> .
<https://data.nasa.gov/ontologies/atmonto/data#metarReportType> <http://www.w3.org/2000/01/rdf-schema#domain> <https://data.nasa.gov/ontologies/atmonto/data#METARreport> .
_:B5f8fce50X2Dc5d8X2D48daX2Db7c6X2D7c1b6f6af3c4 <http://www.w3.org/1999/02/22-rdf-syntax-ns#first> "shower" .
_:B9c90bf4aX2D2609X2D4c54X2Db976X2D6348225f7b0f <http://www.w3.org/1999/02/22-rdf-syntax-ns#first> "forecast" .
_:B97bda6f7X2D7997X2D45d8X2Db9c2X2D9a780815a7ee <http://www.w3.org/1999/02/22-rdf-syntax-ns#first> "low drifting" .
_:B6f05af65X2D3ac3X2D4eabX2D8ba2X2D79da922e7fed <http://www.w3.org/2002/07/owl#onProperty> <https://data.nasa.gov/ontologies/atmonto/general#hasFirstItem> .
<https://data.nasa.gov/ontologies/atmonto/data#dataIntervalStartDay> <http://www.w3.org/2000/01/rdf-schema#domain> <https://data.nasa.gov/ontologies/atmonto/data#IntervalData> .
_:B54b31c49X2De49bX2D424aX2D8ca0X2D44c454b589d7 <http://www.w3.org/1999/02/22-rdf-syntax-ns#type> <http://www.w3.org/2000/01/rdf-schema#Datatype> .
_:Bf17cee5bX2D5755X2D4fb7X2D97ebX2Dec73717e59c7 <http://www.w3.org/1999/02/22-rdf-syntax-ns#first> "fog" .
<https://data.nasa.gov/ontologies/atmonto/data#airportArrivalRate> <http://www.w3.org/2000/01/rdf-schema#range> <http://www.w3.org/2001/XMLSchema#integer> .
<https://data.nasa.gov/ontologies/atmonto/data#totalAirborneDelay> <http://www.w3.org/1999/02/22-rdf-syntax-ns#type> <http://www.w3.org/2002/07/owl#FunctionalProperty> .
<https://data.nasa.gov/ontologies/atmonto/data#lowVisibilityWITIhourly> <http://www.w3.org/2000/01/rdf-schema#comment> "The low visibility weather impacted traffic index (WITI) computed for the airport during the specified timeframe (hourly). WITI is an estimate of the number of flights potentially impacted due to inclement weather based on the scheduled traffic demand for a defined geographic region of the air traffic system (in this case, an airport). If the visibility at the airport is below a set threshold, then the low visibility WITI is set to the number of scheduled arrivals for that timeframe." .
_:B8d363893X2D1704X2D4f5cX2Db41dX2D528cd0a7a11e <http://www.w3.org/2002/07/owl#oneOf> _:Be0657408X2Dc1a6X2D446aX2D8e38X2D6dc3b0f5ac14 .
<https://data.nasa.gov/ontologies/atmonto/data#SectorFlow> <http://www.w3.org/2000/01/rdf-schema#label> "Sector flow" .
<https://data.nasa.gov/ontologies/atmonto/data#hasCloudLayerProfile> <http://www.w3.org/2000/01/rdf-schema#label> "has cloud layer profile" .
_:B97306119X2D6454X2D46caX2Da1d6X2Dee39ce88006f <http://www.w3.org/1999/02/22-rdf-syntax-ns#type> <http://www.w3.org/2002/07/owl#Restriction> .
_:B0fea9690X2Da2d4X2D4976X2Daa0cX2D1f5129c61150 <http://www.w3.org/2002/07/owl#allValuesFrom> _:B4455496dX2Db59fX2D4b8eX2D85b7X2D501844a10d5d .
_:B1c6feb5eX2Ded53X2D4a66X2D8040X2D8209c323332e <http://www.w3.org/2002/07/owl#allValuesFrom> <https://data.nasa.gov/ontologies/atmonto/data#CloudLayer> .
<https://data.nasa.gov/ontologies/atmonto/data#cloudCover> <http://www.w3.org/2000/01/rdf-schema#range> <http://www.w3.org/2001/XMLSchema#string> .
<https://data.nasa.gov/ontologies/atmonto/data#airportDepartureRate> <http://www.w3.org/2000/01/rdf-schema#label> "airport departure rate" .
<https://data.nasa.gov/ontologies/atmonto/data#TAFreport> <http://www.w3.org/2000/01/rdf-schema#subClassOf> _:B6f05af65X2D3ac3X2D4eabX2D8ba2X2D79da922e7fed .
_:Beb087fa3X2D0133X2D4787X2Dbfb4X2De9880898c35a <http://www.w3.org/2002/07/owl#allValuesFrom> _:B528d25d8X2D078fX2D473aX2D8212X2D8f61edadc910 .
<https://data.nasa.gov/ontologies/atmonto/data#tafReportType> <http://www.w3.org/2000/01/rdf-schema#comment> "Type of Terminal Area Forecast (TAF) report: a routine report (TAF), an amended report (AMD), a corrected report (COR), or a delayed report (RTD). An amended TAF is issued when the current TAF no longer adequately describes the ongoing weather or the forecaster feels the TAF is not representative of the current or expected weather." .
<https://data.nasa.gov/ontologies/atmonto/data#windShearHeight> <http://www.w3.org/1999/02/22-rdf-syntax-ns#type> <http://www.w3.org/2002/07/owl#DatatypeProperty> .
<https://data.nasa.gov/ontologies/atmonto/data#CloudLayer> <http://www.w3.org/2000/01/rdf-schema#comment> "Represents a cloud layer, providing its bottom and top altitude, its cloud type, and its degree of coverage." .
_:B0a10f0e0X2D2618X2D4ab2X2D9d35X2D0f79d669b21e <http://www.w3.org/1999/02/22-rdf-syntax-ns#first> "towering cumulus" .
<https://data.nasa.gov/ontologies/atmonto/data#TAFreport> <http://www.w3.org/1999/02/22-rdf-syntax-ns#type> <http://www.w3.org/2002/07/owl#Class> .
_:Bd270744aX2D8b58X2D4e82X2D84aeX2Dbec1f8e37e13 <http://www.w3.org/1999/02/22-rdf-syntax-ns#type> <http://www.w3.org/2002/07/owl#Restriction> .
<https://data.nasa.gov/ontologies/atmonto/data#cloudCover> <http://www.w3.org/2000/01/rdf-schema#domain> <https://data.nasa.gov/ontologies/atmonto/data#CloudLayer> .
<https://data.nasa.gov/ontologies/atmonto/data#departureDemand> <http://www.w3.org/2000/01/rdf-schema#domain> <https://data.nasa.gov/ontologies/atmonto/data#AirportData> .
<https://data.nasa.gov/ontologies/atmonto/data#VisibilityCondition> <http://www.w3.org/2000/01/rdf-schema#label> "Visibility condition" .
<https://data.nasa.gov/ontologies/atmonto/data#totalAirborneDelay> <http://www.w3.org/2000/01/rdf-schema#range> <http://www.w3.org/2001/XMLSchema#float> .
<https://data.nasa.gov/ontologies/atmonto/data#aspmFlightRules> <http://www.w3.org/2000/01/rdf-schema#comment> "Indicates what flight rule conditions the airport is operating under during the specified time period (I-instrument, V-Visual)." .
_:Bd6384cdeX2Dd08aX2D4cf2X2D882fX2Dd0745776d655 <http://www.w3.org/2002/07/owl#onProperty> <https://data.nasa.gov/ontologies/atmonto/data#runwayStatus> .
<https://data.nasa.gov/ontologies/atmonto/data#SurfaceWindCondition> <http://www.w3.org/2000/01/rdf-schema#comment> "The current or forecast surface wind conditions." .
<https://data.nasa.gov/ontologies/atmonto/data#TAFmeteorologicalCondition> <http://www.w3.org/1999/02/22-rdf-syntax-ns#type> <http://www.w3.org/2002/07/owl#Class> .
<https://data.nasa.gov/ontologies/atmonto/data#etmsDepartures> <http://www.w3.org/2000/01/rdf-schema#range> <http://www.w3.org/2001/XMLSchema#integer> .
_:B97bda6f7X2D7997X2D45d8X2Db9c2X2D9a780815a7ee <http://www.w3.org/1999/02/22-rdf-syntax-ns#rest> _:Bc0b04394X2D0f2aX2D495aX2Db48aX2D3909da332a75 .
<https://data.nasa.gov/ontologies/atmonto/data#metarReportString> <http://www.w3.org/2000/01/rdf-schema#domain> <https://data.nasa.gov/ontologies/atmonto/data#METARreport> .
<https://data.nasa.gov/ontologies/atmonto/data#metConditionProbability> <http://www.w3.org/2000/01/rdf-schema#comment> "For a forecast meteorological condition, the percent probability associated with the forecast occurrence." .
_:B3de3ba09X2Dd947X2D476cX2D82b9X2D81581c658d84 <http://www.w3.org/1999/02/22-rdf-syntax-ns#first> "smoke" .
<https://data.nasa.gov/ontologies/atmonto/data#forecastingAirport> <http://www.w3.org/2000/01/rdf-schema#label> "forecasting airport" .
<https://data.nasa.gov/ontologies/atmonto/data#hasMETARreport> <http://www.w3.org/1999/02/22-rdf-syntax-ns#type> <http://www.w3.org/2002/07/owl#ObjectProperty> .
_:Bd616d3c5X2D5a5aX2D4e0bX2D8540X2D04e9934f4846 <http://www.w3.org/1999/02/22-rdf-syntax-ns#rest> _:B8f07340fX2D4b3fX2D42f7X2Da7a2X2Da835853aa3d2 .
_:B964063e1X2D598aX2D4833X2Da717X2D006b0ad56c4f <http://www.w3.org/1999/02/22-rdf-syntax-ns#first> "amended" .
<https://data.nasa.gov/ontologies/atmonto/data#WeatherCondition> <http://www.w3.org/2000/01/rdf-schema#subClassOf> <https://data.nasa.gov/ontologies/atmonto/data#MetCondition> .
<https://data.nasa.gov/ontologies/atmonto/data#hasWeatherCondition> <http://www.w3.org/2000/01/rdf-schema#comment> "Associates a meteorological condition with the details of the weather conditions at the reporting location." .
<https://data.nasa.gov/ontologies/atmonto/data#tafReportString> <http://www.w3.org/2000/01/rdf-schema#range> <http://www.w3.org/2001/XMLSchema#string> .
_:B8e425b69X2D6e28X2D45ceX2Dbe5aX2D37148e4c513b <http://www.w3.org/1999/02/22-rdf-syntax-ns#type> <http://www.w3.org/2002/07/owl#Restriction> .
<https://data.nasa.gov/ontologies/atmonto/data#surfaceWindDirectionStatus> <http://www.w3.org/2000/01/rdf-schema#label> "surface wind direction status" .
<https://data.nasa.gov/ontologies/atmonto/data#WeatherCondition> <http://www.w3.org/2000/01/rdf-schema#label> "Weather condition" .
<https://data.nasa.gov/ontologies/atmonto/data#windDirectionFixed> <http://www.w3.org/2000/01/rdf-schema#domain> <https://data.nasa.gov/ontologies/atmonto/data#SurfaceWindCondition> .
<https://data.nasa.gov/ontologies/atmonto/data#MetCondition> <http://www.w3.org/2000/01/rdf-schema#comment> "A superclass over the various types of meteorological conditions." .
_:B513700a8X2D8864X2D4f03X2Da59bX2D3276a521415d <http://www.w3.org/1999/02/22-rdf-syntax-ns#rest> _:Bcffad628X2Dfcf7X2D4d00X2Dbaa1X2De1d98d14a19d .
<https://data.nasa.gov/ontologies/atmonto/data#TAFreport> <http://www.w3.org/2000/01/rdf-schema#subClassOf> <https://data.nasa.gov/ontologies/atmonto/data#IntervalData> .
_:B250d7406X2D0509X2D47c9X2Dac7aX2Daee37a2553ab <http://www.w3.org/1999/02/22-rdf-syntax-ns#type> <http://www.w3.org/2000/01/rdf-schema#Datatype> .
_:Bd2d0bf49X2D78c9X2D45fdX2D868bX2D977560253335 <http://www.w3.org/1999/02/22-rdf-syntax-ns#rest> _:B230cdf26X2D6a04X2D4dceX2Daf60X2D2c2e2894276a .
<https://data.nasa.gov/ontologies/atmonto/data#windDirectionUpper> <http://www.w3.org/2000/01/rdf-schema#domain> <https://data.nasa.gov/ontologies/atmonto/data#SurfaceWindCondition> .
<https://data.nasa.gov/ontologies/atmonto/data#oagGateDepartureDelay> <http://www.w3.org/1999/02/22-rdf-syntax-ns#type> <http://www.w3.org/2002/07/owl#DatatypeProperty> .
<https://data.nasa.gov/ontologies/atmonto/data#oagArrivalDelay> <http://www.w3.org/2000/01/rdf-schema#label> "OAG arrival delay" .
<https://data.nasa.gov/ontologies/atmonto/data#scheduledArrivals> <http://www.w3.org/1999/02/22-rdf-syntax-ns#type> <http://www.w3.org/2002/07/owl#DatatypeProperty> .
<https://data.nasa.gov/ontologies/atmonto/data#hasSurfaceWindCondition> <http://www.w3.org/1999/02/22-rdf-syntax-ns#type> <http://www.w3.org/2002/07/owl#ObjectProperty> .
<https://data.nasa.gov/ontologies/atmonto/data#hasSurfaceWindCondition> <http://www.w3.org/2000/01/rdf-schema#range> <https://data.nasa.gov/ontologies/atmonto/data#SurfaceWindCondition> .
<https://data.nasa.gov/ontologies/atmonto/data#surfaceTemperature> <http://www.w3.org/2000/01/rdf-schema#domain> <https://data.nasa.gov/ontologies/atmonto/data#MeteorologicalCondition> .
<https://data.nasa.gov/ontologies/atmonto/data#MetCondition> <http://www.w3.org/2000/01/rdf-schema#label> "Meteorological condition" .
<https://data.nasa.gov/ontologies/atmonto/data#etmsArrivals> <http://www.w3.org/2000/01/rdf-schema#comment> "Count of arrivals at airport based on ETMS (Enhanced Traffic Management System) data." .
_:B76f6ed19X2D8a0eX2D4874X2D9d77X2De04bbb907796 <http://www.w3.org/1999/02/22-rdf-syntax-ns#rest> _:B707feedbX2Dbc93X2D4d7aX2D9954X2D1fff0050275c .
<https://data.nasa.gov/ontologies/atmonto/data#forecastIssueTime> <http://www.w3.org/2000/01/rdf-schema#comment> "The time that the TAF (Terminal Area Forecast) report was issued." .
<https://data.nasa.gov/ontologies/atmonto/data#runwaySurfaceFriction> <http://www.w3.org/2000/01/rdf-schema#domain> <https://data.nasa.gov/ontologies/atmonto/data#RunwayStatusData> .
<https://data.nasa.gov/ontologies/atmonto/data#highWindWITIhourly> <http://www.w3.org/2000/01/rdf-schema#comment> "The high wind weather impacted traffic index (WITI) computed for the airport during the specified timeframe (hourly). WITI is an estimate of the number of flights potentially impacted due to inclement weather based on the scheduled traffic demand for a defined geographic region of the air traffic system (in this case, an airport). If the winds at the airport are above a set threshold, then the high wind WITI is set to the number of scheduled arrivals for that timeframe." .
<https://data.nasa.gov/ontologies/atmonto/data#hasMETARreport> <http://www.w3.org/2000/01/rdf-schema#label> "has METARreport" .
<https://data.nasa.gov/ontologies/atmonto/data#edctArrivalHold> <http://www.w3.org/2000/01/rdf-schema#domain> <https://data.nasa.gov/ontologies/atmonto/data#AirportData> .
_:Becd96e69X2Db94eX2D423dX2Dbc6aX2Da7f962e9579c <http://www.w3.org/2002/07/owl#onProperty> <https://data.nasa.gov/ontologies/atmonto/data#metarReportModifier> .
_:B805beb7dX2De0a6X2D4d92X2Dbc13X2Dff6a40662f87 <http://www.w3.org/1999/02/22-rdf-syntax-ns#type> <http://www.w3.org/2002/07/owl#Restriction> .
<https://data.nasa.gov/ontologies/atmonto/data#dataIntervalEndDay> <http://www.w3.org/2000/01/rdf-schema#range> <https://data.nasa.gov/ontologies/atmonto/NAS#NASday> .
_:Beb087fa3X2D0133X2D4787X2Dbfb4X2De9880898c35a <http://www.w3.org/2002/07/owl#onProperty> <https://data.nasa.gov/ontologies/atmonto/data#tafReportType> .
<https://data.nasa.gov/ontologies/atmonto/data#METARreport> <http://www.w3.org/2000/01/rdf-schema#label> "METAR Report" .
<https://data.nasa.gov/ontologies/atmonto/data#tafReportType> <http://www.w3.org/1999/02/22-rdf-syntax-ns#type> <http://www.w3.org/2002/07/owl#DatatypeProperty> .
<https://data.nasa.gov/ontologies/atmonto/data#FixCapacity> <http://www.w3.org/2000/01/rdf-schema#label> "Fix capacity" .
<https://data.nasa.gov/ontologies/atmonto/data#airportArrivalRate> <http://www.w3.org/1999/02/22-rdf-syntax-ns#type> <http://www.w3.org/2002/07/owl#FunctionalProperty> .
<https://data.nasa.gov/ontologies/atmonto/data#baseAltitude> <http://www.w3.org/2000/01/rdf-schema#label> "base altitude" .
<https://data.nasa.gov/ontologies/atmonto/data#metarReportModifier> <http://www.w3.org/2000/01/rdf-schema#range> <http://www.w3.org/2001/XMLSchema#string> .
_:Bd270744aX2D8b58X2D4e82X2D84aeX2Dbec1f8e37e13 <http://www.w3.org/2002/07/owl#onProperty> <https://data.nasa.gov/ontologies/atmonto/general#hasSequencedItem> .
_:B46fafbb9X2D8a44X2D44f2X2Da251X2D9afc5da3912e <http://www.w3.org/1999/02/22-rdf-syntax-ns#rest> <http://www.w3.org/1999/02/22-rdf-syntax-ns#nil> .
_:Bcfbdc0bdX2Daa20X2D44ffX2D9949X2De9daeac6a1bf <http://www.w3.org/1999/02/22-rdf-syntax-ns#first> "vertical visibility layer" .
<https://data.nasa.gov/ontologies/atmonto/data#unlimitedVisibility> <http://www.w3.org/2000/01/rdf-schema#range> <http://www.w3.org/2001/XMLSchema#boolean> .
<https://data.nasa.gov/ontologies/atmonto/data#CloudLayerProfile> <http://www.w3.org/2000/01/rdf-schema#label> "Cloud layer profile" .
<https://data.nasa.gov/ontologies/atmonto/data#scheduledArrivals> <http://www.w3.org/2000/01/rdf-schema#label> "scheduled arrivals" .
<https://data.nasa.gov/ontologies/atmonto/data#ASPMmeteorologicalCondition> <http://www.w3.org/2000/01/rdf-schema#label> "ASPM meteorological condition" .
_:B7b5530c5X2D489cX2D4cc0X2Da132X2Dccd6bb298bac <http://www.w3.org/1999/02/22-rdf-syntax-ns#rest> <http://www.w3.org/1999/02/22-rdf-syntax-ns#nil> .
<https://data.nasa.gov/ontologies/atmonto/data#SurfaceWindCondition> <http://www.w3.org/1999/02/22-rdf-syntax-ns#type> <http://www.w3.org/2002/07/owl#Class> .
<https://data.nasa.gov/ontologies/atmonto/data#weatherIntensity> <http://www.w3.org/2000/01/rdf-schema#label> "weather intensity" .
_:Bed0be29bX2D57deX2D4f76X2Db3c4X2Dc697a028d67d <http://www.w3.org/2002/07/owl#allValuesFrom> _:B8d363893X2D1704X2D4f5cX2Db41dX2D528cd0a7a11e .
<https://data.nasa.gov/ontologies/atmonto/data#metarReportString> <http://www.w3.org/2000/01/rdf-schema#comment> "Entire text of METAR report." .
_:B76f6ed19X2D8a0eX2D4874X2D9d77X2De04bbb907796 <http://www.w3.org/1999/02/22-rdf-syntax-ns#first> "well-developed dust/sand whirls" .
<https://data.nasa.gov/ontologies/atmonto/data#weatherPhenomenon> <http://www.w3.org/2000/01/rdf-schema#domain> <https://data.nasa.gov/ontologies/atmonto/data#WeatherCondition> .
_:B69d15ecaX2D4fa3X2D45edX2Da7d1X2D16ba12529690 <http://www.w3.org/1999/02/22-rdf-syntax-ns#rest> _:B97bda6f7X2D7997X2D45d8X2Db9c2X2D9a780815a7ee .
<https://data.nasa.gov/ontologies/atmonto/data#METARreport> <http://www.w3.org/2000/01/rdf-schema#subClassOf> _:Bb2447386X2D2e28X2D4c69X2Dba49X2De5dfe47e13ba .
_:B9ce34d7bX2De1c2X2D4ef2X2Db0ebX2D036a7350e4a1 <http://www.w3.org/2002/07/owl#allValuesFrom> <https://data.nasa.gov/ontologies/atmonto/data#CloudLayer> .
_:B035d8c87X2D8e8bX2D4c64X2D80c1X2Dc15f119e4b26 <http://www.w3.org/1999/02/22-rdf-syntax-ns#type> <http://www.w3.org/2002/07/owl#Restriction> .
<https://data.nasa.gov/ontologies/atmonto/data#seaLevelPressure> <http://www.w3.org/2000/01/rdf-schema#range> <http://www.w3.org/2001/XMLSchema#float> .
<https://data.nasa.gov/ontologies/atmonto/data#windShearHeight> <http://www.w3.org/2000/01/rdf-schema#comment> "The height in hundreds of feet above ground level associated with a wind shear phenomenon." .
<https://data.nasa.gov/ontologies/atmonto/data#WITIproperty> <http://www.w3.org/2000/01/rdf-schema#subClassOf> <http://www.w3.org/2002/07/owl#DatatypeProperty> .
<https://data.nasa.gov/ontologies/atmonto/data#lowVisibilityWITIdaily> <http://www.w3.org/2000/01/rdf-schema#comment> "The low visibility weather impacted traffic index (WITI) computed for the airport during the specified timeframe (daily). WITI is an estimate of the number of flights potentially impacted due to inclement weather based on the scheduled traffic demand for a defined geographic region of the air traffic system (in this case, an airport). If the visibility at the airport is below a set threshold, then the low visibility WITI is set to the number of scheduled arrivals for that timeframe." .
_:B2b621779X2D2b0eX2D4b01X2D8daaX2D4ca45b169260 <http://www.w3.org/1999/02/22-rdf-syntax-ns#first> "in vicinity" .
<https://data.nasa.gov/ontologies/atmonto/data#edctArrivalHold> <http://www.w3.org/2000/01/rdf-schema#label> "EDCT arrival hold" .
<https://data.nasa.gov/ontologies/atmonto/data#highWindWITIhourly> <http://www.w3.org/2000/01/rdf-schema#domain> <https://data.nasa.gov/ontologies/atmonto/data#AirportData> .
_:Be07d6f98X2D2f29X2D4301X2Db3a4X2D6815000d445d <http://www.w3.org/2002/07/owl#onProperty> <https://data.nasa.gov/ontologies/atmonto/ATM#flowMeasurementRegion> .
_:B230cdf26X2D6a04X2D4dceX2Daf60X2D2c2e2894276a <http://www.w3.org/1999/02/22-rdf-syntax-ns#rest> _:Bcfbdc0bdX2Daa20X2D44ffX2D9949X2De9daeac6a1bf .
<https://data.nasa.gov/ontologies/atmonto/data#runwaySurfaceFriction> <http://www.w3.org/2000/01/rdf-schema#range> <http://www.w3.org/2001/XMLSchema#float> .
<https://data.nasa.gov/ontologies/atmonto/data#lowCeilingWITIhourly> <http://www.w3.org/2000/01/rdf-schema#label> "low ceiling WITI hourly" .
<https://data.nasa.gov/ontologies/atmonto/data#baseAltitude> <http://www.w3.org/2000/01/rdf-schema#domain> <https://data.nasa.gov/ontologies/atmonto/data#CloudLayer> .
_:B25ba395bX2D0846X2D4d82X2D82d9X2D21ac99c733ef <http://www.w3.org/2002/07/owl#oneOf> _:B513700a8X2D8864X2D4f03X2Da59bX2D3276a521415d .
_:Bb2447386X2D2e28X2D4c69X2Dba49X2De5dfe47e13ba <http://www.w3.org/2002/07/owl#onProperty> <https://data.nasa.gov/ontologies/atmonto/data#metarReportType> .
<https://data.nasa.gov/ontologies/atmonto/data#weatherPhenomenon> <http://www.w3.org/1999/02/22-rdf-syntax-ns#type> <http://www.w3.org/2002/07/owl#DatatypeProperty> .
<https://data.nasa.gov/ontologies/atmonto/data#airportArrivalRate> <http://www.w3.org/2000/01/rdf-schema#comment> "The arrival rate per hour set by the airport during the specified interval. This is the total number of aircraft that can arrive on all runways combined during an hour." .
_:B99eb8123X2D4b4cX2D4ea1X2Da30cX2D98f3275b841f <http://www.w3.org/1999/02/22-rdf-syntax-ns#type> <http://www.w3.org/2002/07/owl#Restriction> .
<https://data.nasa.gov/ontologies/atmonto/data#dataIntervalEndDay> <http://www.w3.org/1999/02/22-rdf-syntax-ns#type> <http://www.w3.org/2002/07/owl#ObjectProperty> .
_:B4e280221X2Db9eaX2D4d95X2Db31cX2D56635ce48129 <http://www.w3.org/1999/02/22-rdf-syntax-ns#rest> _:B14b9247fX2D1e6fX2D4a13X2Da9a1X2D0429fef1984c .
_:B54b31c49X2De49bX2D424aX2D8ca0X2D44c454b589d7 <http://www.w3.org/2002/07/owl#oneOf> _:Bc416aebdX2D893bX2D40e2X2Dbbe6X2D9efbb3d57b65 .
<https://data.nasa.gov/ontologies/atmonto/data#hasVisibilityCondition> <http://www.w3.org/2000/01/rdf-schema#range> <https://data.nasa.gov/ontologies/atmonto/data#VisibilityCondition> .
<https://data.nasa.gov/ontologies/atmonto/data#forecastIssueTime> <http://www.w3.org/2000/01/rdf-schema#label> "forecast issue time" .
<https://data.nasa.gov/ontologies/atmonto/data#aspmFlightRules> <http://www.w3.org/1999/02/22-rdf-syntax-ns#type> <http://www.w3.org/2002/07/owl#DatatypeProperty> .
_:B1af074b8X2D5962X2D4fcbX2Daca3X2Da844f3426735 <http://www.w3.org/2002/07/owl#onProperty> <https://data.nasa.gov/ontologies/atmonto/data#cloudType> .
<https://data.nasa.gov/ontologies/atmonto/data#hasSkyCondition> <http://www.w3.org/1999/02/22-rdf-syntax-ns#type> <http://www.w3.org/2002/07/owl#ObjectProperty> .
<https://data.nasa.gov/ontologies/atmonto/data#METARreport> <http://www.w3.org/2000/01/rdf-schema#subClassOf> _:Becd96e69X2Db94eX2D423dX2Dbc6aX2Da7f962e9579c .
_:Bf27add84X2D9124X2D4875X2Da3aeX2Dae2ca2ff433f <http://www.w3.org/1999/02/22-rdf-syntax-ns#first> "delayed" .
_:B4c7117e3X2Df7ceX2D41b2X2D9a3eX2Deb7cb89d18ff <http://www.w3.org/2002/07/owl#onProperty> <https://data.nasa.gov/ontologies/atmonto/data#meteorologicalConditionStatus> .
<https://data.nasa.gov/ontologies/atmonto/data#aspmFlightRules> <http://www.w3.org/2000/01/rdf-schema#label> "ASPM Flight Rules" .
<https://data.nasa.gov/ontologies/atmonto/data#highWindWITIhourly> <http://www.w3.org/2000/01/rdf-schema#range> <http://www.w3.org/2001/XMLSchema#float> .
<https://data.nasa.gov/ontologies/atmonto/data#SurfaceWindCondition> <http://www.w3.org/2000/01/rdf-schema#label> "Surface wind condition" .
_:Bebd0d737X2D5b76X2D489dX2D8cb9X2D2aad44a9506d <http://www.w3.org/2002/07/owl#onProperty> <https://data.nasa.gov/ontologies/atmonto/ATM#flowMeasurementRegion> .
<https://data.nasa.gov/ontologies/atmonto/data#MeteorologicalCondition> <http://www.w3.org/1999/02/22-rdf-syntax-ns#type> <http://www.w3.org/2002/07/owl#Class> .
_:B795569e6X2D13d8X2D47e9X2Dbf2aX2D18d54d334b74 <http://www.w3.org/1999/02/22-rdf-syntax-ns#rest> _:Bebcc5a6dX2D4c71X2D4c01X2Dbb24X2D303e16cf078c .
<https://data.nasa.gov/ontologies/atmonto/data#limitedVisibilityDistance> <http://www.w3.org/2000/01/rdf-schema#range> <http://www.w3.org/2001/XMLSchema#float> .
<https://data.nasa.gov/ontologies/atmonto/data#VisibilityCondition> <http://www.w3.org/2000/01/rdf-schema#comment> "The current or forecast surface visibility conditions at a given airport or other reporting station." .
_:Bb0924366X2Da055X2D481bX2Dac3aX2D179dc523f9ab <http://www.w3.org/2002/07/owl#allValuesFrom> _:B25ba395bX2D0846X2D4d82X2D82d9X2D21ac99c733ef .
<https://data.nasa.gov/ontologies/atmonto/data#hasAirportData> <http://www.w3.org/2000/01/rdf-schema#comment> "Links an airport to a collection of temporally-dependent data pertinent to the airport conditions, including a variety of data collected in the ASPM system." .
<https://data.nasa.gov/ontologies/atmonto/data> <http://www.w3.org/2002/07/owl#versionInfo> "Created with TopBraid Composer" .
<https://data.nasa.gov/ontologies/atmonto/data#weatherQualifier> <http://www.w3.org/2000/01/rdf-schema#label> "weather qualifier" .
<https://data.nasa.gov/ontologies/atmonto/data#lowVisibilityWITIhourly> <http://www.w3.org/1999/02/22-rdf-syntax-ns#type> <http://www.w3.org/2002/07/owl#FunctionalProperty> .
<https://data.nasa.gov/ontologies/atmonto/data#scheduledDepartures> <http://www.w3.org/2000/01/rdf-schema#label> "scheduled departures" .
_:B9ce34d7bX2De1c2X2D4ef2X2Db0ebX2D036a7350e4a1 <http://www.w3.org/1999/02/22-rdf-syntax-ns#type> <http://www.w3.org/2002/07/owl#Restriction> .
<https://data.nasa.gov/ontologies/atmonto/data#airportDepartureRate> <http://www.w3.org/1999/02/22-rdf-syntax-ns#type> <http://www.w3.org/2002/07/owl#FunctionalProperty> .
<https://data.nasa.gov/ontologies/atmonto/data#oagGateDepartureDelay> <http://www.w3.org/2000/01/rdf-schema#label> "OAG gate departure delay" .
<https://data.nasa.gov/ontologies/atmonto/data#baseAltitude> <http://www.w3.org/1999/02/22-rdf-syntax-ns#type> <http://www.w3.org/2002/07/owl#DatatypeProperty> .
_:B3e86c2f0X2Dd810X2D42a7X2D9fceX2D5d86be533d87 <http://www.w3.org/1999/02/22-rdf-syntax-ns#rest> _:B76f6ed19X2D8a0eX2D4874X2D9d77X2De04bbb907796 .
_:B97306119X2D6454X2D46caX2Da1d6X2Dee39ce88006f <http://www.w3.org/2002/07/owl#onProperty> <https://data.nasa.gov/ontologies/atmonto/data#weatherQualifier> .
<https://data.nasa.gov/ontologies/atmonto/data#arrivalDemand> <http://www.w3.org/2000/01/rdf-schema#label> "arrival demand" .
_:B3720f7beX2Dc05dX2D4ad7X2D9f53X2D0bf28577eadf <http://www.w3.org/1999/02/22-rdf-syntax-ns#rest> _:B7c0bd641X2Dd3c5X2D4dfbX2Db8faX2D67cf310a0048 .
<https://data.nasa.gov/ontologies/atmonto/data#metarReportModifier> <http://www.w3.org/2000/01/rdf-schema#comment> "Automation status information pertaining to a METAR report: AUTO indicates a fully automated report with no human intervention; COR indicates a corrected observation; no modifier indicates either human observer/reporter or automated report with human oversight." .
_:Bfac1032cX2Dd316X2D4b77X2Da395X2D41ef2744759a <http://www.w3.org/1999/02/22-rdf-syntax-ns#rest> _:B31730194X2Da2aeX2D4755X2D9b1eX2D53849b794653 .
<https://data.nasa.gov/ontologies/atmonto/data#oagArrivalDelay> <http://www.w3.org/1999/02/22-rdf-syntax-ns#type> <http://www.w3.org/2002/07/owl#DatatypeProperty> .
<https://data.nasa.gov/ontologies/atmonto/data#departureDemand> <http://www.w3.org/2000/01/rdf-schema#range> <http://www.w3.org/2001/XMLSchema#integer> .
<https://data.nasa.gov/ontologies/atmonto/data#cloudType> <http://www.w3.org/2000/01/rdf-schema#range> <http://www.w3.org/2001/XMLSchema#string> .
_:B8c48c716X2D963cX2D4959X2Db42cX2Dbd4a96019db6 <http://www.w3.org/2002/07/owl#cardinality> "1"^^<http://www.w3.org/2001/XMLSchema#nonNegativeInteger> .
_:B4c7117e3X2Df7ceX2D41b2X2D9a3eX2Deb7cb89d18ff <http://www.w3.org/2002/07/owl#cardinality> "1"^^<http://www.w3.org/2001/XMLSchema#nonNegativeInteger> .
<https://data.nasa.gov/ontologies/atmonto/data#etmsArrivals> <http://www.w3.org/1999/02/22-rdf-syntax-ns#type> <http://www.w3.org/2002/07/owl#DatatypeProperty> .
<https://data.nasa.gov/ontologies/atmonto/data#hasTAFreport> <http://www.w3.org/1999/02/22-rdf-syntax-ns#type> <http://www.w3.org/2002/07/owl#ObjectProperty> .
<https://data.nasa.gov/ontologies/atmonto/data#surfaceTemperature> <http://www.w3.org/1999/02/22-rdf-syntax-ns#type> <http://www.w3.org/2002/07/owl#DatatypeProperty> .
<https://data.nasa.gov/ontologies/atmonto/data#MeteorologicalCondition> <http://www.w3.org/2000/01/rdf-schema#subClassOf> <https://data.nasa.gov/ontologies/atmonto/data#IntervalData> .
<https://data.nasa.gov/ontologies/atmonto/data#windDirectionLower> <http://www.w3.org/2000/01/rdf-schema#domain> <https://data.nasa.gov/ontologies/atmonto/data#SurfaceWindCondition> .
<https://data.nasa.gov/ontologies/atmonto/data#MeteorologicalCondition> <http://www.w3.org/2000/01/rdf-schema#comment> "A representation of the meteorological status for the specified time period, including sky, wind, visibility, and weather subcomponents." .
<https://data.nasa.gov/ontologies/atmonto/data#arrivalDemand> <http://www.w3.org/1999/02/22-rdf-syntax-ns#type> <http://www.w3.org/2002/07/owl#FunctionalProperty> .
_:B4fc00ab9X2Dd8e6X2D499dX2D8a46X2D29e6d0403d01 <http://www.w3.org/1999/02/22-rdf-syntax-ns#first> "unknown precipitation" .
<https://data.nasa.gov/ontologies/atmonto/data#edctArrivalHold> <http://www.w3.org/2000/01/rdf-schema#range> <http://www.w3.org/2001/XMLSchema#float> .
_:B69d15ecaX2D4fa3X2D45edX2Da7d1X2D16ba12529690 <http://www.w3.org/1999/02/22-rdf-syntax-ns#first> "patchy" .
<https://data.nasa.gov/ontologies/atmonto/data#RunwayStatusData> <http://www.w3.org/2000/01/rdf-schema#label> "Runway status data" .
<https://data.nasa.gov/ontologies/atmonto/data#SkyCondition> <http://www.w3.org/2000/01/rdf-schema#comment> "The current or forecast sky conditions, including the ceiling and information on the cloud layers present." .
_:B25ba395bX2D0846X2D4d82X2D82d9X2D21ac99c733ef <http://www.w3.org/1999/02/22-rdf-syntax-ns#type> <http://www.w3.org/2000/01/rdf-schema#Datatype> .
_:B2635a848X2Dce68X2D4e2bX2Db928X2Dd7161a537f11 <http://www.w3.org/1999/02/22-rdf-syntax-ns#first> "funnel cloud" .
<https://data.nasa.gov/ontologies/atmonto/data#runwayStatus> <http://www.w3.org/1999/02/22-rdf-syntax-ns#type> <http://www.w3.org/2002/07/owl#DatatypeProperty> .
_:Bc6eac04aX2D276dX2D4b24X2Dbb5fX2Ddaf57af65002 <http://www.w3.org/1999/02/22-rdf-syntax-ns#first> "heavy" .
<https://data.nasa.gov/ontologies/atmonto/data#etmsDepartures> <http://www.w3.org/2000/01/rdf-schema#domain> <https://data.nasa.gov/ontologies/atmonto/data#AirportData> .
<https://data.nasa.gov/ontologies/atmonto/data#weatherPhenomenon> <http://www.w3.org/2000/01/rdf-schema#comment> "Describes the type of weather phenomena experienced during the specified period: drizzle, rain, snow, snow grains, ice crystals, ice pellets, hail, small hail and/or snow pellets, unknown precipitation, mist, fog, smoke, volcanic ash, widespread dust, sand, haze, spray, well-developed dust/sand whirls, squalls, funnel cloud, tornado/waterspout, sandstorm, duststorm" .
<https://data.nasa.gov/ontologies/atmonto/data#CloudLayer> <http://www.w3.org/2000/01/rdf-schema#subClassOf> _:B8c48c716X2D963cX2D4959X2Db42cX2Dbd4a96019db6 .
<https://data.nasa.gov/ontologies/atmonto/data#ceiling> <http://www.w3.org/1999/02/22-rdf-syntax-ns#type> <http://www.w3.org/2002/07/owl#DatatypeProperty> .
<https://data.nasa.gov/ontologies/atmonto/data#hasTAFreport> <http://www.w3.org/2000/01/rdf-schema#comment> "Associates an airport with TAF weather reports generated for that airport." .
_:B2635a848X2Dce68X2D4e2bX2Db928X2Dd7161a537f11 <http://www.w3.org/1999/02/22-rdf-syntax-ns#rest> _:Bbf6eefb7X2D4f53X2D441dX2D97a5X2D04b495a23c9c .
<https://data.nasa.gov/ontologies/atmonto/data#metarStationHasPrecipitationSensor> <http://www.w3.org/2000/01/rdf-schema#domain> <https://data.nasa.gov/ontologies/atmonto/data#METARreport> .
<https://data.nasa.gov/ontologies/atmonto/data#runwayVisibleRange> <http://www.w3.org/2000/01/rdf-schema#label> "runway visible range" .
<https://data.nasa.gov/ontologies/atmonto/data#hourlyPrecipitation> <http://www.w3.org/1999/02/22-rdf-syntax-ns#type> <http://www.w3.org/2002/07/owl#DatatypeProperty> .
_:Bc93945cdX2Dbbb5X2D4eacX2Da84cX2D697ea4b10cb0 <http://www.w3.org/2002/07/owl#onProperty> <https://data.nasa.gov/ontologies/atmonto/data#weatherIntensity> .
<https://data.nasa.gov/ontologies/atmonto/data#hasMETARreport> <http://www.w3.org/2000/01/rdf-schema#comment> "Associates a METAR reporting station with METAR weather reports generated for that station." .
_:B6401bc46X2D5951X2D460fX2D8449X2D8cac8d53dacc <http://www.w3.org/2002/07/owl#onProperty> <https://data.nasa.gov/ontologies/atmonto/data#metarReportType> .
<https://data.nasa.gov/ontologies/atmonto/data#SkyCondition> <http://www.w3.org/1999/02/22-rdf-syntax-ns#type> <http://www.w3.org/2002/07/owl#Class> .
_:B9ce34d7bX2De1c2X2D4ef2X2Db0ebX2D036a7350e4a1 <http://www.w3.org/2002/07/owl#onProperty> <https://data.nasa.gov/ontologies/atmonto/general#hasSequencedItem> .
<https://data.nasa.gov/ontologies/atmonto/data#surfaceGustSpeed> <http://www.w3.org/2000/01/rdf-schema#domain> <https://data.nasa.gov/ontologies/atmonto/data#SurfaceWindCondition> .
<https://data.nasa.gov/ontologies/atmonto/data#edctDepartureHold> <http://www.w3.org/2000/01/rdf-schema#label> "EDCT departure hold" .
_:B6a6d732fX2D3d9dX2D4ff2X2D9ca9X2Da4c8cfd7aad4 <http://www.w3.org/1999/02/22-rdf-syntax-ns#rest> _:Bd4a3a582X2D9a9fX2D415aX2D9694X2Dc01bdb73db07 .
<https://data.nasa.gov/ontologies/atmonto/data#CloudLayerProfile> <http://www.w3.org/2000/01/rdf-schema#subClassOf> _:B195faeccX2D24b1X2D411bX2D84cdX2D8418f3dd35e1 .
<https://data.nasa.gov/ontologies/atmonto/data#WeatherCondition> <http://www.w3.org/2000/01/rdf-schema#subClassOf> _:B97306119X2D6454X2D46caX2Da1d6X2Dee39ce88006f .
_:B6f05af65X2D3ac3X2D4eabX2D8ba2X2D79da922e7fed <http://www.w3.org/2002/07/owl#allValuesFrom> <https://data.nasa.gov/ontologies/atmonto/data#TAFmeteorologicalCondition> .
<https://data.nasa.gov/ontologies/atmonto/data#hourlyPrecipitation> <http://www.w3.org/2000/01/rdf-schema#domain> <https://data.nasa.gov/ontologies/atmonto/data#WeatherCondition> .
_:B5d4f6142X2Da1f0X2D4072X2Da809X2D852ce5e44b4d <http://www.w3.org/2002/07/owl#oneOf> _:Bd616d3c5X2D5a5aX2D4e0bX2D8540X2D04e9934f4846 .
_:B8914685fX2D58a2X2D466cX2Daf8bX2D76835b10c083 <http://www.w3.org/1999/02/22-rdf-syntax-ns#type> <http://www.w3.org/2002/07/owl#Restriction> .
_:B95a67ad0X2Dd63eX2D4c80X2Dbfd0X2D73fbdfc02689 <http://www.w3.org/1999/02/22-rdf-syntax-ns#rest> _:Bf17cee5bX2D5755X2D4fb7X2D97ebX2Dec73717e59c7 .
_:B513700a8X2D8864X2D4f03X2Da59bX2D3276a521415d <http://www.w3.org/1999/02/22-rdf-syntax-ns#first> "light" .
_:B2c6b6bcfX2Dea96X2D4171X2D8b43X2D9ee49ed8f0a1 <http://www.w3.org/1999/02/22-rdf-syntax-ns#type> <http://www.w3.org/2000/01/rdf-schema#Datatype> .
_:Bdaeec009X2D8f1bX2D49e4X2D9273X2De4481e737d48 <http://www.w3.org/2002/07/owl#onProperty> <https://data.nasa.gov/ontologies/atmonto/data#meteorologicalConditionStatus> .
_:B2c6b6bcfX2Dea96X2D4171X2D8b43X2D9ee49ed8f0a1 <http://www.w3.org/2002/07/owl#oneOf> _:B6a6d732fX2D3d9dX2D4ff2X2D9ca9X2Da4c8cfd7aad4 .
<https://data.nasa.gov/ontologies/atmonto/data#forecastIssueTime> <http://www.w3.org/1999/02/22-rdf-syntax-ns#type> <http://www.w3.org/2002/07/owl#DatatypeProperty> .
<https://data.nasa.gov/ontologies/atmonto/data#cloudCover> <http://www.w3.org/1999/02/22-rdf-syntax-ns#type> <http://www.w3.org/2002/07/owl#DatatypeProperty> .
<https://data.nasa.gov/ontologies/atmonto/data#forecastIssueTime> <http://www.w3.org/2000/01/rdf-schema#range> <http://www.w3.org/2001/XMLSchema#dateTime> .
<https://data.nasa.gov/ontologies/atmonto/data#airportDepartureRate> <http://www.w3.org/2000/01/rdf-schema#comment> "The departure rate per hour set by the airport during the specified interval. This is the total number of aircraft that can depart from all runways combined during an hour." .
_:B6401bc46X2D5951X2D460fX2D8449X2D8cac8d53dacc <http://www.w3.org/2002/07/owl#allValuesFrom> _:B31ecb3a2X2D633bX2D4b66X2D8d6eX2De894ef9060a9 .
_:B8e425b69X2D6e28X2D45ceX2Dbe5aX2D37148e4c513b <http://www.w3.org/2002/07/owl#onProperty> <https://data.nasa.gov/ontologies/atmonto/general#hasLastItem> .
<https://data.nasa.gov/ontologies/atmonto/data#hasVisibilityCondition> <http://www.w3.org/2000/01/rdf-schema#label> "has visibility condition" .
<https://data.nasa.gov/ontologies/atmonto/data#lowCeilingWITIdaily> <http://www.w3.org/1999/02/22-rdf-syntax-ns#type> <https://data.nasa.gov/ontologies/atmonto/data#WITIproperty> .
_:B95a67ad0X2Dd63eX2D4c80X2Dbfd0X2D73fbdfc02689 <http://www.w3.org/1999/02/22-rdf-syntax-ns#first> "mist" .
<https://data.nasa.gov/ontologies/atmonto/data#runwaySurfaceFriction> <http://www.w3.org/2000/01/rdf-schema#comment> "The surface friction (mu) value of the runway for the specified period. Runway surface friction is directly relevant to the braking action which will be available to an aircraft decelerating after touch down, or after a decision to reject a take off." .
<https://data.nasa.gov/ontologies/atmonto/data#metarReportString> <http://www.w3.org/1999/02/22-rdf-syntax-ns#type> <http://www.w3.org/2002/07/owl#FunctionalProperty> .
<https://data.nasa.gov/ontologies/atmonto/data#topAltitude> <http://www.w3.org/2000/01/rdf-schema#label> "top altitude" .
<https://data.nasa.gov/ontologies/atmonto/data#METARreport> <http://www.w3.org/1999/02/22-rdf-syntax-ns#type> <http://www.w3.org/2002/07/owl#Class> .
<https://data.nasa.gov/ontologies/atmonto/data#SectorFlow> <http://www.w3.org/2000/01/rdf-schema#subClassOf> <https://data.nasa.gov/ontologies/atmonto/ATM#AircraftFlow> .
<https://data.nasa.gov/ontologies/atmonto/data#scheduledDepartures> <http://www.w3.org/1999/02/22-rdf-syntax-ns#type> <http://www.w3.org/2002/07/owl#DatatypeProperty> .
_:Be0657408X2Dc1a6X2D446aX2D8e38X2D6dc3b0f5ac14 <http://www.w3.org/1999/02/22-rdf-syntax-ns#first> "I" .
<https://data.nasa.gov/ontologies/atmonto/data#dataIntervalStartTime> <http://www.w3.org/2000/01/rdf-schema#domain> <https://data.nasa.gov/ontologies/atmonto/data#IntervalData> .
<https://data.nasa.gov/ontologies/atmonto/data#limitedVisibilityDistance> <http://www.w3.org/2000/01/rdf-schema#seeAlso> <https://data.nasa.gov/ontologies/atmonto/data#unlimitedVisibility> .
<https://data.nasa.gov/ontologies/atmonto/data#edctDepartureHold> <http://www.w3.org/1999/02/22-rdf-syntax-ns#type> <http://www.w3.org/2002/07/owl#DatatypeProperty> .
<https://data.nasa.gov/ontologies/atmonto/data#totalAirborneDelay> <http://www.w3.org/2000/01/rdf-schema#domain> <https://data.nasa.gov/ontologies/atmonto/data#AirportData> .
<https://data.nasa.gov/ontologies/atmonto/data#hasWeatherCondition> <http://www.w3.org/2000/01/rdf-schema#range> <https://data.nasa.gov/ontologies/atmonto/data#WeatherCondition> .
<https://data.nasa.gov/ontologies/atmonto/data#surfaceGustSpeed> <http://www.w3.org/2000/01/rdf-schema#comment> "Surface gust speed measured under the associated surface wind conditions." .
<https://data.nasa.gov/ontologies/atmonto/data#metarReportType> <http://www.w3.org/2000/01/rdf-schema#label> "metar report type" .
<https://data.nasa.gov/ontologies/atmonto/data#surfaceGustSpeed> <http://www.w3.org/2000/01/rdf-schema#range> <http://www.w3.org/2001/XMLSchema#float> .
<https://data.nasa.gov/ontologies/atmonto/data#windDirectionFixed> <http://www.w3.org/2000/01/rdf-schema#comment> "Steady wind direction (in degrees), when winds are fixed and not variable." .
_:Bc6eac04aX2D276dX2D4b24X2Dbb5fX2Ddaf57af65002 <http://www.w3.org/1999/02/22-rdf-syntax-ns#rest> <http://www.w3.org/1999/02/22-rdf-syntax-ns#nil> .
_:B195faeccX2D24b1X2D411bX2D84cdX2D8418f3dd35e1 <http://www.w3.org/2002/07/owl#onProperty> <https://data.nasa.gov/ontologies/atmonto/general#hasLastItem> .
_:B1bfa9b51X2Dccd1X2D46e9X2Db402X2D287ac5521893 <http://www.w3.org/1999/02/22-rdf-syntax-ns#rest> _:B0c83ab22X2Dd668X2D47a1X2D9e72X2Dc5f247057922 .
_:B32e8d549X2D4b04X2D4ec9X2Daca6X2De401856abf2a <http://www.w3.org/1999/02/22-rdf-syntax-ns#first> "METAR" .
_:B909dd746X2D45deX2D42daX2D9cc2X2D69a07074a11a <http://www.w3.org/2002/07/owl#oneOf> _:B8ebf7271X2Db1a5X2D4b4aX2Daa9cX2D74891abd525a .
<https://data.nasa.gov/ontologies/atmonto/data#airportDepartureRate> <http://www.w3.org/1999/02/22-rdf-syntax-ns#type> <http://www.w3.org/2002/07/owl#DatatypeProperty> .
_:B37b4539cX2Defd3X2D4968X2D8828X2D0816c74be323 <http://www.w3.org/1999/02/22-rdf-syntax-ns#type> <http://www.w3.org/2000/01/rdf-schema#Datatype> .
_:B8d363893X2D1704X2D4f5cX2Db41dX2D528cd0a7a11e <http://www.w3.org/1999/02/22-rdf-syntax-ns#type> <http://www.w3.org/2000/01/rdf-schema#Datatype> .
<https://data.nasa.gov/ontologies/atmonto/data#unlimitedVisibility> <http://www.w3.org/2000/01/rdf-schema#comment> "A binary property indicating whether the visibility conditions are unlimited." .
<https://data.nasa.gov/ontologies/atmonto/data#highWindWITIhourly> <http://www.w3.org/1999/02/22-rdf-syntax-ns#type> <https://data.nasa.gov/ontologies/atmonto/data#WITIproperty> .
<https://data.nasa.gov/ontologies/atmonto/data#dataIntervalEndTime> <http://www.w3.org/2000/01/rdf-schema#label> "data interval end time" .
<https://data.nasa.gov/ontologies/atmonto/data#aspmFlightRules> <http://www.w3.org/1999/02/22-rdf-syntax-ns#type> <http://www.w3.org/2002/07/owl#FunctionalProperty> .
<https://data.nasa.gov/ontologies/atmonto/data#AirportData> <http://www.w3.org/1999/02/22-rdf-syntax-ns#type> <http://www.w3.org/2002/07/owl#Class> .
_:Bc0b04394X2D0f2aX2D495aX2Db48aX2D3909da332a75 <http://www.w3.org/1999/02/22-rdf-syntax-ns#first> "blowing" .
<https://data.nasa.gov/ontologies/atmonto/data#ASPMmeteorologicalCondition> <http://www.w3.org/1999/02/22-rdf-syntax-ns#type> <http://www.w3.org/2002/07/owl#Class> .
<https://data.nasa.gov/ontologies/atmonto/data#RunwayStatusData> <http://www.w3.org/2000/01/rdf-schema#subClassOf> <https://data.nasa.gov/ontologies/atmonto/data#IntervalData> .
<https://data.nasa.gov/ontologies/atmonto/data#SectorFlow> <http://www.w3.org/2000/01/rdf-schema#comment> "A subclass of interval-based data representing the number of aircraft flowing through a sector during some interval of time." .
<https://data.nasa.gov/ontologies/atmonto/data#MetCondition> <http://www.w3.org/1999/02/22-rdf-syntax-ns#type> <http://www.w3.org/2002/07/owl#Class> .
<https://data.nasa.gov/ontologies/atmonto/data#RunwayStatusData> <http://www.w3.org/1999/02/22-rdf-syntax-ns#type> <http://www.w3.org/2002/07/owl#Class> .
<https://data.nasa.gov/ontologies/atmonto/data#runwayStatus> <http://www.w3.org/1999/02/22-rdf-syntax-ns#type> <http://www.w3.org/2002/07/owl#FunctionalProperty> .
<https://data.nasa.gov/ontologies/atmonto/data#hasMETARreport> <http://www.w3.org/2002/07/owl#inverseOf> <https://data.nasa.gov/ontologies/atmonto/data#associatedMETARreportingStation> .
<https://data.nasa.gov/ontologies/atmonto/data#surfaceWindSpeed> <http://www.w3.org/2000/01/rdf-schema#label> "surface wind speed" .
<https://data.nasa.gov/ontologies/atmonto/data#SurfaceWindCondition> <http://www.w3.org/2000/01/rdf-schema#subClassOf> _:B1eed5083X2D3b8dX2D4c08X2Dadf1X2D1eea74c97d5c .
<https://data.nasa.gov/ontologies/atmonto/data#SkyCondition> <http://www.w3.org/2000/01/rdf-schema#label> "Sky condition" .
_:B8c48c716X2D963cX2D4959X2Db42cX2Dbd4a96019db6 <http://www.w3.org/1999/02/22-rdf-syntax-ns#type> <http://www.w3.org/2002/07/owl#Restriction> .
_:B4c7117e3X2Df7ceX2D41b2X2D9a3eX2Deb7cb89d18ff <http://www.w3.org/1999/02/22-rdf-syntax-ns#type> <http://www.w3.org/2002/07/owl#Restriction> .
_:B70d3bda9X2D6639X2D4f0eX2D8d65X2D7c412969f5f8 <http://www.w3.org/1999/02/22-rdf-syntax-ns#type> <http://www.w3.org/2002/07/owl#Restriction> .
<https://data.nasa.gov/ontologies/atmonto/data#AirportData> <http://www.w3.org/2000/01/rdf-schema#subClassOf> <https://data.nasa.gov/ontologies/atmonto/data#IntervalData> .
_:Bf27add84X2D9124X2D4875X2Da3aeX2Dae2ca2ff433f <http://www.w3.org/1999/02/22-rdf-syntax-ns#rest> <http://www.w3.org/1999/02/22-rdf-syntax-ns#nil> .
<https://data.nasa.gov/ontologies/atmonto/data#metConditionProbability> <http://www.w3.org/2000/01/rdf-schema#label> "met condition probability" .
_:Bb0924366X2Da055X2D481bX2Dac3aX2D179dc523f9ab <http://www.w3.org/1999/02/22-rdf-syntax-ns#type> <http://www.w3.org/2002/07/owl#Restriction> .
<http://spinrdf.org/arg#property> <http://www.w3.org/2000/01/rdf-schema#subPropertyOf> <http://spinrdf.org/sp#arg> .
_:Bf17cee5bX2D5755X2D4fb7X2D97ebX2Dec73717e59c7 <http://www.w3.org/1999/02/22-rdf-syntax-ns#rest> _:B3de3ba09X2Dd947X2D476cX2D82b9X2D81581c658d84 .
<https://data.nasa.gov/ontologies/atmonto/data#oagArrivalDelay> <http://www.w3.org/1999/02/22-rdf-syntax-ns#type> <http://www.w3.org/2002/07/owl#FunctionalProperty> .
_:Bfa09714cX2DdcfbX2D4b9eX2D9927X2Dad5d6499080b <http://www.w3.org/2002/07/owl#oneOf> _:B0a10f0e0X2D2618X2D4ab2X2D9d35X2D0f79d669b21e .
<https://data.nasa.gov/ontologies/atmonto/data#hasVisibilityCondition> <http://www.w3.org/2000/01/rdf-schema#domain> <https://data.nasa.gov/ontologies/atmonto/data#MeteorologicalCondition> .
<https://data.nasa.gov/ontologies/atmonto/data#CloudLayer> <http://www.w3.org/2000/01/rdf-schema#subClassOf> <https://data.nasa.gov/ontologies/atmonto/general#SequencedItem> .
<https://data.nasa.gov/ontologies/atmonto/data#arrivalDemand> <http://www.w3.org/1999/02/22-rdf-syntax-ns#type> <http://www.w3.org/2002/07/owl#DatatypeProperty> .
_:B195faeccX2D24b1X2D411bX2D84cdX2D8418f3dd35e1 <http://www.w3.org/2002/07/owl#allValuesFrom> <https://data.nasa.gov/ontologies/atmonto/data#CloudLayer> .
<https://data.nasa.gov/ontologies/atmonto/data#totalAirborneDelay> <http://www.w3.org/2000/01/rdf-schema#label> "total airborne delay" .
<https://data.nasa.gov/ontologies/atmonto/data#etmsArrivals> <http://www.w3.org/1999/02/22-rdf-syntax-ns#type> <http://www.w3.org/2002/07/owl#FunctionalProperty> .
_:B72137fc5X2D81ccX2D4df0X2D8a6fX2D197abe2a15e1 <http://www.w3.org/1999/02/22-rdf-syntax-ns#first> "rain" .
_:Bd2d0bf49X2D78c9X2D45fdX2D868bX2D977560253335 <http://www.w3.org/1999/02/22-rdf-syntax-ns#first> "broken clouds" .
<https://data.nasa.gov/ontologies/atmonto/data#forecastingAirport> <http://www.w3.org/2002/07/owl#inverseOf> <https://data.nasa.gov/ontologies/atmonto/data#hasTAFreport> .
<https://data.nasa.gov/ontologies/atmonto/data#dataIntervalEndTime> <http://www.w3.org/2000/01/rdf-schema#domain> <https://data.nasa.gov/ontologies/atmonto/data#IntervalData> .
<https://data.nasa.gov/ontologies/atmonto/data#dewpoint> <http://www.w3.org/1999/02/22-rdf-syntax-ns#type> <http://www.w3.org/2002/07/owl#DatatypeProperty> .
<https://data.nasa.gov/ontologies/atmonto/data#etmsDepartures> <http://www.w3.org/2000/01/rdf-schema#label> "etms arrivals" .
<https://data.nasa.gov/ontologies/atmonto/data#seaLevelPressure> <http://www.w3.org/2000/01/rdf-schema#comment> "Sea level pressure measured under the associated meteorological conditions." .
<https://data.nasa.gov/ontologies/atmonto/data#surfaceTemperature> <http://www.w3.org/2000/01/rdf-schema#comment> "Surface temperature measured under the associated meteorological conditions." .
<https://data.nasa.gov/ontologies/atmonto/data#ceiling> <http://www.w3.org/2000/01/rdf-schema#domain> <https://data.nasa.gov/ontologies/atmonto/data#SkyCondition> .
<https://data.nasa.gov/ontologies/atmonto/data#hasCloudLayerProfile> <http://www.w3.org/1999/02/22-rdf-syntax-ns#type> <http://www.w3.org/2002/07/owl#ObjectProperty> .
<https://data.nasa.gov/ontologies/atmonto/data#meteorologicalConditionStatus> <http://www.w3.org/1999/02/22-rdf-syntax-ns#type> <http://www.w3.org/2002/07/owl#DatatypeProperty> .
_:B32708683X2D2838X2D496bX2Db4d3X2Da7511750f66b <http://www.w3.org/1999/02/22-rdf-syntax-ns#first> "thunderstorm" .
<https://data.nasa.gov/ontologies/atmonto/data#FixFlow> <http://www.w3.org/2000/01/rdf-schema#subClassOf> <https://data.nasa.gov/ontologies/atmonto/ATM#AircraftFlow> .
<https://data.nasa.gov/ontologies/atmonto/data#runwaySurfaceFriction> <http://www.w3.org/2000/01/rdf-schema#label> "runway surface friction (mu)" .
_:B0c83ab22X2Dd668X2D47a1X2D9e72X2Dc5f247057922 <http://www.w3.org/1999/02/22-rdf-syntax-ns#rest> _:B72bab791X2D0b7cX2D4affX2Dafe5X2Dfdcf7d4a9f3c .
_:Bc9c398a1X2Dd4dcX2D4f15X2D8c3bX2D3e579a6ee161 <http://www.w3.org/1999/02/22-rdf-syntax-ns#type> <http://www.w3.org/2002/07/owl#Restriction> .
_:B872639bbX2D4805X2D484bX2Db538X2D2f7feb5abf7c <http://www.w3.org/1999/02/22-rdf-syntax-ns#type> <http://www.w3.org/2000/01/rdf-schema#Datatype> .
<https://data.nasa.gov/ontologies/atmonto/data#dataIntervalStartTime> <http://www.w3.org/2000/01/rdf-schema#label> "data interval start time" .
_:B8914685fX2D58a2X2D466cX2Daf8bX2D76835b10c083 <http://www.w3.org/2002/07/owl#allValuesFrom> <https://data.nasa.gov/ontologies/atmonto/ATM#NavigationFix> .
_:Bfae980e0X2De811X2D47caX2Da09bX2D9125d95d22d5 <http://www.w3.org/1999/02/22-rdf-syntax-ns#type> <http://www.w3.org/2002/07/owl#Restriction> .
_:B3de3ba09X2Dd947X2D476cX2D82b9X2D81581c658d84 <http://www.w3.org/1999/02/22-rdf-syntax-ns#rest> _:Bf9bf06dbX2D3d8bX2D49ddX2Da012X2Dc9846897439f .
<https://data.nasa.gov/ontologies/atmonto/data#lowVisibilityWITIdaily> <http://www.w3.org/1999/02/22-rdf-syntax-ns#type> <http://www.w3.org/2002/07/owl#FunctionalProperty> .
<https://data.nasa.gov/ontologies/atmonto/data#SkyCondition> <http://www.w3.org/2000/01/rdf-schema#subClassOf> <https://data.nasa.gov/ontologies/atmonto/data#MetCondition> .
<https://data.nasa.gov/ontologies/atmonto/data#hasSurfaceWindCondition> <http://www.w3.org/2000/01/rdf-schema#label> "has surface wind condition" .
<https://data.nasa.gov/ontologies/atmonto/data#edctDepartureHold> <http://www.w3.org/1999/02/22-rdf-syntax-ns#type> <http://www.w3.org/2002/07/owl#FunctionalProperty> .
_:B2b069507X2Dcd7aX2D4102X2DaedbX2Dc5cf54058891 <http://www.w3.org/1999/02/22-rdf-syntax-ns#rest> _:B4fc00ab9X2Dd8e6X2D499dX2D8a46X2D29e6d0403d01 .
<https://data.nasa.gov/ontologies/atmonto/data#windDirectionLower> <http://www.w3.org/2000/01/rdf-schema#range> <http://www.w3.org/2001/XMLSchema#float> .
<https://data.nasa.gov/ontologies/atmonto/data#scheduledDepartures> <http://www.w3.org/1999/02/22-rdf-syntax-ns#type> <http://www.w3.org/2002/07/owl#FunctionalProperty> .
<https://data.nasa.gov/ontologies/atmonto/data#METARreportingStation> <http://www.w3.org/2000/01/rdf-schema#comment> "A weather reporting station that provides sensor data for a METAR report. Many airports are also METAR reporting stations." .
_:B707feedbX2Dbc93X2D4d7aX2D9954X2D1fff0050275c <http://www.w3.org/1999/02/22-rdf-syntax-ns#first> "squalls" .
<https://data.nasa.gov/ontologies/atmonto/data#lowCeilingWITIdaily> <http://www.w3.org/2000/01/rdf-schema#range> <http://www.w3.org/2001/XMLSchema#float> .
_:B31ecb3a2X2D633bX2D4b66X2D8d6eX2De894ef9060a9 <http://www.w3.org/1999/02/22-rdf-syntax-ns#type> <http://www.w3.org/2000/01/rdf-schema#Datatype> .
<https://data.nasa.gov/ontologies/atmonto/data#lowCeilingWITIdaily> <http://www.w3.org/2000/01/rdf-schema#label> "low ceiling WITI daily" .
<https://data.nasa.gov/ontologies/atmonto/data#CloudLayer> <http://www.w3.org/2000/01/rdf-schema#subClassOf> _:Bfae980e0X2De811X2D47caX2Da09bX2D9125d95d22d5 .
<https://data.nasa.gov/ontologies/atmonto/data#surfaceWindDirectionStatus> <http://www.w3.org/2000/01/rdf-schema#range> <http://www.w3.org/2001/XMLSchema#string> .
<https://data.nasa.gov/ontologies/atmonto/data#associatedMETARreportingStation> <http://www.w3.org/1999/02/22-rdf-syntax-ns#type> <http://www.w3.org/2002/07/owl#ObjectProperty> .
_:Bd4a3a582X2D9a9fX2D415aX2D9694X2Dc01bdb73db07 <http://www.w3.org/1999/02/22-rdf-syntax-ns#first> "partial" .
<https://data.nasa.gov/ontologies/atmonto/data#windDirectionUpper> <http://www.w3.org/2000/01/rdf-schema#label> "lower wind direction" .
<https://data.nasa.gov/ontologies/atmonto/data#TAFreport> <http://www.w3.org/2000/01/rdf-schema#label> "TAF report" .
<https://data.nasa.gov/ontologies/atmonto/data#TAFreport> <http://www.w3.org/2000/01/rdf-schema#subClassOf> _:Beb087fa3X2D0133X2D4787X2Dbfb4X2De9880898c35a .
_:B25e3a789X2Da464X2D4768X2Db69fX2D2b31e7ea7980 <http://www.w3.org/1999/02/22-rdf-syntax-ns#first> "closed" .
_:Bdaeec009X2D8f1bX2D49e4X2D9273X2De4481e737d48 <http://www.w3.org/1999/02/22-rdf-syntax-ns#type> <http://www.w3.org/2002/07/owl#Restriction> .
_:B25e3a789X2Da464X2D4768X2Db69fX2D2b31e7ea7980 <http://www.w3.org/1999/02/22-rdf-syntax-ns#rest> <http://www.w3.org/1999/02/22-rdf-syntax-ns#nil> .
<https://data.nasa.gov/ontologies/atmonto/data#RunwayReport> <http://www.w3.org/2000/01/rdf-schema#comment> "A report on runway conditions during a specified interval of time, focusing on runway status (open vs. closed) and surface friction during winter precipitation." .
<https://data.nasa.gov/ontologies/atmonto/data#CloudLayerProfile> <http://www.w3.org/1999/02/22-rdf-syntax-ns#type> <http://www.w3.org/2002/07/owl#Class> .
<https://data.nasa.gov/ontologies/atmonto/data#CloudLayer> <http://www.w3.org/2000/01/rdf-schema#subClassOf> _:Bc9c398a1X2Dd4dcX2D4f15X2D8c3bX2D3e579a6ee161 .
<https://data.nasa.gov/ontologies/atmonto/data#METARreportingStation> <http://www.w3.org/2000/01/rdf-schema#subClassOf> <http://www.w3.org/2002/07/owl#Thing> .
<https://data.nasa.gov/ontologies/atmonto/data#scheduledDepartures> <http://www.w3.org/2000/01/rdf-schema#comment> "Count of scheduled departures. (Most probably from OAG (Official Airline Guide))" .
_:B6df800f8X2D7b0fX2D4f0dX2D96f1X2D3b5354db0cb9 <http://www.w3.org/1999/02/22-rdf-syntax-ns#first> "fixed" .
<https://data.nasa.gov/ontologies/atmonto/data#metConditionProbability> <http://www.w3.org/2000/01/rdf-schema#range> <http://www.w3.org/2001/XMLSchema#float> .
<https://data.nasa.gov/ontologies/atmonto/data#SectorCapacity> <http://www.w3.org/2000/01/rdf-schema#comment> "A subclass of interval-based data representing the maximum number of controllable aircraft flowing through a sector during some interval of time." .
<https://data.nasa.gov/ontologies/atmonto/data#FixFlow> <http://www.w3.org/2000/01/rdf-schema#comment> "A subclass of interval-based data representing the number of aircraft flowing through a fix per some interval of time." .
_:B872639bbX2D4805X2D484bX2Db538X2D2f7feb5abf7c <http://www.w3.org/2002/07/owl#oneOf> _:B8cf977bcX2D2117X2D4e12X2D8f80X2Da16200b800f9 .
<https://data.nasa.gov/ontologies/atmonto/data#metarReportString> <http://www.w3.org/1999/02/22-rdf-syntax-ns#type> <http://www.w3.org/2002/07/owl#DatatypeProperty> .
_:B795569e6X2D13d8X2D47e9X2Dbf2aX2D18d54d334b74 <http://www.w3.org/1999/02/22-rdf-syntax-ns#first> "few clouds" .
<https://data.nasa.gov/ontologies/atmonto/data#lowCeilingWITIhourly> <http://www.w3.org/2000/01/rdf-schema#comment> "The low ceiling weather impacted traffic index (WITI) computed for the airport during the specified timeframe (hourly). WITI is an estimate of the number of flights potentially impacted due to inclement weather based on the scheduled traffic demand for a defined geographic region of the air traffic system (in this case, an airport). If the ceiling at the airport is below a set threshold, then the low ceiling WITI is set to the number of scheduled arrivals for that timeframe." .
<https://data.nasa.gov/ontologies/atmonto/data#forecastingAirport> <http://www.w3.org/2000/01/rdf-schema#comment> "Links to the airport for which the TAF (Terminal Area Forecast) report was compiled." .
_:B4e280221X2Db9eaX2D4d95X2Db31cX2D56635ce48129 <http://www.w3.org/1999/02/22-rdf-syntax-ns#first> "ice pellets" .
<https://data.nasa.gov/ontologies/atmonto/data#associatedMETARreportingStation> <http://www.w3.org/2002/07/owl#inverseOf> <https://data.nasa.gov/ontologies/atmonto/data#hasMETARreport> .
<https://data.nasa.gov/ontologies/atmonto/data#dataIntervalEndDay> <http://www.w3.org/2000/01/rdf-schema#label> "data interval end day" .
_:B528d25d8X2D078fX2D473aX2D8212X2D8f61edadc910 <http://www.w3.org/2002/07/owl#oneOf> _:Bf568bd21X2Df8efX2D464fX2D83abX2D64c80580b5a6 .
<https://data.nasa.gov/ontologies/atmonto/data#weatherIntensity> <http://www.w3.org/1999/02/22-rdf-syntax-ns#type> <http://www.w3.org/2002/07/owl#DatatypeProperty> .
_:B31730194X2Da2aeX2D4755X2D9b1eX2D53849b794653 <http://www.w3.org/1999/02/22-rdf-syntax-ns#rest> <http://www.w3.org/1999/02/22-rdf-syntax-ns#nil> .
<https://data.nasa.gov/ontologies/atmonto/data#metarStationHasPrecipitationSensor> <http://www.w3.org/2000/01/rdf-schema#label> "metar station has precipitation sensor" .
<https://data.nasa.gov/ontologies/atmonto/data#CloudLayerProfile> <http://www.w3.org/2000/01/rdf-schema#subClassOf> _:B9ce34d7bX2De1c2X2D4ef2X2Db0ebX2D036a7350e4a1 .
<https://data.nasa.gov/ontologies/atmonto/data#MeteorologicalCondition> <http://www.w3.org/2000/01/rdf-schema#label> "Meteorological condition" .
<https://data.nasa.gov/ontologies/atmonto/data#cloudType> <http://www.w3.org/2000/01/rdf-schema#label> "cloud type" .
<https://data.nasa.gov/ontologies/atmonto/data#hasSurfaceWindCondition> <http://www.w3.org/2000/01/rdf-schema#comment> "Associates a meteorological condition with the details of the surface wind conditions at the reporting location.." .
_:B4fc00ab9X2Dd8e6X2D499dX2D8a46X2D29e6d0403d01 <http://www.w3.org/1999/02/22-rdf-syntax-ns#rest> _:B95a67ad0X2Dd63eX2D4c80X2Dbfd0X2D73fbdfc02689 .
<https://data.nasa.gov/ontologies/atmonto/data#SectorCapacity> <http://www.w3.org/2000/01/rdf-schema#subClassOf> _:B9381954aX2Dcd8eX2D4902X2DbddbX2D1acd0d5d9150 .
<https://data.nasa.gov/ontologies/atmonto/data#lowCeilingWITIdaily> <http://www.w3.org/2000/01/rdf-schema#domain> <https://data.nasa.gov/ontologies/atmonto/data#AirportData> .
<https://data.nasa.gov/ontologies/atmonto/data#ASPMmeteorologicalCondition> <http://www.w3.org/2000/01/rdf-schema#comment> "Meteorological conditions reported as part of the ASPM hourly airport data. Includes sky, wind, visibility and weather components." .
<https://data.nasa.gov/ontologies/atmonto/data#windDirectionUpper> <http://www.w3.org/2000/01/rdf-schema#comment> "Upper bound (in degrees) of two bounding values describing a variable wind direction." .
_:B4455496dX2Db59fX2D4b8eX2D85b7X2D501844a10d5d <http://www.w3.org/2002/07/owl#oneOf> _:B6df800f8X2D7b0fX2D4f0dX2D96f1X2D3b5354db0cb9 .
_:Becd96e69X2Db94eX2D423dX2Dbc6aX2Da7f962e9579c <http://www.w3.org/2002/07/owl#allValuesFrom> _:B5d4f6142X2Da1f0X2D4072X2Da809X2D852ce5e44b4d .
<https://data.nasa.gov/ontologies/atmonto/data#metarReportType> <http://www.w3.org/2000/01/rdf-schema#range> <http://www.w3.org/2001/XMLSchema#string> .
<https://data.nasa.gov/ontologies/atmonto/data#weatherIntensity> <http://www.w3.org/2000/01/rdf-schema#domain> <https://data.nasa.gov/ontologies/atmonto/data#WeatherCondition> .
<https://data.nasa.gov/ontologies/atmonto/data#oagGateDepartureDelay> <http://www.w3.org/1999/02/22-rdf-syntax-ns#type> <http://www.w3.org/2002/07/owl#FunctionalProperty> .
<https://data.nasa.gov/ontologies/atmonto/data#hasTAFreport> <http://www.w3.org/2002/07/owl#inverseOf> <https://data.nasa.gov/ontologies/atmonto/data#forecastingAirport> .
<https://data.nasa.gov/ontologies/atmonto/data#FixCapacity> <http://www.w3.org/2000/01/rdf-schema#subClassOf> _:Be07d6f98X2D2f29X2D4301X2Db3a4X2D6815000d445d .
_:B528d25d8X2D078fX2D473aX2D8212X2D8f61edadc910 <http://www.w3.org/1999/02/22-rdf-syntax-ns#type> <http://www.w3.org/2000/01/rdf-schema#Datatype> .
<https://data.nasa.gov/ontologies/atmonto/data#rapidityOfWeatherChange> <http://www.w3.org/2000/01/rdf-schema#label> "rapidity of weather change" .
_:B4b2a0e6eX2Df449X2D48edX2D911eX2D9e65301dbe01 <http://www.w3.org/1999/02/22-rdf-syntax-ns#first> "varyingWithinRange" .
<https://data.nasa.gov/ontologies/atmonto/data#limitedVisibilityDistance> <http://www.w3.org/2000/01/rdf-schema#label> "limited visibility distance" .
<https://data.nasa.gov/ontologies/atmonto/data#dataIntervalEndDay> <http://www.w3.org/2000/01/rdf-schema#domain> <https://data.nasa.gov/ontologies/atmonto/data#IntervalData> .
_:B6a6d732fX2D3d9dX2D4ff2X2D9ca9X2Da4c8cfd7aad4 <http://www.w3.org/1999/02/22-rdf-syntax-ns#first> "shallow" .
_:B4b2a0e6eX2Df449X2D48edX2D911eX2D9e65301dbe01 <http://www.w3.org/1999/02/22-rdf-syntax-ns#rest> _:Bb4bc8a40X2Db4beX2D4bcdX2D812eX2D895e29907502 .
<https://data.nasa.gov/ontologies/atmonto/data#runwayStatus> <http://www.w3.org/2000/01/rdf-schema#label> "runway status" .
_:Bc416aebdX2D893bX2D40e2X2Dbbe6X2D9efbb3d57b65 <http://www.w3.org/1999/02/22-rdf-syntax-ns#rest> _:B9c90bf4aX2D2609X2D4c54X2Db976X2D6348225f7b0f .
_:B0a10f0e0X2D2618X2D4ab2X2D9d35X2D0f79d669b21e <http://www.w3.org/1999/02/22-rdf-syntax-ns#rest> _:B1b277598X2Dd23fX2D4f2aX2Db4caX2D14883857655f .
<https://data.nasa.gov/ontologies/atmonto/data#scheduledArrivals> <http://www.w3.org/1999/02/22-rdf-syntax-ns#type> <http://www.w3.org/2002/07/owl#FunctionalProperty> .
<https://data.nasa.gov/ontologies/atmonto/data#lowCeilingWITIhourly> <http://www.w3.org/1999/02/22-rdf-syntax-ns#type> <http://www.w3.org/2002/07/owl#FunctionalProperty> .
<https://data.nasa.gov/ontologies/atmonto/data#topAltitude> <http://www.w3.org/2000/01/rdf-schema#range> <http://www.w3.org/2001/XMLSchema#integer> .
<https://data.nasa.gov/ontologies/atmonto/data#WeatherCondition> <http://www.w3.org/1999/02/22-rdf-syntax-ns#type> <http://www.w3.org/2002/07/owl#Class> .
<https://data.nasa.gov/ontologies/atmonto/data#SectorCapacity> <http://www.w3.org/1999/02/22-rdf-syntax-ns#type> <http://www.w3.org/2002/07/owl#Class> .
<https://data.nasa.gov/ontologies/atmonto/data#TAFmeteorologicalCondition> <http://www.w3.org/2000/01/rdf-schema#subClassOf> _:B049b6b81X2Dfb65X2D461cX2Da676X2D8c02cc81e607 .
_:B8cf977bcX2D2117X2D4e12X2D8f80X2Da16200b800f9 <http://www.w3.org/1999/02/22-rdf-syntax-ns#first> "rapid" .
<https://data.nasa.gov/ontologies/atmonto/data#surfaceWindSpeed> <http://www.w3.org/1999/02/22-rdf-syntax-ns#type> <http://www.w3.org/2002/07/owl#DatatypeProperty> .
_:Becd96e69X2Db94eX2D423dX2Dbc6aX2Da7f962e9579c <http://www.w3.org/1999/02/22-rdf-syntax-ns#type> <http://www.w3.org/2002/07/owl#Restriction> .
_:B6df800f8X2D7b0fX2D4f0dX2D96f1X2D3b5354db0cb9 <http://www.w3.org/1999/02/22-rdf-syntax-ns#rest> _:B4b2a0e6eX2Df449X2D48edX2D911eX2D9e65301dbe01 .
<https://data.nasa.gov/ontologies/atmonto/data#highWindWITIdaily> <http://www.w3.org/1999/02/22-rdf-syntax-ns#type> <http://www.w3.org/2002/07/owl#FunctionalProperty> .
<https://data.nasa.gov/ontologies/atmonto/data#metarReportType> <http://www.w3.org/2000/01/rdf-schema#comment> "METAR report type indicator specifies whether this report is a regularly scheduled hourly report (METAR) or a special unscheduled report (SPECI). SPECIs are issued more frequently than hourly when adverse weather conditions prevail." .
<https://data.nasa.gov/ontologies/atmonto/data#SurfaceWindCondition> <http://www.w3.org/2000/01/rdf-schema#subClassOf> _:B0fea9690X2Da2d4X2D4976X2Daa0cX2D1f5129c61150 .
<https://data.nasa.gov/ontologies/atmonto/data#tafReportString> <http://www.w3.org/2000/01/rdf-schema#domain> <https://data.nasa.gov/ontologies/atmonto/data#TAFreport> .
<https://data.nasa.gov/ontologies/atmonto/data#meteorologicalConditionStatus> <http://www.w3.org/2000/01/rdf-schema#domain> <https://data.nasa.gov/ontologies/atmonto/data#MeteorologicalCondition> .
<https://data.nasa.gov/ontologies/atmonto/data#FixCapacity> <http://www.w3.org/2000/01/rdf-schema#subClassOf> <https://data.nasa.gov/ontologies/atmonto/ATM#AircraftCapacity> .
<https://data.nasa.gov/ontologies/atmonto/data#SurfaceWindCondition> <http://www.w3.org/2000/01/rdf-schema#subClassOf> <https://data.nasa.gov/ontologies/atmonto/data#MetCondition> .
_:Bdaeec009X2D8f1bX2D49e4X2D9273X2De4481e737d48 <http://www.w3.org/2002/07/owl#allValuesFrom> _:B54b31c49X2De49bX2D424aX2D8ca0X2D44c454b589d7 .
_:B195faeccX2D24b1X2D411bX2D84cdX2D8418f3dd35e1 <http://www.w3.org/1999/02/22-rdf-syntax-ns#type> <http://www.w3.org/2002/07/owl#Restriction> .
<https://data.nasa.gov/ontologies/atmonto/data#weatherProximity> <http://www.w3.org/2000/01/rdf-schema#range> <http://www.w3.org/2001/XMLSchema#string> .
_:B9381954aX2Dcd8eX2D4902X2DbddbX2D1acd0d5d9150 <http://www.w3.org/2002/07/owl#onProperty> <https://data.nasa.gov/ontologies/atmonto/ATM#flowMeasurementRegion> .
<https://data.nasa.gov/ontologies/atmonto/data#airportArrivalRate> <http://www.w3.org/1999/02/22-rdf-syntax-ns#type> <http://www.w3.org/2002/07/owl#DatatypeProperty> .
<https://data.nasa.gov/ontologies/atmonto/data> <http://www.w3.org/1999/02/22-rdf-syntax-ns#type> <http://www.w3.org/2002/07/owl#Ontology> .
_:B5ba85c47X2D6e17X2D4e4bX2Dba3eX2D2d76ff83a78e <http://www.w3.org/1999/02/22-rdf-syntax-ns#first> "sandstorm" .
<https://data.nasa.gov/ontologies/atmonto/data#hasCloudLayerProfile> <http://www.w3.org/2000/01/rdf-schema#comment> "Links a sky condition to a representation of the cloud layers present." .
<https://data.nasa.gov/ontologies/atmonto/data#metarStationHasPrecipitationSensor> <http://www.w3.org/1999/02/22-rdf-syntax-ns#type> <http://www.w3.org/2002/07/owl#DatatypeProperty> .
_:B14b9247fX2D1e6fX2D4a13X2Da9a1X2D0429fef1984c <http://www.w3.org/1999/02/22-rdf-syntax-ns#rest> _:B2b069507X2Dcd7aX2D4102X2DaedbX2Dc5cf54058891 .
<https://data.nasa.gov/ontologies/atmonto/data#dewpoint> <http://www.w3.org/2000/01/rdf-schema#domain> <https://data.nasa.gov/ontologies/atmonto/data#MeteorologicalCondition> .
<https://data.nasa.gov/ontologies/atmonto/data#hasTAFreport> <http://www.w3.org/2000/01/rdf-schema#domain> <https://data.nasa.gov/ontologies/atmonto/NAS#Airport> .
<https://data.nasa.gov/ontologies/atmonto/data#surfaceWindDirectionStatus> <http://www.w3.org/2000/01/rdf-schema#domain> <https://data.nasa.gov/ontologies/atmonto/data#SurfaceWindCondition> .
<https://data.nasa.gov/ontologies/atmonto/data#RunwayStatusData> <http://www.w3.org/2000/01/rdf-schema#comment> "This class describes a temporally-dependent set of data about the operating status of a physical runway." .
_:Bed0be29bX2D57deX2D4f76X2Db3c4X2Dc697a028d67d <http://www.w3.org/2002/07/owl#onProperty> <https://data.nasa.gov/ontologies/atmonto/data#aspmFlightRules> .
_:Bb855cbbbX2De2e6X2D4090X2D875cX2D7250d013f1b5 <http://www.w3.org/2002/07/owl#allValuesFrom> _:B250d7406X2D0509X2D47c9X2Dac7aX2Daee37a2553ab .
<https://data.nasa.gov/ontologies/atmonto/data#topAltitude> <http://www.w3.org/2000/01/rdf-schema#comment> "The top altitude of a homogenous cloud layer." .
_:B72bab791X2D0b7cX2D4affX2Dafe5X2Dfdcf7d4a9f3c <http://www.w3.org/1999/02/22-rdf-syntax-ns#first> "haze" .
_:B805beb7dX2De0a6X2D4d92X2Dbc13X2Dff6a40662f87 <http://www.w3.org/2002/07/owl#cardinality> "1"^^<http://www.w3.org/2001/XMLSchema#nonNegativeInteger> .
_:B32708683X2D2838X2D496bX2Db4d3X2Da7511750f66b <http://www.w3.org/1999/02/22-rdf-syntax-ns#rest> _:B41ecb1f3X2D60e9X2D435eX2Dad0eX2D1d88e2ff9118 .
<https://data.nasa.gov/ontologies/atmonto/data#runwayReportedOn> <http://www.w3.org/2000/01/rdf-schema#label> "runway reported on" .
<https://data.nasa.gov/ontologies/atmonto/data#weatherQualifier> <http://www.w3.org/1999/02/22-rdf-syntax-ns#type> <http://www.w3.org/2002/07/owl#DatatypeProperty> .
<https://data.nasa.gov/ontologies/atmonto/data#windDirectionFixed> <http://www.w3.org/2000/01/rdf-schema#range> <http://www.w3.org/2001/XMLSchema#float> .
<https://data.nasa.gov/ontologies/atmonto/data#hasCloudLayerProfile> <http://www.w3.org/2000/01/rdf-schema#range> <https://data.nasa.gov/ontologies/atmonto/data#CloudLayerProfile> .
<https://data.nasa.gov/ontologies/atmonto/data#arrivalDemand> <http://www.w3.org/2000/01/rdf-schema#comment> "The number of aircraft intending to arrive at an airport during the specified time period." .
<https://data.nasa.gov/ontologies/atmonto/data#metarStationHasPrecipitationSensor> <http://www.w3.org/2000/01/rdf-schema#comment> "A boolean value indicating whether the reporting METAR station has a precipitation sensor." .
<https://data.nasa.gov/ontologies/atmonto/data#cloudType> <http://www.w3.org/2000/01/rdf-schema#comment> "For a given homogeneous cloud layer, the type of cloud present: towering cumulus, cumulonimbus, altocumulus castellanus." .
<http://spinrdf.org/arg#property> <http://www.w3.org/1999/02/22-rdf-syntax-ns#type> <http://www.w3.org/1999/02/22-rdf-syntax-ns#Property> .
_:B049b6b81X2Dfb65X2D461cX2Da676X2D8c02cc81e607 <http://www.w3.org/2002/07/owl#onProperty> <https://data.nasa.gov/ontologies/atmonto/data#rapidityOfWeatherChange> .
_:B7c0bd641X2Dd3c5X2D4dfbX2Db8faX2D67cf310a0048 <http://www.w3.org/1999/02/22-rdf-syntax-ns#first> "ice crystals" .
<https://data.nasa.gov/ontologies/atmonto/data#baseAltitude> <http://www.w3.org/2000/01/rdf-schema#comment> "For a given homogeonous cloud layer, this is the lowest altitude." .
<https://data.nasa.gov/ontologies/atmonto/data#dataIntervalStartDay> <http://www.w3.org/2000/01/rdf-schema#label> "data interval start day" .
_:Bb4bc8a40X2Db4beX2D4bcdX2D812eX2D895e29907502 <http://www.w3.org/1999/02/22-rdf-syntax-ns#first> "variable" .
<https://data.nasa.gov/ontologies/atmonto/data#rapidityOfWeatherChange> <http://www.w3.org/1999/02/22-rdf-syntax-ns#type> <http://www.w3.org/2002/07/owl#DatatypeProperty> .
<https://data.nasa.gov/ontologies/atmonto/data#weatherQualifier> <http://www.w3.org/2000/01/rdf-schema#domain> <https://data.nasa.gov/ontologies/atmonto/data#WeatherCondition> .
<https://data.nasa.gov/ontologies/atmonto/data#hasTAFreport> <http://www.w3.org/2000/01/rdf-schema#range> <https://data.nasa.gov/ontologies/atmonto/data#TAFreport> .
<https://data.nasa.gov/ontologies/atmonto/data#edctDepartureHold> <http://www.w3.org/2000/01/rdf-schema#comment> "EDCT (Estimated Departure Clearance Time) hold minutes at other airports departing this airport." .
_:B1b277598X2Dd23fX2D4f2aX2Db4caX2D14883857655f <http://www.w3.org/1999/02/22-rdf-syntax-ns#first> "cumulonimbus" .
<https://data.nasa.gov/ontologies/atmonto/data#dataIntervalStartTime> <http://www.w3.org/2000/01/rdf-schema#comment> "For temporally-dependent data, the starting time of the data's period of validity." .
<https://data.nasa.gov/ontologies/atmonto/data#windDirectionLower> <http://www.w3.org/2000/01/rdf-schema#label> "lower wind direction" .
<https://data.nasa.gov/ontologies/atmonto/data#TAFmeteorologicalCondition> <http://www.w3.org/2000/01/rdf-schema#label> "TAF meteorological condition" .
_:Beb087fa3X2D0133X2D4787X2Dbfb4X2De9880898c35a <http://www.w3.org/1999/02/22-rdf-syntax-ns#type> <http://www.w3.org/2002/07/owl#Restriction> .
<https://data.nasa.gov/ontologies/atmonto/data#hasWeatherCondition> <http://www.w3.org/2000/01/rdf-schema#domain> <https://data.nasa.gov/ontologies/atmonto/data#MeteorologicalCondition> .
<https://data.nasa.gov/ontologies/atmonto/data#windDirectionUpper> <http://www.w3.org/2000/01/rdf-schema#range> <http://www.w3.org/2001/XMLSchema#float> .
<https://data.nasa.gov/ontologies/atmonto/data#runwayVisibleRange> <http://www.w3.org/1999/02/22-rdf-syntax-ns#type> <http://www.w3.org/2002/07/owl#ObjectProperty> .
