<http://def.seegrid.csiro.au/isotc211/iso19103/2005/basic#DateTime>
        a       <http://www.w3.org/2000/01/rdf-schema#Datatype> ;
        <http://www.w3.org/2000/01/rdf-schema#comment>
                "Temporal position expressed as a time and date" ;
        <http://www.w3.org/2000/01/rdf-schema#isDefinedBy>
                <http://def.seegrid.csiro.au/isotc211/iso19103/2005/basic> ;
        <http://www.w3.org/2000/01/rdf-schema#label>
                "dateTime" ;
        <http://www.w3.org/2002/07/owl#equivalentClass>
                <http://www.w3.org/2001/XMLSchema#dateTime> .

<http://def.seegrid.csiro.au/isotc211/iso19103/2005/basic#Angle>
        a       <http://www.w3.org/2002/07/owl#Class> ;
        <http://www.w3.org/2000/01/rdf-schema#comment>
                "measure of arc length or rotation" ;
        <http://www.w3.org/2000/01/rdf-schema#isDefinedBy>
                <http://def.seegrid.csiro.au/isotc211/iso19103/2005/basic> ;
        <http://www.w3.org/2000/01/rdf-schema#label>
                "Angle" ;
        <http://www.w3.org/2000/01/rdf-schema#subClassOf>
                <http://def.seegrid.csiro.au/isotc211/iso19103/2005/basic#Measure> .

<http://def.seegrid.csiro.au/isotc211/iso19103/2005/basic#Acceleration>
        a       <http://www.w3.org/2002/07/owl#Class> ;
        <http://www.w3.org/2000/01/rdf-schema#comment>
                "Measure of rate of change of velocity" ;
        <http://www.w3.org/2000/01/rdf-schema#isDefinedBy>
                <http://def.seegrid.csiro.au/isotc211/iso19103/2005/basic> ;
        <http://www.w3.org/2000/01/rdf-schema#label>
                "Acceleration"@en ;
        <http://www.w3.org/2000/01/rdf-schema#subClassOf>
                <http://def.seegrid.csiro.au/isotc211/iso19103/2005/basic#Measure> .

<http://def.seegrid.csiro.au/isotc211/iso19103/2005/basic#CharacterString>
        a       <http://www.w3.org/2000/01/rdf-schema#Datatype> ;
        <http://www.w3.org/2000/01/rdf-schema#comment>
                "sequence of characters" ;
        <http://www.w3.org/2000/01/rdf-schema#isDefinedBy>
                <http://def.seegrid.csiro.au/isotc211/iso19103/2005/basic> ;
        <http://www.w3.org/2000/01/rdf-schema#label>
                "characterString" ;
        <http://www.w3.org/2002/07/owl#equivalentClass>
                <http://www.w3.org/2001/XMLSchema#string> .

<http://def.seegrid.csiro.au/isotc211/iso19103/2005/basic>
        a       <http://purl.org/vocommons/voaf#Vocabulary> , <http://www.w3.org/2002/07/owl#Ontology> ;
        <http://www.w3.org/2000/01/rdf-schema#comment>
                "An OWL representation of (some of) the basic types described in ISO 19103:2005, required as primitives in other ontologies based on ISO 19100 series standards. \r\n\r\nThis vocabulary is provisional, pending finalization of ISO 19150-2.\r\n\r\nThe URI stem http://def.seegrid.csiro.au/isotc211/ is temporary. The vocabulary is expected to be ultimately published in the domain http://def.isotc211.org/" ;
        <http://purl.org/dc/elements/1.1/creator>
                "Simon Jonathan David COX, CSIRO Australia" ;
        <http://purl.org/dc/elements/1.1/description>
                "An OWL representation of (some of) the basic types described in ISO 19103:2005, required as primitives in other ontologies based on ISO 19100 series standards. " ;
        <http://purl.org/dc/elements/1.1/rights>
                "Copyright Â© 2012-2013 CSIRO" ;
        <http://purl.org/dc/elements/1.1/source>
                "ISO 19103:2005" ;
        <http://purl.org/dc/elements/1.1/title>
                "OWL representation of ISO 19103 (Basic types package)" ;
        <http://purl.org/dc/terms/created>
                "2011-01-01T00:00:00"^^<http://www.w3.org/2001/XMLSchema#dateTime> ;
        <http://purl.org/dc/terms/hasPart>
                <http://def.seegrid.csiro.au/isotc211/iso19103/2005/basic#dimension> , <http://def.seegrid.csiro.au/isotc211/iso19103/2005/basic#uom> , <http://def.seegrid.csiro.au/isotc211/iso19103/2005/basic#ordinates> , <http://def.seegrid.csiro.au/isotc211/iso19103/2005/basic#value> , <http://def.seegrid.csiro.au/isotc211/iso19103/2005/basic#Decimal> , <http://def.seegrid.csiro.au/isotc211/iso19103/2005/basic#Length> , <http://def.seegrid.csiro.au/isotc211/iso19103/2005/basic#Real> , <http://def.seegrid.csiro.au/isotc211/iso19103/2005/basic#Area> , <http://def.seegrid.csiro.au/isotc211/iso19103/2005/basic#LocalName> , <http://def.seegrid.csiro.au/isotc211/iso19103/2005/basic#Number> , <http://def.seegrid.csiro.au/isotc211/iso19103/2005/basic#Measure> , <http://def.seegrid.csiro.au/isotc211/iso19103/2005/basic#Volume> , <http://def.seegrid.csiro.au/isotc211/iso19103/2005/basic#Date> , <http://def.seegrid.csiro.au/isotc211/iso19103/2005/basic#DateTime> , <http://def.seegrid.csiro.au/isotc211/iso19103/2005/basic#Distance> , <http://def.seegrid.csiro.au/isotc211/iso19103/2005/basic#Time> , <http://def.seegrid.csiro.au/isotc211/iso19103/2005/basic#Currency> , <http://def.seegrid.csiro.au/isotc211/iso19103/2005/basic#measure> , <http://def.seegrid.csiro.au/isotc211/iso19103/2005/basic#Acceleration> , <http://def.seegrid.csiro.au/isotc211/iso19103/2005/basic#CharacterString> , <http://def.seegrid.csiro.au/isotc211/iso19103/2005/basic#Mass> , <http://def.seegrid.csiro.au/isotc211/iso19103/2005/basic#Angle> , <http://def.seegrid.csiro.au/isotc211/iso19103/2005/basic#Velocity> , <http://def.seegrid.csiro.au/isotc211/iso19103/2005/basic#AngularVelocity> , <http://def.seegrid.csiro.au/isotc211/iso19103/2005/basic#UnitOfMeasure> , <http://def.seegrid.csiro.au/isotc211/iso19103/2005/basic#Integer> , <http://def.seegrid.csiro.au/isotc211/iso19103/2005/basic#Weight> , <http://def.seegrid.csiro.au/isotc211/iso19103/2005/basic#Vector> , <http://def.seegrid.csiro.au/isotc211/iso19103/2005/basic#Boolean> , <http://def.seegrid.csiro.au/isotc211/iso19103/2005/basic#Scale> ;
        <http://purl.org/dc/terms/license>
                <http://creativecommons.org/licenses/by/3.0/> ;
        <http://purl.org/dc/terms/modified>
                "2013-11-14T00:00:00"^^<http://www.w3.org/2001/XMLSchema#dateTime> ;
        <http://purl.org/vocab/vann/preferredNamespacePrefix>
                "basic" ;
        <http://purl.org/vocab/vann/preferredNamespaceUri>
                <http://def.seegrid.csiro.au/isotc211/iso19103/2005/basic#> ;
        <http://www.w3.org/2002/07/owl#imports>
                <http://purl.org/dc/elements/1.1/> ;
        <http://www.w3.org/2002/07/owl#priorVersion>
                <https://www.seegrid.csiro.au/subversion/xmml/ontologies/tags/201305/ISOTC211/HM/basic.rdf> ;
        <http://www.w3.org/2002/07/owl#versionIRI>
                <https://www.seegrid.csiro.au/subversion/xmml/ontologies/tags/201311/ISOTC211/HM/basic.rdf> .

<http://def.seegrid.csiro.au/isotc211/iso19103/2005/basic#ordinates>
        a       <http://www.w3.org/2002/07/owl#DatatypeProperty> ;
        <http://www.w3.org/2000/01/rdf-schema#comment>
                "Numerical values of the vector components" ;
        <http://www.w3.org/2000/01/rdf-schema#domain>
                <http://def.seegrid.csiro.au/isotc211/iso19103/2005/basic#Vector> ;
        <http://www.w3.org/2000/01/rdf-schema#isDefinedBy>
                <http://def.seegrid.csiro.au/isotc211/iso19103/2005/basic> ;
        <http://www.w3.org/2000/01/rdf-schema#label>
                "ordinates" .

<http://def.seegrid.csiro.au/isotc211/iso19103/2005/basic#Integer>
        a       <http://www.w3.org/2000/01/rdf-schema#Datatype> ;
        <http://www.w3.org/2000/01/rdf-schema#comment>
                "An exact integer value, with no fractional part. " ;
        <http://www.w3.org/2000/01/rdf-schema#isDefinedBy>
                <http://def.seegrid.csiro.au/isotc211/iso19103/2005/basic> ;
        <http://www.w3.org/2000/01/rdf-schema#label>
                "integer" ;
        <http://www.w3.org/2002/07/owl#equivalentClass>
                <http://www.w3.org/2001/XMLSchema#integer> .

<http://def.seegrid.csiro.au/isotc211/iso19103/2005/basic#Volume>
        a       <http://www.w3.org/2002/07/owl#Class> ;
        <http://www.w3.org/2000/01/rdf-schema#comment>
                "Measure of 3-D extent" ;
        <http://www.w3.org/2000/01/rdf-schema#isDefinedBy>
                <http://def.seegrid.csiro.au/isotc211/iso19103/2005/basic> ;
        <http://www.w3.org/2000/01/rdf-schema#label>
                "Volume" ;
        <http://www.w3.org/2000/01/rdf-schema#subClassOf>
                <http://def.seegrid.csiro.au/isotc211/iso19103/2005/basic#Measure> ;
        <http://www.w3.org/2004/02/skos/core#notation>
                "Volume"^^<http://def.seegrid.csiro.au/isotc211/iso19103/2005/basic#ISOClassName> .

<http://def.seegrid.csiro.au/isotc211/iso19103/2005/basic#UnitOfMeasure>
        a       <http://www.w3.org/2002/07/owl#Class> ;
        <http://www.w3.org/2000/01/rdf-schema#comment>
                "Scale for a number describing size or extent" ;
        <http://www.w3.org/2000/01/rdf-schema#isDefinedBy>
                <http://def.seegrid.csiro.au/isotc211/iso19103/2005/basic> ;
        <http://www.w3.org/2000/01/rdf-schema#label>
                "Unit of measure" ;
        <http://www.w3.org/2002/07/owl#disjointWith>
                <http://def.seegrid.csiro.au/isotc211/iso19103/2005/basic#Measure> .

<http://def.seegrid.csiro.au/isotc211/iso19103/2005/basic#Currency>
        a       <http://www.w3.org/2002/07/owl#Class> ;
        <http://www.w3.org/2000/01/rdf-schema#comment>
                "Measure of exchange value" ;
        <http://www.w3.org/2000/01/rdf-schema#isDefinedBy>
                <http://def.seegrid.csiro.au/isotc211/iso19103/2005/basic> ;
        <http://www.w3.org/2000/01/rdf-schema#label>
                "Currency" ;
        <http://www.w3.org/2000/01/rdf-schema#subClassOf>
                <http://def.seegrid.csiro.au/isotc211/iso19103/2005/basic#Measure> .

<http://def.seegrid.csiro.au/isotc211/iso19103/2005/basic#Vector>
        a       <http://www.w3.org/2002/07/owl#Class> ;
        <http://www.w3.org/2000/01/rdf-schema#comment>
                "A vector is a sequence of a fixed length of Numbers. Normally, the numbers represent some measures, and thus vectors are often used where records of Numbers would be more appropriate. In geometry for example, direct positions are given by undistinguished coordinate vectors, which can be interpreted through the use of coordinate reference systems." ;
        <http://www.w3.org/2000/01/rdf-schema#isDefinedBy>
                <http://def.seegrid.csiro.au/isotc211/iso19103/2005/basic> ;
        <http://www.w3.org/2000/01/rdf-schema#label>
                "Vector" ;
        <http://www.w3.org/2000/01/rdf-schema#subClassOf>
                [ a       <http://www.w3.org/2002/07/owl#Restriction> ;
                  <http://www.w3.org/2002/07/owl#cardinality>
                          "1"^^<http://www.w3.org/2001/XMLSchema#nonNegativeInteger> ;
                  <http://www.w3.org/2002/07/owl#onProperty>
                          <http://def.seegrid.csiro.au/isotc211/iso19103/2005/basic#dimension>
                ] ;
        <http://www.w3.org/2000/01/rdf-schema#subClassOf>
                [ a       <http://www.w3.org/2002/07/owl#Restriction> ;
                  <http://www.w3.org/2002/07/owl#cardinality>
                          "1"^^<http://www.w3.org/2001/XMLSchema#nonNegativeInteger> ;
                  <http://www.w3.org/2002/07/owl#onProperty>
                          <http://def.seegrid.csiro.au/isotc211/iso19103/2005/basic#ordinates>
                ] .

<http://def.seegrid.csiro.au/isotc211/iso19103/2005/basic#Measure>
        a       <http://www.w3.org/2002/07/owl#Class> ;
        <http://www.w3.org/2000/01/rdf-schema#comment>
                "Scaled number" ;
        <http://www.w3.org/2000/01/rdf-schema#isDefinedBy>
                <http://def.seegrid.csiro.au/isotc211/iso19103/2005/basic> ;
        <http://www.w3.org/2000/01/rdf-schema#label>
                "Measure"@en , "Mesure"@fr ;
        <http://www.w3.org/2000/01/rdf-schema#subClassOf>
                [ a       <http://www.w3.org/2002/07/owl#Restriction> ;
                  <http://www.w3.org/2002/07/owl#cardinality>
                          "1"^^<http://www.w3.org/2001/XMLSchema#nonNegativeInteger> ;
                  <http://www.w3.org/2002/07/owl#onProperty>
                          <http://def.seegrid.csiro.au/isotc211/iso19103/2005/basic#value>
                ] ;
        <http://www.w3.org/2000/01/rdf-schema#subClassOf>
                [ a       <http://www.w3.org/2002/07/owl#Restriction> ;
                  <http://www.w3.org/2002/07/owl#cardinality>
                          "1"^^<http://www.w3.org/2001/XMLSchema#nonNegativeInteger> ;
                  <http://www.w3.org/2002/07/owl#onProperty>
                          <http://def.seegrid.csiro.au/isotc211/iso19103/2005/basic#uom>
                ] ;
        <http://www.w3.org/2002/07/owl#disjointWith>
                <http://def.seegrid.csiro.au/isotc211/iso19103/2005/basic#UnitOfMeasure> .

<http://def.seegrid.csiro.au/isotc211/iso19103/2005/basic#Boolean>
        a       <http://www.w3.org/2000/01/rdf-schema#Datatype> ;
        <http://www.w3.org/2000/01/rdf-schema#comment>
                "Truth value. Most valuable in the predicate calculus, where items are either True or False, unless they are ill formed." ;
        <http://www.w3.org/2000/01/rdf-schema#isDefinedBy>
                <http://def.seegrid.csiro.au/isotc211/iso19103/2005/basic> ;
        <http://www.w3.org/2000/01/rdf-schema#label>
                "boolean" ;
        <http://www.w3.org/2002/07/owl#equivalentClass>
                <http://www.w3.org/2001/XMLSchema#boolean> .

<http://def.seegrid.csiro.au/isotc211/iso19103/2005/basic#Distance>
        a       <http://www.w3.org/2002/07/owl#Class> ;
        <http://www.w3.org/2000/01/rdf-schema#comment>
                "Measure of spatial separation along some 1-D manifold" ;
        <http://www.w3.org/2000/01/rdf-schema#isDefinedBy>
                <http://def.seegrid.csiro.au/isotc211/iso19103/2005/basic> ;
        <http://www.w3.org/2000/01/rdf-schema#label>
                "Distance" ;
        <http://www.w3.org/2000/01/rdf-schema#subClassOf>
                <http://def.seegrid.csiro.au/isotc211/iso19103/2005/basic#Length> .

<http://def.seegrid.csiro.au/isotc211/iso19103/2005/basic#uom>
        a       <http://www.w3.org/2002/07/owl#ObjectProperty> ;
        <http://www.w3.org/2000/01/rdf-schema#comment>
                "The value of this property designates the units of measure or scale for the quantity" ;
        <http://www.w3.org/2000/01/rdf-schema#isDefinedBy>
                <http://def.seegrid.csiro.au/isotc211/iso19103/2005/basic> ;
        <http://www.w3.org/2000/01/rdf-schema#label>
                "unit of measure" ;
        <http://www.w3.org/2000/01/rdf-schema#range>
                <http://def.seegrid.csiro.au/isotc211/iso19103/2005/basic#UnitOfMeasure> .

<http://def.seegrid.csiro.au/isotc211/iso19103/2005/basic#value>
        a       <http://www.w3.org/2002/07/owl#DatatypeProperty> ;
        <http://www.w3.org/2000/01/rdf-schema#comment>
                "The value of this property is a number" ;
        <http://www.w3.org/2000/01/rdf-schema#isDefinedBy>
                <http://def.seegrid.csiro.au/isotc211/iso19103/2005/basic> ;
        <http://www.w3.org/2000/01/rdf-schema#label>
                "value" ;
        <http://www.w3.org/2000/01/rdf-schema#range>
                <http://def.seegrid.csiro.au/isotc211/iso19103/2005/basic#Number> ;
        <http://www.w3.org/2000/01/rdf-schema#subPropertyOf>
                <http://www.w3.org/1999/02/22-rdf-syntax-ns#value> .

<http://def.seegrid.csiro.au/isotc211/iso19103/2005/basic#Weight>
        a       <http://www.w3.org/2002/07/owl#Class> ;
        <http://www.w3.org/2000/01/rdf-schema#comment>
                "Measure of force due to a mass in a specific gravitational field" ;
        <http://www.w3.org/2000/01/rdf-schema#isDefinedBy>
                <http://def.seegrid.csiro.au/isotc211/iso19103/2005/basic> ;
        <http://www.w3.org/2000/01/rdf-schema#label>
                "Weight" ;
        <http://www.w3.org/2000/01/rdf-schema#subClassOf>
                <http://def.seegrid.csiro.au/isotc211/iso19103/2005/basic#Measure> .

<http://def.seegrid.csiro.au/isotc211/iso19103/2005/basic#Length>
        a       <http://www.w3.org/2002/07/owl#Class> ;
        <http://www.w3.org/2000/01/rdf-schema#comment>
                "Measure of 1-D extent" ;
        <http://www.w3.org/2000/01/rdf-schema#isDefinedBy>
                <http://def.seegrid.csiro.au/isotc211/iso19103/2005/basic> ;
        <http://www.w3.org/2000/01/rdf-schema#label>
                "Length" ;
        <http://www.w3.org/2000/01/rdf-schema#subClassOf>
                <http://def.seegrid.csiro.au/isotc211/iso19103/2005/basic#Measure> .

<http://def.seegrid.csiro.au/isotc211/iso19103/2005/basic#Area>
        a       <http://www.w3.org/2002/07/owl#Class> ;
        <http://www.w3.org/2000/01/rdf-schema#comment>
                "Measure of 2-D extent" ;
        <http://www.w3.org/2000/01/rdf-schema#isDefinedBy>
                <http://def.seegrid.csiro.au/isotc211/iso19103/2005/basic> ;
        <http://www.w3.org/2000/01/rdf-schema#label>
                "Area" ;
        <http://www.w3.org/2000/01/rdf-schema#subClassOf>
                <http://def.seegrid.csiro.au/isotc211/iso19103/2005/basic#Measure> .

<http://def.seegrid.csiro.au/isotc211/iso19103/2005/basic#LocalName>
        a       <http://www.w3.org/2000/01/rdf-schema#Datatype> ;
        <http://www.w3.org/2000/01/rdf-schema#comment>
                "Name in some local context" ;
        <http://www.w3.org/2000/01/rdf-schema#isDefinedBy>
                <http://def.seegrid.csiro.au/isotc211/iso19103/2005/basic> ;
        <http://www.w3.org/2000/01/rdf-schema#label>
                "localName" ;
        <http://www.w3.org/2002/07/owl#equivalentClass>
                <http://www.w3.org/2001/XMLSchema#NCName> .

<http://def.seegrid.csiro.au/isotc211/iso19103/2005/basic#Number>
        a       <http://www.w3.org/2000/01/rdf-schema#Datatype> ;
        <http://www.w3.org/2000/01/rdf-schema#comment>
                "Note: integer is a specialization of decimal" , "The set of numbers" ;
        <http://www.w3.org/2000/01/rdf-schema#isDefinedBy>
                <http://def.seegrid.csiro.au/isotc211/iso19103/2005/basic> ;
        <http://www.w3.org/2000/01/rdf-schema#label>
                "Number" ;
        <http://www.w3.org/2002/07/owl#equivalentClass>
                [ a       <http://www.w3.org/2002/07/owl#Class> ;
                  <http://www.w3.org/2002/07/owl#unionOf>
                          ( <http://www.w3.org/2001/XMLSchema#double> <http://www.w3.org/2001/XMLSchema#float> <http://www.w3.org/2001/XMLSchema#decimal> <http://www.w3.org/2001/XMLSchema#integer> )
                ] .

<http://def.seegrid.csiro.au/isotc211/iso19103/2005/basic#Date>
        a       <http://www.w3.org/2000/01/rdf-schema#Datatype> ;
        <http://www.w3.org/2000/01/rdf-schema#comment>
                "Temporal position expressed with precision of days" ;
        <http://www.w3.org/2000/01/rdf-schema#isDefinedBy>
                <http://def.seegrid.csiro.au/isotc211/iso19103/2005/basic> ;
        <http://www.w3.org/2000/01/rdf-schema#label>
                "date" ;
        <http://www.w3.org/2002/07/owl#equivalentClass>
                <http://www.w3.org/2001/XMLSchema#date> .

<http://def.seegrid.csiro.au/isotc211/iso19103/2005/basic#AngularVelocity>
        a       <http://www.w3.org/2002/07/owl#Class> ;
        <http://www.w3.org/2000/01/rdf-schema#comment>
                "Measure of rate of change of angular position" ;
        <http://www.w3.org/2000/01/rdf-schema#isDefinedBy>
                <http://def.seegrid.csiro.au/isotc211/iso19103/2005/basic> ;
        <http://www.w3.org/2000/01/rdf-schema#label>
                "AngularVelocity" ;
        <http://www.w3.org/2000/01/rdf-schema#subClassOf>
                <http://def.seegrid.csiro.au/isotc211/iso19103/2005/basic#Measure> .

<http://def.seegrid.csiro.au/isotc211/iso19103/2005/basic#Real>
        a       <http://www.w3.org/2000/01/rdf-schema#Datatype> ;
        <http://www.w3.org/2000/01/rdf-schema#comment>
                "The common binary Real finite implementation using base 2. Since such reals can approximate any measure where absolute accuracy is not possible, this form of numeric is most often used for measures. In cases were absolute accuracy is needed, such as currencies, then a decimal representation may be preferred (assuming the currency is decimal, such as the US dollar, British pound, etc.). Where there are no subunits possible, Integer numbers may be preferred.  \n\nCan be thought of as an integer part followed by a fractional part given in multiples of powers of 1/2 (halves)." ;
        <http://www.w3.org/2000/01/rdf-schema#isDefinedBy>
                <http://def.seegrid.csiro.au/isotc211/iso19103/2005/basic> ;
        <http://www.w3.org/2000/01/rdf-schema#label>
                "realNumber" ;
        <http://www.w3.org/2002/07/owl#equivalentClass>
                [ a       <http://www.w3.org/2000/01/rdf-schema#Datatype> ;
                  <http://www.w3.org/2002/07/owl#unionOf>
                          ( <http://www.w3.org/2001/XMLSchema#double> <http://www.w3.org/2001/XMLSchema#float> )
                ] .

<http://def.seegrid.csiro.au/isotc211/iso19103/2005/basic#Scale>
        a       <http://www.w3.org/2002/07/owl#Class> ;
        <http://www.w3.org/2000/01/rdf-schema#comment>
                "Factor by which a representation should be magnified to match the geomstric size of the thing it represents." ;
        <http://www.w3.org/2000/01/rdf-schema#isDefinedBy>
                <http://def.seegrid.csiro.au/isotc211/iso19103/2005/basic> ;
        <http://www.w3.org/2000/01/rdf-schema#label>
                "Scale" ;
        <http://www.w3.org/2000/01/rdf-schema#subClassOf>
                <http://def.seegrid.csiro.au/isotc211/iso19103/2005/basic#Measure> .

<http://def.seegrid.csiro.au/isotc211/iso19103/2005/basic#dimension>
        a       <http://www.w3.org/2002/07/owl#DatatypeProperty> ;
        <http://www.w3.org/2000/01/rdf-schema#comment>
                "Number of components in the vector" ;
        <http://www.w3.org/2000/01/rdf-schema#domain>
                <http://def.seegrid.csiro.au/isotc211/iso19103/2005/basic#Vector> ;
        <http://www.w3.org/2000/01/rdf-schema#isDefinedBy>
                <http://def.seegrid.csiro.au/isotc211/iso19103/2005/basic> ;
        <http://www.w3.org/2000/01/rdf-schema#label>
                "dimension" ;
        <http://www.w3.org/2000/01/rdf-schema#range>
                <http://www.w3.org/2001/XMLSchema#positiveInteger> .

<http://def.seegrid.csiro.au/isotc211/iso19103/2005/basic#Time>
        a       <http://www.w3.org/2002/07/owl#Class> ;
        <http://www.w3.org/2000/01/rdf-schema#comment>
                "Measure of temporal extent" ;
        <http://www.w3.org/2000/01/rdf-schema#isDefinedBy>
                <http://def.seegrid.csiro.au/isotc211/iso19103/2005/basic> ;
        <http://www.w3.org/2000/01/rdf-schema#label>
                "Time" ;
        <http://www.w3.org/2000/01/rdf-schema#subClassOf>
                <http://def.seegrid.csiro.au/isotc211/iso19103/2005/basic#Measure> .

<http://def.seegrid.csiro.au/isotc211/iso19103/2005/basic#Mass>
        a       <http://www.w3.org/2002/07/owl#Class> ;
        <http://www.w3.org/2000/01/rdf-schema#comment>
                "Measure of amount of substance" ;
        <http://www.w3.org/2000/01/rdf-schema#isDefinedBy>
                <http://def.seegrid.csiro.au/isotc211/iso19103/2005/basic> ;
        <http://www.w3.org/2000/01/rdf-schema#label>
                "Mass" ;
        <http://www.w3.org/2000/01/rdf-schema#subClassOf>
                <http://def.seegrid.csiro.au/isotc211/iso19103/2005/basic#Measure> .

<http://def.seegrid.csiro.au/isotc211/iso19103/2005/basic#measure>
        a       <http://www.w3.org/2002/07/owl#ObjectProperty> ;
        <http://www.w3.org/2000/01/rdf-schema#comment>
                "The value of this property is a scaled number" ;
        <http://www.w3.org/2000/01/rdf-schema#isDefinedBy>
                <http://def.seegrid.csiro.au/isotc211/iso19103/2005/basic> ;
        <http://www.w3.org/2000/01/rdf-schema#label>
                "measure" ;
        <http://www.w3.org/2000/01/rdf-schema#range>
                <http://def.seegrid.csiro.au/isotc211/iso19103/2005/basic#Measure> .

<http://def.seegrid.csiro.au/isotc211/iso19103/2005/basic#Velocity>
        a       <http://www.w3.org/2002/07/owl#Class> ;
        <http://www.w3.org/2000/01/rdf-schema#comment>
                "Measure of rate of change of position" ;
        <http://www.w3.org/2000/01/rdf-schema#isDefinedBy>
                <http://def.seegrid.csiro.au/isotc211/iso19103/2005/basic> ;
        <http://www.w3.org/2000/01/rdf-schema#label>
                "Velocity" ;
        <http://www.w3.org/2000/01/rdf-schema#subClassOf>
                <http://def.seegrid.csiro.au/isotc211/iso19103/2005/basic#Measure> .

<http://def.seegrid.csiro.au/isotc211/iso19103/2005/basic#Decimal>
        a       <http://www.w3.org/2000/01/rdf-schema#Datatype> ;
        <http://www.w3.org/2000/01/rdf-schema#comment>
                "The usually finite representation of a decimal number. It differs from the common binary Real implementation in that it can represent 1/10 (one-tenth) without error, while binary real representation can only represent powers of 1/2 (one-half) exactly. Since many currencies are decimal, these representations are preferred in dealing with such moneys. This is also true for mile markers, which are often given in decimals.\r\n\r\nCan be thought of as an integer part followed by a fractional part given in multiples of powers of 1/10 (tenths)." ;
        <http://www.w3.org/2000/01/rdf-schema#isDefinedBy>
                <http://def.seegrid.csiro.au/isotc211/iso19103/2005/basic> ;
        <http://www.w3.org/2000/01/rdf-schema#label>
                "decimal" ;
        <http://www.w3.org/2002/07/owl#equivalentClass>
                <http://www.w3.org/2001/XMLSchema#decimal> .
