<http://purl.org/makolab/caont/Audio>
        a       <http://www.w3.org/2002/07/owl#Class> ;
        <http://www.w3.org/2000/01/rdf-schema#comment>
                "Audio file format suported by receiver's audio module"@en ;
        <http://www.w3.org/2000/01/rdf-schema#isDefinedBy>
                "http://purl.org/makolab/caont/" ;
        <http://www.w3.org/2000/01/rdf-schema#label>
                "Audio module"@en ;
        <http://www.w3.org/2000/01/rdf-schema#subClassOf>
                <http://purl.org/makolab/caont/Feature> ;
        <http://www.w3.org/2002/07/owl#disjointWith>
                <http://purl.org/makolab/caont/Tuner> , <http://purl.org/makolab/caont/Display> .

<http://purl.org/makolab/caont/Speaker>
        a       <http://www.w3.org/2002/07/owl#Class> ;
        <http://www.w3.org/2000/01/rdf-schema#comment>
                "Car speakers are largely functionally identical to any other loudspeaker design with key components specialized for use in mobile environments, and generally serve an identical purpose. One major key design difference is mult-axial mounting of different types of loudspeakers in the same footprint, such as a tweeter directly mounted over a woofer. Another key difference is non-circular cone shapes, such as square, oval, or even triangular. Both of these features reflect a significant reduction in space and size that a speaker may occupy in a vehicle cabin.\n\nSource:\nhttp://en.wikipedia.org/wiki/Car_audio#Speakers"@en ;
        <http://www.w3.org/2000/01/rdf-schema#isDefinedBy>
                "http://purl.org/makolab/caont/" ;
        <http://www.w3.org/2000/01/rdf-schema#label>
                "Car speaker"@en ;
        <http://www.w3.org/2000/01/rdf-schema#subClassOf>
                <http://purl.org/goodrelations/v1#ProductOrService> .

<http://purl.org/makolab/caont/hasUnit>
        a       <http://www.w3.org/2002/07/owl#ObjectProperty> ;
        <http://www.w3.org/2000/01/rdf-schema#comment>
                "The unit of measurement for a gr:QuantitativeValue, a gr:UnitPriceSpecification, or a gr:TypeAndQuantityNode given using the instance, i.e. \nVoltage\t-\thttp://dbpedia.org/resource/Volt \n"@en ;
        <http://www.w3.org/2000/01/rdf-schema#domain>
                [ a       <http://www.w3.org/2002/07/owl#Class> ;
                  <http://www.w3.org/2002/07/owl#unionOf>
                          ( <http://purl.org/goodrelations/v1#QuantitativeValue> <http://purl.org/goodrelations/v1#TypeAndQuantityNode> <http://purl.org/goodrelations/v1#UnitPriceSpecification> )
                ] ;
        <http://www.w3.org/2000/01/rdf-schema#isDefinedBy>
                "http://purl.org/makolab/caont/" ;
        <http://www.w3.org/2000/01/rdf-schema#label>
                "unit of measurement"@en .

<http://purl.org/makolab/caont/displaySize>
        a       <http://www.w3.org/2002/07/owl#ObjectProperty> ;
        <http://www.w3.org/2000/01/rdf-schema#comment>
                "The diagonal, usually measured in inches. The diagonal measurement of a display as the actual viewable area is also dependent on the aspect ratio of the display. For a display device of the same area, the diagonal achieves a larger value in a widescreen than compared to a more square screen. There is a risk of manufacturers making displays wider than what is actually most convenient in order to make the diagonal achieve a larger value.\n\nSource:\nhttp://en.wikipedia.org/wiki/Display_size"@en ;
        <http://www.w3.org/2000/01/rdf-schema#domain>
                <http://purl.org/makolab/caont/Display> ;
        <http://www.w3.org/2000/01/rdf-schema#isDefinedBy>
                "http://purl.org/makolab/caont/" ;
        <http://www.w3.org/2000/01/rdf-schema#label>
                "Display diagonal"@en ;
        <http://www.w3.org/2000/01/rdf-schema#range>
                <http://purl.org/goodrelations/v1#QuantitativeValueFloat> ;
        <http://www.w3.org/2000/01/rdf-schema#subPropertyOf>
                <http://purl.org/goodrelations/v1#quantitativeProductOrServiceProperty> .

<http://purl.org/makolab/caont/DataFormat>
        a       <http://www.w3.org/2002/07/owl#Class> ;
        <http://www.w3.org/2000/01/rdf-schema#comment>
                "A file format is a particular way that information is encoded for storage in a computer file.\n\nSource:\nhttp://en.wikipedia.org/wiki/File_format"@en ;
        <http://www.w3.org/2000/01/rdf-schema#isDefinedBy>
                "http://purl.org/makolab/caont/" ;
        <http://www.w3.org/2000/01/rdf-schema#label>
                "Audio Video data format"@en ;
        <http://www.w3.org/2000/01/rdf-schema#subClassOf>
                <http://purl.org/goodrelations/v1#QualitativeValue> .

<http://purl.org/makolab/caont/hasConnectivity>
        a       <http://www.w3.org/2002/07/owl#ObjectProperty> ;
        <http://www.w3.org/2000/01/rdf-schema#comment>
                "Connection possibilities of electronical devices."@en ;
        <http://www.w3.org/2000/01/rdf-schema#domain>
                [ a       <http://www.w3.org/2002/07/owl#Class> ;
                  <http://www.w3.org/2002/07/owl#unionOf>
                          ( <http://purl.org/makolab/caont/CDChanger> <http://purl.org/makolab/caont/Receiver> )
                ] ;
        <http://www.w3.org/2000/01/rdf-schema#isDefinedBy>
                "http://purl.org/makolab/caont/" ;
        <http://www.w3.org/2000/01/rdf-schema#label>
                "Connection ports of a device"@en ;
        <http://www.w3.org/2000/01/rdf-schema#range>
                <http://purl.org/makolab/caont/Connectivity> ;
        <http://www.w3.org/2000/01/rdf-schema#subPropertyOf>
                <http://purl.org/goodrelations/v1#qualitativeProductOrServiceProperty> .

<http://purl.org/makolab/caont/Connectivity>
        a       <http://www.w3.org/2002/07/owl#Class> ;
        <http://www.w3.org/2000/01/rdf-schema#comment>
                "Possible connections on an audio/video receiver's module"@en ;
        <http://www.w3.org/2000/01/rdf-schema#isDefinedBy>
                "http://purl.org/makolab/caont/" ;
        <http://www.w3.org/2000/01/rdf-schema#label>
                "Connectivity"@en ;
        <http://www.w3.org/2000/01/rdf-schema#subClassOf>
                <http://purl.org/goodrelations/v1#QualitativeValue> .

<http://purl.org/makolab/caont/hasFeature>
        a       <http://www.w3.org/2002/07/owl#ObjectProperty> ;
        <http://www.w3.org/2000/01/rdf-schema#comment>
                "Defines features of a audio/video receiver."@en ;
        <http://www.w3.org/2000/01/rdf-schema#domain>
                <http://purl.org/makolab/caont/Receiver> ;
        <http://www.w3.org/2000/01/rdf-schema#isDefinedBy>
                "http://purl.org/makolab/caont/" ;
        <http://www.w3.org/2000/01/rdf-schema#label>
                "Feature"@en ;
        <http://www.w3.org/2000/01/rdf-schema#range>
                <http://purl.org/makolab/caont/Feature> ;
        <http://www.w3.org/2000/01/rdf-schema#subPropertyOf>
                <http://purl.org/goodrelations/v1#qualitativeProductOrServiceProperty> .

<http://purl.org/makolab/caont/Amplifier>
        a       <http://www.w3.org/2002/07/owl#Class> ;
        <http://www.w3.org/2000/01/rdf-schema#comment>
                "Amplifier feature"@en ;
        <http://www.w3.org/2000/01/rdf-schema#isDefinedBy>
                "http://purl.org/makolab/caont/" ;
        <http://www.w3.org/2000/01/rdf-schema#label>
                "Amplifier"@en ;
        <http://www.w3.org/2000/01/rdf-schema#subClassOf>
                <http://purl.org/makolab/caont/Feature> ;
        <http://www.w3.org/2002/07/owl#disjointWith>
                <http://purl.org/makolab/caont/Audio> , <http://purl.org/makolab/caont/Display> , <http://purl.org/makolab/caont/Tuner> .

<http://purl.org/makolab/caont/hasRDS>
        a       <http://www.w3.org/2002/07/owl#DatatypeProperty> ;
        <http://www.w3.org/2000/01/rdf-schema#comment>
                "Radio Data System, or RDS, is a communications protocol standard for embedding small amounts of digital information in conventional FM radio broadcasts. RDS standardises several types of information transmitted, including time, station identification and programme information.\n\nSource:\nhttp://en.wikipedia.org/wiki/Radio_Data_System"@en ;
        <http://www.w3.org/2000/01/rdf-schema#domain>
                <http://purl.org/makolab/caont/Tuner> ;
        <http://www.w3.org/2000/01/rdf-schema#isDefinedBy>
                "http://purl.org/makolab/caont/" ;
        <http://www.w3.org/2000/01/rdf-schema#label>
                "Radio Data System"@en ;
        <http://www.w3.org/2000/01/rdf-schema#range>
                <http://www.w3.org/2001/XMLSchema#boolean> ;
        <http://www.w3.org/2000/01/rdf-schema#subPropertyOf>
                <http://purl.org/goodrelations/v1#datatypeProductOrServiceProperty> .

<http://purl.org/makolab/caont/hasRemoteControl>
        a       <http://www.w3.org/2002/07/owl#DatatypeProperty> ;
        <http://www.w3.org/2000/01/rdf-schema#comment>
                "A remote control is a component of an electronics device, most commonly a television set, DVD player and home theater systems originally used for operating the television device wirelessly from a short line-of-sight distance. Remote control has continually evolved and advanced over recent years to include Bluetooth connectivity, motion sensor enabled capabilities and voice control.\n\nSource:\nhttp://en.wikipedia.org/wiki/Remote_control"@en ;
        <http://www.w3.org/2000/01/rdf-schema#domain>
                <http://purl.org/makolab/caont/Receiver> ;
        <http://www.w3.org/2000/01/rdf-schema#isDefinedBy>
                "http://purl.org/makolab/caont/" ;
        <http://www.w3.org/2000/01/rdf-schema#label>
                "Remote control"@en ;
        <http://www.w3.org/2000/01/rdf-schema#range>
                <http://www.w3.org/2001/XMLSchema#boolean> ;
        <http://www.w3.org/2000/01/rdf-schema#subPropertyOf>
                <http://purl.org/goodrelations/v1#datatypeProductOrServiceProperty> .

<http://purl.org/makolab/caont/hasDataFormat>
        a       <http://www.w3.org/2002/07/owl#ObjectProperty> ;
        <http://www.w3.org/2000/01/rdf-schema#comment>
                "Supported audio/video formats."@en ;
        <http://www.w3.org/2000/01/rdf-schema#domain>
                [ a       <http://www.w3.org/2002/07/owl#Class> ;
                  <http://www.w3.org/2002/07/owl#unionOf>
                          ( <http://purl.org/makolab/caont/Audio> <http://purl.org/makolab/caont/Display> )
                ] ;
        <http://www.w3.org/2000/01/rdf-schema#isDefinedBy>
                "http://purl.org/makolab/caont/" ;
        <http://www.w3.org/2000/01/rdf-schema#label>
                "Data format"@en ;
        <http://www.w3.org/2000/01/rdf-schema#range>
                <http://purl.org/makolab/caont/DataFormat> ;
        <http://www.w3.org/2000/01/rdf-schema#subPropertyOf>
                <http://purl.org/goodrelations/v1#qualitativeProductOrServiceProperty> .

<http://purl.org/makolab/caont/hasAudioPower>
        a       <http://www.w3.org/2002/07/owl#ObjectProperty> ;
        <http://www.w3.org/2000/01/rdf-schema#comment>
                "Audio power is the electrical power transferred from an audio amplifier to a loudspeaker, measured in watts. The electrical power delivered to the loudspeaker, together with its sensitivity, determines the sound power level generated (with the rest being converted to heat).\n\nSource:\nhttp://en.wikipedia.org/wiki/Audio_power"@en ;
        <http://www.w3.org/2000/01/rdf-schema#domain>
                [ a       <http://www.w3.org/2002/07/owl#Class> ;
                  <http://www.w3.org/2002/07/owl#unionOf>
                          ( <http://purl.org/makolab/caont/Amplifier> <http://purl.org/makolab/caont/Speaker> )
                ] ;
        <http://www.w3.org/2000/01/rdf-schema#isDefinedBy>
                "http://purl.org/makolab/caont/" ;
        <http://www.w3.org/2000/01/rdf-schema#label>
                "Amplifier/speaker power"@en ;
        <http://www.w3.org/2000/01/rdf-schema#range>
                <http://purl.org/goodrelations/v1#QuantitativeValueFloat> ;
        <http://www.w3.org/2000/01/rdf-schema#subPropertyOf>
                <http://purl.org/goodrelations/v1#quantitativeProductOrServiceProperty> .

<http://purl.org/makolab/caont/CDChanger>
        a       <http://www.w3.org/2002/07/owl#Class> ;
        <http://www.w3.org/2000/01/rdf-schema#comment>
                "A CD changer holds multiple Compact Discs, usually in a cartridge, and allows the user to access (or play) any of them, one at a time. CD changers were commonly found in home cinema systems, in cars and, less frequently, in computer equipment.\n\nSource:\nhttp://en.wikipedia.org/wiki/CD_Changer#CD_changer"@en ;
        <http://www.w3.org/2000/01/rdf-schema#isDefinedBy>
                "http://purl.org/makolab/caont/" ;
        <http://www.w3.org/2000/01/rdf-schema#label>
                "External cartridge CD changer"@en ;
        <http://www.w3.org/2000/01/rdf-schema#subClassOf>
                <http://purl.org/goodrelations/v1#ProductOrService> ;
        <http://www.w3.org/2000/01/rdf-schema#subClassOf>
                [ a       <http://www.w3.org/2002/07/owl#Restriction> ;
                  <http://www.w3.org/2002/07/owl#maxCardinality>
                          "1"^^<http://www.w3.org/2001/XMLSchema#nonNegativeInteger> ;
                  <http://www.w3.org/2002/07/owl#onProperty>
                          <http://purl.org/makolab/caont/cdChangerCapacity>
                ] .

<http://purl.org/makolab/caont/diameter>
        a       <http://www.w3.org/2002/07/owl#ObjectProperty> ;
        <http://www.w3.org/2000/01/rdf-schema#comment>
                "The diameter of the speaker.\nTypical unit code(s): CMT for centimeters, INH for inches"@en ;
        <http://www.w3.org/2000/01/rdf-schema#domain>
                <http://purl.org/makolab/caont/Speaker> ;
        <http://www.w3.org/2000/01/rdf-schema#isDefinedBy>
                "http://purl.org/makolab/caont/" ;
        <http://www.w3.org/2000/01/rdf-schema#label>
                "Diameter"@en ;
        <http://www.w3.org/2000/01/rdf-schema#range>
                <http://purl.org/goodrelations/v1#QuantitativeValue> ;
        <http://www.w3.org/2000/01/rdf-schema#subPropertyOf>
                <http://purl.org/goodrelations/v1#quantitativeProductOrServiceProperty> .

<http://purl.org/makolab/caont/hasRemovableFrontPanel>
        a       <http://www.w3.org/2002/07/owl#DatatypeProperty> ;
        <http://www.w3.org/2000/01/rdf-schema#comment>
                "Determines whether the panel of the device is removable."@en ;
        <http://www.w3.org/2000/01/rdf-schema#domain>
                <http://purl.org/makolab/caont/Receiver> ;
        <http://www.w3.org/2000/01/rdf-schema#isDefinedBy>
                "http://purl.org/makolab/caont/" ;
        <http://www.w3.org/2000/01/rdf-schema#label>
                "Removable front panel"@en ;
        <http://www.w3.org/2000/01/rdf-schema#range>
                <http://www.w3.org/2001/XMLSchema#boolean> ;
        <http://www.w3.org/2000/01/rdf-schema#subPropertyOf>
                <http://purl.org/goodrelations/v1#datatypeProductOrServiceProperty> .

<http://purl.org/makolab/caont/cdChangerCapacity>
        a       <http://www.w3.org/2002/07/owl#ObjectProperty> , <http://www.w3.org/2002/07/owl#FunctionalProperty> ;
        <http://www.w3.org/2000/01/rdf-schema#comment>
                "CD Changer Capacity"@en ;
        <http://www.w3.org/2000/01/rdf-schema#domain>
                <http://purl.org/makolab/caont/CDChanger> ;
        <http://www.w3.org/2000/01/rdf-schema#isDefinedBy>
                "http://purl.org/makolab/caont/" ;
        <http://www.w3.org/2000/01/rdf-schema#label>
                "CD Changer Capacity"@en ;
        <http://www.w3.org/2000/01/rdf-schema#range>
                <http://purl.org/goodrelations/v1#QuantitativeValueInteger> ;
        <http://www.w3.org/2000/01/rdf-schema#subPropertyOf>
                <http://purl.org/goodrelations/v1#quantitativeProductOrServiceProperty> .

<http://purl.org/makolab/caont/hasFrequencyResponse>
        a       <http://www.w3.org/2002/07/owl#ObjectProperty> ;
        <http://www.w3.org/2000/01/rdf-schema#comment>
                "An audio frequency (abbreviation: AF) or audible frequency is characterized as a periodic vibration whose frequency is audible to the average human. It is the property of sound that most determines pitch and is measured in hertz (Hz).\n\nSource:\nhttp://en.wikipedia.org/wiki/Audio_frequency"@en ;
        <http://www.w3.org/2000/01/rdf-schema#domain>
                [ a       <http://www.w3.org/2002/07/owl#Class> ;
                  <http://www.w3.org/2002/07/owl#unionOf>
                          ( <http://purl.org/makolab/caont/Amplifier> <http://purl.org/makolab/caont/Speaker> )
                ] ;
        <http://www.w3.org/2000/01/rdf-schema#isDefinedBy>
                "http://purl.org/makolab/caont/" ;
        <http://www.w3.org/2000/01/rdf-schema#label>
                "Frequency response range"@en ;
        <http://www.w3.org/2000/01/rdf-schema#range>
                <http://purl.org/goodrelations/v1#QuantitativeValueFloat> ;
        <http://www.w3.org/2000/01/rdf-schema#subPropertyOf>
                <http://purl.org/goodrelations/v1#quantitativeProductOrServiceProperty> .

<http://purl.org/makolab/caont/>
        a       <http://www.w3.org/2002/07/owl#Ontology> ;
        <http://www.w3.org/2000/01/rdf-schema#comment>
                "CAO: Car Audio Ontology\n    \nA Web vocabulary for describings car audio/video systems for e-commerce.\n\nVocabulary:    http://purl.org/makolab/caont/\nNamespace:     http://purl.org/makolab/caont/\n\nDesigned to be used in combination with GoodRelations, a standard vocabulary for the commercial aspects of offers for sale or rental. \n\nSee http://purl.org/goodrelations/ for more information."@en ;
        <http://www.w3.org/2000/01/rdf-schema#label>
                "CAO: Car Audio Ontology"@en ;
        <http://purl.org/dc/elements/1.1/creator>
                "Makolab S.A.\nhttp://makolab.com"@en ;
        <http://purl.org/dc/elements/1.1/title>
                "CAO: Car Audio Ontology"@en ;
        <http://purl.org/dc/terms/license>
                "http://creativecommons.org/licenses/by/3.0/"@en ;
        <http://purl.org/makolab/caont/lastActualisationDate>
                "2012-10-09" ;
        <http://www.w3.org/2002/07/owl#imports>
                <http://purl.org/goodrelations/v1> ;
        <http://www.w3.org/2002/07/owl#versionInfo>
                "0.8.5" .

<http://purl.org/makolab/caont/Tuner>
        a       <http://www.w3.org/2002/07/owl#Class> ;
        <http://www.w3.org/2000/01/rdf-schema#comment>
                "AV receivers though primarily used for amplification may or may not have an inbuilt AM/FM radio tuner among other features such as LAN connectivity for various Internet applications and some with multi-room audio solutions.\n\nResource:\nhttp://en.wikipedia.org/wiki/AV_receiver#Radio_on_AVRs"@en ;
        <http://www.w3.org/2000/01/rdf-schema#isDefinedBy>
                "http://purl.org/makolab/caont/" ;
        <http://www.w3.org/2000/01/rdf-schema#label>
                "Audio/Video receiver's module"@en ;
        <http://www.w3.org/2000/01/rdf-schema#subClassOf>
                <http://purl.org/makolab/caont/Feature> .

<http://purl.org/makolab/caont/iPodControl>
        a       <http://www.w3.org/2002/07/owl#DatatypeProperty> ;
        <http://www.w3.org/2000/01/rdf-schema#comment>
                "Determines whether the receiver has iPod connection."@en ;
        <http://www.w3.org/2000/01/rdf-schema#domain>
                <http://purl.org/makolab/caont/Receiver> ;
        <http://www.w3.org/2000/01/rdf-schema#isDefinedBy>
                "http://purl.org/makolab/caont/" ;
        <http://www.w3.org/2000/01/rdf-schema#label>
                "Supported iPod® connection"@en ;
        <http://www.w3.org/2000/01/rdf-schema#range>
                <http://www.w3.org/2001/XMLSchema#boolean> ;
        <http://www.w3.org/2000/01/rdf-schema#subPropertyOf>
                <http://purl.org/goodrelations/v1#datatypeProductOrServiceProperty> .

<http://purl.org/makolab/caont/touchPanel>
        a       <http://www.w3.org/2002/07/owl#DatatypeProperty> ;
        <http://www.w3.org/2000/01/rdf-schema#comment>
                "A touchscreen is an electronic visual display that can detect the presence and location of a touch within the display area. The term generally refers to touching the display of the device with a finger or hand. Touchscreens can also sense other passive objects, such as a stylus. Touchscreens are common in devices such as game consoles, all-in-one computers, tablet computers, and smartphones.\n\nSource:\nhttp://en.wikipedia.org/wiki/Touchscreen"@en ;
        <http://www.w3.org/2000/01/rdf-schema#domain>
                <http://purl.org/makolab/caont/Display> ;
        <http://www.w3.org/2000/01/rdf-schema#isDefinedBy>
                "http://purl.org/makolab/caont/" ;
        <http://www.w3.org/2000/01/rdf-schema#label>
                "Touchscreen feature"@en ;
        <http://www.w3.org/2000/01/rdf-schema#range>
                <http://www.w3.org/2001/XMLSchema#boolean> ;
        <http://www.w3.org/2000/01/rdf-schema#subPropertyOf>
                <http://purl.org/goodrelations/v1#datatypeProductOrServiceProperty> .

<http://purl.org/makolab/caont/Display>
        a       <http://www.w3.org/2002/07/owl#Class> ;
        <http://www.w3.org/2000/01/rdf-schema#comment>
                "Specification of a display audio/video receiver's module"@en ;
        <http://www.w3.org/2000/01/rdf-schema#isDefinedBy>
                "http://purl.org/makolab/caont/" ;
        <http://www.w3.org/2000/01/rdf-schema#label>
                "Display"@en ;
        <http://www.w3.org/2000/01/rdf-schema#subClassOf>
                <http://purl.org/makolab/caont/Feature> ;
        <http://www.w3.org/2002/07/owl#disjointWith>
                <http://purl.org/makolab/caont/Tuner> .

<http://purl.org/makolab/caont/madeOfMaterial>
        a       <http://www.w3.org/2002/07/owl#DatatypeProperty> ;
        <http://www.w3.org/2000/01/rdf-schema#comment>
                "Material used for the speaker."@en ;
        <http://www.w3.org/2000/01/rdf-schema#domain>
                <http://purl.org/makolab/caont/Speaker> ;
        <http://www.w3.org/2000/01/rdf-schema#isDefinedBy>
                "http://purl.org/makolab/caont/" ;
        <http://www.w3.org/2000/01/rdf-schema#label>
                "Made of material"@en ;
        <http://www.w3.org/2000/01/rdf-schema#range>
                <http://www.w3.org/2001/XMLSchema#string> ;
        <http://www.w3.org/2000/01/rdf-schema#subPropertyOf>
                <http://purl.org/goodrelations/v1#datatypeProductOrServiceProperty> .

<http://purl.org/makolab/caont/hasImpedance>
        a       <http://www.w3.org/2002/07/owl#ObjectProperty> ;
        <http://www.w3.org/2000/01/rdf-schema#comment>
                "The nominal impedance rating of consumer loudspeakers systems can aid in choosing the correct loudspeaker for a given amplifier (or vice versa). If a home hi-fi amplifier specifies 8 ohm or greater loads, care should be taken that loudspeakers with a lower impedance are not used, lest the amplifier be required to produce more current than it was designed to handle. Using a 4 ohm loudspeaker system on an amplifier specifying 8 ohms or greater could lead to amplifier failure.\n\nSource:\nhttp://en.wikipedia.org/wiki/Electrical_characteristics_of_dynamic_loudspeakers#Nominal_impedance"@en ;
        <http://www.w3.org/2000/01/rdf-schema#domain>
                <http://purl.org/makolab/caont/Speaker> ;
        <http://www.w3.org/2000/01/rdf-schema#isDefinedBy>
                "http://purl.org/makolab/caont/" ;
        <http://www.w3.org/2000/01/rdf-schema#label>
                "Speaker impedance"@en ;
        <http://www.w3.org/2000/01/rdf-schema#range>
                <http://purl.org/goodrelations/v1#QuantitativeValueInteger> ;
        <http://www.w3.org/2000/01/rdf-schema#subPropertyOf>
                <http://purl.org/goodrelations/v1#quantitativeProductOrServiceProperty> .

<http://purl.org/makolab/caont/Feature>
        a       <http://www.w3.org/2002/07/owl#Class> ;
        <http://www.w3.org/2000/01/rdf-schema#comment>
                "Audio/Video Receiver feature."@en ;
        <http://www.w3.org/2000/01/rdf-schema#isDefinedBy>
                "http://purl.org/makolab/caont/" ;
        <http://www.w3.org/2000/01/rdf-schema#label>
                "Feature"@en ;
        <http://www.w3.org/2000/01/rdf-schema#subClassOf>
                <http://purl.org/goodrelations/v1#QualitativeValue> .

<http://purl.org/makolab/caont/Receiver>
        a       <http://www.w3.org/2002/07/owl#Class> ;
        <http://www.w3.org/2000/01/rdf-schema#comment>
                "In modern cars, the primary control device for an audio system is commonly referred to as a head unit, and is installed in the center of the dash panel between the driver and the passenger. In older vehicles that had audio components as an option, such devices were mounted externally to the top of or underneath the dash. In rarer occasions, head units have also been mounted vertically.\n\nThe headunit itself is usually a multi-purpose device that houses multiple types of components in its housing. The most common components are a radio receiver/tuner usually with AM and FM bands, and a small amplifier for driving an audio signal to speakers. Other possible components include various media devices, such as (in older vehicles) a tape player (either 8-track or cassette), CD player, DVD player, HD Radio, Satelite Radio, USB flash memory, and even a portable hard disk drive typically used in notebook computing. Many head units also feature a DSP component, and equalization component (such as bass and treble controls), or a control interface for another feature on the car (such as a back-up/parking camera, navigation system, trip odometer, etc.).\n\nSource:\nhttp://en.wikipedia.org/wiki/Car_audio#Head_unit"@en ;
        <http://www.w3.org/2000/01/rdf-schema#isDefinedBy>
                "http://purl.org/makolab/caont/" ;
        <http://www.w3.org/2000/01/rdf-schema#label>
                "Primary control device for an audio/video system"@en ;
        <http://www.w3.org/2000/01/rdf-schema#subClassOf>
                <http://purl.org/goodrelations/v1#ProductOrService> .

<http://purl.org/makolab/caont/lastActualisationDate>
        a       <http://www.w3.org/2002/07/owl#AnnotationProperty> ;
        <http://www.w3.org/2000/01/rdf-schema#range>
                <http://www.w3.org/2001/XMLSchema#dateTime> .
