_:B5d3bac10X2Dd039X2D4aadX2D984fX2Dc6a1bb911c65 <http://www.w3.org/1999/02/22-rdf-syntax-ns#type> <http://purl.org/linked-data/cube#ComponentSpecification> .
<https://privatealpha.com/ontology/content-inventory/1#target> <http://www.w3.org/2000/01/rdf-schema#label> "target"^^<http://www.w3.org/2001/XMLSchema#token> .
<https://privatealpha.com/ontology/content-inventory/1#link> <http://www.w3.org/2000/01/rdf-schema#domain> <http://xmlns.com/foaf/0.1/Document> .
<https://privatealpha.com/ontology/content-inventory/1#tentative-merge> <http://www.w3.org/2000/01/rdf-schema#comment> "Merge this document into some other document, though unspecified at this time as to which."@en .
<https://privatealpha.com/ontology/content-inventory/1#Action> <http://www.w3.org/2000/01/rdf-schema#isDefinedBy> <https://privatealpha.com/ontology/content-inventory/1#> .
<https://privatealpha.com/ontology/content-inventory/1#indegree> <http://www.w3.org/1999/02/22-rdf-syntax-ns#type> <http://purl.org/linked-data/cube#MeasureProperty> .
<https://privatealpha.com/ontology/content-inventory/1#action> <http://www.w3.org/1999/02/22-rdf-syntax-ns#type> <http://www.w3.org/2002/07/owl#ObjectProperty> .
<https://privatealpha.com/ontology/content-inventory/1#blocks> <http://www.w3.org/2000/01/rdf-schema#range> <http://www.w3.org/2001/XMLSchema#nonNegativeInteger> .
<https://privatealpha.com/ontology/content-inventory/1#words-and-blocks> <http://purl.org/linked-data/cube#component> _:B1cd34ff5X2De048X2D4730X2D9610X2Dc6fb30037588 .
<https://privatealpha.com/ontology/content-inventory/1#> <http://purl.org/dc/terms/modified> "2019-07-07T22:10:55Z"^^<http://www.w3.org/2001/XMLSchema#dateTime> .
<https://privatealpha.com/ontology/content-inventory/1#landing> <http://www.w3.org/2000/01/rdf-schema#isDefinedBy> <https://privatealpha.com/ontology/content-inventory/1#> .
<https://privatealpha.com/ontology/content-inventory/1#> <http://purl.org/dc/terms/references> <http://publishing-statistical-data.googlecode.com/svn/trunk/specs/src/main/html/cube.html#ref_qb_Observation> .
<https://privatealpha.com/ontology/content-inventory/1#desired-outcome> <http://www.w3.org/2000/01/rdf-schema#label> "desired-outcome"^^<http://www.w3.org/2001/XMLSchema#token> .
<https://privatealpha.com/ontology/content-inventory/1#outdegree> <http://www.w3.org/2000/01/rdf-schema#label> "outdegree"^^<http://www.w3.org/2001/XMLSchema#token> .
<https://privatealpha.com/ontology/content-inventory/1#empty> <http://www.w3.org/2000/01/rdf-schema#comment> "The document contains no content."@en .
<https://privatealpha.com/ontology/content-inventory/1#Advertisement> <http://www.w3.org/2000/01/rdf-schema#comment> "This is intended to be a decorator class to indicate that the subject is an advertisement. It can therefore be combined with other classes such as foaf:Image."@en .
<https://privatealpha.com/ontology/content-inventory/1#keep> <http://www.w3.org/1999/02/22-rdf-syntax-ns#type> <https://privatealpha.com/ontology/content-inventory/1#Action> .
<https://privatealpha.com/ontology/content-inventory/1#sd> <http://www.w3.org/2000/01/rdf-schema#comment> "Standard Deviation"@en .
<https://privatealpha.com/ontology/content-inventory/1#sd> <http://www.w3.org/1999/02/22-rdf-syntax-ns#type> <http://purl.org/linked-data/cube#MeasureProperty> .
<https://privatealpha.com/ontology/content-inventory/1#incomplete> <http://www.w3.org/2000/01/rdf-schema#isDefinedBy> <https://privatealpha.com/ontology/content-inventory/1#> .
<https://privatealpha.com/ontology/content-inventory/1#> <http://purl.org/dc/terms/references> <http://en.wikipedia.org/wiki/Content_strategy> .
<https://privatealpha.com/ontology/content-inventory/1#low-quartile> <http://www.w3.org/2000/01/rdf-schema#range> <http://www.w3.org/2001/XMLSchema#number> .
<https://privatealpha.com/ontology/content-inventory/1#> <http://purl.org/dc/terms/references> <http://www.w3.org/TR/vocab-data-cube/#ref_qb_DataSet> .
<https://privatealpha.com/ontology/content-inventory/1#low-quartile> <http://www.w3.org/2000/01/rdf-schema#domain> <http://purl.org/linked-data/cube#Observation> .
<https://privatealpha.com/ontology/content-inventory/1#low-quartile> <http://www.w3.org/2000/01/rdf-schema#isDefinedBy> <https://privatealpha.com/ontology/content-inventory/1#> .
<https://privatealpha.com/ontology/content-inventory/1#Audience> <http://www.w3.org/2000/01/rdf-schema#subClassOf> <http://purl.org/dc/terms/AgentClass> .
<https://privatealpha.com/ontology/content-inventory/1#Advertisement> <http://www.w3.org/1999/02/22-rdf-syntax-ns#type> <http://www.w3.org/2002/07/owl#Class> .
<https://privatealpha.com/ontology/content-inventory/1#Merge> <http://www.w3.org/1999/02/22-rdf-syntax-ns#type> <http://www.w3.org/2002/07/owl#Class> .
<https://privatealpha.com/ontology/content-inventory/1#desired-outcome> <http://www.w3.org/1999/02/22-rdf-syntax-ns#type> <http://www.w3.org/2002/07/owl#ObjectProperty> .
<https://privatealpha.com/ontology/content-inventory/1#indegree> <http://www.w3.org/2000/01/rdf-schema#seeAlso> <http://en.wikipedia.org/wiki/Directed_graph#Indegree_and_outdegree> .
<https://privatealpha.com/ontology/content-inventory/1#desired-outcome> <http://www.w3.org/2000/01/rdf-schema#subPropertyOf> <http://purl.org/dc/terms/type> .
<https://privatealpha.com/ontology/content-inventory/1#link> <http://www.w3.org/2000/01/rdf-schema#subPropertyOf> <http://purl.org/dc/terms/references> .
<https://privatealpha.com/ontology/content-inventory/1#empty> <http://www.w3.org/2000/01/rdf-schema#isDefinedBy> <https://privatealpha.com/ontology/content-inventory/1#> .
<https://privatealpha.com/ontology/content-inventory/1#orphan> <http://www.w3.org/2000/01/rdf-schema#comment> "The resource is not explicitly pending or removed from publication, however it has managed to be disconnected from the rest of the site: There is no path to it from a landing page, and it is not a landing page on its own. That is to say that the resource either has no inbound links, or if it does, those links are from other resources that are in the same situation. Documents which are only linked from retired documents are also considered orphans."@en .
<https://privatealpha.com/ontology/content-inventory/1#incomplete> <http://www.w3.org/2000/01/rdf-schema#comment> "The document has been started, but is clearly not finished."@en .
<https://privatealpha.com/ontology/content-inventory/1#non-audience> <http://www.w3.org/2000/01/rdf-schema#isDefinedBy> <https://privatealpha.com/ontology/content-inventory/1#> .
<https://privatealpha.com/ontology/content-inventory/1#aware-of> <http://www.w3.org/1999/02/22-rdf-syntax-ns#type> <http://www.w3.org/2002/07/owl#ObjectProperty> .
<https://privatealpha.com/ontology/content-inventory/1#> <http://purl.org/dc/terms/modified> "2019-09-04T20:27:32Z"^^<http://www.w3.org/2001/XMLSchema#dateTime> .
<https://privatealpha.com/ontology/content-inventory/1#landing> <http://www.w3.org/2000/01/rdf-schema#comment> "The resource is a landing page from some other medium (e.g. e-mail, television, billboard). This status is a hint to automated systems which would otherwise orphan or retire a landing page with no inbound links."@en .
<https://privatealpha.com/ontology/content-inventory/1#retire> <http://www.w3.org/1999/02/22-rdf-syntax-ns#type> <https://privatealpha.com/ontology/content-inventory/1#Action> .
<https://privatealpha.com/ontology/content-inventory/1#update-metadata> <http://www.w3.org/2000/01/rdf-schema#isDefinedBy> <https://privatealpha.com/ontology/content-inventory/1#> .
<https://privatealpha.com/ontology/content-inventory/1#slug> <http://www.w3.org/2000/01/rdf-schema#comment> "The slug is a text token which represents either the full path or terminal path segment of an HTTP(S) URL by which a resource can be located. This property is mainly for the purpose of archiving old or alternative URL paths in a content inventory, for such tasks as generating URL rewriting maps."@en .
<https://privatealpha.com/ontology/content-inventory/1#> <http://purl.org/dc/terms/modified> "2018-10-06T16:23:52Z"^^<http://www.w3.org/2001/XMLSchema#dateTime> .
<https://privatealpha.com/ontology/content-inventory/1#max> <http://www.w3.org/2000/01/rdf-schema#domain> <http://purl.org/linked-data/cube#Observation> .
<https://privatealpha.com/ontology/content-inventory/1#max> <http://www.w3.org/2000/01/rdf-schema#isDefinedBy> <https://privatealpha.com/ontology/content-inventory/1#> .
<https://privatealpha.com/ontology/content-inventory/1#> <http://purl.org/dc/terms/modified> "2019-04-18T01:01:09Z"^^<http://www.w3.org/2001/XMLSchema#dateTime> .
<https://privatealpha.com/ontology/content-inventory/1#max> <http://www.w3.org/2000/01/rdf-schema#range> <http://www.w3.org/2001/XMLSchema#number> .
<https://privatealpha.com/ontology/content-inventory/1#embed> <http://www.w3.org/2000/01/rdf-schema#comment> "This property specifies an embedded resource which is visible in the subject's user interface."@en .
<https://privatealpha.com/ontology/content-inventory/1#high-quartile> <http://www.w3.org/2000/01/rdf-schema#range> <http://www.w3.org/2001/XMLSchema#number> .
<https://privatealpha.com/ontology/content-inventory/1#indexed> <http://www.w3.org/1999/02/22-rdf-syntax-ns#type> <http://www.w3.org/2002/07/owl#DatatypeProperty> .
<https://privatealpha.com/ontology/content-inventory/1#words-and-blocks> <http://www.w3.org/1999/02/22-rdf-syntax-ns#type> <http://purl.org/linked-data/cube#DataStructureDefinition> .
<https://privatealpha.com/ontology/content-inventory/1#max> <http://www.w3.org/2000/01/rdf-schema#comment> "Maximum"@en .
<https://privatealpha.com/ontology/content-inventory/1#indexed> <http://www.w3.org/2000/01/rdf-schema#range> <http://www.w3.org/2001/XMLSchema#boolean> .
<https://privatealpha.com/ontology/content-inventory/1#eschews> <http://www.w3.org/2000/01/rdf-schema#label> "eschews"^^<http://www.w3.org/2001/XMLSchema#token> .
<https://privatealpha.com/ontology/content-inventory/1#high-quartile> <http://www.w3.org/2000/01/rdf-schema#domain> <http://purl.org/linked-data/cube#Observation> .
<https://privatealpha.com/ontology/content-inventory/1#high-quartile> <http://www.w3.org/2000/01/rdf-schema#isDefinedBy> <https://privatealpha.com/ontology/content-inventory/1#> .
<https://privatealpha.com/ontology/content-inventory/1#understands> <http://www.w3.org/2000/01/rdf-schema#domain> <https://privatealpha.com/ontology/content-inventory/1#audience> .
<https://privatealpha.com/ontology/content-inventory/1#canonical-slug> <http://www.w3.org/2000/01/rdf-schema#comment> "This is the canonical slug associated with the resource, and should be populated with the slug which is actually in use."@en .
<https://privatealpha.com/ontology/content-inventory/1#link> <http://www.w3.org/2000/01/rdf-schema#label> "link"^^<http://www.w3.org/2001/XMLSchema#token> .
<https://privatealpha.com/ontology/content-inventory/1#desired-outcome> <http://www.w3.org/2000/01/rdf-schema#domain> <http://xmlns.com/foaf/0.1/Document> .
<https://privatealpha.com/ontology/content-inventory/1#words-and-blocks> <http://purl.org/linked-data/cube#component> _:B07c650f3X2D053eX2D46baX2D978dX2D09e37ca141e4 .
<https://privatealpha.com/ontology/content-inventory/1> <http://xmlns.com/foaf/0.1/primaryTopic> <https://privatealpha.com/ontology/content-inventory/1#> .
<https://privatealpha.com/ontology/content-inventory/1#document> <http://www.w3.org/1999/02/22-rdf-syntax-ns#type> <http://purl.org/linked-data/cube#DimensionProperty> .
<https://privatealpha.com/ontology/content-inventory/1#eschews> <http://www.w3.org/1999/02/22-rdf-syntax-ns#type> <http://www.w3.org/2002/07/owl#ObjectProperty> .
<https://privatealpha.com/ontology/content-inventory/1#> <http://purl.org/dc/terms/modified> "2015-02-03T14:39:00-08:00"^^<http://www.w3.org/2001/XMLSchema#dateTime> .
<https://privatealpha.com/ontology/content-inventory/1#indegree> <http://www.w3.org/2000/01/rdf-schema#label> "indegree"^^<http://www.w3.org/2001/XMLSchema#token> .
<https://privatealpha.com/ontology/content-inventory/1#high-quartile> <http://www.w3.org/2000/01/rdf-schema#label> "high-quartile"^^<http://www.w3.org/2001/XMLSchema#token> .
<https://privatealpha.com/ontology/content-inventory/1#> <http://purl.org/dc/terms/creator> <https://doriantaylor.com/person/dorian-taylor#me> .
<https://privatealpha.com/ontology/content-inventory/1#> <http://www.w3.org/2000/01/rdf-schema#comment> "This vocabulary defines a number of concepts peculiar to content strategy which are not accounted for by other vocabularies."@en .
<https://privatealpha.com/ontology/content-inventory/1#proofread> <http://www.w3.org/2000/01/rdf-schema#label> "proofread"^^<http://www.w3.org/2001/XMLSchema#token> .
<https://privatealpha.com/ontology/content-inventory/1#Audience> <http://www.w3.org/2000/01/rdf-schema#label> "Audience"^^<http://www.w3.org/2001/XMLSchema#token> .
<https://privatealpha.com/ontology/content-inventory/1#proofread> <http://www.w3.org/2000/01/rdf-schema#comment> "Proofread this document."@en .
<https://privatealpha.com/ontology/content-inventory/1#aware-of> <http://www.w3.org/2000/01/rdf-schema#comment> "This property relates an Audience to a SKOS concept that is likely to be in the orbit of the audience's members: they are aware that the concept exists, although they may not necessarily understand it."@en .
<https://privatealpha.com/ontology/content-inventory/1#non-audience> <http://www.w3.org/2000/01/rdf-schema#seeAlso> <http://purl.org/dc/terms/audience> .
<https://privatealpha.com/ontology/content-inventory/1#tentative-merge> <http://www.w3.org/2000/01/rdf-schema#isDefinedBy> <https://privatealpha.com/ontology/content-inventory/1#> .
<https://privatealpha.com/ontology/content-inventory/1#> <http://purl.org/dc/terms/modified> "2019-04-07T16:36:10Z"^^<http://www.w3.org/2001/XMLSchema#dateTime> .
<https://privatealpha.com/ontology/content-inventory/1#action> <http://www.w3.org/2000/01/rdf-schema#domain> <http://xmlns.com/foaf/0.1/Document> .
<https://privatealpha.com/ontology/content-inventory/1#> <http://purl.org/dc/terms/references> <http://en.wikipedia.org/wiki/Five-number_summary> .
<https://privatealpha.com/ontology/content-inventory/1#document> <http://www.w3.org/2000/01/rdf-schema#domain> <http://purl.org/linked-data/cube#Observation> .
<https://privatealpha.com/ontology/content-inventory/1#min> <http://www.w3.org/2000/01/rdf-schema#label> "min"^^<http://www.w3.org/2001/XMLSchema#token> .
<https://privatealpha.com/ontology/content-inventory/1#document> <http://www.w3.org/2000/01/rdf-schema#isDefinedBy> <https://privatealpha.com/ontology/content-inventory/1#> .
<https://privatealpha.com/ontology/content-inventory/1#mean> <http://www.w3.org/2000/01/rdf-schema#comment> "Mean"@en .
<https://privatealpha.com/ontology/content-inventory/1#circulated> <http://www.w3.org/2000/01/rdf-schema#comment> "The document is available for select people to see, but not published in the strict literal sense."@en .
<https://privatealpha.com/ontology/content-inventory/1#median> <http://www.w3.org/2000/01/rdf-schema#range> <http://www.w3.org/2001/XMLSchema#number> .
<https://privatealpha.com/ontology/content-inventory/1#sections> <http://www.w3.org/2000/01/rdf-schema#isDefinedBy> <https://privatealpha.com/ontology/content-inventory/1#> .
<https://privatealpha.com/ontology/content-inventory/1#retired> <http://www.w3.org/2000/01/rdf-schema#label> "retired"^^<http://www.w3.org/2001/XMLSchema#token> .
<https://privatealpha.com/ontology/content-inventory/1#update-metadata> <http://www.w3.org/2000/01/rdf-schema#comment> "Update the metadata of this document, such as keywords, audience, etc."@en .
<https://privatealpha.com/ontology/content-inventory/1#link> <http://www.w3.org/1999/02/22-rdf-syntax-ns#type> <http://www.w3.org/2002/07/owl#ObjectProperty> .
<https://privatealpha.com/ontology/content-inventory/1#median> <http://www.w3.org/2000/01/rdf-schema#isDefinedBy> <https://privatealpha.com/ontology/content-inventory/1#> .
<https://privatealpha.com/ontology/content-inventory/1#median> <http://www.w3.org/2000/01/rdf-schema#domain> <http://purl.org/linked-data/cube#Observation> .
<https://privatealpha.com/ontology/content-inventory/1#circulated> <http://www.w3.org/2000/01/rdf-schema#isDefinedBy> <https://privatealpha.com/ontology/content-inventory/1#> .
<https://privatealpha.com/ontology/content-inventory/1#blocks> <http://www.w3.org/1999/02/22-rdf-syntax-ns#type> <http://purl.org/linked-data/cube#MeasureProperty> .
<https://privatealpha.com/ontology/content-inventory/1#assumes> <http://www.w3.org/2000/01/rdf-schema#label> "assumes"^^<http://www.w3.org/2001/XMLSchema#token> .
<https://privatealpha.com/ontology/content-inventory/1#indegree> <http://www.w3.org/2000/01/rdf-schema#comment> "The number of links pointing at the specified resource."@en .
<https://privatealpha.com/ontology/content-inventory/1> <http://purl.org/dc/terms/subject> <https://privatealpha.com/ontology/content-inventory/1#> .
<https://privatealpha.com/ontology/content-inventory/1#words-and-blocks> <http://www.w3.org/2000/01/rdf-schema#comment> "A set of descriptive statistics pertaining to the number of words per block of text in a given document."@en .
<https://privatealpha.com/ontology/content-inventory/1#values> <http://www.w3.org/2000/01/rdf-schema#domain> <https://privatealpha.com/ontology/content-inventory/1#audience> .
_:Bfd383f50X2D9fc1X2D479bX2D87deX2Ddbc543ff3f94 <http://www.w3.org/1999/02/22-rdf-syntax-ns#type> <http://purl.org/linked-data/cube#ComponentSpecification> .
<https://privatealpha.com/ontology/content-inventory/1#canonical-slug> <http://www.w3.org/1999/02/22-rdf-syntax-ns#type> <http://www.w3.org/2002/07/owl#DatatypeProperty> .
<https://privatealpha.com/ontology/content-inventory/1#canonical-slug> <http://www.w3.org/2000/01/rdf-schema#subPropertyOf> <https://privatealpha.com/ontology/content-inventory/1#slug> .
<https://privatealpha.com/ontology/content-inventory/1#obsolete> <http://www.w3.org/2000/01/rdf-schema#comment> "The content of this document was correct and relevant at one point, but external circumstances have caused it to lapse in relevance or factual accuracy."@en .
_:B1ad310fdX2Dbce0X2D42f6X2D92a9X2D7326c4bb67df <http://www.w3.org/1999/02/22-rdf-syntax-ns#type> <http://purl.org/linked-data/cube#ComponentSpecification> .
<https://privatealpha.com/ontology/content-inventory/1#link> <http://www.w3.org/2000/01/rdf-schema#isDefinedBy> <https://privatealpha.com/ontology/content-inventory/1#> .
<https://privatealpha.com/ontology/content-inventory/1#orphan> <http://www.w3.org/2000/01/rdf-schema#isDefinedBy> <https://privatealpha.com/ontology/content-inventory/1#> .
<https://privatealpha.com/ontology/content-inventory/1#eschews> <http://www.w3.org/2000/01/rdf-schema#range> <http://www.w3.org/2004/02/skos/core#Concept> .
<https://privatealpha.com/ontology/content-inventory/1#> <http://purl.org/dc/terms/references> <http://publishing-statistical-data.googlecode.com/svn/trunk/specs/src/main/html/cube.html#ref_qb_DimensionProperty> .
<https://privatealpha.com/ontology/content-inventory/1#words-and-blocks> <http://purl.org/linked-data/cube#component> _:Bfd383f50X2D9fc1X2D479bX2D87deX2Ddbc543ff3f94 .
<https://privatealpha.com/ontology/content-inventory/1#retired> <http://www.w3.org/1999/02/22-rdf-syntax-ns#type> <http://purl.org/ontology/bibo/DocumentStatus> .
<https://privatealpha.com/ontology/content-inventory/1#alias-for> <http://www.w3.org/2000/01/rdf-schema#label> "alias-for"^^<http://www.w3.org/2001/XMLSchema#token> .
_:Bcc48f0eaX2D2180X2D4228X2Dbe25X2D32444277b9f8 <http://purl.org/linked-data/cube#measure> <https://privatealpha.com/ontology/content-inventory/1#median> .
<https://privatealpha.com/ontology/content-inventory/1#Audience> <http://www.w3.org/2000/01/rdf-schema#isDefinedBy> <https://privatealpha.com/ontology/content-inventory/1#> .
<https://privatealpha.com/ontology/content-inventory/1#proofread> <http://www.w3.org/2000/01/rdf-schema#isDefinedBy> <https://privatealpha.com/ontology/content-inventory/1#> .
<https://privatealpha.com/ontology/content-inventory/1#Merge> <http://www.w3.org/2000/01/rdf-schema#label> "Merge"^^<http://www.w3.org/2001/XMLSchema#token> .
<https://privatealpha.com/ontology/content-inventory/1#indexed> <http://www.w3.org/2000/01/rdf-schema#isDefinedBy> <https://privatealpha.com/ontology/content-inventory/1#> .
<https://privatealpha.com/ontology/content-inventory/1#words> <http://www.w3.org/2000/01/rdf-schema#domain> <http://purl.org/linked-data/cube#Observation> .
<https://privatealpha.com/ontology/content-inventory/1#words> <http://www.w3.org/2000/01/rdf-schema#isDefinedBy> <https://privatealpha.com/ontology/content-inventory/1#> .
<https://privatealpha.com/ontology/content-inventory/1#retire> <http://www.w3.org/2000/01/rdf-schema#label> "retire"^^<http://www.w3.org/2001/XMLSchema#token> .
<https://privatealpha.com/ontology/content-inventory/1#canonical> <http://www.w3.org/1999/02/22-rdf-syntax-ns#type> <http://www.w3.org/2002/07/owl#FunctionalProperty> .
<https://privatealpha.com/ontology/content-inventory/1#orphan> <http://www.w3.org/2000/01/rdf-schema#label> "orphan"^^<http://www.w3.org/2001/XMLSchema#token> .
<https://privatealpha.com/ontology/content-inventory/1#rewrite> <http://www.w3.org/2000/01/rdf-schema#label> "rewrite"^^<http://www.w3.org/2001/XMLSchema#token> .
<https://privatealpha.com/ontology/content-inventory/1#mean> <http://www.w3.org/2000/01/rdf-schema#label> "mean"^^<http://www.w3.org/2001/XMLSchema#token> .
<https://privatealpha.com/ontology/content-inventory/1#> <http://purl.org/dc/terms/modified> "2019-07-21T23:05:32Z"^^<http://www.w3.org/2001/XMLSchema#dateTime> .
<https://privatealpha.com/ontology/content-inventory/1#eschews> <http://www.w3.org/2000/01/rdf-schema#seeAlso> <https://privatealpha.com/ontology/content-inventory/1#values> .
_:Ba7283634X2D00bbX2D4e75X2Da641X2D67b5556457c0 <http://www.w3.org/1999/02/22-rdf-syntax-ns#type> <http://purl.org/linked-data/cube#ComponentSpecification> .
_:B5d3bac10X2Dd039X2D4aadX2D984fX2Dc6a1bb911c65 <http://purl.org/linked-data/cube#measure> <https://privatealpha.com/ontology/content-inventory/1#words> .
<https://privatealpha.com/ontology/content-inventory/1#incorrect> <http://www.w3.org/1999/02/22-rdf-syntax-ns#type> <http://purl.org/ontology/bibo/DocumentStatus> .
<https://privatealpha.com/ontology/content-inventory/1#outdegree> <http://www.w3.org/2000/01/rdf-schema#domain> <http://purl.org/linked-data/cube#Observation> .
<https://privatealpha.com/ontology/content-inventory/1#outdegree> <http://www.w3.org/2000/01/rdf-schema#isDefinedBy> <https://privatealpha.com/ontology/content-inventory/1#> .
_:B1cd34ff5X2De048X2D4730X2D9610X2Dc6fb30037588 <http://purl.org/linked-data/cube#measure> <https://privatealpha.com/ontology/content-inventory/1#max> .
<https://privatealpha.com/ontology/content-inventory/1#assumes> <http://www.w3.org/2000/01/rdf-schema#comment> "The document assumes the audience is familiar with this concept, and may not mention it explicitly."@en .
<https://privatealpha.com/ontology/content-inventory/1#outdegree> <http://www.w3.org/2000/01/rdf-schema#range> <http://www.w3.org/2001/XMLSchema#number> .
_:B8151917aX2D1a15X2D42dfX2D91a7X2De5106cce1e93 <http://www.w3.org/1999/02/22-rdf-syntax-ns#type> <http://purl.org/linked-data/cube#ComponentSpecification> .
<https://privatealpha.com/ontology/content-inventory/1#> <http://purl.org/dc/terms/references> <http://en.wikipedia.org/wiki/Mean> .
<https://privatealpha.com/ontology/content-inventory/1#max> <http://www.w3.org/2000/01/rdf-schema#seeAlso> <http://en.wikipedia.org/wiki/Sample_maximum> .
<https://privatealpha.com/ontology/content-inventory/1#characters> <http://www.w3.org/1999/02/22-rdf-syntax-ns#type> <http://purl.org/linked-data/cube#MeasureProperty> .
<https://privatealpha.com/ontology/content-inventory/1#eschews> <http://www.w3.org/2000/01/rdf-schema#subPropertyOf> <http://www.w3.org/2004/02/skos/core#related> .
<https://privatealpha.com/ontology/content-inventory/1#mean> <http://www.w3.org/2000/01/rdf-schema#seeAlso> <http://en.wikipedia.org/wiki/Mean> .
<https://privatealpha.com/ontology/content-inventory/1#tentative-merge> <http://www.w3.org/2000/01/rdf-schema#label> "tentative-merge"^^<http://www.w3.org/2001/XMLSchema#token> .
<https://privatealpha.com/ontology/content-inventory/1#non-audience> <http://www.w3.org/2000/01/rdf-schema#domain> <http://xmlns.com/foaf/0.1/Document> .
<https://privatealpha.com/ontology/content-inventory/1#unavailable> <http://www.w3.org/2000/01/rdf-schema#isDefinedBy> <https://privatealpha.com/ontology/content-inventory/1#> .
<https://privatealpha.com/ontology/content-inventory/1#incorrect> <http://www.w3.org/2000/01/rdf-schema#label> "incorrect"^^<http://www.w3.org/2001/XMLSchema#token> .
<https://privatealpha.com/ontology/content-inventory/1#understands> <http://www.w3.org/2000/01/rdf-schema#comment> "This property relates an Audience to a SKOS concept that members of the audience are known to comprehend, and thereby do not need any additional explanation."@en .
<https://privatealpha.com/ontology/content-inventory/1#blocks> <http://www.w3.org/2000/01/rdf-schema#label> "blocks"^^<http://www.w3.org/2001/XMLSchema#token> .
<https://privatealpha.com/ontology/content-inventory/1#canonical-slug> <http://www.w3.org/2000/01/rdf-schema#isDefinedBy> <https://privatealpha.com/ontology/content-inventory/1#> .
<https://privatealpha.com/ontology/content-inventory/1#confidential> <http://www.w3.org/2000/01/rdf-schema#isDefinedBy> <https://privatealpha.com/ontology/content-inventory/1#> .
<https://privatealpha.com/ontology/content-inventory/1#characters> <http://www.w3.org/2000/01/rdf-schema#comment> "This indicates the number of characters in a document, with punctuation and the XPath normalize-space function applied. Note this is characters, not bytes."@en .
<https://privatealpha.com/ontology/content-inventory/1#target> <http://www.w3.org/2000/01/rdf-schema#range> <http://xmlns.com/foaf/0.1/Document> .
<https://privatealpha.com/ontology/content-inventory/1#keep> <http://www.w3.org/2000/01/rdf-schema#comment> "Keep this document to which this is associated; make no changes to it at this time."@en .
<https://privatealpha.com/ontology/content-inventory/1#split> <http://www.w3.org/2000/01/rdf-schema#label> "split"^^<http://www.w3.org/2001/XMLSchema#token> .
<https://privatealpha.com/ontology/content-inventory/1#eschews> <http://www.w3.org/2000/01/rdf-schema#isDefinedBy> <https://privatealpha.com/ontology/content-inventory/1#> .
<https://privatealpha.com/ontology/content-inventory/1#document> <http://www.w3.org/2000/01/rdf-schema#comment> "Document Reference"@en .
<https://privatealpha.com/ontology/content-inventory/1#slug> <http://www.w3.org/2000/01/rdf-schema#range> <http://www.w3.org/2001/XMLSchema#string> .
<https://privatealpha.com/ontology/content-inventory/1#aware-of> <http://www.w3.org/2000/01/rdf-schema#isDefinedBy> <https://privatealpha.com/ontology/content-inventory/1#> .
<https://privatealpha.com/ontology/content-inventory/1#mean> <http://www.w3.org/1999/02/22-rdf-syntax-ns#type> <http://purl.org/linked-data/cube#MeasureProperty> .
<https://privatealpha.com/ontology/content-inventory/1#obsolete> <http://www.w3.org/2000/01/rdf-schema#isDefinedBy> <https://privatealpha.com/ontology/content-inventory/1#> .
<https://privatealpha.com/ontology/content-inventory/1#non-audience> <http://www.w3.org/1999/02/22-rdf-syntax-ns#type> <http://www.w3.org/2002/07/owl#ObjectProperty> .
<https://privatealpha.com/ontology/content-inventory/1#canonical> <http://www.w3.org/2000/01/rdf-schema#comment> "Asserts the canonical URI of the subject resource, i.e., the one you always want to publish in content or redirect Web requests to."@en .
<https://privatealpha.com/ontology/content-inventory/1#sections> <http://www.w3.org/2000/01/rdf-schema#comment> "For document types that have a concrete representation of sections, this property may be used to capture their sum."@en .
<https://privatealpha.com/ontology/content-inventory/1#canonical> <http://www.w3.org/2000/01/rdf-schema#label> "canonical"^^<http://www.w3.org/2001/XMLSchema#token> .
<https://privatealpha.com/ontology/content-inventory/1#introduces> <http://www.w3.org/2000/01/rdf-schema#subPropertyOf> <https://privatealpha.com/ontology/content-inventory/1#mentions> .
<https://privatealpha.com/ontology/content-inventory/1#Advertisement> <http://www.w3.org/2000/01/rdf-schema#label> "Advertisement"^^<http://www.w3.org/2001/XMLSchema#token> .
<https://privatealpha.com/ontology/content-inventory/1#desired-outcome> <http://www.w3.org/2000/01/rdf-schema#isDefinedBy> <https://privatealpha.com/ontology/content-inventory/1#> .
<https://privatealpha.com/ontology/content-inventory/1#rewrite> <http://www.w3.org/1999/02/22-rdf-syntax-ns#type> <https://privatealpha.com/ontology/content-inventory/1#Action> .
_:Bfbbe042bX2Dd590X2D4ff4X2Db1f9X2D47f0a34e8b98 <http://purl.org/linked-data/cube#measure> <https://privatealpha.com/ontology/content-inventory/1#characters> .
<https://privatealpha.com/ontology/content-inventory/1#words-and-blocks> <http://purl.org/linked-data/cube#component> _:Bcbbc9d5fX2D1b1dX2D4342X2D9009X2D72d442a1e643 .
<https://privatealpha.com/ontology/content-inventory/1#Audience> <http://www.w3.org/2000/01/rdf-schema#seeAlso> <http://www.w3.org/ns/org#Role> .
<https://privatealpha.com/ontology/content-inventory/1#characters> <http://www.w3.org/2000/01/rdf-schema#range> <http://www.w3.org/2001/XMLSchema#nonNegativeInteger> .
<https://privatealpha.com/ontology/content-inventory/1#words-and-blocks> <http://purl.org/linked-data/cube#component> _:Ba3d85955X2Dc6c8X2D41d5X2Db10bX2D082014a2959c .
<https://privatealpha.com/ontology/content-inventory/1#min> <http://www.w3.org/2000/01/rdf-schema#comment> "The smallest observation in the sample."@en .
<https://privatealpha.com/ontology/content-inventory/1#aware-of> <http://www.w3.org/2000/01/rdf-schema#subPropertyOf> <http://www.w3.org/2004/02/skos/core#related> .
<https://privatealpha.com/ontology/content-inventory/1#> <http://purl.org/ontology/bibo/uri> <https://privatealpha.com/ontology/content-inventory/1#> .
_:Bcbbc9d5fX2D1b1dX2D4342X2D9009X2D72d442a1e643 <http://purl.org/linked-data/cube#measure> <https://privatealpha.com/ontology/content-inventory/1#min> .
_:B1cd34ff5X2De048X2D4730X2D9610X2Dc6fb30037588 <http://www.w3.org/1999/02/22-rdf-syntax-ns#type> <http://purl.org/linked-data/cube#ComponentSpecification> .
<https://privatealpha.com/ontology/content-inventory/1#min> <http://www.w3.org/2000/01/rdf-schema#range> <http://www.w3.org/2001/XMLSchema#number> .
<https://privatealpha.com/ontology/content-inventory/1#keep> <http://www.w3.org/2000/01/rdf-schema#label> "keep"^^<http://www.w3.org/2001/XMLSchema#token> .
<https://privatealpha.com/ontology/content-inventory/1#non-audience> <http://www.w3.org/2000/01/rdf-schema#label> "non-audience"^^<http://www.w3.org/2001/XMLSchema#token> .
<https://privatealpha.com/ontology/content-inventory/1#min> <http://www.w3.org/2000/01/rdf-schema#domain> <http://purl.org/linked-data/cube#Observation> .
<https://privatealpha.com/ontology/content-inventory/1#action> <http://www.w3.org/2000/01/rdf-schema#isDefinedBy> <https://privatealpha.com/ontology/content-inventory/1#> .
<https://privatealpha.com/ontology/content-inventory/1#mentions> <http://www.w3.org/2000/01/rdf-schema#label> "mentions"^^<http://www.w3.org/2001/XMLSchema#token> .
<https://privatealpha.com/ontology/content-inventory/1#min> <http://www.w3.org/2000/01/rdf-schema#isDefinedBy> <https://privatealpha.com/ontology/content-inventory/1#> .
<https://privatealpha.com/ontology/content-inventory/1#action> <http://www.w3.org/2000/01/rdf-schema#subPropertyOf> <http://purl.org/NET/c4dm/event.owl#factor_of> .
<https://privatealpha.com/ontology/content-inventory/1#sections> <http://www.w3.org/2000/01/rdf-schema#domain> <http://xmlns.com/foaf/0.1/Document> .
<https://privatealpha.com/ontology/content-inventory/1#split> <http://www.w3.org/2000/01/rdf-schema#isDefinedBy> <https://privatealpha.com/ontology/content-inventory/1#> .
<https://privatealpha.com/ontology/content-inventory/1#non-audience> <http://www.w3.org/2000/01/rdf-schema#comment> "This property complements dct:audience insofar as enabling the author or editor to designate a set of entities who are explicitly not the intended audience of the document."@en .
<https://privatealpha.com/ontology/content-inventory/1#> <http://purl.org/dc/terms/modified> "2017-04-06T15:24:00-07:00"^^<http://www.w3.org/2001/XMLSchema#dateTime> .
<https://privatealpha.com/ontology/content-inventory/1#alias-for> <http://www.w3.org/2000/01/rdf-schema#seeAlso> <https://privatealpha.com/ontology/content-inventory/1#canonical> .
<https://privatealpha.com/ontology/content-inventory/1#revise> <http://www.w3.org/1999/02/22-rdf-syntax-ns#type> <https://privatealpha.com/ontology/content-inventory/1#Action> .
<https://privatealpha.com/ontology/content-inventory/1#characters> <http://www.w3.org/2000/01/rdf-schema#seeAlso> <http://www.w3.org/TR/xpath/#function-normalize-space> .
<https://privatealpha.com/ontology/content-inventory/1#rewrite> <http://www.w3.org/2000/01/rdf-schema#comment> "Rewrite this document from scratch."@en .
<https://privatealpha.com/ontology/content-inventory/1#Audience> <http://www.w3.org/2000/01/rdf-schema#seeAlso> <http://purl.org/dc/terms/audience> .
<https://privatealpha.com/ontology/content-inventory/1#aware-of> <http://www.w3.org/2000/01/rdf-schema#range> <http://www.w3.org/2004/02/skos/core#Concept> .
<https://privatealpha.com/ontology/content-inventory/1#Merge> <http://www.w3.org/2000/01/rdf-schema#subClassOf> <https://privatealpha.com/ontology/content-inventory/1#Action> .
<https://privatealpha.com/ontology/content-inventory/1#low-quartile> <http://www.w3.org/2000/01/rdf-schema#comment> "Equivalent to the bottom quarter, or 25th percentile, of the observed data."@en .
<https://privatealpha.com/ontology/content-inventory/1#circulated> <http://www.w3.org/2000/01/rdf-schema#label> "circulated"^^<http://www.w3.org/2001/XMLSchema#token> .
<https://privatealpha.com/ontology/content-inventory/1#target> <http://www.w3.org/2000/01/rdf-schema#comment> "Specify the URI of the target resource into which this document should be merged."@en .
<https://privatealpha.com/ontology/content-inventory/1#> <http://www.w3.org/2002/07/owl#imports> <http://purl.org/linked-data/cube#> .
<https://privatealpha.com/ontology/content-inventory/1#> <http://purl.org/vocab/vann/preferredNamespacePrefix> "ci" .
<https://privatealpha.com/ontology/content-inventory/1#retired> <http://www.w3.org/2000/01/rdf-schema#comment> "The document has been explicitly retired by an editor or curator, but still exists in the archive."@en .
_:B8151917aX2D1a15X2D42dfX2D91a7X2De5106cce1e93 <http://purl.org/linked-data/cube#measure> <https://privatealpha.com/ontology/content-inventory/1#sd> .
<https://privatealpha.com/ontology/content-inventory/1#Audience> <http://www.w3.org/1999/02/22-rdf-syntax-ns#type> <http://www.w3.org/2002/07/owl#Class> .
<https://privatealpha.com/ontology/content-inventory/1#min> <http://www.w3.org/2000/01/rdf-schema#seeAlso> <http://en.wikipedia.org/wiki/Sample_minimum> .
<https://privatealpha.com/ontology/content-inventory/1#confidential> <http://www.w3.org/2000/01/rdf-schema#comment> "The document is confidential and not for publication."@en .
<https://privatealpha.com/ontology/content-inventory/1#words-and-blocks> <http://www.w3.org/2000/01/rdf-schema#label> "words-and-blocks"^^<http://www.w3.org/2001/XMLSchema#token> .
<https://privatealpha.com/ontology/content-inventory/1#introduces> <http://www.w3.org/1999/02/22-rdf-syntax-ns#type> <http://www.w3.org/2002/07/owl#ObjectProperty> .
<https://privatealpha.com/ontology/content-inventory/1#high-quartile> <http://www.w3.org/1999/02/22-rdf-syntax-ns#type> <http://purl.org/linked-data/cube#MeasureProperty> .
<https://privatealpha.com/ontology/content-inventory/1#retire> <http://www.w3.org/2000/01/rdf-schema#comment> "Remove all references to this document and consign it to the archive."@en .
<https://privatealpha.com/ontology/content-inventory/1#> <http://purl.org/dc/terms/modified> "2019-03-05T23:38:59Z"^^<http://www.w3.org/2001/XMLSchema#dateTime> .
<https://privatealpha.com/ontology/content-inventory/1#> <http://www.w3.org/2002/07/owl#imports> <http://xmlns.com/foaf/0.1/> .
<https://privatealpha.com/ontology/content-inventory/1#mentions> <http://www.w3.org/2000/01/rdf-schema#domain> <http://xmlns.com/foaf/0.1/Document> .
<https://privatealpha.com/ontology/content-inventory/1#alias> <http://www.w3.org/1999/02/22-rdf-syntax-ns#type> <http://www.w3.org/2002/07/owl#ObjectProperty> .
<https://privatealpha.com/ontology/content-inventory/1#aware-of> <http://www.w3.org/2000/01/rdf-schema#domain> <https://privatealpha.com/ontology/content-inventory/1#audience> .
<https://privatealpha.com/ontology/content-inventory/1#empty> <http://www.w3.org/1999/02/22-rdf-syntax-ns#type> <http://purl.org/ontology/bibo/DocumentStatus> .
<https://privatealpha.com/ontology/content-inventory/1#alias> <http://www.w3.org/2000/01/rdf-schema#comment> "Denotes an alternate URI for the subject resource. It extends owl:sameAs insofar as asserting that the object is somehow less canonical than the subject."@en .
<https://privatealpha.com/ontology/content-inventory/1#Action> <http://www.w3.org/2000/01/rdf-schema#label> "Action"^^<http://www.w3.org/2001/XMLSchema#token> .
<https://privatealpha.com/ontology/content-inventory/1#median> <http://www.w3.org/2000/01/rdf-schema#label> "median"^^<http://www.w3.org/2001/XMLSchema#token> .
<https://privatealpha.com/ontology/content-inventory/1#words-and-blocks> <http://purl.org/linked-data/cube#component> _:B1fbf547cX2D3f36X2D42b5X2D92cfX2D39448acfe13e .
<https://privatealpha.com/ontology/content-inventory/1#words-and-blocks> <http://purl.org/linked-data/cube#component> _:Bcc48f0eaX2D2180X2D4228X2Dbe25X2D32444277b9f8 .
<https://privatealpha.com/ontology/content-inventory/1#values> <http://www.w3.org/2000/01/rdf-schema#label> "values"^^<http://www.w3.org/2001/XMLSchema#token> .
<https://privatealpha.com/ontology/content-inventory/1#> <http://purl.org/dc/terms/references> <http://publishing-statistical-data.googlecode.com/svn/trunk/specs/src/main/html/cube.html#ref_qb_DataStructureDefinition> .
<https://privatealpha.com/ontology/content-inventory/1#alias> <http://www.w3.org/2002/07/owl#inverseOf> <https://privatealpha.com/ontology/content-inventory/1#alias-for> .
<https://privatealpha.com/ontology/content-inventory/1#values> <http://www.w3.org/2000/01/rdf-schema#comment> "This property relates an Audience to a SKOS concept that members of the audience are known to value, that is, to find meaningful in an axiological sense."@en .
<https://privatealpha.com/ontology/content-inventory/1#canonical> <http://www.w3.org/1999/02/22-rdf-syntax-ns#type> <http://www.w3.org/2002/07/owl#ObjectProperty> .
<https://privatealpha.com/ontology/content-inventory/1#blocks> <http://www.w3.org/2000/01/rdf-schema#domain> <http://purl.org/linked-data/cube#Observation> .
<https://privatealpha.com/ontology/content-inventory/1#unavailable> <http://www.w3.org/2000/01/rdf-schema#comment> "The resource at the subject address is unavailable for reasons other than explicit retirement, e.g. HTTP 404 or 403, or going out of print."@en .
<https://privatealpha.com/ontology/content-inventory/1#blocks> <http://www.w3.org/2000/01/rdf-schema#isDefinedBy> <https://privatealpha.com/ontology/content-inventory/1#> .
<https://privatealpha.com/ontology/content-inventory/1#desired-outcome> <http://www.w3.org/2000/01/rdf-schema#comment> "This property is intended to indicate what the document is supposed to do—what material effect it is supposed to produce. It is intentionally open-ended, and as such can point to something like a skos:Concept, another document, or a literal string of text describing the outcome."@en .
<https://privatealpha.com/ontology/content-inventory/1#words-and-blocks> <http://purl.org/linked-data/cube#component> _:Ba7283634X2D00bbX2D4e75X2Da641X2D67b5556457c0 .
<https://privatealpha.com/ontology/content-inventory/1#target> <http://www.w3.org/2000/01/rdf-schema#domain> <https://privatealpha.com/ontology/content-inventory/1#Merge> .
<https://privatealpha.com/ontology/content-inventory/1#incomplete> <http://www.w3.org/1999/02/22-rdf-syntax-ns#type> <http://purl.org/ontology/bibo/DocumentStatus> .
<https://privatealpha.com/ontology/content-inventory/1#low-quartile> <http://www.w3.org/2000/01/rdf-schema#seeAlso> <http://en.wikipedia.org/wiki/Quartile> .
<https://privatealpha.com/ontology/content-inventory/1#Action> <http://www.w3.org/2000/01/rdf-schema#subClassOf> <http://purl.org/NET/c4dm/event.owl#Event> .
<https://privatealpha.com/ontology/content-inventory/1#Merge> <http://www.w3.org/2000/01/rdf-schema#comment> "In order to merge a document, we must define the target to which it ought to be merged. This class is identical to an Action, save for such a property."@en .
<https://privatealpha.com/ontology/content-inventory/1#embed> <http://www.w3.org/1999/02/22-rdf-syntax-ns#type> <http://www.w3.org/2002/07/owl#ObjectProperty> .
<https://privatealpha.com/ontology/content-inventory/1#assumes> <http://www.w3.org/1999/02/22-rdf-syntax-ns#type> <http://www.w3.org/2002/07/owl#ObjectProperty> .
<https://privatealpha.com/ontology/content-inventory/1#mentions> <http://www.w3.org/2000/01/rdf-schema#subPropertyOf> <http://purl.org/dc/terms/references> .
_:B1ad310fdX2Dbce0X2D42f6X2D92a9X2D7326c4bb67df <http://purl.org/linked-data/cube#measure> <https://privatealpha.com/ontology/content-inventory/1#high-quartile> .
<https://privatealpha.com/ontology/content-inventory/1#median> <http://www.w3.org/1999/02/22-rdf-syntax-ns#type> <http://purl.org/linked-data/cube#MeasureProperty> .
<https://privatealpha.com/ontology/content-inventory/1#indexed> <http://www.w3.org/2000/01/rdf-schema#label> "indexed"^^<http://www.w3.org/2001/XMLSchema#token> .
<https://privatealpha.com/ontology/content-inventory/1#assumes> <http://www.w3.org/2000/01/rdf-schema#seeAlso> <http://purl.org/dc/terms/educationLevel> .
<https://privatealpha.com/ontology/content-inventory/1#landing> <http://www.w3.org/1999/02/22-rdf-syntax-ns#type> <http://purl.org/ontology/bibo/DocumentStatus> .
<https://privatealpha.com/ontology/content-inventory/1#proofread> <http://www.w3.org/1999/02/22-rdf-syntax-ns#type> <https://privatealpha.com/ontology/content-inventory/1#Action> .
<https://privatealpha.com/ontology/content-inventory/1#sections> <http://www.w3.org/1999/02/22-rdf-syntax-ns#type> <http://purl.org/linked-data/cube#MeasureProperty> .
<https://privatealpha.com/ontology/content-inventory/1#outdegree> <http://www.w3.org/2000/01/rdf-schema#comment> "The number of links emanating from the specified resource."@en .
<https://privatealpha.com/ontology/content-inventory/1#sd> <http://www.w3.org/2000/01/rdf-schema#domain> <http://purl.org/linked-data/cube#Observation> .
<https://privatealpha.com/ontology/content-inventory/1#sd> <http://www.w3.org/2000/01/rdf-schema#isDefinedBy> <https://privatealpha.com/ontology/content-inventory/1#> .
<https://privatealpha.com/ontology/content-inventory/1#values> <http://www.w3.org/1999/02/22-rdf-syntax-ns#type> <http://www.w3.org/2002/07/owl#ObjectProperty> .
<https://privatealpha.com/ontology/content-inventory/1#> <http://www.w3.org/2002/07/owl#imports> <http://purl.org/ontology/bibo/> .
<https://privatealpha.com/ontology/content-inventory/1#> <http://purl.org/dc/terms/references> <http://en.wikipedia.org/wiki/Standard_deviation> .
<https://privatealpha.com/ontology/content-inventory/1#circulated> <http://www.w3.org/1999/02/22-rdf-syntax-ns#type> <http://purl.org/ontology/bibo/DocumentStatus> .
<https://privatealpha.com/ontology/content-inventory/1#sections> <http://www.w3.org/2000/01/rdf-schema#range> <http://www.w3.org/2001/XMLSchema#nonNegativeInteger> .
<https://privatealpha.com/ontology/content-inventory/1#aware-of> <http://www.w3.org/2000/01/rdf-schema#label> "aware-of"^^<http://www.w3.org/2001/XMLSchema#token> .
<https://privatealpha.com/ontology/content-inventory/1#sd> <http://www.w3.org/2000/01/rdf-schema#range> <http://www.w3.org/2001/XMLSchema#number> .
_:B1fbf547cX2D3f36X2D42b5X2D92cfX2D39448acfe13e <http://purl.org/linked-data/cube#measure> <https://privatealpha.com/ontology/content-inventory/1#low-quartile> .
<https://privatealpha.com/ontology/content-inventory/1#embed> <http://www.w3.org/2000/01/rdf-schema#domain> <http://xmlns.com/foaf/0.1/Document> .
<https://privatealpha.com/ontology/content-inventory/1#action> <http://www.w3.org/2000/01/rdf-schema#range> <https://privatealpha.com/ontology/content-inventory/1#Action> .
<https://privatealpha.com/ontology/content-inventory/1#assumes> <http://www.w3.org/2000/01/rdf-schema#domain> <http://xmlns.com/foaf/0.1/Document> .
<https://privatealpha.com/ontology/content-inventory/1#indexed> <http://www.w3.org/2000/01/rdf-schema#comment> "This is a boolean value to indicate whether or not a resource ought to be indexed. It does not necessarily ascribe a policy: an absence of an explicit true value does not necessarily imply the resource ought not be indexed, but the presence of a false value probably should."@en .
<https://privatealpha.com/ontology/content-inventory/1#sections> <http://www.w3.org/2000/01/rdf-schema#label> "sections"^^<http://www.w3.org/2001/XMLSchema#token> .
<https://privatealpha.com/ontology/content-inventory/1#alias> <http://www.w3.org/2000/01/rdf-schema#subPropertyOf> <http://www.w3.org/2002/07/owl#sameAs> .
<https://privatealpha.com/ontology/content-inventory/1#obsolete> <http://www.w3.org/2000/01/rdf-schema#label> "obsolete"^^<http://www.w3.org/2001/XMLSchema#token> .
<https://privatealpha.com/ontology/content-inventory/1#low-quartile> <http://www.w3.org/1999/02/22-rdf-syntax-ns#type> <http://purl.org/linked-data/cube#MeasureProperty> .
<https://privatealpha.com/ontology/content-inventory/1#understands> <http://www.w3.org/2000/01/rdf-schema#label> "understands"^^<http://www.w3.org/2001/XMLSchema#token> .
<https://privatealpha.com/ontology/content-inventory/1#alias-for> <http://www.w3.org/2000/01/rdf-schema#isDefinedBy> <https://privatealpha.com/ontology/content-inventory/1#> .
<https://privatealpha.com/ontology/content-inventory/1#revise> <http://www.w3.org/2000/01/rdf-schema#isDefinedBy> <https://privatealpha.com/ontology/content-inventory/1#> .
_:B07c650f3X2D053eX2D46baX2D978dX2D09e37ca141e4 <http://www.w3.org/1999/02/22-rdf-syntax-ns#type> <http://purl.org/linked-data/cube#ComponentSpecification> .
<https://privatealpha.com/ontology/content-inventory/1#target> <http://www.w3.org/1999/02/22-rdf-syntax-ns#type> <http://www.w3.org/2002/07/owl#ObjectProperty> .
<https://privatealpha.com/ontology/content-inventory/1#> <http://www.w3.org/1999/xhtml/vocab#license> <http://creativecommons.org/licenses/by/2.5/ca/> .
<https://privatealpha.com/ontology/content-inventory/1#indegree> <http://www.w3.org/2000/01/rdf-schema#range> <http://www.w3.org/2001/XMLSchema#number> .
<https://privatealpha.com/ontology/content-inventory/1#> <http://purl.org/dc/terms/references> <http://www.w3.org/TR/vocab-data-cube/> .
<https://privatealpha.com/ontology/content-inventory/1#confidential> <http://www.w3.org/2000/01/rdf-schema#label> "confidential"^^<http://www.w3.org/2001/XMLSchema#token> .
<https://privatealpha.com/ontology/content-inventory/1#split> <http://www.w3.org/1999/02/22-rdf-syntax-ns#type> <https://privatealpha.com/ontology/content-inventory/1#Action> .
<https://privatealpha.com/ontology/content-inventory/1#indegree> <http://www.w3.org/2000/01/rdf-schema#domain> <http://purl.org/linked-data/cube#Observation> .
<https://privatealpha.com/ontology/content-inventory/1#indegree> <http://www.w3.org/2000/01/rdf-schema#isDefinedBy> <https://privatealpha.com/ontology/content-inventory/1#> .
<https://privatealpha.com/ontology/content-inventory/1#revise> <http://www.w3.org/2000/01/rdf-schema#comment> "Revise or restructure this document."@en .
<https://privatealpha.com/ontology/content-inventory/1#assumes> <http://www.w3.org/2000/01/rdf-schema#subPropertyOf> <http://purl.org/dc/terms/references> .
<https://privatealpha.com/ontology/content-inventory/1#canonical-slug> <http://www.w3.org/2000/01/rdf-schema#range> <http://www.w3.org/2001/XMLSchema#string> .
<https://privatealpha.com/ontology/content-inventory/1#document> <http://www.w3.org/2000/01/rdf-schema#range> <http://xmlns.com/foaf/0.1/Document> .
<https://privatealpha.com/ontology/content-inventory/1#tentative-merge> <http://www.w3.org/1999/02/22-rdf-syntax-ns#type> <https://privatealpha.com/ontology/content-inventory/1#Merge> .
<https://privatealpha.com/ontology/content-inventory/1#document> <http://www.w3.org/2000/01/rdf-schema#label> "document"^^<http://www.w3.org/2001/XMLSchema#token> .
<https://privatealpha.com/ontology/content-inventory/1#low-quartile> <http://www.w3.org/2000/01/rdf-schema#label> "low-quartile"^^<http://www.w3.org/2001/XMLSchema#token> .
<https://privatealpha.com/ontology/content-inventory/1#introduces> <http://www.w3.org/2000/01/rdf-schema#label> "introduces"^^<http://www.w3.org/2001/XMLSchema#token> .
<https://privatealpha.com/ontology/content-inventory/1#revise> <http://www.w3.org/2000/01/rdf-schema#label> "revise"^^<http://www.w3.org/2001/XMLSchema#token> .
<https://privatealpha.com/ontology/content-inventory/1#understands> <http://www.w3.org/2000/01/rdf-schema#seeAlso> <http://purl.org/dc/terms/educationLevel> .
<https://privatealpha.com/ontology/content-inventory/1#eschews> <http://www.w3.org/2000/01/rdf-schema#domain> <https://privatealpha.com/ontology/content-inventory/1#audience> .
_:Ba3d85955X2Dc6c8X2D41d5X2Db10bX2D082014a2959c <http://www.w3.org/1999/02/22-rdf-syntax-ns#type> <http://purl.org/linked-data/cube#ComponentSpecification> .
<https://privatealpha.com/ontology/content-inventory/1#slug> <http://www.w3.org/2000/01/rdf-schema#isDefinedBy> <https://privatealpha.com/ontology/content-inventory/1#> .
<https://privatealpha.com/ontology/content-inventory/1#max> <http://www.w3.org/1999/02/22-rdf-syntax-ns#type> <http://purl.org/linked-data/cube#MeasureProperty> .
<https://privatealpha.com/ontology/content-inventory/1#action> <http://www.w3.org/2000/01/rdf-schema#label> "action"^^<http://www.w3.org/2001/XMLSchema#token> .
<https://privatealpha.com/ontology/content-inventory/1#alias-for> <http://www.w3.org/2002/07/owl#inverseOf> <https://privatealpha.com/ontology/content-inventory/1#alias> .
<https://privatealpha.com/ontology/content-inventory/1#high-quartile> <http://www.w3.org/2000/01/rdf-schema#seeAlso> <http://en.wikipedia.org/wiki/Quartile> .
<https://privatealpha.com/ontology/content-inventory/1#slug> <http://www.w3.org/2000/01/rdf-schema#label> "slug"^^<http://www.w3.org/2001/XMLSchema#token> .
<https://privatealpha.com/ontology/content-inventory/1#words-and-blocks> <http://purl.org/linked-data/cube#component> _:B5d3bac10X2Dd039X2D4aadX2D984fX2Dc6a1bb911c65 .
<https://privatealpha.com/ontology/content-inventory/1#alias-for> <http://www.w3.org/2000/01/rdf-schema#comment> "Denotes that the subject is the alias URI, and the object is more canonical (though not necessarily the most canonical)."@en .
<https://privatealpha.com/ontology/content-inventory/1#words-and-blocks> <http://purl.org/linked-data/cube#component> _:B1ad310fdX2Dbce0X2D42f6X2D92a9X2D7326c4bb67df .
<https://privatealpha.com/ontology/content-inventory/1#mentions> <http://www.w3.org/2000/01/rdf-schema#comment> "The document explicitly mentions this concept."@en .
<https://privatealpha.com/ontology/content-inventory/1#> <http://www.w3.org/2000/01/rdf-schema#isDefinedBy> <https://privatealpha.com/ontology/content-inventory/1#> .
<https://privatealpha.com/ontology/content-inventory/1#high-quartile> <http://www.w3.org/2000/01/rdf-schema#comment> "Third Quartile"@en .
<https://privatealpha.com/ontology/content-inventory/1#introduces> <http://www.w3.org/2000/01/rdf-schema#domain> <http://xmlns.com/foaf/0.1/Document> .
<https://privatealpha.com/ontology/content-inventory/1#rewrite> <http://www.w3.org/2000/01/rdf-schema#isDefinedBy> <https://privatealpha.com/ontology/content-inventory/1#> .
_:B07c650f3X2D053eX2D46baX2D978dX2D09e37ca141e4 <http://purl.org/linked-data/cube#measure> <https://privatealpha.com/ontology/content-inventory/1#blocks> .
<https://privatealpha.com/ontology/content-inventory/1#understands> <http://www.w3.org/1999/02/22-rdf-syntax-ns#type> <http://www.w3.org/2002/07/owl#ObjectProperty> .
<https://privatealpha.com/ontology/content-inventory/1#mentions> <http://www.w3.org/1999/02/22-rdf-syntax-ns#type> <http://www.w3.org/2002/07/owl#ObjectProperty> .
<https://privatealpha.com/ontology/content-inventory/1#canonical> <http://www.w3.org/2000/01/rdf-schema#subPropertyOf> <https://privatealpha.com/ontology/content-inventory/1#alias-for> .
<https://privatealpha.com/ontology/content-inventory/1#unavailable> <http://www.w3.org/1999/02/22-rdf-syntax-ns#type> <http://purl.org/ontology/bibo/DocumentStatus> .
<https://privatealpha.com/ontology/content-inventory/1#update-metadata> <http://www.w3.org/1999/02/22-rdf-syntax-ns#type> <https://privatealpha.com/ontology/content-inventory/1#Action> .
<https://privatealpha.com/ontology/content-inventory/1#split> <http://www.w3.org/2000/01/rdf-schema#comment> "Split this document into multiple pieces."@en .
<https://privatealpha.com/ontology/content-inventory/1#confidential> <http://www.w3.org/1999/02/22-rdf-syntax-ns#type> <http://purl.org/ontology/bibo/DocumentStatus> .
<https://privatealpha.com/ontology/content-inventory/1#retire> <http://www.w3.org/2000/01/rdf-schema#isDefinedBy> <https://privatealpha.com/ontology/content-inventory/1#> .
<https://privatealpha.com/ontology/content-inventory/1#> <http://purl.org/dc/terms/modified> "2014-02-06T14:10:00-08:00"^^<http://www.w3.org/2001/XMLSchema#dateTime> .
<https://privatealpha.com/ontology/content-inventory/1#> <http://purl.org/dc/terms/created> "2012-01-23T11:52:00-08:00"^^<http://www.w3.org/2001/XMLSchema#dateTime> .
<https://privatealpha.com/ontology/content-inventory/1#update-metadata> <http://www.w3.org/2000/01/rdf-schema#label> "update-metadata"^^<http://www.w3.org/2001/XMLSchema#token> .
<https://privatealpha.com/ontology/content-inventory/1> <http://www.w3.org/1999/02/22-rdf-syntax-ns#type> <http://purl.org/ontology/bibo/Webpage> .
<https://privatealpha.com/ontology/content-inventory/1#> <http://purl.org/dc/terms/references> <http://publishing-statistical-data.googlecode.com/svn/trunk/specs/src/main/html/cube.html#ref_qb_MeasureProperty> .
<https://privatealpha.com/ontology/content-inventory/1#> <http://www.w3.org/1999/02/22-rdf-syntax-ns#type> <http://www.w3.org/2002/07/owl#Ontology> .
<https://privatealpha.com/ontology/content-inventory/1#Action> <http://www.w3.org/1999/02/22-rdf-syntax-ns#type> <http://www.w3.org/2002/07/owl#Class> .
_:Bfd383f50X2D9fc1X2D479bX2D87deX2Ddbc543ff3f94 <http://purl.org/linked-data/cube#dimension> <https://privatealpha.com/ontology/content-inventory/1#document> .
<https://privatealpha.com/ontology/content-inventory/1#understands> <http://www.w3.org/2000/01/rdf-schema#isDefinedBy> <https://privatealpha.com/ontology/content-inventory/1#> .
<https://privatealpha.com/ontology/content-inventory/1#Action> <http://www.w3.org/2000/01/rdf-schema#comment> "An action, as its name implies, is meant to represent something a person or other agent ought to do to a document."@en .
<https://privatealpha.com/ontology/content-inventory/1#values> <http://www.w3.org/2000/01/rdf-schema#range> <http://www.w3.org/2004/02/skos/core#Concept> .
<https://privatealpha.com/ontology/content-inventory/1#mentions> <http://www.w3.org/2000/01/rdf-schema#isDefinedBy> <https://privatealpha.com/ontology/content-inventory/1#> .
<https://privatealpha.com/ontology/content-inventory/1#mean> <http://www.w3.org/2000/01/rdf-schema#range> <http://www.w3.org/2001/XMLSchema#number> .
_:Ba3d85955X2Dc6c8X2D41d5X2Db10bX2D082014a2959c <http://purl.org/linked-data/cube#measure> <https://privatealpha.com/ontology/content-inventory/1#mean> .
<https://privatealpha.com/ontology/content-inventory/1#mean> <http://www.w3.org/2000/01/rdf-schema#isDefinedBy> <https://privatealpha.com/ontology/content-inventory/1#> .
<https://privatealpha.com/ontology/content-inventory/1#mean> <http://www.w3.org/2000/01/rdf-schema#domain> <http://purl.org/linked-data/cube#Observation> .
<https://privatealpha.com/ontology/content-inventory/1#sd> <http://www.w3.org/2000/01/rdf-schema#seeAlso> <http://en.wikipedia.org/wiki/Standard_deviation> .
_:B1fbf547cX2D3f36X2D42b5X2D92cfX2D39448acfe13e <http://www.w3.org/1999/02/22-rdf-syntax-ns#type> <http://purl.org/linked-data/cube#ComponentSpecification> .
_:Bcc48f0eaX2D2180X2D4228X2Dbe25X2D32444277b9f8 <http://www.w3.org/1999/02/22-rdf-syntax-ns#type> <http://purl.org/linked-data/cube#ComponentSpecification> .
<https://privatealpha.com/ontology/content-inventory/1#embed> <http://www.w3.org/2000/01/rdf-schema#label> "embed"^^<http://www.w3.org/2001/XMLSchema#token> .
_:Ba7283634X2D00bbX2D4e75X2Da641X2D67b5556457c0 <http://purl.org/linked-data/cube#measure> <https://privatealpha.com/ontology/content-inventory/1#sections> .
<https://privatealpha.com/ontology/content-inventory/1#> <http://purl.org/dc/terms/references> <http://vocab.org/frbr/extended> .
<https://privatealpha.com/ontology/content-inventory/1#alias-for> <http://www.w3.org/1999/02/22-rdf-syntax-ns#type> <http://www.w3.org/2002/07/owl#ObjectProperty> .
<https://privatealpha.com/ontology/content-inventory/1#slug> <http://www.w3.org/1999/02/22-rdf-syntax-ns#type> <http://www.w3.org/2002/07/owl#DatatypeProperty> .
<https://privatealpha.com/ontology/content-inventory/1#keep> <http://www.w3.org/2000/01/rdf-schema#isDefinedBy> <https://privatealpha.com/ontology/content-inventory/1#> .
<https://privatealpha.com/ontology/content-inventory/1#characters> <http://www.w3.org/2000/01/rdf-schema#label> "characters"^^<http://www.w3.org/2001/XMLSchema#token> .
<https://privatealpha.com/ontology/content-inventory/1#incorrect> <http://www.w3.org/2000/01/rdf-schema#isDefinedBy> <https://privatealpha.com/ontology/content-inventory/1#> .
<https://privatealpha.com/ontology/content-inventory/1#Advertisement> <http://www.w3.org/2000/01/rdf-schema#subClassOf> <http://xmlns.com/foaf/0.1/Document> .
<https://privatealpha.com/ontology/content-inventory/1#Merge> <http://www.w3.org/2000/01/rdf-schema#isDefinedBy> <https://privatealpha.com/ontology/content-inventory/1#> .
<https://privatealpha.com/ontology/content-inventory/1#Advertisement> <http://www.w3.org/2000/01/rdf-schema#isDefinedBy> <https://privatealpha.com/ontology/content-inventory/1#> .
<https://privatealpha.com/ontology/content-inventory/1#incorrect> <http://www.w3.org/2000/01/rdf-schema#comment> "The content of this document is factually wrong."@en .
<https://privatealpha.com/ontology/content-inventory/1#words> <http://www.w3.org/2000/01/rdf-schema#range> <http://www.w3.org/2001/XMLSchema#nonNegativeInteger> .
<https://privatealpha.com/ontology/content-inventory/1#max> <http://www.w3.org/2000/01/rdf-schema#label> "max"^^<http://www.w3.org/2001/XMLSchema#token> .
_:Bfbbe042bX2Dd590X2D4ff4X2Db1f9X2D47f0a34e8b98 <http://www.w3.org/1999/02/22-rdf-syntax-ns#type> <http://purl.org/linked-data/cube#ComponentSpecification> .
<https://privatealpha.com/ontology/content-inventory/1#Audience> <http://www.w3.org/2000/01/rdf-schema#comment> "An audience represents the set of people who are the intended recipients of the resource. This class is at once an agent class as well as a conceptual entity, capable of being mixed into a SKOS concept scheme."@en .
<https://privatealpha.com/ontology/content-inventory/1#median> <http://www.w3.org/2000/01/rdf-schema#comment> "The median of a population "@en .
<https://privatealpha.com/ontology/content-inventory/1#> <http://purl.org/dc/terms/modified> "2019-07-10T22:28:06Z"^^<http://www.w3.org/2001/XMLSchema#dateTime> .
<https://privatealpha.com/ontology/content-inventory/1#mentions> <http://www.w3.org/2000/01/rdf-schema#range> <http://www.w3.org/2004/02/skos/core#Concept> .
<https://privatealpha.com/ontology/content-inventory/1#landing> <http://www.w3.org/2000/01/rdf-schema#label> "landing"^^<http://www.w3.org/2001/XMLSchema#token> .
<https://privatealpha.com/ontology/content-inventory/1#values> <http://www.w3.org/2000/01/rdf-schema#isDefinedBy> <https://privatealpha.com/ontology/content-inventory/1#> .
<https://privatealpha.com/ontology/content-inventory/1#understands> <http://www.w3.org/2000/01/rdf-schema#range> <http://www.w3.org/2004/02/skos/core#Concept> .
<https://privatealpha.com/ontology/content-inventory/1#min> <http://www.w3.org/1999/02/22-rdf-syntax-ns#type> <http://purl.org/linked-data/cube#MeasureProperty> .
<https://privatealpha.com/ontology/content-inventory/1#> <http://purl.org/dc/terms/references> <http://vocab.org/frbr/core> .
<https://privatealpha.com/ontology/content-inventory/1#> <http://www.w3.org/2002/07/owl#versionInfo> "0.11" .
<https://privatealpha.com/ontology/content-inventory/1#orphan> <http://www.w3.org/1999/02/22-rdf-syntax-ns#type> <http://purl.org/ontology/bibo/DocumentStatus> .
<https://privatealpha.com/ontology/content-inventory/1#Audience> <http://www.w3.org/2000/01/rdf-schema#subClassOf> <http://www.w3.org/2004/02/skos/core#Concept> .
<https://privatealpha.com/ontology/content-inventory/1#retired> <http://www.w3.org/2000/01/rdf-schema#isDefinedBy> <https://privatealpha.com/ontology/content-inventory/1#> .
<https://privatealpha.com/ontology/content-inventory/1#values> <http://www.w3.org/2000/01/rdf-schema#subPropertyOf> <http://www.w3.org/2004/02/skos/core#related> .
<https://privatealpha.com/ontology/content-inventory/1#non-audience> <http://www.w3.org/2000/01/rdf-schema#range> <http://purl.org/dc/terms/AgentClass> .
<https://privatealpha.com/ontology/content-inventory/1#target> <http://www.w3.org/2000/01/rdf-schema#isDefinedBy> <https://privatealpha.com/ontology/content-inventory/1#> .
<https://doriantaylor.com/person/dorian-taylor#me> <http://xmlns.com/foaf/0.1/name> "Dorian Taylor"@en .
<https://privatealpha.com/ontology/content-inventory/1#introduces> <http://www.w3.org/2000/01/rdf-schema#range> <http://www.w3.org/2004/02/skos/core#Concept> .
<https://privatealpha.com/ontology/content-inventory/1#assumes> <http://www.w3.org/2000/01/rdf-schema#isDefinedBy> <https://privatealpha.com/ontology/content-inventory/1#> .
<https://privatealpha.com/ontology/content-inventory/1#embed> <http://www.w3.org/2000/01/rdf-schema#isDefinedBy> <https://privatealpha.com/ontology/content-inventory/1#> .
<https://privatealpha.com/ontology/content-inventory/1#sd> <http://www.w3.org/2000/01/rdf-schema#label> "sd"^^<http://www.w3.org/2001/XMLSchema#token> .
<https://privatealpha.com/ontology/content-inventory/1#words> <http://www.w3.org/2000/01/rdf-schema#comment> "This indicates the number of words in a document, similar to the familiar function in a word processor. The exact method of counting words may vary by document type, language etc., and is thus out of scope from this document."@en .
<https://privatealpha.com/ontology/content-inventory/1#canonical> <http://www.w3.org/2000/01/rdf-schema#isDefinedBy> <https://privatealpha.com/ontology/content-inventory/1#> .
<https://privatealpha.com/ontology/content-inventory/1#incomplete> <http://www.w3.org/2000/01/rdf-schema#label> "incomplete"^^<http://www.w3.org/2001/XMLSchema#token> .
<https://privatealpha.com/ontology/content-inventory/1#values> <http://www.w3.org/2000/01/rdf-schema#seeAlso> <https://privatealpha.com/ontology/content-inventory/1#eschews> .
<https://privatealpha.com/ontology/content-inventory/1#outdegree> <http://www.w3.org/1999/02/22-rdf-syntax-ns#type> <http://purl.org/linked-data/cube#MeasureProperty> .
<https://privatealpha.com/ontology/content-inventory/1#indexed> <http://www.w3.org/1999/02/22-rdf-syntax-ns#type> <http://www.w3.org/2002/07/owl#FunctionalProperty> .
<https://privatealpha.com/ontology/content-inventory/1#embed> <http://www.w3.org/2000/01/rdf-schema#subPropertyOf> <http://purl.org/dc/terms/hasPart> .
<https://privatealpha.com/ontology/content-inventory/1#words> <http://www.w3.org/1999/02/22-rdf-syntax-ns#type> <http://purl.org/linked-data/cube#MeasureProperty> .
<https://privatealpha.com/ontology/content-inventory/1#words-and-blocks> <http://purl.org/linked-data/cube#component> _:Bfbbe042bX2Dd590X2D4ff4X2Db1f9X2D47f0a34e8b98 .
<https://privatealpha.com/ontology/content-inventory/1#> <http://purl.org/dc/terms/modified> "2012-12-11T22:22:00-08:00"^^<http://www.w3.org/2001/XMLSchema#dateTime> .
<https://privatealpha.com/ontology/content-inventory/1#words> <http://www.w3.org/2000/01/rdf-schema#label> "words"^^<http://www.w3.org/2001/XMLSchema#token> .
<https://privatealpha.com/ontology/content-inventory/1#> <http://www.w3.org/2002/07/owl#imports> <http://purl.org/dc/terms/> .
<https://privatealpha.com/ontology/content-inventory/1#outdegree> <http://www.w3.org/2000/01/rdf-schema#seeAlso> <http://en.wikipedia.org/wiki/Directed_graph#Indegree_and_outdegree> .
<https://privatealpha.com/ontology/content-inventory/1#blocks> <http://www.w3.org/2000/01/rdf-schema#comment> "A block count is conceptually similar to a word or section count, though it counts the total of elements in the document considered to be text blocks, such as paragraphs, tables, lists and figures. It is suited for document types that have no concept of (semantic) sections, such as HTML. The purpose of this measurement is to provide a sort of ratio to the word count, to glean how well-proportioned the document is."@en .
<https://privatealpha.com/ontology/content-inventory/1#introduces> <http://www.w3.org/2000/01/rdf-schema#comment> "The document defines, describes, or otherwise introduces the audience to this concept."@en .
_:Bcbbc9d5fX2D1b1dX2D4342X2D9009X2D72d442a1e643 <http://www.w3.org/1999/02/22-rdf-syntax-ns#type> <http://purl.org/linked-data/cube#ComponentSpecification> .
<https://privatealpha.com/ontology/content-inventory/1#empty> <http://www.w3.org/2000/01/rdf-schema#label> "empty"^^<http://www.w3.org/2001/XMLSchema#token> .
<https://privatealpha.com/ontology/content-inventory/1#canonical-slug> <http://www.w3.org/1999/02/22-rdf-syntax-ns#type> <http://www.w3.org/2002/07/owl#FunctionalProperty> .
<https://privatealpha.com/ontology/content-inventory/1#unavailable> <http://www.w3.org/2000/01/rdf-schema#label> "unavailable"^^<http://www.w3.org/2001/XMLSchema#token> .
<https://privatealpha.com/ontology/content-inventory/1#action> <http://www.w3.org/2000/01/rdf-schema#comment> "use this to signal an action to take with the document in question."@en .
<https://privatealpha.com/ontology/content-inventory/1#understands> <http://www.w3.org/2000/01/rdf-schema#subPropertyOf> <https://privatealpha.com/ontology/content-inventory/1#aware-of> .
<https://privatealpha.com/ontology/content-inventory/1#eschews> <http://www.w3.org/2000/01/rdf-schema#comment> "This property relates an Audience to a SKOS concept that members of the audience are known to actively avoid or regard with contempt. This relation is intended to represent the complement of values."@en .
<https://privatealpha.com/ontology/content-inventory/1#obsolete> <http://www.w3.org/1999/02/22-rdf-syntax-ns#type> <http://purl.org/ontology/bibo/DocumentStatus> .
<https://privatealpha.com/ontology/content-inventory/1#characters> <http://www.w3.org/2000/01/rdf-schema#domain> <http://purl.org/linked-data/cube#Observation> .
<https://privatealpha.com/ontology/content-inventory/1#characters> <http://www.w3.org/2000/01/rdf-schema#isDefinedBy> <https://privatealpha.com/ontology/content-inventory/1#> .
<https://privatealpha.com/ontology/content-inventory/1#canonical-slug> <http://www.w3.org/2000/01/rdf-schema#label> "canonical-slug"^^<http://www.w3.org/2001/XMLSchema#token> .
<https://privatealpha.com/ontology/content-inventory/1#words-and-blocks> <http://purl.org/linked-data/cube#component> _:B8151917aX2D1a15X2D42dfX2D91a7X2De5106cce1e93 .
<https://privatealpha.com/ontology/content-inventory/1#median> <http://www.w3.org/2000/01/rdf-schema#seeAlso> <http://en.wikipedia.org/wiki/Median> .
<https://privatealpha.com/ontology/content-inventory/1#> <http://purl.org/dc/terms/title> "A Content Inventory Vocabulary"@en .
<https://privatealpha.com/ontology/content-inventory/1#> <http://www.w3.org/2002/07/owl#imports> <http://purl.org/NET/c4dm/event.owl#> .
<https://privatealpha.com/ontology/content-inventory/1#alias> <http://www.w3.org/2000/01/rdf-schema#isDefinedBy> <https://privatealpha.com/ontology/content-inventory/1#> .
<https://privatealpha.com/ontology/content-inventory/1#assumes> <http://www.w3.org/2000/01/rdf-schema#range> <http://www.w3.org/2004/02/skos/core#Concept> .
<https://privatealpha.com/ontology/content-inventory/1#alias> <http://www.w3.org/2000/01/rdf-schema#label> "alias"^^<http://www.w3.org/2001/XMLSchema#token> .
<https://privatealpha.com/ontology/content-inventory/1#introduces> <http://www.w3.org/2000/01/rdf-schema#isDefinedBy> <https://privatealpha.com/ontology/content-inventory/1#> .
<https://privatealpha.com/ontology/content-inventory/1#alias-for> <http://www.w3.org/2000/01/rdf-schema#subPropertyOf> <http://www.w3.org/2002/07/owl#sameAs> .
<https://privatealpha.com/ontology/content-inventory/1#link> <http://www.w3.org/2000/01/rdf-schema#comment> "This property specifies a linked resource which is visible in the subject's user interface."@en .
