<http://purl.org/csm/1.0#hasRewardMechanism> <http://www.w3.org/2000/01/rdf-schema#label> "has Reward Mechanism" .
<http://purl.org/csm/1.0#title> <http://www.w3.org/2000/01/rdf-schema#comment> "The data property csm:title is a short phrase to improve the human readability of an instance." .
<http://purl.org/csm/1.0#hardwareDevice> <http://www.w3.org/2000/01/rdf-schema#comment> "any hardware device (e.g., personal computer, mobile phone, smartphone, tablet computer)" .
<http://purl.org/csm/1.0#Proportional> <http://www.w3.org/1999/02/22-rdf-syntax-ns#type> <http://www.w3.org/2002/07/owl#NamedIndividual> .
<http://purl.org/csm/1.0#External> <http://www.w3.org/2000/01/rdf-schema#comment> "Example: to gain insights about service experience,  provide ideas for new product design" .
<http://purl.org/csm/1.0#Code> <http://www.w3.org/1999/02/22-rdf-syntax-ns#type> <http://purl.org/csm/1.0#ActionType> .
<http://purl.org/csm/1.0#External> <http://www.w3.org/2000/01/rdf-schema#label> "external" .
<http://purl.org/csm/1.0#NoReward> <http://www.w3.org/1999/02/22-rdf-syntax-ns#type> <http://www.w3.org/2002/07/owl#NamedIndividual> .
<http://purl.org/csm/1.0#category> <http://www.w3.org/2000/01/rdf-schema#range> <http://www.w3.org/2000/01/rdf-schema#Literal> .
<http://purl.org/csm/1.0#ActionType> <http://www.w3.org/1999/02/22-rdf-syntax-ns#type> <http://www.w3.org/2002/07/owl#Class> .
<http://purl.org/csm/1.0#PerformanceBased> <http://www.w3.org/2000/01/rdf-schema#label> "performance based" .
<http://purl.org/csm/1.0#hardwareDevice> <http://www.w3.org/2000/01/rdf-schema#range> <http://www.w3.org/2000/01/rdf-schema#Literal> .
<http://purl.org/csm/1.0#Iterative> <http://www.w3.org/1999/02/22-rdf-syntax-ns#type> <http://www.w3.org/2002/07/owl#NamedIndividual> .
<http://purl.org/csm/1.0#amount> <http://www.w3.org/1999/02/22-rdf-syntax-ns#type> <http://www.w3.org/2002/07/owl#DatatypeProperty> .
<http://purl.org/csm/1.0#AcceptReject> <http://www.w3.org/2000/01/rdf-schema#label> "accept or reject" .
<http://purl.org/csm/1.0#amount> <http://www.w3.org/2000/01/rdf-schema#domain> <http://purl.org/csm/1.0#RewardMechanism> .
<http://purl.org/csm/1.0#hasNext> <http://www.w3.org/1999/02/22-rdf-syntax-ns#type> <http://www.w3.org/2002/07/owl#ObjectProperty> .
<http://purl.org/csm/1.0#qualificationType> <http://www.w3.org/2000/01/rdf-schema#domain> <http://purl.org/csm/1.0#HumanRequirement> .
<http://purl.org/csm/1.0#ageMin> <http://www.w3.org/2000/01/rdf-schema#range> <http://www.w3.org/2001/XMLSchema#unsignedByte> .
<http://purl.org/csm/1.0#Project> <http://www.w3.org/2000/01/rdf-schema#label> "Project" .
<http://purl.org/csm/1.0#ageMin> <http://www.w3.org/2000/01/rdf-schema#label> "minimum age" .
<http://purl.org/csm/1.0#ageMin> <http://www.w3.org/1999/02/22-rdf-syntax-ns#type> <http://www.w3.org/2002/07/owl#DatatypeProperty> .
<http://purl.org/csm/1.0#Verify> <http://www.w3.org/2000/01/rdf-schema#label> "verify" .
<http://purl.org/csm/1.0#User> <http://www.w3.org/2000/01/rdf-schema#comment> "The class csm:User defines a  person or an organization that is involved in a crowdsourcing activity." .
<http://purl.org/csm/1.0#Simultaneously> <http://www.w3.org/2000/01/rdf-schema#label> "simultaneously" .
<http://purl.org/csm/1.0#SolveProblem> <http://www.w3.org/2000/01/rdf-schema#label> "solve problem" .
<http://purl.org/csm/1.0#EvaluationMechanism> <http://www.w3.org/1999/02/22-rdf-syntax-ns#type> <http://www.w3.org/2002/07/owl#Class> .
<http://purl.org/csm/1.0#hasNext> <http://www.w3.org/2000/01/rdf-schema#range> <http://purl.org/csm/1.0#Task> .
<http://purl.org/csm/1.0#priorityLevel> <http://www.w3.org/2000/01/rdf-schema#label> "priority level" .
<http://purl.org/csm/1.0#NeutralPriority> <http://www.w3.org/1999/02/22-rdf-syntax-ns#type> <http://www.w3.org/2002/07/owl#NamedIndividual> .
<http://purl.org/csm/1.0#hasPayoutMethod> <http://www.w3.org/1999/02/22-rdf-syntax-ns#type> <http://www.w3.org/2002/07/owl#ObjectProperty> .
<http://purl.org/csm/1.0#country> <http://www.w3.org/2000/01/rdf-schema#range> <http://www.w3.org/2001/XMLSchema#string> .
<http://purl.org/csm/1.0#softwarePlatform> <http://www.w3.org/2000/01/rdf-schema#comment> "any operating system independent platform (e.g., Java, Firefox)" .
<http://purl.org/csm/1.0#gender> <http://www.w3.org/2000/01/rdf-schema#range> <http://www.w3.org/2001/XMLSchema#unsignedByte> .
<http://purl.org/csm/1.0#MajorityDecision> <http://www.w3.org/1999/02/22-rdf-syntax-ns#type> <http://www.w3.org/2002/07/owl#NamedIndividual> .
<http://purl.org/csm/1.0#ageMax> <http://www.w3.org/2000/01/rdf-schema#comment> "The data property csm:ageMax defines the maximum age in years." .
<http://purl.org/csm/1.0#hasPayoutMethod> <http://www.w3.org/2000/01/rdf-schema#domain> <http://purl.org/csm/1.0#RewardMechanism> .
<http://purl.org/csm/1.0#AllParticipants> <http://www.w3.org/2000/01/rdf-schema#label> "all participants" .
<http://purl.org/csm/1.0#User> <http://www.w3.org/2002/07/owl#equivalentClass> _:B29bdffeaX2Daa8dX2D45b1X2D86f4X2D0d62657c2eed .
<http://purl.org/csm/1.0#Lottery> <http://www.w3.org/1999/02/22-rdf-syntax-ns#type> <http://www.w3.org/2002/07/owl#NamedIndividual> .
<http://purl.org/csm/1.0#jobTitle> <http://www.w3.org/2000/01/rdf-schema#label> "job title" .
<http://purl.org/csm/1.0#gender> <http://www.w3.org/1999/02/22-rdf-syntax-ns#type> <http://www.w3.org/2002/07/owl#DatatypeProperty> .
<http://purl.org/csm/1.0#AssessmentForm> <http://www.w3.org/1999/02/22-rdf-syntax-ns#type> <http://purl.org/csm/1.0#EvaluationSpecificity> .
<http://purl.org/csm/1.0#SolveProblem> <http://www.w3.org/2000/01/rdf-schema#comment> "to solve complex theoretical and practical problems, e.g, finding an algorithm" .
<http://purl.org/csm/1.0#country> <http://www.w3.org/2000/01/rdf-schema#comment> "The data property csm:country defines the country in which a participant should live (use 3-digit country code according to ISO 3166-1 alpha-3)." .
<http://purl.org/csm/1.0#ageMin> <http://www.w3.org/2000/01/rdf-schema#comment> "The data property csm:ageMin defines the minimum age in years." .
<http://purl.org/csm/1.0#numberOfAssignments> <http://www.w3.org/2000/01/rdf-schema#range> <http://www.w3.org/2001/XMLSchema#unsignedInt> .
<http://purl.org/csm/1.0#ThirdParty> <http://www.w3.org/1999/02/22-rdf-syntax-ns#type> <http://www.w3.org/2002/07/owl#NamedIndividual> .
<http://purl.org/csm/1.0#description> <http://www.w3.org/2000/01/rdf-schema#domain> <http://purl.org/csm/1.0#Task> .
<http://purl.org/csm/1.0#language> <http://www.w3.org/1999/02/22-rdf-syntax-ns#type> <http://www.w3.org/2002/07/owl#DatatypeProperty> .
<http://purl.org/csm/1.0#goal> <http://www.w3.org/1999/02/22-rdf-syntax-ns#type> <http://www.w3.org/2002/07/owl#DatatypeProperty> .
<http://purl.org/csm/1.0#Discount> <http://www.w3.org/2000/01/rdf-schema#label> "discount" .
<http://purl.org/csm/1.0#operatingSystem> <http://www.w3.org/2000/01/rdf-schema#comment> "The data property csm:operatingSystem defines any operating system for personal computers or mobile devices (e.g., Microsoft Windows, OS X, Linux, Android, Windows Phone, iOS)." .
<http://purl.org/csm/1.0#RewardMechanism> <http://www.w3.org/1999/02/22-rdf-syntax-ns#type> <http://www.w3.org/2002/07/owl#Class> .
<http://purl.org/csm/1.0#GenerateIdea> <http://www.w3.org/2000/01/rdf-schema#comment> "to collect innovative product or service ideas using brainstorming" .
<http://purl.org/csm/1.0#estimatedDuration> <http://www.w3.org/2000/01/rdf-schema#domain> <http://purl.org/csm/1.0#Task> .
<http://purl.org/csm/1.0#ResourceAccess> <http://www.w3.org/1999/02/22-rdf-syntax-ns#type> <http://purl.org/csm/1.0#RewardType> .
<http://purl.org/csm/1.0#ActionType> <http://www.w3.org/2000/01/rdf-schema#seeAlso> "Doan, A., Ramakrishnan, R., & Halevy, A. Y. (2011). Crowdsourcing systems on the World-Wide Web. Communications of the ACM, 54(4), 86–96." .
<http://purl.org/csm/1.0#amount> <http://www.w3.org/2000/01/rdf-schema#label> "amount" .
<http://purl.org/csm/1.0#numberOfAssignments> <http://www.w3.org/2000/01/rdf-schema#comment> "The data property csm:numberOfAssignments defines the number of participants who will be assigned to one task." .
<http://purl.org/csm/1.0#estimatedDuration> <http://www.w3.org/2000/01/rdf-schema#range> <http://www.w3.org/2001/XMLSchema#int> .
<http://purl.org/csm/1.0#issues> <http://www.w3.org/2000/01/rdf-schema#range> <http://purl.org/csm/1.0#Project> .
<http://purl.org/csm/1.0#Write> <http://www.w3.org/2000/01/rdf-schema#comment> "to describe something or someone" .
<http://purl.org/csm/1.0#GenerateIdea> <http://www.w3.org/1999/02/22-rdf-syntax-ns#type> <http://www.w3.org/2002/07/owl#NamedIndividual> .
<http://purl.org/csm/1.0#description> <http://www.w3.org/2000/01/rdf-schema#comment> "The data property csm:description describes the instance readable for humans." .
<http://purl.org/csm/1.0#softwarePlatform> <http://www.w3.org/2000/01/rdf-schema#label> "software platform" .
<http://purl.org/csm/1.0#EvaluationSpecificity> <http://www.w3.org/2000/01/rdf-schema#label> "Evaluation Specificity" .
<http://purl.org/csm/1.0#numberOfAssignments> <http://www.w3.org/1999/02/22-rdf-syntax-ns#type> <http://www.w3.org/2002/07/owl#DatatypeProperty> .
<http://purl.org/csm/1.0#Simultaneously> <http://www.w3.org/2000/01/rdf-schema#comment> "The evaluation subject is simultaneously evaluated during solving the crowdsourcing task. This applies to both participants and contributions." .
<http://purl.org/csm/1.0#closureTime> <http://www.w3.org/2000/01/rdf-schema#comment> "The data property csm:closureTime defines the time when the task expires." .
<http://purl.org/csm/1.0#hasActionType> <http://www.w3.org/2000/01/rdf-schema#domain> <http://purl.org/csm/1.0#Task> .
<http://purl.org/csm/1.0#approvalRate> <http://www.w3.org/2000/01/rdf-schema#comment> "The data property csm:approval Rate defines the ratio of properly solved tasks to the number of submitted tasks." .
<http://purl.org/csm/1.0#hasRewardNature> <http://www.w3.org/2000/01/rdf-schema#label> "has Reward Nature" .
<http://purl.org/csm/1.0#Contribution> <http://www.w3.org/2000/01/rdf-schema#label> "Contribution" .
<http://purl.org/csm/1.0#currency> <http://www.w3.org/2000/01/rdf-schema#label> "currency" .
<http://purl.org/csm/1.0#Requester> <http://www.w3.org/1999/02/22-rdf-syntax-ns#type> <http://www.w3.org/2002/07/owl#Class> .
<http://purl.org/csm/1.0#submits> <http://www.w3.org/2000/01/rdf-schema#label> "submits" .
<http://purl.org/csm/1.0#Integrative> <http://www.w3.org/2000/01/rdf-schema#label> "integrative" .
<http://purl.org/csm/1.0#interactionMode> <http://www.w3.org/2000/01/rdf-schema#label> "interaction mode" .
<http://purl.org/csm/1.0#interactionMode> <http://www.w3.org/2000/01/rdf-schema#domain> <http://purl.org/csm/1.0#Task> .
<http://purl.org/csm/1.0#Rank> <http://www.w3.org/2000/01/rdf-schema#comment> "to put someone or something in order (synonym: order, arrange)" .
<http://purl.org/csm/1.0#country> <http://www.w3.org/2000/01/rdf-schema#label> "country" .
<http://purl.org/csm/1.0#category> <http://www.w3.org/2000/01/rdf-schema#label> "category" .
<http://purl.org/csm/1.0#GenerateIdea> <http://www.w3.org/1999/02/22-rdf-syntax-ns#type> <http://purl.org/csm/1.0#ActionType> .
<http://purl.org/csm/1.0#ControlGroup> <http://www.w3.org/2000/01/rdf-schema#comment> "The control group approach assigns the task to one worker who completes the task. Afterwards, the crowdsourcing system sends the control group multiple validation tasks with the request to rate the submitted solutions. The solution will be accepted if the majority of the control group members decide it is correct." .
<http://purl.org/csm/1.0#ThirdParty> <http://www.w3.org/1999/02/22-rdf-syntax-ns#type> <http://purl.org/csm/1.0#EvaluationSource> .
<http://purl.org/csm/1.0#hasEvaluationMethod> <http://www.w3.org/2000/01/rdf-schema#range> <http://purl.org/csm/1.0#EvaluationMethod> .
<http://purl.org/csm/1.0> <http://purl.org/dc/elements/1.1/rights> "This work is distributed under a Creative Commons Attribution License (http://creativecommons.org/licenses/by/3.0/)."@en .
<http://purl.org/csm/1.0#TopXParticipants> <http://www.w3.org/2000/01/rdf-schema#label> "top X participants" .
<http://purl.org/csm/1.0#hasExternalResource> <http://www.w3.org/2000/01/rdf-schema#domain> <http://purl.org/csm/1.0#Task> .
<http://purl.org/csm/1.0#category> <http://www.w3.org/1999/02/22-rdf-syntax-ns#type> <http://www.w3.org/2002/07/owl#DatatypeProperty> .
<http://purl.org/csm/1.0#hardwareDevice> <http://www.w3.org/1999/02/22-rdf-syntax-ns#type> <http://www.w3.org/2002/07/owl#DatatypeProperty> .
<http://purl.org/csm/1.0#HumanRequirement> <http://www.w3.org/2000/01/rdf-schema#comment> "The class csm:HumanRequirement configures the characteristics of the crowd, such as the gender, the age, the spoken language, or the country of origin. Other attributes considered in the ontology define the qualifications of the participant. These are the job title, the qualification type, the corresponding qualification level, and the number of approved tasks of a certain qualification." .
<http://purl.org/csm/1.0#Immediate> <http://www.w3.org/2000/01/rdf-schema#label> "immediate" .
<http://purl.org/csm/1.0#estimatedDuration> <http://www.w3.org/2000/01/rdf-schema#label> "estimated duration" .
<http://purl.org/csm/1.0#amount> <http://www.w3.org/2000/01/rdf-schema#range> <http://www.w3.org/2001/XMLSchema#float> .
<http://purl.org/csm/1.0#Code> <http://www.w3.org/1999/02/22-rdf-syntax-ns#type> <http://www.w3.org/2002/07/owl#NamedIndividual> .
<http://purl.org/csm/1.0#goal> <http://www.w3.org/2000/01/rdf-schema#range> <http://www.w3.org/2000/01/rdf-schema#Literal> .
<http://purl.org/csm/1.0#submissionTime> <http://www.w3.org/2000/01/rdf-schema#label> "submission time" .
<http://purl.org/csm/1.0#EvaluationSpecificity> <http://www.w3.org/2000/01/rdf-schema#comment> "The class csm:EvaluationSpecificity refers to the specificity of the evaluation, which may be a simple acceptance or rejection, a rating, for example, on a five star rating scale, an assessment form that codifies domain knowledge into pre-authored statements, or a custom free text response." .
<http://purl.org/csm/1.0#title> <http://www.w3.org/2000/01/rdf-schema#domain> <http://purl.org/csm/1.0#Task> .
<http://purl.org/csm/1.0#EvaluationTime> <http://www.w3.org/2000/01/rdf-schema#seeAlso> "Corney, J. R., Torres-Sánchez, C., Jagadeesan, A. P., Yan, X. T., Regli, W. C., & Medellin, H. (2010). Putting the crowd to work in a knowledge-based factory. Advanced Engineering Informatics, 24(3), 243–250.\n\nMashhadi, A. J., & Capra, L. (2011). Quality control for real-time ubiquitous crowdsourcing. In Proceedings of the 2nd International Workshop on Ubiquitous Crowdsouring (pp. 5–8). New York, NY, USA: ACM." .
<http://purl.org/csm/1.0#EvaluationMechanism> <http://www.w3.org/2000/01/rdf-schema#comment> "The class csm:EvaluationMechanism contains aspects of how a crowdsourcing user or contribution is evaluated." .
<http://purl.org/csm/1.0#VirtualPoints> <http://www.w3.org/2000/01/rdf-schema#label> "virtual points" .
<http://purl.org/csm/1.0#External> <http://www.w3.org/1999/02/22-rdf-syntax-ns#type> <http://www.w3.org/2002/07/owl#NamedIndividual> .
<http://purl.org/csm/1.0#gender> <http://www.w3.org/2000/01/rdf-schema#label> "gender" .
<http://purl.org/csm/1.0#EvaluationSource> <http://www.w3.org/2000/01/rdf-schema#seeAlso> "Zhao, Y., & Zhu, Q. (2012). Evaluation on crowdsourcing research: Current status and future direction. Information Systems Frontiers, 1–18.\n\nDow, S., Kulkarni, A., Klemmer, S., & Hartmann, B. (2012). Shepherding the crowd yields better work. In Proceedings of the ACM 2012 Conference on Computer Supported Cooperative Work (pp. 1013–1022). New York, NY, USA: ACM." .
<http://purl.org/csm/1.0#VirtualPoints> <http://www.w3.org/1999/02/22-rdf-syntax-ns#type> <http://www.w3.org/2002/07/owl#NamedIndividual> .
<http://purl.org/csm/1.0#hasExternalResource> <http://www.w3.org/2000/01/rdf-schema#label> "has External Resource" .
<http://purl.org/csm/1.0#GenerateIdea> <http://www.w3.org/2000/01/rdf-schema#label> "generate idea" .
<http://purl.org/csm/1.0#Write> <http://www.w3.org/2000/01/rdf-schema#label> "write" .
<http://purl.org/csm/1.0#confidentialityLevel> <http://www.w3.org/1999/02/22-rdf-syntax-ns#type> <http://www.w3.org/2002/07/owl#DatatypeProperty> .
<http://purl.org/csm/1.0#ResourceAccess> <http://www.w3.org/2000/01/rdf-schema#label> "resource access" .
<http://purl.org/csm/1.0#numberOfApprovedTask> <http://www.w3.org/2000/01/rdf-schema#range> <http://www.w3.org/2001/XMLSchema#unsignedInt> .
<http://purl.org/csm/1.0#Translate> <http://www.w3.org/2000/01/rdf-schema#label> "translate" .
<http://purl.org/csm/1.0#WinnerParticipants> <http://www.w3.org/2000/01/rdf-schema#label> "winner participant" .
<http://purl.org/csm/1.0#hasLatencyType> <http://www.w3.org/2000/01/rdf-schema#label> "has Latency Type" .
<http://purl.org/csm/1.0#closureTime> <http://www.w3.org/2000/01/rdf-schema#label> "closure time" .
<http://purl.org/csm/1.0#Simple> <http://www.w3.org/1999/02/22-rdf-syntax-ns#type> <http://www.w3.org/2002/07/owl#NamedIndividual> .
<http://purl.org/csm/1.0#priorityLevel> <http://www.w3.org/2000/01/rdf-schema#comment> "The data property csm:priorityLevel defines the priority of a crowdsourcing task. Depending on the importance of concurrent tasks, the requester may either increase or decrease the attention of the crowd." .
<http://purl.org/csm/1.0#PerformanceBased> <http://www.w3.org/1999/02/22-rdf-syntax-ns#type> <http://purl.org/csm/1.0#RewardNature> .
<http://purl.org/csm/1.0#Verify> <http://www.w3.org/2000/01/rdf-schema#comment> "to check if data or information is correct or true (synonym: check)\n(apply csm:test to check products and services)" .
<http://purl.org/csm/1.0#Categorize> <http://www.w3.org/2000/01/rdf-schema#label> "categorize" .
<http://purl.org/csm/1.0#instruction> <http://www.w3.org/2000/01/rdf-schema#domain> <http://purl.org/csm/1.0#Task> .
<http://purl.org/csm/1.0#Label> <http://www.w3.org/2000/01/rdf-schema#comment> "to give someone or something a title or a name (synonym: tag)" .
<http://purl.org/csm/1.0#submits> <http://www.w3.org/1999/02/22-rdf-syntax-ns#type> <http://www.w3.org/2002/07/owl#ObjectProperty> .
<http://purl.org/csm/1.0#complexityLevel> <http://www.w3.org/2000/01/rdf-schema#seeAlso> "Brabham, D. C. (2008). Crowdsourcing as a Model for Problem Solving: An Introduction and Cases. Convergence: The International Journal of Research into New Media Technologies, 14(1), 75–90.\n\nRouse, A. C. (2010). A preliminary taxonomy of crowdsourcing. In ACIS 2010 Proceedings.\n\nSchenk, E., & Guittard, C. (2010). Towards a characterization of crowdsourcing practices. Journal of Innovation Economics, 7(1)." .
<http://purl.org/csm/1.0#hasEvaluationSpecificity> <http://www.w3.org/1999/02/22-rdf-syntax-ns#type> <http://www.w3.org/2002/07/owl#ObjectProperty> .
<http://purl.org/csm/1.0#operatingSystem> <http://www.w3.org/2000/01/rdf-schema#domain> <http://purl.org/csm/1.0#TechnicalRequirement> .
<http://purl.org/csm/1.0#numberOfApprovedTask> <http://www.w3.org/1999/02/22-rdf-syntax-ns#type> <http://www.w3.org/2002/07/owl#DatatypeProperty> .
<http://purl.org/csm/1.0#Voluntary> <http://www.w3.org/1999/02/22-rdf-syntax-ns#type> <http://www.w3.org/2002/07/owl#NamedIndividual> .
<http://purl.org/csm/1.0#hasTargetAudience> <http://www.w3.org/2000/01/rdf-schema#domain> <http://purl.org/csm/1.0#Task> .
<http://purl.org/csm/1.0#TechnicalRequirement> <http://www.w3.org/2000/01/rdf-schema#subClassOf> <http://purl.org/csm/1.0#Requirement> .
<http://purl.org/csm/1.0#Selective> <http://www.w3.org/2000/01/rdf-schema#label> "selective" .
<http://purl.org/csm/1.0#jobTitle> <http://www.w3.org/2000/01/rdf-schema#comment> "The data property csm:jobTitle defines the job title that a participant should have (use 6-digit code of the standard occupational classification (SOC))." .
<http://purl.org/csm/1.0#User> <http://www.w3.org/2000/01/rdf-schema#subClassOf> <http://purl.org/csm/1.0#EvaluationSource> .
<http://purl.org/csm/1.0#hasAggregationType> <http://www.w3.org/2000/01/rdf-schema#domain> <http://purl.org/csm/1.0#Task> .
<http://purl.org/csm/1.0#HumanRequirement> <http://www.w3.org/1999/02/22-rdf-syntax-ns#type> <http://www.w3.org/2002/07/owl#Class> .
<http://purl.org/csm/1.0#Internal> <http://www.w3.org/1999/02/22-rdf-syntax-ns#type> <http://www.w3.org/2002/07/owl#NamedIndividual> .
<http://purl.org/csm/1.0#Share> <http://www.w3.org/2000/01/rdf-schema#comment> "to share an artifact" .
<http://purl.org/csm/1.0#hasEvaluationMechanism> <http://www.w3.org/1999/02/22-rdf-syntax-ns#type> <http://www.w3.org/2002/07/owl#ObjectProperty> .
<http://purl.org/csm/1.0#Good> <http://www.w3.org/2000/01/rdf-schema#label> "good" .
<http://purl.org/csm/1.0#Rate> <http://www.w3.org/2000/01/rdf-schema#comment> "to give someone or something a quality value, e.g., on a five star rating scale" .
<http://purl.org/csm/1.0#TechnicalRequirement> <http://www.w3.org/2000/01/rdf-schema#label> "Technical Requirement" .
<http://purl.org/csm/1.0#Code> <http://www.w3.org/2000/01/rdf-schema#comment> "to develop software" .
<http://purl.org/csm/1.0#Transcribe> <http://www.w3.org/2000/01/rdf-schema#comment> "to digitize audio and video" .
<http://purl.org/csm/1.0#Design> <http://www.w3.org/2000/01/rdf-schema#label> "design" .
<http://purl.org/csm/1.0#issues> <http://www.w3.org/2000/01/rdf-schema#domain> <http://purl.org/csm/1.0#Requester> .
<http://purl.org/csm/1.0#ExternalResource> <http://www.w3.org/1999/02/22-rdf-syntax-ns#type> <http://www.w3.org/2002/07/owl#Class> .
<http://purl.org/csm/1.0#Test> <http://www.w3.org/2000/01/rdf-schema#comment> "to check if a product or service works properly, e.g., search relevance, product usability, functionality, security, localization" .
<http://purl.org/csm/1.0#hasPrevious> <http://www.w3.org/2000/01/rdf-schema#domain> <http://purl.org/csm/1.0#Task> .
<http://purl.org/csm/1.0#Label> <http://www.w3.org/2000/01/rdf-schema#label> "label" .
<http://purl.org/csm/1.0#operatingSystem> <http://www.w3.org/2000/01/rdf-schema#range> <http://www.w3.org/2000/01/rdf-schema#Literal> .
<http://purl.org/csm/1.0#qualificationType> <http://www.w3.org/2000/01/rdf-schema#range> <http://www.w3.org/2000/01/rdf-schema#Literal> .
<http://purl.org/csm/1.0#Untimed> <http://www.w3.org/1999/02/22-rdf-syntax-ns#type> <http://www.w3.org/2002/07/owl#NamedIndividual> .
<http://purl.org/csm/1.0#hasExternalResource> <http://www.w3.org/2000/01/rdf-schema#range> <http://purl.org/csm/1.0#ExternalResource> .
<http://purl.org/csm/1.0#Internal> <http://www.w3.org/2000/01/rdf-schema#comment> "Example: to discover knowledge within the company that might be confidential" .
<http://purl.org/csm/1.0#Play> <http://www.w3.org/2000/01/rdf-schema#label> "play" .
<http://purl.org/csm/1.0#Untimed> <http://www.w3.org/1999/02/22-rdf-syntax-ns#type> <http://purl.org/csm/1.0#LatencyType> .
<http://purl.org/csm/1.0#Code> <http://www.w3.org/2000/01/rdf-schema#label> "code" .
<http://purl.org/csm/1.0#hasTargetAudience> <http://www.w3.org/2000/01/rdf-schema#label> "has Target Audience" .
<http://purl.org/csm/1.0#hasPayoutMethod> <http://www.w3.org/2000/01/rdf-schema#label> "has Payout Method" .
<http://purl.org/csm/1.0#EvaluationMethod> <http://www.w3.org/2000/01/rdf-schema#label> "Evaluation Method" .
<http://purl.org/csm/1.0#owns> <http://www.w3.org/2000/01/rdf-schema#label> "owns" .
<http://purl.org/csm/1.0#submits> <http://www.w3.org/2000/01/rdf-schema#domain> <http://purl.org/csm/1.0#Participant> .
<http://purl.org/csm/1.0#hasActionType> <http://www.w3.org/2000/01/rdf-schema#range> <http://purl.org/csm/1.0#ActionType> .
<http://purl.org/csm/1.0#LowConfidential> <http://www.w3.org/1999/02/22-rdf-syntax-ns#type> <http://www.w3.org/2002/07/owl#NamedIndividual> .
<http://purl.org/csm/1.0#goal> <http://www.w3.org/2000/01/rdf-schema#domain> <http://purl.org/csm/1.0#Project> .
<http://purl.org/csm/1.0#SolveProblem> <http://www.w3.org/1999/02/22-rdf-syntax-ns#type> <http://purl.org/csm/1.0#ActionType> .
<http://purl.org/csm/1.0#Selective> <http://www.w3.org/2000/01/rdf-schema#comment> "(similar to competitive crowdsourcing, tournament-based crowdsourcing)" .
<http://purl.org/csm/1.0#Selective> <http://www.w3.org/1999/02/22-rdf-syntax-ns#type> <http://purl.org/csm/1.0#AggregationType> .
<http://purl.org/csm/1.0#currency> <http://www.w3.org/2000/01/rdf-schema#range> <http://www.w3.org/2001/XMLSchema#string> .
<http://purl.org/csm/1.0#hasRewardType> <http://www.w3.org/2000/01/rdf-schema#label> "has Reward Type" .
_:Bdf186945X2D7f0eX2D4a65X2Db934X2D00f1e241aa66 <http://www.w3.org/1999/02/22-rdf-syntax-ns#rest> _:Bdb74931eX2Ddeb4X2D4942X2Da3d8X2De97a0985f6aa .
<http://purl.org/csm/1.0#Integrative> <http://www.w3.org/1999/02/22-rdf-syntax-ns#type> <http://www.w3.org/2002/07/owl#NamedIndividual> .
<http://purl.org/csm/1.0#Transcribe> <http://www.w3.org/1999/02/22-rdf-syntax-ns#type> <http://purl.org/csm/1.0#ActionType> .
<http://purl.org/csm/1.0#hasLatencyType> <http://www.w3.org/1999/02/22-rdf-syntax-ns#type> <http://www.w3.org/2002/07/owl#ObjectProperty> .
<http://purl.org/csm/1.0#Task> <http://www.w3.org/2000/01/rdf-schema#label> "Task" .
<http://purl.org/csm/1.0#ExternalResource> <http://www.w3.org/2000/01/rdf-schema#label> "External Resource" .
<http://purl.org/csm/1.0#visibilityMode> <http://www.w3.org/2000/01/rdf-schema#range> <http://www.w3.org/2001/XMLSchema#boolean> .
<http://purl.org/csm/1.0#numberOfApprovedTask> <http://www.w3.org/2000/01/rdf-schema#domain> <http://purl.org/csm/1.0#HumanRequirement> .
<http://purl.org/csm/1.0#RewardNature> <http://www.w3.org/2000/01/rdf-schema#comment> "The class csm:RewardNature describes how a worker’s contribution is rewarded. A reward may either be fixed, such as a certain amount of money disbursed after completing a task, proportional, such as a share of virtual points, or performance-based, such as a prize that depends on the ranking in a competition. If no reward is stated, the nature of the reward is marked as voluntary." .
<http://purl.org/csm/1.0#Good> <http://www.w3.org/1999/02/22-rdf-syntax-ns#type> <http://www.w3.org/2002/07/owl#NamedIndividual> .
<http://purl.org/csm/1.0#Participant> <http://www.w3.org/2000/01/rdf-schema#subClassOf> <http://purl.org/csm/1.0#User> .
<http://purl.org/csm/1.0#Discount> <http://www.w3.org/1999/02/22-rdf-syntax-ns#type> <http://purl.org/csm/1.0#RewardType> .
<http://purl.org/csm/1.0#AggregationType> <http://www.w3.org/2000/01/rdf-schema#comment> "The class csm:AggregationType specifies the mechanism of how the contributions of the crowd are combined." .
<http://purl.org/csm/1.0#visibilityMode> <http://www.w3.org/1999/02/22-rdf-syntax-ns#type> <http://www.w3.org/2002/07/owl#DatatypeProperty> .
<http://purl.org/csm/1.0#EvaluationMethod> <http://www.w3.org/1999/02/22-rdf-syntax-ns#type> <http://www.w3.org/2002/07/owl#Class> .
<http://purl.org/csm/1.0#Fixed> <http://www.w3.org/1999/02/22-rdf-syntax-ns#type> <http://purl.org/csm/1.0#RewardNature> .
<http://purl.org/csm/1.0#hasAggregationType> <http://www.w3.org/2000/01/rdf-schema#label> "has Aggregation Type" .
<http://purl.org/csm/1.0#RewardType> <http://www.w3.org/2000/01/rdf-schema#label> "Reward Type" .
<http://purl.org/csm/1.0#Project> <http://www.w3.org/2000/01/rdf-schema#comment> "The class csm:Project defines parameters of the crowdsourcing project, such as the goal, the category, or the submission and closure time." .
<http://purl.org/csm/1.0#Translate> <http://www.w3.org/2000/01/rdf-schema#comment> "to translate words, phrases, or documents from one language into another language" .
<http://purl.org/csm/1.0#confidentialityLevel> <http://www.w3.org/2000/01/rdf-schema#seeAlso> "Corney, J. R., Torres-Sánchez, C., Jagadeesan, A. P., Yan, X. T., Regli, W. C., & Medellin, H. (2010). Putting the crowd to work in a knowledge-based factory. Advanced Engineering Informatics, 24(3), 243–250." .
<http://purl.org/csm/1.0#Coupon> <http://www.w3.org/1999/02/22-rdf-syntax-ns#type> <http://www.w3.org/2002/07/owl#NamedIndividual> .
<http://purl.org/csm/1.0#owns> <http://www.w3.org/1999/02/22-rdf-syntax-ns#type> <http://www.w3.org/2002/07/owl#ObjectProperty> .
<http://purl.org/csm/1.0#Before> <http://www.w3.org/2000/01/rdf-schema#label> "before" .
<http://purl.org/csm/1.0#jobTitle> <http://www.w3.org/2000/01/rdf-schema#range> <http://www.w3.org/2001/XMLSchema#string> .
<http://purl.org/csm/1.0#Simultaneously> <http://www.w3.org/1999/02/22-rdf-syntax-ns#type> <http://purl.org/csm/1.0#EvaluationTime> .
<http://purl.org/csm/1.0#hasEvaluationMechanism> <http://www.w3.org/2000/01/rdf-schema#label> "has Evaluation Mechanism" .
<http://purl.org/csm/1.0#Hybrid> <http://www.w3.org/1999/02/22-rdf-syntax-ns#type> <http://purl.org/csm/1.0#TargetAudience> .
<http://purl.org/csm/1.0#Complex> <http://www.w3.org/1999/02/22-rdf-syntax-ns#type> <http://www.w3.org/2002/07/owl#NamedIndividual> .
<http://purl.org/csm/1.0#Task> <http://www.w3.org/2000/01/rdf-schema#comment> "The class csm:Task describes the smallest indivisible unit of work in a crowdsourcing process." .
<http://purl.org/csm/1.0#Lottery> <http://www.w3.org/2000/01/rdf-schema#label> "lottery" .
<http://purl.org/csm/1.0#Rating> <http://www.w3.org/2000/01/rdf-schema#label> "rating" .
<http://purl.org/csm/1.0#Share> <http://www.w3.org/2000/01/rdf-schema#label> "share" .
<http://purl.org/csm/1.0#operatingSystem> <http://www.w3.org/1999/02/22-rdf-syntax-ns#type> <http://www.w3.org/2002/07/owl#DatatypeProperty> .
<http://purl.org/csm/1.0#qualificationType> <http://www.w3.org/1999/02/22-rdf-syntax-ns#type> <http://www.w3.org/2002/07/owl#DatatypeProperty> .
<http://purl.org/csm/1.0#priorityLevel> <http://www.w3.org/2000/01/rdf-schema#domain> <http://purl.org/csm/1.0#Task> .
<http://purl.org/csm/1.0#Execute> <http://www.w3.org/2000/01/rdf-schema#comment> "to execute a task, e.g., do research, general office work, or" .
<http://purl.org/csm/1.0#Requirement> <http://www.w3.org/2000/01/rdf-schema#comment> "The class csm:Requirement defines any human or technical aspect that is required to solve a crowdsourcing task." .
<http://purl.org/csm/1.0#AggregationType> <http://www.w3.org/2000/01/rdf-schema#label> "Aggregation Type" .
<http://purl.org/csm/1.0#gender> <http://www.w3.org/2000/01/rdf-schema#comment> "The data property csm:gender defines the gender that a participant should have (use 1-digit gender code according to ISO/IEC 5218; 0 = not known, 1 = male, 2 = female, 9 = not applicable)." .
<http://purl.org/csm/1.0#ageMin> <http://www.w3.org/2000/01/rdf-schema#domain> <http://purl.org/csm/1.0#HumanRequirement> .
<http://purl.org/csm/1.0#numberOfAssignments> <http://www.w3.org/2000/01/rdf-schema#label> "number of assignments" .
<http://purl.org/csm/1.0#EvaluationMethod> <http://www.w3.org/2000/01/rdf-schema#comment> "The class csm:EvaluationMethod describes the evaluation method used. There are two major evaluation methods: the majority decision and the control group approach." .
<http://purl.org/csm/1.0#Participant> <http://www.w3.org/2000/01/rdf-schema#comment> "The class csm:Participant defines a person who submits a contribution.\n(related terms: crowdsourcees, crowd, human cloud, recipient, worker, provider, designated agent)" .
<http://purl.org/csm/1.0#currency> <http://www.w3.org/2000/01/rdf-schema#comment> "The data property csm:currency defines the currency of a monetary reward (use 3-digit currency code according to ISO 4217)." .
<http://purl.org/csm/1.0#Transcribe> <http://www.w3.org/1999/02/22-rdf-syntax-ns#type> <http://www.w3.org/2002/07/owl#NamedIndividual> .
<http://purl.org/csm/1.0#Proportional> <http://www.w3.org/2000/01/rdf-schema#label> "proportional" .
<http://purl.org/csm/1.0#hasRewardMechanism> <http://www.w3.org/2000/01/rdf-schema#range> <http://purl.org/csm/1.0#RewardMechanism> .
<http://purl.org/csm/1.0#Requirement> <http://www.w3.org/2000/01/rdf-schema#label> "Requirement" .
<http://purl.org/csm/1.0#operatingSystem> <http://www.w3.org/2000/01/rdf-schema#label> "operating system" .
<http://purl.org/csm/1.0#complexityLevel> <http://www.w3.org/2000/01/rdf-schema#domain> <http://purl.org/csm/1.0#Task> .
<http://purl.org/csm/1.0#AssessmentForm> <http://www.w3.org/1999/02/22-rdf-syntax-ns#type> <http://www.w3.org/2002/07/owl#NamedIndividual> .
<http://purl.org/csm/1.0#hardwareFeature> <http://www.w3.org/2000/01/rdf-schema#label> "hardware feature" .
<http://purl.org/csm/1.0#RewardType> <http://www.w3.org/1999/02/22-rdf-syntax-ns#type> <http://www.w3.org/2002/07/owl#Class> .
<http://purl.org/csm/1.0#EvaluationSubject> <http://www.w3.org/2000/01/rdf-schema#label> "Evaluation Subject" .
<http://purl.org/csm/1.0#MaleParticipant> <http://www.w3.org/1999/02/22-rdf-syntax-ns#type> <http://www.w3.org/2002/07/owl#NamedIndividual> .
<http://purl.org/csm/1.0#ThirdParty> <http://www.w3.org/2000/01/rdf-schema#comment> "A third party organization is contracted to evaluate the contributions or participants." .
<http://purl.org/csm/1.0#MajorityDecision> <http://www.w3.org/1999/02/22-rdf-syntax-ns#type> <http://purl.org/csm/1.0#EvaluationMethod> .
<http://purl.org/csm/1.0#title> <http://www.w3.org/2000/01/rdf-schema#label> "title" .
<http://purl.org/csm/1.0#hasEvaluationTime> <http://www.w3.org/2000/01/rdf-schema#range> <http://purl.org/csm/1.0#EvaluationTime> .
<http://purl.org/csm/1.0#hasRewardType> <http://www.w3.org/1999/02/22-rdf-syntax-ns#type> <http://www.w3.org/2002/07/owl#ObjectProperty> .
<http://purl.org/csm/1.0#hasEvaluationSource> <http://www.w3.org/2000/01/rdf-schema#range> <http://purl.org/csm/1.0#EvaluationSource> .
<http://purl.org/csm/1.0> <http://www.w3.org/2002/07/owl#imports> <http://purl.org/goodrelations/v1> .
<http://purl.org/csm/1.0#hasRewardType> <http://www.w3.org/2000/01/rdf-schema#domain> <http://purl.org/csm/1.0#RewardMechanism> .
<http://purl.org/csm/1.0#hasEvaluationSubject> <http://www.w3.org/2000/01/rdf-schema#label> "has Evaluation Subject" .
<http://purl.org/csm/1.0#PayoutMethod> <http://www.w3.org/2000/01/rdf-schema#comment> "The class csm:PayoutMethod defines which participants in the crowdsourcing activity are rewarded — for example, all, the winner only, or the top ten participants." .
<http://purl.org/csm/1.0#hasRewardMechanism> <http://www.w3.org/2000/01/rdf-schema#domain> <http://purl.org/csm/1.0#Task> .
<http://purl.org/csm/1.0#Transcribe> <http://www.w3.org/2000/01/rdf-schema#label> "transcribe" .
<http://purl.org/csm/1.0#hasEvaluationSpecificity> <http://www.w3.org/2000/01/rdf-schema#domain> <http://purl.org/csm/1.0#EvaluationMechanism> .
<http://purl.org/csm/1.0#hardwareDevice> <http://www.w3.org/2000/01/rdf-schema#domain> <http://purl.org/csm/1.0#TechnicalRequirement> .
<http://purl.org/csm/1.0#AggregationType> <http://www.w3.org/1999/02/22-rdf-syntax-ns#type> <http://www.w3.org/2002/07/owl#Class> .
<http://purl.org/csm/1.0#FemaleParticipant> <http://www.w3.org/1999/02/22-rdf-syntax-ns#type> <http://www.w3.org/2002/07/owl#NamedIndividual> .
<http://purl.org/csm/1.0#imposes> <http://www.w3.org/2000/01/rdf-schema#label> "imposes" .
<http://purl.org/csm/1.0#imposes> <http://www.w3.org/1999/02/22-rdf-syntax-ns#type> <http://www.w3.org/2002/07/owl#ObjectProperty> .
<http://purl.org/csm/1.0#Categorize> <http://www.w3.org/2000/01/rdf-schema#comment> "to put someone or something into groups (synonym: classify, organize)" .
<http://purl.org/csm/1.0#Algorithm> <http://www.w3.org/2000/01/rdf-schema#label> "algorithm" .
<http://purl.org/csm/1.0#Simultaneously> <http://www.w3.org/1999/02/22-rdf-syntax-ns#type> <http://www.w3.org/2002/07/owl#NamedIndividual> .
<http://purl.org/csm/1.0> <http://purl.org/dc/elements/1.1/description> <http://www.larshetmank.com/vocabulary/csm-content/csm.png> .
<http://purl.org/csm/1.0#MajorityDecision> <http://www.w3.org/2000/01/rdf-schema#label> "majority decision" .
<http://purl.org/csm/1.0#gender> <http://www.w3.org/2000/01/rdf-schema#domain> <http://purl.org/csm/1.0#HumanRequirement> .
<http://purl.org/csm/1.0#SolveProblem> <http://www.w3.org/1999/02/22-rdf-syntax-ns#type> <http://www.w3.org/2002/07/owl#NamedIndividual> .
<http://purl.org/csm/1.0#Money> <http://www.w3.org/1999/02/22-rdf-syntax-ns#type> <http://purl.org/csm/1.0#RewardType> .
<http://purl.org/csm/1.0#category> <http://www.w3.org/2000/01/rdf-schema#domain> <http://purl.org/csm/1.0#Project> .
<http://purl.org/csm/1.0#Create> <http://www.w3.org/2000/01/rdf-schema#comment> "to create an artifact or a prototype" .
<http://purl.org/csm/1.0#hasRewardType> <http://www.w3.org/2000/01/rdf-schema#range> <http://purl.org/csm/1.0#RewardType> .
<http://purl.org/csm/1.0#goal> <http://www.w3.org/2000/01/rdf-schema#label> "goal" .
<http://purl.org/csm/1.0#LowPriority> <http://www.w3.org/1999/02/22-rdf-syntax-ns#type> <http://www.w3.org/2002/07/owl#NamedIndividual> .
<http://purl.org/csm/1.0#language> <http://www.w3.org/2000/01/rdf-schema#domain> <http://purl.org/csm/1.0#HumanRequirement> .
<http://purl.org/csm/1.0#EvaluationSpecificity> <http://www.w3.org/2000/01/rdf-schema#seeAlso> "Dow, S., Kulkarni, A., Klemmer, S., & Hartmann, B. (2012). Shepherding the crowd yields better work. In Proceedings of the ACM 2012 Conference on Computer Supported Cooperative Work (pp. 1013–1022). New York, NY, USA: ACM." .
<http://purl.org/csm/1.0#hasEvaluationSource> <http://www.w3.org/2000/01/rdf-schema#domain> <http://purl.org/csm/1.0#EvaluationMechanism> .
<http://purl.org/csm/1.0#country> <http://www.w3.org/1999/02/22-rdf-syntax-ns#type> <http://www.w3.org/2002/07/owl#DatatypeProperty> .
<http://purl.org/csm/1.0#hasPrevious> <http://www.w3.org/2000/01/rdf-schema#label> "has Previous" .
<http://purl.org/csm/1.0#ageMax> <http://www.w3.org/2000/01/rdf-schema#domain> <http://purl.org/csm/1.0#HumanRequirement> .
<http://purl.org/csm/1.0#hasPrevious> <http://www.w3.org/1999/02/22-rdf-syntax-ns#type> <http://www.w3.org/2002/07/owl#ObjectProperty> .
<http://purl.org/csm/1.0#RewardType> <http://www.w3.org/2000/01/rdf-schema#comment> "The class csm:RewardType specifies what kind of reward is offered. On the one hand, a reward may be of immaterial value, such as providing virtual points that improve the worker’s reputation, money in the form of a bonus that increases the salary, or access to a resource, which may or may not be related to the actual crowdsourcing initiative itself, such as, for example, a knowledge repository. In addition, physical goods may be used to compensate workers for their efforts." .
<http://purl.org/csm/1.0#Participant> <http://www.w3.org/1999/02/22-rdf-syntax-ns#type> <http://www.w3.org/2002/07/owl#Class> .
<http://purl.org/csm/1.0#visibilityMode> <http://www.w3.org/2000/01/rdf-schema#domain> <http://purl.org/csm/1.0#Task> .
<http://purl.org/csm/1.0> <http://purl.org/dc/elements/1.1/date> "2013-09-22" .
<http://purl.org/csm/1.0#hasActionType> <http://www.w3.org/2000/01/rdf-schema#label> "has Action Type" .
<http://purl.org/csm/1.0#PayoutMethod> <http://www.w3.org/1999/02/22-rdf-syntax-ns#type> <http://www.w3.org/2002/07/owl#Class> .
<http://purl.org/csm/1.0#hasEvaluationMethod> <http://www.w3.org/2000/01/rdf-schema#domain> <http://purl.org/csm/1.0#EvaluationMechanism> .
<http://purl.org/csm/1.0#Verify> <http://www.w3.org/1999/02/22-rdf-syntax-ns#type> <http://purl.org/csm/1.0#ActionType> .
<http://purl.org/csm/1.0#hasAggregationType> <http://www.w3.org/1999/02/22-rdf-syntax-ns#type> <http://www.w3.org/2002/07/owl#ObjectProperty> .
<http://purl.org/csm/1.0#confidentialityLevel> <http://www.w3.org/2000/01/rdf-schema#label> "confidentiality level" .
<http://purl.org/csm/1.0#goal> <http://www.w3.org/2000/01/rdf-schema#comment> "The data property csm:goal is a free text that contains the goal of the task." .
<http://purl.org/csm/1.0#Proportional> <http://www.w3.org/1999/02/22-rdf-syntax-ns#type> <http://purl.org/csm/1.0#RewardNature> .
<http://purl.org/csm/1.0#hasPrevious> <http://www.w3.org/2000/01/rdf-schema#range> <http://purl.org/csm/1.0#Task> .
<http://purl.org/csm/1.0#description> <http://www.w3.org/2000/01/rdf-schema#domain> <http://purl.org/csm/1.0#Contribution> .
<http://purl.org/csm/1.0#numberOfApprovedTask> <http://www.w3.org/2000/01/rdf-schema#label> "number of approved task" .
<http://purl.org/csm/1.0#EvaluationSource> <http://www.w3.org/1999/02/22-rdf-syntax-ns#type> <http://www.w3.org/2002/07/owl#Class> .
<http://purl.org/csm/1.0#Play> <http://www.w3.org/1999/02/22-rdf-syntax-ns#type> <http://www.w3.org/2002/07/owl#NamedIndividual> .
<http://purl.org/csm/1.0#hasEvaluationMechanism> <http://www.w3.org/2000/01/rdf-schema#domain> <http://purl.org/csm/1.0#Task> .
<http://purl.org/csm/1.0#NoReward> <http://www.w3.org/1999/02/22-rdf-syntax-ns#type> <http://purl.org/csm/1.0#RewardType> .
<http://purl.org/csm/1.0#hasEvaluationSubject> <http://www.w3.org/2000/01/rdf-schema#range> <http://purl.org/csm/1.0#EvaluationSubject> .
<http://purl.org/csm/1.0#Contribution> <http://www.w3.org/1999/02/22-rdf-syntax-ns#type> <http://www.w3.org/2002/07/owl#Class> .
<http://purl.org/csm/1.0#hardwareFeature> <http://www.w3.org/1999/02/22-rdf-syntax-ns#type> <http://www.w3.org/2002/07/owl#DatatypeProperty> .
_:B29bdffeaX2Daa8dX2D45b1X2D86f4X2D0d62657c2eed <http://www.w3.org/1999/02/22-rdf-syntax-ns#type> <http://www.w3.org/2002/07/owl#Class> .
<http://purl.org/csm/1.0#Label> <http://www.w3.org/1999/02/22-rdf-syntax-ns#type> <http://purl.org/csm/1.0#ActionType> .
<http://purl.org/csm/1.0#complexityLevel> <http://www.w3.org/2000/01/rdf-schema#label> "complexity level" .
<http://purl.org/csm/1.0#submissionTime> <http://www.w3.org/2000/01/rdf-schema#domain> <http://purl.org/csm/1.0#Project> .
<http://purl.org/csm/1.0#Create> <http://www.w3.org/1999/02/22-rdf-syntax-ns#type> <http://purl.org/csm/1.0#ActionType> .
<http://purl.org/csm/1.0#HighPriority> <http://www.w3.org/1999/02/22-rdf-syntax-ns#type> <http://www.w3.org/2002/07/owl#NamedIndividual> .
<http://purl.org/csm/1.0#TargetAudience> <http://www.w3.org/2000/01/rdf-schema#comment> "The class csm:TargetAudience sets the target audience to either internal crowd (the employees of the enterprise), external crowd (the public domain), or hybrid crowd (both employees and the public domain)." .
<http://purl.org/csm/1.0#After> <http://www.w3.org/1999/02/22-rdf-syntax-ns#type> <http://www.w3.org/2002/07/owl#NamedIndividual> .
<http://purl.org/csm/1.0#Rating> <http://www.w3.org/1999/02/22-rdf-syntax-ns#type> <http://purl.org/csm/1.0#EvaluationSpecificity> .
<http://purl.org/csm/1.0#Categorize> <http://www.w3.org/1999/02/22-rdf-syntax-ns#type> <http://www.w3.org/2002/07/owl#NamedIndividual> .
<http://purl.org/csm/1.0#EvaluationMethod> <http://www.w3.org/2000/01/rdf-schema#seeAlso> "Hirth, M., Hossfeld, T., & Tran-Gia, P. (2011). Cost-Optimal Validation Mechanisms and Cheat-Detection for Crowdsourcing Platforms. In Innovative Mobile and Internet Services in Ubiquitous Computing (IMIS), 2011 Fifth International Conference On (pp. 316–321)." .
<http://purl.org/csm/1.0#WinnerParticipants> <http://www.w3.org/1999/02/22-rdf-syntax-ns#type> <http://purl.org/csm/1.0#PayoutMethod> .
<http://purl.org/csm/1.0#Project> <http://www.w3.org/1999/02/22-rdf-syntax-ns#type> <http://www.w3.org/2002/07/owl#Class> .
<http://purl.org/csm/1.0#User> <http://www.w3.org/2000/01/rdf-schema#label> "User" .
_:B29bdffeaX2Daa8dX2D45b1X2D86f4X2D0d62657c2eed <http://www.w3.org/2002/07/owl#unionOf> _:Bdf186945X2D7f0eX2D4a65X2Db934X2D00f1e241aa66 .
<http://purl.org/csm/1.0#EvaluationMechanism> <http://www.w3.org/2000/01/rdf-schema#label> "Evaluation Mechanism" .
<http://purl.org/csm/1.0#Coupon> <http://www.w3.org/2000/01/rdf-schema#label> "coupon" .
<http://purl.org/csm/1.0#description> <http://www.w3.org/2000/01/rdf-schema#domain> <http://purl.org/csm/1.0#Project> .
<http://purl.org/csm/1.0#qualificationLevel> <http://www.w3.org/2000/01/rdf-schema#comment> "The data property csm:qualificationLevel defines the proficiency level of a certain qualification (poor, fair, good, very good, excellent)." .
<http://purl.org/csm/1.0#qualificationType> <http://www.w3.org/2000/01/rdf-schema#comment> "The data property csm:qualificationType defines any academic degree, certificate, or skill required to solve the task." .
<http://purl.org/csm/1.0#complexityLevel> <http://www.w3.org/2000/01/rdf-schema#range> <http://www.w3.org/2000/01/rdf-schema#Literal> .
<http://purl.org/csm/1.0#Before> <http://www.w3.org/1999/02/22-rdf-syntax-ns#type> <http://www.w3.org/2002/07/owl#NamedIndividual> .
<http://purl.org/csm/1.0#External> <http://www.w3.org/1999/02/22-rdf-syntax-ns#type> <http://purl.org/csm/1.0#TargetAudience> .
<http://purl.org/csm/1.0#hasLatencyType> <http://www.w3.org/2000/01/rdf-schema#domain> <http://purl.org/csm/1.0#Task> .
<http://purl.org/csm/1.0#title> <http://www.w3.org/2000/01/rdf-schema#domain> <http://purl.org/csm/1.0#ExternalResource> .
<http://purl.org/csm/1.0#Translate> <http://www.w3.org/1999/02/22-rdf-syntax-ns#type> <http://purl.org/csm/1.0#ActionType> .
<http://purl.org/csm/1.0#visibilityMode> <http://www.w3.org/2000/01/rdf-schema#label> "visibility mode" .
<http://purl.org/csm/1.0#ResourceAccess> <http://www.w3.org/1999/02/22-rdf-syntax-ns#type> <http://www.w3.org/2002/07/owl#NamedIndividual> .
<http://purl.org/csm/1.0#ExternalResource> <http://www.w3.org/2000/01/rdf-schema#comment> "The class csm:TechnicalResource refers to all inputs, such as software applications, documents, or datasets, that are required to accomplish the crowdsourcing task. A software application may be an online survey tool that is not part of the crowdsourcing system itself but has to be used to solve the problem. Often, the instructions for a task cannot be described in short sentences. In these cases, additional information in the form of a combination of text, audio, or video elements must be included." .
<http://purl.org/csm/1.0#hasTask> <http://www.w3.org/2000/01/rdf-schema#label> "has Task" .
<http://purl.org/csm/1.0#hasEvaluationTime> <http://www.w3.org/2000/01/rdf-schema#domain> <http://purl.org/csm/1.0#EvaluationMechanism> .
<http://purl.org/csm/1.0#issues> <http://www.w3.org/1999/02/22-rdf-syntax-ns#type> <http://www.w3.org/2002/07/owl#ObjectProperty> .
<http://purl.org/csm/1.0#qualificationLevel> <http://www.w3.org/2000/01/rdf-schema#range> <http://www.w3.org/2000/01/rdf-schema#Literal> .
<http://purl.org/csm/1.0#qualificationType> <http://www.w3.org/2000/01/rdf-schema#label> "qualification type" .
<http://purl.org/csm/1.0#hasTask> <http://www.w3.org/2000/01/rdf-schema#domain> <http://purl.org/csm/1.0#Project> .
<http://purl.org/csm/1.0#hasEvaluationMethod> <http://www.w3.org/2000/01/rdf-schema#label> "has Evaluation Method" .
<http://purl.org/csm/1.0#softwarePlatform> <http://www.w3.org/2000/01/rdf-schema#domain> <http://purl.org/csm/1.0#TechnicalRequirement> .
<http://purl.org/csm/1.0#description> <http://www.w3.org/2000/01/rdf-schema#domain> <http://purl.org/csm/1.0#EvaluationMechanism> .
<http://purl.org/csm/1.0#Requester> <http://www.w3.org/2000/01/rdf-schema#label> "Requester" .
<http://purl.org/csm/1.0#Requirement> <http://www.w3.org/1999/02/22-rdf-syntax-ns#type> <http://www.w3.org/2002/07/owl#Class> .
<http://purl.org/csm/1.0#owns> <http://www.w3.org/2000/01/rdf-schema#domain> <http://purl.org/csm/1.0#Task> .
<http://purl.org/csm/1.0#Execute> <http://www.w3.org/1999/02/22-rdf-syntax-ns#type> <http://purl.org/csm/1.0#ActionType> .
<http://purl.org/csm/1.0#Lottery> <http://www.w3.org/1999/02/22-rdf-syntax-ns#type> <http://purl.org/csm/1.0#RewardType> .
<http://purl.org/csm/1.0#Hybrid> <http://www.w3.org/2000/01/rdf-schema#label> "hybrid" .
<http://purl.org/csm/1.0#Algorithm> <http://www.w3.org/2000/01/rdf-schema#comment> "An algorithm is applied to evaluate the contributions or participants." .
<http://purl.org/csm/1.0#EvaluationTime> <http://www.w3.org/2000/01/rdf-schema#comment> "The class csm:Evaluation defines the point of time when the user or the contribution is evaluated. A user may be evaluated before starting the first task (ex-ante) or after finishing a task (ex-post). The former applies to entry questions, pre-qualification tasks, or gold standard data to determine the expertise or skill level of a worker. The latter considers acceptance and rejection decisions about historic contributions. The users may also get feedback on the quality of the contribution during the work in progress." .
<http://purl.org/csm/1.0#WinnerParticipants> <http://www.w3.org/1999/02/22-rdf-syntax-ns#type> <http://www.w3.org/2002/07/owl#NamedIndividual> .
<http://purl.org/csm/1.0#hardwareFeature> <http://www.w3.org/2000/01/rdf-schema#range> <http://www.w3.org/2000/01/rdf-schema#Literal> .
<http://purl.org/csm/1.0#FreeForm> <http://www.w3.org/1999/02/22-rdf-syntax-ns#type> <http://purl.org/csm/1.0#EvaluationSpecificity> .
<http://purl.org/csm/1.0#Translate> <http://www.w3.org/1999/02/22-rdf-syntax-ns#type> <http://www.w3.org/2002/07/owl#NamedIndividual> .
<http://purl.org/csm/1.0#title> <http://www.w3.org/2000/01/rdf-schema#domain> <http://purl.org/csm/1.0#Contribution> .
<http://purl.org/csm/1.0#language> <http://www.w3.org/2000/01/rdf-schema#range> <http://www.w3.org/2001/XMLSchema#language> .
<http://purl.org/csm/1.0#LatencyType> <http://www.w3.org/2000/01/rdf-schema#comment> "The class csm:LatencyType specifies if the answer is untimed or if an immediate reply is expected. For some tasks, such as the collaborative creation of a knowledge repository, the focus lies on the accuracy of the contribution. In this case, the latency between issuing a task and getting an answer to the task does not matter. These tasks are defined as untimed. In other cases, such as an instant translation during a meeting, receiving an immediate reply is critical for the quality experience of the requester." .
<http://purl.org/csm/1.0#Integrative> <http://www.w3.org/1999/02/22-rdf-syntax-ns#type> <http://purl.org/csm/1.0#AggregationType> .
<http://purl.org/csm/1.0#Moderate> <http://www.w3.org/1999/02/22-rdf-syntax-ns#type> <http://www.w3.org/2002/07/owl#NamedIndividual> .
<http://purl.org/csm/1.0> <http://purl.org/dc/elements/1.1/title> "CSM Ontology – An Enterprise Crowdsourcing Ontology" .
<http://purl.org/csm/1.0#Selective> <http://www.w3.org/1999/02/22-rdf-syntax-ns#type> <http://www.w3.org/2002/07/owl#NamedIndividual> .
<http://purl.org/csm/1.0> <http://www.w3.org/2000/01/rdf-schema#comment> "The CSM ontology provides concepts and properties for capturing, storing, and linking crowdsourcing data. The designed ontology contains 24 classes, 22 object properties, and 30 data properties to describe the key aspects of a typical enterprise crowdsourcing activity. All semantic entities of the ontology are supplemented with additional annotation information, whereas the rdfs:comment property is applied to explain the meaning of the entity and the rdfs:seeAlso property offers literature references and suggestions for further reading (currently not rendered by the documentation generator).\n\nThe anticipated benefits for the crowdsourcing domain are in detail:\n\n- Providing of a controlled vocabulary that reduces ambiguity and ensures consistency\n- Enhanced semantic and intelligent search, navigation, and browsing capabilities\n- Support of proactive recommendation mechanisms\n- Improved data exchange and integration\n- Foundation for knowledge discovery, data mining, and machine learning\n\n\nReferences:\n\n[1] Hetmank, L. (2013). Components and Functions of Crowdsourcing Systems – A Systematic Literature Review. In 11th International Conference on Wirtschaftsinformatik (WI). Leipzig.\n\n[2] Hetmank, L. (2013). Towards a Semantic Standard for Enterprise Crowdsourcing – A Scenario-based Evaluation of a Conceptual Prototype. In 21st European Conference on In-formation Systems (ECIS). Utrecht.\n\n[3] Hetmank, L. (2014). Developing an Ontology for Enterprise Crowdsourcing. In Multikonferenz Wirtschaftsinformatik (MKWI). Paderborn." .
<http://purl.org/csm/1.0#hasEvaluationSubject> <http://www.w3.org/2000/01/rdf-schema#domain> <http://purl.org/csm/1.0#EvaluationMechanism> .
<http://purl.org/csm/1.0#After> <http://www.w3.org/1999/02/22-rdf-syntax-ns#type> <http://purl.org/csm/1.0#EvaluationTime> .
<http://purl.org/csm/1.0#visibilityMode> <http://www.w3.org/2000/01/rdf-schema#comment> "The data property csm:visibilityMode  defines whether the workers can or can not see each other’s contributions." .
<http://purl.org/csm/1.0#ThirdParty> <http://www.w3.org/2000/01/rdf-schema#label> "third party" .
<http://purl.org/csm/1.0#closureTime> <http://www.w3.org/1999/02/22-rdf-syntax-ns#type> <http://www.w3.org/2002/07/owl#DatatypeProperty> .
<http://purl.org/csm/1.0#RewardNature> <http://www.w3.org/1999/02/22-rdf-syntax-ns#type> <http://www.w3.org/2002/07/owl#Class> .
<http://purl.org/csm/1.0#LatencyType> <http://www.w3.org/2000/01/rdf-schema#seeAlso> "Liu, Y., Lehdonvirta, V., Kleppe, M., Alexandrova, T., Kimura, H., & Nakajima, T. (2010). A crowdsourcing based mobile image translation and knowledge sharing service. In Proceedings of the 9th International Conference on Mobile and Ubiquitous Multimedia (pp. 1–9). New York, NY, USA: ACM." .
<http://purl.org/csm/1.0#issues> <http://www.w3.org/2000/01/rdf-schema#comment> "The object property csm:issues defines the projects that a requester issues." .
<http://purl.org/csm/1.0#RewardMechanism> <http://www.w3.org/2000/01/rdf-schema#label> "Reward Mechanism" .
<http://purl.org/csm/1.0#Untimed> <http://www.w3.org/2000/01/rdf-schema#label> "untimed" .
<http://purl.org/csm/1.0#Execute> <http://www.w3.org/1999/02/22-rdf-syntax-ns#type> <http://www.w3.org/2002/07/owl#NamedIndividual> .
<http://purl.org/csm/1.0#Internal> <http://www.w3.org/2000/01/rdf-schema#label> "internal" .
<http://purl.org/csm/1.0#approvalRate> <http://www.w3.org/2000/01/rdf-schema#domain> <http://purl.org/csm/1.0#HumanRequirement> .
<http://purl.org/csm/1.0#description> <http://www.w3.org/2000/01/rdf-schema#label> "description" .
<http://purl.org/csm/1.0#AggregationType> <http://www.w3.org/2000/01/rdf-schema#seeAlso> "\nSchenk, E., & Guittard, C. (2010). Towards a characterization of crowdsourcing practices. Journal of Innovation Economics, 7(1)." .
<http://purl.org/csm/1.0#Fixed> <http://www.w3.org/2000/01/rdf-schema#label> "fixed" .
<http://purl.org/csm/1.0#title> <http://www.w3.org/2000/01/rdf-schema#domain> <http://purl.org/csm/1.0#Project> .
<http://purl.org/csm/1.0#NoReward> <http://www.w3.org/2000/01/rdf-schema#label> "no reward" .
<http://purl.org/csm/1.0#qualificationLevel> <http://www.w3.org/2000/01/rdf-schema#label> "qualification level" .
<http://purl.org/csm/1.0#Verify> <http://www.w3.org/1999/02/22-rdf-syntax-ns#type> <http://www.w3.org/2002/07/owl#NamedIndividual> .
<http://purl.org/csm/1.0#ControlGroup> <http://www.w3.org/1999/02/22-rdf-syntax-ns#type> <http://purl.org/csm/1.0#EvaluationMethod> .
<http://purl.org/csm/1.0> <http://www.w3.org/2002/07/owl#imports> <http://xmlns.com/foaf/0.1/> .
<http://purl.org/csm/1.0#imposes> <http://www.w3.org/2000/01/rdf-schema#domain> <http://purl.org/csm/1.0#Task> .
<http://purl.org/csm/1.0#Play> <http://www.w3.org/1999/02/22-rdf-syntax-ns#type> <http://purl.org/csm/1.0#ActionType> .
<http://purl.org/csm/1.0#TargetAudience> <http://www.w3.org/2000/01/rdf-schema#label> "Target Audience" .
<http://purl.org/csm/1.0#imposes> <http://www.w3.org/2000/01/rdf-schema#range> <http://purl.org/csm/1.0#Requirement> .
<http://purl.org/csm/1.0#description> <http://www.w3.org/2000/01/rdf-schema#domain> <http://purl.org/csm/1.0#ExternalResource> .
<http://purl.org/csm/1.0#qualificationLevel> <http://www.w3.org/1999/02/22-rdf-syntax-ns#type> <http://www.w3.org/2002/07/owl#DatatypeProperty> .
<http://purl.org/csm/1.0#Before> <http://www.w3.org/1999/02/22-rdf-syntax-ns#type> <http://purl.org/csm/1.0#EvaluationTime> .
<http://purl.org/csm/1.0#HumanRequirement> <http://www.w3.org/2000/01/rdf-schema#subClassOf> <http://purl.org/csm/1.0#Requirement> .
<http://purl.org/csm/1.0#priorityLevel> <http://www.w3.org/1999/02/22-rdf-syntax-ns#type> <http://www.w3.org/2002/07/owl#DatatypeProperty> .
<http://purl.org/csm/1.0#AssessmentForm> <http://www.w3.org/2000/01/rdf-schema#label> "assessment form" .
<http://purl.org/csm/1.0#estimatedDuration> <http://www.w3.org/2000/01/rdf-schema#comment> "The data property csm:estimatedDuration specifies the estimated time required to complete the crowdsourcing task." .
<http://purl.org/csm/1.0#Requester> <http://www.w3.org/2000/01/rdf-schema#comment> "The class csm:Requester defines the initiator of a crowdsourcing project, such as an individual, a company, or a public organization.\n(related terms: crowdsourcer, client, system owner)" .
<http://purl.org/csm/1.0#Execute> <http://www.w3.org/2000/01/rdf-schema#label> "execute" .
<http://purl.org/csm/1.0#hardwareDevice> <http://www.w3.org/2000/01/rdf-schema#label> "hardware device" .
<http://purl.org/csm/1.0#hasRewardMechanism> <http://www.w3.org/1999/02/22-rdf-syntax-ns#type> <http://www.w3.org/2002/07/owl#ObjectProperty> .
<http://purl.org/csm/1.0#EvaluationTime> <http://www.w3.org/2000/01/rdf-schema#label> "Evaluation Time" .
<http://purl.org/csm/1.0#closureTime> <http://www.w3.org/2000/01/rdf-schema#range> <http://www.w3.org/2001/XMLSchema#dateTime> .
<http://purl.org/csm/1.0#AcceptReject> <http://www.w3.org/1999/02/22-rdf-syntax-ns#type> <http://www.w3.org/2002/07/owl#NamedIndividual> .
<http://purl.org/csm/1.0#Voluntary> <http://www.w3.org/1999/02/22-rdf-syntax-ns#type> <http://purl.org/csm/1.0#RewardNature> .
<http://purl.org/csm/1.0#category> <http://www.w3.org/2000/01/rdf-schema#comment> "The data property csm:category defines the class of a crowdsourcing activity (e.g., idea generation, problem-solving, or content creation)." .
<http://purl.org/csm/1.0#Design> <http://www.w3.org/2000/01/rdf-schema#comment> "to plan or develop something that should be created in the future (compare: create)" .
<http://purl.org/csm/1.0#PayoutMethod> <http://www.w3.org/2000/01/rdf-schema#label> "Payout Method" .
<http://purl.org/csm/1.0#VirtualPoints> <http://www.w3.org/1999/02/22-rdf-syntax-ns#type> <http://purl.org/csm/1.0#RewardType> .
<http://purl.org/csm/1.0#Create> <http://www.w3.org/1999/02/22-rdf-syntax-ns#type> <http://www.w3.org/2002/07/owl#NamedIndividual> .
<http://purl.org/csm/1.0#instruction> <http://www.w3.org/2000/01/rdf-schema#label> "instruction" .
<http://purl.org/csm/1.0#title> <http://www.w3.org/2000/01/rdf-schema#domain> <http://purl.org/csm/1.0#EvaluationMechanism> .
<http://purl.org/csm/1.0#Contribution> <http://www.w3.org/2000/01/rdf-schema#comment> "The class csm:Contribution comprises all data records, content items, documents, or code fragments that contributes to the solution of a crowdsourcing task." .
<http://purl.org/csm/1.0#Categorize> <http://www.w3.org/1999/02/22-rdf-syntax-ns#type> <http://purl.org/csm/1.0#ActionType> .
<http://purl.org/csm/1.0#Rank> <http://www.w3.org/2000/01/rdf-schema#label> "rank" .
<http://purl.org/csm/1.0#ageMax> <http://www.w3.org/2000/01/rdf-schema#label> "maximum age" .
<http://purl.org/csm/1.0#After> <http://www.w3.org/2000/01/rdf-schema#label> "after" .
<http://purl.org/csm/1.0#TechnicalRequirement> <http://www.w3.org/2000/01/rdf-schema#comment> "The class csm:Technical Requirement determines the required hardware and software specifications." .
<http://purl.org/csm/1.0#jobTitle> <http://www.w3.org/2000/01/rdf-schema#domain> <http://purl.org/csm/1.0#HumanRequirement> .
<http://purl.org/csm/1.0#hasPayoutMethod> <http://www.w3.org/2000/01/rdf-schema#range> <http://purl.org/csm/1.0#PayoutMethod> .
<http://purl.org/csm/1.0#language> <http://www.w3.org/2000/01/rdf-schema#label> "language" .
<http://purl.org/csm/1.0#PerformanceBased> <http://www.w3.org/1999/02/22-rdf-syntax-ns#type> <http://www.w3.org/2002/07/owl#NamedIndividual> .
<http://purl.org/csm/1.0#complexityLevel> <http://www.w3.org/1999/02/22-rdf-syntax-ns#type> <http://www.w3.org/2002/07/owl#DatatypeProperty> .
<http://purl.org/csm/1.0#After> <http://www.w3.org/2000/01/rdf-schema#comment> "The evaluation subject is evaluated after finishing the crowdsourcing task. This applies to both participants and contributions." .
<http://purl.org/csm/1.0#TargetAudience> <http://www.w3.org/2000/01/rdf-schema#seeAlso> "Vukovic, M., & Bartolini, C. (2010). Towards a Research Agenda for Enterprise. In T. Margaria & B. Steffen (Eds.), ISoLA 2010 (Vol. 6415, pp. 425–434). Springer Berlin / Heidelberg." .
<http://purl.org/csm/1.0#Label> <http://www.w3.org/1999/02/22-rdf-syntax-ns#type> <http://www.w3.org/2002/07/owl#NamedIndividual> .
<http://purl.org/csm/1.0#hasTargetAudience> <http://www.w3.org/2000/01/rdf-schema#range> <http://purl.org/csm/1.0#TargetAudience> .
<http://purl.org/csm/1.0#issues> <http://www.w3.org/2000/01/rdf-schema#label> "issues" .
<http://purl.org/csm/1.0#EvaluationTime> <http://www.w3.org/1999/02/22-rdf-syntax-ns#type> <http://www.w3.org/2002/07/owl#Class> .
<http://purl.org/csm/1.0#AcceptReject> <http://www.w3.org/1999/02/22-rdf-syntax-ns#type> <http://purl.org/csm/1.0#EvaluationSpecificity> .
<http://purl.org/csm/1.0#description> <http://www.w3.org/1999/02/22-rdf-syntax-ns#type> <http://www.w3.org/2002/07/owl#DatatypeProperty> .
<http://purl.org/csm/1.0#Voluntary> <http://www.w3.org/2000/01/rdf-schema#label> "voluntary" .
<http://purl.org/csm/1.0#submissionTime> <http://www.w3.org/2000/01/rdf-schema#range> <http://www.w3.org/2001/XMLSchema#dateTime> .
<http://purl.org/csm/1.0#Design> <http://www.w3.org/1999/02/22-rdf-syntax-ns#type> <http://purl.org/csm/1.0#ActionType> .
<http://purl.org/csm/1.0#EvaluationSource> <http://www.w3.org/2000/01/rdf-schema#comment> "The class csm:EvaluationSource addresses the choice of the evaluation source. The quality of contributions may either be checked manually by experts or peer workers, often by using a voting and rating mechanism, or automatically by the crowdsourcing system itself, using a specific data processing technique, such as a data mining or machine learning algorithm. Additionally, evaluations services offered by third party organizations may be employed. Finally, the contributors may assess their own work or the requesters may process the evaluation themselves." .
<http://purl.org/csm/1.0#Immediate> <http://www.w3.org/1999/02/22-rdf-syntax-ns#type> <http://purl.org/csm/1.0#LatencyType> .
<http://purl.org/csm/1.0#instruction> <http://www.w3.org/2000/01/rdf-schema#range> <http://www.w3.org/2000/01/rdf-schema#Literal> .
<http://purl.org/csm/1.0#approvalRate> <http://www.w3.org/1999/02/22-rdf-syntax-ns#type> <http://www.w3.org/2002/07/owl#DatatypeProperty> .
<http://purl.org/csm/1.0#TopXParticipants> <http://www.w3.org/1999/02/22-rdf-syntax-ns#type> <http://www.w3.org/2002/07/owl#NamedIndividual> .
<http://purl.org/csm/1.0#language> <http://www.w3.org/2000/01/rdf-schema#comment> "The data property csm:language defines the language that a participant should speak (use 2-digit language code according to ISO 639-1)." .
_:Bdb74931eX2Ddeb4X2D4942X2Da3d8X2De97a0985f6aa <http://www.w3.org/1999/02/22-rdf-syntax-ns#rest> <http://www.w3.org/1999/02/22-rdf-syntax-ns#nil> .
<http://purl.org/csm/1.0#ControlGroup> <http://www.w3.org/2000/01/rdf-schema#label> "control group" .
<http://purl.org/csm/1.0#LatencyType> <http://www.w3.org/2000/01/rdf-schema#label> "Latency Type" .
<http://purl.org/csm/1.0#Participant> <http://www.w3.org/2000/01/rdf-schema#label> "Participant" .
<http://purl.org/csm/1.0#softwarePlatform> <http://www.w3.org/1999/02/22-rdf-syntax-ns#type> <http://www.w3.org/2002/07/owl#DatatypeProperty> .
<http://purl.org/csm/1.0#Immediate> <http://www.w3.org/1999/02/22-rdf-syntax-ns#type> <http://www.w3.org/2002/07/owl#NamedIndividual> .
<http://purl.org/csm/1.0#LatencyType> <http://www.w3.org/1999/02/22-rdf-syntax-ns#type> <http://www.w3.org/2002/07/owl#Class> .
<http://purl.org/csm/1.0#Rate> <http://www.w3.org/2000/01/rdf-schema#label> "rate" .
<http://purl.org/csm/1.0> <http://purl.org/dc/elements/1.1/creator> "Lars Hetmank" .
<http://purl.org/csm/1.0#hasEvaluationMethod> <http://www.w3.org/1999/02/22-rdf-syntax-ns#type> <http://www.w3.org/2002/07/owl#ObjectProperty> .
<http://purl.org/csm/1.0#numberOfAssignments> <http://www.w3.org/2000/01/rdf-schema#domain> <http://purl.org/csm/1.0#Task> .
<http://purl.org/csm/1.0#interactionMode> <http://www.w3.org/2000/01/rdf-schema#comment> "The data property csm:interactionMode enables or disables peer-to-peer collaboration by forbidding or permitting direct communication between the participants." .
<http://purl.org/csm/1.0#hasNext> <http://www.w3.org/2000/01/rdf-schema#domain> <http://purl.org/csm/1.0#Task> .
<http://purl.org/csm/1.0#ControlGroup> <http://www.w3.org/1999/02/22-rdf-syntax-ns#type> <http://www.w3.org/2002/07/owl#NamedIndividual> .
<http://purl.org/csm/1.0#description> <http://www.w3.org/2000/01/rdf-schema#domain> <http://purl.org/csm/1.0#RewardMechanism> .
<http://purl.org/csm/1.0#hasEvaluationMechanism> <http://www.w3.org/2000/01/rdf-schema#range> <http://purl.org/csm/1.0#EvaluationMechanism> .
<http://purl.org/csm/1.0#TechnicalRequirement> <http://www.w3.org/1999/02/22-rdf-syntax-ns#type> <http://www.w3.org/2002/07/owl#Class> .
<http://purl.org/csm/1.0#estimatedDuration> <http://www.w3.org/1999/02/22-rdf-syntax-ns#type> <http://www.w3.org/2002/07/owl#DatatypeProperty> .
<http://purl.org/csm/1.0#title> <http://www.w3.org/2000/01/rdf-schema#range> <http://www.w3.org/2000/01/rdf-schema#Literal> .
<http://purl.org/csm/1.0#ActionType> <http://www.w3.org/2000/01/rdf-schema#label> "Action Type" .
<http://purl.org/csm/1.0#hasLatencyType> <http://www.w3.org/2000/01/rdf-schema#range> <http://purl.org/csm/1.0#LatencyType> .
<http://purl.org/csm/1.0#hasEvaluationSource> <http://www.w3.org/1999/02/22-rdf-syntax-ns#type> <http://www.w3.org/2002/07/owl#ObjectProperty> .
<http://purl.org/csm/1.0#owns> <http://www.w3.org/2000/01/rdf-schema#range> <http://purl.org/csm/1.0#Contribution> .
<http://purl.org/csm/1.0#Rank> <http://www.w3.org/1999/02/22-rdf-syntax-ns#type> <http://purl.org/csm/1.0#ActionType> .
<http://purl.org/csm/1.0#hardwareFeature> <http://www.w3.org/2000/01/rdf-schema#domain> <http://purl.org/csm/1.0#TechnicalRequirement> .
<http://purl.org/csm/1.0#Write> <http://www.w3.org/1999/02/22-rdf-syntax-ns#type> <http://purl.org/csm/1.0#ActionType> .
<http://purl.org/csm/1.0#Contribution> <http://www.w3.org/2000/01/rdf-schema#subClassOf> <http://purl.org/csm/1.0#EvaluationSubject> .
<http://purl.org/csm/1.0#Rate> <http://www.w3.org/1999/02/22-rdf-syntax-ns#type> <http://www.w3.org/2002/07/owl#NamedIndividual> .
<http://purl.org/csm/1.0#currency> <http://www.w3.org/2000/01/rdf-schema#domain> <http://purl.org/csm/1.0#RewardMechanism> .
<http://purl.org/csm/1.0#Fixed> <http://www.w3.org/1999/02/22-rdf-syntax-ns#type> <http://www.w3.org/2002/07/owl#NamedIndividual> .
<http://purl.org/csm/1.0#AllParticipants> <http://www.w3.org/1999/02/22-rdf-syntax-ns#type> <http://www.w3.org/2002/07/owl#NamedIndividual> .
<http://purl.org/csm/1.0#HighConfidential> <http://www.w3.org/1999/02/22-rdf-syntax-ns#type> <http://www.w3.org/2002/07/owl#NamedIndividual> .
<http://purl.org/csm/1.0#hasEvaluationTime> <http://www.w3.org/1999/02/22-rdf-syntax-ns#type> <http://www.w3.org/2002/07/owl#ObjectProperty> .
<http://purl.org/csm/1.0#jobTitle> <http://www.w3.org/1999/02/22-rdf-syntax-ns#type> <http://www.w3.org/2002/07/owl#DatatypeProperty> .
<http://purl.org/csm/1.0#EvaluationSpecificity> <http://www.w3.org/1999/02/22-rdf-syntax-ns#type> <http://www.w3.org/2002/07/owl#Class> .
<http://purl.org/csm/1.0#description> <http://www.w3.org/2000/01/rdf-schema#domain> <http://purl.org/csm/1.0#Requirement> .
<http://purl.org/csm/1.0#User> <http://www.w3.org/1999/02/22-rdf-syntax-ns#type> <http://www.w3.org/2002/07/owl#Class> .
<http://purl.org/csm/1.0#Algorithm> <http://www.w3.org/1999/02/22-rdf-syntax-ns#type> <http://purl.org/csm/1.0#EvaluationSource> .
<http://purl.org/csm/1.0#Coupon> <http://www.w3.org/1999/02/22-rdf-syntax-ns#type> <http://purl.org/csm/1.0#RewardType> .
<http://purl.org/csm/1.0#Share> <http://www.w3.org/1999/02/22-rdf-syntax-ns#type> <http://purl.org/csm/1.0#ActionType> .
<http://purl.org/csm/1.0#hardwareFeature> <http://www.w3.org/2000/01/rdf-schema#comment> "The data property csm:hardwareFeature defines any build-in feature of the hardware device (e.g., processor, memory, GPS, camera, accelerometer, gyrometer)." .
<http://purl.org/csm/1.0#Participant> <http://www.w3.org/2000/01/rdf-schema#subClassOf> <http://purl.org/csm/1.0#EvaluationSubject> .
<http://purl.org/csm/1.0#qualificationLevel> <http://www.w3.org/2000/01/rdf-schema#domain> <http://purl.org/csm/1.0#HumanRequirement> .
<http://purl.org/csm/1.0#Test> <http://www.w3.org/2000/01/rdf-schema#label> "test" .
<http://purl.org/csm/1.0#FreeForm> <http://www.w3.org/1999/02/22-rdf-syntax-ns#type> <http://www.w3.org/2002/07/owl#NamedIndividual> .
_:Bdf186945X2D7f0eX2D4a65X2Db934X2D00f1e241aa66 <http://www.w3.org/1999/02/22-rdf-syntax-ns#first> <http://schema.org/Organization> .
<http://purl.org/csm/1.0#Discount> <http://www.w3.org/1999/02/22-rdf-syntax-ns#type> <http://www.w3.org/2002/07/owl#NamedIndividual> .
<http://purl.org/csm/1.0#hasTask> <http://www.w3.org/1999/02/22-rdf-syntax-ns#type> <http://www.w3.org/2002/07/owl#ObjectProperty> .
<http://purl.org/csm/1.0#Good> <http://www.w3.org/1999/02/22-rdf-syntax-ns#type> <http://purl.org/csm/1.0#RewardType> .
<http://purl.org/csm/1.0#submissionTime> <http://www.w3.org/1999/02/22-rdf-syntax-ns#type> <http://www.w3.org/2002/07/owl#DatatypeProperty> .
<http://purl.org/csm/1.0#Test> <http://www.w3.org/1999/02/22-rdf-syntax-ns#type> <http://purl.org/csm/1.0#ActionType> .
<http://purl.org/csm/1.0#hasEvaluationSpecificity> <http://www.w3.org/2000/01/rdf-schema#range> <http://purl.org/csm/1.0#EvaluationSpecificity> .
<http://purl.org/csm/1.0#EvaluationSubject> <http://www.w3.org/2000/01/rdf-schema#comment> "The class:EvaluationSubject defines the subject of the evaluation (contribution, participant)." .
<http://purl.org/csm/1.0#owns> <http://www.w3.org/2000/01/rdf-schema#comment> "The object property csm:owns defines the contributions that belong to a crowdsourcing task." .
<http://purl.org/csm/1.0#currency> <http://www.w3.org/1999/02/22-rdf-syntax-ns#type> <http://www.w3.org/2002/07/owl#DatatypeProperty> .
<http://purl.org/csm/1.0#hasTask> <http://www.w3.org/2000/01/rdf-schema#range> <http://purl.org/csm/1.0#Task> .
<http://purl.org/csm/1.0#hasEvaluationTime> <http://www.w3.org/2000/01/rdf-schema#label> "has Evaluation Time" .
<http://purl.org/csm/1.0#hasPrevious> <http://www.w3.org/2002/07/owl#inverseOf> <http://purl.org/csm/1.0#hasNext> .
<http://purl.org/csm/1.0#TargetAudience> <http://www.w3.org/1999/02/22-rdf-syntax-ns#type> <http://www.w3.org/2002/07/owl#Class> .
<http://purl.org/csm/1.0#confidentialityLevel> <http://www.w3.org/2000/01/rdf-schema#domain> <http://purl.org/csm/1.0#Task> .
<http://purl.org/csm/1.0#complexityLevel> <http://www.w3.org/2000/01/rdf-schema#comment> "The data property csm:complexityLevel specifies the amount of skills, experiences and knowledge that is required to solve the crowdsourcing task.\n\nUse 'simple', 'moderate', 'complex' to determine the complexity level." .
<http://purl.org/csm/1.0#submits> <http://www.w3.org/2000/01/rdf-schema#comment> "The object property csm:submits defines the contributions that a participant submits." .
<http://purl.org/csm/1.0#Internal> <http://www.w3.org/1999/02/22-rdf-syntax-ns#type> <http://purl.org/csm/1.0#TargetAudience> .
<http://purl.org/csm/1.0#Write> <http://www.w3.org/1999/02/22-rdf-syntax-ns#type> <http://www.w3.org/2002/07/owl#NamedIndividual> .
<http://purl.org/csm/1.0#confidentialityLevel> <http://www.w3.org/2000/01/rdf-schema#comment> "The data property csm:confidentialityLevel classifies if the task and the associated documents that can be shared with third parties." .
<http://purl.org/csm/1.0#Rate> <http://www.w3.org/1999/02/22-rdf-syntax-ns#type> <http://purl.org/csm/1.0#ActionType> .
<http://purl.org/csm/1.0#hasEvaluationSubject> <http://www.w3.org/1999/02/22-rdf-syntax-ns#type> <http://www.w3.org/2002/07/owl#ObjectProperty> .
<http://purl.org/csm/1.0#ActionType> <http://www.w3.org/2000/01/rdf-schema#comment> "The class csm:ActionType specifies the type of action that is required to solve a crowdsourcing task." .
<http://purl.org/csm/1.0#title> <http://www.w3.org/1999/02/22-rdf-syntax-ns#type> <http://www.w3.org/2002/07/owl#DatatypeProperty> .
<http://purl.org/csm/1.0#Before> <http://www.w3.org/2000/01/rdf-schema#comment> "The evaluation subject is evaluated before starting the crowdsourcing task. This only applies to participants." .
<http://purl.org/csm/1.0#hasEvaluationSpecificity> <http://www.w3.org/2000/01/rdf-schema#label> "has Evaluation Specificity" .
<http://purl.org/csm/1.0#hasRewardNature> <http://www.w3.org/1999/02/22-rdf-syntax-ns#type> <http://www.w3.org/2002/07/owl#ObjectProperty> .
<http://purl.org/csm/1.0#amount> <http://www.w3.org/2000/01/rdf-schema#comment> "The data property csm:amount defines the number of points or monetary value." .
<http://purl.org/csm/1.0#hasEvaluationSource> <http://www.w3.org/2000/01/rdf-schema#label> "has Evaluation Source" .
<http://purl.org/csm/1.0#hasActionType> <http://www.w3.org/1999/02/22-rdf-syntax-ns#type> <http://www.w3.org/2002/07/owl#ObjectProperty> .
<http://purl.org/csm/1.0#Create> <http://www.w3.org/2000/01/rdf-schema#label> "create" .
<http://purl.org/csm/1.0#hasExternalResource> <http://www.w3.org/1999/02/22-rdf-syntax-ns#type> <http://www.w3.org/2002/07/owl#ObjectProperty> .
<http://purl.org/csm/1.0#ageMax> <http://www.w3.org/1999/02/22-rdf-syntax-ns#type> <http://www.w3.org/2002/07/owl#DatatypeProperty> .
<http://purl.org/csm/1.0#country> <http://www.w3.org/2000/01/rdf-schema#domain> <http://purl.org/csm/1.0#HumanRequirement> .
<http://purl.org/csm/1.0#Test> <http://www.w3.org/1999/02/22-rdf-syntax-ns#type> <http://www.w3.org/2002/07/owl#NamedIndividual> .
<http://purl.org/csm/1.0#approvalRate> <http://www.w3.org/2000/01/rdf-schema#label> "approval rate" .
<http://purl.org/csm/1.0#submissionTime> <http://www.w3.org/2000/01/rdf-schema#comment> "The data property csm:submissionTime defines the time when the task is accessible for the crowd." .
<http://purl.org/csm/1.0#Algorithm> <http://www.w3.org/1999/02/22-rdf-syntax-ns#type> <http://www.w3.org/2002/07/owl#NamedIndividual> .
<http://purl.org/csm/1.0#TopXParticipants> <http://www.w3.org/1999/02/22-rdf-syntax-ns#type> <http://purl.org/csm/1.0#PayoutMethod> .
<http://purl.org/csm/1.0#title> <http://www.w3.org/2000/01/rdf-schema#domain> <http://purl.org/csm/1.0#RewardMechanism> .
<http://purl.org/csm/1.0#description> <http://www.w3.org/2000/01/rdf-schema#range> <http://www.w3.org/2000/01/rdf-schema#Literal> .
<http://purl.org/csm/1.0#RewardNature> <http://www.w3.org/2000/01/rdf-schema#label> "Reward Nature" .
<http://purl.org/csm/1.0#FreeForm> <http://www.w3.org/2000/01/rdf-schema#label> "free form" .
<http://purl.org/csm/1.0#ageMax> <http://www.w3.org/2000/01/rdf-schema#range> <http://www.w3.org/2001/XMLSchema#unsignedByte> .
<http://purl.org/csm/1.0#instruction> <http://www.w3.org/2000/01/rdf-schema#comment> "The data property csm:instruction is a free text that contains the instruction for the task." .
<http://purl.org/csm/1.0#hasAggregationType> <http://www.w3.org/2000/01/rdf-schema#range> <http://purl.org/csm/1.0#AggregationType> .
<http://purl.org/csm/1.0#Share> <http://www.w3.org/1999/02/22-rdf-syntax-ns#type> <http://www.w3.org/2002/07/owl#NamedIndividual> .
<http://purl.org/csm/1.0> <http://www.w3.org/2002/07/owl#versionInfo> "Revision: 1.0" .
<http://purl.org/csm/1.0#instruction> <http://www.w3.org/1999/02/22-rdf-syntax-ns#type> <http://www.w3.org/2002/07/owl#DatatypeProperty> .
<http://purl.org/csm/1.0#Iterative> <http://www.w3.org/2000/01/rdf-schema#label> "iterative" .
<http://purl.org/csm/1.0#Task> <http://www.w3.org/1999/02/22-rdf-syntax-ns#type> <http://www.w3.org/2002/07/owl#Class> .
<http://purl.org/csm/1.0#softwarePlatform> <http://www.w3.org/2000/01/rdf-schema#range> <http://www.w3.org/2000/01/rdf-schema#Literal> .
<http://purl.org/csm/1.0#Design> <http://www.w3.org/1999/02/22-rdf-syntax-ns#type> <http://www.w3.org/2002/07/owl#NamedIndividual> .
<http://purl.org/csm/1.0#Play> <http://www.w3.org/2000/01/rdf-schema#comment> "to play a game" .
<http://purl.org/csm/1.0#Iterative> <http://www.w3.org/1999/02/22-rdf-syntax-ns#type> <http://purl.org/csm/1.0#AggregationType> .
<http://purl.org/csm/1.0#approvalRate> <http://www.w3.org/2000/01/rdf-schema#range> <http://www.w3.org/2001/XMLSchema#float> .
<http://purl.org/csm/1.0#title> <http://www.w3.org/2000/01/rdf-schema#domain> <http://purl.org/csm/1.0#Requirement> .
<http://purl.org/csm/1.0#hasNext> <http://www.w3.org/2000/01/rdf-schema#label> "has Next" .
<http://purl.org/csm/1.0#EvaluationSubject> <http://www.w3.org/1999/02/22-rdf-syntax-ns#type> <http://www.w3.org/2002/07/owl#Class> .
<http://purl.org/csm/1.0#HumanRequirement> <http://www.w3.org/2000/01/rdf-schema#label> "Human Requirement" .
<http://purl.org/csm/1.0#imposes> <http://www.w3.org/2000/01/rdf-schema#comment> "The object property csm:imposes defines the requirements of a crowdsourcing task." .
<http://purl.org/csm/1.0#User> <http://www.w3.org/2002/07/owl#equivalentClass> <http://purl.org/goodrelations/v1#BusinessEntity> .
<http://purl.org/csm/1.0#Money> <http://www.w3.org/1999/02/22-rdf-syntax-ns#type> <http://www.w3.org/2002/07/owl#NamedIndividual> .
<http://purl.org/csm/1.0#Rating> <http://www.w3.org/1999/02/22-rdf-syntax-ns#type> <http://www.w3.org/2002/07/owl#NamedIndividual> .
<http://purl.org/csm/1.0#hasRewardNature> <http://www.w3.org/2000/01/rdf-schema#domain> <http://purl.org/csm/1.0#RewardMechanism> .
<http://purl.org/csm/1.0#Integrative> <http://www.w3.org/2000/01/rdf-schema#comment> "Example: knowledge acquisition and aggregation\n(similar to accumulative crowdsourcing, collaboration-based)" .
<http://purl.org/csm/1.0#User> <http://www.w3.org/2002/07/owl#equivalentClass> <http://xmlns.com/foaf/0.1/Person> .
<http://purl.org/csm/1.0#MajorityDecision> <http://www.w3.org/2000/01/rdf-schema#comment> "The majority decision approach assigns the task to multiple users who submit their individual results to the crowdsourcing system, and finally selects the most frequent result." .
<http://purl.org/csm/1.0#hasTargetAudience> <http://www.w3.org/1999/02/22-rdf-syntax-ns#type> <http://www.w3.org/2002/07/owl#ObjectProperty> .
<http://purl.org/csm/1.0#Hybrid> <http://www.w3.org/1999/02/22-rdf-syntax-ns#type> <http://www.w3.org/2002/07/owl#NamedIndividual> .
<http://purl.org/csm/1.0#Rank> <http://www.w3.org/1999/02/22-rdf-syntax-ns#type> <http://www.w3.org/2002/07/owl#NamedIndividual> .
<http://purl.org/csm/1.0#EvaluationSource> <http://www.w3.org/2000/01/rdf-schema#label> "Evaluation Source" .
<http://purl.org/csm/1.0#Requester> <http://www.w3.org/2000/01/rdf-schema#subClassOf> <http://purl.org/csm/1.0#User> .
<http://purl.org/csm/1.0> <http://www.w3.org/1999/02/22-rdf-syntax-ns#type> <http://www.w3.org/2002/07/owl#Ontology> .
<http://purl.org/csm/1.0#interactionMode> <http://www.w3.org/1999/02/22-rdf-syntax-ns#type> <http://www.w3.org/2002/07/owl#DatatypeProperty> .
<http://purl.org/csm/1.0#numberOfApprovedTask> <http://www.w3.org/2000/01/rdf-schema#comment> "The data property csm:numberOfApprovedTask defines the number of properly solved tasks." .
<http://purl.org/csm/1.0#closureTime> <http://www.w3.org/2000/01/rdf-schema#domain> <http://purl.org/csm/1.0#Project> .
<http://purl.org/csm/1.0#hasRewardNature> <http://www.w3.org/2000/01/rdf-schema#range> <http://purl.org/csm/1.0#RewardNature> .
<http://purl.org/csm/1.0#Money> <http://www.w3.org/2000/01/rdf-schema#label> "money" .
<http://purl.org/csm/1.0#AllParticipants> <http://www.w3.org/1999/02/22-rdf-syntax-ns#type> <http://purl.org/csm/1.0#PayoutMethod> .
<http://purl.org/csm/1.0#interactionMode> <http://www.w3.org/2000/01/rdf-schema#range> <http://www.w3.org/2001/XMLSchema#boolean> .
<http://purl.org/csm/1.0#RewardMechanism> <http://www.w3.org/2000/01/rdf-schema#comment> "The class csm:RewardMechanism describes the configuration of a certain type of reward mechanism." .
_:Bdb74931eX2Ddeb4X2D4942X2Da3d8X2De97a0985f6aa <http://www.w3.org/1999/02/22-rdf-syntax-ns#first> <http://schema.org/Person> .
