<https://w3id.org/ibp/CTRLont#hasMedium>
        a       <http://www.w3.org/2002/07/owl#ObjectProperty> ;
        <http://www.w3.org/2000/01/rdf-schema#comment>
                "Object property to annotate an input, output or parameter with its medium."@en ;
        <http://www.w3.org/2000/01/rdf-schema#domain>
                <https://w3id.org/ibp/CTRLont#AnnotatedElement> ;
        <http://www.w3.org/2000/01/rdf-schema#isDefinedBy>
                <https://w3id.org/ibp/CTRLont#ctrl> ;
        <http://www.w3.org/2000/01/rdf-schema#label>
                "hasMedium"@en ;
        <http://www.w3.org/2000/01/rdf-schema#range>
                <https://w3id.org/ibp/CTRLont#Medium> ;
        <http://www.w3.org/2003/06/sw-vocab-status/ns#term_status>
                "stable" .

<https://w3id.org/ibp/CTRLont#Unit>
        a       <http://www.w3.org/2002/07/owl#Class> ;
        <http://www.w3.org/2000/01/rdf-schema#comment>
                "Placeholder concept to stipulate reuse of existing ontologies such as Ontology for Units and Measures (OM) or QUDT."@en ;
        <http://www.w3.org/2000/01/rdf-schema#isDefinedBy>
                <https://w3id.org/ibp/CTRLont#ctrl> ;
        <http://www.w3.org/2000/01/rdf-schema#label>
                "Unit"@en ;
        <http://www.w3.org/2003/06/sw-vocab-status/ns#term_status>
                "stable" .

<https://w3id.org/ibp/CTRLont>
        a       <http://www.w3.org/2002/07/owl#Ontology> , <http://www.w3.org/2002/07/owl#NamedIndividual> , <http://purl.org/vocommons/voaf#Vocabulary> ;
        <http://www.w3.org/2000/01/rdf-schema#comment>
                "CTRLont specifies concepts and relationships of control actors on a high level."@en ;
        <http://www.w3.org/2000/01/rdf-schema#label>
                "CTRLont"@en ;
        <http://purl.org/dc/terms/creator>
                "Georg Ferdinand Schneider" ;
        <http://purl.org/dc/terms/creator>
                <https://www.researchgate.net/profile/Georg_Schneider3> , <https://orcid.org/0000-0002-2033-859X> ;
        <http://purl.org/dc/terms/description>
                "The ontology and its use are described in [1]. The ontology is implemented using the free protege tool (protege.stanford.edu) [2].\n\n[1] Schneider, G.F., Pauwels, P. and Steiger, S. (2017): \"Ontology-based Modelling of Control Logic in Building Automation Systems\" in IEEE Transactions on Industrial Informatics, vol. 13, no. 6, pp. 3350-3360, DOI: 10.1109/TII.2017.2743221.\n\n[2] M. A. Musen (2015): The protege project: a look back and a look forward. AI matters, 1(4):4-12, doi: 10.1145/2757001.2757003."@en ;
        <http://purl.org/dc/terms/identifier>
                "https://w3id.org/ibp/CTRLont#" ;
        <http://purl.org/dc/terms/issued>
                "2016-11-01"^^<http://www.w3.org/2001/XMLSchema#date> ;
        <http://purl.org/dc/terms/license>
                <http://creativecommons.org/licenses/by-sa/4.0> ;
        <http://purl.org/dc/terms/modified>
                "2019-04-29"^^<http://www.w3.org/2001/XMLSchema#date> ;
        <http://purl.org/dc/terms/publisher>
                <https://www.ibp.fraunhofer.de> ;
        <http://purl.org/dc/terms/rights>
                "Copyright (c) 2019 Georg Ferdinand Schneider/ Fraunhofer Institute for Building Physics IBP. This ontology is distributed under a Creative Commons Attribution \nShare Alike License (CC BY-SA 4.0) http://creativecommons.org/licenses/by-sa/4.0"@en ;
        <http://purl.org/dc/terms/title>
                "CTRLont - An ontology to formally specify the control domain."@en ;
        <http://purl.org/vocab/vann/preferredNamespacePrefix>
                "ctrl" ;
        <http://purl.org/vocab/vann/preferredNamespaceUri>
                <https://w3id.org/ibp/CTRLont#> ;
        <http://www.w3.org/2002/07/owl#priorVersion>
                <https://w3id.org/ibp/CTRLont-0.0.1> ;
        <http://www.w3.org/2002/07/owl#versionIRI>
                <https://w3id.org/ibp/CTRLont-0.3.0> ;
        <http://www.w3.org/2002/07/owl#versionInfo>
                "v0.3.0" .

<https://w3id.org/ibp/CTRLont#Output>
        a       <http://www.w3.org/2002/07/owl#Class> ;
        <http://www.w3.org/2000/01/rdf-schema#comment>
                "An output allows compute results by the application logic of an control actor to be fowarded to outside entities such as actuators or other control actors."@en ;
        <http://www.w3.org/2000/01/rdf-schema#isDefinedBy>
                <https://w3id.org/ibp/CTRLont#ctrl> ;
        <http://www.w3.org/2000/01/rdf-schema#label>
                "Output"@en ;
        <http://www.w3.org/2000/01/rdf-schema#subClassOf>
                <https://w3id.org/ibp/CTRLont#AnnotatedElement> ;
        <http://www.w3.org/2002/07/owl#disjointWith>
                <https://w3id.org/ibp/CTRLont#Parameter> ;
        <http://www.w3.org/2003/06/sw-vocab-status/ns#term_status>
                "stable" .

<https://w3id.org/ibp/CTRLont#hasInput>
        a       <http://www.w3.org/2002/07/owl#ObjectProperty> ;
        <http://www.w3.org/2000/01/rdf-schema#comment>
                "Object property to relate a control actor to its inputs."@en ;
        <http://www.w3.org/2000/01/rdf-schema#domain>
                <https://w3id.org/ibp/CTRLont#ControlActor> ;
        <http://www.w3.org/2000/01/rdf-schema#isDefinedBy>
                <https://w3id.org/ibp/CTRLont#ctrl> ;
        <http://www.w3.org/2000/01/rdf-schema#label>
                "hasInput"@en ;
        <http://www.w3.org/2000/01/rdf-schema#range>
                <https://w3id.org/ibp/CTRLont#Input> ;
        <http://www.w3.org/2003/06/sw-vocab-status/ns#term_status>
                "stable" .

<https://w3id.org/ibp/CTRLont#hasQuantity>
        a       <http://www.w3.org/2002/07/owl#ObjectProperty> ;
        <http://www.w3.org/2000/01/rdf-schema#comment>
                "Object property to annotate an input, output or parameter with its quantity."@en ;
        <http://www.w3.org/2000/01/rdf-schema#domain>
                <https://w3id.org/ibp/CTRLont#AnnotatedElement> ;
        <http://www.w3.org/2000/01/rdf-schema#isDefinedBy>
                <https://w3id.org/ibp/CTRLont#ctrl> ;
        <http://www.w3.org/2000/01/rdf-schema#label>
                "hasQuantity"@en ;
        <http://www.w3.org/2000/01/rdf-schema#range>
                <https://w3id.org/ibp/CTRLont#Quantity> ;
        <http://www.w3.org/2003/06/sw-vocab-status/ns#term_status>
                "stable" .

<https://w3id.org/ibp/CTRLont#logicOutput>
        a       <http://www.w3.org/2002/07/owl#ObjectProperty> ;
        <http://www.w3.org/2000/01/rdf-schema#comment>
                "Object property to express the relationship of some application logic concept to an output."@en ;
        <http://www.w3.org/2000/01/rdf-schema#isDefinedBy>
                <https://w3id.org/ibp/CTRLont#ctrl> ;
        <http://www.w3.org/2000/01/rdf-schema#label>
                "logicOutput"@en ;
        <http://www.w3.org/2000/01/rdf-schema#range>
                <https://w3id.org/ibp/CTRLont#Output> ;
        <http://www.w3.org/2003/06/sw-vocab-status/ns#term_status>
                "stable" .

<https://w3id.org/ibp/CTRLont#hasOutput>
        a       <http://www.w3.org/2002/07/owl#ObjectProperty> ;
        <http://www.w3.org/2000/01/rdf-schema#comment>
                "Object property to relate a control actor to its outputs."@en ;
        <http://www.w3.org/2000/01/rdf-schema#domain>
                <https://w3id.org/ibp/CTRLont#ControlActor> ;
        <http://www.w3.org/2000/01/rdf-schema#isDefinedBy>
                <https://w3id.org/ibp/CTRLont#ctrl> ;
        <http://www.w3.org/2000/01/rdf-schema#label>
                "hasOutput"@en ;
        <http://www.w3.org/2000/01/rdf-schema#range>
                <https://w3id.org/ibp/CTRLont#Output> ;
        <http://www.w3.org/2003/06/sw-vocab-status/ns#term_status>
                "stable" .

<https://w3id.org/ibp/CTRLont#ApplicationLogic>
        a       <http://www.w3.org/2002/07/owl#Class> ;
        <http://www.w3.org/2000/01/rdf-schema#comment>
                "Concept to specify the application logic of a control actor. Seperate ontologies may be used to further specify this concept."@en ;
        <http://www.w3.org/2000/01/rdf-schema#isDefinedBy>
                <https://w3id.org/ibp/CTRLont#ctrl> ;
        <http://www.w3.org/2000/01/rdf-schema#label>
                "Application Logic"@en ;
        <http://www.w3.org/2003/06/sw-vocab-status/ns#term_status>
                "stable" .

<https://w3id.org/ibp/CTRLont#logicParameter>
        a       <http://www.w3.org/2002/07/owl#ObjectProperty> ;
        <http://www.w3.org/2000/01/rdf-schema#comment>
                "Object property to express the relationship of some application logic concept to an parameter."@en ;
        <http://www.w3.org/2000/01/rdf-schema#isDefinedBy>
                <https://w3id.org/ibp/CTRLont#ctrl> ;
        <http://www.w3.org/2000/01/rdf-schema#label>
                "logicParameter"@en ;
        <http://www.w3.org/2000/01/rdf-schema#range>
                <https://w3id.org/ibp/CTRLont#Parameter> ;
        <http://www.w3.org/2003/06/sw-vocab-status/ns#term_status>
                "stable" .

<https://w3id.org/ibp/CTRLont#DataType>
        a       <http://www.w3.org/2002/07/owl#Class> ;
        <http://www.w3.org/2000/01/rdf-schema#comment>
                "Placeholder class for the specification of basic data types such as, e.g. integer, boolean or double."@en ;
        <http://www.w3.org/2000/01/rdf-schema#isDefinedBy>
                <https://w3id.org/ibp/CTRLont#ctrl> ;
        <http://www.w3.org/2000/01/rdf-schema#label>
                "Data type"@en ;
        <http://www.w3.org/2000/01/rdf-schema#seeAlso>
                "https://www.w3.org/TR/xmlschema-2/#built-in-datatypes"^^<http://www.w3.org/2001/XMLSchema#anyURI> ;
        <http://www.w3.org/2003/06/sw-vocab-status/ns#term_status>
                "stable" .

<https://w3id.org/ibp/CTRLont#AnnotatedElement>
        a       <http://www.w3.org/2002/07/owl#Class> ;
        <http://www.w3.org/2000/01/rdf-schema#comment>
                "An annotated element is a generic superclass for ctrl:Input, ctrl:Output and ctrl:Parameter"@en ;
        <http://www.w3.org/2000/01/rdf-schema#isDefinedBy>
                <https://w3id.org/ibp/CTRLont#ctrl> ;
        <http://www.w3.org/2000/01/rdf-schema#label>
                "Annotated Element"@en ;
        <http://www.w3.org/2000/01/rdf-schema#subClassOf>
                [ a       <http://www.w3.org/2002/07/owl#Restriction> ;
                  <http://www.w3.org/2002/07/owl#allValuesFrom>
                          <https://w3id.org/ibp/CTRLont#SemanticType> ;
                  <http://www.w3.org/2002/07/owl#onProperty>
                          <https://w3id.org/ibp/CTRLont#hasSemanticType>
                ] ;
        <http://www.w3.org/2000/01/rdf-schema#subClassOf>
                [ a       <http://www.w3.org/2002/07/owl#Restriction> ;
                  <http://www.w3.org/2002/07/owl#allValuesFrom>
                          <https://w3id.org/ibp/CTRLont#Unit> ;
                  <http://www.w3.org/2002/07/owl#onProperty>
                          <https://w3id.org/ibp/CTRLont#hasUnit>
                ] ;
        <http://www.w3.org/2000/01/rdf-schema#subClassOf>
                [ a       <http://www.w3.org/2002/07/owl#Restriction> ;
                  <http://www.w3.org/2002/07/owl#allValuesFrom>
                          <https://w3id.org/ibp/CTRLont#DataType> ;
                  <http://www.w3.org/2002/07/owl#onProperty>
                          <https://w3id.org/ibp/CTRLont#hasDataType>
                ] ;
        <http://www.w3.org/2000/01/rdf-schema#subClassOf>
                [ a       <http://www.w3.org/2002/07/owl#Restriction> ;
                  <http://www.w3.org/2002/07/owl#allValuesFrom>
                          <https://w3id.org/ibp/CTRLont#Quantity> ;
                  <http://www.w3.org/2002/07/owl#onProperty>
                          <https://w3id.org/ibp/CTRLont#hasQuantity>
                ] ;
        <http://www.w3.org/2000/01/rdf-schema#subClassOf>
                [ a       <http://www.w3.org/2002/07/owl#Restriction> ;
                  <http://www.w3.org/2002/07/owl#allValuesFrom>
                          <https://w3id.org/ibp/CTRLont#Medium> ;
                  <http://www.w3.org/2002/07/owl#onProperty>
                          <https://w3id.org/ibp/CTRLont#hasMedium>
                ] ;
        <http://www.w3.org/2003/06/sw-vocab-status/ns#term_status>
                "stable" .

<https://w3id.org/ibp/CTRLont#ControlActor>
        a       <http://www.w3.org/2002/07/owl#Class> ;
        <http://www.w3.org/2000/01/rdf-schema#comment>
                "Concept to describe the in general accepted Sense-Process-Actuate\npattern in automation systems, e.g. function blocks from IEC 61499."@en ;
        <http://www.w3.org/2000/01/rdf-schema#isDefinedBy>
                <https://w3id.org/ibp/CTRLont#ctrl> ;
        <http://www.w3.org/2000/01/rdf-schema#label>
                "Control Actor"@en ;
        <http://www.w3.org/2000/01/rdf-schema#subClassOf>
                [ a       <http://www.w3.org/2002/07/owl#Restriction> ;
                  <http://www.w3.org/2002/07/owl#onProperty>
                          <https://w3id.org/ibp/CTRLont#hasApplicationLogic> ;
                  <http://www.w3.org/2002/07/owl#someValuesFrom>
                          <https://w3id.org/ibp/CTRLont#ApplicationLogic>
                ] ;
        <http://www.w3.org/2000/01/rdf-schema#subClassOf>
                [ a       <http://www.w3.org/2002/07/owl#Restriction> ;
                  <http://www.w3.org/2002/07/owl#allValuesFrom>
                          <https://w3id.org/ibp/CTRLont#Output> ;
                  <http://www.w3.org/2002/07/owl#onProperty>
                          <https://w3id.org/ibp/CTRLont#hasOutput>
                ] ;
        <http://www.w3.org/2000/01/rdf-schema#subClassOf>
                [ a       <http://www.w3.org/2002/07/owl#Restriction> ;
                  <http://www.w3.org/2002/07/owl#allValuesFrom>
                          <https://w3id.org/ibp/CTRLont#Parameter> ;
                  <http://www.w3.org/2002/07/owl#onProperty>
                          <https://w3id.org/ibp/CTRLont#hasParameter>
                ] ;
        <http://www.w3.org/2000/01/rdf-schema#subClassOf>
                [ a       <http://www.w3.org/2002/07/owl#Restriction> ;
                  <http://www.w3.org/2002/07/owl#onProperty>
                          <https://w3id.org/ibp/CTRLont#hasOutput> ;
                  <http://www.w3.org/2002/07/owl#someValuesFrom>
                          <https://w3id.org/ibp/CTRLont#Output>
                ] ;
        <http://www.w3.org/2000/01/rdf-schema#subClassOf>
                [ a       <http://www.w3.org/2002/07/owl#Restriction> ;
                  <http://www.w3.org/2002/07/owl#allValuesFrom>
                          <https://w3id.org/ibp/CTRLont#ApplicationLogic> ;
                  <http://www.w3.org/2002/07/owl#onProperty>
                          <https://w3id.org/ibp/CTRLont#hasApplicationLogic>
                ] ;
        <http://www.w3.org/2000/01/rdf-schema#subClassOf>
                [ a       <http://www.w3.org/2002/07/owl#Restriction> ;
                  <http://www.w3.org/2002/07/owl#allValuesFrom>
                          <https://w3id.org/ibp/CTRLont#Input> ;
                  <http://www.w3.org/2002/07/owl#onProperty>
                          <https://w3id.org/ibp/CTRLont#hasInput>
                ] ;
        <http://www.w3.org/2003/06/sw-vocab-status/ns#term_status>
                "stable" .

<https://w3id.org/ibp/CTRLont#isConnectedTo>
        a       <http://www.w3.org/2002/07/owl#ObjectProperty> ;
        <http://www.w3.org/2000/01/rdf-schema#comment>
                "Object property to describe the topological relationship between an input of one control actor and the output of another."@en ;
        <http://www.w3.org/2000/01/rdf-schema#domain>
                <https://w3id.org/ibp/CTRLont#Output> ;
        <http://www.w3.org/2000/01/rdf-schema#isDefinedBy>
                <https://w3id.org/ibp/CTRLont#ctrl> ;
        <http://www.w3.org/2000/01/rdf-schema#label>
                "isConnectedTo"@en ;
        <http://www.w3.org/2000/01/rdf-schema#range>
                <https://w3id.org/ibp/CTRLont#Input> ;
        <http://www.w3.org/2003/06/sw-vocab-status/ns#term_status>
                "stable" .

<https://w3id.org/ibp/CTRLont#supervises>
        a       <http://www.w3.org/2002/07/owl#ObjectProperty> ;
        <http://www.w3.org/2000/01/rdf-schema#comment>
                "Object property to describe if one control actor supervises another."@en ;
        <http://www.w3.org/2000/01/rdf-schema#domain>
                <https://w3id.org/ibp/CTRLont#ControlActor> ;
        <http://www.w3.org/2000/01/rdf-schema#isDefinedBy>
                <https://w3id.org/ibp/CTRLont#ctrl> ;
        <http://www.w3.org/2000/01/rdf-schema#label>
                "supervises"@en ;
        <http://www.w3.org/2000/01/rdf-schema#range>
                <https://w3id.org/ibp/CTRLont#ControlActor> ;
        <http://www.w3.org/2003/06/sw-vocab-status/ns#term_status>
                "stable" .

<https://w3id.org/ibp/CTRLont#hasParameter>
        a       <http://www.w3.org/2002/07/owl#ObjectProperty> ;
        <http://www.w3.org/2000/01/rdf-schema#comment>
                "Object property to relate a control actor to its parameter."@en ;
        <http://www.w3.org/2000/01/rdf-schema#domain>
                <https://w3id.org/ibp/CTRLont#ControlActor> ;
        <http://www.w3.org/2000/01/rdf-schema#isDefinedBy>
                <https://w3id.org/ibp/CTRLont#ctrl> ;
        <http://www.w3.org/2000/01/rdf-schema#label>
                "hasParameter"@en ;
        <http://www.w3.org/2000/01/rdf-schema#range>
                <https://w3id.org/ibp/CTRLont#Parameter> ;
        <http://www.w3.org/2003/06/sw-vocab-status/ns#term_status>
                "stable" .

<https://w3id.org/ibp/CTRLont#Medium>
        a       <http://www.w3.org/2002/07/owl#Class> ;
        <http://www.w3.org/2000/01/rdf-schema#comment>
                "Placeholder concept to stipulate reuse of existing ontologies such as dbpedia or  \thttp://www.productontology.org/id/"@en ;
        <http://www.w3.org/2000/01/rdf-schema#isDefinedBy>
                <https://w3id.org/ibp/CTRLont#ctrl> ;
        <http://www.w3.org/2000/01/rdf-schema#label>
                "Medium"@en ;
        <http://www.w3.org/2000/01/rdf-schema#seeAlso>
                <http://wiki.dbpedia.org/> , <http://www.productontology.org/id/> ;
        <http://www.w3.org/2003/06/sw-vocab-status/ns#term_status>
                "stable" .

<https://w3id.org/ibp/CTRLont#hasApplicationLogic>
        a       <http://www.w3.org/2002/07/owl#ObjectProperty> ;
        <http://www.w3.org/2000/01/rdf-schema#comment>
                "Object property to relate a control actor to its specific application logic"@en ;
        <http://www.w3.org/2000/01/rdf-schema#isDefinedBy>
                <https://w3id.org/ibp/CTRLont#ctrl> ;
        <http://www.w3.org/2000/01/rdf-schema#label>
                "hasApplicationLogic"@en ;
        <http://www.w3.org/2000/01/rdf-schema#range>
                <https://w3id.org/ibp/CTRLont#ApplicationLogic> ;
        <http://www.w3.org/2003/06/sw-vocab-status/ns#term_status>
                "stable" .

<https://w3id.org/ibp/CTRLont#hasDataType>
        a       <http://www.w3.org/2002/07/owl#ObjectProperty> ;
        <http://www.w3.org/2000/01/rdf-schema#comment>
                "Object property to annotate a input, output or parameter with its data type."@en ;
        <http://www.w3.org/2000/01/rdf-schema#domain>
                <https://w3id.org/ibp/CTRLont#AnnotatedElement> ;
        <http://www.w3.org/2000/01/rdf-schema#isDefinedBy>
                <https://w3id.org/ibp/CTRLont#ctrl> ;
        <http://www.w3.org/2000/01/rdf-schema#label>
                "hasDataType"@en ;
        <http://www.w3.org/2000/01/rdf-schema#range>
                <https://w3id.org/ibp/CTRLont#DataType> ;
        <http://www.w3.org/2003/06/sw-vocab-status/ns#term_status>
                "stable" .

<https://w3id.org/ibp/CTRLont#logicInput>
        a       <http://www.w3.org/2002/07/owl#ObjectProperty> ;
        <http://www.w3.org/2000/01/rdf-schema#comment>
                "Object property to express the relationship of some application logic concept to an input."@en ;
        <http://www.w3.org/2000/01/rdf-schema#isDefinedBy>
                <https://w3id.org/ibp/CTRLont#ctrl> ;
        <http://www.w3.org/2000/01/rdf-schema#label>
                "logicInput"@en ;
        <http://www.w3.org/2000/01/rdf-schema#range>
                <https://w3id.org/ibp/CTRLont#Input> ;
        <http://www.w3.org/2003/06/sw-vocab-status/ns#term_status>
                "stable" .

<https://w3id.org/ibp/CTRLont#isSupervisedBy>
        a       <http://www.w3.org/2002/07/owl#ObjectProperty> ;
        <http://www.w3.org/2000/01/rdf-schema#comment>
                "Object property to describe hierarchical composition of control actors."@en ;
        <http://www.w3.org/2000/01/rdf-schema#domain>
                <https://w3id.org/ibp/CTRLont#ControlActor> ;
        <http://www.w3.org/2000/01/rdf-schema#isDefinedBy>
                <https://w3id.org/ibp/CTRLont#ctrl> ;
        <http://www.w3.org/2000/01/rdf-schema#label>
                "isSupervisedBy"@en ;
        <http://www.w3.org/2000/01/rdf-schema#range>
                <https://w3id.org/ibp/CTRLont#ControlActor> ;
        <http://www.w3.org/2002/07/owl#inverseOf>
                <https://w3id.org/ibp/CTRLont#supervises> ;
        <http://www.w3.org/2003/06/sw-vocab-status/ns#term_status>
                "stable" .

<https://w3id.org/ibp/CTRLont#Quantity>
        a       <http://www.w3.org/2002/07/owl#Class> ;
        <http://www.w3.org/2000/01/rdf-schema#comment>
                "Placeholder concept to stipulate reuse of existing ontologies such as Ontology for Units and Measures (OM) or QUDT."@en ;
        <http://www.w3.org/2000/01/rdf-schema#isDefinedBy>
                <https://w3id.org/ibp/CTRLont#ctrl> ;
        <http://www.w3.org/2000/01/rdf-schema#label>
                "Quantity"@en ;
        <http://www.w3.org/2000/01/rdf-schema#seeAlso>
                <http://www.ontology-of-units-of-measure.org/resource/om-2/> , <http://qudt.org/schema/qudt> ;
        <http://www.w3.org/2003/06/sw-vocab-status/ns#term_status>
                "stable" .

<https://w3id.org/ibp/CTRLont#Parameter>
        a       <http://www.w3.org/2002/07/owl#Class> ;
        <http://www.w3.org/2000/01/rdf-schema#comment>
                "Parameter describe time-invariant values and settings of the respective control actor. Thus thay can be added dependent on the respective application logic."@en ;
        <http://www.w3.org/2000/01/rdf-schema#isDefinedBy>
                <https://w3id.org/ibp/CTRLont#ctrl> ;
        <http://www.w3.org/2000/01/rdf-schema#label>
                "Parameter"@en ;
        <http://www.w3.org/2000/01/rdf-schema#subClassOf>
                <https://w3id.org/ibp/CTRLont#AnnotatedElement> ;
        <http://www.w3.org/2003/06/sw-vocab-status/ns#term_status>
                "stable" .

<https://w3id.org/ibp/CTRLont#hasSemanticType>
        a       <http://www.w3.org/2002/07/owl#ObjectProperty> ;
        <http://www.w3.org/2000/01/rdf-schema#comment>
                "Object property to relate an input, output or parameter with its semantic type."@en ;
        <http://www.w3.org/2000/01/rdf-schema#domain>
                <https://w3id.org/ibp/CTRLont#AnnotatedElement> ;
        <http://www.w3.org/2000/01/rdf-schema#isDefinedBy>
                <https://w3id.org/ibp/CTRLont#ctrl> ;
        <http://www.w3.org/2000/01/rdf-schema#label>
                "hasSemanticType"@en ;
        <http://www.w3.org/2000/01/rdf-schema#range>
                <https://w3id.org/ibp/CTRLont#SemanticType> ;
        <http://www.w3.org/2003/06/sw-vocab-status/ns#term_status>
                "stable" .

<https://w3id.org/ibp/CTRLont#hasUnit>
        a       <http://www.w3.org/2002/07/owl#ObjectProperty> ;
        <http://www.w3.org/2000/01/rdf-schema#comment>
                "Object property to relate an input, output or parameter with its unit."@en ;
        <http://www.w3.org/2000/01/rdf-schema#domain>
                <https://w3id.org/ibp/CTRLont#AnnotatedElement> ;
        <http://www.w3.org/2000/01/rdf-schema#isDefinedBy>
                <https://w3id.org/ibp/CTRLont#ctrl> ;
        <http://www.w3.org/2000/01/rdf-schema#label>
                "hasUnit"@en ;
        <http://www.w3.org/2000/01/rdf-schema#range>
                <https://w3id.org/ibp/CTRLont#Unit> ;
        <http://www.w3.org/2003/06/sw-vocab-status/ns#term_status>
                "stable" .

<http://purl.org/dc/terms/contributor>
        a       <http://www.w3.org/2002/07/owl#AnnotationProperty> .

<http://purl.org/dc/terms/issued>
        a       <http://www.w3.org/2002/07/owl#AnnotationProperty> .

<https://w3id.org/ibp/CTRLont#Input>
        a       <http://www.w3.org/2002/07/owl#Class> ;
        <http://www.w3.org/2000/01/rdf-schema#comment>
                "An input allow flows of information to enter a control actor. Inputs are processed by the respective application logic of the control actor to compute the outputs."@en ;
        <http://www.w3.org/2000/01/rdf-schema#isDefinedBy>
                <https://w3id.org/ibp/CTRLont#ctrl> ;
        <http://www.w3.org/2000/01/rdf-schema#label>
                "Input"@en ;
        <http://www.w3.org/2000/01/rdf-schema#subClassOf>
                <https://w3id.org/ibp/CTRLont#AnnotatedElement> ;
        <http://www.w3.org/2002/07/owl#disjointWith>
                <https://w3id.org/ibp/CTRLont#Parameter> ;
        <http://www.w3.org/2003/06/sw-vocab-status/ns#term_status>
                "stable" .

<http://purl.org/vocommons/voaf#Vocabulary>
        a       <http://www.w3.org/2002/07/owl#Class> .

<http://www.w3.org/2000/01/rdf-schema#isDefinedBy>
        a       <http://www.w3.org/2002/07/owl#AnnotationProperty> .

<http://purl.org/dc/terms/publisher>
        a       <http://www.w3.org/2002/07/owl#AnnotationProperty> .

<http://purl.org/dc/terms/description>
        a       <http://www.w3.org/2002/07/owl#AnnotationProperty> .

<https://w3id.org/ibp/CTRLont#SemanticType>
        a       <http://www.w3.org/2002/07/owl#Class> ;
        <http://www.w3.org/2000/01/rdf-schema#comment>
                "It may be required to further annotate an Input, Output or Parameter with a specific Semantic Type. For example in building automation to differ between room air temperature or outdoor air temperature."@en ;
        <http://www.w3.org/2000/01/rdf-schema#isDefinedBy>
                <https://w3id.org/ibp/CTRLont#ctrl> ;
        <http://www.w3.org/2000/01/rdf-schema#label>
                "Semantic Type"@en ;
        <http://www.w3.org/2003/06/sw-vocab-status/ns#term_status>
                "stable" .

<http://purl.org/dc/terms/license>
        a       <http://www.w3.org/2002/07/owl#AnnotationProperty> .

<http://purl.org/dc/terms/creator>
        a       <http://www.w3.org/2002/07/owl#AnnotationProperty> .

<http://purl.org/dc/terms/title>
        a       <http://www.w3.org/2002/07/owl#AnnotationProperty> .

<http://purl.org/dc/terms/modified>
        a       <http://www.w3.org/2002/07/owl#AnnotationProperty> .

<http://www.w3.org/2003/06/sw-vocab-status/ns#term_status>
        a       <http://www.w3.org/2002/07/owl#AnnotationProperty> .

<http://www.w3.org/2000/01/rdf-schema#comment>
        a       <http://www.w3.org/2002/07/owl#AnnotationProperty> .

<http://purl.org/dc/terms/rights>
        a       <http://www.w3.org/2002/07/owl#AnnotationProperty> .

<http://purl.org/dc/terms/identifier>
        a       <http://www.w3.org/2002/07/owl#AnnotationProperty> .

<http://www.w3.org/2000/01/rdf-schema#seeAlso>
        a       <http://www.w3.org/2002/07/owl#AnnotationProperty> .

<http://purl.org/vocab/vann/preferredNamespaceUri>
        a       <http://www.w3.org/2002/07/owl#AnnotationProperty> .

<http://www.w3.org/2000/01/rdf-schema#label>
        a       <http://www.w3.org/2002/07/owl#AnnotationProperty> .

<http://www.w3.org/2002/07/owl#Thing>
        a       <http://www.w3.org/2002/07/owl#Class> .

<http://purl.org/vocab/vann/preferredNamespacePrefix>
        a       <http://www.w3.org/2002/07/owl#AnnotationProperty> .
