<http://www.ontologydesignpatterns.org/ont/dul/DUL.owl#Place>
        <http://www.w3.org/2000/01/rdf-schema#subClassOf>
                <http://www.ontologydesignpatterns.org/ont/d0.owl#Location> .

<http://www.ontologydesignpatterns.org/ont/dul/DUL.owl#Action>
        <http://www.w3.org/2000/01/rdf-schema#subClassOf>
                <http://www.ontologydesignpatterns.org/ont/d0.owl#Activity> .

<http://www.ontologydesignpatterns.org/ont/d0.owl#Event>
        a       <http://www.w3.org/2002/07/owl#Class> ;
        <http://www.w3.org/2000/01/rdf-schema#comment>
                "Any natural event, independently of its possible causes. E.g. avalanche, earthquake, brainwave, bonfire, etc." ;
        <http://www.w3.org/2000/01/rdf-schema#label>
                "natural event"@en , "event"@en ;
        <http://www.w3.org/2000/01/rdf-schema#subClassOf>
                <http://www.w3.org/2002/07/owl#Thing> ;
        <http://www.w3.org/2002/07/owl#equivalentClass>
                [ a       <http://www.w3.org/2002/07/owl#Class> ;
                  <http://www.w3.org/2002/07/owl#unionOf>
                          ( <http://www.ontologydesignpatterns.org/ont/dul/DUL.owl#Event> <http://www.ontologydesignpatterns.org/ont/dul/DUL.owl#EventType> )
                ] .

<http://www.ontologydesignpatterns.org/ont/d0.owl>
        a       <http://www.w3.org/2002/07/owl#Ontology> ;
        <http://www.w3.org/2002/07/owl#imports>
                <http://www.ontologydesignpatterns.org/ont/dul/Supplements.owl> , <http://www.ontologydesignpatterns.org/ont/dul/ontopic.owl> , <http://www.ontologydesignpatterns.org/ont/dul/Conceptualization.owl> , <http://www.ontologydesignpatterns.org/ont/dul/Roles.owl> , <http://www.ontologydesignpatterns.org/ont/dul/CollectionsLite.owl> .

<http://www.ontologydesignpatterns.org/ont/d0.owl#System>
        a       <http://www.w3.org/2002/07/owl#Class> ;
        <http://www.w3.org/2000/01/rdf-schema#comment>
                "Physical, social, political systems.\t viticulture, non-linear system, democracy, water system, etc. E.g. viticulture, non-linear system, democracy, water system, etc." ;
        <http://www.w3.org/2000/01/rdf-schema#label>
                "system"@en ;
        <http://www.w3.org/2000/01/rdf-schema#subClassOf>
                <http://www.w3.org/2002/07/owl#Thing> .

<http://www.ontologydesignpatterns.org/ont/dul/DUL.owl#Event>
        <http://www.w3.org/2000/01/rdf-schema#subClassOf>
                <http://www.ontologydesignpatterns.org/ont/d0.owl#Event> .

<http://www.ontologydesignpatterns.org/ont/d0.owl#CognitiveEntity>
        a       <http://www.w3.org/2002/07/owl#Class> ;
        <http://www.w3.org/2000/01/rdf-schema#comment>
                "Attitudes, cognitive abilities, ideologies, psychological phenomena, mind, etc. E.g. discernment, homophobia, precognition, etc." ;
        <http://www.w3.org/2000/01/rdf-schema#label>
                "cognitive entity"@en ;
        <http://www.w3.org/2000/01/rdf-schema#subClassOf>
                <http://www.w3.org/2002/07/owl#Thing> .

<http://www.ontologydesignpatterns.org/ont/d0.owl#Characteristic>
        a       <http://www.w3.org/2002/07/owl#Class> ;
        <http://www.w3.org/2000/01/rdf-schema#comment>
                "An aspect or quality of a thing. E.g. radial symmetry, poker face, alkalinity, attractiveness, darkness, etc." ;
        <http://www.w3.org/2000/01/rdf-schema#label>
                "characteristic"@en ;
        <http://www.w3.org/2002/07/owl#equivalentClass>
                [ a       <http://www.w3.org/2002/07/owl#Class> ;
                  <http://www.w3.org/2002/07/owl#unionOf>
                          ( <http://www.ontologydesignpatterns.org/ont/dul/DUL.owl#Quality> <http://www.ontologydesignpatterns.org/ont/dul/DUL.owl#Parameter> <http://www.ontologydesignpatterns.org/ont/dul/DUL.owl#Region> )
                ] .

<http://www.ontologydesignpatterns.org/ont/d0.owl#Topic>
        a       <http://www.w3.org/2002/07/owl#Class> ;
        <http://www.w3.org/2000/01/rdf-schema#comment>
                "Any area, discipline, subject of knowledge. E.g. algebra, avionics, ballet, theology, engineering, etc." ;
        <http://www.w3.org/2000/01/rdf-schema#label>
                "topic"@en ;
        <http://www.w3.org/2000/01/rdf-schema#subClassOf>
                <http://www.w3.org/2002/07/owl#Thing> .

<http://www.ontologydesignpatterns.org/ont/d0.owl#Location>
        a       <http://www.w3.org/2002/07/owl#Class> ;
        <http://www.w3.org/2000/01/rdf-schema#comment>
                "A location, in a very generic sense e.g. geo-political entities, or physical object that are inherently located. E.g. Oslo, Australia, Inner Mongolia, resort area, intergalactic space, tundra, tunnel, etc." ;
        <http://www.w3.org/2000/01/rdf-schema#label>
                "location"@en ;
        <http://www.w3.org/2002/07/owl#equivalentClass>
                [ a       <http://www.w3.org/2002/07/owl#Class> ;
                  <http://www.w3.org/2002/07/owl#unionOf>
                          ( <http://www.ontologydesignpatterns.org/ont/dul/DUL.owl#Place> <http://www.ontologydesignpatterns.org/ont/dul/DUL.owl#PhysicalPlace> <http://www.ontologydesignpatterns.org/ont/dul/DUL.owl#SpaceRegion> )
                ] .

<http://www.ontologydesignpatterns.org/ont/d0.owl#Activity>
        a       <http://www.w3.org/2002/07/owl#Class> ;
        <http://www.w3.org/2000/01/rdf-schema#comment>
                "Any action or task planned or executed by an agent intentionally causing and participating in it.\tE.g. swimming, shopping, knowledge sharing, etc." ;
        <http://www.w3.org/2000/01/rdf-schema#label>
                "activity"@en ;
        <http://www.w3.org/2002/07/owl#equivalentClass>
                [ a       <http://www.w3.org/2002/07/owl#Class> ;
                  <http://www.w3.org/2002/07/owl#unionOf>
                          ( <http://www.ontologydesignpatterns.org/ont/dul/DUL.owl#Task> <http://www.ontologydesignpatterns.org/ont/dul/DUL.owl#Action> )
                ] .

<http://www.ontologydesignpatterns.org/ont/dul/DUL.owl#Region>
        <http://www.w3.org/2000/01/rdf-schema#subClassOf>
                <http://www.ontologydesignpatterns.org/ont/d0.owl#Characteristic> .

<http://www.ontologydesignpatterns.org/ont/dul/DUL.owl#Quality>
        <http://www.w3.org/2000/01/rdf-schema#subClassOf>
                <http://www.ontologydesignpatterns.org/ont/d0.owl#Characteristic> .

<http://www.ontologydesignpatterns.org/ont/dul/DUL.owl#Task>
        <http://www.w3.org/2000/01/rdf-schema#subClassOf>
                <http://www.ontologydesignpatterns.org/ont/d0.owl#Activity> .

<http://www.ontologydesignpatterns.org/ont/dul/DUL.owl#EventType>
        <http://www.w3.org/2000/01/rdf-schema#subClassOf>
                <http://www.ontologydesignpatterns.org/ont/d0.owl#Event> .

<http://www.ontologydesignpatterns.org/ont/dul/DUL.owl#SpaceRegion>
        <http://www.w3.org/2000/01/rdf-schema#subClassOf>
                <http://www.ontologydesignpatterns.org/ont/d0.owl#Location> .

<http://www.ontologydesignpatterns.org/ont/dul/DUL.owl#PhysicalPlace>
        <http://www.w3.org/2000/01/rdf-schema#subClassOf>
                <http://www.ontologydesignpatterns.org/ont/d0.owl#Location> .

<http://www.ontologydesignpatterns.org/ont/dul/Conceptualization.owl#InternalRepresentation>
        <http://www.w3.org/2000/01/rdf-schema#subClassOf>
                <http://www.ontologydesignpatterns.org/ont/d0.owl#CognitiveEntity> .

<http://www.ontologydesignpatterns.org/ont/dul/DUL.owl#Parameter>
        <http://www.w3.org/2000/01/rdf-schema#subClassOf>
                <http://www.ontologydesignpatterns.org/ont/d0.owl#Characteristic> .
