<http://www.openlinksw.com/ontology/dbms-app-ontology#dataAccessAPI>
        a       <http://www.w3.org/2002/07/owl#ObjectProperty> ;
        <http://www.w3.org/2000/01/rdf-schema#altLabel>
                "Data Access API" ;
        <http://www.w3.org/2000/01/rdf-schema#comment>
                "Associates a Database Management System (DBMS) with supported Data\r\n\t\t\t\tAccess Programming Interfaces e.g., ODBC, JDBC, ADO.NET, OLE-DB, \r\n\t\t\t\tXMLA, HTTP etc.\r\n\t\t\t " ;
        <http://www.w3.org/2000/01/rdf-schema#domain>
                <http://www.openlinksw.com/ontology/dbms-app-ontology#DatabaseManagementSystem> ;
        <http://www.w3.org/2000/01/rdf-schema#isDefinedBy>
                <http://www.openlinksw.com/ontology/dbms-app-ontology#> ;
        <http://www.w3.org/2000/01/rdf-schema#label>
                "dataAccessAPI" ;
        <http://www.w3.org/2000/01/rdf-schema#range>
                <http://dbpedia.org/class/yago/WikicatComputerLibraries> ;
        <http://www.w3.org/2004/02/skos/core#related>
                <http://data.openlinksw.com/oplweb/glossary-term/OpenDatabaseConnectivity#this> .

<http://www.openlinksw.com/ontology/dbms-app-ontology#benchmarkStandards>
        a       <http://www.w3.org/2002/07/owl#ObjectProperty> ;
        <http://www.w3.org/2000/01/rdf-schema#comment>
                "Associates a Database Management System (DBMS) with supported industry standard\r\n\t\t\t\tbenchmarks e.g., TPC-A, TPC-D, TPC-H, LDBC, LUBM, Berlin SPARQL Benchmark etc..\r\n\t\t\t " ;
        <http://www.w3.org/2000/01/rdf-schema#domain>
                <http://www.openlinksw.com/ontology/dbms-app-ontology#DatabaseManagementSystem> ;
        <http://www.w3.org/2000/01/rdf-schema#isDefinedBy>
                <http://www.openlinksw.com/ontology/dbms-app-ontology#> ;
        <http://www.w3.org/2000/01/rdf-schema#label>
                "benchmarkStandards" ;
        <http://www.w3.org/2000/01/rdf-schema#range>
                <http://dbpedia.org/class/yago/Identifier107270601> ;
        <http://www.w3.org/2004/02/skos/core#altLabel>
                "Industry Standard Performance Benchmarks" ;
        <http://www.w3.org/2004/02/skos/core#related>
                <http://ldbcouncil.org/this> , <http://www.tpc.org/tpca/default.asp#this> , <http://ldbcouncil.org/benchmarks/spb#this> , <https://github.com/hobbit-project/faceted-benchmark#this> , <http://wifo5-03.informatik.uni-mannheim.de/bizer/berlinsparqlbenchmark/this> , <http://www.tpc.org/tpcc/default.asp#this> , <http://www.tpc.org/tpch/default.asp#this> , <http://swat.cse.lehigh.edu/projects/lubm/this> .

<http://www.openlinksw.com/ontology/dbms-app-ontology#relationPartitioning>
        a       <http://www.w3.org/2002/07/owl#ObjectProperty> ;
        <http://www.w3.org/2000/01/rdf-schema#comment>
                "Associates a Database Management System (DBMS) with how it partitions relations\r\n                for unambiguous identification using namespacing. For example: catalog.schema.relation,\r\n\t\t\t\tdatabase.schema.relation, schema.relation, urn:xyz:data, http://example.com/entity/,\r\n\t\t\t\tor http://example.com/entity#this etc.\r\n\t\t\t " ;
        <http://www.w3.org/2000/01/rdf-schema#domain>
                <http://www.openlinksw.com/ontology/dbms-app-ontology#DatabaseManagementSystem> ;
        <http://www.w3.org/2000/01/rdf-schema#isDefinedBy>
                <http://www.openlinksw.com/ontology/dbms-app-ontology#> ;
        <http://www.w3.org/2000/01/rdf-schema#label>
                "relationPartitioning" ;
        <http://www.w3.org/2000/01/rdf-schema#range>
                <http://www.w3.org/2001/XMLSchema#literal> ;
        <http://www.w3.org/2004/02/skos/core#related>
                <http://dbpedia.org/resource/Semantic_triple> , <http://dbpedia.org/resource/Tuple> , <http://data.openlinksw.com/oplweb/glossary-term/Tuple#this> .

<http://www.openlinksw.com/ontology/dbms-app-ontology#declarativeDataManipulationLang>
        a       <http://www.w3.org/2002/07/owl#ObjectProperty> ;
        <http://www.w3.org/2000/01/rdf-schema#comment>
                "Associates a Database Management System (DBMS) with supported declarative \r\n\t\t\t\tData Manipulation Languages.\r\n\t\t\t " ;
        <http://www.w3.org/2000/01/rdf-schema#domain>
                <http://www.openlinksw.com/ontology/dbms-app-ontology#DatabaseManagementSystem> ;
        <http://www.w3.org/2000/01/rdf-schema#isDefinedBy>
                <http://www.openlinksw.com/ontology/dbms-app-ontology#> ;
        <http://www.w3.org/2000/01/rdf-schema#label>
                "declarativeDataManipulationLang" ;
        <http://www.w3.org/2000/01/rdf-schema#range>
                <http://dbpedia.org/class/yago/WikicatQueryLanguages> ;
        <http://www.w3.org/2004/02/skos/core#altLabel>
                "DML" ;
        <http://www.w3.org/2004/02/skos/core#related>
                <http://data.openlinksw.com/oplweb/glossary-term/RDF#this> , <http://data.openlinksw.com/oplweb/glossary-term/SQL#this> , <http://data.openlinksw.com/oplweb/glossary-term/SPARQL#this> , <http://data.openlinksw.com/oplweb/glossary-term/RDFSchema#this> , <http://data.openlinksw.com/oplweb/glossary-term/OWL#this> .

<http://www.openlinksw.com/ontology/dbms-app-ontology#relationsModeledAs>
        a       <http://www.w3.org/2002/07/owl#ObjectProperty> ;
        <http://www.w3.org/2000/01/rdf-schema#comment>
                "Associates a Database Management System (DBMS) with how it models Entity Relationship Types (Relations)" ;
        <http://www.w3.org/2000/01/rdf-schema#domain>
                <http://www.openlinksw.com/ontology/dbms-app-ontology#DatabaseManagementSystem> ;
        <http://www.w3.org/2000/01/rdf-schema#isDefinedBy>
                <http://www.openlinksw.com/ontology/dbms-app-ontology#> ;
        <http://www.w3.org/2000/01/rdf-schema#label>
                "relationsModeledAs" ;
        <http://www.w3.org/2000/01/rdf-schema#range>
                <http://dbpedia.org/class/yago/Sequence108459252> ;
        <http://www.w3.org/2004/02/skos/core#related>
                <http://dbpedia.org/resource/Directed_graph> , <http://data.openlinksw.com/oplweb/glossary-term/RDFRelation#this> , <http://data.openlinksw.com/oplweb/glossary-term/SQLRelation#this> .

<http://www.openlinksw.com/ontology/dbms-app-ontology#identifierQuoteChar>
        a       <http://www.w3.org/2002/07/owl#ObjectProperty> ;
        <http://www.w3.org/2000/01/rdf-schema#comment>
                "Associates a Database Management System (DBMS) with supported Identifier Quotation character \r\n                for system artificat naming/identification (relations/tables, inferred-relations/views, stored procedures)\r\n\t\t\t\te.g., double-quotes, single-quotes, less-than and greater-than characters" ;
        <http://www.w3.org/2000/01/rdf-schema#domain>
                <http://www.openlinksw.com/ontology/dbms-app-ontology#DatabaseManagementSystem> ;
        <http://www.w3.org/2000/01/rdf-schema#isDefinedBy>
                <http://www.openlinksw.com/ontology/dbms-app-ontology#> ;
        <http://www.w3.org/2000/01/rdf-schema#label>
                "identifierQuoteChar" ;
        <http://www.w3.org/2000/01/rdf-schema#range>
                <http://www.w3.org/2001/XMLSchema#literal> ;
        <http://www.w3.org/2004/02/skos/core#related>
                <http://data.openlinksw.com/oplweb/glossary-term/URI#this> , <http://data.openlinksw.com/oplweb/glossary-term/IRI#this> .

<http://www.openlinksw.com/ontology/dbms-app-ontology#declarativeReasoningLang>
        a       <http://www.w3.org/2002/07/owl#ObjectProperty> ;
        <http://www.w3.org/2000/01/rdf-schema#comment>
                "Associates a Database Management System (DBMS) with supported declarative \r\n\t\t\t\tReasoning & Inference Languages.\r\n\t\t\t " ;
        <http://www.w3.org/2000/01/rdf-schema#domain>
                <http://www.openlinksw.com/ontology/dbms-app-ontology#DatabaseManagementSystem> ;
        <http://www.w3.org/2000/01/rdf-schema#isDefinedBy>
                <http://www.openlinksw.com/ontology/dbms-app-ontology#> ;
        <http://www.w3.org/2000/01/rdf-schema#label>
                "declarativeReasoningLang" ;
        <http://www.w3.org/2000/01/rdf-schema#range>
                <http://dbpedia.org/class/yago/WikicatQueryLanguages> , <http://dbpedia.org/class/yago/ArtificialLanguage106894544> ;
        <http://www.w3.org/2004/02/skos/core#related>
                <http://data.openlinksw.com/oplweb/glossary-term/SPINRulesVocab#this> , <http://data.openlinksw.com/oplweb/glossary-term/SPARQL#this> , <http://data.openlinksw.com/oplweb/glossary-term/SQL#this> .

<http://www.openlinksw.com/ontology/dbms-app-ontology#transactionSemantics>
        a       <http://www.w3.org/2002/07/owl#ObjectProperty> ;
        <http://www.w3.org/2000/01/rdf-schema#comment>
                "Associates a Database Management System (DBMS) with supported Transaction Semantics e.g.,\r\n                Atomicity (A), Consistency (C), Isolation (I), and Durability (D).\r\n\t\t\t " ;
        <http://www.w3.org/2000/01/rdf-schema#domain>
                <http://www.openlinksw.com/ontology/dbms-app-ontology#DatabaseManagementSystem> ;
        <http://www.w3.org/2000/01/rdf-schema#isDefinedBy>
                <http://www.openlinksw.com/ontology/dbms-app-ontology#> ;
        <http://www.w3.org/2000/01/rdf-schema#label>
                "transactionSemantics" ;
        <http://www.w3.org/2000/01/rdf-schema#range>
                <http://www.w3.org/2004/02/skos/core#Concept> ;
        <http://www.w3.org/2004/02/skos/core#altLabel>
                "ACID" ;
        <http://www.w3.org/2004/02/skos/core#related>
                <http://dbpedia.org/resource/Transaction_processing> , <http://dbpedia.org/resource/ACID> .

<http://dbpedia.org/class/yago/WikicatComputerLibraries>
        <http://www.w3.org/2000/01/rdf-schema#label>
                "Class: Computer Library" .

<http://www.openlinksw.com/ontology/dbms-app-ontology#DatabaseManagementSystem>
        <http://www.w3.org/2000/01/rdf-schema#comment>
                "A Software Application that provides Structured Data Definition and Manipulation functionality." ;
        <http://www.w3.org/2000/01/rdf-schema#isDefinedBy>
                <http://www.openlinksw.com/ontology/dbms-app-ontology#> ;
        <http://www.w3.org/2000/01/rdf-schema#label>
                "Database Management System" ;
        <http://www.w3.org/2000/01/rdf-schema#subClassOf>
                <http://schema.org/Application> ;
        <http://schema.org/maninEntityOfPage>
                <http://www.openlinksw.com/data/turtle/general/tabulated-data-comparison.ttl> , <http://linkeddata.uriburner.com/describe/?url=https%3A%2F%2Fwww.openlinksw.com%2Fdata%2Fturtle%2Fgeneral%2Ftabulated-data-comparison.ttl%23content&graph=http%3A%2F%2Fwww.openlinksw.com%2Fdata%2Fturtle%2Fgeneral%2Ftabulated-data-comparison.ttl&distinct=1> , <https://docs.google.com/spreadsheets/d/1QHbPEsZqyNb6k0JB5j8vHkuI514c44mkNu-SaO8DekM/edit#gid=1757189899> ;
        <http://www.w3.org/2002/07/owl#equivalentClass>
                <http://dbpedia.org/class/yago/DatabaseManagementSystem106588785> ;
        <http://www.w3.org/2004/02/skos/core#altLabel>
                "DBMS" .

<http://www.openlinksw.com/ontology/dbms-app-ontology#declarativeDataDefinitionLang>
        a       <http://www.w3.org/2002/07/owl#ObjectProperty> ;
        <http://www.w3.org/2000/01/rdf-schema#comment>
                "Associates a Database Management System (DBMS) with supported declarative \r\n\t\t\t\tData Definition Languages.\r\n\t\t\t " ;
        <http://www.w3.org/2000/01/rdf-schema#domain>
                <http://www.openlinksw.com/ontology/dbms-app-ontology#DatabaseManagementSystem> ;
        <http://www.w3.org/2000/01/rdf-schema#isDefinedBy>
                <http://www.openlinksw.com/ontology/dbms-app-ontology#> ;
        <http://www.w3.org/2000/01/rdf-schema#label>
                "declarativeDataDefinitionLang" ;
        <http://www.w3.org/2000/01/rdf-schema#range>
                <http://dbpedia.org/class/yago/WikicatDataModelingLanguages> ;
        <http://www.w3.org/2004/02/skos/core#altLabel>
                "DDL" ;
        <http://www.w3.org/2004/02/skos/core#related>
                <http://data.openlinksw.com/oplweb/glossary-term/OWL#this> , <http://data.openlinksw.com/oplweb/glossary-term/RDF#this> , <http://data.openlinksw.com/oplweb/glossary-term/SQL#this> .

<http://www.openlinksw.com/ontology/dbms#this>
        a       <http://www.w3.org/2002/07/owl#Ontology> .

<http://www.openlinksw.com/ontology/dbms#declarativeDataManipulationLang>
        a       <http://www.w3.org/2002/07/owl#ObjectProperty> .

<http://data.openlinksw.com/oplweb/product/Virtuoso#this>
        a       <http://www.openlinksw.com/ontology/dbms-app-ontology#DatabaseManagementSystem> .

<http://www.openlinksw.com/DAV/data/turtle/dbms-app-ontology.ttl>
        a                              <http://schema.org/CreativeWork> ;
        <http://creativecommons.org/ns#attributionName>
                "OpenLink Software" ;
        <http://creativecommons.org/ns#attributionURL>
                <http://www.openlinksw.com/dataspace/organization/openlink#this> ;
        <http://schema.org/author>     <http://www.openlinksw.com/#this> ;
        <http://schema.org/dateCreated>
                "2019-04-17T13:00:00-05:00"^^<http://www.w3.org/2001/XMLSchema#dateTime> ;
        <http://schema.org/dateModified>
                "2019-04-18T15:00:00-05:00"^^<http://www.w3.org/2001/XMLSchema#dateTime> ;
        <http://schema.org/datePublished>
                "2019-04-18T13:00:00-05:00"^^<http://www.w3.org/2001/XMLSchema#dateTime> ;
        <http://schema.org/description>
                "Document that describes an Ontology of terms associated with \r\n\t\t\t\t\t\t   Database Management Systems (DBMS) genres. Terms in this ontology enable\r\n\t\t\t\t\t\t   structured descriptions of DBMS products.  \r\n\t\t\t\t\t\t " ;
        <http://schema.org/keywords>   "ODBC, ODBC Driver, JDBC, JDBC Driver, ADO.NET, ADO.NET Provider, OLE-DB, OLE-DB Provider, \r\n\t\t\t\t\t\tUDA, Data Access, Data Access Driver, Data Access Middleware, Database, Database Management System, \r\n\t\t\t\t\t\tDBMS, Relational Database Management System, RDBMS, Resource Description Framework, RDF, Relation,\r\n\t\t\t\t\t\tNoSQL, SQL, SPARQL.\r\n\t\t \t\t\t " ;
        <http://schema.org/mainEnity>  <http://www.openlinksw.com/ontology/dbms-app-ontology#> ;
        <http://schema.org/name>       "OpenLink Database Management System Ontology Document " ;
        <http://www.w3.org/1999/xhtml/vocab#license>
                <http://creativecommons.org/licenses/by/4.0/deed.en_US> ;
        <http://www.w3.org/2002/07/owl#sameAs>
                <http://www.openlinksw.com/ontology/dbms-app-ontology#> .

<http://www.openlinksw.com/ontology/dbms-app-ontology#dataAccessControl>
        a       <http://www.w3.org/2002/07/owl#ObjectProperty> ;
        <http://www.w3.org/2000/01/rdf-schema#comment>
                "Associates a Database Management System (DBMS) with supported modalities\r\n\t\t\t\tfor controlling access to data e.g., Role-based Access Control (RBAC) or \r\n\t\t\t\tAttributed-based Access Control (ABAC).\r\n\t\t\t " ;
        <http://www.w3.org/2000/01/rdf-schema#domain>
                <http://www.openlinksw.com/ontology/dbms-app-ontology#DatabaseManagementSystem> ;
        <http://www.w3.org/2000/01/rdf-schema#isDefinedBy>
                <http://www.openlinksw.com/ontology/dbms-app-ontology#> ;
        <http://www.w3.org/2000/01/rdf-schema#label>
                "dataAccessControl" ;
        <http://www.w3.org/2000/01/rdf-schema#range>
                <http://dbpedia.org/class/yago/Identifier107270601> ;
        <http://www.w3.org/2004/02/skos/core#altLabel>
                "Data Security" ;
        <http://www.w3.org/2004/02/skos/core#related>
                <http://data.openlinksw.com/oplweb/glossary-term/ABAC#this> , <http://data.openlinksw.com/oplweb/glossary-term/RBAC#this> .

<http://www.openlinksw.com/ontology/dbms-app-ontology#tupleNotation>
        a       <http://www.w3.org/2002/07/owl#ObjectProperty> ;
        <http://www.w3.org/2000/01/rdf-schema#comment>
                "Associates a Database Management System (DBMS) with the supported notations for\r\n\t\t\t\trepresenting N-Tuples, 3-Tuples etc.\r\n\t\t\t " ;
        <http://www.w3.org/2000/01/rdf-schema#domain>
                <http://www.openlinksw.com/ontology/dbms-app-ontology#DatabaseManagementSystem> ;
        <http://www.w3.org/2000/01/rdf-schema#isDefinedBy>
                <http://www.openlinksw.com/ontology/dbms-app-ontology#> ;
        <http://www.w3.org/2000/01/rdf-schema#label>
                "tupleNotation" ;
        <http://www.w3.org/2000/01/rdf-schema#range>
                <http://dbpedia.org/class/yago/Notation106808493> ;
        <http://www.w3.org/2004/02/skos/core#related>
                <http://data.openlinksw.com/oplweb/glossary-term/CSV#this> , <http://data.openlinksw.com/oplweb/glossary-term/Tuple#this> , <http://data.openlinksw.com/oplweb/glossary-term/Turtle#this> , <http://data.openlinksw.com/oplweb/glossary-term/RDFa#this> , <http://data.openlinksw.com/oplweb/glossary-term/Microdata#this> , <http://data.openlinksw.com/oplweb/glossary-term/NTriples#this> , <http://data.openlinksw.com/oplweb/glossary-term/JSONLD#this> , <http://data.openlinksw.com/oplweb/glossary-term/RDFXML#this> .

<http://www.openlinksw.com/ontology/dbms#transactionSemantics>
        a       <http://www.w3.org/2002/07/owl#ObjectProperty> .

<http://www.openlinksw.com/ontology/dbms-app-ontology#supportsIdentifierType>
        a       <http://www.w3.org/2002/07/owl#ObjectProperty> ;
        <http://www.w3.org/2000/01/rdf-schema#comment>
                "Associates a Database Management System (DBMS) with supported Identifier Types. Examples include\r\n              IRIs, URIs, and other" ;
        <http://www.w3.org/2000/01/rdf-schema#domain>
                <http://www.openlinksw.com/ontology/dbms-app-ontology#DatabaseManagementSystem> ;
        <http://www.w3.org/2000/01/rdf-schema#isDefinedBy>
                <http://www.openlinksw.com/ontology/dbms-app-ontology#> ;
        <http://www.w3.org/2000/01/rdf-schema#label>
                "supportsIdentifierType" ;
        <http://www.w3.org/2000/01/rdf-schema#range>
                <http://dbpedia.org/class/yago/Identifier107270601> ;
        <http://www.w3.org/2004/02/skos/core#related>
                <http://data.openlinksw.com/oplweb/glossary-term/IRI#this> , <http://data.openlinksw.com/oplweb/glossary-term/URI#this> .

<http://www.openlinksw.com/ontology/dbms#identifierQuoteChar>
        a       <http://www.w3.org/2002/07/owl#ObjectProperty> .

<http://www.openlinksw.com/ontology/dbms-app-ontology#>
        a                            <http://www.w3.org/2002/07/owl#Ontology> ;
        <http://www.w3.org/2000/01/rdf-schema#comment>
                "Ontology that defines entity and relation types used to describe \r\n\t\t\t  Database Management Systems software.\r\n\t\t   "@en ;
        <http://www.w3.org/2000/01/rdf-schema#label>
                "OpenLink Database Management Systems Ontology" ;
        <http://purl.org/dc/terms/created>
                "2019-04-17T13:00:00-05:00"^^<http://www.w3.org/2001/XMLSchema#dateTime> ;
        <http://purl.org/dc/terms/modified>
                "2019-04-22T16:21:00-05:00"^^<http://www.w3.org/2001/XMLSchema#dateTime> ;
        <http://purl.org/dc/terms/title>
                "OpenLink Database Management Systems Ontology" ;
        <http://schema.org/creator>  <http://www.openlinksw.com/#this> ;
        <http://www.w3.org/2002/07/owl#versionInfo>
                "1.0.0" ;
        <http://www.w3.org/2007/05/powder-s#describedby>
                <http://www.openlinksw.com/DAV/data/turtle/dbms-app-ontology.ttl> .

<http://www.openlinksw.com/ontology/dbms#supportsIdentifierType>
        a       <http://www.w3.org/2002/07/owl#ObjectProperty> .

<http://www.openlinksw.com/ontology/dbms#declarativeReasoningLang>
        a       <http://www.w3.org/2002/07/owl#ObjectProperty> .

<http://www.openlinksw.com/ontology/dbms#declarativeDataDefinitionLang>
        a       <http://www.w3.org/2002/07/owl#ObjectProperty> .

<http://www.openlinksw.com/ontology/dbms#tupleNotation>
        a       <http://www.w3.org/2002/07/owl#ObjectProperty> .

<http://www.openlinksw.com/ontology/dbms-app-ontology#relationStructure>
        a       <http://www.w3.org/2002/07/owl#ObjectProperty> ;
        <http://www.w3.org/2000/01/rdf-schema#comment>
                "Associates a Database Management System (DBMS) with how it Entity Relationship Types (Relations) \r\n\t\t\t\tare structured e.g., N-Tuples, 3-Tuples etc.\r\n\t\t\t " ;
        <http://www.w3.org/2000/01/rdf-schema#domain>
                <http://www.openlinksw.com/ontology/dbms-app-ontology#DatabaseManagementSystem> ;
        <http://www.w3.org/2000/01/rdf-schema#isDefinedBy>
                <http://www.openlinksw.com/ontology/dbms-app-ontology#> ;
        <http://www.w3.org/2000/01/rdf-schema#label>
                "relationStructure" ;
        <http://www.w3.org/2000/01/rdf-schema#range>
                <http://dbpedia.org/class/yago/DataStructure105728493> ;
        <http://www.w3.org/2004/02/skos/core#related>
                <http://data.openlinksw.com/oplweb/glossary-term/Tuple#this> , <http://dbpedia.org/resource/Semantic_triple> , <http://dbpedia.org/resource/Tuple> .

<http://www.openlinksw.com/ontology/dbms#dataAccessControl>
        a       <http://www.w3.org/2002/07/owl#ObjectProperty> .

<http://dbpedia.org/class/yago/DataStructure105728493>
        <http://www.w3.org/2000/01/rdf-schema#label>
                "Class: Data Structure" .

<http://www.openlinksw.com/ontology/dbms#dataAccessAPI>
        a       <http://www.w3.org/2002/07/owl#ObjectProperty> .

<http://dbpedia.org/class/yago/DatabaseManagementSystem106588785>
        <http://www.w3.org/2000/01/rdf-schema#label>
                "Class: Database Management System" .

<http://www.openlinksw.com/ontology/dbms#benchmarkStandards>
        a       <http://www.w3.org/2002/07/owl#ObjectProperty> .

<http://dbpedia.org/class/yago/WikicatDataModelingLanguages>
        <http://www.w3.org/2000/01/rdf-schema#label>
                "Class: Modeling Language" .

<http://dbpedia.org/class/yago/Identifier107270601>
        <http://www.w3.org/2000/01/rdf-schema#label>
                "Class: Identifier" .

<http://dbpedia.org/class/yago/ArtificialLanguage106894544>
        <http://www.w3.org/2000/01/rdf-schema#label>
                "Class: Artificial Language" .

<http://www.openlinksw.com/ontology/dbms#relationStructure>
        a       <http://www.w3.org/2002/07/owl#ObjectProperty> .

<http://dbpedia.org/class/yago/Sequence108459252>
        <http://www.w3.org/2000/01/rdf-schema#label>
                "Class: Sequence" .

<http://www.openlinksw.com/ontology/dbms#relationPartitioning>
        a       <http://www.w3.org/2002/07/owl#ObjectProperty> .

<http://dbpedia.org/class/yago/WikicatQueryLanguages>
        <http://www.w3.org/2000/01/rdf-schema#label>
                "Class: Query Language" .

<http://www.openlinksw.com/ontology/dbms-app-ontology#this>
        a       <http://www.w3.org/2002/07/owl#Ontology> .

<http://dbpedia.org/class/yago/Notation106808493>
        <http://www.w3.org/2000/01/rdf-schema#label>
                "Class: Notation" .

<http://www.openlinksw.com/ontology/dbms#relationsModeledAs>
        a       <http://www.w3.org/2002/07/owl#ObjectProperty> .
