<http://purl.org/dc/terms/Jurisdiction>
        a       <http://www.w3.org/2002/07/owl#Class> ;
        <http://www.w3.org/2000/01/rdf-schema#comment>
                "The extent or range of judicial, law enforcement, or other authority."@en ;
        <http://www.w3.org/2000/01/rdf-schema#isDefinedBy>
                <http://purl.org/dc/terms/> ;
        <http://www.w3.org/2000/01/rdf-schema#label>
                "Jurisdiction"@en ;
        <http://www.w3.org/2000/01/rdf-schema#subClassOf>
                <http://purl.org/dc/terms/LocationPeriodOrJurisdiction> ;
        <http://purl.org/dc/terms/hasVersion>
                <http://dublincore.org/usage/terms/history/#Jurisdiction-001> ;
        <http://purl.org/dc/terms/issued>
                "2008-01-14"^^<http://www.w3.org/2001/XMLSchema#date> .

<http://purl.org/dc/terms/temporal>
        a       <http://www.w3.org/2002/07/owl#AnnotationProperty> , <http://www.w3.org/2002/07/owl#ObjectProperty> ;
        <http://www.w3.org/2000/01/rdf-schema#comment>
                "Temporal characteristics of the resource."@en ;
        <http://www.w3.org/2000/01/rdf-schema#isDefinedBy>
                <http://purl.org/dc/terms/> ;
        <http://www.w3.org/2000/01/rdf-schema#label>
                "Temporal Coverage"@en ;
        <http://www.w3.org/2000/01/rdf-schema#range>
                <http://purl.org/dc/terms/PeriodOfTime> ;
        <http://www.w3.org/2000/01/rdf-schema#subPropertyOf>
                <http://purl.org/dc/elements/1.1/coverage> , <http://purl.org/dc/terms/coverage> ;
        <http://purl.org/dc/terms/hasVersion>
                <http://dublincore.org/usage/terms/history/#temporal-003> ;
        <http://purl.org/dc/terms/issued>
                "2000-07-11"^^<http://www.w3.org/2001/XMLSchema#date> ;
        <http://purl.org/dc/terms/modified>
                "2008-01-14"^^<http://www.w3.org/2001/XMLSchema#date> .

<http://purl.org/dc/terms/valid>
        a       <http://www.w3.org/2002/07/owl#DatatypeProperty> , <http://www.w3.org/2002/07/owl#AnnotationProperty> ;
        <http://www.w3.org/2000/01/rdf-schema#comment>
                "Date (often a range) of validity of a resource."@en ;
        <http://www.w3.org/2000/01/rdf-schema#isDefinedBy>
                <http://purl.org/dc/terms/> ;
        <http://www.w3.org/2000/01/rdf-schema#label>
                "Date Valid"@en ;
        <http://www.w3.org/2000/01/rdf-schema#range>
                <http://www.w3.org/2000/01/rdf-schema#Literal> ;
        <http://www.w3.org/2000/01/rdf-schema#subPropertyOf>
                <http://purl.org/dc/elements/1.1/date> , <http://purl.org/dc/terms/date> ;
        <http://purl.org/dc/terms/hasVersion>
                <http://dublincore.org/usage/terms/history/#valid-003> ;
        <http://purl.org/dc/terms/issued>
                "2000-07-11"^^<http://www.w3.org/2001/XMLSchema#date> ;
        <http://purl.org/dc/terms/modified>
                "2008-01-14"^^<http://www.w3.org/2001/XMLSchema#date> .

<http://www.demcare.eu/ontologies/demlab.owl#handTrajectory>
        a       <http://www.w3.org/2002/07/owl#ObjectProperty> ;
        <http://www.w3.org/2000/01/rdf-schema#comment>
                "Associates an instance of FunctionalAbilitiesData with a hand trajectory type"@en ;
        <http://www.w3.org/2000/01/rdf-schema#domain>
                <http://www.demcare.eu/ontologies/demlab.owl#FunctionalAbilitiesData> ;
        <http://www.w3.org/2000/01/rdf-schema#range>
                <http://www.demcare.eu/ontologies/demlab.owl#HandTrajectoryType> ;
        <http://www.w3.org/2000/01/rdf-schema#seeAlso>
                <http://www.demcare.eu/ontologies/demlab.owl#FunctionalAbilitiesData> , <http://www.demcare.eu/ontologies/demlab.owl#HandTrajectoryType> .

<http://www.demcare.eu/ontologies/demlab.owl#repetitions>
        a       <http://www.w3.org/2002/07/owl#DatatypeProperty> ;
        <http://www.w3.org/2000/01/rdf-schema#comment>
                "Number of repetitions during semi-directed activities"@en ;
        <http://www.w3.org/2000/01/rdf-schema#domain>
                <http://www.demcare.eu/ontologies/demlab.owl#CognitiveAbilitiesData> ;
        <http://www.w3.org/2000/01/rdf-schema#seeAlso>
                <http://www.demcare.eu/ontologies/demlab.owl#SemiDirectedTask> .

<http://purl.org/dc/terms/FileFormat>
        a       <http://www.w3.org/2002/07/owl#Class> ;
        <http://www.w3.org/2000/01/rdf-schema#comment>
                "A digital resource format."@en ;
        <http://www.w3.org/2000/01/rdf-schema#isDefinedBy>
                <http://purl.org/dc/terms/> ;
        <http://www.w3.org/2000/01/rdf-schema#label>
                "File Format"@en ;
        <http://www.w3.org/2000/01/rdf-schema#subClassOf>
                <http://purl.org/dc/terms/MediaType> ;
        <http://purl.org/dc/terms/description>
                "Examples include the formats defined by the list of Internet Media Types."@en ;
        <http://purl.org/dc/terms/hasVersion>
                <http://dublincore.org/usage/terms/history/#FileFormat-001> ;
        <http://purl.org/dc/terms/issued>
                "2008-01-14"^^<http://www.w3.org/2001/XMLSchema#date> .

<http://purl.org/dc/terms/MethodOfAccrual>
        a       <http://www.w3.org/2002/07/owl#Class> ;
        <http://www.w3.org/2000/01/rdf-schema#comment>
                "A method by which resources are added to a collection."@en ;
        <http://www.w3.org/2000/01/rdf-schema#isDefinedBy>
                <http://purl.org/dc/terms/> ;
        <http://www.w3.org/2000/01/rdf-schema#label>
                "Method of Accrual"@en ;
        <http://purl.org/dc/terms/hasVersion>
                <http://dublincore.org/usage/terms/history/#MethodOfAccrual-001> ;
        <http://purl.org/dc/terms/issued>
                "2008-01-14"^^<http://www.w3.org/2001/XMLSchema#date> .

<http://www.demcare.eu/ontologies/demlab.owl#PrepareHotTeaTask>
        a       <http://www.w3.org/2002/07/owl#Class> ;
        <http://www.w3.org/2000/01/rdf-schema#comment>
                "- The participant has to switch on the electric kettle. \n- The participant has to pour the hot water on the glass containing the tea bag."@en ;
        <http://www.w3.org/2000/01/rdf-schema#subClassOf>
                <http://www.demcare.eu/ontologies/demlab.owl#SemiDirectedTask> .

<http://purl.org/dc/terms/LCC>
        a       <http://www.w3.org/2002/07/owl#NamedIndividual> , <http://purl.org/dc/dcam/VocabularyEncodingScheme> ;
        <http://www.w3.org/2000/01/rdf-schema#comment>
                "The set of conceptual resources specified by the Library of Congress Classification."@en ;
        <http://www.w3.org/2000/01/rdf-schema#isDefinedBy>
                <http://purl.org/dc/terms/> ;
        <http://www.w3.org/2000/01/rdf-schema#label>
                "LCC"@en ;
        <http://www.w3.org/2000/01/rdf-schema#seeAlso>
                <http://lcweb.loc.gov/catdir/cpso/lcco/lcco.html> ;
        <http://purl.org/dc/terms/hasVersion>
                <http://dublincore.org/usage/terms/history/#LCC-003> ;
        <http://purl.org/dc/terms/issued>
                "2000-07-11"^^<http://www.w3.org/2001/XMLSchema#date> ;
        <http://purl.org/dc/terms/modified>
                "2008-01-14"^^<http://www.w3.org/2001/XMLSchema#date> .

<http://purl.org/dc/terms/issued>
        a       <http://www.w3.org/2002/07/owl#AnnotationProperty> , <http://www.w3.org/2002/07/owl#DatatypeProperty> ;
        <http://www.w3.org/2000/01/rdf-schema#comment>
                "Date of formal issuance (e.g., publication) of the resource."@en ;
        <http://www.w3.org/2000/01/rdf-schema#isDefinedBy>
                <http://purl.org/dc/terms/> ;
        <http://www.w3.org/2000/01/rdf-schema#label>
                "Date Issued"@en ;
        <http://www.w3.org/2000/01/rdf-schema#range>
                <http://www.w3.org/2000/01/rdf-schema#Literal> ;
        <http://www.w3.org/2000/01/rdf-schema#subPropertyOf>
                <http://purl.org/dc/terms/date> , <http://purl.org/dc/elements/1.1/date> ;
        <http://purl.org/dc/terms/hasVersion>
                <http://dublincore.org/usage/terms/history/#issued-003> ;
        <http://purl.org/dc/terms/issued>
                "2000-07-11"^^<http://www.w3.org/2001/XMLSchema#date> ;
        <http://purl.org/dc/terms/modified>
                "2008-01-14"^^<http://www.w3.org/2001/XMLSchema#date> .

<http://purl.org/dc/terms/isRequiredBy>
        a       <http://www.w3.org/2002/07/owl#AnnotationProperty> ;
        <http://www.w3.org/2000/01/rdf-schema#comment>
                "A related resource that requires the described resource to support its function, delivery, or coherence."@en ;
        <http://www.w3.org/2000/01/rdf-schema#isDefinedBy>
                <http://purl.org/dc/terms/> ;
        <http://www.w3.org/2000/01/rdf-schema#label>
                "Is Required By"@en ;
        <http://www.w3.org/2000/01/rdf-schema#subPropertyOf>
                <http://purl.org/dc/elements/1.1/relation> , <http://purl.org/dc/terms/relation> ;
        <http://purl.org/dc/terms/hasVersion>
                <http://dublincore.org/usage/terms/history/#isRequiredBy-003> ;
        <http://purl.org/dc/terms/issued>
                "2000-07-11"^^<http://www.w3.org/2001/XMLSchema#date> ;
        <http://purl.org/dc/terms/modified>
                "2008-01-14"^^<http://www.w3.org/2001/XMLSchema#date> ;
        <http://www.w3.org/2004/02/skos/core#note>
                "This term is intended to be used with non-literal values as defined in the DCMI Abstract Model (http://dublincore.org/documents/abstract-model/).  As of December 2007, the DCMI Usage Board is seeking a way to express this intention with a formal range declaration."@en .

<http://www.demcare.eu/ontologies/demlab.owl#stressLevel>
        a       <http://www.w3.org/2002/07/owl#DatatypeProperty> ;
        <http://www.w3.org/2000/01/rdf-schema#domain>
                <http://www.demcare.eu/ontologies/demlab.owl#StressData> ;
        <http://www.w3.org/2000/01/rdf-schema#seeAlso>
                "Stress level"@en ;
        <http://www.w3.org/2000/01/rdf-schema#seeAlso>
                <http://www.demcare.eu/ontologies/demlab.owl#StressData> .

<http://purl.org/dc/terms/hasFormat>
        a       <http://www.w3.org/2002/07/owl#AnnotationProperty> ;
        <http://www.w3.org/2000/01/rdf-schema#comment>
                "A related resource that is substantially the same as the pre-existing described resource, but in another format."@en ;
        <http://www.w3.org/2000/01/rdf-schema#isDefinedBy>
                <http://purl.org/dc/terms/> ;
        <http://www.w3.org/2000/01/rdf-schema#label>
                "Has Format"@en ;
        <http://www.w3.org/2000/01/rdf-schema#subPropertyOf>
                <http://purl.org/dc/terms/relation> , <http://purl.org/dc/elements/1.1/relation> ;
        <http://purl.org/dc/terms/hasVersion>
                <http://dublincore.org/usage/terms/history/#hasFormat-003> ;
        <http://purl.org/dc/terms/issued>
                "2000-07-11"^^<http://www.w3.org/2001/XMLSchema#date> ;
        <http://purl.org/dc/terms/modified>
                "2008-01-14"^^<http://www.w3.org/2001/XMLSchema#date> ;
        <http://www.w3.org/2004/02/skos/core#note>
                "This term is intended to be used with non-literal values as defined in the DCMI Abstract Model (http://dublincore.org/documents/abstract-model/).  As of December 2007, the DCMI Usage Board is seeking a way to express this intention with a formal range declaration."@en .

<http://purl.org/dc/terms/publisher>
        a       <http://www.w3.org/2002/07/owl#ObjectProperty> , <http://www.w3.org/2002/07/owl#AnnotationProperty> ;
        <http://www.w3.org/2000/01/rdf-schema#comment>
                "An entity responsible for making the resource available."@en ;
        <http://www.w3.org/2000/01/rdf-schema#isDefinedBy>
                <http://purl.org/dc/terms/> ;
        <http://www.w3.org/2000/01/rdf-schema#label>
                "Publisher"@en ;
        <http://www.w3.org/2000/01/rdf-schema#range>
                <http://purl.org/dc/terms/Agent> ;
        <http://www.w3.org/2000/01/rdf-schema#subPropertyOf>
                <http://purl.org/dc/elements/1.1/publisher> ;
        <http://purl.org/dc/terms/description>
                "Examples of a Publisher include a person, an organization, or a service."@en ;
        <http://purl.org/dc/terms/hasVersion>
                <http://dublincore.org/usage/terms/history/#publisherT-001> ;
        <http://purl.org/dc/terms/issued>
                "2008-01-14"^^<http://www.w3.org/2001/XMLSchema#date> ;
        <http://purl.org/dc/terms/modified>
                "2010-10-11"^^<http://www.w3.org/2001/XMLSchema#date> .

<http://www.demcare.eu/ontologies/demlab.owl#apathyInventory>
        a       <http://www.w3.org/2002/07/owl#DatatypeProperty> ;
        <http://www.w3.org/2000/01/rdf-schema#comment>
                "Apathy Inventory (AI) and diagnostic criteria for apathy"@en ;
        <http://www.w3.org/2000/01/rdf-schema#domain>
                <http://www.demcare.eu/ontologies/demlab.owl#NeuropsychiatricAndMoodAssessment> ;
        <http://www.w3.org/2000/01/rdf-schema#seeAlso>
                <http://www.demcare.eu/ontologies/demlab.owl#NeuropsychiatricAndMoodAssessment> .

<http://www.demcare.eu/ontologies/demlab.owl#dsm_ivDepressionCriteria>
        a       <http://www.w3.org/2002/07/owl#DatatypeProperty> ;
        <http://www.w3.org/2000/01/rdf-schema#comment>
                "DSM-IV Criteria for depression"@en ;
        <http://www.w3.org/2000/01/rdf-schema#domain>
                <http://www.demcare.eu/ontologies/demlab.owl#NeuropsychiatricAndMoodAssessment> ;
        <http://www.w3.org/2000/01/rdf-schema#seeAlso>
                "http://en.wikipedia.org/wiki/Diagnostic_and_Statistical_Manual_of_Mental_Disorders"@en .

<http://www.demcare.eu/ontologies/demlab.owl#Task>
        a       <http://www.w3.org/2002/07/owl#Class> ;
        <http://www.w3.org/2000/01/rdf-schema#comment>
                "Each Task involves the collection of one or more measurements (MeasuredData instances)."@en , "" ;
        <http://www.w3.org/2000/01/rdf-schema#subClassOf>
                [ a       <http://www.w3.org/2002/07/owl#Restriction> ;
                  <http://www.w3.org/2002/07/owl#onClass>
                          <http://www.w3.org/2006/time#Instant> ;
                  <http://www.w3.org/2002/07/owl#onProperty>
                          <http://www.w3.org/2006/time#hasBeginning> ;
                  <http://www.w3.org/2002/07/owl#qualifiedCardinality>
                          "1"^^<http://www.w3.org/2001/XMLSchema#nonNegativeInteger>
                ] ;
        <http://www.w3.org/2000/01/rdf-schema#subClassOf>
                [ a       <http://www.w3.org/2002/07/owl#Restriction> ;
                  <http://www.w3.org/2002/07/owl#onClass>
                          <http://www.w3.org/2006/time#Instant> ;
                  <http://www.w3.org/2002/07/owl#onProperty>
                          <http://www.w3.org/2006/time#hasEnd> ;
                  <http://www.w3.org/2002/07/owl#qualifiedCardinality>
                          "1"^^<http://www.w3.org/2001/XMLSchema#nonNegativeInteger>
                ] ;
        <http://www.w3.org/2000/01/rdf-schema#subClassOf>
                [ a       <http://www.w3.org/2002/07/owl#Restriction> ;
                  <http://www.w3.org/2002/07/owl#onProperty>
                          <http://www.demcare.eu/ontologies/demlab.owl#measuredData> ;
                  <http://www.w3.org/2002/07/owl#someValuesFrom>
                          <http://www.demcare.eu/ontologies/demlab.owl#MeasuredData>
                ] .

<http://purl.org/dc/terms/isReferencedBy>
        a       <http://www.w3.org/2002/07/owl#AnnotationProperty> ;
        <http://www.w3.org/2000/01/rdf-schema#comment>
                "A related resource that references, cites, or otherwise points to the described resource."@en ;
        <http://www.w3.org/2000/01/rdf-schema#isDefinedBy>
                <http://purl.org/dc/terms/> ;
        <http://www.w3.org/2000/01/rdf-schema#label>
                "Is Referenced By"@en ;
        <http://www.w3.org/2000/01/rdf-schema#subPropertyOf>
                <http://purl.org/dc/terms/relation> , <http://purl.org/dc/elements/1.1/relation> ;
        <http://purl.org/dc/terms/hasVersion>
                <http://dublincore.org/usage/terms/history/#isReferencedBy-003> ;
        <http://purl.org/dc/terms/issued>
                "2000-07-11"^^<http://www.w3.org/2001/XMLSchema#date> ;
        <http://purl.org/dc/terms/modified>
                "2008-01-14"^^<http://www.w3.org/2001/XMLSchema#date> ;
        <http://www.w3.org/2004/02/skos/core#note>
                "This term is intended to be used with non-literal values as defined in the DCMI Abstract Model (http://dublincore.org/documents/abstract-model/).  As of December 2007, the DCMI Usage Board is seeking a way to express this intention with a formal range declaration."@en .

<http://purl.org/dc/terms/Period>
        a       <http://www.w3.org/2000/01/rdf-schema#Datatype> ;
        <http://www.w3.org/2000/01/rdf-schema#comment>
                "The set of time intervals defined by their limits according to the DCMI Period Encoding Scheme."@en ;
        <http://www.w3.org/2000/01/rdf-schema#isDefinedBy>
                <http://purl.org/dc/terms/> ;
        <http://www.w3.org/2000/01/rdf-schema#label>
                "DCMI Period"@en ;
        <http://www.w3.org/2000/01/rdf-schema#seeAlso>
                <http://dublincore.org/documents/dcmi-period/> ;
        <http://purl.org/dc/terms/hasVersion>
                <http://dublincore.org/usage/terms/history/#Period-003> ;
        <http://purl.org/dc/terms/issued>
                "2000-07-11"^^<http://www.w3.org/2001/XMLSchema#date> ;
        <http://purl.org/dc/terms/modified>
                "2008-01-14"^^<http://www.w3.org/2001/XMLSchema#date> .

<http://purl.org/dc/terms/NLM>
        a       <http://purl.org/dc/dcam/VocabularyEncodingScheme> , <http://www.w3.org/2002/07/owl#NamedIndividual> ;
        <http://www.w3.org/2000/01/rdf-schema#comment>
                "The set of conceptual resources specified by the National Library of Medicine Classification."@en ;
        <http://www.w3.org/2000/01/rdf-schema#isDefinedBy>
                <http://purl.org/dc/terms/> ;
        <http://www.w3.org/2000/01/rdf-schema#label>
                "NLM"@en ;
        <http://www.w3.org/2000/01/rdf-schema#seeAlso>
                <http://wwwcf.nlm.nih.gov/class/> ;
        <http://purl.org/dc/terms/hasVersion>
                <http://dublincore.org/usage/terms/history/#NLM-002> ;
        <http://purl.org/dc/terms/issued>
                "2005-06-13"^^<http://www.w3.org/2001/XMLSchema#date> ;
        <http://purl.org/dc/terms/modified>
                "2008-01-14"^^<http://www.w3.org/2001/XMLSchema#date> .

<http://purl.org/dc/terms/references>
        a       <http://www.w3.org/2002/07/owl#AnnotationProperty> ;
        <http://www.w3.org/2000/01/rdf-schema#comment>
                "A related resource that is referenced, cited, or otherwise pointed to by the described resource."@en ;
        <http://www.w3.org/2000/01/rdf-schema#isDefinedBy>
                <http://purl.org/dc/terms/> ;
        <http://www.w3.org/2000/01/rdf-schema#label>
                "References"@en ;
        <http://www.w3.org/2000/01/rdf-schema#subPropertyOf>
                <http://purl.org/dc/elements/1.1/relation> , <http://purl.org/dc/terms/relation> ;
        <http://purl.org/dc/terms/hasVersion>
                <http://dublincore.org/usage/terms/history/#references-003> ;
        <http://purl.org/dc/terms/issued>
                "2000-07-11"^^<http://www.w3.org/2001/XMLSchema#date> ;
        <http://purl.org/dc/terms/modified>
                "2008-01-14"^^<http://www.w3.org/2001/XMLSchema#date> ;
        <http://www.w3.org/2004/02/skos/core#note>
                "This term is intended to be used with non-literal values as defined in the DCMI Abstract Model (http://dublincore.org/documents/abstract-model/).  As of December 2007, the DCMI Usage Board is seeking a way to express this intention with a formal range declaration."@en .

<http://www.demcare.eu/ontologies/demlab.owl#stepLength>
        a       <http://www.w3.org/2002/07/owl#DatatypeProperty> ;
        <http://www.w3.org/2000/01/rdf-schema#comment>
                "Step length"@en ;
        <http://www.w3.org/2000/01/rdf-schema#domain>
                <http://www.demcare.eu/ontologies/demlab.owl#GaitData> ;
        <http://www.w3.org/2000/01/rdf-schema#seeAlso>
                <http://www.demcare.eu/ontologies/demlab.owl#GaitData> .

<http://purl.org/dc/terms/RFC5646>
        a       <http://www.w3.org/2000/01/rdf-schema#Datatype> ;
        <http://www.w3.org/2000/01/rdf-schema#comment>
                "The set of tags constructed according to RFC 5646 for the identification of languages."@en ;
        <http://www.w3.org/2000/01/rdf-schema#isDefinedBy>
                <http://purl.org/dc/terms/> ;
        <http://www.w3.org/2000/01/rdf-schema#label>
                "RFC 5646"@en ;
        <http://www.w3.org/2000/01/rdf-schema#seeAlso>
                <http://www.ietf.org/rfc/rfc5646.txt> ;
        <http://purl.org/dc/terms/description>
                "RFC 5646 obsoletes RFC 4646."@en ;
        <http://purl.org/dc/terms/hasVersion>
                <http://dublincore.org/usage/terms/history/#RFC5646-001> ;
        <http://purl.org/dc/terms/issued>
                "2010-10-11"^^<http://www.w3.org/2001/XMLSchema#date> .

<http://purl.org/dc/terms/BibliographicResource>
        a       <http://www.w3.org/2002/07/owl#Class> ;
        <http://www.w3.org/2000/01/rdf-schema#comment>
                "A book, article, or other documentary resource."@en ;
        <http://www.w3.org/2000/01/rdf-schema#isDefinedBy>
                <http://purl.org/dc/terms/> ;
        <http://www.w3.org/2000/01/rdf-schema#label>
                "Bibliographic Resource"@en ;
        <http://purl.org/dc/terms/hasVersion>
                <http://dublincore.org/usage/terms/history/#BibliographicResource-001> ;
        <http://purl.org/dc/terms/issued>
                "2008-01-14"^^<http://www.w3.org/2001/XMLSchema#date> .

<http://purl.org/dc/terms/MESH>
        a       <http://www.w3.org/2002/07/owl#NamedIndividual> , <http://purl.org/dc/dcam/VocabularyEncodingScheme> ;
        <http://www.w3.org/2000/01/rdf-schema#comment>
                "The set of labeled concepts specified by the Medical Subject Headings."@en ;
        <http://www.w3.org/2000/01/rdf-schema#isDefinedBy>
                <http://purl.org/dc/terms/> ;
        <http://www.w3.org/2000/01/rdf-schema#label>
                "MeSH"@en ;
        <http://www.w3.org/2000/01/rdf-schema#seeAlso>
                <http://www.nlm.nih.gov/mesh/meshhome.html> ;
        <http://purl.org/dc/terms/hasVersion>
                <http://dublincore.org/usage/terms/history/#MESH-003> ;
        <http://purl.org/dc/terms/issued>
                "2000-07-11"^^<http://www.w3.org/2001/XMLSchema#date> ;
        <http://purl.org/dc/terms/modified>
                "2008-01-14"^^<http://www.w3.org/2001/XMLSchema#date> .

<http://purl.org/dc/terms/replaces>
        a       <http://www.w3.org/2002/07/owl#AnnotationProperty> ;
        <http://www.w3.org/2000/01/rdf-schema#comment>
                "A related resource that is supplanted, displaced, or superseded by the described resource."@en ;
        <http://www.w3.org/2000/01/rdf-schema#isDefinedBy>
                <http://purl.org/dc/terms/> ;
        <http://www.w3.org/2000/01/rdf-schema#label>
                "Replaces"@en ;
        <http://www.w3.org/2000/01/rdf-schema#subPropertyOf>
                <http://purl.org/dc/terms/relation> , <http://purl.org/dc/elements/1.1/relation> ;
        <http://purl.org/dc/terms/hasVersion>
                <http://dublincore.org/usage/terms/history/#replaces-003> ;
        <http://purl.org/dc/terms/issued>
                "2000-07-11"^^<http://www.w3.org/2001/XMLSchema#date> ;
        <http://purl.org/dc/terms/modified>
                "2008-01-14"^^<http://www.w3.org/2001/XMLSchema#date> ;
        <http://www.w3.org/2004/02/skos/core#note>
                "This term is intended to be used with non-literal values as defined in the DCMI Abstract Model (http://dublincore.org/documents/abstract-model/).  As of December 2007, the DCMI Usage Board is seeking a way to express this intention with a formal range declaration."@en .

<http://www.demcare.eu/ontologies/demlab.owl#PrepareDrugBoxTask>
        a       <http://www.w3.org/2002/07/owl#Class> ;
        <http://www.w3.org/2000/01/rdf-schema#comment>
                "- 4 types of drugs are proposed to the participant. \n- The participant has to respect the posology prescribed (2 types of drugs at different moment of the day) and the date (day and moment of the day)."@en ;
        <http://www.w3.org/2000/01/rdf-schema#subClassOf>
                <http://www.demcare.eu/ontologies/demlab.owl#SemiDirectedTask> .

<http://www.demcare.eu/ontologies/demlab.owl#DiscussionWithClinicianStep>
        a       <http://www.w3.org/2002/07/owl#Class> ;
        <http://www.w3.org/2000/01/rdf-schema#comment>
                "This ProtocolStep involves two Tasks. The first task (DirectedExpressionTask) is a directed discussion during which the clinician assesses the episodic memory of participant through questions related to events and activities of SemiDirectedActivitiesStep. The second task (PictureDescriptionTask) assesses the verbal fluency and mood of participant using a picture that the participant has to describe (with the picture in the eyes) and then to involve a discussion about their interests for the activity represented. This part is done with two different pictures."@en ;
        <http://www.w3.org/2000/01/rdf-schema#subClassOf>
                <http://www.demcare.eu/ontologies/demlab.owl#ProtocolStep> ;
        <http://www.w3.org/2000/01/rdf-schema#subClassOf>
                [ a       <http://www.w3.org/2002/07/owl#Restriction> ;
                  <http://www.w3.org/2002/07/owl#allValuesFrom>
                          [ a       <http://www.w3.org/2002/07/owl#Class> ;
                            <http://www.w3.org/2002/07/owl#unionOf>
                                    ( <http://www.demcare.eu/ontologies/demlab.owl#DirectedExpressionTask> <http://www.demcare.eu/ontologies/demlab.owl#PictureDescriptionTask> <http://www.demcare.eu/ontologies/demlab.owl#PictureDiscussionTask> )
                          ] ;
                  <http://www.w3.org/2002/07/owl#onProperty>
                          <http://www.demcare.eu/ontologies/demlab.owl#involvesTask>
                ] .

<http://purl.org/dc/terms/ProvenanceStatement>
        a       <http://www.w3.org/2002/07/owl#Class> ;
        <http://www.w3.org/2000/01/rdf-schema#comment>
                "A statement of any changes in ownership and custody of a resource since its creation that are significant for its authenticity, integrity, and interpretation."@en ;
        <http://www.w3.org/2000/01/rdf-schema#isDefinedBy>
                <http://purl.org/dc/terms/> ;
        <http://www.w3.org/2000/01/rdf-schema#label>
                "Provenance Statement"@en ;
        <http://purl.org/dc/terms/hasVersion>
                <http://dublincore.org/usage/terms/history/#ProvenanceStatement-001> ;
        <http://purl.org/dc/terms/issued>
                "2008-01-14"^^<http://www.w3.org/2001/XMLSchema#date> .

<http://www.demcare.eu/ontologies/demlab.owl#CognitiveAbilitiesData>
        a       <http://www.w3.org/2002/07/owl#Class> ;
        <http://www.w3.org/2000/01/rdf-schema#comment>
                "Explore functional abilities for the completion of specific activities"@en ;
        <http://www.w3.org/2000/01/rdf-schema#subClassOf>
                <http://www.demcare.eu/ontologies/demlab.owl#MeasuredData> ;
        <http://www.w3.org/2000/01/rdf-schema#subClassOf>
                [ a       <http://www.w3.org/2002/07/owl#Restriction> ;
                  <http://www.w3.org/2002/07/owl#onClass>
                          <http://www.demcare.eu/ontologies/demlab.owl#ActivityStatusType> ;
                  <http://www.w3.org/2002/07/owl#onProperty>
                          <http://www.demcare.eu/ontologies/demlab.owl#activityStatus> ;
                  <http://www.w3.org/2002/07/owl#qualifiedCardinality>
                          "1"^^<http://www.w3.org/2001/XMLSchema#nonNegativeInteger>
                ] ;
        <http://www.w3.org/2000/01/rdf-schema#subClassOf>
                [ a       <http://www.w3.org/2002/07/owl#Restriction> ;
                  <http://www.w3.org/2002/07/owl#cardinality>
                          "1"^^<http://www.w3.org/2001/XMLSchema#nonNegativeInteger> ;
                  <http://www.w3.org/2002/07/owl#onProperty>
                          <http://www.demcare.eu/ontologies/demlab.owl#repetitions>
                ] ;
        <http://www.w3.org/2000/01/rdf-schema#subClassOf>
                [ a       <http://www.w3.org/2002/07/owl#Restriction> ;
                  <http://www.w3.org/2002/07/owl#onDataRange>
                          <http://www.w3.org/2001/XMLSchema#boolean> ;
                  <http://www.w3.org/2002/07/owl#onProperty>
                          <http://www.demcare.eu/ontologies/demlab.owl#compliantInstructionsOrder> ;
                  <http://www.w3.org/2002/07/owl#qualifiedCardinality>
                          "1"^^<http://www.w3.org/2001/XMLSchema#nonNegativeInteger>
                ] .

<http://purl.org/dc/terms/dateSubmitted>
        a       <http://www.w3.org/2002/07/owl#AnnotationProperty> , <http://www.w3.org/2002/07/owl#DatatypeProperty> ;
        <http://www.w3.org/2000/01/rdf-schema#comment>
                "Date of submission of the resource."@en ;
        <http://www.w3.org/2000/01/rdf-schema#isDefinedBy>
                <http://purl.org/dc/terms/> ;
        <http://www.w3.org/2000/01/rdf-schema#label>
                "Date Submitted"@en ;
        <http://www.w3.org/2000/01/rdf-schema#range>
                <http://www.w3.org/2000/01/rdf-schema#Literal> ;
        <http://www.w3.org/2000/01/rdf-schema#subPropertyOf>
                <http://purl.org/dc/terms/date> , <http://purl.org/dc/elements/1.1/date> ;
        <http://purl.org/dc/terms/description>
                "Examples of resources to which a Date Submitted may be relevant are a thesis (submitted to a university department) or an article (submitted to a journal)."@en ;
        <http://purl.org/dc/terms/hasVersion>
                <http://dublincore.org/usage/terms/history/#dateSubmitted-002> ;
        <http://purl.org/dc/terms/issued>
                "2002-07-13"^^<http://www.w3.org/2001/XMLSchema#date> ;
        <http://purl.org/dc/terms/modified>
                "2008-01-14"^^<http://www.w3.org/2001/XMLSchema#date> .

<http://purl.org/dc/terms/description>
        a       <http://www.w3.org/2002/07/owl#AnnotationProperty> ;
        <http://www.w3.org/2000/01/rdf-schema#comment>
                "An account of the resource."@en ;
        <http://www.w3.org/2000/01/rdf-schema#isDefinedBy>
                <http://purl.org/dc/terms/> ;
        <http://www.w3.org/2000/01/rdf-schema#label>
                "Description"@en ;
        <http://www.w3.org/2000/01/rdf-schema#subPropertyOf>
                <http://purl.org/dc/elements/1.1/description> ;
        <http://purl.org/dc/terms/description>
                "Description may include but is not limited to: an abstract, a table of contents, a graphical representation, or a free-text account of the resource."@en ;
        <http://purl.org/dc/terms/hasVersion>
                <http://dublincore.org/usage/terms/history/#descriptionT-001> ;
        <http://purl.org/dc/terms/issued>
                "2008-01-14"^^<http://www.w3.org/2001/XMLSchema#date> ;
        <http://purl.org/dc/terms/modified>
                "2008-01-14"^^<http://www.w3.org/2001/XMLSchema#date> .

<http://www.demcare.eu/ontologies/demlab.owl#ClinicalAssessment>
        a       <http://www.w3.org/2002/07/owl#Class> ;
        <http://www.w3.org/2000/01/rdf-schema#comment>
                "Root concept for the five types of clinical assessment"@en ;
        <http://www.w3.org/2000/01/rdf-schema#seeAlso>
                <http://www.demcare.eu/ontologies/demlab.owl#CognitiveAbilitiesAssessment> , <http://www.demcare.eu/ontologies/demlab.owl#MotricityAbilitiesAssessment> , <http://www.demcare.eu/ontologies/demlab.owl#NeuropsychiatricAndMoodAssessment> , <http://www.demcare.eu/ontologies/demlab.owl#AutonomyAssessment> , <http://www.demcare.eu/ontologies/demlab.owl#DiagnosisAssessment> .

<http://purl.org/dc/terms/W3CDTF>
        a       <http://www.w3.org/2000/01/rdf-schema#Datatype> ;
        <http://www.w3.org/2000/01/rdf-schema#comment>
                "The set of dates and times constructed according to the W3C Date and Time Formats Specification."@en ;
        <http://www.w3.org/2000/01/rdf-schema#isDefinedBy>
                <http://purl.org/dc/terms/> ;
        <http://www.w3.org/2000/01/rdf-schema#label>
                "W3C-DTF"@en ;
        <http://www.w3.org/2000/01/rdf-schema#seeAlso>
                <http://www.w3.org/TR/NOTE-datetime> ;
        <http://purl.org/dc/terms/hasVersion>
                <http://dublincore.org/usage/terms/history/#W3CDTF-003> ;
        <http://purl.org/dc/terms/issued>
                "2000-07-11"^^<http://www.w3.org/2001/XMLSchema#date> ;
        <http://purl.org/dc/terms/modified>
                "2008-01-14"^^<http://www.w3.org/2001/XMLSchema#date> .

<http://www.demcare.eu/ontologies/demlab.owl#ReadArticleTask>
        a       <http://www.w3.org/2002/07/owl#Class> ;
        <http://www.w3.org/2000/01/rdf-schema#comment>
                "Three articles are proposed to the participant (Topics: Collection Cars; Cooking; Sightseeing). The three articles have the same words number and level of difficulty. Below each articles, the 3 following questions are asked\n- Q1/ What is the topic of the article? \n- Q2/ What is the percentage of French interested in the … (Collection Car / Cooking / Sightseeing, text adapted to the article topic)? \n- Q3/ Who is interviewed?"@en ;
        <http://www.w3.org/2000/01/rdf-schema#subClassOf>
                <http://www.demcare.eu/ontologies/demlab.owl#SemiDirectedTask> .

<http://www.demcare.eu/ontologies/demlab.owl#stoppingDisplacement>
        a       <http://www.w3.org/2002/07/owl#DatatypeProperty> ;
        <http://www.w3.org/2000/01/rdf-schema#comment>
                "Stopping displacement during walking"@en ;
        <http://www.w3.org/2000/01/rdf-schema#domain>
                <http://www.demcare.eu/ontologies/demlab.owl#GaitData> ;
        <http://www.w3.org/2000/01/rdf-schema#seeAlso>
                <http://www.demcare.eu/ontologies/demlab.owl#GaitData> .

<http://purl.org/dc/terms/audience>
        a       <http://www.w3.org/2002/07/owl#ObjectProperty> ;
        <http://www.w3.org/2000/01/rdf-schema#comment>
                "A class of entity for whom the resource is intended or useful."@en ;
        <http://www.w3.org/2000/01/rdf-schema#isDefinedBy>
                <http://purl.org/dc/terms/> ;
        <http://www.w3.org/2000/01/rdf-schema#label>
                "Audience"@en ;
        <http://www.w3.org/2000/01/rdf-schema#range>
                <http://purl.org/dc/terms/AgentClass> ;
        <http://purl.org/dc/terms/hasVersion>
                <http://dublincore.org/usage/terms/history/#audience-003> ;
        <http://purl.org/dc/terms/issued>
                "2001-05-21"^^<http://www.w3.org/2001/XMLSchema#date> ;
        <http://purl.org/dc/terms/modified>
                "2008-01-14"^^<http://www.w3.org/2001/XMLSchema#date> .

<http://purl.org/dc/terms/Standard>
        a       <http://www.w3.org/2002/07/owl#Class> ;
        <http://www.w3.org/2000/01/rdf-schema#comment>
                "A basis for comparison; a reference point against which other things can be evaluated."@en ;
        <http://www.w3.org/2000/01/rdf-schema#isDefinedBy>
                <http://purl.org/dc/terms/> ;
        <http://www.w3.org/2000/01/rdf-schema#label>
                "Standard"@en ;
        <http://purl.org/dc/terms/hasVersion>
                <http://dublincore.org/usage/terms/history/#Standard-001> ;
        <http://purl.org/dc/terms/issued>
                "2008-01-14"^^<http://www.w3.org/2001/XMLSchema#date> .

<http://purl.org/dc/terms/DCMIType>
        a       <http://www.w3.org/2002/07/owl#NamedIndividual> , <http://purl.org/dc/dcam/VocabularyEncodingScheme> ;
        <http://www.w3.org/2000/01/rdf-schema#comment>
                "The set of classes specified by the DCMI Type Vocabulary, used to categorize the nature or genre of the resource."@en ;
        <http://www.w3.org/2000/01/rdf-schema#isDefinedBy>
                <http://purl.org/dc/terms/> ;
        <http://www.w3.org/2000/01/rdf-schema#label>
                "DCMI Type Vocabulary"@en ;
        <http://www.w3.org/2000/01/rdf-schema#seeAlso>
                <http://purl.org/dc/dcmitype/> ;
        <http://purl.org/dc/terms/hasVersion>
                <http://dublincore.org/usage/terms/history/#DCMIType-005> ;
        <http://purl.org/dc/terms/issued>
                "2000-07-11"^^<http://www.w3.org/2001/XMLSchema#date> ;
        <http://purl.org/dc/terms/modified>
                "2012-06-14"^^<http://www.w3.org/2001/XMLSchema#date> .

<http://purl.org/dc/terms/contributor>
        a       <http://www.w3.org/2002/07/owl#ObjectProperty> , <http://www.w3.org/2002/07/owl#AnnotationProperty> ;
        <http://www.w3.org/2000/01/rdf-schema#comment>
                "An entity responsible for making contributions to the resource."@en ;
        <http://www.w3.org/2000/01/rdf-schema#isDefinedBy>
                <http://purl.org/dc/terms/> ;
        <http://www.w3.org/2000/01/rdf-schema#label>
                "Contributor"@en ;
        <http://www.w3.org/2000/01/rdf-schema#range>
                <http://purl.org/dc/terms/Agent> ;
        <http://www.w3.org/2000/01/rdf-schema#subPropertyOf>
                <http://purl.org/dc/elements/1.1/contributor> ;
        <http://purl.org/dc/terms/description>
                "Examples of a Contributor include a person, an organization, or a service."@en ;
        <http://purl.org/dc/terms/hasVersion>
                <http://dublincore.org/usage/terms/history/#contributorT-001> ;
        <http://purl.org/dc/terms/issued>
                "2008-01-14"^^<http://www.w3.org/2001/XMLSchema#date> ;
        <http://purl.org/dc/terms/modified>
                "2010-10-11"^^<http://www.w3.org/2001/XMLSchema#date> .

<http://www.demcare.eu/ontologies/demlab.owl#verbalReactionSpontaneity>
        a       <http://www.w3.org/2002/07/owl#DatatypeProperty> ;
        <http://www.w3.org/2000/01/rdf-schema#comment>
                "Time between the end of assessor’s speech and the beginning of participant’s speech (Discussion Task)"@en ;
        <http://www.w3.org/2000/01/rdf-schema#domain>
                <http://www.demcare.eu/ontologies/demlab.owl#DiscussionInvolvementData> ;
        <http://www.w3.org/2000/01/rdf-schema#seeAlso>
                <http://www.demcare.eu/ontologies/demlab.owl#DiscussionInvolvementData> .

<http://purl.org/dc/terms/LicenseDocument>
        a       <http://www.w3.org/2002/07/owl#Class> ;
        <http://www.w3.org/2000/01/rdf-schema#comment>
                "A legal document giving official permission to do something with a Resource."@en ;
        <http://www.w3.org/2000/01/rdf-schema#isDefinedBy>
                <http://purl.org/dc/terms/> ;
        <http://www.w3.org/2000/01/rdf-schema#label>
                "License Document"@en ;
        <http://www.w3.org/2000/01/rdf-schema#subClassOf>
                <http://purl.org/dc/terms/RightsStatement> ;
        <http://purl.org/dc/terms/hasVersion>
                <http://dublincore.org/usage/terms/history/#LicenseDocument-001> ;
        <http://purl.org/dc/terms/issued>
                "2008-01-14"^^<http://www.w3.org/2001/XMLSchema#date> .

<http://www.demcare.eu/ontologies/demlab.owl#WalkingCountingBackwardsTask>
        a       <http://www.w3.org/2002/07/owl#Class> ;
        <http://www.w3.org/2000/01/rdf-schema#comment>
                "(DualTask) The clinician asks the participant to walk and count aloud backwards simultaneously: \n- From 305 until the end of the walking tasks; or \n- From 20 to 0 for participants who don’t manage to count backwards from 305 to 285 during the CountingBackwardsTask\n\nThis task is used for assessing:\n- Gait: walking speed, step length, etc.\n- Latency: time of latency between the end of instructions (stimulation) and the beginning of the task\n- Stress level\n- Voice: e.g. speech fluency and articulation"@en ;
        <http://www.w3.org/2000/01/rdf-schema#subClassOf>
                <http://www.demcare.eu/ontologies/demlab.owl#DirectedTask> ;
        <http://www.w3.org/2000/01/rdf-schema#subClassOf>
                [ a       <http://www.w3.org/2002/07/owl#Restriction> ;
                  <http://www.w3.org/2002/07/owl#allValuesFrom>
                          [ a       <http://www.w3.org/2002/07/owl#Class> ;
                            <http://www.w3.org/2002/07/owl#unionOf>
                                    ( <http://www.demcare.eu/ontologies/demlab.owl#GaitData> <http://www.demcare.eu/ontologies/demlab.owl#LatencyData> <http://www.demcare.eu/ontologies/demlab.owl#StressData> <http://www.demcare.eu/ontologies/demlab.owl#VoiceData> )
                          ] ;
                  <http://www.w3.org/2002/07/owl#onProperty>
                          <http://www.demcare.eu/ontologies/demlab.owl#measuredData>
                ] .

<http://www.demcare.eu/ontologies/demlab.owl#speechFluency>
        a       <http://www.w3.org/2002/07/owl#DatatypeProperty> ;
        <http://www.w3.org/2000/01/rdf-schema#comment>
                "Speech fluency during sentence repetition and picture description tasks"@en ;
        <http://www.w3.org/2000/01/rdf-schema#domain>
                <http://www.demcare.eu/ontologies/demlab.owl#VoiceData> ;
        <http://www.w3.org/2000/01/rdf-schema#seeAlso>
                <http://www.demcare.eu/ontologies/demlab.owl#VoiceData> .

<http://purl.org/dc/terms/Location>
        a       <http://www.w3.org/2002/07/owl#Class> ;
        <http://www.w3.org/2000/01/rdf-schema#comment>
                "A spatial region or named place."@en ;
        <http://www.w3.org/2000/01/rdf-schema#isDefinedBy>
                <http://purl.org/dc/terms/> ;
        <http://www.w3.org/2000/01/rdf-schema#label>
                "Location"@en ;
        <http://www.w3.org/2000/01/rdf-schema#subClassOf>
                <http://purl.org/dc/terms/LocationPeriodOrJurisdiction> ;
        <http://purl.org/dc/terms/hasVersion>
                <http://dublincore.org/usage/terms/history/#Location-001> ;
        <http://purl.org/dc/terms/issued>
                "2008-01-14"^^<http://www.w3.org/2001/XMLSchema#date> .

<http://purl.org/dc/terms/Box>
        a       <http://www.w3.org/2000/01/rdf-schema#Datatype> ;
        <http://www.w3.org/2000/01/rdf-schema#comment>
                "The set of regions in space defined by their geographic coordinates according to the DCMI Box Encoding Scheme."@en ;
        <http://www.w3.org/2000/01/rdf-schema#isDefinedBy>
                <http://purl.org/dc/terms/> ;
        <http://www.w3.org/2000/01/rdf-schema#label>
                "DCMI Box"@en ;
        <http://www.w3.org/2000/01/rdf-schema#seeAlso>
                <http://dublincore.org/documents/dcmi-box/> ;
        <http://purl.org/dc/terms/hasVersion>
                <http://dublincore.org/usage/terms/history/#Box-003> ;
        <http://purl.org/dc/terms/issued>
                "2000-07-11"^^<http://www.w3.org/2001/XMLSchema#date> ;
        <http://purl.org/dc/terms/modified>
                "2008-01-14"^^<http://www.w3.org/2001/XMLSchema#date> .

<http://purl.org/dc/terms/RFC1766>
        a       <http://www.w3.org/2000/01/rdf-schema#Datatype> ;
        <http://www.w3.org/2000/01/rdf-schema#comment>
                "The set of tags, constructed according to RFC 1766, for the identification of languages."@en ;
        <http://www.w3.org/2000/01/rdf-schema#isDefinedBy>
                <http://purl.org/dc/terms/> ;
        <http://www.w3.org/2000/01/rdf-schema#label>
                "RFC 1766"@en ;
        <http://www.w3.org/2000/01/rdf-schema#seeAlso>
                <http://www.ietf.org/rfc/rfc1766.txt> ;
        <http://purl.org/dc/terms/hasVersion>
                <http://dublincore.org/usage/terms/history/#RFC1766-003> ;
        <http://purl.org/dc/terms/issued>
                "2000-07-11"^^<http://www.w3.org/2001/XMLSchema#date> ;
        <http://purl.org/dc/terms/modified>
                "2008-01-14"^^<http://www.w3.org/2001/XMLSchema#date> .

<http://purl.org/dc/terms/tableOfContents>
        a       <http://www.w3.org/2002/07/owl#AnnotationProperty> ;
        <http://www.w3.org/2000/01/rdf-schema#comment>
                "A list of subunits of the resource."@en ;
        <http://www.w3.org/2000/01/rdf-schema#isDefinedBy>
                <http://purl.org/dc/terms/> ;
        <http://www.w3.org/2000/01/rdf-schema#label>
                "Table Of Contents"@en ;
        <http://www.w3.org/2000/01/rdf-schema#subPropertyOf>
                <http://purl.org/dc/terms/description> , <http://purl.org/dc/elements/1.1/description> ;
        <http://purl.org/dc/terms/hasVersion>
                <http://dublincore.org/usage/terms/history/#tableOfContents-003> ;
        <http://purl.org/dc/terms/issued>
                "2000-07-11"^^<http://www.w3.org/2001/XMLSchema#date> ;
        <http://purl.org/dc/terms/modified>
                "2008-01-14"^^<http://www.w3.org/2001/XMLSchema#date> .

<http://www.demcare.eu/ontologies/demlab.owl#FindBusLineOnMapTask>
        a       <http://www.w3.org/2002/07/owl#Class> ;
        <http://www.w3.org/2000/01/rdf-schema#comment>
                "- A real bus map is showed to the participant with the indication of the current location of the participant. \n- The participant has to write on a sheet of paper located next to the bus map the bus lines to take for the itinerary (From Hospital to Station train). Two itineraries are accepted."@en ;
        <http://www.w3.org/2000/01/rdf-schema#subClassOf>
                <http://www.demcare.eu/ontologies/demlab.owl#SemiDirectedTask> .

<http://purl.org/dc/terms/RFC4646>
        a       <http://www.w3.org/2000/01/rdf-schema#Datatype> ;
        <http://www.w3.org/2000/01/rdf-schema#comment>
                "The set of tags constructed according to RFC 4646 for the identification of languages."@en ;
        <http://www.w3.org/2000/01/rdf-schema#isDefinedBy>
                <http://purl.org/dc/terms/> ;
        <http://www.w3.org/2000/01/rdf-schema#label>
                "RFC 4646"@en ;
        <http://www.w3.org/2000/01/rdf-schema#seeAlso>
                <http://www.ietf.org/rfc/rfc4646.txt> ;
        <http://purl.org/dc/terms/description>
                "RFC 4646 obsoletes RFC 3066."@en ;
        <http://purl.org/dc/terms/hasVersion>
                <http://dublincore.org/usage/terms/history/#RFC4646-001> ;
        <http://purl.org/dc/terms/issued>
                "2008-01-14"^^<http://www.w3.org/2001/XMLSchema#date> .

<http://purl.org/dc/terms/license>
        a       <http://www.w3.org/2002/07/owl#AnnotationProperty> , <http://www.w3.org/2002/07/owl#ObjectProperty> ;
        <http://www.w3.org/2000/01/rdf-schema#comment>
                "A legal document giving official permission to do something with the resource."@en ;
        <http://www.w3.org/2000/01/rdf-schema#isDefinedBy>
                <http://purl.org/dc/terms/> ;
        <http://www.w3.org/2000/01/rdf-schema#label>
                "License"@en ;
        <http://www.w3.org/2000/01/rdf-schema#range>
                <http://purl.org/dc/terms/LicenseDocument> ;
        <http://www.w3.org/2000/01/rdf-schema#subPropertyOf>
                <http://purl.org/dc/terms/rights> , <http://purl.org/dc/elements/1.1/rights> ;
        <http://purl.org/dc/terms/hasVersion>
                <http://dublincore.org/usage/terms/history/#license-002> ;
        <http://purl.org/dc/terms/issued>
                "2004-06-14"^^<http://www.w3.org/2001/XMLSchema#date> ;
        <http://purl.org/dc/terms/modified>
                "2008-01-14"^^<http://www.w3.org/2001/XMLSchema#date> .

<http://www.demcare.eu/ontologies/demlab.owl#DiscussionTask>
        a       <http://www.w3.org/2002/07/owl#Class> ;
        <http://www.w3.org/2000/01/rdf-schema#comment>
                "Root concept for grouping the Tasks relevant to the DiscussionWithClinicianStep\n\nThe relevant tasks are used for assessing:\n- Stress level\n- Voice: e.g. speech rate, pause rate etc."@en ;
        <http://www.w3.org/2000/01/rdf-schema#subClassOf>
                <http://www.demcare.eu/ontologies/demlab.owl#Task> ;
        <http://www.w3.org/2000/01/rdf-schema#subClassOf>
                [ a       <http://www.w3.org/2002/07/owl#Restriction> ;
                  <http://www.w3.org/2002/07/owl#allValuesFrom>
                          [ a       <http://www.w3.org/2002/07/owl#Class> ;
                            <http://www.w3.org/2002/07/owl#unionOf>
                                    ( <http://www.demcare.eu/ontologies/demlab.owl#StressData> <http://www.demcare.eu/ontologies/demlab.owl#VoiceData> )
                          ] ;
                  <http://www.w3.org/2002/07/owl#onProperty>
                          <http://www.demcare.eu/ontologies/demlab.owl#measuredData>
                ] .

<http://www.iti.gr/iti/people/Ioannis_Kompatsiaris.html#ikom>
        a       <http://xmlns.com/foaf/0.1/Person> ;
        <http://xmlns.com/foaf/0.1/homepage>
                <http://www.iti.gr/iti/people/Ioannis_Kompatsiaris.html> ;
        <http://xmlns.com/foaf/0.1/name>
                "Ioannis Kompatsiaris" .

<http://purl.org/dc/terms/type>
        a       <http://www.w3.org/2002/07/owl#AnnotationProperty> , <http://www.w3.org/2002/07/owl#ObjectProperty> ;
        <http://www.w3.org/2000/01/rdf-schema#comment>
                "The nature or genre of the resource."@en ;
        <http://www.w3.org/2000/01/rdf-schema#isDefinedBy>
                <http://purl.org/dc/terms/> ;
        <http://www.w3.org/2000/01/rdf-schema#label>
                "Type"@en ;
        <http://www.w3.org/2000/01/rdf-schema#range>
                <http://www.w3.org/2000/01/rdf-schema#Class> ;
        <http://www.w3.org/2000/01/rdf-schema#subPropertyOf>
                <http://purl.org/dc/elements/1.1/type> ;
        <http://purl.org/dc/terms/description>
                "Recommended best practice is to use a controlled vocabulary such as the DCMI Type Vocabulary [DCMITYPE]. To describe the file format, physical medium, or dimensions of the resource, use the Format element."@en ;
        <http://purl.org/dc/terms/hasVersion>
                <http://dublincore.org/usage/terms/history/#typeT-001> ;
        <http://purl.org/dc/terms/issued>
                "2008-01-14"^^<http://www.w3.org/2001/XMLSchema#date> ;
        <http://purl.org/dc/terms/modified>
                "2008-01-14"^^<http://www.w3.org/2001/XMLSchema#date> .

<http://purl.org/dc/elements/1.1/publisher>
        a       <http://www.w3.org/2002/07/owl#AnnotationProperty> .

<http://purl.org/dc/terms/language>
        a       <http://www.w3.org/2002/07/owl#AnnotationProperty> , <http://www.w3.org/2002/07/owl#ObjectProperty> ;
        <http://www.w3.org/2000/01/rdf-schema#comment>
                "A language of the resource."@en ;
        <http://www.w3.org/2000/01/rdf-schema#isDefinedBy>
                <http://purl.org/dc/terms/> ;
        <http://www.w3.org/2000/01/rdf-schema#label>
                "Language"@en ;
        <http://www.w3.org/2000/01/rdf-schema#range>
                <http://purl.org/dc/terms/LinguisticSystem> ;
        <http://www.w3.org/2000/01/rdf-schema#subPropertyOf>
                <http://purl.org/dc/elements/1.1/language> ;
        <http://purl.org/dc/terms/description>
                "Recommended best practice is to use a controlled vocabulary such as RFC 4646 [RFC4646]."@en ;
        <http://purl.org/dc/terms/hasVersion>
                <http://dublincore.org/usage/terms/history/#languageT-001> ;
        <http://purl.org/dc/terms/issued>
                "2008-01-14"^^<http://www.w3.org/2001/XMLSchema#date> ;
        <http://purl.org/dc/terms/modified>
                "2008-01-14"^^<http://www.w3.org/2001/XMLSchema#date> .

<http://purl.org/dc/terms/IMT>
        a       <http://purl.org/dc/dcam/VocabularyEncodingScheme> , <http://www.w3.org/2002/07/owl#NamedIndividual> ;
        <http://www.w3.org/2000/01/rdf-schema#comment>
                "The set of media types specified by the Internet Assigned Numbers Authority."@en ;
        <http://www.w3.org/2000/01/rdf-schema#isDefinedBy>
                <http://purl.org/dc/terms/> ;
        <http://www.w3.org/2000/01/rdf-schema#label>
                "IMT"@en ;
        <http://www.w3.org/2000/01/rdf-schema#seeAlso>
                <http://www.iana.org/assignments/media-types/> ;
        <http://purl.org/dc/terms/hasVersion>
                <http://dublincore.org/usage/terms/history/#IMT-004> ;
        <http://purl.org/dc/terms/issued>
                "2000-07-11"^^<http://www.w3.org/2001/XMLSchema#date> ;
        <http://purl.org/dc/terms/modified>
                "2008-01-14"^^<http://www.w3.org/2001/XMLSchema#date> .

<http://purl.org/dc/terms/Point>
        a       <http://www.w3.org/2000/01/rdf-schema#Datatype> ;
        <http://www.w3.org/2000/01/rdf-schema#comment>
                "The set of points in space defined by their geographic coordinates according to the DCMI Point Encoding Scheme."@en ;
        <http://www.w3.org/2000/01/rdf-schema#isDefinedBy>
                <http://purl.org/dc/terms/> ;
        <http://www.w3.org/2000/01/rdf-schema#label>
                "DCMI Point"@en ;
        <http://www.w3.org/2000/01/rdf-schema#seeAlso>
                <http://dublincore.org/documents/dcmi-point/> ;
        <http://purl.org/dc/terms/hasVersion>
                <http://dublincore.org/usage/terms/history/#Point-003> ;
        <http://purl.org/dc/terms/issued>
                "2000-07-11"^^<http://www.w3.org/2001/XMLSchema#date> ;
        <http://purl.org/dc/terms/modified>
                "2008-01-14"^^<http://www.w3.org/2001/XMLSchema#date> .

<http://www.demcare.eu/ontologies/demlab.owl#PersonWithDementia>
        a       <http://www.w3.org/2002/07/owl#Class> ;
        <http://www.w3.org/2000/01/rdf-schema#comment>
                "A Person with Dementia is defined as the participant whose clinical record contains a dementia clinical diagnosis"@en ;
        <http://www.w3.org/2000/01/rdf-schema#seeAlso>
                <http://www.demcare.eu/ontologies/demlab.owl#DiagnosisAssessment> , <http://www.demcare.eu/ontologies/demlab.owl#DiagnosisType> , <http://www.demcare.eu/ontologies/demlab.owl#ClinicalRecord> , <http://www.demcare.eu/ontologies/demlab.owl#dementia> ;
        <http://www.w3.org/2000/01/rdf-schema#subClassOf>
                <http://www.demcare.eu/ontologies/demlab.owl#Participant> ;
        <http://www.w3.org/2002/07/owl#equivalentClass>
                [ a       <http://www.w3.org/2002/07/owl#Restriction> ;
                  <http://www.w3.org/2002/07/owl#onProperty>
                          <http://www.demcare.eu/ontologies/demlab.owl#hasClinicalRecord> ;
                  <http://www.w3.org/2002/07/owl#someValuesFrom>
                          [ a       <http://www.w3.org/2002/07/owl#Class> ;
                            <http://www.w3.org/2002/07/owl#intersectionOf>
                                    ( <http://www.demcare.eu/ontologies/demlab.owl#ClinicalRecord>
                                      [ a       <http://www.w3.org/2002/07/owl#Restriction> ;
                                        <http://www.w3.org/2002/07/owl#onProperty>
                                                <http://www.demcare.eu/ontologies/demlab.owl#containsAssessment> ;
                                        <http://www.w3.org/2002/07/owl#someValuesFrom>
                                                [ a       <http://www.w3.org/2002/07/owl#Class> ;
                                                  <http://www.w3.org/2002/07/owl#intersectionOf>
                                                          ( <http://www.demcare.eu/ontologies/demlab.owl#DiagnosisAssessment>
                                                            [ a       <http://www.w3.org/2002/07/owl#Restriction> ;
                                                              <http://www.w3.org/2002/07/owl#onProperty>
                                                                      <http://www.demcare.eu/ontologies/demlab.owl#hasClinicalDiagnosis> ;
                                                              <http://www.w3.org/2002/07/owl#someValuesFrom>
                                                                      [ a       <http://www.w3.org/2002/07/owl#Class> ;
                                                                        <http://www.w3.org/2002/07/owl#oneOf>
                                                                                ( <http://www.demcare.eu/ontologies/demlab.owl#dementia> )
                                                                      ]
                                                            ]
                                                          )
                                                ]
                                      ]
                                    )
                          ]
                ] .

<http://purl.org/dc/terms/PhysicalMedium>
        a       <http://www.w3.org/2002/07/owl#Class> ;
        <http://www.w3.org/2000/01/rdf-schema#comment>
                "A physical material or carrier."@en ;
        <http://www.w3.org/2000/01/rdf-schema#isDefinedBy>
                <http://purl.org/dc/terms/> ;
        <http://www.w3.org/2000/01/rdf-schema#label>
                "Physical Medium"@en ;
        <http://www.w3.org/2000/01/rdf-schema#subClassOf>
                <http://purl.org/dc/terms/MediaType> ;
        <http://purl.org/dc/terms/description>
                "Examples include paper, canvas, or DVD."@en ;
        <http://purl.org/dc/terms/hasVersion>
                <http://dublincore.org/usage/terms/history/#PhysicalMedium-001> ;
        <http://purl.org/dc/terms/issued>
                "2008-01-14"^^<http://www.w3.org/2001/XMLSchema#date> .

<http://www.demcare.eu/ontologies/demlab.owl#OrganisationEfficiencyData>
        a       <http://www.w3.org/2002/07/owl#Class> ;
        <http://www.w3.org/2000/01/rdf-schema#comment>
                "Explore ability to organize with efficiency the different activities"@en ;
        <http://www.w3.org/2000/01/rdf-schema#subClassOf>
                <http://www.demcare.eu/ontologies/demlab.owl#MeasuredData> ;
        <http://www.w3.org/2000/01/rdf-schema#subClassOf>
                [ a       <http://www.w3.org/2002/07/owl#Restriction> ;
                  <http://www.w3.org/2002/07/owl#onProperty>
                          <http://www.demcare.eu/ontologies/demlab.owl#areasOfInterestExplored> ;
                  <http://www.w3.org/2002/07/owl#someValuesFrom>
                          <http://www.demcare.eu/ontologies/demlab.owl#Zone>
                ] ;
        <http://www.w3.org/2000/01/rdf-schema#subClassOf>
                [ a       <http://www.w3.org/2002/07/owl#Restriction> ;
                  <http://www.w3.org/2002/07/owl#onProperty>
                          <http://www.demcare.eu/ontologies/demlab.owl#areasOfNoInterestExplored> ;
                  <http://www.w3.org/2002/07/owl#someValuesFrom>
                          <http://www.demcare.eu/ontologies/demlab.owl#Zone>
                ] ;
        <http://www.w3.org/2000/01/rdf-schema#subClassOf>
                [ a       <http://www.w3.org/2002/07/owl#Restriction> ;
                  <http://www.w3.org/2002/07/owl#cardinality>
                          "1"^^<http://www.w3.org/2001/XMLSchema#nonNegativeInteger> ;
                  <http://www.w3.org/2002/07/owl#onProperty>
                          <http://www.demcare.eu/ontologies/demlab.owl#distanceWalked>
                ] .

<http://www.demcare.eu/ontologies/demlab.owl#HealthyControlParticipant>
        a       <http://www.w3.org/2002/07/owl#Class> ;
        <http://www.w3.org/2000/01/rdf-schema#comment>
                "A Healthy Control Participant is defined as the participant whose clinical record contains a healthy clinical diagnosis"@en ;
        <http://www.w3.org/2000/01/rdf-schema#seeAlso>
                <http://www.demcare.eu/ontologies/demlab.owl#DiagnosisType> , <http://www.demcare.eu/ontologies/demlab.owl#DiagnosisAssessment> , <http://www.demcare.eu/ontologies/demlab.owl#healthy> , <http://www.demcare.eu/ontologies/demlab.owl#ClinicalRecord> ;
        <http://www.w3.org/2000/01/rdf-schema#subClassOf>
                <http://www.demcare.eu/ontologies/demlab.owl#Participant> ;
        <http://www.w3.org/2002/07/owl#equivalentClass>
                [ a       <http://www.w3.org/2002/07/owl#Restriction> ;
                  <http://www.w3.org/2002/07/owl#onProperty>
                          <http://www.demcare.eu/ontologies/demlab.owl#hasClinicalRecord> ;
                  <http://www.w3.org/2002/07/owl#someValuesFrom>
                          [ a       <http://www.w3.org/2002/07/owl#Class> ;
                            <http://www.w3.org/2002/07/owl#intersectionOf>
                                    ( <http://www.demcare.eu/ontologies/demlab.owl#ClinicalRecord>
                                      [ a       <http://www.w3.org/2002/07/owl#Restriction> ;
                                        <http://www.w3.org/2002/07/owl#onProperty>
                                                <http://www.demcare.eu/ontologies/demlab.owl#containsAssessment> ;
                                        <http://www.w3.org/2002/07/owl#someValuesFrom>
                                                [ a       <http://www.w3.org/2002/07/owl#Class> ;
                                                  <http://www.w3.org/2002/07/owl#intersectionOf>
                                                          ( <http://www.demcare.eu/ontologies/demlab.owl#DiagnosisAssessment>
                                                            [ a       <http://www.w3.org/2002/07/owl#Restriction> ;
                                                              <http://www.w3.org/2002/07/owl#onProperty>
                                                                      <http://www.demcare.eu/ontologies/demlab.owl#hasClinicalDiagnosis> ;
                                                              <http://www.w3.org/2002/07/owl#someValuesFrom>
                                                                      [ a       <http://www.w3.org/2002/07/owl#Class> ;
                                                                        <http://www.w3.org/2002/07/owl#oneOf>
                                                                                ( <http://www.demcare.eu/ontologies/demlab.owl#healthy> )
                                                                      ]
                                                            ]
                                                          )
                                                ]
                                      ]
                                    )
                          ]
                ] .

<http://purl.org/dc/terms/conformsTo>
        a       <http://www.w3.org/2002/07/owl#AnnotationProperty> , <http://www.w3.org/2002/07/owl#ObjectProperty> ;
        <http://www.w3.org/2000/01/rdf-schema#comment>
                "An established standard to which the described resource conforms."@en ;
        <http://www.w3.org/2000/01/rdf-schema#isDefinedBy>
                <http://purl.org/dc/terms/> ;
        <http://www.w3.org/2000/01/rdf-schema#label>
                "Conforms To"@en ;
        <http://www.w3.org/2000/01/rdf-schema#range>
                <http://purl.org/dc/terms/Standard> ;
        <http://www.w3.org/2000/01/rdf-schema#subPropertyOf>
                <http://purl.org/dc/elements/1.1/relation> , <http://purl.org/dc/terms/relation> ;
        <http://purl.org/dc/terms/hasVersion>
                <http://dublincore.org/usage/terms/history/#conformsTo-003> ;
        <http://purl.org/dc/terms/issued>
                "2001-05-21"^^<http://www.w3.org/2001/XMLSchema#date> ;
        <http://purl.org/dc/terms/modified>
                "2008-01-14"^^<http://www.w3.org/2001/XMLSchema#date> .

<http://purl.org/dc/elements/1.1/identifier>
        a       <http://www.w3.org/2002/07/owl#AnnotationProperty> .

<http://www.demcare.eu/ontologies/demlab.owl#hasUPDRSScore>
        a       <http://www.w3.org/2002/07/owl#DatatypeProperty> ;
        <http://www.w3.org/2000/01/rdf-schema#comment>
                "Part III of the Unified Parkinson’s Disease Rating Scale"@en ;
        <http://www.w3.org/2000/01/rdf-schema#domain>
                <http://www.demcare.eu/ontologies/demlab.owl#MotricityAbilitiesAssessment> ;
        <http://www.w3.org/2000/01/rdf-schema#seeAlso>
                <http://www.demcare.eu/ontologies/demlab.owl#MotricityAbilitiesAssessment> .

<http://purl.org/dc/terms/created>
        a       <http://www.w3.org/2002/07/owl#AnnotationProperty> , <http://www.w3.org/2002/07/owl#DatatypeProperty> ;
        <http://www.w3.org/2000/01/rdf-schema#comment>
                "Date of creation of the resource."@en ;
        <http://www.w3.org/2000/01/rdf-schema#isDefinedBy>
                <http://purl.org/dc/terms/> ;
        <http://www.w3.org/2000/01/rdf-schema#label>
                "Date Created"@en ;
        <http://www.w3.org/2000/01/rdf-schema#range>
                <http://www.w3.org/2000/01/rdf-schema#Literal> ;
        <http://www.w3.org/2000/01/rdf-schema#subPropertyOf>
                <http://purl.org/dc/terms/date> , <http://purl.org/dc/elements/1.1/date> ;
        <http://purl.org/dc/terms/hasVersion>
                <http://dublincore.org/usage/terms/history/#created-003> ;
        <http://purl.org/dc/terms/issued>
                "2000-07-11"^^<http://www.w3.org/2001/XMLSchema#date> ;
        <http://purl.org/dc/terms/modified>
                "2008-01-14"^^<http://www.w3.org/2001/XMLSchema#date> .

<http://www.demcare.eu/ontologies/demlab.owl#WalkingTask>
        a       <http://www.w3.org/2002/07/owl#Class> ;
        <http://www.w3.org/2000/01/rdf-schema#comment>
                "(MonoTask) The clinician asks the participant to walk 4 meters across the room, to turn and then to come back (total walking distance: 8m).\n\nThis task is used for assessing:\n- Gait: walking speed, step length, etc.\n- Latency: time of latency between the end of instructions (stimulation) and the beginning of the task\n- Stress level"@en ;
        <http://www.w3.org/2000/01/rdf-schema#subClassOf>
                <http://www.demcare.eu/ontologies/demlab.owl#DirectedTask> ;
        <http://www.w3.org/2000/01/rdf-schema#subClassOf>
                [ a       <http://www.w3.org/2002/07/owl#Restriction> ;
                  <http://www.w3.org/2002/07/owl#onProperty>
                          <http://www.demcare.eu/ontologies/demlab.owl#measuredData> ;
                  <http://www.w3.org/2002/07/owl#someValuesFrom>
                          <http://www.demcare.eu/ontologies/demlab.owl#GaitData>
                ] ;
        <http://www.w3.org/2000/01/rdf-schema#subClassOf>
                [ a       <http://www.w3.org/2002/07/owl#Restriction> ;
                  <http://www.w3.org/2002/07/owl#allValuesFrom>
                          [ a       <http://www.w3.org/2002/07/owl#Class> ;
                            <http://www.w3.org/2002/07/owl#unionOf>
                                    ( <http://www.demcare.eu/ontologies/demlab.owl#GaitData> <http://www.demcare.eu/ontologies/demlab.owl#LatencyData> <http://www.demcare.eu/ontologies/demlab.owl#StressData> )
                          ] ;
                  <http://www.w3.org/2002/07/owl#onProperty>
                          <http://www.demcare.eu/ontologies/demlab.owl#measuredData>
                ] ;
        <http://www.w3.org/2000/01/rdf-schema#subClassOf>
                [ a       <http://www.w3.org/2002/07/owl#Restriction> ;
                  <http://www.w3.org/2002/07/owl#onProperty>
                          <http://www.demcare.eu/ontologies/demlab.owl#measuredData> ;
                  <http://www.w3.org/2002/07/owl#someValuesFrom>
                          <http://www.demcare.eu/ontologies/demlab.owl#LatencyData>
                ] .

<http://purl.org/dc/terms/instructionalMethod>
        a       <http://www.w3.org/2002/07/owl#ObjectProperty> ;
        <http://www.w3.org/2000/01/rdf-schema#comment>
                "A process, used to engender knowledge, attitudes and skills, that the described resource is designed to support."@en ;
        <http://www.w3.org/2000/01/rdf-schema#isDefinedBy>
                <http://purl.org/dc/terms/> ;
        <http://www.w3.org/2000/01/rdf-schema#label>
                "Instructional Method"@en ;
        <http://www.w3.org/2000/01/rdf-schema#range>
                <http://purl.org/dc/terms/MethodOfInstruction> ;
        <http://purl.org/dc/terms/description>
                "Instructional Method will typically include ways of presenting instructional materials or conducting instructional activities, patterns of learner-to-learner and learner-to-instructor interactions, and mechanisms by which group and individual levels of learning are measured.  Instructional methods include all aspects of the instruction and learning processes from planning and implementation through evaluation and feedback."@en ;
        <http://purl.org/dc/terms/hasVersion>
                <http://dublincore.org/usage/terms/history/#instructionalMethod-002> ;
        <http://purl.org/dc/terms/issued>
                "2005-06-13"^^<http://www.w3.org/2001/XMLSchema#date> ;
        <http://purl.org/dc/terms/modified>
                "2008-01-14"^^<http://www.w3.org/2001/XMLSchema#date> .

<http://purl.org/dc/terms/ISO639-2>
        a       <http://www.w3.org/2000/01/rdf-schema#Datatype> ;
        <http://www.w3.org/2000/01/rdf-schema#comment>
                "The three-letter alphabetic codes listed in ISO639-2 for the representation of names of languages."@en ;
        <http://www.w3.org/2000/01/rdf-schema#isDefinedBy>
                <http://purl.org/dc/terms/> ;
        <http://www.w3.org/2000/01/rdf-schema#label>
                "ISO 639-2"@en ;
        <http://www.w3.org/2000/01/rdf-schema#seeAlso>
                <http://lcweb.loc.gov/standards/iso639-2/langhome.html> ;
        <http://purl.org/dc/terms/hasVersion>
                <http://dublincore.org/usage/terms/history/#ISO639-2-003> ;
        <http://purl.org/dc/terms/issued>
                "2000-07-11"^^<http://www.w3.org/2001/XMLSchema#date> ;
        <http://purl.org/dc/terms/modified>
                "2008-01-14"^^<http://www.w3.org/2001/XMLSchema#date> .

<http://www.demcare.eu/ontologies/demlab.owl#containsAssessment>
        a       <http://www.w3.org/2002/07/owl#ObjectProperty> ;
        <http://www.w3.org/2000/01/rdf-schema#comment>
                "A ClinicalRecord contains a ClinicalAssessment" ;
        <http://www.w3.org/2000/01/rdf-schema#domain>
                <http://www.demcare.eu/ontologies/demlab.owl#ClinicalRecord> ;
        <http://www.w3.org/2000/01/rdf-schema#range>
                <http://www.demcare.eu/ontologies/demlab.owl#ClinicalAssessment> ;
        <http://www.w3.org/2000/01/rdf-schema#seeAlso>
                <http://www.demcare.eu/ontologies/demlab.owl#ClinicalAssessment> , <http://www.demcare.eu/ontologies/demlab.owl#ClinicalRecord> .

<http://www.demcare.eu/ontologies/demlab.owl#StressData>
        a       <http://www.w3.org/2002/07/owl#Class> ;
        <http://www.w3.org/2000/01/rdf-schema#comment>
                "Explore stress level"@en ;
        <http://www.w3.org/2000/01/rdf-schema#subClassOf>
                <http://www.demcare.eu/ontologies/demlab.owl#MeasuredData> ;
        <http://www.w3.org/2000/01/rdf-schema#subClassOf>
                [ a       <http://www.w3.org/2002/07/owl#Restriction> ;
                  <http://www.w3.org/2002/07/owl#cardinality>
                          "1"^^<http://www.w3.org/2001/XMLSchema#nonNegativeInteger> ;
                  <http://www.w3.org/2002/07/owl#onProperty>
                          <http://www.demcare.eu/ontologies/demlab.owl#stressLevel>
                ] .

<http://www.demcare.eu/ontologies/demlab.owl#articulation>
        a       <http://www.w3.org/2002/07/owl#DatatypeProperty> ;
        <http://www.w3.org/2000/01/rdf-schema#comment>
                "Measures the articulation control of the participant"@en ;
        <http://www.w3.org/2000/01/rdf-schema#domain>
                <http://www.demcare.eu/ontologies/demlab.owl#VoiceData> .

<http://www.demcare.eu/ontologies/demlab.owl#compliantInstructionsOrder>
        a       <http://www.w3.org/2002/07/owl#DatatypeProperty> ;
        <http://www.w3.org/2000/01/rdf-schema#comment>
                "Whether the participant followed the activity order suggested by the instructions sheet"@en ;
        <http://www.w3.org/2000/01/rdf-schema#domain>
                <http://www.demcare.eu/ontologies/demlab.owl#CognitiveAbilitiesData> ;
        <http://www.w3.org/2000/01/rdf-schema#seeAlso>
                <http://www.demcare.eu/ontologies/demlab.owl#CognitiveAbilitiesData> .

<http://purl.org/dc/terms/bibliographicCitation>
        a       <http://www.w3.org/2002/07/owl#AnnotationProperty> , <http://www.w3.org/2002/07/owl#DatatypeProperty> ;
        <http://www.w3.org/2000/01/rdf-schema#comment>
                "A bibliographic reference for the resource."@en ;
        <http://www.w3.org/2000/01/rdf-schema#domain>
                <http://purl.org/dc/terms/BibliographicResource> ;
        <http://www.w3.org/2000/01/rdf-schema#isDefinedBy>
                <http://purl.org/dc/terms/> ;
        <http://www.w3.org/2000/01/rdf-schema#label>
                "Bibliographic Citation"@en ;
        <http://www.w3.org/2000/01/rdf-schema#range>
                <http://www.w3.org/2000/01/rdf-schema#Literal> ;
        <http://www.w3.org/2000/01/rdf-schema#subPropertyOf>
                <http://purl.org/dc/elements/1.1/identifier> , <http://purl.org/dc/terms/identifier> ;
        <http://purl.org/dc/terms/description>
                "Recommended practice is to include sufficient bibliographic detail to identify the resource as unambiguously as possible."@en ;
        <http://purl.org/dc/terms/hasVersion>
                <http://dublincore.org/usage/terms/history/#bibliographicCitation-002> ;
        <http://purl.org/dc/terms/issued>
                "2003-02-15"^^<http://www.w3.org/2001/XMLSchema#date> ;
        <http://purl.org/dc/terms/modified>
                "2008-01-14"^^<http://www.w3.org/2001/XMLSchema#date> .

<http://purl.org/dc/terms/hasPart>
        a       <http://www.w3.org/2002/07/owl#AnnotationProperty> ;
        <http://www.w3.org/2000/01/rdf-schema#comment>
                "A related resource that is included either physically or logically in the described resource."@en ;
        <http://www.w3.org/2000/01/rdf-schema#isDefinedBy>
                <http://purl.org/dc/terms/> ;
        <http://www.w3.org/2000/01/rdf-schema#label>
                "Has Part"@en ;
        <http://www.w3.org/2000/01/rdf-schema#subPropertyOf>
                <http://purl.org/dc/elements/1.1/relation> , <http://purl.org/dc/terms/relation> ;
        <http://purl.org/dc/terms/hasVersion>
                <http://dublincore.org/usage/terms/history/#hasPart-003> ;
        <http://purl.org/dc/terms/issued>
                "2000-07-11"^^<http://www.w3.org/2001/XMLSchema#date> ;
        <http://purl.org/dc/terms/modified>
                "2008-01-14"^^<http://www.w3.org/2001/XMLSchema#date> ;
        <http://www.w3.org/2004/02/skos/core#note>
                "This term is intended to be used with non-literal values as defined in the DCMI Abstract Model (http://dublincore.org/documents/abstract-model/).  As of December 2007, the DCMI Usage Board is seeking a way to express this intention with a formal range declaration."@en .

<http://purl.org/dc/terms/creator>
        a       <http://www.w3.org/2002/07/owl#AnnotationProperty> , <http://www.w3.org/2002/07/owl#ObjectProperty> ;
        <http://www.w3.org/2000/01/rdf-schema#comment>
                "An entity primarily responsible for making the resource."@en ;
        <http://www.w3.org/2000/01/rdf-schema#isDefinedBy>
                <http://purl.org/dc/terms/> ;
        <http://www.w3.org/2000/01/rdf-schema#label>
                "Creator"@en ;
        <http://www.w3.org/2000/01/rdf-schema#range>
                <http://purl.org/dc/terms/Agent> ;
        <http://www.w3.org/2000/01/rdf-schema#subPropertyOf>
                <http://purl.org/dc/elements/1.1/creator> , <http://purl.org/dc/terms/contributor> ;
        <http://purl.org/dc/terms/description>
                "Examples of a Creator include a person, an organization, or a service."@en ;
        <http://purl.org/dc/terms/hasVersion>
                <http://dublincore.org/usage/terms/history/#creatorT-002> ;
        <http://purl.org/dc/terms/issued>
                "2008-01-14"^^<http://www.w3.org/2001/XMLSchema#date> ;
        <http://purl.org/dc/terms/modified>
                "2010-10-11"^^<http://www.w3.org/2001/XMLSchema#date> .

<http://www.demcare.eu/ontologies/demlab.owl#Protocol>
        a       <http://www.w3.org/2002/07/owl#Class> ;
        <http://www.w3.org/2000/01/rdf-schema#comment>
                "A Protocol instance contains information regarding the participant and the duration of the protocol session. It can be also associated with one or more ProtocolSteps that define the Tasks and the corresponding MeasuredData."@en ;
        <http://www.w3.org/2000/01/rdf-schema#seeAlso>
                <http://www.demcare.eu/ontologies/demlab.owl#Task> , <http://www.demcare.eu/ontologies/demlab.owl#MeasuredData> , <http://www.demcare.eu/ontologies/demlab.owl#ProtocolStep> ;
        <http://www.w3.org/2000/01/rdf-schema#subClassOf>
                [ a       <http://www.w3.org/2002/07/owl#Restriction> ;
                  <http://www.w3.org/2002/07/owl#onClass>
                          <http://www.w3.org/2006/time#Instant> ;
                  <http://www.w3.org/2002/07/owl#onProperty>
                          <http://www.w3.org/2006/time#hasEnd> ;
                  <http://www.w3.org/2002/07/owl#qualifiedCardinality>
                          "1"^^<http://www.w3.org/2001/XMLSchema#nonNegativeInteger>
                ] ;
        <http://www.w3.org/2000/01/rdf-schema#subClassOf>
                [ a       <http://www.w3.org/2002/07/owl#Restriction> ;
                  <http://www.w3.org/2002/07/owl#onProperty>
                          <http://www.demcare.eu/ontologies/demlab.owl#hasProtocolStep> ;
                  <http://www.w3.org/2002/07/owl#someValuesFrom>
                          <http://www.demcare.eu/ontologies/demlab.owl#ProtocolStep>
                ] ;
        <http://www.w3.org/2000/01/rdf-schema#subClassOf>
                [ a       <http://www.w3.org/2002/07/owl#Restriction> ;
                  <http://www.w3.org/2002/07/owl#onClass>
                          <http://xmlns.com/foaf/0.1/Person> ;
                  <http://www.w3.org/2002/07/owl#onProperty>
                          <http://www.demcare.eu/ontologies/demlab.owl#hasParticipant> ;
                  <http://www.w3.org/2002/07/owl#qualifiedCardinality>
                          "1"^^<http://www.w3.org/2001/XMLSchema#nonNegativeInteger>
                ] ;
        <http://www.w3.org/2000/01/rdf-schema#subClassOf>
                [ a       <http://www.w3.org/2002/07/owl#Restriction> ;
                  <http://www.w3.org/2002/07/owl#onClass>
                          <http://www.w3.org/2006/time#Instant> ;
                  <http://www.w3.org/2002/07/owl#onProperty>
                          <http://www.w3.org/2006/time#hasBeginning> ;
                  <http://www.w3.org/2002/07/owl#qualifiedCardinality>
                          "1"^^<http://www.w3.org/2001/XMLSchema#nonNegativeInteger>
                ] .

<http://purl.org/dc/terms/hasVersion>
        a       <http://www.w3.org/2002/07/owl#AnnotationProperty> ;
        <http://www.w3.org/2000/01/rdf-schema#comment>
                "A related resource that is a version, edition, or adaptation of the described resource."@en ;
        <http://www.w3.org/2000/01/rdf-schema#isDefinedBy>
                <http://purl.org/dc/terms/> ;
        <http://www.w3.org/2000/01/rdf-schema#label>
                "Has Version"@en ;
        <http://www.w3.org/2000/01/rdf-schema#subPropertyOf>
                <http://purl.org/dc/elements/1.1/relation> , <http://purl.org/dc/terms/relation> ;
        <http://purl.org/dc/terms/hasVersion>
                <http://dublincore.org/usage/terms/history/#hasVersion-003> ;
        <http://purl.org/dc/terms/issued>
                "2000-07-11"^^<http://www.w3.org/2001/XMLSchema#date> ;
        <http://purl.org/dc/terms/modified>
                "2008-01-14"^^<http://www.w3.org/2001/XMLSchema#date> ;
        <http://www.w3.org/2004/02/skos/core#note>
                "This term is intended to be used with non-literal values as defined in the DCMI Abstract Model (http://dublincore.org/documents/abstract-model/).  As of December 2007, the DCMI Usage Board is seeking a way to express this intention with a formal range declaration."@en .

<http://www.demcare.eu/ontologies/demlab.owl#AutonomyAssessment>
        a       <http://www.w3.org/2002/07/owl#Class> ;
        <http://www.w3.org/2000/01/rdf-schema#comment>
                "Autonomy is assessed based on the performance of the participant during the SemiDirectedActivitiesStep. The property iadl_e (Instrumental Activities of Daily Living for Elderly) can be used to quantify autonomy"@en ;
        <http://www.w3.org/2000/01/rdf-schema#seeAlso>
                <http://www.demcare.eu/ontologies/demlab.owl#iadl_e> , <http://www.demcare.eu/ontologies/demlab.owl#SemiDirectedActivitiesStep> ;
        <http://www.w3.org/2000/01/rdf-schema#subClassOf>
                <http://www.demcare.eu/ontologies/demlab.owl#ClinicalAssessment> ;
        <http://www.w3.org/2000/01/rdf-schema#subClassOf>
                [ a       <http://www.w3.org/2002/07/owl#Restriction> ;
                  <http://www.w3.org/2002/07/owl#cardinality>
                          "1"^^<http://www.w3.org/2001/XMLSchema#nonNegativeInteger> ;
                  <http://www.w3.org/2002/07/owl#onProperty>
                          <http://www.demcare.eu/ontologies/demlab.owl#iadl_e>
                ] .

<http://www.demcare.eu/ontologies/demlab.owl>
        a       <http://www.w3.org/2002/07/owl#Ontology> , <http://www.w3.org/2002/07/owl#NamedIndividual> ;
        <http://www.w3.org/2000/01/rdf-schema#seeAlso>
                "http://www.demcare.eu/downloads/D8.1ExperimentationProtocols.pdf" , "http://www.demcare.eu/" ;
        <http://creativecommons.org/ns#license>
                <http://creativecommons.org/licenses/by/3.0/> ;
        <http://purl.org/dc/elements/1.1/creator>
                <http://www.iti.gr/iti/people/Georgios_Meditskos.html#gmeditsk> , <http://www.iti.gr/iti/people/Ioannis_Kompatsiaris.html#ikom> ;
        <http://purl.org/dc/elements/1.1/description>
                "The ontology has been developed in the framework of the Dem@Care project for representing the experimentation protocol towards diagnostic support and assessment of Dementia in a controlled environment. The aim of the protocol is to provide a brief overview of their health status of the participants during consultation (cognition, behaviours and function), and to correlate the system (sensor) data with the data collected using typical dementia care assessment tools.\n\nThe ontology describes the basic Steps of the experimentation protocol (Directed Activities, Semi-directed Activities and Free Discussion with the Clinician), the Tasks that are involved, as well as the measurement types relevant to each Task. The defined protocol can be reused and further extended, adding new steps, tasks and measured data.\n\nDocumentation regarding the ontology vocabulary can be found at http://www.demcare.eu/ontologies/demlab.html"@en ;
        <http://purl.org/dc/terms/date>
                "2014-09-02" ;
        <http://purl.org/dc/terms/rights>
                "This ontology is licensed under Creative Commons CC BY 3.0 It is developed in the framework of the Dem@Care project (http://www.demcare.eu/) and supported by the Information Technologies Institute (http://www.iti.gr) of the Centre for Research and Technology Hellas."@en ;
        <http://purl.org/dc/terms/title>
                "Dem@Care Lab Ontology for Dementia Assessment"@en ;
        <http://purl.org/vocab/vann/preferredNamespacePrefix>
                "demlab" ;
        <http://www.w3.org/2002/07/owl#imports>
                <http://www.w3.org/2006/time> , <http://xmlns.com/foaf/0.1/> ;
        <http://www.w3.org/2002/07/owl#versionIRI>
                <http://www.demcare.eu/ontologies/demlab.owl/1.0> ;
        <http://www.w3.org/2002/07/owl#versionInfo>
                1.0 .

<http://purl.org/dc/terms/date>
        a       <http://www.w3.org/2002/07/owl#DatatypeProperty> , <http://www.w3.org/2002/07/owl#AnnotationProperty> ;
        <http://www.w3.org/2000/01/rdf-schema#comment>
                "A point or period of time associated with an event in the lifecycle of the resource."@en ;
        <http://www.w3.org/2000/01/rdf-schema#isDefinedBy>
                <http://purl.org/dc/terms/> ;
        <http://www.w3.org/2000/01/rdf-schema#label>
                "Date"@en ;
        <http://www.w3.org/2000/01/rdf-schema#range>
                <http://www.w3.org/2000/01/rdf-schema#Literal> ;
        <http://www.w3.org/2000/01/rdf-schema#subPropertyOf>
                <http://purl.org/dc/elements/1.1/date> ;
        <http://purl.org/dc/terms/description>
                "Date may be used to express temporal information at any level of granularity.  Recommended best practice is to use an encoding scheme, such as the W3CDTF profile of ISO 8601 [W3CDTF]."@en ;
        <http://purl.org/dc/terms/hasVersion>
                <http://dublincore.org/usage/terms/history/#dateT-001> ;
        <http://purl.org/dc/terms/issued>
                "2008-01-14"^^<http://www.w3.org/2001/XMLSchema#date> ;
        <http://purl.org/dc/terms/modified>
                "2008-01-14"^^<http://www.w3.org/2001/XMLSchema#date> .

<http://www.demcare.eu/ontologies/demlab.owl#predementia>
        a       <http://www.demcare.eu/ontologies/demlab.owl#DiagnosisType> , <http://www.w3.org/2002/07/owl#NamedIndividual> .

<http://www.demcare.eu/ontologies/demlab.owl#DirectedDiscussionTask>
        a       <http://www.w3.org/2002/07/owl#Class> ;
        <http://www.w3.org/2000/01/rdf-schema#subClassOf>
                <http://www.demcare.eu/ontologies/demlab.owl#DiscussionTask> .

<http://www.demcare.eu/ontologies/demlab.owl#SemiDirectedActivitiesStep>
        a       <http://www.w3.org/2002/07/owl#Class> ;
        <http://www.w3.org/2000/01/rdf-schema#comment>
                "This ProtocolStep consists of assessing the autonomy of the participant. The participant has to organize himself/herself and correctly perform a list of Instrumental Activities of Daily Living (e.g., managing finance, using phone, preparing tea) within a timeframe of 15minutes. For this step, the participant is alone in the experimental setting and can refer to the instruction sheet of paper with the IADLs to perform at any time."@en ;
        <http://www.w3.org/2000/01/rdf-schema#subClassOf>
                <http://www.demcare.eu/ontologies/demlab.owl#ProtocolStep> ;
        <http://www.w3.org/2000/01/rdf-schema#subClassOf>
                [ a       <http://www.w3.org/2002/07/owl#Restriction> ;
                  <http://www.w3.org/2002/07/owl#allValuesFrom>
                          [ a       <http://www.w3.org/2002/07/owl#Class> ;
                            <http://www.w3.org/2002/07/owl#unionOf>
                                    ( <http://www.demcare.eu/ontologies/demlab.owl#AnswerPhoneTask> <http://www.demcare.eu/ontologies/demlab.owl#CallPsychologistTask> <http://www.demcare.eu/ontologies/demlab.owl#EstablishAccountBalanceTask> <http://www.demcare.eu/ontologies/demlab.owl#FindBusLineOnMapTask> <http://www.demcare.eu/ontologies/demlab.owl#LeaveRoomTask> <http://www.demcare.eu/ontologies/demlab.owl#PayBillTask> <http://www.demcare.eu/ontologies/demlab.owl#PrepareDrugBoxTask> <http://www.demcare.eu/ontologies/demlab.owl#PrepareHotTeaTask> <http://www.demcare.eu/ontologies/demlab.owl#Task> <http://www.demcare.eu/ontologies/demlab.owl#TurnOnTVTask> <http://www.demcare.eu/ontologies/demlab.owl#WaterPlantTask> )
                          ] ;
                  <http://www.w3.org/2002/07/owl#onProperty>
                          <http://www.demcare.eu/ontologies/demlab.owl#involvesTask>
                ] .

<http://purl.org/dc/terms/URI>
        a       <http://www.w3.org/2000/01/rdf-schema#Datatype> ;
        <http://www.w3.org/2000/01/rdf-schema#comment>
                "The set of identifiers constructed according to the generic syntax for Uniform Resource Identifiers as specified by the Internet Engineering Task Force."@en ;
        <http://www.w3.org/2000/01/rdf-schema#isDefinedBy>
                <http://purl.org/dc/terms/> ;
        <http://www.w3.org/2000/01/rdf-schema#label>
                "URI"@en ;
        <http://www.w3.org/2000/01/rdf-schema#seeAlso>
                <http://www.ietf.org/rfc/rfc3986.txt> ;
        <http://purl.org/dc/terms/hasVersion>
                <http://dublincore.org/usage/terms/history/#URI-003> ;
        <http://purl.org/dc/terms/issued>
                "2000-07-11"^^<http://www.w3.org/2001/XMLSchema#date> ;
        <http://purl.org/dc/terms/modified>
                "2008-01-14"^^<http://www.w3.org/2001/XMLSchema#date> .

<http://purl.org/dc/terms/modified>
        a       <http://www.w3.org/2002/07/owl#DatatypeProperty> , <http://www.w3.org/2002/07/owl#AnnotationProperty> ;
        <http://www.w3.org/2000/01/rdf-schema#comment>
                "Date on which the resource was changed."@en ;
        <http://www.w3.org/2000/01/rdf-schema#isDefinedBy>
                <http://purl.org/dc/terms/> ;
        <http://www.w3.org/2000/01/rdf-schema#label>
                "Date Modified"@en ;
        <http://www.w3.org/2000/01/rdf-schema#range>
                <http://www.w3.org/2000/01/rdf-schema#Literal> ;
        <http://www.w3.org/2000/01/rdf-schema#subPropertyOf>
                <http://purl.org/dc/elements/1.1/date> , <http://purl.org/dc/terms/date> ;
        <http://purl.org/dc/terms/hasVersion>
                <http://dublincore.org/usage/terms/history/#modified-003> ;
        <http://purl.org/dc/terms/issued>
                "2000-07-11"^^<http://www.w3.org/2001/XMLSchema#date> ;
        <http://purl.org/dc/terms/modified>
                "2008-01-14"^^<http://www.w3.org/2001/XMLSchema#date> .

<http://www.demcare.eu/ontologies/demlab.owl#ArticulationControlTask>
        a       <http://www.w3.org/2002/07/owl#Class> ;
        <http://www.w3.org/2000/01/rdf-schema#comment>
                "The participant is asked to pronounce repeatedly a predefined diadochokinetic “Pataka” token as rapid as possible stopping this action upon a sign by the clinician. The clinician will stop the action in 10 sec.\n\nThis task is used for assessing:\n- Latency: time of latency between the end of instructions (stimulation) and the beginning of the task\n- Stress level\n- Voice: e.g. speech rate, pause rate etc."@en ;
        <http://www.w3.org/2000/01/rdf-schema#subClassOf>
                <http://www.demcare.eu/ontologies/demlab.owl#DirectedTask> ;
        <http://www.w3.org/2000/01/rdf-schema#subClassOf>
                [ a       <http://www.w3.org/2002/07/owl#Restriction> ;
                  <http://www.w3.org/2002/07/owl#allValuesFrom>
                          [ a       <http://www.w3.org/2002/07/owl#Class> ;
                            <http://www.w3.org/2002/07/owl#unionOf>
                                    ( <http://www.demcare.eu/ontologies/demlab.owl#LatencyData> <http://www.demcare.eu/ontologies/demlab.owl#StressData> <http://www.demcare.eu/ontologies/demlab.owl#VoiceData> )
                          ] ;
                  <http://www.w3.org/2002/07/owl#onProperty>
                          <http://www.demcare.eu/ontologies/demlab.owl#measuredData>
                ] .

<http://purl.org/dc/terms/accrualPolicy>
        a       <http://www.w3.org/2002/07/owl#ObjectProperty> , <http://www.w3.org/2002/07/owl#AnnotationProperty> ;
        <http://www.w3.org/2000/01/rdf-schema#comment>
                "The policy governing the addition of items to a collection."@en ;
        <http://www.w3.org/2000/01/rdf-schema#domain>
                <http://purl.org/dc/dcmitype/Collection> ;
        <http://www.w3.org/2000/01/rdf-schema#isDefinedBy>
                <http://purl.org/dc/terms/> ;
        <http://www.w3.org/2000/01/rdf-schema#label>
                "Accrual Policy"@en ;
        <http://www.w3.org/2000/01/rdf-schema#range>
                <http://purl.org/dc/terms/Policy> ;
        <http://purl.org/dc/terms/hasVersion>
                <http://dublincore.org/usage/terms/history/#accrualPolicy-003> ;
        <http://purl.org/dc/terms/issued>
                "2005-06-13"^^<http://www.w3.org/2001/XMLSchema#date> ;
        <http://purl.org/dc/terms/modified>
                "2010-10-11"^^<http://www.w3.org/2001/XMLSchema#date> .

<http://purl.org/dc/terms/rights>
        a       <http://www.w3.org/2002/07/owl#ObjectProperty> , <http://www.w3.org/2002/07/owl#AnnotationProperty> ;
        <http://www.w3.org/2000/01/rdf-schema#comment>
                "Information about rights held in and over the resource."@en ;
        <http://www.w3.org/2000/01/rdf-schema#isDefinedBy>
                <http://purl.org/dc/terms/> ;
        <http://www.w3.org/2000/01/rdf-schema#label>
                "Rights"@en ;
        <http://www.w3.org/2000/01/rdf-schema#range>
                <http://purl.org/dc/terms/RightsStatement> ;
        <http://www.w3.org/2000/01/rdf-schema#subPropertyOf>
                <http://purl.org/dc/elements/1.1/rights> ;
        <http://purl.org/dc/terms/description>
                "Typically, rights information includes a statement about various property rights associated with the resource, including intellectual property rights."@en ;
        <http://purl.org/dc/terms/hasVersion>
                <http://dublincore.org/usage/terms/history/#rightsT-001> ;
        <http://purl.org/dc/terms/issued>
                "2008-01-14"^^<http://www.w3.org/2001/XMLSchema#date> ;
        <http://purl.org/dc/terms/modified>
                "2008-01-14"^^<http://www.w3.org/2001/XMLSchema#date> .

<http://www.demcare.eu/ontologies/demlab.owl#NeuropsychiatricAndMoodAssessment>
        a       <http://www.w3.org/2002/07/owl#Class> ;
        <http://www.w3.org/2000/01/rdf-schema#comment>
                "Neuropsychiatric/Mood assessments:\n- NPI \n- DSM-IV Criteria for depression \n- Apathy Inventory (AI) and diagnostic criteria for apathy."@en ;
        <http://www.w3.org/2000/01/rdf-schema#seeAlso>
                <http://www.demcare.eu/ontologies/demlab.owl#npi> , <http://www.demcare.eu/ontologies/demlab.owl#apathyInventory> , <http://www.demcare.eu/ontologies/demlab.owl#dsm_ivDepressionCriteria> ;
        <http://www.w3.org/2000/01/rdf-schema#subClassOf>
                <http://www.demcare.eu/ontologies/demlab.owl#ClinicalAssessment> ;
        <http://www.w3.org/2000/01/rdf-schema#subClassOf>
                [ a       <http://www.w3.org/2002/07/owl#Restriction> ;
                  <http://www.w3.org/2002/07/owl#cardinality>
                          "1"^^<http://www.w3.org/2001/XMLSchema#nonNegativeInteger> ;
                  <http://www.w3.org/2002/07/owl#onProperty>
                          <http://www.demcare.eu/ontologies/demlab.owl#npi>
                ] ;
        <http://www.w3.org/2000/01/rdf-schema#subClassOf>
                [ a       <http://www.w3.org/2002/07/owl#Restriction> ;
                  <http://www.w3.org/2002/07/owl#cardinality>
                          "1"^^<http://www.w3.org/2001/XMLSchema#nonNegativeInteger> ;
                  <http://www.w3.org/2002/07/owl#onProperty>
                          <http://www.demcare.eu/ontologies/demlab.owl#apathyInventory>
                ] ;
        <http://www.w3.org/2000/01/rdf-schema#subClassOf>
                [ a       <http://www.w3.org/2002/07/owl#Restriction> ;
                  <http://www.w3.org/2002/07/owl#cardinality>
                          "1"^^<http://www.w3.org/2001/XMLSchema#nonNegativeInteger> ;
                  <http://www.w3.org/2002/07/owl#onProperty>
                          <http://www.demcare.eu/ontologies/demlab.owl#dsm_ivDepressionCriteria>
                ] .

<http://purl.org/dc/terms/Agent>
        a       <http://purl.org/dc/terms/AgentClass> , <http://www.w3.org/2002/07/owl#NamedIndividual> , <http://www.w3.org/2002/07/owl#Class> ;
        <http://www.w3.org/2000/01/rdf-schema#comment>
                "A resource that acts or has the power to act."@en ;
        <http://www.w3.org/2000/01/rdf-schema#isDefinedBy>
                <http://purl.org/dc/terms/> ;
        <http://www.w3.org/2000/01/rdf-schema#label>
                "Agent"@en ;
        <http://purl.org/dc/terms/description>
                "Examples of Agent include person, organization, and software agent."@en ;
        <http://purl.org/dc/terms/hasVersion>
                <http://dublincore.org/usage/terms/history/#Agent-001> ;
        <http://purl.org/dc/terms/issued>
                "2008-01-14"^^<http://www.w3.org/2001/XMLSchema#date> .

<http://www.demcare.eu/ontologies/demlab.owl#pauseRate>
        a       <http://www.w3.org/2002/07/owl#DatatypeProperty> ;
        <http://www.w3.org/2000/01/rdf-schema#comment>
                "Pause rate during sentence repetition and mono/dual tasks"@en ;
        <http://www.w3.org/2000/01/rdf-schema#domain>
                <http://www.demcare.eu/ontologies/demlab.owl#VoiceData> ;
        <http://www.w3.org/2000/01/rdf-schema#seeAlso>
                <http://www.demcare.eu/ontologies/demlab.owl#SentenceRepeatingTask> , <http://www.demcare.eu/ontologies/demlab.owl#VoiceData> , <http://www.demcare.eu/ontologies/demlab.owl#CountingBackwardsTask> , <http://www.demcare.eu/ontologies/demlab.owl#WalkingCountingBackwardsTask> , <http://www.demcare.eu/ontologies/demlab.owl#ArticulationControlTask> .

<http://www.demcare.eu/ontologies/demlab.owl#freeAndCuedRemindingAssessment>
        a       <http://www.w3.org/2002/07/owl#DatatypeProperty> ;
        <http://www.w3.org/2000/01/rdf-schema#comment>
                "The Free and Cued Selective Reminding Test"@en ;
        <http://www.w3.org/2000/01/rdf-schema#domain>
                <http://www.demcare.eu/ontologies/demlab.owl#CognitiveAbilitiesAssessment> ;
        <http://www.w3.org/2000/01/rdf-schema#seeAlso>
                <http://www.demcare.eu/ontologies/demlab.owl#CognitiveAbilitiesAssessment> .

<http://www.demcare.eu/ontologies/demlab.owl#PersonWithPredementia>
        a       <http://www.w3.org/2002/07/owl#Class> ;
        <http://www.w3.org/2000/01/rdf-schema#comment>
                "A Person with Predementia is defined as the participant whose clinical record contains a predementia clinical diagnosis"@en ;
        <http://www.w3.org/2000/01/rdf-schema#seeAlso>
                <http://www.demcare.eu/ontologies/demlab.owl#predementia> , <http://www.demcare.eu/ontologies/demlab.owl#ClinicalRecord> , <http://www.demcare.eu/ontologies/demlab.owl#DiagnosisType> , <http://www.demcare.eu/ontologies/demlab.owl#DiagnosisAssessment> ;
        <http://www.w3.org/2000/01/rdf-schema#subClassOf>
                <http://www.demcare.eu/ontologies/demlab.owl#Participant> ;
        <http://www.w3.org/2002/07/owl#equivalentClass>
                [ a       <http://www.w3.org/2002/07/owl#Restriction> ;
                  <http://www.w3.org/2002/07/owl#onProperty>
                          <http://www.demcare.eu/ontologies/demlab.owl#hasClinicalRecord> ;
                  <http://www.w3.org/2002/07/owl#someValuesFrom>
                          [ a       <http://www.w3.org/2002/07/owl#Class> ;
                            <http://www.w3.org/2002/07/owl#intersectionOf>
                                    ( <http://www.demcare.eu/ontologies/demlab.owl#ClinicalRecord>
                                      [ a       <http://www.w3.org/2002/07/owl#Restriction> ;
                                        <http://www.w3.org/2002/07/owl#onProperty>
                                                <http://www.demcare.eu/ontologies/demlab.owl#containsAssessment> ;
                                        <http://www.w3.org/2002/07/owl#someValuesFrom>
                                                [ a       <http://www.w3.org/2002/07/owl#Class> ;
                                                  <http://www.w3.org/2002/07/owl#intersectionOf>
                                                          ( <http://www.demcare.eu/ontologies/demlab.owl#DiagnosisAssessment>
                                                            [ a       <http://www.w3.org/2002/07/owl#Restriction> ;
                                                              <http://www.w3.org/2002/07/owl#onProperty>
                                                                      <http://www.demcare.eu/ontologies/demlab.owl#hasClinicalDiagnosis> ;
                                                              <http://www.w3.org/2002/07/owl#someValuesFrom>
                                                                      [ a       <http://www.w3.org/2002/07/owl#Class> ;
                                                                        <http://www.w3.org/2002/07/owl#oneOf>
                                                                                ( <http://www.demcare.eu/ontologies/demlab.owl#predementia> )
                                                                      ]
                                                            ]
                                                          )
                                                ]
                                      ]
                                    )
                          ]
                ] .

<http://purl.org/dc/terms/alternative>
        a       <http://www.w3.org/2002/07/owl#DatatypeProperty> , <http://www.w3.org/2002/07/owl#AnnotationProperty> ;
        <http://www.w3.org/2000/01/rdf-schema#comment>
                "An alternative name for the resource."@en ;
        <http://www.w3.org/2000/01/rdf-schema#isDefinedBy>
                <http://purl.org/dc/terms/> ;
        <http://www.w3.org/2000/01/rdf-schema#label>
                "Alternative Title"@en ;
        <http://www.w3.org/2000/01/rdf-schema#range>
                <http://www.w3.org/2000/01/rdf-schema#Literal> ;
        <http://www.w3.org/2000/01/rdf-schema#subPropertyOf>
                <http://purl.org/dc/terms/title> , <http://purl.org/dc/elements/1.1/title> ;
        <http://purl.org/dc/terms/description>
                "The distinction between titles and alternative titles is application-specific."@en ;
        <http://purl.org/dc/terms/hasVersion>
                <http://dublincore.org/usage/terms/history/#alternative-003> ;
        <http://purl.org/dc/terms/issued>
                "2000-07-11"^^<http://www.w3.org/2001/XMLSchema#date> ;
        <http://purl.org/dc/terms/modified>
                "2010-10-11"^^<http://www.w3.org/2001/XMLSchema#date> .

<http://www.demcare.eu/ontologies/demlab.owl#GaitData>
        a       <http://www.w3.org/2002/07/owl#Class> ;
        <http://www.w3.org/2000/01/rdf-schema#comment>
                "Gait assessment and impact of a cognitive activity on gait performance"@en ;
        <http://www.w3.org/2000/01/rdf-schema#subClassOf>
                <http://www.demcare.eu/ontologies/demlab.owl#MeasuredData> ;
        <http://www.w3.org/2000/01/rdf-schema#subClassOf>
                [ a       <http://www.w3.org/2002/07/owl#Restriction> ;
                  <http://www.w3.org/2002/07/owl#cardinality>
                          "1"^^<http://www.w3.org/2001/XMLSchema#nonNegativeInteger> ;
                  <http://www.w3.org/2002/07/owl#onProperty>
                          <http://www.demcare.eu/ontologies/demlab.owl#walkingSpeed>
                ] ;
        <http://www.w3.org/2000/01/rdf-schema#subClassOf>
                [ a       <http://www.w3.org/2002/07/owl#Restriction> ;
                  <http://www.w3.org/2002/07/owl#cardinality>
                          "1"^^<http://www.w3.org/2001/XMLSchema#nonNegativeInteger> ;
                  <http://www.w3.org/2002/07/owl#onProperty>
                          <http://www.demcare.eu/ontologies/demlab.owl#dynamicBalance>
                ] ;
        <http://www.w3.org/2000/01/rdf-schema#subClassOf>
                [ a       <http://www.w3.org/2002/07/owl#Restriction> ;
                  <http://www.w3.org/2002/07/owl#cardinality>
                          "1"^^<http://www.w3.org/2001/XMLSchema#nonNegativeInteger> ;
                  <http://www.w3.org/2002/07/owl#onProperty>
                          <http://www.demcare.eu/ontologies/demlab.owl#walkingSpeedInstantaneous>
                ] ;
        <http://www.w3.org/2000/01/rdf-schema#subClassOf>
                [ a       <http://www.w3.org/2002/07/owl#Restriction> ;
                  <http://www.w3.org/2002/07/owl#onDataRange>
                          <http://www.w3.org/2001/XMLSchema#boolean> ;
                  <http://www.w3.org/2002/07/owl#onProperty>
                          <http://www.demcare.eu/ontologies/demlab.owl#stoppingDisplacement> ;
                  <http://www.w3.org/2002/07/owl#qualifiedCardinality>
                          "1"^^<http://www.w3.org/2001/XMLSchema#nonNegativeInteger>
                ] ;
        <http://www.w3.org/2000/01/rdf-schema#subClassOf>
                [ a       <http://www.w3.org/2002/07/owl#Restriction> ;
                  <http://www.w3.org/2002/07/owl#cardinality>
                          "1"^^<http://www.w3.org/2001/XMLSchema#nonNegativeInteger> ;
                  <http://www.w3.org/2002/07/owl#onProperty>
                          <http://www.demcare.eu/ontologies/demlab.owl#stepLength>
                ] .

<http://purl.org/dc/terms/dateCopyrighted>
        a       <http://www.w3.org/2002/07/owl#DatatypeProperty> , <http://www.w3.org/2002/07/owl#AnnotationProperty> ;
        <http://www.w3.org/2000/01/rdf-schema#comment>
                "Date of copyright."@en ;
        <http://www.w3.org/2000/01/rdf-schema#isDefinedBy>
                <http://purl.org/dc/terms/> ;
        <http://www.w3.org/2000/01/rdf-schema#label>
                "Date Copyrighted"@en ;
        <http://www.w3.org/2000/01/rdf-schema#range>
                <http://www.w3.org/2000/01/rdf-schema#Literal> ;
        <http://www.w3.org/2000/01/rdf-schema#subPropertyOf>
                <http://purl.org/dc/elements/1.1/date> , <http://purl.org/dc/terms/date> ;
        <http://purl.org/dc/terms/hasVersion>
                <http://dublincore.org/usage/terms/history/#dateCopyrighted-002> ;
        <http://purl.org/dc/terms/issued>
                "2002-07-13"^^<http://www.w3.org/2001/XMLSchema#date> ;
        <http://purl.org/dc/terms/modified>
                "2008-01-14"^^<http://www.w3.org/2001/XMLSchema#date> .

<http://www.demcare.eu/ontologies/demlab.owl#ProtocolStep>
        a       <http://www.w3.org/2002/07/owl#Class> ;
        <http://www.w3.org/2000/01/rdf-schema#comment>
                "A ProtocolStep defines the Tasks of interest. Three ProtocolStep types are currently defined in Dem@Care: DirectedActivities, SemiDirectedActivities and DiscussionWithTheClinician"@en ;
        <http://www.w3.org/2000/01/rdf-schema#seeAlso>
                <http://www.demcare.eu/ontologies/demlab.owl#DiscussionWithClinicianStep> , <http://www.demcare.eu/ontologies/demlab.owl#SemiDirectedActivitiesStep> , <http://www.demcare.eu/ontologies/demlab.owl#Task> , <http://www.demcare.eu/ontologies/demlab.owl#DirectedActivitiesStep> ;
        <http://www.w3.org/2000/01/rdf-schema#subClassOf>
                [ a       <http://www.w3.org/2002/07/owl#Restriction> ;
                  <http://www.w3.org/2002/07/owl#onProperty>
                          <http://www.demcare.eu/ontologies/demlab.owl#involvesTask> ;
                  <http://www.w3.org/2002/07/owl#someValuesFrom>
                          <http://www.demcare.eu/ontologies/demlab.owl#Task>
                ] ;
        <http://www.w3.org/2000/01/rdf-schema#subClassOf>
                [ a       <http://www.w3.org/2002/07/owl#Restriction> ;
                  <http://www.w3.org/2002/07/owl#onClass>
                          <http://www.w3.org/2006/time#Instant> ;
                  <http://www.w3.org/2002/07/owl#onProperty>
                          <http://www.w3.org/2006/time#hasEnd> ;
                  <http://www.w3.org/2002/07/owl#qualifiedCardinality>
                          "1"^^<http://www.w3.org/2001/XMLSchema#nonNegativeInteger>
                ] ;
        <http://www.w3.org/2000/01/rdf-schema#subClassOf>
                [ a       <http://www.w3.org/2002/07/owl#Restriction> ;
                  <http://www.w3.org/2002/07/owl#onClass>
                          <http://www.w3.org/2006/time#Instant> ;
                  <http://www.w3.org/2002/07/owl#onProperty>
                          <http://www.w3.org/2006/time#hasBeginning> ;
                  <http://www.w3.org/2002/07/owl#qualifiedCardinality>
                          "1"^^<http://www.w3.org/2001/XMLSchema#nonNegativeInteger>
                ] .

<http://purl.org/dc/terms/relation>
        a       <http://www.w3.org/2002/07/owl#AnnotationProperty> ;
        <http://www.w3.org/2000/01/rdf-schema#comment>
                "A related resource."@en ;
        <http://www.w3.org/2000/01/rdf-schema#isDefinedBy>
                <http://purl.org/dc/terms/> ;
        <http://www.w3.org/2000/01/rdf-schema#label>
                "Relation"@en ;
        <http://www.w3.org/2000/01/rdf-schema#subPropertyOf>
                <http://purl.org/dc/elements/1.1/relation> ;
        <http://purl.org/dc/terms/description>
                "Recommended best practice is to identify the related resource by means of a string conforming to a formal identification system. "@en ;
        <http://purl.org/dc/terms/hasVersion>
                <http://dublincore.org/usage/terms/history/#relationT-001> ;
        <http://purl.org/dc/terms/issued>
                "2008-01-14"^^<http://www.w3.org/2001/XMLSchema#date> ;
        <http://purl.org/dc/terms/modified>
                "2008-01-14"^^<http://www.w3.org/2001/XMLSchema#date> ;
        <http://www.w3.org/2004/02/skos/core#note>
                "This term is intended to be used with non-literal values as defined in the DCMI Abstract Model (http://dublincore.org/documents/abstract-model/).  As of December 2007, the DCMI Usage Board is seeking a way to express this intention with a formal range declaration."@en .

<http://purl.org/dc/terms/educationLevel>
        a       <http://www.w3.org/2002/07/owl#ObjectProperty> , <http://www.w3.org/2002/07/owl#AnnotationProperty> ;
        <http://www.w3.org/2000/01/rdf-schema#comment>
                "A class of entity, defined in terms of progression through an educational or training context, for which the described resource is intended."@en ;
        <http://www.w3.org/2000/01/rdf-schema#isDefinedBy>
                <http://purl.org/dc/terms/> ;
        <http://www.w3.org/2000/01/rdf-schema#label>
                "Audience Education Level"@en ;
        <http://www.w3.org/2000/01/rdf-schema#range>
                <http://purl.org/dc/terms/AgentClass> ;
        <http://www.w3.org/2000/01/rdf-schema#subPropertyOf>
                <http://purl.org/dc/terms/audience> ;
        <http://purl.org/dc/terms/hasVersion>
                <http://dublincore.org/usage/terms/history/#educationLevel-002> ;
        <http://purl.org/dc/terms/issued>
                "2002-07-13"^^<http://www.w3.org/2001/XMLSchema#date> ;
        <http://purl.org/dc/terms/modified>
                "2008-01-14"^^<http://www.w3.org/2001/XMLSchema#date> .

<http://www.demcare.eu/ontologies/demlab.owl#walkingSpeed>
        a       <http://www.w3.org/2002/07/owl#DatatypeProperty> ;
        <http://www.w3.org/2000/01/rdf-schema#comment>
                "Walking speed"@en ;
        <http://www.w3.org/2000/01/rdf-schema#domain>
                <http://www.demcare.eu/ontologies/demlab.owl#GaitData> ;
        <http://www.w3.org/2000/01/rdf-schema#seeAlso>
                <http://www.demcare.eu/ontologies/demlab.owl#GaitData> .

<http://purl.org/dc/terms/RFC3066>
        a       <http://www.w3.org/2000/01/rdf-schema#Datatype> ;
        <http://www.w3.org/2000/01/rdf-schema#comment>
                "The set of tags constructed according to RFC 3066 for the identification of languages."@en ;
        <http://www.w3.org/2000/01/rdf-schema#isDefinedBy>
                <http://purl.org/dc/terms/> ;
        <http://www.w3.org/2000/01/rdf-schema#label>
                "RFC 3066"@en ;
        <http://www.w3.org/2000/01/rdf-schema#seeAlso>
                <http://www.ietf.org/rfc/rfc3066.txt> ;
        <http://purl.org/dc/terms/description>
                "RFC 3066 has been obsoleted by RFC 4646."@en ;
        <http://purl.org/dc/terms/hasVersion>
                <http://dublincore.org/usage/terms/history/#RFC3066-002> ;
        <http://purl.org/dc/terms/issued>
                "2002-07-13"^^<http://www.w3.org/2001/XMLSchema#date> ;
        <http://purl.org/dc/terms/modified>
                "2008-01-14"^^<http://www.w3.org/2001/XMLSchema#date> .

<http://purl.org/dc/terms/SizeOrDuration>
        a       <http://www.w3.org/2002/07/owl#Class> ;
        <http://www.w3.org/2000/01/rdf-schema#comment>
                "A dimension or extent, or a time taken to play or execute."@en ;
        <http://www.w3.org/2000/01/rdf-schema#isDefinedBy>
                <http://purl.org/dc/terms/> ;
        <http://www.w3.org/2000/01/rdf-schema#label>
                "Size or Duration"@en ;
        <http://www.w3.org/2000/01/rdf-schema#subClassOf>
                <http://purl.org/dc/terms/MediaTypeOrExtent> ;
        <http://purl.org/dc/terms/description>
                "Examples include a number of pages, a specification of length, width, and breadth, or a period in hours, minutes, and seconds."@en ;
        <http://purl.org/dc/terms/hasVersion>
                <http://dublincore.org/usage/terms/history/#SizeOrDuration-001> ;
        <http://purl.org/dc/terms/issued>
                "2008-01-14"^^<http://www.w3.org/2001/XMLSchema#date> .

<http://purl.org/dc/terms/AgentClass>
        a       <http://www.w3.org/2002/07/owl#Class> ;
        <http://www.w3.org/2000/01/rdf-schema#comment>
                "A group of agents."@en ;
        <http://www.w3.org/2000/01/rdf-schema#isDefinedBy>
                <http://purl.org/dc/terms/> ;
        <http://www.w3.org/2000/01/rdf-schema#label>
                "Agent Class"@en ;
        <http://www.w3.org/2000/01/rdf-schema#subClassOf>
                <http://www.w3.org/2000/01/rdf-schema#Class> ;
        <http://purl.org/dc/terms/description>
                "Examples of Agent Class include groups seen as classes, such as students, women, charities, lecturers."@en ;
        <http://purl.org/dc/terms/hasVersion>
                <http://dublincore.org/usage/terms/history/#AgentClass-003> ;
        <http://purl.org/dc/terms/issued>
                "2008-01-14"^^<http://www.w3.org/2001/XMLSchema#date> ;
        <http://purl.org/dc/terms/modified>
                "2012-06-14"^^<http://www.w3.org/2001/XMLSchema#date> .

<http://purl.org/dc/terms/requires>
        a       <http://www.w3.org/2002/07/owl#AnnotationProperty> ;
        <http://www.w3.org/2000/01/rdf-schema#comment>
                "A related resource that is required by the described resource to support its function, delivery, or coherence."@en ;
        <http://www.w3.org/2000/01/rdf-schema#isDefinedBy>
                <http://purl.org/dc/terms/> ;
        <http://www.w3.org/2000/01/rdf-schema#label>
                "Requires"@en ;
        <http://www.w3.org/2000/01/rdf-schema#subPropertyOf>
                <http://purl.org/dc/elements/1.1/relation> , <http://purl.org/dc/terms/relation> ;
        <http://purl.org/dc/terms/hasVersion>
                <http://dublincore.org/usage/terms/history/#requires-003> ;
        <http://purl.org/dc/terms/issued>
                "2000-07-11"^^<http://www.w3.org/2001/XMLSchema#date> ;
        <http://purl.org/dc/terms/modified>
                "2008-01-14"^^<http://www.w3.org/2001/XMLSchema#date> ;
        <http://www.w3.org/2004/02/skos/core#note>
                "This term is intended to be used with non-literal values as defined in the DCMI Abstract Model (http://dublincore.org/documents/abstract-model/).  As of December 2007, the DCMI Usage Board is seeking a way to express this intention with a formal range declaration."@en .

<http://www.demcare.eu/ontologies/demlab.owl#dementia>
        a       <http://www.demcare.eu/ontologies/demlab.owl#DiagnosisType> , <http://www.w3.org/2002/07/owl#NamedIndividual> .

<http://purl.org/dc/terms/accessRights>
        a       <http://www.w3.org/2002/07/owl#AnnotationProperty> , <http://www.w3.org/2002/07/owl#ObjectProperty> ;
        <http://www.w3.org/2000/01/rdf-schema#comment>
                "Information about who can access the resource or an indication of its security status."@en ;
        <http://www.w3.org/2000/01/rdf-schema#isDefinedBy>
                <http://purl.org/dc/terms/> ;
        <http://www.w3.org/2000/01/rdf-schema#label>
                "Access Rights"@en ;
        <http://www.w3.org/2000/01/rdf-schema#range>
                <http://purl.org/dc/terms/RightsStatement> ;
        <http://www.w3.org/2000/01/rdf-schema#subPropertyOf>
                <http://purl.org/dc/elements/1.1/rights> , <http://purl.org/dc/terms/rights> ;
        <http://purl.org/dc/terms/description>
                "Access Rights may include information regarding access or restrictions based on privacy, security, or other policies."@en ;
        <http://purl.org/dc/terms/hasVersion>
                <http://dublincore.org/usage/terms/history/#accessRights-002> ;
        <http://purl.org/dc/terms/issued>
                "2003-02-15"^^<http://www.w3.org/2001/XMLSchema#date> ;
        <http://purl.org/dc/terms/modified>
                "2008-01-14"^^<http://www.w3.org/2001/XMLSchema#date> .

<http://purl.org/dc/terms/isFormatOf>
        a       <http://www.w3.org/2002/07/owl#AnnotationProperty> ;
        <http://www.w3.org/2000/01/rdf-schema#comment>
                "A related resource that is substantially the same as the described resource, but in another format."@en ;
        <http://www.w3.org/2000/01/rdf-schema#isDefinedBy>
                <http://purl.org/dc/terms/> ;
        <http://www.w3.org/2000/01/rdf-schema#label>
                "Is Format Of"@en ;
        <http://www.w3.org/2000/01/rdf-schema#subPropertyOf>
                <http://purl.org/dc/terms/relation> , <http://purl.org/dc/elements/1.1/relation> ;
        <http://purl.org/dc/terms/hasVersion>
                <http://dublincore.org/usage/terms/history/#isFormatOf-003> ;
        <http://purl.org/dc/terms/issued>
                "2000-07-11"^^<http://www.w3.org/2001/XMLSchema#date> ;
        <http://purl.org/dc/terms/modified>
                "2008-01-14"^^<http://www.w3.org/2001/XMLSchema#date> ;
        <http://www.w3.org/2004/02/skos/core#note>
                "This term is intended to be used with non-literal values as defined in the DCMI Abstract Model (http://dublincore.org/documents/abstract-model/).  As of December 2007, the DCMI Usage Board is seeking a way to express this intention with a formal range declaration."@en .

<http://purl.org/dc/terms/source>
        a       <http://www.w3.org/2002/07/owl#AnnotationProperty> ;
        <http://www.w3.org/2000/01/rdf-schema#comment>
                "A related resource from which the described resource is derived."@en ;
        <http://www.w3.org/2000/01/rdf-schema#isDefinedBy>
                <http://purl.org/dc/terms/> ;
        <http://www.w3.org/2000/01/rdf-schema#label>
                "Source"@en ;
        <http://www.w3.org/2000/01/rdf-schema#subPropertyOf>
                <http://purl.org/dc/terms/relation> , <http://purl.org/dc/elements/1.1/source> ;
        <http://purl.org/dc/terms/description>
                "The described resource may be derived from the related resource in whole or in part. Recommended best practice is to identify the related resource by means of a string conforming to a formal identification system."@en ;
        <http://purl.org/dc/terms/hasVersion>
                <http://dublincore.org/usage/terms/history/#sourceT-001> ;
        <http://purl.org/dc/terms/issued>
                "2008-01-14"^^<http://www.w3.org/2001/XMLSchema#date> ;
        <http://purl.org/dc/terms/modified>
                "2008-01-14"^^<http://www.w3.org/2001/XMLSchema#date> ;
        <http://www.w3.org/2004/02/skos/core#note>
                "This term is intended to be used with non-literal values as defined in the DCMI Abstract Model (http://dublincore.org/documents/abstract-model/).  As of December 2007, the DCMI Usage Board is seeking a way to express this intention with a formal range declaration."@en .

<http://purl.org/dc/terms/spatial>
        a       <http://www.w3.org/2002/07/owl#ObjectProperty> , <http://www.w3.org/2002/07/owl#AnnotationProperty> ;
        <http://www.w3.org/2000/01/rdf-schema#comment>
                "Spatial characteristics of the resource."@en ;
        <http://www.w3.org/2000/01/rdf-schema#isDefinedBy>
                <http://purl.org/dc/terms/> ;
        <http://www.w3.org/2000/01/rdf-schema#label>
                "Spatial Coverage"@en ;
        <http://www.w3.org/2000/01/rdf-schema#range>
                <http://purl.org/dc/terms/Location> ;
        <http://www.w3.org/2000/01/rdf-schema#subPropertyOf>
                <http://purl.org/dc/terms/coverage> , <http://purl.org/dc/elements/1.1/coverage> ;
        <http://purl.org/dc/terms/hasVersion>
                <http://dublincore.org/usage/terms/history/#spatial-003> ;
        <http://purl.org/dc/terms/issued>
                "2000-07-11"^^<http://www.w3.org/2001/XMLSchema#date> ;
        <http://purl.org/dc/terms/modified>
                "2008-01-14"^^<http://www.w3.org/2001/XMLSchema#date> .

<http://purl.org/dc/terms/accrualPeriodicity>
        a       <http://www.w3.org/2002/07/owl#ObjectProperty> , <http://www.w3.org/2002/07/owl#AnnotationProperty> ;
        <http://www.w3.org/2000/01/rdf-schema#comment>
                "The frequency with which items are added to a collection."@en ;
        <http://www.w3.org/2000/01/rdf-schema#domain>
                <http://purl.org/dc/dcmitype/Collection> ;
        <http://www.w3.org/2000/01/rdf-schema#isDefinedBy>
                <http://purl.org/dc/terms/> ;
        <http://www.w3.org/2000/01/rdf-schema#label>
                "Accrual Periodicity"@en ;
        <http://www.w3.org/2000/01/rdf-schema#range>
                <http://purl.org/dc/terms/Frequency> ;
        <http://purl.org/dc/terms/hasVersion>
                <http://dublincore.org/usage/terms/history/#accrualPeriodicity-003> ;
        <http://purl.org/dc/terms/issued>
                "2005-06-13"^^<http://www.w3.org/2001/XMLSchema#date> ;
        <http://purl.org/dc/terms/modified>
                "2010-10-11"^^<http://www.w3.org/2001/XMLSchema#date> .

<http://www.demcare.eu/ontologies/demlab.owl#dynamicBalance>
        a       <http://www.w3.org/2002/07/owl#DatatypeProperty> ;
        <http://www.w3.org/2000/01/rdf-schema#comment>
                "Dynamical balance during the walking (e.g., people trajectory study)"@en ;
        <http://www.w3.org/2000/01/rdf-schema#domain>
                <http://www.demcare.eu/ontologies/demlab.owl#GaitData> ;
        <http://www.w3.org/2000/01/rdf-schema#seeAlso>
                <http://www.demcare.eu/ontologies/demlab.owl#GaitData> .

<http://www.demcare.eu/ontologies/demlab.owl#DirectedTask>
        a       <http://www.w3.org/2002/07/owl#Class> ;
        <http://www.w3.org/2000/01/rdf-schema#comment>
                "Root concept for grouping the Tasks relevant to the DirectedActivitiesStep"@en ;
        <http://www.w3.org/2000/01/rdf-schema#seeAlso>
                <http://www.demcare.eu/ontologies/demlab.owl#DirectedActivitiesStep> , <http://www.demcare.eu/ontologies/demlab.owl#Task> ;
        <http://www.w3.org/2000/01/rdf-schema#subClassOf>
                <http://www.demcare.eu/ontologies/demlab.owl#Task> .

<http://purl.org/dc/terms/Policy>
        a       <http://www.w3.org/2002/07/owl#Class> ;
        <http://www.w3.org/2000/01/rdf-schema#comment>
                "A plan or course of action by an authority, intended to influence and determine decisions, actions, and other matters."@en ;
        <http://www.w3.org/2000/01/rdf-schema#isDefinedBy>
                <http://purl.org/dc/terms/> ;
        <http://www.w3.org/2000/01/rdf-schema#label>
                "Policy"@en ;
        <http://purl.org/dc/terms/hasVersion>
                <http://dublincore.org/usage/terms/history/#Policy-001> ;
        <http://purl.org/dc/terms/issued>
                "2008-01-14"^^<http://www.w3.org/2001/XMLSchema#date> .

<http://www.demcare.eu/ontologies/demlab.owl#LatencyData>
        a       <http://www.w3.org/2002/07/owl#Class> ;
        <http://www.w3.org/2000/01/rdf-schema#comment>
                "Explore the time of latency [stimulation, response] during the DirectedActivitiesTask (Explore sensitivity of this measure for assessing the apathy)"@en ;
        <http://www.w3.org/2000/01/rdf-schema#subClassOf>
                <http://www.demcare.eu/ontologies/demlab.owl#MeasuredData> ;
        <http://www.w3.org/2000/01/rdf-schema#subClassOf>
                [ a       <http://www.w3.org/2002/07/owl#Restriction> ;
                  <http://www.w3.org/2002/07/owl#cardinality>
                          "1"^^<http://www.w3.org/2001/XMLSchema#nonNegativeInteger> ;
                  <http://www.w3.org/2002/07/owl#onProperty>
                          <http://www.demcare.eu/ontologies/demlab.owl#latency>
                ] .

<http://purl.org/dc/terms/LCSH>
        a       <http://purl.org/dc/dcam/VocabularyEncodingScheme> , <http://www.w3.org/2002/07/owl#NamedIndividual> ;
        <http://www.w3.org/2000/01/rdf-schema#comment>
                "The set of labeled concepts specified by the Library of Congress Subject Headings."@en ;
        <http://www.w3.org/2000/01/rdf-schema#isDefinedBy>
                <http://purl.org/dc/terms/> ;
        <http://www.w3.org/2000/01/rdf-schema#label>
                "LCSH"@en ;
        <http://purl.org/dc/terms/hasVersion>
                <http://dublincore.org/usage/terms/history/#LCSH-003> ;
        <http://purl.org/dc/terms/issued>
                "2000-07-11"^^<http://www.w3.org/2001/XMLSchema#date> ;
        <http://purl.org/dc/terms/modified>
                "2008-01-14"^^<http://www.w3.org/2001/XMLSchema#date> .

<http://purl.org/dc/terms/UDC>
        a       <http://www.w3.org/2002/07/owl#NamedIndividual> , <http://purl.org/dc/dcam/VocabularyEncodingScheme> ;
        <http://www.w3.org/2000/01/rdf-schema#comment>
                "The set of conceptual resources specified by the Universal Decimal Classification."@en ;
        <http://www.w3.org/2000/01/rdf-schema#isDefinedBy>
                <http://purl.org/dc/terms/> ;
        <http://www.w3.org/2000/01/rdf-schema#label>
                "UDC"@en ;
        <http://www.w3.org/2000/01/rdf-schema#seeAlso>
                <http://www.udcc.org/> ;
        <http://purl.org/dc/terms/hasVersion>
                <http://dublincore.org/usage/terms/history/#UDC-003> ;
        <http://purl.org/dc/terms/issued>
                "2000-07-11"^^<http://www.w3.org/2001/XMLSchema#date> ;
        <http://purl.org/dc/terms/modified>
                "2008-01-14"^^<http://www.w3.org/2001/XMLSchema#date> .

<http://www.demcare.eu/ontologies/demlab.owl#omitted>
        a       <http://www.w3.org/2002/07/owl#NamedIndividual> , <http://www.demcare.eu/ontologies/demlab.owl#ActivityStatusType> .

<http://www.demcare.eu/ontologies/demlab.owl#DiagnosisAssessment>
        a       <http://www.w3.org/2002/07/owl#Class> ;
        <http://www.w3.org/2000/01/rdf-schema#comment>
                "Diagnosis established the day of the recording session. Participant is assigned to one of this 3 categories: Healthy Control participants, Alzheimer’s disease at pre-dementia stage, Alzheimer ’s disease at dementia stage"@en ;
        <http://www.w3.org/2000/01/rdf-schema#seeAlso>
                <http://www.demcare.eu/ontologies/demlab.owl#PersonWithPredementia> , <http://www.demcare.eu/ontologies/demlab.owl#hasClinicalDiagnosis> , <http://www.demcare.eu/ontologies/demlab.owl#PersonWithDementia> , <http://www.demcare.eu/ontologies/demlab.owl#DiagnosisType> , <http://www.demcare.eu/ontologies/demlab.owl#HealthyControlParticipant> ;
        <http://www.w3.org/2000/01/rdf-schema#subClassOf>
                <http://www.demcare.eu/ontologies/demlab.owl#ClinicalAssessment> ;
        <http://www.w3.org/2000/01/rdf-schema#subClassOf>
                [ a       <http://www.w3.org/2002/07/owl#Restriction> ;
                  <http://www.w3.org/2002/07/owl#onClass>
                          <http://www.demcare.eu/ontologies/demlab.owl#DiagnosisType> ;
                  <http://www.w3.org/2002/07/owl#onProperty>
                          <http://www.demcare.eu/ontologies/demlab.owl#hasClinicalDiagnosis> ;
                  <http://www.w3.org/2002/07/owl#qualifiedCardinality>
                          "1"^^<http://www.w3.org/2001/XMLSchema#nonNegativeInteger>
                ] .

<http://purl.org/dc/terms/MediaType>
        a       <http://www.w3.org/2002/07/owl#Class> ;
        <http://www.w3.org/2000/01/rdf-schema#comment>
                "A file format or physical medium."@en ;
        <http://www.w3.org/2000/01/rdf-schema#isDefinedBy>
                <http://purl.org/dc/terms/> ;
        <http://www.w3.org/2000/01/rdf-schema#label>
                "Media Type"@en ;
        <http://www.w3.org/2000/01/rdf-schema#subClassOf>
                <http://purl.org/dc/terms/MediaTypeOrExtent> ;
        <http://purl.org/dc/terms/hasVersion>
                <http://dublincore.org/usage/terms/history/#MediaType-001> ;
        <http://purl.org/dc/terms/issued>
                "2008-01-14"^^<http://www.w3.org/2001/XMLSchema#date> .

<http://www.demcare.eu/ontologies/demlab.owl#DirectedActivitiesStep>
        a       <http://www.w3.org/2002/07/owl#Class> ;
        <http://www.w3.org/2000/01/rdf-schema#comment>
                "This ProtocolStep is conducted by a clinician, who details step by step the different activities to do by the participant. This step involves five Tasks. The tasks Walking, CountingBackwards and WalkingAndCountingBackwards are used for characterizing participants’ gait in mono and dual tasks, and the impact of cognitive activity on gait (e.g., walking speed, step length, stops during the walking exercise done in dual task). The tasks SentenceRepeating and ArticulationControl are vocally-directed tasks: one task consists of repeating a sentence after the clinician (this task is repeated with three sentences), and the other is an articulation control exercise done to evaluate the neuromuscular mechanism of speech production."@en ;
        <http://www.w3.org/2000/01/rdf-schema#subClassOf>
                <http://www.demcare.eu/ontologies/demlab.owl#ProtocolStep> ;
        <http://www.w3.org/2000/01/rdf-schema#subClassOf>
                [ a       <http://www.w3.org/2002/07/owl#Restriction> ;
                  <http://www.w3.org/2002/07/owl#allValuesFrom>
                          [ a       <http://www.w3.org/2002/07/owl#Class> ;
                            <http://www.w3.org/2002/07/owl#unionOf>
                                    ( <http://www.demcare.eu/ontologies/demlab.owl#ArticulationControlTask> <http://www.demcare.eu/ontologies/demlab.owl#CountingBackwardsTask> <http://www.demcare.eu/ontologies/demlab.owl#SentenceRepeatingTask> <http://www.demcare.eu/ontologies/demlab.owl#Task> <http://www.demcare.eu/ontologies/demlab.owl#WalkingCountingBackwardsTask> <http://www.demcare.eu/ontologies/demlab.owl#WalkingTask> )
                          ] ;
                  <http://www.w3.org/2002/07/owl#onProperty>
                          <http://www.demcare.eu/ontologies/demlab.owl#involvesTask>
                ] .

<http://purl.org/dc/terms/coverage>
        a       <http://www.w3.org/2002/07/owl#AnnotationProperty> , <http://www.w3.org/2002/07/owl#ObjectProperty> ;
        <http://www.w3.org/2000/01/rdf-schema#comment>
                "The spatial or temporal topic of the resource, the spatial applicability of the resource, or the jurisdiction under which the resource is relevant."@en ;
        <http://www.w3.org/2000/01/rdf-schema#isDefinedBy>
                <http://purl.org/dc/terms/> ;
        <http://www.w3.org/2000/01/rdf-schema#label>
                "Coverage"@en ;
        <http://www.w3.org/2000/01/rdf-schema#range>
                <http://purl.org/dc/terms/LocationPeriodOrJurisdiction> ;
        <http://www.w3.org/2000/01/rdf-schema#subPropertyOf>
                <http://purl.org/dc/elements/1.1/coverage> ;
        <http://purl.org/dc/terms/description>
                "Spatial topic and spatial applicability may be a named place or a location specified by its geographic coordinates. Temporal topic may be a named period, date, or date range. A jurisdiction may be a named administrative entity or a geographic place to which the resource applies. Recommended best practice is to use a controlled vocabulary such as the Thesaurus of Geographic Names [TGN]. Where appropriate, named places or time periods can be used in preference to numeric identifiers such as sets of coordinates or date ranges."@en ;
        <http://purl.org/dc/terms/hasVersion>
                <http://dublincore.org/usage/terms/history/#coverageT-001> ;
        <http://purl.org/dc/terms/issued>
                "2008-01-14"^^<http://www.w3.org/2001/XMLSchema#date> ;
        <http://purl.org/dc/terms/modified>
                "2008-01-14"^^<http://www.w3.org/2001/XMLSchema#date> .

<http://purl.org/dc/terms/provenance>
        a       <http://www.w3.org/2002/07/owl#ObjectProperty> ;
        <http://www.w3.org/2000/01/rdf-schema#comment>
                "A statement of any changes in ownership and custody of the resource since its creation that are significant for its authenticity, integrity, and interpretation."@en ;
        <http://www.w3.org/2000/01/rdf-schema#isDefinedBy>
                <http://purl.org/dc/terms/> ;
        <http://www.w3.org/2000/01/rdf-schema#label>
                "Provenance"@en ;
        <http://www.w3.org/2000/01/rdf-schema#range>
                <http://purl.org/dc/terms/ProvenanceStatement> ;
        <http://purl.org/dc/terms/description>
                "The statement may include a description of any changes successive custodians made to the resource."@en ;
        <http://purl.org/dc/terms/hasVersion>
                <http://dublincore.org/usage/terms/history/#provenance-002> ;
        <http://purl.org/dc/terms/issued>
                "2004-09-20"^^<http://www.w3.org/2001/XMLSchema#date> ;
        <http://purl.org/dc/terms/modified>
                "2008-01-14"^^<http://www.w3.org/2001/XMLSchema#date> .

<http://purl.org/dc/terms/isPartOf>
        a       <http://www.w3.org/2002/07/owl#AnnotationProperty> ;
        <http://www.w3.org/2000/01/rdf-schema#comment>
                "A related resource in which the described resource is physically or logically included."@en ;
        <http://www.w3.org/2000/01/rdf-schema#isDefinedBy>
                <http://purl.org/dc/terms/> ;
        <http://www.w3.org/2000/01/rdf-schema#label>
                "Is Part Of"@en ;
        <http://www.w3.org/2000/01/rdf-schema#subPropertyOf>
                <http://purl.org/dc/elements/1.1/relation> , <http://purl.org/dc/terms/relation> ;
        <http://purl.org/dc/terms/hasVersion>
                <http://dublincore.org/usage/terms/history/#isPartOf-003> ;
        <http://purl.org/dc/terms/issued>
                "2000-07-11"^^<http://www.w3.org/2001/XMLSchema#date> ;
        <http://purl.org/dc/terms/modified>
                "2008-01-14"^^<http://www.w3.org/2001/XMLSchema#date> ;
        <http://www.w3.org/2004/02/skos/core#note>
                "This term is intended to be used with non-literal values as defined in the DCMI Abstract Model (http://dublincore.org/documents/abstract-model/).  As of December 2007, the DCMI Usage Board is seeking a way to express this intention with a formal range declaration."@en .

<http://purl.org/dc/terms/subject>
        a       <http://www.w3.org/2002/07/owl#AnnotationProperty> ;
        <http://www.w3.org/2000/01/rdf-schema#comment>
                "The topic of the resource."@en ;
        <http://www.w3.org/2000/01/rdf-schema#isDefinedBy>
                <http://purl.org/dc/terms/> ;
        <http://www.w3.org/2000/01/rdf-schema#label>
                "Subject"@en ;
        <http://www.w3.org/2000/01/rdf-schema#subPropertyOf>
                <http://purl.org/dc/elements/1.1/subject> ;
        <http://purl.org/dc/terms/description>
                "Typically, the subject will be represented using keywords, key phrases, or classification codes. Recommended best practice is to use a controlled vocabulary."@en ;
        <http://purl.org/dc/terms/hasVersion>
                <http://dublincore.org/usage/terms/history/#subjectT-002> ;
        <http://purl.org/dc/terms/issued>
                "2008-01-14"^^<http://www.w3.org/2001/XMLSchema#date> ;
        <http://purl.org/dc/terms/modified>
                "2012-06-14"^^<http://www.w3.org/2001/XMLSchema#date> ;
        <http://www.w3.org/2004/02/skos/core#note>
                "This term is intended to be used with non-literal values as defined in the DCMI Abstract Model (http://dublincore.org/documents/abstract-model/).  As of December 2007, the DCMI Usage Board is seeking a way to express this intention with a formal range declaration."@en .

<http://www.demcare.eu/ontologies/demlab.owl#DiscussionInvolvementData>
        a       <http://www.w3.org/2002/07/owl#Class> ;
        <http://www.w3.org/2000/01/rdf-schema#comment>
                "- Assessment of the impact of cognitive load imposed by the picture description task on speech fluency\n- Memory and self-appraisal assessment\n- Verbal fluency and mood (Apathy) assessment"@en ;
        <http://www.w3.org/2000/01/rdf-schema#subClassOf>
                <http://www.demcare.eu/ontologies/demlab.owl#MeasuredData> ;
        <http://www.w3.org/2000/01/rdf-schema#subClassOf>
                [ a       <http://www.w3.org/2002/07/owl#Restriction> ;
                  <http://www.w3.org/2002/07/owl#cardinality>
                          "1"^^<http://www.w3.org/2001/XMLSchema#nonNegativeInteger> ;
                  <http://www.w3.org/2002/07/owl#onProperty>
                          <http://www.demcare.eu/ontologies/demlab.owl#verbalReactionSpontaneity>
                ] .

<http://www.demcare.eu/ontologies/demlab.owl#hasParticipant>
        a       <http://www.w3.org/2002/07/owl#ObjectProperty> ;
        <http://www.w3.org/2000/01/rdf-schema#comment>
                "The participant of the protocol"@en ;
        <http://www.w3.org/2000/01/rdf-schema#domain>
                <http://www.demcare.eu/ontologies/demlab.owl#Protocol> ;
        <http://www.w3.org/2000/01/rdf-schema#range>
                <http://www.demcare.eu/ontologies/demlab.owl#Participant> ;
        <http://www.w3.org/2000/01/rdf-schema#seeAlso>
                <http://www.demcare.eu/ontologies/demlab.owl#Protocol> , <http://www.demcare.eu/ontologies/demlab.owl#Person> .

<http://www.demcare.eu/ontologies/demlab.owl#areasOfNoInterestExplored>
        a       <http://www.w3.org/2002/07/owl#ObjectProperty> ;
        <http://www.w3.org/2000/01/rdf-schema#comment>
                "Zones of interest"@en ;
        <http://www.w3.org/2000/01/rdf-schema#domain>
                <http://www.demcare.eu/ontologies/demlab.owl#OrganisationEfficiencyData> ;
        <http://www.w3.org/2000/01/rdf-schema#range>
                <http://www.demcare.eu/ontologies/demlab.owl#Zone> ;
        <http://www.w3.org/2000/01/rdf-schema#seeAlso>
                <http://www.demcare.eu/ontologies/demlab.owl#OrganisationEfficiencyData> .

<http://www.demcare.eu/ontologies/demlab.owl#latency>
        a       <http://www.w3.org/2002/07/owl#DatatypeProperty> ;
        <http://www.w3.org/2000/01/rdf-schema#comment>
                "Time of latency between the end of instructions (stimulation) and the beginning of the task"@en ;
        <http://www.w3.org/2000/01/rdf-schema#domain>
                <http://www.demcare.eu/ontologies/demlab.owl#LatencyData> ;
        <http://www.w3.org/2000/01/rdf-schema#seeAlso>
                <http://www.demcare.eu/ontologies/demlab.owl#LatencyData> .

<http://www.demcare.eu/ontologies/demlab.owl#distanceWalked>
        a       <http://www.w3.org/2002/07/owl#DatatypeProperty> ;
        <http://www.w3.org/2000/01/rdf-schema#comment>
                "Total distance walked"@en ;
        <http://www.w3.org/2000/01/rdf-schema#domain>
                <http://www.demcare.eu/ontologies/demlab.owl#OrganisationEfficiencyData> ;
        <http://www.w3.org/2000/01/rdf-schema#seeAlso>
                <http://www.demcare.eu/ontologies/demlab.owl#OrganisationEfficiencyData> .

<http://purl.org/dc/terms/RightsStatement>
        a       <http://www.w3.org/2002/07/owl#Class> ;
        <http://www.w3.org/2000/01/rdf-schema#comment>
                "A statement about the intellectual property rights (IPR) held in or over a Resource, a legal document giving official permission to do something with a resource, or a statement about access rights."@en ;
        <http://www.w3.org/2000/01/rdf-schema#isDefinedBy>
                <http://purl.org/dc/terms/> ;
        <http://www.w3.org/2000/01/rdf-schema#label>
                "Rights Statement"@en ;
        <http://purl.org/dc/terms/hasVersion>
                <http://dublincore.org/usage/terms/history/#RightsStatement-001> ;
        <http://purl.org/dc/terms/issued>
                "2008-01-14"^^<http://www.w3.org/2001/XMLSchema#date> .

<http://www.demcare.eu/ontologies/demlab.owl#PictureDiscussionTask>
        a       <http://www.w3.org/2002/07/owl#Class> ;
        <http://www.w3.org/2000/01/rdf-schema#comment>
                "The clinician asks if the participant likes doing this activity and why"@en ;
        <http://www.w3.org/2000/01/rdf-schema#subClassOf>
                <http://www.demcare.eu/ontologies/demlab.owl#FreeDiscussionTask> .

<http://purl.org/dc/terms/ISO3166>
        a       <http://www.w3.org/2000/01/rdf-schema#Datatype> ;
        <http://www.w3.org/2000/01/rdf-schema#comment>
                "The set of codes listed in ISO 3166-1 for the representation of names of countries."@en ;
        <http://www.w3.org/2000/01/rdf-schema#isDefinedBy>
                <http://purl.org/dc/terms/> ;
        <http://www.w3.org/2000/01/rdf-schema#label>
                "ISO 3166"@en ;
        <http://www.w3.org/2000/01/rdf-schema#seeAlso>
                <http://www.iso.org/iso/en/prods-services/iso3166ma/02iso-3166-code-lists/list-en1.html> ;
        <http://purl.org/dc/terms/hasVersion>
                <http://dublincore.org/usage/terms/history/#ISO3166-004> ;
        <http://purl.org/dc/terms/issued>
                "2000-07-11"^^<http://www.w3.org/2001/XMLSchema#date> ;
        <http://purl.org/dc/terms/modified>
                "2008-01-14"^^<http://www.w3.org/2001/XMLSchema#date> .

<http://www.demcare.eu/ontologies/demlab.owl#DirectedExpressionTask>
        a       <http://www.w3.org/2002/07/owl#Class> ;
        <http://www.w3.org/2000/01/rdf-schema#comment>
                "The clinician asks the same questions than the ones asked on the read article, e.g. What is the topic of the article?"@en ;
        <http://www.w3.org/2000/01/rdf-schema#subClassOf>
                <http://www.demcare.eu/ontologies/demlab.owl#DirectedDiscussionTask> .

<http://purl.org/dc/terms/medium>
        a       <http://www.w3.org/2002/07/owl#AnnotationProperty> , <http://www.w3.org/2002/07/owl#ObjectProperty> ;
        <http://www.w3.org/2000/01/rdf-schema#comment>
                "The material or physical carrier of the resource."@en ;
        <http://www.w3.org/2000/01/rdf-schema#domain>
                <http://purl.org/dc/terms/PhysicalResource> ;
        <http://www.w3.org/2000/01/rdf-schema#isDefinedBy>
                <http://purl.org/dc/terms/> ;
        <http://www.w3.org/2000/01/rdf-schema#label>
                "Medium"@en ;
        <http://www.w3.org/2000/01/rdf-schema#range>
                <http://purl.org/dc/terms/PhysicalMedium> ;
        <http://www.w3.org/2000/01/rdf-schema#subPropertyOf>
                <http://purl.org/dc/terms/format> , <http://purl.org/dc/elements/1.1/format> ;
        <http://purl.org/dc/terms/hasVersion>
                <http://dublincore.org/usage/terms/history/#medium-003> ;
        <http://purl.org/dc/terms/issued>
                "2000-07-11"^^<http://www.w3.org/2001/XMLSchema#date> ;
        <http://purl.org/dc/terms/modified>
                "2008-01-14"^^<http://www.w3.org/2001/XMLSchema#date> .

<http://www.demcare.eu/ontologies/demlab.owl#ClinicalRecord>
        a       <http://www.w3.org/2002/07/owl#Class> ;
        <http://www.w3.org/2000/01/rdf-schema#comment>
                "A ClinicalRecord contains information about the five types of clinical assessment"@en ;
        <http://www.w3.org/2000/01/rdf-schema#seeAlso>
                <http://www.demcare.eu/ontologies/demlab.owl#ClinicalAssessment> , <http://www.demcare.eu/ontologies/demlab.owl#containsAssessment> ;
        <http://www.w3.org/2000/01/rdf-schema#subClassOf>
                [ a       <http://www.w3.org/2002/07/owl#Restriction> ;
                  <http://www.w3.org/2002/07/owl#onClass>
                          <http://www.demcare.eu/ontologies/demlab.owl#Participant> ;
                  <http://www.w3.org/2002/07/owl#onProperty>
                          <http://www.demcare.eu/ontologies/demlab.owl#isClinicalRecordOf> ;
                  <http://www.w3.org/2002/07/owl#qualifiedCardinality>
                          "1"^^<http://www.w3.org/2001/XMLSchema#nonNegativeInteger>
                ] ;
        <http://www.w3.org/2000/01/rdf-schema#subClassOf>
                [ a       <http://www.w3.org/2002/07/owl#Restriction> ;
                  <http://www.w3.org/2002/07/owl#allValuesFrom>
                          [ a       <http://www.w3.org/2002/07/owl#Class> ;
                            <http://www.w3.org/2002/07/owl#unionOf>
                                    ( <http://www.demcare.eu/ontologies/demlab.owl#AutonomyAssessment> <http://www.demcare.eu/ontologies/demlab.owl#CognitiveAbilitiesAssessment> <http://www.demcare.eu/ontologies/demlab.owl#DiagnosisAssessment> <http://www.demcare.eu/ontologies/demlab.owl#MotricityAbilitiesAssessment> <http://www.demcare.eu/ontologies/demlab.owl#NeuropsychiatricAndMoodAssessment> )
                          ] ;
                  <http://www.w3.org/2002/07/owl#onProperty>
                          <http://www.demcare.eu/ontologies/demlab.owl#containsAssessment>
                ] .

<http://www.demcare.eu/ontologies/demlab.owl#MotricityAbilitiesAssessment>
        a       <http://www.w3.org/2002/07/owl#Class> ;
        <http://www.w3.org/2000/01/rdf-schema#comment>
                "Motricity abilities assessment:\n- Part III of the Unified Parkinson’s Disease Rating Scale (UPDRS) ."@en ;
        <http://www.w3.org/2000/01/rdf-schema#seeAlso>
                <http://www.demcare.eu/ontologies/demlab.owl#hasUPDRSScore> ;
        <http://www.w3.org/2000/01/rdf-schema#subClassOf>
                <http://www.demcare.eu/ontologies/demlab.owl#ClinicalAssessment> ;
        <http://www.w3.org/2000/01/rdf-schema#subClassOf>
                [ a       <http://www.w3.org/2002/07/owl#Restriction> ;
                  <http://www.w3.org/2002/07/owl#onDataRange>
                          <http://www.w3.org/2001/XMLSchema#int> ;
                  <http://www.w3.org/2002/07/owl#onProperty>
                          <http://www.demcare.eu/ontologies/demlab.owl#hasUPDRSScore> ;
                  <http://www.w3.org/2002/07/owl#qualifiedCardinality>
                          "1"^^<http://www.w3.org/2001/XMLSchema#nonNegativeInteger>
                ] .

<http://purl.org/dc/terms/PhysicalResource>
        a       <http://www.w3.org/2002/07/owl#Class> ;
        <http://www.w3.org/2000/01/rdf-schema#comment>
                "A material thing."@en ;
        <http://www.w3.org/2000/01/rdf-schema#isDefinedBy>
                <http://purl.org/dc/terms/> ;
        <http://www.w3.org/2000/01/rdf-schema#label>
                "Physical Resource"@en ;
        <http://purl.org/dc/terms/hasVersion>
                <http://dublincore.org/usage/terms/history/#PhysicalResource-001> ;
        <http://purl.org/dc/terms/issued>
                "2008-01-14"^^<http://www.w3.org/2001/XMLSchema#date> .

<http://purl.org/dc/terms/MediaTypeOrExtent>
        a       <http://www.w3.org/2002/07/owl#Class> ;
        <http://www.w3.org/2000/01/rdf-schema#comment>
                "A media type or extent."@en ;
        <http://www.w3.org/2000/01/rdf-schema#isDefinedBy>
                <http://purl.org/dc/terms/> ;
        <http://www.w3.org/2000/01/rdf-schema#label>
                "Media Type or Extent"@en ;
        <http://purl.org/dc/terms/hasVersion>
                <http://dublincore.org/usage/terms/history/#MediaTypeOrExtent-001> ;
        <http://purl.org/dc/terms/issued>
                "2008-01-14"^^<http://www.w3.org/2001/XMLSchema#date> .

<http://www.demcare.eu/ontologies/demlab.owl#participates>
        a       <http://www.w3.org/2002/07/owl#ObjectProperty> ;
        <http://www.w3.org/2000/01/rdf-schema#seeAlso>
                <http://www.demcare.eu/ontologies/demlab.owl#hasParticipant> ;
        <http://www.w3.org/2002/07/owl#inverseOf>
                <http://www.demcare.eu/ontologies/demlab.owl#hasParticipant> .

<http://www.demcare.eu/ontologies/demlab.owl#SemiDirectedTask>
        a       <http://www.w3.org/2002/07/owl#Class> ;
        <http://www.w3.org/2000/01/rdf-schema#comment>
                "In this Task the participant has to organize himself/herself and correctly perform a list of Instrumental Activities of Daily Living (e.g., managing finance, using phone, preparing tea) within a timeframe of 15minutes.\n\nThe relevant tasks are used for assessing:\n- Cognitive abilities through activity repetitions, missed activities, order of activities\n- Functional abilities for the completion of specific activities: e.g. hand trajectories\n- Stress level"@en ;
        <http://www.w3.org/2000/01/rdf-schema#subClassOf>
                <http://www.demcare.eu/ontologies/demlab.owl#Task> ;
        <http://www.w3.org/2000/01/rdf-schema#subClassOf>
                [ a       <http://www.w3.org/2002/07/owl#Restriction> ;
                  <http://www.w3.org/2002/07/owl#allValuesFrom>
                          [ a       <http://www.w3.org/2002/07/owl#Class> ;
                            <http://www.w3.org/2002/07/owl#unionOf>
                                    ( <http://www.demcare.eu/ontologies/demlab.owl#CognitiveAbilitiesData> <http://www.demcare.eu/ontologies/demlab.owl#FunctionalAbilitiesData> <http://www.demcare.eu/ontologies/demlab.owl#StressData> )
                          ] ;
                  <http://www.w3.org/2002/07/owl#onProperty>
                          <http://www.demcare.eu/ontologies/demlab.owl#measuredData>
                ] .

<http://purl.org/dc/terms/isVersionOf>
        a       <http://www.w3.org/2002/07/owl#AnnotationProperty> ;
        <http://www.w3.org/2000/01/rdf-schema#comment>
                "A related resource of which the described resource is a version, edition, or adaptation."@en ;
        <http://www.w3.org/2000/01/rdf-schema#isDefinedBy>
                <http://purl.org/dc/terms/> ;
        <http://www.w3.org/2000/01/rdf-schema#label>
                "Is Version Of"@en ;
        <http://www.w3.org/2000/01/rdf-schema#subPropertyOf>
                <http://purl.org/dc/terms/relation> , <http://purl.org/dc/elements/1.1/relation> ;
        <http://purl.org/dc/terms/description>
                "Changes in version imply substantive changes in content rather than differences in format."@en ;
        <http://purl.org/dc/terms/hasVersion>
                <http://dublincore.org/usage/terms/history/#isVersionOf-003> ;
        <http://purl.org/dc/terms/issued>
                "2000-07-11"^^<http://www.w3.org/2001/XMLSchema#date> ;
        <http://purl.org/dc/terms/modified>
                "2008-01-14"^^<http://www.w3.org/2001/XMLSchema#date> ;
        <http://www.w3.org/2004/02/skos/core#note>
                "This term is intended to be used with non-literal values as defined in the DCMI Abstract Model (http://dublincore.org/documents/abstract-model/).  As of December 2007, the DCMI Usage Board is seeking a way to express this intention with a formal range declaration."@en .

<http://purl.org/dc/elements/1.1/language>
        a       <http://www.w3.org/2002/07/owl#AnnotationProperty> .

<http://www.demcare.eu/ontologies/demlab.owl#ActivityStatusType>
        a       <http://www.w3.org/2002/07/owl#Class> ;
        <http://www.w3.org/2002/07/owl#equivalentClass>
                [ a       <http://www.w3.org/2002/07/owl#Class> ;
                  <http://www.w3.org/2002/07/owl#oneOf>
                          ( <http://www.demcare.eu/ontologies/demlab.owl#completed> <http://www.demcare.eu/ontologies/demlab.owl#incomplete> <http://www.demcare.eu/ontologies/demlab.owl#omitted> )
                ] .

<http://purl.org/dc/terms/ISO639-3>
        a       <http://www.w3.org/2000/01/rdf-schema#Datatype> ;
        <http://www.w3.org/2000/01/rdf-schema#comment>
                "The set of three-letter codes listed in ISO 639-3 for the representation of names of languages."@en ;
        <http://www.w3.org/2000/01/rdf-schema#isDefinedBy>
                <http://purl.org/dc/terms/> ;
        <http://www.w3.org/2000/01/rdf-schema#label>
                "ISO 639-3"@en ;
        <http://www.w3.org/2000/01/rdf-schema#seeAlso>
                <http://www.sil.org/iso639-3/> ;
        <http://purl.org/dc/terms/hasVersion>
                <http://dublincore.org/usage/terms/history/#ISO639-3-001> ;
        <http://purl.org/dc/terms/issued>
                "2008-01-14"^^<http://www.w3.org/2001/XMLSchema#date> .

<http://www.demcare.eu/ontologies/demlab.owl#healthy>
        a       <http://www.w3.org/2002/07/owl#NamedIndividual> , <http://www.demcare.eu/ontologies/demlab.owl#DiagnosisType> ;
        <http://www.demcare.eu/ontologies/demlab.owl#hasClinicalDiagnosis>
                <http://www.demcare.eu/ontologies/demlab.owl#dementia> .

<http://purl.org/dc/elements/1.1/contributor>
        a       <http://www.w3.org/2002/07/owl#AnnotationProperty> .

<http://www.demcare.eu/ontologies/demlab.owl#FunctionalAbilitiesData>
        a       <http://www.w3.org/2002/07/owl#Class> ;
        <http://www.w3.org/2000/01/rdf-schema#comment>
                "Explore functional abilities for the completion of specific activities"@en ;
        <http://www.w3.org/2000/01/rdf-schema#subClassOf>
                <http://www.demcare.eu/ontologies/demlab.owl#MeasuredData> ;
        <http://www.w3.org/2000/01/rdf-schema#subClassOf>
                [ a       <http://www.w3.org/2002/07/owl#Restriction> ;
                  <http://www.w3.org/2002/07/owl#onClass>
                          <http://www.demcare.eu/ontologies/demlab.owl#HandTrajectoryType> ;
                  <http://www.w3.org/2002/07/owl#onProperty>
                          <http://www.demcare.eu/ontologies/demlab.owl#handTrajectory> ;
                  <http://www.w3.org/2002/07/owl#qualifiedCardinality>
                          "1"^^<http://www.w3.org/2001/XMLSchema#nonNegativeInteger>
                ] .

<http://purl.org/dc/terms/format>
        a       <http://www.w3.org/2002/07/owl#ObjectProperty> , <http://www.w3.org/2002/07/owl#AnnotationProperty> ;
        <http://www.w3.org/2000/01/rdf-schema#comment>
                "The file format, physical medium, or dimensions of the resource."@en ;
        <http://www.w3.org/2000/01/rdf-schema#isDefinedBy>
                <http://purl.org/dc/terms/> ;
        <http://www.w3.org/2000/01/rdf-schema#label>
                "Format"@en ;
        <http://www.w3.org/2000/01/rdf-schema#range>
                <http://purl.org/dc/terms/MediaTypeOrExtent> ;
        <http://www.w3.org/2000/01/rdf-schema#subPropertyOf>
                <http://purl.org/dc/elements/1.1/format> ;
        <http://purl.org/dc/terms/description>
                "Examples of dimensions include size and duration. Recommended best practice is to use a controlled vocabulary such as the list of Internet Media Types [MIME]."@en ;
        <http://purl.org/dc/terms/hasVersion>
                <http://dublincore.org/usage/terms/history/#formatT-001> ;
        <http://purl.org/dc/terms/issued>
                "2008-01-14"^^<http://www.w3.org/2001/XMLSchema#date> ;
        <http://purl.org/dc/terms/modified>
                "2008-01-14"^^<http://www.w3.org/2001/XMLSchema#date> .

<http://www.demcare.eu/ontologies/demlab.owl#PictureDescriptionTask>
        a       <http://www.w3.org/2002/07/owl#Class> ;
        <http://www.w3.org/2000/01/rdf-schema#comment>
                "The clinician shows to the participant one picture representing daily activity and asks the participants to give a verbal description of the picture in a few sentences"@en ;
        <http://www.w3.org/2000/01/rdf-schema#subClassOf>
                <http://www.demcare.eu/ontologies/demlab.owl#FreeDiscussionTask> .

<http://www.iti.gr/iti/people/Georgios_Meditskos.html#gmeditsk>
        a       <http://xmlns.com/foaf/0.1/Person> ;
        <http://xmlns.com/foaf/0.1/homepage>
                <http://www.iti.gr/iti/people/Georgios_Meditskos.html> ;
        <http://xmlns.com/foaf/0.1/name>
                "Georgios Meditskos" .

<http://purl.org/dc/terms/Frequency>
        a       <http://www.w3.org/2002/07/owl#Class> ;
        <http://www.w3.org/2000/01/rdf-schema#comment>
                "A rate at which something recurs."@en ;
        <http://www.w3.org/2000/01/rdf-schema#isDefinedBy>
                <http://purl.org/dc/terms/> ;
        <http://www.w3.org/2000/01/rdf-schema#label>
                "Frequency"@en ;
        <http://purl.org/dc/terms/hasVersion>
                <http://dublincore.org/usage/terms/history/#Frequency-001> ;
        <http://purl.org/dc/terms/issued>
                "2008-01-14"^^<http://www.w3.org/2001/XMLSchema#date> .

<http://purl.org/dc/terms/dateAccepted>
        a       <http://www.w3.org/2002/07/owl#DatatypeProperty> , <http://www.w3.org/2002/07/owl#AnnotationProperty> ;
        <http://www.w3.org/2000/01/rdf-schema#comment>
                "Date of acceptance of the resource."@en ;
        <http://www.w3.org/2000/01/rdf-schema#isDefinedBy>
                <http://purl.org/dc/terms/> ;
        <http://www.w3.org/2000/01/rdf-schema#label>
                "Date Accepted"@en ;
        <http://www.w3.org/2000/01/rdf-schema#range>
                <http://www.w3.org/2000/01/rdf-schema#Literal> ;
        <http://www.w3.org/2000/01/rdf-schema#subPropertyOf>
                <http://purl.org/dc/elements/1.1/date> , <http://purl.org/dc/terms/date> ;
        <http://purl.org/dc/terms/description>
                "Examples of resources to which a Date Accepted may be relevant are a thesis (accepted by a university department) or an article (accepted by a journal)."@en ;
        <http://purl.org/dc/terms/hasVersion>
                <http://dublincore.org/usage/terms/history/#dateAccepted-002> ;
        <http://purl.org/dc/terms/issued>
                "2002-07-13"^^<http://www.w3.org/2001/XMLSchema#date> ;
        <http://purl.org/dc/terms/modified>
                "2008-01-14"^^<http://www.w3.org/2001/XMLSchema#date> .

<http://purl.org/dc/terms/TGN>
        a       <http://www.w3.org/2002/07/owl#NamedIndividual> , <http://purl.org/dc/dcam/VocabularyEncodingScheme> ;
        <http://www.w3.org/2000/01/rdf-schema#comment>
                "The set of places specified by the Getty Thesaurus of Geographic Names."@en ;
        <http://www.w3.org/2000/01/rdf-schema#isDefinedBy>
                <http://purl.org/dc/terms/> ;
        <http://www.w3.org/2000/01/rdf-schema#label>
                "TGN"@en ;
        <http://www.w3.org/2000/01/rdf-schema#seeAlso>
                <http://www.getty.edu/research/tools/vocabulary/tgn/index.html> ;
        <http://purl.org/dc/terms/hasVersion>
                <http://dublincore.org/usage/terms/history/#TGN-003> ;
        <http://purl.org/dc/terms/issued>
                "2000-07-11"^^<http://www.w3.org/2001/XMLSchema#date> ;
        <http://purl.org/dc/terms/modified>
                "2008-01-14"^^<http://www.w3.org/2001/XMLSchema#date> .

<http://purl.org/dc/terms/title>
        a       <http://www.w3.org/2002/07/owl#DatatypeProperty> , <http://www.w3.org/2002/07/owl#AnnotationProperty> ;
        <http://www.w3.org/2000/01/rdf-schema#comment>
                "A name given to the resource."@en ;
        <http://www.w3.org/2000/01/rdf-schema#isDefinedBy>
                <http://purl.org/dc/terms/> ;
        <http://www.w3.org/2000/01/rdf-schema#label>
                "Title"@en ;
        <http://www.w3.org/2000/01/rdf-schema#range>
                <http://www.w3.org/2000/01/rdf-schema#Literal> ;
        <http://www.w3.org/2000/01/rdf-schema#subPropertyOf>
                <http://purl.org/dc/elements/1.1/title> ;
        <http://purl.org/dc/terms/hasVersion>
                <http://dublincore.org/usage/terms/history/#titleT-002> ;
        <http://purl.org/dc/terms/issued>
                "2008-01-14"^^<http://www.w3.org/2001/XMLSchema#date> ;
        <http://purl.org/dc/terms/modified>
                "2010-10-11"^^<http://www.w3.org/2001/XMLSchema#date> .

<http://purl.org/dc/terms/isReplacedBy>
        a       <http://www.w3.org/2002/07/owl#AnnotationProperty> ;
        <http://www.w3.org/2000/01/rdf-schema#comment>
                "A related resource that supplants, displaces, or supersedes the described resource."@en ;
        <http://www.w3.org/2000/01/rdf-schema#isDefinedBy>
                <http://purl.org/dc/terms/> ;
        <http://www.w3.org/2000/01/rdf-schema#label>
                "Is Replaced By"@en ;
        <http://www.w3.org/2000/01/rdf-schema#subPropertyOf>
                <http://purl.org/dc/terms/relation> , <http://purl.org/dc/elements/1.1/relation> ;
        <http://purl.org/dc/terms/hasVersion>
                <http://dublincore.org/usage/terms/history/#isReplacedBy-003> ;
        <http://purl.org/dc/terms/issued>
                "2000-07-11"^^<http://www.w3.org/2001/XMLSchema#date> ;
        <http://purl.org/dc/terms/modified>
                "2008-01-14"^^<http://www.w3.org/2001/XMLSchema#date> ;
        <http://www.w3.org/2004/02/skos/core#note>
                "This term is intended to be used with non-literal values as defined in the DCMI Abstract Model (http://dublincore.org/documents/abstract-model/).  As of December 2007, the DCMI Usage Board is seeking a way to express this intention with a formal range declaration."@en .

<http://purl.org/dc/terms/mediator>
        a       <http://www.w3.org/2002/07/owl#AnnotationProperty> , <http://www.w3.org/2002/07/owl#ObjectProperty> ;
        <http://www.w3.org/2000/01/rdf-schema#comment>
                "An entity that mediates access to the resource and for whom the resource is intended or useful."@en ;
        <http://www.w3.org/2000/01/rdf-schema#isDefinedBy>
                <http://purl.org/dc/terms/> ;
        <http://www.w3.org/2000/01/rdf-schema#label>
                "Mediator"@en ;
        <http://www.w3.org/2000/01/rdf-schema#range>
                <http://purl.org/dc/terms/AgentClass> ;
        <http://www.w3.org/2000/01/rdf-schema#subPropertyOf>
                <http://purl.org/dc/terms/audience> ;
        <http://purl.org/dc/terms/description>
                "In an educational context, a mediator might be a parent, teacher, teaching assistant, or care-giver."@en ;
        <http://purl.org/dc/terms/hasVersion>
                <http://dublincore.org/usage/terms/history/#mediator-003> ;
        <http://purl.org/dc/terms/issued>
                "2001-05-21"^^<http://www.w3.org/2001/XMLSchema#date> ;
        <http://purl.org/dc/terms/modified>
                "2008-01-14"^^<http://www.w3.org/2001/XMLSchema#date> .

<http://purl.org/dc/terms/PeriodOfTime>
        a       <http://www.w3.org/2002/07/owl#Class> ;
        <http://www.w3.org/2000/01/rdf-schema#comment>
                "An interval of time that is named or defined by its start and end dates."@en ;
        <http://www.w3.org/2000/01/rdf-schema#isDefinedBy>
                <http://purl.org/dc/terms/> ;
        <http://www.w3.org/2000/01/rdf-schema#label>
                "Period of Time"@en ;
        <http://www.w3.org/2000/01/rdf-schema#subClassOf>
                <http://purl.org/dc/terms/LocationPeriodOrJurisdiction> ;
        <http://purl.org/dc/terms/hasVersion>
                <http://dublincore.org/usage/terms/history/#PeriodOfTime-001> ;
        <http://purl.org/dc/terms/issued>
                "2008-01-14"^^<http://www.w3.org/2001/XMLSchema#date> .

<http://www.demcare.eu/ontologies/demlab.owl#vowelDuration>
        a       <http://www.w3.org/2002/07/owl#DatatypeProperty> ;
        <http://www.w3.org/2000/01/rdf-schema#comment>
                <http://www.demcare.eu/ontologies/demlab.owl#VoiceData> ;
        <http://www.w3.org/2000/01/rdf-schema#domain>
                <http://www.demcare.eu/ontologies/demlab.owl#VoiceData> ;
        <http://www.w3.org/2000/01/rdf-schema#seeAlso>
                "Vowel duration"@en ;
        <http://www.w3.org/2000/01/rdf-schema#subPropertyOf>
                <http://www.w3.org/2002/07/owl#topDataProperty> .

<http://purl.org/vocab/vann/preferredNamespacePrefix>
        a       <http://www.w3.org/2002/07/owl#AnnotationProperty> .

<http://purl.org/dc/terms/identifier>
        a       <http://www.w3.org/2002/07/owl#DatatypeProperty> , <http://www.w3.org/2002/07/owl#AnnotationProperty> ;
        <http://www.w3.org/2000/01/rdf-schema#comment>
                "An unambiguous reference to the resource within a given context."@en ;
        <http://www.w3.org/2000/01/rdf-schema#isDefinedBy>
                <http://purl.org/dc/terms/> ;
        <http://www.w3.org/2000/01/rdf-schema#label>
                "Identifier"@en ;
        <http://www.w3.org/2000/01/rdf-schema#range>
                <http://www.w3.org/2000/01/rdf-schema#Literal> ;
        <http://www.w3.org/2000/01/rdf-schema#subPropertyOf>
                <http://purl.org/dc/elements/1.1/identifier> ;
        <http://purl.org/dc/terms/description>
                "Recommended best practice is to identify the resource by means of a string conforming to a formal identification system. "@en ;
        <http://purl.org/dc/terms/hasVersion>
                <http://dublincore.org/usage/terms/history/#identifierT-001> ;
        <http://purl.org/dc/terms/issued>
                "2008-01-14"^^<http://www.w3.org/2001/XMLSchema#date> ;
        <http://purl.org/dc/terms/modified>
                "2008-01-14"^^<http://www.w3.org/2001/XMLSchema#date> .

<http://www.demcare.eu/ontologies/demlab.owl#npi>
        a       <http://www.w3.org/2002/07/owl#DatatypeProperty> ;
        <http://www.w3.org/2000/01/rdf-schema#comment>
                "Neuropsychiatric Inventory"@en ;
        <http://www.w3.org/2000/01/rdf-schema#domain>
                <http://www.demcare.eu/ontologies/demlab.owl#NeuropsychiatricAndMoodAssessment> ;
        <http://www.w3.org/2000/01/rdf-schema#seeAlso>
                <http://www.demcare.eu/ontologies/demlab.owl#NeuropsychiatricAndMoodAssessment> .

<http://purl.org/dc/terms/accrualMethod>
        a       <http://www.w3.org/2002/07/owl#ObjectProperty> , <http://www.w3.org/2002/07/owl#AnnotationProperty> ;
        <http://www.w3.org/2000/01/rdf-schema#comment>
                "The method by which items are added to a collection."@en ;
        <http://www.w3.org/2000/01/rdf-schema#domain>
                <http://purl.org/dc/dcmitype/Collection> ;
        <http://www.w3.org/2000/01/rdf-schema#isDefinedBy>
                <http://purl.org/dc/terms/> ;
        <http://www.w3.org/2000/01/rdf-schema#label>
                "Accrual Method"@en ;
        <http://www.w3.org/2000/01/rdf-schema#range>
                <http://purl.org/dc/terms/MethodOfAccrual> ;
        <http://purl.org/dc/terms/hasVersion>
                <http://dublincore.org/usage/terms/history/#accrualMethod-003> ;
        <http://purl.org/dc/terms/issued>
                "2005-06-13"^^<http://www.w3.org/2001/XMLSchema#date> ;
        <http://purl.org/dc/terms/modified>
                "2010-10-11"^^<http://www.w3.org/2001/XMLSchema#date> .

<http://www.demcare.eu/ontologies/demlab.owl#PayBillTask>
        a       <http://www.w3.org/2002/07/owl#Class> ;
        <http://www.w3.org/2000/01/rdf-schema#comment>
                "- Three bills (Electricity/Gaz/Phone) are proposed. The participant has to pay the phone bill by check. \n- The check is well completed if the amount, order (i.e. Phone Company), date and signature are right."@en ;
        <http://www.w3.org/2000/01/rdf-schema#subClassOf>
                <http://www.demcare.eu/ontologies/demlab.owl#SemiDirectedTask> .

<http://purl.org/dc/terms/extent>
        a       <http://www.w3.org/2002/07/owl#ObjectProperty> , <http://www.w3.org/2002/07/owl#AnnotationProperty> ;
        <http://www.w3.org/2000/01/rdf-schema#comment>
                "The size or duration of the resource."@en ;
        <http://www.w3.org/2000/01/rdf-schema#isDefinedBy>
                <http://purl.org/dc/terms/> ;
        <http://www.w3.org/2000/01/rdf-schema#label>
                "Extent"@en ;
        <http://www.w3.org/2000/01/rdf-schema#range>
                <http://purl.org/dc/terms/SizeOrDuration> ;
        <http://www.w3.org/2000/01/rdf-schema#subPropertyOf>
                <http://purl.org/dc/elements/1.1/format> , <http://purl.org/dc/terms/format> ;
        <http://purl.org/dc/terms/hasVersion>
                <http://dublincore.org/usage/terms/history/#extent-003> ;
        <http://purl.org/dc/terms/issued>
                "2000-07-11"^^<http://www.w3.org/2001/XMLSchema#date> ;
        <http://purl.org/dc/terms/modified>
                "2008-01-14"^^<http://www.w3.org/2001/XMLSchema#date> .

<http://purl.org/dc/terms/LinguisticSystem>
        a       <http://www.w3.org/2002/07/owl#Class> ;
        <http://www.w3.org/2000/01/rdf-schema#comment>
                "A system of signs, symbols, sounds, gestures, or rules used in communication."@en ;
        <http://www.w3.org/2000/01/rdf-schema#isDefinedBy>
                <http://purl.org/dc/terms/> ;
        <http://www.w3.org/2000/01/rdf-schema#label>
                "Linguistic System"@en ;
        <http://purl.org/dc/terms/description>
                "Examples include written, spoken, sign, and computer languages."@en ;
        <http://purl.org/dc/terms/hasVersion>
                <http://dublincore.org/usage/terms/history/#LinguisticSystem-001> ;
        <http://purl.org/dc/terms/issued>
                "2008-01-14"^^<http://www.w3.org/2001/XMLSchema#date> .

<http://purl.org/dc/terms/>
        <http://purl.org/dc/terms/modified>
                "2012-06-14"^^<http://www.w3.org/2001/XMLSchema#date> ;
        <http://purl.org/dc/terms/publisher>
                <http://purl.org/dc/aboutdcmi#DCMI> ;
        <http://purl.org/dc/terms/title>
                "DCMI Metadata Terms - other"@en .

<http://purl.org/dc/terms/abstract>
        a       <http://www.w3.org/2002/07/owl#AnnotationProperty> ;
        <http://www.w3.org/2000/01/rdf-schema#comment>
                "A summary of the resource."@en ;
        <http://www.w3.org/2000/01/rdf-schema#isDefinedBy>
                <http://purl.org/dc/terms/> ;
        <http://www.w3.org/2000/01/rdf-schema#label>
                "Abstract"@en ;
        <http://www.w3.org/2000/01/rdf-schema#subPropertyOf>
                <http://purl.org/dc/elements/1.1/description> , <http://purl.org/dc/terms/description> ;
        <http://purl.org/dc/terms/hasVersion>
                <http://dublincore.org/usage/terms/history/#abstract-003> ;
        <http://purl.org/dc/terms/issued>
                "2000-07-11"^^<http://www.w3.org/2001/XMLSchema#date> ;
        <http://purl.org/dc/terms/modified>
                "2008-01-14"^^<http://www.w3.org/2001/XMLSchema#date> .

<http://purl.org/dc/terms/LocationPeriodOrJurisdiction>
        a       <http://www.w3.org/2002/07/owl#Class> ;
        <http://www.w3.org/2000/01/rdf-schema#comment>
                "A location, period of time, or jurisdiction."@en ;
        <http://www.w3.org/2000/01/rdf-schema#isDefinedBy>
                <http://purl.org/dc/terms/> ;
        <http://www.w3.org/2000/01/rdf-schema#label>
                "Location, Period, or Jurisdiction"@en ;
        <http://purl.org/dc/terms/hasVersion>
                <http://dublincore.org/usage/terms/history/#LocationPeriodOrJurisdiction-001> ;
        <http://purl.org/dc/terms/issued>
                "2008-01-14"^^<http://www.w3.org/2001/XMLSchema#date> .

<http://purl.org/dc/elements/1.1/subject>
        a       <http://www.w3.org/2002/07/owl#AnnotationProperty> .

<http://www.demcare.eu/ontologies/demlab.owl#areasOfInterestExplored>
        a       <http://www.w3.org/2002/07/owl#ObjectProperty> ;
        <http://www.w3.org/2000/01/rdf-schema#comment>
                "Zones of no interest"@en ;
        <http://www.w3.org/2000/01/rdf-schema#domain>
                <http://www.demcare.eu/ontologies/demlab.owl#OrganisationEfficiencyData> ;
        <http://www.w3.org/2000/01/rdf-schema#range>
                <http://www.demcare.eu/ontologies/demlab.owl#Zone> ;
        <http://www.w3.org/2000/01/rdf-schema#seeAlso>
                <http://www.demcare.eu/ontologies/demlab.owl#OrganisationEfficiencyData> .

<http://www.demcare.eu/ontologies/demlab.owl#AnswerPhoneTask>
        a       <http://www.w3.org/2002/07/owl#Class> ;
        <http://www.w3.org/2000/01/rdf-schema#comment>
                "- The phone is scheduled to ring 10 minutes after the entering of the participant inside the room. \n- During this task, the clinician explains that there is a mistake on the phone bill: the amount was wrong. Consequently, it is expected that the participant corrects his/her phone check and corrects the account balance (tasks normally established before the phone call according to the constraint)."@en ;
        <http://www.w3.org/2000/01/rdf-schema#subClassOf>
                <http://www.demcare.eu/ontologies/demlab.owl#SemiDirectedTask> .

<http://www.demcare.eu/ontologies/demlab.owl#VoiceData>
        a       <http://www.w3.org/2002/07/owl#Class> ;
        <http://www.w3.org/2000/01/rdf-schema#comment>
                "- Vocal biomarkers extraction for cognitive load assessment\n- Assessment of mutual influence of cognitive activities an motor activities\n- Assessment of the verbal reaction time and the impact of cognitive load imposed by the sentence recall task on speech fluency\n- Assessment of the level of the participants’ control over the neuromuscular mechanism of speech production"@en ;
        <http://www.w3.org/2000/01/rdf-schema#subClassOf>
                <http://www.demcare.eu/ontologies/demlab.owl#MeasuredData> ;
        <http://www.w3.org/2000/01/rdf-schema#subClassOf>
                [ a       <http://www.w3.org/2002/07/owl#Restriction> ;
                  <http://www.w3.org/2002/07/owl#cardinality>
                          "1"^^<http://www.w3.org/2001/XMLSchema#nonNegativeInteger> ;
                  <http://www.w3.org/2002/07/owl#onProperty>
                          <http://www.demcare.eu/ontologies/demlab.owl#vowelDuration>
                ] ;
        <http://www.w3.org/2000/01/rdf-schema#subClassOf>
                [ a       <http://www.w3.org/2002/07/owl#Restriction> ;
                  <http://www.w3.org/2002/07/owl#cardinality>
                          "1"^^<http://www.w3.org/2001/XMLSchema#nonNegativeInteger> ;
                  <http://www.w3.org/2002/07/owl#onProperty>
                          <http://www.demcare.eu/ontologies/demlab.owl#speechFluency>
                ] ;
        <http://www.w3.org/2000/01/rdf-schema#subClassOf>
                [ a       <http://www.w3.org/2002/07/owl#Restriction> ;
                  <http://www.w3.org/2002/07/owl#cardinality>
                          "1"^^<http://www.w3.org/2001/XMLSchema#nonNegativeInteger> ;
                  <http://www.w3.org/2002/07/owl#onProperty>
                          <http://www.demcare.eu/ontologies/demlab.owl#pauseRate>
                ] ;
        <http://www.w3.org/2000/01/rdf-schema#subClassOf>
                [ a       <http://www.w3.org/2002/07/owl#Restriction> ;
                  <http://www.w3.org/2002/07/owl#cardinality>
                          "1"^^<http://www.w3.org/2001/XMLSchema#nonNegativeInteger> ;
                  <http://www.w3.org/2002/07/owl#onProperty>
                          <http://www.demcare.eu/ontologies/demlab.owl#speechRate>
                ] ;
        <http://www.w3.org/2000/01/rdf-schema#subClassOf>
                [ a       <http://www.w3.org/2002/07/owl#Restriction> ;
                  <http://www.w3.org/2002/07/owl#cardinality>
                          "1"^^<http://www.w3.org/2001/XMLSchema#nonNegativeInteger> ;
                  <http://www.w3.org/2002/07/owl#onProperty>
                          <http://www.demcare.eu/ontologies/demlab.owl#verbalReactionTime>
                ] ;
        <http://www.w3.org/2000/01/rdf-schema#subClassOf>
                [ a       <http://www.w3.org/2002/07/owl#Restriction> ;
                  <http://www.w3.org/2002/07/owl#cardinality>
                          "1"^^<http://www.w3.org/2001/XMLSchema#nonNegativeInteger> ;
                  <http://www.w3.org/2002/07/owl#onProperty>
                          <http://www.demcare.eu/ontologies/demlab.owl#articulation>
                ] .

<http://purl.org/dc/terms/DDC>
        a       <http://www.w3.org/2002/07/owl#NamedIndividual> , <http://purl.org/dc/dcam/VocabularyEncodingScheme> ;
        <http://www.w3.org/2000/01/rdf-schema#comment>
                "The set of conceptual resources specified by the Dewey Decimal Classification."@en ;
        <http://www.w3.org/2000/01/rdf-schema#isDefinedBy>
                <http://purl.org/dc/terms/> ;
        <http://www.w3.org/2000/01/rdf-schema#label>
                "DDC"@en ;
        <http://www.w3.org/2000/01/rdf-schema#seeAlso>
                <http://www.oclc.org/dewey/> ;
        <http://purl.org/dc/terms/hasVersion>
                <http://dublincore.org/usage/terms/history/#DDC-003> ;
        <http://purl.org/dc/terms/issued>
                "2000-07-11"^^<http://www.w3.org/2001/XMLSchema#date> ;
        <http://purl.org/dc/terms/modified>
                "2008-01-14"^^<http://www.w3.org/2001/XMLSchema#date> .

<http://www.demcare.eu/ontologies/demlab.owl#CognitiveAbilitiesAssessment>
        a       <http://www.w3.org/2002/07/owl#Class> ;
        <http://www.w3.org/2000/01/rdf-schema#comment>
                "The Cognitive abilities assessment is performed in terms of five scores:\n- Mini-Mental State Exam (MMSE). \n- Frontal Assessment Battery (FAB). \n- Trail making test A and B. \n- Short Cognitive Battery. \n- The Free and Cued Selective Reminding Test"@en ;
        <http://www.w3.org/2000/01/rdf-schema#seeAlso>
                <http://www.demcare.eu/ontologies/demlab.owl#fabScore> , <http://www.demcare.eu/ontologies/demlab.owl#freeAndCuedRemindingAssessment> , <http://www.demcare.eu/ontologies/demlab.owl#hasMMSEScore> , <http://www.demcare.eu/ontologies/demlab.owl#shortCognitiveBatteryAssessment> , <http://www.demcare.eu/ontologies/demlab.owl#trailMakingTest> ;
        <http://www.w3.org/2000/01/rdf-schema#subClassOf>
                <http://www.demcare.eu/ontologies/demlab.owl#ClinicalAssessment> ;
        <http://www.w3.org/2000/01/rdf-schema#subClassOf>
                [ a       <http://www.w3.org/2002/07/owl#Restriction> ;
                  <http://www.w3.org/2002/07/owl#cardinality>
                          "1"^^<http://www.w3.org/2001/XMLSchema#nonNegativeInteger> ;
                  <http://www.w3.org/2002/07/owl#onProperty>
                          <http://www.demcare.eu/ontologies/demlab.owl#trailMakingTest>
                ] ;
        <http://www.w3.org/2000/01/rdf-schema#subClassOf>
                [ a       <http://www.w3.org/2002/07/owl#Restriction> ;
                  <http://www.w3.org/2002/07/owl#cardinality>
                          "1"^^<http://www.w3.org/2001/XMLSchema#nonNegativeInteger> ;
                  <http://www.w3.org/2002/07/owl#onProperty>
                          <http://www.demcare.eu/ontologies/demlab.owl#fabScore>
                ] ;
        <http://www.w3.org/2000/01/rdf-schema#subClassOf>
                [ a       <http://www.w3.org/2002/07/owl#Restriction> ;
                  <http://www.w3.org/2002/07/owl#cardinality>
                          "1"^^<http://www.w3.org/2001/XMLSchema#nonNegativeInteger> ;
                  <http://www.w3.org/2002/07/owl#onProperty>
                          <http://www.demcare.eu/ontologies/demlab.owl#freeAndCuedRemindingAssessment>
                ] ;
        <http://www.w3.org/2000/01/rdf-schema#subClassOf>
                [ a       <http://www.w3.org/2002/07/owl#Restriction> ;
                  <http://www.w3.org/2002/07/owl#cardinality>
                          "1"^^<http://www.w3.org/2001/XMLSchema#nonNegativeInteger> ;
                  <http://www.w3.org/2002/07/owl#onProperty>
                          <http://www.demcare.eu/ontologies/demlab.owl#shortCognitiveBatteryAssessment>
                ] ;
        <http://www.w3.org/2000/01/rdf-schema#subClassOf>
                [ a       <http://www.w3.org/2002/07/owl#Restriction> ;
                  <http://www.w3.org/2002/07/owl#cardinality>
                          "1"^^<http://www.w3.org/2001/XMLSchema#nonNegativeInteger> ;
                  <http://www.w3.org/2002/07/owl#onProperty>
                          <http://www.demcare.eu/ontologies/demlab.owl#hasMMSEScore>
                ] .

<http://www.demcare.eu/ontologies/demlab.owl#FreeDiscussionTask>
        a       <http://www.w3.org/2002/07/owl#Class> ;
        <http://www.w3.org/2000/01/rdf-schema#subClassOf>
                <http://www.demcare.eu/ontologies/demlab.owl#DiscussionTask> .

<http://www.demcare.eu/ontologies/demlab.owl#EstablishAccountBalanceTask>
        a       <http://www.w3.org/2002/07/owl#Class> ;
        <http://www.w3.org/2000/01/rdf-schema#comment>
                "- Three bills (Electricity/Gaz/Phone) are proposed. The account balance is given. \n- The participant has to establish the amount balance after having taken into account the three bills."@en ;
        <http://www.w3.org/2000/01/rdf-schema#subClassOf>
                <http://www.demcare.eu/ontologies/demlab.owl#SemiDirectedTask> .

<http://www.demcare.eu/ontologies/demlab.owl#hasClinicalRecord>
        a       <http://www.w3.org/2002/07/owl#ObjectProperty> ;
        <http://www.w3.org/2000/01/rdf-schema#comment>
                "Each participant is associated with a clinical record"@en ;
        <http://www.w3.org/2000/01/rdf-schema#domain>
                <http://www.demcare.eu/ontologies/demlab.owl#Participant> ;
        <http://www.w3.org/2000/01/rdf-schema#range>
                <http://www.demcare.eu/ontologies/demlab.owl#ClinicalRecord> ;
        <http://www.w3.org/2000/01/rdf-schema#seeAlso>
                <http://www.demcare.eu/ontologies/demlab.owl#ClinicalRecord> .

<http://www.demcare.eu/ontologies/demlab.owl#Participant>
        a       <http://www.w3.org/2002/07/owl#Class> ;
        <http://www.w3.org/2000/01/rdf-schema#subClassOf>
                <http://xmlns.com/foaf/0.1/Person> ;
        <http://www.w3.org/2000/01/rdf-schema#subClassOf>
                [ a       <http://www.w3.org/2002/07/owl#Restriction> ;
                  <http://www.w3.org/2002/07/owl#onClass>
                          <http://www.demcare.eu/ontologies/demlab.owl#ClinicalRecord> ;
                  <http://www.w3.org/2002/07/owl#onProperty>
                          <http://www.demcare.eu/ontologies/demlab.owl#hasClinicalRecord> ;
                  <http://www.w3.org/2002/07/owl#qualifiedCardinality>
                          "1"^^<http://www.w3.org/2001/XMLSchema#nonNegativeInteger>
                ] ;
        <http://www.w3.org/2000/01/rdf-schema#subClassOf>
                [ a       <http://www.w3.org/2002/07/owl#Restriction> ;
                  <http://www.w3.org/2002/07/owl#onProperty>
                          <http://www.demcare.eu/ontologies/demlab.owl#participates> ;
                  <http://www.w3.org/2002/07/owl#someValuesFrom>
                          <http://www.demcare.eu/ontologies/demlab.owl#Protocol>
                ] .

<http://www.demcare.eu/ontologies/demlab.owl#CountingBackwardsTask>
        a       <http://www.w3.org/2002/07/owl#Class> ;
        <http://www.w3.org/2000/01/rdf-schema#comment>
                "(MonoTask) The participant is standing and the clinician asks him/her to count aloud backwards: \n- From 305 to 285 (to change tens and hundreds) one by one; or \n- From 20 to 0 if they make counting mistakes after 2 attempts of the previous backwards counting\n\nThis task is used for assessing:\n- Latency: time of latency between the end of instructions (stimulation) and the beginning of the task\n- Stress level\n- Voice: e.g. speech fluency and articulation"@en ;
        <http://www.w3.org/2000/01/rdf-schema#subClassOf>
                <http://www.demcare.eu/ontologies/demlab.owl#DirectedTask> ;
        <http://www.w3.org/2000/01/rdf-schema#subClassOf>
                [ a       <http://www.w3.org/2002/07/owl#Restriction> ;
                  <http://www.w3.org/2002/07/owl#allValuesFrom>
                          [ a       <http://www.w3.org/2002/07/owl#Class> ;
                            <http://www.w3.org/2002/07/owl#unionOf>
                                    ( <http://www.demcare.eu/ontologies/demlab.owl#LatencyData> <http://www.demcare.eu/ontologies/demlab.owl#StressData> <http://www.demcare.eu/ontologies/demlab.owl#VoiceData> )
                          ] ;
                  <http://www.w3.org/2002/07/owl#onProperty>
                          <http://www.demcare.eu/ontologies/demlab.owl#measuredData>
                ] .

<http://www.demcare.eu/ontologies/demlab.owl#hasMMSEScore>
        a       <http://www.w3.org/2002/07/owl#DatatypeProperty> ;
        <http://www.w3.org/2000/01/rdf-schema#comment>
                "Mini-Mental State Exam score"@en ;
        <http://www.w3.org/2000/01/rdf-schema#domain>
                <http://www.demcare.eu/ontologies/demlab.owl#CognitiveAbilitiesAssessment> ;
        <http://www.w3.org/2000/01/rdf-schema#seeAlso>
                <http://www.demcare.eu/ontologies/demlab.owl#CognitiveAbilitiesAssessment> .

<http://www.demcare.eu/ontologies/demlab.owl#TurnOnTVTask>
        a       <http://www.w3.org/2002/07/owl#Class> ;
        <http://www.w3.org/2000/01/rdf-schema#comment>
                "The TV is turn off. The participant has to take the remote control and turns on the TV"@en ;
        <http://www.w3.org/2000/01/rdf-schema#subClassOf>
                <http://www.demcare.eu/ontologies/demlab.owl#SemiDirectedTask> .

<http://purl.org/dc/terms/rightsHolder>
        a       <http://www.w3.org/2002/07/owl#ObjectProperty> ;
        <http://www.w3.org/2000/01/rdf-schema#comment>
                "A person or organization owning or managing rights over the resource."@en ;
        <http://www.w3.org/2000/01/rdf-schema#isDefinedBy>
                <http://purl.org/dc/terms/> ;
        <http://www.w3.org/2000/01/rdf-schema#label>
                "Rights Holder"@en ;
        <http://www.w3.org/2000/01/rdf-schema#range>
                <http://purl.org/dc/terms/Agent> ;
        <http://purl.org/dc/terms/hasVersion>
                <http://dublincore.org/usage/terms/history/#rightsHolder-002> ;
        <http://purl.org/dc/terms/issued>
                "2004-06-14"^^<http://www.w3.org/2001/XMLSchema#date> ;
        <http://purl.org/dc/terms/modified>
                "2008-01-14"^^<http://www.w3.org/2001/XMLSchema#date> .

<http://www.demcare.eu/ontologies/demlab.owl#walkingSpeedInstantaneous>
        a       <http://www.w3.org/2002/07/owl#DatatypeProperty> ;
        <http://www.w3.org/2000/01/rdf-schema#comment>
                "Walking speed instantaneous (mono task walking activity/dual task)"@en ;
        <http://www.w3.org/2000/01/rdf-schema#domain>
                <http://www.demcare.eu/ontologies/demlab.owl#GaitData> ;
        <http://www.w3.org/2000/01/rdf-schema#seeAlso>
                <http://www.demcare.eu/ontologies/demlab.owl#GaitData> .

<http://www.demcare.eu/ontologies/demlab.owl#iadl_e>
        a       <http://www.w3.org/2002/07/owl#DatatypeProperty> ;
        <http://www.w3.org/2000/01/rdf-schema#comment>
                "Allows the quantification of autonomy"@en ;
        <http://www.w3.org/2000/01/rdf-schema#domain>
                <http://www.demcare.eu/ontologies/demlab.owl#AutonomyAssessment> ;
        <http://www.w3.org/2000/01/rdf-schema#seeAlso>
                <http://www.demcare.eu/ontologies/demlab.owl#AutonomyAssessment> .

<http://www.demcare.eu/ontologies/demlab.owl#measuredData>
        a       <http://www.w3.org/2002/07/owl#ObjectProperty> ;
        <http://www.w3.org/2000/01/rdf-schema#domain>
                <http://www.demcare.eu/ontologies/demlab.owl#Task> ;
        <http://www.w3.org/2000/01/rdf-schema#range>
                <http://www.demcare.eu/ontologies/demlab.owl#MeasuredData> ;
        <http://www.w3.org/2000/01/rdf-schema#seeAlso>
                "Associates a Task with a MeasuredData instance"@en ;
        <http://www.w3.org/2000/01/rdf-schema#seeAlso>
                <http://www.demcare.eu/ontologies/demlab.owl#Task> , <http://www.demcare.eu/ontologies/demlab.owl#MeasuredData> .

<http://purl.org/dc/terms/MethodOfInstruction>
        a       <http://www.w3.org/2002/07/owl#Class> ;
        <http://www.w3.org/2000/01/rdf-schema#comment>
                "A process that is used to engender knowledge, attitudes, and skills."@en ;
        <http://www.w3.org/2000/01/rdf-schema#isDefinedBy>
                <http://purl.org/dc/terms/> ;
        <http://www.w3.org/2000/01/rdf-schema#label>
                "Method of Instruction"@en ;
        <http://purl.org/dc/terms/hasVersion>
                <http://dublincore.org/usage/terms/history/#MethodOfInstruction-001> ;
        <http://purl.org/dc/terms/issued>
                "2008-01-14"^^<http://www.w3.org/2001/XMLSchema#date> .

<http://purl.org/dc/terms/available>
        a       <http://www.w3.org/2002/07/owl#AnnotationProperty> , <http://www.w3.org/2002/07/owl#DatatypeProperty> ;
        <http://www.w3.org/2000/01/rdf-schema#comment>
                "Date (often a range) that the resource became or will become available."@en ;
        <http://www.w3.org/2000/01/rdf-schema#isDefinedBy>
                <http://purl.org/dc/terms/> ;
        <http://www.w3.org/2000/01/rdf-schema#label>
                "Date Available"@en ;
        <http://www.w3.org/2000/01/rdf-schema#range>
                <http://www.w3.org/2000/01/rdf-schema#Literal> ;
        <http://www.w3.org/2000/01/rdf-schema#subPropertyOf>
                <http://purl.org/dc/terms/date> , <http://purl.org/dc/elements/1.1/date> ;
        <http://purl.org/dc/terms/hasVersion>
                <http://dublincore.org/usage/terms/history/#available-003> ;
        <http://purl.org/dc/terms/issued>
                "2000-07-11"^^<http://www.w3.org/2001/XMLSchema#date> ;
        <http://purl.org/dc/terms/modified>
                "2008-01-14"^^<http://www.w3.org/2001/XMLSchema#date> .

<http://www.demcare.eu/ontologies/demlab.owl#Zone>
        a       <http://www.w3.org/2002/07/owl#Class> ;
        <http://www.w3.org/2000/01/rdf-schema#comment>
                "Allows the definition of zones (areas) of interest, e.g. phone zone"@en .

<http://www.demcare.eu/ontologies/demlab.owl#LeaveRoomTask>
        a       <http://www.w3.org/2002/07/owl#Class> ;
        <http://www.w3.org/2000/01/rdf-schema#comment>
                "The participant has to leave the room when he/she feels that all activities are performed and achieved"@en ;
        <http://www.w3.org/2000/01/rdf-schema#subClassOf>
                <http://www.demcare.eu/ontologies/demlab.owl#SemiDirectedTask> .

<http://www.demcare.eu/ontologies/demlab.owl#fabScore>
        a       <http://www.w3.org/2002/07/owl#DatatypeProperty> ;
        <http://www.w3.org/2000/01/rdf-schema#comment>
                "Frontal Assessment Battery score"@en ;
        <http://www.w3.org/2000/01/rdf-schema#domain>
                <http://www.demcare.eu/ontologies/demlab.owl#CognitiveAbilitiesAssessment> ;
        <http://www.w3.org/2000/01/rdf-schema#seeAlso>
                <http://www.demcare.eu/ontologies/demlab.owl#CognitiveAbilitiesAssessment> .

<http://purl.org/dc/elements/1.1/type>
        a       <http://www.w3.org/2002/07/owl#AnnotationProperty> .

<http://www.demcare.eu/ontologies/demlab.owl#hasProtocolStep>
        a       <http://www.w3.org/2002/07/owl#ObjectProperty> ;
        <http://www.w3.org/2000/01/rdf-schema#comment>
                "Each Protocol consists of one or more ProtocolSteps"@en ;
        <http://www.w3.org/2000/01/rdf-schema#domain>
                <http://www.demcare.eu/ontologies/demlab.owl#Protocol> ;
        <http://www.w3.org/2000/01/rdf-schema#range>
                <http://www.demcare.eu/ontologies/demlab.owl#ProtocolStep> ;
        <http://www.w3.org/2000/01/rdf-schema#seeAlso>
                <http://www.demcare.eu/ontologies/demlab.owl#Protocol> , <http://www.demcare.eu/ontologies/demlab.owl#ProtocolStep> .

<http://www.w3.org/2004/02/skos/core#note>
        a       <http://www.w3.org/2002/07/owl#AnnotationProperty> .

<http://www.demcare.eu/ontologies/demlab.owl#speechRate>
        a       <http://www.w3.org/2002/07/owl#DatatypeProperty> ;
        <http://www.w3.org/2000/01/rdf-schema#comment>
                "Speech fluency during sentence repetition and picture description tasks"@en ;
        <http://www.w3.org/2000/01/rdf-schema#domain>
                <http://www.demcare.eu/ontologies/demlab.owl#VoiceData> ;
        <http://www.w3.org/2000/01/rdf-schema#seeAlso>
                <http://www.demcare.eu/ontologies/demlab.owl#VoiceData> .

<http://www.demcare.eu/ontologies/demlab.owl#DiagnosisType>
        a       <http://www.w3.org/2002/07/owl#Class> ;
        <http://www.w3.org/2002/07/owl#equivalentClass>
                [ a       <http://www.w3.org/2002/07/owl#Class> ;
                  <http://www.w3.org/2002/07/owl#oneOf>
                          ( <http://www.demcare.eu/ontologies/demlab.owl#healthy> <http://www.demcare.eu/ontologies/demlab.owl#dementia> <http://www.demcare.eu/ontologies/demlab.owl#predementia> )
                ] .

<http://www.demcare.eu/ontologies/demlab.owl#shortCognitiveBatteryAssessment>
        a       <http://www.w3.org/2002/07/owl#DatatypeProperty> ;
        <http://www.w3.org/2000/01/rdf-schema#comment>
                "Short Cognitive Battery"@en ;
        <http://www.w3.org/2000/01/rdf-schema#domain>
                <http://www.demcare.eu/ontologies/demlab.owl#CognitiveAbilitiesAssessment> ;
        <http://www.w3.org/2000/01/rdf-schema#seeAlso>
                <http://www.demcare.eu/ontologies/demlab.owl#CognitiveAbilitiesAssessment> .

<http://www.demcare.eu/ontologies/demlab.owl#SentenceRepeatingTask>
        a       <http://www.w3.org/2002/07/owl#Class> ;
        <http://www.w3.org/2000/01/rdf-schema#comment>
                "- The participant is asked to repeat a short sentence after the assessor. \n- The assessor reads aloud a sentence. The participant repeats the sentence. The action is done once by sentence. Three sentences must be repeated.\n\nThis task is used for assessing:\n- Latency: time of latency between the end of instructions (stimulation) and the beginning of the task\n- Stress level\n- Voice: e.g. verbal reaction time"@en ;
        <http://www.w3.org/2000/01/rdf-schema#subClassOf>
                <http://www.demcare.eu/ontologies/demlab.owl#DirectedTask> ;
        <http://www.w3.org/2000/01/rdf-schema#subClassOf>
                [ a       <http://www.w3.org/2002/07/owl#Restriction> ;
                  <http://www.w3.org/2002/07/owl#allValuesFrom>
                          [ a       <http://www.w3.org/2002/07/owl#Class> ;
                            <http://www.w3.org/2002/07/owl#unionOf>
                                    ( <http://www.demcare.eu/ontologies/demlab.owl#LatencyData> <http://www.demcare.eu/ontologies/demlab.owl#StressData> <http://www.demcare.eu/ontologies/demlab.owl#VoiceData> )
                          ] ;
                  <http://www.w3.org/2002/07/owl#onProperty>
                          <http://www.demcare.eu/ontologies/demlab.owl#measuredData>
                ] .

<http://www.demcare.eu/ontologies/demlab.owl#verbalReactionTime>
        a       <http://www.w3.org/2002/07/owl#DatatypeProperty> ;
        <http://www.w3.org/2000/01/rdf-schema#comment>
                "Time interval between the end of assessor’s speech and the beginning of participant’s speech (Sentence Repetition Task)"@en ;
        <http://www.w3.org/2000/01/rdf-schema#domain>
                <http://www.demcare.eu/ontologies/demlab.owl#VoiceData> ;
        <http://www.w3.org/2000/01/rdf-schema#seeAlso>
                <http://www.demcare.eu/ontologies/demlab.owl#VoiceData> .

<http://www.demcare.eu/ontologies/demlab.owl#MeasuredData>
        a       <http://www.w3.org/2002/07/owl#Class> ;
        <http://www.w3.org/2000/01/rdf-schema#comment>
                "MeasuredData is the root concept that groups the measurement types that are collected during the Tasks." .

<http://purl.org/dc/elements/1.1/relation>
        a       <http://www.w3.org/2002/07/owl#AnnotationProperty> .

<http://www.demcare.eu/ontologies/demlab.owl#trailMakingTest>
        a       <http://www.w3.org/2002/07/owl#DatatypeProperty> ;
        <http://www.w3.org/2000/01/rdf-schema#comment>
                "Trail making test A and B"@en ;
        <http://www.w3.org/2000/01/rdf-schema#domain>
                <http://www.demcare.eu/ontologies/demlab.owl#CognitiveAbilitiesAssessment> ;
        <http://www.w3.org/2000/01/rdf-schema#seeAlso>
                <http://www.demcare.eu/ontologies/demlab.owl#CognitiveAbilitiesAssessment> .

<http://www.demcare.eu/ontologies/demlab.owl#CallPsychologistTask>
        a       <http://www.w3.org/2002/07/owl#Class> ;
        <http://www.w3.org/2000/01/rdf-schema#comment>
                "- The participant has to call the psychologist. Two phone numbers are proposed to the participant (1 visit card of the hair dressing,+ 1 visit card of the CHUN with phone number of a psychologist). \n- According the constraint, the participant has to call the psychologist within the 5 first minutes."@en ;
        <http://www.w3.org/2000/01/rdf-schema#subClassOf>
                <http://www.demcare.eu/ontologies/demlab.owl#SemiDirectedTask> .

<http://www.demcare.eu/ontologies/demlab.owl#activityStatus>
        a       <http://www.w3.org/2002/07/owl#ObjectProperty> ;
        <http://www.w3.org/2000/01/rdf-schema#comment>
                "The status of a semi-directed activity" ;
        <http://www.w3.org/2000/01/rdf-schema#domain>
                <http://www.demcare.eu/ontologies/demlab.owl#CognitiveAbilitiesData> ;
        <http://www.w3.org/2000/01/rdf-schema#range>
                <http://www.demcare.eu/ontologies/demlab.owl#ActivityStatusType> ;
        <http://www.w3.org/2000/01/rdf-schema#seeAlso>
                <http://www.demcare.eu/ontologies/demlab.owl#CognitiveAbilitiesData> , <http://www.demcare.eu/ontologies/demlab.owl#ActivityStatusType> .

<http://www.demcare.eu/ontologies/demlab.owl#hasClinicalDiagnosis>
        a       <http://www.w3.org/2002/07/owl#ObjectProperty> ;
        <http://www.w3.org/2000/01/rdf-schema#comment>
                "The value of the DiagnosisAssessment"@en ;
        <http://www.w3.org/2000/01/rdf-schema#domain>
                <http://www.demcare.eu/ontologies/demlab.owl#DiagnosisAssessment> ;
        <http://www.w3.org/2000/01/rdf-schema#range>
                <http://www.demcare.eu/ontologies/demlab.owl#DiagnosisType> ;
        <http://www.w3.org/2000/01/rdf-schema#seeAlso>
                <http://www.demcare.eu/ontologies/demlab.owl#DiagnosisAssessment> , <http://www.demcare.eu/ontologies/demlab.owl#DiagnosisType> ;
        <http://www.w3.org/2000/01/rdf-schema#subPropertyOf>
                <http://www.w3.org/2002/07/owl#topObjectProperty> .

<http://www.demcare.eu/ontologies/demlab.owl#involvesTask>
        a       <http://www.w3.org/2002/07/owl#ObjectProperty> ;
        <http://www.w3.org/2000/01/rdf-schema#comment>
                "Each ProtocolStep involves one or more Tasks"@en ;
        <http://www.w3.org/2000/01/rdf-schema#domain>
                <http://www.demcare.eu/ontologies/demlab.owl#ProtocolStep> ;
        <http://www.w3.org/2000/01/rdf-schema#range>
                <http://www.demcare.eu/ontologies/demlab.owl#Task> ;
        <http://www.w3.org/2000/01/rdf-schema#seeAlso>
                <http://www.demcare.eu/ontologies/demlab.owl#ProtocolStep> , <http://www.demcare.eu/ontologies/demlab.owl#Task> .

<http://purl.org/dc/elements/1.1/creator>
        a       <http://www.w3.org/2002/07/owl#AnnotationProperty> .

<http://purl.org/dc/elements/1.1/format>
        a       <http://www.w3.org/2002/07/owl#AnnotationProperty> .

<http://purl.org/dc/elements/1.1/rights>
        a       <http://www.w3.org/2002/07/owl#AnnotationProperty> .

<http://www.demcare.eu/ontologies/demlab.owl#WaterPlantTask>
        a       <http://www.w3.org/2002/07/owl#Class> ;
        <http://www.w3.org/2000/01/rdf-schema#comment>
                "The participant has to take the water can, and water the plant nearby."@en ;
        <http://www.w3.org/2000/01/rdf-schema#subClassOf>
                <http://www.demcare.eu/ontologies/demlab.owl#SemiDirectedTask> .

<http://www.w3.org/2001/XMLSchema#date>
        a       <http://www.w3.org/2000/01/rdf-schema#Datatype> .

<http://www.demcare.eu/ontologies/demlab.owl#incomplete>
        a       <http://www.w3.org/2002/07/owl#NamedIndividual> , <http://www.demcare.eu/ontologies/demlab.owl#ActivityStatusType> .

<http://www.demcare.eu/ontologies/demlab.owl#isClinicalRecordOf>
        a       <http://www.w3.org/2002/07/owl#ObjectProperty> ;
        <http://www.w3.org/2002/07/owl#inverseOf>
                <http://www.demcare.eu/ontologies/demlab.owl#hasClinicalRecord> .

<http://www.demcare.eu/ontologies/demlab.owl#HandTrajectoryType>
        a       <http://www.w3.org/2002/07/owl#Class> .

<http://purl.org/dc/elements/1.1/source>
        a       <http://www.w3.org/2002/07/owl#AnnotationProperty> .

<http://purl.org/dc/dcam/VocabularyEncodingScheme>
        a       <http://www.w3.org/2002/07/owl#Class> .

<http://purl.org/dc/elements/1.1/coverage>
        a       <http://www.w3.org/2002/07/owl#AnnotationProperty> .

<http://www.demcare.eu/ontologies/demlab.owl#completed>
        a       <http://www.demcare.eu/ontologies/demlab.owl#ActivityStatusType> , <http://www.w3.org/2002/07/owl#NamedIndividual> .
