<http://purl.org/dqm-vocabulary/v1/dqm#TestedClass>
        a       <http://www.w3.org/2002/07/owl#Class> ;
        <http://www.w3.org/2000/01/rdf-schema#comment>
                "A tested class is a class that holds the instances that shall be analyzed for data quality problems."@en ;
        <http://www.w3.org/2000/01/rdf-schema#label>
                "Tested Class"@en ;
        <http://www.w3.org/2000/01/rdf-schema#subClassOf>
                <http://purl.org/dqm-vocabulary/v1/dqm#DataElement> .

<http://purl.org/dqm-vocabulary/v1/dqm#reqSource>
        a       <http://www.w3.org/2002/07/owl#DatatypeProperty> ;
        <http://www.w3.org/2000/01/rdf-schema#comment>
                "Specifies the source of a data requirement."@en ;
        <http://www.w3.org/2000/01/rdf-schema#domain>
                [ a       <http://www.w3.org/2002/07/owl#Class> ;
                  <http://www.w3.org/2002/07/owl#unionOf>
                          ( <http://purl.org/dqm-vocabulary/v1/dqm#DataCleansingRule> <http://purl.org/dqm-vocabulary/v1/dqm#DataRequirement> )
                ] ;
        <http://www.w3.org/2000/01/rdf-schema#label>
                "Requirement Source"@en ;
        <http://www.w3.org/2000/01/rdf-schema#range>
                <http://www.w3.org/2001/XMLSchema#string> ;
        <http://www.w3.org/2000/01/rdf-schema#subPropertyOf>
                <http://purl.org/dqm-vocabulary/v1/dqm#reqMetadata> .

<http://purl.org/dqm-vocabulary/v1/dqm#IllegalValueRule>
        a       <http://www.w3.org/2002/07/owl#Class> ;
        <http://www.w3.org/2000/01/rdf-schema#comment>
                "An illegal value rule is a property requirement that specifies the values that a certain property must not obtain. Illegal value rules, therefore, refer to reference properties that hold all disallowed values."@en ;
        <http://www.w3.org/2000/01/rdf-schema#label>
                "Illegal Value Rule"@en ;
        <http://www.w3.org/2000/01/rdf-schema#subClassOf>
                <http://purl.org/dqm-vocabulary/v1/dqm#PropertyRequirement> .

<http://purl.org/dqm-vocabulary/v1/dqm#hasCondition>
        a       <http://www.w3.org/2002/07/owl#ObjectProperty> ;
        <http://www.w3.org/2000/01/rdf-schema#comment>
                "Connects a conditional rule with a certain condition"@en ;
        <http://www.w3.org/2000/01/rdf-schema#label>
                "Condition"@en ;
        <http://www.w3.org/2000/01/rdf-schema#range>
                <http://purl.org/dqm-vocabulary/v1/dqm#Condition> ;
        <http://www.w3.org/2000/01/rdf-schema#subPropertyOf>
                <http://purl.org/dqm-vocabulary/v1/dqm#dataElementRelationship> .

<http://purl.org/dqm-vocabulary/v1/dqm#FuncDepReferenceRule>
        a       <http://www.w3.org/2002/07/owl#Class> ;
        <http://www.w3.org/2000/01/rdf-schema#comment>
                "A functional dependency reference rule is a multi property requirement that specifies legal value combinations for two or more properties that are allowed to occur within the same instance. Functional dependency reference rules refer to reference properties of classes that hold instances with all allowed value combinations."@en ;
        <http://www.w3.org/2000/01/rdf-schema#label>
                "Functional Dependency Reference Rule"@en ;
        <http://www.w3.org/2000/01/rdf-schema#subClassOf>
                <http://purl.org/dqm-vocabulary/v1/dqm#MatchingValueRule> .

<http://purl.org/dqm-vocabulary/v1/dqm#blacklistClass>
        a       <http://www.w3.org/2002/07/owl#ObjectProperty> , <http://www.w3.org/2002/07/owl#FunctionalProperty> ;
        <http://www.w3.org/2000/01/rdf-schema#comment>
                "A blacklist class holds instances with values that are disallowed for a certain data set."@en ;
        <http://www.w3.org/2000/01/rdf-schema#domain>
                <http://purl.org/dqm-vocabulary/v1/dqm#IllegalValueRule> ;
        <http://www.w3.org/2000/01/rdf-schema#label>
                "Blacklist Class"@en ;
        <http://www.w3.org/2000/01/rdf-schema#range>
                <http://purl.org/dqm-vocabulary/v1/dqm#BlacklistClass> ;
        <http://www.w3.org/2000/01/rdf-schema#subPropertyOf>
                <http://purl.org/dqm-vocabulary/v1/dqm#dataElementRelationship> .

<http://purl.org/dqm-vocabulary/v1/dqm#MultiPropertyCleansingRule>
        a       <http://www.w3.org/2002/07/owl#Class> ;
        <http://www.w3.org/2000/01/rdf-schema#comment>
                "Multi property cleansing rules can be used to cleanse the literal values of two or more dependent properties."@en ;
        <http://www.w3.org/2000/01/rdf-schema#label>
                "Multi Property Cleansing Rule"@en ;
        <http://www.w3.org/2000/01/rdf-schema#subClassOf>
                <http://purl.org/dqm-vocabulary/v1/dqm#DataCleansingRule> .

<http://purl.org/dqm-vocabulary/v1/dqm#unitDescription>
        a       <http://www.w3.org/2002/07/owl#DatatypeProperty> ;
        <http://www.w3.org/2000/01/rdf-schema#comment>
                "Description of a unit of measurement."@en ;
        <http://www.w3.org/2000/01/rdf-schema#domain>
                <http://purl.org/dqm-vocabulary/v1/dqm#Unit> ;
        <http://www.w3.org/2000/01/rdf-schema#label>
                "Unit Description"@en ;
        <http://www.w3.org/2000/01/rdf-schema#range>
                <http://www.w3.org/2001/XMLSchema#string> .

<http://purl.org/dqm-vocabulary/v1/dqm#affectedClass>
        a       <http://www.w3.org/2002/07/owl#ObjectProperty> ;
        <http://www.w3.org/2000/01/rdf-schema#comment>
                "An affected class holds one or more instances with one or more data requirement violations."@en ;
        <http://www.w3.org/2000/01/rdf-schema#domain>
                <http://purl.org/dqm-vocabulary/v1/dqm#DataRequirementViolation> ;
        <http://www.w3.org/2000/01/rdf-schema#label>
                "Affected Class"@en ;
        <http://www.w3.org/2000/01/rdf-schema#range>
                <http://purl.org/dqm-vocabulary/v1/dqm#AffectedClass> ;
        <http://www.w3.org/2000/01/rdf-schema#subPropertyOf>
                <http://purl.org/dqm-vocabulary/v1/dqm#dataElementRelationship> .

<http://purl.org/dqm-vocabulary/v1/dqm#IllegalValueRangeRule>
        a       <http://www.w3.org/2002/07/owl#Class> ;
        <http://www.w3.org/2000/01/rdf-schema#comment>
                "An illegal value range rule is a property requirement that specifies the upper and/or lower boundary of numeric values that a certain property must not obtain."@en ;
        <http://www.w3.org/2000/01/rdf-schema#label>
                "Illegal Value Range Rule"@en ;
        <http://www.w3.org/2000/01/rdf-schema#subClassOf>
                <http://purl.org/dqm-vocabulary/v1/dqm#PropertyRequirement> .

<http://purl.org/dqm-vocabulary/v1/dqm#unitName>
        a       <http://www.w3.org/2002/07/owl#DatatypeProperty> ;
        <http://www.w3.org/2000/01/rdf-schema#comment>
                "Name of a unit of measurement."@en ;
        <http://www.w3.org/2000/01/rdf-schema#domain>
                <http://purl.org/dqm-vocabulary/v1/dqm#Unit> ;
        <http://www.w3.org/2000/01/rdf-schema#label>
                "Unit Name"@en ;
        <http://www.w3.org/2000/01/rdf-schema#range>
                <http://www.w3.org/2001/XMLSchema#string> .

<http://purl.org/dqm-vocabulary/v1/dqm#currentValue>
        a       <http://www.w3.org/2002/07/owl#FunctionalProperty> , <http://www.w3.org/2002/07/owl#DatatypeProperty> ;
        <http://www.w3.org/2000/01/rdf-schema#comment>
                "The current value propertiy specifies the value to be removed."@en ;
        <http://www.w3.org/2000/01/rdf-schema#domain>
                <http://purl.org/dqm-vocabulary/v1/dqm#ValueSubstitution> ;
        <http://www.w3.org/2000/01/rdf-schema#label>
                "Current Value"@en ;
        <http://www.w3.org/2000/01/rdf-schema#range>
                <http://www.w3.org/2001/XMLSchema#string> ;
        <http://www.w3.org/2000/01/rdf-schema#subPropertyOf>
                <http://purl.org/dqm-vocabulary/v1/dqm#cleansingProperty> .

<http://purl.org/dqm-vocabulary/v1/dqm#referenceProperty1>
        a       <http://www.w3.org/2002/07/owl#ObjectProperty> , <http://www.w3.org/2002/07/owl#FunctionalProperty> ;
        <http://www.w3.org/2000/01/rdf-schema#comment>
                "The reference property points to the URI of a property that holds trusted values, i.e. values of high quality"@en ;
        <http://www.w3.org/2000/01/rdf-schema#domain>
                [ a       <http://www.w3.org/2002/07/owl#Class> ;
                  <http://www.w3.org/2002/07/owl#unionOf>
                          ( <http://purl.org/dqm-vocabulary/v1/dqm#FuncDepReferenceRule> <http://purl.org/dqm-vocabulary/v1/dqm#LegalValueRule> )
                ] ;
        <http://www.w3.org/2000/01/rdf-schema#label>
                "Reference Property 1"@en ;
        <http://www.w3.org/2000/01/rdf-schema#subPropertyOf>
                <http://purl.org/dqm-vocabulary/v1/dqm#referenceProperty> .

<http://purl.org/dqm-vocabulary/v1/dqm#MissingElement>
        a       <http://www.w3.org/2002/07/owl#Class> ;
        <http://www.w3.org/2000/01/rdf-schema#comment>
                "A missing element is a data requirement violation that occurs when schema elements, instances, or data values are missing, but required."@en ;
        <http://www.w3.org/2000/01/rdf-schema#label>
                "Missing Element"@en ;
        <http://www.w3.org/2000/01/rdf-schema#subClassOf>
                <http://purl.org/dqm-vocabulary/v1/dqm#DataRequirementViolation> .

<http://purl.org/dqm-vocabulary/v1/dqm#referenceProperty2>
        a       <http://www.w3.org/2002/07/owl#ObjectProperty> , <http://www.w3.org/2002/07/owl#FunctionalProperty> ;
        <http://www.w3.org/2000/01/rdf-schema#comment>
                "The reference property points to the URI of a property that holds trusted values, i.e. values of high quality"@en ;
        <http://www.w3.org/2000/01/rdf-schema#domain>
                <http://purl.org/dqm-vocabulary/v1/dqm#FuncDepReferenceRule> ;
        <http://www.w3.org/2000/01/rdf-schema#label>
                "Reference Property 2"@en ;
        <http://www.w3.org/2000/01/rdf-schema#subPropertyOf>
                <http://purl.org/dqm-vocabulary/v1/dqm#referenceProperty> .

<http://purl.org/dqm-vocabulary/v1/dqm#referenceProperty3>
        a       <http://www.w3.org/2002/07/owl#ObjectProperty> , <http://www.w3.org/2002/07/owl#FunctionalProperty> ;
        <http://www.w3.org/2000/01/rdf-schema#comment>
                "The reference property points to the URI of a property that holds trusted values, i.e. values of high quality"@en ;
        <http://www.w3.org/2000/01/rdf-schema#domain>
                <http://purl.org/dqm-vocabulary/v1/dqm#FuncDepReferenceRule> ;
        <http://www.w3.org/2000/01/rdf-schema#label>
                "Reference Property 3"@en ;
        <http://www.w3.org/2000/01/rdf-schema#subPropertyOf>
                <http://purl.org/dqm-vocabulary/v1/dqm#referenceProperty> .

<http://purl.org/dqm-vocabulary/v1/dqm#referenceProperty4>
        a       <http://www.w3.org/2002/07/owl#ObjectProperty> , <http://www.w3.org/2002/07/owl#FunctionalProperty> ;
        <http://www.w3.org/2000/01/rdf-schema#comment>
                "The reference property points to the URI of a property that holds trusted values, i.e. values of high quality"@en ;
        <http://www.w3.org/2000/01/rdf-schema#domain>
                <http://purl.org/dqm-vocabulary/v1/dqm#FuncDepReferenceRule> ;
        <http://www.w3.org/2000/01/rdf-schema#label>
                "Reference Property 4"@en ;
        <http://www.w3.org/2000/01/rdf-schema#subPropertyOf>
                <http://purl.org/dqm-vocabulary/v1/dqm#referenceProperty> .

<http://purl.org/dqm-vocabulary/v1/dqm#referenceProperty5>
        a       <http://www.w3.org/2002/07/owl#ObjectProperty> , <http://www.w3.org/2002/07/owl#FunctionalProperty> ;
        <http://www.w3.org/2000/01/rdf-schema#comment>
                "The reference property points to the URI of a property that holds trusted values, i.e. values of high quality"@en ;
        <http://www.w3.org/2000/01/rdf-schema#domain>
                <http://purl.org/dqm-vocabulary/v1/dqm#FuncDepReferenceRule> ;
        <http://www.w3.org/2000/01/rdf-schema#label>
                "Reference Property 5"@en ;
        <http://www.w3.org/2000/01/rdf-schema#subPropertyOf>
                <http://purl.org/dqm-vocabulary/v1/dqm#referenceProperty> .

<http://purl.org/dqm-vocabulary/v1/dqm#importance>
        a       <http://www.w3.org/2002/07/owl#DatatypeProperty> , <http://www.w3.org/2002/07/owl#FunctionalProperty> ;
        <http://www.w3.org/2000/01/rdf-schema#comment>
                "Specifies the importance of a task, a data quality rule, or a data element."@en ;
        <http://www.w3.org/2000/01/rdf-schema#domain>
                [ a       <http://www.w3.org/2002/07/owl#Class> ;
                  <http://www.w3.org/2002/07/owl#unionOf>
                          ( <http://purl.org/dqm-vocabulary/v1/dqm#DataElement> <http://purl.org/dqm-vocabulary/v1/dqm#DataRequirement> <http://purl.org/dqm-vocabulary/v1/dqm#Task> )
                ] ;
        <http://www.w3.org/2000/01/rdf-schema#label>
                "Importance"@en ;
        <http://www.w3.org/2000/01/rdf-schema#range>
                <http://www.w3.org/2000/01/rdf-schema#Literal> ;
        <http://www.w3.org/2000/01/rdf-schema#subPropertyOf>
                <http://purl.org/dqm-vocabulary/v1/dqm#reqMetadata> .

<http://purl.org/dqm-vocabulary/v1/dqm#lastModified>
        a       <http://www.w3.org/2002/07/owl#FunctionalProperty> , <http://www.w3.org/2002/07/owl#DatatypeProperty> ;
        <http://www.w3.org/2000/01/rdf-schema#comment>
                "The property lastModified indicates the date and time when the rule was last modified."@en ;
        <http://www.w3.org/2000/01/rdf-schema#domain>
                <http://purl.org/dqm-vocabulary/v1/dqm#DataRequirement> ;
        <http://www.w3.org/2000/01/rdf-schema#label>
                "Last Modified"@en ;
        <http://www.w3.org/2000/01/rdf-schema#range>
                <http://www.w3.org/2001/XMLSchema#dateTime> ;
        <http://www.w3.org/2000/01/rdf-schema#subPropertyOf>
                <http://purl.org/dqm-vocabulary/v1/dqm#reqMetadata> .

<http://purl.org/dqm-vocabulary/v1/dqm#cleansesClass>
        a       <http://www.w3.org/2002/07/owl#FunctionalProperty> , <http://www.w3.org/2002/07/owl#ObjectProperty> ;
        <http://www.w3.org/2000/01/rdf-schema#comment>
                "This property identifies classes that contain instances that shall be cleansed via a data cleansing rule."@en ;
        <http://www.w3.org/2000/01/rdf-schema#domain>
                <http://purl.org/dqm-vocabulary/v1/dqm#DataCleansingRule> ;
        <http://www.w3.org/2000/01/rdf-schema#label>
                "Cleanses Class"@en ;
        <http://www.w3.org/2000/01/rdf-schema#range>
                <http://purl.org/dqm-vocabulary/v1/dqm#TestedClass> ;
        <http://www.w3.org/2000/01/rdf-schema#subPropertyOf>
                <http://purl.org/dqm-vocabulary/v1/dqm#dataCleansingRuleRelationship> .

<http://purl.org/dqm-vocabulary/v1/dqm#validFrom>
        a       <http://www.w3.org/2002/07/owl#FunctionalProperty> , <http://www.w3.org/2002/07/owl#DatatypeProperty> ;
        <http://www.w3.org/2000/01/rdf-schema#comment>
                "Specifies the date and time from which a rule is valid."@en ;
        <http://www.w3.org/2000/01/rdf-schema#domain>
                [ a       <http://www.w3.org/2002/07/owl#Class> ;
                  <http://www.w3.org/2002/07/owl#unionOf>
                          ( <http://purl.org/dqm-vocabulary/v1/dqm#DataCleansingRule> <http://purl.org/dqm-vocabulary/v1/dqm#DataRequirement> )
                ] ;
        <http://www.w3.org/2000/01/rdf-schema#label>
                "Valid From"@en ;
        <http://www.w3.org/2000/01/rdf-schema#range>
                <http://www.w3.org/2001/XMLSchema#dateTime> ;
        <http://www.w3.org/2000/01/rdf-schema#subPropertyOf>
                <http://purl.org/dqm-vocabulary/v1/dqm#reqMetadata> .

<http://purl.org/dqm-vocabulary/v1/dqm#greaterThan>
        a       <http://www.w3.org/2002/07/owl#DatatypeProperty> , <http://www.w3.org/2002/07/owl#FunctionalProperty> ;
        <http://www.w3.org/2000/01/rdf-schema#comment>
                "Holds a numeric value that is used to identify values of a property that are greater than the value of this property."@en ;
        <http://www.w3.org/2000/01/rdf-schema#domain>
                [ a       <http://www.w3.org/2002/07/owl#Class> ;
                  <http://www.w3.org/2002/07/owl#unionOf>
                          ( <http://purl.org/dqm-vocabulary/v1/dqm#Condition> <http://purl.org/dqm-vocabulary/v1/dqm#FuncDepValueRule> )
                ] ;
        <http://www.w3.org/2000/01/rdf-schema#label>
                "Greater Than"@en ;
        <http://www.w3.org/2000/01/rdf-schema#range>
                <http://www.w3.org/2001/XMLSchema#float> ;
        <http://www.w3.org/2000/01/rdf-schema#subPropertyOf>
                <http://purl.org/dqm-vocabulary/v1/dqm#operatedValue> .

<http://purl.org/dqm-vocabulary/v1/dqm#Uniqueness>
        a       <http://www.w3.org/2002/07/owl#Class> ;
        <http://www.w3.org/2000/01/rdf-schema#comment>
                "Uniqueness is the degree to which properties and classes are free of duplicate values and instances."@en ;
        <http://www.w3.org/2000/01/rdf-schema#label>
                "Uniqueness"@en ;
        <http://www.w3.org/2000/01/rdf-schema#subClassOf>
                <http://purl.org/dqm-vocabulary/v1/dqm#DataQualityScore> .

<http://purl.org/dqm-vocabulary/v1/dqm#IllegalValue>
        a       <http://www.w3.org/2002/07/owl#Class> ;
        <http://www.w3.org/2000/01/rdf-schema#comment>
                "An illegal value is a data value that must not be used for a property."@en ;
        <http://www.w3.org/2000/01/rdf-schema#label>
                "Illegal Value"@en ;
        <http://www.w3.org/2000/01/rdf-schema#subClassOf>
                <http://purl.org/dqm-vocabulary/v1/dqm#DataRequirementViolation> .

<http://purl.org/dqm-vocabulary/v1/dqm#dataElementRelationship>
        a       <http://www.w3.org/2002/07/owl#ObjectProperty> ;
        <http://www.w3.org/2000/01/rdf-schema#comment>
                "The data element relationship property is an abstract property that holds object properties that are used to define internal and external relationships of data elements."@en ;
        <http://www.w3.org/2000/01/rdf-schema#label>
                "Data Element Relationship"@en .

<http://purl.org/dqm-vocabulary/v1/dqm#SyntacticAccuracy>
        a       <http://www.w3.org/2002/07/owl#Class> ;
        <http://www.w3.org/2000/01/rdf-schema#comment>
                "Syntactic accuracy is the degree to which data values of a property represent legal values and are free from syntax violations."@en ;
        <http://www.w3.org/2000/01/rdf-schema#label>
                "Syntactic Accuracy"@en ;
        <http://www.w3.org/2000/01/rdf-schema#subClassOf>
                <http://purl.org/dqm-vocabulary/v1/dqm#Accuracy> .

<http://purl.org/dqm-vocabulary/v1/dqm#basedOn>
        a       <http://www.w3.org/2002/07/owl#ObjectProperty> ;
        <http://www.w3.org/2000/01/rdf-schema#comment>
                "Connects a data quality score with the data requirements that were used to calculate the score."@en ;
        <http://www.w3.org/2000/01/rdf-schema#domain>
                <http://purl.org/dqm-vocabulary/v1/dqm#DataQualityScore> ;
        <http://www.w3.org/2000/01/rdf-schema#label>
                "Based On"@en ;
        <http://www.w3.org/2000/01/rdf-schema#range>
                <http://purl.org/dqm-vocabulary/v1/dqm#DataRequirement> ;
        <http://www.w3.org/2000/01/rdf-schema#subPropertyOf>
                <http://purl.org/dqm-vocabulary/v1/dqm#dataRequirementsRelationship> ;
        <http://www.w3.org/2002/07/owl#inverseOf>
                <http://purl.org/dqm-vocabulary/v1/dqm#hasScore> .

<http://purl.org/dqm-vocabulary/v1/dqm#rank>
        a       <http://www.w3.org/2002/07/owl#DatatypeProperty> , <http://www.w3.org/2002/07/owl#FunctionalProperty> ;
        <http://www.w3.org/2000/01/rdf-schema#comment>
                "Position of a value in an ordinal scale."@en ;
        <http://www.w3.org/2000/01/rdf-schema#domain>
                <http://purl.org/dqm-vocabulary/v1/dqm#ScaleValue> ;
        <http://www.w3.org/2000/01/rdf-schema#label>
                "Rank"@en ;
        <http://www.w3.org/2000/01/rdf-schema#range>
                <http://www.w3.org/2001/XMLSchema#int> .

<http://purl.org/dqm-vocabulary/v1/dqm#hasCondition3>
        a       <http://www.w3.org/2002/07/owl#FunctionalProperty> , <http://www.w3.org/2002/07/owl#ObjectProperty> ;
        <http://www.w3.org/2000/01/rdf-schema#comment>
                "Connects a conditional rule with a certain condition."@en ;
        <http://www.w3.org/2000/01/rdf-schema#domain>
                [ a       <http://www.w3.org/2002/07/owl#Class> ;
                  <http://www.w3.org/2002/07/owl#unionOf>
                          ( <http://purl.org/dqm-vocabulary/v1/dqm#ConditionalRule> <http://purl.org/dqm-vocabulary/v1/dqm#MultiPropertyCleansingRule> )
                ] ;
        <http://www.w3.org/2000/01/rdf-schema#label>
                "Has Condition 3"@en ;
        <http://www.w3.org/2000/01/rdf-schema#subPropertyOf>
                <http://purl.org/dqm-vocabulary/v1/dqm#hasCondition> .

<http://purl.org/dqm-vocabulary/v1/dqm#hasCondition4>
        a       <http://www.w3.org/2002/07/owl#FunctionalProperty> , <http://www.w3.org/2002/07/owl#ObjectProperty> ;
        <http://www.w3.org/2000/01/rdf-schema#comment>
                "Connects a conditional rule with a certain condition."@en ;
        <http://www.w3.org/2000/01/rdf-schema#domain>
                [ a       <http://www.w3.org/2002/07/owl#Class> ;
                  <http://www.w3.org/2002/07/owl#unionOf>
                          ( <http://purl.org/dqm-vocabulary/v1/dqm#ConditionalRule> <http://purl.org/dqm-vocabulary/v1/dqm#MultiPropertyCleansingRule> )
                ] ;
        <http://www.w3.org/2000/01/rdf-schema#label>
                "Has Condition 4"@en ;
        <http://www.w3.org/2000/01/rdf-schema#subPropertyOf>
                <http://purl.org/dqm-vocabulary/v1/dqm#hasCondition> .

<http://purl.org/dqm-vocabulary/v1/dqm#startsWith>
        a       <http://www.w3.org/2002/07/owl#FunctionalProperty> , <http://www.w3.org/2002/07/owl#DatatypeProperty> ;
        <http://www.w3.org/2000/01/rdf-schema#comment>
                "Holds one or more consecutive characters that are supposed to be found at the beginning of strings of another property."@en ;
        <http://www.w3.org/2000/01/rdf-schema#domain>
                [ a       <http://www.w3.org/2002/07/owl#Class> ;
                  <http://www.w3.org/2002/07/owl#unionOf>
                          ( <http://purl.org/dqm-vocabulary/v1/dqm#Condition> <http://purl.org/dqm-vocabulary/v1/dqm#FuncDepValueRule> )
                ] ;
        <http://www.w3.org/2000/01/rdf-schema#label>
                "Starts With"@en ;
        <http://www.w3.org/2000/01/rdf-schema#range>
                <http://www.w3.org/2001/XMLSchema#string> ;
        <http://www.w3.org/2000/01/rdf-schema#subPropertyOf>
                <http://purl.org/dqm-vocabulary/v1/dqm#operatedValue> .

<http://purl.org/dqm-vocabulary/v1/dqm#hasCondition5>
        a       <http://www.w3.org/2002/07/owl#FunctionalProperty> , <http://www.w3.org/2002/07/owl#ObjectProperty> ;
        <http://www.w3.org/2000/01/rdf-schema#comment>
                "Connects a conditional rule with a certain condition."@en ;
        <http://www.w3.org/2000/01/rdf-schema#domain>
                [ a       <http://www.w3.org/2002/07/owl#Class> ;
                  <http://www.w3.org/2002/07/owl#unionOf>
                          ( <http://purl.org/dqm-vocabulary/v1/dqm#ConditionalRule> <http://purl.org/dqm-vocabulary/v1/dqm#MultiPropertyCleansingRule> )
                ] ;
        <http://www.w3.org/2000/01/rdf-schema#label>
                "Has Condition 5"@en ;
        <http://www.w3.org/2000/01/rdf-schema#subPropertyOf>
                <http://purl.org/dqm-vocabulary/v1/dqm#hasCondition> .

<http://purl.org/dqm-vocabulary/v1/dqm#ExpiryRule>
        a       <http://www.w3.org/2002/07/owl#Class> ;
        <http://www.w3.org/2000/01/rdf-schema#comment>
                "An expiry rule is an outdated instance rule that specifies the expiration date of an instance that must not exceed the current date and time. Therefore, expiry rules require date information about the validity period of an instance."@en ;
        <http://www.w3.org/2000/01/rdf-schema#label>
                "Expiry Rule"@en ;
        <http://www.w3.org/2000/01/rdf-schema#subClassOf>
                <http://purl.org/dqm-vocabulary/v1/dqm#OutdatedInstanceRule> .

<http://purl.org/dqm-vocabulary/v1/dqm#hasCondition1>
        a       <http://www.w3.org/2002/07/owl#FunctionalProperty> , <http://www.w3.org/2002/07/owl#ObjectProperty> ;
        <http://www.w3.org/2000/01/rdf-schema#comment>
                "Connects a conditional rule with a certain condition."@en ;
        <http://www.w3.org/2000/01/rdf-schema#domain>
                [ a       <http://www.w3.org/2002/07/owl#Class> ;
                  <http://www.w3.org/2002/07/owl#unionOf>
                          ( <http://purl.org/dqm-vocabulary/v1/dqm#ConditionalRule> <http://purl.org/dqm-vocabulary/v1/dqm#MultiPropertyCleansingRule> )
                ] ;
        <http://www.w3.org/2000/01/rdf-schema#label>
                "Has Condition 1"@en ;
        <http://www.w3.org/2000/01/rdf-schema#subPropertyOf>
                <http://purl.org/dqm-vocabulary/v1/dqm#hasCondition> .

<http://purl.org/dqm-vocabulary/v1/dqm#hasCondition2>
        a       <http://www.w3.org/2002/07/owl#FunctionalProperty> , <http://www.w3.org/2002/07/owl#ObjectProperty> ;
        <http://www.w3.org/2000/01/rdf-schema#comment>
                "Connects a conditional rule with a certain condition."@en ;
        <http://www.w3.org/2000/01/rdf-schema#domain>
                [ a       <http://www.w3.org/2002/07/owl#Class> ;
                  <http://www.w3.org/2002/07/owl#unionOf>
                          ( <http://purl.org/dqm-vocabulary/v1/dqm#ConditionalRule> <http://purl.org/dqm-vocabulary/v1/dqm#MultiPropertyCleansingRule> )
                ] ;
        <http://www.w3.org/2000/01/rdf-schema#label>
                "Has Condition 2"@en ;
        <http://www.w3.org/2000/01/rdf-schema#subPropertyOf>
                <http://purl.org/dqm-vocabulary/v1/dqm#hasCondition> .

<http://purl.org/dqm-vocabulary/v1/dqm#validation>
        a       <http://www.w3.org/2002/07/owl#FunctionalProperty> , <http://www.w3.org/2002/07/owl#DatatypeProperty> ;
        <http://www.w3.org/2000/01/rdf-schema#comment>
                "Validation indicates whether a data quality rule shall be used for validation during data entry."@en ;
        <http://www.w3.org/2000/01/rdf-schema#domain>
                <http://purl.org/dqm-vocabulary/v1/dqm#DataRequirement> ;
        <http://www.w3.org/2000/01/rdf-schema#label>
                "Validation"@en ;
        <http://www.w3.org/2000/01/rdf-schema#range>
                <http://www.w3.org/2001/XMLSchema#boolean> .

<http://purl.org/dqm-vocabulary/v1/dqm#PopulationUniqueness>
        a       <http://www.w3.org/2002/07/owl#Class> ;
        <http://www.w3.org/2000/01/rdf-schema#comment>
                "Entity uniqueness is the degree to which entities (that must be uniquely represented within a certain class) are unique."@en ;
        <http://www.w3.org/2000/01/rdf-schema#label>
                "Population Uniqueness"@en ;
        <http://www.w3.org/2000/01/rdf-schema#subClassOf>
                <http://purl.org/dqm-vocabulary/v1/dqm#Uniqueness> .

<http://purl.org/dc/elements/1.1/title>
        a       <http://www.w3.org/2002/07/owl#AnnotationProperty> .

<http://purl.org/dqm-vocabulary/v1/dqm#SyntaxViolation>
        a       <http://www.w3.org/2002/07/owl#Class> ;
        <http://www.w3.org/2000/01/rdf-schema#comment>
                "A syntax violation is a data requirement violation that occurs when a data value contains disallowed characters or does not match a predefined pattern."@en ;
        <http://www.w3.org/2000/01/rdf-schema#label>
                "Syntax Violation"@en ;
        <http://www.w3.org/2000/01/rdf-schema#subClassOf>
                <http://purl.org/dqm-vocabulary/v1/dqm#DataRequirementViolation> .

<http://purl.org/dqm-vocabulary/v1/dqm#regex>
        a       <http://www.w3.org/2002/07/owl#FunctionalProperty> , <http://www.w3.org/2002/07/owl#DatatypeProperty> ;
        <http://www.w3.org/2000/01/rdf-schema#comment>
                "The regular expressions property can be used to express legal character ranges and data patterns for values of a certain property via regular expressions."@en ;
        <http://www.w3.org/2000/01/rdf-schema#domain>
                [ a       <http://www.w3.org/2002/07/owl#Class> ;
                  <http://www.w3.org/2002/07/owl#unionOf>
                          ( <http://purl.org/dqm-vocabulary/v1/dqm#ConditionalSyntaxRule> <http://purl.org/dqm-vocabulary/v1/dqm#SyntaxRule> )
                ] ;
        <http://www.w3.org/2000/01/rdf-schema#label>
                "Regular Expression"@en ;
        <http://www.w3.org/2000/01/rdf-schema#range>
                <http://www.w3.org/2001/XMLSchema#string> .

<http://purl.org/dqm-vocabulary/v1/dqm#contains>
        a       <http://www.w3.org/2002/07/owl#DatatypeProperty> , <http://www.w3.org/2002/07/owl#FunctionalProperty> ;
        <http://www.w3.org/2000/01/rdf-schema#comment>
                "Holds one or more consecutive characters that are supposed to be found in strings of another property."@en ;
        <http://www.w3.org/2000/01/rdf-schema#domain>
                [ a       <http://www.w3.org/2002/07/owl#Class> ;
                  <http://www.w3.org/2002/07/owl#unionOf>
                          ( <http://purl.org/dqm-vocabulary/v1/dqm#Condition> <http://purl.org/dqm-vocabulary/v1/dqm#FuncDepValueRule> )
                ] ;
        <http://www.w3.org/2000/01/rdf-schema#label>
                "Contains"@en ;
        <http://www.w3.org/2000/01/rdf-schema#range>
                <http://www.w3.org/2001/XMLSchema#string> ;
        <http://www.w3.org/2000/01/rdf-schema#subPropertyOf>
                <http://purl.org/dqm-vocabulary/v1/dqm#operatedValue> .

<http://purl.org/dqm-vocabulary/v1/dqm#AffectedInstance>
        a       <http://www.w3.org/2002/07/owl#Class> ;
        <http://www.w3.org/2000/01/rdf-schema#comment>
                "An affected instance is a data instance that contains one or more data quality problems."@en ;
        <http://www.w3.org/2000/01/rdf-schema#label>
                "Affected Instance"@en ;
        <http://www.w3.org/2000/01/rdf-schema#subClassOf>
                <http://purl.org/dqm-vocabulary/v1/dqm#DataElement> .

<http://purl.org/dqm-vocabulary/v1/dqm#expectedUpdateInterval>
        a       <http://www.w3.org/2002/07/owl#DatatypeProperty> , <http://www.w3.org/2002/07/owl#FunctionalProperty> ;
        <http://www.w3.org/2000/01/rdf-schema#comment>
                "The expected update interval specifies the time interval in which instances of a specific class must be updated in order to be current."@en ;
        <http://www.w3.org/2000/01/rdf-schema#domain>
                <http://purl.org/dqm-vocabulary/v1/dqm#UpdateRule> ;
        <http://www.w3.org/2000/01/rdf-schema#label>
                "Expected Update Interval"@en ;
        <http://www.w3.org/2000/01/rdf-schema#range>
                <http://www.w3.org/2001/XMLSchema#duration> .

<http://purl.org/dqm-vocabulary/v1/dqm#requiredProperty>
        a       <http://www.w3.org/2002/07/owl#FunctionalProperty> , <http://www.w3.org/2002/07/owl#DatatypeProperty> ;
        <http://www.w3.org/2000/01/rdf-schema#comment>
                "Specifies whether a property must exist."@en ;
        <http://www.w3.org/2000/01/rdf-schema#domain>
                [ a       <http://www.w3.org/2002/07/owl#Class> ;
                  <http://www.w3.org/2002/07/owl#unionOf>
                          ( <http://purl.org/dqm-vocabulary/v1/dqm#ConditionalPropertyCompletenessRule> <http://purl.org/dqm-vocabulary/v1/dqm#PropertyCompletenessRule> )
                ] ;
        <http://www.w3.org/2000/01/rdf-schema#label>
                "Required Property"@en ;
        <http://www.w3.org/2000/01/rdf-schema#range>
                <http://www.w3.org/2001/XMLSchema#boolean> .

<http://purl.org/dqm-vocabulary/v1/dqm#subTaskOf>
        a       <http://www.w3.org/2002/07/owl#ObjectProperty> , <http://www.w3.org/2002/07/owl#TransitiveProperty> ;
        <http://www.w3.org/2000/01/rdf-schema#comment>
                "Property that can be used to represent hierachies of between tasks."@en ;
        <http://www.w3.org/2000/01/rdf-schema#domain>
                <http://purl.org/dqm-vocabulary/v1/dqm#Task> ;
        <http://www.w3.org/2000/01/rdf-schema#label>
                "Sub Task Of"@en ;
        <http://www.w3.org/2000/01/rdf-schema#range>
                <http://purl.org/dqm-vocabulary/v1/dqm#Task> ;
        <http://www.w3.org/2000/01/rdf-schema#subPropertyOf>
                <http://purl.org/dqm-vocabulary/v1/dqm#dataRequirementsRelationship> .

<http://purl.org/dqm-vocabulary/v1/dqm#ruleViolation>
        a       <http://www.w3.org/2002/07/owl#ObjectProperty> ;
        <http://www.w3.org/2000/01/rdf-schema#comment>
                "Connects data requirements with data quality problems that have been identified using the requirement."@en ;
        <http://www.w3.org/2000/01/rdf-schema#domain>
                <http://purl.org/dqm-vocabulary/v1/dqm#DataRequirement> ;
        <http://www.w3.org/2000/01/rdf-schema#label>
                "Rule Violation"@en ;
        <http://www.w3.org/2000/01/rdf-schema#range>
                <http://purl.org/dqm-vocabulary/v1/dqm#DataRequirementViolation> ;
        <http://www.w3.org/2000/01/rdf-schema#subPropertyOf>
                <http://purl.org/dqm-vocabulary/v1/dqm#dataRequirementsRelationship> ;
        <http://www.w3.org/2002/07/owl#inverseOf>
                <http://purl.org/dqm-vocabulary/v1/dqm#ruleOfIdentification> .

<http://purl.org/dqm-vocabulary/v1/dqm#TrustedProperty>
        a       <http://www.w3.org/2002/07/owl#Class> ;
        <http://www.w3.org/2000/01/rdf-schema#comment>
                "A trusted property holds the values that serve as a trusted reference in legal value rules / functional dependency reference rules, e.g. to define legal values for a tested property."@en ;
        <http://www.w3.org/2000/01/rdf-schema#label>
                "Trusted Property"@en ;
        <http://www.w3.org/2000/01/rdf-schema#subClassOf>
                <http://purl.org/dqm-vocabulary/v1/dqm#DataElement> .

<http://purl.org/dqm-vocabulary/v1/dqm#Condition>
        a       <http://www.w3.org/2002/07/owl#Class> ;
        <http://www.w3.org/2000/01/rdf-schema#comment>
                "A condition constrains instances of a class to a certain subset for which certain data quality rules apply."@en ;
        <http://www.w3.org/2000/01/rdf-schema#label>
                "Condition"@en .

<http://purl.org/dqm-vocabulary/v1/dqm#ValueSubstitution>
        a       <http://www.w3.org/2002/07/owl#Class> ;
        <http://www.w3.org/2000/01/rdf-schema#comment>
                "A value substitution rule specifies a value to be removed and a new value that shall substitute the removed value."@en ;
        <http://www.w3.org/2000/01/rdf-schema#label>
                "Value Substitution Rule"@en ;
        <http://www.w3.org/2000/01/rdf-schema#subClassOf>
                <http://purl.org/dqm-vocabulary/v1/dqm#LiteralCleansingRule> .

<http://purl.org/dqm-vocabulary/v1/dqm#BlacklistClass>
        a       <http://www.w3.org/2002/07/owl#Class> ;
        <http://www.w3.org/2000/01/rdf-schema#comment>
                "A blacklist class holds instances with values that are disallowed for a certain data set. Thus, illegal value rules refer to such classes over the blacklist class property."@en ;
        <http://www.w3.org/2000/01/rdf-schema#label>
                "Blacklist Class"@en ;
        <http://www.w3.org/2000/01/rdf-schema#subClassOf>
                <http://purl.org/dqm-vocabulary/v1/dqm#DataElement> .

<http://purl.org/dqm-vocabulary/v1/dqm#testedClass>
        a       <http://www.w3.org/2002/07/owl#FunctionalProperty> , <http://www.w3.org/2002/07/owl#ObjectProperty> ;
        <http://www.w3.org/2000/01/rdf-schema#comment>
                "The tested class property specifies the class that holds the instances that shall be tested for data quality problems."@en ;
        <http://www.w3.org/2000/01/rdf-schema#domain>
                <http://purl.org/dqm-vocabulary/v1/dqm#DataRequirement> ;
        <http://www.w3.org/2000/01/rdf-schema#label>
                "Tested Class"@en ;
        <http://www.w3.org/2000/01/rdf-schema#range>
                <http://purl.org/dqm-vocabulary/v1/dqm#TestedClass> ;
        <http://www.w3.org/2000/01/rdf-schema#subPropertyOf>
                <http://purl.org/dqm-vocabulary/v1/dqm#dataElementRelationship> .

<http://purl.org/dqm-vocabulary/v1/dqm#appliesFor>
        a       <http://www.w3.org/2002/07/owl#ObjectProperty> ;
        <http://www.w3.org/2000/01/rdf-schema#comment>
                "Connects data requirements with the tasks in which the requirement applies."@en ;
        <http://www.w3.org/2000/01/rdf-schema#domain>
                <http://purl.org/dqm-vocabulary/v1/dqm#DataRequirement> ;
        <http://www.w3.org/2000/01/rdf-schema#label>
                "Applies For"@en ;
        <http://www.w3.org/2000/01/rdf-schema#range>
                <http://purl.org/dqm-vocabulary/v1/dqm#Task> ;
        <http://www.w3.org/2000/01/rdf-schema#subPropertyOf>
                <http://purl.org/dqm-vocabulary/v1/dqm#dataRequirementsRelationship> ;
        <http://www.w3.org/2002/07/owl#inverseOf>
                <http://purl.org/dqm-vocabulary/v1/dqm#hasRequirement> .

<http://purl.org/dqm-vocabulary/v1/dqm#dataRequirementsRelationship>
        a       <http://www.w3.org/2002/07/owl#ObjectProperty> ;
        <http://www.w3.org/2000/01/rdf-schema#comment>
                "The data requirements relationship property is an abstract property that holds object properties that are used to define internal and external relationships of data requirements."@en ;
        <http://www.w3.org/2000/01/rdf-schema#label>
                "Data Requirements Relationship"@en .

<http://purl.org/dqm-vocabulary/v1/dqm#MissingPropertyAndValue>
        a       <http://www.w3.org/2002/07/owl#Class> ;
        <http://www.w3.org/2000/01/rdf-schema#comment>
                "Class for instances that miss both a property and its value."@en ;
        <http://www.w3.org/2000/01/rdf-schema#label>
                "Missing Property and Value"@en ;
        <http://www.w3.org/2000/01/rdf-schema#subClassOf>
                <http://purl.org/dqm-vocabulary/v1/dqm#MissingElement> .

<http://purl.org/dqm-vocabulary/v1/dqm#referenceProperty>
        a       <http://www.w3.org/2002/07/owl#ObjectProperty> ;
        <http://www.w3.org/2000/01/rdf-schema#comment>
                "The reference property points to the URI of a property that holds trusted values, i.e. values of high quality"@en ;
        <http://www.w3.org/2000/01/rdf-schema#label>
                "Reference Property"@en ;
        <http://www.w3.org/2000/01/rdf-schema#range>
                <http://purl.org/dqm-vocabulary/v1/dqm#TrustedProperty> ;
        <http://www.w3.org/2000/01/rdf-schema#subPropertyOf>
                <http://purl.org/dqm-vocabulary/v1/dqm#dataElementRelationship> .

<http://purl.org/dqm-vocabulary/v1/dqm#hasProperties>
        a       <http://www.w3.org/2002/07/owl#ObjectProperty> ;
        <http://www.w3.org/2000/01/rdf-schema#comment>
                "Reconnects mapped classes and properties with each other."@en ;
        <http://www.w3.org/2000/01/rdf-schema#domain>
                [ a       <http://www.w3.org/2002/07/owl#Class> ;
                  <http://www.w3.org/2002/07/owl#unionOf>
                          ( <http://purl.org/dqm-vocabulary/v1/dqm#AffectedClass> <http://purl.org/dqm-vocabulary/v1/dqm#BlacklistClass> <http://purl.org/dqm-vocabulary/v1/dqm#TestedClass> <http://purl.org/dqm-vocabulary/v1/dqm#TrustedClass> )
                ] ;
        <http://www.w3.org/2000/01/rdf-schema#label>
                "Has Properties"@en ;
        <http://www.w3.org/2000/01/rdf-schema#range>
                [ a       <http://www.w3.org/2002/07/owl#Class> ;
                  <http://www.w3.org/2002/07/owl#unionOf>
                          ( <http://purl.org/dqm-vocabulary/v1/dqm#AffectedProperty> <http://purl.org/dqm-vocabulary/v1/dqm#BlacklistProperty> <http://purl.org/dqm-vocabulary/v1/dqm#TestedProperty> <http://purl.org/dqm-vocabulary/v1/dqm#TrustedProperty> )
                ] ;
        <http://www.w3.org/2000/01/rdf-schema#subPropertyOf>
                <http://purl.org/dqm-vocabulary/v1/dqm#dataElementRelationship> .

<http://purl.org/dqm-vocabulary/v1/dqm#notEqualTo>
        a       <http://www.w3.org/2002/07/owl#FunctionalProperty> , <http://www.w3.org/2002/07/owl#DatatypeProperty> ;
        <http://www.w3.org/2000/01/rdf-schema#comment>
                "Holds one or more consecutive characters that are used to identify values of another property that do not match with the value of this property."@en ;
        <http://www.w3.org/2000/01/rdf-schema#domain>
                [ a       <http://www.w3.org/2002/07/owl#Class> ;
                  <http://www.w3.org/2002/07/owl#unionOf>
                          ( <http://purl.org/dqm-vocabulary/v1/dqm#Condition> <http://purl.org/dqm-vocabulary/v1/dqm#FuncDepValueRule> )
                ] ;
        <http://www.w3.org/2000/01/rdf-schema#label>
                "Not Equal To"@en ;
        <http://www.w3.org/2000/01/rdf-schema#range>
                <http://www.w3.org/2001/XMLSchema#string> ;
        <http://www.w3.org/2000/01/rdf-schema#subPropertyOf>
                <http://purl.org/dqm-vocabulary/v1/dqm#operatedValue> .

<http://purl.org/dqm-vocabulary/v1/dqm#assessedProperty>
        a       <http://www.w3.org/2002/07/owl#ObjectProperty> ;
        <http://www.w3.org/2000/01/rdf-schema#comment>
                "The assessed property represents all properties that have been tested for rule violations during the computation of the assessment score."@en ;
        <http://www.w3.org/2000/01/rdf-schema#domain>
                <http://purl.org/dqm-vocabulary/v1/dqm#DataQualityScore> ;
        <http://www.w3.org/2000/01/rdf-schema#label>
                "Assessed Property"@en ;
        <http://www.w3.org/2000/01/rdf-schema#range>
                <http://purl.org/dqm-vocabulary/v1/dqm#TestedProperty> ;
        <http://www.w3.org/2000/01/rdf-schema#subPropertyOf>
                <http://purl.org/dqm-vocabulary/v1/dqm#dataElementRelationship> .

<http://purl.org/dqm-vocabulary/v1/dqm#assessment>
        a       <http://www.w3.org/2002/07/owl#FunctionalProperty> , <http://www.w3.org/2002/07/owl#DatatypeProperty> ;
        <http://www.w3.org/2000/01/rdf-schema#comment>
                "The assessment property indicates whether the rule shall be used for data quality assessment."@en ;
        <http://www.w3.org/2000/01/rdf-schema#domain>
                <http://purl.org/dqm-vocabulary/v1/dqm#DataRequirement> ;
        <http://www.w3.org/2000/01/rdf-schema#label>
                "Assessment"@en ;
        <http://www.w3.org/2000/01/rdf-schema#range>
                <http://www.w3.org/2001/XMLSchema#boolean> ;
        <http://www.w3.org/2000/01/rdf-schema#subPropertyOf>
                <http://purl.org/dqm-vocabulary/v1/dqm#reqMetadata> .

<http://purl.org/dqm-vocabulary/v1/dqm#reqName>
        a       <http://www.w3.org/2002/07/owl#DatatypeProperty> ;
        <http://www.w3.org/2000/01/rdf-schema#comment>
                "Specifies the name of a data requirement in natural language."@en ;
        <http://www.w3.org/2000/01/rdf-schema#domain>
                [ a       <http://www.w3.org/2002/07/owl#Class> ;
                  <http://www.w3.org/2002/07/owl#unionOf>
                          ( <http://purl.org/dqm-vocabulary/v1/dqm#DataCleansingRule> <http://purl.org/dqm-vocabulary/v1/dqm#DataRequirement> )
                ] ;
        <http://www.w3.org/2000/01/rdf-schema#label>
                "Requirement Name"@en ;
        <http://www.w3.org/2000/01/rdf-schema#range>
                <http://www.w3.org/2001/XMLSchema#string> ;
        <http://www.w3.org/2000/01/rdf-schema#subPropertyOf>
                <http://purl.org/dqm-vocabulary/v1/dqm#reqMetadata> .

<http://purl.org/dqm-vocabulary/v1/dqm#UniquenessViolation>
        a       <http://www.w3.org/2002/07/owl#Class> ;
        <http://www.w3.org/2000/01/rdf-schema#comment>
                "A uniqueness violation occurs when two or more identical values are assigned to a property that requires unique values."@en ;
        <http://www.w3.org/2000/01/rdf-schema#label>
                "Uniqueness Violation"@en ;
        <http://www.w3.org/2000/01/rdf-schema#subClassOf>
                <http://purl.org/dqm-vocabulary/v1/dqm#DataRequirementViolation> .

<http://purl.org/dqm-vocabulary/v1/dqm#unitOfMeasurement>
        a       <http://www.w3.org/2002/07/owl#FunctionalProperty> , <http://www.w3.org/2002/07/owl#ObjectProperty> ;
        <http://www.w3.org/2000/01/rdf-schema#comment>
                "Indicates the unit of measurement, e.g. of data quality scores. It is recommended to use UN/CEFACT common codes to specify the unit of measurement, e.g. \"P1\" stands for percent."@en ;
        <http://www.w3.org/2000/01/rdf-schema#domain>
                <http://purl.org/dqm-vocabulary/v1/dqm#DataQualityScore> ;
        <http://www.w3.org/2000/01/rdf-schema#label>
                "Unit of Measurement"@en ;
        <http://www.w3.org/2000/01/rdf-schema#range>
                <http://purl.org/dqm-vocabulary/v1/dqm#Unit> .

<http://purl.org/dqm-vocabulary/v1/dqm#PropertyCompletenessRule>
        a       <http://www.w3.org/2002/07/owl#Class> ;
        <http://www.w3.org/2000/01/rdf-schema#comment>
                "A property completeness rule is a data requirement that specifies that a certain property and/or its value must exist in all instances of a certain class."@en ;
        <http://www.w3.org/2000/01/rdf-schema#label>
                "Property Completeness Rule"@en ;
        <http://www.w3.org/2000/01/rdf-schema#subClassOf>
                <http://purl.org/dqm-vocabulary/v1/dqm#PropertyRequirement> .

<http://purl.org/dqm-vocabulary/v1/dqm#hasScore>
        a       <http://www.w3.org/2002/07/owl#ObjectProperty> ;
        <http://www.w3.org/2000/01/rdf-schema#comment>
                "Connects data requirements with the data quality score which was calculated based on the requirement."@en ;
        <http://www.w3.org/2000/01/rdf-schema#domain>
                <http://purl.org/dqm-vocabulary/v1/dqm#DataRequirement> ;
        <http://www.w3.org/2000/01/rdf-schema#label>
                "Has Score"@en ;
        <http://www.w3.org/2000/01/rdf-schema#range>
                <http://purl.org/dqm-vocabulary/v1/dqm#DataQualityScore> ;
        <http://www.w3.org/2000/01/rdf-schema#subPropertyOf>
                <http://purl.org/dqm-vocabulary/v1/dqm#dataRequirementsRelationship> .

<http://purl.org/dqm-vocabulary/v1/dqm#weightedScore>
        a       <http://www.w3.org/2002/07/owl#DatatypeProperty> , <http://www.w3.org/2002/07/owl#FunctionalProperty> ;
        <http://www.w3.org/2000/01/rdf-schema#comment>
                "A weighted score is a data quality dimension score that is computed by integration of importance values of data requirements, tasks, or data elements."@en ;
        <http://www.w3.org/2000/01/rdf-schema#domain>
                <http://purl.org/dqm-vocabulary/v1/dqm#DataQualityScore> ;
        <http://www.w3.org/2000/01/rdf-schema#label>
                "Weighted Score"@en ;
        <http://www.w3.org/2000/01/rdf-schema#range>
                <http://www.w3.org/2000/01/rdf-schema#Literal> .

<http://purl.org/dc/elements/1.1/creator>
        a       <http://www.w3.org/2002/07/owl#AnnotationProperty> .

<http://purl.org/dqm-vocabulary/v1/dqm#blacklistProperty>
        a       <http://www.w3.org/2002/07/owl#ObjectProperty> , <http://www.w3.org/2002/07/owl#FunctionalProperty> ;
        <http://www.w3.org/2000/01/rdf-schema#comment>
                "A blacklist property holds the values that are disallowed for a certain data set."@en ;
        <http://www.w3.org/2000/01/rdf-schema#domain>
                <http://purl.org/dqm-vocabulary/v1/dqm#IllegalValueRule> ;
        <http://www.w3.org/2000/01/rdf-schema#label>
                "Blacklist Property"@en ;
        <http://www.w3.org/2000/01/rdf-schema#range>
                <http://purl.org/dqm-vocabulary/v1/dqm#BlacklistProperty> ;
        <http://www.w3.org/2000/01/rdf-schema#subPropertyOf>
                <http://purl.org/dqm-vocabulary/v1/dqm#dataElementRelationship> .

<http://purl.org/dqm-vocabulary/v1/dqm#timeOfAssessment>
        a       <http://www.w3.org/2002/07/owl#DatatypeProperty> ;
        <http://www.w3.org/2000/01/rdf-schema#comment>
                "The time of assessment represents the data and time when the data quality score was computed."@en ;
        <http://www.w3.org/2000/01/rdf-schema#domain>
                <http://purl.org/dqm-vocabulary/v1/dqm#DataQualityScore> ;
        <http://www.w3.org/2000/01/rdf-schema#label>
                "Time Of Assessment"@en ;
        <http://www.w3.org/2000/01/rdf-schema#range>
                <http://www.w3.org/2001/XMLSchema#dateTime> .

<http://purl.org/dqm-vocabulary/v1/dqm#ruleOfIdentification>
        a       <http://www.w3.org/2002/07/owl#ObjectProperty> ;
        <http://www.w3.org/2000/01/rdf-schema#comment>
                "The rule of identification property connects the data quality problem instances with the instance of the data requirement that has detected the problem."@en ;
        <http://www.w3.org/2000/01/rdf-schema#domain>
                <http://purl.org/dqm-vocabulary/v1/dqm#DataRequirementViolation> ;
        <http://www.w3.org/2000/01/rdf-schema#label>
                "Rule Of Identification"@en ;
        <http://www.w3.org/2000/01/rdf-schema#range>
                <http://purl.org/dqm-vocabulary/v1/dqm#DataRequirement> ;
        <http://www.w3.org/2000/01/rdf-schema#subPropertyOf>
                <http://purl.org/dqm-vocabulary/v1/dqm#dataRequirementsRelationship> .

<http://purl.org/dqm-vocabulary/v1/dqm#referenceClass>
        a       <http://www.w3.org/2002/07/owl#ObjectProperty> , <http://www.w3.org/2002/07/owl#FunctionalProperty> ;
        <http://www.w3.org/2000/01/rdf-schema#comment>
                "The reference class property points to the URI of a class that contains trusted instances, i.e. instances of high quality."@en ;
        <http://www.w3.org/2000/01/rdf-schema#domain>
                [ a       <http://www.w3.org/2002/07/owl#Class> ;
                  <http://www.w3.org/2002/07/owl#unionOf>
                          ( <http://purl.org/dqm-vocabulary/v1/dqm#FuncDepReferenceRule> <http://purl.org/dqm-vocabulary/v1/dqm#LegalValueRule> )
                ] ;
        <http://www.w3.org/2000/01/rdf-schema#label>
                "Reference Class"@en ;
        <http://www.w3.org/2000/01/rdf-schema#range>
                <http://purl.org/dqm-vocabulary/v1/dqm#TrustedClass> ;
        <http://www.w3.org/2000/01/rdf-schema#subPropertyOf>
                <http://purl.org/dqm-vocabulary/v1/dqm#dataElementRelationship> .

<http://purl.org/dqm-vocabulary/v1/dqm#BlacklistProperty>
        a       <http://www.w3.org/2002/07/owl#Class> ;
        <http://www.w3.org/2000/01/rdf-schema#comment>
                "A blacklist property holds the values that are disallowed for a certain data set."@en ;
        <http://www.w3.org/2000/01/rdf-schema#label>
                "Blacklist Property"@en ;
        <http://www.w3.org/2000/01/rdf-schema#subClassOf>
                <http://purl.org/dqm-vocabulary/v1/dqm#DataElement> .

<http://purl.org/dqm-vocabulary/v1/dqm#OutdatedInstanceRule>
        a       <http://www.w3.org/2002/07/owl#Class> ;
        <http://www.w3.org/2000/01/rdf-schema#comment>
                "An outdated instance rule is a data requirement that specifies the point in time when an instance is not current anymore."@en ;
        <http://www.w3.org/2000/01/rdf-schema#label>
                "Outdated Instance Rule"@en ;
        <http://www.w3.org/2000/01/rdf-schema#subClassOf>
                <http://purl.org/dqm-vocabulary/v1/dqm#ClassRequirement> .

<http://purl.org/dqm-vocabulary/v1/dqm#confidence>
        a       <http://www.w3.org/2002/07/owl#DatatypeProperty> , <http://www.w3.org/2002/07/owl#FunctionalProperty> ;
        <http://www.w3.org/2000/01/rdf-schema#comment>
                "The confidence property indicates how confident a rule creators is regarding the correctness of the rule."@en ;
        <http://www.w3.org/2000/01/rdf-schema#domain>
                <http://purl.org/dqm-vocabulary/v1/dqm#DataRequirement> ;
        <http://www.w3.org/2000/01/rdf-schema#label>
                "Confidence"@en ;
        <http://www.w3.org/2000/01/rdf-schema#range>
                <http://www.w3.org/2000/01/rdf-schema#Literal> ;
        <http://www.w3.org/2000/01/rdf-schema#subPropertyOf>
                <http://purl.org/dqm-vocabulary/v1/dqm#reqMetadata> .

<http://purl.org/dqm-vocabulary/v1/dqm#upperLimit>
        a       <http://www.w3.org/2002/07/owl#DatatypeProperty> , <http://www.w3.org/2002/07/owl#FunctionalProperty> ;
        <http://www.w3.org/2000/01/rdf-schema#comment>
                "Specifies the upper limit a numeric property value shall obtain."@en ;
        <http://www.w3.org/2000/01/rdf-schema#domain>
                [ a       <http://www.w3.org/2002/07/owl#Class> ;
                  <http://www.w3.org/2002/07/owl#unionOf>
                          ( <http://purl.org/dqm-vocabulary/v1/dqm#IllegalValueRangeRule> <http://purl.org/dqm-vocabulary/v1/dqm#LegalValueRangeRule> <http://purl.org/dqm-vocabulary/v1/dqm#Unit> )
                ] ;
        <http://www.w3.org/2000/01/rdf-schema#label>
                "Upper Limit"@en ;
        <http://www.w3.org/2000/01/rdf-schema#range>
                <http://www.w3.org/2001/XMLSchema#float> .

<http://purl.org/dqm-vocabulary/v1/dqm#cleansing>
        a       <http://www.w3.org/2002/07/owl#FunctionalProperty> , <http://www.w3.org/2002/07/owl#DatatypeProperty> ;
        <http://www.w3.org/2000/01/rdf-schema#comment>
                "The data cleansing property specifies whether the rule shall be applied to cleanse the data in a data source."@en ;
        <http://www.w3.org/2000/01/rdf-schema#domain>
                <http://purl.org/dqm-vocabulary/v1/dqm#DataRequirement> ;
        <http://www.w3.org/2000/01/rdf-schema#label>
                "Cleansing"@en ;
        <http://www.w3.org/2000/01/rdf-schema#range>
                <http://www.w3.org/2001/XMLSchema#boolean> ;
        <http://www.w3.org/2000/01/rdf-schema#subPropertyOf>
                <http://purl.org/dqm-vocabulary/v1/dqm#reqMetadata> .

<http://purl.org/dqm-vocabulary/v1/dqm#filtering>
        a       <http://www.w3.org/2002/07/owl#FunctionalProperty> , <http://www.w3.org/2002/07/owl#DatatypeProperty> ;
        <http://www.w3.org/2000/01/rdf-schema#comment>
                "The filtering property indicates whether the rule shall be used for information filtering, i.e. only high quality data is retrieved."@en ;
        <http://www.w3.org/2000/01/rdf-schema#domain>
                <http://purl.org/dqm-vocabulary/v1/dqm#DataRequirement> ;
        <http://www.w3.org/2000/01/rdf-schema#label>
                "Filtering"@en ;
        <http://www.w3.org/2000/01/rdf-schema#range>
                <http://www.w3.org/2001/XMLSchema#boolean> ;
        <http://www.w3.org/2000/01/rdf-schema#subPropertyOf>
                <http://purl.org/dqm-vocabulary/v1/dqm#reqMetadata> .

<http://purl.org/dqm-vocabulary/v1/dqm#Task>
        a       <http://www.w3.org/2002/07/owl#Class> ;
        <http://www.w3.org/2000/01/rdf-schema#comment>
                "Classifies the tasks for which the data quality rule shall apply for."@en ;
        <http://www.w3.org/2000/01/rdf-schema#label>
                "Task"@en .

<http://purl.org/dqm-vocabulary/v1/dqm#technicalName>
        a       <http://www.w3.org/2002/07/owl#FunctionalProperty> , <http://www.w3.org/2002/07/owl#DatatypeProperty> ;
        <http://www.w3.org/2000/01/rdf-schema#comment>
                "Technical name of a value."@en ;
        <http://www.w3.org/2000/01/rdf-schema#domain>
                <http://purl.org/dqm-vocabulary/v1/dqm#ScaleValue> ;
        <http://www.w3.org/2000/01/rdf-schema#label>
                "Technical Name"@en ;
        <http://www.w3.org/2000/01/rdf-schema#range>
                <http://www.w3.org/2001/XMLSchema#string> .

<http://purl.org/dqm-vocabulary/v1/dqm#OutOfRangeValue>
        a       <http://www.w3.org/2002/07/owl#Class> ;
        <http://www.w3.org/2000/01/rdf-schema#comment>
                "A value is out of range when it is not part of the legal value range or when it is part of the illegal value range."@en ;
        <http://www.w3.org/2000/01/rdf-schema#label>
                "Out of Range Value" ;
        <http://www.w3.org/2000/01/rdf-schema#subClassOf>
                <http://purl.org/dqm-vocabulary/v1/dqm#DataRequirementViolation> .

<http://purl.org/dqm-vocabulary/v1/dqm#commonCode>
        a       <http://www.w3.org/2002/07/owl#FunctionalProperty> , <http://www.w3.org/2002/07/owl#DatatypeProperty> ;
        <http://www.w3.org/2000/01/rdf-schema#comment>
                "UN/CEFACT common code of a unit of measurement."@en ;
        <http://www.w3.org/2000/01/rdf-schema#domain>
                <http://purl.org/dqm-vocabulary/v1/dqm#Unit> ;
        <http://www.w3.org/2000/01/rdf-schema#label>
                "UN/CEFACT common code"@en ;
        <http://www.w3.org/2000/01/rdf-schema#range>
                <http://www.w3.org/2001/XMLSchema#string> .

<http://purl.org/dc/terms/license>
        a       <http://www.w3.org/2002/07/owl#AnnotationProperty> .

<http://purl.org/dqm-vocabulary/v1/dqm#affectedProperty>
        a       <http://www.w3.org/2002/07/owl#ObjectProperty> ;
        <http://www.w3.org/2000/01/rdf-schema#comment>
                "An affected property specifies the property of a data instance that contains one or more data requirement violations. Some data requirement violations, such as functional dependency violations, have more than one affected property."@de ;
        <http://www.w3.org/2000/01/rdf-schema#domain>
                <http://purl.org/dqm-vocabulary/v1/dqm#DataRequirementViolation> ;
        <http://www.w3.org/2000/01/rdf-schema#label>
                "Affected Property"@de ;
        <http://www.w3.org/2000/01/rdf-schema#range>
                <http://purl.org/dqm-vocabulary/v1/dqm#AffectedProperty> ;
        <http://www.w3.org/2000/01/rdf-schema#subPropertyOf>
                <http://purl.org/dqm-vocabulary/v1/dqm#dataElementRelationship> .

<http://purl.org/dqm-vocabulary/v1/dqm#FunctionalDependencyViolation>
        a       <http://www.w3.org/2002/07/owl#Class> ;
        <http://www.w3.org/2000/01/rdf-schema#comment>
                "A functional dependency violation is a combination of different property values within the same instance that must not occur together. E.g. an instance describing the man “Peter Miller” has the value “Mr.” as salutation property, but the value “female” as sex."@en ;
        <http://www.w3.org/2000/01/rdf-schema#label>
                "Functional Dependency Violation"@en ;
        <http://www.w3.org/2000/01/rdf-schema#subClassOf>
                <http://purl.org/dqm-vocabulary/v1/dqm#DataRequirementViolation> .

<http://purl.org/dqm-vocabulary/v1/dqm#endsWith>
        a       <http://www.w3.org/2002/07/owl#FunctionalProperty> , <http://www.w3.org/2002/07/owl#DatatypeProperty> ;
        <http://www.w3.org/2000/01/rdf-schema#comment>
                "Holds one or more consecutive characters that are supposed to be found at the end of strings of another property."@en ;
        <http://www.w3.org/2000/01/rdf-schema#domain>
                [ a       <http://www.w3.org/2002/07/owl#Class> ;
                  <http://www.w3.org/2002/07/owl#unionOf>
                          ( <http://purl.org/dqm-vocabulary/v1/dqm#Condition> <http://purl.org/dqm-vocabulary/v1/dqm#FuncDepValueRule> )
                ] ;
        <http://www.w3.org/2000/01/rdf-schema#label>
                "Ends With"@en ;
        <http://www.w3.org/2000/01/rdf-schema#range>
                <http://www.w3.org/2001/XMLSchema#string> ;
        <http://www.w3.org/2000/01/rdf-schema#subPropertyOf>
                <http://purl.org/dqm-vocabulary/v1/dqm#operatedValue> .

<http://purl.org/dqm-vocabulary/v1/dqm#DataCleansingRule>
        a       <http://www.w3.org/2002/07/owl#Class> ;
        <http://www.w3.org/2000/01/rdf-schema#comment>
                "A data cleansing rule is an unambiguous rule that precisely specifies the required state of a data value."@en ;
        <http://www.w3.org/2000/01/rdf-schema#label>
                "Data Cleansing Rule"@en .

<http://purl.org/dqm-vocabulary/v1/dqm#addValue>
        a       <http://www.w3.org/2002/07/owl#DatatypeProperty> , <http://www.w3.org/2002/07/owl#FunctionalProperty> ;
        <http://www.w3.org/2000/01/rdf-schema#comment>
                "A value that shall be added to a property of an instance."@en ;
        <http://www.w3.org/2000/01/rdf-schema#domain>
                <http://purl.org/dqm-vocabulary/v1/dqm#PropertyCompletion> ;
        <http://www.w3.org/2000/01/rdf-schema#label>
                "Add Value"@en ;
        <http://www.w3.org/2000/01/rdf-schema#range>
                <http://www.w3.org/2001/XMLSchema#string> ;
        <http://www.w3.org/2000/01/rdf-schema#subPropertyOf>
                <http://purl.org/dqm-vocabulary/v1/dqm#cleansingProperty> .

<http://purl.org/dqm-vocabulary/v1/dqm#MultiPropertyRequirement>
        a       <http://www.w3.org/2002/07/owl#Class> ;
        <http://www.w3.org/2000/01/rdf-schema#comment>
                "Multi property requirements are data requirements that consider values from two or more properties."@en ;
        <http://www.w3.org/2000/01/rdf-schema#label>
                "Multi Property Requirement"@en ;
        <http://www.w3.org/2000/01/rdf-schema#subClassOf>
                <http://purl.org/dqm-vocabulary/v1/dqm#DataRequirement> .

<http://purl.org/dqm-vocabulary/v1/dqm#taskDescription>
        a       <http://www.w3.org/2002/07/owl#DatatypeProperty> ;
        <http://www.w3.org/2000/01/rdf-schema#comment>
                "Describes the task in natural language."@en ;
        <http://www.w3.org/2000/01/rdf-schema#domain>
                <http://purl.org/dqm-vocabulary/v1/dqm#Task> ;
        <http://www.w3.org/2000/01/rdf-schema#label>
                "Task Description"@en ;
        <http://www.w3.org/2000/01/rdf-schema#range>
                <http://www.w3.org/2001/XMLSchema#string> .

<http://purl.org/dqm-vocabulary/v1/dqm#LegalValueRangeRule>
        a       <http://www.w3.org/2002/07/owl#Class> ;
        <http://www.w3.org/2000/01/rdf-schema#comment>
                "A legal value range rule is a property requirement that specifies the upper and/or lower boundary of numeric values that a certain property is allowed to obtain."@en ;
        <http://www.w3.org/2000/01/rdf-schema#label>
                "Legal Value Range Rule"@en ;
        <http://www.w3.org/2000/01/rdf-schema#subClassOf>
                <http://purl.org/dqm-vocabulary/v1/dqm#PropertyRequirement> .

<http://purl.org/dqm-vocabulary/v1/dqm#unitOfConfidence>
        a       <http://www.w3.org/2002/07/owl#ObjectProperty> , <http://www.w3.org/2002/07/owl#FunctionalProperty> ;
        <http://www.w3.org/2000/01/rdf-schema#comment>
                "The unit in which confidence is expressed."@en ;
        <http://www.w3.org/2000/01/rdf-schema#domain>
                <http://purl.org/dqm-vocabulary/v1/dqm#DataRequirement> ;
        <http://www.w3.org/2000/01/rdf-schema#label>
                "Unit of Confidence"@en ;
        <http://www.w3.org/2000/01/rdf-schema#range>
                <http://purl.org/dqm-vocabulary/v1/dqm#Unit> .

<http://purl.org/dqm-vocabulary/v1/dqm#conditionalProperty>
        a       <http://www.w3.org/2002/07/owl#ObjectProperty> , <http://www.w3.org/2002/07/owl#FunctionalProperty> ;
        <http://www.w3.org/2000/01/rdf-schema#comment>
                "The conditional property property indicates the URI of a property that holds values that can be used to filter the relevant subset of data for which a rule applies."@en ;
        <http://www.w3.org/2000/01/rdf-schema#domain>
                <http://purl.org/dqm-vocabulary/v1/dqm#Condition> ;
        <http://www.w3.org/2000/01/rdf-schema#label>
                "Conditional Property"@en ;
        <http://www.w3.org/2000/01/rdf-schema#range>
                <http://purl.org/dqm-vocabulary/v1/dqm#TestedProperty> ;
        <http://www.w3.org/2000/01/rdf-schema#subPropertyOf>
                <http://purl.org/dqm-vocabulary/v1/dqm#dataElementRelationship> .

<http://purl.org/dqm-vocabulary/v1/dqm#DataQualityScore>
        a       <http://www.w3.org/2002/07/owl#Class> ;
        <http://www.w3.org/2000/01/rdf-schema#comment>
                "Data quality score is an abstract class that can be used to structure data quality dimension scores that indicate the quality state of classes and/or properties."@en ;
        <http://www.w3.org/2000/01/rdf-schema#label>
                "Data Quality Assessment"@en .

<http://purl.org/dqm-vocabulary/v1/dqm#unitOfImportance>
        a       <http://www.w3.org/2002/07/owl#FunctionalProperty> , <http://www.w3.org/2002/07/owl#ObjectProperty> ;
        <http://www.w3.org/2000/01/rdf-schema#comment>
                "The unit in which importance is expressed."@en ;
        <http://www.w3.org/2000/01/rdf-schema#domain>
                [ a       <http://www.w3.org/2002/07/owl#Class> ;
                  <http://www.w3.org/2002/07/owl#unionOf>
                          ( <http://purl.org/dqm-vocabulary/v1/dqm#DataElement> <http://purl.org/dqm-vocabulary/v1/dqm#DataRequirement> <http://purl.org/dqm-vocabulary/v1/dqm#Task> )
                ] ;
        <http://www.w3.org/2000/01/rdf-schema#label>
                "Unit of Importance"@en ;
        <http://www.w3.org/2000/01/rdf-schema#range>
                <http://purl.org/dqm-vocabulary/v1/dqm#Unit> .

<http://purl.org/dqm-vocabulary/v1/dqm#validUntil>
        a       <http://www.w3.org/2002/07/owl#DatatypeProperty> , <http://www.w3.org/2002/07/owl#FunctionalProperty> ;
        <http://www.w3.org/2000/01/rdf-schema#comment>
                "Specifies the date and time until a rule stays valid."@en ;
        <http://www.w3.org/2000/01/rdf-schema#domain>
                [ a       <http://www.w3.org/2002/07/owl#Class> ;
                  <http://www.w3.org/2002/07/owl#unionOf>
                          ( <http://purl.org/dqm-vocabulary/v1/dqm#DataCleansingRule> <http://purl.org/dqm-vocabulary/v1/dqm#DataRequirement> )
                ] ;
        <http://www.w3.org/2000/01/rdf-schema#label>
                "Valid Until"@en ;
        <http://www.w3.org/2000/01/rdf-schema#range>
                <http://www.w3.org/2001/XMLSchema#dateTime> ;
        <http://www.w3.org/2000/01/rdf-schema#subPropertyOf>
                <http://purl.org/dqm-vocabulary/v1/dqm#reqMetadata> .

<http://purl.org/dqm-vocabulary/v1/dqm#MatchingValueRule>
        a       <http://www.w3.org/2002/07/owl#Class> ;
        <http://www.w3.org/2000/01/rdf-schema#comment>
                "Matching value rules are multi property requirements in which the property values of other instances are used to identify data requirements violations in an instance."@en ;
        <http://www.w3.org/2000/01/rdf-schema#label>
                "Matching Value Rule"@en ;
        <http://www.w3.org/2000/01/rdf-schema#subClassOf>
                <http://purl.org/dqm-vocabulary/v1/dqm#MultiPropertyRequirement> .

<http://purl.org/dqm-vocabulary/v1/dqm#taskName>
        a       <http://www.w3.org/2002/07/owl#DatatypeProperty> ;
        <http://www.w3.org/2000/01/rdf-schema#comment>
                "Specifies the name of the task."@en ;
        <http://www.w3.org/2000/01/rdf-schema#domain>
                <http://purl.org/dqm-vocabulary/v1/dqm#Task> ;
        <http://www.w3.org/2000/01/rdf-schema#label>
                "Task Name"@en ;
        <http://www.w3.org/2000/01/rdf-schema#range>
                <http://www.w3.org/2001/XMLSchema#string> .

<http://purl.org/dqm-vocabulary/v1/dqm#cleansesProperty1>
        a       <http://www.w3.org/2002/07/owl#FunctionalProperty> , <http://www.w3.org/2002/07/owl#ObjectProperty> ;
        <http://www.w3.org/2000/01/rdf-schema#comment>
                "This property identifies a property that holds values that shall be cleansed."@en ;
        <http://www.w3.org/2000/01/rdf-schema#domain>
                <http://purl.org/dqm-vocabulary/v1/dqm#DataCleansingRule> ;
        <http://www.w3.org/2000/01/rdf-schema#label>
                "Cleanses Property 1"@en ;
        <http://www.w3.org/2000/01/rdf-schema#range>
                <http://purl.org/dqm-vocabulary/v1/dqm#TestedProperty> ;
        <http://www.w3.org/2000/01/rdf-schema#subPropertyOf>
                <http://purl.org/dqm-vocabulary/v1/dqm#dataCleansingRuleRelationship> .

<http://purl.org/dqm-vocabulary/v1/dqm#pattern>
        a       <http://www.w3.org/2002/07/owl#FunctionalProperty> , <http://www.w3.org/2002/07/owl#DatatypeProperty> ;
        <http://www.w3.org/2000/01/rdf-schema#comment>
                "The pattern property can be used to express value patterns based on a simple syntax without the need for knowing regular expressions. E.g. the pattern \"AaaaaNN\" where \"A\" stands for capital letters, \"a\" for small letters, and \"N\" for numbers."@en ;
        <http://www.w3.org/2000/01/rdf-schema#domain>
                [ a       <http://www.w3.org/2002/07/owl#Class> ;
                  <http://www.w3.org/2002/07/owl#unionOf>
                          ( <http://purl.org/dqm-vocabulary/v1/dqm#ConditionalSyntaxRule> <http://purl.org/dqm-vocabulary/v1/dqm#SyntaxRule> )
                ] ;
        <http://www.w3.org/2000/01/rdf-schema#label>
                "Pattern"@en ;
        <http://www.w3.org/2000/01/rdf-schema#range>
                <http://www.w3.org/2001/XMLSchema#string> .

<http://purl.org/dqm-vocabulary/v1/dqm#UniqueValueRule>
        a       <http://www.w3.org/2002/07/owl#Class> ;
        <http://www.w3.org/2000/01/rdf-schema#comment>
                "A unique value rule is a property requirement that specifies that each value of a certain property must be unique in instances of a certain class."@en ;
        <http://www.w3.org/2000/01/rdf-schema#label>
                "Unique Value Rule"@en ;
        <http://www.w3.org/2000/01/rdf-schema#subClassOf>
                <http://purl.org/dqm-vocabulary/v1/dqm#PropertyRequirement> .

<http://purl.org/dqm-vocabulary/v1/dqm>
        a       <http://www.w3.org/2002/07/owl#Ontology> ;
        <http://www.w3.org/2000/01/rdf-schema#comment>
                "The Data Quality Management Vocabulary provides an ontology for the structured representation of data requirements, data quality assessment results, data cleansing rules, and data requirement violations connected to their origin. It, therefore, supports data quality monitoring, data quality assessment, and data cleansing in Semantic Web architectures."@en ;
        <http://www.w3.org/2000/01/rdf-schema#label>
                "The Data Quality Management Vocabulary - An Ontology for Data Requirements Management, Data Quality Monitoring, Data Quality Assessment, and Data Cleansing"@en ;
        <http://purl.org/dc/elements/1.1/creator>
                "Christian Fürber and Martin Hepp" ;
        <http://purl.org/dc/elements/1.1/rights>
                "The Data Quality Management Vocabulary is available under the Creative Commons Attribution - Non Commercial - Share Alike 3.0 Unported license; see http://creativecommons.org/licenses/by-nc-sa/3.0/. In a nutshell, you are free to copy, distribute and transmit the work and to remix/adapt the work (e.g. to import the ontology and create specializations of its elements) for non commercial purposes, as long as you attribute the work in the manner specified by the author or licensor (but not in any way that suggests that they endorse you or your use of the work). Proper Attribution: Simply include the statement \"This work is based on the Data Quality Management Vocabulary, developed by Christian Fürber and Martin Hepp\" and link back to http://purl.org/dqm-vocabulary ." ;
        <http://purl.org/dc/elements/1.1/subject>
                "Data Quality Management, Data Quality Assessment, Data Quality Monitoring, Data Profiling, Data Cleansing, Data Requirements Management" ;
        <http://purl.org/dc/elements/1.1/title>
                "The Data Quality Management Vocabulary" ;
        <http://purl.org/dc/terms/license>
                "http://creativecommons.org/licenses/by-nc-sa/3.0/" ;
        <http://www.w3.org/2002/07/owl#versionInfo>
                "V 1.00, Release 09-10-2011" .

<http://purl.org/dqm-vocabulary/v1/dqm#lowerLimit>
        a       <http://www.w3.org/2002/07/owl#DatatypeProperty> , <http://www.w3.org/2002/07/owl#FunctionalProperty> ;
        <http://www.w3.org/2000/01/rdf-schema#comment>
                "Specifies the lower limit a numeric property value shall obtain."@en ;
        <http://www.w3.org/2000/01/rdf-schema#domain>
                [ a       <http://www.w3.org/2002/07/owl#Class> ;
                  <http://www.w3.org/2002/07/owl#unionOf>
                          ( <http://purl.org/dqm-vocabulary/v1/dqm#IllegalValueRangeRule> <http://purl.org/dqm-vocabulary/v1/dqm#LegalValueRangeRule> <http://purl.org/dqm-vocabulary/v1/dqm#Unit> )
                ] ;
        <http://www.w3.org/2000/01/rdf-schema#label>
                "Lower Limit"@en ;
        <http://www.w3.org/2000/01/rdf-schema#range>
                <http://www.w3.org/2001/XMLSchema#float> .

<http://purl.org/dqm-vocabulary/v1/dqm#PropertyRequirement>
        a       <http://www.w3.org/2002/07/owl#Class> ;
        <http://www.w3.org/2000/01/rdf-schema#comment>
                "Property requirements are data requirements that are related to values of a single property."@en ;
        <http://www.w3.org/2000/01/rdf-schema#label>
                "Property Requirement"@en ;
        <http://www.w3.org/2000/01/rdf-schema#subClassOf>
                <http://purl.org/dqm-vocabulary/v1/dqm#DataRequirement> .

<http://purl.org/dqm-vocabulary/v1/dqm#testedProperty5>
        a       <http://www.w3.org/2002/07/owl#ObjectProperty> , <http://www.w3.org/2002/07/owl#FunctionalProperty> ;
        <http://www.w3.org/2000/01/rdf-schema#comment>
                "The property with the values that shall be tested for data quality problems."@en ;
        <http://www.w3.org/2000/01/rdf-schema#domain>
                <http://purl.org/dqm-vocabulary/v1/dqm#MatchingValueRule> ;
        <http://www.w3.org/2000/01/rdf-schema#label>
                "Tested Property 5"@en ;
        <http://www.w3.org/2000/01/rdf-schema#subPropertyOf>
                <http://purl.org/dqm-vocabulary/v1/dqm#testedProperty> .

<http://purl.org/dqm-vocabulary/v1/dqm#testedProperty4>
        a       <http://www.w3.org/2002/07/owl#ObjectProperty> , <http://www.w3.org/2002/07/owl#FunctionalProperty> ;
        <http://www.w3.org/2000/01/rdf-schema#comment>
                "The property with the values that shall be tested for data quality problems."@en ;
        <http://www.w3.org/2000/01/rdf-schema#domain>
                <http://purl.org/dqm-vocabulary/v1/dqm#MatchingValueRule> ;
        <http://www.w3.org/2000/01/rdf-schema#label>
                "Tested Property 4"@en ;
        <http://www.w3.org/2000/01/rdf-schema#subPropertyOf>
                <http://purl.org/dqm-vocabulary/v1/dqm#testedProperty> .

<http://purl.org/dqm-vocabulary/v1/dqm#testedProperty1>
        a       <http://www.w3.org/2002/07/owl#ObjectProperty> , <http://www.w3.org/2002/07/owl#FunctionalProperty> ;
        <http://www.w3.org/2000/01/rdf-schema#comment>
                "The property with the values that shall be tested for data quality problems."@en ;
        <http://www.w3.org/2000/01/rdf-schema#domain>
                <http://purl.org/dqm-vocabulary/v1/dqm#DataRequirement> ;
        <http://www.w3.org/2000/01/rdf-schema#label>
                "Tested Property 1"@en ;
        <http://www.w3.org/2000/01/rdf-schema#subPropertyOf>
                <http://purl.org/dqm-vocabulary/v1/dqm#testedProperty> .

<http://purl.org/dqm-vocabulary/v1/dqm#testedProperty2>
        a       <http://www.w3.org/2002/07/owl#ObjectProperty> , <http://www.w3.org/2002/07/owl#FunctionalProperty> ;
        <http://www.w3.org/2000/01/rdf-schema#comment>
                "The property with the values that shall be tested for data quality problems."@en ;
        <http://www.w3.org/2000/01/rdf-schema#domain>
                <http://purl.org/dqm-vocabulary/v1/dqm#MatchingValueRule> ;
        <http://www.w3.org/2000/01/rdf-schema#label>
                "Tested Property 2"@en ;
        <http://www.w3.org/2000/01/rdf-schema#subPropertyOf>
                <http://purl.org/dqm-vocabulary/v1/dqm#testedProperty> .

<http://purl.org/dqm-vocabulary/v1/dqm#testedProperty3>
        a       <http://www.w3.org/2002/07/owl#ObjectProperty> , <http://www.w3.org/2002/07/owl#FunctionalProperty> ;
        <http://www.w3.org/2000/01/rdf-schema#comment>
                "The property with the values that shall be tested for data quality problems."@en ;
        <http://www.w3.org/2000/01/rdf-schema#domain>
                <http://purl.org/dqm-vocabulary/v1/dqm#MatchingValueRule> ;
        <http://www.w3.org/2000/01/rdf-schema#label>
                "Tested Property 3"@en ;
        <http://www.w3.org/2000/01/rdf-schema#subPropertyOf>
                <http://purl.org/dqm-vocabulary/v1/dqm#testedProperty> .

<http://purl.org/dqm-vocabulary/v1/dqm#addProperty>
        a       <http://www.w3.org/2002/07/owl#FunctionalProperty> , <http://www.w3.org/2002/07/owl#DatatypeProperty> ;
        <http://www.w3.org/2000/01/rdf-schema#comment>
                "A property that shall be added to an instance."@en ;
        <http://www.w3.org/2000/01/rdf-schema#domain>
                <http://purl.org/dqm-vocabulary/v1/dqm#PropertyCompletion> ;
        <http://www.w3.org/2000/01/rdf-schema#label>
                "Add Property"@en ;
        <http://www.w3.org/2000/01/rdf-schema#range>
                <http://www.w3.org/2001/XMLSchema#anyURI> ;
        <http://www.w3.org/2000/01/rdf-schema#subPropertyOf>
                <http://purl.org/dqm-vocabulary/v1/dqm#cleansingProperty> .

<http://purl.org/dqm-vocabulary/v1/dqm#DataRequirement>
        a       <http://www.w3.org/2002/07/owl#Class> ;
        <http://www.w3.org/2000/01/rdf-schema#comment>
                "A data requirement is a prescribed directive or consensual agreement that defines the content and/or structure that constitute high quality data instances and values."@en ;
        <http://www.w3.org/2000/01/rdf-schema#label>
                "Data Requirement"@en .

<http://purl.org/dqm-vocabulary/v1/dqm#SyntaxRule>
        a       <http://www.w3.org/2002/07/owl#Class> ;
        <http://www.w3.org/2000/01/rdf-schema#comment>
                "A syntax rule is a property requirement that specifies the allowed characters and/or character pattern to be used in values for a certain property in instances of a certain class."@en ;
        <http://www.w3.org/2000/01/rdf-schema#label>
                "Syntax Rule"@en ;
        <http://www.w3.org/2000/01/rdf-schema#subClassOf>
                <http://purl.org/dqm-vocabulary/v1/dqm#PropertyRequirement> .

<http://purl.org/dqm-vocabulary/v1/dqm#hasURI>
        a       <http://www.w3.org/2002/07/owl#FunctionalProperty> , <http://www.w3.org/2002/07/owl#DatatypeProperty> ;
        <http://www.w3.org/2000/01/rdf-schema#comment>
                "The hasURI property is used to map properties to instances of a class."@en ;
        <http://www.w3.org/2000/01/rdf-schema#domain>
                <http://purl.org/dqm-vocabulary/v1/dqm#DataElement> ;
        <http://www.w3.org/2000/01/rdf-schema#label>
                "Has URI"@en ;
        <http://www.w3.org/2000/01/rdf-schema#range>
                <http://www.w3.org/2001/XMLSchema#anyURI> .

<http://purl.org/dqm-vocabulary/v1/dqm#PropertyUniqueness>
        a       <http://www.w3.org/2002/07/owl#Class> ;
        <http://www.w3.org/2000/01/rdf-schema#comment>
                "Property uniqueness is the degree to which the values of a property (that must only contain unique values within instances of a certain class) are unique."@en ;
        <http://www.w3.org/2000/01/rdf-schema#label>
                "Property Uniqueness"@en ;
        <http://www.w3.org/2000/01/rdf-schema#subClassOf>
                <http://purl.org/dqm-vocabulary/v1/dqm#Uniqueness> .

<http://purl.org/dqm-vocabulary/v1/dqm#MissingValue>
        a       <http://www.w3.org/2002/07/owl#Class> ;
        <http://www.w3.org/2000/01/rdf-schema#comment>
                "A missing value occurs when a property of an instance does not hold a value."@en ;
        <http://www.w3.org/2000/01/rdf-schema#label>
                "Missing Value"@en ;
        <http://www.w3.org/2000/01/rdf-schema#subClassOf>
                <http://purl.org/dqm-vocabulary/v1/dqm#MissingElement> .

<http://purl.org/dc/elements/1.1/rights>
        a       <http://www.w3.org/2002/07/owl#AnnotationProperty> .

<http://purl.org/dqm-vocabulary/v1/dqm#sparqlrule>
        a       <http://www.w3.org/2002/07/owl#DatatypeProperty> , <http://www.w3.org/2002/07/owl#FunctionalProperty> ;
        <http://www.w3.org/2000/01/rdf-schema#comment>
                "This property can store custom data requirements that are expressed via SPARQL queries."@en ;
        <http://www.w3.org/2000/01/rdf-schema#domain>
                <http://purl.org/dqm-vocabulary/v1/dqm#CustomRequirement> ;
        <http://www.w3.org/2000/01/rdf-schema#label>
                "SPARQL rule"@en ;
        <http://www.w3.org/2000/01/rdf-schema#range>
                <http://www.w3.org/2001/XMLSchema#string> .

<http://purl.org/dqm-vocabulary/v1/dqm#ClassRequirement>
        a       <http://www.w3.org/2002/07/owl#Class> ;
        <http://www.w3.org/2000/01/rdf-schema#comment>
                "A class requirement is a data requirement that refers to the instances of a class as a whole."@en ;
        <http://www.w3.org/2000/01/rdf-schema#label>
                "Class Requirement"@en ;
        <http://www.w3.org/2000/01/rdf-schema#subClassOf>
                <http://purl.org/dqm-vocabulary/v1/dqm#DataRequirement> .

<http://purl.org/dqm-vocabulary/v1/dqm#StrictValueCombination>
        a       <http://www.w3.org/2002/07/owl#Class> ;
        <http://www.w3.org/2000/01/rdf-schema#comment>
                "A strict value combination is a combination of two values of different properties that may only be assigned to each other, but not to other values."@en ;
        <http://www.w3.org/2000/01/rdf-schema#label>
                "Strict Value Combination Rule"@en ;
        <http://www.w3.org/2000/01/rdf-schema#subClassOf>
                <http://purl.org/dqm-vocabulary/v1/dqm#MultiPropertyCleansingRule> .

<http://purl.org/dqm-vocabulary/v1/dqm#scaleValues>
        a       <http://www.w3.org/2002/07/owl#ObjectProperty> ;
        <http://www.w3.org/2000/01/rdf-schema#comment>
                "Links to values of a certain ordinal or nominal scale."@en ;
        <http://www.w3.org/2000/01/rdf-schema#domain>
                <http://purl.org/dqm-vocabulary/v1/dqm#Unit> ;
        <http://www.w3.org/2000/01/rdf-schema#label>
                "Scale Values"@en ;
        <http://www.w3.org/2000/01/rdf-schema#range>
                <http://purl.org/dqm-vocabulary/v1/dqm#ScaleValue> .

<http://purl.org/dqm-vocabulary/v1/dqm#ConditionalRule>
        a       <http://www.w3.org/2002/07/owl#Class> ;
        <http://www.w3.org/2000/01/rdf-schema#comment>
                "A conditional rule is a multi property requirement that can be used to specify that values of a tested property A must always obtain a certain state under the condition that values of another property B obtain a certain state (condition)."@en ;
        <http://www.w3.org/2000/01/rdf-schema#label>
                "Conditional Rule"@en ;
        <http://www.w3.org/2000/01/rdf-schema#subClassOf>
                <http://purl.org/dqm-vocabulary/v1/dqm#MultiPropertyRequirement> .

<http://purl.org/dqm-vocabulary/v1/dqm#DataElement>
        a       <http://www.w3.org/2002/07/owl#Class> ;
        <http://www.w3.org/2000/01/rdf-schema#comment>
                "A data element is a class, a property, an instance, or a literal value."@en ;
        <http://www.w3.org/2000/01/rdf-schema#label>
                "Data Element"@en .

<http://purl.org/dqm-vocabulary/v1/dqm#ScaleValue>
        a       <http://www.w3.org/2002/07/owl#Class> ;
        <http://www.w3.org/2000/01/rdf-schema#comment>
                "A scale value is a value of a nominal or ordinal scale."@en ;
        <http://www.w3.org/2000/01/rdf-schema#label>
                "Scale Value"@en .

<http://purl.org/dqm-vocabulary/v1/dqm#DuplicateInstanceRule>
        a       <http://www.w3.org/2002/07/owl#Class> ;
        <http://www.w3.org/2000/01/rdf-schema#comment>
                "A duplicate instance rule is a multi property requirement which specifies the properties that (when seen together) uniquely identify an entity. I.e. if the properties of two or more different instances represent the same state, then the instances represent the same entity. Thus, the instances are considered to be duplicates."@en ;
        <http://www.w3.org/2000/01/rdf-schema#label>
                "Duplicate Instance Rule"@en ;
        <http://www.w3.org/2000/01/rdf-schema#subClassOf>
                <http://purl.org/dqm-vocabulary/v1/dqm#MatchingValueRule> .

<http://purl.org/dqm-vocabulary/v1/dqm#WhitespaceRemoval>
        a       <http://www.w3.org/2002/07/owl#Class> ;
        <http://www.w3.org/2000/01/rdf-schema#comment>
                "A white space removal rule states that whitespaces at the beginning of a string and at the end of a string shall be removed for the specified property."@en ;
        <http://www.w3.org/2000/01/rdf-schema#label>
                "White Space Removal Rule"@en ;
        <http://www.w3.org/2000/01/rdf-schema#subClassOf>
                <http://purl.org/dqm-vocabulary/v1/dqm#LiteralCleansingRule> .

<http://purl.org/dqm-vocabulary/v1/dqm#lessThan>
        a       <http://www.w3.org/2002/07/owl#FunctionalProperty> , <http://www.w3.org/2002/07/owl#DatatypeProperty> ;
        <http://www.w3.org/2000/01/rdf-schema#comment>
                "Holds a numeric value that is used to identify values of a property that are less than the value of this property."@en ;
        <http://www.w3.org/2000/01/rdf-schema#domain>
                [ a       <http://www.w3.org/2002/07/owl#Class> ;
                  <http://www.w3.org/2002/07/owl#unionOf>
                          ( <http://purl.org/dqm-vocabulary/v1/dqm#Condition> <http://purl.org/dqm-vocabulary/v1/dqm#FuncDepValueRule> )
                ] ;
        <http://www.w3.org/2000/01/rdf-schema#label>
                "Less Than"@en ;
        <http://www.w3.org/2000/01/rdf-schema#range>
                <http://www.w3.org/2001/XMLSchema#float> ;
        <http://www.w3.org/2000/01/rdf-schema#subPropertyOf>
                <http://purl.org/dqm-vocabulary/v1/dqm#operatedValue> .

<http://purl.org/dqm-vocabulary/v1/dqm#newValue>
        a       <http://www.w3.org/2002/07/owl#DatatypeProperty> , <http://www.w3.org/2002/07/owl#FunctionalProperty> ;
        <http://www.w3.org/2000/01/rdf-schema#comment>
                "The new value property specifies the new value which shall substitute the current value."@en ;
        <http://www.w3.org/2000/01/rdf-schema#domain>
                <http://purl.org/dqm-vocabulary/v1/dqm#ValueSubstitution> ;
        <http://www.w3.org/2000/01/rdf-schema#label>
                "New Value"@en ;
        <http://www.w3.org/2000/01/rdf-schema#range>
                <http://www.w3.org/2001/XMLSchema#string> ;
        <http://www.w3.org/2000/01/rdf-schema#subPropertyOf>
                <http://purl.org/dqm-vocabulary/v1/dqm#cleansingProperty> .

<http://purl.org/dqm-vocabulary/v1/dqm#AffectedProperty>
        a       <http://www.w3.org/2002/07/owl#Class> ;
        <http://www.w3.org/2000/01/rdf-schema#comment>
                "An affected property specifies the property of a data instance that contains one or more data quality problems."@en ;
        <http://www.w3.org/2000/01/rdf-schema#label>
                "Affected Property" ;
        <http://www.w3.org/2000/01/rdf-schema#subClassOf>
                <http://purl.org/dqm-vocabulary/v1/dqm#DataElement> .

<http://purl.org/dqm-vocabulary/v1/dqm#MissingProperty>
        a       <http://www.w3.org/2002/07/owl#Class> ;
        <http://www.w3.org/2000/01/rdf-schema#comment>
                "A property is missing when an instances does not contain a specific property that is required."@en ;
        <http://www.w3.org/2000/01/rdf-schema#label>
                "Missing Property"@en ;
        <http://www.w3.org/2000/01/rdf-schema#subClassOf>
                <http://purl.org/dqm-vocabulary/v1/dqm#MissingElement> .

<http://purl.org/dqm-vocabulary/v1/dqm#officialName>
        a       <http://www.w3.org/2002/07/owl#DatatypeProperty> , <http://www.w3.org/2002/07/owl#FunctionalProperty> ;
        <http://www.w3.org/2000/01/rdf-schema#comment>
                "Official name of a value."@en ;
        <http://www.w3.org/2000/01/rdf-schema#domain>
                <http://purl.org/dqm-vocabulary/v1/dqm#ScaleValue> ;
        <http://www.w3.org/2000/01/rdf-schema#label>
                "Official Name"@en ;
        <http://www.w3.org/2000/01/rdf-schema#range>
                <http://www.w3.org/2001/XMLSchema#string> .

<http://purl.org/dqm-vocabulary/v1/dqm#SemanticAccuracy>
        a       <http://www.w3.org/2002/07/owl#Class> ;
        <http://www.w3.org/2000/01/rdf-schema#comment>
                "Semantic accuracy is the degree to which the data values of an instance represent the correct state of an entity’s property."@en ;
        <http://www.w3.org/2000/01/rdf-schema#label>
                "Semantic Accuracy"@en ;
        <http://www.w3.org/2000/01/rdf-schema#subClassOf>
                <http://purl.org/dqm-vocabulary/v1/dqm#Accuracy> .

<http://purl.org/dqm-vocabulary/v1/dqm#hasRequirement>
        a       <http://www.w3.org/2002/07/owl#ObjectProperty> ;
        <http://www.w3.org/2000/01/rdf-schema#comment>
                "Specifies the data requirements that have to be fulfilled to perform the task."@en ;
        <http://www.w3.org/2000/01/rdf-schema#domain>
                <http://purl.org/dqm-vocabulary/v1/dqm#Task> ;
        <http://www.w3.org/2000/01/rdf-schema#label>
                "Has Requirement"@en ;
        <http://www.w3.org/2000/01/rdf-schema#range>
                <http://purl.org/dqm-vocabulary/v1/dqm#DataRequirement> ;
        <http://www.w3.org/2000/01/rdf-schema#subPropertyOf>
                <http://purl.org/dqm-vocabulary/v1/dqm#dataRequirementsRelationship> .

<http://purl.org/dqm-vocabulary/v1/dqm#reqDescription>
        a       <http://www.w3.org/2002/07/owl#DatatypeProperty> ;
        <http://www.w3.org/2000/01/rdf-schema#comment>
                "Describes a data requirement in natural language."@en ;
        <http://www.w3.org/2000/01/rdf-schema#domain>
                <http://purl.org/dqm-vocabulary/v1/dqm#DataRequirement> ;
        <http://www.w3.org/2000/01/rdf-schema#label>
                "Requirement Description"@en ;
        <http://www.w3.org/2000/01/rdf-schema#range>
                <http://www.w3.org/2001/XMLSchema#string> ;
        <http://www.w3.org/2000/01/rdf-schema#subPropertyOf>
                <http://purl.org/dqm-vocabulary/v1/dqm#reqMetadata> .

<http://purl.org/dqm-vocabulary/v1/dqm#taskDependent>
        a       <http://www.w3.org/2002/07/owl#FunctionalProperty> , <http://www.w3.org/2002/07/owl#DatatypeProperty> ;
        <http://www.w3.org/2000/01/rdf-schema#comment>
                "Specifies whether the data quality rule is task dependent."@en ;
        <http://www.w3.org/2000/01/rdf-schema#domain>
                <http://purl.org/dqm-vocabulary/v1/dqm#DataRequirement> ;
        <http://www.w3.org/2000/01/rdf-schema#label>
                "Task Dependent"@en ;
        <http://www.w3.org/2000/01/rdf-schema#range>
                <http://www.w3.org/2001/XMLSchema#boolean> ;
        <http://www.w3.org/2000/01/rdf-schema#subPropertyOf>
                <http://purl.org/dqm-vocabulary/v1/dqm#reqMetadata> .

<http://purl.org/dqm-vocabulary/v1/dqm#DuplicateInstance>
        a       <http://www.w3.org/2002/07/owl#Class> ;
        <http://www.w3.org/2000/01/rdf-schema#comment>
                "Two or more instances are duplicates when they represent the same real world entity."@en ;
        <http://www.w3.org/2000/01/rdf-schema#label>
                "Duplicate Instance"@en ;
        <http://www.w3.org/2000/01/rdf-schema#subClassOf>
                <http://purl.org/dqm-vocabulary/v1/dqm#DataRequirementViolation> .

<http://purl.org/dqm-vocabulary/v1/dqm#requiredValue>
        a       <http://www.w3.org/2002/07/owl#FunctionalProperty> , <http://www.w3.org/2002/07/owl#DatatypeProperty> ;
        <http://www.w3.org/2000/01/rdf-schema#comment>
                "Specifies whether a value for a property must exist."@en ;
        <http://www.w3.org/2000/01/rdf-schema#domain>
                [ a       <http://www.w3.org/2002/07/owl#Class> ;
                  <http://www.w3.org/2002/07/owl#unionOf>
                          ( <http://purl.org/dqm-vocabulary/v1/dqm#ConditionalPropertyCompletenessRule> <http://purl.org/dqm-vocabulary/v1/dqm#PropertyCompletenessRule> )
                ] ;
        <http://www.w3.org/2000/01/rdf-schema#label>
                "Required Value"@en ;
        <http://www.w3.org/2000/01/rdf-schema#range>
                <http://www.w3.org/2001/XMLSchema#boolean> .

<http://purl.org/dqm-vocabulary/v1/dqm#scaleType>
        a       <http://www.w3.org/2002/07/owl#DatatypeProperty> , <http://www.w3.org/2002/07/owl#FunctionalProperty> ;
        <http://www.w3.org/2000/01/rdf-schema#comment>
                "Type of statistical scale."@en ;
        <http://www.w3.org/2000/01/rdf-schema#domain>
                <http://purl.org/dqm-vocabulary/v1/dqm#Unit> ;
        <http://www.w3.org/2000/01/rdf-schema#label>
                "Scale Type"@en ;
        <http://www.w3.org/2000/01/rdf-schema#range>
                [ a       <http://www.w3.org/2002/07/owl#DataRange> ;
                  <http://www.w3.org/2002/07/owl#oneOf>
                          ( "interval" "nominal" "ordinal" "ratio" )
                ] .

<http://purl.org/dqm-vocabulary/v1/dqm#reqMetadata>
        a       <http://www.w3.org/2002/07/owl#DatatypeProperty> ;
        <http://www.w3.org/2000/01/rdf-schema#comment>
                "An abstract property that holds generic datatype properties that describe a data requirement."@en ;
        <http://www.w3.org/2000/01/rdf-schema#label>
                "Requirement Metadata"@en .

<http://purl.org/dqm-vocabulary/v1/dqm#PropertyCompleteness>
        a       <http://www.w3.org/2002/07/owl#Class> ;
        <http://www.w3.org/2000/01/rdf-schema#comment>
                "Property completeness is the degree to which values for a specific property are missing in entities of a specific class."@en ;
        <http://www.w3.org/2000/01/rdf-schema#label>
                "Property Completeness"@en ;
        <http://www.w3.org/2000/01/rdf-schema#subClassOf>
                <http://purl.org/dqm-vocabulary/v1/dqm#Completeness> .

<http://purl.org/dqm-vocabulary/v1/dqm#AffectedClass>
        a       <http://www.w3.org/2002/07/owl#Class> ;
        <http://www.w3.org/2000/01/rdf-schema#comment>
                "An affected class holds one or more affected instances"@en ;
        <http://www.w3.org/2000/01/rdf-schema#label>
                "Affected Class" ;
        <http://www.w3.org/2000/01/rdf-schema#subClassOf>
                <http://purl.org/dqm-vocabulary/v1/dqm#DataElement> .

<http://purl.org/dqm-vocabulary/v1/dqm#LiteralCleansingRule>
        a       <http://www.w3.org/2002/07/owl#Class> ;
        <http://www.w3.org/2000/01/rdf-schema#comment>
                "Literal cleansing rules can be used to cleanse the literal values of a certain property."@en ;
        <http://www.w3.org/2000/01/rdf-schema#label>
                "Literal Cleansing Rule"@en ;
        <http://www.w3.org/2000/01/rdf-schema#subClassOf>
                <http://purl.org/dqm-vocabulary/v1/dqm#DataCleansingRule> .

<http://purl.org/dqm-vocabulary/v1/dqm#DataRequirementViolation>
        a       <http://www.w3.org/2002/07/owl#Class> ;
        <http://www.w3.org/2000/01/rdf-schema#comment>
                "A data requirement violation occurs when a data value or a data instance does not meet its requirements."@en ;
        <http://www.w3.org/2000/01/rdf-schema#label>
                "Data Requirement Violation"@en .

<http://purl.org/dqm-vocabulary/v1/dqm#ConditionalSyntaxRule>
        a       <http://www.w3.org/2002/07/owl#Class> ;
        <http://www.w3.org/2000/01/rdf-schema#comment>
                "Conditional syntax rules define that the literal values of a tested property must follow a certain syntax when the value of another property obtains a certain state. E.g. the property foo:state must have a value with two capital letters when the property foo:country obtains the value \"USA\"."@en ;
        <http://www.w3.org/2000/01/rdf-schema#label>
                "Conditional Syntax Rule"@en ;
        <http://www.w3.org/2000/01/rdf-schema#subClassOf>
                <http://purl.org/dqm-vocabulary/v1/dqm#ConditionalRule> .

<http://purl.org/dqm-vocabulary/v1/dqm#affectedInstance>
        a       <http://www.w3.org/2002/07/owl#ObjectProperty> ;
        <http://www.w3.org/2000/01/rdf-schema#comment>
                "An affected instance is the data instance that contains one or more data requirement violations."@de ;
        <http://www.w3.org/2000/01/rdf-schema#domain>
                <http://purl.org/dqm-vocabulary/v1/dqm#DataRequirementViolation> ;
        <http://www.w3.org/2000/01/rdf-schema#label>
                "Affected Instance"@de ;
        <http://www.w3.org/2000/01/rdf-schema#range>
                <http://purl.org/dqm-vocabulary/v1/dqm#AffectedInstance> ;
        <http://www.w3.org/2000/01/rdf-schema#subPropertyOf>
                <http://purl.org/dqm-vocabulary/v1/dqm#dataElementRelationship> .

<http://purl.org/dqm-vocabulary/v1/dqm#assessedClass>
        a       <http://www.w3.org/2002/07/owl#ObjectProperty> ;
        <http://www.w3.org/2000/01/rdf-schema#comment>
                "The assessed class is the class that holds the instances that have been analyzed to compute the assessment score."@en ;
        <http://www.w3.org/2000/01/rdf-schema#domain>
                <http://purl.org/dqm-vocabulary/v1/dqm#DataQualityScore> ;
        <http://www.w3.org/2000/01/rdf-schema#label>
                "Assessed Class"@en ;
        <http://www.w3.org/2000/01/rdf-schema#range>
                <http://purl.org/dqm-vocabulary/v1/dqm#TestedClass> ;
        <http://www.w3.org/2000/01/rdf-schema#subPropertyOf>
                <http://purl.org/dqm-vocabulary/v1/dqm#dataElementRelationship> .

<http://purl.org/dqm-vocabulary/v1/dqm#equals>
        a       <http://www.w3.org/2002/07/owl#DatatypeProperty> , <http://www.w3.org/2002/07/owl#FunctionalProperty> ;
        <http://www.w3.org/2000/01/rdf-schema#comment>
                "Holds one or more consecutive characters that are supposed to be found in the same order in strings of another property."@en ;
        <http://www.w3.org/2000/01/rdf-schema#domain>
                [ a       <http://www.w3.org/2002/07/owl#Class> ;
                  <http://www.w3.org/2002/07/owl#unionOf>
                          ( <http://purl.org/dqm-vocabulary/v1/dqm#Condition> <http://purl.org/dqm-vocabulary/v1/dqm#FuncDepValueRule> )
                ] ;
        <http://www.w3.org/2000/01/rdf-schema#label>
                "Equals"@en ;
        <http://www.w3.org/2000/01/rdf-schema#range>
                <http://www.w3.org/2001/XMLSchema#string> ;
        <http://www.w3.org/2000/01/rdf-schema#subPropertyOf>
                <http://purl.org/dqm-vocabulary/v1/dqm#operatedValue> .

<http://purl.org/dqm-vocabulary/v1/dqm#ConditionalPropertyCompletenessRule>
        a       <http://www.w3.org/2002/07/owl#Class> ;
        <http://www.w3.org/2000/01/rdf-schema#comment>
                "Conditional property completeness rules specify that a tested property and/or its literal values must exist when the value of another property obtains a certain state. E.g. the property foo:state must exist and have a value when the property foo:country obtains the value \"USA\"."@en ;
        <http://www.w3.org/2000/01/rdf-schema#label>
                "Conditional Data Competeness Rule"@en ;
        <http://www.w3.org/2000/01/rdf-schema#subClassOf>
                <http://purl.org/dqm-vocabulary/v1/dqm#ConditionalRule> .

<http://purl.org/dqm-vocabulary/v1/dqm#FuncDepValueRule>
        a       <http://www.w3.org/2002/07/owl#Class> ;
        <http://www.w3.org/2000/01/rdf-schema#comment>
                "A functionally dependent value rule defines that the value of a tested property must have a certain value when the values of other properties obtain certain states (conditions). E.g. the property foo:inStock must have value \"true\" when the property foo:availableAmount is greater than zero."@en ;
        <http://www.w3.org/2000/01/rdf-schema#label>
                "Functionally Dependent Value Rule"@en ;
        <http://www.w3.org/2000/01/rdf-schema#subClassOf>
                <http://purl.org/dqm-vocabulary/v1/dqm#ConditionalRule> .

<http://purl.org/dqm-vocabulary/v1/dqm#testedProperty>
        a       <http://www.w3.org/2002/07/owl#ObjectProperty> ;
        <http://www.w3.org/2000/01/rdf-schema#comment>
                "The property with the values that shall be tested for data quality problems."@en ;
        <http://www.w3.org/2000/01/rdf-schema#label>
                "Tested Property"@en ;
        <http://www.w3.org/2000/01/rdf-schema#range>
                <http://purl.org/dqm-vocabulary/v1/dqm#TestedProperty> ;
        <http://www.w3.org/2000/01/rdf-schema#subPropertyOf>
                <http://purl.org/dqm-vocabulary/v1/dqm#dataElementRelationship> .

<http://purl.org/dqm-vocabulary/v1/dqm#PopulationCompleteness>
        a       <http://www.w3.org/2002/07/owl#Class> ;
        <http://www.w3.org/2000/01/rdf-schema#comment>
                "Population completeness is the degree to which all objects of a certain reference are represented in a specific class."@en ;
        <http://www.w3.org/2000/01/rdf-schema#label>
                "Population Completeness"@en ;
        <http://www.w3.org/2000/01/rdf-schema#subClassOf>
                <http://purl.org/dqm-vocabulary/v1/dqm#Completeness> .

<http://purl.org/dqm-vocabulary/v1/dqm#CustomRequirement>
        a       <http://www.w3.org/2002/07/owl#Class> ;
        <http://www.w3.org/2000/01/rdf-schema#comment>
                "A custom requirement is a data requirement that is expressed via a SPARQL query."@en ;
        <http://www.w3.org/2000/01/rdf-schema#label>
                "Custom Requirement"@en ;
        <http://www.w3.org/2000/01/rdf-schema#subClassOf>
                <http://purl.org/dqm-vocabulary/v1/dqm#DataRequirement> .

<http://purl.org/dqm-vocabulary/v1/dqm#timeOfIdentification>
        a       <http://www.w3.org/2002/07/owl#DatatypeProperty> ;
        <http://www.w3.org/2000/01/rdf-schema#comment>
                "The time of identification property specifies the date and time in which the data quality problem was detected"@en ;
        <http://www.w3.org/2000/01/rdf-schema#domain>
                <http://purl.org/dqm-vocabulary/v1/dqm#DataRequirementViolation> ;
        <http://www.w3.org/2000/01/rdf-schema#label>
                "Time Of Identification"@en ;
        <http://www.w3.org/2000/01/rdf-schema#range>
                <http://www.w3.org/2001/XMLSchema#dateTime> .

<http://purl.org/dqm-vocabulary/v1/dqm#OutdatedInstance>
        a       <http://www.w3.org/2002/07/owl#Class> ;
        <http://www.w3.org/2000/01/rdf-schema#comment>
                "An instance is outdated when it represents an outdated state of its corresponding real-world entity."@en ;
        <http://www.w3.org/2000/01/rdf-schema#label>
                "Outdated Instance"@en ;
        <http://www.w3.org/2000/01/rdf-schema#subClassOf>
                <http://purl.org/dqm-vocabulary/v1/dqm#DataRequirementViolation> .

<http://purl.org/dqm-vocabulary/v1/dqm#dataCleansingRuleRelationship>
        a       <http://www.w3.org/2002/07/owl#ObjectProperty> ;
        <http://www.w3.org/2000/01/rdf-schema#comment>
                "Data cleansing rule relationships are object properties of the data cleansing rules."@en ;
        <http://www.w3.org/2000/01/rdf-schema#label>
                "Data Cleansing Rule Relationship"@en .

<http://purl.org/dqm-vocabulary/v1/dqm#next>
        a       <http://www.w3.org/2002/07/owl#ObjectProperty> ;
        <http://www.w3.org/2000/01/rdf-schema#comment>
                "Links an instances to the next instance in an ordinal scale."@en ;
        <http://www.w3.org/2000/01/rdf-schema#domain>
                <http://purl.org/dqm-vocabulary/v1/dqm#ScaleValue> ;
        <http://www.w3.org/2000/01/rdf-schema#range>
                <http://purl.org/dqm-vocabulary/v1/dqm#ScaleValue> .

<http://purl.org/dqm-vocabulary/v1/dqm#Completeness>
        a       <http://www.w3.org/2002/07/owl#Class> ;
        <http://www.w3.org/2000/01/rdf-schema#comment>
                "Completeness is the extent to which data are of sufficient breadth, depth, and scope for the task at hand."@en ;
        <http://www.w3.org/2000/01/rdf-schema#label>
                "Completeness"@en ;
        <http://www.w3.org/2000/01/rdf-schema#subClassOf>
                <http://purl.org/dqm-vocabulary/v1/dqm#DataQualityScore> .

<http://purl.org/dqm-vocabulary/v1/dqm#LegalValueRule>
        a       <http://www.w3.org/2002/07/owl#Class> ;
        <http://www.w3.org/2000/01/rdf-schema#comment>
                "A legal value rule is a property requirement that specifies all values that a certain property is allowed to obtain. Legal value rules, therefore, refer to reference properties of classes that hold instances with all allowed values."@en ;
        <http://www.w3.org/2000/01/rdf-schema#label>
                "Legal Value Rule"@en ;
        <http://www.w3.org/2000/01/rdf-schema#subClassOf>
                <http://purl.org/dqm-vocabulary/v1/dqm#PropertyRequirement> .

<http://purl.org/dqm-vocabulary/v1/dqm#Timeliness>
        a       <http://www.w3.org/2002/07/owl#Class> ;
        <http://www.w3.org/2000/01/rdf-schema#comment>
                "Timeliness is the degree to which instances of a specific class (1) are updated within an expected time or (2) have not exceeded their expiration date."@en ;
        <http://www.w3.org/2000/01/rdf-schema#label>
                "Timeliness"@en ;
        <http://www.w3.org/2000/01/rdf-schema#subClassOf>
                <http://purl.org/dqm-vocabulary/v1/dqm#DataQualityScore> .

<http://purl.org/dc/elements/1.1/contributor>
        a       <http://www.w3.org/2002/07/owl#AnnotationProperty> .

<http://purl.org/dqm-vocabulary/v1/dqm#Accuracy>
        a       <http://www.w3.org/2002/07/owl#Class> ;
        <http://www.w3.org/2000/01/rdf-schema#comment>
                "Accuracy is the degree to which a data value represents the desired state regarding its syntax and semantics."@en ;
        <http://www.w3.org/2000/01/rdf-schema#label>
                "Accuracy"@en ;
        <http://www.w3.org/2000/01/rdf-schema#subClassOf>
                <http://purl.org/dqm-vocabulary/v1/dqm#DataQualityScore> .

<http://purl.org/dqm-vocabulary/v1/dqm#UpdateRule>
        a       <http://www.w3.org/2002/07/owl#Class> ;
        <http://www.w3.org/2000/01/rdf-schema#comment>
                "An update rule is an outdated instance rule that specifies the maximum duration tolerated without any updates. Update rules require timestamps about the last update of an instance."@en ;
        <http://www.w3.org/2000/01/rdf-schema#label>
                "Update Rule"@en ;
        <http://www.w3.org/2000/01/rdf-schema#subClassOf>
                <http://purl.org/dqm-vocabulary/v1/dqm#OutdatedInstanceRule> .

<http://purl.org/dqm-vocabulary/v1/dqm#valueMeaning>
        a       <http://www.w3.org/2002/07/owl#DatatypeProperty> ;
        <http://www.w3.org/2000/01/rdf-schema#comment>
                "Meaning of a value."@en ;
        <http://www.w3.org/2000/01/rdf-schema#domain>
                <http://purl.org/dqm-vocabulary/v1/dqm#ScaleValue> ;
        <http://www.w3.org/2000/01/rdf-schema#label>
                "Value Meaning"@en ;
        <http://www.w3.org/2000/01/rdf-schema#range>
                <http://www.w3.org/2001/XMLSchema#string> .

<http://purl.org/dqm-vocabulary/v1/dqm#plainScore>
        a       <http://www.w3.org/2002/07/owl#FunctionalProperty> , <http://www.w3.org/2002/07/owl#DatatypeProperty> ;
        <http://www.w3.org/2000/01/rdf-schema#comment>
                "The plain score represents a data quality dimension score that was assessed by using a certain formula that accounts for the violations of data quality rules related to the size of the relevant data set."@en ;
        <http://www.w3.org/2000/01/rdf-schema#domain>
                <http://purl.org/dqm-vocabulary/v1/dqm#DataQualityScore> ;
        <http://www.w3.org/2000/01/rdf-schema#label>
                "Plain Score"@en ;
        <http://www.w3.org/2000/01/rdf-schema#range>
                <http://www.w3.org/2000/01/rdf-schema#Literal> .

<http://purl.org/dc/elements/1.1/subject>
        a       <http://www.w3.org/2002/07/owl#AnnotationProperty> .

<http://purl.org/dqm-vocabulary/v1/dqm#cleansingProperty>
        a       <http://www.w3.org/2002/07/owl#DatatypeProperty> ;
        <http://www.w3.org/2000/01/rdf-schema#comment>
                "Cleansing properties are properties of data cleansing rules."@en ;
        <http://www.w3.org/2000/01/rdf-schema#label>
                "Cleansing Property"@en .

<http://purl.org/dqm-vocabulary/v1/dqm#operatedValue>
        a       <http://www.w3.org/2002/07/owl#DatatypeProperty> ;
        <http://www.w3.org/2000/01/rdf-schema#comment>
                "The operated value property is an abstract property for datatype properties that are used to express string filtering criteria."@en ;
        <http://www.w3.org/2000/01/rdf-schema#label>
                "Operated Value"@en .

<http://purl.org/dqm-vocabulary/v1/dqm#TestedProperty>
        a       <http://www.w3.org/2002/07/owl#Class> ;
        <http://www.w3.org/2000/01/rdf-schema#comment>
                "A tested property holds the values to be analyzed for data quality problems."@en ;
        <http://www.w3.org/2000/01/rdf-schema#label>
                "Tested Property"@en ;
        <http://www.w3.org/2000/01/rdf-schema#subClassOf>
                <http://purl.org/dqm-vocabulary/v1/dqm#DataElement> .

<http://purl.org/dqm-vocabulary/v1/dqm#PropertyCompletion>
        a       <http://www.w3.org/2002/07/owl#Class> ;
        <http://www.w3.org/2000/01/rdf-schema#comment>
                "A property completion rule specifies a property and value that shall be added to certain instances."@en ;
        <http://www.w3.org/2000/01/rdf-schema#label>
                "Property Completion Rule"@en ;
        <http://www.w3.org/2000/01/rdf-schema#subClassOf>
                <http://purl.org/dqm-vocabulary/v1/dqm#MultiPropertyCleansingRule> .

<http://purl.org/dqm-vocabulary/v1/dqm#TrustedClass>
        a       <http://www.w3.org/2002/07/owl#Class> ;
        <http://www.w3.org/2000/01/rdf-schema#comment>
                "Legal value rules and functional dependency reference rules require the specification of a trusted class as a reference that holds instances with legal values / legal value combinations."@en ;
        <http://www.w3.org/2000/01/rdf-schema#label>
                "Trusted Class"@en ;
        <http://www.w3.org/2000/01/rdf-schema#subClassOf>
                <http://purl.org/dqm-vocabulary/v1/dqm#DataElement> .

<http://purl.org/dqm-vocabulary/v1/dqm#Unit>
        a       <http://www.w3.org/2002/07/owl#Class> ;
        <http://www.w3.org/2000/01/rdf-schema#comment>
                "Class for units of numerical values that are used to express certain property states."@en ;
        <http://www.w3.org/2000/01/rdf-schema#label>
                "Unit"@en .
