<https://ns.eccenca.com/Eccenca> <http://www.w3.org/2004/02/skos/core#prefLabel> "eccenca GmbH"@de .
<https://ns.eccenca.com/CorporateMemory> <http://www.w3.org/2000/01/rdf-schema#comment> "For the first occurence of the name in a text, use the complete name eccenca Corporate Memory. In the following text, you can skip eccenca. Write the product name exactly in the spelling given in all texts and user interfaces." .
<https://ns.eccenca.com/CorporateMemorySync> <http://www.w3.org/2004/02/skos/core#altLabel> "eccenca Corporate Memory SYNC"@de .
<https://ns.eccenca.com/Mapping> <http://www.w3.org/2000/01/rdf-schema#label> "mapping" .
<https://ns.eccenca.com/Eccenca> <http://www.w3.org/2004/02/skos/core#altLabel> "eccenca"@en .
<https://ns.eccenca.com/BroxITSolutions> <http://www.w3.org/2004/02/skos/core#hiddenLabel> "Brox" .
<https://ns.eccenca.com/Eccenca> <http://www.w3.org/2000/01/rdf-schema#comment> "Write eccenca always in lowercase, also at the beginning of sentences, headings or titles." .
<https://ns.eccenca.com/DataPlatform> <http://www.w3.org/2004/02/skos/core#hiddenLabel> "Data Platform" .
<https://ns.eccenca.com/> <http://purl.org/dc/terms/creator> <https://ns.eccenca.com/aweilandt> .
<https://ns.eccenca.com/DataManager> <http://www.w3.org/2004/02/skos/core#definition> "Software to create and manage knowledge graphs."@en .
<https://ns.eccenca.com/CorporateMemory> <http://www.w3.org/2004/02/skos/core#altLabel> "eccenca Corporate Memory"@de .
<https://ns.eccenca.com/DataPlatform> <http://www.w3.org/1999/02/22-rdf-syntax-ns#type> <http://www.w3.org/2004/02/skos/core#Concept> .
<https://ns.eccenca.com/ProductName> <http://www.w3.org/2004/02/skos/core#definition> "Proper name of a product." .
<https://ns.eccenca.com/DataPlatform> <http://www.w3.org/2004/02/skos/core#hiddenLabel> "Backend" .
<https://ns.eccenca.com/HierarchicalMapping> <http://www.w3.org/2004/02/skos/core#definition> "Mapping with subordinate levels."@en .
<https://ns.eccenca.com/eccenca-GmbH> <http://www.w3.org/1999/02/22-rdf-syntax-ns#type> <http://xmlns.com/foaf/0.1/Organization> .
<https://ns.eccenca.com/mbruemmer> <http://www.w3.org/1999/02/22-rdf-syntax-ns#type> <http://xmlns.com/foaf/0.1/Person> .
<https://ns.eccenca.com/HierarchicalMapping> <http://www.w3.org/2004/02/skos/core#broader> <https://ns.eccenca.com/Mapping> .
<https://ns.eccenca.com/mbruemmer> <http://www.w3.org/1999/02/22-rdf-syntax-ns#type> <http://purl.org/dc/terms/Agent> .
<https://ns.eccenca.com/eccenca-GmbH> <http://www.w3.org/1999/02/22-rdf-syntax-ns#type> <http://purl.org/dc/terms/Agent> .
<https://ns.eccenca.com/Feature> <http://www.w3.org/2000/01/rdf-schema#label> "Feature" .
<https://ns.eccenca.com/ProductName> <http://www.w3.org/1999/02/22-rdf-syntax-ns#type> <http://www.w3.org/2004/02/skos/core#Concept> .
<https://ns.eccenca.com/Feature> <http://www.w3.org/2004/02/skos/core#inScheme> <https://ns.eccenca.com/EccencaCorporateTerminology> .
<https://ns.eccenca.com/Mapping> <http://www.w3.org/2004/02/skos/core#inScheme> <https://ns.eccenca.com/EccencaCorporateTerminology> .
<https://ns.eccenca.com/CorporateMemorySync> <http://www.w3.org/2000/01/rdf-schema#comment> "For the first occurence of the name in a text, use the complete name eccenca Corporate Memory SYNC. In the following text, you can skip eccenca. Write the product name exactly in the spelling given in all texts and user interfaces." .
<https://ns.eccenca.com/URIPattern> <http://www.w3.org/1999/02/22-rdf-syntax-ns#type> <http://www.w3.org/2004/02/skos/core#Concept> .
<https://ns.eccenca.com/DataManager> <http://www.w3.org/2004/02/skos/core#inScheme> <https://ns.eccenca.com/EccencaCorporateTerminology> .
<https://ns.eccenca.com/CorporateMemorySync> <http://www.w3.org/2004/02/skos/core#hiddenLabel> "CMEM-SYNC" .
<https://ns.eccenca.com/BroxITSolutions> <http://www.w3.org/2004/02/skos/core#altLabel> "brox"@de .
<https://ns.eccenca.com/BroxITSolutions> <http://www.w3.org/2004/02/skos/core#broader> <https://ns.eccenca.com/CompanyName> .
<https://ns.eccenca.com/> <http://www.w3.org/2000/01/rdf-schema#comment> "TODO describe"@en .
<https://ns.eccenca.com/> <http://rdfs.org/ns/void#entities> "23"^^<http://www.w3.org/2001/XMLSchema#integer> .
<https://ns.eccenca.com/Eccenca> <http://www.w3.org/1999/02/22-rdf-syntax-ns#type> <http://www.w3.org/2004/02/skos/core#Concept> .
<https://ns.eccenca.com/CompanyName> <http://www.w3.org/2004/02/skos/core#prefLabel> "company name"@en .
<https://ns.eccenca.com/HierarchicalMapping> <http://www.w3.org/2004/02/skos/core#prefLabel> "hierarchical mapping"@en .
<https://ns.eccenca.com/Mapping> <http://www.w3.org/2004/02/skos/core#prefLabel> "Mapping"@de .
<https://ns.eccenca.com/CorporateMemorySync> <http://www.w3.org/2004/02/skos/core#prefLabel> "Corporate Memory SYNC"@de .
<https://ns.eccenca.com/CorporateMemory> <http://www.w3.org/2004/02/skos/core#hiddenLabel> "eLDS" .
<https://ns.eccenca.com/ObjectMapping> <http://www.w3.org/2000/01/rdf-schema#label> "object mapping" .
<https://ns.eccenca.com/> <http://purl.org/dc/terms/issued> "2017-08-07"^^<http://www.w3.org/2001/XMLSchema#date> .
<https://ns.eccenca.com/Mapping> <http://www.w3.org/2004/02/skos/core#prefLabel> "mapping"@en .
<https://ns.eccenca.com/ObjectMapping> <http://www.w3.org/1999/02/22-rdf-syntax-ns#type> <http://www.w3.org/2004/02/skos/core#Concept> .
<https://ns.eccenca.com/CompanyName> <http://www.w3.org/1999/02/22-rdf-syntax-ns#type> <http://www.w3.org/2004/02/skos/core#Concept> .
<https://ns.eccenca.com/DataIntegration> <http://www.w3.org/2004/02/skos/core#inScheme> <https://ns.eccenca.com/EccencaCorporateTerminology> .
<https://ns.eccenca.com/DataIntegration> <http://www.w3.org/2004/02/skos/core#prefLabel> "DataIntegration"@en .
<https://ns.eccenca.com/rnavarropiris> <http://xmlns.com/foaf/0.1/name> "Rub√©n Navarro Piris" .
<https://ns.eccenca.com/Mapping> <http://www.w3.org/2004/02/skos/core#definition> "Set of transformations that assign data elements in a source dataset to data elements in a target dataset."@en .
<https://ns.eccenca.com/DataPlatform> <http://www.w3.org/2004/02/skos/core#prefLabel> "DataPlatform"@en .
<https://ns.eccenca.com/Eccenca> <http://www.w3.org/2004/02/skos/core#broader> <https://ns.eccenca.com/CompanyName> .
<https://ns.eccenca.com/BroxITSolutions> <http://www.w3.org/2000/01/rdf-schema#comment> "Write brox always in lowercase, also at the beginning of sentences, headings or titles. Use the term brox only after the correct name brox IT-Solutions has been mentioned once." .
<https://ns.eccenca.com/BroxITSolutions> <http://www.w3.org/1999/02/22-rdf-syntax-ns#type> <http://www.w3.org/2004/02/skos/core#Concept> .
<https://ns.eccenca.com/DataPlatform> <http://www.w3.org/2004/02/skos/core#altLabel> "eccenca DataPlatform"@en .
<https://ns.eccenca.com/Eccenca> <http://www.w3.org/2000/01/rdf-schema#label> "eccenca GmbH" .
<https://ns.eccenca.com/CorporateMemory> <http://www.w3.org/1999/02/22-rdf-syntax-ns#type> <http://www.w3.org/2004/02/skos/core#Concept> .
<https://ns.eccenca.com/CorporateMemorySync> <http://www.w3.org/2004/02/skos/core#broader> <https://ns.eccenca.com/ProductName> .
<https://ns.eccenca.com/HierarchicalMapping> <http://www.w3.org/1999/02/22-rdf-syntax-ns#type> <http://www.w3.org/2004/02/skos/core#Concept> .
<https://ns.eccenca.com/CorporateMemory> <http://www.w3.org/2004/02/skos/core#inScheme> <https://ns.eccenca.com/EccencaCorporateTerminology> .
<https://ns.eccenca.com/BroxITSolutions> <http://www.w3.org/2004/02/skos/core#inScheme> <https://ns.eccenca.com/EccencaCorporateTerminology> .
<https://ns.eccenca.com/DataManager> <http://www.w3.org/2004/02/skos/core#hiddenLabel> "Data Manager" .
<https://ns.eccenca.com/> <http://www.w3.org/2002/07/owl#versionInfo> "SNAPSHOT" .
<https://ns.eccenca.com/rpietzsch> <http://www.w3.org/1999/02/22-rdf-syntax-ns#type> <http://xmlns.com/foaf/0.1/Person> .
<https://ns.eccenca.com/rpietzsch> <http://www.w3.org/1999/02/22-rdf-syntax-ns#type> <http://purl.org/dc/terms/Agent> .
<https://ns.eccenca.com/DataIntegration> <http://www.w3.org/2000/01/rdf-schema#label> "DataIntegration" .
<https://ns.eccenca.com/ObjectMapping> <http://www.w3.org/2004/02/skos/core#inScheme> <https://ns.eccenca.com/EccencaCorporateTerminology> .
<https://ns.eccenca.com/CompanyName> <http://www.w3.org/2004/02/skos/core#inScheme> <https://ns.eccenca.com/EccencaCorporateTerminology> .
<https://ns.eccenca.com/DataIntegration> <http://www.w3.org/2004/02/skos/core#altLabel> "eccenca DataIntegration"@de .
<https://ns.eccenca.com/DataIntegration> <http://www.w3.org/1999/02/22-rdf-syntax-ns#type> <http://www.w3.org/2004/02/skos/core#Concept> .
<https://ns.eccenca.com/> <http://www.w3.org/2000/01/rdf-schema#isDefinedBy> <https://ns.eccenca.com/> .
<https://ns.eccenca.com/Eccenca> <http://www.w3.org/2004/02/skos/core#prefLabel> "eccenca GmbH"@en .
<https://ns.eccenca.com/ObjectMapping> <http://www.w3.org/2004/02/skos/core#prefLabel> "object mapping"@en .
<https://ns.eccenca.com/CorporateMemorySync> <http://www.w3.org/2004/02/skos/core#altLabel> "eccenca Corporate Memory SYNC"@en .
<https://ns.eccenca.com/Eccenca> <http://www.w3.org/2004/02/skos/core#altLabel> "eccenca"@de .
<https://ns.eccenca.com/CorporateMemory> <http://www.w3.org/2000/01/rdf-schema#label> "Corporate Memory" .
<https://ns.eccenca.com/CorporateMemory> <http://www.w3.org/2004/02/skos/core#historyNote> "eccenca Linked Data Suite (eLDS) is an obsolete name for eccenca Corporate Memory. Do not use it anymore. Do not use CMEM in external communication." .
<https://ns.eccenca.com/CorporateMemorySync> <http://www.w3.org/2004/02/skos/core#definition> "Product solution of eccenca for exchanging and sharing data among organizations. Composed of DataManager and DataPlatform."@en .
<https://ns.eccenca.com/ValuePath> <http://www.w3.org/2004/02/skos/core#definition> "Path expression - not unlike XPath or CSS selectors - that selects the value of the source dataset data element specified by that path."@en .
<https://ns.eccenca.com/Feature> <http://www.w3.org/1999/02/22-rdf-syntax-ns#type> <http://www.w3.org/2004/02/skos/core#Collection> .
<https://ns.eccenca.com/ValuePath> <http://www.w3.org/2004/02/skos/core#prefLabel> "value path"@en .
<https://ns.eccenca.com/CompanyName> <http://www.w3.org/2004/02/skos/core#prefLabel> "Firmenname"@de .
<https://ns.eccenca.com/URIPattern> <http://www.w3.org/2004/02/skos/core#prefLabel> "URI pattern"@en .
<https://ns.eccenca.com/Eccenca> <http://www.w3.org/2004/02/skos/core#inScheme> <https://ns.eccenca.com/EccencaCorporateTerminology> .
<https://ns.eccenca.com/CorporateMemory> <http://www.w3.org/2004/02/skos/core#prefLabel> "Corporate Memory"@de .
<https://ns.eccenca.com/ObjectMapping> <http://www.w3.org/2004/02/skos/core#broader> <https://ns.eccenca.com/Mapping> .
<https://ns.eccenca.com/URIPattern> <http://www.w3.org/2000/01/rdf-schema#label> "URI pattern" .
<https://ns.eccenca.com/ProductName> <http://www.w3.org/2004/02/skos/core#inScheme> <https://ns.eccenca.com/EccencaCorporateTerminology> .
<https://ns.eccenca.com/Mapping> <http://www.w3.org/1999/02/22-rdf-syntax-ns#type> <http://www.w3.org/2004/02/skos/core#Concept> .
<https://ns.eccenca.com/DataIntegration> <http://www.w3.org/2004/02/skos/core#hiddenLabel> "Link Discovery" .
<https://ns.eccenca.com/Eccenca> <http://www.w3.org/2004/02/skos/core#hiddenLabel> "Eccenca" .
<https://ns.eccenca.com/mbruemmer> <http://xmlns.com/foaf/0.1/name> "Martin Br√ºmmer" .
<https://ns.eccenca.com/URIPattern> <http://www.w3.org/2004/02/skos/core#inScheme> <https://ns.eccenca.com/EccencaCorporateTerminology> .
<https://ns.eccenca.com/DataManager> <http://www.w3.org/1999/02/22-rdf-syntax-ns#type> <http://www.w3.org/2004/02/skos/core#Concept> .
<https://ns.eccenca.com/ValueMapping> <http://www.w3.org/2000/01/rdf-schema#label> "value mapping" .
<https://ns.eccenca.com/rnavarropiris> <http://www.w3.org/1999/02/22-rdf-syntax-ns#type> <http://xmlns.com/foaf/0.1/Person> .
<https://ns.eccenca.com/> <http://rdfs.org/ns/void#vocabulary> <http://purl.org/vocab/vann/> .
<https://ns.eccenca.com/rnavarropiris> <http://www.w3.org/1999/02/22-rdf-syntax-ns#type> <http://purl.org/dc/terms/Agent> .
<https://ns.eccenca.com/BroxITSolutions> <http://www.w3.org/2004/02/skos/core#definition> "Company for IT consulting and information management with headquarter in Hanover, founded in 1998 and parent company of eccenca GmbH."@en .
<https://ns.eccenca.com/DataIntegration> <http://www.w3.org/2004/02/skos/core#definition> "Software to link, integrate, map and transform data as well as to manage KPI trees."@en .
<https://ns.eccenca.com/> <http://purl.org/dc/terms/publisher> <https://ns.eccenca.com/GmbH> .
<https://ns.eccenca.com/DataManager> <http://www.w3.org/2004/02/skos/core#altLabel> "eccenca DataManager"@de .
<https://ns.eccenca.com/stramp> <http://xmlns.com/foaf/0.1/name> "Sebastian Tramp" .
<https://ns.eccenca.com/DataPlatform> <http://www.w3.org/2004/02/skos/core#inScheme> <https://ns.eccenca.com/EccencaCorporateTerminology> .
<https://ns.eccenca.com/BroxITSolutions> <http://www.w3.org/2004/02/skos/core#altLabel> "brox IT-Solutions"@de .
<https://ns.eccenca.com/HierarchicalMapping> <http://www.w3.org/2000/01/rdf-schema#label> "hierarchical mapping" .
<https://ns.eccenca.com/rpietzsch> <http://xmlns.com/foaf/0.1/name> "Ren√© Pietzsch" .
<https://ns.eccenca.com/> <http://rdfs.org/ns/void#vocabulary> <http://purl.org/dc/terms/> .
<https://ns.eccenca.com/Mapping> <http://www.w3.org/2004/02/skos/core#narrower> <https://ns.eccenca.com/ObjectMapping> .
<https://ns.eccenca.com/ValueMapping> <http://www.w3.org/2004/02/skos/core#hiddenLabel> "direct mapping" .
<https://ns.eccenca.com/DataIntegration> <http://www.w3.org/2004/02/skos/core#hiddenLabel> "Data Integration" .
<https://ns.eccenca.com/stramp> <http://www.w3.org/1999/02/22-rdf-syntax-ns#type> <http://purl.org/dc/terms/Agent> .
<https://ns.eccenca.com/stramp> <http://www.w3.org/1999/02/22-rdf-syntax-ns#type> <http://xmlns.com/foaf/0.1/Person> .
<https://ns.eccenca.com/Eccenca> <http://www.w3.org/2004/02/skos/core#related> <https://ns.eccenca.com/BroxITSolutions> .
<https://ns.eccenca.com/ValuePath> <http://www.w3.org/2000/01/rdf-schema#label> "value path" .
<https://ns.eccenca.com/CorporateMemory> <http://www.w3.org/2004/02/skos/core#broader> <https://ns.eccenca.com/ProductName> .
<https://ns.eccenca.com/CorporateMemorySync> <http://www.w3.org/1999/02/22-rdf-syntax-ns#type> <http://www.w3.org/2004/02/skos/core#Concept> .
<https://ns.eccenca.com/CorporateMemory> <http://www.w3.org/2004/02/skos/core#prefLabel> "Corporate Memory"@en .
<https://ns.eccenca.com/BroxITSolutions> <http://www.w3.org/2004/02/skos/core#altLabel> "brox"@en .
<https://ns.eccenca.com/ValueMapping> <http://www.w3.org/1999/02/22-rdf-syntax-ns#type> <http://www.w3.org/2004/02/skos/core#Concept> .
<https://ns.eccenca.com/> <http://rdfs.org/ns/void#vocabulary> <http://xmlns.com/foaf/0.1/> .
<https://ns.eccenca.com/DataManager> <http://www.w3.org/2000/01/rdf-schema#label> "DataManager" .
<https://ns.eccenca.com/> <http://www.w3.org/1999/02/22-rdf-syntax-ns#type> <http://www.w3.org/2002/07/owl#Ontology> .
<https://ns.eccenca.com/> <http://purl.org/dc/terms/rights> "Copyright ¬© 2017 eccenca GmbH" .
<https://ns.eccenca.com/CorporateMemorySync> <http://www.w3.org/2004/02/skos/core#hiddenLabel> "CMEM SYNC" .
<https://ns.eccenca.com/CorporateMemory> <http://www.w3.org/2004/02/skos/core#hiddenLabel> "eccenca Linked Data Suite" .
<https://ns.eccenca.com/BroxITSolutions> <http://www.w3.org/2004/02/skos/core#prefLabel> "brox IT-Solutions GmbH"@de .
<https://ns.eccenca.com/Eccenca> <http://www.w3.org/2004/02/skos/core#definition> "Company for software development with headquarter in Leipzig, founded in 2013 as a subsidiary of brox IT-Solutions GmbH."@en .
<https://ns.eccenca.com/BroxITSolutions> <http://www.w3.org/2004/02/skos/core#altLabel> "brox IT-Solutions"@en .
<https://ns.eccenca.com/ValuePath> <http://www.w3.org/2004/02/skos/core#inScheme> <https://ns.eccenca.com/EccencaCorporateTerminology> .
<https://ns.eccenca.com/CorporateMemorySync> <http://www.w3.org/2000/01/rdf-schema#label> "Corporate Memory SYNC" .
<https://ns.eccenca.com/> <http://rdfs.org/ns/void#classes> "0"^^<http://www.w3.org/2001/XMLSchema#integer> .
<https://ns.eccenca.com/CorporateMemory> <http://www.w3.org/2004/02/skos/core#hiddenLabel> "CorporateMemory" .
<https://ns.eccenca.com/> <http://purl.org/dc/terms/modified> "2017-08-11"^^<http://www.w3.org/2001/XMLSchema#date> .
<https://ns.eccenca.com/URIPattern> <http://www.w3.org/2004/02/skos/core#definition> "Template that specifies how object URIs are created. It consists of static strings, usually defining URI scheme, authority and some paths, as well as references to source paths, which are replaced with source dataset data values during transformation."@en .
<https://ns.eccenca.com/DataPlatform> <http://www.w3.org/2004/02/skos/core#definition> "Software to provides storage abstraction and virtualization."@en .
<https://ns.eccenca.com/DataIntegration> <http://www.w3.org/2004/02/skos/core#hiddenLabel> "Data Integrator" .
<https://ns.eccenca.com/CorporateMemory> <http://www.w3.org/2004/02/skos/core#hiddenLabel> "CMEM" .
<https://ns.eccenca.com/DataPlatform> <http://www.w3.org/2004/02/skos/core#broader> <https://ns.eccenca.com/ProductName> .
<https://ns.eccenca.com/DataManager> <http://www.w3.org/2004/02/skos/core#prefLabel> "DataManager"@en .
<https://ns.eccenca.com/Feature> <http://www.w3.org/2004/02/skos/core#prefLabel> "Feature"@en .
<https://ns.eccenca.com/ValueMapping> <http://www.w3.org/2004/02/skos/core#definition> "Mapping that transforms a data element value, like a string, number or data, in a source dataset to a data element value in a target dataset. If the target dataset is an RDF graph, value mappings result in triples with literal objects and are thus suitable to map datatype properties."@en .
<https://ns.eccenca.com/DataPlatform> <http://www.w3.org/2000/01/rdf-schema#comment> "For the first occurence of the name in a text, use the complete name eccenca DataIntegration. In the following text, you can skip eccenca. Write the product name exactly in the spelling given in all texts and user interfaces." .
<https://ns.eccenca.com/DataManager> <http://www.w3.org/2004/02/skos/core#altLabel> "eccenca DataManager"@en .
<https://ns.eccenca.com/ProductName> <http://www.w3.org/2004/02/skos/core#prefLabel> "Produktname"@de .
<https://ns.eccenca.com/DataManager> <http://www.w3.org/2000/01/rdf-schema#comment> "For the first occurence of the name in a text, use the complete name eccenca DataManager. In the following text, you can skip eccenca. Write the product name exactly in the spelling given in all texts and user interfaces." .
<https://ns.eccenca.com/ValueMapping> <http://www.w3.org/2004/02/skos/core#broader> <https://ns.eccenca.com/Mapping> .
<https://ns.eccenca.com/DataIntegration> <http://www.w3.org/2004/02/skos/core#prefLabel> "DataIntegration"@de .
<https://ns.eccenca.com/> <http://rdfs.org/ns/void#properties> "0"^^<http://www.w3.org/2001/XMLSchema#integer> .
<https://ns.eccenca.com/ValueMapping> <http://www.w3.org/2004/02/skos/core#prefLabel> "value mapping"@en .
<https://ns.eccenca.com/DataManager> <http://www.w3.org/2004/02/skos/core#prefLabel> "DataManager"@de .
<https://ns.eccenca.com/BroxITSolutions> <http://www.w3.org/2004/02/skos/core#prefLabel> "brox IT-Solutions GmbH"@en .
<https://ns.eccenca.com/eccenca-GmbH> <http://xmlns.com/foaf/0.1/name> "eccenca GmbH" .
<https://ns.eccenca.com/Feature> <http://www.w3.org/2004/02/skos/core#member> <https://ns.eccenca.com/HierachicalMapping> .
<https://ns.eccenca.com/BroxITSolutions> <http://www.w3.org/2000/01/rdf-schema#label> "brox IT-Solutions GmbH" .
<https://ns.eccenca.com/EccencaCorporateTerminology> <http://purl.org/dc/terms/title> "eccenca Corporate Terminology" .
<https://ns.eccenca.com/DataPlatform> <http://www.w3.org/2004/02/skos/core#historyNote> "Backend is an obsolete name for DataPlatform. Do not use it anymore." .
<https://ns.eccenca.com/> <http://www.w3.org/2000/01/rdf-schema#label> "eccenca Corporate Terminology"@en .
<https://ns.eccenca.com/DataPlatform> <http://www.w3.org/2000/01/rdf-schema#label> "DataPlatform" .
<https://ns.eccenca.com/ValuePath> <http://www.w3.org/1999/02/22-rdf-syntax-ns#type> <http://www.w3.org/2004/02/skos/core#Concept> .
<https://ns.eccenca.com/> <http://purl.org/vocab/vann/preferredNamespaceUri> "https://ns.eccenca.com/" .
<https://ns.eccenca.com/CorporateMemory> <http://www.w3.org/2004/02/skos/core#altLabel> "eccenca Corporate Memory"@en .
<https://ns.eccenca.com/CorporateMemorySync> <http://www.w3.org/2004/02/skos/core#hiddenLabel> "Data Sharing" .
<https://ns.eccenca.com/ProductName> <http://www.w3.org/2000/01/rdf-schema#label> "Product name" .
<https://ns.eccenca.com/CorporateMemorySync> <http://www.w3.org/2004/02/skos/core#hiddenLabel> "CorporateMemory Sync" .
<https://ns.eccenca.com/CompanyName> <http://www.w3.org/2000/01/rdf-schema#label> "Company name" .
<https://ns.eccenca.com/DataManager> <http://www.w3.org/2004/02/skos/core#broader> <https://ns.eccenca.com/ProductName> .
<https://ns.eccenca.com/Mapping> <http://www.w3.org/2004/02/skos/core#hiddenLabel> "linking" .
<https://ns.eccenca.com/EccencaCorporateTerminology> <http://www.w3.org/2000/01/rdf-schema#label> "eccenca Corporate Terminology"@en .
<https://ns.eccenca.com/HierarchicalMapping> <http://www.w3.org/2004/02/skos/core#prefLabel> "hierarchisches Mapping"@de .
<https://ns.eccenca.com/DataPlatform> <http://www.w3.org/2004/02/skos/core#prefLabel> "DataPlatform"@de .
<https://ns.eccenca.com/> <http://purl.org/vocab/vann/preferredNamespacePrefix> "ecc" .
<https://ns.eccenca.com/> <http://rdfs.org/ns/void#triples> "180"^^<http://www.w3.org/2001/XMLSchema#integer> .
<https://ns.eccenca.com/ValueMapping> <http://www.w3.org/2004/02/skos/core#inScheme> <https://ns.eccenca.com/EccencaCorporateTerminology> .
<https://ns.eccenca.com/CorporateMemory> <http://www.w3.org/2004/02/skos/core#definition> "Product solution of eccenca for managing data landscapes including preparation, integration and browsing of data. Composed of DataManager, DataIntegration and DataPlatform with optional add-ons for Hadoop and/or HDFS."@en .
<https://ns.eccenca.com/DataPlatform> <http://www.w3.org/2004/02/skos/core#altLabel> "eccenca DataPlatform"@de .
<https://ns.eccenca.com/ProductName> <http://www.w3.org/2004/02/skos/core#prefLabel> "product name"@en .
<https://ns.eccenca.com/CompanyName> <http://www.w3.org/2004/02/skos/core#definition> "Proper name of a company." .
<https://ns.eccenca.com/BroxITSolutions> <http://www.w3.org/2004/02/skos/core#related> <https://ns.eccenca.com/Eccenca> .
<https://ns.eccenca.com/ObjectMapping> <http://www.w3.org/2004/02/skos/core#definition> "Mapping that transforms a data element in a source dataset to a data element in a target dataset. If the target dataset is an RDF graph, object mappings result in triples with resource objects and are thus suitable to map object properties. Object mappings create a new subordinate level in the (hierarchical) mapping view of Corporate Memory."@en .
<https://ns.eccenca.com/EccencaCorporateTerminology> <http://www.w3.org/1999/02/22-rdf-syntax-ns#type> <http://www.w3.org/2004/02/skos/core#ConceptScheme> .
<https://ns.eccenca.com/DataIntegration> <http://www.w3.org/2004/02/skos/core#broader> <https://ns.eccenca.com/ProductName> .
<https://ns.eccenca.com/DataIntegration> <http://www.w3.org/2004/02/skos/core#altLabel> "eccenca DataIntegration"@en .
<https://ns.eccenca.com/CorporateMemorySync> <http://www.w3.org/2004/02/skos/core#inScheme> <https://ns.eccenca.com/EccencaCorporateTerminology> .
<https://ns.eccenca.com/CorporateMemorySync> <http://www.w3.org/2004/02/skos/core#prefLabel> "Corporate Memory SYNC"@en .
<https://ns.eccenca.com/Mapping> <http://www.w3.org/2004/02/skos/core#narrower> <https://ns.eccenca.com/ValueMapping> .
<https://ns.eccenca.com/DataIntegration> <http://www.w3.org/2000/01/rdf-schema#comment> "For the first occurence of the name in a text, use the complete name eccenca DataIntegration. In the following text, you can skip eccenca. Write the product name exactly in the spelling given in all texts and user interfaces." .
