<https://ns.eccenca.com/Eccenca>
        a       <http://www.w3.org/2004/02/skos/core#Concept> ;
        <http://www.w3.org/2000/01/rdf-schema#comment>
                "Write eccenca always in lowercase, also at the beginning of sentences, headings or titles." ;
        <http://www.w3.org/2000/01/rdf-schema#label>
                "eccenca GmbH" ;
        <http://www.w3.org/2004/02/skos/core#altLabel>
                "eccenca"@en , "eccenca"@de ;
        <http://www.w3.org/2004/02/skos/core#broader>
                <https://ns.eccenca.com/CompanyName> ;
        <http://www.w3.org/2004/02/skos/core#definition>
                "Company for software development with headquarter in Leipzig, founded in 2013 as a subsidiary of brox IT-Solutions GmbH."@en ;
        <http://www.w3.org/2004/02/skos/core#hiddenLabel>
                "Eccenca" ;
        <http://www.w3.org/2004/02/skos/core#inScheme>
                <https://ns.eccenca.com/EccencaCorporateTerminology> ;
        <http://www.w3.org/2004/02/skos/core#prefLabel>
                "eccenca GmbH"@de , "eccenca GmbH"@en ;
        <http://www.w3.org/2004/02/skos/core#related>
                <https://ns.eccenca.com/BroxITSolutions> .

<https://ns.eccenca.com/CorporateMemory>
        a       <http://www.w3.org/2004/02/skos/core#Concept> ;
        <http://www.w3.org/2000/01/rdf-schema#comment>
                "For the first occurence of the name in a text, use the complete name eccenca Corporate Memory. In the following text, you can skip eccenca. Write the product name exactly in the spelling given in all texts and user interfaces." ;
        <http://www.w3.org/2000/01/rdf-schema#label>
                "Corporate Memory" ;
        <http://www.w3.org/2004/02/skos/core#altLabel>
                "eccenca Corporate Memory"@de , "eccenca Corporate Memory"@en ;
        <http://www.w3.org/2004/02/skos/core#broader>
                <https://ns.eccenca.com/ProductName> ;
        <http://www.w3.org/2004/02/skos/core#definition>
                "Product solution of eccenca for managing data landscapes including preparation, integration and browsing of data. Composed of DataManager, DataIntegration and DataPlatform with optional add-ons for Hadoop and/or HDFS."@en ;
        <http://www.w3.org/2004/02/skos/core#hiddenLabel>
                "eLDS" , "eccenca Linked Data Suite" , "CorporateMemory" , "CMEM" ;
        <http://www.w3.org/2004/02/skos/core#historyNote>
                "eccenca Linked Data Suite (eLDS) is an obsolete name for eccenca Corporate Memory. Do not use it anymore. Do not use CMEM in external communication." ;
        <http://www.w3.org/2004/02/skos/core#inScheme>
                <https://ns.eccenca.com/EccencaCorporateTerminology> ;
        <http://www.w3.org/2004/02/skos/core#prefLabel>
                "Corporate Memory"@de , "Corporate Memory"@en .

<https://ns.eccenca.com/CorporateMemorySync>
        a       <http://www.w3.org/2004/02/skos/core#Concept> ;
        <http://www.w3.org/2000/01/rdf-schema#comment>
                "For the first occurence of the name in a text, use the complete name eccenca Corporate Memory SYNC. In the following text, you can skip eccenca. Write the product name exactly in the spelling given in all texts and user interfaces." ;
        <http://www.w3.org/2000/01/rdf-schema#label>
                "Corporate Memory SYNC" ;
        <http://www.w3.org/2004/02/skos/core#altLabel>
                "eccenca Corporate Memory SYNC"@de , "eccenca Corporate Memory SYNC"@en ;
        <http://www.w3.org/2004/02/skos/core#broader>
                <https://ns.eccenca.com/ProductName> ;
        <http://www.w3.org/2004/02/skos/core#definition>
                "Product solution of eccenca for exchanging and sharing data among organizations. Composed of DataManager and DataPlatform."@en ;
        <http://www.w3.org/2004/02/skos/core#hiddenLabel>
                "CMEM-SYNC" , "CMEM SYNC" , "Data Sharing" , "CorporateMemory Sync" ;
        <http://www.w3.org/2004/02/skos/core#inScheme>
                <https://ns.eccenca.com/EccencaCorporateTerminology> ;
        <http://www.w3.org/2004/02/skos/core#prefLabel>
                "Corporate Memory SYNC"@de , "Corporate Memory SYNC"@en .

<https://ns.eccenca.com/Mapping>
        a       <http://www.w3.org/2004/02/skos/core#Concept> ;
        <http://www.w3.org/2000/01/rdf-schema#label>
                "mapping" ;
        <http://www.w3.org/2004/02/skos/core#definition>
                "Set of transformations that assign data elements in a source dataset to data elements in a target dataset."@en ;
        <http://www.w3.org/2004/02/skos/core#hiddenLabel>
                "linking" ;
        <http://www.w3.org/2004/02/skos/core#inScheme>
                <https://ns.eccenca.com/EccencaCorporateTerminology> ;
        <http://www.w3.org/2004/02/skos/core#narrower>
                <https://ns.eccenca.com/ObjectMapping> , <https://ns.eccenca.com/ValueMapping> ;
        <http://www.w3.org/2004/02/skos/core#prefLabel>
                "Mapping"@de , "mapping"@en .

<https://ns.eccenca.com/BroxITSolutions>
        a       <http://www.w3.org/2004/02/skos/core#Concept> ;
        <http://www.w3.org/2000/01/rdf-schema#comment>
                "Write brox always in lowercase, also at the beginning of sentences, headings or titles. Use the term brox only after the correct name brox IT-Solutions has been mentioned once." ;
        <http://www.w3.org/2000/01/rdf-schema#label>
                "brox IT-Solutions GmbH" ;
        <http://www.w3.org/2004/02/skos/core#altLabel>
                "brox"@de , "brox IT-Solutions"@de , "brox"@en , "brox IT-Solutions"@en ;
        <http://www.w3.org/2004/02/skos/core#broader>
                <https://ns.eccenca.com/CompanyName> ;
        <http://www.w3.org/2004/02/skos/core#definition>
                "Company for IT consulting and information management with headquarter in Hanover, founded in 1998 and parent company of eccenca GmbH."@en ;
        <http://www.w3.org/2004/02/skos/core#hiddenLabel>
                "Brox" ;
        <http://www.w3.org/2004/02/skos/core#inScheme>
                <https://ns.eccenca.com/EccencaCorporateTerminology> ;
        <http://www.w3.org/2004/02/skos/core#prefLabel>
                "brox IT-Solutions GmbH"@de , "brox IT-Solutions GmbH"@en ;
        <http://www.w3.org/2004/02/skos/core#related>
                <https://ns.eccenca.com/Eccenca> .

<https://ns.eccenca.com/DataPlatform>
        a       <http://www.w3.org/2004/02/skos/core#Concept> ;
        <http://www.w3.org/2000/01/rdf-schema#comment>
                "For the first occurence of the name in a text, use the complete name eccenca DataIntegration. In the following text, you can skip eccenca. Write the product name exactly in the spelling given in all texts and user interfaces." ;
        <http://www.w3.org/2000/01/rdf-schema#label>
                "DataPlatform" ;
        <http://www.w3.org/2004/02/skos/core#altLabel>
                "eccenca DataPlatform"@en , "eccenca DataPlatform"@de ;
        <http://www.w3.org/2004/02/skos/core#broader>
                <https://ns.eccenca.com/ProductName> ;
        <http://www.w3.org/2004/02/skos/core#definition>
                "Software to provides storage abstraction and virtualization."@en ;
        <http://www.w3.org/2004/02/skos/core#hiddenLabel>
                "Data Platform" , "Backend" ;
        <http://www.w3.org/2004/02/skos/core#historyNote>
                "Backend is an obsolete name for DataPlatform. Do not use it anymore." ;
        <http://www.w3.org/2004/02/skos/core#inScheme>
                <https://ns.eccenca.com/EccencaCorporateTerminology> ;
        <http://www.w3.org/2004/02/skos/core#prefLabel>
                "DataPlatform"@en , "DataPlatform"@de .

<https://ns.eccenca.com/>
        a       <http://www.w3.org/2002/07/owl#Ontology> ;
        <http://www.w3.org/2000/01/rdf-schema#comment>
                "TODO describe"@en ;
        <http://www.w3.org/2000/01/rdf-schema#isDefinedBy>
                <https://ns.eccenca.com/> ;
        <http://www.w3.org/2000/01/rdf-schema#label>
                "eccenca Corporate Terminology"@en ;
        <http://purl.org/dc/terms/creator>
                <https://ns.eccenca.com/aweilandt> ;
        <http://purl.org/dc/terms/issued>
                "2017-08-07"^^<http://www.w3.org/2001/XMLSchema#date> ;
        <http://purl.org/dc/terms/modified>
                "2017-08-11"^^<http://www.w3.org/2001/XMLSchema#date> ;
        <http://purl.org/dc/terms/publisher>
                <https://ns.eccenca.com/GmbH> ;
        <http://purl.org/dc/terms/rights>
                "Copyright © 2017 eccenca GmbH" ;
        <http://purl.org/vocab/vann/preferredNamespacePrefix>
                "ecc" ;
        <http://purl.org/vocab/vann/preferredNamespaceUri>
                "https://ns.eccenca.com/" ;
        <http://rdfs.org/ns/void#classes>
                0 ;
        <http://rdfs.org/ns/void#entities>
                23 ;
        <http://rdfs.org/ns/void#properties>
                0 ;
        <http://rdfs.org/ns/void#triples>
                180 ;
        <http://rdfs.org/ns/void#vocabulary>
                <http://purl.org/vocab/vann/> , <http://purl.org/dc/terms/> , <http://xmlns.com/foaf/0.1/> ;
        <http://www.w3.org/2002/07/owl#versionInfo>
                "SNAPSHOT" .

<https://ns.eccenca.com/DataManager>
        a       <http://www.w3.org/2004/02/skos/core#Concept> ;
        <http://www.w3.org/2000/01/rdf-schema#comment>
                "For the first occurence of the name in a text, use the complete name eccenca DataManager. In the following text, you can skip eccenca. Write the product name exactly in the spelling given in all texts and user interfaces." ;
        <http://www.w3.org/2000/01/rdf-schema#label>
                "DataManager" ;
        <http://www.w3.org/2004/02/skos/core#altLabel>
                "eccenca DataManager"@de , "eccenca DataManager"@en ;
        <http://www.w3.org/2004/02/skos/core#broader>
                <https://ns.eccenca.com/ProductName> ;
        <http://www.w3.org/2004/02/skos/core#definition>
                "Software to create and manage knowledge graphs."@en ;
        <http://www.w3.org/2004/02/skos/core#hiddenLabel>
                "Data Manager" ;
        <http://www.w3.org/2004/02/skos/core#inScheme>
                <https://ns.eccenca.com/EccencaCorporateTerminology> ;
        <http://www.w3.org/2004/02/skos/core#prefLabel>
                "DataManager"@en , "DataManager"@de .

<https://ns.eccenca.com/ProductName>
        a       <http://www.w3.org/2004/02/skos/core#Concept> ;
        <http://www.w3.org/2000/01/rdf-schema#label>
                "Product name" ;
        <http://www.w3.org/2004/02/skos/core#definition>
                "Proper name of a product." ;
        <http://www.w3.org/2004/02/skos/core#inScheme>
                <https://ns.eccenca.com/EccencaCorporateTerminology> ;
        <http://www.w3.org/2004/02/skos/core#prefLabel>
                "Produktname"@de , "product name"@en .

<https://ns.eccenca.com/HierarchicalMapping>
        a       <http://www.w3.org/2004/02/skos/core#Concept> ;
        <http://www.w3.org/2000/01/rdf-schema#label>
                "hierarchical mapping" ;
        <http://www.w3.org/2004/02/skos/core#broader>
                <https://ns.eccenca.com/Mapping> ;
        <http://www.w3.org/2004/02/skos/core#definition>
                "Mapping with subordinate levels."@en ;
        <http://www.w3.org/2004/02/skos/core#prefLabel>
                "hierarchical mapping"@en , "hierarchisches Mapping"@de .

<https://ns.eccenca.com/eccenca-GmbH>
        a       <http://xmlns.com/foaf/0.1/Organization> , <http://purl.org/dc/terms/Agent> ;
        <http://xmlns.com/foaf/0.1/name>
                "eccenca GmbH" .

<https://ns.eccenca.com/mbruemmer>
        a       <http://xmlns.com/foaf/0.1/Person> , <http://purl.org/dc/terms/Agent> ;
        <http://xmlns.com/foaf/0.1/name>
                "Martin Brümmer" .

<https://ns.eccenca.com/Feature>
        a       <http://www.w3.org/2004/02/skos/core#Collection> ;
        <http://www.w3.org/2000/01/rdf-schema#label>
                "Feature" ;
        <http://www.w3.org/2004/02/skos/core#inScheme>
                <https://ns.eccenca.com/EccencaCorporateTerminology> ;
        <http://www.w3.org/2004/02/skos/core#member>
                <https://ns.eccenca.com/HierachicalMapping> ;
        <http://www.w3.org/2004/02/skos/core#prefLabel>
                "Feature"@en .

<https://ns.eccenca.com/URIPattern>
        a       <http://www.w3.org/2004/02/skos/core#Concept> ;
        <http://www.w3.org/2000/01/rdf-schema#label>
                "URI pattern" ;
        <http://www.w3.org/2004/02/skos/core#definition>
                "Template that specifies how object URIs are created. It consists of static strings, usually defining URI scheme, authority and some paths, as well as references to source paths, which are replaced with source dataset data values during transformation."@en ;
        <http://www.w3.org/2004/02/skos/core#inScheme>
                <https://ns.eccenca.com/EccencaCorporateTerminology> ;
        <http://www.w3.org/2004/02/skos/core#prefLabel>
                "URI pattern"@en .

<https://ns.eccenca.com/CompanyName>
        a       <http://www.w3.org/2004/02/skos/core#Concept> ;
        <http://www.w3.org/2000/01/rdf-schema#label>
                "Company name" ;
        <http://www.w3.org/2004/02/skos/core#definition>
                "Proper name of a company." ;
        <http://www.w3.org/2004/02/skos/core#inScheme>
                <https://ns.eccenca.com/EccencaCorporateTerminology> ;
        <http://www.w3.org/2004/02/skos/core#prefLabel>
                "company name"@en , "Firmenname"@de .

<https://ns.eccenca.com/ObjectMapping>
        a       <http://www.w3.org/2004/02/skos/core#Concept> ;
        <http://www.w3.org/2000/01/rdf-schema#label>
                "object mapping" ;
        <http://www.w3.org/2004/02/skos/core#broader>
                <https://ns.eccenca.com/Mapping> ;
        <http://www.w3.org/2004/02/skos/core#definition>
                "Mapping that transforms a data element in a source dataset to a data element in a target dataset. If the target dataset is an RDF graph, object mappings result in triples with resource objects and are thus suitable to map object properties. Object mappings create a new subordinate level in the (hierarchical) mapping view of Corporate Memory."@en ;
        <http://www.w3.org/2004/02/skos/core#inScheme>
                <https://ns.eccenca.com/EccencaCorporateTerminology> ;
        <http://www.w3.org/2004/02/skos/core#prefLabel>
                "object mapping"@en .

<https://ns.eccenca.com/DataIntegration>
        a       <http://www.w3.org/2004/02/skos/core#Concept> ;
        <http://www.w3.org/2000/01/rdf-schema#comment>
                "For the first occurence of the name in a text, use the complete name eccenca DataIntegration. In the following text, you can skip eccenca. Write the product name exactly in the spelling given in all texts and user interfaces." ;
        <http://www.w3.org/2000/01/rdf-schema#label>
                "DataIntegration" ;
        <http://www.w3.org/2004/02/skos/core#altLabel>
                "eccenca DataIntegration"@de , "eccenca DataIntegration"@en ;
        <http://www.w3.org/2004/02/skos/core#broader>
                <https://ns.eccenca.com/ProductName> ;
        <http://www.w3.org/2004/02/skos/core#definition>
                "Software to link, integrate, map and transform data as well as to manage KPI trees."@en ;
        <http://www.w3.org/2004/02/skos/core#hiddenLabel>
                "Link Discovery" , "Data Integration" , "Data Integrator" ;
        <http://www.w3.org/2004/02/skos/core#inScheme>
                <https://ns.eccenca.com/EccencaCorporateTerminology> ;
        <http://www.w3.org/2004/02/skos/core#prefLabel>
                "DataIntegration"@en , "DataIntegration"@de .

<https://ns.eccenca.com/rnavarropiris>
        a       <http://xmlns.com/foaf/0.1/Person> , <http://purl.org/dc/terms/Agent> ;
        <http://xmlns.com/foaf/0.1/name>
                "Rubén Navarro Piris" .

<https://ns.eccenca.com/rpietzsch>
        a       <http://xmlns.com/foaf/0.1/Person> , <http://purl.org/dc/terms/Agent> ;
        <http://xmlns.com/foaf/0.1/name>
                "René Pietzsch" .

<https://ns.eccenca.com/ValuePath>
        a       <http://www.w3.org/2004/02/skos/core#Concept> ;
        <http://www.w3.org/2000/01/rdf-schema#label>
                "value path" ;
        <http://www.w3.org/2004/02/skos/core#definition>
                "Path expression - not unlike XPath or CSS selectors - that selects the value of the source dataset data element specified by that path."@en ;
        <http://www.w3.org/2004/02/skos/core#inScheme>
                <https://ns.eccenca.com/EccencaCorporateTerminology> ;
        <http://www.w3.org/2004/02/skos/core#prefLabel>
                "value path"@en .

<https://ns.eccenca.com/ValueMapping>
        a       <http://www.w3.org/2004/02/skos/core#Concept> ;
        <http://www.w3.org/2000/01/rdf-schema#label>
                "value mapping" ;
        <http://www.w3.org/2004/02/skos/core#broader>
                <https://ns.eccenca.com/Mapping> ;
        <http://www.w3.org/2004/02/skos/core#definition>
                "Mapping that transforms a data element value, like a string, number or data, in a source dataset to a data element value in a target dataset. If the target dataset is an RDF graph, value mappings result in triples with literal objects and are thus suitable to map datatype properties."@en ;
        <http://www.w3.org/2004/02/skos/core#hiddenLabel>
                "direct mapping" ;
        <http://www.w3.org/2004/02/skos/core#inScheme>
                <https://ns.eccenca.com/EccencaCorporateTerminology> ;
        <http://www.w3.org/2004/02/skos/core#prefLabel>
                "value mapping"@en .

<https://ns.eccenca.com/stramp>
        a       <http://purl.org/dc/terms/Agent> , <http://xmlns.com/foaf/0.1/Person> ;
        <http://xmlns.com/foaf/0.1/name>
                "Sebastian Tramp" .

<https://ns.eccenca.com/EccencaCorporateTerminology>
        a       <http://www.w3.org/2004/02/skos/core#ConceptScheme> ;
        <http://www.w3.org/2000/01/rdf-schema#label>
                "eccenca Corporate Terminology"@en ;
        <http://purl.org/dc/terms/title>
                "eccenca Corporate Terminology" .
