<http://purl.org/cerif/frapo/hasIPROwner>
        a       <http://www.w3.org/2002/07/owl#ObjectProperty> ;
        <http://www.w3.org/2000/01/rdf-schema#comment>
                "An object property linking an entity such as a project, an endeavour or an output to an agent who owns the IPR arising from or related to that entity."@en ;
        <http://www.w3.org/2000/01/rdf-schema#label>
                "has IPR owner"@en ;
        <http://www.w3.org/2000/01/rdf-schema#range>
                <http://xmlns.com/foaf/0.1/Agent> ;
        <http://www.w3.org/2000/01/rdf-schema#subPropertyOf>
                <http://purl.org/cerif/frapo/isOwnedBy> ;
        <http://www.w3.org/2002/07/owl#inverseOf>
                <http://purl.org/cerif/frapo/ownsIRPOf> .

<http://purl.org/cerif/frapo/manufactures>
        a       <http://www.w3.org/2002/07/owl#ObjectProperty> ;
        <http://www.w3.org/2000/01/rdf-schema#comment>
                "An object property relating a manufacturer to a manufactured entity."@en ;
        <http://www.w3.org/2000/01/rdf-schema#domain>
                <http://purl.org/cerif/frapo/Manufacturer> ;
        <http://www.w3.org/2000/01/rdf-schema#label>
                "manufactures"@en .

<http://purl.org/cerif/frapo/Endeavour>
        a       <http://www.w3.org/2002/07/owl#Class> ;
        <http://www.w3.org/2000/01/rdf-schema#comment>
                "In FRAPO, an endeavour is an activity such as a research investigation that is enabled by a project.  An endeavour relate to the academic and practical aspects of undertaking that endeavour - thus for a research investigation the research itself, including the hypotheses being investigated, the experiments being undertaken, the data being gathered and analysed, the interpretations being drawn from the data, and the results obtained.  In contrast, the project relates to the administrative aspects of undertaking an endeavour, including the funding obtained, the people employed, and the management of the project in terms of deadlines and deliverables."@en ;
        <http://www.w3.org/2000/01/rdf-schema#label>
                "endeavour"@en ;
        <http://www.w3.org/2000/01/rdf-schema#subClassOf>
                <http://www.w3.org/2002/07/owl#Thing> .

<http://purl.org/cerif/frapo/hasAccountNumber>
        a       <http://www.w3.org/2002/07/owl#DatatypeProperty> ;
        <http://www.w3.org/2000/01/rdf-schema#comment>
                "A data property linking a financial account to an identifying number for that account."@en ;
        <http://www.w3.org/2000/01/rdf-schema#domain>
                <http://purl.org/cerif/frapo/Account> ;
        <http://www.w3.org/2000/01/rdf-schema#label>
                "has account number"@en ;
        <http://www.w3.org/2000/01/rdf-schema#subPropertyOf>
                <http://purl.org/dc/terms/identifier> .

<http://purl.org/cerif/frapo/Repository>
        a       <http://www.w3.org/2002/07/owl#Class> ;
        <http://www.w3.org/2000/01/rdf-schema#comment>
                "A facility in which entities can be deposited for long-term preservation."@en ;
        <http://www.w3.org/2000/01/rdf-schema#label>
                "repository"@en ;
        <http://www.w3.org/2000/01/rdf-schema#subClassOf>
                <http://purl.org/cerif/frapo/Facility> ;
        <http://purl.org/dc/elements/1.1/description>
                "May also be described as an archive, or as a database."@en .

<http://purl.org/cerif/frapo/owns>
        a       <http://www.w3.org/2002/07/owl#ObjectProperty> ;
        <http://www.w3.org/2000/01/rdf-schema#comment>
                "An object property linking an agent to an entity owned by that agent."@en ;
        <http://www.w3.org/2000/01/rdf-schema#domain>
                <http://xmlns.com/foaf/0.1/Agent> ;
        <http://www.w3.org/2000/01/rdf-schema#label>
                "owns"@en .

<http://purl.org/cerif/frapo/estates-costs>
        a       <http://purl.org/cerif/frapo/BudgetCategory> , <http://www.w3.org/2002/07/owl#NamedIndividual> ;
        <http://www.w3.org/2000/01/rdf-schema#comment>
                "A budget category to cover the 'overhead' costs of maintaining the premises in which work is undertaken."@en ;
        <http://www.w3.org/2000/01/rdf-schema#label>
                "estates costs"@en .

<http://purl.org/cerif/frapo/FinancialControlSystem>
        a       <http://www.w3.org/2002/07/owl#Class> ;
        <http://www.w3.org/2000/01/rdf-schema#comment>
                "A software system controlling the financial activities of an organization, for example determining full economic cost budgets for grant applications, and managing the funding of funded projects."@en ;
        <http://www.w3.org/2000/01/rdf-schema#label>
                "financial control system"@en ;
        <http://www.w3.org/2000/01/rdf-schema#subClassOf>
                <http://purl.org/cerif/frapo/ComputationalService> .

<http://purl.org/cerif/frapo/Legacy>
        a       <http://www.w3.org/2002/07/owl#Class> ;
        <http://www.w3.org/2000/01/rdf-schema#comment>
                "A gift of money or property specified in the will of a person, that is made after that person's death."@en ;
        <http://www.w3.org/2000/01/rdf-schema#label>
                "legacy"@en ;
        <http://www.w3.org/2000/01/rdf-schema#subClassOf>
                <http://purl.org/cerif/frapo/Gift> .

<http://purl.org/cerif/frapo/hasDeliverable>
        a       <http://www.w3.org/2002/07/owl#DatatypeProperty> ;
        <http://www.w3.org/2000/01/rdf-schema#comment>
                "A data property that permits one to define a deliverable of a project."@en ;
        <http://www.w3.org/2000/01/rdf-schema#label>
                "has deliverable"@en .

<http://purl.org/cerif/frapo/isManufacturedBy>
        a       <http://www.w3.org/2002/07/owl#ObjectProperty> ;
        <http://www.w3.org/2000/01/rdf-schema#comment>
                "An object property relating a manufactured entity to its manufacturer."@en ;
        <http://www.w3.org/2000/01/rdf-schema#label>
                "is manufactured by"@en ;
        <http://www.w3.org/2000/01/rdf-schema#range>
                <http://purl.org/cerif/frapo/Manufacturer> ;
        <http://www.w3.org/2002/07/owl#inverseOf>
                <http://purl.org/cerif/frapo/manufactures> .

<http://purl.org/cerif/frapo/Service>
        a       <http://www.w3.org/2002/07/owl#Class> ;
        <http://www.w3.org/2000/01/rdf-schema#comment>
                "A service of help to others, often requiring funding, employees, equipment and/or facilities for its provision, for example a library service, a transportation service, a DNA sequencing service."@en ;
        <http://www.w3.org/2000/01/rdf-schema#label>
                "service"@en ;
        <http://www.w3.org/2000/01/rdf-schema#subClassOf>
                <http://purl.org/cerif/frapo/InfrastructureEntity> .

<http://purl.org/cerif/frapo/hasProjectIdentifier>
        a       <http://www.w3.org/2002/07/owl#AnnotationProperty> , <http://www.w3.org/2002/07/owl#DatatypeProperty> ;
        <http://www.w3.org/2000/01/rdf-schema#comment>
                "A data property linking a project to an identifier for that project."@en ;
        <http://www.w3.org/2000/01/rdf-schema#domain>
                <http://xmlns.com/foaf/0.1/Project> ;
        <http://www.w3.org/2000/01/rdf-schema#label>
                "has project identifier"@en ;
        <http://www.w3.org/2000/01/rdf-schema#subPropertyOf>
                <http://purl.org/dc/terms/identifier> .

<http://purl.org/cerif/frapo/Division>
        a       <http://www.w3.org/2002/07/owl#Class> ;
        <http://www.w3.org/2000/01/rdf-schema#comment>
                "A grouping of similar departments within a larger organization.  In the university context, also known as a school or a faculty, for example the Humanities Division, the Mathematics Faculty, or the School of Medicine."@en ;
        <http://www.w3.org/2000/01/rdf-schema#label>
                "division"@en ;
        <http://www.w3.org/2000/01/rdf-schema#subClassOf>
                <http://xmlns.com/foaf/0.1/Organization> .

<http://purl.org/cerif/frapo/hasAgentInformation>
        a       <http://www.w3.org/2002/07/owl#DatatypeProperty> ;
        <http://www.w3.org/2000/01/rdf-schema#comment>
                "A data property linking an agent to information about that agent."@en ;
        <http://www.w3.org/2000/01/rdf-schema#domain>
                <http://xmlns.com/foaf/0.1/Agent> ;
        <http://www.w3.org/2000/01/rdf-schema#label>
                "has information"@en .

<http://purl.org/cerif/frapo/GovernmentOrganization>
        a       <http://www.w3.org/2002/07/owl#Class> ;
        <http://www.w3.org/2000/01/rdf-schema#comment>
                "An organization that is part of, or funded by, central or local goverment."@en ;
        <http://www.w3.org/2000/01/rdf-schema#label>
                "government organization"@en ;
        <http://www.w3.org/2000/01/rdf-schema#subClassOf>
                <http://xmlns.com/foaf/0.1/Organization> .

<http://purl.org/cerif/frapo/isSuppliedBy>
        a       <http://www.w3.org/2002/07/owl#ObjectProperty> ;
        <http://www.w3.org/2000/01/rdf-schema#comment>
                "An object property relating an entity that is supplied, or an agent to whom an entity is supplied, to the supplier."@en ;
        <http://www.w3.org/2000/01/rdf-schema#label>
                "is supplied by"@en ;
        <http://www.w3.org/2000/01/rdf-schema#range>
                <http://purl.org/cerif/frapo/Supplier> ;
        <http://www.w3.org/2002/07/owl#inverseOf>
                <http://purl.org/cerif/frapo/supplies> .

<http://purl.org/cerif/frapo/business-angel>
        a       <http://www.w3.org/2002/07/owl#NamedIndividual> , <http://xmlns.com/foaf/0.1/Person> ;
        <http://www.w3.org/2000/01/rdf-schema#comment>
                "A person willing to invest in start-up companies."@en ;
        <http://www.w3.org/2000/01/rdf-schema#label>
                "business angel"@en .

<http://purl.org/cerif/frapo/hasLanguageCode>
        a       <http://www.w3.org/2002/07/owl#DatatypeProperty> ;
        <http://www.w3.org/2000/01/rdf-schema#comment>
                "A data property specifying the two-letter or three-letter lower-case code used to identify a language (e.g. fr/fra for French, de/deu for Germany) (see http://en.wikipedia.org/wiki/List_of_ISO_639-1_codes)."@en ;
        <http://www.w3.org/2000/01/rdf-schema#label>
                "has language code"@en ;
        <http://www.w3.org/2000/01/rdf-schema#subPropertyOf>
                <http://purl.org/cerif/frapo/hasCode> .

<http://purl.org/cerif/frapo/familyNameInitial>
        a       <http://www.w3.org/2002/07/owl#DatatypeProperty> ;
        <http://www.w3.org/2000/01/rdf-schema#comment>
                "A data property permitting specification of the initial(s) of a person's family name."@en ;
        <http://www.w3.org/2000/01/rdf-schema#label>
                "family name initial"@en ;
        <http://www.w3.org/2000/01/rdf-schema#subPropertyOf>
                <http://purl.org/cerif/frapo/initial> .

<http://purl.org/cerif/frapo/FundingAgency>
        a       <http://www.w3.org/2002/07/owl#Class> ;
        <http://www.w3.org/2000/01/rdf-schema#comment>
                "An organization that provides funding for projects or resources, often in the form of grants awarded on the basis of competitive application."@en ;
        <http://www.w3.org/2000/01/rdf-schema#label>
                "funding agency"@en ;
        <http://www.w3.org/2000/01/rdf-schema#subClassOf>
                <http://xmlns.com/foaf/0.1/Organization> .

<http://purl.org/cerif/frapo/DocumentRepository>
        a       <http://www.w3.org/2002/07/owl#Class> ;
        <http://www.w3.org/2000/01/rdf-schema#comment>
                "A facility in which digital documents are deposited for long-term preservation and (optional) publication."@en ;
        <http://www.w3.org/2000/01/rdf-schema#label>
                "document repository"@en ;
        <http://www.w3.org/2000/01/rdf-schema#subClassOf>
                <http://purl.org/cerif/frapo/Repository> ;
        <http://purl.org/dc/elements/1.1/description>
                "May also be described as a document archive, or a digital library."@en .

<http://xmlns.com/foaf/0.1/Project>
        a       <http://www.w3.org/2002/07/owl#Class> ;
        <http://www.w3.org/2000/01/rdf-schema#comment>
                "In FRAPO, a project is an administrative entity that enables an endeavour such as a research investigation.  A project relates to the administrative aspects of undertaking an endeavour, including the funding obtained, the people employed, and the management of the project in terms of deadlines and deliverables.  In contrast, an endeavour such as a research investigation relate to the academic and practical aspects of undertaking that endeavour - thus for a research investigation: the research itself, including the hypotheses being investigated, the experiments being undertaken, the data being gathered and analysed, the interpretations being drawn from the data, and the results obtained."@en ;
        <http://www.w3.org/2000/01/rdf-schema#label>
                "project"@en ;
        <http://www.w3.org/2000/01/rdf-schema#subClassOf>
                <http://www.w3.org/2002/07/owl#Thing> ;
        <http://purl.org/dc/elements/1.1/description>
                "Super-class of cerif:Project."@en .

<http://purl.org/cerif/frapo/AdmissionApplication>
        a       <http://www.w3.org/2002/07/owl#Class> ;
        <http://www.w3.org/2000/01/rdf-schema#comment>
                "The activity of applying for admission to some group or institution, for example a learned society or a university."@en ;
        <http://www.w3.org/2000/01/rdf-schema#label>
                "admission application"@en ;
        <http://www.w3.org/2000/01/rdf-schema#subClassOf>
                <http://purl.org/cerif/frapo/Application> .

<http://purl.org/cerif/frapo/building-costs>
        a       <http://www.w3.org/2002/07/owl#NamedIndividual> , <http://purl.org/cerif/frapo/BudgetCategory> ;
        <http://www.w3.org/2000/01/rdf-schema#comment>
                "A budget category to cover the costs of constructing, renovating or modifying a physical building."@en ;
        <http://www.w3.org/2000/01/rdf-schema#label>
                "building costs"@en .

<http://purl.org/cerif/frapo/hasPersonalInformation>
        a       <http://www.w3.org/2002/07/owl#DatatypeProperty> ;
        <http://www.w3.org/2000/01/rdf-schema#comment>
                "A data property linking a person to information about that person."@en ;
        <http://www.w3.org/2000/01/rdf-schema#domain>
                <http://xmlns.com/foaf/0.1/Person> ;
        <http://www.w3.org/2000/01/rdf-schema#label>
                "has contact information"@en ;
        <http://www.w3.org/2000/01/rdf-schema#subPropertyOf>
                <http://purl.org/cerif/frapo/hasAgentInformation> .

<http://purl.org/cerif/frapo>
        a       <http://www.w3.org/2002/07/owl#Ontology> ;
        <http://www.w3.org/2000/01/rdf-schema#comment>
                "The Funding, Research Administration and Projects Ontology (FRAPO) is an ontology for describing the administrative information of research projects, e.g., grant applications, funding bodies, project partners, etc.\n\n**URL:** http://purl.org/cerif/frapo\n\n**Creators**: [David Shotton](http://orcid.org/0000-0001-5506-523X)\n\n**Contributors**: [Silvio Peroni](http://orcid.org/0000-0003-0530-4305)\n\n**License:** [Creative Commons Attribution 4.0 International](https://creativecommons.org/licenses/by/4.0/legalcode)\n\n**Website:** http://www.sparontologies.net/ontologies/frapo" ;
        <http://purl.org/dc/elements/1.1/contributor>
                "Silvio Peroni" ;
        <http://purl.org/dc/elements/1.1/creator>
                "David Shotton" ;
        <http://purl.org/dc/elements/1.1/date>
                "2017-09-04" ;
        <http://purl.org/dc/elements/1.1/description>
                "FRAPO is an ontology for use to describe research project administrative information and to work with CRIS (Current Research Information Systems). It can be used for the characterization of grant applications, funding bodies, projects, project partners, etc.  It can also be used to describe other types of projects, for example building projects and educational projects.  \n\nFRAPO imports FOAF and is designed to work with SCoRO, the Scholarly Contributions and Roles Ontology (http://purl.org/spar/scoro), which is used to characterize the contributions and time-limited roles that may exist between agents such as people and organizations and entities such as projects, research investigations or research outputs.\n\nFaBiO, the FRBR-alightned bibliographic ontology (http://purl.org/spar/fabio), provides terms for documents of relevance, such as grant applications, project plans, project reports, datasets and journal articles, which are therefore not included within FRAPO.\n\nFRAPO is not intended to describe the details of research investigations enabled by funded research projects, nor their component studies and assays, which are the domain of a complementary ontology, ISA-RDF (under development - add URL)." ;
        <http://purl.org/dc/elements/1.1/rights>
                "This work is distributed under a Creative Commons Attribution License (http://creativecommons.org/licenses/by/3.0/)."@en ;
        <http://purl.org/dc/elements/1.1/title>
                "FRAPO, the Funding, Research Administration and Projects Ontology" ;
        <http://www.w3.org/2002/07/owl#imports>
                <https://w3id.org/spar/foaf> ;
        <http://www.w3.org/2002/07/owl#priorVersion>
                <http://svn.code.sf.net/p/cerif/code/trunk/FRAPO/2014-01-31-FRAPO-1_1.owl> ;
        <http://www.w3.org/2002/07/owl#versionIRI>
                <http://purl.org/cerif/frapo/2017-09-04> ;
        <http://www.w3.org/2002/07/owl#versionInfo>
                "1.1.1" .

<http://purl.org/cerif/frapo/hasPurchaseDate>
        a       <http://www.w3.org/2002/07/owl#FunctionalProperty> , <http://www.w3.org/2002/07/owl#DatatypeProperty> ;
        <http://www.w3.org/2000/01/rdf-schema#comment>
                "A data property linking something to its purchase date."@en ;
        <http://www.w3.org/2000/01/rdf-schema#label>
                "has purchase date"@en ;
        <http://www.w3.org/2000/01/rdf-schema#range>
                <http://www.w3.org/2001/XMLSchema#dateTime> ;
        <http://www.w3.org/2000/01/rdf-schema#subPropertyOf>
                <http://purl.org/dc/terms/date> .

<http://purl.org/cerif/frapo/hasPostCode>
        a       <http://www.w3.org/2002/07/owl#DatatypeProperty> ;
        <http://www.w3.org/2000/01/rdf-schema#comment>
                "A data property defining the postal code of an address."@en ;
        <http://www.w3.org/2000/01/rdf-schema#label>
                "has post code"@en ;
        <http://www.w3.org/2000/01/rdf-schema#subPropertyOf>
                <http://purl.org/cerif/frapo/hasCode> .

<http://purl.org/cerif/frapo/hasFundingAgency>
        a       <http://www.w3.org/2002/07/owl#ObjectProperty> ;
        <http://www.w3.org/2000/01/rdf-schema#comment>
                "An object property linking something to a funding agency that provides funding for it."@en ;
        <http://www.w3.org/2000/01/rdf-schema#label>
                "has funding agency"@en ;
        <http://www.w3.org/2000/01/rdf-schema#range>
                <http://purl.org/cerif/frapo/FundingAgency> ;
        <http://www.w3.org/2000/01/rdf-schema#subPropertyOf>
                <http://purl.org/cerif/frapo/isSupportedBy> ;
        <http://www.w3.org/2002/07/owl#inverseOf>
                <http://purl.org/cerif/frapo/isFundingAgencyFor> .

<http://purl.org/cerif/frapo/Deliverable>
        a       <http://www.w3.org/2002/07/owl#Class> ;
        <http://www.w3.org/2000/01/rdf-schema#comment>
                "A class defining a 'deliverable' of a project, i.e. something that the project set out to deliver, or succeeds in delivering."@en ;
        <http://www.w3.org/2000/01/rdf-schema#label>
                "deliverable"@en ;
        <http://www.w3.org/2000/01/rdf-schema#subClassOf>
                <http://purl.org/cerif/frapo/Output> .

<http://purl.org/cerif/frapo/funded>
        a       <http://www.w3.org/2002/07/owl#NamedIndividual> , <http://purl.org/cerif/frapo/Status> ;
        <http://www.w3.org/2000/01/rdf-schema#comment>
                "The status of something such as an investigation or a project as being funded."@en ;
        <http://www.w3.org/2000/01/rdf-schema#label>
                "funded"@en .

<http://purl.org/cerif/frapo/hasRegistrationDeadline>
        a       <http://www.w3.org/2002/07/owl#FunctionalProperty> , <http://www.w3.org/2002/07/owl#DatatypeProperty> ;
        <http://www.w3.org/2000/01/rdf-schema#comment>
                "The date by which registration must be made, for example renewal of an internet domain name."@en ;
        <http://www.w3.org/2000/01/rdf-schema#label>
                "has registration deadline"@en ;
        <http://www.w3.org/2000/01/rdf-schema#range>
                <http://www.w3.org/2001/XMLSchema#dateTime> ;
        <http://www.w3.org/2000/01/rdf-schema#subPropertyOf>
                <http://purl.org/dc/terms/date> .

<http://purl.org/cerif/frapo/InfrastructureEntity>
        a       <http://www.w3.org/2002/07/owl#Class> ;
        <http://www.w3.org/2000/01/rdf-schema#comment>
                "An entity that facilitates work."@en ;
        <http://www.w3.org/2000/01/rdf-schema#label>
                "infrastructure entity"@en ;
        <http://www.w3.org/2000/01/rdf-schema#subClassOf>
                <http://www.w3.org/2002/07/owl#Thing> ;
        <http://purl.org/dc/elements/1.1/description>
                "owl:equivalentClass cerif:InfrastructureEntity ."@en .

<http://purl.org/cerif/frapo/isAppliedForBy>
        a       <http://www.w3.org/2002/07/owl#ObjectProperty> ;
        <http://www.w3.org/2000/01/rdf-schema#comment>
                "An object property linking something applied for to the agent making the application."@en ;
        <http://www.w3.org/2000/01/rdf-schema#label>
                "is applied for by"@en ;
        <http://www.w3.org/2000/01/rdf-schema#range>
                <http://xmlns.com/foaf/0.1/Agent> .

<http://purl.org/cerif/frapo/submits>
        a       <http://www.w3.org/2002/07/owl#ObjectProperty> ;
        <http://www.w3.org/2000/01/rdf-schema#comment>
                "An object property linking an agent to an entity that is submitted to some third party, for example a grant application submitted to a funding agency, a manuscript submitted to a publisher, a quotation submitted by a vendor, or a dataset submitted by a researcher to a data repository."@en ;
        <http://www.w3.org/2000/01/rdf-schema#domain>
                <http://xmlns.com/foaf/0.1/Agent> ;
        <http://www.w3.org/2000/01/rdf-schema#label>
                "submits"@en .

<http://xmlns.com/foaf/0.1/Organization>
        a       <http://www.w3.org/2002/07/owl#Class> ;
        <http://purl.org/dc/elements/1.1/description>
                "owl:equivalentClass cerf:OrganizationalUnit ."@en .

<http://purl.org/cerif/frapo/publishing-costs>
        a       <http://purl.org/cerif/frapo/BudgetCategory> , <http://www.w3.org/2002/07/owl#NamedIndividual> ;
        <http://www.w3.org/2000/01/rdf-schema#comment>
                "A budget category to cover the cost of publishing outpots from a project, for example author fees for journal articles in an open access journal."@en ;
        <http://www.w3.org/2000/01/rdf-schema#label>
                "publishing costs"@en .

<http://purl.org/cerif/frapo/hasPostalAddressLine>
        a       <http://www.w3.org/2002/07/owl#DatatypeProperty> ;
        <http://www.w3.org/2000/01/rdf-schema#comment>
                "A data property permitting specification of a single line of a postal address."@en ;
        <http://www.w3.org/2000/01/rdf-schema#domain>
                <http://purl.org/cerif/frapo/PostalAddress> ;
        <http://www.w3.org/2000/01/rdf-schema#label>
                "has postal address line"@en ;
        <http://www.w3.org/2000/01/rdf-schema#subPropertyOf>
                <http://purl.org/cerif/frapo/hasAgentInformation> .

<http://xmlns.com/foaf/0.1/surname>
        a       <http://www.w3.org/2002/07/owl#DatatypeProperty> , <http://www.w3.org/2002/07/owl#AnnotationProperty> ;
        <http://www.w3.org/2000/01/rdf-schema#subPropertyOf>
                <http://purl.org/cerif/frapo/hasPersonalInformation> .

<http://xmlns.com/foaf/0.1/name>
        a       <http://www.w3.org/2002/07/owl#DatatypeProperty> , <http://www.w3.org/2002/07/owl#AnnotationProperty> ;
        <http://www.w3.org/2000/01/rdf-schema#subPropertyOf>
                <http://purl.org/cerif/frapo/hasPersonalInformation> .

<http://purl.org/cerif/frapo/ComputationalAgent>
        a       <http://www.w3.org/2002/07/owl#Class> ;
        <http://www.w3.org/2000/01/rdf-schema#comment>
                "A computer system or software program whose action has an effect on external events, for example a laboratory robot that undertakes your experiments, or the financial control system that controls an institution's payrole, or that, following programmed business rules, prevents the principal investigator from placing an order for research equipment because there is insufficient money left in the project budget."@en ;
        <http://www.w3.org/2000/01/rdf-schema#label>
                "computational agent"@en ;
        <http://www.w3.org/2000/01/rdf-schema#subClassOf>
                <http://xmlns.com/foaf/0.1/Agent> .

<http://purl.org/cerif/frapo/Faculty>
        a       <http://www.w3.org/2002/07/owl#Class> ;
        <http://www.w3.org/2000/01/rdf-schema#comment>
                "A grouping of similar departments within a university context, also known as a school or a division, for example the Humanities Division, the Mathematics Faculty, or the School of Medicine."@en ;
        <http://www.w3.org/2000/01/rdf-schema#label>
                "faculty"@en ;
        <http://www.w3.org/2000/01/rdf-schema#subClassOf>
                <http://purl.org/cerif/frapo/Division> .

<http://purl.org/dc/elements/1.1/title>
        a       <http://www.w3.org/2002/07/owl#AnnotationProperty> .

<http://xmlns.com/foaf/0.1/nick>
        a       <http://www.w3.org/2002/07/owl#DatatypeProperty> , <http://www.w3.org/2002/07/owl#AnnotationProperty> ;
        <http://www.w3.org/2000/01/rdf-schema#subPropertyOf>
                <http://purl.org/cerif/frapo/hasPersonalInformation> .

<http://purl.org/cerif/frapo/Endowment>
        a       <http://www.w3.org/2002/07/owl#Class> ;
        <http://www.w3.org/2000/01/rdf-schema#comment>
                "A transfer, generally as a gift, of money or property to an institution to provide a permanent fund, the income from which is to be used for a particular purpose.  (Abbreviated from http://legal-dictionary.thefreedictionary.com/endowment)."@en ;
        <http://www.w3.org/2000/01/rdf-schema#label>
                "endowment"@en ;
        <http://www.w3.org/2000/01/rdf-schema#subClassOf>
                <http://purl.org/cerif/frapo/Gift> .

<http://purl.org/cerif/frapo/employs>
        a       <http://www.w3.org/2002/07/owl#ObjectProperty> ;
        <http://www.w3.org/2000/01/rdf-schema#comment>
                "An object property relating an employing agent to an employed agent, for example a person or an organization, who is typically employed to undertaking specified work in exchange for payment."@en ;
        <http://www.w3.org/2000/01/rdf-schema#domain>
                <http://xmlns.com/foaf/0.1/Agent> ;
        <http://www.w3.org/2000/01/rdf-schema#label>
                "employs"@en ;
        <http://www.w3.org/2000/01/rdf-schema#range>
                <http://xmlns.com/foaf/0.1/Agent> ;
        <http://purl.org/dc/elements/1.1/description>
                "This property should not be used for the other meaning of 'employ', meaning to use something, e.g. 'He employed great skill . . .'/"@en ;
        <http://www.w3.org/2002/07/owl#inverseOf>
                <http://purl.org/cerif/frapo/isEmployedBy> .

<http://purl.org/cerif/frapo/Manufacturer>
        a       <http://www.w3.org/2002/07/owl#Class> ;
        <http://www.w3.org/2000/01/rdf-schema#comment>
                "An agent who manufactures goods or equipment."@en ;
        <http://www.w3.org/2000/01/rdf-schema#label>
                "manufacturer"@en ;
        <http://www.w3.org/2000/01/rdf-schema#subClassOf>
                <http://xmlns.com/foaf/0.1/Agent> .

<http://purl.org/cerif/frapo/isAwardedBy>
        a       <http://www.w3.org/2002/07/owl#ObjectProperty> , <http://www.w3.org/2002/07/owl#FunctionalProperty> ;
        <http://www.w3.org/2000/01/rdf-schema#comment>
                "An object property linking something awarded to the agent making the award, for example linking a grant to a funding agency, a degree to a university, or a prize to the awarding organization."@en ;
        <http://www.w3.org/2000/01/rdf-schema#label>
                "is awarded by"@en ;
        <http://www.w3.org/2000/01/rdf-schema#range>
                <http://xmlns.com/foaf/0.1/Agent> ;
        <http://purl.org/dc/elements/1.1/description>
                "Domain constraints have been removed from this object property to permit it to be used in unforeseen ways."@en .

<http://purl.org/cerif/frapo/providesService>
        a       <http://www.w3.org/2002/07/owl#ObjectProperty> ;
        <http://www.w3.org/2000/01/rdf-schema#comment>
                "An agent that provides a service."@en ;
        <http://www.w3.org/2000/01/rdf-schema#domain>
                <http://xmlns.com/foaf/0.1/Agent> ;
        <http://www.w3.org/2000/01/rdf-schema#label>
                "provides service"@en ;
        <http://purl.org/dc/elements/1.1/description>
                "Range constraints have been removed from this object property to permit it to be used in unforeseen ways."@en .

<http://purl.org/cerif/frapo/ComputationalService>
        a       <http://www.w3.org/2002/07/owl#Class> ;
        <http://www.w3.org/2000/01/rdf-schema#comment>
                "A service provided by a computer system."@en ;
        <http://www.w3.org/2000/01/rdf-schema#label>
                "computational service"@en ;
        <http://www.w3.org/2000/01/rdf-schema#subClassOf>
                <http://purl.org/cerif/frapo/Service> .

<http://purl.org/cerif/frapo/isEvaluatedBy>
        a       <http://www.w3.org/2002/07/owl#ObjectProperty> ;
        <http://www.w3.org/2000/01/rdf-schema#comment>
                "An object property linking an entity to an agent that evaluates it."@en ;
        <http://www.w3.org/2000/01/rdf-schema#label>
                "is evaluated by"@en ;
        <http://www.w3.org/2000/01/rdf-schema#range>
                <http://xmlns.com/foaf/0.1/Agent> .

<http://purl.org/cerif/frapo/Tender>
        a       <http://www.w3.org/2002/07/owl#Class> ;
        <http://www.w3.org/2000/01/rdf-schema#comment>
                "Sealed bid or offer document submitted in response to a request for tenders, containing detailed information on costs, requirements and terms associated with a potential contract.  (Adapted from http://www.businessdictionary.com/definition/tender.html)."@en ;
        <http://www.w3.org/2000/01/rdf-schema#label>
                "tender"@en ;
        <http://www.w3.org/2000/01/rdf-schema#subClassOf>
                <http://purl.org/cerif/frapo/FinancialEntity> .

<http://purl.org/cerif/frapo/hasCallIdentifier>
        a       <http://www.w3.org/2002/07/owl#DatatypeProperty> ;
        <http://www.w3.org/2000/01/rdf-schema#comment>
                "A data property specifying the identifying number of a call for applications issued by a funding agency."@en ;
        <http://www.w3.org/2000/01/rdf-schema#label>
                "has call identifier"@en ;
        <http://www.w3.org/2000/01/rdf-schema#subPropertyOf>
                <http://purl.org/dc/terms/identifier> .

<http://purl.org/cerif/frapo/hasProvenance>
        a       <http://www.w3.org/2002/07/owl#DatatypeProperty> ;
        <http://www.w3.org/2000/01/rdf-schema#comment>
                "A data property that permits the provenance of an entity to be described."@en ;
        <http://www.w3.org/2000/01/rdf-schema#label>
                "has provenance"@en ;
        <http://www.w3.org/2000/01/rdf-schema#subPropertyOf>
                <http://www.w3.org/2002/07/owl#topDataProperty> .

<http://purl.org/cerif/frapo/isSupportedBy>
        a       <http://www.w3.org/2002/07/owl#ObjectProperty> ;
        <http://www.w3.org/2000/01/rdf-schema#comment>
                "An object property linking something to an agent that provides funding or other support for it."@en ;
        <http://www.w3.org/2000/01/rdf-schema#label>
                "is supported by"@en ;
        <http://www.w3.org/2000/01/rdf-schema#range>
                [ a       <http://www.w3.org/2002/07/owl#Class> ;
                  <http://www.w3.org/2002/07/owl#unionOf>
                          ( <http://purl.org/cerif/frapo/Funding> <http://xmlns.com/foaf/0.1/Agent> )
                ] ;
        <http://purl.org/dc/elements/1.1/description>
                "This property is not intended for use to describe mechanical or physical support, as in 'The statue is supported by the plinth'. "@en ;
        <http://www.w3.org/2002/07/owl#inverseOf>
                <http://purl.org/cerif/frapo/supports> .

<http://purl.org/cerif/frapo/hasEndDate>
        a       <http://www.w3.org/2002/07/owl#FunctionalProperty> , <http://www.w3.org/2002/07/owl#DatatypeProperty> ;
        <http://www.w3.org/2000/01/rdf-schema#comment>
                "A data property linking something such as a project to its end date."@en ;
        <http://www.w3.org/2000/01/rdf-schema#label>
                "has end date"@en ;
        <http://www.w3.org/2000/01/rdf-schema#range>
                <http://www.w3.org/2001/XMLSchema#dateTime> ;
        <http://www.w3.org/2000/01/rdf-schema#subPropertyOf>
                <http://purl.org/dc/terms/date> .

<http://purl.org/cerif/frapo/hasApplicationDeadline>
        a       <http://www.w3.org/2002/07/owl#AnnotationProperty> , <http://www.w3.org/2002/07/owl#FunctionalProperty> , <http://www.w3.org/2002/07/owl#DatatypeProperty> ;
        <http://www.w3.org/2000/01/rdf-schema#comment>
                "The date by which an application, for example a job application, a fellowship application or a grant application, has to be submitted if it is to be considered for acceptance or funding."@en ;
        <http://www.w3.org/2000/01/rdf-schema#domain>
                <http://purl.org/cerif/frapo/Application> ;
        <http://www.w3.org/2000/01/rdf-schema#label>
                "has application deadline"@en ;
        <http://www.w3.org/2000/01/rdf-schema#range>
                <http://www.w3.org/2001/XMLSchema#dateTime> ;
        <http://www.w3.org/2000/01/rdf-schema#subPropertyOf>
                <http://purl.org/dc/terms/date> ;
        <http://purl.org/dc/elements/1.1/description>
                "owl:equivalentProperty fabio:hasApplicationDeadline ."@en .

<http://purl.org/cerif/frapo/hasFunderIdentifier>
        a       <http://www.w3.org/2002/07/owl#DatatypeProperty> ;
        <http://www.w3.org/2000/01/rdf-schema#comment>
                "A data property linking a funding agency to an identifier for that funding agency."@en ;
        <http://www.w3.org/2000/01/rdf-schema#domain>
                <http://purl.org/cerif/frapo/FundingAgency> ;
        <http://www.w3.org/2000/01/rdf-schema#label>
                "has funder identifer"@en ;
        <http://www.w3.org/2000/01/rdf-schema#subPropertyOf>
                <http://purl.org/dc/terms/identifier> .

<http://purl.org/cerif/frapo/College>
        a       <http://www.w3.org/2002/07/owl#Class> ;
        <http://www.w3.org/2000/01/rdf-schema#comment>
                "An academic organization that is either a small degree-giving university, or (in the OxBridge sense) an independent corporation of scholars within a larger university, providing undergraduate tuition and a social environment for its students and fellows."@en ;
        <http://www.w3.org/2000/01/rdf-schema#label>
                "college"@en ;
        <http://www.w3.org/2000/01/rdf-schema#subClassOf>
                <http://xmlns.com/foaf/0.1/Organization> .

<http://purl.org/cerif/frapo/ProjectBudget>
        a       <http://www.w3.org/2002/07/owl#Class> ;
        <http://www.w3.org/2000/01/rdf-schema#comment>
                "A budget for a research project."@en ;
        <http://www.w3.org/2000/01/rdf-schema#label>
                "project budget"@en ;
        <http://www.w3.org/2000/01/rdf-schema#subClassOf>
                <http://purl.org/cerif/frapo/Budget> .

<http://purl.org/cerif/frapo/appliesFor>
        a       <http://www.w3.org/2002/07/owl#ObjectProperty> ;
        <http://www.w3.org/2000/01/rdf-schema#comment>
                "An object property linking an agent to something for which that agent applies, for example a job, membership of an organization, or a grant from a funding agency."@en ;
        <http://www.w3.org/2000/01/rdf-schema#domain>
                <http://xmlns.com/foaf/0.1/Agent> ;
        <http://www.w3.org/2000/01/rdf-schema#label>
                "applies for"@en ;
        <http://www.w3.org/2002/07/owl#inverseOf>
                <http://purl.org/cerif/frapo/isAppliedForBy> .

<http://purl.org/cerif/frapo/hasStartDate>
        a       <http://www.w3.org/2002/07/owl#DatatypeProperty> , <http://www.w3.org/2002/07/owl#FunctionalProperty> ;
        <http://www.w3.org/2000/01/rdf-schema#comment>
                "A data property linking something such as a project to its start date."@en ;
        <http://www.w3.org/2000/01/rdf-schema#label>
                "has start date"@en ;
        <http://www.w3.org/2000/01/rdf-schema#range>
                <http://www.w3.org/2001/XMLSchema#dateTime> ;
        <http://www.w3.org/2000/01/rdf-schema#subPropertyOf>
                <http://purl.org/dc/terms/date> .

<http://purl.org/cerif/frapo/enables>
        a       <http://www.w3.org/2002/07/owl#ObjectProperty> ;
        <http://www.w3.org/2000/01/rdf-schema#comment>
                "An object property relating an entity to another entity that it enables, e.g. linking a project to an endeavour that the project enables."@en ;
        <http://www.w3.org/2000/01/rdf-schema#label>
                "enables"@en ;
        <http://purl.org/dc/elements/1.1/description>
                "Domain and range constraints have been removed from this object property to permit it to be used in unforeseen ways."@en ;
        <http://www.w3.org/2002/07/owl#inverseOf>
                <http://purl.org/cerif/frapo/isEnabledBy> .

<http://purl.org/cerif/frapo/NotForProfitOrganization>
        a       <http://www.w3.org/2002/07/owl#Class> ;
        <http://www.w3.org/2000/01/rdf-schema#comment>
                "An organization that does not primarily exist to make profit, for example a charity or charitable foundation, a learned society, or a standards body such as the World Wide Web Consortium."@en ;
        <http://www.w3.org/2000/01/rdf-schema#label>
                "not-for-profit organization"@en ;
        <http://www.w3.org/2000/01/rdf-schema#subClassOf>
                <http://xmlns.com/foaf/0.1/Organization> .

<http://purl.org/cerif/frapo/hasORCID>
        a       <http://www.w3.org/2002/07/owl#DatatypeProperty> ;
        <http://www.w3.org/2000/01/rdf-schema#comment>
                "A data property relating an individual to his/her Open Researcher and Contributor ID (ORCID), an alphanumeric identifier for individual scholars described at http://about.orcid.org/."@en ;
        <http://www.w3.org/2000/01/rdf-schema#label>
                "has ORCID"@en ;
        <http://www.w3.org/2000/01/rdf-schema#subPropertyOf>
                <http://purl.org/cerif/frapo/hasPersonalIdentifier> ;
        <http://purl.org/dc/elements/1.1/description>
                "owl:equivalentProperty <http://purl.org/spar/scoro/hasORCID> ."@en .

<http://purl.org/cerif/frapo/supports>
        a       <http://www.w3.org/2002/07/owl#ObjectProperty> ;
        <http://www.w3.org/2000/01/rdf-schema#comment>
                "An object property linking an agent to something that the agent supports by financial or other means."@en ;
        <http://www.w3.org/2000/01/rdf-schema#domain>
                [ a       <http://www.w3.org/2002/07/owl#Class> ;
                  <http://www.w3.org/2002/07/owl#unionOf>
                          ( <http://purl.org/cerif/frapo/Funding> <http://xmlns.com/foaf/0.1/Agent> )
                ] ;
        <http://www.w3.org/2000/01/rdf-schema#label>
                "supports"@en ;
        <http://purl.org/dc/elements/1.1/description>
                "This property is not intended for use to describe mechanical or physical support, as in 'The plinth supports the statue'. "@en .

<http://purl.org/cerif/frapo/other-costs>
        a       <http://www.w3.org/2002/07/owl#NamedIndividual> , <http://purl.org/cerif/frapo/BudgetCategory> ;
        <http://www.w3.org/2000/01/rdf-schema#comment>
                "A budget category to cover costs not covered in other budget categories."@en ;
        <http://www.w3.org/2000/01/rdf-schema#label>
                "other costs"@en .

<http://purl.org/cerif/frapo/isEmployedBy>
        a       <http://www.w3.org/2002/07/owl#ObjectProperty> ;
        <http://www.w3.org/2000/01/rdf-schema#comment>
                "An object property relating an employed agent, typically a person or an organization, to an employing agent."@en ;
        <http://www.w3.org/2000/01/rdf-schema#domain>
                <http://xmlns.com/foaf/0.1/Agent> ;
        <http://www.w3.org/2000/01/rdf-schema#label>
                "is employed by"@en ;
        <http://www.w3.org/2000/01/rdf-schema#range>
                <http://xmlns.com/foaf/0.1/Agent> ;
        <http://www.w3.org/2000/01/rdf-schema#subPropertyOf>
                <http://www.w3.org/2002/07/owl#topObjectProperty> ;
        <http://purl.org/dc/elements/1.1/description>
                "This property should not be used for the other meaning of 'employ', meaning to use something, e.g. 'Great skill is employed by master craftsmen . . .'/"@en .

<http://purl.org/cerif/frapo/DataRepository>
        a       <http://www.w3.org/2002/07/owl#Class> ;
        <http://www.w3.org/2000/01/rdf-schema#comment>
                "A facility in which digital data are deposited for long-term preservation and (optional) publication."@en ;
        <http://www.w3.org/2000/01/rdf-schema#label>
                "data repository"@en ;
        <http://www.w3.org/2000/01/rdf-schema#subClassOf>
                <http://purl.org/cerif/frapo/Repository> ;
        <http://purl.org/dc/elements/1.1/description>
                "May also be described as a data archive, or as a database."@en .

<http://xmlns.com/foaf/0.1/title>
        a       <http://www.w3.org/2002/07/owl#AnnotationProperty> , <http://www.w3.org/2002/07/owl#DatatypeProperty> ;
        <http://www.w3.org/2000/01/rdf-schema#subPropertyOf>
                <http://purl.org/cerif/frapo/hasPersonalInformation> .

<http://purl.org/cerif/frapo/hasAwardDate>
        a       <http://www.w3.org/2002/07/owl#FunctionalProperty> , <http://www.w3.org/2002/07/owl#DatatypeProperty> ;
        <http://www.w3.org/2000/01/rdf-schema#comment>
                "The date on which notification is given or received that something, for example a scholarship or a grant, has been awarded.  [See also frapo:hasDecisionDate.]"@en ;
        <http://www.w3.org/2000/01/rdf-schema#label>
                "has award date"@en ;
        <http://www.w3.org/2000/01/rdf-schema#range>
                <http://www.w3.org/2001/XMLSchema#date> ;
        <http://www.w3.org/2000/01/rdf-schema#subPropertyOf>
                <http://purl.org/dc/terms/date> .

<http://purl.org/cerif/frapo/Commitments>
        a       <http://www.w3.org/2002/07/owl#Class> ;
        <http://www.w3.org/2000/01/rdf-schema#comment>
                "Money set aside to honour expenditures already made but for which no invoices have yet been received, or expenditures planned for the future, for example for salaries."@en ;
        <http://www.w3.org/2000/01/rdf-schema#label>
                "commitments"@en ;
        <http://www.w3.org/2000/01/rdf-schema#subClassOf>
                <http://purl.org/cerif/frapo/BudgetInformation> .

<http://purl.org/cerif/frapo/BudgetCategory>
        a       <http://www.w3.org/2002/07/owl#Class> ;
        <http://www.w3.org/2000/01/rdf-schema#comment>
                "A category of expenditure within a budget, determining what the allocated money can be spent on, for example salaries, equipment, travel."@en ;
        <http://www.w3.org/2000/01/rdf-schema#label>
                "budget category"@en ;
        <http://www.w3.org/2000/01/rdf-schema#subClassOf>
                <http://purl.org/cerif/frapo/FinancialEntity> .

<http://purl.org/dc/elements/1.1/creator>
        a       <http://www.w3.org/2002/07/owl#AnnotationProperty> .

<http://purl.org/cerif/frapo/ConsortiumAgreement>
        a       <http://www.w3.org/2002/07/owl#Class> ;
        <http://www.w3.org/2000/01/rdf-schema#comment>
                "A formal agreement between members of a consortium, for example between research groups at different universities engaged in a multi-partner research project."@en ;
        <http://www.w3.org/2000/01/rdf-schema#label>
                "consortium agreement"@en ;
        <http://www.w3.org/2000/01/rdf-schema#subClassOf>
                <http://purl.org/cerif/frapo/Contract> .

<http://purl.org/cerif/frapo/Bursary>
        a       <http://www.w3.org/2002/07/owl#Class> ;
        <http://www.w3.org/2000/01/rdf-schema#comment>
                "An amount of money given to a person by an organization, for example by a university to a university student in need to enable that student to continue his/her studies."@en ;
        <http://www.w3.org/2000/01/rdf-schema#label>
                "bursary"@en ;
        <http://www.w3.org/2000/01/rdf-schema#subClassOf>
                <http://purl.org/cerif/frapo/Funding> .

<http://purl.org/cerif/frapo/hasCost>
        a       <http://www.w3.org/2002/07/owl#DatatypeProperty> ;
        <http://www.w3.org/2000/01/rdf-schema#comment>
                "A data property enabling the cost of something that can be paid for to be defined."@en ;
        <http://www.w3.org/2000/01/rdf-schema#label>
                "has cost"@en .

<http://purl.org/cerif/frapo/sellsTo>
        a       <http://www.w3.org/2002/07/owl#ObjectProperty> ;
        <http://www.w3.org/2000/01/rdf-schema#comment>
                "An object property relating a supplier to a purchaser to whom an entity is sold."@en ;
        <http://www.w3.org/2000/01/rdf-schema#domain>
                <http://xmlns.com/foaf/0.1/Agent> ;
        <http://www.w3.org/2000/01/rdf-schema#label>
                "sells to"@en ;
        <http://www.w3.org/2000/01/rdf-schema#range>
                <http://xmlns.com/foaf/0.1/Agent> ;
        <http://purl.org/dc/elements/1.1/description>
                "Domain and range constraints on this object property have been relaxed to permit it to be used in unforeseen ways."@en .

<http://purl.org/cerif/frapo/hasInvoiceDate>
        a       <http://www.w3.org/2002/07/owl#AnnotationProperty> , <http://www.w3.org/2002/07/owl#DatatypeProperty> , <http://www.w3.org/2002/07/owl#FunctionalProperty> ;
        <http://www.w3.org/2000/01/rdf-schema#comment>
                "A data property linking an invoice to its date."@en ;
        <http://www.w3.org/2000/01/rdf-schema#domain>
                <http://purl.org/cerif/frapo/Invoice> ;
        <http://www.w3.org/2000/01/rdf-schema#label>
                "has invoice date"@en ;
        <http://www.w3.org/2000/01/rdf-schema#range>
                <http://www.w3.org/2001/XMLSchema#date> ;
        <http://www.w3.org/2000/01/rdf-schema#subPropertyOf>
                <http://purl.org/dc/terms/date> .

<http://purl.org/cerif/frapo/Fee>
        a       <http://www.w3.org/2002/07/owl#Class> ;
        <http://www.w3.org/2000/01/rdf-schema#comment>
                "An amount of money paid for something that is not purchased."@en ;
        <http://www.w3.org/2000/01/rdf-schema#label>
                "fee"@en ;
        <http://www.w3.org/2000/01/rdf-schema#subClassOf>
                <http://purl.org/cerif/frapo/FinancialEntity> .

<http://purl.org/cerif/frapo/Expenditure>
        a       <http://www.w3.org/2002/07/owl#Class> ;
        <http://www.w3.org/2000/01/rdf-schema#comment>
                "Money going out of an account, because of expenditure on various entities. May be associated with a particular budget category."@en ;
        <http://www.w3.org/2000/01/rdf-schema#label>
                "expenditure"@en ;
        <http://www.w3.org/2000/01/rdf-schema#subClassOf>
                <http://purl.org/cerif/frapo/BudgetInformation> .

<http://purl.org/cerif/frapo/hasProfessionalName>
        a       <http://www.w3.org/2002/07/owl#DatatypeProperty> ;
        <http://www.w3.org/2000/01/rdf-schema#comment>
                "An alternative name that a person uses for professional purposes, for example the pen name of an author, or a married woman's maiden name used as her professional name. "@en ;
        <http://www.w3.org/2000/01/rdf-schema#label>
                "has alternate name"@en ;
        <http://www.w3.org/2000/01/rdf-schema#subPropertyOf>
                <http://purl.org/cerif/frapo/hasPersonalInformation> .

<http://purl.org/cerif/frapo/Funding>
        a       <http://www.w3.org/2002/07/owl#Class> ;
        <http://www.w3.org/2000/01/rdf-schema#comment>
                "An amount of money available to finance some project or activity. "@en ;
        <http://www.w3.org/2000/01/rdf-schema#label>
                "funding"@en ;
        <http://www.w3.org/2000/01/rdf-schema#subClassOf>
                <http://purl.org/cerif/frapo/FinancialEntity> .

<http://purl.org/cerif/frapo/usesService>
        a       <http://www.w3.org/2002/07/owl#ObjectProperty> ;
        <http://www.w3.org/2000/01/rdf-schema#comment>
                "An object property linking an activity such as an expedition, a research project or an investigation, to a service employed in that activity."@en ;
        <http://www.w3.org/2000/01/rdf-schema#label>
                "uses service"@en ;
        <http://www.w3.org/2000/01/rdf-schema#range>
                <http://purl.org/cerif/frapo/Service> ;
        <http://purl.org/dc/elements/1.1/description>
                "Domain constraints have been removed from this object property to permit it to be used in unforeseen ways."@en .

<http://purl.org/cerif/frapo/Application>
        a       <http://www.w3.org/2002/07/owl#Class> ;
        <http://www.w3.org/2000/01/rdf-schema#comment>
                "The activity of making an application, for example for a job, or for funding."@en ;
        <http://www.w3.org/2000/01/rdf-schema#label>
                "application"@en ;
        <http://www.w3.org/2000/01/rdf-schema#subClassOf>
                <http://www.w3.org/2002/07/owl#Thing> .

<http://purl.org/cerif/frapo/usesFacility>
        a       <http://www.w3.org/2002/07/owl#ObjectProperty> ;
        <http://www.w3.org/2000/01/rdf-schema#comment>
                "An object property linking an activity such as an expedition, a research project or an investigation, to a facility employed in that activity."@en ;
        <http://www.w3.org/2000/01/rdf-schema#label>
                "uses facility"@en ;
        <http://www.w3.org/2000/01/rdf-schema#range>
                <http://purl.org/cerif/frapo/Facility> ;
        <http://www.w3.org/2000/01/rdf-schema#subPropertyOf>
                <http://www.w3.org/2002/07/owl#topObjectProperty> ;
        <http://purl.org/dc/elements/1.1/description>
                "Domain constraints have been removed from this object property to permit it to be used in unforeseen ways."@en .

<http://purl.org/cerif/frapo/Income>
        a       <http://www.w3.org/2002/07/owl#Class> ;
        <http://www.w3.org/2000/01/rdf-schema#comment>
                "Money coming into an account.  May be associated with a particular budget category."@en ;
        <http://www.w3.org/2000/01/rdf-schema#label>
                "income"@en ;
        <http://www.w3.org/2000/01/rdf-schema#subClassOf>
                <http://purl.org/cerif/frapo/BudgetInformation> .

<http://purl.org/cerif/frapo/Investment>
        a       <http://www.w3.org/2002/07/owl#Class> ;
        <http://www.w3.org/2000/01/rdf-schema#comment>
                "An investment of money, generally in stocks and shares, or in property, for the purpose of safeguarding the capital and yielding an income."@en ;
        <http://www.w3.org/2000/01/rdf-schema#label>
                "investment"@en ;
        <http://www.w3.org/2000/01/rdf-schema#subClassOf>
                <http://purl.org/cerif/frapo/FinancialEntity> .

<http://purl.org/cerif/frapo/hasHonorificSuffix>
        a       <http://www.w3.org/2002/07/owl#DatatypeProperty> ;
        <http://www.w3.org/2000/01/rdf-schema#comment>
                "The letters that should be displayed after a person's name to indicate qualification, membership or fellowship in a professional society, honours or elite status, e.g. MRCVS, FRCS, FRS, OBE, Kt."@en ;
        <http://www.w3.org/2000/01/rdf-schema#label>
                "post-nominals"@en ;
        <http://www.w3.org/2000/01/rdf-schema#subPropertyOf>
                <http://purl.org/cerif/frapo/hasNameSuffix> .

<http://xmlns.com/foaf/0.1/firstName>
        a       <http://www.w3.org/2002/07/owl#DatatypeProperty> , <http://www.w3.org/2002/07/owl#AnnotationProperty> ;
        <http://www.w3.org/2000/01/rdf-schema#subPropertyOf>
                <http://purl.org/cerif/frapo/hasPersonalInformation> .

<http://purl.org/cerif/frapo/feeOrFree>
        a       <http://www.w3.org/2002/07/owl#DatatypeProperty> ;
        <http://www.w3.org/2000/01/rdf-schema#comment>
                "A data property defining whether participation in an event is free, or requires payment of a fee."@en ;
        <http://www.w3.org/2000/01/rdf-schema#label>
                "fee or free"@en .

<http://purl.org/cerif/frapo/isOutputOf>
        a       <http://www.w3.org/2002/07/owl#ObjectProperty> ;
        <http://www.w3.org/2000/01/rdf-schema#comment>
                "An object property linking something that is created or produced to the activity that created or produced it."@en ;
        <http://www.w3.org/2000/01/rdf-schema#label>
                "is output of"@en ;
        <http://purl.org/dc/elements/1.1/description>
                "Domain and range constraints have been removed from this object property to permit it to be used in unforeseen ways."@en .

<http://purl.org/cerif/frapo/hasCurrencyCode>
        a       <http://www.w3.org/2002/07/owl#DatatypeProperty> ;
        <http://www.w3.org/2000/01/rdf-schema#comment>
                "A data property specifying the three-letter currency code used to identify a currency, as defined by ISO 4217 (e.g. EUR or GBP) (see http://en.wikipedia.org/wiki/ISO_4217).  \n\nNot to be confused with the symbol used with numbers to denote an amount of money in a particular currency (e.g.€500; £3.40)"@en ;
        <http://www.w3.org/2000/01/rdf-schema#label>
                "has currency code"@en ;
        <http://www.w3.org/2000/01/rdf-schema#subPropertyOf>
                <http://purl.org/cerif/frapo/hasCode> .

<http://purl.org/cerif/frapo/BudgetInformation>
        a       <http://www.w3.org/2002/07/owl#Class> ;
        <http://www.w3.org/2000/01/rdf-schema#comment>
                "Information about an aspect of a budget."@en ;
        <http://www.w3.org/2000/01/rdf-schema#label>
                "budget information"@en ;
        <http://www.w3.org/2000/01/rdf-schema#subClassOf>
                <http://purl.org/cerif/frapo/FinancialEntity> .

<http://purl.org/cerif/frapo/hasModelNumber>
        a       <http://www.w3.org/2002/07/owl#DatatypeProperty> ;
        <http://www.w3.org/2000/01/rdf-schema#comment>
                "A data property linking something, for example a piece of equipment, to its model number."@en ;
        <http://www.w3.org/2000/01/rdf-schema#label>
                "has model number"@en ;
        <http://www.w3.org/2000/01/rdf-schema#subPropertyOf>
                <http://purl.org/dc/terms/identifier> .

<http://purl.org/cerif/frapo/Fellowship>
        a       <http://www.w3.org/2002/07/owl#Class> ;
        <http://www.w3.org/2000/01/rdf-schema#comment>
                "The stipend paid to a fellow in a college or university."@en ;
        <http://www.w3.org/2000/01/rdf-schema#label>
                "fellowship"@en ;
        <http://www.w3.org/2000/01/rdf-schema#subClassOf>
                <http://purl.org/cerif/frapo/Stipend> .

<http://purl.org/cerif/frapo/University>
        a       <http://www.w3.org/2002/07/owl#Class> ;
        <http://www.w3.org/2000/01/rdf-schema#comment>
                "A university at which higher education and research is conducted."@en ;
        <http://www.w3.org/2000/01/rdf-schema#label>
                "university"@en ;
        <http://www.w3.org/2000/01/rdf-schema#subClassOf>
                <http://xmlns.com/foaf/0.1/Organization> .

<http://purl.org/cerif/frapo/hasDecisionDate>
        a       <http://www.w3.org/2002/07/owl#DatatypeProperty> , <http://www.w3.org/2002/07/owl#FunctionalProperty> ;
        <http://www.w3.org/2000/01/rdf-schema#comment>
                "The date on which a particular action is or will be decided upon, or when an application, such as a grant application, is or will be approved or rejected. [See also frapo:hasAwardDate.]"@en ;
        <http://www.w3.org/2000/01/rdf-schema#label>
                "has decision date"@en ;
        <http://www.w3.org/2000/01/rdf-schema#range>
                <http://www.w3.org/2001/XMLSchema#dateTime> ;
        <http://www.w3.org/2000/01/rdf-schema#seeAlso>
                <http://purl.org/spar/fabio/hasDecisionDate> ;
        <http://www.w3.org/2000/01/rdf-schema#subPropertyOf>
                <http://purl.org/dc/terms/date> ;
        <http://purl.org/dc/elements/1.1/description>
                "This same data property appears in FaBiO, the FRBR-aligned Bibliographic Ontology (http://purl.org/spar/fabio/)."@en .

<http://purl.org/cerif/frapo/hasBirthDate>
        a       <http://www.w3.org/2002/07/owl#DatatypeProperty> ;
        <http://www.w3.org/2000/01/rdf-schema#comment>
                "A data property permitting specification of the birth date of a person."@en ;
        <http://www.w3.org/2000/01/rdf-schema#domain>
                <http://xmlns.com/foaf/0.1/Person> ;
        <http://www.w3.org/2000/01/rdf-schema#label>
                "has birth date"@en ;
        <http://www.w3.org/2000/01/rdf-schema#range>
                <http://www.w3.org/2001/XMLSchema#dateTime> ;
        <http://www.w3.org/2000/01/rdf-schema#subPropertyOf>
                <http://xmlns.com/foaf/0.1/birthday> .

<http://purl.org/cerif/frapo/Contract>
        a       <http://www.w3.org/2002/07/owl#Class> ;
        <http://www.w3.org/2000/01/rdf-schema#comment>
                "A legally binding agreement between parties."@en ;
        <http://www.w3.org/2000/01/rdf-schema#label>
                "contract"@en ;
        <http://www.w3.org/2000/01/rdf-schema#subClassOf>
                <http://purl.org/cerif/frapo/FinancialEntity> .

<http://purl.org/dc/terms/identifier>
        a       <http://www.w3.org/2002/07/owl#DatatypeProperty> ;
        <http://www.w3.org/2000/01/rdf-schema#comment>
                "A unique and unambiguous reference to the resource within a given context.\n\nRecommended best practice is to identify the resource by means of a string conforming to a formal identification system."@en ;
        <http://www.w3.org/2000/01/rdf-schema#label>
                "identifier"@en .

<http://purl.org/cerif/frapo/ConferenceFee>
        a       <http://www.w3.org/2002/07/owl#Class> ;
        <http://www.w3.org/2000/01/rdf-schema#comment>
                "A fee paid to attend a conference."@en ;
        <http://www.w3.org/2000/01/rdf-schema#label>
                "conference fee"@en ;
        <http://www.w3.org/2000/01/rdf-schema#subClassOf>
                <http://purl.org/cerif/frapo/Fee> .

<http://purl.org/cerif/frapo/supplies>
        a       <http://www.w3.org/2002/07/owl#ObjectProperty> ;
        <http://www.w3.org/2000/01/rdf-schema#comment>
                "An object property relating a supplier to a supplied entity, or to an agent to whom the entity is supplied."@en ;
        <http://www.w3.org/2000/01/rdf-schema#domain>
                <http://xmlns.com/foaf/0.1/Agent> ;
        <http://www.w3.org/2000/01/rdf-schema#label>
                "supplies"@en ;
        <http://purl.org/dc/elements/1.1/description>
                "Domain constraints on this object property have been relaxed to permit it to be used in unforeseen ways."@en .

<http://purl.org/cerif/frapo/AvailableFunds>
        a       <http://www.w3.org/2002/07/owl#Class> ;
        <http://www.w3.org/2000/01/rdf-schema#comment>
                "The amount available to spend in a budget category, equalling the income minus the expenditure to date plus future expenditure commitments. "@en ;
        <http://www.w3.org/2000/01/rdf-schema#label>
                "available funds"@en ;
        <http://www.w3.org/2000/01/rdf-schema#subClassOf>
                <http://purl.org/cerif/frapo/BudgetInformation> .

<http://purl.org/cerif/frapo/Supplier>
        a       <http://www.w3.org/2002/07/owl#Class> ;
        <http://www.w3.org/2000/01/rdf-schema#comment>
                "An agent who supplies something, such as goods or services."@en ;
        <http://www.w3.org/2000/01/rdf-schema#label>
                "supplier"@en ;
        <http://www.w3.org/2000/01/rdf-schema#subClassOf>
                <http://xmlns.com/foaf/0.1/Agent> .

<http://purl.org/cerif/frapo/Gift>
        a       <http://www.w3.org/2002/07/owl#Class> ;
        <http://www.w3.org/2000/01/rdf-schema#comment>
                "A gift, donation, benefaction or legacy, typically of money."@en ;
        <http://www.w3.org/2000/01/rdf-schema#label>
                "gift"@en ;
        <http://www.w3.org/2000/01/rdf-schema#subClassOf>
                <http://purl.org/cerif/frapo/Funding> .

<http://purl.org/dc/terms/created>
        a       <http://www.w3.org/2002/07/owl#FunctionalProperty> , <http://www.w3.org/2002/07/owl#DatatypeProperty> ;
        <http://www.w3.org/2000/01/rdf-schema#comment>
                "A data property linking something to its date of creation."@en ;
        <http://www.w3.org/2000/01/rdf-schema#label>
                "has creation date"@en ;
        <http://www.w3.org/2000/01/rdf-schema#range>
                <http://www.w3.org/2001/XMLSchema#dateTime> ;
        <http://www.w3.org/2000/01/rdf-schema#subPropertyOf>
                <http://purl.org/dc/terms/date> .

<http://purl.org/cerif/frapo/hasGrantNumber>
        a       <http://www.w3.org/2002/07/owl#DatatypeProperty> ;
        <http://www.w3.org/2000/01/rdf-schema#comment>
                "A data property specifying the grant number of a grant provided by a funding agency."@en ;
        <http://www.w3.org/2000/01/rdf-schema#domain>
                <http://purl.org/cerif/frapo/Grant> ;
        <http://www.w3.org/2000/01/rdf-schema#label>
                "has grant number"@en ;
        <http://www.w3.org/2000/01/rdf-schema#subPropertyOf>
                <http://purl.org/dc/terms/identifier> .

<http://purl.org/cerif/frapo/hasCompletionDate>
        a       <http://www.w3.org/2002/07/owl#DatatypeProperty> , <http://www.w3.org/2002/07/owl#FunctionalProperty> ;
        <http://www.w3.org/2000/01/rdf-schema#comment>
                "A data property linking something such as a building or a contract to its date of completion."@en ;
        <http://www.w3.org/2000/01/rdf-schema#label>
                "has completion date"@en ;
        <http://www.w3.org/2000/01/rdf-schema#range>
                <http://www.w3.org/2001/XMLSchema#dateTime> ;
        <http://www.w3.org/2000/01/rdf-schema#subPropertyOf>
                <http://purl.org/dc/terms/date> .

<http://purl.org/cerif/frapo/full-economic-costs>
        a       <http://www.w3.org/2002/07/owl#NamedIndividual> , <http://purl.org/cerif/frapo/BudgetCategory> ;
        <http://www.w3.org/2000/01/rdf-schema#comment>
                "A budget category to cover all the direct and indirect costs of a project. "@en ;
        <http://www.w3.org/2000/01/rdf-schema#label>
                "full economic costs"@en ;
        <http://purl.org/dc/elements/1.1/description>
                "Frequently abbreviated 'FEC'."@en .

<http://purl.org/cerif/frapo/overhead-costs>
        a       <http://www.w3.org/2002/07/owl#NamedIndividual> , <http://purl.org/cerif/frapo/BudgetCategory> ;
        <http://www.w3.org/2000/01/rdf-schema#comment>
                "A budget category to cover all the non-directly incurred costs of a project, including estates costs and indirect costs, that enable an institution to host an externally-funded project. "@en ;
        <http://www.w3.org/2000/01/rdf-schema#label>
                "overhead costs"@en .

<http://purl.org/cerif/frapo/SME>
        a       <http://www.w3.org/2002/07/owl#Class> ;
        <http://www.w3.org/2000/01/rdf-schema#comment>
                "A small to medium enterprise, having up to 250 employees."@en ;
        <http://www.w3.org/2000/01/rdf-schema#label>
                "sme"@en , "small to medium enterprise"@en ;
        <http://www.w3.org/2000/01/rdf-schema#subClassOf>
                <http://purl.org/cerif/frapo/Company> .

<http://purl.org/cerif/frapo/hasPurchaseOrderNumber>
        a       <http://www.w3.org/2002/07/owl#DatatypeProperty> ;
        <http://www.w3.org/2000/01/rdf-schema#comment>
                "A data property identifying an official purchase order issued by a purchasing agent to a supplier of goods or services, and used by the supplier to identify the order when delivering goods or submitting an invoice."@en ;
        <http://www.w3.org/2000/01/rdf-schema#domain>
                <http://purl.org/cerif/frapo/PurchaseOrder> ;
        <http://www.w3.org/2000/01/rdf-schema#label>
                "has purchase order number"@en ;
        <http://www.w3.org/2000/01/rdf-schema#subPropertyOf>
                <http://purl.org/dc/terms/identifier> .

<http://purl.org/cerif/frapo/hasCountryCode>
        a       <http://www.w3.org/2002/07/owl#DatatypeProperty> ;
        <http://www.w3.org/2000/01/rdf-schema#comment>
                "A data property specifying the two-letter or three-letter upper-case country code used to identify a country (e.g. FR/FRA for France, DE/DEU for Germany) (see http://countrycode.org/)."@en ;
        <http://www.w3.org/2000/01/rdf-schema#label>
                "has country code"@en ;
        <http://www.w3.org/2000/01/rdf-schema#subPropertyOf>
                <http://purl.org/cerif/frapo/hasCode> .

<http://purl.org/cerif/frapo/funds>
        a       <http://www.w3.org/2002/07/owl#ObjectProperty> ;
        <http://www.w3.org/2000/01/rdf-schema#comment>
                "An object property that links a grant to something that it funds (i.e. that it finances or pays for), or that links an agent providing funding to something that it funds.  This flexibility is given because of alternative usages of the English word 'funds'.  [See also frapo:awards and frapo:supports.]"@en ;
        <http://www.w3.org/2000/01/rdf-schema#label>
                "funds"@en ;
        <http://www.w3.org/2000/01/rdf-schema#subPropertyOf>
                <http://purl.org/cerif/frapo/supports> ;
        <http://www.w3.org/2002/07/owl#inverseOf>
                <http://purl.org/cerif/frapo/isFundedBy> .

<http://purl.org/cerif/frapo/hasOrganizationalInformation>
        a       <http://www.w3.org/2002/07/owl#DatatypeProperty> ;
        <http://www.w3.org/2000/01/rdf-schema#comment>
                "It describes information about the organization."@en ;
        <http://www.w3.org/2000/01/rdf-schema#domain>
                <http://xmlns.com/foaf/0.1/Organization> ;
        <http://www.w3.org/2000/01/rdf-schema#label>
                "has organizational information"@en ;
        <http://www.w3.org/2000/01/rdf-schema#subPropertyOf>
                <http://purl.org/cerif/frapo/hasAgentInformation> .

<http://purl.org/cerif/frapo/ExpenditureToDate>
        a       <http://www.w3.org/2002/07/owl#Class> ;
        <http://www.w3.org/2000/01/rdf-schema#comment>
                "Total money expended to date from an an account, or from a particular budget category."@en ;
        <http://www.w3.org/2000/01/rdf-schema#label>
                "expenditure to date"@en ;
        <http://www.w3.org/2000/01/rdf-schema#subClassOf>
                <http://purl.org/cerif/frapo/Expenditure> .

<http://purl.org/cerif/frapo/isFundingAgencyFor>
        a       <http://www.w3.org/2002/07/owl#ObjectProperty> ;
        <http://www.w3.org/2000/01/rdf-schema#comment>
                "An object property linking a funding agency to an entity for which it provides funding."@en ;
        <http://www.w3.org/2000/01/rdf-schema#domain>
                <http://purl.org/cerif/frapo/FundingAgency> ;
        <http://www.w3.org/2000/01/rdf-schema#label>
                "is funding agency for"@en ;
        <http://www.w3.org/2000/01/rdf-schema#subPropertyOf>
                <http://purl.org/cerif/frapo/supports> .

<http://purl.org/cerif/frapo/unfunded>
        a       <http://purl.org/cerif/frapo/Status> , <http://www.w3.org/2002/07/owl#NamedIndividual> ;
        <http://www.w3.org/2000/01/rdf-schema#comment>
                "The status of something such as an investigation or a project as being unfunded."@en ;
        <http://www.w3.org/2000/01/rdf-schema#label>
                "unfunded"@en .

<http://purl.org/cerif/frapo/hasPersonalIdentifier>
        a       <http://www.w3.org/2002/07/owl#DatatypeProperty> ;
        <http://www.w3.org/2000/01/rdf-schema#comment>
                "A unique and unambiguous identifier for an individual person within a given context."@en ;
        <http://www.w3.org/2000/01/rdf-schema#domain>
                <http://xmlns.com/foaf/0.1/Person> ;
        <http://www.w3.org/2000/01/rdf-schema#label>
                "has personal identifier"@en ;
        <http://www.w3.org/2000/01/rdf-schema#subPropertyOf>
                <http://purl.org/cerif/frapo/hasPersonalInformation> , <http://purl.org/dc/terms/identifier> ;
        <http://purl.org/dc/elements/1.1/description>
                "owl:equivalentProperty <http://purl.org/spar/scoro/hasPersonalIdentifier> ."@en , "owl:equivalentProperty <http://purl.org/spar/datacite/hasPersonalIdentifier> ." .

<http://purl.org/cerif/frapo/purchases>
        a       <http://www.w3.org/2002/07/owl#ObjectProperty> ;
        <http://www.w3.org/2000/01/rdf-schema#comment>
                "An object property relating a purchaser to a purchased entity."@en ;
        <http://www.w3.org/2000/01/rdf-schema#domain>
                <http://xmlns.com/foaf/0.1/Agent> ;
        <http://www.w3.org/2000/01/rdf-schema#label>
                "purchases"@en ;
        <http://purl.org/dc/elements/1.1/description>
                "Range constraints have been removed from this object property to permit it to be used in unforeseen ways."@en .

<http://purl.org/cerif/frapo/directly-incurred-costs>
        a       <http://www.w3.org/2002/07/owl#NamedIndividual> , <http://purl.org/cerif/frapo/BudgetCategory> ;
        <http://www.w3.org/2000/01/rdf-schema#comment>
                "A budget category to cover all costs directly incurred because of a legitimate expenditure on a project, for example the purchase of reagents or the employment of a post-doctoral researcher."@en ;
        <http://www.w3.org/2000/01/rdf-schema#label>
                "directly incurred costs"@en ;
        <http://purl.org/dc/elements/1.1/description>
                "Also known as the 'direct costs' of the project."@en .

<http://xmlns.com/foaf/0.1/birthday>
        a       <http://www.w3.org/2002/07/owl#DatatypeProperty> ;
        <http://www.w3.org/2000/01/rdf-schema#range>
                <http://www.w3.org/2001/XMLSchema#date> ;
        <http://www.w3.org/2000/01/rdf-schema#subPropertyOf>
                <http://purl.org/dc/terms/date> .

<http://purl.org/cerif/frapo/academic>
        a       <http://www.w3.org/2002/07/owl#NamedIndividual> , <http://xmlns.com/foaf/0.1/Person> ;
        <http://www.w3.org/2000/01/rdf-schema#comment>
                "A member of the academic staff of an academic institution such as a university."@en ;
        <http://www.w3.org/2000/01/rdf-schema#label>
                "academic"@en .

<http://purl.org/cerif/frapo/Equipment>
        a       <http://www.w3.org/2002/07/owl#Class> ;
        <http://www.w3.org/2000/01/rdf-schema#comment>
                "An item of equipment or apparatus, or a laboratory instrument, for example a refrigerated centrifuge."@en ;
        <http://www.w3.org/2000/01/rdf-schema#label>
                "equipment"@en ;
        <http://www.w3.org/2000/01/rdf-schema#subClassOf>
                <http://purl.org/cerif/frapo/InfrastructureEntity> .

<http://purl.org/cerif/frapo/hasQualification>
        a       <http://www.w3.org/2002/07/owl#DatatypeProperty> ;
        <http://www.w3.org/2000/01/rdf-schema#comment>
                "A data property permitting specification of the qualification held by a person."@en ;
        <http://www.w3.org/2000/01/rdf-schema#label>
                "has qualification"@en ;
        <http://www.w3.org/2000/01/rdf-schema#subPropertyOf>
                <http://purl.org/cerif/frapo/hasPersonalInformation> .

<http://purl.org/cerif/frapo/hasApplicationOutcome>
        a       <http://www.w3.org/2002/07/owl#DatatypeProperty> ;
        <http://www.w3.org/2000/01/rdf-schema#comment>
                "A data property that permits the outcome of an application to be described, for example that a job has been offered or that a grant has been awarded."@en ;
        <http://www.w3.org/2000/01/rdf-schema#label>
                "has application outcome"@en ;
        <http://www.w3.org/2000/01/rdf-schema#subPropertyOf>
                <http://www.w3.org/2002/07/owl#topDataProperty> .

<http://purl.org/cerif/frapo/hasFaxNumber>
        a       <http://www.w3.org/2002/07/owl#DatatypeProperty> ;
        <http://www.w3.org/2000/01/rdf-schema#comment>
                "A data property identifying a Fax number for an agent."@en ;
        <http://www.w3.org/2000/01/rdf-schema#label>
                "has fax number"@en ;
        <http://www.w3.org/2000/01/rdf-schema#subPropertyOf>
                <http://purl.org/cerif/frapo/hasAgentInformation> .

<http://purl.org/cerif/frapo/indirect-costs>
        a       <http://purl.org/cerif/frapo/BudgetCategory> , <http://www.w3.org/2002/07/owl#NamedIndividual> ;
        <http://www.w3.org/2000/01/rdf-schema#comment>
                "A budget category to cover the indirect costs of running a project, for example heating and lighting, and the employment of non-project staff including administrators, accountants and cleaners."@en ;
        <http://www.w3.org/2000/01/rdf-schema#label>
                "indirect costs"@en .

<http://purl.org/cerif/frapo/hasPhoneNumber>
        a       <http://www.w3.org/2002/07/owl#DatatypeProperty> ;
        <http://www.w3.org/2000/01/rdf-schema#comment>
                "A data property identifying a telephone number for an agent."@en ;
        <http://www.w3.org/2000/01/rdf-schema#label>
                "has phone number"@en ;
        <http://www.w3.org/2000/01/rdf-schema#subPropertyOf>
                <http://purl.org/cerif/frapo/hasAgentInformation> .

<http://purl.org/cerif/frapo/software-costs>
        a       <http://www.w3.org/2002/07/owl#NamedIndividual> , <http://purl.org/cerif/frapo/BudgetCategory> ;
        <http://www.w3.org/2000/01/rdf-schema#comment>
                "A budget category to cover the costs of software licenses required by a project."@en ;
        <http://www.w3.org/2000/01/rdf-schema#label>
                "software costs"@en .

<http://purl.org/cerif/frapo/donates>
        a       <http://www.w3.org/2002/07/owl#ObjectProperty> ;
        <http://www.w3.org/2000/01/rdf-schema#comment>
                "An object property linking a benefactor to a gift."@en ;
        <http://www.w3.org/2000/01/rdf-schema#domain>
                <http://xmlns.com/foaf/0.1/Agent> ;
        <http://www.w3.org/2000/01/rdf-schema#label>
                "donates"@en ;
        <http://purl.org/dc/elements/1.1/description>
                "Range constraints have been removed from this object property to permit it to be used in unforeseen ways."@en ;
        <http://www.w3.org/2002/07/owl#inverseOf>
                <http://purl.org/cerif/frapo/isDonatedBy> .

<http://purl.org/cerif/frapo/Laboratory>
        a       <http://www.w3.org/2002/07/owl#Class> ;
        <http://www.w3.org/2000/01/rdf-schema#comment>
                "A facility in which research can be conducted."@en ;
        <http://www.w3.org/2000/01/rdf-schema#label>
                "laboratory"@en ;
        <http://www.w3.org/2000/01/rdf-schema#subClassOf>
                <http://purl.org/cerif/frapo/Facility> .

<http://purl.org/cerif/frapo/entrepreneur>
        a       <http://xmlns.com/foaf/0.1/Person> , <http://www.w3.org/2002/07/owl#NamedIndividual> ;
        <http://www.w3.org/2000/01/rdf-schema#comment>
                "A person who invests in novel enterprises."@en ;
        <http://www.w3.org/2000/01/rdf-schema#label>
                "entrepreneur"@en .

<http://purl.org/cerif/frapo/initial>
        a       <http://www.w3.org/2002/07/owl#DatatypeProperty> ;
        <http://www.w3.org/2000/01/rdf-schema#comment>
                "A data property permitting specification of the initial(s) of a person's name."@en ;
        <http://www.w3.org/2000/01/rdf-schema#label>
                "initials"@en ;
        <http://www.w3.org/2000/01/rdf-schema#subPropertyOf>
                <http://purl.org/cerif/frapo/hasPersonalInformation> .

<http://purl.org/cerif/frapo/hasMonetaryValue>
        a       <http://www.w3.org/2002/07/owl#DatatypeProperty> ;
        <http://www.w3.org/2000/01/rdf-schema#comment>
                "A data property enabling one to specify the monetary value of a financial entity such as a grant, a gift or a budget category.  Use in conjuction with frapo:hasCurrency."@en ;
        <http://www.w3.org/2000/01/rdf-schema#label>
                "has value"@en .

<http://purl.org/cerif/frapo/ScholarshipApplication>
        a       <http://www.w3.org/2002/07/owl#Class> ;
        <http://www.w3.org/2000/01/rdf-schema#comment>
                "The activity of applying for an educational scholarship."@en ;
        <http://www.w3.org/2000/01/rdf-schema#label>
                "scholarship application"@en ;
        <http://www.w3.org/2000/01/rdf-schema#subClassOf>
                <http://purl.org/cerif/frapo/Application> .

<http://purl.org/cerif/frapo/Subscription>
        a       <http://www.w3.org/2002/07/owl#Class> ;
        <http://www.w3.org/2000/01/rdf-schema#comment>
                "Payment, commonly made annually, to obtain access to something on a periodic or continuing basis, such as a journal."@en ;
        <http://www.w3.org/2000/01/rdf-schema#label>
                "subscription"@en ;
        <http://www.w3.org/2000/01/rdf-schema#subClassOf>
                <http://purl.org/cerif/frapo/Fee> .

<http://purl.org/cerif/frapo/EmploymentContract>
        a       <http://www.w3.org/2002/07/owl#Class> ;
        <http://www.w3.org/2000/01/rdf-schema#comment>
                "A contract of employment between a person and an organization."@en ;
        <http://www.w3.org/2000/01/rdf-schema#label>
                "employment contract"@en ;
        <http://www.w3.org/2000/01/rdf-schema#subClassOf>
                <http://purl.org/cerif/frapo/Contract> .

<http://www.w3.org/2000/01/rdf-schema#comment>
        a       <http://www.w3.org/2002/07/owl#AnnotationProperty> .

<http://purl.org/cerif/frapo/Library>
        a       <http://www.w3.org/2002/07/owl#Class> ;
        <http://www.w3.org/2000/01/rdf-schema#comment>
                "A facility in which printed documents (for example books and journals) are deposited for long-term preservation and access."@en ;
        <http://www.w3.org/2000/01/rdf-schema#label>
                "library"@en ;
        <http://www.w3.org/2000/01/rdf-schema#subClassOf>
                <http://purl.org/cerif/frapo/Repository> .

<http://purl.org/cerif/frapo/ServiceContractFee>
        a       <http://www.w3.org/2002/07/owl#Class> ;
        <http://www.w3.org/2000/01/rdf-schema#comment>
                "A fee paid periodically, typically annually, to obtain access when required to a service such as an equipment maintenance contract.\""@en ;
        <http://www.w3.org/2000/01/rdf-schema#label>
                "service contract fee"@en ;
        <http://www.w3.org/2000/01/rdf-schema#subClassOf>
                <http://purl.org/cerif/frapo/Fee> .

<http://purl.org/cerif/frapo/hasSerialNumber>
        a       <http://www.w3.org/2002/07/owl#DatatypeProperty> ;
        <http://www.w3.org/2000/01/rdf-schema#comment>
                "A data property linking something, for example a piece of equipment, to its serial number."@en ;
        <http://www.w3.org/2000/01/rdf-schema#label>
                "has serial number"@en ;
        <http://www.w3.org/2000/01/rdf-schema#subPropertyOf>
                <http://purl.org/dc/terms/identifier> .

<http://purl.org/cerif/frapo/hasSupplierNumber>
        a       <http://www.w3.org/2002/07/owl#DatatypeProperty> ;
        <http://www.w3.org/2000/01/rdf-schema#comment>
                "A data property linking a supplier to an identifying number for that supplier, typically used by the accounting system of the purchasing institution when placing and tracking orders."@en ;
        <http://www.w3.org/2000/01/rdf-schema#domain>
                <http://purl.org/cerif/frapo/Supplier> ;
        <http://www.w3.org/2000/01/rdf-schema#label>
                "has supplier number"@en ;
        <http://www.w3.org/2000/01/rdf-schema#subPropertyOf>
                <http://purl.org/dc/terms/identifier> .

<http://purl.org/dc/elements/1.1/rights>
        a       <http://www.w3.org/2002/07/owl#AnnotationProperty> .

<http://purl.org/cerif/frapo/hasExpertise>
        a       <http://www.w3.org/2002/07/owl#DatatypeProperty> ;
        <http://www.w3.org/2000/01/rdf-schema#comment>
                "A data property identifying the area(s) of expertise and skills posessed by an individual or an organization."@en ;
        <http://www.w3.org/2000/01/rdf-schema#label>
                "has expertise"@en ;
        <http://www.w3.org/2000/01/rdf-schema#subPropertyOf>
                <http://purl.org/cerif/frapo/hasAgentInformation> .

<http://purl.org/cerif/frapo/AccountStatement>
        a       <http://www.w3.org/2002/07/owl#Class> ;
        <http://www.w3.org/2000/01/rdf-schema#comment>
                "A statement of income and expenditure for an account, typically presented as dated income receipts and outgoings against categories in a budget for that account."@en ;
        <http://www.w3.org/2000/01/rdf-schema#label>
                "account statement"@en ;
        <http://www.w3.org/2000/01/rdf-schema#subClassOf>
                <http://purl.org/cerif/frapo/FinancialEntity> .

<http://purl.org/cerif/frapo/givenNameInitial>
        a       <http://www.w3.org/2002/07/owl#DatatypeProperty> ;
        <http://www.w3.org/2000/01/rdf-schema#comment>
                "A data property permitting specification of the initial(s) of a person's given name(s)."@en ;
        <http://www.w3.org/2000/01/rdf-schema#label>
                "given name initial"@en ;
        <http://www.w3.org/2000/01/rdf-schema#subPropertyOf>
                <http://purl.org/cerif/frapo/initial> .

<http://purl.org/cerif/frapo/hasQuotationDate>
        a       <http://www.w3.org/2002/07/owl#DatatypeProperty> ;
        <http://www.w3.org/2000/01/rdf-schema#comment>
                "A data property linking a quotation to its date."@en ;
        <http://www.w3.org/2000/01/rdf-schema#label>
                "has quotation date"@en ;
        <http://www.w3.org/2000/01/rdf-schema#range>
                <http://www.w3.org/2001/XMLSchema#dateTime> ;
        <http://www.w3.org/2000/01/rdf-schema#subPropertyOf>
                <http://purl.org/dc/terms/date> .

<http://purl.org/cerif/frapo/providesFractionOfTotalFunding>
        a       <http://www.w3.org/2002/07/owl#ObjectProperty> ;
        <http://www.w3.org/2000/01/rdf-schema#comment>
                "An object property linking funding to a budget, specifying what fraction of the total budget is provided by that source of funding."@en ;
        <http://www.w3.org/2000/01/rdf-schema#domain>
                <http://purl.org/cerif/frapo/Funding> ;
        <http://www.w3.org/2000/01/rdf-schema#label>
                "percentage of total funding"@en ;
        <http://www.w3.org/2000/01/rdf-schema#range>
                <http://purl.org/cerif/frapo/Budget> .

<http://purl.org/cerif/frapo/accepted>
        a       <http://purl.org/cerif/frapo/Status> , <http://www.w3.org/2002/07/owl#NamedIndividual> ;
        <http://www.w3.org/2000/01/rdf-schema#comment>
                "The status of something such as an application as having been accepted."@en ;
        <http://www.w3.org/2000/01/rdf-schema#label>
                "accepted"@en .

<http://xmlns.com/foaf/0.1/Document>
        a       <http://www.w3.org/2002/07/owl#Class> ;
        <http://purl.org/dc/elements/1.1/description>
                "Ontology terms and definitions for many documents relevant to FRAPO are given as 'Expression' classes in FaBiO, the FRBR-aligned Bibliographic Ontology, e.g. fabio:CallForApplications, fabio:DataManagementPlan, fabio:GrantApplicationDocument, fabio:ProjectPlan.  Others are given as sub-classes of this class."@en .

<http://purl.org/cerif/frapo/hasMilestone>
        a       <http://www.w3.org/2002/07/owl#DatatypeProperty> ;
        <http://www.w3.org/2000/01/rdf-schema#comment>
                "A data property that permits one to define a significant event (a 'milestone') in the progress of a project."@en ;
        <http://www.w3.org/2000/01/rdf-schema#label>
                "has milestone"@en .

<http://purl.org/cerif/frapo/Stipend>
        a       <http://www.w3.org/2002/07/owl#Class> ;
        <http://www.w3.org/2000/01/rdf-schema#comment>
                "A sum of money allotted on a regular basis, usually for some specific purpose."@en ;
        <http://www.w3.org/2000/01/rdf-schema#label>
                "stipend"@en ;
        <http://www.w3.org/2000/01/rdf-schema#subClassOf>
                <http://purl.org/cerif/frapo/Funding> .

<http://purl.org/cerif/frapo/directly-allocated-costs>
        a       <http://purl.org/cerif/frapo/BudgetCategory> , <http://www.w3.org/2002/07/owl#NamedIndividual> ;
        <http://www.w3.org/2000/01/rdf-schema#comment>
                "A budget category to cover those costs normally borne by an institution, that are assigned to the budget of an externally funded project to cover the value of contributions to that project, for example to pay for the salary of a permanent member of staff seconded to work on the project, to compensate the employing organization for the loss of that person's efforts on other activities that he or she would otherwise be undertaking were it not for that secondment."@en ;
        <http://www.w3.org/2000/01/rdf-schema#label>
                "directly allocated costs"@en .

<http://purl.org/cerif/frapo/ConsultancyAgreement>
        a       <http://www.w3.org/2002/07/owl#Class> ;
        <http://www.w3.org/2000/01/rdf-schema#comment>
                "A contract between an employer and a consultant, detailing the terms of the consultancy."@en ;
        <http://www.w3.org/2000/01/rdf-schema#label>
                "consultancy agreement"@en ;
        <http://www.w3.org/2000/01/rdf-schema#subClassOf>
                <http://purl.org/cerif/frapo/Contract> .

<http://purl.org/cerif/frapo/ResearchInformationSystem>
        a       <http://www.w3.org/2002/07/owl#Class> ;
        <http://www.w3.org/2000/01/rdf-schema#comment>
                "A database containing administrative information about the research undertaken in an institution, and the publications and other outputs from such research."@en ;
        <http://www.w3.org/2000/01/rdf-schema#label>
                "research information system"@en ;
        <http://www.w3.org/2000/01/rdf-schema#subClassOf>
                <http://purl.org/cerif/frapo/ComputationalService> .

<http://purl.org/cerif/frapo/isSubmittedBy>
        a       <http://www.w3.org/2002/07/owl#ObjectProperty> ;
        <http://www.w3.org/2000/01/rdf-schema#comment>
                "An object property linking an entity that is submitted (to some third party) to the agent who submits it."@en ;
        <http://www.w3.org/2000/01/rdf-schema#label>
                "is submitted by"@en ;
        <http://www.w3.org/2000/01/rdf-schema#range>
                <http://xmlns.com/foaf/0.1/Agent> ;
        <http://www.w3.org/2002/07/owl#inverseOf>
                <http://purl.org/cerif/frapo/submits> .

<http://purl.org/cerif/frapo/RegistrationAgency>
        a       <http://www.w3.org/2002/07/owl#Class> ;
        <http://www.w3.org/2000/01/rdf-schema#comment>
                "An institution or organization officially appointed by a Registration Authority that acts to register things. For example, CrossRef is a registration agency for DOIs relating to documents, while DataCite is a registration agency for DOIs relating to datasets, acting for the Registration Authority for DOIs, namely the International DOI Foundation (IDF)."@en ;
        <http://www.w3.org/2000/01/rdf-schema#label>
                "registration agency"@en ;
        <http://www.w3.org/2000/01/rdf-schema#subClassOf>
                <http://xmlns.com/foaf/0.1/Organization> .

<http://www.w3.org/2000/01/rdf-schema#label>
        a       <http://www.w3.org/2002/07/owl#AnnotationProperty> .

<http://purl.org/cerif/frapo/hasCode>
        a       <http://www.w3.org/2002/07/owl#DatatypeProperty> ;
        <http://www.w3.org/2000/01/rdf-schema#comment>
                "A data property defining a code."@en ;
        <http://www.w3.org/2000/01/rdf-schema#label>
                "has code"@en .

<http://purl.org/cerif/frapo/rejected>
        a       <http://purl.org/cerif/frapo/Status> , <http://www.w3.org/2002/07/owl#NamedIndividual> ;
        <http://www.w3.org/2000/01/rdf-schema#comment>
                "The status of something such as an application as having been rejected."@en ;
        <http://www.w3.org/2000/01/rdf-schema#label>
                "rejected"@en .

<http://purl.org/cerif/frapo/purchasesFrom>
        a       <http://www.w3.org/2002/07/owl#ObjectProperty> ;
        <http://www.w3.org/2000/01/rdf-schema#comment>
                "An object property relating a purchaser to a supplier from whom the purchase is made."@en ;
        <http://www.w3.org/2000/01/rdf-schema#domain>
                <http://xmlns.com/foaf/0.1/Agent> ;
        <http://www.w3.org/2000/01/rdf-schema#label>
                "purchases from"@en ;
        <http://www.w3.org/2000/01/rdf-schema#range>
                <http://xmlns.com/foaf/0.1/Agent> ;
        <http://purl.org/dc/elements/1.1/description>
                "Domain and range constraints on this object property have been relaxed to permit it to be used in unforeseen ways."@en ;
        <http://www.w3.org/2002/07/owl#inverseOf>
                <http://purl.org/cerif/frapo/sellsTo> .

<http://purl.org/cerif/frapo/FundingApplication>
        a       <http://www.w3.org/2002/07/owl#Class> ;
        <http://www.w3.org/2000/01/rdf-schema#comment>
                "The activity of applying for funding."@en ;
        <http://www.w3.org/2000/01/rdf-schema#label>
                "funding application"@en ;
        <http://www.w3.org/2000/01/rdf-schema#subClassOf>
                <http://purl.org/cerif/frapo/Application> ;
        <http://purl.org/dc/elements/1.1/description>
                "For the documents supporting a funding application, use fabio:GrantApplicationDocument and fabio:CaseForSupportDocument."@en .

<http://purl.org/cerif/frapo/Business_angel>
        a       <http://www.w3.org/2002/07/owl#AnnotationProperty> ;
        <http://www.w3.org/2000/01/rdf-schema#subPropertyOf>
                <http://www.w3.org/2000/01/rdf-schema#label> .

<http://purl.org/cerif/frapo/PostalAddress>
        a       <http://www.w3.org/2002/07/owl#Class> ;
        <http://www.w3.org/2000/01/rdf-schema#comment>
                "A postal address."@en ;
        <http://www.w3.org/2000/01/rdf-schema#label>
                "postal address"@en ;
        <http://www.w3.org/2000/01/rdf-schema#subClassOf>
                <http://www.w3.org/2002/07/owl#Thing> .

<http://purl.org/cerif/frapo/usesEquipment>
        a       <http://www.w3.org/2002/07/owl#ObjectProperty> ;
        <http://www.w3.org/2000/01/rdf-schema#comment>
                "An object property linking an activity such as an expedition, a research project or an investigation, to an item of equipment employed in that activity."@en ;
        <http://www.w3.org/2000/01/rdf-schema#label>
                "uses equipment"@en ;
        <http://www.w3.org/2000/01/rdf-schema#range>
                <http://purl.org/cerif/frapo/Equipment> ;
        <http://www.w3.org/2000/01/rdf-schema#subPropertyOf>
                <http://www.w3.org/2002/07/owl#topObjectProperty> ;
        <http://purl.org/dc/elements/1.1/description>
                "Domain constraints have been removed from this object property to permit it to be used in unforeseen ways."@en .

<http://purl.org/cerif/frapo/hasDegreeSuffix>
        a       <http://www.w3.org/2002/07/owl#DatatypeProperty> ;
        <http://www.w3.org/2000/01/rdf-schema#comment>
                "The letters that should be displayed after a person's name to indicate an academic degree, e.g. BA, BVSc, PhD, DSc."@en ;
        <http://www.w3.org/2000/01/rdf-schema#label>
                "has degrees"@en ;
        <http://www.w3.org/2000/01/rdf-schema#subPropertyOf>
                <http://purl.org/cerif/frapo/hasNameSuffix> .

<http://purl.org/cerif/frapo/hasCurriculumVitae>
        a       <http://www.w3.org/2002/07/owl#ObjectProperty> ;
        <http://www.w3.org/2000/01/rdf-schema#comment>
                "An object property linking a person to an on-line version of that person's curriculum vitae."@en ;
        <http://www.w3.org/2000/01/rdf-schema#domain>
                <http://xmlns.com/foaf/0.1/Person> ;
        <http://www.w3.org/2000/01/rdf-schema#label>
                "has curriculum vitae"@en ;
        <http://www.w3.org/2000/01/rdf-schema#range>
                <http://xmlns.com/foaf/0.1/Document> .

<http://purl.org/cerif/frapo/EmploymentApplication>
        a       <http://www.w3.org/2002/07/owl#Class> ;
        <http://www.w3.org/2000/01/rdf-schema#comment>
                "The activity of applying for a job."@en ;
        <http://www.w3.org/2000/01/rdf-schema#label>
                "employment application"@en ;
        <http://www.w3.org/2000/01/rdf-schema#subClassOf>
                <http://purl.org/cerif/frapo/Application> .

<http://purl.org/cerif/frapo/non-staff-costs>
        a       <http://purl.org/cerif/frapo/BudgetCategory> , <http://www.w3.org/2002/07/owl#NamedIndividual> ;
        <http://www.w3.org/2000/01/rdf-schema#comment>
                "A budget category to cover all the costs associated with a project that do not involve the employment of staff by the institution, thus, for example, including consumables purchase, travel costs and consultancy fees, but excluding the salary, estates and indirect costs associated with the allocation of the PI's time to the project and the direct employment of a project manager."@en ;
        <http://www.w3.org/2000/01/rdf-schema#label>
                "non-staff costs"@en .

<http://purl.org/cerif/frapo/isPurchasedBy>
        a       <http://www.w3.org/2002/07/owl#ObjectProperty> ;
        <http://www.w3.org/2000/01/rdf-schema#comment>
                "An object property relating a purchased entity to its purchaser."@en ;
        <http://www.w3.org/2000/01/rdf-schema#label>
                "was purchased by"@en ;
        <http://www.w3.org/2000/01/rdf-schema#range>
                <http://xmlns.com/foaf/0.1/Agent> ;
        <http://purl.org/dc/elements/1.1/description>
                "Domain constraints have been removed from this object property to permit it to be used in unforeseen ways."@en ;
        <http://www.w3.org/2002/07/owl#inverseOf>
                <http://purl.org/cerif/frapo/purchases> .

<http://purl.org/cerif/frapo/facilities-costs>
        a       <http://www.w3.org/2002/07/owl#NamedIndividual> , <http://purl.org/cerif/frapo/BudgetCategory> ;
        <http://www.w3.org/2000/01/rdf-schema#comment>
                "A budget category to cover the costs of maintaining facilities used by a project, for example an electron microscopy facility."@en ;
        <http://www.w3.org/2000/01/rdf-schema#label>
                "facilities costs"@en .

<http://purl.org/cerif/frapo/contributions-in-kind>
        a       <http://www.w3.org/2002/07/owl#NamedIndividual> , <http://purl.org/cerif/frapo/BudgetCategory> ;
        <http://www.w3.org/2000/01/rdf-schema#comment>
                "A budget category to categorize the financial worth of contributions in kind (e.g. staff effort, access to facilities, sharing of know-how) given to a project by an agent, for example by the host institution or by a commerical partner in an academic project. "@en ;
        <http://www.w3.org/2000/01/rdf-schema#label>
                "contributions in kind"@en .

<http://xmlns.com/foaf/0.1/givenname>
        a       <http://www.w3.org/2002/07/owl#DatatypeProperty> , <http://www.w3.org/2002/07/owl#AnnotationProperty> ;
        <http://www.w3.org/2000/01/rdf-schema#subPropertyOf>
                <http://purl.org/cerif/frapo/hasPersonalInformation> .

<http://purl.org/cerif/frapo/hasPostalAddress>
        a       <http://www.w3.org/2002/07/owl#DatatypeProperty> ;
        <http://www.w3.org/2000/01/rdf-schema#comment>
                "A data property identifying a postal address for an agent."@en ;
        <http://www.w3.org/2000/01/rdf-schema#label>
                "has postal address"@en ;
        <http://www.w3.org/2000/01/rdf-schema#subPropertyOf>
                <http://purl.org/cerif/frapo/hasAgentInformation> .

<http://purl.org/cerif/frapo/hasLocation>
        a       <http://www.w3.org/2002/07/owl#DatatypeProperty> ;
        <http://www.w3.org/2000/01/rdf-schema#comment>
                "A data property link an entity to a relevant location, which might be geographical (e.g. New York City) or local (e.g. Freezer B, second shelf)."@en ;
        <http://www.w3.org/2000/01/rdf-schema#label>
                "has location"@en .

<http://purl.org/cerif/frapo/FinancialEntity>
        a       <http://www.w3.org/2002/07/owl#Class> ;
        <http://www.w3.org/2000/01/rdf-schema#comment>
                "An entity primarily to do with money."@en ;
        <http://www.w3.org/2000/01/rdf-schema#label>
                "financial entity"@en ;
        <http://www.w3.org/2000/01/rdf-schema#subClassOf>
                <http://www.w3.org/2002/07/owl#Thing> .

<http://purl.org/cerif/frapo/hasDeliveryDate>
        a       <http://www.w3.org/2002/07/owl#DatatypeProperty> ;
        <http://www.w3.org/2000/01/rdf-schema#comment>
                "The date on which something is delivered, or is due to be delivered."@en ;
        <http://www.w3.org/2000/01/rdf-schema#label>
                "has delivery date"@en ;
        <http://www.w3.org/2000/01/rdf-schema#range>
                <http://www.w3.org/2001/XMLSchema#dateTime> ;
        <http://www.w3.org/2000/01/rdf-schema#subPropertyOf>
                <http://purl.org/dc/terms/date> .

<http://purl.org/cerif/frapo/service-costs>
        a       <http://purl.org/cerif/frapo/BudgetCategory> , <http://www.w3.org/2002/07/owl#NamedIndividual> ;
        <http://www.w3.org/2000/01/rdf-schema#comment>
                "A budget category to cover the costs of services used by a project, for example a DNA sequencing service, or an equipment maintenance service."@en ;
        <http://www.w3.org/2000/01/rdf-schema#label>
                "service costs"@en .

<http://purl.org/cerif/frapo/hasExchangeRate>
        a       <http://www.w3.org/2002/07/owl#DatatypeProperty> ;
        <http://www.w3.org/2000/01/rdf-schema#comment>
                "A data property specifying the currency exchange rate between two specified currencies."@en ;
        <http://www.w3.org/2000/01/rdf-schema#label>
                "has exchange rate"@en .

<http://www.w3.org/2006/timezone#TimeZone>
        a       <http://www.w3.org/2002/07/owl#DatatypeProperty> , <http://www.w3.org/2002/07/owl#FunctionalProperty> ;
        <http://www.w3.org/2000/01/rdf-schema#comment>
                "A data property that permits the time zone relating to an entity to be specified."@en ;
        <http://www.w3.org/2000/01/rdf-schema#label>
                "has time zone"@en .

<http://purl.org/cerif/frapo/hasCityOrTown>
        a       <http://www.w3.org/2002/07/owl#DatatypeProperty> ;
        <http://www.w3.org/2000/01/rdf-schema#comment>
                "A data property specifying a city or town, for example as the location of an event."@en ;
        <http://www.w3.org/2000/01/rdf-schema#label>
                "has city or town"@en .

<http://purl.org/cerif/frapo/hasBatchNumber>
        a       <http://www.w3.org/2002/07/owl#DatatypeProperty> ;
        <http://www.w3.org/2000/01/rdf-schema#comment>
                "A data property linking something, for example a chemical or drug, to its manufacturing batch number."@en ;
        <http://www.w3.org/2000/01/rdf-schema#label>
                "has batch number"@en ;
        <http://www.w3.org/2000/01/rdf-schema#subPropertyOf>
                <http://purl.org/dc/terms/identifier> .

<http://purl.org/cerif/frapo/travel-and-subsistence-costs>
        a       <http://www.w3.org/2002/07/owl#NamedIndividual> , <http://purl.org/cerif/frapo/BudgetCategory> ;
        <http://www.w3.org/2000/01/rdf-schema#comment>
                "A budget category to cover the costs of travel and subsistence incurred on behalf of the project."@en ;
        <http://www.w3.org/2000/01/rdf-schema#label>
                "travel and subsistence costs"@en .

<http://purl.org/cerif/frapo/awards>
        a       <http://www.w3.org/2002/07/owl#ObjectProperty> , <http://www.w3.org/2002/07/owl#InverseFunctionalProperty> ;
        <http://www.w3.org/2000/01/rdf-schema#comment>
                "An object property linking an agent to something the agent awards, for example linking a funding agency to a grant, a university to a degree, or an organization to a prize."@en ;
        <http://www.w3.org/2000/01/rdf-schema#domain>
                <http://xmlns.com/foaf/0.1/Agent> ;
        <http://www.w3.org/2000/01/rdf-schema#label>
                "awards"@en ;
        <http://www.w3.org/2002/07/owl#inverseOf>
                <http://purl.org/cerif/frapo/isAwardedBy> .

<http://purl.org/cerif/frapo/Output>
        a       <http://www.w3.org/2002/07/owl#Class> ;
        <http://www.w3.org/2000/01/rdf-schema#comment>
                "Something that is created or produced as a result of a project or an endeavour. Examples include a building resulting from a building project, educated students graduating from an educational programme, and a journal article published as a result of a research project.  Research outputs can also include reports, datasets, experimental protocols, workflows and mathematical models, and material outputs such as a cell line, a mouse mutant or a new form of microscope."@en ;
        <http://www.w3.org/2000/01/rdf-schema#label>
                "output"@en ;
        <http://www.w3.org/2000/01/rdf-schema#subClassOf>
                <http://purl.org/cerif/frapo/Equipment> , <http://www.w3.org/2002/07/owl#Thing> ;
        <http://purl.org/dc/elements/1.1/description>
                "Ontology terms and definitions for most publishable project outputs are given as 'Expression' classes in FaBiO, the FRBR-aligned Bibliographic Ontology, e.g. fabio:JournalArticle, fabio:DataSet.  For 'deliverables', use frapo:Deliverable.  For material outputs, use frapo:MaterialOutput."@en .

<http://purl.org/cerif/frapo/hasCurrency>
        a       <http://www.w3.org/2002/07/owl#DatatypeProperty> ;
        <http://www.w3.org/2000/01/rdf-schema#comment>
                "A data property defining the currency used to specify a financial entity.  Use in conjection with frapo:hasMonetaryValue."@en ;
        <http://www.w3.org/2000/01/rdf-schema#label>
                "has currency"@en .

<http://purl.org/cerif/frapo/owl:sameAs>
        a       <http://www.w3.org/2002/07/owl#AnnotationProperty> .

<http://purl.org/cerif/frapo/hasManufactureDate>
        a       <http://www.w3.org/2002/07/owl#DatatypeProperty> , <http://www.w3.org/2002/07/owl#FunctionalProperty> ;
        <http://www.w3.org/2000/01/rdf-schema#comment>
                "A data property linking something to its date of manufacture."@en ;
        <http://www.w3.org/2000/01/rdf-schema#label>
                "has data of manufacture"@en ;
        <http://www.w3.org/2000/01/rdf-schema#range>
                <http://www.w3.org/2001/XMLSchema#dateTime> ;
        <http://www.w3.org/2000/01/rdf-schema#subPropertyOf>
                <http://purl.org/dc/terms/date> .

<http://purl.org/cerif/frapo/hasHeadcount>
        a       <http://www.w3.org/2002/07/owl#DatatypeProperty> ;
        <http://www.w3.org/2000/01/rdf-schema#comment>
                "A data property specifying the number of people employed by an organization."@en ;
        <http://www.w3.org/2000/01/rdf-schema#label>
                "has headcount"@en ;
        <http://www.w3.org/2000/01/rdf-schema#subPropertyOf>
                <http://purl.org/cerif/frapo/hasOrganizationalInformation> .

<http://xmlns.com/foaf/0.1/gender>
        a       <http://www.w3.org/2002/07/owl#DatatypeProperty> , <http://www.w3.org/2002/07/owl#AnnotationProperty> ;
        <http://www.w3.org/2000/01/rdf-schema#subPropertyOf>
                <http://purl.org/cerif/frapo/hasPersonalInformation> .

<http://purl.org/cerif/frapo/hasOutput>
        a       <http://www.w3.org/2002/07/owl#ObjectProperty> ;
        <http://www.w3.org/2000/01/rdf-schema#comment>
                "An object property linking an activity such as a project or endeavour to something that is created or produced as a result of that activity.  Examples include a building created as a result of a building project, and a journal article published to describe the results of a research investigation.  "@en ;
        <http://www.w3.org/2000/01/rdf-schema#label>
                "has output"@en ;
        <http://purl.org/dc/elements/1.1/description>
                "Domain and range constraints have been removed from this object property to permit it to be used in unforeseen ways."@en ;
        <http://www.w3.org/2002/07/owl#inverseOf>
                <http://purl.org/cerif/frapo/isOutputOf> .

<http://purl.org/cerif/frapo/Investigation>
        a       <http://www.w3.org/2002/07/owl#Class> ;
        <http://www.w3.org/2000/01/rdf-schema#comment>
                "An investigation is an endeavour that involves research, enabled by a project.  \n\nThe investigation relate to the scholarly and practical aspects of conducting the research itself, including the hypotheses being investigated, the experiments being undertaken, the data being gathered and analysed, the interpretations being drawn from the data, and the results obtained.  \n\nIn contrast, the project that enables it encompasses the administrative aspects of undertaking the endeavour, including the funding obtained, the people employed, and the management of the project in terms of deadlines and deliverables."@en ;
        <http://www.w3.org/2000/01/rdf-schema#label>
                "investigation"@en ;
        <http://www.w3.org/2000/01/rdf-schema#subClassOf>
                <http://purl.org/cerif/frapo/Endeavour> ;
        <http://purl.org/dc/elements/1.1/description>
                "Equivalent class in ISA-RDF: 'Investigation'."@en .

<http://purl.org/cerif/frapo/ownsIRPOf>
        a       <http://www.w3.org/2002/07/owl#ObjectProperty> ;
        <http://www.w3.org/2000/01/rdf-schema#comment>
                "An object property linking an agent who owns IPR arising from or relating to an entity to that entity."@en ;
        <http://www.w3.org/2000/01/rdf-schema#domain>
                <http://xmlns.com/foaf/0.1/Agent> ;
        <http://www.w3.org/2000/01/rdf-schema#label>
                "owns IPR of"@en ;
        <http://www.w3.org/2000/01/rdf-schema#subPropertyOf>
                <http://purl.org/cerif/frapo/owns> .

<http://purl.org/dc/terms/date>
        a       <http://www.w3.org/2002/07/owl#DatatypeProperty> .

<http://purl.org/cerif/frapo/Owner>
        a       <http://www.w3.org/2002/07/owl#Class> ;
        <http://www.w3.org/2000/01/rdf-schema#comment>
                "The agent who owns an entity."@en ;
        <http://www.w3.org/2000/01/rdf-schema#label>
                "owner"@en ;
        <http://www.w3.org/2000/01/rdf-schema#subClassOf>
                <http://xmlns.com/foaf/0.1/Agent> .

<http://purl.org/cerif/frapo/evaluates>
        a       <http://www.w3.org/2002/07/owl#ObjectProperty> ;
        <http://www.w3.org/2000/01/rdf-schema#comment>
                "An object property linking an agent to an entity which that agent evaluates, for example a funding agency that is evaluating a grant application to determine whether the proposed project is worthy of funding, or a publisher evaluating a manuscript to determine whether it is suitable for publication."@en ;
        <http://www.w3.org/2000/01/rdf-schema#domain>
                <http://xmlns.com/foaf/0.1/Agent> ;
        <http://www.w3.org/2000/01/rdf-schema#label>
                "evaluates"@en ;
        <http://www.w3.org/2002/07/owl#inverseOf>
                <http://purl.org/cerif/frapo/isEvaluatedBy> .

<http://purl.org/cerif/frapo/hasJobTitle>
        a       <http://www.w3.org/2002/07/owl#DatatypeProperty> ;
        <http://www.w3.org/2000/01/rdf-schema#comment>
                "A data property permitting specification of the job title held by a person, such as might appear next to the name in a directory or on a conference name badge.  For example, the person's specific Job Title might be 'Linacre Professor of Zoology' or 'Regius Professor of Moral Philosophy'. \n\nThis job title properly refers to the **role** held by that person (e.g. 'Head of Department'), which can be separately defined using SCoRO, the Scholarly Contributions and Roles Ontology (http://purl.org/spar/scoro/). [see scoro:withJobTitle].\n\n"@en ;
        <http://www.w3.org/2000/01/rdf-schema#domain>
                <http://xmlns.com/foaf/0.1/Person> ;
        <http://www.w3.org/2000/01/rdf-schema#label>
                "has job title"@en ;
        <http://www.w3.org/2000/01/rdf-schema#subPropertyOf>
                <http://purl.org/cerif/frapo/hasPersonalInformation> .

<http://purl.org/cerif/frapo/ServiceContract>
        a       <http://www.w3.org/2002/07/owl#Class> ;
        <http://www.w3.org/2000/01/rdf-schema#comment>
                "A contract for the provision of a service such as a cleaning service, or for the regular servicing, maintenance and repair of some item of equipment or infrastructure."@en ;
        <http://www.w3.org/2000/01/rdf-schema#label>
                "service contract"@en ;
        <http://www.w3.org/2000/01/rdf-schema#subClassOf>
                <http://purl.org/cerif/frapo/Contract> .

<http://purl.org/cerif/frapo/BudgetedAmount>
        a       <http://www.w3.org/2002/07/owl#Class> ;
        <http://www.w3.org/2000/01/rdf-schema#comment>
                "The amount of money originally available to spend in a particular budget category."@en ;
        <http://www.w3.org/2000/01/rdf-schema#label>
                "budgeted amount"@en ;
        <http://www.w3.org/2000/01/rdf-schema#subClassOf>
                <http://purl.org/cerif/frapo/BudgetInformation> .

<http://purl.org/cerif/frapo/MaterialOutput>
        a       <http://www.w3.org/2002/07/owl#Class> ;
        <http://www.w3.org/2000/01/rdf-schema#comment>
                "A material or physical output created or produced as a result of a project or an endeavour such as a research investigation. Examples include a building constructed as a result of a building project, and research outputs such as a cell line, a mouse mutant or a new form of microscope."@en ;
        <http://www.w3.org/2000/01/rdf-schema#label>
                "material output"@en ;
        <http://www.w3.org/2000/01/rdf-schema#subClassOf>
                <http://purl.org/cerif/frapo/Output> .

<http://purl.org/cerif/frapo/hasTemporalDuration>
        a       <http://www.w3.org/2002/07/owl#DatatypeProperty> ;
        <http://www.w3.org/2000/01/rdf-schema#comment>
                "A data property enabling one to define the temporal duration of some entity such as an event or a project."@en ;
        <http://www.w3.org/2000/01/rdf-schema#label>
                "has temporal duration"@en ;
        <http://www.w3.org/2000/01/rdf-schema#range>
                <http://www.w3.org/2001/XMLSchema#dateTime> .

<http://purl.org/cerif/frapo/isDonatedBy>
        a       <http://www.w3.org/2002/07/owl#ObjectProperty> ;
        <http://www.w3.org/2000/01/rdf-schema#comment>
                "An object property linking a gift to the benefactor who provided it."@en ;
        <http://www.w3.org/2000/01/rdf-schema#label>
                "is donated by"@en ;
        <http://www.w3.org/2000/01/rdf-schema#range>
                <http://xmlns.com/foaf/0.1/Agent> ;
        <http://purl.org/dc/elements/1.1/description>
                "Domain constraints have been removed from this object property to permit it to be used in unforeseen ways."@en .

<http://xmlns.com/foaf/0.1/Person>
        a       <http://www.w3.org/2002/07/owl#Class> .

<http://purl.org/cerif/frapo/consumables-costs>
        a       <http://www.w3.org/2002/07/owl#NamedIndividual> , <http://purl.org/cerif/frapo/BudgetCategory> ;
        <http://www.w3.org/2000/01/rdf-schema#comment>
                "A budget category to cover the costs of purchasing consumables."@en ;
        <http://www.w3.org/2000/01/rdf-schema#label>
                "consumables costs"@en .

<http://purl.org/cerif/frapo/hasAcronym>
        a       <http://www.w3.org/2002/07/owl#DatatypeProperty> ;
        <http://www.w3.org/2000/01/rdf-schema#comment>
                "A data property linking an entity to an acronym used to identify it, based on its full name or title.  For example, this ontology has the full name 'Funding, Research Administration and Projects Ontology' and the acronym 'FRAPO'."@en ;
        <http://www.w3.org/2000/01/rdf-schema#label>
                "has acronym"@en .

<http://purl.org/cerif/frapo/hasDomainName>
        a       <http://www.w3.org/2002/07/owl#DatatypeProperty> ;
        <http://www.w3.org/2000/01/rdf-schema#comment>
                "A data property linking an entity to an internet domain name that has been registered for that entity, for example http://www.miidi.org for MIIDI, the Minimal Information standard for reporting an Infectious Disease Investigation."@en ;
        <http://www.w3.org/2000/01/rdf-schema#label>
                "has domain name"@en .

<http://purl.org/cerif/frapo/isFundedBy>
        a       <http://www.w3.org/2002/07/owl#ObjectProperty> ;
        <http://www.w3.org/2000/01/rdf-schema#comment>
                "An object property linking something to the funding that funds it (i.e. that finances or pays for it), or to the funding agency providing that funding.  This flexibility is given because of alternative usages of the English word 'funds'.  [See also frapo:isAwardedBy and frapo:hasFundingAgency and frapo:isSupportedBy.]"@en ;
        <http://www.w3.org/2000/01/rdf-schema#label>
                "is funded by"@en ;
        <http://www.w3.org/2000/01/rdf-schema#subPropertyOf>
                <http://purl.org/cerif/frapo/isSupportedBy> .

<http://xmlns.com/foaf/0.1/Group>
        a       <http://www.w3.org/2002/07/owl#Class> .

<http://purl.org/cerif/frapo/hasKeyword>
        a       <http://www.w3.org/2002/07/owl#DatatypeProperty> ;
        <http://www.w3.org/2000/01/rdf-schema#comment>
                "A data property permitting specification of a keyword relating to an entity."@en ;
        <http://www.w3.org/2000/01/rdf-schema#label>
                "has keyword"@en .

<http://purl.org/cerif/cerro/results_in_beginning>
        a       <http://www.w3.org/2002/07/owl#AnnotationProperty> ;
        <http://www.w3.org/2000/01/rdf-schema#subPropertyOf>
                <http://www.w3.org/2000/01/rdf-schema#label> .

<http://xmlns.com/foaf/0.1/family_name>
        a       <http://www.w3.org/2002/07/owl#AnnotationProperty> , <http://www.w3.org/2002/07/owl#DatatypeProperty> ;
        <http://www.w3.org/2000/01/rdf-schema#subPropertyOf>
                <http://purl.org/cerif/frapo/hasPersonalInformation> .

<http://purl.org/cerif/frapo/hasDispatchDate>
        a       <http://www.w3.org/2002/07/owl#DatatypeProperty> ;
        <http://www.w3.org/2000/01/rdf-schema#comment>
                "The date on which something, for example an item of equipment, is dispatched by the supplier."@en ;
        <http://www.w3.org/2000/01/rdf-schema#label>
                "has dispatch date"@en ;
        <http://www.w3.org/2000/01/rdf-schema#range>
                <http://www.w3.org/2001/XMLSchema#dateTime> ;
        <http://www.w3.org/2000/01/rdf-schema#subPropertyOf>
                <http://purl.org/dc/terms/date> .

<http://purl.org/cerif/frapo/consultancy-costs>
        a       <http://purl.org/cerif/frapo/BudgetCategory> , <http://www.w3.org/2002/07/owl#NamedIndividual> ;
        <http://www.w3.org/2000/01/rdf-schema#comment>
                "A budget category to cover the costs of consultancy fees."@en ;
        <http://www.w3.org/2000/01/rdf-schema#label>
                "consultancy costs"@en .

<http://purl.org/cerif/frapo/ArticleProcessingCharge>
        a       <http://www.w3.org/2002/07/owl#Class> ;
        <http://www.w3.org/2000/01/rdf-schema#comment>
                "A fee levied by a publisher on an author or an institution to cover the cost of publishing an Open Access journal article.  Also knows as Article Processing Fee, Article Publication Charge, Author Processing Charge or Author Publishing Charge."@en ;
        <http://www.w3.org/2000/01/rdf-schema#label>
                "article processing charge"@en ;
        <http://www.w3.org/2000/01/rdf-schema#subClassOf>
                <http://purl.org/cerif/frapo/Fee> .

<http://purl.org/cerif/frapo/Scholarship>
        a       <http://www.w3.org/2002/07/owl#Class> ;
        <http://www.w3.org/2000/01/rdf-schema#comment>
                "A financial grant to a scholar to enable him/her to undertake advanced academic study."@en ;
        <http://www.w3.org/2000/01/rdf-schema#label>
                "scholarship"@en ;
        <http://www.w3.org/2000/01/rdf-schema#subClassOf>
                <http://purl.org/cerif/frapo/Stipend> .

<http://purl.org/cerif/frapo/Status>
        a       <http://www.w3.org/2002/07/owl#Class> ;
        <http://www.w3.org/2000/01/rdf-schema#comment>
                "The status of something such as an application, an investigation or a project."@en ;
        <http://www.w3.org/2000/01/rdf-schema#label>
                "status"@en ;
        <http://www.w3.org/2000/01/rdf-schema#subClassOf>
                <http://www.w3.org/2002/07/owl#Thing> .

<http://purl.org/cerif/frapo/hasCountry>
        a       <http://www.w3.org/2002/07/owl#DatatypeProperty> ;
        <http://www.w3.org/2000/01/rdf-schema#comment>
                "A data property specifying a country, for example as the location of an event."@en ;
        <http://www.w3.org/2000/01/rdf-schema#label>
                "has country"@en .

<http://purl.org/cerif/frapo/Company>
        a       <http://www.w3.org/2002/07/owl#Class> ;
        <http://www.w3.org/2000/01/rdf-schema#comment>
                "A commercial company or business run for profit."@en ;
        <http://www.w3.org/2000/01/rdf-schema#label>
                "company"@en ;
        <http://www.w3.org/2000/01/rdf-schema#subClassOf>
                <http://xmlns.com/foaf/0.1/Organization> .

<http://purl.org/dc/elements/1.1/contributor>
        a       <http://www.w3.org/2002/07/owl#AnnotationProperty> .

<http://purl.org/cerif/frapo/Grant>
        a       <http://www.w3.org/2002/07/owl#Class> ;
        <http://www.w3.org/2000/01/rdf-schema#comment>
                "A financial award by a funding agency for a particular project or purpose, usually awarded on the basis of a competitive application."@en ;
        <http://www.w3.org/2000/01/rdf-schema#label>
                "grant"@en ;
        <http://www.w3.org/2000/01/rdf-schema#subClassOf>
                <http://purl.org/cerif/frapo/Funding> .

<http://purl.org/cerif/frapo/hasNameSuffix>
        a       <http://www.w3.org/2002/07/owl#DatatypeProperty> ;
        <http://www.w3.org/2000/01/rdf-schema#comment>
                "The letters that should be displayed after a person's name."@en ;
        <http://www.w3.org/2000/01/rdf-schema#label>
                "has name suffix"@en ;
        <http://www.w3.org/2000/01/rdf-schema#subPropertyOf>
                <http://purl.org/cerif/frapo/hasPersonalInformation> .

<http://purl.org/cerif/frapo/isOwnedBy>
        a       <http://www.w3.org/2002/07/owl#ObjectProperty> ;
        <http://www.w3.org/2000/01/rdf-schema#comment>
                "An object property linking an entity to the agent that owns it."@en ;
        <http://www.w3.org/2000/01/rdf-schema#label>
                "is owned by"@en ;
        <http://www.w3.org/2000/01/rdf-schema#range>
                <http://xmlns.com/foaf/0.1/Agent> ;
        <http://www.w3.org/2002/07/owl#inverseOf>
                <http://purl.org/cerif/frapo/owns> .

<http://purl.org/cerif/frapo/FundingProgramme>
        a       <http://www.w3.org/2002/07/owl#Class> ;
        <http://www.w3.org/2000/01/rdf-schema#comment>
                "A programme of related funded activities or projects, typically established by a funding agency.  Often associated with publication of a call for applications (fabio:CallForApplications)."@en ;
        <http://www.w3.org/2000/01/rdf-schema#label>
                "funding programme"@en ;
        <http://www.w3.org/2000/01/rdf-schema#subClassOf>
                <http://www.w3.org/2002/07/owl#Thing> .

<http://purl.org/cerif/frapo/Purchaser>
        a       <http://www.w3.org/2002/07/owl#Class> ;
        <http://www.w3.org/2000/01/rdf-schema#comment>
                "An agent who purchases something from a supplier."@en ;
        <http://www.w3.org/2000/01/rdf-schema#label>
                "purchaser"@en ;
        <http://www.w3.org/2000/01/rdf-schema#subClassOf>
                <http://xmlns.com/foaf/0.1/Agent> .

<http://purl.org/cerif/frapo/AnnualTurnover>
        a       <http://www.w3.org/2002/07/owl#Class> ;
        <http://www.w3.org/2000/01/rdf-schema#comment>
                "The anual financial turnover of an organization (in a specified currency)."@en ;
        <http://www.w3.org/2000/01/rdf-schema#label>
                "annual turnover"@en ;
        <http://www.w3.org/2000/01/rdf-schema#subClassOf>
                <http://purl.org/cerif/frapo/FinancialEntity> .

<http://purl.org/cerif/frapo/specifiesExpediture>
        a       <http://www.w3.org/2002/07/owl#ObjectProperty> ;
        <http://www.w3.org/2000/01/rdf-schema#comment>
                "An object property relating an agent or a budget to the expenditure specified by that agent or budget."@en ;
        <http://www.w3.org/2000/01/rdf-schema#domain>
                [ a       <http://www.w3.org/2002/07/owl#Class> ;
                  <http://www.w3.org/2002/07/owl#unionOf>
                          ( <http://purl.org/cerif/frapo/Budget> <http://xmlns.com/foaf/0.1/Agent> )
                ] ;
        <http://www.w3.org/2000/01/rdf-schema#label>
                "specifies expenditure"@en ;
        <http://purl.org/dc/elements/1.1/description>
                "Range constraints have been removed from this object property to permit it to be used in unforeseen ways."@en .

<http://purl.org/cerif/frapo/PurchaseOrder>
        a       <http://www.w3.org/2002/07/owl#Class> ;
        <http://www.w3.org/2000/01/rdf-schema#comment>
                "An official order from a purchasing institution to a supplier for the purchase of goods or services, often issued in response to the receipt of a quotation from the supplier."@en ;
        <http://www.w3.org/2000/01/rdf-schema#label>
                "purchase order"@en ;
        <http://www.w3.org/2000/01/rdf-schema#subClassOf>
                <http://purl.org/cerif/frapo/FinancialEntity> .

<http://purl.org/cerif/frapo/benefactor>
        a       <http://xmlns.com/foaf/0.1/Person> , <http://www.w3.org/2002/07/owl#NamedIndividual> ;
        <http://www.w3.org/2000/01/rdf-schema#comment>
                "A person who gives a gift."@en ;
        <http://www.w3.org/2000/01/rdf-schema#label>
                "benefactor"@en .

<http://purl.org/cerif/frapo/Payment>
        a       <http://www.w3.org/2002/07/owl#Class> ;
        <http://www.w3.org/2000/01/rdf-schema#comment>
                "A financial payment made, for example in exchange for something purchased such as property, goods or services, or to refund expenses incurred."@en ;
        <http://www.w3.org/2000/01/rdf-schema#label>
                "payment"@en ;
        <http://www.w3.org/2000/01/rdf-schema#subClassOf>
                <http://purl.org/cerif/frapo/FinancialEntity> .

<http://purl.org/cerif/frapo/ResearchInstitute>
        a       <http://www.w3.org/2002/07/owl#Class> ;
        <http://www.w3.org/2000/01/rdf-schema#comment>
                "An organization primarily dedicated to undertaking research, that might be part of a university or of a commercial company, or might be independently funded by a research funding agency.  "@en ;
        <http://www.w3.org/2000/01/rdf-schema#label>
                "research institute"@en ;
        <http://www.w3.org/2000/01/rdf-schema#subClassOf>
                <http://xmlns.com/foaf/0.1/Organization> .

<http://purl.org/cerif/frapo/ResearchGroup>
        a       <http://www.w3.org/2002/07/owl#Class> ;
        <http://www.w3.org/2000/01/rdf-schema#comment>
                "A group of people, usually within a university department or a research institute, and typically under a single group leader, dedicated to working together to undertake research on one or more topics. May also be called a research unit."@en ;
        <http://www.w3.org/2000/01/rdf-schema#label>
                "research group"@en ;
        <http://www.w3.org/2000/01/rdf-schema#subClassOf>
                <http://xmlns.com/foaf/0.1/Group> .

<http://purl.org/cerif/frapo/hasExpiryDate>
        a       <http://www.w3.org/2002/07/owl#DatatypeProperty> , <http://www.w3.org/2002/07/owl#FunctionalProperty> ;
        <http://www.w3.org/2000/01/rdf-schema#comment>
                "A data property linking something, for example a drug, to its expiry date, beyond which the manufacture recommends that it should not be used."@en ;
        <http://www.w3.org/2000/01/rdf-schema#label>
                "has expiry date"@en ;
        <http://www.w3.org/2000/01/rdf-schema#range>
                <http://www.w3.org/2001/XMLSchema#dateTime> ;
        <http://www.w3.org/2000/01/rdf-schema#subPropertyOf>
                <http://purl.org/dc/terms/date> .

<http://www.w3.org/2001/XMLSchema#date>
        a       <http://www.w3.org/2000/01/rdf-schema#Datatype> .

<http://purl.org/cerif/frapo/Invoice>
        a       <http://www.w3.org/2002/07/owl#Class> ;
        <http://www.w3.org/2000/01/rdf-schema#comment>
                "An invoice for payment of goods or services."@en ;
        <http://www.w3.org/2000/01/rdf-schema#label>
                "invoice"@en ;
        <http://www.w3.org/2000/01/rdf-schema#subClassOf>
                <http://purl.org/cerif/frapo/FinancialEntity> .

<http://purl.org/cerif/frapo/collaboratesWith>
        a       <http://www.w3.org/2002/07/owl#ObjectProperty> , <http://www.w3.org/2002/07/owl#SymmetricProperty> ;
        <http://www.w3.org/2000/01/rdf-schema#comment>
                "An object property linking agents, for example different organizations, or people typically from different groups or organizations, that work together on a common task, project or endeavour, or towards a common goal."@en ;
        <http://www.w3.org/2000/01/rdf-schema#domain>
                <http://xmlns.com/foaf/0.1/Agent> ;
        <http://www.w3.org/2000/01/rdf-schema#label>
                "collaborates with"@en ;
        <http://www.w3.org/2000/01/rdf-schema#range>
                <http://xmlns.com/foaf/0.1/Agent> .

<http://purl.org/cerif/frapo/Account>
        a       <http://www.w3.org/2002/07/owl#Class> ;
        <http://www.w3.org/2000/01/rdf-schema#comment>
                "A mechanism for administering money, typically owned by an agent and dedicated to a particular purpose, for example the equipment account of a university department, to be used only for the purchase or maintenance of items of equipment. "@en ;
        <http://www.w3.org/2000/01/rdf-schema#label>
                "account"@en ;
        <http://www.w3.org/2000/01/rdf-schema#subClassOf>
                <http://purl.org/cerif/frapo/FinancialEntity> .

<http://purl.org/cerif/frapo/Studentship>
        a       <http://www.w3.org/2002/07/owl#Class> ;
        <http://www.w3.org/2000/01/rdf-schema#comment>
                "A financial grant to a student to enable him/her to undertake advanced academic study."@en ;
        <http://www.w3.org/2000/01/rdf-schema#label>
                "studentship"@en ;
        <http://www.w3.org/2000/01/rdf-schema#subClassOf>
                <http://purl.org/cerif/frapo/Stipend> .

<http://purl.org/cerif/frapo/SpinOffCompany>
        a       <http://www.w3.org/2002/07/owl#Class> ;
        <http://www.w3.org/2000/01/rdf-schema#comment>
                "A company that has been established by a university or research institute to mature and market the results of research conducted at that research institution."@en ;
        <http://www.w3.org/2000/01/rdf-schema#label>
                "spin-off company"@en ;
        <http://www.w3.org/2000/01/rdf-schema#subClassOf>
                <http://purl.org/cerif/frapo/Company> .

<http://purl.org/cerif/frapo/hasCatalogNumber>
        a       <http://www.w3.org/2002/07/owl#DatatypeProperty> ;
        <http://www.w3.org/2000/01/rdf-schema#comment>
                "A data property linking something to its catalog number."@en ;
        <http://www.w3.org/2000/01/rdf-schema#label>
                "has catalog number"@en ;
        <http://www.w3.org/2000/01/rdf-schema#subPropertyOf>
                <http://purl.org/dc/terms/identifier> .

<http://purl.org/cerif/frapo/hasReferenceNumber>
        a       <http://www.w3.org/2002/07/owl#DatatypeProperty> ;
        <http://www.w3.org/2000/01/rdf-schema#comment>
                "A data property linking something to a reference number for that item."@en ;
        <http://www.w3.org/2000/01/rdf-schema#label>
                "has reference number"@en ;
        <http://www.w3.org/2000/01/rdf-schema#subPropertyOf>
                <http://purl.org/dc/terms/identifier> .

<http://purl.org/cerif/frapo/Purchase>
        a       <http://www.w3.org/2002/07/owl#Class> ;
        <http://www.w3.org/2000/01/rdf-schema#comment>
                "The payment for obtaining something, for example property, goods or services."@en ;
        <http://www.w3.org/2000/01/rdf-schema#label>
                "purchase"@en ;
        <http://www.w3.org/2000/01/rdf-schema#subClassOf>
                <http://purl.org/cerif/frapo/FinancialEntity> .

<http://purl.org/cerif/frapo/Vendor>
        a       <http://www.w3.org/2002/07/owl#Class> ;
        <http://www.w3.org/2000/01/rdf-schema#comment>
                "An agent who supplies goods or services in exchange for payment, in response to receipt of payment or of an official purchase order from a purchaser that is responded to by submission of an invoice for what is supplied."@en ;
        <http://www.w3.org/2000/01/rdf-schema#label>
                "vendor"@en ;
        <http://www.w3.org/2000/01/rdf-schema#subClassOf>
                <http://purl.org/cerif/frapo/Supplier> .

<http://www.w3.org/2002/07/owl#versionInfo>
        a       <http://www.w3.org/2002/07/owl#AnnotationProperty> .

<http://purl.org/cerif/frapo/RegistrationAuthority>
        a       <http://www.w3.org/2002/07/owl#Class> ;
        <http://www.w3.org/2000/01/rdf-schema#comment>
                "An agent with responsibility for registering and maintaining international standards, internet domain names, patents, controlled vocabularies and other similar entities required for reliable international cooperatative activities. For example, the International DOI Foundation (IDF) is the Registration Authority for DOIs."@en ;
        <http://www.w3.org/2000/01/rdf-schema#label>
                "registration authority"@en ;
        <http://www.w3.org/2000/01/rdf-schema#subClassOf>
                <http://xmlns.com/foaf/0.1/Organization> .

<http://purl.org/cerif/frapo/Quotation>
        a       <http://www.w3.org/2002/07/owl#Class> ;
        <http://www.w3.org/2000/01/rdf-schema#comment>
                "A formal statement of promise (usually provided in response to a request for quotation) by potential supplier to supply goods or services at specified prices and within a specified period. Acceptance of the quotation by the buyer constitutes an agreement binding on both parties.  (Shortened from http://www.businessdictionary.com/definition/quotation.html).\n"@en ;
        <http://www.w3.org/2000/01/rdf-schema#label>
                "quotation"@en ;
        <http://www.w3.org/2000/01/rdf-schema#subClassOf>
                <http://purl.org/cerif/frapo/FinancialEntity> .

<http://purl.org/dc/elements/1.1/date>
        a       <http://www.w3.org/2002/07/owl#AnnotationProperty> .

<http://purl.org/cerif/frapo/HostInstitution>
        a       <http://www.w3.org/2002/07/owl#Class> ;
        <http://www.w3.org/2000/01/rdf-schema#comment>
                "An institution that acts as a host, for example of a project, a resource or a person, for example by providing accommodation, services, operational support and/or funding."@en ;
        <http://www.w3.org/2000/01/rdf-schema#label>
                "host institution"@en ;
        <http://www.w3.org/2000/01/rdf-schema#subClassOf>
                <http://xmlns.com/foaf/0.1/Organization> .

<http://purl.org/cerif/frapo/hasCustomerNumber>
        a       <http://www.w3.org/2002/07/owl#DatatypeProperty> ;
        <http://www.w3.org/2000/01/rdf-schema#comment>
                "A data property linking an agent to an identifying number for that agent, typically used by the accounting system of the supplier when issuing quotations, fulfilling orders and submitting invoices."@en ;
        <http://www.w3.org/2000/01/rdf-schema#domain>
                <http://purl.org/cerif/frapo/Purchaser> ;
        <http://www.w3.org/2000/01/rdf-schema#label>
                "has customer number"@en ;
        <http://www.w3.org/2000/01/rdf-schema#subPropertyOf>
                <http://purl.org/dc/terms/identifier> .

<http://purl.org/cerif/frapo/Budget>
        a       <http://www.w3.org/2002/07/owl#Class> ;
        <http://www.w3.org/2000/01/rdf-schema#comment>
                "A structured statement of how funds are to be used for expenditure in defined budget categories.  A budget is created, for example, when applying for funding for a project, and is subsequently used to manage the expenditure from the awarded grant for that project."@en ;
        <http://www.w3.org/2000/01/rdf-schema#label>
                "budget"@en ;
        <http://www.w3.org/2000/01/rdf-schema#subClassOf>
                <http://purl.org/cerif/frapo/FinancialEntity> .

<http://purl.org/cerif/frapo/isEnabledBy>
        a       <http://www.w3.org/2002/07/owl#ObjectProperty> ;
        <http://www.w3.org/2000/01/rdf-schema#comment>
                "An object property relating an entity to another entity that enables it, e.g. linking an investigation to a project that enables it."@en ;
        <http://www.w3.org/2000/01/rdf-schema#label>
                "is enabled by"@en ;
        <http://purl.org/dc/elements/1.1/description>
                "Domain and range constraints have been removed from this object property to permit it to be used in unforeseen ways."@en .

<http://xmlns.com/foaf/0.1/Agent>
        a       <http://www.w3.org/2002/07/owl#Class> .

<http://purl.org/cerif/frapo/hasFamilialSuffix>
        a       <http://www.w3.org/2002/07/owl#DatatypeProperty> ;
        <http://www.w3.org/2000/01/rdf-schema#comment>
                "The letters that may be displayed after a person's name to indicate familial status, e.g. Sn., Jn., III, 3rd."@en ;
        <http://www.w3.org/2000/01/rdf-schema#label>
                "has familiar suffix"@en ;
        <http://www.w3.org/2000/01/rdf-schema#subPropertyOf>
                <http://purl.org/cerif/frapo/hasNameSuffix> .

<http://purl.org/cerif/frapo/Department>
        a       <http://www.w3.org/2002/07/owl#Class> ;
        <http://www.w3.org/2000/01/rdf-schema#comment>
                "A department or sub-section within a larger organization, for example a university academic department."@en ;
        <http://www.w3.org/2000/01/rdf-schema#label>
                "department"@en ;
        <http://www.w3.org/2000/01/rdf-schema#subClassOf>
                <http://xmlns.com/foaf/0.1/Organization> .

<http://www.w3.org/2000/01/rdf-schema#seeAlso>
        a       <http://www.w3.org/2002/07/owl#AnnotationProperty> .

<http://purl.org/dc/elements/1.1/description>
        a       <http://www.w3.org/2002/07/owl#AnnotationProperty> .

<http://purl.org/cerif/frapo/Facility>
        a       <http://www.w3.org/2002/07/owl#Class> ;
        <http://www.w3.org/2000/01/rdf-schema#comment>
                "A place or installation built or designed to serve a specific function or provide a specific service, for example an animal breeding centre, a DNA sequencing facility or a confocal imaging laboratory."@en ;
        <http://www.w3.org/2000/01/rdf-schema#label>
                "facility"@en ;
        <http://www.w3.org/2000/01/rdf-schema#subClassOf>
                <http://purl.org/cerif/frapo/InfrastructureEntity> .
