<http://linked.data.gov.au/def/geofabric> <http://www.w3.org/2002/07/owl#versionInfo> "Beta version"@en .
<http://linked.data.gov.au/def/geofabric#RiverRegion> <http://www.w3.org/2000/01/rdf-schema#subClassOf> <http://www.opengis.net/ont/geosparql#Feature> .
_:Bc0254babce19175c3e91079fc96c0f85 <https://schema.org/identifier> <http://catalogue.linked.data.gov.au/org/csiro> .
_:B284bc2e7a5f2190407d62828b5105ed7 <http://www.w3.org/1999/02/22-rdf-syntax-ns#type> <http://www.w3.org/2002/07/owl#Restriction> .
_:Be3b61f29b77409e2d388e9722746c75d <https://schema.org/name> "Nicholas J. Car" .
<http://linked.data.gov.au/def/geofabric#RiverRegion> <http://www.w3.org/2000/01/rdf-schema#subClassOf> <https://www.opengis.net/def/appschema/hy_features/hyf/HY_CatchmentAggregate> .
<http://linked.data.gov.au/def/geofabric#ReportingRegion> <http://www.w3.org/2000/01/rdf-schema#label> "Geofabric Hydrology reporting region" .
<http://linked.data.gov.au/def/geofabric#ContractedCatchment> <http://www.w3.org/2000/01/rdf-schema#comment> "The Geofabric's Hydrology Reporting Catchments product's AHGF Contracted Catchment object.\n\nContracted Catchments are always within River Revions."@en .
_:B284bc2e7a5f2190407d62828b5105ed7 <http://www.w3.org/2002/07/owl#onClass> <http://linked.data.gov.au/def/geofabric#DrainageDivision> .
<http://linked.data.gov.au/def/geofabric#DrainageDivision> <http://www.w3.org/2000/01/rdf-schema#subClassOf> <https://www.opengis.net/def/appschema/hy_features/hyf/HY_CatchmentAggregate> .
<https://www.opengis.net/def/appschema/hy_features/hyf/HY_Catchment> <http://www.w3.org/2000/01/rdf-schema#comment> "The HY Features Ontology's generic class for a catchment"@en .
_:B680b1aafe8be8d4b4b6ddb06a1024273 <https://schema.org/name> "CSIRO" .
_:B738f77d6e389fb671d376b9d1754f146 <http://www.w3.org/1999/02/22-rdf-syntax-ns#type> <http://www.w3.org/2002/07/owl#Restriction> .
<https://www.opengis.net/def/appschema/hy_features/hyf/HY_CatchmentAggregate> <http://www.w3.org/2000/01/rdf-schema#comment> "The HY Features Ontology's generic class for an aggregation of catchments"@en .
<http://linked.data.gov.au/def/geofabric> <http://purl.org/dc/terms/created> "2019-06-07"^^<http://www.w3.org/2001/XMLSchema#date> .
<http://linked.data.gov.au/def/geofabric#ContractedCatchment> <http://purl.org/dc/elements/1.1/source> "Section 5.4.3 Page 40 in the Australian Hydrological Geospatial Fabric (Geofabric) v3.0 Product Guide"@en .
_:Bd06b23f60a1f5897e137e7832491c0ed <https://schema.org/identifier> <http://catalogue.linked.data.gov.au/org/csiro> .
<http://linked.data.gov.au/def/geofabric#DrainageDivision> <http://www.w3.org/2000/01/rdf-schema#subClassOf> <http://www.opengis.net/ont/geosparql#Feature> .
<http://www.opengis.net/ont/geosparql#Feature> <http://www.w3.org/1999/02/22-rdf-syntax-ns#type> <http://www.w3.org/2002/07/owl#Class> .
_:B187c66ed7b9f4b7f5f5313e69b20a48b <https://schema.org/name> "CSIRO" .
<https://www.opengis.net/def/appschema/hy_features/hyf/HY_Catchment> <http://www.w3.org/2000/01/rdf-schema#label> "Catchment" .
<http://linked.data.gov.au/def/geofabric#DrainageDivision> <http://www.w3.org/2000/01/rdf-schema#comment> "The Geofabric's Hydrology Reporting Region product's AWRA Drainage Division object.\n\nDrainage Division is defined for the purpose of providing a stable set of reporting regions specifically for the purpose of the Bureau’s Australian Water Resources Assessment (AWRA) and are referred to as the 2010 and 2012 Assessment Reporting Regions"@en .
<http://purl.org/dc/elements/1.1/source> <http://www.w3.org/1999/02/22-rdf-syntax-ns#type> <http://www.w3.org/2002/07/owl#AnnotationProperty> .
_:Be3b61f29b77409e2d388e9722746c75d <https://schema.org/identifier> <http://orcid.org/0000-0002-8742-7730> .
_:B284bc2e7a5f2190407d62828b5105ed7 <http://www.w3.org/2002/07/owl#onProperty> <http://www.opengis.net/ont/geosparql#sfWithin> .
<https://schema.org/identifier> <http://www.w3.org/1999/02/22-rdf-syntax-ns#type> <http://www.w3.org/2002/07/owl#AnnotationProperty> .
_:B6162819902b0dc0d6c42797657c381ac <https://schema.org/name> "CSIRO" .
<http://linked.data.gov.au/def/geofabric#RiverRegion> <http://www.w3.org/2000/01/rdf-schema#subClassOf> <http://linked.data.gov.au/def/geofabric#ReportingRegion> .
<http://linked.data.gov.au/def/geofabric#ReportingRegion> <http://www.w3.org/2000/01/rdf-schema#subClassOf> <http://www.opengis.net/ont/geosparql#Feature> .
<http://linked.data.gov.au/def/geofabric> <http://www.w3.org/2000/01/rdf-schema#comment> "A bare-bones ontology for the Australian Hydrological Geospatial Fabric.\n\nThis small ontology characterises major parts of the [Australian Hydrological Geospatial Fabric](http://www.bom.gov.au/water/geofabric/) for their delivery as [Linked Data](https://www.w3.org/wiki/LinkedData) via the [Geofabric LDAPI](http://linked.data.gov.au/dataset/geofabric).\n\nThis ontology accords with the [Loc-I Project](http://locationindex.org)'s requirements for the delivery of spatial [Semantic Web](https://www.w3.org/standards/semanticweb/) objects."@en .
_:B738f77d6e389fb671d376b9d1754f146 <http://www.w3.org/2002/07/owl#onProperty> <http://www.opengis.net/ont/geosparql#sfWithin> .
<http://linked.data.gov.au/def/geofabric#ContractedCatchment> <http://www.w3.org/1999/02/22-rdf-syntax-ns#type> <http://www.w3.org/2002/07/owl#Class> .
<http://linked.data.gov.au/def/geofabric#DrainageDivision> <http://purl.org/dc/elements/1.1/source> "Page 44 in the Australian Hydrological Geospatial Fabric (Geofabric) v3.0 Product Guide"@en .
<http://linked.data.gov.au/def/geofabric#ReportingRegion> <http://www.w3.org/2000/01/rdf-schema#subClassOf> <https://www.opengis.net/def/appschema/hy_features/hyf/HY_CatchmentAggregate> .
<http://linked.data.gov.au/def/geofabric#RiverRegion> <http://www.w3.org/2000/01/rdf-schema#label> "River Region" .
<http://linked.data.gov.au/def/geofabric#DrainageDivision> <http://www.w3.org/2000/01/rdf-schema#label> "Drainage Division" .
<http://linked.data.gov.au/def/geofabric#DrainageDivision> <http://www.w3.org/2000/01/rdf-schema#subClassOf> <http://linked.data.gov.au/def/geofabric#ReportingRegion> .
_:B6162819902b0dc0d6c42797657c381ac <https://schema.org/identifier> <http://catalogue.linked.data.gov.au/org/csiro> .
<http://linked.data.gov.au/def/geofabric#ContractedCatchment> <http://www.w3.org/2000/01/rdf-schema#label> "Contracted Catchment" .
<http://linked.data.gov.au/def/geofabric#RiverRegion> <http://www.w3.org/1999/02/22-rdf-syntax-ns#type> <http://www.w3.org/2002/07/owl#Class> .
_:B284bc2e7a5f2190407d62828b5105ed7 <http://www.w3.org/2002/07/owl#qualifiedCardinality> "1"^^<http://www.w3.org/2001/XMLSchema#nonNegativeInteger> .
_:Bc97368400aeef93595f36397b36b90f1 <https://schema.org/name> "Nicholas J. Car" .
<http://linked.data.gov.au/def/geofabric> <http://www.w3.org/2000/01/rdf-schema#seeAlso> "http://github.com/CSIRO-enviro-informatics/geofabric-ont/"@en .
<http://linked.data.gov.au/def/geofabric> <http://www.w3.org/2002/07/owl#imports> <http://www.opengis.net/ont/geosparql#> .
_:B1f7c1c9aa927c7f524b20ab63fa6ab10 <https://schema.org/name> "Nicholas J. Car" .
_:B92d492f0c98eddf7582466af474b17fc <https://schema.org/name> "Nicholas J. Car" .
<http://linked.data.gov.au/def/geofabric#RiverRegion> <http://purl.org/dc/elements/1.1/description> "The River Regions were based on a specification developed by Bureau hydrologists involved in\r\nwater resources assessment in consultation with the Geofabric team and scientists from\r\nCSIRO and ANU. These boundaries were developed for use in regional scale reporting and\r\nhydrological modelling. The River Region boundaries were not used in the Australian Water\r\nResources Assessment 2010 and 2012 but may be considered in the future as the resolution\r\nof reporting increases." .
_:B738f77d6e389fb671d376b9d1754f146 <http://www.w3.org/2002/07/owl#qualifiedCardinality> "1"^^<http://www.w3.org/2001/XMLSchema#nonNegativeInteger> .
<http://linked.data.gov.au/def/geofabric> <http://www.w3.org/1999/02/22-rdf-syntax-ns#type> <http://www.w3.org/2002/07/owl#Ontology> .
<http://linked.data.gov.au/def/geofabric> <http://www.w3.org/2002/07/owl#versionInfo> "Version 1.0 only characterises 3 types of Feature - Contracted Catchment, River Region & Drianage Division - and requires that each CC be within a RR and that an RR be within a DD."@en .
<http://linked.data.gov.au/def/geofabric> <http://purl.org/dc/terms/contributor> <https://orcid.org/0000-0002-3884-3420> .
<http://linked.data.gov.au/def/geofabric> <http://purl.org/dc/terms/publisher> _:B680b1aafe8be8d4b4b6ddb06a1024273 .
<https://schema.org/name> <http://www.w3.org/1999/02/22-rdf-syntax-ns#type> <http://www.w3.org/2002/07/owl#AnnotationProperty> .
<http://linked.data.gov.au/def/geofabric#DrainageDivision> <http://www.w3.org/1999/02/22-rdf-syntax-ns#type> <http://www.w3.org/2002/07/owl#Class> .
_:Bc1f6687f9ead4d0676f6a4ddb05d8c5c <https://schema.org/name> "Nicholas J. Car" .
<http://linked.data.gov.au/def/geofabric#ContractedCatchment> <http://www.w3.org/2000/01/rdf-schema#subClassOf> _:B738f77d6e389fb671d376b9d1754f146 .
<http://linked.data.gov.au/def/geofabric#ContractedCatchment> <http://purl.org/dc/elements/1.1/description> "All contracted catchment features of type ContractedArea are aggregations of the\r\nAHGFCatchment units that participate in a relationship of common geographic extent based\r\nupon the location of a contracted node from both Geofabric Surface Cartography and\r\nGeofabric Surface Network or a data sink as defined within the DEM-1S. Levels of confidence\r\nfor contracted nodes are further described in the following section of the Geofabric Product\r\nGuide.\r\n\r\nEach ContractedArea is assigned with the contracted node identifier (ConNodeID) and the\r\nconfidence level (ConLevel) of the contracted node to which they drain. The ContractedArea\r\nfeatures are the drainage areas of a combination of Levels 1 and 2 contracted nodes. These\r\ndrainage areas also incorporate catchment areas where there is no discernable flow (at\r\n1:250,000 scale) in the form of stream flow segment features. The allocation of no flow areas\r\nto contracted catchments is performed based on the most likely destination of water falling in\r\nthese areas in flood type conditions. \r\n\r\nContracted catchment hierarchy\r\n\r\nIn previous versions of the Geofabric, the set of contracted catchment features provided a\r\ncollection of drainage areas for a set of persistent contracted nodes. In V2.1 these areas have\r\nbeen further processed to aggregate these features into a contracted catchment hierarchy.\r\nThis hierarchy of contracted catchments includes only those catchments for key contracted\r\nnodes taken from a full set of contractible river confluences, sinks, monitoring points and the\r\ninflow and outflow points of water storages. These key contracted nodes form a stable,\r\nlogical, dendritic hierarchy of catchments that can be reliably reproduced when moving to\r\nhigher resolution or larger scaled data. The contracted catchment hierarchy provides a\r\nreliable and stable set of catchments that, among other things, can be mapped to a number\r\nof types of water reporting areas (depending on the use case) as exemplified by the stable\r\nreporting regions given in Hydrology Reporting Regions." .
<https://www.opengis.net/def/appschema/hy_features/hyf/HY_Catchment> <http://www.w3.org/1999/02/22-rdf-syntax-ns#type> <http://www.w3.org/2002/07/owl#Class> .
<http://linked.data.gov.au/def/geofabric> <http://purl.org/dc/terms/creator> _:B92d492f0c98eddf7582466af474b17fc .
<http://linked.data.gov.au/def/geofabric#ReportingRegion> <http://purl.org/dc/elements/1.1/source> "Section 5.5 Page 44 in the Australian Hydrological Geospatial Fabric (Geofabric) v3.0 Product Guide"@en .
_:Bc0254babce19175c3e91079fc96c0f85 <https://schema.org/name> "CSIRO" .
_:Bc97368400aeef93595f36397b36b90f1 <https://schema.org/identifier> <http://orcid.org/0000-0002-8742-7730> .
<http://linked.data.gov.au/def/geofabric#ContractedCatchment> <http://www.w3.org/2000/01/rdf-schema#subClassOf> <https://www.opengis.net/def/appschema/hy_features/hyf/HY_Catchment> .
<http://linked.data.gov.au/def/geofabric#RiverRegion> <http://www.w3.org/2000/01/rdf-schema#subClassOf> _:B284bc2e7a5f2190407d62828b5105ed7 .
_:B1f7c1c9aa927c7f524b20ab63fa6ab10 <https://schema.org/identifier> <http://orcid.org/0000-0002-8742-7730> .
<http://linked.data.gov.au/def/geofabric> <http://www.w3.org/2000/01/rdf-schema#label> "Geofabric Ontology"@en .
<http://linked.data.gov.au/def/geofabric#RiverRegion> <http://www.w3.org/2000/01/rdf-schema#comment> "The Geofabric's Hydrology Reporting Region product's River Region object.\n\nReporting Regions are derived from aggregations of Contracted Catchments for regional scale reporting purposes.\n\nA River Regions is always within one and only one Drainage Division."@en .
<http://linked.data.gov.au/def/geofabric> <http://purl.org/dc/terms/modified> "2019-07-29"^^<http://www.w3.org/2001/XMLSchema#date> .
<http://linked.data.gov.au/def/geofabric#ReportingRegion> <http://purl.org/dc/elements/1.1/description> "Geofabric Hydrology Reporting Regions are derived from aggregations of contracted\r\ncatchments from Geofabric Hydrology Reporting Catchments. This product contains two\r\ncandidate reporting regions, namely AWRA Drainage Division for national scale reporting\r\npurposes and River Region for regional scale reporting purposes. More reporting regions may\r\nbe added in future releases based on user requirements.\r\n\r\nThe AWRA Drainage Division is defined for the purpose of providing a stable set of reporting\r\nregions specifically for the purpose of the Bureau’s Australian Water Resources Assessment\r\nand are referred to as the 2010 and 2012 Assessment Reporting Regions.\r\n\r\nThe River Regions were based on a specification developed by Bureau hydrologists involved in\r\nwater resources assessment in consultation with the Geofabric team and scientists from\r\nCSIRO and ANU. These boundaries were developed for use in regional scale reporting and\r\nhydrological modelling. The River Region boundaries were not used in the Australian Water\r\nResources Assessment 2010 and 2012 but may be considered in the future as the resolution\r\nof reporting increases.\r\n\r\nThough the Geofabric Hydrology Reporting Regions have been developed for the purposes of\r\nthe Australian Water Resources Assessment, it is envisaged that these units can be used more\r\ngenerally as a standard for hydrological reporting at the national and regional scale, and thus\r\nreplace the Australia River Basins 1997 (http://www.ga.gov.au/metadatagateway/metadata/record/gcat_42343).\r\nTable 31 shows the Geofabric Hydrology Reporting Regions feature class terminology and\r\nfeature subtypes. " .
_:B92d492f0c98eddf7582466af474b17fc <https://schema.org/identifier> <http://orcid.org/0000-0002-8742-7730> .
<http://linked.data.gov.au/def/geofabric#ReportingRegion> <http://www.w3.org/1999/02/22-rdf-syntax-ns#type> <http://www.w3.org/2002/07/owl#Class> .
_:B680b1aafe8be8d4b4b6ddb06a1024273 <https://schema.org/identifier> <http://catalogue.linked.data.gov.au/org/csiro> .
<http://linked.data.gov.au/def/geofabric#ContractedCatchment> <http://www.w3.org/2000/01/rdf-schema#subClassOf> <http://www.opengis.net/ont/geosparql#Feature> .
<http://linked.data.gov.au/def/geofabric> <http://www.w3.org/2000/01/rdf-schema#seeAlso> <http://www.bom.gov.au/water/geofabric/documents/v2_1/AHGF_GDB_ProductRelationships_V2_1_release.pdf> .
<http://linked.data.gov.au/def/geofabric> <http://purl.org/dc/terms/source> <http://www.bom.gov.au/water/geofabric/documents/v3_0/ahgf_productguide_V3_0_release.pdf> .
<https://www.opengis.net/def/appschema/hy_features/hyf/HY_CatchmentAggregate> <http://www.w3.org/1999/02/22-rdf-syntax-ns#type> <http://www.w3.org/2002/07/owl#Class> .
_:Bc1f6687f9ead4d0676f6a4ddb05d8c5c <https://schema.org/identifier> <http://orcid.org/0000-0002-8742-7730> .
<http://linked.data.gov.au/def/geofabric> <http://www.w3.org/2002/07/owl#versionIRI> <http://linked.data.gov.au/def/geofabric/1.0> .
<http://linked.data.gov.au/def/geofabric#DrainageDivision> <http://purl.org/dc/elements/1.1/description> "The AWRA Drainage Division is defined for the purpose of providing a stable set of reporting\r\nregions specifically for the purpose of the Bureau’s Australian Water Resources Assessment\r\nand are referred to as the 2010 and 2012 Assessment Reporting Regions." .
_:B187c66ed7b9f4b7f5f5313e69b20a48b <https://schema.org/identifier> <http://catalogue.linked.data.gov.au/org/csiro> .
_:B738f77d6e389fb671d376b9d1754f146 <http://www.w3.org/2002/07/owl#onClass> <http://linked.data.gov.au/def/geofabric#RiverRegion> .
<https://www.opengis.net/def/appschema/hy_features/hyf/HY_CatchmentAggregate> <http://www.w3.org/2000/01/rdf-schema#label> "Catchment Aggregate" .
_:Bd06b23f60a1f5897e137e7832491c0ed <https://schema.org/name> "CSIRO" .
