<http://vocabularies.wikipathways.org/gpml#textlabel>
        a       <http://www.w3.org/2002/07/owl#DatatypeProperty> ;
        <http://www.w3.org/2000/01/rdf-schema#comment>
                "TextLabel of an object (DataNode, Group, Label, Shape, State)."@en ;
        <http://www.w3.org/2000/01/rdf-schema#label>
                "textlabel"@en ;
        <http://www.w3.org/2000/01/rdf-schema#range>
                <http://vocabularies.wikipathways.org/gpml#Label> , <http://vocabularies.wikipathways.org/gpml#Shape> , <http://vocabularies.wikipathways.org/gpml#Group> , <http://vocabularies.wikipathways.org/gpml#DataNode> , <http://vocabularies.wikipathways.org/gpml#State> , <http://www.w3.org/2001/XMLSchema#string> ;
        <http://www.w3.org/2004/02/skos/core#inScheme>
                <http://vocabularies.wikipathways.org/gpml#> .

<http://vocabularies.wikipathways.org/gpml#width>
        a       <http://www.w3.org/2002/07/owl#DatatypeProperty> ;
        <http://www.w3.org/2000/01/rdf-schema#comment>
                "The pixel value for the x-dimensional length of a given object."@en ;
        <http://www.w3.org/2000/01/rdf-schema#label>
                "width"@en ;
        <http://www.w3.org/2000/01/rdf-schema#range>
                <http://vocabularies.wikipathways.org/gpml#Shape> , <http://www.w3.org/2001/XMLSchema#float> , <http://vocabularies.wikipathways.org/gpml#Label> , <http://vocabularies.wikipathways.org/gpml#State> , <http://vocabularies.wikipathways.org/gpml#DataNode> ;
        <http://www.w3.org/2004/02/skos/core#inScheme>
                <http://vocabularies.wikipathways.org/gpml#> .

<http://vocabularies.wikipathways.org/gpml#hasComment>
        a       <http://www.w3.org/2002/07/owl#ObjectProperty> ;
        <http://www.w3.org/2000/01/rdf-schema#comment>
                "Boolean property for the existence of a Comment class associated with a given object."@en ;
        <http://www.w3.org/2000/01/rdf-schema#label>
                "hasComment"@en ;
        <http://www.w3.org/2000/01/rdf-schema#range>
                <http://vocabularies.wikipathways.org/gpml#Shape> , <http://vocabularies.wikipathways.org/gpml#Group> , <http://vocabularies.wikipathways.org/gpml#Interaction> , <http://vocabularies.wikipathways.org/gpml#Label> , <http://vocabularies.wikipathways.org/gpml#GraphicalLine> , <http://vocabularies.wikipathways.org/gpml#State> , <http://vocabularies.wikipathways.org/gpml#Pathway> , <http://vocabularies.wikipathways.org/gpml#DataNode> , <http://vocabularies.wikipathways.org/gpml#Comment> ;
        <http://www.w3.org/2004/02/skos/core#inScheme>
                <http://vocabularies.wikipathways.org/gpml#> .

<http://vocabularies.wikipathways.org/gpml#centerY>
        a       <http://www.w3.org/2002/07/owl#DatatypeProperty> ;
        <http://www.w3.org/2000/01/rdf-schema#comment>
                "Middle of a pathway element in the y-direction."@en ;
        <http://www.w3.org/2000/01/rdf-schema#label>
                "centerY"@en ;
        <http://www.w3.org/2000/01/rdf-schema#range>
                <http://vocabularies.wikipathways.org/gpml#Label> , <http://www.w3.org/2001/XMLSchema#float> , <http://vocabularies.wikipathways.org/gpml#Legend> , <http://vocabularies.wikipathways.org/gpml#Shape> , <http://vocabularies.wikipathways.org/gpml#InfoBox> , <http://vocabularies.wikipathways.org/gpml#DataNode> ;
        <http://www.w3.org/2004/02/skos/core#inScheme>
                <http://vocabularies.wikipathways.org/gpml#> .

<http://vocabularies.wikipathways.org/gpml#centerX>
        a       <http://www.w3.org/2002/07/owl#DatatypeProperty> ;
        <http://www.w3.org/2000/01/rdf-schema#comment>
                "Middle of a pathway element in the x-direction."@en ;
        <http://www.w3.org/2000/01/rdf-schema#label>
                "centerX"@en ;
        <http://www.w3.org/2000/01/rdf-schema#range>
                <http://vocabularies.wikipathways.org/gpml#Label> , <http://www.w3.org/2001/XMLSchema#float> , <http://vocabularies.wikipathways.org/gpml#Legend> , <http://vocabularies.wikipathways.org/gpml#Shape> , <http://vocabularies.wikipathways.org/gpml#InfoBox> , <http://vocabularies.wikipathways.org/gpml#DataNode> ;
        <http://www.w3.org/2004/02/skos/core#inScheme>
                <http://vocabularies.wikipathways.org/gpml#> .

<http://vocabularies.wikipathways.org/gpml#hasBiopax>
        a       <http://www.w3.org/2002/07/owl#ObjectProperty> ;
        <http://www.w3.org/2000/01/rdf-schema#comment>
                "Boolean property for the existence of a BioPax class associated with a given pathway."@en ;
        <http://www.w3.org/2000/01/rdf-schema#label>
                "hasBiopax"@en ;
        <http://www.w3.org/2000/01/rdf-schema#range>
                <http://vocabularies.wikipathways.org/gpml#Pathway> , <http://vocabularies.wikipathways.org/gpml#Biopax> ;
        <http://www.w3.org/2004/02/skos/core#inScheme>
                <http://vocabularies.wikipathways.org/gpml#> .

<http://vocabularies.wikipathways.org/gpml#href>
        a       <http://www.w3.org/2002/07/owl#DatatypeProperty> ;
        <http://www.w3.org/2000/01/rdf-schema#comment>
                "The hyperlink optionally specified in a Label."@en ;
        <http://www.w3.org/2000/01/rdf-schema#label>
                "href"@en ;
        <http://www.w3.org/2000/01/rdf-schema#range>
                <http://vocabularies.wikipathways.org/gpml#Label> , <http://www.w3.org/2001/XMLSchema#string> ;
        <http://www.w3.org/2004/02/skos/core#inScheme>
                <http://vocabularies.wikipathways.org/gpml#> .

<http://vocabularies.wikipathways.org/gpml#lineThickness>
        a       <http://www.w3.org/2002/07/owl#DatatypeProperty> ;
        <http://www.w3.org/2000/01/rdf-schema#comment>
                "The pixel value for the width of a given line, interaction or border."@en ;
        <http://www.w3.org/2000/01/rdf-schema#label>
                "lineThickness"@en ;
        <http://www.w3.org/2000/01/rdf-schema#range>
                <http://vocabularies.wikipathways.org/gpml#Shape> , <http://vocabularies.wikipathways.org/gpml#Interaction> , <http://vocabularies.wikipathways.org/gpml#Label> , <http://vocabularies.wikipathways.org/gpml#GraphicalLine> , <http://www.w3.org/2001/XMLSchema#string> , <http://vocabularies.wikipathways.org/gpml#State> , <http://vocabularies.wikipathways.org/gpml#DataNode> ;
        <http://www.w3.org/2004/02/skos/core#inScheme>
                <http://vocabularies.wikipathways.org/gpml#> .

<http://vocabularies.wikipathways.org/gpml#graphId>
        a       <http://www.w3.org/2002/07/owl#DatatypeProperty> ;
        <http://www.w3.org/2000/01/rdf-schema#comment>
                "A GraphId is a unique (per Pathway) identifier for a pathway element, such as DataNode, Interaction, GraphicalLine, Label, Point, Group, Shape, State and Anchor."@en ;
        <http://www.w3.org/2000/01/rdf-schema#label>
                "graphId"@en ;
        <http://www.w3.org/2000/01/rdf-schema#range>
                <http://vocabularies.wikipathways.org/gpml#Shape> , <http://vocabularies.wikipathways.org/gpml#Anchor> , <http://vocabularies.wikipathways.org/gpml#Group> , <http://vocabularies.wikipathways.org/gpml#Point> , <http://vocabularies.wikipathways.org/gpml#Interaction> , <http://vocabularies.wikipathways.org/gpml#Label> , <http://vocabularies.wikipathways.org/gpml#GraphicalLine> , <http://www.w3.org/2001/XMLSchema#string> , <http://vocabularies.wikipathways.org/gpml#State> , <http://vocabularies.wikipathways.org/gpml#DataNode> ;
        <http://www.w3.org/2004/02/skos/core#inScheme>
                <http://vocabularies.wikipathways.org/gpml#> .

<http://vocabularies.wikipathways.org/gpml#Label>
        a       <http://www.w3.org/2002/07/owl#Class> ;
        <http://www.w3.org/2000/01/rdf-schema#Label>
                "Label"@en ;
        <http://www.w3.org/2000/01/rdf-schema#comment>
                "A text field which can be used to annotate any aspect of a pathway."@en ;
        <http://www.w3.org/2004/02/skos/core#inScheme>
                <http://vocabularies.wikipathways.org/gpml#> .

<http://vocabularies.wikipathways.org/gpml#DataNode>
        a       <http://www.w3.org/2002/07/owl#Class> ;
        <http://www.w3.org/2000/01/rdf-schema#comment>
                "Denotes a biological entity that forms a node in a pathway and has some biological meaning associated with it. For a list of the gpml:DataNode types supported at WikiPathways, see subclasses of wp:DataNode or the wpTypes vocabulary defined for use in applications.."@en ;
        <http://www.w3.org/2000/01/rdf-schema#label>
                "DataNode"@en ;
        <http://www.w3.org/2004/02/skos/core#inScheme>
                <http://vocabularies.wikipathways.org/gpml#> .

<http://vocabularies.wikipathways.org/gpml#color>
        a       <http://www.w3.org/2002/07/owl#DatatypeProperty> ;
        <http://www.w3.org/2000/01/rdf-schema#comment>
                "The color to be used for visualization."@en ;
        <http://www.w3.org/2000/01/rdf-schema#label>
                "color"@en ;
        <http://www.w3.org/2000/01/rdf-schema#range>
                <http://vocabularies.wikipathways.org/gpml#DataNode> , <http://vocabularies.wikipathways.org/gpml#State> , <http://www.w3.org/2001/XMLSchema#hexBinary> , <http://vocabularies.wikipathways.org/gpml#Shape> , <http://vocabularies.wikipathways.org/gpml#GraphicalLine> , <http://vocabularies.wikipathways.org/gpml#Label> , <http://vocabularies.wikipathways.org/gpml#Interaction> ;
        <http://www.w3.org/2004/02/skos/core#inScheme>
                <http://vocabularies.wikipathways.org/gpml#> .

<http://vocabularies.wikipathways.org/gpml#connectorType>
        a       <http://www.w3.org/2002/07/owl#DatatypeProperty> ;
        <http://www.w3.org/2000/01/rdf-schema#comment>
                "Specifies a set of rules to govern layout of Graphical Lines and Interactions.  PathVisio (Java): Line Type and GPML: ConnectorType"@en ;
        <http://www.w3.org/2000/01/rdf-schema#label>
                "connectorType"@en ;
        <http://www.w3.org/2000/01/rdf-schema#range>
                <http://vocabularies.wikipathways.org/gpml#Interaction> , <http://vocabularies.wikipathways.org/gpml#GraphicalLine> , <http://www.w3.org/2001/XMLSchema#string> ;
        <http://www.w3.org/2004/02/skos/core#inScheme>
                <http://vocabularies.wikipathways.org/gpml#> .

<http://vocabularies.wikipathways.org/gpml#style>
        a       <http://www.w3.org/2002/07/owl#DatatypeProperty> ;
        <http://www.w3.org/2000/01/rdf-schema#comment>
                "The type of Group, e.g., Complex."@en ;
        <http://www.w3.org/2000/01/rdf-schema#label>
                "style"@en ;
        <http://www.w3.org/2000/01/rdf-schema#range>
                <http://vocabularies.wikipathways.org/gpml#Group> , <http://www.w3.org/2001/XMLSchema#string> ;
        <http://www.w3.org/2004/02/skos/core#inScheme>
                <http://vocabularies.wikipathways.org/gpml#> .

<http://vocabularies.wikipathways.org/gpml#value>
        a       <http://www.w3.org/2002/07/owl#DatatypeProperty> ;
        <http://www.w3.org/2000/01/rdf-schema#comment>
                "Value of the key/value pair in the Attribute class."@en ;
        <http://www.w3.org/2000/01/rdf-schema#label>
                "value"@en ;
        <http://www.w3.org/2000/01/rdf-schema#range>
                <http://www.w3.org/2001/XMLSchema#string> , <http://vocabularies.wikipathways.org/gpml#Attribute> ;
        <http://www.w3.org/2004/02/skos/core#inScheme>
                <http://vocabularies.wikipathways.org/gpml#> .

<http://vocabularies.wikipathways.org/gpml#height>
        a       <http://www.w3.org/2002/07/owl#DatatypeProperty> ;
        <http://www.w3.org/2000/01/rdf-schema#comment>
                "The pixel value for the y-dimensional length of a given object."@en ;
        <http://www.w3.org/2000/01/rdf-schema#label>
                "height"@en ;
        <http://www.w3.org/2000/01/rdf-schema#range>
                <http://vocabularies.wikipathways.org/gpml#Shape> , <http://www.w3.org/2001/XMLSchema#float> , <http://vocabularies.wikipathways.org/gpml#Label> , <http://vocabularies.wikipathways.org/gpml#State> , <http://vocabularies.wikipathways.org/gpml#DataNode> ;
        <http://www.w3.org/2004/02/skos/core#inScheme>
                <http://vocabularies.wikipathways.org/gpml#> .

<http://vocabularies.wikipathways.org/gpml#hasAttribute>
        a       <http://www.w3.org/2002/07/owl#ObjectProperty> ;
        <http://www.w3.org/2000/01/rdf-schema#comment>
                "Boolean property for the existence of an Attribute class associated with a given object."@en ;
        <http://www.w3.org/2000/01/rdf-schema#label>
                "hasAttribute"@en ;
        <http://www.w3.org/2000/01/rdf-schema#range>
                <http://vocabularies.wikipathways.org/gpml#Pathway> , <http://vocabularies.wikipathways.org/gpml#DataNode> , <http://vocabularies.wikipathways.org/gpml#State> , <http://vocabularies.wikipathways.org/gpml#Attribute> , <http://vocabularies.wikipathways.org/gpml#Group> , <http://vocabularies.wikipathways.org/gpml#Shape> , <http://vocabularies.wikipathways.org/gpml#GraphicalLine> , <http://vocabularies.wikipathways.org/gpml#Label> , <http://vocabularies.wikipathways.org/gpml#Interaction> ;
        <http://www.w3.org/2004/02/skos/core#inScheme>
                <http://vocabularies.wikipathways.org/gpml#> .

<http://vocabularies.wikipathways.org/gpml#Anchor>
        a       <http://www.w3.org/2002/07/owl#Class> ;
        <http://www.w3.org/2000/01/rdf-schema#comment>
                "A connection point on a graphical line or an interaction, where another graphical line or interaction can be connected."@en ;
        <http://www.w3.org/2000/01/rdf-schema#label>
                "Anchor"@en ;
        <http://www.w3.org/2004/02/skos/core#inScheme>
                <http://vocabularies.wikipathways.org/gpml#> .

<http://vocabularies.wikipathways.org/gpml#groupId>
        a       <http://www.w3.org/2002/07/owl#DatatypeProperty> ;
        <http://www.w3.org/2000/01/rdf-schema#comment>
                "Uniquely identifies a gpml:Group in a gpml:Pathway."@en ;
        <http://www.w3.org/2000/01/rdf-schema#label>
                "groupId"@en ;
        <http://www.w3.org/2000/01/rdf-schema#range>
                <http://www.w3.org/2001/XMLSchema#string> , <http://vocabularies.wikipathways.org/gpml#Group> ;
        <http://www.w3.org/2004/02/skos/core#inScheme>
                <http://vocabularies.wikipathways.org/gpml#> .

<http://vocabularies.wikipathways.org/gpml#hasLegend>
        a       <http://www.w3.org/2002/07/owl#ObjectProperty> ;
        <http://www.w3.org/2000/01/rdf-schema#comment>
                "Boolean property for the existence of a Legend in a given pathway."@en ;
        <http://www.w3.org/2000/01/rdf-schema#label>
                "hasLegend"@en ;
        <http://www.w3.org/2000/01/rdf-schema#range>
                <http://vocabularies.wikipathways.org/gpml#Legend> , <http://vocabularies.wikipathways.org/gpml#Pathway> ;
        <http://www.w3.org/2004/02/skos/core#inScheme>
                <http://vocabularies.wikipathways.org/gpml#> .

<http://vocabularies.wikipathways.org/gpml#lineStyle>
        a       <http://www.w3.org/2002/07/owl#DatatypeProperty> ;
        <http://www.w3.org/2000/01/rdf-schema#comment>
                "The visual appearance of a line or border, e.g., Solid or Broken."@en ;
        <http://www.w3.org/2000/01/rdf-schema#label>
                "lineStyle"@en ;
        <http://www.w3.org/2000/01/rdf-schema#range>
                <http://vocabularies.wikipathways.org/gpml#Shape> , <http://vocabularies.wikipathways.org/gpml#Interaction> , <http://vocabularies.wikipathways.org/gpml#GraphicalLine> , <http://vocabularies.wikipathways.org/gpml#Label> , <http://vocabularies.wikipathways.org/gpml#State> , <http://www.w3.org/2001/XMLSchema#string> , <http://vocabularies.wikipathways.org/gpml#DataNode> ;
        <http://www.w3.org/2004/02/skos/core#inScheme>
                <http://vocabularies.wikipathways.org/gpml#> .

<http://vocabularies.wikipathways.org/gpml#maintainer>
        a       <http://www.w3.org/2002/07/owl#DatatypeProperty> ;
        <http://www.w3.org/2000/01/rdf-schema#comment>
                "The maintainer of the pathway. Currently not used in WP."@en ;
        <http://www.w3.org/2000/01/rdf-schema#label>
                "maintainer"@en ;
        <http://www.w3.org/2000/01/rdf-schema#range>
                <http://www.w3.org/2001/XMLSchema#string> , <http://vocabularies.wikipathways.org/gpml#Pathway> ;
        <http://www.w3.org/2004/02/skos/core#inScheme>
                <http://vocabularies.wikipathways.org/gpml#> .

<http://vocabularies.wikipathways.org/gpml#Group>
        a       <http://www.w3.org/2002/07/owl#Class> ;
        <http://www.w3.org/2000/01/rdf-schema#comment>
                "A collection of structurally or functionally similar or related pathway elements."@en ;
        <http://www.w3.org/2000/01/rdf-schema#label>
                "Group"@en ;
        <http://www.w3.org/2004/02/skos/core#inScheme>
                <http://vocabularies.wikipathways.org/gpml#> .

<http://vocabularies.wikipathways.org/gpml#hasInfoBox>
        a       <http://www.w3.org/2002/07/owl#ObjectProperty> ;
        <http://www.w3.org/2000/01/rdf-schema#comment>
                "Boolean property for the existence of an InfroBox in a given pathway."@en ;
        <http://www.w3.org/2000/01/rdf-schema#label>
                "hasInfoBox"@en ;
        <http://www.w3.org/2000/01/rdf-schema#range>
                <http://vocabularies.wikipathways.org/gpml#Pathway> , <http://vocabularies.wikipathways.org/gpml#InfoBox> ;
        <http://www.w3.org/2004/02/skos/core#inScheme>
                <http://vocabularies.wikipathways.org/gpml#> .

<http://vocabularies.wikipathways.org/gpml#fontStyle>
        a       <http://www.w3.org/2002/07/owl#DatatypeProperty> ;
        <http://www.w3.org/2000/01/rdf-schema#comment>
                "The typographic style or font face applied to displayed text, e.g., Arial."@en ;
        <http://www.w3.org/2000/01/rdf-schema#label>
                "fontStyle"@en ;
        <http://www.w3.org/2000/01/rdf-schema#range>
                <http://vocabularies.wikipathways.org/gpml#DataNode> , <http://www.w3.org/2001/XMLSchema#string> , <http://vocabularies.wikipathways.org/gpml#Shape> , <http://vocabularies.wikipathways.org/gpml#Label> ;
        <http://www.w3.org/2004/02/skos/core#inScheme>
                <http://vocabularies.wikipathways.org/gpml#> .

<http://vocabularies.wikipathways.org/gpml#type>
        a       <http://www.w3.org/2002/07/owl#DatatypeProperty> ;
        <http://www.w3.org/2000/01/rdf-schema#comment>
                "Specifies the type of an object (DataNode, GraphicalLine, Interaction)."@en ;
        <http://www.w3.org/2000/01/rdf-schema#label>
                "type"@en ;
        <http://www.w3.org/2000/01/rdf-schema#range>
                <http://vocabularies.wikipathways.org/gpml#GraphicalLine> , <http://vocabularies.wikipathways.org/gpml#Interaction> , <http://vocabularies.wikipathways.org/gpml#DataNode> , <http://www.w3.org/2001/XMLSchema#string> ;
        <http://www.w3.org/2004/02/skos/core#inScheme>
                <http://vocabularies.wikipathways.org/gpml#> .

<http://vocabularies.wikipathways.org/gpml#>
        a       <http://www.w3.org/2002/07/owl#Ontology> , <http://www.w3.org/2004/02/skos/core#ConceptScheme> ;
        <http://www.w3.org/2000/01/rdf-schema#label>
                "WikiPathways GPML Vocabulary"@en ;
        <http://www.w3.org/2000/01/rdf-schema#seeAlso>
                <http://www.wikipathways.org/> ;
        <http://www.w3.org/2002/07/owl#versionIRI>
                <http://www.w3.org/2012/pyRdfa/extract?uri=http://vocabularies.wikipathways.org/gpml#> .

<http://vocabularies.wikipathways.org/gpml#author>
        a       <http://www.w3.org/2002/07/owl#DatatypeProperty> ;
        <http://www.w3.org/2000/01/rdf-schema#comment>
                "The person who created or edited the pathway in question."@en ;
        <http://www.w3.org/2000/01/rdf-schema#label>
                "author"@en ;
        <http://www.w3.org/2000/01/rdf-schema#range>
                <http://www.w3.org/2001/XMLSchema#string> , <http://vocabularies.wikipathways.org/gpml#Pathway> ;
        <http://www.w3.org/2004/02/skos/core#inScheme>
                <http://vocabularies.wikipathways.org/gpml#> .

<http://vocabularies.wikipathways.org/gpml#zorder>
        a       <http://www.w3.org/2002/07/owl#DatatypeProperty> ;
        <http://www.w3.org/2000/01/rdf-schema#comment>
                "Indicates the zorder of the object in the pathway."@en ;
        <http://www.w3.org/2000/01/rdf-schema#label>
                "zorder"@en ;
        <http://www.w3.org/2000/01/rdf-schema#range>
                <http://vocabularies.wikipathways.org/gpml#State> , <http://vocabularies.wikipathways.org/gpml#DataNode> , <http://vocabularies.wikipathways.org/gpml#Interaction> , <http://vocabularies.wikipathways.org/gpml#Label> , <http://vocabularies.wikipathways.org/gpml#GraphicalLine> , <http://vocabularies.wikipathways.org/gpml#Shape> , <http://www.w3.org/2001/XMLSchema#integer> ;
        <http://www.w3.org/2004/02/skos/core#inScheme>
                <http://vocabularies.wikipathways.org/gpml#> .

<http://vocabularies.wikipathways.org/gpml#name>
        a       <http://www.w3.org/2002/07/owl#DatatypeProperty> ;
        <http://www.w3.org/2000/01/rdf-schema#comment>
                "The name of a pathway."@en ;
        <http://www.w3.org/2000/01/rdf-schema#label>
                "name"@en ;
        <http://www.w3.org/2000/01/rdf-schema#range>
                <http://www.w3.org/2001/XMLSchema#string> , <http://vocabularies.wikipathways.org/gpml#Pathway> ;
        <http://www.w3.org/2004/02/skos/core#inScheme>
                <http://vocabularies.wikipathways.org/gpml#> .

<http://vocabularies.wikipathways.org/gpml#y>
        a       <http://www.w3.org/2002/07/owl#DatatypeProperty> ;
        <http://www.w3.org/2000/01/rdf-schema#comment>
                "The y-coordinate of a point in the 2-dimensional plane in which a pathway is drawn."@en ;
        <http://www.w3.org/2000/01/rdf-schema#label>
                "y"@en ;
        <http://www.w3.org/2000/01/rdf-schema#range>
                <http://vocabularies.wikipathways.org/gpml#Point> , <http://www.w3.org/2001/XMLSchema#float> ;
        <http://www.w3.org/2004/02/skos/core#inScheme>
                <http://vocabularies.wikipathways.org/gpml#> .

<http://vocabularies.wikipathways.org/gpml#Xref>
        a       <http://www.w3.org/2002/07/owl#Class> ;
        <http://www.w3.org/2000/01/rdf-schema#comment>
                "Reference to a database entry that matches the node\nin the pathway. It is a combination of an identifier of the entity and an\nidentifier of the database in which the entity is found."@en ;
        <http://www.w3.org/2000/01/rdf-schema#label>
                "Xref"@en ;
        <http://www.w3.org/2004/02/skos/core#inScheme>
                <http://vocabularies.wikipathways.org/gpml#> .

<http://vocabularies.wikipathways.org/gpml#fontWeight>
        a       <http://www.w3.org/2002/07/owl#DatatypeProperty> ;
        <http://www.w3.org/2000/01/rdf-schema#comment>
                "Thickness of the font used, e.g a bold font would have more weight. Used for DataNodes, Labels and Shapes."@en ;
        <http://www.w3.org/2000/01/rdf-schema#label>
                "fontWeight"@en ;
        <http://www.w3.org/2000/01/rdf-schema#range>
                <http://vocabularies.wikipathways.org/gpml#Shape> , <http://vocabularies.wikipathways.org/gpml#Label> , <http://vocabularies.wikipathways.org/gpml#DataNode> , <http://www.w3.org/2001/XMLSchema#string> ;
        <http://www.w3.org/2004/02/skos/core#inScheme>
                <http://vocabularies.wikipathways.org/gpml#> .

<http://vocabularies.wikipathways.org/gpml#last-Modified>
        a       <http://www.w3.org/2002/07/owl#DatatypeProperty> ;
        <http://www.w3.org/2000/01/rdf-schema#comment>
                "The date of the last modification of the pathway."@en ;
        <http://www.w3.org/2000/01/rdf-schema#label>
                "last-Modified"@en ;
        <http://www.w3.org/2000/01/rdf-schema#range>
                <http://www.w3.org/2001/XMLSchema#string> , <http://vocabularies.wikipathways.org/gpml#Pathway> ;
        <http://www.w3.org/2004/02/skos/core#inScheme>
                <http://vocabularies.wikipathways.org/gpml#> .

<http://vocabularies.wikipathways.org/gpml#align>
        a       <http://www.w3.org/2002/07/owl#DatatypeProperty> ;
        <http://www.w3.org/2000/01/rdf-schema#comment>
                "Horizontal alignment of displayed text, e.g., Left, Center, Right."@en ;
        <http://www.w3.org/2000/01/rdf-schema#label>
                "align"@en ;
        <http://www.w3.org/2000/01/rdf-schema#range>
                <http://vocabularies.wikipathways.org/gpml#DataNode> , <http://www.w3.org/2001/XMLSchema#string> , <http://vocabularies.wikipathways.org/gpml#Shape> , <http://vocabularies.wikipathways.org/gpml#Label> ;
        <http://www.w3.org/2004/02/skos/core#inScheme>
                <http://vocabularies.wikipathways.org/gpml#> .

<http://vocabularies.wikipathways.org/gpml#InfoBox>
        a       <http://www.w3.org/2002/07/owl#Class> ;
        <http://www.w3.org/2000/01/rdf-schema#comment>
                "Currently just a placeholder -- not used."@en ;
        <http://www.w3.org/2000/01/rdf-schema#label>
                "InfoBox"@en ;
        <http://www.w3.org/2004/02/skos/core#inScheme>
                <http://vocabularies.wikipathways.org/gpml#> .

<http://vocabularies.wikipathways.org/gpml#hasDataNode>
        a       <http://www.w3.org/2002/07/owl#ObjectProperty> ;
        <http://www.w3.org/2000/01/rdf-schema#comment>
                "Boolean property for the existence of a DataNode in a given pathway."@en ;
        <http://www.w3.org/2000/01/rdf-schema#label>
                "hasDataNode"@en ;
        <http://www.w3.org/2000/01/rdf-schema#range>
                <http://vocabularies.wikipathways.org/gpml#Pathway> , <http://vocabularies.wikipathways.org/gpml#DataNode> ;
        <http://www.w3.org/2004/02/skos/core#inScheme>
                <http://vocabularies.wikipathways.org/gpml#> .

<http://vocabularies.wikipathways.org/gpml#Interaction>
        a       <http://www.w3.org/2002/07/owl#Class> ;
        <http://www.w3.org/2000/01/rdf-schema#comment>
                "Defines the biochemical relationship between DataNodes or with Anchors on other Interactions. An Xref can be specified for Interactions (in contrast to GraphicalLines)."@en ;
        <http://www.w3.org/2000/01/rdf-schema#label>
                "Interaction"@en ;
        <http://www.w3.org/2004/02/skos/core#inScheme>
                <http://vocabularies.wikipathways.org/gpml#> .

<http://vocabularies.wikipathways.org/gpml#fontSize>
        a       <http://www.w3.org/2002/07/owl#DatatypeProperty> ;
        <http://www.w3.org/2000/01/rdf-schema#comment>
                "The point value for the size of the font."@en ;
        <http://www.w3.org/2000/01/rdf-schema#label>
                "fontSize"@en ;
        <http://www.w3.org/2000/01/rdf-schema#range>
                <http://vocabularies.wikipathways.org/gpml#Label> , <http://vocabularies.wikipathways.org/gpml#Shape> , <http://www.w3.org/2001/XMLSchema#nonNegativeInteger> ;
        <http://www.w3.org/2004/02/skos/core#inScheme>
                <http://vocabularies.wikipathways.org/gpml#> .

<http://vocabularies.wikipathways.org/gpml#shapeType>
        a       <http://www.w3.org/2002/07/owl#DatatypeProperty> ;
        <http://www.w3.org/2000/01/rdf-schema#comment>
                "Currently: Specifies the glyph (graphical representation) to use for GPML elements (DataNode, Label, Shape, State).\n\nProposed: Expand it to also describe Anchors. It should replace the term currently used to specify the graphical representation of an Anchor. The current term is \"Shape,\" which conflicts with the GPML element named \"Shape.\" See details for term \"Shape.\""@en ;
        <http://www.w3.org/2000/01/rdf-schema#label>
                "shapeType"@en ;
        <http://www.w3.org/2000/01/rdf-schema#range>
                <http://vocabularies.wikipathways.org/gpml#Label> , <http://vocabularies.wikipathways.org/gpml#Shape> , <http://vocabularies.wikipathways.org/gpml#DataNode> , <http://www.w3.org/2001/XMLSchema#string> , <http://vocabularies.wikipathways.org/gpml#State> ;
        <http://www.w3.org/2004/02/skos/core#inScheme>
                <http://vocabularies.wikipathways.org/gpml#> .

<http://vocabularies.wikipathways.org/gpml#rotation>
        a       <http://www.w3.org/2002/07/owl#DatatypeProperty> ;
        <http://www.w3.org/2000/01/rdf-schema#comment>
                "The degree value of angular offset relative to the center of a given object."@en ;
        <http://www.w3.org/2000/01/rdf-schema#label>
                "rotation"@en ;
        <http://www.w3.org/2000/01/rdf-schema#range>
                <http://www.w3.org/2001/XMLSchema#float> , <http://vocabularies.wikipathways.org/gpml#Shape> ;
        <http://www.w3.org/2004/02/skos/core#inScheme>
                <http://vocabularies.wikipathways.org/gpml#> .

<http://vocabularies.wikipathways.org/gpml#PublicationXref>
        a       <http://www.w3.org/2002/07/owl#Class> ;
        <http://www.w3.org/2000/01/rdf-schema#comment>
                "Defines a literature reference. Refers to a BioPAX definition."@en ;
        <http://www.w3.org/2000/01/rdf-schema#label>
                "PublicationXref"@en ;
        <http://www.w3.org/2000/01/rdf-schema#seeAlso>
                <http://www.biopax.org/owldoc/Level3/classes/PublicationXref___-1968381200.html> ;
        <http://www.w3.org/2004/02/skos/core#inScheme>
                <http://vocabularies.wikipathways.org/gpml#> .

<http://vocabularies.wikipathways.org/gpml#organism>
        a       <http://www.w3.org/2002/07/owl#DatatypeProperty> ;
        <http://www.w3.org/2000/01/rdf-schema#comment>
                "The scientific name (e.g., Homo sapiens) of the species being described by the pathway."@en ;
        <http://www.w3.org/2000/01/rdf-schema#label>
                "organism"@en ;
        <http://www.w3.org/2000/01/rdf-schema#range>
                <http://vocabularies.wikipathways.org/gpml#Pathway> , <http://www.w3.org/2001/XMLSchema#string> ;
        <http://www.w3.org/2004/02/skos/core#inScheme>
                <http://vocabularies.wikipathways.org/gpml#> .

<http://vocabularies.wikipathways.org/gpml#valign>
        a       <http://www.w3.org/2002/07/owl#DatatypeProperty> ;
        <http://www.w3.org/2000/01/rdf-schema#comment>
                " Vertical alignment of displayed text, e.g., Top, Middle, Bottom."@en ;
        <http://www.w3.org/2000/01/rdf-schema#label>
                "valign"@en ;
        <http://www.w3.org/2000/01/rdf-schema#range>
                <http://vocabularies.wikipathways.org/gpml#Shape> , <http://vocabularies.wikipathways.org/gpml#Label> , <http://vocabularies.wikipathways.org/gpml#DataNode> , <http://www.w3.org/2001/XMLSchema#string> ;
        <http://www.w3.org/2004/02/skos/core#inScheme>
                <http://vocabularies.wikipathways.org/gpml#> .

<http://vocabularies.wikipathways.org/gpml#Pathway>
        a       <http://www.w3.org/2002/07/owl#Class> ;
        <http://www.w3.org/2000/01/rdf-schema#comment>
                "A graph diagram representing a biological process as a set of interactions and relationships among genes, proteins, metabolites, and other factors in the context of cellular compartments, tissues and organisms."@en ;
        <http://www.w3.org/2000/01/rdf-schema#label>
                "Pathway"@en ;
        <http://www.w3.org/2004/02/skos/core#inScheme>
                <http://vocabularies.wikipathways.org/gpml#> .

<http://vocabularies.wikipathways.org/gpml#fontName>
        a       <http://www.w3.org/2002/07/owl#DatatypeProperty> ;
        <http://www.w3.org/2000/01/rdf-schema#comment>
                "The name of the set of printable text characters to be used for visualization."@en ;
        <http://www.w3.org/2000/01/rdf-schema#label>
                "fontName"@en ;
        <http://www.w3.org/2000/01/rdf-schema#range>
                <http://www.w3.org/2001/XMLSchema#string> , <http://vocabularies.wikipathways.org/gpml#Shape> , <http://vocabularies.wikipathways.org/gpml#Label> ;
        <http://www.w3.org/2004/02/skos/core#inScheme>
                <http://vocabularies.wikipathways.org/gpml#> .

<http://vocabularies.wikipathways.org/gpml#database>
        a       <http://www.w3.org/2002/07/owl#DatatypeProperty> ;
        <http://www.w3.org/2000/01/rdf-schema#comment>
                "Specifies the datasource for the identifier provided as an Xref.  Equivalent to http://vocabularies.bridgedb.org/ops#DataSource conventional name ."@en ;
        <http://www.w3.org/2000/01/rdf-schema#label>
                "database"@en ;
        <http://www.w3.org/2000/01/rdf-schema#range>
                <http://vocabularies.wikipathways.org/gpml#Xref> , <http://www.w3.org/2001/XMLSchema#string> ;
        <http://www.w3.org/2000/01/rdf-schema#seeAlso>
                <http://vocabularies.bridgedb.org/ops#DataSource> ;
        <http://www.w3.org/2004/02/skos/core#inScheme>
                <http://vocabularies.wikipathways.org/gpml#> .

<http://vocabularies.wikipathways.org/gpml#stateType>
        a       <http://www.w3.org/2002/07/owl#DatatypeProperty> ;
        <http://www.w3.org/2000/01/rdf-schema#comment>
                "A free text field to describe the nature or category of a given state."@en ;
        <http://www.w3.org/2000/01/rdf-schema#label>
                "stateType"@en ;
        <http://www.w3.org/2000/01/rdf-schema#range>
                <http://www.w3.org/2001/XMLSchema#string> , <http://vocabularies.wikipathways.org/gpml#State> ;
        <http://www.w3.org/2004/02/skos/core#inScheme>
                <http://vocabularies.wikipathways.org/gpml#> .

<http://vocabularies.wikipathways.org/gpml#hasGroup>
        a       <http://www.w3.org/2002/07/owl#ObjectProperty> ;
        <http://www.w3.org/2000/01/rdf-schema#comment>
                "Boolean property for the existence of a Group in a given pathway."@en ;
        <http://www.w3.org/2000/01/rdf-schema#label>
                "hasGroup"@en ;
        <http://www.w3.org/2000/01/rdf-schema#range>
                <http://vocabularies.wikipathways.org/gpml#Pathway> , <http://vocabularies.wikipathways.org/gpml#Group> ;
        <http://www.w3.org/2004/02/skos/core#inScheme>
                <http://vocabularies.wikipathways.org/gpml#> .

<http://vocabularies.wikipathways.org/gpml#boardHeight>
        a       <http://www.w3.org/2002/07/owl#DatatypeProperty> ;
        <http://www.w3.org/2000/01/rdf-schema#comment>
                "Range minimum is zero."@en ;
        <http://www.w3.org/2000/01/rdf-schema#label>
                "boardHeight"@en ;
        <http://www.w3.org/2000/01/rdf-schema#range>
                <http://www.w3.org/2001/XMLSchema#float> , <http://vocabularies.wikipathways.org/gpml#Pathway> ;
        <http://www.w3.org/2004/02/skos/core#inScheme>
                <http://vocabularies.wikipathways.org/gpml#> .

<http://vocabularies.wikipathways.org/gpml#key>
        a       <http://www.w3.org/2002/07/owl#DatatypeProperty> ;
        <http://www.w3.org/2000/01/rdf-schema#comment>
                "Key of the key/value pair in the Attribute class."@en ;
        <http://www.w3.org/2000/01/rdf-schema#label>
                "key"@en ;
        <http://www.w3.org/2000/01/rdf-schema#range>
                <http://www.w3.org/2001/XMLSchema#string> , <http://vocabularies.wikipathways.org/gpml#Attribute> ;
        <http://www.w3.org/2004/02/skos/core#inScheme>
                <http://vocabularies.wikipathways.org/gpml#> .

<http://vocabularies.wikipathways.org/gpml#hasShape>
        a       <http://www.w3.org/2002/07/owl#ObjectProperty> ;
        <http://www.w3.org/2000/01/rdf-schema#comment>
                "Boolean property for the existence of a Shape in a given pathway."@en ;
        <http://www.w3.org/2000/01/rdf-schema#label>
                "hasShape"@en ;
        <http://www.w3.org/2000/01/rdf-schema#range>
                <http://vocabularies.wikipathways.org/gpml#Pathway> , <http://vocabularies.wikipathways.org/gpml#Shape> ;
        <http://www.w3.org/2004/02/skos/core#inScheme>
                <http://vocabularies.wikipathways.org/gpml#> .

<http://vocabularies.wikipathways.org/gpml#hasPoint>
        a       <http://www.w3.org/2002/07/owl#ObjectProperty> ;
        <http://www.w3.org/2000/01/rdf-schema#comment>
                "Boolean property for the existence of a Point in a given line or interaction."@en ;
        <http://www.w3.org/2000/01/rdf-schema#label>
                "hasPoint"@en ;
        <http://www.w3.org/2000/01/rdf-schema#range>
                <http://vocabularies.wikipathways.org/gpml#Interaction> , <http://vocabularies.wikipathways.org/gpml#GraphicalLine> , <http://vocabularies.wikipathways.org/gpml#Point> ;
        <http://www.w3.org/2004/02/skos/core#inScheme>
                <http://vocabularies.wikipathways.org/gpml#> .

<http://vocabularies.wikipathways.org/gpml#State>
        a       <http://www.w3.org/2002/07/owl#Class> ;
        <http://www.w3.org/2000/01/rdf-schema#comment>
                "A particular condition, mode or modification of an entity, e.g., phosphorylated, activated, mutated, SNP, etc."@en ;
        <http://www.w3.org/2000/01/rdf-schema#label>
                "State"@en ;
        <http://www.w3.org/2004/02/skos/core#inScheme>
                <http://vocabularies.wikipathways.org/gpml#> .

<http://vocabularies.wikipathways.org/gpml#hasState>
        a       <http://www.w3.org/2002/07/owl#ObjectProperty> ;
        <http://www.w3.org/2000/01/rdf-schema#comment>
                "Boolean property for the existence of a State in a given pathway."@en ;
        <http://www.w3.org/2000/01/rdf-schema#label>
                "hasState"@en ;
        <http://www.w3.org/2000/01/rdf-schema#range>
                <http://vocabularies.wikipathways.org/gpml#Pathway> , <http://vocabularies.wikipathways.org/gpml#State> ;
        <http://www.w3.org/2004/02/skos/core#inScheme>
                <http://vocabularies.wikipathways.org/gpml#> .

<http://vocabularies.wikipathways.org/gpml#Attribute>
        a       <http://www.w3.org/2002/07/owl#Class> ;
        <http://www.w3.org/2000/01/rdf-schema#comment>
                "Element used to specify key/value paired information for a given object."@en ;
        <http://www.w3.org/2000/01/rdf-schema#label>
                "Attribute"@en ;
        <http://www.w3.org/2004/02/skos/core#inScheme>
                <http://vocabularies.wikipathways.org/gpml#> .

<http://vocabularies.wikipathways.org/gpml#email>
        a       <http://www.w3.org/2002/07/owl#DatatypeProperty> ;
        <http://www.w3.org/2000/01/rdf-schema#comment>
                "Deprecated: An electronic mail address. Used to reference the author or maintainer of a pathway prior to WikiPathways."@en ;
        <http://www.w3.org/2000/01/rdf-schema#label>
                "email"@en ;
        <http://www.w3.org/2000/01/rdf-schema#range>
                <http://vocabularies.wikipathways.org/gpml#Pathway> , <http://www.w3.org/2001/XMLSchema#string> ;
        <http://www.w3.org/2004/02/skos/core#inScheme>
                <http://vocabularies.wikipathways.org/gpml#> .

<http://vocabularies.wikipathways.org/gpml#Point>
        a       <http://www.w3.org/2002/07/owl#Class> ;
        <http://www.w3.org/2000/01/rdf-schema#comment>
                "A location in 2-dimensional space defined by x and y coordinates."@en ;
        <http://www.w3.org/2000/01/rdf-schema#label>
                "Point"@en ;
        <http://www.w3.org/2004/02/skos/core#inScheme>
                <http://vocabularies.wikipathways.org/gpml#> .

<http://vocabularies.wikipathways.org/gpml#hasAnchor>
        a       <http://www.w3.org/2002/07/owl#ObjectProperty> ;
        <http://www.w3.org/2000/01/rdf-schema#comment>
                "Boolean property for the existence of an Anchor on a given line or interaction."@en ;
        <http://www.w3.org/2000/01/rdf-schema#label>
                "hasAnchor"@en ;
        <http://www.w3.org/2000/01/rdf-schema#range>
                <http://vocabularies.wikipathways.org/gpml#Anchor> , <http://vocabularies.wikipathways.org/gpml#GraphicalLine> , <http://vocabularies.wikipathways.org/gpml#Interaction> ;
        <http://www.w3.org/2004/02/skos/core#inScheme>
                <http://vocabularies.wikipathways.org/gpml#> .

<http://vocabularies.wikipathways.org/gpml#Shape>
        a       <http://www.w3.org/2002/07/owl#Class> ;
        <http://www.w3.org/2000/01/rdf-schema#comment>
                "Shape can refer to two different things in GPML, both of which are associated with graphical elements."@en ;
        <http://www.w3.org/2000/01/rdf-schema#label>
                "Shape"@en ;
        <http://www.w3.org/2004/02/skos/core#inScheme>
                <http://vocabularies.wikipathways.org/gpml#> .

<http://vocabularies.wikipathways.org/gpml#hasLabel>
        a       <http://www.w3.org/2002/07/owl#ObjectProperty> ;
        <http://www.w3.org/2000/01/rdf-schema#comment>
                "Boolean property for the existence of a Label in a given pathway."@en ;
        <http://www.w3.org/2000/01/rdf-schema#label>
                "hasLabel"@en ;
        <http://www.w3.org/2000/01/rdf-schema#range>
                <http://vocabularies.wikipathways.org/gpml#Pathway> , <http://vocabularies.wikipathways.org/gpml#Label> ;
        <http://www.w3.org/2004/02/skos/core#inScheme>
                <http://vocabularies.wikipathways.org/gpml#> .

<http://vocabularies.wikipathways.org/gpml#hasXref>
        a       <http://www.w3.org/2002/07/owl#ObjectProperty> ;
        <http://www.w3.org/2000/01/rdf-schema#comment>
                "Boolean property for the existence of an Xref associated with a given object."@en ;
        <http://www.w3.org/2000/01/rdf-schema#label>
                "hasXref"@en ;
        <http://www.w3.org/2000/01/rdf-schema#range>
                <http://vocabularies.wikipathways.org/gpml#Interaction> , <http://vocabularies.wikipathways.org/gpml#DataNode> , <http://vocabularies.wikipathways.org/gpml#State> , <http://vocabularies.wikipathways.org/gpml#Xref> ;
        <http://www.w3.org/2004/02/skos/core#inScheme>
                <http://vocabularies.wikipathways.org/gpml#> .

<http://vocabularies.wikipathways.org/gpml#id>
        a       <http://www.w3.org/2002/07/owl#DatatypeProperty> ;
        <http://www.w3.org/2000/01/rdf-schema#comment>
                "The identifier of a PublicationXref or Xref object."@en ;
        <http://www.w3.org/2000/01/rdf-schema#label>
                "id"@en ;
        <http://www.w3.org/2000/01/rdf-schema#range>
                <http://vocabularies.wikipathways.org/gpml#Xref> , <http://www.w3.org/2001/XMLSchema#string> , <http://vocabularies.wikipathways.org/gpml#PublicationXref> ;
        <http://www.w3.org/2000/01/rdf-schema#seeAlso>
                <http://www.biopax.org/release/biopax-level3.owl#id> ;
        <http://www.w3.org/2004/02/skos/core#inScheme>
                <http://vocabularies.wikipathways.org/gpml#> .

<http://vocabularies.wikipathways.org/gpml#source>
        a       <http://www.w3.org/2002/07/owl#DatatypeProperty> ;
        <http://www.w3.org/2000/01/rdf-schema#comment>
                "The author, reference or category of a comment. Used to help parse pathway-level comments, e.g., the descriptions displayed at WikiPathways.org are comments with source=\"WikiPathways-description\"."@en ;
        <http://www.w3.org/2000/01/rdf-schema#label>
                "source"@en ;
        <http://www.w3.org/2000/01/rdf-schema#range>
                <http://www.w3.org/2001/XMLSchema#string> , <http://vocabularies.wikipathways.org/gpml#Commnet> ;
        <http://www.w3.org/2004/02/skos/core#inScheme>
                <http://vocabularies.wikipathways.org/gpml#> .

<http://vocabularies.wikipathways.org/gpml#fillColor>
        a       <http://www.w3.org/2002/07/owl#DatatypeProperty> ;
        <http://www.w3.org/2000/01/rdf-schema#comment>
                "The hexidecimal color value used to paint the area of an object, not including its border."@en ;
        <http://www.w3.org/2000/01/rdf-schema#label>
                "fillColor"@en ;
        <http://www.w3.org/2000/01/rdf-schema#range>
                <http://vocabularies.wikipathways.org/gpml#Label> , <http://vocabularies.wikipathways.org/gpml#Shape> , <http://www.w3.org/2001/XMLSchema#hexBinary> , <http://vocabularies.wikipathways.org/gpml#State> , <http://vocabularies.wikipathways.org/gpml#DataNode> ;
        <http://www.w3.org/2004/02/skos/core#inScheme>
                <http://vocabularies.wikipathways.org/gpml#> .

<http://vocabularies.wikipathways.org/gpml#groupRef>
        a       <http://www.w3.org/2002/07/owl#DatatypeProperty> ;
        <http://www.w3.org/2000/01/rdf-schema#comment>
                "A GroupRef indicates that its element is part of the gpml:Group with the specified GroupId.\nDataNode, GraphicalLine, Group, Interaction, Label and Shape can be part of a group."@en ;
        <http://www.w3.org/2000/01/rdf-schema#label>
                "groupRef"@en ;
        <http://www.w3.org/2000/01/rdf-schema#range>
                <http://www.w3.org/2001/XMLSchema#string> , <http://vocabularies.wikipathways.org/gpml#DataNode> , <http://vocabularies.wikipathways.org/gpml#Interaction> , <http://vocabularies.wikipathways.org/gpml#GraphicalLine> , <http://vocabularies.wikipathways.org/gpml#Label> , <http://vocabularies.wikipathways.org/gpml#Group> , <http://vocabularies.wikipathways.org/gpml#Shape> ;
        <http://www.w3.org/2004/02/skos/core#inScheme>
                <http://vocabularies.wikipathways.org/gpml#> .

<http://vocabularies.wikipathways.org/gpml#license>
        a       <http://www.w3.org/2002/07/owl#DatatypeProperty> ;
        <http://www.w3.org/2000/01/rdf-schema#comment>
                "The license of a pathway."@en ;
        <http://www.w3.org/2000/01/rdf-schema#label>
                "license"@en ;
        <http://www.w3.org/2000/01/rdf-schema#range>
                <http://vocabularies.wikipathways.org/gpml#Pathway> , <http://www.w3.org/2001/XMLSchema#string> ;
        <http://www.w3.org/2004/02/skos/core#inScheme>
                <http://vocabularies.wikipathways.org/gpml#> .

<http://vocabularies.wikipathways.org/gpml#fontStrikethru>
        a       <http://www.w3.org/2002/07/owl#DatatypeProperty> ;
        <http://www.w3.org/2000/01/rdf-schema#comment>
                "Deprecated: Not in use."@en ;
        <http://www.w3.org/2000/01/rdf-schema#label>
                "fontStrikethru"@en ;
        <http://www.w3.org/2000/01/rdf-schema#range>
                <http://vocabularies.wikipathways.org/gpml#Label> , <http://vocabularies.wikipathways.org/gpml#Shape> , <http://www.w3.org/2001/XMLSchema#string> , <http://vocabularies.wikipathways.org/gpml#DataNode> ;
        <http://www.w3.org/2004/02/skos/core#inScheme>
                <http://vocabularies.wikipathways.org/gpml#> .

<http://vocabularies.wikipathways.org/gpml#hasInteraction>
        a       <http://www.w3.org/2002/07/owl#ObjectProperty> ;
        <http://www.w3.org/2000/01/rdf-schema#comment>
                "Boolean property for the existence of an Interaction in a given pathway."@en ;
        <http://www.w3.org/2000/01/rdf-schema#label>
                "hasInteraction"@en ;
        <http://www.w3.org/2000/01/rdf-schema#range>
                <http://vocabularies.wikipathways.org/gpml#Pathway> , <http://vocabularies.wikipathways.org/gpml#Interaction> ;
        <http://www.w3.org/2004/02/skos/core#inScheme>
                <http://vocabularies.wikipathways.org/gpml#> .

<http://vocabularies.wikipathways.org/gpml#Comment>
        a       <http://www.w3.org/2002/07/owl#Class> ;
        <http://www.w3.org/2000/01/rdf-schema#comment>
                "Elements used to provide descriptions and arbitrary notes for a given object."@en ;
        <http://www.w3.org/2000/01/rdf-schema#label>
                "Comment"@en ;
        <http://www.w3.org/2004/02/skos/core#inScheme>
                <http://vocabularies.wikipathways.org/gpml#> .

<http://vocabularies.wikipathways.org/gpml#hasPublicationXref>
        a       <http://www.w3.org/2002/07/owl#ObjectProperty> ;
        <http://www.w3.org/2000/01/rdf-schema#comment>
                "Boolean property for the existence of a PublicationXref associated with a given object."@en ;
        <http://www.w3.org/2000/01/rdf-schema#label>
                "hasPublicationXref"@en ;
        <http://www.w3.org/2000/01/rdf-schema#range>
                <http://vocabularies.wikipathways.org/gpml#DataNode> , <http://vocabularies.wikipathways.org/gpml#Pathway> , <http://vocabularies.wikipathways.org/gpml#PublicationXref> , <http://vocabularies.wikipathways.org/gpml#State> , <http://vocabularies.wikipathways.org/gpml#Label> , <http://vocabularies.wikipathways.org/gpml#GraphicalLine> , <http://vocabularies.wikipathways.org/gpml#Interaction> , <http://vocabularies.wikipathways.org/gpml#Shape> , <http://vocabularies.wikipathways.org/gpml#Group> ;
        <http://www.w3.org/2004/02/skos/core#inScheme>
                <http://vocabularies.wikipathways.org/gpml#> .

<http://vocabularies.wikipathways.org/gpml#relY>
        a       <http://www.w3.org/2002/07/owl#DatatypeProperty> ;
        <http://www.w3.org/2000/01/rdf-schema#comment>
                "RelY is the y-coordinate used when a point or state is linked to a another object - relative coordinate to the object that it is linked to (0,0 - center, 1,1 - bottom-right)."@en ;
        <http://www.w3.org/2000/01/rdf-schema#label>
                "relY"@en ;
        <http://www.w3.org/2000/01/rdf-schema#range>
                <http://vocabularies.wikipathways.org/gpml#State> , <http://vocabularies.wikipathways.org/gpml#Point> , <http://www.w3.org/2001/XMLSchema#float> ;
        <http://www.w3.org/2004/02/skos/core#inScheme>
                <http://vocabularies.wikipathways.org/gpml#> .

<http://vocabularies.wikipathways.org/gpml#shape>
        a       <http://www.w3.org/2002/07/owl#DatatypeProperty> ;
        <http://www.w3.org/2000/01/rdf-schema#comment>
                "The visual representation of an anchor, e.g., Circle or None."@en ;
        <http://www.w3.org/2000/01/rdf-schema#label>
                "shape"@en ;
        <http://www.w3.org/2000/01/rdf-schema#range>
                <http://vocabularies.wikipathways.org/gpml#Anchor> , <http://www.w3.org/2001/XMLSchema#string> ;
        <http://www.w3.org/2004/02/skos/core#inScheme>
                <http://vocabularies.wikipathways.org/gpml#> .

<http://vocabularies.wikipathways.org/gpml#graphRef>
        a       <http://www.w3.org/2002/07/owl#DatatypeProperty> ;
        <http://www.w3.org/2000/01/rdf-schema#comment>
                "A GraphRef indicates a \"depends on\" or child/parent relationship between two Pathway elements. The element with the GraphRef is the child, and the element referred to by the GraphRef is the parent. The parent's GraphId will be specified by the child's GraphRef."@en ;
        <http://www.w3.org/2000/01/rdf-schema#label>
                "graphRef"@en ;
        <http://www.w3.org/2000/01/rdf-schema#range>
                <http://www.w3.org/2001/XMLSchema#string> , <http://vocabularies.wikipathways.org/gpml#State> , <http://vocabularies.wikipathways.org/gpml#Point> ;
        <http://www.w3.org/2004/02/skos/core#inScheme>
                <http://vocabularies.wikipathways.org/gpml#> .

<http://vocabularies.wikipathways.org/gpml#biopaxRef>
        a       <http://www.w3.org/2002/07/owl#DatatypeProperty> ;
        <http://www.w3.org/2000/01/rdf-schema#comment>
                "Reuse of references defined by BioPAX."@en ;
        <http://www.w3.org/2000/01/rdf-schema#label>
                "biopaxRef"@en ;
        <http://www.w3.org/2000/01/rdf-schema#range>
                <http://www.w3.org/2001/XMLSchema#string> , <http://vocabularies.wikipathways.org/gpml#State> , <http://vocabularies.wikipathways.org/gpml#DataNode> , <http://vocabularies.wikipathways.org/gpml#Pathway> , <http://vocabularies.wikipathways.org/gpml#Interaction> , <http://vocabularies.wikipathways.org/gpml#Label> , <http://vocabularies.wikipathways.org/gpml#GraphicalLine> , <http://vocabularies.wikipathways.org/gpml#Shape> , <http://vocabularies.wikipathways.org/gpml#Group> ;
        <http://www.w3.org/2000/01/rdf-schema#seeAlso>
                <http://www.biopax.org/release/biopax-level3.owl#PublicationXref> ;
        <http://www.w3.org/2004/02/skos/core#inScheme>
                <http://vocabularies.wikipathways.org/gpml#> .

<http://vocabularies.wikipathways.org/gpml#x>
        a       <http://www.w3.org/2002/07/owl#DatatypeProperty> ;
        <http://www.w3.org/2000/01/rdf-schema#comment>
                "The x-coordinate of a point in the 2-dimensional plane in which a pathway is drawn."@en ;
        <http://www.w3.org/2000/01/rdf-schema#label>
                "x"@en ;
        <http://www.w3.org/2000/01/rdf-schema#range>
                <http://vocabularies.wikipathways.org/gpml#Point> , <http://www.w3.org/2001/XMLSchema#float> ;
        <http://www.w3.org/2004/02/skos/core#inScheme>
                <http://vocabularies.wikipathways.org/gpml#> .

<http://vocabularies.wikipathways.org/gpml#GraphicalLine>
        a       <http://www.w3.org/2002/07/owl#Class> ;
        <http://www.w3.org/2000/01/rdf-schema#comment>
                "A visual annotation, often used to partition space or connect other annotation, e.g., Shapes. An Xref can not be specified for GraphicalLines (in contrast to Interactions)."@en ;
        <http://www.w3.org/2000/01/rdf-schema#label>
                "GraphicalLine"@en ;
        <http://www.w3.org/2004/02/skos/core#inScheme>
                <http://vocabularies.wikipathways.org/gpml#> .

<http://vocabularies.wikipathways.org/gpml#RequiresCurationAttention>
        a       <http://www.w3.org/2002/07/owl#Class> ;
        <http://www.w3.org/2000/01/rdf-schema#comment>
                "Deprecated: Not in use."@en ;
        <http://www.w3.org/2000/01/rdf-schema#label>
                "RequiresCurationAttention"@en ;
        <http://www.w3.org/2004/02/skos/core#inScheme>
                <http://vocabularies.wikipathways.org/gpml#> .

<http://vocabularies.wikipathways.org/gpml#data-Source>
        a       <http://www.w3.org/2002/07/owl#DatatypeProperty> ;
        <http://www.w3.org/2000/01/rdf-schema#comment>
                "Deprecated: Not in use."@en ;
        <http://www.w3.org/2000/01/rdf-schema#label>
                "data-Source"@en ;
        <http://www.w3.org/2000/01/rdf-schema#range>
                <http://vocabularies.wikipathways.org/gpml#Pathway> , <http://www.w3.org/2001/XMLSchema#string> ;
        <http://www.w3.org/2004/02/skos/core#inScheme>
                <http://vocabularies.wikipathways.org/gpml#> .

<http://vocabularies.wikipathways.org/gpml#fontDecoration>
        a       <http://www.w3.org/2002/07/owl#DatatypeProperty> ;
        <http://www.w3.org/2000/01/rdf-schema#comment>
                "Deprecated: Not in use."@en ;
        <http://www.w3.org/2000/01/rdf-schema#label>
                "fontDecoration"@en ;
        <http://www.w3.org/2000/01/rdf-schema#range>
                <http://www.w3.org/2001/XMLSchema#string> , <http://vocabularies.wikipathways.org/gpml#Label> , <http://vocabularies.wikipathways.org/gpml#Shape> ;
        <http://www.w3.org/2004/02/skos/core#inScheme>
                <http://vocabularies.wikipathways.org/gpml#> .

<http://vocabularies.wikipathways.org/gpml#version>
        a       <http://www.w3.org/2002/07/owl#DatatypeProperty> ;
        <http://www.w3.org/2000/01/rdf-schema#comment>
                "The version of a Pathway (currently not used in WP)."@en ;
        <http://www.w3.org/2000/01/rdf-schema#label>
                "version"@en ;
        <http://www.w3.org/2000/01/rdf-schema#range>
                <http://www.w3.org/2001/XMLSchema#string> , <http://vocabularies.wikipathways.org/gpml#Pathway> ;
        <http://www.w3.org/2004/02/skos/core#inScheme>
                <http://vocabularies.wikipathways.org/gpml#> .

<http://vocabularies.wikipathways.org/gpml#boardWidth>
        a       <http://www.w3.org/2002/07/owl#DatatypeProperty> ;
        <http://www.w3.org/2000/01/rdf-schema#comment>
                "Range minimum is zero."@en ;
        <http://www.w3.org/2000/01/rdf-schema#label>
                "boardWidth"@en ;
        <http://www.w3.org/2000/01/rdf-schema#range>
                <http://vocabularies.wikipathways.org/gpml#Pathway> , <http://www.w3.org/2001/XMLSchema#float> ;
        <http://www.w3.org/2004/02/skos/core#inScheme>
                <http://vocabularies.wikipathways.org/gpml#> .

<http://vocabularies.wikipathways.org/gpml#Legend>
        a       <http://www.w3.org/2002/07/owl#Class> ;
        <http://www.w3.org/2000/01/rdf-schema#comment>
                "An explanatory list of the colors used for visualizing data on the pathway. Not currently used."@en ;
        <http://www.w3.org/2000/01/rdf-schema#label>
                "Legend"@en ;
        <http://www.w3.org/2004/02/skos/core#inScheme>
                <http://vocabularies.wikipathways.org/gpml#> .

<http://vocabularies.wikipathways.org/gpml#arrowHead>
        a       <http://www.w3.org/2002/07/owl#DatatypeProperty> ;
        <http://www.w3.org/2000/01/rdf-schema#comment>
                "Specifies the glyph at the ends of lines and interactions."@en ;
        <http://www.w3.org/2000/01/rdf-schema#label>
                "arrowHead"@en ;
        <http://www.w3.org/2000/01/rdf-schema#range>
                <http://www.w3.org/2001/XMLSchema#string> , <http://vocabularies.wikipathways.org/gpml#Point> ;
        <http://www.w3.org/2004/02/skos/core#inScheme>
                <http://vocabularies.wikipathways.org/gpml#> .

<http://vocabularies.wikipathways.org/gpml#Biopax>
        a       <http://www.w3.org/2002/07/owl#Class> ;
        <http://www.w3.org/2000/01/rdf-schema#comment>
                "Element used to embed Biopax (namespace: http://www.biopax.org/release/biopax-level3.owl) content in a GPML document."@en ;
        <http://www.w3.org/2000/01/rdf-schema#label>
                "Biopax"@en ;
        <http://www.w3.org/2004/02/skos/core#inScheme>
                <http://vocabularies.wikipathways.org/gpml#> .

<http://vocabularies.wikipathways.org/gpml#relX>
        a       <http://www.w3.org/2002/07/owl#DatatypeProperty> ;
        <http://www.w3.org/2000/01/rdf-schema#comment>
                "RelX is the x-coordinate used when a point or state is linked to a another object - relative coordinate to the object that it is linked to (0,0 - center, 1,1 - bottom-right)."@en ;
        <http://www.w3.org/2000/01/rdf-schema#label>
                "relX"@en ;
        <http://www.w3.org/2000/01/rdf-schema#range>
                <http://vocabularies.wikipathways.org/gpml#State> , <http://vocabularies.wikipathways.org/gpml#Point> , <http://www.w3.org/2001/XMLSchema#float> ;
        <http://www.w3.org/2004/02/skos/core#inScheme>
                <http://vocabularies.wikipathways.org/gpml#> .

<http://vocabularies.wikipathways.org/gpml#hasGraphicalLine>
        a       <http://www.w3.org/2002/07/owl#ObjectProperty> ;
        <http://www.w3.org/2000/01/rdf-schema#comment>
                "Boolean property for the existence of a GraphicalLine in a given pathway."@en ;
        <http://www.w3.org/2000/01/rdf-schema#label>
                "hasGraphicalLine"@en ;
        <http://www.w3.org/2000/01/rdf-schema#range>
                <http://vocabularies.wikipathways.org/gpml#Pathway> , <http://vocabularies.wikipathways.org/gpml#GraphicalLine> ;
        <http://www.w3.org/2004/02/skos/core#inScheme>
                <http://vocabularies.wikipathways.org/gpml#> .

<http://vocabularies.wikipathways.org/gpml#position>
        a       <http://www.w3.org/2002/07/owl#DatatypeProperty> ;
        <http://www.w3.org/2000/01/rdf-schema#comment>
                "Proportional distance of an anchor along the line it belongs to, between 0 and 1."@en ;
        <http://www.w3.org/2000/01/rdf-schema#label>
                "position"@en ;
        <http://www.w3.org/2000/01/rdf-schema#range>
                <http://vocabularies.wikipathways.org/gpml#Anchor> , <http://www.w3.org/2001/XMLSchema#float> ;
        <http://www.w3.org/2004/02/skos/core#inScheme>
                <http://vocabularies.wikipathways.org/gpml#> .
