<https://vocab.eccenca.com/geniustex/rechargeable>
        a       <http://www.w3.org/2002/07/owl#DatatypeProperty> ;
        <http://www.w3.org/2000/01/rdf-schema#comment>
                "if a power supply module can be recharged, i.e., if electrical energy can be restored by connecting it to another power supply (yes/no)" ;
        <http://www.w3.org/2000/01/rdf-schema#domain>
                <https://vocab.eccenca.com/geniustex/PowerSupplyModule> ;
        <http://www.w3.org/2000/01/rdf-schema#isDefinedBy>
                <https://vocab.eccenca.com/geniustex/> ;
        <http://www.w3.org/2000/01/rdf-schema#label>
                "rechargeable" ;
        <http://www.w3.org/2000/01/rdf-schema#range>
                <http://www.w3.org/2001/XMLSchema#boolean> ;
        <http://purl.org/dc/terms/issued>
                "2018-10-03"^^<http://www.w3.org/2001/XMLSchema#date> ;
        <http://purl.org/dc/terms/modified>
                "2019-04-15"^^<http://www.w3.org/2001/XMLSchema#date> .

<https://vocab.eccenca.com/geniustex/thermicalsensor>
        a       <https://vocab.eccenca.com/geniustex/SensorType> ;
        <http://www.w3.org/2000/01/rdf-schema#comment>
                " sensors that detect changes in temperature" ;
        <http://www.w3.org/2000/01/rdf-schema#isDefinedBy>
                <https://vocab.eccenca.com/geniustex/> ;
        <http://www.w3.org/2000/01/rdf-schema#label>
                "thermical sensor" ;
        <http://purl.org/dc/terms/issued>
                "2018-08-15"^^<http://www.w3.org/2001/XMLSchema#date> ;
        <http://purl.org/dc/terms/modified>
                "2019-09-18"^^<http://www.w3.org/2001/XMLSchema#date> .

<https://vocab.eccenca.com/geniustex/finewash>
        a       <https://vocab.eccenca.com/geniustex/CareInstructions> ;
        <http://www.w3.org/2000/01/rdf-schema#comment>
                "a material can be washed with fine wash 30째C" ;
        <http://www.w3.org/2000/01/rdf-schema#isDefinedBy>
                <https://vocab.eccenca.com/geniustex/> ;
        <http://www.w3.org/2000/01/rdf-schema#label>
                "fine wash" ;
        <http://purl.org/dc/terms/issued>
                "2019-02-28"^^<http://www.w3.org/2001/XMLSchema#date> .

<https://vocab.eccenca.com/geniustex/automated>
        a       <http://www.w3.org/2002/07/owl#DatatypeProperty> ;
        <http://www.w3.org/2000/01/rdf-schema#comment>
                "degree of automation of a process, i.e., how much automatic equipment is used in a manufacturing or other process or facility (high/medium/low)" ;
        <http://www.w3.org/2000/01/rdf-schema#domain>
                <https://vocab.eccenca.com/geniustex/Process> ;
        <http://www.w3.org/2000/01/rdf-schema#isDefinedBy>
                <https://vocab.eccenca.com/geniustex/> ;
        <http://www.w3.org/2000/01/rdf-schema#label>
                "degree of automation" ;
        <http://www.w3.org/2000/01/rdf-schema#range>
                <http://www.w3.org/2001/XMLSchema#string> ;
        <http://purl.org/dc/terms/issued>
                "2018-08-15"^^<http://www.w3.org/2001/XMLSchema#date> ;
        <http://purl.org/dc/terms/modified>
                "2019-04-15"^^<http://www.w3.org/2001/XMLSchema#date> .

<https://vocab.eccenca.com/geniustex/usesComponent>
        a       <http://www.w3.org/2002/07/owl#ObjectProperty> ;
        <http://www.w3.org/2000/01/rdf-schema#comment>
                "a collaboration concept can use/refer to a component" ;
        <http://www.w3.org/2000/01/rdf-schema#domain>
                <https://vocab.eccenca.com/geniustex/CollaborationConcept> ;
        <http://www.w3.org/2000/01/rdf-schema#isDefinedBy>
                <https://vocab.eccenca.com/geniustex/> ;
        <http://www.w3.org/2000/01/rdf-schema#label>
                "uses component" ;
        <http://www.w3.org/2000/01/rdf-schema#range>
                <https://vocab.eccenca.com/geniustex/Component> ;
        <http://purl.org/dc/terms/issued>
                "2018-09-30"^^<http://www.w3.org/2001/XMLSchema#date> .

<https://vocab.eccenca.com/geniustex/crosswise>
        a       <https://vocab.eccenca.com/geniustex/ElasticityType> ;
        <http://www.w3.org/2000/01/rdf-schema#comment>
                "elasticity only crosswise, i.e., able to resume its normal shape spontaneously after being stretched or compressed crosswise" ;
        <http://www.w3.org/2000/01/rdf-schema#isDefinedBy>
                <https://vocab.eccenca.com/geniustex/> ;
        <http://www.w3.org/2000/01/rdf-schema#label>
                "crosswise" ;
        <http://purl.org/dc/terms/issued>
                "2018-09-30"^^<http://www.w3.org/2001/XMLSchema#date> ;
        <http://purl.org/dc/terms/modified>
                "2019-04-15"^^<http://www.w3.org/2001/XMLSchema#date> .

<https://vocab.eccenca.com/geniustex/smd>
        a       <https://vocab.eccenca.com/geniustex/PackageType> ;
        <http://www.w3.org/2000/01/rdf-schema#comment>
                "component is packaged as surface mount device, i.e., it has leads that are designed to be soldered on the side of a circuit board that the body of the component is mounted on" ;
        <http://www.w3.org/2000/01/rdf-schema#isDefinedBy>
                <https://vocab.eccenca.com/geniustex/> ;
        <http://www.w3.org/2000/01/rdf-schema#label>
                "surface mount device" ;
        <http://purl.org/dc/terms/issued>
                "2018-09-30"^^<http://www.w3.org/2001/XMLSchema#date> ;
        <http://purl.org/dc/terms/modified>
                "2019-04-15"^^<http://www.w3.org/2001/XMLSchema#date> .

<https://vocab.eccenca.com/geniustex/contacts>
        a       <http://www.w3.org/2002/07/owl#ObjectProperty> ;
        <http://www.w3.org/2000/01/rdf-schema#comment>
                "process contacts components on circuit boards or interconnection modules" ;
        <http://www.w3.org/2000/01/rdf-schema#domain>
                <https://vocab.eccenca.com/geniustex/Contacting> ;
        <http://www.w3.org/2000/01/rdf-schema#isDefinedBy>
                <https://vocab.eccenca.com/geniustex/> ;
        <http://www.w3.org/2000/01/rdf-schema#label>
                "contacts" ;
        <http://www.w3.org/2000/01/rdf-schema#range>
                <https://vocab.eccenca.com/geniustex/Component> ;
        <http://purl.org/dc/terms/issued>
                "2018-05-21"^^<http://www.w3.org/2001/XMLSchema#date> ;
        <http://purl.org/dc/terms/modified>
                "2019-04-15"^^<http://www.w3.org/2001/XMLSchema#date> .

<https://vocab.eccenca.com/geniustex/medtech>
        a       <https://vocab.eccenca.com/geniustex/ApplicationArea> ;
        <http://www.w3.org/2000/01/rdf-schema#comment>
                "Medicine, hygiene, work clothing, implants  (Source: Gries et al. Textile Fertigungsverfahren: Eine Einf체hrung; Carl Hanser\nVerlag)" ;
        <http://www.w3.org/2000/01/rdf-schema#isDefinedBy>
                <https://vocab.eccenca.com/geniustex/> ;
        <http://www.w3.org/2000/01/rdf-schema#label>
                "medtech" ;
        <http://purl.org/dc/terms/issued>
                "2019-04-15"^^<http://www.w3.org/2001/XMLSchema#date> .

<https://vocab.eccenca.com/geniustex/detachable>
        a       <http://www.w3.org/2002/07/owl#DatatypeProperty> ;
        <http://www.w3.org/2000/01/rdf-schema#comment>
                "if a casing can be detached from the item is surrounds (yes/no)" ;
        <http://www.w3.org/2000/01/rdf-schema#domain>
                <https://vocab.eccenca.com/geniustex/Casing> ;
        <http://www.w3.org/2000/01/rdf-schema#isDefinedBy>
                <https://vocab.eccenca.com/geniustex/> ;
        <http://www.w3.org/2000/01/rdf-schema#label>
                "detachale" ;
        <http://www.w3.org/2000/01/rdf-schema#range>
                <http://www.w3.org/2001/XMLSchema#boolean> ;
        <http://purl.org/dc/terms/issued>
                "2018-10-03"^^<http://www.w3.org/2001/XMLSchema#date> ;
        <http://purl.org/dc/terms/modified>
                "2019-04-15"^^<http://www.w3.org/2001/XMLSchema#date> .

<https://vocab.eccenca.com/geniustex/Marking>
        a       <http://www.w3.org/2002/07/owl#Class> ;
        <http://www.w3.org/2000/01/rdf-schema#comment>
                "a process step where a small spot or area is made as an indication or record of some information" ;
        <http://www.w3.org/2000/01/rdf-schema#isDefinedBy>
                <https://vocab.eccenca.com/geniustex/> ;
        <http://www.w3.org/2000/01/rdf-schema#label>
                "Marking" ;
        <http://www.w3.org/2000/01/rdf-schema#subClassOf>
                <https://vocab.eccenca.com/geniustex/QualityControl> ;
        <http://purl.org/dc/terms/issued>
                "2018-09-19"^^<http://www.w3.org/2001/XMLSchema#date> ;
        <http://purl.org/dc/terms/modified>
                "2019-04-15"^^<http://www.w3.org/2001/XMLSchema#date> .

<https://vocab.eccenca.com/geniustex/freedomGeometry>
        a       <http://www.w3.org/2002/07/owl#DatatypeProperty> ;
        <http://www.w3.org/2000/01/rdf-schema#comment>
                "freedom of geometry achieved by integrating process (very high freedom = 5 / high  = 4 /medium a = 3 / low  = 2 / no freedom of geometry = 1; i.e., 5 represents most desirable evaluation)" ;
        <http://www.w3.org/2000/01/rdf-schema#domain>
                <https://vocab.eccenca.com/geniustex/Integrating> ;
        <http://www.w3.org/2000/01/rdf-schema#isDefinedBy>
                <https://vocab.eccenca.com/geniustex/> ;
        <http://www.w3.org/2000/01/rdf-schema#label>
                "freedom of geometry" ;
        <http://www.w3.org/2000/01/rdf-schema#range>
                <http://www.w3.org/2001/XMLSchema#integer> ;
        <http://purl.org/dc/terms/issued>
                "2018-08-15"^^<http://www.w3.org/2001/XMLSchema#date> .

<https://vocab.eccenca.com/geniustex/hasMatTestResult>
        a       <http://www.w3.org/2002/07/owl#ObjectProperty> ;
        <http://www.w3.org/2000/01/rdf-schema#comment>
                "a material has a certain result in the property test that it conforms with" ;
        <http://www.w3.org/2000/01/rdf-schema#domain>
                <https://vocab.eccenca.com/geniustex/Material> ;
        <http://www.w3.org/2000/01/rdf-schema#isDefinedBy>
                <https://vocab.eccenca.com/geniustex/> ;
        <http://www.w3.org/2000/01/rdf-schema#label>
                "has material test result" ;
        <http://www.w3.org/2000/01/rdf-schema#range>
                <https://vocab.eccenca.com/geniustex/TestResult> ;
        <http://purl.org/dc/terms/issued>
                "2018-08-30"^^<http://www.w3.org/2001/XMLSchema#date> .

<https://vocab.eccenca.com/geniustex/integrates>
        a       <http://www.w3.org/2002/07/owl#ObjectProperty> ;
        <http://www.w3.org/2000/01/rdf-schema#comment>
                "process joins components to each other " ;
        <http://www.w3.org/2000/01/rdf-schema#domain>
                <https://vocab.eccenca.com/geniustex/Integrating> ;
        <http://www.w3.org/2000/01/rdf-schema#isDefinedBy>
                <https://vocab.eccenca.com/geniustex/> ;
        <http://www.w3.org/2000/01/rdf-schema#label>
                "integrates" ;
        <http://www.w3.org/2000/01/rdf-schema#range>
                <https://vocab.eccenca.com/geniustex/Component> ;
        <http://purl.org/dc/terms/issued>
                "2018-05-21"^^<http://www.w3.org/2001/XMLSchema#date> ;
        <http://purl.org/dc/terms/modified>
                "2018-08-15"^^<http://www.w3.org/2001/XMLSchema#date> .

<http://www.w3.org/ns/ssn/systems/hasSystemCapability>
        a       <http://www.w3.org/2002/07/owl#ObjectProperty> ;
        <http://www.w3.org/2000/01/rdf-schema#comment>
                "Relation from a System to a SystemCapability describing the capabilities of the System under certain Conditions."@en ;
        <http://www.w3.org/2000/01/rdf-schema#domain>
                <https://vocab.eccenca.com/geniustex/FunctionalModule> ;
        <http://www.w3.org/2000/01/rdf-schema#isDefinedBy>
                <http://www.w3.org/ns/ssn/systems/> ;
        <http://www.w3.org/2000/01/rdf-schema#label>
                "has system capability"@en ;
        <http://www.w3.org/2000/01/rdf-schema#range>
                <http://www.w3.org/ns/ssn/systems/SystemCapability> ;
        <http://www.w3.org/2000/01/rdf-schema#subPropertyOf>
                <http://www.w3.org/ns/ssn/hasProperty> .

<https://vocab.eccenca.com/geniustex/IncludesFunctComp>
        a       <http://www.w3.org/2002/07/owl#ObjectProperty> ;
        <http://www.w3.org/2000/01/rdf-schema#comment>
                "a component includes other functional modules (besides the module/class is has been applied to)" ;
        <http://www.w3.org/2000/01/rdf-schema#domain>
                <https://vocab.eccenca.com/geniustex/Component> ;
        <http://www.w3.org/2000/01/rdf-schema#isDefinedBy>
                <https://vocab.eccenca.com/geniustex/> ;
        <http://www.w3.org/2000/01/rdf-schema#label>
                "includes functional component" ;
        <http://www.w3.org/2000/01/rdf-schema#range>
                <https://vocab.eccenca.com/geniustex/FunctionalModule> ;
        <http://purl.org/dc/terms/issued>
                "2018-08-30"^^<http://www.w3.org/2001/XMLSchema#date> ;
        <http://purl.org/dc/terms/modified>
                "2019-02-14"^^<http://www.w3.org/2001/XMLSchema#date> .

<https://vocab.eccenca.com/geniustex/opticsignal>
        a       <https://vocab.eccenca.com/geniustex/SignalType> ;
        <http://www.w3.org/2000/01/rdf-schema#comment>
                "optic signal, e.g., a light" ;
        <http://www.w3.org/2000/01/rdf-schema#isDefinedBy>
                <https://vocab.eccenca.com/geniustex/> ;
        <http://www.w3.org/2000/01/rdf-schema#label>
                "optic actuator signal" ;
        <http://purl.org/dc/terms/issued>
                "2018-08-15"^^<http://www.w3.org/2001/XMLSchema#date> ;
        <http://purl.org/dc/terms/modified>
                "2019-04-15"^^<http://www.w3.org/2001/XMLSchema#date> .

<https://vocab.eccenca.com/geniustex/geotech>
        a       <https://vocab.eccenca.com/geniustex/ApplicationArea> ;
        <http://www.w3.org/2000/01/rdf-schema#comment>
                "Civil engineering, road construction, dam construction, landfill construction and mining  (Source: Gries et al. Textile Fertigungsverfahren: Eine Einf체hrung; Carl Hanser\nVerlag)" ;
        <http://www.w3.org/2000/01/rdf-schema#isDefinedBy>
                <https://vocab.eccenca.com/geniustex/> ;
        <http://www.w3.org/2000/01/rdf-schema#label>
                "geotech" ;
        <http://purl.org/dc/terms/issued>
                "2018-06-15"^^<http://www.w3.org/2001/XMLSchema#date> ;
        <http://purl.org/dc/terms/modified>
                "2019-04-15"^^<http://www.w3.org/2001/XMLSchema#date> .

<https://vocab.eccenca.com/geniustex/usesProcess>
        a       <http://www.w3.org/2002/07/owl#ObjectProperty> ;
        <http://www.w3.org/2000/01/rdf-schema#comment>
                "a collaboration concept can use/refer to a process" ;
        <http://www.w3.org/2000/01/rdf-schema#domain>
                <https://vocab.eccenca.com/geniustex/CollaborationConcept> ;
        <http://www.w3.org/2000/01/rdf-schema#isDefinedBy>
                <https://vocab.eccenca.com/geniustex/> ;
        <http://www.w3.org/2000/01/rdf-schema#label>
                "uses process" ;
        <http://www.w3.org/2000/01/rdf-schema#range>
                <https://vocab.eccenca.com/geniustex/Process> ;
        <http://purl.org/dc/terms/issued>
                "2018-09-30"^^<http://www.w3.org/2001/XMLSchema#date> .

<https://vocab.eccenca.com/geniustex/pinDistance>
        a       <http://www.w3.org/2002/07/owl#ObjectProperty> ;
        <http://www.w3.org/2000/01/rdf-schema#comment>
                "distance between connecting pins of a functional module" ;
        <http://www.w3.org/2000/01/rdf-schema#domain>
                <https://vocab.eccenca.com/geniustex/FunctionalModule> ;
        <http://www.w3.org/2000/01/rdf-schema#isDefinedBy>
                <https://vocab.eccenca.com/geniustex/> ;
        <http://www.w3.org/2000/01/rdf-schema#label>
                "pin distance " ;
        <http://purl.org/dc/terms/issued>
                "2018-08-15"^^<http://www.w3.org/2001/XMLSchema#date> ;
        <http://purl.org/dc/terms/modified>
                "2019-04-15"^^<http://www.w3.org/2001/XMLSchema#date> .

<https://vocab.eccenca.com/geniustex/needsProcess>
        a       <http://www.w3.org/2002/07/owl#ObjectProperty> ;
        <http://www.w3.org/2000/01/rdf-schema#comment>
                "a process needs another process to function properly" ;
        <http://www.w3.org/2000/01/rdf-schema#domain>
                <https://vocab.eccenca.com/geniustex/Process> ;
        <http://www.w3.org/2000/01/rdf-schema#isDefinedBy>
                <https://vocab.eccenca.com/geniustex/> ;
        <http://www.w3.org/2000/01/rdf-schema#label>
                "needs a process" ;
        <http://www.w3.org/2000/01/rdf-schema#range>
                <https://vocab.eccenca.com/geniustex/Process> ;
        <http://purl.org/dc/terms/issued>
                "2019-02-13"^^<http://www.w3.org/2001/XMLSchema#date> ;
        <http://purl.org/dc/terms/modified>
                "2019-04-15"^^<http://www.w3.org/2001/XMLSchema#date> .

<https://vocab.eccenca.com/geniustex/trackClearance>
        a       <http://www.w3.org/2002/07/owl#DatatypeProperty> ;
        <http://www.w3.org/2000/01/rdf-schema#comment>
                "track clearance of interconnection modules like circuit boards (micrometers)" ;
        <http://www.w3.org/2000/01/rdf-schema#domain>
                <https://vocab.eccenca.com/geniustex/InterconnectionModule> ;
        <http://www.w3.org/2000/01/rdf-schema#isDefinedBy>
                <https://vocab.eccenca.com/geniustex/> ;
        <http://www.w3.org/2000/01/rdf-schema#label>
                "track clearance" ;
        <http://www.w3.org/2000/01/rdf-schema#range>
                <http://www.w3.org/2001/XMLSchema#float> ;
        <http://purl.org/dc/terms/issued>
                "2018-08-15"^^<http://www.w3.org/2001/XMLSchema#date> ;
        <http://purl.org/dc/terms/modified>
                "2019-04-15"^^<http://www.w3.org/2001/XMLSchema#date> .

<https://vocab.eccenca.com/geniustex/packtech>
        a       <https://vocab.eccenca.com/geniustex/ApplicationArea> ;
        <http://www.w3.org/2000/01/rdf-schema#comment>
                "Packaging, insulation, covering  (Source: Gries et al. Textile Fertigungsverfahren: Eine Einf체hrung; Carl Hanser\nVerlag)" ;
        <http://www.w3.org/2000/01/rdf-schema#isDefinedBy>
                <https://vocab.eccenca.com/geniustex/> ;
        <http://www.w3.org/2000/01/rdf-schema#label>
                "packtech" ;
        <http://purl.org/dc/terms/issued>
                "2018-06-15"^^<http://www.w3.org/2001/XMLSchema#date> ;
        <http://purl.org/dc/terms/modified>
                "2019-04-15"^^<http://www.w3.org/2001/XMLSchema#date> .

<https://vocab.eccenca.com/geniustex/maxTransmissionRate>
        a       <http://www.w3.org/2002/07/owl#ObjectProperty> ;
        <http://www.w3.org/2000/01/rdf-schema#comment>
                "maximum transmission rate of the data transmission module, i.e., the amount of data (given in Mbit) that can be sent or received in a time interval" ;
        <http://www.w3.org/2000/01/rdf-schema#domain>
                <https://vocab.eccenca.com/geniustex/DataTransmissionModule> ;
        <http://www.w3.org/2000/01/rdf-schema#isDefinedBy>
                <https://vocab.eccenca.com/geniustex/> ;
        <http://www.w3.org/2000/01/rdf-schema#label>
                "maximum transmission rate" ;
        <http://purl.org/dc/terms/issued>
                "2018-08-15"^^<http://www.w3.org/2001/XMLSchema#date> ;
        <http://purl.org/dc/terms/modified>
                "2019-04-15"^^<http://www.w3.org/2001/XMLSchema#date> .

<https://vocab.eccenca.com/geniustex/protectionLevel>
        a       <http://www.w3.org/2002/07/owl#DatatypeProperty> ;
        <http://www.w3.org/2000/01/rdf-schema#comment>
                "protection provided by casing (very high protection = 5 / high  = 4 /medium  = 3 / low  = 2 / no protection = 1)" ;
        <http://www.w3.org/2000/01/rdf-schema#domain>
                <https://vocab.eccenca.com/geniustex/Casing> ;
        <http://www.w3.org/2000/01/rdf-schema#isDefinedBy>
                <https://vocab.eccenca.com/geniustex/> ;
        <http://www.w3.org/2000/01/rdf-schema#label>
                "protection level" ;
        <http://www.w3.org/2000/01/rdf-schema#range>
                <http://www.w3.org/2001/XMLSchema#integer> ;
        <http://purl.org/dc/terms/issued>
                "2018-08-15"^^<http://www.w3.org/2001/XMLSchema#date> .

<https://vocab.eccenca.com/geniustex/productID>
        a       <http://www.w3.org/2002/07/owl#DatatypeProperty> ;
        <http://www.w3.org/2000/01/rdf-schema#comment>
                "an identification key given by a supplier to a specific product" ;
        <http://www.w3.org/2000/01/rdf-schema#domain>
                <https://vocab.eccenca.com/geniustex/Component> ;
        <http://www.w3.org/2000/01/rdf-schema#isDefinedBy>
                <https://vocab.eccenca.com/geniustex/> ;
        <http://www.w3.org/2000/01/rdf-schema#label>
                "ID of a component or product" ;
        <http://www.w3.org/2000/01/rdf-schema#range>
                <http://www.w3.org/2001/XMLSchema#string> ;
        <http://purl.org/dc/terms/issued>
                "2018-07-10"^^<http://www.w3.org/2001/XMLSchema#date> .

<https://vocab.eccenca.com/geniustex/temperatureMatCuring>
        a       <http://www.w3.org/2002/07/owl#ObjectProperty> ;
        <http://www.w3.org/2000/01/rdf-schema#comment>
                "curing temperature of a material " ;
        <http://www.w3.org/2000/01/rdf-schema#domain>
                <https://vocab.eccenca.com/geniustex/Material> ;
        <http://www.w3.org/2000/01/rdf-schema#isDefinedBy>
                <https://vocab.eccenca.com/geniustex/> ;
        <http://www.w3.org/2000/01/rdf-schema#label>
                "curing temperature of a material" ;
        <http://purl.org/dc/terms/issued>
                "2019-02-13"^^<http://www.w3.org/2001/XMLSchema#date> ;
        <http://purl.org/dc/terms/modified>
                "2019-04-15"^^<http://www.w3.org/2001/XMLSchema#date> .

<http://www.w3.org/ns/ssn/systems/Condition>
        a       <http://www.w3.org/2002/07/owl#Class> ;
        <http://www.w3.org/2000/01/rdf-schema#comment>
                "Used to specify ranges for qualities that act as conditions on a system/sensor's operation.  For example, wind speed of 10-60m/s may be used as the condition on a SystemProperty, for example, to state that a sensor has a particular accuracy in that condition."@en ;
        <http://www.w3.org/2000/01/rdf-schema#isDefinedBy>
                <http://www.w3.org/ns/ssn/systems/> ;
        <http://www.w3.org/2000/01/rdf-schema#label>
                "Condition"@en ;
        <http://www.w3.org/2000/01/rdf-schema#subClassOf>
                <http://www.w3.org/ns/ssn/Property> .

<http://www.w3.org/ns/ssn/systems/SystemProperty>
        a       <http://www.w3.org/2002/07/owl#Class> ;
        <http://www.w3.org/2000/01/rdf-schema#comment>
                "An identifiable and observable characteristic that represents the System's ability to operate its primary purpose: a Sensor to make Observations, an Actuator to make Actuations, or a Sampler to make Samplings."@en ;
        <http://www.w3.org/2000/01/rdf-schema#isDefinedBy>
                <http://www.w3.org/ns/ssn/systems/> ;
        <http://www.w3.org/2000/01/rdf-schema#label>
                "System Property"@en ;
        <http://www.w3.org/2000/01/rdf-schema#subClassOf>
                <http://www.w3.org/ns/ssn/Property> .

<https://vocab.eccenca.com/geniustex/conformsWith>
        a       <http://www.w3.org/2002/07/owl#ObjectProperty> ;
        <http://www.w3.org/2000/01/rdf-schema#comment>
                "a smart product meets the requirements of a property test" ;
        <http://www.w3.org/2000/01/rdf-schema#domain>
                <https://vocab.eccenca.com/geniustex/SmartProduct> ;
        <http://www.w3.org/2000/01/rdf-schema#isDefinedBy>
                <https://vocab.eccenca.com/geniustex/> ;
        <http://www.w3.org/2000/01/rdf-schema#label>
                "conforms with" ;
        <http://www.w3.org/2000/01/rdf-schema#range>
                <https://vocab.eccenca.com/geniustex/PropertyTest> ;
        <http://purl.org/dc/terms/issued>
                "2018-06-23"^^<http://www.w3.org/2001/XMLSchema#date> .

<https://vocab.eccenca.com/geniustex/IEC%5F56%2F1579%2FCD%3A2014>
        a       <https://vocab.eccenca.com/geniustex/FmeaTest> ;
        <http://www.w3.org/2000/01/rdf-schema#comment>
                "the international IED ID of the FMEA test" ;
        <http://www.w3.org/2000/01/rdf-schema#isDefinedBy>
                <https://vocab.eccenca.com/geniustex/> ;
        <http://www.w3.org/2000/01/rdf-schema#label>
                "FMEA test norm" ;
        <http://purl.org/dc/terms/issued>
                "2018-10-12"^^<http://www.w3.org/2001/XMLSchema#date> .

<https://vocab.eccenca.com/geniustex/measures>
        a       <http://www.w3.org/2002/07/owl#ObjectProperty> ;
        <http://www.w3.org/2000/01/rdf-schema#comment>
                "sensors can measure quantifiable aspects" ;
        <http://www.w3.org/2000/01/rdf-schema#domain>
                <https://vocab.eccenca.com/geniustex/Sensor> ;
        <http://www.w3.org/2000/01/rdf-schema#isDefinedBy>
                <https://vocab.eccenca.com/geniustex/> ;
        <http://www.w3.org/2000/01/rdf-schema#label>
                "measures" ;
        <http://www.w3.org/2000/01/rdf-schema#range>
                <https://vocab.eccenca.com/geniustex/Quantity> ;
        <http://purl.org/dc/terms/issued>
                "2018-07-10"^^<http://www.w3.org/2001/XMLSchema#date> .

<https://vocab.eccenca.com/geniustex/adhesivebond>
        a       <https://vocab.eccenca.com/geniustex/ConnectionType> ;
        <http://www.w3.org/2000/01/rdf-schema#comment>
                "connection in joining process created by an adhesive bond. Adhesive bonding describes a technique where an intermediate layer (e.g., a glue) is applied to connect substrates of different types of materials" ;
        <http://www.w3.org/2000/01/rdf-schema#isDefinedBy>
                <https://vocab.eccenca.com/geniustex/> ;
        <http://www.w3.org/2000/01/rdf-schema#label>
                "adhesive bond" ;
        <http://purl.org/dc/terms/issued>
                "2018-09-30"^^<http://www.w3.org/2001/XMLSchema#date> ;
        <http://purl.org/dc/terms/modified>
                "2019-04-15"^^<http://www.w3.org/2001/XMLSchema#date> .

<https://vocab.eccenca.com/geniustex/ConnectionType>
        a       <http://www.w3.org/2002/07/owl#Class> ;
        <http://www.w3.org/2000/01/rdf-schema#comment>
                "type of connection that is created in a production process between two or more components" ;
        <http://www.w3.org/2000/01/rdf-schema#isDefinedBy>
                <https://vocab.eccenca.com/geniustex/> ;
        <http://www.w3.org/2000/01/rdf-schema#label>
                "Type of Connection" ;
        <http://purl.org/dc/terms/issued>
                "2018-09-30"^^<http://www.w3.org/2001/XMLSchema#date> ;
        <http://purl.org/dc/terms/modified>
                "2019-04-12"^^<http://www.w3.org/2001/XMLSchema#date> .

<https://vocab.eccenca.com/geniustex/hasCareInstructions>
        a       <http://www.w3.org/2002/07/owl#ObjectProperty> ;
        <http://www.w3.org/2000/01/rdf-schema#comment>
                "a material has certain care instructions, e.g., how it should be cleaned or washed" ;
        <http://www.w3.org/2000/01/rdf-schema#domain>
                <https://vocab.eccenca.com/geniustex/Material> ;
        <http://www.w3.org/2000/01/rdf-schema#isDefinedBy>
                <https://vocab.eccenca.com/geniustex/> ;
        <http://www.w3.org/2000/01/rdf-schema#label>
                "has care instruction" ;
        <http://www.w3.org/2000/01/rdf-schema#range>
                <https://vocab.eccenca.com/geniustex/CareInstructions> ;
        <http://purl.org/dc/terms/issued>
                "2018-08-30"^^<http://www.w3.org/2001/XMLSchema#date> ;
        <http://purl.org/dc/terms/modified>
                "2019-04-15"^^<http://www.w3.org/2001/XMLSchema#date> .

<https://vocab.eccenca.com/geniustex/ElasticityType>
        a       <http://www.w3.org/2002/07/owl#Class> ;
        <http://www.w3.org/2000/01/rdf-schema#comment>
                "describes how a textile is elastic, i.e., if it is able to resume its normal shape spontaneously after being stretched or compressed (none/bidirectional/lengthwise/crosswise)" ;
        <http://www.w3.org/2000/01/rdf-schema#isDefinedBy>
                <https://vocab.eccenca.com/geniustex/> ;
        <http://www.w3.org/2000/01/rdf-schema#label>
                "Type of Elasticity" ;
        <http://purl.org/dc/terms/issued>
                "2018-09-30"^^<http://www.w3.org/2001/XMLSchema#date> ;
        <http://purl.org/dc/terms/modified>
                "2019-04-15"^^<http://www.w3.org/2001/XMLSchema#date> .

<https://vocab.eccenca.com/geniustex/User>
        a       <http://www.w3.org/2002/07/owl#Class> ;
        <http://www.w3.org/2000/01/rdf-schema#comment>
                "user of the platform, working with smart products" ;
        <http://www.w3.org/2000/01/rdf-schema#isDefinedBy>
                <https://vocab.eccenca.com/geniustex/> ;
        <http://www.w3.org/2000/01/rdf-schema#label>
                "User" ;
        <http://purl.org/dc/terms/issued>
                "2018-09-30"^^<http://www.w3.org/2001/XMLSchema#date> .

<https://vocab.eccenca.com/geniustex/Process>
        a       <http://www.w3.org/2002/07/owl#Class> ;
        <http://www.w3.org/2000/01/rdf-schema#comment>
                "a process step during the production/system integration of the smart product" ;
        <http://www.w3.org/2000/01/rdf-schema#isDefinedBy>
                <https://vocab.eccenca.com/geniustex/> ;
        <http://www.w3.org/2000/01/rdf-schema#label>
                "Process Module" ;
        <http://www.w3.org/2000/01/rdf-schema#subClassOf>
                <https://vocab.eccenca.com/geniustex/SmartProduct> ;
        <http://purl.org/dc/terms/issued>
                "2018-05-21"^^<http://www.w3.org/2001/XMLSchema#date> ;
        <http://purl.org/dc/terms/modified>
                "2018-06-14"^^<http://www.w3.org/2001/XMLSchema#date> .

<https://vocab.eccenca.com/geniustex/consistsOf>
        a       <http://www.w3.org/2002/07/owl#ObjectProperty> ;
        <http://www.w3.org/2000/01/rdf-schema#comment>
                "a component consists of a certain material" ;
        <http://www.w3.org/2000/01/rdf-schema#domain>
                <https://vocab.eccenca.com/geniustex/Component> ;
        <http://www.w3.org/2000/01/rdf-schema#isDefinedBy>
                <https://vocab.eccenca.com/geniustex/> ;
        <http://www.w3.org/2000/01/rdf-schema#label>
                "consists of" ;
        <http://www.w3.org/2000/01/rdf-schema#range>
                <https://vocab.eccenca.com/geniustex/Material> ;
        <http://purl.org/dc/terms/issued>
                "2018-08-30"^^<http://www.w3.org/2001/XMLSchema#date> .

<https://vocab.eccenca.com/geniustex/processableLength>
        a       <http://www.w3.org/2002/07/owl#ObjectProperty> ;
        <http://www.w3.org/2000/01/rdf-schema#comment>
                "the processable length dimension (min and max) for the process" ;
        <http://www.w3.org/2000/01/rdf-schema#domain>
                <https://vocab.eccenca.com/geniustex/Process> ;
        <http://www.w3.org/2000/01/rdf-schema#isDefinedBy>
                <https://vocab.eccenca.com/geniustex/> ;
        <http://www.w3.org/2000/01/rdf-schema#label>
                "processable length" ;
        <http://purl.org/dc/terms/issued>
                "2019-07-09"^^<http://www.w3.org/2001/XMLSchema#date> .

<https://vocab.eccenca.com/geniustex/suppliedBy>
        a       <http://www.w3.org/2002/07/owl#ObjectProperty> ;
        <http://www.w3.org/2000/01/rdf-schema#comment>
                "Provider supplies the smart product component or process" ;
        <http://www.w3.org/2000/01/rdf-schema#domain>
                <https://vocab.eccenca.com/geniustex/SmartProduct> ;
        <http://www.w3.org/2000/01/rdf-schema#isDefinedBy>
                <https://vocab.eccenca.com/geniustex/> ;
        <http://www.w3.org/2000/01/rdf-schema#label>
                "is supplied by" ;
        <http://www.w3.org/2000/01/rdf-schema#range>
                <https://vocab.eccenca.com/geniustex/Provider> ;
        <http://purl.org/dc/terms/issued>
                "2018-05-21"^^<http://www.w3.org/2001/XMLSchema#date> ;
        <http://purl.org/dc/terms/modified>
                "2018-06-14"^^<http://www.w3.org/2001/XMLSchema#date> .

<https://vocab.eccenca.com/geniustex/hapticsignal>
        a       <https://vocab.eccenca.com/geniustex/SignalType> ;
        <http://www.w3.org/2000/01/rdf-schema#comment>
                "haptic signal, e.g., a vibration" ;
        <http://www.w3.org/2000/01/rdf-schema#isDefinedBy>
                <https://vocab.eccenca.com/geniustex/> ;
        <http://www.w3.org/2000/01/rdf-schema#label>
                "haptic actuator signal" ;
        <http://purl.org/dc/terms/issued>
                "2018-08-15"^^<http://www.w3.org/2001/XMLSchema#date> ;
        <http://purl.org/dc/terms/modified>
                "2019-04-15"^^<http://www.w3.org/2001/XMLSchema#date> .

<https://vocab.eccenca.com/geniustex/PropertyTest>
        a       <http://www.w3.org/2002/07/owl#Class> ;
        <http://www.w3.org/2000/01/rdf-schema#comment>
                "a one-time property test that checks if a certain property is fulfilled according to some given specification" ;
        <http://www.w3.org/2000/01/rdf-schema#isDefinedBy>
                <https://vocab.eccenca.com/geniustex/> ;
        <http://www.w3.org/2000/01/rdf-schema#label>
                "PropertyTest" ;
        <http://www.w3.org/2000/01/rdf-schema#subClassOf>
                <https://vocab.eccenca.com/geniustex/QualityControl> ;
        <http://purl.org/dc/terms/issued>
                "2018-06-15"^^<http://www.w3.org/2001/XMLSchema#date> ;
        <http://purl.org/dc/terms/modified>
                "2019-04-15"^^<http://www.w3.org/2001/XMLSchema#date> .

<https://vocab.eccenca.com/geniustex/hasSupplyType>
        a       <http://www.w3.org/2002/07/owl#ObjectProperty> ;
        <http://www.w3.org/2000/01/rdf-schema#comment>
                "how a component can be supplied (instant sample; instant series; sample lead time > 1 week; series lead time > 1 week)" ;
        <http://www.w3.org/2000/01/rdf-schema#domain>
                <https://vocab.eccenca.com/geniustex/Component> ;
        <http://www.w3.org/2000/01/rdf-schema#isDefinedBy>
                <https://vocab.eccenca.com/geniustex/> ;
        <http://www.w3.org/2000/01/rdf-schema#label>
                "has a supply type" ;
        <http://www.w3.org/2000/01/rdf-schema#range>
                <https://vocab.eccenca.com/geniustex/SupplyType> ;
        <http://purl.org/dc/terms/issued>
                "2018-09-30"^^<http://www.w3.org/2001/XMLSchema#date> .

<https://vocab.eccenca.com/geniustex/relatedTo>
        a       <http://www.w3.org/2002/07/owl#ObjectProperty> ;
        <http://www.w3.org/2000/01/rdf-schema#comment>
                "some components can be used with others" ;
        <http://www.w3.org/2000/01/rdf-schema#domain>
                <https://vocab.eccenca.com/geniustex/Component> ;
        <http://www.w3.org/2000/01/rdf-schema#isDefinedBy>
                <https://vocab.eccenca.com/geniustex/> ;
        <http://www.w3.org/2000/01/rdf-schema#label>
                "is related to" ;
        <http://www.w3.org/2000/01/rdf-schema#range>
                <https://vocab.eccenca.com/geniustex/Component> ;
        <http://purl.org/dc/terms/issued>
                "2018-05-21"^^<http://www.w3.org/2001/XMLSchema#date> ;
        <http://purl.org/dc/terms/modified>
                "2018-06-14"^^<http://www.w3.org/2001/XMLSchema#date> .

<https://vocab.eccenca.com/geniustex/hasEletricConnectionType>
        a       <http://www.w3.org/2002/07/owl#ObjectProperty> ;
        <http://www.w3.org/2000/01/rdf-schema#comment>
                "a functional module has a certain electric connection type " ;
        <http://www.w3.org/2000/01/rdf-schema#domain>
                <https://vocab.eccenca.com/geniustex/FunctionalModule> ;
        <http://www.w3.org/2000/01/rdf-schema#isDefinedBy>
                <https://vocab.eccenca.com/geniustex/> ;
        <http://www.w3.org/2000/01/rdf-schema#label>
                "has electric connection type" ;
        <http://www.w3.org/2000/01/rdf-schema#range>
                <https://vocab.eccenca.com/geniustex/ElectricConnectionType> ;
        <http://purl.org/dc/terms/issued>
                "2019-02-18"^^<http://www.w3.org/2001/XMLSchema#date> .

<http://www.ontology-of-units-of-measure.org/resource/om-2/Quantity>
        a       <http://www.w3.org/2002/07/owl#Class> ;
        <http://www.w3.org/2000/01/rdf-schema#comment>
                "A quantity is a representation of a quantifiable (standardised) aspect (such as length, mass, and time) of a phenomenon (e.g., a star, a molecule, or a food product). Quantities are classified according to similarity in their (implicit) metrological aspect, e.g. the length of my table and the length of my chair are both classified as length."@en ;
        <http://www.w3.org/2000/01/rdf-schema#isDefinedBy>
                <http://www.ontology-of-units-of-measure.org/resource/om-2/> ;
        <http://www.w3.org/2000/01/rdf-schema#label>
                "quantity"@en .

<https://vocab.eccenca.com/geniustex/appliedIn>
        a       <http://www.w3.org/2002/07/owl#ObjectProperty> ;
        <http://www.w3.org/2000/01/rdf-schema#comment>
                "a smart product is applied in certain application areas" ;
        <http://www.w3.org/2000/01/rdf-schema#domain>
                <https://vocab.eccenca.com/geniustex/SmartProduct> ;
        <http://www.w3.org/2000/01/rdf-schema#isDefinedBy>
                <https://vocab.eccenca.com/geniustex/> ;
        <http://www.w3.org/2000/01/rdf-schema#label>
                "is applied in" ;
        <http://www.w3.org/2000/01/rdf-schema#range>
                <https://vocab.eccenca.com/geniustex/ApplicationArea> ;
        <http://purl.org/dc/terms/issued>
                "2018-06-21"^^<http://www.w3.org/2001/XMLSchema#date> ;
        <http://purl.org/dc/terms/modified>
                "2018-06-21"^^<http://www.w3.org/2001/XMLSchema#date> .

<https://vocab.eccenca.com/geniustex/gripElastic>
        a       <http://www.w3.org/2002/07/owl#DatatypeProperty> ;
        <http://www.w3.org/2000/01/rdf-schema#comment>
                "boolean value to represent if the gripping of elastic materials feasible or not" ;
        <http://www.w3.org/2000/01/rdf-schema#domain>
                <https://vocab.eccenca.com/geniustex/Handling> ;
        <http://www.w3.org/2000/01/rdf-schema#isDefinedBy>
                <https://vocab.eccenca.com/geniustex/> ;
        <http://www.w3.org/2000/01/rdf-schema#label>
                "gripping of elastic materials feasible" ;
        <http://www.w3.org/2000/01/rdf-schema#range>
                <http://www.w3.org/2001/XMLSchema#boolean> ;
        <http://purl.org/dc/terms/issued>
                "2018-08-17"^^<http://www.w3.org/2001/XMLSchema#date> .

<https://vocab.eccenca.com/geniustex/Idea>
        a       <http://www.w3.org/2002/07/owl#Class> ;
        <http://www.w3.org/2000/01/rdf-schema#comment>
                "an idea for a smart product, can be missing technical/commercial implementation know how" ;
        <http://www.w3.org/2000/01/rdf-schema#isDefinedBy>
                <https://vocab.eccenca.com/geniustex/> ;
        <http://www.w3.org/2000/01/rdf-schema#label>
                "Idea" ;
        <http://www.w3.org/2000/01/rdf-schema#subClassOf>
                <https://vocab.eccenca.com/geniustex/CollaborationConcept> ;
        <http://purl.org/dc/terms/issued>
                "2018-09-30"^^<http://www.w3.org/2001/XMLSchema#date> .

<https://vocab.eccenca.com/geniustex/Sensor>
        a       <http://www.w3.org/2002/07/owl#Class> ;
        <http://www.w3.org/2000/01/rdf-schema#comment>
                "a component which detect events or changes in its environment" ;
        <http://www.w3.org/2000/01/rdf-schema#isDefinedBy>
                <https://vocab.eccenca.com/geniustex/> ;
        <http://www.w3.org/2000/01/rdf-schema#label>
                "Sensor" ;
        <http://www.w3.org/2000/01/rdf-schema#subClassOf>
                <https://vocab.eccenca.com/geniustex/FunctionalModule> ;
        <http://purl.org/dc/terms/issued>
                "2018-05-21"^^<http://www.w3.org/2001/XMLSchema#date> ;
        <http://purl.org/dc/terms/modified>
                "2018-06-14"^^<http://www.w3.org/2001/XMLSchema#date> .

<https://vocab.eccenca.com/geniustex/openness>
        a       <http://www.w3.org/2002/07/owl#DatatypeProperty> ;
        <http://www.w3.org/2000/01/rdf-schema#comment>
                "open or closed structure of data processing module. Outputs of open modules can be accessed and manipulated for further applications, e.g., via an interface (API)" ;
        <http://www.w3.org/2000/01/rdf-schema#domain>
                <https://vocab.eccenca.com/geniustex/DataProcessingModule> ;
        <http://www.w3.org/2000/01/rdf-schema#isDefinedBy>
                <https://vocab.eccenca.com/geniustex/> ;
        <http://www.w3.org/2000/01/rdf-schema#label>
                "openness" ;
        <http://www.w3.org/2000/01/rdf-schema#range>
                <http://www.w3.org/2001/XMLSchema#string> ;
        <http://purl.org/dc/terms/issued>
                "2018-08-15"^^<http://www.w3.org/2001/XMLSchema#date> ;
        <http://purl.org/dc/terms/modified>
                "2019-04-15"^^<http://www.w3.org/2001/XMLSchema#date> .

<https://vocab.eccenca.com/geniustex/printedpath>
        a       <https://vocab.eccenca.com/geniustex/ElectricConnectionType> ;
        <http://www.w3.org/2000/01/rdf-schema#comment>
                "a functional component has a printed path as electric connection type" ;
        <http://www.w3.org/2000/01/rdf-schema#isDefinedBy>
                <https://vocab.eccenca.com/geniustex/> ;
        <http://www.w3.org/2000/01/rdf-schema#label>
                "printed path" ;
        <http://purl.org/dc/terms/issued>
                "2019-02-22"^^<http://www.w3.org/2001/XMLSchema#date> .

<http://purl.org/vocab/vann/preferredNamespacePrefix>
        a       <http://www.w3.org/2002/07/owl#AnnotationProperty> ;
        <http://www.w3.org/2000/01/rdf-schema#isDefinedBy>
                <http://purl.org/vocab/vann/> .

<https://vocab.eccenca.com/geniustex/functionTested>
        a       <http://www.w3.org/2002/07/owl#DatatypeProperty> ;
        <http://www.w3.org/2000/01/rdf-schema#comment>
                "function tested by a functional control test" ;
        <http://www.w3.org/2000/01/rdf-schema#domain>
                <https://vocab.eccenca.com/geniustex/FunctionalControl> ;
        <http://www.w3.org/2000/01/rdf-schema#isDefinedBy>
                <https://vocab.eccenca.com/geniustex/> ;
        <http://www.w3.org/2000/01/rdf-schema#label>
                "function tested" ;
        <http://www.w3.org/2000/01/rdf-schema#range>
                <http://www.w3.org/2001/XMLSchema#string> ;
        <http://purl.org/dc/terms/issued>
                "2018-08-17"^^<http://www.w3.org/2001/XMLSchema#date> .

<https://vocab.eccenca.com/geniustex/invest>
        a       <http://www.w3.org/2002/07/owl#DatatypeProperty> ;
        <http://www.w3.org/2000/01/rdf-schema#comment>
                "relative investment costs of a process (high/medium/low, on 1-5 likert scale)" ;
        <http://www.w3.org/2000/01/rdf-schema#domain>
                <https://vocab.eccenca.com/geniustex/Process> ;
        <http://www.w3.org/2000/01/rdf-schema#isDefinedBy>
                <https://vocab.eccenca.com/geniustex/> ;
        <http://www.w3.org/2000/01/rdf-schema#label>
                "invest" ;
        <http://www.w3.org/2000/01/rdf-schema#range>
                <http://www.w3.org/2001/XMLSchema#integer> ;
        <http://purl.org/dc/terms/issued>
                "2018-10-03"^^<http://www.w3.org/2001/XMLSchema#date> .

<https://vocab.eccenca.com/geniustex/Separating>
        a       <http://www.w3.org/2002/07/owl#Class> ;
        <http://www.w3.org/2000/01/rdf-schema#comment>
                "a process step that disconnects two or more objects or divides an object into multiple distinct units" ;
        <http://www.w3.org/2000/01/rdf-schema#isDefinedBy>
                <https://vocab.eccenca.com/geniustex/> ;
        <http://www.w3.org/2000/01/rdf-schema#label>
                "Separating" ;
        <http://www.w3.org/2000/01/rdf-schema#subClassOf>
                <https://vocab.eccenca.com/geniustex/Process> ;
        <http://purl.org/dc/terms/issued>
                "2018-06-15"^^<http://www.w3.org/2001/XMLSchema#date> ;
        <http://purl.org/dc/terms/modified>
                "2019-04-15"^^<http://www.w3.org/2001/XMLSchema#date> .

<https://vocab.eccenca.com/geniustex/Component>
        a       <http://www.w3.org/2002/07/owl#Class> ;
        <http://www.w3.org/2000/01/rdf-schema#comment>
                "a (physical) component that is part of the smart product" ;
        <http://www.w3.org/2000/01/rdf-schema#isDefinedBy>
                <https://vocab.eccenca.com/geniustex/> ;
        <http://www.w3.org/2000/01/rdf-schema#label>
                "Component Module" ;
        <http://www.w3.org/2000/01/rdf-schema#subClassOf>
                <https://vocab.eccenca.com/geniustex/SmartProduct> ;
        <http://purl.org/dc/terms/issued>
                "2018-05-21"^^<http://www.w3.org/2001/XMLSchema#date> ;
        <http://purl.org/dc/terms/modified>
                "2018-06-14"^^<http://www.w3.org/2001/XMLSchema#date> .

<https://vocab.eccenca.com/geniustex/bidirectional>
        a       <https://vocab.eccenca.com/geniustex/ElasticityType> ;
        <http://www.w3.org/2000/01/rdf-schema#comment>
                "elasticity lengthwise and crosswise, i.e., able to resume its normal shape spontaneously after being stretched or compressed in either direction" ;
        <http://www.w3.org/2000/01/rdf-schema#isDefinedBy>
                <https://vocab.eccenca.com/geniustex/> ;
        <http://www.w3.org/2000/01/rdf-schema#label>
                "bidirectional" ;
        <http://purl.org/dc/terms/issued>
                "2018-09-30"^^<http://www.w3.org/2001/XMLSchema#date> ;
        <http://purl.org/dc/terms/modified>
                "2019-04-15"^^<http://www.w3.org/2001/XMLSchema#date> .

<https://vocab.eccenca.com/geniustex/oekotexstandard100>
        a       <https://vocab.eccenca.com/geniustex/NormedPropertyTest> ;
        <http://www.w3.org/2000/01/rdf-schema#comment>
                "oekotex standard 100 for testing ecological properties of textiles" ;
        <http://www.w3.org/2000/01/rdf-schema#isDefinedBy>
                <https://vocab.eccenca.com/geniustex/> ;
        <http://www.w3.org/2000/01/rdf-schema#label>
                "Oekotex Standard 100" ;
        <http://purl.org/dc/terms/issued>
                "2018-08-30"^^<http://www.w3.org/2001/XMLSchema#date> .

<https://vocab.eccenca.com/geniustex/SignalType>
        a       <http://www.w3.org/2002/07/owl#Class> ;
        <http://www.w3.org/2000/01/rdf-schema#comment>
                "signal type of an actuator (e.g., haptic, acoustic)" ;
        <http://www.w3.org/2000/01/rdf-schema#isDefinedBy>
                <https://vocab.eccenca.com/geniustex/> ;
        <http://www.w3.org/2000/01/rdf-schema#label>
                "Signal Type" ;
        <http://purl.org/dc/terms/issued>
                "2018-08-15"^^<http://www.w3.org/2001/XMLSchema#date> ;
        <http://purl.org/dc/terms/modified>
                "2019-04-15"^^<http://www.w3.org/2001/XMLSchema#date> .

<https://vocab.eccenca.com/geniustex/1weekseries>
        a       <https://vocab.eccenca.com/geniustex/SupplyType> ;
        <http://www.w3.org/2000/01/rdf-schema#comment>
                "supply of sample volume with lead time > 1 week" ;
        <http://www.w3.org/2000/01/rdf-schema#isDefinedBy>
                <https://vocab.eccenca.com/geniustex/> ;
        <http://www.w3.org/2000/01/rdf-schema#label>
                "series lead time > 1 week" ;
        <http://purl.org/dc/terms/issued>
                "2018-09-30"^^<http://www.w3.org/2001/XMLSchema#date> .

<https://vocab.eccenca.com/geniustex/chemicalsensor>
        a       <https://vocab.eccenca.com/geniustex/SensorType> ;
        <http://www.w3.org/2000/01/rdf-schema#comment>
                "sensors that detect chemical signals, e.g., certain substances" ;
        <http://www.w3.org/2000/01/rdf-schema#isDefinedBy>
                <https://vocab.eccenca.com/geniustex/> ;
        <http://www.w3.org/2000/01/rdf-schema#label>
                "chemical sensor" ;
        <http://purl.org/dc/terms/issued>
                "2018-08-15"^^<http://www.w3.org/2001/XMLSchema#date> ;
        <http://purl.org/dc/terms/modified>
                "2019-09-18"^^<http://www.w3.org/2001/XMLSchema#date> .

<https://vocab.eccenca.com/geniustex/SupplyType>
        a       <http://www.w3.org/2002/07/owl#Class> ;
        <http://www.w3.org/2000/01/rdf-schema#comment>
                "how a material or component can be supplied (instant sample; instant series; sample lead time > 1 week; series lead time > 1 week)" ;
        <http://www.w3.org/2000/01/rdf-schema#isDefinedBy>
                <https://vocab.eccenca.com/geniustex/> ;
        <http://www.w3.org/2000/01/rdf-schema#label>
                "Supply Type" ;
        <http://purl.org/dc/terms/issued>
                "2018-09-30"^^<http://www.w3.org/2001/XMLSchema#date> .

<https://vocab.eccenca.com/geniustex/processesComponent>
        a       <http://www.w3.org/2002/07/owl#ObjectProperty> ;
        <http://www.w3.org/2000/01/rdf-schema#comment>
                "process can work with component types" ;
        <http://www.w3.org/2000/01/rdf-schema#domain>
                <https://vocab.eccenca.com/geniustex/Process> ;
        <http://www.w3.org/2000/01/rdf-schema#isDefinedBy>
                <https://vocab.eccenca.com/geniustex/> ;
        <http://www.w3.org/2000/01/rdf-schema#label>
                "processes a component" ;
        <http://www.w3.org/2000/01/rdf-schema#range>
                <https://vocab.eccenca.com/geniustex/Component> ;
        <http://purl.org/dc/terms/issued>
                "2018-08-17"^^<http://www.w3.org/2001/XMLSchema#date> ;
        <http://purl.org/dc/terms/modified>
                "2018-08-30"^^<http://www.w3.org/2001/XMLSchema#date> .

<http://www.w3.org/ns/ssn/systems/Sensitivity>
        a       <http://www.w3.org/2002/07/owl#Class> ;
        <http://www.w3.org/2000/01/rdf-schema#comment>
                "As a Sensor Property: Sensitivity is the quotient of the change in a Result of Observation and the corresponding change in a value of an ObservableProperty being observed, under the defined Conditions.\n\n   As an Actuator Property: Sensitivity is the quotient of the change in a command of Actuation and the corresponding change in a value of an ActuatableProperty being acted on, under the defined Conditions."@en ;
        <http://www.w3.org/2000/01/rdf-schema#isDefinedBy>
                <http://www.w3.org/ns/ssn/systems/> ;
        <http://www.w3.org/2000/01/rdf-schema#label>
                "Sensitivity"@en ;
        <http://www.w3.org/2000/01/rdf-schema#subClassOf>
                <http://www.w3.org/ns/ssn/systems/SystemProperty> .

<https://vocab.eccenca.com/geniustex/woven>
        a       <https://vocab.eccenca.com/geniustex/PackageType> ;
        <http://www.w3.org/2000/01/rdf-schema#comment>
                "component is packaged within a woven fabric structure, e.g., for textile based or textile integrated components" ;
        <http://www.w3.org/2000/01/rdf-schema#isDefinedBy>
                <https://vocab.eccenca.com/geniustex/> ;
        <http://www.w3.org/2000/01/rdf-schema#label>
                "woven" ;
        <http://purl.org/dc/terms/issued>
                "2018-09-30"^^<http://www.w3.org/2001/XMLSchema#date> .

<https://vocab.eccenca.com/geniustex/ExtraLayerReelingDevice>
        a       <http://www.w3.org/2002/07/owl#Class> ;
        <http://www.w3.org/2000/01/rdf-schema#comment>
                "extra handling step needed when using reeling device" ;
        <http://www.w3.org/2000/01/rdf-schema#isDefinedBy>
                <https://vocab.eccenca.com/geniustex/> ;
        <http://www.w3.org/2000/01/rdf-schema#label>
                "Extra Layer for Reeling Device" ;
        <http://www.w3.org/2000/01/rdf-schema#subClassOf>
                <https://vocab.eccenca.com/geniustex/Handling> ;
        <http://purl.org/dc/terms/issued>
                "2018-09-19"^^<http://www.w3.org/2001/XMLSchema#date> ;
        <http://purl.org/dc/terms/modified>
                "2019-04-15"^^<http://www.w3.org/2001/XMLSchema#date> .

<https://vocab.eccenca.com/geniustex/robustness>
        a       <http://www.w3.org/2002/07/owl#DatatypeProperty> ;
        <http://www.w3.org/2000/01/rdf-schema#comment>
                "robustness/reproducibility of a process, i.e., if specified outcome can be achieved reliably over multiple iterations of the process (high/medium/low, on 1-5 likert scale)" ;
        <http://www.w3.org/2000/01/rdf-schema#domain>
                <https://vocab.eccenca.com/geniustex/Process> ;
        <http://www.w3.org/2000/01/rdf-schema#isDefinedBy>
                <https://vocab.eccenca.com/geniustex/> ;
        <http://www.w3.org/2000/01/rdf-schema#label>
                "robustness of process" ;
        <http://www.w3.org/2000/01/rdf-schema#range>
                <http://www.w3.org/2001/XMLSchema#string> ;
        <http://purl.org/dc/terms/issued>
                "2018-08-30"^^<http://www.w3.org/2001/XMLSchema#date> ;
        <http://purl.org/dc/terms/modified>
                "2019-04-15"^^<http://www.w3.org/2001/XMLSchema#date> .

<https://vocab.eccenca.com/geniustex/Cleaning>
        a       <http://www.w3.org/2002/07/owl#Class> ;
        <http://www.w3.org/2000/01/rdf-schema#comment>
                "a process step that removes dirt, marks, or stains from a part (Source: https://en.oxforddictionaries.com/definition/clean)" ;
        <http://www.w3.org/2000/01/rdf-schema#isDefinedBy>
                <https://vocab.eccenca.com/geniustex/> ;
        <http://www.w3.org/2000/01/rdf-schema#label>
                "Cleaning" ;
        <http://www.w3.org/2000/01/rdf-schema#subClassOf>
                <https://vocab.eccenca.com/geniustex/Handling> ;
        <http://purl.org/dc/terms/issued>
                "2018-09-19"^^<http://www.w3.org/2001/XMLSchema#date> ;
        <http://purl.org/dc/terms/modified>
                "2019-04-12"^^<http://www.w3.org/2001/XMLSchema#date> .

<https://vocab.eccenca.com/geniustex/infotext>
        a       <http://www.w3.org/2002/07/owl#DatatypeProperty> ;
        <http://www.w3.org/2000/01/rdf-schema#comment>
                "textual guideline for component usage" ;
        <http://www.w3.org/2000/01/rdf-schema#isDefinedBy>
                <https://vocab.eccenca.com/geniustex/> ;
        <http://www.w3.org/2000/01/rdf-schema#label>
                "information text" ;
        <http://www.w3.org/2000/01/rdf-schema#range>
                <http://www.w3.org/2001/XMLSchema#string> ;
        <http://purl.org/dc/terms/issued>
                "2019-05-15"^^<http://www.w3.org/2001/XMLSchema#date> .

<https://vocab.eccenca.com/geniustex/integrated>
        a       <https://vocab.eccenca.com/geniustex/LevelTextileIntegration> ;
        <http://www.w3.org/2000/01/rdf-schema#comment>
                "textile-integrated smart products (between based and adapted) (Source: Bosowski et al. Design and manufacture\nof textile-based sensors. In Electronic Textiles: Smart Fabrics and Wearable Technology)" ;
        <http://www.w3.org/2000/01/rdf-schema#isDefinedBy>
                <https://vocab.eccenca.com/geniustex/> ;
        <http://www.w3.org/2000/01/rdf-schema#label>
                "integrated" ;
        <http://purl.org/dc/terms/issued>
                "2018-08-15"^^<http://www.w3.org/2001/XMLSchema#date> ;
        <http://purl.org/dc/terms/modified>
                "2019-04-15"^^<http://www.w3.org/2001/XMLSchema#date> .

<https://vocab.eccenca.com/geniustex/includesComponent>
        a       <http://www.w3.org/2002/07/owl#ObjectProperty> ;
        <http://www.w3.org/2000/01/rdf-schema#comment>
                "a component includes other component (besides the module/class is has been applied to)" ;
        <http://www.w3.org/2000/01/rdf-schema#domain>
                <https://vocab.eccenca.com/geniustex/Component> ;
        <http://www.w3.org/2000/01/rdf-schema#isDefinedBy>
                <https://vocab.eccenca.com/geniustex/> ;
        <http://www.w3.org/2000/01/rdf-schema#label>
                "includes a component" ;
        <http://www.w3.org/2000/01/rdf-schema#range>
                <https://vocab.eccenca.com/geniustex/Component> ;
        <http://purl.org/dc/terms/issued>
                "2019-02-14"^^<http://www.w3.org/2001/XMLSchema#date> .

<https://vocab.eccenca.com/geniustex/hasPackageType>
        a       <http://www.w3.org/2002/07/owl#ObjectProperty> ;
        <http://www.w3.org/2000/01/rdf-schema#comment>
                "every component has a package or mounting type" ;
        <http://www.w3.org/2000/01/rdf-schema#domain>
                <https://vocab.eccenca.com/geniustex/Component> ;
        <http://www.w3.org/2000/01/rdf-schema#isDefinedBy>
                <https://vocab.eccenca.com/geniustex/> ;
        <http://www.w3.org/2000/01/rdf-schema#label>
                "has a package type" ;
        <http://www.w3.org/2000/01/rdf-schema#range>
                <https://vocab.eccenca.com/geniustex/PackageType> ;
        <http://purl.org/dc/terms/issued>
                "2018-09-30"^^<http://www.w3.org/2001/XMLSchema#date> .

<https://vocab.eccenca.com/geniustex/QualityControl>
        a       <http://www.w3.org/2002/07/owl#Class> ;
        <http://www.w3.org/2000/01/rdf-schema#comment>
                "a  process step where the quality of a process or product is checked" ;
        <http://www.w3.org/2000/01/rdf-schema#isDefinedBy>
                <https://vocab.eccenca.com/geniustex/> ;
        <http://www.w3.org/2000/01/rdf-schema#label>
                "Quality Control" ;
        <http://www.w3.org/2000/01/rdf-schema#subClassOf>
                <https://vocab.eccenca.com/geniustex/Process> ;
        <http://purl.org/dc/terms/issued>
                "2018-06-15"^^<http://www.w3.org/2001/XMLSchema#date> ;
        <http://purl.org/dc/terms/modified>
                "2019-04-15"^^<http://www.w3.org/2001/XMLSchema#date> .

<https://vocab.eccenca.com/geniustex/thermicalsignal>
        a       <https://vocab.eccenca.com/geniustex/SignalType> ;
        <http://www.w3.org/2000/01/rdf-schema#comment>
                "the signal of a thermical actuator, e.g., change in temperature" ;
        <http://www.w3.org/2000/01/rdf-schema#isDefinedBy>
                <https://vocab.eccenca.com/geniustex/> ;
        <http://www.w3.org/2000/01/rdf-schema#label>
                "thermical actuator signal" ;
        <http://purl.org/dc/terms/issued>
                "2018-08-15"^^<http://www.w3.org/2001/XMLSchema#date> ;
        <http://purl.org/dc/terms/modified>
                "2019-04-15"^^<http://www.w3.org/2001/XMLSchema#date> .

<https://vocab.eccenca.com/geniustex/usesMaterial>
        a       <http://www.w3.org/2002/07/owl#ObjectProperty> ;
        <http://www.w3.org/2000/01/rdf-schema#comment>
                "a collaboration concept can use/refer to a material" ;
        <http://www.w3.org/2000/01/rdf-schema#domain>
                <https://vocab.eccenca.com/geniustex/CollaborationConcept> ;
        <http://www.w3.org/2000/01/rdf-schema#isDefinedBy>
                <https://vocab.eccenca.com/geniustex/> ;
        <http://www.w3.org/2000/01/rdf-schema#label>
                "uses material" ;
        <http://www.w3.org/2000/01/rdf-schema#range>
                <https://vocab.eccenca.com/geniustex/Material> ;
        <http://purl.org/dc/terms/issued>
                "2018-09-30"^^<http://www.w3.org/2001/XMLSchema#date> .

<https://vocab.eccenca.com/geniustex/Calibrating>
        a       <http://www.w3.org/2002/07/owl#Class> ;
        <http://www.w3.org/2000/01/rdf-schema#comment>
                "a process step to mark (a gauge or instrument) with a standard scale of readings (Source: https://en.oxforddictionaries.com/definition/calibrate)" ;
        <http://www.w3.org/2000/01/rdf-schema#isDefinedBy>
                <https://vocab.eccenca.com/geniustex/> ;
        <http://www.w3.org/2000/01/rdf-schema#label>
                "Calibrating" ;
        <http://www.w3.org/2000/01/rdf-schema#subClassOf>
                <https://vocab.eccenca.com/geniustex/QualityControl> ;
        <http://purl.org/dc/terms/issued>
                "2018-06-15"^^<http://www.w3.org/2001/XMLSchema#date> ;
        <http://purl.org/dc/terms/modified>
                "2019-04-12"^^<http://www.w3.org/2001/XMLSchema#date> .

<https://vocab.eccenca.com/geniustex/processableHeigth>
        a       <http://www.w3.org/2002/07/owl#ObjectProperty> ;
        <http://www.w3.org/2000/01/rdf-schema#comment>
                "the processable heigth dimension (min and max) for the process" ;
        <http://www.w3.org/2000/01/rdf-schema#domain>
                <https://vocab.eccenca.com/geniustex/Process> ;
        <http://www.w3.org/2000/01/rdf-schema#isDefinedBy>
                <https://vocab.eccenca.com/geniustex/> ;
        <http://www.w3.org/2000/01/rdf-schema#label>
                "processable height" ;
        <http://purl.org/dc/terms/issued>
                "2019-07-09"^^<http://www.w3.org/2001/XMLSchema#date> .

<https://vocab.eccenca.com/geniustex/SensorType>
        a       <http://www.w3.org/2002/07/owl#Class> ;
        <http://www.w3.org/2000/01/rdf-schema#comment>
                "type of a sensor, i.e., which type of signals can be detected by a sensor (e.g., optical, or thermical signals)" ;
        <http://www.w3.org/2000/01/rdf-schema#isDefinedBy>
                <https://vocab.eccenca.com/geniustex/> ;
        <http://www.w3.org/2000/01/rdf-schema#label>
                "Sensor Type" ;
        <http://purl.org/dc/terms/issued>
                "2018-08-15"^^<http://www.w3.org/2001/XMLSchema#date> ;
        <http://purl.org/dc/terms/modified>
                "2019-04-15"^^<http://www.w3.org/2001/XMLSchema#date> .

<https://vocab.eccenca.com/geniustex/payload>
        a       <http://www.w3.org/2002/07/owl#DatatypeProperty> ;
        <http://www.w3.org/2000/01/rdf-schema#comment>
                "payload that can be moved or carried by a handling device (kg)" ;
        <http://www.w3.org/2000/01/rdf-schema#domain>
                <https://vocab.eccenca.com/geniustex/Handling> ;
        <http://www.w3.org/2000/01/rdf-schema#isDefinedBy>
                <https://vocab.eccenca.com/geniustex/> ;
        <http://www.w3.org/2000/01/rdf-schema#label>
                "payload" ;
        <http://www.w3.org/2000/01/rdf-schema#range>
                <http://www.w3.org/2001/XMLSchema#float> ;
        <http://purl.org/dc/terms/issued>
                "2018-08-15"^^<http://www.w3.org/2001/XMLSchema#date> ;
        <http://purl.org/dc/terms/modified>
                "2019-04-15"^^<http://www.w3.org/2001/XMLSchema#date> .

<https://vocab.eccenca.com/geniustex/supplyVoltage>
        a       <http://www.w3.org/2002/07/owl#ObjectProperty> ;
        <http://www.w3.org/2000/01/rdf-schema#comment>
                "voltage needed to operate a component" ;
        <http://www.w3.org/2000/01/rdf-schema#domain>
                <https://vocab.eccenca.com/geniustex/FunctionalModule> ;
        <http://www.w3.org/2000/01/rdf-schema#isDefinedBy>
                <https://vocab.eccenca.com/geniustex/> ;
        <http://www.w3.org/2000/01/rdf-schema#label>
                "supply voltage" ;
        <http://purl.org/dc/terms/issued>
                "2018-05-23"^^<http://www.w3.org/2001/XMLSchema#date> ;
        <http://purl.org/dc/terms/modified>
                "2019-04-15"^^<http://www.w3.org/2001/XMLSchema#date> .

<https://vocab.eccenca.com/geniustex/skincontact>
        a       <https://vocab.eccenca.com/geniustex/Usability> ;
        <http://www.w3.org/2000/01/rdf-schema#comment>
                "a product has skin contact" ;
        <http://www.w3.org/2000/01/rdf-schema#isDefinedBy>
                <https://vocab.eccenca.com/geniustex/> ;
        <http://www.w3.org/2000/01/rdf-schema#label>
                "skincontact" ;
        <http://purl.org/dc/terms/issued>
                "2018-10-03"^^<http://www.w3.org/2001/XMLSchema#date> .

<https://vocab.eccenca.com/geniustex/CollaborationConcept>
        a       <http://www.w3.org/2002/07/owl#Class> ;
        <http://www.w3.org/2000/01/rdf-schema#comment>
                "a collaboration concept is a setting where multiple users work together on a common topic" ;
        <http://www.w3.org/2000/01/rdf-schema#isDefinedBy>
                <https://vocab.eccenca.com/geniustex/> ;
        <http://www.w3.org/2000/01/rdf-schema#label>
                "Collaboration Concept" ;
        <http://purl.org/dc/terms/issued>
                "2018-09-30"^^<http://www.w3.org/2001/XMLSchema#date> ;
        <http://purl.org/dc/terms/modified>
                "2019-04-12"^^<http://www.w3.org/2001/XMLSchema#date> .

<https://vocab.eccenca.com/geniustex/stability>
        a       <http://www.w3.org/2002/07/owl#DatatypeProperty> ;
        <http://www.w3.org/2000/01/rdf-schema#comment>
                "mechanical stability of a contact (high/medium/low, on 1-5 likert scale)" ;
        <http://www.w3.org/2000/01/rdf-schema#domain>
                <https://vocab.eccenca.com/geniustex/Contacting> ;
        <http://www.w3.org/2000/01/rdf-schema#isDefinedBy>
                <https://vocab.eccenca.com/geniustex/> ;
        <http://www.w3.org/2000/01/rdf-schema#label>
                "mechanical stability" ;
        <http://www.w3.org/2000/01/rdf-schema#range>
                <http://www.w3.org/2001/XMLSchema#integer> ;
        <http://purl.org/dc/terms/issued>
                "2018-08-15"^^<http://www.w3.org/2001/XMLSchema#date> .

<http://www.w3.org/ns/ssn/systems/DetectionLimit>
        a       <http://www.w3.org/2002/07/owl#Class> ;
        <http://www.w3.org/2000/01/rdf-schema#comment>
                "An observed value for which the probability of falsely claiming the absence of a component in a material is beta, given a probability alpha of falsely claiming its presence."@en ;
        <http://www.w3.org/2000/01/rdf-schema#isDefinedBy>
                <http://www.w3.org/ns/ssn/systems/> ;
        <http://www.w3.org/2000/01/rdf-schema#label>
                "Detection Limit"@en ;
        <http://www.w3.org/2000/01/rdf-schema#subClassOf>
                <http://www.w3.org/ns/ssn/systems/SystemProperty> ;
        <http://www.w3.org/2000/01/rdf-schema#subClassOf>
                [ a       <http://www.w3.org/2002/07/owl#Restriction> ;
                  <http://www.w3.org/2002/07/owl#allValuesFrom>
                          [ a       <http://www.w3.org/2002/07/owl#Restriction> ;
                            <http://www.w3.org/2002/07/owl#allValuesFrom>
                                    <http://www.w3.org/ns/sosa/Sensor> ;
                            <http://www.w3.org/2002/07/owl#onProperty>
                                    [ <http://www.w3.org/2002/07/owl#inverseOf>
                                              <http://www.w3.org/ns/ssn/systems/hasSystemCapability> ]
                          ] ;
                  <http://www.w3.org/2002/07/owl#onProperty>
                          [ <http://www.w3.org/2002/07/owl#inverseOf>
                                    <http://www.w3.org/ns/ssn/systems/hasSystemProperty> ]
                ] .

<https://vocab.eccenca.com/geniustex/protech>
        a       <https://vocab.eccenca.com/geniustex/ApplicationArea> ;
        <http://www.w3.org/2000/01/rdf-schema#comment>
                "Personal, building and property protection  (Source: Gries et al. Textile Fertigungsverfahren: Eine Einf체hrung; Carl Hanser\nVerlag)" ;
        <http://www.w3.org/2000/01/rdf-schema#isDefinedBy>
                <https://vocab.eccenca.com/geniustex/> ;
        <http://www.w3.org/2000/01/rdf-schema#label>
                "protech" ;
        <http://purl.org/dc/terms/issued>
                "2019-04-15"^^<http://www.w3.org/2001/XMLSchema#date> .

<https://vocab.eccenca.com/geniustex/hasSignalType>
        a       <http://www.w3.org/2002/07/owl#ObjectProperty> ;
        <http://www.w3.org/2000/01/rdf-schema#comment>
                "an actuator gives signals of a certain type" ;
        <http://www.w3.org/2000/01/rdf-schema#domain>
                <https://vocab.eccenca.com/geniustex/Actuator> ;
        <http://www.w3.org/2000/01/rdf-schema#isDefinedBy>
                <https://vocab.eccenca.com/geniustex/> ;
        <http://www.w3.org/2000/01/rdf-schema#label>
                "has signal type" ;
        <http://www.w3.org/2000/01/rdf-schema#range>
                <https://vocab.eccenca.com/geniustex/SignalType> ;
        <http://purl.org/dc/terms/issued>
                "2018-08-15"^^<http://www.w3.org/2001/XMLSchema#date> ;
        <http://purl.org/dc/terms/modified>
                "2019-04-15"^^<http://www.w3.org/2001/XMLSchema#date> .

<https://vocab.eccenca.com/geniustex/instantseries>
        a       <https://vocab.eccenca.com/geniustex/SupplyType> ;
        <http://www.w3.org/2000/01/rdf-schema#comment>
                "supply of series volume instantaneously feasible" ;
        <http://www.w3.org/2000/01/rdf-schema#isDefinedBy>
                <https://vocab.eccenca.com/geniustex/> ;
        <http://www.w3.org/2000/01/rdf-schema#label>
                "instant series supply" ;
        <http://purl.org/dc/terms/issued>
                "2018-09-30"^^<http://www.w3.org/2001/XMLSchema#date> .

<https://vocab.eccenca.com/geniustex/temperatureJoining>
        a       <http://www.w3.org/2002/07/owl#ObjectProperty> ;
        <http://www.w3.org/2000/01/rdf-schema#comment>
                "temperature of joining process" ;
        <http://www.w3.org/2000/01/rdf-schema#domain>
                <https://vocab.eccenca.com/geniustex/Joining> ;
        <http://www.w3.org/2000/01/rdf-schema#isDefinedBy>
                <https://vocab.eccenca.com/geniustex/> ;
        <http://www.w3.org/2000/01/rdf-schema#label>
                "temperature (joining)" ;
        <http://purl.org/dc/terms/issued>
                "2018-08-15"^^<http://www.w3.org/2001/XMLSchema#date> ;
        <http://purl.org/dc/terms/modified>
                "2019-04-15"^^<http://www.w3.org/2001/XMLSchema#date> .

<https://vocab.eccenca.com/geniustex/hasSensorType>
        a       <http://www.w3.org/2002/07/owl#ObjectProperty> ;
        <http://www.w3.org/2000/01/rdf-schema#comment>
                "sensor detects signals of a certain type" ;
        <http://www.w3.org/2000/01/rdf-schema#domain>
                <https://vocab.eccenca.com/geniustex/Sensor> ;
        <http://www.w3.org/2000/01/rdf-schema#isDefinedBy>
                <https://vocab.eccenca.com/geniustex/> ;
        <http://www.w3.org/2000/01/rdf-schema#label>
                "has sensor type" ;
        <http://www.w3.org/2000/01/rdf-schema#range>
                <https://vocab.eccenca.com/geniustex/SensorType> ;
        <http://purl.org/dc/terms/issued>
                "2018-08-15"^^<http://www.w3.org/2001/XMLSchema#date> ;
        <http://purl.org/dc/terms/modified>
                "2019-04-15"^^<http://www.w3.org/2001/XMLSchema#date> .

<https://vocab.eccenca.com/geniustex/handcleaning>
        a       <https://vocab.eccenca.com/geniustex/Usability> ;
        <http://www.w3.org/2000/01/rdf-schema#comment>
                "a product needs to be cleaned just by hand (not machine)" ;
        <http://www.w3.org/2000/01/rdf-schema#isDefinedBy>
                <https://vocab.eccenca.com/geniustex/> ;
        <http://www.w3.org/2000/01/rdf-schema#label>
                "handcleaning" ;
        <http://purl.org/dc/terms/issued>
                "2018-10-03"^^<http://www.w3.org/2001/XMLSchema#date> .

<https://vocab.eccenca.com/geniustex/fibreyarnwire>
        a       <https://vocab.eccenca.com/geniustex/ElectricConnectionType> ;
        <http://www.w3.org/2000/01/rdf-schema#comment>
                "a functional component has a fibre or yarn ot wire as eletric connection type" ;
        <http://www.w3.org/2000/01/rdf-schema#isDefinedBy>
                <https://vocab.eccenca.com/geniustex/> ;
        <http://www.w3.org/2000/01/rdf-schema#label>
                "fibre or yarn or wire " ;
        <http://purl.org/dc/terms/issued>
                "2019-02-22"^^<http://www.w3.org/2001/XMLSchema#date> .

<http://purl.org/dc/terms/creator>
        a       <http://www.w3.org/2002/07/owl#AnnotationProperty> ;
        <http://www.w3.org/2000/01/rdf-schema#isDefinedBy>
                <http://purl.org/dc/terms/> .

<https://vocab.eccenca.com/geniustex/description>
        a       <http://www.w3.org/2002/07/owl#DatatypeProperty> ;
        <http://www.w3.org/2000/01/rdf-schema#comment>
                "a description of a process or component in text format" ;
        <http://www.w3.org/2000/01/rdf-schema#domain>
                <https://vocab.eccenca.com/geniustex/SmartProduct> ;
        <http://www.w3.org/2000/01/rdf-schema#isDefinedBy>
                <https://vocab.eccenca.com/geniustex/> ;
        <http://www.w3.org/2000/01/rdf-schema#label>
                "description of a product of process" ;
        <http://www.w3.org/2000/01/rdf-schema#range>
                <http://www.w3.org/2001/XMLSchema#string> ;
        <http://purl.org/dc/terms/issued>
                "2018-07-10"^^<http://www.w3.org/2001/XMLSchema#date> .

<https://vocab.eccenca.com/geniustex/indutech>
        a       <https://vocab.eccenca.com/geniustex/ApplicationArea> ;
        <http://www.w3.org/2000/01/rdf-schema#comment>
                "Filtration, cleaning, mechanical engineering, chemical and electrical industry  (Source: Gries et al. Textile Fertigungsverfahren: Eine Einf체hrung; Carl Hanser\nVerlag)" ;
        <http://www.w3.org/2000/01/rdf-schema#isDefinedBy>
                <https://vocab.eccenca.com/geniustex/> ;
        <http://www.w3.org/2000/01/rdf-schema#label>
                "indutech" ;
        <http://purl.org/dc/terms/issued>
                "2018-06-15"^^<http://www.w3.org/2001/XMLSchema#date> ;
        <http://purl.org/dc/terms/modified>
                "2019-04-15"^^<http://www.w3.org/2001/XMLSchema#date> .

<https://vocab.eccenca.com/geniustex/Handling>
        a       <http://www.w3.org/2002/07/owl#Class> ;
        <http://www.w3.org/2000/01/rdf-schema#comment>
                "a handling process step" ;
        <http://www.w3.org/2000/01/rdf-schema#isDefinedBy>
                <https://vocab.eccenca.com/geniustex/> ;
        <http://www.w3.org/2000/01/rdf-schema#label>
                "Handling" ;
        <http://www.w3.org/2000/01/rdf-schema#subClassOf>
                <https://vocab.eccenca.com/geniustex/Process> ;
        <http://purl.org/dc/terms/issued>
                "2018-06-15"^^<http://www.w3.org/2001/XMLSchema#date> .

<https://vocab.eccenca.com/geniustex/fineness>
        a       <http://www.w3.org/2002/07/owl#ObjectProperty> ;
        <http://www.w3.org/2000/01/rdf-schema#comment>
                "fineness of material in dtex" ;
        <http://www.w3.org/2000/01/rdf-schema#domain>
                <https://vocab.eccenca.com/geniustex/Material> ;
        <http://www.w3.org/2000/01/rdf-schema#isDefinedBy>
                <https://vocab.eccenca.com/geniustex/> ;
        <http://www.w3.org/2000/01/rdf-schema#label>
                "fineness of material" ;
        <http://purl.org/dc/terms/issued>
                "2018-08-30"^^<http://www.w3.org/2001/XMLSchema#date> ;
        <http://purl.org/dc/terms/modified>
                "2019-04-15"^^<http://www.w3.org/2001/XMLSchema#date> .

<https://vocab.eccenca.com/geniustex/hasSupplyTypeMat>
        a       <http://www.w3.org/2002/07/owl#ObjectProperty> ;
        <http://www.w3.org/2000/01/rdf-schema#comment>
                "how a material can be supplied (instant sample; instant series; sample lead time > 1 week; series lead time > 1 week)" ;
        <http://www.w3.org/2000/01/rdf-schema#domain>
                <https://vocab.eccenca.com/geniustex/Material> ;
        <http://www.w3.org/2000/01/rdf-schema#isDefinedBy>
                <https://vocab.eccenca.com/geniustex/> ;
        <http://www.w3.org/2000/01/rdf-schema#label>
                "has a material supply type" ;
        <http://www.w3.org/2000/01/rdf-schema#range>
                <https://vocab.eccenca.com/geniustex/SupplyType> ;
        <http://purl.org/dc/terms/issued>
                "2018-09-30"^^<http://www.w3.org/2001/XMLSchema#date> .

<https://vocab.eccenca.com/geniustex/FunctionalModule>
        a       <http://www.w3.org/2002/07/owl#Class> ;
        <http://www.w3.org/2000/01/rdf-schema#comment>
                "a component that adds (part of a ) functionality to the smart product" ;
        <http://www.w3.org/2000/01/rdf-schema#isDefinedBy>
                <https://vocab.eccenca.com/geniustex/> ;
        <http://www.w3.org/2000/01/rdf-schema#label>
                "Functional Module" ;
        <http://www.w3.org/2000/01/rdf-schema#subClassOf>
                <https://vocab.eccenca.com/geniustex/Component> ;
        <http://purl.org/dc/terms/issued>
                "2018-05-21"^^<http://www.w3.org/2001/XMLSchema#date> ;
        <http://purl.org/dc/terms/modified>
                "2018-06-14"^^<http://www.w3.org/2001/XMLSchema#date> .

<https://vocab.eccenca.com/geniustex/DataProcessingModule>
        a       <http://www.w3.org/2002/07/owl#Class> ;
        <http://www.w3.org/2000/01/rdf-schema#comment>
                "A module that is carrying out operations on data to retrieve, transform, or classify information, e.g., a microchip or a computer" ;
        <http://www.w3.org/2000/01/rdf-schema#isDefinedBy>
                <https://vocab.eccenca.com/geniustex/> ;
        <http://www.w3.org/2000/01/rdf-schema#label>
                "Data Processing Module" ;
        <http://www.w3.org/2000/01/rdf-schema#subClassOf>
                <https://vocab.eccenca.com/geniustex/FunctionalModule> ;
        <http://purl.org/dc/terms/issued>
                "2018-05-21"^^<http://www.w3.org/2001/XMLSchema#date> ;
        <http://purl.org/dc/terms/modified>
                "2019-04-15"^^<http://www.w3.org/2001/XMLSchema#date> .

<https://vocab.eccenca.com/geniustex/contactarea>
        a       <https://vocab.eccenca.com/geniustex/ElectricConnectionType> ;
        <http://www.w3.org/2000/01/rdf-schema#comment>
                "a functional component has a contact area in general as electric connection type which can not be further specified by the other instances of  \"ElectricConnectionType\"  (e.g. a plane or convex contact surface)" ;
        <http://www.w3.org/2000/01/rdf-schema#isDefinedBy>
                <https://vocab.eccenca.com/geniustex/> ;
        <http://www.w3.org/2000/01/rdf-schema#label>
                "contact area" ;
        <http://purl.org/dc/terms/issued>
                "2019-02-22"^^<http://www.w3.org/2001/XMLSchema#date> .

<https://vocab.eccenca.com/geniustex/SmartProduct>
        a       <http://www.w3.org/2002/07/owl#Class> ;
        <http://www.w3.org/2000/01/rdf-schema#comment>
                "a product with \"smart\" functionality " ;
        <http://www.w3.org/2000/01/rdf-schema#isDefinedBy>
                <https://vocab.eccenca.com/geniustex/> ;
        <http://www.w3.org/2000/01/rdf-schema#label>
                "Smart Product" ;
        <http://purl.org/dc/terms/issued>
                "2018-05-21"^^<http://www.w3.org/2001/XMLSchema#date> ;
        <http://purl.org/dc/terms/modified>
                "2018-06-14"^^<http://www.w3.org/2001/XMLSchema#date> .

<https://vocab.eccenca.com/geniustex/nobleach>
        a       <https://vocab.eccenca.com/geniustex/CareInstructions> ;
        <http://www.w3.org/2000/01/rdf-schema#comment>
                "a material cannot be bleached" ;
        <http://www.w3.org/2000/01/rdf-schema#isDefinedBy>
                <https://vocab.eccenca.com/geniustex/> ;
        <http://www.w3.org/2000/01/rdf-schema#label>
                "no bleaching" ;
        <http://purl.org/dc/terms/issued>
                "2019-02-28"^^<http://www.w3.org/2001/XMLSchema#date> .

<https://vocab.eccenca.com/geniustex/homepage>
        a       <http://www.w3.org/2002/07/owl#DatatypeProperty> ;
        <http://www.w3.org/2000/01/rdf-schema#comment>
                "link to further information on the smart product" ;
        <http://www.w3.org/2000/01/rdf-schema#domain>
                <https://vocab.eccenca.com/geniustex/SmartProduct> ;
        <http://www.w3.org/2000/01/rdf-schema#isDefinedBy>
                <https://vocab.eccenca.com/geniustex/> ;
        <http://www.w3.org/2000/01/rdf-schema#label>
                "homepage" ;
        <http://www.w3.org/2000/01/rdf-schema#range>
                <http://www.w3.org/2001/XMLSchema#string> ;
        <http://purl.org/dc/terms/issued>
                "2019-02-28"^^<http://www.w3.org/2001/XMLSchema#date> .

<https://ns.eccenca.com/mknuth>
        a       <http://xmlns.com/foaf/0.1/Person> , <http://purl.org/dc/terms/Agent> ;
        <http://xmlns.com/foaf/0.1/name>
                "Magnus Knuth" .

<https://vocab.eccenca.com/geniustex/Contacting>
        a       <http://www.w3.org/2002/07/owl#Class> ;
        <http://www.w3.org/2000/01/rdf-schema#comment>
                "a process step where electrical contacts with component modules are created. An electrical contact is an electrical circuit component that consists of  electrically conductive material. When a pair of contacts touch, they can pass an electrical current with a certain contact resistance, dependent on surface structure, surface chemistry and contact time; when the pair is separated by an insulating gap, then the pair does not pass a current. (Source: https://en.wikipedia.org/wiki/Electrical_contacts)" ;
        <http://www.w3.org/2000/01/rdf-schema#isDefinedBy>
                <https://vocab.eccenca.com/geniustex/> ;
        <http://www.w3.org/2000/01/rdf-schema#label>
                "Contacting" ;
        <http://www.w3.org/2000/01/rdf-schema#subClassOf>
                <https://vocab.eccenca.com/geniustex/Joining> ;
        <http://purl.org/dc/terms/issued>
                "2018-08-15"^^<http://www.w3.org/2001/XMLSchema#date> ;
        <http://purl.org/dc/terms/modified>
                "2019-04-12"^^<http://www.w3.org/2001/XMLSchema#date> .

<https://vocab.eccenca.com/geniustex/speed>
        a       <http://www.w3.org/2002/07/owl#DatatypeProperty> ;
        <http://www.w3.org/2000/01/rdf-schema#comment>
                "relative speed of a process (high/medium/low, on 1-5 likert scale)" ;
        <http://www.w3.org/2000/01/rdf-schema#domain>
                <https://vocab.eccenca.com/geniustex/Process> ;
        <http://www.w3.org/2000/01/rdf-schema#isDefinedBy>
                <https://vocab.eccenca.com/geniustex/> ;
        <http://www.w3.org/2000/01/rdf-schema#label>
                "speed of process" ;
        <http://www.w3.org/2000/01/rdf-schema#range>
                <http://www.w3.org/2001/XMLSchema#integer> ;
        <http://purl.org/dc/terms/issued>
                "2018-08-15"^^<http://www.w3.org/2001/XMLSchema#date> ;
        <http://purl.org/dc/terms/modified>
                "2019-04-15"^^<http://www.w3.org/2001/XMLSchema#date> .

<http://www.w3.org/ns/ssn/systems/OperatingRange>
        a       <http://www.w3.org/2002/07/owl#Class> ;
        <http://www.w3.org/2000/01/rdf-schema#comment>
                "Describes normal OperatingProperties of a System under some specified Conditions. For example, to the power requirement or maintenance schedule of a System under a specified temperature range.\n\n    In the absence of OperatingProperties, simply describes the Conditions in which a System is expected to operate.\n\n    The System continues to operate as defined using SystemCapability. If, however, the SurvivalRange is violated, the System is 'damaged' and SystemCapability specifications may no longer hold."@en ;
        <http://www.w3.org/2000/01/rdf-schema#isDefinedBy>
                <http://www.w3.org/ns/ssn/systems/> ;
        <http://www.w3.org/2000/01/rdf-schema#label>
                "Operating Range"@en ;
        <http://www.w3.org/2000/01/rdf-schema#subClassOf>
                <http://www.w3.org/ns/ssn/Property> .

<https://vocab.eccenca.com/geniustex/DataTransmissionModule>
        a       <http://www.w3.org/2002/07/owl#Class> ;
        <http://www.w3.org/2000/01/rdf-schema#comment>
                "a component which is dedicated to send and receive data by implementing a specific communication protocol" ;
        <http://www.w3.org/2000/01/rdf-schema#isDefinedBy>
                <https://vocab.eccenca.com/geniustex/> ;
        <http://www.w3.org/2000/01/rdf-schema#label>
                "Data Transmission Module" ;
        <http://www.w3.org/2000/01/rdf-schema#subClassOf>
                <https://vocab.eccenca.com/geniustex/FunctionalModule> ;
        <http://purl.org/dc/terms/issued>
                "2018-05-21"^^<http://www.w3.org/2001/XMLSchema#date> ;
        <http://purl.org/dc/terms/modified>
                "2018-06-14"^^<http://www.w3.org/2001/XMLSchema#date> .

<https://vocab.eccenca.com/geniustex/testNormID>
        a       <http://www.w3.org/2002/07/owl#DatatypeProperty> ;
        <http://www.w3.org/2000/01/rdf-schema#comment>
                "any normed property test has an ID by the norming institution (DIN, ISO,); international ID to be used (--> check if Database linking DIN names to IEC names can be used)" ;
        <http://www.w3.org/2000/01/rdf-schema#domain>
                <https://vocab.eccenca.com/geniustex/NormedPropertyTest> ;
        <http://www.w3.org/2000/01/rdf-schema#isDefinedBy>
                <https://vocab.eccenca.com/geniustex/> ;
        <http://www.w3.org/2000/01/rdf-schema#label>
                "ID of normed property test" ;
        <http://www.w3.org/2000/01/rdf-schema#range>
                <http://www.w3.org/2001/XMLSchema#string> ;
        <http://purl.org/dc/terms/issued>
                "2018-06-23"^^<http://www.w3.org/2001/XMLSchema#date> .

<https://vocab.eccenca.com/geniustex/solvesProblemDefinition>
        a       <http://www.w3.org/2002/07/owl#ObjectProperty> ;
        <http://www.w3.org/2000/01/rdf-schema#comment>
                "a solution refers to a problem definition" ;
        <http://www.w3.org/2000/01/rdf-schema#domain>
                <https://vocab.eccenca.com/geniustex/ProposedSolution> ;
        <http://www.w3.org/2000/01/rdf-schema#isDefinedBy>
                <https://vocab.eccenca.com/geniustex/> ;
        <http://www.w3.org/2000/01/rdf-schema#label>
                "solves problem definition" ;
        <http://www.w3.org/2000/01/rdf-schema#range>
                <https://vocab.eccenca.com/geniustex/ProblemDefinition> ;
        <http://purl.org/dc/terms/issued>
                "2018-09-30"^^<http://www.w3.org/2001/XMLSchema#date> .

<https://vocab.eccenca.com/geniustex/>
        a       <http://purl.org/vocommons/voaf#Vocabulary> , <http://www.w3.org/2002/07/owl#Ontology> ;
        <http://www.w3.org/2000/01/rdf-schema#comment>
                "Ontology for the modularization of Smart Textiles components."@en ;
        <http://www.w3.org/2000/01/rdf-schema#isDefinedBy>
                <https://vocab.eccenca.com/geniustex/> ;
        <http://www.w3.org/2000/01/rdf-schema#label>
                "GeniusTex - Smart Textiles Ontology"@en ;
        <http://purl.org/dc/terms/creator>
                <https://ns.eccenca.com/stramp> , <https://ns.eccenca.com/mknuth> , <https://ns.eccenca.com/extern.igehrke> ;
        <http://purl.org/dc/terms/issued>
                "2018-05-24"^^<http://www.w3.org/2001/XMLSchema#date> ;
        <http://purl.org/dc/terms/modified>
                "2018-09-21"^^<http://www.w3.org/2001/XMLSchema#date> ;
        <http://purl.org/dc/terms/publisher>
                <https://ns.eccenca.com/eccenca-GmbH> ;
        <http://purl.org/dc/terms/rights>
                "Copyright 짤 2018 GeniusTex Consortium" ;
        <http://purl.org/vocab/vann/preferredNamespacePrefix>
                "gt" ;
        <http://purl.org/vocab/vann/preferredNamespaceUri>
                "https://vocab.eccenca.com/geniustex/" ;
        <http://rdfs.org/ns/void#vocabulary>
                <http://xmlns.com/foaf/0.1/> , <http://purl.org/vocab/vann/> , <http://purl.org/dc/terms/> ;
        <http://www.w3.org/2002/07/owl#versionInfo>
                "v1.2.0-4-g058acee-dirty" .

<https://vocab.eccenca.com/geniustex/ElectricConnectionType>
        a       <http://www.w3.org/2002/07/owl#Class> ;
        <http://www.w3.org/2000/01/rdf-schema#comment>
                "Electric or electronic connection type of a functional component for external connection" ;
        <http://www.w3.org/2000/01/rdf-schema#isDefinedBy>
                <https://vocab.eccenca.com/geniustex/> ;
        <http://www.w3.org/2000/01/rdf-schema#label>
                "Electric connection type" ;
        <http://purl.org/dc/terms/issued>
                "2019-02-18"^^<http://www.w3.org/2001/XMLSchema#date> .

<https://vocab.eccenca.com/geniustex/DIN%5FEN%5FISO%5F10993-5>
        a       <https://vocab.eccenca.com/geniustex/NormedPropertyTest> ;
        <http://www.w3.org/2000/01/rdf-schema#comment>
                "DIN standard for testing cytotoxicity. Cytotoxicity is the quality of being toxic to cells. (Source: https://en.wikipedia.org/wiki/Cytotoxicity)" ;
        <http://www.w3.org/2000/01/rdf-schema#isDefinedBy>
                <https://vocab.eccenca.com/geniustex/> ;
        <http://www.w3.org/2000/01/rdf-schema#label>
                "cytotoxicity test" ;
        <http://purl.org/dc/terms/issued>
                "2018-08-30"^^<http://www.w3.org/2001/XMLSchema#date> ;
        <http://purl.org/dc/terms/modified>
                "2019-04-15"^^<http://www.w3.org/2001/XMLSchema#date> .

<https://vocab.eccenca.com/geniustex/Actuator>
        a       <http://www.w3.org/2002/07/owl#Class> ;
        <http://www.w3.org/2000/01/rdf-schema#comment>
                "a component which is responsible for moving and controlling a mechanism or system" ;
        <http://www.w3.org/2000/01/rdf-schema#isDefinedBy>
                <https://vocab.eccenca.com/geniustex/> ;
        <http://www.w3.org/2000/01/rdf-schema#label>
                "Actuator" ;
        <http://www.w3.org/2000/01/rdf-schema#subClassOf>
                <https://vocab.eccenca.com/geniustex/FunctionalModule> ;
        <http://purl.org/dc/terms/issued>
                "2018-05-21"^^<http://www.w3.org/2001/XMLSchema#date> ;
        <http://purl.org/dc/terms/modified>
                "2018-06-14"^^<http://www.w3.org/2001/XMLSchema#date> .

<https://vocab.eccenca.com/geniustex/hometech>
        a       <https://vocab.eccenca.com/geniustex/ApplicationArea> ;
        <http://www.w3.org/2000/01/rdf-schema#comment>
                "Furniture, upholstery, interior equipment, floor and wall coverings  (Source: Gries et al. Textile Fertigungsverfahren: Eine Einf체hrung; Carl Hanser\nVerlag)" ;
        <http://www.w3.org/2000/01/rdf-schema#isDefinedBy>
                <https://vocab.eccenca.com/geniustex/> ;
        <http://www.w3.org/2000/01/rdf-schema#label>
                "hometech" ;
        <http://purl.org/dc/terms/issued>
                "2018-06-15"^^<http://www.w3.org/2001/XMLSchema#date> ;
        <http://purl.org/dc/terms/modified>
                "2019-04-15"^^<http://www.w3.org/2001/XMLSchema#date> .

<https://vocab.eccenca.com/geniustex/gripFlexible>
        a       <http://www.w3.org/2002/07/owl#DatatypeProperty> ;
        <http://www.w3.org/2000/01/rdf-schema#comment>
                "boolean value to represent if gripping of flexible materials possible or not" ;
        <http://www.w3.org/2000/01/rdf-schema#domain>
                <https://vocab.eccenca.com/geniustex/Handling> ;
        <http://www.w3.org/2000/01/rdf-schema#isDefinedBy>
                <https://vocab.eccenca.com/geniustex/> ;
        <http://www.w3.org/2000/01/rdf-schema#label>
                "gripping of flexible materials possible" ;
        <http://www.w3.org/2000/01/rdf-schema#range>
                <http://www.w3.org/2001/XMLSchema#boolean> ;
        <http://purl.org/dc/terms/issued>
                "2018-08-17"^^<http://www.w3.org/2001/XMLSchema#date> .

<https://vocab.eccenca.com/geniustex/Quantity>
        a       <http://www.w3.org/2002/07/owl#Class> ;
        <http://www.w3.org/2000/01/rdf-schema#comment>
                "an aspect, usually an amount or numeric value, that can be measured by a sensor" ;
        <http://www.w3.org/2000/01/rdf-schema#isDefinedBy>
                <https://vocab.eccenca.com/geniustex/> ;
        <http://www.w3.org/2000/01/rdf-schema#label>
                "Quantity" ;
        <http://www.w3.org/2000/01/rdf-schema#subClassOf>
                <http://www.ontology-of-units-of-measure.org/resource/om-2/Quantity> ;
        <http://purl.org/dc/terms/issued>
                "2018-05-21"^^<http://www.w3.org/2001/XMLSchema#date> ;
        <http://purl.org/dc/terms/modified>
                "2019-04-15"^^<http://www.w3.org/2001/XMLSchema#date> .

<http://www.w3.org/ns/ssn/isPropertyOf>
        a       <http://www.w3.org/2002/07/owl#ObjectProperty> ;
        <http://www.w3.org/2000/01/rdf-schema#comment>
                "Relation between a Property and the entity it belongs to."@en ;
        <http://www.w3.org/2000/01/rdf-schema#isDefinedBy>
                <http://www.w3.org/ns/ssn/> ;
        <http://www.w3.org/2000/01/rdf-schema#label>
                "is property of"@en ;
        <http://www.w3.org/2002/07/owl#inverseOf>
                <http://www.w3.org/ns/ssn/hasProperty> .

<http://www.w3.org/ns/ssn/systems/Selectivity>
        a       <http://www.w3.org/2002/07/owl#Class> ;
        <http://www.w3.org/2000/01/rdf-schema#comment>
                "As a Sensor Property: Selectivity is a Property of a Sensor whereby it provides observed values for one or more ObservableProperties such that the Results for each ObservableProperty are independent of other Properties in the FeatureOfInterest being investigated,  under the defined Conditions.\n\n  As an Actuator Property: Selectivity is a Property of an Actuator whereby it acts on one or more ActuatableProperties such as the Results for each ActuatableProperty are independent of other Properties in the FeatureOfInterest being acted on, under the defined Conditions."@en ;
        <http://www.w3.org/2000/01/rdf-schema#isDefinedBy>
                <http://www.w3.org/ns/ssn/systems/> ;
        <http://www.w3.org/2000/01/rdf-schema#label>
                "Selectivity"@en ;
        <http://www.w3.org/2000/01/rdf-schema#subClassOf>
                <http://www.w3.org/ns/ssn/systems/SystemProperty> .

<https://vocab.eccenca.com/geniustex/title>
        a       <http://www.w3.org/2002/07/owl#DatatypeProperty> ;
        <http://www.w3.org/2000/01/rdf-schema#comment>
                "title of a collaboration concept" ;
        <http://www.w3.org/2000/01/rdf-schema#domain>
                <https://vocab.eccenca.com/geniustex/CollaborationConcept> ;
        <http://www.w3.org/2000/01/rdf-schema#isDefinedBy>
                <https://vocab.eccenca.com/geniustex/> ;
        <http://www.w3.org/2000/01/rdf-schema#label>
                "title" ;
        <http://www.w3.org/2000/01/rdf-schema#range>
                <http://www.w3.org/2001/XMLSchema#string> ;
        <http://purl.org/dc/terms/issued>
                "2018-09-30"^^<http://www.w3.org/2001/XMLSchema#date> .

<http://purl.org/vocab/vann/preferredNamespaceUri>
        a       <http://www.w3.org/2002/07/owl#AnnotationProperty> ;
        <http://www.w3.org/2000/01/rdf-schema#isDefinedBy>
                <http://purl.org/vocab/vann/> .

<http://www.w3.org/ns/ssn/systems/Resolution>
        a       <http://www.w3.org/2002/07/owl#Class> ;
        <http://www.w3.org/2000/01/rdf-schema#comment>
                "As a Sensor Property: the smallest difference in the value of a ObservableProperty being observed that would result in perceptably different values of Observation Results, under the defined Conditions. \n\n  As an Actuator Property: the smallest difference in the value of an Actuation command that would result in a value change of the ActuatableProperty being acted on, under the defined Conditions."@en ;
        <http://www.w3.org/2000/01/rdf-schema#isDefinedBy>
                <http://www.w3.org/ns/ssn/systems/> ;
        <http://www.w3.org/2000/01/rdf-schema#label>
                "Resolution"@en ;
        <http://www.w3.org/2000/01/rdf-schema#subClassOf>
                <http://www.w3.org/ns/ssn/systems/SystemProperty> .

<https://vocab.eccenca.com/geniustex/tht%5Fconnection>
        a       <https://vocab.eccenca.com/geniustex/ElectricConnectionType> ;
        <http://www.w3.org/2000/01/rdf-schema#comment>
                "a functional component has a Through-the-Hole-Technology connection type, i.e., for components having leads which are designed to go through holes to the other side of a circuit board for soldering." ;
        <http://www.w3.org/2000/01/rdf-schema#isDefinedBy>
                <https://vocab.eccenca.com/geniustex/> ;
        <http://www.w3.org/2000/01/rdf-schema#label>
                "Trough-the-Hole-Technology-connection" ;
        <http://purl.org/dc/terms/issued>
                "2019-02-22"^^<http://www.w3.org/2001/XMLSchema#date> ;
        <http://purl.org/dc/terms/modified>
                "2019-04-15"^^<http://www.w3.org/2001/XMLSchema#date> .

<https://vocab.eccenca.com/geniustex/constantContactResistance>
        a       <http://www.w3.org/2002/07/owl#DatatypeProperty> ;
        <http://www.w3.org/2000/01/rdf-schema#comment>
                "constant contact resistance of a contact (const to very fluctuating, on a 1-3 scale )" ;
        <http://www.w3.org/2000/01/rdf-schema#domain>
                <https://vocab.eccenca.com/geniustex/Contacting> ;
        <http://www.w3.org/2000/01/rdf-schema#isDefinedBy>
                <https://vocab.eccenca.com/geniustex/> ;
        <http://www.w3.org/2000/01/rdf-schema#label>
                "constant contact resistance" ;
        <http://www.w3.org/2000/01/rdf-schema#range>
                <http://www.w3.org/2001/XMLSchema#integer> ;
        <http://purl.org/dc/terms/issued>
                "2019-04-25"^^<http://www.w3.org/2001/XMLSchema#date> .

<https://vocab.eccenca.com/geniustex/Material>
        a       <http://www.w3.org/2002/07/owl#Class> ;
        <http://www.w3.org/2000/01/rdf-schema#comment>
                "material type" ;
        <http://www.w3.org/2000/01/rdf-schema#isDefinedBy>
                <https://vocab.eccenca.com/geniustex/> ;
        <http://www.w3.org/2000/01/rdf-schema#label>
                "Material" ;
        <http://purl.org/dc/terms/issued>
                "2018-08-30"^^<http://www.w3.org/2001/XMLSchema#date> .

<https://vocab.eccenca.com/geniustex/Carrier>
        a       <http://www.w3.org/2002/07/owl#Class> ;
        <http://www.w3.org/2000/01/rdf-schema#comment>
                "a (textile) material, often also called substrate, where functional components can be integrated and are thus \"carried\" by the textile substrate" ;
        <http://www.w3.org/2000/01/rdf-schema#isDefinedBy>
                <https://vocab.eccenca.com/geniustex/> ;
        <http://www.w3.org/2000/01/rdf-schema#label>
                "Carrier / Substrate" ;
        <http://www.w3.org/2000/01/rdf-schema#subClassOf>
                <https://vocab.eccenca.com/geniustex/Component> ;
        <http://purl.org/dc/terms/issued>
                "2018-05-21"^^<http://www.w3.org/2001/XMLSchema#date> ;
        <http://purl.org/dc/terms/modified>
                "2019-04-12"^^<http://www.w3.org/2001/XMLSchema#date> .

<https://vocab.eccenca.com/geniustex/nominalVoltage>
        a       <http://www.w3.org/2002/07/owl#ObjectProperty> ;
        <http://www.w3.org/2000/01/rdf-schema#comment>
                "nominal voltage of power supply module" ;
        <http://www.w3.org/2000/01/rdf-schema#domain>
                <https://vocab.eccenca.com/geniustex/PowerSupplyModule> ;
        <http://www.w3.org/2000/01/rdf-schema#isDefinedBy>
                <https://vocab.eccenca.com/geniustex/> ;
        <http://www.w3.org/2000/01/rdf-schema#label>
                "nominal voltage" ;
        <http://purl.org/dc/terms/issued>
                "2018-08-15"^^<http://www.w3.org/2001/XMLSchema#date> ;
        <http://purl.org/dc/terms/modified>
                "2019-04-15"^^<http://www.w3.org/2001/XMLSchema#date> .

<https://vocab.eccenca.com/geniustex/formclosure>
        a       <https://vocab.eccenca.com/geniustex/ConnectionType> ;
        <http://www.w3.org/2000/01/rdf-schema#comment>
                "connection in joining process created by form closure where two or more components are positioned against each other so that they block loosening the connection, e.g., screws or nuts" ;
        <http://www.w3.org/2000/01/rdf-schema#isDefinedBy>
                <https://vocab.eccenca.com/geniustex/> ;
        <http://www.w3.org/2000/01/rdf-schema#label>
                "form closure" ;
        <http://purl.org/dc/terms/issued>
                "2018-09-30"^^<http://www.w3.org/2001/XMLSchema#date> ;
        <http://purl.org/dc/terms/modified>
                "2019-04-15"^^<http://www.w3.org/2001/XMLSchema#date> .

<https://vocab.eccenca.com/geniustex/hasProposedSolution>
        a       <http://www.w3.org/2002/07/owl#ObjectProperty> ;
        <http://www.w3.org/2000/01/rdf-schema#comment>
                "a problem definition can have multiple proposed solutions" ;
        <http://www.w3.org/2000/01/rdf-schema#domain>
                <https://vocab.eccenca.com/geniustex/ProblemDefinition> ;
        <http://www.w3.org/2000/01/rdf-schema#isDefinedBy>
                <https://vocab.eccenca.com/geniustex/> ;
        <http://www.w3.org/2000/01/rdf-schema#label>
                "Has proposed Solution" ;
        <http://www.w3.org/2000/01/rdf-schema#range>
                <https://vocab.eccenca.com/geniustex/ProposedSolution> ;
        <http://purl.org/dc/terms/issued>
                "2018-09-30"^^<http://www.w3.org/2001/XMLSchema#date> .

<https://vocab.eccenca.com/geniustex/clothtech>
        a       <https://vocab.eccenca.com/geniustex/ApplicationArea> ;
        <http://www.w3.org/2000/01/rdf-schema#comment>
                "Clothing, shoes  (Source: Gries et al. Textile Fertigungsverfahren: Eine Einf체hrung; Carl Hanser\nVerlag)" ;
        <http://www.w3.org/2000/01/rdf-schema#isDefinedBy>
                <https://vocab.eccenca.com/geniustex/> ;
        <http://www.w3.org/2000/01/rdf-schema#label>
                "clothtech" ;
        <http://purl.org/dc/terms/issued>
                "2018-06-15"^^<http://www.w3.org/2001/XMLSchema#date> ;
        <http://purl.org/dc/terms/modified>
                "2019-04-15"^^<http://www.w3.org/2001/XMLSchema#date> .

<https://vocab.eccenca.com/geniustex/Joining>
        a       <http://www.w3.org/2002/07/owl#Class> ;
        <http://www.w3.org/2000/01/rdf-schema#comment>
                "a process step that unite two or more components to form one entity" ;
        <http://www.w3.org/2000/01/rdf-schema#isDefinedBy>
                <https://vocab.eccenca.com/geniustex/> ;
        <http://www.w3.org/2000/01/rdf-schema#label>
                "Joining" ;
        <http://www.w3.org/2000/01/rdf-schema#subClassOf>
                <https://vocab.eccenca.com/geniustex/Process> ;
        <http://purl.org/dc/terms/issued>
                "2018-06-15"^^<http://www.w3.org/2001/XMLSchema#date> ;
        <http://purl.org/dc/terms/modified>
                "2019-04-15"^^<http://www.w3.org/2001/XMLSchema#date> .

<https://vocab.eccenca.com/geniustex/hasTestResult>
        a       <http://www.w3.org/2002/07/owl#ObjectProperty> ;
        <http://www.w3.org/2000/01/rdf-schema#comment>
                "a smart product has a certain result in the property test that it conforms with" ;
        <http://www.w3.org/2000/01/rdf-schema#domain>
                <https://vocab.eccenca.com/geniustex/SmartProduct> ;
        <http://www.w3.org/2000/01/rdf-schema#isDefinedBy>
                <https://vocab.eccenca.com/geniustex/> ;
        <http://www.w3.org/2000/01/rdf-schema#label>
                "has test result" ;
        <http://www.w3.org/2000/01/rdf-schema#range>
                <https://vocab.eccenca.com/geniustex/TestResult> ;
        <http://purl.org/dc/terms/issued>
                "2018-08-30"^^<http://www.w3.org/2001/XMLSchema#date> .

<https://vocab.eccenca.com/geniustex/UnitOfMeasure>
        a       <http://www.w3.org/2002/07/owl#Class> ;
        <http://www.w3.org/2000/01/rdf-schema#comment>
                "a unit of measure" ;
        <http://www.w3.org/2000/01/rdf-schema#isDefinedBy>
                <https://vocab.eccenca.com/geniustex/> ;
        <http://www.w3.org/2000/01/rdf-schema#label>
                "Unit of measure" ;
        <http://www.w3.org/2000/01/rdf-schema#subClassOf>
                <http://www.ontology-of-units-of-measure.org/resource/om-2/Unit> ;
        <http://purl.org/dc/terms/issued>
                "2018-07-10"^^<http://www.w3.org/2001/XMLSchema#date> .

<http://www.w3.org/ns/ssn/systems/ActuationRange>
        a       <http://www.w3.org/2002/07/owl#Class> ;
        <http://www.w3.org/2000/01/rdf-schema#comment>
                "The set of values that the Actuator can return as the Result of an Actuation under the defined Conditions with the defined system properties."@en ;
        <http://www.w3.org/2000/01/rdf-schema#isDefinedBy>
                <http://www.w3.org/ns/ssn/systems/> ;
        <http://www.w3.org/2000/01/rdf-schema#label>
                "Actuation Range"@en ;
        <http://www.w3.org/2000/01/rdf-schema#subClassOf>
                <http://www.w3.org/ns/ssn/systems/SystemProperty> ;
        <http://www.w3.org/2000/01/rdf-schema#subClassOf>
                [ a       <http://www.w3.org/2002/07/owl#Restriction> ;
                  <http://www.w3.org/2002/07/owl#allValuesFrom>
                          [ a       <http://www.w3.org/2002/07/owl#Restriction> ;
                            <http://www.w3.org/2002/07/owl#allValuesFrom>
                                    <http://www.w3.org/ns/sosa/Actuator> ;
                            <http://www.w3.org/2002/07/owl#onProperty>
                                    [ <http://www.w3.org/2002/07/owl#inverseOf>
                                              <http://www.w3.org/ns/ssn/systems/hasSystemCapability> ]
                          ] ;
                  <http://www.w3.org/2002/07/owl#onProperty>
                          [ <http://www.w3.org/2002/07/owl#inverseOf>
                                    <http://www.w3.org/ns/ssn/systems/hasSystemProperty> ]
                ] .

<http://www.w3.org/ns/ssn/systems/Latency>
        a       <http://www.w3.org/2002/07/owl#Class> ;
        <http://www.w3.org/2000/01/rdf-schema#comment>
                "The time between a command for an Observation (resp. Actuation) and the Sensor providing a Result (resp. the Actuator operating the Actuation), under the defined Conditions."@en ;
        <http://www.w3.org/2000/01/rdf-schema#isDefinedBy>
                <http://www.w3.org/ns/ssn/systems/> ;
        <http://www.w3.org/2000/01/rdf-schema#label>
                "Latency"@en ;
        <http://www.w3.org/2000/01/rdf-schema#subClassOf>
                <http://www.w3.org/ns/ssn/systems/SystemProperty> .

<https://vocab.eccenca.com/geniustex/FmeaTest>
        a       <http://www.w3.org/2002/07/owl#Class> ;
        <http://www.w3.org/2000/01/rdf-schema#comment>
                "a failure mode and effect analysis (FMEA). An FMEA is often the first step of a system reliability study. It involves reviewing as many components, assemblies, and subsystems as possible to identify failure modes, and their causes and effects. For each component, the failure modes and their resulting effects on the rest of the system are recorded in a specific FMEA worksheet (Source: https://en.wikipedia.org/wiki/Failure_mode_and_effects_analysis)" ;
        <http://www.w3.org/2000/01/rdf-schema#isDefinedBy>
                <https://vocab.eccenca.com/geniustex/> ;
        <http://www.w3.org/2000/01/rdf-schema#label>
                "FMEA test" ;
        <http://www.w3.org/2000/01/rdf-schema#subClassOf>
                <https://vocab.eccenca.com/geniustex/NormedPropertyTest> ;
        <http://purl.org/dc/terms/issued>
                "2018-06-23"^^<http://www.w3.org/2001/XMLSchema#date> ;
        <http://purl.org/dc/terms/modified>
                "2019-04-15"^^<http://www.w3.org/2001/XMLSchema#date> .

<https://vocab.eccenca.com/geniustex/controls>
        a       <http://www.w3.org/2002/07/owl#ObjectProperty> ;
        <http://www.w3.org/2000/01/rdf-schema#comment>
                "a quality control step control a certain process" ;
        <http://www.w3.org/2000/01/rdf-schema#domain>
                <https://vocab.eccenca.com/geniustex/QualityControl> ;
        <http://www.w3.org/2000/01/rdf-schema#isDefinedBy>
                <https://vocab.eccenca.com/geniustex/> ;
        <http://www.w3.org/2000/01/rdf-schema#label>
                "controls" ;
        <http://www.w3.org/2000/01/rdf-schema#range>
                <https://vocab.eccenca.com/geniustex/Process> ;
        <http://purl.org/dc/terms/issued>
                "2018-08-15"^^<http://www.w3.org/2001/XMLSchema#date> .

<https://vocab.eccenca.com/geniustex/visibility>
        a       <http://www.w3.org/2002/07/owl#DatatypeProperty> ;
        <http://www.w3.org/2000/01/rdf-schema#comment>
                "visibility of a collaboration concept, i.e., which users can access, read and edit it" ;
        <http://www.w3.org/2000/01/rdf-schema#domain>
                <https://vocab.eccenca.com/geniustex/CollaborationConcept> ;
        <http://www.w3.org/2000/01/rdf-schema#isDefinedBy>
                <https://vocab.eccenca.com/geniustex/> ;
        <http://www.w3.org/2000/01/rdf-schema#label>
                "visibility" ;
        <http://www.w3.org/2000/01/rdf-schema#range>
                <http://www.w3.org/2001/XMLSchema#string> ;
        <http://purl.org/dc/terms/issued>
                "2018-09-30"^^<http://www.w3.org/2001/XMLSchema#date> ;
        <http://purl.org/dc/terms/modified>
                "2019-04-15"^^<http://www.w3.org/2001/XMLSchema#date> .

<https://vocab.eccenca.com/geniustex/mobilityTransmission>
        a       <http://www.w3.org/2002/07/owl#DatatypeProperty> ;
        <http://www.w3.org/2000/01/rdf-schema#comment>
                "if a data transmission module is suitable for mobile use (yes/no)" ;
        <http://www.w3.org/2000/01/rdf-schema#domain>
                <https://vocab.eccenca.com/geniustex/DataTransmissionModule> ;
        <http://www.w3.org/2000/01/rdf-schema#isDefinedBy>
                <https://vocab.eccenca.com/geniustex/> ;
        <http://www.w3.org/2000/01/rdf-schema#label>
                "mobility data transmission module" ;
        <http://www.w3.org/2000/01/rdf-schema#range>
                <http://www.w3.org/2001/XMLSchema#boolean> ;
        <http://purl.org/dc/terms/issued>
                "2018-10-03"^^<http://www.w3.org/2001/XMLSchema#date> .

<https://vocab.eccenca.com/geniustex/price>
        a       <http://www.w3.org/2002/07/owl#ObjectProperty> ;
        <http://www.w3.org/2000/01/rdf-schema#comment>
                "price of component (unit cost)" ;
        <http://www.w3.org/2000/01/rdf-schema#domain>
                <https://vocab.eccenca.com/geniustex/Component> ;
        <http://www.w3.org/2000/01/rdf-schema#isDefinedBy>
                <https://vocab.eccenca.com/geniustex/> ;
        <http://www.w3.org/2000/01/rdf-schema#label>
                "price" ;
        <http://purl.org/dc/terms/issued>
                "2018-05-21"^^<http://www.w3.org/2001/XMLSchema#date> ;
        <http://purl.org/dc/terms/modified>
                "2019-04-15"^^<http://www.w3.org/2001/XMLSchema#date> .

<https://vocab.eccenca.com/geniustex/componentGeometry>
        a       <http://www.w3.org/2002/07/owl#ObjectProperty> ;
        <http://www.w3.org/2000/01/rdf-schema#comment>
                "the geometric form of the component (length, width, height)" ;
        <http://www.w3.org/2000/01/rdf-schema#domain>
                <https://vocab.eccenca.com/geniustex/Component> ;
        <http://www.w3.org/2000/01/rdf-schema#isDefinedBy>
                <https://vocab.eccenca.com/geniustex/> ;
        <http://www.w3.org/2000/01/rdf-schema#label>
                "has component geometry" ;
        <http://www.w3.org/2000/01/rdf-schema#range>
                <https://vocab.eccenca.com/geniustex/ComponentGeometry> ;
        <http://purl.org/dc/terms/issued>
                "2018-10-15"^^<http://www.w3.org/2001/XMLSchema#date> ;
        <http://purl.org/dc/terms/modified>
                "2019-04-15"^^<http://www.w3.org/2001/XMLSchema#date> .

<https://vocab.eccenca.com/geniustex/consumptionCosts>
        a       <http://www.w3.org/2002/07/owl#DatatypeProperty> ;
        <http://www.w3.org/2000/01/rdf-schema#comment>
                "relative consumption costs of a process (high/medium/low, on 1-5 likert scale)" ;
        <http://www.w3.org/2000/01/rdf-schema#domain>
                <https://vocab.eccenca.com/geniustex/Process> ;
        <http://www.w3.org/2000/01/rdf-schema#isDefinedBy>
                <https://vocab.eccenca.com/geniustex/> ;
        <http://www.w3.org/2000/01/rdf-schema#label>
                "consumption costs" ;
        <http://www.w3.org/2000/01/rdf-schema#range>
                <http://www.w3.org/2001/XMLSchema#string> ;
        <http://purl.org/dc/terms/issued>
                "2018-10-03"^^<http://www.w3.org/2001/XMLSchema#date> .

<https://vocab.eccenca.com/geniustex/1weeksample>
        a       <https://vocab.eccenca.com/geniustex/SupplyType> ;
        <http://www.w3.org/2000/01/rdf-schema#comment>
                "supply of series volume with lead time > 1 week" ;
        <http://www.w3.org/2000/01/rdf-schema#isDefinedBy>
                <https://vocab.eccenca.com/geniustex/> ;
        <http://www.w3.org/2000/01/rdf-schema#label>
                "sample lead time > 1 week" ;
        <http://purl.org/dc/terms/issued>
                "2018-09-30"^^<http://www.w3.org/2001/XMLSchema#date> .

<https://vocab.eccenca.com/geniustex/transmissionRange>
        a       <http://www.w3.org/2002/07/owl#DatatypeProperty> ;
        <http://www.w3.org/2000/01/rdf-schema#comment>
                "range of data transmission" ;
        <http://www.w3.org/2000/01/rdf-schema#domain>
                <https://vocab.eccenca.com/geniustex/DataTransmissionModule> ;
        <http://www.w3.org/2000/01/rdf-schema#isDefinedBy>
                <https://vocab.eccenca.com/geniustex/> ;
        <http://www.w3.org/2000/01/rdf-schema#label>
                "transmission range" ;
        <http://www.w3.org/2000/01/rdf-schema#range>
                <http://www.w3.org/2001/XMLSchema#float> ;
        <http://purl.org/dc/terms/issued>
                "2018-08-15"^^<http://www.w3.org/2001/XMLSchema#date> .

<https://vocab.eccenca.com/geniustex/Curing>
        a       <http://www.w3.org/2002/07/owl#Class> ;
        <http://www.w3.org/2000/01/rdf-schema#comment>
                "a process step where a part undergoes hardening by a chemical process (with or without additional temperature) " ;
        <http://www.w3.org/2000/01/rdf-schema#isDefinedBy>
                <https://vocab.eccenca.com/geniustex/> ;
        <http://www.w3.org/2000/01/rdf-schema#label>
                "Curing" ;
        <http://www.w3.org/2000/01/rdf-schema#subClassOf>
                <https://vocab.eccenca.com/geniustex/Handling> ;
        <http://purl.org/dc/terms/issued>
                "2018-06-15"^^<http://www.w3.org/2001/XMLSchema#date> ;
        <http://purl.org/dc/terms/modified>
                "2019-04-12"^^<http://www.w3.org/2001/XMLSchema#date> .

<https://vocab.eccenca.com/geniustex/temperatureCuring>
        a       <http://www.w3.org/2002/07/owl#ObjectProperty> ;
        <http://www.w3.org/2000/01/rdf-schema#comment>
                "temperature of curing process" ;
        <http://www.w3.org/2000/01/rdf-schema#domain>
                <https://vocab.eccenca.com/geniustex/Curing> ;
        <http://www.w3.org/2000/01/rdf-schema#isDefinedBy>
                <https://vocab.eccenca.com/geniustex/> ;
        <http://www.w3.org/2000/01/rdf-schema#label>
                "temperature (curing)" ;
        <http://purl.org/dc/terms/issued>
                "2018-08-15"^^<http://www.w3.org/2001/XMLSchema#date> ;
        <http://purl.org/dc/terms/modified>
                "2019-04-15"^^<http://www.w3.org/2001/XMLSchema#date> .

<https://vocab.eccenca.com/geniustex/magneticsensor>
        a       <https://vocab.eccenca.com/geniustex/SensorType> ;
        <http://www.w3.org/2000/01/rdf-schema#comment>
                "sensors that detect changes in magnetic fields" ;
        <http://www.w3.org/2000/01/rdf-schema#isDefinedBy>
                <https://vocab.eccenca.com/geniustex/> ;
        <http://www.w3.org/2000/01/rdf-schema#label>
                "magnetic sensor" ;
        <http://purl.org/dc/terms/issued>
                "2018-08-15"^^<http://www.w3.org/2001/XMLSchema#date> ;
        <http://purl.org/dc/terms/modified>
                "2019-09-18"^^<http://www.w3.org/2001/XMLSchema#date> .

<https://vocab.eccenca.com/geniustex/hasUsability>
        a       <http://www.w3.org/2002/07/owl#ObjectProperty> ;
        <http://www.w3.org/2000/01/rdf-schema#comment>
                "a smart product has certain usability context requirements" ;
        <http://www.w3.org/2000/01/rdf-schema#domain>
                <https://vocab.eccenca.com/geniustex/SmartProduct> ;
        <http://www.w3.org/2000/01/rdf-schema#isDefinedBy>
                <https://vocab.eccenca.com/geniustex/> ;
        <http://www.w3.org/2000/01/rdf-schema#label>
                "has usability requirements" ;
        <http://www.w3.org/2000/01/rdf-schema#range>
                <https://vocab.eccenca.com/geniustex/Usability> ;
        <http://purl.org/dc/terms/issued>
                "2018-10-03"^^<http://www.w3.org/2001/XMLSchema#date> .

<https://vocab.eccenca.com/geniustex/flexibility>
        a       <http://www.w3.org/2002/07/owl#DatatypeProperty> ;
        <http://www.w3.org/2000/01/rdf-schema#comment>
                "flexibility of a component, i.e., if it is capable of bending easily without breaking (yes/no), applies mainly to interconnection modules" ;
        <http://www.w3.org/2000/01/rdf-schema#domain>
                <https://vocab.eccenca.com/geniustex/InterconnectionModule> ;
        <http://www.w3.org/2000/01/rdf-schema#isDefinedBy>
                <https://vocab.eccenca.com/geniustex/> ;
        <http://www.w3.org/2000/01/rdf-schema#label>
                "flexibility" ;
        <http://www.w3.org/2000/01/rdf-schema#range>
                <http://www.w3.org/2001/XMLSchema#boolean> ;
        <http://purl.org/dc/terms/issued>
                "2018-08-15"^^<http://www.w3.org/2001/XMLSchema#date> ;
        <http://purl.org/dc/terms/modified>
                "2019-04-15"^^<http://www.w3.org/2001/XMLSchema#date> .

<https://vocab.eccenca.com/geniustex/adapted>
        a       <https://vocab.eccenca.com/geniustex/LevelTextileIntegration> ;
        <http://www.w3.org/2000/01/rdf-schema#comment>
                "textile-adapted smart products (no textile integration) (Source: Bosowski et al. Design and manufacture\nof textile-based sensors. In Electronic Textiles: Smart Fabrics and Wearable Technology)" ;
        <http://www.w3.org/2000/01/rdf-schema#isDefinedBy>
                <https://vocab.eccenca.com/geniustex/> ;
        <http://www.w3.org/2000/01/rdf-schema#label>
                "adapted" ;
        <http://purl.org/dc/terms/issued>
                "2018-08-15"^^<http://www.w3.org/2001/XMLSchema#date> ;
        <http://purl.org/dc/terms/modified>
                "2019-04-15"^^<http://www.w3.org/2001/XMLSchema#date> .

<https://vocab.eccenca.com/geniustex/knitted>
        a       <https://vocab.eccenca.com/geniustex/PackageType> ;
        <http://www.w3.org/2000/01/rdf-schema#comment>
                "component is packaged within a knitted fabric structure, e.g., for textile based or textile integrated components" ;
        <http://www.w3.org/2000/01/rdf-schema#isDefinedBy>
                <https://vocab.eccenca.com/geniustex/> ;
        <http://www.w3.org/2000/01/rdf-schema#label>
                "knitted" ;
        <http://purl.org/dc/terms/issued>
                "2018-09-30"^^<http://www.w3.org/2001/XMLSchema#date> .

<https://vocab.eccenca.com/geniustex/AdditiveForming>
        a       <http://www.w3.org/2002/07/owl#Class> ;
        <http://www.w3.org/2000/01/rdf-schema#comment>
                "a forming process step that uses additive manufacturing techniques to permanently deform the part processed, e.g., 3D printing" ;
        <http://www.w3.org/2000/01/rdf-schema#isDefinedBy>
                <https://vocab.eccenca.com/geniustex/> ;
        <http://www.w3.org/2000/01/rdf-schema#label>
                "Additive forming" ;
        <http://www.w3.org/2000/01/rdf-schema#subClassOf>
                <https://vocab.eccenca.com/geniustex/Forming> ;
        <http://purl.org/dc/terms/issued>
                "2018-09-26"^^<http://www.w3.org/2001/XMLSchema#date> ;
        <http://purl.org/dc/terms/modified>
                "2019-04-12"^^<http://www.w3.org/2001/XMLSchema#date> .

<https://vocab.eccenca.com/geniustex/processesMaterial>
        a       <http://www.w3.org/2002/07/owl#ObjectProperty> ;
        <http://www.w3.org/2000/01/rdf-schema#comment>
                "process can process a certain material" ;
        <http://www.w3.org/2000/01/rdf-schema#domain>
                <https://vocab.eccenca.com/geniustex/Process> ;
        <http://www.w3.org/2000/01/rdf-schema#isDefinedBy>
                <https://vocab.eccenca.com/geniustex/> ;
        <http://www.w3.org/2000/01/rdf-schema#label>
                "processes a material" ;
        <http://www.w3.org/2000/01/rdf-schema#range>
                <https://vocab.eccenca.com/geniustex/Material> ;
        <http://purl.org/dc/terms/issued>
                "2018-08-30"^^<http://www.w3.org/2001/XMLSchema#date> .

<https://vocab.eccenca.com/geniustex/accuracyPosition>
        a       <http://www.w3.org/2002/07/owl#DatatypeProperty> ;
        <http://www.w3.org/2000/01/rdf-schema#comment>
                "This value represents the accuracy of positioning in mm" ;
        <http://www.w3.org/2000/01/rdf-schema#domain>
                <https://vocab.eccenca.com/geniustex/Handling> ;
        <http://www.w3.org/2000/01/rdf-schema#isDefinedBy>
                <https://vocab.eccenca.com/geniustex/> ;
        <http://www.w3.org/2000/01/rdf-schema#label>
                "accuracy of positioning" ;
        <http://www.w3.org/2000/01/rdf-schema#range>
                <http://www.w3.org/2001/XMLSchema#float> ;
        <http://purl.org/dc/terms/issued>
                "2018-08-17"^^<http://www.w3.org/2001/XMLSchema#date> .

<https://vocab.eccenca.com/geniustex/ApplicationArea>
        a       <http://www.w3.org/2002/07/owl#Class> ;
        <http://www.w3.org/2000/01/rdf-schema#comment>
                "application area where a smart textile or a functional module is usually applied as defined by Gries, T.; Veit, D.; Wulfhorst, B. Textile Fertigungsverfahren: Eine Einf체hrung; Carl Hanser\nVerlag GmbH Co. KG: Munich, Germany, 2014." ;
        <http://www.w3.org/2000/01/rdf-schema#isDefinedBy>
                <https://vocab.eccenca.com/geniustex/> ;
        <http://www.w3.org/2000/01/rdf-schema#label>
                "Application Area" ;
        <http://purl.org/dc/terms/issued>
                "2018-05-24"^^<http://www.w3.org/2001/XMLSchema#date> ;
        <http://purl.org/dc/terms/modified>
                "2019-04-12"^^<http://www.w3.org/2001/XMLSchema#date> .

<https://vocab.eccenca.com/geniustex/agrotech>
        a       <https://vocab.eccenca.com/geniustex/ApplicationArea> ;
        <http://www.w3.org/2000/01/rdf-schema#comment>
                "agricultural application, e.g., gardening and landscaping, agriculture and forestry, animal husbandry (Source: Gries et al. Textile Fertigungsverfahren: Eine Einf체hrung; Carl Hanser\nVerlag)" ;
        <http://www.w3.org/2000/01/rdf-schema#isDefinedBy>
                <https://vocab.eccenca.com/geniustex/> ;
        <http://www.w3.org/2000/01/rdf-schema#label>
                "agrotech" ;
        <http://purl.org/dc/terms/issued>
                "2018-06-15"^^<http://www.w3.org/2001/XMLSchema#date> ;
        <http://purl.org/dc/terms/modified>
                "2019-04-15"^^<http://www.w3.org/2001/XMLSchema#date> .

<https://vocab.eccenca.com/geniustex/hole>
        a       <https://vocab.eccenca.com/geniustex/ElectricConnectionType> ;
        <http://www.w3.org/2000/01/rdf-schema#comment>
                "a functional component has a hole as electric connection type " ;
        <http://www.w3.org/2000/01/rdf-schema#isDefinedBy>
                <https://vocab.eccenca.com/geniustex/> ;
        <http://www.w3.org/2000/01/rdf-schema#label>
                "hole" ;
        <http://purl.org/dc/terms/issued>
                "2019-02-22"^^<http://www.w3.org/2001/XMLSchema#date> .

<https://vocab.eccenca.com/geniustex/InterconnectionModule>
        a       <http://www.w3.org/2002/07/owl#Class> ;
        <http://www.w3.org/2000/01/rdf-schema#comment>
                "a functional module that provides (electrically or thermically) conductive connections between other moduels. It can be either a standard electronic component attached to a textile, e.g., a thin rigid of flexible board containing an electric circuit, or it can be a textile-based  connection, e.g. a conductive yarn weaved into a carrier fabric" ;
        <http://www.w3.org/2000/01/rdf-schema#isDefinedBy>
                <https://vocab.eccenca.com/geniustex/> ;
        <http://www.w3.org/2000/01/rdf-schema#label>
                "Interconnection module" ;
        <http://www.w3.org/2000/01/rdf-schema#subClassOf>
                <https://vocab.eccenca.com/geniustex/FunctionalModule> ;
        <http://purl.org/dc/terms/issued>
                "2018-05-21"^^<http://www.w3.org/2001/XMLSchema#date> ;
        <http://purl.org/dc/terms/modified>
                "2019-04-12"^^<http://www.w3.org/2001/XMLSchema#date> .

<http://www.w3.org/ns/ssn/systems/SystemCapability>
        a       <http://www.w3.org/2002/07/owl#Class> ;
        <http://www.w3.org/2000/01/rdf-schema#comment>
                "Describes normal measurement, actuation, sampling properties such as accuracy, range, precision, etc. of a System under some specified Conditions such as a temperature range.\n\nThe capabilities specified here are those that affect the primary purpose of the System, while those in OperatingRange represent the system's normal operating environment, including conditions that don't affect the observations or the actuations."@en ;
        <http://www.w3.org/2000/01/rdf-schema#isDefinedBy>
                <http://www.w3.org/ns/ssn/systems/> ;
        <http://www.w3.org/2000/01/rdf-schema#label>
                "System Capability"@en ;
        <http://www.w3.org/2000/01/rdf-schema#subClassOf>
                <http://www.w3.org/ns/ssn/Property> .

<https://vocab.eccenca.com/geniustex/corrosionResistance>
        a       <http://www.w3.org/2002/07/owl#DatatypeProperty> ;
        <http://www.w3.org/2000/01/rdf-schema#comment>
                "corrosion resistance of a contact (high/medium/low, on 1-3 likert scale)" ;
        <http://www.w3.org/2000/01/rdf-schema#domain>
                <https://vocab.eccenca.com/geniustex/Contacting> ;
        <http://www.w3.org/2000/01/rdf-schema#isDefinedBy>
                <https://vocab.eccenca.com/geniustex/> ;
        <http://www.w3.org/2000/01/rdf-schema#label>
                "corrosion resistance" ;
        <http://www.w3.org/2000/01/rdf-schema#range>
                <http://www.w3.org/2001/XMLSchema#integer> ;
        <http://purl.org/dc/terms/issued>
                "2019-04-25"^^<http://www.w3.org/2001/XMLSchema#date> .

<https://vocab.eccenca.com/geniustex/fibre>
        a       <https://vocab.eccenca.com/geniustex/PackageType> ;
        <http://www.w3.org/2000/01/rdf-schema#comment>
                "component is packaged as fibre, e.g., for textile based components" ;
        <http://www.w3.org/2000/01/rdf-schema#isDefinedBy>
                <https://vocab.eccenca.com/geniustex/> ;
        <http://www.w3.org/2000/01/rdf-schema#label>
                "fibre" ;
        <http://purl.org/dc/terms/issued>
                "2018-09-30"^^<http://www.w3.org/2001/XMLSchema#date> .

<https://vocab.eccenca.com/geniustex/conductivityContacting>
        a       <http://www.w3.org/2002/07/owl#DatatypeProperty> ;
        <http://www.w3.org/2000/01/rdf-schema#comment>
                "electrical conductivity (measure of a material's ability to conduct an electric current) of a connection created by a contacting process (S/m)" ;
        <http://www.w3.org/2000/01/rdf-schema#domain>
                <https://vocab.eccenca.com/geniustex/Contacting> ;
        <http://www.w3.org/2000/01/rdf-schema#isDefinedBy>
                <https://vocab.eccenca.com/geniustex/> ;
        <http://www.w3.org/2000/01/rdf-schema#label>
                "conductivity of contact" ;
        <http://www.w3.org/2000/01/rdf-schema#range>
                <http://www.w3.org/2001/XMLSchema#integer> ;
        <http://purl.org/dc/terms/issued>
                "2018-08-30"^^<http://www.w3.org/2001/XMLSchema#date> ;
        <http://purl.org/dc/terms/modified>
                "2019-04-15"^^<http://www.w3.org/2001/XMLSchema#date> .

<https://vocab.eccenca.com/geniustex/PowerSupplyModule>
        a       <http://www.w3.org/2002/07/owl#Class> ;
        <http://www.w3.org/2000/01/rdf-schema#comment>
                "a component which provides a source of energy (for other components)" ;
        <http://www.w3.org/2000/01/rdf-schema#isDefinedBy>
                <https://vocab.eccenca.com/geniustex/> ;
        <http://www.w3.org/2000/01/rdf-schema#label>
                "Power Supply Module" ;
        <http://www.w3.org/2000/01/rdf-schema#subClassOf>
                <https://vocab.eccenca.com/geniustex/FunctionalModule> ;
        <http://purl.org/dc/terms/issued>
                "2018-05-21"^^<http://www.w3.org/2001/XMLSchema#date> ;
        <http://purl.org/dc/terms/modified>
                "2018-06-14"^^<http://www.w3.org/2001/XMLSchema#date> .

<http://www.w3.org/ns/ssn/systems/hasSurvivalRange>
        a       <http://www.w3.org/2002/07/owl#ObjectProperty> ;
        <http://www.w3.org/2000/01/rdf-schema#comment>
                "Relation from a System to a SurvivalRange."@en ;
        <http://www.w3.org/2000/01/rdf-schema#domain>
                <https://vocab.eccenca.com/geniustex/FunctionalModule> ;
        <http://www.w3.org/2000/01/rdf-schema#isDefinedBy>
                <http://www.w3.org/ns/ssn/systems/> ;
        <http://www.w3.org/2000/01/rdf-schema#label>
                "has survival range"@en ;
        <http://www.w3.org/2000/01/rdf-schema#range>
                <http://www.w3.org/ns/ssn/systems/SurvivalRange> ;
        <http://www.w3.org/2000/01/rdf-schema#subPropertyOf>
                <http://www.w3.org/ns/ssn/hasProperty> .

<https://vocab.eccenca.com/geniustex/acusticsignal>
        a       <https://vocab.eccenca.com/geniustex/SignalType> ;
        <http://www.w3.org/2000/01/rdf-schema#comment>
                "acustic signals, like sound" ;
        <http://www.w3.org/2000/01/rdf-schema#isDefinedBy>
                <https://vocab.eccenca.com/geniustex/> ;
        <http://www.w3.org/2000/01/rdf-schema#label>
                "acustic actuator signal" ;
        <http://purl.org/dc/terms/issued>
                "2018-08-15"^^<http://www.w3.org/2001/XMLSchema#date> ;
        <http://purl.org/dc/terms/modified>
                "2019-04-15"^^<http://www.w3.org/2001/XMLSchema#date> .

<https://vocab.eccenca.com/geniustex/drapability>
        a       <http://www.w3.org/2002/07/owl#DatatypeProperty> ;
        <http://www.w3.org/2000/01/rdf-schema#comment>
                "drapability of a carrier component (very high drapability = 5 / high = 4 /medium = 3 / low = 2 / no drapability = 1)" ;
        <http://www.w3.org/2000/01/rdf-schema#domain>
                <https://vocab.eccenca.com/geniustex/Carrier> ;
        <http://www.w3.org/2000/01/rdf-schema#isDefinedBy>
                <https://vocab.eccenca.com/geniustex/> ;
        <http://www.w3.org/2000/01/rdf-schema#label>
                "drapability of a carrier" ;
        <http://www.w3.org/2000/01/rdf-schema#range>
                <http://www.w3.org/2001/XMLSchema#integer> ;
        <http://purl.org/dc/terms/issued>
                "2018-08-15"^^<http://www.w3.org/2001/XMLSchema#date> ;
        <http://purl.org/dc/terms/modified>
                "2019-04-15"^^<http://www.w3.org/2001/XMLSchema#date> .

<https://ns.eccenca.com/stramp>
        a       <http://purl.org/dc/terms/Agent> , <http://xmlns.com/foaf/0.1/Person> ;
        <http://xmlns.com/foaf/0.1/name>
                "Sebastian Tramp" .

<https://vocab.eccenca.com/geniustex/ProblemDefinition>
        a       <http://www.w3.org/2002/07/owl#Class> ;
        <http://www.w3.org/2000/01/rdf-schema#comment>
                "a problem to be solved for a smart product" ;
        <http://www.w3.org/2000/01/rdf-schema#isDefinedBy>
                <https://vocab.eccenca.com/geniustex/> ;
        <http://www.w3.org/2000/01/rdf-schema#label>
                "Problem Definition" ;
        <http://www.w3.org/2000/01/rdf-schema#subClassOf>
                <https://vocab.eccenca.com/geniustex/CollaborationConcept> ;
        <http://purl.org/dc/terms/issued>
                "2018-09-30"^^<http://www.w3.org/2001/XMLSchema#date> .

<https://vocab.eccenca.com/geniustex/Integrating>
        a       <http://www.w3.org/2002/07/owl#Class> ;
        <http://www.w3.org/2000/01/rdf-schema#comment>
                "a joining process step where components are  combined with textiles to form a whole" ;
        <http://www.w3.org/2000/01/rdf-schema#isDefinedBy>
                <https://vocab.eccenca.com/geniustex/> ;
        <http://www.w3.org/2000/01/rdf-schema#label>
                "Integrating" ;
        <http://www.w3.org/2000/01/rdf-schema#subClassOf>
                <https://vocab.eccenca.com/geniustex/Joining> ;
        <http://purl.org/dc/terms/issued>
                "2018-08-15"^^<http://www.w3.org/2001/XMLSchema#date> ;
        <http://purl.org/dc/terms/modified>
                "2019-07-22"^^<http://www.w3.org/2001/XMLSchema#date> .

<http://www.w3.org/ns/ssn/systems/SurvivalRange>
        a       <http://www.w3.org/2002/07/owl#Class> ;
        <http://www.w3.org/2000/01/rdf-schema#comment>
                "Describes survival capabilities of a System under some specified Conditions. For example, to the lifetime of a System under a specified temperature range.\n\nIn the absence of SurvivalProperties, simply describes the Conditions a System can be exposed to without damage. For example, the temperature range a System can withstand before being considered damaged.\n\nThe System continues to operate as defined using SystemCapability. If, however, the OperatingProperty is violated, the System is operating 'out of operating range' and SystemCapability specifications may no longer hold."@en ;
        <http://www.w3.org/2000/01/rdf-schema#isDefinedBy>
                <http://www.w3.org/ns/ssn/systems/> ;
        <http://www.w3.org/2000/01/rdf-schema#label>
                "Survival Range"@en ;
        <http://www.w3.org/2000/01/rdf-schema#subClassOf>
                <http://www.w3.org/ns/ssn/Property> .

<https://vocab.eccenca.com/geniustex/hasTestID>
        a       <http://www.w3.org/2002/07/owl#ObjectProperty> ;
        <http://www.w3.org/2000/01/rdf-schema#comment>
                "any normed property test has an ID by a norming institution (DIN, ISO,)" ;
        <http://www.w3.org/2000/01/rdf-schema#domain>
                <https://vocab.eccenca.com/geniustex/NormedPropertyTest> ;
        <http://www.w3.org/2000/01/rdf-schema#isDefinedBy>
                <https://vocab.eccenca.com/geniustex/> ;
        <http://www.w3.org/2000/01/rdf-schema#label>
                "has official ID" ;
        <http://www.w3.org/2000/01/rdf-schema#range>
                <https://vocab.eccenca.com/geniustex/NormedPropertyTest> ;
        <http://purl.org/dc/terms/issued>
                "2018-06-23"^^<http://www.w3.org/2001/XMLSchema#date> ;
        <http://purl.org/dc/terms/modified>
                "2019-04-15"^^<http://www.w3.org/2001/XMLSchema#date> .

<https://vocab.eccenca.com/geniustex/capacity>
        a       <http://www.w3.org/2002/07/owl#ObjectProperty> ;
        <http://www.w3.org/2000/01/rdf-schema#comment>
                "the amount of electric charge a power supply module can deliver at the rated voltage" ;
        <http://www.w3.org/2000/01/rdf-schema#domain>
                <https://vocab.eccenca.com/geniustex/PowerSupplyModule> ;
        <http://www.w3.org/2000/01/rdf-schema#isDefinedBy>
                <https://vocab.eccenca.com/geniustex/> ;
        <http://www.w3.org/2000/01/rdf-schema#label>
                "capacity" ;
        <http://purl.org/dc/terms/issued>
                "2018-08-15"^^<http://www.w3.org/2001/XMLSchema#date> ;
        <http://purl.org/dc/terms/modified>
                "2019-04-15"^^<http://www.w3.org/2001/XMLSchema#date> .

<https://vocab.eccenca.com/geniustex/Casing>
        a       <http://www.w3.org/2002/07/owl#Class> ;
        <http://www.w3.org/2000/01/rdf-schema#comment>
                "a non-textile cover or shell that protects or encloses the functional components of a smart textile" ;
        <http://www.w3.org/2000/01/rdf-schema#isDefinedBy>
                <https://vocab.eccenca.com/geniustex/> ;
        <http://www.w3.org/2000/01/rdf-schema#label>
                "Casing" ;
        <http://www.w3.org/2000/01/rdf-schema#subClassOf>
                <https://vocab.eccenca.com/geniustex/Carrier> ;
        <http://purl.org/dc/terms/issued>
                "2018-05-21"^^<http://www.w3.org/2001/XMLSchema#date> ;
        <http://purl.org/dc/terms/modified>
                "2019-04-12"^^<http://www.w3.org/2001/XMLSchema#date> .

<https://vocab.eccenca.com/geniustex/Provider>
        a       <http://www.w3.org/2002/07/owl#Class> ;
        <http://www.w3.org/2000/01/rdf-schema#comment>
                "a provider of a smart product process/component/." ;
        <http://www.w3.org/2000/01/rdf-schema#isDefinedBy>
                <https://vocab.eccenca.com/geniustex/> ;
        <http://www.w3.org/2000/01/rdf-schema#label>
                "Provider of Service / Product" ;
        <http://www.w3.org/2000/01/rdf-schema#subClassOf>
                <https://vocab.eccenca.com/geniustex/User> ;
        <http://purl.org/dc/terms/issued>
                "2018-05-21"^^<http://www.w3.org/2001/XMLSchema#date> ;
        <http://purl.org/dc/terms/modified>
                "2018-09-30"^^<http://www.w3.org/2001/XMLSchema#date> .

<https://vocab.eccenca.com/geniustex/Cutting>
        a       <http://www.w3.org/2002/07/owl#Class> ;
        <http://www.w3.org/2000/01/rdf-schema#comment>
                "a process step where a part is divided into pieces with a sharp implement" ;
        <http://www.w3.org/2000/01/rdf-schema#isDefinedBy>
                <https://vocab.eccenca.com/geniustex/> ;
        <http://www.w3.org/2000/01/rdf-schema#label>
                "Cutting " ;
        <http://www.w3.org/2000/01/rdf-schema#subClassOf>
                <https://vocab.eccenca.com/geniustex/Separating> ;
        <http://purl.org/dc/terms/issued>
                "2018-06-15"^^<http://www.w3.org/2001/XMLSchema#date> ;
        <http://purl.org/dc/terms/modified>
                "2019-04-12"^^<http://www.w3.org/2001/XMLSchema#date> .

<https://vocab.eccenca.com/geniustex/hasConnectionType>
        a       <http://www.w3.org/2002/07/owl#ObjectProperty> ;
        <http://www.w3.org/2000/01/rdf-schema#comment>
                "a joining process creates a connection of a certain type" ;
        <http://www.w3.org/2000/01/rdf-schema#domain>
                <https://vocab.eccenca.com/geniustex/Joining> ;
        <http://www.w3.org/2000/01/rdf-schema#isDefinedBy>
                <https://vocab.eccenca.com/geniustex/> ;
        <http://www.w3.org/2000/01/rdf-schema#label>
                "has a certain type of connection" ;
        <http://www.w3.org/2000/01/rdf-schema#range>
                <https://vocab.eccenca.com/geniustex/ConnectionType> ;
        <http://purl.org/dc/terms/issued>
                "2018-09-30"^^<http://www.w3.org/2001/XMLSchema#date> .

<https://vocab.eccenca.com/geniustex/Reach>
        a       <https://vocab.eccenca.com/geniustex/NormedPropertyTest> ;
        <http://www.w3.org/2000/01/rdf-schema#comment>
                "conforms with EU Registration, Evaluation, Authorisation and Restriction of Chemicals law" ;
        <http://www.w3.org/2000/01/rdf-schema#isDefinedBy>
                <https://vocab.eccenca.com/geniustex/> ;
        <http://www.w3.org/2000/01/rdf-schema#label>
                "Registration, Evaluation, Authorisation and Restriction of Chemicals" ;
        <http://purl.org/dc/terms/issued>
                "2018-08-30"^^<http://www.w3.org/2001/XMLSchema#date> .

<https://vocab.eccenca.com/geniustex/NormedPropertyTest>
        a       <http://www.w3.org/2002/07/owl#Class> ;
        <http://www.w3.org/2000/01/rdf-schema#comment>
                "a one-time property test according to a defined norm/standard" ;
        <http://www.w3.org/2000/01/rdf-schema#isDefinedBy>
                <https://vocab.eccenca.com/geniustex/> ;
        <http://www.w3.org/2000/01/rdf-schema#label>
                "Normed property test" ;
        <http://www.w3.org/2000/01/rdf-schema#subClassOf>
                <https://vocab.eccenca.com/geniustex/PropertyTest> ;
        <http://purl.org/dc/terms/issued>
                "2018-06-23"^^<http://www.w3.org/2001/XMLSchema#date> .

<https://vocab.eccenca.com/geniustex/LevelTextileIntegration>
        a       <http://www.w3.org/2002/07/owl#Class> ;
        <http://www.w3.org/2000/01/rdf-schema#comment>
                "the level of textile integration of a smart product. Textile-adapted: the textile does not cover an electronic function (0%), but\nelectronic components can be attached to the textile, e.g., a pocket for an MP3 player.\nTextile-integrated: the textile covers between 0 and 100% of the electronic\nfunction, creating an interface between the textile and the electronics. For example,\nflexible circuit boards can be integrated into textiles in this manner.\nTextile-based: electronic function is 100% covered by the textile.\nWhen considering an intelligent textile material, this can involve the realization of\nconductor paths and sensors made of conductive yarns (Source: Bosowski et al. Design and manufacture\nof textile-based sensors. In Electronic Textiles: Smart Fabrics and Wearable Technology)" ;
        <http://www.w3.org/2000/01/rdf-schema#isDefinedBy>
                <https://vocab.eccenca.com/geniustex/> ;
        <http://www.w3.org/2000/01/rdf-schema#label>
                "Textile Integration" ;
        <http://purl.org/dc/terms/issued>
                "2018-08-15"^^<http://www.w3.org/2001/XMLSchema#date> ;
        <http://purl.org/dc/terms/modified>
                "2019-04-15"^^<http://www.w3.org/2001/XMLSchema#date> .

<https://vocab.eccenca.com/geniustex/TestResult>
        a       <http://www.w3.org/2002/07/owl#Class> ;
        <http://www.w3.org/2000/01/rdf-schema#comment>
                "result of a conducted property test" ;
        <http://www.w3.org/2000/01/rdf-schema#isDefinedBy>
                <https://vocab.eccenca.com/geniustex/> ;
        <http://www.w3.org/2000/01/rdf-schema#label>
                "Result of Property Test" ;
        <http://www.w3.org/2000/01/rdf-schema#subClassOf>
                <https://vocab.eccenca.com/geniustex/PropertyTest> ;
        <http://purl.org/dc/terms/issued>
                "2018-08-30"^^<http://www.w3.org/2001/XMLSchema#date> .

<https://vocab.eccenca.com/geniustex/noiron>
        a       <https://vocab.eccenca.com/geniustex/CareInstructions> ;
        <http://www.w3.org/2000/01/rdf-schema#comment>
                "a material cannot be ironed" ;
        <http://www.w3.org/2000/01/rdf-schema#isDefinedBy>
                <https://vocab.eccenca.com/geniustex/> ;
        <http://www.w3.org/2000/01/rdf-schema#label>
                "no ironing" ;
        <http://purl.org/dc/terms/issued>
                "2019-02-28"^^<http://www.w3.org/2001/XMLSchema#date> .

<https://vocab.eccenca.com/geniustex/paste>
        a       <https://vocab.eccenca.com/geniustex/PackageType> ;
        <http://www.w3.org/2000/01/rdf-schema#comment>
                "component is packaged as paste, e.g., for textile based components" ;
        <http://www.w3.org/2000/01/rdf-schema#isDefinedBy>
                <https://vocab.eccenca.com/geniustex/> ;
        <http://www.w3.org/2000/01/rdf-schema#label>
                "paste" ;
        <http://purl.org/dc/terms/issued>
                "2019-02-15"^^<http://www.w3.org/2001/XMLSchema#date> .

<https://vocab.eccenca.com/geniustex/mechanicsensor>
        a       <https://vocab.eccenca.com/geniustex/SensorType> ;
        <http://www.w3.org/2000/01/rdf-schema#comment>
                "sensors that detect changes in mechanic properties, e.g., pressure" ;
        <http://www.w3.org/2000/01/rdf-schema#isDefinedBy>
                <https://vocab.eccenca.com/geniustex/> ;
        <http://www.w3.org/2000/01/rdf-schema#label>
                "mechanic sensor" ;
        <http://purl.org/dc/terms/issued>
                "2018-08-15"^^<http://www.w3.org/2001/XMLSchema#date> ;
        <http://purl.org/dc/terms/modified>
                "2019-09-18"^^<http://www.w3.org/2001/XMLSchema#date> .

<https://vocab.eccenca.com/geniustex/ComponentGeometry>
        a       <http://www.w3.org/2002/07/owl#Class> ;
        <http://www.w3.org/2000/01/rdf-schema#comment>
                "the geometric form of a component given by width, heigth and length" ;
        <http://www.w3.org/2000/01/rdf-schema#isDefinedBy>
                <https://vocab.eccenca.com/geniustex/> ;
        <http://www.w3.org/2000/01/rdf-schema#label>
                "Component Geometry" ;
        <http://purl.org/dc/terms/issued>
                "2018-10-15"^^<http://www.w3.org/2001/XMLSchema#date> ;
        <http://purl.org/dc/terms/modified>
                "2019-04-12"^^<http://www.w3.org/2001/XMLSchema#date> .

<http://www.w3.org/ns/ssn/systems/inCondition>
        a       <http://www.w3.org/2002/07/owl#ObjectProperty> ;
        <http://www.w3.org/2000/01/rdf-schema#comment>
                "Describes the prevailing environmental conditions for SystemCapabilites, OperatingRanges and SurvivalRanges."@en ;
        <http://www.w3.org/2000/01/rdf-schema#isDefinedBy>
                <http://www.w3.org/ns/ssn/systems/> ;
        <http://www.w3.org/2000/01/rdf-schema#label>
                "in condition"@en .

<https://ns.eccenca.com/extern.igehrke>
        a       <http://purl.org/dc/terms/Agent> , <http://xmlns.com/foaf/0.1/Person> ;
        <http://xmlns.com/foaf/0.1/name>
                "Inga Gehrke" .

<https://vocab.eccenca.com/geniustex/Usability>
        a       <http://www.w3.org/2002/07/owl#Class> ;
        <http://www.w3.org/2000/01/rdf-schema#comment>
                "usage context requirements of a smart product" ;
        <http://www.w3.org/2000/01/rdf-schema#isDefinedBy>
                <https://vocab.eccenca.com/geniustex/> ;
        <http://www.w3.org/2000/01/rdf-schema#label>
                "Usability" ;
        <http://purl.org/dc/terms/issued>
                "2018-10-03"^^<http://www.w3.org/2001/XMLSchema#date> .

<http://www.w3.org/ns/ssn/systems/Accuracy>
        a       <http://www.w3.org/2002/07/owl#Class> ;
        <http://www.w3.org/2000/01/rdf-schema#comment>
                "The closeness of agreement between the Result of an Observation (resp. the command of an Actuation) and the true value of the observed ObservableProperty (resp. of the acted on ActuatableProperty) under the defined Conditions."@en ;
        <http://www.w3.org/2000/01/rdf-schema#isDefinedBy>
                <http://www.w3.org/ns/ssn/systems/> ;
        <http://www.w3.org/2000/01/rdf-schema#label>
                "Accuracy"@en ;
        <http://www.w3.org/2000/01/rdf-schema#subClassOf>
                <http://www.w3.org/ns/ssn/systems/SystemProperty> .

<https://vocab.eccenca.com/geniustex/notumbledry>
        a       <https://vocab.eccenca.com/geniustex/CareInstructions> ;
        <http://www.w3.org/2000/01/rdf-schema#comment>
                "a material cannot be tumble dryed" ;
        <http://www.w3.org/2000/01/rdf-schema#isDefinedBy>
                <https://vocab.eccenca.com/geniustex/> ;
        <http://www.w3.org/2000/01/rdf-schema#label>
                "no tumble drying" ;
        <http://purl.org/dc/terms/issued>
                "2019-02-28"^^<http://www.w3.org/2001/XMLSchema#date> .

<https://vocab.eccenca.com/geniustex/mobiltech>
        a       <https://vocab.eccenca.com/geniustex/ApplicationArea> ;
        <http://www.w3.org/2000/01/rdf-schema#comment>
                "Vehicles of all kinds, ships, aviation and space travel  (Source: Gries et al. Textile Fertigungsverfahren: Eine Einf체hrung; Carl Hanser\nVerlag)" ;
        <http://www.w3.org/2000/01/rdf-schema#isDefinedBy>
                <https://vocab.eccenca.com/geniustex/> ;
        <http://www.w3.org/2000/01/rdf-schema#label>
                "mobiltech" ;
        <http://purl.org/dc/terms/issued>
                "2019-04-15"^^<http://www.w3.org/2001/XMLSchema#date> .

<https://vocab.eccenca.com/geniustex/TRL>
        a       <http://www.w3.org/2002/07/owl#DatatypeProperty> ;
        <http://www.w3.org/2000/01/rdf-schema#comment>
                "TRL of a smart product (or subclasses), given as integer 1-9" ;
        <http://www.w3.org/2000/01/rdf-schema#domain>
                <https://vocab.eccenca.com/geniustex/SmartProduct> ;
        <http://www.w3.org/2000/01/rdf-schema#isDefinedBy>
                <https://vocab.eccenca.com/geniustex/> ;
        <http://www.w3.org/2000/01/rdf-schema#label>
                "technology readiness level" ;
        <http://www.w3.org/2000/01/rdf-schema#range>
                <http://www.w3.org/2001/XMLSchema#integer> ;
        <http://purl.org/dc/terms/issued>
                "2018-08-15"^^<http://www.w3.org/2001/XMLSchema#date> .

<https://vocab.eccenca.com/geniustex/processableWidth>
        a       <http://www.w3.org/2002/07/owl#ObjectProperty> ;
        <http://www.w3.org/2000/01/rdf-schema#comment>
                "the processable width dimension (min and max) for the process" ;
        <http://www.w3.org/2000/01/rdf-schema#domain>
                <https://vocab.eccenca.com/geniustex/Process> ;
        <http://www.w3.org/2000/01/rdf-schema#isDefinedBy>
                <https://vocab.eccenca.com/geniustex/> ;
        <http://www.w3.org/2000/01/rdf-schema#label>
                "processable width" ;
        <http://purl.org/dc/terms/issued>
                "2019-07-09"^^<http://www.w3.org/2001/XMLSchema#date> .

<https://vocab.eccenca.com/geniustex/linearComponentGeometry>
        a       <https://vocab.eccenca.com/geniustex/ComponentGeometry> ;
        <http://www.w3.org/2000/01/rdf-schema#comment>
                "one-dimensional form" ;
        <http://www.w3.org/2000/01/rdf-schema#isDefinedBy>
                <https://vocab.eccenca.com/geniustex/> ;
        <http://www.w3.org/2000/01/rdf-schema#label>
                "linear" ;
        <http://purl.org/dc/terms/issued>
                "2018-10-15"^^<http://www.w3.org/2001/XMLSchema#date> .

<https://vocab.eccenca.com/geniustex/protects>
        a       <http://www.w3.org/2002/07/owl#ObjectProperty> ;
        <http://www.w3.org/2000/01/rdf-schema#comment>
                "a casing protects functional modules against outer influences" ;
        <http://www.w3.org/2000/01/rdf-schema#domain>
                <https://vocab.eccenca.com/geniustex/Casing> ;
        <http://www.w3.org/2000/01/rdf-schema#isDefinedBy>
                <https://vocab.eccenca.com/geniustex/> ;
        <http://www.w3.org/2000/01/rdf-schema#label>
                "protects against outer influences" ;
        <http://www.w3.org/2000/01/rdf-schema#range>
                <https://vocab.eccenca.com/geniustex/FunctionalModule> ;
        <http://purl.org/dc/terms/issued>
                "2018-08-15"^^<http://www.w3.org/2001/XMLSchema#date> .

<https://vocab.eccenca.com/geniustex/trackFineness>
        a       <http://www.w3.org/2002/07/owl#DatatypeProperty> ;
        <http://www.w3.org/2000/01/rdf-schema#comment>
                "track fineness that can be handled by an integrating process" ;
        <http://www.w3.org/2000/01/rdf-schema#domain>
                <https://vocab.eccenca.com/geniustex/Integrating> ;
        <http://www.w3.org/2000/01/rdf-schema#isDefinedBy>
                <https://vocab.eccenca.com/geniustex/> ;
        <http://www.w3.org/2000/01/rdf-schema#label>
                "track fineness" ;
        <http://www.w3.org/2000/01/rdf-schema#range>
                <http://www.w3.org/2001/XMLSchema#float> ;
        <http://purl.org/dc/terms/issued>
                "2018-08-15"^^<http://www.w3.org/2001/XMLSchema#date> .

<https://vocab.eccenca.com/geniustex/contactResistance>
        a       <http://www.w3.org/2002/07/owl#DatatypeProperty> ;
        <http://www.w3.org/2000/01/rdf-schema#comment>
                "contact reistance of a contact (low to high, on 1-3 scale)" ;
        <http://www.w3.org/2000/01/rdf-schema#domain>
                <https://vocab.eccenca.com/geniustex/Contacting> ;
        <http://www.w3.org/2000/01/rdf-schema#isDefinedBy>
                <https://vocab.eccenca.com/geniustex/> ;
        <http://www.w3.org/2000/01/rdf-schema#label>
                "contact resistance" ;
        <http://www.w3.org/2000/01/rdf-schema#range>
                <http://www.w3.org/2001/XMLSchema#integer> ;
        <http://purl.org/dc/terms/issued>
                "2019-04-25"^^<http://www.w3.org/2001/XMLSchema#date> .

<https://vocab.eccenca.com/geniustex/CareInstructions>
        a       <http://www.w3.org/2002/07/owl#Class> ;
        <http://www.w3.org/2000/01/rdf-schema#comment>
                "instructions that describe how a (smart) textile product should be treated to maintain function and condition, e.g., how to clean it" ;
        <http://www.w3.org/2000/01/rdf-schema#isDefinedBy>
                <https://vocab.eccenca.com/geniustex/> ;
        <http://www.w3.org/2000/01/rdf-schema#label>
                "Care Instructions" ;
        <http://purl.org/dc/terms/issued>
                "2018-08-30"^^<http://www.w3.org/2001/XMLSchema#date> ;
        <http://purl.org/dc/terms/modified>
                "2019-04-12"^^<http://www.w3.org/2001/XMLSchema#date> .

<https://vocab.eccenca.com/geniustex/PackageType>
        a       <http://www.w3.org/2002/07/owl#Class> ;
        <http://www.w3.org/2000/01/rdf-schema#comment>
                "how a component is packaged and can be mounted (SMD/SMT, woven, fibrous,.)" ;
        <http://www.w3.org/2000/01/rdf-schema#isDefinedBy>
                <https://vocab.eccenca.com/geniustex/> ;
        <http://www.w3.org/2000/01/rdf-schema#label>
                "Packaging or Mounting Type" ;
        <http://purl.org/dc/terms/issued>
                "2018-09-30"^^<http://www.w3.org/2001/XMLSchema#date> .

<https://vocab.eccenca.com/geniustex/hasElasticityTypeMat>
        a       <http://www.w3.org/2002/07/owl#ObjectProperty> ;
        <http://www.w3.org/2000/01/rdf-schema#comment>
                "a material has a certain type of elasticity that describes how a textile is elastic, i.e., if it is able to resume its normal shape spontaneously after being stretched or compressed  (none/bidirectional/lengthwise/crosswise)" ;
        <http://www.w3.org/2000/01/rdf-schema#domain>
                <https://vocab.eccenca.com/geniustex/Material> ;
        <http://www.w3.org/2000/01/rdf-schema#isDefinedBy>
                <https://vocab.eccenca.com/geniustex/> ;
        <http://www.w3.org/2000/01/rdf-schema#label>
                "has a certain type of material elasticity" ;
        <http://www.w3.org/2000/01/rdf-schema#range>
                <https://vocab.eccenca.com/geniustex/ElasticityType> ;
        <http://purl.org/dc/terms/issued>
                "2018-09-30"^^<http://www.w3.org/2001/XMLSchema#date> ;
        <http://purl.org/dc/terms/modified>
                "2019-04-15"^^<http://www.w3.org/2001/XMLSchema#date> .

<https://vocab.eccenca.com/geniustex/hasUnit>
        a       <http://www.w3.org/2002/07/owl#ObjectProperty> ;
        <http://www.w3.org/2000/01/rdf-schema#comment>
                "every measured value has a certain unit of measure" ;
        <http://www.w3.org/2000/01/rdf-schema#isDefinedBy>
                <https://vocab.eccenca.com/geniustex/> ;
        <http://www.w3.org/2000/01/rdf-schema#label>
                "has a unit of measure" ;
        <http://www.w3.org/2000/01/rdf-schema#range>
                <https://vocab.eccenca.com/geniustex/UnitOfMeasure> ;
        <http://www.w3.org/2000/01/rdf-schema#subPropertyOf>
                <http://www.ontology-of-units-of-measure.org/resource/om-2/hasUnit> ;
        <http://purl.org/dc/terms/issued>
                "2018-07-10"^^<http://www.w3.org/2001/XMLSchema#date> ;
        <http://purl.org/dc/terms/modified>
                "2018-09-20"^^<http://www.w3.org/2001/XMLSchema#date> .

<https://vocab.eccenca.com/geniustex/cubicComponentGeometry>
        a       <https://vocab.eccenca.com/geniustex/ComponentGeometry> ;
        <http://www.w3.org/2000/01/rdf-schema#comment>
                "three-dimensional" ;
        <http://www.w3.org/2000/01/rdf-schema#isDefinedBy>
                <https://vocab.eccenca.com/geniustex/> ;
        <http://www.w3.org/2000/01/rdf-schema#label>
                "cubic" ;
        <http://purl.org/dc/terms/issued>
                "2018-10-15"^^<http://www.w3.org/2001/XMLSchema#date> .

<http://www.w3.org/ns/ssn/systems/MeasurementRange>
        a       <http://www.w3.org/2002/07/owl#Class> ;
        <http://www.w3.org/2000/01/rdf-schema#comment>
                "The set of values that the Sensor can return as the Result of an Observation under the defined Conditions."@en ;
        <http://www.w3.org/2000/01/rdf-schema#isDefinedBy>
                <http://www.w3.org/ns/ssn/systems/> ;
        <http://www.w3.org/2000/01/rdf-schema#label>
                "Measurement Range"@en ;
        <http://www.w3.org/2000/01/rdf-schema#subClassOf>
                <http://www.w3.org/ns/ssn/systems/SystemProperty> ;
        <http://www.w3.org/2000/01/rdf-schema#subClassOf>
                [ a       <http://www.w3.org/2002/07/owl#Restriction> ;
                  <http://www.w3.org/2002/07/owl#allValuesFrom>
                          [ a       <http://www.w3.org/2002/07/owl#Restriction> ;
                            <http://www.w3.org/2002/07/owl#allValuesFrom>
                                    <http://www.w3.org/ns/sosa/Sensor> ;
                            <http://www.w3.org/2002/07/owl#onProperty>
                                    [ <http://www.w3.org/2002/07/owl#inverseOf>
                                              <http://www.w3.org/ns/ssn/systems/hasSystemCapability> ]
                          ] ;
                  <http://www.w3.org/2002/07/owl#onProperty>
                          [ <http://www.w3.org/2002/07/owl#inverseOf>
                                    <http://www.w3.org/ns/ssn/systems/hasSystemProperty> ]
                ] .

<https://vocab.eccenca.com/geniustex/yarn>
        a       <https://vocab.eccenca.com/geniustex/PackageType> ;
        <http://www.w3.org/2000/01/rdf-schema#comment>
                "component is packaged within a yarn structure, e.g., for textile based or textile integrated components" ;
        <http://www.w3.org/2000/01/rdf-schema#isDefinedBy>
                <https://vocab.eccenca.com/geniustex/> ;
        <http://www.w3.org/2000/01/rdf-schema#label>
                "yarn" ;
        <http://purl.org/dc/terms/issued>
                "2018-09-30"^^<http://www.w3.org/2001/XMLSchema#date> .

<https://vocab.eccenca.com/geniustex/reversible>
        a       <http://www.w3.org/2002/07/owl#DatatypeProperty> ;
        <http://www.w3.org/2000/01/rdf-schema#comment>
                "boolean value to represent if the contacting process is reversible or not" ;
        <http://www.w3.org/2000/01/rdf-schema#domain>
                <https://vocab.eccenca.com/geniustex/Contacting> ;
        <http://www.w3.org/2000/01/rdf-schema#isDefinedBy>
                <https://vocab.eccenca.com/geniustex/> ;
        <http://www.w3.org/2000/01/rdf-schema#label>
                "reversible contacting process" ;
        <http://www.w3.org/2000/01/rdf-schema#range>
                <http://www.w3.org/2001/XMLSchema#boolean> ;
        <http://purl.org/dc/terms/issued>
                "2018-08-17"^^<http://www.w3.org/2001/XMLSchema#date> ;
        <http://purl.org/dc/terms/modified>
                "2019-04-15"^^<http://www.w3.org/2001/XMLSchema#date> .

<https://vocab.eccenca.com/geniustex/suppliedMatBy>
        a       <http://www.w3.org/2002/07/owl#ObjectProperty> ;
        <http://www.w3.org/2000/01/rdf-schema#comment>
                "Provider supplies a material" ;
        <http://www.w3.org/2000/01/rdf-schema#domain>
                <https://vocab.eccenca.com/geniustex/Material> ;
        <http://www.w3.org/2000/01/rdf-schema#isDefinedBy>
                <https://vocab.eccenca.com/geniustex/> ;
        <http://www.w3.org/2000/01/rdf-schema#label>
                "is supplied (material) by" ;
        <http://www.w3.org/2000/01/rdf-schema#range>
                <https://vocab.eccenca.com/geniustex/Provider> ;
        <http://purl.org/dc/terms/issued>
                "2018-08-30"^^<http://www.w3.org/2001/XMLSchema#date> .

<https://vocab.eccenca.com/geniustex/DIN%5FEN%5FISO%5F2062>
        a       <https://vocab.eccenca.com/geniustex/NormedPropertyTest> ;
        <http://www.w3.org/2000/01/rdf-schema#comment>
                "testing elongation (i.e.,  the amount of extension of an object under stress, usually expressed as a percentage of the original length) and tear resistance" ;
        <http://www.w3.org/2000/01/rdf-schema#isDefinedBy>
                <https://vocab.eccenca.com/geniustex/> ;
        <http://www.w3.org/2000/01/rdf-schema#label>
                "tear and elongation test" ;
        <http://purl.org/dc/terms/issued>
                "2018-08-30"^^<http://www.w3.org/2001/XMLSchema#date> ;
        <http://purl.org/dc/terms/modified>
                "2019-04-15"^^<http://www.w3.org/2001/XMLSchema#date> .

<http://www.w3.org/ns/ssn/systems/ResponseTime>
        a       <http://www.w3.org/2002/07/owl#Class> ;
        <http://www.w3.org/2000/01/rdf-schema#comment>
                "As a Sensor Property: the time between a (step) change in the value of an observed ObservableProperty and a Sensor (possibly with specified error) 'settling' on an observed value, under the defined Conditions.\n\n  As an Actuator property: the time between a (step) change in the command of an Actuator and the 'settling' of the value of the acted on ActuatableProperty, under the defined Conditions."@en ;
        <http://www.w3.org/2000/01/rdf-schema#isDefinedBy>
                <http://www.w3.org/ns/ssn/systems/> ;
        <http://www.w3.org/2000/01/rdf-schema#label>
                "Response Time"@en ;
        <http://www.w3.org/2000/01/rdf-schema#subClassOf>
                <http://www.w3.org/ns/ssn/systems/SystemProperty> .

<http://www.w3.org/ns/ssn/systems/Drift>
        a       <http://www.w3.org/2002/07/owl#Class> ;
        <http://www.w3.org/2000/01/rdf-schema#comment>
                "As a Sensor Property: a continuous or incremental change in the reported values of Observations over time for an unchanging Property under the defined Conditions. \n\n  As an Actuator Property: a continuous or incremental change in the true value of the acted on ActuatableProperty over time for an unchanging command under the defined Conditions."@en ;
        <http://www.w3.org/2000/01/rdf-schema#isDefinedBy>
                <http://www.w3.org/ns/ssn/systems/> ;
        <http://www.w3.org/2000/01/rdf-schema#label>
                "Drift"@en ;
        <http://www.w3.org/2000/01/rdf-schema#subClassOf>
                <http://www.w3.org/ns/ssn/systems/SystemProperty> .

<https://vocab.eccenca.com/geniustex/based>
        a       <https://vocab.eccenca.com/geniustex/LevelTextileIntegration> ;
        <http://www.w3.org/2000/01/rdf-schema#comment>
                "textile-based smart products (fully textile) (Source: Bosowski et al. Design and manufacture\nof textile-based sensors. In Electronic Textiles: Smart Fabrics and Wearable Technology)" ;
        <http://www.w3.org/2000/01/rdf-schema#isDefinedBy>
                <https://vocab.eccenca.com/geniustex/> ;
        <http://www.w3.org/2000/01/rdf-schema#label>
                "based" ;
        <http://purl.org/dc/terms/issued>
                "2018-08-15"^^<http://www.w3.org/2001/XMLSchema#date> ;
        <http://purl.org/dc/terms/modified>
                "2019-04-15"^^<http://www.w3.org/2001/XMLSchema#date> .

<https://vocab.eccenca.com/geniustex/energyConsumption>
        a       <http://www.w3.org/2002/07/owl#ObjectProperty> ;
        <http://www.w3.org/2000/01/rdf-schema#comment>
                "energy consumption of a functional module" ;
        <http://www.w3.org/2000/01/rdf-schema#domain>
                <https://vocab.eccenca.com/geniustex/FunctionalModule> ;
        <http://www.w3.org/2000/01/rdf-schema#isDefinedBy>
                <https://vocab.eccenca.com/geniustex/> ;
        <http://www.w3.org/2000/01/rdf-schema#label>
                "energy consumption" ;
        <http://purl.org/dc/terms/issued>
                "2018-06-21"^^<http://www.w3.org/2001/XMLSchema#date> ;
        <http://purl.org/dc/terms/modified>
                "2019-04-15"^^<http://www.w3.org/2001/XMLSchema#date> .

<http://www.ontology-of-units-of-measure.org/resource/om-2/Unit>
        a       <http://www.w3.org/2002/07/owl#Class> ;
        <http://www.w3.org/2000/01/rdf-schema#comment>
                "A unit of measure is a definite magnitude of a quantity, defined and adopted by convention or by law. It is used as a standard for measurement of the same quantity, where any other value of the quantity can be expressed as a simple multiple of the unit. For example, length is a quantity; the metre is a unit of length that represents a definite predetermined length. When we say 10 metre (or 10 m), we actually mean 10 times the definite predetermined length called \"metre\"."@en ;
        <http://www.w3.org/2000/01/rdf-schema#isDefinedBy>
                <http://www.ontology-of-units-of-measure.org/resource/om-2/> ;
        <http://www.w3.org/2000/01/rdf-schema#label>
                "unit"@en .

<http://www.w3.org/ns/ssn/systems/hasOperatingRange>
        a       <http://www.w3.org/2002/07/owl#ObjectProperty> ;
        <http://www.w3.org/2000/01/rdf-schema#comment>
                "Relation from a System to an OperatingRange describing the normal operating environment of the System."@en ;
        <http://www.w3.org/2000/01/rdf-schema#domain>
                <https://vocab.eccenca.com/geniustex/FunctionalModule> ;
        <http://www.w3.org/2000/01/rdf-schema#isDefinedBy>
                <http://www.w3.org/ns/ssn/systems/> ;
        <http://www.w3.org/2000/01/rdf-schema#label>
                "has operating range"@en ;
        <http://www.w3.org/2000/01/rdf-schema#range>
                <http://www.w3.org/ns/ssn/systems/OperatingRange> ;
        <http://www.w3.org/2000/01/rdf-schema#subPropertyOf>
                <http://www.w3.org/ns/ssn/hasProperty> .

<https://vocab.eccenca.com/geniustex/Folding>
        a       <http://www.w3.org/2002/07/owl#Class> ;
        <http://www.w3.org/2000/01/rdf-schema#comment>
                "a process step where something flexible and relatively flat (e.g., the textile)  is bent over on itself so that one part of it covers another" ;
        <http://www.w3.org/2000/01/rdf-schema#isDefinedBy>
                <https://vocab.eccenca.com/geniustex/> ;
        <http://www.w3.org/2000/01/rdf-schema#label>
                "Folding" ;
        <http://www.w3.org/2000/01/rdf-schema#subClassOf>
                <https://vocab.eccenca.com/geniustex/Handling> ;
        <http://purl.org/dc/terms/issued>
                "2018-06-15"^^<http://www.w3.org/2001/XMLSchema#date> ;
        <http://purl.org/dc/terms/modified>
                "2019-04-15"^^<http://www.w3.org/2001/XMLSchema#date> .

<https://vocab.eccenca.com/geniustex/none>
        a       <https://vocab.eccenca.com/geniustex/ElasticityType> ;
        <http://www.w3.org/2000/01/rdf-schema#comment>
                "no elasticity of textile material, i.e., it is not able to resume its normal shape spontaneously after being stretched or compressed " ;
        <http://www.w3.org/2000/01/rdf-schema#isDefinedBy>
                <https://vocab.eccenca.com/geniustex/> ;
        <http://www.w3.org/2000/01/rdf-schema#label>
                "none" ;
        <http://purl.org/dc/terms/issued>
                "2018-09-30"^^<http://www.w3.org/2001/XMLSchema#date> ;
        <http://purl.org/dc/terms/modified>
                "2019-04-15"^^<http://www.w3.org/2001/XMLSchema#date> .

<https://vocab.eccenca.com/geniustex/Packaging>
        a       <http://www.w3.org/2002/07/owl#Class> ;
        <http://www.w3.org/2000/01/rdf-schema#comment>
                "a packaging step where the product or a group of products is wrapped or packed in a sort of box" ;
        <http://www.w3.org/2000/01/rdf-schema#isDefinedBy>
                <https://vocab.eccenca.com/geniustex/> ;
        <http://www.w3.org/2000/01/rdf-schema#label>
                "Packaging" ;
        <http://www.w3.org/2000/01/rdf-schema#subClassOf>
                <https://vocab.eccenca.com/geniustex/Handling> ;
        <http://purl.org/dc/terms/issued>
                "2018-06-15"^^<http://www.w3.org/2001/XMLSchema#date> ;
        <http://purl.org/dc/terms/modified>
                "2019-04-15"^^<http://www.w3.org/2001/XMLSchema#date> .

<https://vocab.eccenca.com/geniustex/hasElasticityType>
        a       <http://www.w3.org/2002/07/owl#ObjectProperty> ;
        <http://www.w3.org/2000/01/rdf-schema#comment>
                "a carrier has a certain type of elasticity that describes how a textile is elastic, i.e., if it is able to resume its normal shape spontaneously after being stretched or compressed  (none/bidirectional/lengthwise/crosswise)" ;
        <http://www.w3.org/2000/01/rdf-schema#domain>
                <https://vocab.eccenca.com/geniustex/Carrier> ;
        <http://www.w3.org/2000/01/rdf-schema#isDefinedBy>
                <https://vocab.eccenca.com/geniustex/> ;
        <http://www.w3.org/2000/01/rdf-schema#label>
                "has a certain type of carrier elasticity" ;
        <http://www.w3.org/2000/01/rdf-schema#range>
                <https://vocab.eccenca.com/geniustex/ElasticityType> ;
        <http://purl.org/dc/terms/issued>
                "2018-09-30"^^<http://www.w3.org/2001/XMLSchema#date> ;
        <http://purl.org/dc/terms/modified>
                "2019-04-15"^^<http://www.w3.org/2001/XMLSchema#date> .

<https://vocab.eccenca.com/geniustex/RoHS>
        a       <https://vocab.eccenca.com/geniustex/NormedPropertyTest> ;
        <http://www.w3.org/2000/01/rdf-schema#comment>
                "conforms with EU Restriction of Hazardous Substances " ;
        <http://www.w3.org/2000/01/rdf-schema#isDefinedBy>
                <https://vocab.eccenca.com/geniustex/> ;
        <http://www.w3.org/2000/01/rdf-schema#label>
                "Restriction of Hazardous Substances" ;
        <http://purl.org/dc/terms/issued>
                "2018-08-30"^^<http://www.w3.org/2001/XMLSchema#date> .

<https://vocab.eccenca.com/geniustex/buildtech>
        a       <https://vocab.eccenca.com/geniustex/ApplicationArea> ;
        <http://www.w3.org/2000/01/rdf-schema#comment>
                "Engineering and industrial construction, interior fittings, earthworks, waterworks and traffic route construction  (Source: Gries et al. Textile Fertigungsverfahren: Eine Einf체hrung; Carl Hanser\nVerlag)" ;
        <http://www.w3.org/2000/01/rdf-schema#isDefinedBy>
                <https://vocab.eccenca.com/geniustex/> ;
        <http://www.w3.org/2000/01/rdf-schema#label>
                "buildtech" ;
        <http://purl.org/dc/terms/issued>
                "2018-06-15"^^<http://www.w3.org/2001/XMLSchema#date> ;
        <http://purl.org/dc/terms/modified>
                "2019-04-15"^^<http://www.w3.org/2001/XMLSchema#date> .

<http://www.w3.org/ns/ssn/systems/hasSystemProperty>
        a       <http://www.w3.org/2002/07/owl#ObjectProperty> ;
        <http://www.w3.org/2000/01/rdf-schema#comment>
                "Relation from an SystemCapability of a System to a SystemProperty describing the capabilities of the System."@en ;
        <http://www.w3.org/2000/01/rdf-schema#isDefinedBy>
                <http://www.w3.org/ns/ssn/systems/> ;
        <http://www.w3.org/2000/01/rdf-schema#label>
                "has system property"@en ;
        <http://www.w3.org/2000/01/rdf-schema#subPropertyOf>
                <http://www.w3.org/ns/ssn/hasProperty> .

<https://vocab.eccenca.com/geniustex/hasIntegrationLevel>
        a       <http://www.w3.org/2002/07/owl#ObjectProperty> ;
        <http://www.w3.org/2000/01/rdf-schema#comment>
                "level of textile integration of a smart product (or subclasses). Textile-adapted: the textile does not cover an electronic function (0%), but electronic components can be attached to the textile, e.g., a pocket for an MP3 player.\nTextile-integrated: the textile covers between 0 and 100% of the electronic function, creating an interface between the textile and the electronics. For example, flexible circuit boards can be integrated into textiles in this manner.\nTextile-based: electronic function is 100% covered by the textile.\nWhen considering an intelligent textile material, this can involve the realization of conductor paths and sensors made of conductive yarns (Source: Bosowski et al. Design and manufacture\nof textile-based sensors. In Electronic Textiles: Smart Fabrics and Wearable Technology)" ;
        <http://www.w3.org/2000/01/rdf-schema#domain>
                <https://vocab.eccenca.com/geniustex/SmartProduct> ;
        <http://www.w3.org/2000/01/rdf-schema#isDefinedBy>
                <https://vocab.eccenca.com/geniustex/> ;
        <http://www.w3.org/2000/01/rdf-schema#label>
                "has a textile integration level" ;
        <http://www.w3.org/2000/01/rdf-schema#range>
                <https://vocab.eccenca.com/geniustex/LevelTextileIntegration> ;
        <http://purl.org/dc/terms/issued>
                "2018-08-15"^^<http://www.w3.org/2001/XMLSchema#date> ;
        <http://purl.org/dc/terms/modified>
                "2019-04-15"^^<http://www.w3.org/2001/XMLSchema#date> .

<https://vocab.eccenca.com/geniustex/IntHandling>
        a       <http://www.w3.org/2002/07/owl#Class> ;
        <http://www.w3.org/2000/01/rdf-schema#comment>
                "an intermediate handling step between process steps not changing the properties of the product" ;
        <http://www.w3.org/2000/01/rdf-schema#isDefinedBy>
                <https://vocab.eccenca.com/geniustex/> ;
        <http://www.w3.org/2000/01/rdf-schema#label>
                "Intermediate Handling" ;
        <http://www.w3.org/2000/01/rdf-schema#subClassOf>
                <https://vocab.eccenca.com/geniustex/Handling> ;
        <http://purl.org/dc/terms/issued>
                "2018-06-15"^^<http://www.w3.org/2001/XMLSchema#date> .

<https://vocab.eccenca.com/geniustex/conformsMatWith>
        a       <http://www.w3.org/2002/07/owl#ObjectProperty> ;
        <http://www.w3.org/2000/01/rdf-schema#comment>
                "a material meets the requirements of a property test" ;
        <http://www.w3.org/2000/01/rdf-schema#domain>
                <https://vocab.eccenca.com/geniustex/Material> ;
        <http://www.w3.org/2000/01/rdf-schema#isDefinedBy>
                <https://vocab.eccenca.com/geniustex/> ;
        <http://www.w3.org/2000/01/rdf-schema#label>
                "conforms (material) with" ;
        <http://www.w3.org/2000/01/rdf-schema#range>
                <https://vocab.eccenca.com/geniustex/PropertyTest> .

<https://vocab.eccenca.com/geniustex/SemifinishedTextile>
        a       <http://www.w3.org/2002/07/owl#Class> ;
        <http://www.w3.org/2000/01/rdf-schema#comment>
                "semifinished textile material acting as carrier" ;
        <http://www.w3.org/2000/01/rdf-schema#isDefinedBy>
                <https://vocab.eccenca.com/geniustex/> ;
        <http://www.w3.org/2000/01/rdf-schema#label>
                "Semifinished Textile" ;
        <http://www.w3.org/2000/01/rdf-schema#subClassOf>
                <https://vocab.eccenca.com/geniustex/Carrier> ;
        <http://purl.org/dc/terms/issued>
                "2018-05-21"^^<http://www.w3.org/2001/XMLSchema#date> ;
        <http://purl.org/dc/terms/modified>
                "2018-06-14"^^<http://www.w3.org/2001/XMLSchema#date> .

<https://vocab.eccenca.com/geniustex/pin>
        a       <https://vocab.eccenca.com/geniustex/ElectricConnectionType> ;
        <http://www.w3.org/2000/01/rdf-schema#comment>
                "a functional component has a pin as electric connection type (only if SMD_connection or THT_connection are not applicable)" ;
        <http://www.w3.org/2000/01/rdf-schema#isDefinedBy>
                <https://vocab.eccenca.com/geniustex/> ;
        <http://www.w3.org/2000/01/rdf-schema#label>
                "pin" ;
        <http://purl.org/dc/terms/issued>
                "2019-02-22"^^<http://www.w3.org/2001/XMLSchema#date> .

<https://vocab.eccenca.com/geniustex/ProposedSolution>
        a       <http://www.w3.org/2002/07/owl#Class> ;
        <http://www.w3.org/2000/01/rdf-schema#comment>
                "a proposal of how to solve a problem" ;
        <http://www.w3.org/2000/01/rdf-schema#isDefinedBy>
                <https://vocab.eccenca.com/geniustex/> ;
        <http://www.w3.org/2000/01/rdf-schema#label>
                "Proposed Solution" ;
        <http://www.w3.org/2000/01/rdf-schema#subClassOf>
                <https://vocab.eccenca.com/geniustex/CollaborationConcept> ;
        <http://purl.org/dc/terms/issued>
                "2018-09-30"^^<http://www.w3.org/2001/XMLSchema#date> .

<https://vocab.eccenca.com/geniustex/FunctionalControl>
        a       <http://www.w3.org/2002/07/owl#Class> ;
        <http://www.w3.org/2000/01/rdf-schema#comment>
                "a process step where a functional testing is carried out, e.g., to check that a component is wokring according to ist specification (In-line)" ;
        <http://www.w3.org/2000/01/rdf-schema#isDefinedBy>
                <https://vocab.eccenca.com/geniustex/> ;
        <http://www.w3.org/2000/01/rdf-schema#label>
                "FunctionalControl" ;
        <http://www.w3.org/2000/01/rdf-schema#subClassOf>
                <https://vocab.eccenca.com/geniustex/QualityControl> ;
        <http://purl.org/dc/terms/issued>
                "2018-06-15"^^<http://www.w3.org/2001/XMLSchema#date> ;
        <http://purl.org/dc/terms/modified>
                "2019-04-15"^^<http://www.w3.org/2001/XMLSchema#date> .

<http://www.w3.org/ns/ssn/systems/Precision>
        a       <http://www.w3.org/2002/07/owl#Class> ;
        <http://www.w3.org/2000/01/rdf-schema#comment>
                "As a Sensor Property: the closeness of agreement between replicate Observations on an unchanged or similar Property value: i.e., a measure of a Sensor's ability to consistently reproduce an Observation, under the defined Conditions.\n\n  As an Actuator Property: the closeness of agreement between replicate Actuations for an unchanged or similar command: i.e., a measure of an Actuator's ability to consistently reproduce an Actuation, under the defined Conditions."@en ;
        <http://www.w3.org/2000/01/rdf-schema#isDefinedBy>
                <http://www.w3.org/ns/ssn/systems/> ;
        <http://www.w3.org/2000/01/rdf-schema#label>
                "Precision"@en ;
        <http://www.w3.org/2000/01/rdf-schema#subClassOf>
                <http://www.w3.org/ns/ssn/systems/SystemProperty> .

<https://vocab.eccenca.com/geniustex/planarComponentGeometry>
        a       <https://vocab.eccenca.com/geniustex/ComponentGeometry> ;
        <http://www.w3.org/2000/01/rdf-schema#comment>
                "two-dimensional form, i.e. flat form" ;
        <http://www.w3.org/2000/01/rdf-schema#isDefinedBy>
                <https://vocab.eccenca.com/geniustex/> ;
        <http://www.w3.org/2000/01/rdf-schema#label>
                "planar" ;
        <http://purl.org/dc/terms/issued>
                "2018-10-15"^^<http://www.w3.org/2001/XMLSchema#date> .

<http://purl.org/dc/terms/modified>
        a       <http://www.w3.org/2002/07/owl#AnnotationProperty> ;
        <http://www.w3.org/2000/01/rdf-schema#isDefinedBy>
                <http://purl.org/dc/terms/> .

<https://vocab.eccenca.com/geniustex/conductivityMaterial>
        a       <http://www.w3.org/2002/07/owl#ObjectProperty> ;
        <http://www.w3.org/2000/01/rdf-schema#comment>
                "electrical conductivity (measure of a material's ability to conduct an electric current) of a material (S/m)" ;
        <http://www.w3.org/2000/01/rdf-schema#domain>
                <https://vocab.eccenca.com/geniustex/Material> ;
        <http://www.w3.org/2000/01/rdf-schema#isDefinedBy>
                <https://vocab.eccenca.com/geniustex/> ;
        <http://www.w3.org/2000/01/rdf-schema#label>
                "conductivity of material" ;
        <http://purl.org/dc/terms/issued>
                "2018-08-15"^^<http://www.w3.org/2001/XMLSchema#date> ;
        <http://purl.org/dc/terms/modified>
                "2019-04-15"^^<http://www.w3.org/2001/XMLSchema#date> .

<https://vocab.eccenca.com/geniustex/baredie>
        a       <https://vocab.eccenca.com/geniustex/PackageType> ;
        <http://www.w3.org/2000/01/rdf-schema#comment>
                "component is packaged as bare die, i.e., without leads for surface-mounting or any packaging" ;
        <http://www.w3.org/2000/01/rdf-schema#isDefinedBy>
                <https://vocab.eccenca.com/geniustex/> ;
        <http://www.w3.org/2000/01/rdf-schema#label>
                "bare die" ;
        <http://purl.org/dc/terms/issued>
                "2018-09-30"^^<http://www.w3.org/2001/XMLSchema#date> ;
        <http://purl.org/dc/terms/modified>
                "2019-04-15"^^<http://www.w3.org/2001/XMLSchema#date> .

<https://vocab.eccenca.com/geniustex/smd%5Fconnection>
        a       <https://vocab.eccenca.com/geniustex/ElectricConnectionType> ;
        <http://www.w3.org/2000/01/rdf-schema#comment>
                "a functional component has a SMD (surface-mount device) connection type" ;
        <http://www.w3.org/2000/01/rdf-schema#isDefinedBy>
                <https://vocab.eccenca.com/geniustex/> ;
        <http://www.w3.org/2000/01/rdf-schema#label>
                "SMD connection" ;
        <http://purl.org/dc/terms/issued>
                "2019-02-22"^^<http://www.w3.org/2001/XMLSchema#date> .

<https://vocab.eccenca.com/geniustex/CE>
        a       <https://vocab.eccenca.com/geniustex/NormedPropertyTest> ;
        <http://www.w3.org/2000/01/rdf-schema#comment>
                "a material or product conforms with CE. CE marking is a certification mark that indicates conformity with health, safety, and environmental protection standards for products sold within the European Economic Area (EEA) (Source: https://en.wikipedia.org/wiki/CE_marking)" ;
        <http://www.w3.org/2000/01/rdf-schema#isDefinedBy>
                <https://vocab.eccenca.com/geniustex/> ;
        <http://www.w3.org/2000/01/rdf-schema#label>
                "Ce certified" ;
        <http://purl.org/dc/terms/issued>
                "2018-08-30"^^<http://www.w3.org/2001/XMLSchema#date> ;
        <http://purl.org/dc/terms/modified>
                "2019-04-15"^^<http://www.w3.org/2001/XMLSchema#date> .

<https://vocab.eccenca.com/geniustex/Forming>
        a       <http://www.w3.org/2002/07/owl#Class> ;
        <http://www.w3.org/2000/01/rdf-schema#comment>
                "a process step where the physical shape of a material is permanently deformed, e.g., by bending, compressing or additive forming" ;
        <http://www.w3.org/2000/01/rdf-schema#isDefinedBy>
                <https://vocab.eccenca.com/geniustex/> ;
        <http://www.w3.org/2000/01/rdf-schema#label>
                "Forming" ;
        <http://www.w3.org/2000/01/rdf-schema#subClassOf>
                <https://vocab.eccenca.com/geniustex/Process> ;
        <http://purl.org/dc/terms/issued>
                "2018-06-15"^^<http://www.w3.org/2001/XMLSchema#date> ;
        <http://purl.org/dc/terms/modified>
                "2019-04-12"^^<http://www.w3.org/2001/XMLSchema#date> .

<https://vocab.eccenca.com/geniustex/mobility>
        a       <http://www.w3.org/2002/07/owl#DatatypeProperty> ;
        <http://www.w3.org/2000/01/rdf-schema#comment>
                "if a power supply module is suitable for mobile use (yes/no)" ;
        <http://www.w3.org/2000/01/rdf-schema#domain>
                <https://vocab.eccenca.com/geniustex/PowerSupplyModule> ;
        <http://www.w3.org/2000/01/rdf-schema#isDefinedBy>
                <https://vocab.eccenca.com/geniustex/> ;
        <http://www.w3.org/2000/01/rdf-schema#label>
                "mobility" ;
        <http://www.w3.org/2000/01/rdf-schema#range>
                <http://www.w3.org/2001/XMLSchema#boolean> ;
        <http://purl.org/dc/terms/issued>
                "2018-10-03"^^<http://www.w3.org/2001/XMLSchema#date> .

<https://vocab.eccenca.com/geniustex/spacerfabric>
        a       <https://vocab.eccenca.com/geniustex/PackageType> ;
        <http://www.w3.org/2000/01/rdf-schema#comment>
                "component is packaged within a spacer fabric structure, e.g., for textile based or textile integrated components" ;
        <http://www.w3.org/2000/01/rdf-schema#isDefinedBy>
                <https://vocab.eccenca.com/geniustex/> ;
        <http://www.w3.org/2000/01/rdf-schema#label>
                "spacer fabric" ;
        <http://purl.org/dc/terms/issued>
                "2018-09-30"^^<http://www.w3.org/2001/XMLSchema#date> .

<https://vocab.eccenca.com/geniustex/PickAndPlace>
        a       <http://www.w3.org/2002/07/owl#Class> ;
        <http://www.w3.org/2000/01/rdf-schema#comment>
                "a handling process step where items are picked up and placed somewhere else, mostly smd components being placed on a circuit board" ;
        <http://www.w3.org/2000/01/rdf-schema#isDefinedBy>
                <https://vocab.eccenca.com/geniustex/> ;
        <http://www.w3.org/2000/01/rdf-schema#label>
                "Pick & Place" ;
        <http://www.w3.org/2000/01/rdf-schema#subClassOf>
                <https://vocab.eccenca.com/geniustex/Handling> ;
        <http://purl.org/dc/terms/issued>
                "2018-10-03"^^<http://www.w3.org/2001/XMLSchema#date> ;
        <http://purl.org/dc/terms/modified>
                "2019-04-15"^^<http://www.w3.org/2001/XMLSchema#date> .

<https://vocab.eccenca.com/geniustex/flexibilityProcess>
        a       <http://www.w3.org/2002/07/owl#DatatypeProperty> ;
        <http://www.w3.org/2000/01/rdf-schema#comment>
                "degree of flexibility of a process (high/medium/low)" ;
        <http://www.w3.org/2000/01/rdf-schema#domain>
                <https://vocab.eccenca.com/geniustex/Process> ;
        <http://www.w3.org/2000/01/rdf-schema#isDefinedBy>
                <https://vocab.eccenca.com/geniustex/> ;
        <http://www.w3.org/2000/01/rdf-schema#label>
                "degree of flexibility" ;
        <http://www.w3.org/2000/01/rdf-schema#range>
                <http://www.w3.org/2001/XMLSchema#string> ;
        <http://purl.org/dc/terms/issued>
                "2019-04-26"^^<http://www.w3.org/2001/XMLSchema#date> .

<https://ns.eccenca.com/eccenca-GmbH>
        a       <http://xmlns.com/foaf/0.1/Organization> , <http://purl.org/dc/terms/Agent> ;
        <http://xmlns.com/foaf/0.1/name>
                "eccenca GmbH" .

<http://www.w3.org/ns/ssn/Property>
        a       <http://www.w3.org/2002/07/owl#Class> ;
        <http://www.w3.org/2000/01/rdf-schema#comment>
                "A quality of an entity. An aspect of an entity that is intrinsic to and cannot exist without the entity."@en ;
        <http://www.w3.org/2000/01/rdf-schema#isDefinedBy>
                <http://www.w3.org/ns/ssn/> ;
        <http://www.w3.org/2000/01/rdf-schema#label>
                "Property"@en .

<https://vocab.eccenca.com/geniustex/traction>
        a       <https://vocab.eccenca.com/geniustex/ConnectionType> ;
        <http://www.w3.org/2000/01/rdf-schema#comment>
                "connection in joining process created by traction. Traction, or tractive force, is the force used to generate motion between a body and a tangential surface, through the use of dry friction, though the use of shear force of the surface is also commonly used (Source: https://en.wikipedia.org/wiki/Traction_(engineering))" ;
        <http://www.w3.org/2000/01/rdf-schema#isDefinedBy>
                <https://vocab.eccenca.com/geniustex/> ;
        <http://www.w3.org/2000/01/rdf-schema#label>
                "traction" ;
        <http://purl.org/dc/terms/issued>
                "2018-09-30"^^<http://www.w3.org/2001/XMLSchema#date> ;
        <http://purl.org/dc/terms/modified>
                "2019-04-15"^^<http://www.w3.org/2001/XMLSchema#date> .

<http://www.w3.org/ns/ssn/System>
        <http://www.w3.org/2000/01/rdf-schema#isDefinedBy>
                <http://www.w3.org/ns/ssn/> ;
        <http://www.w3.org/2000/01/rdf-schema#label>
                "System"@en .

<https://vocab.eccenca.com/geniustex/lengthwise>
        a       <https://vocab.eccenca.com/geniustex/ElasticityType> ;
        <http://www.w3.org/2000/01/rdf-schema#comment>
                "elasticity lengthwise only, i.e., able to resume its normal shape spontaneously after being stretched or compressed lengthwise" ;
        <http://www.w3.org/2000/01/rdf-schema#isDefinedBy>
                <https://vocab.eccenca.com/geniustex/> ;
        <http://www.w3.org/2000/01/rdf-schema#label>
                "lengthwise" ;
        <http://purl.org/dc/terms/issued>
                "2018-09-30"^^<http://www.w3.org/2001/XMLSchema#date> ;
        <http://purl.org/dc/terms/modified>
                "2019-04-15"^^<http://www.w3.org/2001/XMLSchema#date> .

<https://vocab.eccenca.com/geniustex/machinewashable>
        a       <https://vocab.eccenca.com/geniustex/Usability> ;
        <http://www.w3.org/2000/01/rdf-schema#comment>
                "a product needs to be machine washable" ;
        <http://www.w3.org/2000/01/rdf-schema#isDefinedBy>
                <https://vocab.eccenca.com/geniustex/> ;
        <http://www.w3.org/2000/01/rdf-schema#label>
                "machinewashable" ;
        <http://purl.org/dc/terms/issued>
                "2018-10-03"^^<http://www.w3.org/2001/XMLSchema#date> .

<http://www.w3.org/ns/ssn/systems/Frequency>
        a       <http://www.w3.org/2002/07/owl#Class> ;
        <http://www.w3.org/2000/01/rdf-schema#comment>
                "The smallest possible time between one Observation, Actuation, or Sampling and the next, under the defined Conditions."@en ;
        <http://www.w3.org/2000/01/rdf-schema#isDefinedBy>
                <http://www.w3.org/ns/ssn/systems/> ;
        <http://www.w3.org/2000/01/rdf-schema#label>
                "Frequency"@en ;
        <http://www.w3.org/2000/01/rdf-schema#subClassOf>
                <http://www.w3.org/ns/ssn/systems/SystemProperty> .

<https://vocab.eccenca.com/geniustex/ecotech>
        a       <https://vocab.eccenca.com/geniustex/ApplicationArea> ;
        <http://www.w3.org/2000/01/rdf-schema#comment>
                "Environmental protection, recycling, disposal  (Source: Gries et al. Textile Fertigungsverfahren: Eine Einf체hrung; Carl Hanser\nVerlag)" ;
        <http://www.w3.org/2000/01/rdf-schema#isDefinedBy>
                <https://vocab.eccenca.com/geniustex/> ;
        <http://www.w3.org/2000/01/rdf-schema#label>
                "ecotech" ;
        <http://purl.org/dc/terms/issued>
                "2019-04-15"^^<http://www.w3.org/2001/XMLSchema#date> .

<https://vocab.eccenca.com/geniustex/instantsample>
        a       <https://vocab.eccenca.com/geniustex/SupplyType> ;
        <http://www.w3.org/2000/01/rdf-schema#comment>
                "supply of sample volume instantaneously feasible" ;
        <http://www.w3.org/2000/01/rdf-schema#isDefinedBy>
                <https://vocab.eccenca.com/geniustex/> ;
        <http://www.w3.org/2000/01/rdf-schema#label>
                "instant sample supply" ;
        <http://purl.org/dc/terms/issued>
                "2018-09-30"^^<http://www.w3.org/2001/XMLSchema#date> .

<https://vocab.eccenca.com/geniustex/hasAuthor>
        a       <http://www.w3.org/2002/07/owl#ObjectProperty> ;
        <http://www.w3.org/2000/01/rdf-schema#comment>
                "a collaboration concept has an author" ;
        <http://www.w3.org/2000/01/rdf-schema#domain>
                <https://vocab.eccenca.com/geniustex/CollaborationConcept> ;
        <http://www.w3.org/2000/01/rdf-schema#isDefinedBy>
                <https://vocab.eccenca.com/geniustex/> ;
        <http://www.w3.org/2000/01/rdf-schema#label>
                "has an author" ;
        <http://www.w3.org/2000/01/rdf-schema#range>
                <https://vocab.eccenca.com/geniustex/User> ;
        <http://purl.org/dc/terms/issued>
                "2018-09-30"^^<http://www.w3.org/2001/XMLSchema#date> .

<http://www.ontology-of-units-of-measure.org/resource/om-2/hasUnit>
        a       <http://www.w3.org/2002/07/owl#ObjectProperty> ;
        <http://www.w3.org/2000/01/rdf-schema#isDefinedBy>
                <http://www.ontology-of-units-of-measure.org/resource/om-2/> ;
        <http://www.w3.org/2000/01/rdf-schema#label>
                "has unit"@en .

<https://vocab.eccenca.com/geniustex/soc>
        a       <https://vocab.eccenca.com/geniustex/PackageType> ;
        <http://www.w3.org/2000/01/rdf-schema#comment>
                "component is packaged as system on chip" ;
        <http://www.w3.org/2000/01/rdf-schema#isDefinedBy>
                <https://vocab.eccenca.com/geniustex/> ;
        <http://www.w3.org/2000/01/rdf-schema#label>
                "system on chip" ;
        <http://purl.org/dc/terms/issued>
                "2018-10-03"^^<http://www.w3.org/2001/XMLSchema#date> .

<http://purl.org/dc/terms/issued>
        a       <http://www.w3.org/2002/07/owl#AnnotationProperty> ;
        <http://www.w3.org/2000/01/rdf-schema#isDefinedBy>
                <http://purl.org/dc/terms/> .

<https://vocab.eccenca.com/geniustex/fleece>
        a       <https://vocab.eccenca.com/geniustex/PackageType> ;
        <http://www.w3.org/2000/01/rdf-schema#comment>
                "component is packaged within a fleece fabric structure, e.g., for textile based or textile integrated components" ;
        <http://www.w3.org/2000/01/rdf-schema#isDefinedBy>
                <https://vocab.eccenca.com/geniustex/> ;
        <http://www.w3.org/2000/01/rdf-schema#label>
                "fleece" ;
        <http://purl.org/dc/terms/issued>
                "2018-09-30"^^<http://www.w3.org/2001/XMLSchema#date> .

<http://www.w3.org/ns/ssn/hasProperty>
        a       <http://www.w3.org/2002/07/owl#ObjectProperty> ;
        <http://www.w3.org/2000/01/rdf-schema#comment>
                "Relation between an entity and a Property of that entity."@en ;
        <http://www.w3.org/2000/01/rdf-schema#isDefinedBy>
                <http://www.w3.org/ns/ssn/> ;
        <http://www.w3.org/2000/01/rdf-schema#label>
                "has property"@en ;
        <http://www.w3.org/2002/07/owl#inverseOf>
                <http://www.w3.org/ns/ssn/isPropertyOf> .

<https://vocab.eccenca.com/geniustex/sporttech>
        a       <https://vocab.eccenca.com/geniustex/ApplicationArea> ;
        <http://www.w3.org/2000/01/rdf-schema#comment>
                "Sport and leisure, functional sportswear (Source: Gries et al. Textile Fertigungsverfahren: Eine Einf체hrung; Carl Hanser Verlag)" ;
        <http://www.w3.org/2000/01/rdf-schema#isDefinedBy>
                <https://vocab.eccenca.com/geniustex/> ;
        <http://www.w3.org/2000/01/rdf-schema#label>
                "sporttech" ;
        <http://purl.org/dc/terms/issued>
                "2019-04-15"^^<http://www.w3.org/2001/XMLSchema#date> .

<http://creativecommons.org/ns#license>
        a       <http://www.w3.org/2002/07/owl#AnnotationProperty> ;
        <http://www.w3.org/2000/01/rdf-schema#isDefinedBy>
                <http://creativecommons.org/ns> .

<http://purl.org/dc/terms/publisher>
        a       <http://www.w3.org/2002/07/owl#AnnotationProperty> ;
        <http://www.w3.org/2000/01/rdf-schema#isDefinedBy>
                <http://purl.org/dc/terms/> .

<http://purl.org/dc/terms/rights>
        a       <http://www.w3.org/2002/07/owl#AnnotationProperty> ;
        <http://www.w3.org/2000/01/rdf-schema#isDefinedBy>
                <http://purl.org/dc/terms/> .
