<http://www.ontologydesignpatterns.org/cp/owl/informationobjectsandrepresentationlanguages.owl#IconicLanguage>
        a       <http://www.w3.org/2002/07/owl#Class> ;
        <http://www.w3.org/2000/01/rdf-schema#comment>
                "A language made up of graphical elements. It can be natural, artificial, and even formal." ;
        <http://www.w3.org/2000/01/rdf-schema#isDefinedBy>
                <http://www.ontologydesignpatterns.org/cp/owl/informationobjectsandrepresentationlanguages.owl> ;
        <http://www.w3.org/2000/01/rdf-schema#label>
                "Iconic language"@en , "Linguaggio iconico"@it ;
        <http://www.w3.org/2000/01/rdf-schema#subClassOf>
                <http://www.ontologydesignpatterns.org/cp/owl/informationobjectsandrepresentationlanguages.owl#Language> ;
        <http://www.w3.org/2002/07/owl#disjointWith>
                <http://www.ontologydesignpatterns.org/cp/owl/informationobjectsandrepresentationlanguages.owl#NaturalLanguage> .

<http://www.ontologydesignpatterns.org/cp/owl/informationobjectsandrepresentationlanguages.owl#FormalExpression>
        a       <http://www.w3.org/2002/07/owl#Class> ;
        <http://www.w3.org/2000/01/rdf-schema#comment>
                "Any information object represented in a FormalLanguage, usually having a formal interpretation by a dul:FormalEntity, and used to formally represent any Entity" ;
        <http://www.w3.org/2000/01/rdf-schema#isDefinedBy>
                <http://www.ontologydesignpatterns.org/cp/owl/informationobjectsandrepresentationlanguages.owl> ;
        <http://www.w3.org/2000/01/rdf-schema#label>
                "Formal expression"@en , "Espressione formale"@it ;
        <http://www.w3.org/2000/01/rdf-schema#subClassOf>
                <http://www.ontologydesignpatterns.org/cp/owl/intensionextension.owl#InformationObject> ;
        <http://www.w3.org/2000/01/rdf-schema#subClassOf>
                [ a       <http://www.w3.org/2002/07/owl#Restriction> ;
                  <http://www.w3.org/2002/07/owl#onProperty>
                          <http://www.ontologydesignpatterns.org/cp/owl/informationobjectsandrepresentationlanguages.owl#hasRepresentationLanguage> ;
                  <http://www.w3.org/2002/07/owl#someValuesFrom>
                          <http://www.ontologydesignpatterns.org/cp/owl/informationobjectsandrepresentationlanguages.owl#FormalLanguage>
                ] ;
        <http://www.w3.org/2002/07/owl#disjointWith>
                <http://www.ontologydesignpatterns.org/cp/owl/informationobjectsandrepresentationlanguages.owl#LinguisticObject> , <http://www.ontologydesignpatterns.org/cp/owl/informationobjectsandrepresentationlanguages.owl#Language> , <http://www.ontologydesignpatterns.org/cp/owl/informationobjectsandrepresentationlanguages.owl#IconicObject> .

<http://www.ontologydesignpatterns.org/cp/owl/informationobjectsandrepresentationlanguages.owl#IconicObject>
        a       <http://www.w3.org/2002/07/owl#Class> ;
        <http://www.w3.org/2000/01/rdf-schema#comment>
                "An information object represented in an IconicLanguage" ;
        <http://www.w3.org/2000/01/rdf-schema#isDefinedBy>
                <http://www.ontologydesignpatterns.org/cp/owl/informationobjectsandrepresentationlanguages.owl> ;
        <http://www.w3.org/2000/01/rdf-schema#label>
                "Oggetto iconico"@it , "Iconic object"@en ;
        <http://www.w3.org/2000/01/rdf-schema#subClassOf>
                <http://www.ontologydesignpatterns.org/cp/owl/intensionextension.owl#InformationObject> ;
        <http://www.w3.org/2000/01/rdf-schema#subClassOf>
                [ a       <http://www.w3.org/2002/07/owl#Restriction> ;
                  <http://www.w3.org/2002/07/owl#onProperty>
                          <http://www.ontologydesignpatterns.org/cp/owl/informationobjectsandrepresentationlanguages.owl#hasRepresentationLanguage> ;
                  <http://www.w3.org/2002/07/owl#someValuesFrom>
                          <http://www.ontologydesignpatterns.org/cp/owl/informationobjectsandrepresentationlanguages.owl#IconicLanguage>
                ] ;
        <http://www.w3.org/2002/07/owl#disjointWith>
                <http://www.ontologydesignpatterns.org/cp/owl/informationobjectsandrepresentationlanguages.owl#Language> , <http://www.ontologydesignpatterns.org/cp/owl/informationobjectsandrepresentationlanguages.owl#LinguisticObject> .

<http://www.ontologydesignpatterns.org/cp/owl/informationobjectsandrepresentationlanguages.owl#FormalLanguage>
        a       <http://www.w3.org/2002/07/owl#Class> ;
        <http://www.w3.org/2000/01/rdf-schema#comment>
                "A formal language, created by some human, with a fixed grammar, and usually with an explicit formal semantics (i.e. its elements have an interpretation wrt to formal entities such as sets, categories, etc.)." ;
        <http://www.w3.org/2000/01/rdf-schema#isDefinedBy>
                <http://www.ontologydesignpatterns.org/cp/owl/informationobjectsandrepresentationlanguages.owl> ;
        <http://www.w3.org/2000/01/rdf-schema#label>
                "Linguaggio formale"@it , "Formal language"@en ;
        <http://www.w3.org/2000/01/rdf-schema#subClassOf>
                <http://www.ontologydesignpatterns.org/cp/owl/informationobjectsandrepresentationlanguages.owl#Language> ;
        <http://www.w3.org/2000/01/rdf-schema#subClassOf>
                [ a       <http://www.w3.org/2002/07/owl#Restriction> ;
                  <http://www.w3.org/2002/07/owl#allValuesFrom>
                          [ a       <http://www.w3.org/2002/07/owl#Restriction> ;
                            <http://www.w3.org/2002/07/owl#minCardinality>
                                    "1"^^<http://www.w3.org/2001/XMLSchema#nonNegativeInteger> ;
                            <http://www.w3.org/2002/07/owl#onProperty>
                                    <http://www.ontologydesignpatterns.org/cp/owl/informationobjectsandrepresentationlanguages.owl#isFormallyRepresentedIn>
                          ] ;
                  <http://www.w3.org/2002/07/owl#onProperty>
                          <http://www.ontologydesignpatterns.org/cp/owl/partof.owl#hasPart>
                ] ;
        <http://www.w3.org/2002/07/owl#disjointWith>
                <http://www.ontologydesignpatterns.org/cp/owl/informationobjectsandrepresentationlanguages.owl#NaturalLanguage> , <http://www.ontologydesignpatterns.org/cp/owl/informationobjectsandrepresentationlanguages.owl#IconicLanguage> .

<http://www.ontologydesignpatterns.org/cp/owl/informationobjectsandrepresentationlanguages.owl#NaturalLanguage>
        a       <http://www.w3.org/2002/07/owl#Class> ;
        <http://www.w3.org/2000/01/rdf-schema#comment>
                "A natural language, evolved and used in a community across time.\nNatural languages components are 'temporary' and 'reconstructed' out of actual usage. For example, a grammar for a (part of a) natural language has the status of a theory for that language, but alternative ones can exist (e.g. generative vs. construction grammars)." ;
        <http://www.w3.org/2000/01/rdf-schema#isDefinedBy>
                <http://www.ontologydesignpatterns.org/cp/owl/informationobjectsandrepresentationlanguages.owl> ;
        <http://www.w3.org/2000/01/rdf-schema#label>
                "Linguaggio naturale"@it , "Natural language"@en ;
        <http://www.w3.org/2000/01/rdf-schema#subClassOf>
                <http://www.ontologydesignpatterns.org/cp/owl/informationobjectsandrepresentationlanguages.owl#Language> ;
        <http://www.w3.org/2000/01/rdf-schema#subClassOf>
                [ a       <http://www.w3.org/2002/07/owl#Restriction> ;
                  <http://www.w3.org/2002/07/owl#onProperty>
                          <http://www.ontologydesignpatterns.org/cp/owl/informationobjectsandrepresentationlanguages.owl#isConceptualizedBy> ;
                  <http://www.w3.org/2002/07/owl#someValuesFrom>
                          <http://www.ontologydesignpatterns.org/cp/owl/communities.owl#Community>
                ] .

<http://www.ontologydesignpatterns.org/cp/owl/intensionextension.owl#SocialObject>
        a       <http://www.w3.org/2002/07/owl#Class> .

<http://www.ontologydesignpatterns.org/cp/owl/communities.owl#Community>
        a       <http://www.w3.org/2002/07/owl#Class> ;
        <http://www.w3.org/2002/07/owl#disjointWith>
                <http://www.ontologydesignpatterns.org/cp/owl/informationobjectsandrepresentationlanguages.owl#IconicObject> , <http://www.ontologydesignpatterns.org/cp/owl/informationobjectsandrepresentationlanguages.owl#LinguisticObject> , <http://www.ontologydesignpatterns.org/cp/owl/informationobjectsandrepresentationlanguages.owl#Language> , <http://www.ontologydesignpatterns.org/cp/owl/informationobjectsandrepresentationlanguages.owl#FormalExpression> .

<http://www.ontologydesignpatterns.org/cp/owl/informationobjectsandrepresentationlanguages.owl#isFormallyRepresentedIn>
        a       <http://www.w3.org/2002/07/owl#ObjectProperty> ;
        <http://www.w3.org/2000/01/rdf-schema#comment>
                "The relation between formal expressions, and anything that they are supposed to represent.\nE.g., 'the predicate 'MariachiInTijuana' formallyRepresents the dul:Collection of all mariachis in Tijuana'; 'the equivalence relation '<=>' formallyRepresents the concept of two entities having the same properties'.\nNotice that formal expressions are formally interpreted by instances of dul:FormalEntity" ;
        <http://www.w3.org/2000/01/rdf-schema#isDefinedBy>
                <http://www.ontologydesignpatterns.org/cp/owl/informationobjectsandrepresentationlanguages.owl> ;
        <http://www.w3.org/2000/01/rdf-schema#label>
                "is formally represented in"@en , "è rappresentato formalmente in"@it ;
        <http://www.w3.org/2000/01/rdf-schema#range>
                <http://www.ontologydesignpatterns.org/cp/owl/informationobjectsandrepresentationlanguages.owl#FormalExpression> .

<http://www.ontologydesignpatterns.org/cp/owl/informationobjectsandrepresentationlanguages.owl#Language>
        a       <http://www.w3.org/2002/07/owl#Class> ;
        <http://www.w3.org/2000/01/rdf-schema#comment>
                "A natural or artificial language, provided with an alphabet (or vocabulary) and combinatorial rules. In the case of natural languages, their components are 'temporary' and 'reconstructed' out of actual usage. For example, a grammar for a natural language has the status of a theory for that language, and alternative ones can exist (e.g. generative vs. construction grammars).\nAnother distinction, between the general (systemic) rules for a language, and the local (contextual) rules for e.g. a certain context, speaker, place, etc., can be made separately.\nThe most comprehensive classification of languages ha probably been made by Umberto Eco, based on the production modes of the 'signs' that are represented in a certain language. It uses several semiotic dimensions, and will be modeled in a forthcoming ontology." ;
        <http://www.w3.org/2000/01/rdf-schema#isDefinedBy>
                <http://www.ontologydesignpatterns.org/cp/owl/informationobjectsandrepresentationlanguages.owl> ;
        <http://www.w3.org/2000/01/rdf-schema#label>
                "Language"@en , "Linguaggio"@it ;
        <http://www.w3.org/2002/07/owl#disjointWith>
                <http://www.ontologydesignpatterns.org/cp/owl/informationobjectsandrepresentationlanguages.owl#LinguisticObject> .

<http://www.ontologydesignpatterns.org/cp/owl/informationobjectsandrepresentationlanguages.owl#isConceptualizedBy>
        a       <http://www.w3.org/2002/07/owl#ObjectProperty> ;
        <http://www.w3.org/2000/01/rdf-schema#comment>
                "A relation stating that an Agent is internally representing a Description . E.g., 'John believes in the conspiracy theory'; 'Niels Bohr created a solar-system metaphor for his atomic theory'; 'Jacques assumes all swans are white'; 'the task force shares the attack plan'." ;
        <http://www.w3.org/2000/01/rdf-schema#domain>
                <http://www.ontologydesignpatterns.org/cp/owl/intensionextension.owl#SocialObject> ;
        <http://www.w3.org/2000/01/rdf-schema#isDefinedBy>
                <http://www.ontologydesignpatterns.org/cp/owl/informationobjectsandrepresentationlanguages.owl> ;
        <http://www.w3.org/2000/01/rdf-schema#label>
                "è concettualizzato da"@it , "is conceptualized by"@en ;
        <http://www.w3.org/2000/01/rdf-schema#range>
                [ a       <http://www.w3.org/2002/07/owl#Class> ;
                  <http://www.w3.org/2002/07/owl#unionOf>
                          ( <http://www.ontologydesignpatterns.org/cp/owl/agentrole.owl#Agent> <http://www.ontologydesignpatterns.org/cp/owl/communities.owl#Community> )
                ] ;
        <http://www.w3.org/2002/07/owl#inverseOf>
                <http://www.ontologydesignpatterns.org/cp/owl/informationobjectsandrepresentationlanguages.owl#conceptualizes> .

<http://www.ontologydesignpatterns.org/cp/owl/informationobjectsandrepresentationlanguages.owl#isRepresentationLanguageOf>
        a       <http://www.w3.org/2002/07/owl#ObjectProperty> ;
        <http://www.w3.org/2000/01/rdf-schema#domain>
                <http://www.ontologydesignpatterns.org/cp/owl/informationobjectsandrepresentationlanguages.owl#Language> ;
        <http://www.w3.org/2000/01/rdf-schema#isDefinedBy>
                <http://www.ontologydesignpatterns.org/cp/owl/informationobjectsandrepresentationlanguages.owl> ;
        <http://www.w3.org/2000/01/rdf-schema#label>
                "is representation language of"@en , "è il linguaggio di rappresentazione di"@it ;
        <http://www.w3.org/2000/01/rdf-schema#range>
                <http://www.ontologydesignpatterns.org/cp/owl/intensionextension.owl#InformationObject> .

<http://www.ontologydesignpatterns.org/cp/owl/informationobjectsandrepresentationlanguages.owl#hasRepresentationLanguage>
        a       <http://www.w3.org/2002/07/owl#ObjectProperty> ;
        <http://www.w3.org/2000/01/rdf-schema#domain>
                <http://www.ontologydesignpatterns.org/cp/owl/intensionextension.owl#InformationObject> ;
        <http://www.w3.org/2000/01/rdf-schema#isDefinedBy>
                <http://www.ontologydesignpatterns.org/cp/owl/informationobjectsandrepresentationlanguages.owl> ;
        <http://www.w3.org/2000/01/rdf-schema#label>
                "has representation language"@en , "ha linguaggio di rappresentazione"@it ;
        <http://www.w3.org/2000/01/rdf-schema#range>
                <http://www.ontologydesignpatterns.org/cp/owl/informationobjectsandrepresentationlanguages.owl#Language> ;
        <http://www.w3.org/2002/07/owl#inverseOf>
                <http://www.ontologydesignpatterns.org/cp/owl/informationobjectsandrepresentationlanguages.owl#isRepresentationLanguageOf> .

<http://www.ontologydesignpatterns.org/cp/owl/informationobjectsandrepresentationlanguages.owl>
        a       <http://www.w3.org/2002/07/owl#Ontology> ;
        <http://www.w3.org/2002/07/owl#imports>
                <http://www.ontologydesignpatterns.org/cp/owl/intensionextension.owl> , <http://www.ontologydesignpatterns.org/cp/owl/partof.owl> , <http://www.ontologydesignpatterns.org/cp/owl/communities.owl> ;
        <http://www.w3.org/2002/07/owl#versionInfo>
                "1.1 added rdfs:isDefinedBy for all named entities" .

<http://www.ontologydesignpatterns.org/cp/owl/informationobjectsandrepresentationlanguages.owl#LinguisticObject>
        a       <http://www.w3.org/2002/07/owl#Class> ;
        <http://www.w3.org/2000/01/rdf-schema#comment>
                "An information object represented in a NaturalLanguage" ;
        <http://www.w3.org/2000/01/rdf-schema#isDefinedBy>
                <http://www.ontologydesignpatterns.org/cp/owl/informationobjectsandrepresentationlanguages.owl> ;
        <http://www.w3.org/2000/01/rdf-schema#label>
                "Oggetto linguistico"@it , "Linguistic object"@en ;
        <http://www.w3.org/2000/01/rdf-schema#subClassOf>
                <http://www.ontologydesignpatterns.org/cp/owl/intensionextension.owl#InformationObject> ;
        <http://www.w3.org/2000/01/rdf-schema#subClassOf>
                [ a       <http://www.w3.org/2002/07/owl#Restriction> ;
                  <http://www.w3.org/2002/07/owl#onProperty>
                          <http://www.ontologydesignpatterns.org/cp/owl/informationobjectsandrepresentationlanguages.owl#hasRepresentationLanguage> ;
                  <http://www.w3.org/2002/07/owl#someValuesFrom>
                          <http://www.ontologydesignpatterns.org/cp/owl/informationobjectsandrepresentationlanguages.owl#NaturalLanguage>
                ] .

<http://www.ontologydesignpatterns.org/cp/owl/agentrole.owl#Agent>
        a       <http://www.w3.org/2002/07/owl#Class> .

<http://www.ontologydesignpatterns.org/cp/owl/informationobjectsandrepresentationlanguages.owl#formallyRepresents>
        a       <http://www.w3.org/2002/07/owl#ObjectProperty> ;
        <http://www.w3.org/2000/01/rdf-schema#comment>
                "The relation between formal expressions, and anything that they are supposed to represent.\nE.g., 'the predicate 'MariachiInTijuana' formallyRepresents the dul:Collection of all mariachis in Tijuana'; 'the equivalence relation '<=>' formallyRepresents the concept of two entities having the same properties'.\nNotice that formal expressions are formally interpreted by instances of dul:FormalEntity" ;
        <http://www.w3.org/2000/01/rdf-schema#domain>
                <http://www.ontologydesignpatterns.org/cp/owl/informationobjectsandrepresentationlanguages.owl#FormalExpression> ;
        <http://www.w3.org/2000/01/rdf-schema#isDefinedBy>
                <http://www.ontologydesignpatterns.org/cp/owl/informationobjectsandrepresentationlanguages.owl> ;
        <http://www.w3.org/2000/01/rdf-schema#label>
                "formally represents"@en , "rappresenta formalmente"@it ;
        <http://www.w3.org/2002/07/owl#inverseOf>
                <http://www.ontologydesignpatterns.org/cp/owl/informationobjectsandrepresentationlanguages.owl#isFormallyRepresentedIn> .

<http://www.ontologydesignpatterns.org/cp/owl/informationobjectsandrepresentationlanguages.owl#conceptualizes>
        a       <http://www.w3.org/2002/07/owl#ObjectProperty> ;
        <http://www.w3.org/2000/01/rdf-schema#comment>
                "A relation stating that an Agent is internally representing a SocialObject . E.g., 'John believes in the conspiracy theory'; 'Niels Bohr created the solar-system metaphor for the atomic theory'; 'Jacques assumes all swans are white'; 'the task force members share the attack plan'." ;
        <http://www.w3.org/2000/01/rdf-schema#domain>
                [ a       <http://www.w3.org/2002/07/owl#Class> ;
                  <http://www.w3.org/2002/07/owl#unionOf>
                          ( <http://www.ontologydesignpatterns.org/cp/owl/agentrole.owl#Agent> <http://www.ontologydesignpatterns.org/cp/owl/communities.owl#Community> )
                ] ;
        <http://www.w3.org/2000/01/rdf-schema#isDefinedBy>
                <http://www.ontologydesignpatterns.org/cp/owl/informationobjectsandrepresentationlanguages.owl> ;
        <http://www.w3.org/2000/01/rdf-schema#label>
                "concettualizza"@it , "conceptualizes"@en ;
        <http://www.w3.org/2000/01/rdf-schema#range>
                <http://www.ontologydesignpatterns.org/cp/owl/intensionextension.owl#SocialObject> .

<http://www.w3.org/2000/01/rdf-schema#comment>
        a       <http://www.w3.org/2002/07/owl#AnnotationProperty> .

<http://www.ontologydesignpatterns.org/cp/owl/intensionextension.owl#InformationObject>
        a       <http://www.w3.org/2002/07/owl#Class> .

<http://www.w3.org/2002/07/owl#versionInfo>
        a       <http://www.w3.org/2002/07/owl#AnnotationProperty> .

<http://www.w3.org/2000/01/rdf-schema#isDefinedBy>
        a       <http://www.w3.org/2002/07/owl#AnnotationProperty> .

<http://www.w3.org/2000/01/rdf-schema#label>
        a       <http://www.w3.org/2002/07/owl#AnnotationProperty> .

<http://www.w3.org/2002/07/owl#Thing>
        a       <http://www.w3.org/2002/07/owl#Class> .

<http://www.ontologydesignpatterns.org/cp/owl/partof.owl#hasPart>
        a       <http://www.w3.org/2002/07/owl#ObjectProperty> .
