<http://rdfs.co/juso/post_office_box>
        a       <http://www.w3.org/2002/07/owl#DatatypeProperty> ;
        <http://www.w3.org/2000/01/rdf-schema#domain>
                <http://rdfs.co/juso/Address> ;
        <http://www.w3.org/2000/01/rdf-schema#isDefinedBy>
                <http://rdfs.co/juso/> ;
        <http://www.w3.org/2000/01/rdf-schema#range>
                <http://www.w3.org/2001/XMLSchema#string> ;
        <http://purl.org/dc/terms/issued>
                "2015-10-02+09:00"^^<http://www.w3.org/2001/XMLSchema#date> ;
        <http://purl.org/dc/terms/modified>
                "2015-10-02+09:00"^^<http://www.w3.org/2001/XMLSchema#date> ;
        <http://www.w3.org/2002/07/owl#sameAs>
                <http://schema.org/postOfficeBoxNumber> , <http://www.w3.org/ns/locn#poBox> ;
        <http://www.w3.org/2003/06/sw-vocab-status/ns#term_status>
                "unstable"@en ;
        <http://www.w3.org/2004/02/skos/core#definition>
                "\n    This property describes the post office box number for PO box addresses.\n    A post-office box or post office box (commonly referred to as a PO box or a\n    postal box) is a uniquely addressable lockable box located on the premises\n    of a post office station.\n    "@en ;
        <http://www.w3.org/2004/02/skos/core#prefLabel>
                "post office box"@en .

<http://rdfs.co/juso/political_division>
        a       <http://www.w3.org/2002/07/owl#TransitiveProperty> ;
        <http://www.w3.org/2000/01/rdf-schema#domain>
                <http://rdfs.co/juso/Feature> ;
        <http://www.w3.org/2000/01/rdf-schema#isDefinedBy>
                <http://rdfs.co/juso/> ;
        <http://www.w3.org/2000/01/rdf-schema#range>
                <http://rdfs.co/juso/PoliticalDivision> ;
        <http://purl.org/dc/terms/issued>
                "2015-10-02+09:00"^^<http://www.w3.org/2001/XMLSchema#date> ;
        <http://purl.org/dc/terms/modified>
                "2015-10-02+09:00"^^<http://www.w3.org/2001/XMLSchema#date> ;
        <http://www.w3.org/2003/06/sw-vocab-status/ns#term_status>
                "unstable"@en ;
        <http://www.w3.org/2004/02/skos/core#definition>
                "\n    A politial or administrative division that contain the current feature.\n    "@en ;
        <http://www.w3.org/2004/02/skos/core#prefLabel>
                "political division"@en .

<http://rdfs.co/juso/alternate_name>
        a       <http://www.w3.org/2002/07/owl#DatatypeProperty> ;
        <http://www.w3.org/2000/01/rdf-schema#domain>
                <http://rdfs.co/juso/SpatialThing> ;
        <http://www.w3.org/2000/01/rdf-schema#isDefinedBy>
                <http://rdfs.co/juso/> ;
        <http://www.w3.org/2000/01/rdf-schema#range>
                <http://www.w3.org/2001/XMLSchema#string> ;
        <http://www.w3.org/2000/01/rdf-schema#seeAlso>
                <http://www.geonames.org/ontology#alternateName> ;
        <http://www.w3.org/2000/01/rdf-schema#subPropertyOf>
                <http://rdfs.co/juso/name> ;
        <http://purl.org/dc/terms/issued>
                "2015-12-30+09:00"^^<http://www.w3.org/2001/XMLSchema#date> ;
        <http://purl.org/dc/terms/modified>
                "2015-12-30+09:00"^^<http://www.w3.org/2001/XMLSchema#date> ;
        <http://www.w3.org/2002/07/owl#propertyDisjointWith>
                <http://rdfs.co/juso/official_name> ;
        <http://www.w3.org/2003/06/sw-vocab-status/ns#term_status>
                "unstable"@en ;
        <http://www.w3.org/2004/02/skos/core#definition>
                "\n    This property indicates the alternate name of the spatial thing.\n    "@en ;
        <http://www.w3.org/2004/02/skos/core#prefLabel>
                "대체 이름"@ko , "alternate name"@en .

<http://rdfs.co/juso/SecondLevelAdministrativeDivision>
        a       <http://www.w3.org/2002/07/owl#Class> ;
        <http://www.w3.org/2000/01/rdf-schema#isDefinedBy>
                <http://rdfs.co/juso/> ;
        <http://www.w3.org/2000/01/rdf-schema#seeAlso>
                <http://www.geonames.org/ontology#A.ADM2> ;
        <http://www.w3.org/2000/01/rdf-schema#subClassOf>
                <http://rdfs.co/juso/AdministrativeDivision> ;
        <http://purl.org/dc/terms/issued>
                "2015-10-02+09:00"^^<http://www.w3.org/2001/XMLSchema#date> ;
        <http://purl.org/dc/terms/modified>
                "2015-10-02+09:00"^^<http://www.w3.org/2001/XMLSchema#date> ;
        <http://www.w3.org/2003/06/sw-vocab-status/ns#term_status>
                "unstable"@en ;
        <http://www.w3.org/2004/02/skos/core#altLabel>
                "Second-order Administrative Division"@en , "Second Administrative Level"@en ;
        <http://www.w3.org/2004/02/skos/core#definition>
                "\n    A subdivision of a first-level administrative division.\n    "@en ;
        <http://www.w3.org/2004/02/skos/core#prefLabel>
                "Second-level Administrative Division"@en .

<http://rdfs.co/juso/itrf2000_long>
        a       <http://www.w3.org/2002/07/owl#DatatypeProperty> ;
        <http://www.w3.org/2000/01/rdf-schema#domain>
                <http://rdfs.co/juso/Point> ;
        <http://www.w3.org/2000/01/rdf-schema#isDefinedBy>
                <http://rdfs.co/juso/> ;
        <http://www.w3.org/2000/01/rdf-schema#range>
                <http://www.w3.org/2001/XMLSchema#string> ;
        <http://purl.org/dc/terms/issued>
                "2015-11-10+09:00"^^<http://www.w3.org/2001/XMLSchema#date> ;
        <http://purl.org/dc/terms/modified>
                "2015-11-10+09:00"^^<http://www.w3.org/2001/XMLSchema#date> ;
        <http://www.w3.org/2003/06/sw-vocab-status/ns#term_status>
                "unstable"@en ;
        <http://www.w3.org/2004/02/skos/core#definition>
                "\n    The ITRF2000 longitude of a point (decimal degrees).\n    "@en ;
        <http://www.w3.org/2004/02/skos/core#prefLabel>
                "longitude (ITRF2000)"@en , "경도(ITRF2000)"@ko .

<http://rdfs.co/juso/Geometry>
        a       <http://www.w3.org/2002/07/owl#Class> ;
        <http://www.w3.org/2000/01/rdf-schema#isDefinedBy>
                <http://rdfs.co/juso/> ;
        <http://www.w3.org/2000/01/rdf-schema#seeAlso>
                <https://en.wikipedia.org/wiki/Geometry> ;
        <http://www.w3.org/2000/01/rdf-schema#subClassOf>
                <http://rdfs.co/juso/SpatialThing> ;
        <http://purl.org/dc/terms/issued>
                "2015-10-02+09:00"^^<http://www.w3.org/2001/XMLSchema#date> ;
        <http://purl.org/dc/terms/modified>
                "2015-10-02+09:00"^^<http://www.w3.org/2001/XMLSchema#date> ;
        <http://www.w3.org/2002/07/owl#disjointWith>
                <http://rdfs.co/juso/Feature> ;
        <http://www.w3.org/2002/07/owl#sameAs>
                <http://www.w3.org/ns/locn#Geometry> , <http://www.opengis.net/ont/geosparql#Geometry> , <http://geovocab.org/geometry#Geometry> ;
        <http://www.w3.org/2003/06/sw-vocab-status/ns#term_status>
                "unstable"@en ;
        <http://www.w3.org/2004/02/skos/core#definition>
                "\n    Geometry provides \"the means for the quantitative description, by means of\n    coordinates and mathematical functions, of the spatial characteristics of\n    features, including dimension, position, size, shape, and orientation\", as\n    defined in ISO 19107.\n    "@en ;
        <http://www.w3.org/2004/02/skos/core#prefLabel>
                "Geometry"@en , "기하"@ko .

<http://rdfs.co/juso/first_level_administrative_division>
        a       <http://www.w3.org/2002/07/owl#ObjectProperty> ;
        <http://www.w3.org/2000/01/rdf-schema#domain>
                <http://rdfs.co/juso/Address> ;
        <http://www.w3.org/2000/01/rdf-schema#isDefinedBy>
                <http://rdfs.co/juso/> ;
        <http://www.w3.org/2000/01/rdf-schema#range>
                <http://rdfs.co/juso/FirstLevelAdministrativeDivision> ;
        <http://purl.org/dc/terms/issued>
                "2015-10-02+09:00"^^<http://www.w3.org/2001/XMLSchema#date> ;
        <http://purl.org/dc/terms/modified>
                "2015-10-02+09:00"^^<http://www.w3.org/2001/XMLSchema#date> ;
        <http://www.w3.org/2003/06/sw-vocab-status/ns#term_status>
                "unstable"@en ;
        <http://www.w3.org/2004/02/skos/core#definition>
                "\n    The first-level administrative division (region) of the address, usually a\n    county, state or other such area that typically encompasses several\n    localities.\n    "@en ;
        <http://www.w3.org/2004/02/skos/core#prefLabel>
                "first-level administrative division"@en .

<http://rdfs.co/juso/City>
        a       <http://www.w3.org/2002/07/owl#Class> ;
        <http://www.w3.org/2000/01/rdf-schema#isDefinedBy>
                <http://rdfs.co/juso/> ;
        <http://www.w3.org/2000/01/rdf-schema#seeAlso>
                <https://en.wikipedia.org/wiki/City> ;
        <http://www.w3.org/2000/01/rdf-schema#subClassOf>
                <http://schema.org/City> , <http://rdfs.co/juso/AdministrativeDivision> ;
        <http://purl.org/dc/terms/issued>
                "2015-10-02+09:00"^^<http://www.w3.org/2001/XMLSchema#date> ;
        <http://purl.org/dc/terms/modified>
                "2015-10-02+09:00"^^<http://www.w3.org/2001/XMLSchema#date> ;
        <http://www.w3.org/2002/07/owl#sameAs>
                <http://dbpedia.org/ontology/City> , <http://linkedgeodata.org/ontology/City> ;
        <http://www.w3.org/2003/06/sw-vocab-status/ns#term_status>
                "unstable"@en ;
        <http://www.w3.org/2004/02/skos/core#definition>
                "\n    A city is a large and permanent human settlement. Although there is no\n    agreement on how a city is distinguished from a town in general English\n    language meanings, many cities have a particular administrative, legal, or\n    historical status based on local law.\n    "@en ;
        <http://www.w3.org/2004/02/skos/core#prefLabel>
                "시"@ko , "市"@ja , "City"@en .

<http://rdfs.co/juso/endonym>
        a       <http://www.w3.org/2002/07/owl#DatatypeProperty> ;
        <http://www.w3.org/2000/01/rdf-schema#domain>
                <http://rdfs.co/juso/Feature> ;
        <http://www.w3.org/2000/01/rdf-schema#isDefinedBy>
                <http://rdfs.co/juso/> ;
        <http://www.w3.org/2000/01/rdf-schema#range>
                <http://www.w3.org/2001/XMLSchema#string> ;
        <http://www.w3.org/2000/01/rdf-schema#seeAlso>
                <https://en.wikipedia.org/wiki/Exonym_and_endonym> ;
        <http://www.w3.org/2000/01/rdf-schema#subPropertyOf>
                <http://rdfs.co/juso/name> , <http://www.geonames.org/ontology#officialName> , <http://www.w3.org/2004/02/skos/core#prefLabel> ;
        <http://purl.org/dc/terms/issued>
                "2015-10-02+09:00"^^<http://www.w3.org/2001/XMLSchema#date> ;
        <http://purl.org/dc/terms/modified>
                "2015-10-02+09:00"^^<http://www.w3.org/2001/XMLSchema#date> ;
        <http://www.w3.org/2003/06/sw-vocab-status/ns#term_status>
                "unstable"@en ;
        <http://www.w3.org/2004/02/skos/core#definition>
                "\n    The endonym is a name given by members of a particular ethnolinguistic\n    group to its homeland or a specific place within it.\n    "@en ;
        <http://www.w3.org/2004/02/skos/core#prefLabel>
                "endonym"@en .

<http://rdfs.co/juso/itrf2000_lat>
        a       <http://www.w3.org/2002/07/owl#DatatypeProperty> ;
        <http://www.w3.org/2000/01/rdf-schema#domain>
                <http://rdfs.co/juso/Point> ;
        <http://www.w3.org/2000/01/rdf-schema#isDefinedBy>
                <http://rdfs.co/juso/> ;
        <http://www.w3.org/2000/01/rdf-schema#range>
                <http://www.w3.org/2001/XMLSchema#string> ;
        <http://purl.org/dc/terms/issued>
                "2015-11-10+09:00"^^<http://www.w3.org/2001/XMLSchema#date> ;
        <http://purl.org/dc/terms/modified>
                "2015-11-10+09:00"^^<http://www.w3.org/2001/XMLSchema#date> ;
        <http://www.w3.org/2003/06/sw-vocab-status/ns#term_status>
                "unstable"@en ;
        <http://www.w3.org/2004/02/skos/core#definition>
                "\n    The ITRF2000 latitude of a point (decimal degrees).\n    "@en ;
        <http://www.w3.org/2004/02/skos/core#prefLabel>
                "위도(ITRF2000)"@ko , "latitude (ITRF2000)"@en .

<http://rdfs.co/juso/third_level_administrative_division>
        a       <http://www.w3.org/2002/07/owl#ObjectProperty> ;
        <http://www.w3.org/2000/01/rdf-schema#domain>
                <http://rdfs.co/juso/Address> ;
        <http://www.w3.org/2000/01/rdf-schema#isDefinedBy>
                <http://rdfs.co/juso/> ;
        <http://www.w3.org/2000/01/rdf-schema#range>
                <http://rdfs.co/juso/ThirdLevelAdministrativeDivision> ;
        <http://purl.org/dc/terms/issued>
                "2015-10-02+09:00"^^<http://www.w3.org/2001/XMLSchema#date> ;
        <http://purl.org/dc/terms/modified>
                "2015-10-02+09:00"^^<http://www.w3.org/2001/XMLSchema#date> ;
        <http://www.w3.org/2003/06/sw-vocab-status/ns#term_status>
                "unstable"@en ;
        <http://www.w3.org/2004/02/skos/core#definition>
                "\n    The third-level administrative division of the address, if any.\n    "@en ;
        <http://www.w3.org/2004/02/skos/core#prefLabel>
                "third-level administrative division"@en .

<http://rdfs.co/juso/thoroughfare>
        a       <http://www.w3.org/2002/07/owl#ObjectProperty> ;
        <http://www.w3.org/2000/01/rdf-schema#domain>
                <http://rdfs.co/juso/Address> ;
        <http://www.w3.org/2000/01/rdf-schema#isDefinedBy>
                <http://rdfs.co/juso/> ;
        <http://www.w3.org/2000/01/rdf-schema#range>
                <http://rdfs.co/juso/Thoroughfare> ;
        <http://purl.org/dc/terms/issued>
                "2015-10-02+09:00"^^<http://www.w3.org/2001/XMLSchema#date> ;
        <http://purl.org/dc/terms/modified>
                "2015-10-02+09:00"^^<http://www.w3.org/2001/XMLSchema#date> ;
        <http://www.w3.org/2003/06/sw-vocab-status/ns#term_status>
                "unstable"@en ;
        <http://www.w3.org/2004/02/skos/core#definition>
                "\n    An address component that represents the name of a passage or way through\n    from one location to another. A thoroughfare is not necessarily a road, it\n    might be a waterway or some other feature.\n    "@en ;
        <http://www.w3.org/2004/02/skos/core#prefLabel>
                "thoroughfare"@en .

<http://rdfs.co/juso/country>
        a       <http://www.w3.org/2002/07/owl#ObjectProperty> ;
        <http://www.w3.org/2000/01/rdf-schema#domain>
                <http://rdfs.co/juso/Address> ;
        <http://www.w3.org/2000/01/rdf-schema#isDefinedBy>
                <http://rdfs.co/juso/> ;
        <http://www.w3.org/2000/01/rdf-schema#range>
                <http://rdfs.co/juso/Country> ;
        <http://purl.org/dc/terms/issued>
                "2015-10-02+09:00"^^<http://www.w3.org/2001/XMLSchema#date> ;
        <http://purl.org/dc/terms/modified>
                "2015-10-02+09:00"^^<http://www.w3.org/2001/XMLSchema#date> ;
        <http://www.w3.org/2002/07/owl#sameAs>
                <http://ontology.eil.utoronto.ca/icontact.owl#hasCountry> ;
        <http://www.w3.org/2003/06/sw-vocab-status/ns#term_status>
                "unstable"@en ;
        <http://www.w3.org/2004/02/skos/core#definition>
                "\n    The uppermost politial division for the address, almost always a country.\n    "@en ;
        <http://www.w3.org/2004/02/skos/core#prefLabel>
                "country"@en .

<http://rdfs.co/juso/AdministrativeDivision>
        a       <http://www.w3.org/2002/07/owl#Class> ;
        <http://www.w3.org/2000/01/rdf-schema#isDefinedBy>
                <http://rdfs.co/juso/> ;
        <http://www.w3.org/2000/01/rdf-schema#seeAlso>
                <http://www.geonames.org/ontology#A.ADMD> , <https://en.wikipedia.org/wiki/Administrative_division> ;
        <http://www.w3.org/2000/01/rdf-schema#subClassOf>
                <http://rdfs.co/juso/PoliticalDivision> ;
        <http://purl.org/dc/terms/issued>
                "2015-10-02+09:00"^^<http://www.w3.org/2001/XMLSchema#date> ;
        <http://purl.org/dc/terms/modified>
                "2015-10-02+09:00"^^<http://www.w3.org/2001/XMLSchema#date> ;
        <http://www.w3.org/2003/06/sw-vocab-status/ns#term_status>
                "unstable"@en ;
        <http://www.w3.org/2004/02/skos/core#altLabel>
                "Administrative Unit"@en , "Country Subdivision"@en , "Administrative Entity"@en , "Geopolitical Division"@en , "Subnational Entity"@en ;
        <http://www.w3.org/2004/02/skos/core#definition>
                "\n    An administrative division is a portion of a country or other region\n    delineated for the purpose of administration. Administrative divisions are\n    each granted a certain degree of autonomy and are usually required to\n    manage themselves through their own local governments.\n    "@en ;
        <http://www.w3.org/2004/02/skos/core#prefLabel>
                "Administrative Division"@en .

<http://rdfs.co/juso/Township>
        a       <http://www.w3.org/2002/07/owl#Class> ;
        <http://www.w3.org/2000/01/rdf-schema#isDefinedBy>
                <http://rdfs.co/juso/> ;
        <http://www.w3.org/2000/01/rdf-schema#seeAlso>
                <https://en.wikipedia.org/wiki/Township> ;
        <http://www.w3.org/2000/01/rdf-schema#subClassOf>
                <http://rdfs.co/juso/AdministrativeDivision> ;
        <http://purl.org/dc/terms/issued>
                "2015-10-02+09:00"^^<http://www.w3.org/2001/XMLSchema#date> ;
        <http://purl.org/dc/terms/modified>
                "2015-10-02+09:00"^^<http://www.w3.org/2001/XMLSchema#date> ;
        <http://www.w3.org/2003/06/sw-vocab-status/ns#term_status>
                "unstable"@en ;
        <http://www.w3.org/2004/02/skos/core#definition>
                "\n    The word township is used to refer to different kinds of settlements in\n    different countries.\n    "@en ;
        <http://www.w3.org/2004/02/skos/core#prefLabel>
                "면"@ko , "Township"@en .

<http://rdfs.co/juso/Country>
        a       <http://www.w3.org/2002/07/owl#Class> ;
        <http://www.w3.org/2000/01/rdf-schema#isDefinedBy>
                <http://rdfs.co/juso/> ;
        <http://www.w3.org/2000/01/rdf-schema#seeAlso>
                <https://en.wikipedia.org/wiki/Country> ;
        <http://www.w3.org/2000/01/rdf-schema#subClassOf>
                <http://rdfs.co/juso/PoliticalDivision> ;
        <http://purl.org/dc/terms/issued>
                "2015-10-02+09:00"^^<http://www.w3.org/2001/XMLSchema#date> ;
        <http://purl.org/dc/terms/modified>
                "2015-10-02+09:00"^^<http://www.w3.org/2001/XMLSchema#date> ;
        <http://www.w3.org/2002/07/owl#sameAs>
                <http://schema.org/Country> , <http://dbpedia.org/ontology/Country> , <http://linkedgeodata.org/ontology/Country> ;
        <http://www.w3.org/2003/06/sw-vocab-status/ns#term_status>
                "unstable"@en ;
        <http://www.w3.org/2004/02/skos/core#altLabel>
                "국가"@ko , "国家"@ja ;
        <http://www.w3.org/2004/02/skos/core#definition>
                "\n    A country is a region that is identified as a distinct entity in political\n    geography. A country may be an independent sovereign state or one that is\n    occupied by another state, as a non-sovereign or formerly sovereign\n    political division, or a geographic region associated with sets of\n    previously independent or differently associated people with distinct\n    political characteristics.\n    "@en ;
        <http://www.w3.org/2004/02/skos/core#prefLabel>
                "国"@ja , "Country"@en , "나라"@ko .

<http://rdfs.co/juso/Point>
        a       <http://www.w3.org/2002/07/owl#Class> ;
        <http://www.w3.org/2000/01/rdf-schema#isDefinedBy>
                <http://rdfs.co/juso/> ;
        <http://www.w3.org/2000/01/rdf-schema#seeAlso>
                <https://en.wikipedia.org/wiki/Point_(geometry)> ;
        <http://www.w3.org/2000/01/rdf-schema#subClassOf>
                <http://rdfs.co/juso/Geometry> ;
        <http://purl.org/dc/terms/issued>
                "2015-11-10+09:00"^^<http://www.w3.org/2001/XMLSchema#date> ;
        <http://purl.org/dc/terms/modified>
                "2015-11-10+09:00"^^<http://www.w3.org/2001/XMLSchema#date> ;
        <http://www.w3.org/2002/07/owl#sameAs>
                <http://www.w3.org/2003/01/geo/wgs84_pos#Point> ;
        <http://www.w3.org/2003/06/sw-vocab-status/ns#term_status>
                "unstable"@en ;
        <http://www.w3.org/2004/02/skos/core#definition>
                "\n    A point is a geographical point on the surface of the Earth, typically\n    described using a coordinate system relative to the Earth, such as WGS84.\n  "@en ;
        <http://www.w3.org/2004/02/skos/core#prefLabel>
                "점"@ko , "Point"@en .

<http://rdfs.co/juso/fifth_level_administrative_division>
        a       <http://www.w3.org/2002/07/owl#ObjectProperty> ;
        <http://www.w3.org/2000/01/rdf-schema#domain>
                <http://rdfs.co/juso/Address> ;
        <http://www.w3.org/2000/01/rdf-schema#isDefinedBy>
                <http://rdfs.co/juso/> ;
        <http://www.w3.org/2000/01/rdf-schema#range>
                <http://rdfs.co/juso/FifthLevelAdministrativeDivision> ;
        <http://purl.org/dc/terms/issued>
                "2015-10-02+09:00"^^<http://www.w3.org/2001/XMLSchema#date> ;
        <http://purl.org/dc/terms/modified>
                "2015-10-02+09:00"^^<http://www.w3.org/2001/XMLSchema#date> ;
        <http://www.w3.org/2003/06/sw-vocab-status/ns#term_status>
                "unstable"@en ;
        <http://www.w3.org/2004/02/skos/core#definition>
                "\n    The fifth-level administrative division of the address, if any.\n    "@en ;
        <http://www.w3.org/2004/02/skos/core#prefLabel>
                "fifth-level administrative division"@en .

<http://rdfs.co/juso/0.1.2>
        a       <http://creativecommons.org/ns#Work> , <http://www.w3.org/ns/adms#SemanticAsset> , <http://www.w3.org/2002/07/owl#Ontology> , <http://purl.org/vocommons/voaf#Vocabulary> ;
        <http://www.w3.org/2000/01/rdf-schema#comment>
                "\n    There is an extension to this ontology with some country-specific terms for\n    <a href=\"http://rdfs.co/juso/kr/\">South Korea</a>.\n    "@ko , "\n    <div>\n      The master version of this vocabulary is maintained in <a\n      href=\"https://github.com/listinc/juso-ontology\">the GitHub repository</a>\n      so others can contribute edits and improvements.\n    </div>\n    "^^<http://www.w3.org/1999/02/22-rdf-syntax-ns#HTML> , "\n    Most of the descriptions given here are from Wikipedia or from the related\n    ontologies and vocabularies.\n    "@en ;
        <http://www.w3.org/2000/01/rdf-schema#seeAlso>
                <https://github.com/listinc/juso-ontology> ;
        <http://creativecommons.org/ns#license>
                <http://creativecommons.org/licenses/by/4.0/> ;
        <http://purl.org/dc/terms/creator>
                <http://jayg.me/> ;
        <http://purl.org/dc/terms/description>
                "\n    Juso Ontology is a Web vocabulary for describing geographical addresses and\n    features.\n    "@en ;
        <http://purl.org/dc/terms/hasFormat>
                <http://rdfs.co/juso/0.1.2/rdf> , <http://rdfs.co/juso/0.1.2/ttl> , <http://rdfs.co/juso/0.1.2/html> ;
        <http://purl.org/dc/terms/identifier>
                "http://rdfs.co/juso/0.1.2" ;
        <http://purl.org/dc/terms/isVersionOf>
                <http://rdfs.co/juso/> ;
        <http://purl.org/dc/terms/issued>
                "2015-10-02+09:00"^^<http://www.w3.org/2001/XMLSchema#date> ;
        <http://purl.org/dc/terms/modified>
                "2015-12-30+09:00"^^<http://www.w3.org/2001/XMLSchema#date> ;
        <http://purl.org/dc/terms/publisher>
                <http://listinc.kr/id/listinc> ;
        <http://purl.org/dc/terms/replaces>
                <http://rdfs.co/juso/0.1.1> ;
        <http://purl.org/dc/terms/rights>
                "Copyright © 2015 LiST Inc. Some Rights Reserved." ;
        <http://purl.org/dc/terms/title>
                "주소 온톨로지"@ko , "Juso Ontology"@en ;
        <http://purl.org/dc/terms/type>
                <http://purl.org/adms/assettype/Ontology> ;
        <http://purl.org/vocab/vann/example>
                [ <http://www.w3.org/2000/01/rdf-schema#comment>
                          "\n    <pre><code>_:YangyongBldg a juso:Feature ;\n  juso:name \"Yangyong Building\"@en , \"양용빌딩\"@ko ;\n  juso:geometry &lt;http://geohash.org/wydjrzg6ece9&gt; .\n\n_:LiSTInc a juso:SpatialThing , foaf:Organization ;\n  juso:name \"LiST Inc.\"@en , \"주식회사 리스트\"@ko ;\n  juso:within _:YangyongBldg ;\n  juso:historical_address [\n    a juso:Address ;\n    juso:full_address\n      \"대한민국 서울특별시 영등포구 당산동 121-17 양용빌딩 9층 150-040\"@ko ,\n      \"9th Floor, Yangyong Building, 121-17, Dangsan-dong, Yeongdeungpo-gu, Seoul, 150-040, South Korea\"@en ;\n    juso:country &lt;http://sws.geonames.org/1835841/&gt; ;\n    juso:first_level_administrative_division &lt;http://sws.geonames.org/1835847/&gt; ;\n    juso:second_level_administrative_division &lt;http://sws.geonames.org/1832536/&gt; ;\n    juso:third_level_administrative_division &lt;http://sws.geonames.org/8692617/&gt; ;\n    juso:locator _:YangyongBldg ;\n    juso:locator_address \"9층\"@ko , \"9th Floor\"@en ;\n    juso:postal_code [\n      a juso:PostalCode ;\n      rdf:value \"150-040\"\n    ]\n  ] ;\n  juso:address [\n    a juso:Address ;\n    juso:full_address\n      \"대한민국 서울특별시 영등포구 버드나루로19길 3 (당산동) 양용빌딩 9층 07229\"@ko ,\n      \"9th Floor, Yangyong Building, 3, Beodeunaru-ro 19-gil, Yeongdeungpo-gu, Seoul, 07229, South Korea\"@en ;\n    juso:country &lt;http://sws.geonames.org/1835841/&gt; ;\n    juso:first_level_administrative_division &lt;http://sws.geonames.org/1835847/&gt; ;\n    juso:second_level_administrative_division &lt;http://sws.geonames.org/1832536/&gt; ;\n    juso:third_level_administrative_division &lt;http://sws.geonames.org/8692617/&gt; ;\n    juso:thoroughfare [\n      a juso:Street ;\n      juso:name \"Beodeunaru-ro 19-gil\"@en , \"버드나루로19길\"@ko ;\n      juso:parent &lt;http://sws.geonames.org/8692617/&gt;\n    ] ;\n    juso:thoroughfare_address \"3\" ;\n    juso:locator _:YangyongBldg ;\n    juso:locator_address \"9층\"@ko , \"9th Floor\"@en ;\n    juso:postal_code [\n      a juso:PostalCode ;\n      rdf:value \"07229\"\n    ]\n  ] .</code></pre>\n    "^^<http://www.w3.org/1999/02/22-rdf-syntax-ns#HTML> ;
                  <http://www.w3.org/2000/01/rdf-schema#label>
                          "LiST Inc."@en
                ] ;
        <http://purl.org/vocab/vann/preferredNamespacePrefix>
                "juso" ;
        <http://purl.org/vocab/vann/preferredNamespaceUri>
                "http://rdfs.co/juso/" ;
        <http://purl.org/vocab/vann/termGroup>
                <http://rdfs.co/juso/PoliticalDivisionGroup> , <http://rdfs.co/juso/CoreGroup> , <http://rdfs.co/juso/AddressGroup> ;
        <http://www.w3.org/2002/07/owl#versionInfo>
                "0.1.2" ;
        <http://www.w3.org/2004/02/skos/core#changeNote>
                [ <http://www.w3.org/1999/02/22-rdf-syntax-ns#value>
                          "\n      Fixed the wrong use of rdf:XMLLiteral\n      "@en ;
                  <http://purl.org/dc/terms/creator>
                          <http://jayg.me/> ;
                  <http://purl.org/dc/terms/date>
                          "2015-10-07+09:00"^^<http://www.w3.org/2001/XMLSchema#date>
                ] ;
        <http://www.w3.org/2004/02/skos/core#historyNote>
                [ <http://www.w3.org/1999/02/22-rdf-syntax-ns#value>
                          "\n      Added juso:Point, juso:wgs84_lat, juso:wgs84_long,\n      juso:itrf2000_lat, and juso:itrf2000_long\n      "@en ;
                  <http://purl.org/dc/terms/creator>
                          <http://jayg.me/> ;
                  <http://purl.org/dc/terms/date>
                          "2015-11-10+09:00"^^<http://www.w3.org/2001/XMLSchema#date>
                ] ;
        <http://www.w3.org/2004/02/skos/core#historyNote>
                [ <http://www.w3.org/1999/02/22-rdf-syntax-ns#value>
                          "\n      Added juso:official_name, juso:alternate_name, juso:short_name\n      "@en ;
                  <http://purl.org/dc/terms/creator>
                          <http://jayg.me/> ;
                  <http://purl.org/dc/terms/date>
                          "2015-12-30+09:00"^^<http://www.w3.org/2001/XMLSchema#date>
                ] ;
        <http://www.w3.org/ns/adms#status>
                <http://purl.org/adms/status/UnderDevelopment> .

<http://rdfs.co/juso/fourth_level_administrative_division>
        a       <http://www.w3.org/2002/07/owl#ObjectProperty> ;
        <http://www.w3.org/2000/01/rdf-schema#domain>
                <http://rdfs.co/juso/Address> ;
        <http://www.w3.org/2000/01/rdf-schema#isDefinedBy>
                <http://rdfs.co/juso/> ;
        <http://www.w3.org/2000/01/rdf-schema#range>
                <http://rdfs.co/juso/FourthLevelAdministrativeDivision> ;
        <http://purl.org/dc/terms/issued>
                "2015-10-02+09:00"^^<http://www.w3.org/2001/XMLSchema#date> ;
        <http://purl.org/dc/terms/modified>
                "2015-10-02+09:00"^^<http://www.w3.org/2001/XMLSchema#date> ;
        <http://www.w3.org/2003/06/sw-vocab-status/ns#term_status>
                "unstable"@en ;
        <http://www.w3.org/2004/02/skos/core#definition>
                "\n    The fourth-level administrative division of the address, if any.\n    "@en ;
        <http://www.w3.org/2004/02/skos/core#prefLabel>
                "fourth-level administrative division"@en .

<http://rdfs.co/juso/within>
        a       <http://www.w3.org/2002/07/owl#TransitiveProperty> ;
        <http://www.w3.org/2000/01/rdf-schema#domain>
                <http://rdfs.co/juso/SpatialThing> ;
        <http://www.w3.org/2000/01/rdf-schema#isDefinedBy>
                <http://rdfs.co/juso/> ;
        <http://www.w3.org/2000/01/rdf-schema#range>
                <http://rdfs.co/juso/SpatialThing> ;
        <http://www.w3.org/2000/01/rdf-schema#subPropertyOf>
                <http://www.w3.org/2003/01/geo/wgs84_pos#location> , <http://www.w3.org/ns/locn#location> ;
        <http://purl.org/dc/terms/issued>
                "2015-10-02+09:00"^^<http://www.w3.org/2001/XMLSchema#date> ;
        <http://purl.org/dc/terms/modified>
                "2015-10-02+09:00"^^<http://www.w3.org/2001/XMLSchema#date> ;
        <http://www.w3.org/2002/07/owl#inverseOf>
                <http://www.opengis.net/ont/geosparql#sfContains> , <http://geovocab.org/spatial#Pi> ;
        <http://www.w3.org/2002/07/owl#sameAs>
                <http://www.opengis.net/ont/geosparql#sfWithin> , <http://geovocab.org/spatial#P> ;
        <http://www.w3.org/2003/06/sw-vocab-status/ns#term_status>
                "testing"@en ;
        <http://www.w3.org/2004/02/skos/core#definition>
                "\n    A spatial thing that contains the current one within the borders of its own\n    region.\n    "@en ;
        <http://www.w3.org/2004/02/skos/core#prefLabel>
                "within"@en .

<http://rdfs.co/juso/CoreGroup>
        a       <http://www.w3.org/1999/02/22-rdf-syntax-ns#Bag> ;
        <http://www.w3.org/1999/02/22-rdf-syntax-ns#_1>
                <http://rdfs.co/juso/SpatialThing> ;
        <http://www.w3.org/1999/02/22-rdf-syntax-ns#_10>
                <http://rdfs.co/juso/within> ;
        <http://www.w3.org/1999/02/22-rdf-syntax-ns#_11>
                <http://rdfs.co/juso/endonym> ;
        <http://www.w3.org/1999/02/22-rdf-syntax-ns#_12>
                <http://rdfs.co/juso/exonym> ;
        <http://www.w3.org/1999/02/22-rdf-syntax-ns#_13>
                <http://rdfs.co/juso/geometry> ;
        <http://www.w3.org/1999/02/22-rdf-syntax-ns#_14>
                <http://rdfs.co/juso/address> ;
        <http://www.w3.org/1999/02/22-rdf-syntax-ns#_15>
                <http://rdfs.co/juso/historical_address> ;
        <http://www.w3.org/1999/02/22-rdf-syntax-ns#_2>
                <http://rdfs.co/juso/Feature> ;
        <http://www.w3.org/1999/02/22-rdf-syntax-ns#_3>
                <http://rdfs.co/juso/Geometry> ;
        <http://www.w3.org/1999/02/22-rdf-syntax-ns#_4>
                <http://rdfs.co/juso/Point> ;
        <http://www.w3.org/1999/02/22-rdf-syntax-ns#_5>
                <http://rdfs.co/juso/Address> ;
        <http://www.w3.org/1999/02/22-rdf-syntax-ns#_6>
                <http://rdfs.co/juso/name> ;
        <http://www.w3.org/1999/02/22-rdf-syntax-ns#_7>
                <http://rdfs.co/juso/official_name> ;
        <http://www.w3.org/1999/02/22-rdf-syntax-ns#_8>
                <http://rdfs.co/juso/alternate_name> ;
        <http://www.w3.org/1999/02/22-rdf-syntax-ns#_9>
                <http://rdfs.co/juso/short_name> ;
        <http://www.w3.org/2000/01/rdf-schema#comment>
                "\n    These classes and properties form the core of Juso Ontology. They describe\n    fundamental characteristics of geography in relatively broad terms.\n    "@en ;
        <http://www.w3.org/2000/01/rdf-schema#label>
                "Core Terms"@en .

<http://rdfs.co/juso/PostalCode>
        a       <http://www.w3.org/2002/07/owl#Class> ;
        <http://www.w3.org/2000/01/rdf-schema#isDefinedBy>
                <http://rdfs.co/juso/> ;
        <http://www.w3.org/2000/01/rdf-schema#seeAlso>
                <https://en.wikipedia.org/wiki/Postal_code> ;
        <http://purl.org/dc/terms/issued>
                "2015-10-02+09:00"^^<http://www.w3.org/2001/XMLSchema#date> ;
        <http://purl.org/dc/terms/modified>
                "2015-10-02+09:00"^^<http://www.w3.org/2001/XMLSchema#date> ;
        <http://www.w3.org/2003/06/sw-vocab-status/ns#term_status>
                "unstable"@en ;
        <http://www.w3.org/2004/02/skos/core#altLabel>
                "ZIP Code"@en , "PIN Code"@en , "Post Code"@en , "Postcode"@en , "Eircode"@en ;
        <http://www.w3.org/2004/02/skos/core#definition>
                "\n    A postal code is a series of letters and/or digits, sometimes including\n    spaces or punctuation, included in a postal address for the purpose of\n    sorting mail.\n    "@en ;
        <http://www.w3.org/2004/02/skos/core#prefLabel>
                "Postal Code"@en , "우편번호"@ko .

<http://rdfs.co/juso/Town>
        a       <http://www.w3.org/2002/07/owl#Class> ;
        <http://www.w3.org/2000/01/rdf-schema#isDefinedBy>
                <http://rdfs.co/juso/> ;
        <http://www.w3.org/2000/01/rdf-schema#seeAlso>
                <https://en.wikipedia.org/wiki/Town> ;
        <http://www.w3.org/2000/01/rdf-schema#subClassOf>
                <http://rdfs.co/juso/AdministrativeDivision> ;
        <http://purl.org/dc/terms/issued>
                "2015-10-02+09:00"^^<http://www.w3.org/2001/XMLSchema#date> ;
        <http://purl.org/dc/terms/modified>
                "2015-10-02+09:00"^^<http://www.w3.org/2001/XMLSchema#date> ;
        <http://www.w3.org/2002/07/owl#sameAs>
                <http://dbpedia.org/ontology/Town> , <http://linkedgeodata.org/ontology/Town> ;
        <http://www.w3.org/2003/06/sw-vocab-status/ns#term_status>
                "unstable"@en ;
        <http://www.w3.org/2004/02/skos/core#definition>
                "\n    A town is a human settlement larger than a village but smaller than a city.\n    The size definition for what constitutes a \"town\" varies considerably in\n    different parts of the world.\n    "@en ;
        <http://www.w3.org/2004/02/skos/core#prefLabel>
                "Town"@en , "읍"@ko .

<http://rdfs.co/juso/name>
        a       <http://www.w3.org/2002/07/owl#DatatypeProperty> ;
        <http://www.w3.org/2000/01/rdf-schema#domain>
                <http://rdfs.co/juso/SpatialThing> ;
        <http://www.w3.org/2000/01/rdf-schema#isDefinedBy>
                <http://rdfs.co/juso/> ;
        <http://www.w3.org/2000/01/rdf-schema#range>
                <http://www.w3.org/2001/XMLSchema#string> ;
        <http://www.w3.org/2000/01/rdf-schema#subPropertyOf>
                <http://schema.org/name> , <http://purl.org/dc/terms/title> ;
        <http://purl.org/dc/terms/issued>
                "2015-10-02+09:00"^^<http://www.w3.org/2001/XMLSchema#date> ;
        <http://purl.org/dc/terms/modified>
                "2015-10-02+09:00"^^<http://www.w3.org/2001/XMLSchema#date> ;
        <http://www.w3.org/2003/06/sw-vocab-status/ns#term_status>
                "testing"@en ;
        <http://www.w3.org/2004/02/skos/core#definition>
                "\n    This property indicates the name of the spatial thing.\n    "@en ;
        <http://www.w3.org/2004/02/skos/core#prefLabel>
                "name"@en , "이름"@ko .

<http://rdfs.co/juso/Address>
        a       <http://www.w3.org/2002/07/owl#Class> ;
        <http://www.w3.org/2000/01/rdf-schema#isDefinedBy>
                <http://rdfs.co/juso/> ;
        <http://www.w3.org/2000/01/rdf-schema#seeAlso>
                <https://en.wikipedia.org/wiki/Address_(geography)> ;
        <http://purl.org/dc/terms/issued>
                "2015-10-02+09:00"^^<http://www.w3.org/2001/XMLSchema#date> ;
        <http://purl.org/dc/terms/modified>
                "2015-10-02+09:00"^^<http://www.w3.org/2001/XMLSchema#date> ;
        <http://www.w3.org/2002/07/owl#sameAs>
                <http://ontology.eil.utoronto.ca/icontact.owl#Address> , <http://www.w3.org/ns/locn#Address> ;
        <http://www.w3.org/2003/06/sw-vocab-status/ns#term_status>
                "testing"@en ;
        <http://www.w3.org/2004/02/skos/core#altLabel>
                "Geographical Address"@en , "Postal Address"@en ;
        <http://www.w3.org/2004/02/skos/core#definition>
                "\n    An address is a collection of information, presented in a mostly fixed\n    format, used for describing the location of a building, apartment, or other\n    structure or a plot of land, generally using political boundaries and\n    street names as references, along with other identifiers such as house or\n    apartment numbers. Some addresses also contain special codes to aid routing\n    of mail and packages, such as a ZIP code or post code.\n    "@en ;
        <http://www.w3.org/2004/02/skos/core#prefLabel>
                "Address"@en , "주소"@ko .

<http://rdfs.co/juso/CapitalDistrict>
        a       <http://www.w3.org/2002/07/owl#Class> ;
        <http://www.w3.org/2000/01/rdf-schema#isDefinedBy>
                <http://rdfs.co/juso/> ;
        <http://www.w3.org/2000/01/rdf-schema#seeAlso>
                <https://en.wikipedia.org/wiki/Capital_districts_and_territories> ;
        <http://www.w3.org/2000/01/rdf-schema#subClassOf>
                <http://rdfs.co/juso/AdministrativeDivision> ;
        <http://purl.org/dc/terms/issued>
                "2015-10-02+09:00"^^<http://www.w3.org/2001/XMLSchema#date> ;
        <http://purl.org/dc/terms/modified>
                "2015-10-02+09:00"^^<http://www.w3.org/2001/XMLSchema#date> ;
        <http://www.w3.org/2003/06/sw-vocab-status/ns#term_status>
                "unstable"@en ;
        <http://www.w3.org/2004/02/skos/core#altLabel>
                "Capital Territory"@en ;
        <http://www.w3.org/2004/02/skos/core#definition>
                "\n    A capital district or capital territory is normally a specially designated\n    administrative division where a country's seat of government is located.\n    "@en ;
        <http://www.w3.org/2004/02/skos/core#prefLabel>
                "Capital District"@en .

<http://linkedgeodata.org/ontology/Place>
        <http://www.w3.org/2000/01/rdf-schema#subClassOf>
                <http://rdfs.co/juso/SpatialThing> .

<http://rdfs.co/juso/FifthLevelAdministrativeDivision>
        a       <http://www.w3.org/2002/07/owl#Class> ;
        <http://www.w3.org/2000/01/rdf-schema#isDefinedBy>
                <http://rdfs.co/juso/> ;
        <http://www.w3.org/2000/01/rdf-schema#seeAlso>
                <http://www.geonames.org/ontology#A.ADM5> ;
        <http://www.w3.org/2000/01/rdf-schema#subClassOf>
                <http://rdfs.co/juso/AdministrativeDivision> ;
        <http://purl.org/dc/terms/issued>
                "2015-10-02+09:00"^^<http://www.w3.org/2001/XMLSchema#date> ;
        <http://purl.org/dc/terms/modified>
                "2015-10-02+09:00"^^<http://www.w3.org/2001/XMLSchema#date> ;
        <http://www.w3.org/2003/06/sw-vocab-status/ns#term_status>
                "unstable"@en ;
        <http://www.w3.org/2004/02/skos/core#altLabel>
                "Fifth-order Administrative Division"@en , "Fifth Administrative Level"@en ;
        <http://www.w3.org/2004/02/skos/core#definition>
                "\n    A subdivision of a fourth-level administrative division.\n    "@en ;
        <http://www.w3.org/2004/02/skos/core#prefLabel>
                "Fifth-level Administrative Division"@en .

<http://rdfs.co/juso/District>
        a       <http://www.w3.org/2002/07/owl#Class> ;
        <http://www.w3.org/2000/01/rdf-schema#isDefinedBy>
                <http://rdfs.co/juso/> ;
        <http://www.w3.org/2000/01/rdf-schema#seeAlso>
                <https://en.wikipedia.org/wiki/District> ;
        <http://www.w3.org/2000/01/rdf-schema#subClassOf>
                <http://rdfs.co/juso/AdministrativeDivision> ;
        <http://purl.org/dc/terms/issued>
                "2015-10-02+09:00"^^<http://www.w3.org/2001/XMLSchema#date> ;
        <http://purl.org/dc/terms/modified>
                "2015-10-02+09:00"^^<http://www.w3.org/2001/XMLSchema#date> ;
        <http://www.w3.org/2002/07/owl#sameAs>
                <http://dbpedia.org/ontology/District> ;
        <http://www.w3.org/2003/06/sw-vocab-status/ns#term_status>
                "unstable"@en ;
        <http://www.w3.org/2004/02/skos/core#definition>
                "\n    A district is a type of administrative division that, in some countries, is\n    managed by local government. Across the world, areas known as \"districts\"\n    vary greatly in size, spanning entire regions or counties, several\n    municipalities, subdivisions of municipalities, school district, or\n    political district.\n    "@en ;
        <http://www.w3.org/2004/02/skos/core#prefLabel>
                "District"@en , "구"@ko .

<http://rdfs.co/juso/full_address>
        a       <http://www.w3.org/2002/07/owl#DatatypeProperty> ;
        <http://www.w3.org/2000/01/rdf-schema#domain>
                <http://rdfs.co/juso/Address> ;
        <http://www.w3.org/2000/01/rdf-schema#isDefinedBy>
                <http://rdfs.co/juso/> ;
        <http://www.w3.org/2000/01/rdf-schema#range>
                <http://www.w3.org/2001/XMLSchema#string> ;
        <http://purl.org/dc/terms/issued>
                "2015-10-02+09:00"^^<http://www.w3.org/2001/XMLSchema#date> ;
        <http://purl.org/dc/terms/modified>
                "2015-10-02+09:00"^^<http://www.w3.org/2001/XMLSchema#date> ;
        <http://www.w3.org/2002/07/owl#sameAs>
                <http://www.w3.org/ns/locn#fullAddress> ;
        <http://www.w3.org/2003/06/sw-vocab-status/ns#term_status>
                "testing"@en ;
        <http://www.w3.org/2004/02/skos/core#definition>
                "\n    The complete address written as a string, with or without formatting.\n    "@en ;
        <http://www.w3.org/2004/02/skos/core#prefLabel>
                "full address"@en .

<http://rdfs.co/juso/AddressGroup>
        a       <http://www.w3.org/1999/02/22-rdf-syntax-ns#Bag> ;
        <http://www.w3.org/1999/02/22-rdf-syntax-ns#_1>
                <http://rdfs.co/juso/full_address> ;
        <http://www.w3.org/1999/02/22-rdf-syntax-ns#_10>
                <http://rdfs.co/juso/thoroughfare> ;
        <http://www.w3.org/1999/02/22-rdf-syntax-ns#_11>
                <http://rdfs.co/juso/thoroughfare_address> ;
        <http://www.w3.org/1999/02/22-rdf-syntax-ns#_12>
                <http://rdfs.co/juso/locator> ;
        <http://www.w3.org/1999/02/22-rdf-syntax-ns#_13>
                <http://rdfs.co/juso/locator_address> ;
        <http://www.w3.org/1999/02/22-rdf-syntax-ns#_14>
                <http://rdfs.co/juso/po_box> ;
        <http://www.w3.org/1999/02/22-rdf-syntax-ns#_15>
                <http://rdfs.co/juso/PostalCode> ;
        <http://www.w3.org/1999/02/22-rdf-syntax-ns#_16>
                <http://rdfs.co/juso/postal_code> ;
        <http://www.w3.org/1999/02/22-rdf-syntax-ns#_2>
                <http://rdfs.co/juso/country> ;
        <http://www.w3.org/1999/02/22-rdf-syntax-ns#_3>
                <http://rdfs.co/juso/first_level_administrative_division> ;
        <http://www.w3.org/1999/02/22-rdf-syntax-ns#_4>
                <http://rdfs.co/juso/second_level_administrative_division> ;
        <http://www.w3.org/1999/02/22-rdf-syntax-ns#_5>
                <http://rdfs.co/juso/third_level_administrative_division> ;
        <http://www.w3.org/1999/02/22-rdf-syntax-ns#_6>
                <http://rdfs.co/juso/fourth_level_administrative_division> ;
        <http://www.w3.org/1999/02/22-rdf-syntax-ns#_7>
                <http://rdfs.co/juso/fifth_level_administrative_division> ;
        <http://www.w3.org/1999/02/22-rdf-syntax-ns#_8>
                <http://rdfs.co/juso/Thoroughfare> ;
        <http://www.w3.org/1999/02/22-rdf-syntax-ns#_9>
                <http://rdfs.co/juso/Street> ;
        <http://www.w3.org/2000/01/rdf-schema#comment>
                "\n    These classes and properties are used to describe addresses.\n    "@en ;
        <http://www.w3.org/2000/01/rdf-schema#label>
                "Address Terms"@en .

<http://rdfs.co/juso/County>
        a       <http://www.w3.org/2002/07/owl#Class> ;
        <http://www.w3.org/2000/01/rdf-schema#isDefinedBy>
                <http://rdfs.co/juso/> ;
        <http://www.w3.org/2000/01/rdf-schema#seeAlso>
                <https://en.wikipedia.org/wiki/County> ;
        <http://www.w3.org/2000/01/rdf-schema#subClassOf>
                <http://rdfs.co/juso/AdministrativeDivision> ;
        <http://purl.org/dc/terms/issued>
                "2015-10-02+09:00"^^<http://www.w3.org/2001/XMLSchema#date> ;
        <http://purl.org/dc/terms/modified>
                "2015-10-02+09:00"^^<http://www.w3.org/2001/XMLSchema#date> ;
        <http://www.w3.org/2002/07/owl#sameAs>
                <http://linkedgeodata.org/ontology/County> ;
        <http://www.w3.org/2003/06/sw-vocab-status/ns#term_status>
                "unstable"@en ;
        <http://www.w3.org/2004/02/skos/core#altLabel>
                "Co."@en-gb , "Cnty."@en-us ;
        <http://www.w3.org/2004/02/skos/core#definition>
                "\n    A county is a geographical region of a country used for administrative or\n    other purposes, in certain modern nations.\n    "@en ;
        <http://www.w3.org/2004/02/skos/core#prefLabel>
                "군"@ko , "County"@en .

<http://rdfs.co/juso/ThirdLevelAdministrativeDivision>
        a       <http://www.w3.org/2002/07/owl#Class> ;
        <http://www.w3.org/2000/01/rdf-schema#isDefinedBy>
                <http://rdfs.co/juso/> ;
        <http://www.w3.org/2000/01/rdf-schema#seeAlso>
                <http://www.geonames.org/ontology#A.ADM3> ;
        <http://www.w3.org/2000/01/rdf-schema#subClassOf>
                <http://rdfs.co/juso/AdministrativeDivision> ;
        <http://purl.org/dc/terms/issued>
                "2015-10-02+09:00"^^<http://www.w3.org/2001/XMLSchema#date> ;
        <http://purl.org/dc/terms/modified>
                "2015-10-02+09:00"^^<http://www.w3.org/2001/XMLSchema#date> ;
        <http://www.w3.org/2003/06/sw-vocab-status/ns#term_status>
                "unstable"@en ;
        <http://www.w3.org/2004/02/skos/core#altLabel>
                "Third Administrative Level"@en , "Third-order Administrative Division"@en ;
        <http://www.w3.org/2004/02/skos/core#definition>
                "\n    A subdivision of a second-level administrative division.\n    "@en ;
        <http://www.w3.org/2004/02/skos/core#prefLabel>
                "Third-level Administrative Division"@en .

<http://rdfs.co/juso/Neighborhood>
        a       <http://www.w3.org/2002/07/owl#Class> ;
        <http://www.w3.org/2000/01/rdf-schema#isDefinedBy>
                <http://rdfs.co/juso/> ;
        <http://www.w3.org/2000/01/rdf-schema#seeAlso>
                <https://en.wikipedia.org/wiki/Neighbourhood> ;
        <http://www.w3.org/2000/01/rdf-schema#subClassOf>
                <http://rdfs.co/juso/AdministrativeDivision> ;
        <http://purl.org/dc/terms/issued>
                "2015-10-02+09:00"^^<http://www.w3.org/2001/XMLSchema#date> ;
        <http://purl.org/dc/terms/modified>
                "2015-10-02+09:00"^^<http://www.w3.org/2001/XMLSchema#date> ;
        <http://www.w3.org/2003/06/sw-vocab-status/ns#term_status>
                "unstable"@en ;
        <http://www.w3.org/2004/02/skos/core#definition>
                "\n    A neighborhood, or neighbourhood, is a geographically localised community\n    within a larger city, town, suburb or rural area.\n    "@en ;
        <http://www.w3.org/2004/02/skos/core#prefLabel>
                "Neighborhood"@en-us , "동"@ko , "Neighbourhood"@en-gb .

<http://rdfs.co/juso/wgs84_lat>
        a       <http://www.w3.org/2002/07/owl#DatatypeProperty> ;
        <http://www.w3.org/2000/01/rdf-schema#domain>
                <http://rdfs.co/juso/Point> ;
        <http://www.w3.org/2000/01/rdf-schema#isDefinedBy>
                <http://rdfs.co/juso/> ;
        <http://www.w3.org/2000/01/rdf-schema#range>
                <http://www.w3.org/2001/XMLSchema#string> ;
        <http://purl.org/dc/terms/issued>
                "2015-11-10+09:00"^^<http://www.w3.org/2001/XMLSchema#date> ;
        <http://purl.org/dc/terms/modified>
                "2015-11-10+09:00"^^<http://www.w3.org/2001/XMLSchema#date> ;
        <http://www.w3.org/2002/07/owl#sameAs>
                <http://www.w3.org/2003/01/geo/wgs84_pos#lat> ;
        <http://www.w3.org/2003/06/sw-vocab-status/ns#term_status>
                "unstable"@en ;
        <http://www.w3.org/2004/02/skos/core#definition>
                "\n    The WGS84 latitude of a point (decimal degrees).\n    "@en ;
        <http://www.w3.org/2004/02/skos/core#prefLabel>
                "latitude (WGS84)"@en , "위도(WGS84)"@ko .

<http://schema.org/postalCode>
        <http://www.w3.org/2002/07/owl#propertyChainAxiom>
                ( <http://rdfs.co/juso/postal_code> <http://www.w3.org/1999/02/22-rdf-syntax-ns#value> ) .

<http://rdfs.co/juso/PoliticalDivisionGroup>
        a       <http://www.w3.org/1999/02/22-rdf-syntax-ns#Bag> ;
        <http://www.w3.org/1999/02/22-rdf-syntax-ns#_1>
                <http://rdfs.co/juso/PoliticalDivision> ;
        <http://www.w3.org/1999/02/22-rdf-syntax-ns#_10>
                <http://rdfs.co/juso/Province> ;
        <http://www.w3.org/1999/02/22-rdf-syntax-ns#_11>
                <http://rdfs.co/juso/County> ;
        <http://www.w3.org/1999/02/22-rdf-syntax-ns#_12>
                <http://rdfs.co/juso/Parish> ;
        <http://www.w3.org/1999/02/22-rdf-syntax-ns#_13>
                <http://rdfs.co/juso/Borough> ;
        <http://www.w3.org/1999/02/22-rdf-syntax-ns#_14>
                <http://rdfs.co/juso/CapitalDistrict> ;
        <http://www.w3.org/1999/02/22-rdf-syntax-ns#_15>
                <http://rdfs.co/juso/City> ;
        <http://www.w3.org/1999/02/22-rdf-syntax-ns#_16>
                <http://rdfs.co/juso/ConsolidatedCityCounty> ;
        <http://www.w3.org/1999/02/22-rdf-syntax-ns#_17>
                <http://rdfs.co/juso/Municipality> ;
        <http://www.w3.org/1999/02/22-rdf-syntax-ns#_18>
                <http://rdfs.co/juso/District> ;
        <http://www.w3.org/1999/02/22-rdf-syntax-ns#_19>
                <http://rdfs.co/juso/Town> ;
        <http://www.w3.org/1999/02/22-rdf-syntax-ns#_2>
                <http://rdfs.co/juso/Country> ;
        <http://www.w3.org/1999/02/22-rdf-syntax-ns#_20>
                <http://rdfs.co/juso/Township> ;
        <http://www.w3.org/1999/02/22-rdf-syntax-ns#_21>
                <http://rdfs.co/juso/Neighborhood> ;
        <http://www.w3.org/1999/02/22-rdf-syntax-ns#_22>
                <http://rdfs.co/juso/Village> ;
        <http://www.w3.org/1999/02/22-rdf-syntax-ns#_23>
                <http://rdfs.co/juso/Hamlet> ;
        <http://www.w3.org/1999/02/22-rdf-syntax-ns#_24>
                <http://rdfs.co/juso/political_division> ;
        <http://www.w3.org/1999/02/22-rdf-syntax-ns#_25>
                <http://rdfs.co/juso/parent> ;
        <http://www.w3.org/1999/02/22-rdf-syntax-ns#_3>
                <http://rdfs.co/juso/AdministrativeDivision> ;
        <http://www.w3.org/1999/02/22-rdf-syntax-ns#_4>
                <http://rdfs.co/juso/FirstLevelAdministrativeDivision> ;
        <http://www.w3.org/1999/02/22-rdf-syntax-ns#_5>
                <http://rdfs.co/juso/SecondLevelAdministrativeDivision> ;
        <http://www.w3.org/1999/02/22-rdf-syntax-ns#_6>
                <http://rdfs.co/juso/ThirdLevelAdministrativeDivision> ;
        <http://www.w3.org/1999/02/22-rdf-syntax-ns#_7>
                <http://rdfs.co/juso/FourthLevelAdministrativeDivision> ;
        <http://www.w3.org/1999/02/22-rdf-syntax-ns#_8>
                <http://rdfs.co/juso/FifthLevelAdministrativeDivision> ;
        <http://www.w3.org/1999/02/22-rdf-syntax-ns#_9>
                <http://rdfs.co/juso/FederatedState> ;
        <http://www.w3.org/2000/01/rdf-schema#comment>
                "\n    These classes and properties are used to describe political and\n    administrative divisions.\n    "@en ;
        <http://www.w3.org/2000/01/rdf-schema#label>
                "Political Division Terms"@en .

<http://rdfs.co/juso/parent>
        a       <http://www.w3.org/2002/07/owl#ObjectProperty> ;
        <http://www.w3.org/2000/01/rdf-schema#domain>
                <http://rdfs.co/juso/Feature> ;
        <http://www.w3.org/2000/01/rdf-schema#isDefinedBy>
                <http://rdfs.co/juso/> ;
        <http://www.w3.org/2000/01/rdf-schema#range>
                <http://rdfs.co/juso/PoliticalDivision> ;
        <http://www.w3.org/2000/01/rdf-schema#subPropertyOf>
                <http://rdfs.co/juso/political_division> , <http://www.geonames.org/ontology#parentFeature> ;
        <http://purl.org/dc/terms/issued>
                "2015-10-02+09:00"^^<http://www.w3.org/2001/XMLSchema#date> ;
        <http://purl.org/dc/terms/modified>
                "2015-10-02+09:00"^^<http://www.w3.org/2001/XMLSchema#date> ;
        <http://www.w3.org/2003/06/sw-vocab-status/ns#term_status>
                "unstable"@en ;
        <http://www.w3.org/2004/02/skos/core#definition>
                "\n    A politial or administrative division that is a direct parent of the\n    current feature.\n    "@en ;
        <http://www.w3.org/2004/02/skos/core#prefLabel>
                "parent politial division"@en .

<http://rdfs.co/juso/PoliticalDivision>
        a       <http://www.w3.org/2002/07/owl#Class> ;
        <http://www.w3.org/2000/01/rdf-schema#isDefinedBy>
                <http://rdfs.co/juso/> ;
        <http://www.w3.org/2000/01/rdf-schema#seeAlso>
                <https://en.wikipedia.org/wiki/Political_division> ;
        <http://www.w3.org/2000/01/rdf-schema#subClassOf>
                <http://rdfs.co/juso/Feature> ;
        <http://purl.org/dc/terms/issued>
                "2015-10-02+09:00"^^<http://www.w3.org/2001/XMLSchema#date> ;
        <http://purl.org/dc/terms/modified>
                "2015-10-02+09:00"^^<http://www.w3.org/2001/XMLSchema#date> ;
        <http://www.w3.org/2002/07/owl#equivalentClass>
                <http://schema.org/AdministrativeArea> ;
        <http://www.w3.org/2003/06/sw-vocab-status/ns#term_status>
                "unstable"@en ;
        <http://www.w3.org/2004/02/skos/core#definition>
                "\n    A political division is a geographic region accepted to be in the\n    jurisdiction of a particular governmental entity. The particular government\n    entity varies as each organizes its operations by further divisions\n    (subdivisions of the state) to further its tasks and satisfy its\n    responsibilities.\n    "@en ;
        <http://www.w3.org/2004/02/skos/core#prefLabel>
                "Political Division"@en .

<http://rdfs.co/juso/historical_address>
        a       <http://www.w3.org/2002/07/owl#ObjectProperty> ;
        <http://www.w3.org/2000/01/rdf-schema#domain>
                <http://rdfs.co/juso/SpatialThing> ;
        <http://www.w3.org/2000/01/rdf-schema#isDefinedBy>
                <http://rdfs.co/juso/> ;
        <http://www.w3.org/2000/01/rdf-schema#range>
                <http://rdfs.co/juso/Address> ;
        <http://purl.org/dc/terms/issued>
                "2015-10-02+09:00"^^<http://www.w3.org/2001/XMLSchema#date> ;
        <http://purl.org/dc/terms/modified>
                "2015-10-02+09:00"^^<http://www.w3.org/2001/XMLSchema#date> ;
        <http://www.w3.org/2003/06/sw-vocab-status/ns#term_status>
                "unstable"@en ;
        <http://www.w3.org/2004/02/skos/core#definition>
                "\n    This property associates anything with one of its historical address.\n    "@en ;
        <http://www.w3.org/2004/02/skos/core#prefLabel>
                "historical address"@en .

<http://rdfs.co/juso/Feature>
        a       <http://www.w3.org/2002/07/owl#Class> ;
        <http://www.w3.org/2000/01/rdf-schema#isDefinedBy>
                <http://rdfs.co/juso/> ;
        <http://www.w3.org/2000/01/rdf-schema#seeAlso>
                <https://en.wikipedia.org/wiki/Geographical_feature> ;
        <http://www.w3.org/2000/01/rdf-schema#subClassOf>
                <http://rdfs.co/juso/SpatialThing> , <http://www.opengis.net/ont/geosparql#Feature> ;
        <http://purl.org/dc/terms/issued>
                "2015-10-02+09:00"^^<http://www.w3.org/2001/XMLSchema#date> ;
        <http://purl.org/dc/terms/modified>
                "2015-10-02+09:00"^^<http://www.w3.org/2001/XMLSchema#date> ;
        <http://www.w3.org/2002/07/owl#disjointWith>
                <http://rdfs.co/juso/Geometry> ;
        <http://www.w3.org/2002/07/owl#equivalentClass>
                <http://www.geonames.org/ontology#Feature> ;
        <http://www.w3.org/2002/07/owl#sameAs>
                <http://geovocab.org/spatial#Feature> ;
        <http://www.w3.org/2003/06/sw-vocab-status/ns#term_status>
                "unstable"@en ;
        <http://www.w3.org/2004/02/skos/core#altLabel>
                "Feature"@en ;
        <http://www.w3.org/2004/02/skos/core#definition>
                "\n    Geographical features are man-made or naturally-created features associated\n    with a location relative to the Earth.\n    "@en ;
        <http://www.w3.org/2004/02/skos/core#prefLabel>
                "Geographical Feature"@en .

<http://rdfs.co/juso/FourthLevelAdministrativeDivision>
        a       <http://www.w3.org/2002/07/owl#Class> ;
        <http://www.w3.org/2000/01/rdf-schema#isDefinedBy>
                <http://rdfs.co/juso/> ;
        <http://www.w3.org/2000/01/rdf-schema#seeAlso>
                <http://www.geonames.org/ontology#A.ADM4> ;
        <http://www.w3.org/2000/01/rdf-schema#subClassOf>
                <http://rdfs.co/juso/AdministrativeDivision> ;
        <http://purl.org/dc/terms/issued>
                "2015-10-02+09:00"^^<http://www.w3.org/2001/XMLSchema#date> ;
        <http://purl.org/dc/terms/modified>
                "2015-10-02+09:00"^^<http://www.w3.org/2001/XMLSchema#date> ;
        <http://www.w3.org/2003/06/sw-vocab-status/ns#term_status>
                "unstable"@en ;
        <http://www.w3.org/2004/02/skos/core#altLabel>
                "Fourth Administrative Level"@en , "Fourth-order Administrative Division"@en ;
        <http://www.w3.org/2004/02/skos/core#definition>
                "\n    A subdivision of a third-level administrative division.\n    "@en ;
        <http://www.w3.org/2004/02/skos/core#prefLabel>
                "Fourth-level Administrative Division"@en .

<http://listinc.kr/id/listinc>
        a       <http://www.w3.org/ns/org#Organization> , <http://xmlns.com/foaf/0.1/Organization> ;
        <http://xmlns.com/foaf/0.1/homepage>
                <http://listinc.kr/> , <http://li-st.com/> ;
        <http://xmlns.com/foaf/0.1/mbox_sha1sum>
                "de068365487dd2da1f2e88f1eaad0217bff79b40" ;
        <http://xmlns.com/foaf/0.1/member>
                <http://listinc.kr/id/member/jgkim> ;
        <http://xmlns.com/foaf/0.1/name>
                "주식회사 리스트"@ko , "LiST Inc."@en .

<http://rdfs.co/juso/second_level_administrative_division>
        a       <http://www.w3.org/2002/07/owl#ObjectProperty> ;
        <http://www.w3.org/2000/01/rdf-schema#domain>
                <http://rdfs.co/juso/Address> ;
        <http://www.w3.org/2000/01/rdf-schema#isDefinedBy>
                <http://rdfs.co/juso/> ;
        <http://www.w3.org/2000/01/rdf-schema#range>
                <http://rdfs.co/juso/SecondLevelAdministrativeDivision> ;
        <http://purl.org/dc/terms/issued>
                "2015-10-02+09:00"^^<http://www.w3.org/2001/XMLSchema#date> ;
        <http://purl.org/dc/terms/modified>
                "2015-10-02+09:00"^^<http://www.w3.org/2001/XMLSchema#date> ;
        <http://www.w3.org/2003/06/sw-vocab-status/ns#term_status>
                "unstable"@en ;
        <http://www.w3.org/2004/02/skos/core#definition>
                "\n    The second-level administrative division (locality) of the address, usually\n    a city.\n    "@en ;
        <http://www.w3.org/2004/02/skos/core#prefLabel>
                "second-level administrative division"@en .

<http://rdfs.co/juso/official_name>
        a       <http://www.w3.org/2002/07/owl#DatatypeProperty> ;
        <http://www.w3.org/2000/01/rdf-schema#domain>
                <http://rdfs.co/juso/SpatialThing> ;
        <http://www.w3.org/2000/01/rdf-schema#isDefinedBy>
                <http://rdfs.co/juso/> ;
        <http://www.w3.org/2000/01/rdf-schema#range>
                <http://www.w3.org/2001/XMLSchema#string> ;
        <http://www.w3.org/2000/01/rdf-schema#seeAlso>
                <http://www.geonames.org/ontology#officialName> ;
        <http://www.w3.org/2000/01/rdf-schema#subPropertyOf>
                <http://rdfs.co/juso/name> ;
        <http://purl.org/dc/terms/issued>
                "2015-12-30+09:00"^^<http://www.w3.org/2001/XMLSchema#date> ;
        <http://purl.org/dc/terms/modified>
                "2015-12-30+09:00"^^<http://www.w3.org/2001/XMLSchema#date> ;
        <http://www.w3.org/2003/06/sw-vocab-status/ns#term_status>
                "unstable"@en ;
        <http://www.w3.org/2004/02/skos/core#definition>
                "\n    This property indicates the official name of the spatial thing.\n    "@en ;
        <http://www.w3.org/2004/02/skos/core#prefLabel>
                "official name"@en , "공식 이름"@ko .

<http://rdfs.co/juso/SpatialThing>
        a       <http://www.w3.org/2002/07/owl#Class> ;
        <http://www.w3.org/2000/01/rdf-schema#isDefinedBy>
                <http://rdfs.co/juso/> ;
        <http://purl.org/dc/terms/issued>
                "2015-10-02+09:00"^^<http://www.w3.org/2001/XMLSchema#date> ;
        <http://purl.org/dc/terms/modified>
                "2015-10-02+09:00"^^<http://www.w3.org/2001/XMLSchema#date> ;
        <http://www.w3.org/2002/07/owl#sameAs>
                <http://www.opengis.net/ont/geosparql#SpatialObject> , <http://www.w3.org/2003/01/geo/wgs84_pos#SpatialThing> ;
        <http://www.w3.org/2003/06/sw-vocab-status/ns#term_status>
                "testing"@en ;
        <http://www.w3.org/2004/02/skos/core#altLabel>
                "Spatial Object"@en ;
        <http://www.w3.org/2004/02/skos/core#definition>
                "\n    Anything that has a spatial representation, i.e. size, shape, or position.\n    e.g. people, places, objects, as well as abstract areas like cubes.\n    "@en ;
        <http://www.w3.org/2004/02/skos/core#prefLabel>
                "Spatial Thing"@en .

<http://rdfs.co/juso/Village>
        a       <http://www.w3.org/2002/07/owl#Class> ;
        <http://www.w3.org/2000/01/rdf-schema#isDefinedBy>
                <http://rdfs.co/juso/> ;
        <http://www.w3.org/2000/01/rdf-schema#seeAlso>
                <https://en.wikipedia.org/wiki/Village> ;
        <http://www.w3.org/2000/01/rdf-schema#subClassOf>
                <http://rdfs.co/juso/AdministrativeDivision> ;
        <http://purl.org/dc/terms/issued>
                "2015-10-02+09:00"^^<http://www.w3.org/2001/XMLSchema#date> ;
        <http://purl.org/dc/terms/modified>
                "2015-10-02+09:00"^^<http://www.w3.org/2001/XMLSchema#date> ;
        <http://www.w3.org/2002/07/owl#sameAs>
                <http://dbpedia.org/ontology/Village> , <http://linkedgeodata.org/ontology/Village> ;
        <http://www.w3.org/2003/06/sw-vocab-status/ns#term_status>
                "unstable"@en ;
        <http://www.w3.org/2004/02/skos/core#definition>
                "\n    A village is a clustered human settlement or community, larger than a\n    hamlet but smaller than a town, with a population ranging from a few\n    hundred to a few thousand.\n    "@en ;
        <http://www.w3.org/2004/02/skos/core#prefLabel>
                "Village"@en , "리"@ko .

<http://rdfs.co/juso/thoroughfare_address>
        a       <http://www.w3.org/2002/07/owl#DatatypeProperty> ;
        <http://www.w3.org/2000/01/rdf-schema#domain>
                <http://rdfs.co/juso/Address> ;
        <http://www.w3.org/2000/01/rdf-schema#isDefinedBy>
                <http://rdfs.co/juso/> ;
        <http://www.w3.org/2000/01/rdf-schema#range>
                <http://www.w3.org/2001/XMLSchema#string> ;
        <http://www.w3.org/2000/01/rdf-schema#seeAlso>
                <https://en.wikipedia.org/wiki/House_numbering> ;
        <http://purl.org/dc/terms/issued>
                "2015-10-02+09:00"^^<http://www.w3.org/2001/XMLSchema#date> ;
        <http://purl.org/dc/terms/modified>
                "2015-10-02+09:00"^^<http://www.w3.org/2001/XMLSchema#date> ;
        <http://www.w3.org/2003/06/sw-vocab-status/ns#term_status>
                "unstable"@en ;
        <http://www.w3.org/2004/02/skos/core#definition>
                "\n    This property is used to describe a unique number given to each building\n    (residential or not) or vacant lot with a mailbox in a street or other\n    thoroughfares.\n    "@en ;
        <http://www.w3.org/2004/02/skos/core#prefLabel>
                "thoroughfare address"@en .

<http://rdfs.co/juso/FederatedState>
        a       <http://www.w3.org/2002/07/owl#Class> ;
        <http://www.w3.org/2000/01/rdf-schema#isDefinedBy>
                <http://rdfs.co/juso/> ;
        <http://www.w3.org/2000/01/rdf-schema#seeAlso>
                <https://en.wikipedia.org/wiki/Federated_state> ;
        <http://www.w3.org/2000/01/rdf-schema#subClassOf>
                <http://linkedgeodata.org/ontology/State> , <http://dbpedia.org/ontology/State> , <http://rdfs.co/juso/AdministrativeDivision> , <http://schema.org/State> ;
        <http://purl.org/dc/terms/issued>
                "2015-10-02+09:00"^^<http://www.w3.org/2001/XMLSchema#date> ;
        <http://purl.org/dc/terms/modified>
                "2015-10-02+09:00"^^<http://www.w3.org/2001/XMLSchema#date> ;
        <http://www.w3.org/2003/06/sw-vocab-status/ns#term_status>
                "unstable"@en ;
        <http://www.w3.org/2004/02/skos/core#altLabel>
                "State"@en , "주"@ko ;
        <http://www.w3.org/2004/02/skos/core#definition>
                "\n    A federated state is a territorial and constitutional community forming\n    part of a federal union (federation) such as the United States and\n    Australia.\n    "@en ;
        <http://www.w3.org/2004/02/skos/core#prefLabel>
                "연방주"@ko , "Federated State"@en .

<http://rdfs.co/juso/Hamlet>
        a       <http://www.w3.org/2002/07/owl#Class> ;
        <http://www.w3.org/2000/01/rdf-schema#isDefinedBy>
                <http://rdfs.co/juso/> ;
        <http://www.w3.org/2000/01/rdf-schema#seeAlso>
                <https://en.wikipedia.org/wiki/Hamlet_(place)> ;
        <http://www.w3.org/2000/01/rdf-schema#subClassOf>
                <http://rdfs.co/juso/AdministrativeDivision> ;
        <http://purl.org/dc/terms/issued>
                "2015-10-02+09:00"^^<http://www.w3.org/2001/XMLSchema#date> ;
        <http://purl.org/dc/terms/modified>
                "2015-10-02+09:00"^^<http://www.w3.org/2001/XMLSchema#date> ;
        <http://www.w3.org/2002/07/owl#sameAs>
                <http://linkedgeodata.org/ontology/Hamlet> ;
        <http://www.w3.org/2003/06/sw-vocab-status/ns#term_status>
                "unstable"@en ;
        <http://www.w3.org/2004/02/skos/core#definition>
                "\n    A hamlet is a type of settlement. The definition of hamlet varies by\n    country. It usually refers to a small settlement, with a small population\n    that is usually under 100, in a rural area, or a component of a larger\n    settlement or municipality. Hamlets are typically unincorporated\n    communities.\n    "@en ;
        <http://www.w3.org/2004/02/skos/core#prefLabel>
                "Hamlet"@en .

<http://rdfs.co/juso/Province>
        a       <http://www.w3.org/2002/07/owl#Class> ;
        <http://www.w3.org/2000/01/rdf-schema#isDefinedBy>
                <http://rdfs.co/juso/> ;
        <http://www.w3.org/2000/01/rdf-schema#seeAlso>
                <https://en.wikipedia.org/wiki/Province> ;
        <http://www.w3.org/2000/01/rdf-schema#subClassOf>
                <http://rdfs.co/juso/AdministrativeDivision> , <http://schema.org/State> ;
        <http://purl.org/dc/terms/issued>
                "2015-10-02+09:00"^^<http://www.w3.org/2001/XMLSchema#date> ;
        <http://purl.org/dc/terms/modified>
                "2015-10-02+09:00"^^<http://www.w3.org/2001/XMLSchema#date> ;
        <http://www.w3.org/2002/07/owl#sameAs>
                <http://dbpedia.org/ontology/Province> ;
        <http://www.w3.org/2003/06/sw-vocab-status/ns#term_status>
                "unstable"@en ;
        <http://www.w3.org/2004/02/skos/core#definition>
                "\n    A province is almost always an administrative division, within a country or\n    state.\n    "@en ;
        <http://www.w3.org/2004/02/skos/core#prefLabel>
                "Province"@en , "도"@ko .

<http://rdfs.co/juso/short_name>
        a       <http://www.w3.org/2002/07/owl#DatatypeProperty> ;
        <http://www.w3.org/2000/01/rdf-schema#domain>
                <http://rdfs.co/juso/SpatialThing> ;
        <http://www.w3.org/2000/01/rdf-schema#isDefinedBy>
                <http://rdfs.co/juso/> ;
        <http://www.w3.org/2000/01/rdf-schema#range>
                <http://www.w3.org/2001/XMLSchema#string> ;
        <http://www.w3.org/2000/01/rdf-schema#seeAlso>
                <http://www.geonames.org/ontology#shortName> ;
        <http://www.w3.org/2000/01/rdf-schema#subPropertyOf>
                <http://rdfs.co/juso/alternate_name> ;
        <http://purl.org/dc/terms/issued>
                "2015-12-30+09:00"^^<http://www.w3.org/2001/XMLSchema#date> ;
        <http://purl.org/dc/terms/modified>
                "2015-12-30+09:00"^^<http://www.w3.org/2001/XMLSchema#date> ;
        <http://www.w3.org/2003/06/sw-vocab-status/ns#term_status>
                "unstable"@en ;
        <http://www.w3.org/2004/02/skos/core#definition>
                "\n    This property indicates the relatively short name of the spatial thing.\n    "@en ;
        <http://www.w3.org/2004/02/skos/core#prefLabel>
                "short name"@en , "짧은 이름"@ko .

<http://schema.org/containedIn>
        <http://www.w3.org/2000/01/rdf-schema#subPropertyOf>
                <http://rdfs.co/juso/within> .

<http://purl.org/dc/terms/Location>
        <http://www.w3.org/2000/01/rdf-schema#subClassOf>
                <http://rdfs.co/juso/SpatialThing> .

<http://rdfs.co/juso/postal_code>
        a       <http://www.w3.org/2002/07/owl#DatatypeProperty> ;
        <http://www.w3.org/2000/01/rdf-schema#domain>
                <http://rdfs.co/juso/Address> ;
        <http://www.w3.org/2000/01/rdf-schema#isDefinedBy>
                <http://rdfs.co/juso/> ;
        <http://www.w3.org/2000/01/rdf-schema#range>
                <http://rdfs.co/juso/PostalCode> ;
        <http://purl.org/dc/terms/issued>
                "2015-10-02+09:00"^^<http://www.w3.org/2001/XMLSchema#date> ;
        <http://purl.org/dc/terms/modified>
                "2015-10-02+09:00"^^<http://www.w3.org/2001/XMLSchema#date> ;
        <http://www.w3.org/2003/06/sw-vocab-status/ns#term_status>
                "unstable"@en ;
        <http://www.w3.org/2004/02/skos/core#definition>
                "\n    This property associates any address with its postal code.\n    "@en ;
        <http://www.w3.org/2004/02/skos/core#prefLabel>
                "postal code"@en .

<http://rdfs.co/juso/locator_address>
        a       <http://www.w3.org/2002/07/owl#DatatypeProperty> ;
        <http://www.w3.org/2000/01/rdf-schema#domain>
                <http://rdfs.co/juso/Address> ;
        <http://www.w3.org/2000/01/rdf-schema#isDefinedBy>
                <http://rdfs.co/juso/> ;
        <http://www.w3.org/2000/01/rdf-schema#range>
                <http://www.w3.org/2001/XMLSchema#string> ;
        <http://purl.org/dc/terms/issued>
                "2015-10-02+09:00"^^<http://www.w3.org/2001/XMLSchema#date> ;
        <http://purl.org/dc/terms/modified>
                "2015-10-02+09:00"^^<http://www.w3.org/2001/XMLSchema#date> ;
        <http://www.w3.org/2003/06/sw-vocab-status/ns#term_status>
                "unstable"@en ;
        <http://www.w3.org/2004/02/skos/core#definition>
                "\n    This property is used to describe a number or a sequence of characters that\n    uniquely identifies the exact locator within the relevant scope(s), that is\n    described by juso:locator.\n    "@en ;
        <http://www.w3.org/2004/02/skos/core#prefLabel>
                "locator address"@en .

<http://jayg.me/>  a  <http://xmlns.com/foaf/0.1/Person> ;
        <http://www.w3.org/2002/07/owl#sameAs>
                <http://listinc.kr/id/member/jgkim> ;
        <http://www.w3.org/ns/org#memberOf>
                <http://listinc.kr/id/listinc> ;
        <http://xmlns.com/foaf/0.1/homepage>
                <http://jayg.org/> ;
        <http://xmlns.com/foaf/0.1/mbox_sha1sum>
                "f03421e94730da58e8943d3a1d2c4c6b02898e14" ;
        <http://xmlns.com/foaf/0.1/name>
                "James G. Kim"@en , "김보람"@ko .

<http://rdfs.co/juso/FirstLevelAdministrativeDivision>
        a       <http://www.w3.org/2002/07/owl#Class> ;
        <http://www.w3.org/2000/01/rdf-schema#isDefinedBy>
                <http://rdfs.co/juso/> ;
        <http://www.w3.org/2000/01/rdf-schema#seeAlso>
                <http://www.geonames.org/ontology#A.ADM1> ;
        <http://www.w3.org/2000/01/rdf-schema#subClassOf>
                <http://rdfs.co/juso/AdministrativeDivision> ;
        <http://purl.org/dc/terms/issued>
                "2015-10-02+09:00"^^<http://www.w3.org/2001/XMLSchema#date> ;
        <http://purl.org/dc/terms/modified>
                "2015-10-02+09:00"^^<http://www.w3.org/2001/XMLSchema#date> ;
        <http://www.w3.org/2003/06/sw-vocab-status/ns#term_status>
                "unstable"@en ;
        <http://www.w3.org/2004/02/skos/core#altLabel>
                "First Administrative Level"@en , "First-order Administrative Division"@en ;
        <http://www.w3.org/2004/02/skos/core#definition>
                "\n    A primary administrative division of a country, such as a state in the\n    United States.\n    "@en ;
        <http://www.w3.org/2004/02/skos/core#prefLabel>
                "First-level Administrative Division"@en .

<http://rdfs.co/juso/address>
        a       <http://www.w3.org/2002/07/owl#ObjectProperty> ;
        <http://www.w3.org/2000/01/rdf-schema#domain>
                <http://rdfs.co/juso/SpatialThing> ;
        <http://www.w3.org/2000/01/rdf-schema#isDefinedBy>
                <http://rdfs.co/juso/> ;
        <http://www.w3.org/2000/01/rdf-schema#range>
                <http://rdfs.co/juso/Address> ;
        <http://www.w3.org/2000/01/rdf-schema#subPropertyOf>
                <http://ontology.eil.utoronto.ca/icontact.owl#address> , <http://www.w3.org/ns/locn#address> ;
        <http://purl.org/dc/terms/issued>
                "2015-10-02+09:00"^^<http://www.w3.org/2001/XMLSchema#date> ;
        <http://purl.org/dc/terms/modified>
                "2015-10-02+09:00"^^<http://www.w3.org/2001/XMLSchema#date> ;
        <http://www.w3.org/2003/06/sw-vocab-status/ns#term_status>
                "unstable"@en ;
        <http://www.w3.org/2004/02/skos/core#definition>
                "\n    This property associates anything with its address.\n    "@en ;
        <http://www.w3.org/2004/02/skos/core#prefLabel>
                "address"@en .

<http://rdfs.co/juso/Parish>
        a       <http://www.w3.org/2002/07/owl#Class> ;
        <http://www.w3.org/2000/01/rdf-schema#isDefinedBy>
                <http://rdfs.co/juso/> ;
        <http://www.w3.org/2000/01/rdf-schema#seeAlso>
                <https://en.wikipedia.org/wiki/Parish_(administrative_division)> ;
        <http://www.w3.org/2000/01/rdf-schema#subClassOf>
                <http://rdfs.co/juso/AdministrativeDivision> ;
        <http://purl.org/dc/terms/issued>
                "2015-10-02+09:00"^^<http://www.w3.org/2001/XMLSchema#date> ;
        <http://purl.org/dc/terms/modified>
                "2015-10-02+09:00"^^<http://www.w3.org/2001/XMLSchema#date> ;
        <http://www.w3.org/2003/06/sw-vocab-status/ns#term_status>
                "unstable"@en ;
        <http://www.w3.org/2004/02/skos/core#altLabel>
                "Civil Parish"@en-gb ;
        <http://www.w3.org/2004/02/skos/core#definition>
                "\n    A parish is an administrative division used by several countries. In parts\n    of the British Isles it is known as a civil parish to distinguish it from\n    the ecclesiastical parish.\n    "@en ;
        <http://www.w3.org/2004/02/skos/core#prefLabel>
                "Parish"@en .

<http://rdfs.co/juso/wgs84_long>
        a       <http://www.w3.org/2002/07/owl#DatatypeProperty> ;
        <http://www.w3.org/2000/01/rdf-schema#domain>
                <http://rdfs.co/juso/Point> ;
        <http://www.w3.org/2000/01/rdf-schema#isDefinedBy>
                <http://rdfs.co/juso/> ;
        <http://www.w3.org/2000/01/rdf-schema#range>
                <http://www.w3.org/2001/XMLSchema#string> ;
        <http://purl.org/dc/terms/issued>
                "2015-11-10+09:00"^^<http://www.w3.org/2001/XMLSchema#date> ;
        <http://purl.org/dc/terms/modified>
                "2015-11-10+09:00"^^<http://www.w3.org/2001/XMLSchema#date> ;
        <http://www.w3.org/2002/07/owl#sameAs>
                <http://www.w3.org/2003/01/geo/wgs84_pos#long> ;
        <http://www.w3.org/2003/06/sw-vocab-status/ns#term_status>
                "unstable"@en ;
        <http://www.w3.org/2004/02/skos/core#definition>
                "\n    The WGS84 longitude of a point (decimal degrees).\n    "@en ;
        <http://www.w3.org/2004/02/skos/core#prefLabel>
                "longitude (WGS84)"@en , "경도(WGS84)"@ko .

<http://rdfs.co/juso/exonym>
        a       <http://www.w3.org/2002/07/owl#DatatypeProperty> ;
        <http://www.w3.org/2000/01/rdf-schema#domain>
                <http://rdfs.co/juso/Feature> ;
        <http://www.w3.org/2000/01/rdf-schema#isDefinedBy>
                <http://rdfs.co/juso/> ;
        <http://www.w3.org/2000/01/rdf-schema#range>
                <http://www.w3.org/2001/XMLSchema#string> ;
        <http://www.w3.org/2000/01/rdf-schema#seeAlso>
                <https://en.wikipedia.org/wiki/Exonym_and_endonym> ;
        <http://www.w3.org/2000/01/rdf-schema#subPropertyOf>
                <http://rdfs.co/juso/name> , <http://www.geonames.org/ontology#alternateName> , <http://www.w3.org/2004/02/skos/core#altLabel> ;
        <http://purl.org/dc/terms/issued>
                "2015-10-02+09:00"^^<http://www.w3.org/2001/XMLSchema#date> ;
        <http://purl.org/dc/terms/modified>
                "2015-10-02+09:00"^^<http://www.w3.org/2001/XMLSchema#date> ;
        <http://www.w3.org/2003/06/sw-vocab-status/ns#term_status>
                "unstable"@en ;
        <http://www.w3.org/2004/02/skos/core#definition>
                "\n    The exonym is an external name for a geographical place: a common name used\n    only outside the place in question, usually for historical reasons.\n    "@en ;
        <http://www.w3.org/2004/02/skos/core#prefLabel>
                "exonym"@en .

<http://rdfs.co/juso/geometry>
        a       <http://www.w3.org/2002/07/owl#ObjectProperty> ;
        <http://www.w3.org/2000/01/rdf-schema#domain>
                <http://rdfs.co/juso/Feature> ;
        <http://www.w3.org/2000/01/rdf-schema#isDefinedBy>
                <http://rdfs.co/juso/> ;
        <http://www.w3.org/2000/01/rdf-schema#range>
                <http://rdfs.co/juso/Geometry> ;
        <http://www.w3.org/2000/01/rdf-schema#subPropertyOf>
                <http://www.w3.org/ns/locn#geometry> , <http://geovocab.org/geometry#geometry> ;
        <http://purl.org/dc/terms/issued>
                "2015-10-02+09:00"^^<http://www.w3.org/2001/XMLSchema#date> ;
        <http://purl.org/dc/terms/modified>
                "2015-10-02+09:00"^^<http://www.w3.org/2001/XMLSchema#date> ;
        <http://www.w3.org/2003/06/sw-vocab-status/ns#term_status>
                "unstable"@en ;
        <http://www.w3.org/2004/02/skos/core#definition>
                "\n    This property associates any feature with the corresponding geometry.\n    "@en ;
        <http://www.w3.org/2004/02/skos/core#prefLabel>
                "geometry"@en .

<http://rdfs.co/juso/Street>
        a       <http://www.w3.org/2002/07/owl#Class> ;
        <http://www.w3.org/2000/01/rdf-schema#isDefinedBy>
                <http://rdfs.co/juso/> ;
        <http://www.w3.org/2000/01/rdf-schema#seeAlso>
                <http://www.geonames.org/ontology#R.ST> , <https://en.wikipedia.org/wiki/Street> ;
        <http://www.w3.org/2000/01/rdf-schema#subClassOf>
                <http://rdfs.co/juso/Thoroughfare> ;
        <http://purl.org/dc/terms/issued>
                "2015-10-02+09:00"^^<http://www.w3.org/2001/XMLSchema#date> ;
        <http://purl.org/dc/terms/modified>
                "2015-10-02+09:00"^^<http://www.w3.org/2001/XMLSchema#date> ;
        <http://www.w3.org/2003/06/sw-vocab-status/ns#term_status>
                "unstable"@en ;
        <http://www.w3.org/2004/02/skos/core#definition>
                "\n    A street is a public thoroughfare (usually paved) in a built environment.\n    Practically all public streets in Western countries and the majority\n    elsewhere (though not in Japan) are given a street or road name or at least\n    a number to identify them and any addresses located along the streets.\n    Alleys in some places do not have names.\n    "@en ;
        <http://www.w3.org/2004/02/skos/core#prefLabel>
                "Street"@en .

<http://rdfs.co/juso/Municipality>
        a       <http://www.w3.org/2002/07/owl#Class> ;
        <http://www.w3.org/2000/01/rdf-schema#isDefinedBy>
                <http://rdfs.co/juso/> ;
        <http://www.w3.org/2000/01/rdf-schema#seeAlso>
                <https://en.wikipedia.org/wiki/Municipality> ;
        <http://www.w3.org/2000/01/rdf-schema#subClassOf>
                <http://rdfs.co/juso/AdministrativeDivision> ;
        <http://purl.org/dc/terms/issued>
                "2015-10-02+09:00"^^<http://www.w3.org/2001/XMLSchema#date> ;
        <http://purl.org/dc/terms/modified>
                "2015-10-02+09:00"^^<http://www.w3.org/2001/XMLSchema#date> ;
        <http://www.w3.org/2002/07/owl#sameAs>
                <http://dbpedia.org/ontology/Municipality> , <http://linkedgeodata.org/ontology/Municipality> ;
        <http://www.w3.org/2003/06/sw-vocab-status/ns#term_status>
                "unstable"@en ;
        <http://www.w3.org/2004/02/skos/core#definition>
                "\n    A municipality is usually an urban administrative division having corporate\n    status and usually powers of self-government or jurisdiction.\n    "@en ;
        <http://www.w3.org/2004/02/skos/core#prefLabel>
                "Municipality"@en .

<http://rdfs.co/juso/0.1.2/rdf>
        <http://purl.org/dc/terms/format>
                [ a       <http://purl.org/dc/terms/MediaType> ;
                  <http://www.w3.org/1999/02/22-rdf-syntax-ns#value>
                          "application/rdf+xml" ;
                  <http://www.w3.org/2000/01/rdf-schema#label>
                          "RDF/XML"@en ;
                  <http://www.w3.org/2000/01/rdf-schema#seeAlso>
                          <http://www.iana.org/assignments/media-types/application/rdf+xml> ;
                  <http://purl.org/dc/dcam/memberOf>
                          <http://purl.org/dc/terms/IMT> ;
                  <http://www.w3.org/2002/07/owl#sameAs>
                          <https://w3id.org/spar/mediatype/application/rdf%2Bxml>
                ] .

<http://rdfs.co/juso/Thoroughfare>
        a       <http://www.w3.org/2002/07/owl#Class> ;
        <http://www.w3.org/2000/01/rdf-schema#isDefinedBy>
                <http://rdfs.co/juso/> ;
        <http://www.w3.org/2000/01/rdf-schema#seeAlso>
                <https://en.wikipedia.org/wiki/Thoroughfare> ;
        <http://www.w3.org/2000/01/rdf-schema#subClassOf>
                <http://rdfs.co/juso/Feature> ;
        <http://purl.org/dc/terms/issued>
                "2015-10-02+09:00"^^<http://www.w3.org/2001/XMLSchema#date> ;
        <http://purl.org/dc/terms/modified>
                "2015-10-02+09:00"^^<http://www.w3.org/2001/XMLSchema#date> ;
        <http://www.w3.org/2003/06/sw-vocab-status/ns#term_status>
                "unstable"@en ;
        <http://www.w3.org/2004/02/skos/core#definition>
                "\n    A passage or way through from one location to another, which is usually\n    used a component of an address. A thoroughfare is not necessarily a road,\n    it might be a waterway or some other feature.\n    "@en ;
        <http://www.w3.org/2004/02/skos/core#prefLabel>
                "Thoroughfare"@en .

<http://rdfs.co/juso/ConsolidatedCityCounty>
        a       <http://www.w3.org/2002/07/owl#Class> ;
        <http://www.w3.org/2000/01/rdf-schema#isDefinedBy>
                <http://rdfs.co/juso/> ;
        <http://www.w3.org/2000/01/rdf-schema#seeAlso>
                <https://en.wikipedia.org/wiki/Consolidated_city-county> ;
        <http://www.w3.org/2000/01/rdf-schema#subClassOf>
                <http://rdfs.co/juso/City> , <http://rdfs.co/juso/County> ;
        <http://purl.org/dc/terms/issued>
                "2015-10-02+09:00"^^<http://www.w3.org/2001/XMLSchema#date> ;
        <http://purl.org/dc/terms/modified>
                "2015-10-02+09:00"^^<http://www.w3.org/2001/XMLSchema#date> ;
        <http://www.w3.org/2003/06/sw-vocab-status/ns#term_status>
                "unstable"@en ;
        <http://www.w3.org/2004/02/skos/core#definition>
                "\n    A consolidated city-county is a city and county that have been merged into\n    one unified jurisdiction. As such it is simultaneously a city, which is a\n    municipal corporation, and a county, which is an administrative division of\n    a state. It has the powers and responsibilities of both types of entities.\n    "@en ;
        <http://www.w3.org/2004/02/skos/core#prefLabel>
                "Consolidated City-county"@en .

<http://rdfs.co/juso/locator>
        a       <http://www.w3.org/2002/07/owl#ObjectProperty> ;
        <http://www.w3.org/2000/01/rdf-schema#domain>
                <http://rdfs.co/juso/Address> ;
        <http://www.w3.org/2000/01/rdf-schema#isDefinedBy>
                <http://rdfs.co/juso/> ;
        <http://www.w3.org/2000/01/rdf-schema#range>
                <http://rdfs.co/juso/Feature> ;
        <http://purl.org/dc/terms/issued>
                "2015-10-02+09:00"^^<http://www.w3.org/2001/XMLSchema#date> ;
        <http://purl.org/dc/terms/modified>
                "2015-10-02+09:00"^^<http://www.w3.org/2001/XMLSchema#date> ;
        <http://www.w3.org/2003/06/sw-vocab-status/ns#term_status>
                "unstable"@en ;
        <http://www.w3.org/2004/02/skos/core#definition>
                "\n    The real world entity identified by the address. The locator could be the\n    property or complex, of the building or part of the building, of it could\n    be a room inside a building.\n    "@en ;
        <http://www.w3.org/2004/02/skos/core#prefLabel>
                "locator"@en .

<http://schema.org/Place>
        <http://www.w3.org/2000/01/rdf-schema#subClassOf>
                <http://rdfs.co/juso/SpatialThing> .

<http://www.geonames.org/ontology#shortName>
        <http://www.w3.org/2000/01/rdf-schema#subPropertyOf>
                <http://rdfs.co/juso/short_name> .

<http://schema.org/PostalAddress>
        <http://www.w3.org/2000/01/rdf-schema#subClassOf>
                <http://rdfs.co/juso/Address> .

<http://schema.org/address>
        <http://www.w3.org/2000/01/rdf-schema#subPropertyOf>
                <http://rdfs.co/juso/address> .

<http://schema.org/GeoCoordinates>
        <http://www.w3.org/2000/01/rdf-schema#subClassOf>
                <http://rdfs.co/juso/Geometry> .

<http://www.w3.org/ns/locn#postCode>
        <http://www.w3.org/2002/07/owl#propertyChainAxiom>
                ( <http://rdfs.co/juso/postal_code> <http://www.w3.org/1999/02/22-rdf-syntax-ns#value> ) .

<http://www.geonames.org/ontology#officialName>
        <http://www.w3.org/2000/01/rdf-schema#subPropertyOf>
                <http://rdfs.co/juso/official_name> .

<http://www.opengis.net/ont/geosparql#hasGeometry>
        <http://www.w3.org/2000/01/rdf-schema#subPropertyOf>
                <http://rdfs.co/juso/geometry> .

<http://schema.org/geo>
        <http://www.w3.org/2000/01/rdf-schema#subPropertyOf>
                <http://rdfs.co/juso/geometry> .

<http://ontology.eil.utoronto.ca/icontact.owl#hasPostalCode>
        <http://www.w3.org/2002/07/owl#propertyChainAxiom>
                ( <http://rdfs.co/juso/postal_code> <http://www.w3.org/1999/02/22-rdf-syntax-ns#value> ) .

<http://ontology.eil.utoronto.ca/icontact.owl#hasStreetNumber>
        <http://www.w3.org/2000/01/rdf-schema#subPropertyOf>
                <http://rdfs.co/juso/thoroughfare_address> .

<http://schema.org/GeoShape>
        <http://www.w3.org/2000/01/rdf-schema#subClassOf>
                <http://rdfs.co/juso/Geometry> .

<http://rdfs.co/juso/0.1.2/ttl>
        <http://purl.org/dc/terms/format>
                [ a       <http://purl.org/dc/terms/MediaType> ;
                  <http://www.w3.org/1999/02/22-rdf-syntax-ns#value>
                          "text/turtle" ;
                  <http://www.w3.org/2000/01/rdf-schema#label>
                          "Turtle"@en ;
                  <http://www.w3.org/2000/01/rdf-schema#seeAlso>
                          <http://www.iana.org/assignments/media-types/text/turtle> ;
                  <http://purl.org/dc/dcam/memberOf>
                          <http://purl.org/dc/terms/IMT> ;
                  <http://www.w3.org/2002/07/owl#sameAs>
                          <https://w3id.org/spar/mediatype/text/turtle>
                ] .

<http://www.geonames.org/ontology#alternateName>
        <http://www.w3.org/2000/01/rdf-schema#subPropertyOf>
                <http://rdfs.co/juso/alternate_name> .

<http://www.w3.org/2006/vcard/ns#postal-code>
        <http://www.w3.org/2002/07/owl#propertyChainAxiom>
                ( <http://rdfs.co/juso/postal_code> <http://www.w3.org/1999/02/22-rdf-syntax-ns#value> ) .

<http://ontology.eil.utoronto.ca/icontact.owl#hasState>
        <http://www.w3.org/2000/01/rdf-schema#subPropertyOf>
                <http://rdfs.co/juso/first_level_administrative_division> .

<http://rdfs.co/juso/0.1.2/html>
        <http://purl.org/dc/terms/format>
                [ a       <http://purl.org/dc/terms/MediaType> ;
                  <http://www.w3.org/1999/02/22-rdf-syntax-ns#value>
                          "text/html" ;
                  <http://www.w3.org/2000/01/rdf-schema#label>
                          "HTML"@en ;
                  <http://www.w3.org/2000/01/rdf-schema#seeAlso>
                          <http://www.iana.org/assignments/media-types/text/html> ;
                  <http://purl.org/dc/dcam/memberOf>
                          <http://purl.org/dc/terms/IMT> ;
                  <http://www.w3.org/2002/07/owl#sameAs>
                          <https://w3id.org/spar/mediatype/text/html>
                ] .

<http://www.geonames.org/ontology#name>
        <http://www.w3.org/2000/01/rdf-schema#subPropertyOf>
                <http://rdfs.co/juso/name> .

<http://www.w3.org/2006/vcard/ns#Address>
        <http://www.w3.org/2000/01/rdf-schema#subClassOf>
                <http://rdfs.co/juso/Address> .
