<http://rdfs.co/juso/post_office_box> <http://www.w3.org/2004/02/skos/core#prefLabel> "post office box"@en .
_:Bef458c30X2D3ae8X2D4a86X2D8152X2D83d608b43cd5 <http://www.w3.org/1999/02/22-rdf-syntax-ns#first> <http://rdfs.co/juso/postal_code> .
<http://rdfs.co/juso/political_division> <http://www.w3.org/2000/01/rdf-schema#isDefinedBy> <http://rdfs.co/juso/> .
<http://rdfs.co/juso/alternate_name> <http://www.w3.org/2004/02/skos/core#definition> "\n    This property indicates the alternate name of the spatial thing.\n    "@en .
<http://rdfs.co/juso/SecondLevelAdministrativeDivision> <http://www.w3.org/2003/06/sw-vocab-status/ns#term_status> "unstable"@en .
<http://rdfs.co/juso/itrf2000_long> <http://www.w3.org/2004/02/skos/core#prefLabel> "longitude (ITRF2000)"@en .
<http://rdfs.co/juso/Geometry> <http://www.w3.org/2002/07/owl#sameAs> <http://www.w3.org/ns/locn#Geometry> .
<http://rdfs.co/juso/first_level_administrative_division> <http://www.w3.org/2000/01/rdf-schema#isDefinedBy> <http://rdfs.co/juso/> .
<http://rdfs.co/juso/City> <http://www.w3.org/2000/01/rdf-schema#seeAlso> <https://en.wikipedia.org/wiki/City> .
<http://rdfs.co/juso/endonym> <http://www.w3.org/2000/01/rdf-schema#isDefinedBy> <http://rdfs.co/juso/> .
<http://rdfs.co/juso/City> <http://www.w3.org/1999/02/22-rdf-syntax-ns#type> <http://www.w3.org/2002/07/owl#Class> .
<http://rdfs.co/juso/itrf2000_lat> <http://www.w3.org/2000/01/rdf-schema#range> <http://www.w3.org/2001/XMLSchema#string> .
<http://rdfs.co/juso/third_level_administrative_division> <http://www.w3.org/2003/06/sw-vocab-status/ns#term_status> "unstable"@en .
<http://rdfs.co/juso/thoroughfare> <http://www.w3.org/2004/02/skos/core#definition> "\n    An address component that represents the name of a passage or way through\n    from one location to another. A thoroughfare is not necessarily a road, it\n    might be a waterway or some other feature.\n    "@en .
<http://rdfs.co/juso/country> <http://www.w3.org/2004/02/skos/core#prefLabel> "country"@en .
<http://rdfs.co/juso/AdministrativeDivision> <http://www.w3.org/2004/02/skos/core#altLabel> "Administrative Unit"@en .
<http://rdfs.co/juso/Township> <http://www.w3.org/2000/01/rdf-schema#seeAlso> <https://en.wikipedia.org/wiki/Township> .
<http://rdfs.co/juso/Country> <http://purl.org/dc/terms/issued> "2015-10-02+09:00"^^<http://www.w3.org/2001/XMLSchema#date> .
<http://rdfs.co/juso/Point> <http://purl.org/dc/terms/issued> "2015-11-10+09:00"^^<http://www.w3.org/2001/XMLSchema#date> .
<http://rdfs.co/juso/fifth_level_administrative_division> <http://www.w3.org/1999/02/22-rdf-syntax-ns#type> <http://www.w3.org/2002/07/owl#ObjectProperty> .
<http://rdfs.co/juso/0.1.2> <http://www.w3.org/1999/02/22-rdf-syntax-ns#type> <http://creativecommons.org/ns#Work> .
<http://rdfs.co/juso/alternate_name> <http://www.w3.org/2000/01/rdf-schema#domain> <http://rdfs.co/juso/SpatialThing> .
<http://rdfs.co/juso/fourth_level_administrative_division> <http://www.w3.org/1999/02/22-rdf-syntax-ns#type> <http://www.w3.org/2002/07/owl#ObjectProperty> .
<http://rdfs.co/juso/within> <http://www.w3.org/2002/07/owl#inverseOf> <http://www.opengis.net/ont/geosparql#sfContains> .
<http://rdfs.co/juso/City> <http://www.w3.org/2002/07/owl#sameAs> <http://dbpedia.org/ontology/City> .
<http://rdfs.co/juso/CoreGroup> <http://www.w3.org/1999/02/22-rdf-syntax-ns#_9> <http://rdfs.co/juso/short_name> .
<http://rdfs.co/juso/post_office_box> <http://www.w3.org/2000/01/rdf-schema#isDefinedBy> <http://rdfs.co/juso/> .
<http://rdfs.co/juso/PostalCode> <http://www.w3.org/2004/02/skos/core#definition> "\n    A postal code is a series of letters and/or digits, sometimes including\n    spaces or punctuation, included in a postal address for the purpose of\n    sorting mail.\n    "@en .
<http://rdfs.co/juso/City> <http://www.w3.org/2004/02/skos/core#definition> "\n    A city is a large and permanent human settlement. Although there is no\n    agreement on how a city is distinguished from a town in general English\n    language meanings, many cities have a particular administrative, legal, or\n    historical status based on local law.\n    "@en .
<http://rdfs.co/juso/Town> <http://www.w3.org/2000/01/rdf-schema#subClassOf> <http://rdfs.co/juso/AdministrativeDivision> .
<http://rdfs.co/juso/name> <http://www.w3.org/2000/01/rdf-schema#domain> <http://rdfs.co/juso/SpatialThing> .
<http://rdfs.co/juso/country> <http://www.w3.org/1999/02/22-rdf-syntax-ns#type> <http://www.w3.org/2002/07/owl#ObjectProperty> .
<http://rdfs.co/juso/Address> <http://www.w3.org/2004/02/skos/core#definition> "\n    An address is a collection of information, presented in a mostly fixed\n    format, used for describing the location of a building, apartment, or other\n    structure or a plot of land, generally using political boundaries and\n    street names as references, along with other identifiers such as house or\n    apartment numbers. Some addresses also contain special codes to aid routing\n    of mail and packages, such as a ZIP code or post code.\n    "@en .
<http://rdfs.co/juso/CapitalDistrict> <http://www.w3.org/2000/01/rdf-schema#isDefinedBy> <http://rdfs.co/juso/> .
<http://rdfs.co/juso/thoroughfare> <http://www.w3.org/2000/01/rdf-schema#isDefinedBy> <http://rdfs.co/juso/> .
<http://linkedgeodata.org/ontology/Place> <http://www.w3.org/2000/01/rdf-schema#subClassOf> <http://rdfs.co/juso/SpatialThing> .
<http://rdfs.co/juso/post_office_box> <http://www.w3.org/2002/07/owl#sameAs> <http://schema.org/postOfficeBoxNumber> .
<http://rdfs.co/juso/FifthLevelAdministrativeDivision> <http://www.w3.org/2004/02/skos/core#altLabel> "Fifth-order Administrative Division"@en .
<http://rdfs.co/juso/District> <http://www.w3.org/2004/02/skos/core#prefLabel> "District"@en .
<http://rdfs.co/juso/Township> <http://www.w3.org/2004/02/skos/core#prefLabel> "면"@ko .
<http://rdfs.co/juso/full_address> <http://www.w3.org/2000/01/rdf-schema#isDefinedBy> <http://rdfs.co/juso/> .
<http://rdfs.co/juso/0.1.2> <http://purl.org/dc/terms/title> "주소 온톨로지"@ko .
_:Bdb835a76X2D643fX2D4ba0X2Db7efX2De49279b0f79d <http://www.w3.org/1999/02/22-rdf-syntax-ns#value> "\n      Fixed the wrong use of rdf:XMLLiteral\n      "@en .
<http://rdfs.co/juso/SecondLevelAdministrativeDivision> <http://www.w3.org/1999/02/22-rdf-syntax-ns#type> <http://www.w3.org/2002/07/owl#Class> .
<http://rdfs.co/juso/AddressGroup> <http://www.w3.org/1999/02/22-rdf-syntax-ns#_12> <http://rdfs.co/juso/locator> .
<http://rdfs.co/juso/name> <http://www.w3.org/2004/02/skos/core#definition> "\n    This property indicates the name of the spatial thing.\n    "@en .
<http://rdfs.co/juso/Township> <http://www.w3.org/2000/01/rdf-schema#subClassOf> <http://rdfs.co/juso/AdministrativeDivision> .
_:B8944e783X2D91c4X2D4ed8X2Db4ecX2Df633899c71c7 <http://www.w3.org/2000/01/rdf-schema#seeAlso> <http://www.iana.org/assignments/media-types/text/turtle> .
<http://rdfs.co/juso/City> <http://www.w3.org/2003/06/sw-vocab-status/ns#term_status> "unstable"@en .
_:Bc87168a3X2D4f47X2D4915X2Dab29X2D178d859ca892 <http://www.w3.org/1999/02/22-rdf-syntax-ns#rest> _:B6fb959b7X2Db6fbX2D4cbeX2D9eabX2Df833eee3b669 .
<http://rdfs.co/juso/County> <http://www.w3.org/2004/02/skos/core#altLabel> "Co."@en-gb .
<http://rdfs.co/juso/ThirdLevelAdministrativeDivision> <http://www.w3.org/1999/02/22-rdf-syntax-ns#type> <http://www.w3.org/2002/07/owl#Class> .
_:B5f94f7eeX2D87b3X2D4b12X2D952fX2D2915101e3e3b <http://www.w3.org/2002/07/owl#sameAs> <https://w3id.org/spar/mediatype/text/html> .
<http://rdfs.co/juso/Neighborhood> <http://www.w3.org/2000/01/rdf-schema#subClassOf> <http://rdfs.co/juso/AdministrativeDivision> .
<http://rdfs.co/juso/wgs84_lat> <http://purl.org/dc/terms/issued> "2015-11-10+09:00"^^<http://www.w3.org/2001/XMLSchema#date> .
<http://rdfs.co/juso/wgs84_lat> <http://www.w3.org/1999/02/22-rdf-syntax-ns#type> <http://www.w3.org/2002/07/owl#DatatypeProperty> .
<http://rdfs.co/juso/AddressGroup> <http://www.w3.org/1999/02/22-rdf-syntax-ns#_2> <http://rdfs.co/juso/country> .
<http://rdfs.co/juso/country> <http://purl.org/dc/terms/modified> "2015-10-02+09:00"^^<http://www.w3.org/2001/XMLSchema#date> .
<http://rdfs.co/juso/PoliticalDivisionGroup> <http://www.w3.org/1999/02/22-rdf-syntax-ns#_8> <http://rdfs.co/juso/FifthLevelAdministrativeDivision> .
<http://rdfs.co/juso/Address> <http://www.w3.org/2000/01/rdf-schema#isDefinedBy> <http://rdfs.co/juso/> .
<http://rdfs.co/juso/County> <http://www.w3.org/2004/02/skos/core#definition> "\n    A county is a geographical region of a country used for administrative or\n    other purposes, in certain modern nations.\n    "@en .
<http://rdfs.co/juso/parent> <http://purl.org/dc/terms/issued> "2015-10-02+09:00"^^<http://www.w3.org/2001/XMLSchema#date> .
<http://rdfs.co/juso/PoliticalDivision> <http://purl.org/dc/terms/issued> "2015-10-02+09:00"^^<http://www.w3.org/2001/XMLSchema#date> .
<http://rdfs.co/juso/historical_address> <http://www.w3.org/2004/02/skos/core#definition> "\n    This property associates anything with one of its historical address.\n    "@en .
<http://rdfs.co/juso/Feature> <http://www.w3.org/2003/06/sw-vocab-status/ns#term_status> "unstable"@en .
<http://rdfs.co/juso/FourthLevelAdministrativeDivision> <http://www.w3.org/2003/06/sw-vocab-status/ns#term_status> "unstable"@en .
<http://listinc.kr/id/listinc> <http://xmlns.com/foaf/0.1/member> <http://listinc.kr/id/member/jgkim> .
<http://rdfs.co/juso/City> <http://www.w3.org/2004/02/skos/core#prefLabel> "시"@ko .
<http://rdfs.co/juso/second_level_administrative_division> <http://www.w3.org/2000/01/rdf-schema#domain> <http://rdfs.co/juso/Address> .
<http://rdfs.co/juso/official_name> <http://www.w3.org/2000/01/rdf-schema#subPropertyOf> <http://rdfs.co/juso/name> .
<http://rdfs.co/juso/PoliticalDivision> <http://www.w3.org/2000/01/rdf-schema#subClassOf> <http://rdfs.co/juso/Feature> .
<http://rdfs.co/juso/Address> <http://www.w3.org/2004/02/skos/core#prefLabel> "Address"@en .
<http://rdfs.co/juso/FourthLevelAdministrativeDivision> <http://www.w3.org/1999/02/22-rdf-syntax-ns#type> <http://www.w3.org/2002/07/owl#Class> .
<http://rdfs.co/juso/within> <http://www.w3.org/2000/01/rdf-schema#range> <http://rdfs.co/juso/SpatialThing> .
<http://rdfs.co/juso/itrf2000_long> <http://www.w3.org/2000/01/rdf-schema#domain> <http://rdfs.co/juso/Point> .
<http://rdfs.co/juso/Feature> <http://www.w3.org/1999/02/22-rdf-syntax-ns#type> <http://www.w3.org/2002/07/owl#Class> .
<http://rdfs.co/juso/SpatialThing> <http://www.w3.org/2004/02/skos/core#prefLabel> "Spatial Thing"@en .
<http://rdfs.co/juso/CoreGroup> <http://www.w3.org/1999/02/22-rdf-syntax-ns#_13> <http://rdfs.co/juso/geometry> .
<http://rdfs.co/juso/Village> <http://purl.org/dc/terms/modified> "2015-10-02+09:00"^^<http://www.w3.org/2001/XMLSchema#date> .
<http://rdfs.co/juso/PoliticalDivisionGroup> <http://www.w3.org/1999/02/22-rdf-syntax-ns#_2> <http://rdfs.co/juso/Country> .
<http://rdfs.co/juso/AddressGroup> <http://www.w3.org/1999/02/22-rdf-syntax-ns#_10> <http://rdfs.co/juso/thoroughfare> .
<http://rdfs.co/juso/thoroughfare_address> <http://www.w3.org/2004/02/skos/core#prefLabel> "thoroughfare address"@en .
<http://rdfs.co/juso/Address> <http://www.w3.org/2004/02/skos/core#altLabel> "Geographical Address"@en .
<http://rdfs.co/juso/itrf2000_long> <http://purl.org/dc/terms/modified> "2015-11-10+09:00"^^<http://www.w3.org/2001/XMLSchema#date> .
<http://rdfs.co/juso/thoroughfare> <http://www.w3.org/2000/01/rdf-schema#range> <http://rdfs.co/juso/Thoroughfare> .
<http://rdfs.co/juso/FederatedState> <http://purl.org/dc/terms/modified> "2015-10-02+09:00"^^<http://www.w3.org/2001/XMLSchema#date> .
_:B73558d1bX2D2f92X2D4be2X2D9f2fX2Dfc6f492ebfa2 <http://www.w3.org/1999/02/22-rdf-syntax-ns#rest> _:Bd0245b9aX2Db64dX2D4c25X2D8d61X2D041d361c5641 .
<http://rdfs.co/juso/0.1.2> <http://purl.org/dc/terms/issued> "2015-10-02+09:00"^^<http://www.w3.org/2001/XMLSchema#date> .
<http://rdfs.co/juso/Address> <http://www.w3.org/2000/01/rdf-schema#seeAlso> <https://en.wikipedia.org/wiki/Address_(geography)> .
<http://rdfs.co/juso/Hamlet> <http://www.w3.org/2000/01/rdf-schema#isDefinedBy> <http://rdfs.co/juso/> .
<http://rdfs.co/juso/Province> <http://www.w3.org/2000/01/rdf-schema#seeAlso> <https://en.wikipedia.org/wiki/Province> .
<http://rdfs.co/juso/itrf2000_long> <http://www.w3.org/2000/01/rdf-schema#isDefinedBy> <http://rdfs.co/juso/> .
<http://rdfs.co/juso/name> <http://purl.org/dc/terms/issued> "2015-10-02+09:00"^^<http://www.w3.org/2001/XMLSchema#date> .
<http://rdfs.co/juso/PoliticalDivisionGroup> <http://www.w3.org/1999/02/22-rdf-syntax-ns#type> <http://www.w3.org/1999/02/22-rdf-syntax-ns#Bag> .
<http://rdfs.co/juso/0.1.2> <http://www.w3.org/1999/02/22-rdf-syntax-ns#type> <http://www.w3.org/ns/adms#SemanticAsset> .
<http://rdfs.co/juso/itrf2000_lat> <http://www.w3.org/2004/02/skos/core#prefLabel> "위도(ITRF2000)"@ko .
_:B72d2cd9fX2D75e4X2D414bX2D94ceX2Dec81117dce46 <http://www.w3.org/2000/01/rdf-schema#seeAlso> <http://www.iana.org/assignments/media-types/application/rdf+xml> .
<http://rdfs.co/juso/fifth_level_administrative_division> <http://purl.org/dc/terms/modified> "2015-10-02+09:00"^^<http://www.w3.org/2001/XMLSchema#date> .
<http://rdfs.co/juso/PoliticalDivisionGroup> <http://www.w3.org/2000/01/rdf-schema#label> "Political Division Terms"@en .
<http://rdfs.co/juso/FifthLevelAdministrativeDivision> <http://www.w3.org/2000/01/rdf-schema#subClassOf> <http://rdfs.co/juso/AdministrativeDivision> .
<http://rdfs.co/juso/ThirdLevelAdministrativeDivision> <http://www.w3.org/2003/06/sw-vocab-status/ns#term_status> "unstable"@en .
<http://rdfs.co/juso/short_name> <http://www.w3.org/2000/01/rdf-schema#isDefinedBy> <http://rdfs.co/juso/> .
<http://rdfs.co/juso/fourth_level_administrative_division> <http://purl.org/dc/terms/modified> "2015-10-02+09:00"^^<http://www.w3.org/2001/XMLSchema#date> .
<http://rdfs.co/juso/District> <http://purl.org/dc/terms/modified> "2015-10-02+09:00"^^<http://www.w3.org/2001/XMLSchema#date> .
_:Bef458c30X2D3ae8X2D4a86X2D8152X2D83d608b43cd5 <http://www.w3.org/1999/02/22-rdf-syntax-ns#rest> _:B85974e57X2D7cdfX2D4960X2Da14cX2D01aad0844ec3 .
<http://schema.org/containedIn> <http://www.w3.org/2000/01/rdf-schema#subPropertyOf> <http://rdfs.co/juso/within> .
<http://rdfs.co/juso/AddressGroup> <http://www.w3.org/1999/02/22-rdf-syntax-ns#_6> <http://rdfs.co/juso/fourth_level_administrative_division> .
<http://purl.org/dc/terms/Location> <http://www.w3.org/2000/01/rdf-schema#subClassOf> <http://rdfs.co/juso/SpatialThing> .
<http://rdfs.co/juso/Province> <http://purl.org/dc/terms/modified> "2015-10-02+09:00"^^<http://www.w3.org/2001/XMLSchema#date> .
<http://rdfs.co/juso/postal_code> <http://www.w3.org/2000/01/rdf-schema#isDefinedBy> <http://rdfs.co/juso/> .
<http://rdfs.co/juso/locator_address> <http://www.w3.org/2000/01/rdf-schema#domain> <http://rdfs.co/juso/Address> .
<http://rdfs.co/juso/postal_code> <http://www.w3.org/2004/02/skos/core#prefLabel> "postal code"@en .
<http://rdfs.co/juso/wgs84_lat> <http://www.w3.org/2002/07/owl#sameAs> <http://www.w3.org/2003/01/geo/wgs84_pos#lat> .
<http://rdfs.co/juso/full_address> <http://www.w3.org/2000/01/rdf-schema#range> <http://www.w3.org/2001/XMLSchema#string> .
<http://jayg.me/> <http://xmlns.com/foaf/0.1/homepage> <http://jayg.org/> .
<http://rdfs.co/juso/0.1.2> <http://www.w3.org/2002/07/owl#versionInfo> "0.1.2" .
<http://rdfs.co/juso/PoliticalDivisionGroup> <http://www.w3.org/1999/02/22-rdf-syntax-ns#_11> <http://rdfs.co/juso/County> .
<http://rdfs.co/juso/SpatialThing> <http://www.w3.org/2003/06/sw-vocab-status/ns#term_status> "testing"@en .
<http://rdfs.co/juso/SecondLevelAdministrativeDivision> <http://purl.org/dc/terms/issued> "2015-10-02+09:00"^^<http://www.w3.org/2001/XMLSchema#date> .
<http://rdfs.co/juso/AddressGroup> <http://www.w3.org/1999/02/22-rdf-syntax-ns#_4> <http://rdfs.co/juso/second_level_administrative_division> .
<http://rdfs.co/juso/FirstLevelAdministrativeDivision> <http://www.w3.org/2000/01/rdf-schema#seeAlso> <http://www.geonames.org/ontology#A.ADM1> .
<http://rdfs.co/juso/FederatedState> <http://www.w3.org/2000/01/rdf-schema#subClassOf> <http://linkedgeodata.org/ontology/State> .
<http://rdfs.co/juso/CoreGroup> <http://www.w3.org/1999/02/22-rdf-syntax-ns#type> <http://www.w3.org/1999/02/22-rdf-syntax-ns#Bag> .
<http://rdfs.co/juso/address> <http://purl.org/dc/terms/modified> "2015-10-02+09:00"^^<http://www.w3.org/2001/XMLSchema#date> .
<http://rdfs.co/juso/third_level_administrative_division> <http://purl.org/dc/terms/issued> "2015-10-02+09:00"^^<http://www.w3.org/2001/XMLSchema#date> .
<http://rdfs.co/juso/PoliticalDivisionGroup> <http://www.w3.org/1999/02/22-rdf-syntax-ns#_17> <http://rdfs.co/juso/Municipality> .
<http://rdfs.co/juso/PostalCode> <http://www.w3.org/2004/02/skos/core#altLabel> "ZIP Code"@en .
<http://rdfs.co/juso/within> <http://www.w3.org/2002/07/owl#sameAs> <http://www.opengis.net/ont/geosparql#sfWithin> .
<http://rdfs.co/juso/official_name> <http://www.w3.org/2004/02/skos/core#prefLabel> "official name"@en .
<http://rdfs.co/juso/AddressGroup> <http://www.w3.org/1999/02/22-rdf-syntax-ns#_7> <http://rdfs.co/juso/fifth_level_administrative_division> .
<http://rdfs.co/juso/Parish> <http://www.w3.org/2000/01/rdf-schema#isDefinedBy> <http://rdfs.co/juso/> .
<http://rdfs.co/juso/Country> <http://www.w3.org/2003/06/sw-vocab-status/ns#term_status> "unstable"@en .
<http://rdfs.co/juso/0.1.2> <http://purl.org/dc/terms/title> "Juso Ontology"@en .
<http://rdfs.co/juso/Town> <http://www.w3.org/2004/02/skos/core#prefLabel> "Town"@en .
<http://rdfs.co/juso/Country> <http://www.w3.org/1999/02/22-rdf-syntax-ns#type> <http://www.w3.org/2002/07/owl#Class> .
<http://rdfs.co/juso/CapitalDistrict> <http://www.w3.org/2004/02/skos/core#prefLabel> "Capital District"@en .
<http://rdfs.co/juso/wgs84_long> <http://purl.org/dc/terms/issued> "2015-11-10+09:00"^^<http://www.w3.org/2001/XMLSchema#date> .
<http://rdfs.co/juso/CoreGroup> <http://www.w3.org/1999/02/22-rdf-syntax-ns#_5> <http://rdfs.co/juso/Address> .
<http://rdfs.co/juso/official_name> <http://www.w3.org/1999/02/22-rdf-syntax-ns#type> <http://www.w3.org/2002/07/owl#DatatypeProperty> .
<http://rdfs.co/juso/SecondLevelAdministrativeDivision> <http://www.w3.org/2004/02/skos/core#altLabel> "Second-order Administrative Division"@en .
<http://rdfs.co/juso/0.1.2> <http://creativecommons.org/ns#license> <http://creativecommons.org/licenses/by/4.0/> .
<http://rdfs.co/juso/exonym> <http://purl.org/dc/terms/modified> "2015-10-02+09:00"^^<http://www.w3.org/2001/XMLSchema#date> .
<http://rdfs.co/juso/wgs84_long> <http://www.w3.org/1999/02/22-rdf-syntax-ns#type> <http://www.w3.org/2002/07/owl#DatatypeProperty> .
<http://rdfs.co/juso/FirstLevelAdministrativeDivision> <http://www.w3.org/2004/02/skos/core#definition> "\n    A primary administrative division of a country, such as a state in the\n    United States.\n    "@en .
<http://rdfs.co/juso/City> <http://purl.org/dc/terms/issued> "2015-10-02+09:00"^^<http://www.w3.org/2001/XMLSchema#date> .
<http://rdfs.co/juso/geometry> <http://www.w3.org/2004/02/skos/core#definition> "\n    This property associates any feature with the corresponding geometry.\n    "@en .
<http://rdfs.co/juso/itrf2000_lat> <http://www.w3.org/2000/01/rdf-schema#isDefinedBy> <http://rdfs.co/juso/> .
<http://rdfs.co/juso/thoroughfare_address> <http://www.w3.org/1999/02/22-rdf-syntax-ns#type> <http://www.w3.org/2002/07/owl#DatatypeProperty> .
<http://rdfs.co/juso/endonym> <http://www.w3.org/2000/01/rdf-schema#range> <http://www.w3.org/2001/XMLSchema#string> .
<http://rdfs.co/juso/AddressGroup> <http://www.w3.org/1999/02/22-rdf-syntax-ns#_11> <http://rdfs.co/juso/thoroughfare_address> .
<http://rdfs.co/juso/post_office_box> <http://www.w3.org/2000/01/rdf-schema#range> <http://www.w3.org/2001/XMLSchema#string> .
<http://rdfs.co/juso/Street> <http://www.w3.org/2004/02/skos/core#definition> "\n    A street is a public thoroughfare (usually paved) in a built environment.\n    Practically all public streets in Western countries and the majority\n    elsewhere (though not in Japan) are given a street or road name or at least\n    a number to identify them and any addresses located along the streets.\n    Alleys in some places do not have names.\n    "@en .
<http://rdfs.co/juso/alternate_name> <http://www.w3.org/2004/02/skos/core#prefLabel> "대체 이름"@ko .
<http://rdfs.co/juso/PoliticalDivisionGroup> <http://www.w3.org/1999/02/22-rdf-syntax-ns#_15> <http://rdfs.co/juso/City> .
<http://rdfs.co/juso/AddressGroup> <http://www.w3.org/2000/01/rdf-schema#comment> "\n    These classes and properties are used to describe addresses.\n    "@en .
<http://rdfs.co/juso/itrf2000_lat> <http://purl.org/dc/terms/modified> "2015-11-10+09:00"^^<http://www.w3.org/2001/XMLSchema#date> .
<http://rdfs.co/juso/exonym> <http://www.w3.org/2000/01/rdf-schema#seeAlso> <https://en.wikipedia.org/wiki/Exonym_and_endonym> .
<http://rdfs.co/juso/Point> <http://www.w3.org/2000/01/rdf-schema#seeAlso> <https://en.wikipedia.org/wiki/Point_(geometry)> .
<http://rdfs.co/juso/Geometry> <http://www.w3.org/2002/07/owl#disjointWith> <http://rdfs.co/juso/Feature> .
<http://rdfs.co/juso/SecondLevelAdministrativeDivision> <http://www.w3.org/2004/02/skos/core#altLabel> "Second Administrative Level"@en .
<http://rdfs.co/juso/CoreGroup> <http://www.w3.org/1999/02/22-rdf-syntax-ns#_15> <http://rdfs.co/juso/historical_address> .
<http://rdfs.co/juso/FifthLevelAdministrativeDivision> <http://www.w3.org/2004/02/skos/core#prefLabel> "Fifth-level Administrative Division"@en .
_:B72d2cd9fX2D75e4X2D414bX2D94ceX2Dec81117dce46 <http://www.w3.org/2002/07/owl#sameAs> <https://w3id.org/spar/mediatype/application/rdf%2Bxml> .
<http://rdfs.co/juso/itrf2000_lat> <http://www.w3.org/2000/01/rdf-schema#domain> <http://rdfs.co/juso/Point> .
<http://rdfs.co/juso/City> <http://www.w3.org/2000/01/rdf-schema#subClassOf> <http://schema.org/City> .
<http://rdfs.co/juso/parent> <http://www.w3.org/2003/06/sw-vocab-status/ns#term_status> "unstable"@en .
<http://rdfs.co/juso/thoroughfare_address> <http://www.w3.org/2000/01/rdf-schema#domain> <http://rdfs.co/juso/Address> .
<http://rdfs.co/juso/PoliticalDivision> <http://www.w3.org/2003/06/sw-vocab-status/ns#term_status> "unstable"@en .
<http://rdfs.co/juso/historical_address> <http://www.w3.org/2000/01/rdf-schema#isDefinedBy> <http://rdfs.co/juso/> .
_:Bd0245b9aX2Db64dX2D4c25X2D8d61X2D041d361c5641 <http://www.w3.org/1999/02/22-rdf-syntax-ns#first> <http://www.w3.org/1999/02/22-rdf-syntax-ns#value> .
<http://rdfs.co/juso/District> <http://www.w3.org/2000/01/rdf-schema#seeAlso> <https://en.wikipedia.org/wiki/District> .
<http://rdfs.co/juso/wgs84_lat> <http://www.w3.org/2004/02/skos/core#definition> "\n    The WGS84 latitude of a point (decimal degrees).\n    "@en .
<http://rdfs.co/juso/ThirdLevelAdministrativeDivision> <http://www.w3.org/2004/02/skos/core#altLabel> "Third Administrative Level"@en .
<http://rdfs.co/juso/Feature> <http://purl.org/dc/terms/issued> "2015-10-02+09:00"^^<http://www.w3.org/2001/XMLSchema#date> .
<http://rdfs.co/juso/FourthLevelAdministrativeDivision> <http://purl.org/dc/terms/issued> "2015-10-02+09:00"^^<http://www.w3.org/2001/XMLSchema#date> .
<http://rdfs.co/juso/0.1.2> <http://purl.org/dc/terms/publisher> <http://listinc.kr/id/listinc> .
<http://rdfs.co/juso/County> <http://www.w3.org/2004/02/skos/core#prefLabel> "군"@ko .
<http://rdfs.co/juso/0.1.2> <http://purl.org/dc/terms/identifier> "http://rdfs.co/juso/0.1.2" .
<http://rdfs.co/juso/0.1.2/ttl> <http://purl.org/dc/terms/format> _:B8944e783X2D91c4X2D4ed8X2Db4ecX2Df633899c71c7 .
_:Bd0245b9aX2Db64dX2D4c25X2D8d61X2D041d361c5641 <http://www.w3.org/1999/02/22-rdf-syntax-ns#rest> <http://www.w3.org/1999/02/22-rdf-syntax-ns#nil> .
<http://rdfs.co/juso/CoreGroup> <http://www.w3.org/1999/02/22-rdf-syntax-ns#_10> <http://rdfs.co/juso/within> .
<http://rdfs.co/juso/Geometry> <http://www.w3.org/2004/02/skos/core#definition> "\n    Geometry provides \"the means for the quantitative description, by means of\n    coordinates and mathematical functions, of the spatial characteristics of\n    features, including dimension, position, size, shape, and orientation\", as\n    defined in ISO 19107.\n    "@en .
<http://listinc.kr/id/listinc> <http://xmlns.com/foaf/0.1/homepage> <http://listinc.kr/> .
<http://rdfs.co/juso/Geometry> <http://www.w3.org/2000/01/rdf-schema#seeAlso> <https://en.wikipedia.org/wiki/Geometry> .
<http://rdfs.co/juso/SpatialThing> <http://purl.org/dc/terms/modified> "2015-10-02+09:00"^^<http://www.w3.org/2001/XMLSchema#date> .
<http://rdfs.co/juso/alternate_name> <http://purl.org/dc/terms/issued> "2015-12-30+09:00"^^<http://www.w3.org/2001/XMLSchema#date> .
<http://rdfs.co/juso/Municipality> <http://www.w3.org/2002/07/owl#sameAs> <http://dbpedia.org/ontology/Municipality> .
<http://rdfs.co/juso/name> <http://www.w3.org/2000/01/rdf-schema#subPropertyOf> <http://schema.org/name> .
<http://rdfs.co/juso/PostalCode> <http://www.w3.org/2004/02/skos/core#altLabel> "PIN Code"@en .
<http://rdfs.co/juso/Thoroughfare> <http://www.w3.org/2000/01/rdf-schema#isDefinedBy> <http://rdfs.co/juso/> .
<http://rdfs.co/juso/short_name> <http://www.w3.org/2000/01/rdf-schema#range> <http://www.w3.org/2001/XMLSchema#string> .
<http://rdfs.co/juso/FifthLevelAdministrativeDivision> <http://www.w3.org/2004/02/skos/core#definition> "\n    A subdivision of a fourth-level administrative division.\n    "@en .
<http://rdfs.co/juso/itrf2000_long> <http://www.w3.org/2000/01/rdf-schema#range> <http://www.w3.org/2001/XMLSchema#string> .
<http://rdfs.co/juso/PoliticalDivisionGroup> <http://www.w3.org/1999/02/22-rdf-syntax-ns#_16> <http://rdfs.co/juso/ConsolidatedCityCounty> .
<http://rdfs.co/juso/FirstLevelAdministrativeDivision> <http://purl.org/dc/terms/modified> "2015-10-02+09:00"^^<http://www.w3.org/2001/XMLSchema#date> .
<http://rdfs.co/juso/FederatedState> <http://www.w3.org/2000/01/rdf-schema#seeAlso> <https://en.wikipedia.org/wiki/Federated_state> .
<http://rdfs.co/juso/Municipality> <http://www.w3.org/2000/01/rdf-schema#subClassOf> <http://rdfs.co/juso/AdministrativeDivision> .
<http://rdfs.co/juso/CoreGroup> <http://www.w3.org/2000/01/rdf-schema#label> "Core Terms"@en .
<http://rdfs.co/juso/alternate_name> <http://www.w3.org/2000/01/rdf-schema#seeAlso> <http://www.geonames.org/ontology#alternateName> .
<http://rdfs.co/juso/political_division> <http://www.w3.org/2000/01/rdf-schema#domain> <http://rdfs.co/juso/Feature> .
<http://rdfs.co/juso/ConsolidatedCityCounty> <http://www.w3.org/2000/01/rdf-schema#isDefinedBy> <http://rdfs.co/juso/> .
<http://rdfs.co/juso/locator> <http://www.w3.org/2000/01/rdf-schema#domain> <http://rdfs.co/juso/Address> .
<http://rdfs.co/juso/Parish> <http://www.w3.org/2004/02/skos/core#prefLabel> "Parish"@en .
<http://rdfs.co/juso/Township> <http://www.w3.org/2004/02/skos/core#prefLabel> "Township"@en .
<http://rdfs.co/juso/ConsolidatedCityCounty> <http://www.w3.org/2004/02/skos/core#prefLabel> "Consolidated City-county"@en .
<http://rdfs.co/juso/endonym> <http://www.w3.org/2000/01/rdf-schema#domain> <http://rdfs.co/juso/Feature> .
<http://rdfs.co/juso/Country> <http://www.w3.org/2002/07/owl#sameAs> <http://schema.org/Country> .
<http://rdfs.co/juso/fourth_level_administrative_division> <http://www.w3.org/2000/01/rdf-schema#range> <http://rdfs.co/juso/FourthLevelAdministrativeDivision> .
<http://rdfs.co/juso/alternate_name> <http://www.w3.org/2003/06/sw-vocab-status/ns#term_status> "unstable"@en .
<http://rdfs.co/juso/Street> <http://www.w3.org/2000/01/rdf-schema#seeAlso> <http://www.geonames.org/ontology#R.ST> .
<http://rdfs.co/juso/locator_address> <http://www.w3.org/1999/02/22-rdf-syntax-ns#type> <http://www.w3.org/2002/07/owl#DatatypeProperty> .
_:B7af76555X2D95fbX2D4024X2Da653X2D1ecbadf9e9c2 <http://www.w3.org/1999/02/22-rdf-syntax-ns#value> "\n      Added juso:Point, juso:wgs84_lat, juso:wgs84_long,\n      juso:itrf2000_lat, and juso:itrf2000_long\n      "@en .
<http://rdfs.co/juso/ThirdLevelAdministrativeDivision> <http://purl.org/dc/terms/issued> "2015-10-02+09:00"^^<http://www.w3.org/2001/XMLSchema#date> .
<http://rdfs.co/juso/Town> <http://www.w3.org/2002/07/owl#sameAs> <http://dbpedia.org/ontology/Town> .
<http://rdfs.co/juso/Feature> <http://www.w3.org/2004/02/skos/core#definition> "\n    Geographical features are man-made or naturally-created features associated\n    with a location relative to the Earth.\n    "@en .
<http://schema.org/Place> <http://www.w3.org/2000/01/rdf-schema#subClassOf> <http://rdfs.co/juso/SpatialThing> .
<http://rdfs.co/juso/County> <http://www.w3.org/2000/01/rdf-schema#isDefinedBy> <http://rdfs.co/juso/> .
<http://rdfs.co/juso/Street> <http://purl.org/dc/terms/modified> "2015-10-02+09:00"^^<http://www.w3.org/2001/XMLSchema#date> .
<http://rdfs.co/juso/PoliticalDivision> <http://www.w3.org/1999/02/22-rdf-syntax-ns#type> <http://www.w3.org/2002/07/owl#Class> .
<http://rdfs.co/juso/address> <http://www.w3.org/1999/02/22-rdf-syntax-ns#type> <http://www.w3.org/2002/07/owl#ObjectProperty> .
<http://rdfs.co/juso/PoliticalDivisionGroup> <http://www.w3.org/1999/02/22-rdf-syntax-ns#_22> <http://rdfs.co/juso/Village> .
<http://rdfs.co/juso/Country> <http://www.w3.org/2004/02/skos/core#prefLabel> "国"@ja .
<http://rdfs.co/juso/FifthLevelAdministrativeDivision> <http://purl.org/dc/terms/issued> "2015-10-02+09:00"^^<http://www.w3.org/2001/XMLSchema#date> .
<http://rdfs.co/juso/parent> <http://www.w3.org/2000/01/rdf-schema#range> <http://rdfs.co/juso/PoliticalDivision> .
<http://rdfs.co/juso/Street> <http://www.w3.org/2000/01/rdf-schema#isDefinedBy> <http://rdfs.co/juso/> .
<http://rdfs.co/juso/PoliticalDivisionGroup> <http://www.w3.org/2000/01/rdf-schema#comment> "\n    These classes and properties are used to describe political and\n    administrative divisions.\n    "@en .
<http://rdfs.co/juso/within> <http://www.w3.org/2002/07/owl#inverseOf> <http://geovocab.org/spatial#Pi> .
<http://rdfs.co/juso/PostalCode> <http://www.w3.org/2004/02/skos/core#altLabel> "Post Code"@en .
<http://rdfs.co/juso/wgs84_long> <http://www.w3.org/2002/07/owl#sameAs> <http://www.w3.org/2003/01/geo/wgs84_pos#long> .
<http://rdfs.co/juso/Feature> <http://www.w3.org/2004/02/skos/core#prefLabel> "Geographical Feature"@en .
_:B17925ab7X2D4341X2D48e5X2D86bfX2Dfe59340945bd <http://www.w3.org/1999/02/22-rdf-syntax-ns#first> <http://rdfs.co/juso/postal_code> .
<http://rdfs.co/juso/AdministrativeDivision> <http://www.w3.org/2003/06/sw-vocab-status/ns#term_status> "unstable"@en .
<http://rdfs.co/juso/Country> <http://www.w3.org/2004/02/skos/core#altLabel> "국가"@ko .
<http://rdfs.co/juso/County> <http://purl.org/dc/terms/modified> "2015-10-02+09:00"^^<http://www.w3.org/2001/XMLSchema#date> .
<http://rdfs.co/juso/Municipality> <http://www.w3.org/1999/02/22-rdf-syntax-ns#type> <http://www.w3.org/2002/07/owl#Class> .
<http://rdfs.co/juso/locator_address> <http://purl.org/dc/terms/issued> "2015-10-02+09:00"^^<http://www.w3.org/2001/XMLSchema#date> .
<http://rdfs.co/juso/PoliticalDivisionGroup> <http://www.w3.org/1999/02/22-rdf-syntax-ns#_1> <http://rdfs.co/juso/PoliticalDivision> .
<http://rdfs.co/juso/Country> <http://www.w3.org/2004/02/skos/core#altLabel> "国家"@ja .
<http://rdfs.co/juso/official_name> <http://www.w3.org/2004/02/skos/core#definition> "\n    This property indicates the official name of the spatial thing.\n    "@en .
<http://rdfs.co/juso/within> <http://www.w3.org/2000/01/rdf-schema#subPropertyOf> <http://www.w3.org/2003/01/geo/wgs84_pos#location> .
<http://rdfs.co/juso/fifth_level_administrative_division> <http://www.w3.org/2004/02/skos/core#prefLabel> "fifth-level administrative division"@en .
<http://rdfs.co/juso/third_level_administrative_division> <http://www.w3.org/2000/01/rdf-schema#domain> <http://rdfs.co/juso/Address> .
<http://rdfs.co/juso/short_name> <http://www.w3.org/2004/02/skos/core#prefLabel> "short name"@en .
<http://rdfs.co/juso/ConsolidatedCityCounty> <http://purl.org/dc/terms/modified> "2015-10-02+09:00"^^<http://www.w3.org/2001/XMLSchema#date> .
<http://rdfs.co/juso/PoliticalDivisionGroup> <http://www.w3.org/1999/02/22-rdf-syntax-ns#_12> <http://rdfs.co/juso/Parish> .
<http://rdfs.co/juso/FirstLevelAdministrativeDivision> <http://www.w3.org/2000/01/rdf-schema#isDefinedBy> <http://rdfs.co/juso/> .
<http://rdfs.co/juso/official_name> <http://www.w3.org/2000/01/rdf-schema#domain> <http://rdfs.co/juso/SpatialThing> .
<http://rdfs.co/juso/0.1.2/rdf> <http://purl.org/dc/terms/format> _:B72d2cd9fX2D75e4X2D414bX2D94ceX2Dec81117dce46 .
<http://rdfs.co/juso/SpatialThing> <http://www.w3.org/2000/01/rdf-schema#isDefinedBy> <http://rdfs.co/juso/> .
<http://rdfs.co/juso/County> <http://www.w3.org/2004/02/skos/core#prefLabel> "County"@en .
<http://rdfs.co/juso/Thoroughfare> <http://purl.org/dc/terms/modified> "2015-10-02+09:00"^^<http://www.w3.org/2001/XMLSchema#date> .
<http://rdfs.co/juso/Country> <http://www.w3.org/2004/02/skos/core#definition> "\n    A country is a region that is identified as a distinct entity in political\n    geography. A country may be an independent sovereign state or one that is\n    occupied by another state, as a non-sovereign or formerly sovereign\n    political division, or a geographic region associated with sets of\n    previously independent or differently associated people with distinct\n    political characteristics.\n    "@en .
<http://www.w3.org/2006/vcard/ns#postal-code> <http://www.w3.org/2002/07/owl#propertyChainAxiom> _:B73558d1bX2D2f92X2D4be2X2D9f2fX2Dfc6f492ebfa2 .
<http://jayg.me/> <http://xmlns.com/foaf/0.1/name> "James G. Kim"@en .
<http://rdfs.co/juso/short_name> <http://purl.org/dc/terms/modified> "2015-12-30+09:00"^^<http://www.w3.org/2001/XMLSchema#date> .
<http://rdfs.co/juso/Municipality> <http://www.w3.org/2002/07/owl#sameAs> <http://linkedgeodata.org/ontology/Municipality> .
<http://rdfs.co/juso/Neighborhood> <http://purl.org/dc/terms/issued> "2015-10-02+09:00"^^<http://www.w3.org/2001/XMLSchema#date> .
<http://rdfs.co/juso/AdministrativeDivision> <http://www.w3.org/1999/02/22-rdf-syntax-ns#type> <http://www.w3.org/2002/07/owl#Class> .
<http://rdfs.co/juso/geometry> <http://www.w3.org/2003/06/sw-vocab-status/ns#term_status> "unstable"@en .
<http://rdfs.co/juso/0.1.2> <http://purl.org/dc/terms/description> "\n    Juso Ontology is a Web vocabulary for describing geographical addresses and\n    features.\n    "@en .
<http://rdfs.co/juso/Municipality> <http://www.w3.org/2003/06/sw-vocab-status/ns#term_status> "unstable"@en .
<http://rdfs.co/juso/Hamlet> <http://www.w3.org/2002/07/owl#sameAs> <http://linkedgeodata.org/ontology/Hamlet> .
<http://rdfs.co/juso/itrf2000_long> <http://www.w3.org/2004/02/skos/core#definition> "\n    The ITRF2000 longitude of a point (decimal degrees).\n    "@en .
<http://rdfs.co/juso/FederatedState> <http://www.w3.org/2004/02/skos/core#prefLabel> "연방주"@ko .
<http://rdfs.co/juso/wgs84_lat> <http://www.w3.org/2003/06/sw-vocab-status/ns#term_status> "unstable"@en .
<http://rdfs.co/juso/historical_address> <http://purl.org/dc/terms/modified> "2015-10-02+09:00"^^<http://www.w3.org/2001/XMLSchema#date> .
<http://rdfs.co/juso/second_level_administrative_division> <http://www.w3.org/2003/06/sw-vocab-status/ns#term_status> "unstable"@en .
_:B7af76555X2D95fbX2D4024X2Da653X2D1ecbadf9e9c2 <http://purl.org/dc/terms/creator> <http://jayg.me/> .
<http://www.geonames.org/ontology#shortName> <http://www.w3.org/2000/01/rdf-schema#subPropertyOf> <http://rdfs.co/juso/short_name> .
<http://rdfs.co/juso/Geometry> <http://www.w3.org/2003/06/sw-vocab-status/ns#term_status> "unstable"@en .
<http://rdfs.co/juso/PostalCode> <http://www.w3.org/2003/06/sw-vocab-status/ns#term_status> "unstable"@en .
<http://rdfs.co/juso/ThirdLevelAdministrativeDivision> <http://www.w3.org/2004/02/skos/core#prefLabel> "Third-level Administrative Division"@en .
<http://rdfs.co/juso/0.1.2> <http://purl.org/vocab/vann/preferredNamespaceUri> "http://rdfs.co/juso/" .
<http://rdfs.co/juso/full_address> <http://www.w3.org/2004/02/skos/core#definition> "\n    The complete address written as a string, with or without formatting.\n    "@en .
<http://rdfs.co/juso/Township> <http://purl.org/dc/terms/issued> "2015-10-02+09:00"^^<http://www.w3.org/2001/XMLSchema#date> .
<http://rdfs.co/juso/Country> <http://www.w3.org/2004/02/skos/core#prefLabel> "Country"@en .
<http://rdfs.co/juso/thoroughfare_address> <http://purl.org/dc/terms/issued> "2015-10-02+09:00"^^<http://www.w3.org/2001/XMLSchema#date> .
<http://jayg.me/> <http://xmlns.com/foaf/0.1/name> "김보람"@ko .
<http://rdfs.co/juso/within> <http://www.w3.org/1999/02/22-rdf-syntax-ns#type> <http://www.w3.org/2002/07/owl#TransitiveProperty> .
<http://rdfs.co/juso/CoreGroup> <http://www.w3.org/1999/02/22-rdf-syntax-ns#_1> <http://rdfs.co/juso/SpatialThing> .
<http://rdfs.co/juso/third_level_administrative_division> <http://www.w3.org/2004/02/skos/core#definition> "\n    The third-level administrative division of the address, if any.\n    "@en .
<http://rdfs.co/juso/wgs84_long> <http://www.w3.org/2004/02/skos/core#prefLabel> "longitude (WGS84)"@en .
<http://rdfs.co/juso/exonym> <http://www.w3.org/2000/01/rdf-schema#isDefinedBy> <http://rdfs.co/juso/> .
<http://rdfs.co/juso/alternate_name> <http://www.w3.org/2000/01/rdf-schema#subPropertyOf> <http://rdfs.co/juso/name> .
<http://rdfs.co/juso/locator_address> <http://www.w3.org/2004/02/skos/core#definition> "\n    This property is used to describe a number or a sequence of characters that\n    uniquely identifies the exact locator within the relevant scope(s), that is\n    described by juso:locator.\n    "@en .
_:B73558d1bX2D2f92X2D4be2X2D9f2fX2Dfc6f492ebfa2 <http://www.w3.org/1999/02/22-rdf-syntax-ns#first> <http://rdfs.co/juso/postal_code> .
<http://rdfs.co/juso/historical_address> <http://www.w3.org/1999/02/22-rdf-syntax-ns#type> <http://www.w3.org/2002/07/owl#ObjectProperty> .
_:B5f94f7eeX2D87b3X2D4b12X2D952fX2D2915101e3e3b <http://www.w3.org/1999/02/22-rdf-syntax-ns#value> "text/html" .
<http://rdfs.co/juso/PostalCode> <http://www.w3.org/2000/01/rdf-schema#seeAlso> <https://en.wikipedia.org/wiki/Postal_code> .
<http://rdfs.co/juso/PoliticalDivisionGroup> <http://www.w3.org/1999/02/22-rdf-syntax-ns#_18> <http://rdfs.co/juso/District> .
<http://rdfs.co/juso/CoreGroup> <http://www.w3.org/1999/02/22-rdf-syntax-ns#_8> <http://rdfs.co/juso/alternate_name> .
<http://rdfs.co/juso/ConsolidatedCityCounty> <http://www.w3.org/2004/02/skos/core#definition> "\n    A consolidated city-county is a city and county that have been merged into\n    one unified jurisdiction. As such it is simultaneously a city, which is a\n    municipal corporation, and a county, which is an administrative division of\n    a state. It has the powers and responsibilities of both types of entities.\n    "@en .
<http://rdfs.co/juso/Point> <http://www.w3.org/1999/02/22-rdf-syntax-ns#type> <http://www.w3.org/2002/07/owl#Class> .
<http://rdfs.co/juso/Province> <http://www.w3.org/2004/02/skos/core#prefLabel> "Province"@en .
<http://rdfs.co/juso/Parish> <http://purl.org/dc/terms/modified> "2015-10-02+09:00"^^<http://www.w3.org/2001/XMLSchema#date> .
_:B68a7b51bX2Dfa3dX2D4d94X2Dadc1X2D2be21cdb7d78 <http://purl.org/dc/terms/date> "2015-12-30+09:00"^^<http://www.w3.org/2001/XMLSchema#date> .
_:B17925ab7X2D4341X2D48e5X2D86bfX2Dfe59340945bd <http://www.w3.org/1999/02/22-rdf-syntax-ns#rest> _:Bde26aa6aX2D2065X2D4c51X2D8013X2D4cef3dacf87c .
<http://rdfs.co/juso/Point> <http://www.w3.org/2003/06/sw-vocab-status/ns#term_status> "unstable"@en .
<http://rdfs.co/juso/Town> <http://purl.org/dc/terms/issued> "2015-10-02+09:00"^^<http://www.w3.org/2001/XMLSchema#date> .
_:Be368c69eX2Dace7X2D4a9dX2D82a8X2Dae90ab3c5611 <http://www.w3.org/2000/01/rdf-schema#comment> "\n    <pre><code>_:YangyongBldg a juso:Feature ;\n  juso:name \"Yangyong Building\"@en , \"양용빌딩\"@ko ;\n  juso:geometry &lt;http://geohash.org/wydjrzg6ece9&gt; .\n\n_:LiSTInc a juso:SpatialThing , foaf:Organization ;\n  juso:name \"LiST Inc.\"@en , \"주식회사 리스트\"@ko ;\n  juso:within _:YangyongBldg ;\n  juso:historical_address [\n    a juso:Address ;\n    juso:full_address\n      \"대한민국 서울특별시 영등포구 당산동 121-17 양용빌딩 9층 150-040\"@ko ,\n      \"9th Floor, Yangyong Building, 121-17, Dangsan-dong, Yeongdeungpo-gu, Seoul, 150-040, South Korea\"@en ;\n    juso:country &lt;http://sws.geonames.org/1835841/&gt; ;\n    juso:first_level_administrative_division &lt;http://sws.geonames.org/1835847/&gt; ;\n    juso:second_level_administrative_division &lt;http://sws.geonames.org/1832536/&gt; ;\n    juso:third_level_administrative_division &lt;http://sws.geonames.org/8692617/&gt; ;\n    juso:locator _:YangyongBldg ;\n    juso:locator_address \"9층\"@ko , \"9th Floor\"@en ;\n    juso:postal_code [\n      a juso:PostalCode ;\n      rdf:value \"150-040\"\n    ]\n  ] ;\n  juso:address [\n    a juso:Address ;\n    juso:full_address\n      \"대한민국 서울특별시 영등포구 버드나루로19길 3 (당산동) 양용빌딩 9층 07229\"@ko ,\n      \"9th Floor, Yangyong Building, 3, Beodeunaru-ro 19-gil, Yeongdeungpo-gu, Seoul, 07229, South Korea\"@en ;\n    juso:country &lt;http://sws.geonames.org/1835841/&gt; ;\n    juso:first_level_administrative_division &lt;http://sws.geonames.org/1835847/&gt; ;\n    juso:second_level_administrative_division &lt;http://sws.geonames.org/1832536/&gt; ;\n    juso:third_level_administrative_division &lt;http://sws.geonames.org/8692617/&gt; ;\n    juso:thoroughfare [\n      a juso:Street ;\n      juso:name \"Beodeunaru-ro 19-gil\"@en , \"버드나루로19길\"@ko ;\n      juso:parent &lt;http://sws.geonames.org/8692617/&gt;\n    ] ;\n    juso:thoroughfare_address \"3\" ;\n    juso:locator _:YangyongBldg ;\n    juso:locator_address \"9층\"@ko , \"9th Floor\"@en ;\n    juso:postal_code [\n      a juso:PostalCode ;\n      rdf:value \"07229\"\n    ]\n  ] .</code></pre>\n    "^^<http://www.w3.org/1999/02/22-rdf-syntax-ns#HTML> .
<http://schema.org/postalCode> <http://www.w3.org/2002/07/owl#propertyChainAxiom> _:Bc87168a3X2D4f47X2D4915X2Dab29X2D178d859ca892 .
<http://rdfs.co/juso/Parish> <http://www.w3.org/2000/01/rdf-schema#seeAlso> <https://en.wikipedia.org/wiki/Parish_(administrative_division)> .
<http://rdfs.co/juso/0.1.2> <http://purl.org/dc/terms/replaces> <http://rdfs.co/juso/0.1.1> .
<http://rdfs.co/juso/AdministrativeDivision> <http://www.w3.org/2004/02/skos/core#altLabel> "Country Subdivision"@en .
<http://rdfs.co/juso/Village> <http://www.w3.org/2004/02/skos/core#prefLabel> "Village"@en .
<http://rdfs.co/juso/address> <http://www.w3.org/2000/01/rdf-schema#isDefinedBy> <http://rdfs.co/juso/> .
<http://rdfs.co/juso/0.1.2> <http://www.w3.org/2000/01/rdf-schema#comment> "\n    There is an extension to this ontology with some country-specific terms for\n    <a href=\"http://rdfs.co/juso/kr/\">South Korea</a>.\n    "@ko .
<http://schema.org/PostalAddress> <http://www.w3.org/2000/01/rdf-schema#subClassOf> <http://rdfs.co/juso/Address> .
<http://rdfs.co/juso/locator> <http://purl.org/dc/terms/issued> "2015-10-02+09:00"^^<http://www.w3.org/2001/XMLSchema#date> .
<http://jayg.me/> <http://xmlns.com/foaf/0.1/mbox_sha1sum> "f03421e94730da58e8943d3a1d2c4c6b02898e14" .
<http://rdfs.co/juso/CoreGroup> <http://www.w3.org/1999/02/22-rdf-syntax-ns#_6> <http://rdfs.co/juso/name> .
<http://rdfs.co/juso/CapitalDistrict> <http://www.w3.org/2004/02/skos/core#definition> "\n    A capital district or capital territory is normally a specially designated\n    administrative division where a country's seat of government is located.\n    "@en .
<http://rdfs.co/juso/short_name> <http://www.w3.org/2004/02/skos/core#definition> "\n    This property indicates the relatively short name of the spatial thing.\n    "@en .
<http://rdfs.co/juso/Geometry> <http://www.w3.org/1999/02/22-rdf-syntax-ns#type> <http://www.w3.org/2002/07/owl#Class> .
<http://rdfs.co/juso/Municipality> <http://www.w3.org/2000/01/rdf-schema#seeAlso> <https://en.wikipedia.org/wiki/Municipality> .
<http://rdfs.co/juso/PostalCode> <http://www.w3.org/1999/02/22-rdf-syntax-ns#type> <http://www.w3.org/2002/07/owl#Class> .
<http://www.w3.org/ns/locn#postCode> <http://www.w3.org/2002/07/owl#propertyChainAxiom> _:Bef458c30X2D3ae8X2D4a86X2D8152X2D83d608b43cd5 .
<http://rdfs.co/juso/Province> <http://www.w3.org/2000/01/rdf-schema#isDefinedBy> <http://rdfs.co/juso/> .
<http://rdfs.co/juso/geometry> <http://www.w3.org/2000/01/rdf-schema#subPropertyOf> <http://www.w3.org/ns/locn#geometry> .
<http://rdfs.co/juso/Feature> <http://www.w3.org/2002/07/owl#equivalentClass> <http://www.geonames.org/ontology#Feature> .
<http://rdfs.co/juso/postal_code> <http://purl.org/dc/terms/modified> "2015-10-02+09:00"^^<http://www.w3.org/2001/XMLSchema#date> .
<http://rdfs.co/juso/full_address> <http://www.w3.org/2002/07/owl#sameAs> <http://www.w3.org/ns/locn#fullAddress> .
<http://rdfs.co/juso/AddressGroup> <http://www.w3.org/1999/02/22-rdf-syntax-ns#_5> <http://rdfs.co/juso/third_level_administrative_division> .
<http://rdfs.co/juso/District> <http://www.w3.org/2000/01/rdf-schema#isDefinedBy> <http://rdfs.co/juso/> .
<http://rdfs.co/juso/Province> <http://www.w3.org/2002/07/owl#sameAs> <http://dbpedia.org/ontology/Province> .
<http://rdfs.co/juso/Country> <http://www.w3.org/2002/07/owl#sameAs> <http://dbpedia.org/ontology/Country> .
<http://rdfs.co/juso/fourth_level_administrative_division> <http://www.w3.org/2000/01/rdf-schema#isDefinedBy> <http://rdfs.co/juso/> .
<http://jayg.me/> <http://www.w3.org/1999/02/22-rdf-syntax-ns#type> <http://xmlns.com/foaf/0.1/Person> .
<http://rdfs.co/juso/fifth_level_administrative_division> <http://www.w3.org/2000/01/rdf-schema#isDefinedBy> <http://rdfs.co/juso/> .
<http://rdfs.co/juso/postal_code> <http://www.w3.org/2000/01/rdf-schema#range> <http://rdfs.co/juso/PostalCode> .
<http://rdfs.co/juso/full_address> <http://www.w3.org/2003/06/sw-vocab-status/ns#term_status> "testing"@en .
<http://rdfs.co/juso/District> <http://www.w3.org/2002/07/owl#sameAs> <http://dbpedia.org/ontology/District> .
<http://rdfs.co/juso/official_name> <http://www.w3.org/2000/01/rdf-schema#seeAlso> <http://www.geonames.org/ontology#officialName> .
<http://rdfs.co/juso/within> <http://purl.org/dc/terms/issued> "2015-10-02+09:00"^^<http://www.w3.org/2001/XMLSchema#date> .
<http://rdfs.co/juso/PostalCode> <http://www.w3.org/2004/02/skos/core#altLabel> "Postcode"@en .
<http://rdfs.co/juso/FederatedState> <http://www.w3.org/2000/01/rdf-schema#subClassOf> <http://dbpedia.org/ontology/State> .
<http://rdfs.co/juso/Hamlet> <http://purl.org/dc/terms/modified> "2015-10-02+09:00"^^<http://www.w3.org/2001/XMLSchema#date> .
<http://rdfs.co/juso/SpatialThing> <http://www.w3.org/2004/02/skos/core#definition> "\n    Anything that has a spatial representation, i.e. size, shape, or position.\n    e.g. people, places, objects, as well as abstract areas like cubes.\n    "@en .
<http://rdfs.co/juso/FederatedState> <http://www.w3.org/2000/01/rdf-schema#isDefinedBy> <http://rdfs.co/juso/> .
<http://rdfs.co/juso/FifthLevelAdministrativeDivision> <http://www.w3.org/2003/06/sw-vocab-status/ns#term_status> "unstable"@en .
<http://rdfs.co/juso/name> <http://www.w3.org/1999/02/22-rdf-syntax-ns#type> <http://www.w3.org/2002/07/owl#DatatypeProperty> .
<http://rdfs.co/juso/CapitalDistrict> <http://www.w3.org/2000/01/rdf-schema#seeAlso> <https://en.wikipedia.org/wiki/Capital_districts_and_territories> .
<http://rdfs.co/juso/FederatedState> <http://www.w3.org/2004/02/skos/core#altLabel> "State"@en .
<http://rdfs.co/juso/CoreGroup> <http://www.w3.org/1999/02/22-rdf-syntax-ns#_7> <http://rdfs.co/juso/official_name> .
<http://rdfs.co/juso/PoliticalDivisionGroup> <http://www.w3.org/1999/02/22-rdf-syntax-ns#_4> <http://rdfs.co/juso/FirstLevelAdministrativeDivision> .
<http://rdfs.co/juso/first_level_administrative_division> <http://www.w3.org/1999/02/22-rdf-syntax-ns#type> <http://www.w3.org/2002/07/owl#ObjectProperty> .
<http://rdfs.co/juso/ThirdLevelAdministrativeDivision> <http://www.w3.org/2000/01/rdf-schema#subClassOf> <http://rdfs.co/juso/AdministrativeDivision> .
<http://rdfs.co/juso/AdministrativeDivision> <http://purl.org/dc/terms/issued> "2015-10-02+09:00"^^<http://www.w3.org/2001/XMLSchema#date> .
<http://rdfs.co/juso/Village> <http://www.w3.org/2000/01/rdf-schema#isDefinedBy> <http://rdfs.co/juso/> .
<http://rdfs.co/juso/Neighborhood> <http://www.w3.org/1999/02/22-rdf-syntax-ns#type> <http://www.w3.org/2002/07/owl#Class> .
<http://rdfs.co/juso/alternate_name> <http://www.w3.org/1999/02/22-rdf-syntax-ns#type> <http://www.w3.org/2002/07/owl#DatatypeProperty> .
<http://rdfs.co/juso/locator_address> <http://www.w3.org/2003/06/sw-vocab-status/ns#term_status> "unstable"@en .
_:B72d2cd9fX2D75e4X2D414bX2D94ceX2Dec81117dce46 <http://www.w3.org/2000/01/rdf-schema#label> "RDF/XML"@en .
<http://rdfs.co/juso/political_division> <http://www.w3.org/2004/02/skos/core#prefLabel> "political division"@en .
<http://rdfs.co/juso/Thoroughfare> <http://www.w3.org/2004/02/skos/core#prefLabel> "Thoroughfare"@en .
<http://rdfs.co/juso/PoliticalDivision> <http://www.w3.org/2002/07/owl#equivalentClass> <http://schema.org/AdministrativeArea> .
<http://rdfs.co/juso/geometry> <http://purl.org/dc/terms/issued> "2015-10-02+09:00"^^<http://www.w3.org/2001/XMLSchema#date> .
<http://rdfs.co/juso/Neighborhood> <http://www.w3.org/2003/06/sw-vocab-status/ns#term_status> "unstable"@en .
<http://rdfs.co/juso/Point> <http://www.w3.org/2000/01/rdf-schema#subClassOf> <http://rdfs.co/juso/Geometry> .
<http://rdfs.co/juso/Municipality> <http://purl.org/dc/terms/issued> "2015-10-02+09:00"^^<http://www.w3.org/2001/XMLSchema#date> .
<http://rdfs.co/juso/FifthLevelAdministrativeDivision> <http://www.w3.org/1999/02/22-rdf-syntax-ns#type> <http://www.w3.org/2002/07/owl#Class> .
<http://rdfs.co/juso/Address> <http://purl.org/dc/terms/modified> "2015-10-02+09:00"^^<http://www.w3.org/2001/XMLSchema#date> .
<http://schema.org/address> <http://www.w3.org/2000/01/rdf-schema#subPropertyOf> <http://rdfs.co/juso/address> .
<http://schema.org/GeoCoordinates> <http://www.w3.org/2000/01/rdf-schema#subClassOf> <http://rdfs.co/juso/Geometry> .
_:Bc87168a3X2D4f47X2D4915X2Dab29X2D178d859ca892 <http://www.w3.org/1999/02/22-rdf-syntax-ns#first> <http://rdfs.co/juso/postal_code> .
<http://rdfs.co/juso/parent> <http://www.w3.org/2004/02/skos/core#prefLabel> "parent politial division"@en .
<http://rdfs.co/juso/country> <http://www.w3.org/2000/01/rdf-schema#isDefinedBy> <http://rdfs.co/juso/> .
<http://rdfs.co/juso/0.1.2> <http://www.w3.org/1999/02/22-rdf-syntax-ns#type> <http://www.w3.org/2002/07/owl#Ontology> .
<http://rdfs.co/juso/exonym> <http://www.w3.org/2000/01/rdf-schema#domain> <http://rdfs.co/juso/Feature> .
<http://rdfs.co/juso/FourthLevelAdministrativeDivision> <http://www.w3.org/2000/01/rdf-schema#subClassOf> <http://rdfs.co/juso/AdministrativeDivision> .
<http://rdfs.co/juso/Neighborhood> <http://www.w3.org/2004/02/skos/core#prefLabel> "Neighborhood"@en-us .
<http://rdfs.co/juso/AdministrativeDivision> <http://www.w3.org/2004/02/skos/core#altLabel> "Administrative Entity"@en .
<http://rdfs.co/juso/District> <http://www.w3.org/2004/02/skos/core#prefLabel> "구"@ko .
_:Bdb835a76X2D643fX2D4ba0X2Db7efX2De49279b0f79d <http://purl.org/dc/terms/date> "2015-10-07+09:00"^^<http://www.w3.org/2001/XMLSchema#date> .
<http://rdfs.co/juso/thoroughfare> <http://www.w3.org/1999/02/22-rdf-syntax-ns#type> <http://www.w3.org/2002/07/owl#ObjectProperty> .
<http://rdfs.co/juso/AddressGroup> <http://www.w3.org/1999/02/22-rdf-syntax-ns#_13> <http://rdfs.co/juso/locator_address> .
<http://rdfs.co/juso/country> <http://www.w3.org/2004/02/skos/core#definition> "\n    The uppermost politial division for the address, almost always a country.\n    "@en .
<http://listinc.kr/id/listinc> <http://www.w3.org/1999/02/22-rdf-syntax-ns#type> <http://www.w3.org/ns/org#Organization> .
<http://www.geonames.org/ontology#officialName> <http://www.w3.org/2000/01/rdf-schema#subPropertyOf> <http://rdfs.co/juso/official_name> .
<http://www.opengis.net/ont/geosparql#hasGeometry> <http://www.w3.org/2000/01/rdf-schema#subPropertyOf> <http://rdfs.co/juso/geometry> .
<http://rdfs.co/juso/Feature> <http://www.w3.org/2002/07/owl#disjointWith> <http://rdfs.co/juso/Geometry> .
_:B5f94f7eeX2D87b3X2D4b12X2D952fX2D2915101e3e3b <http://www.w3.org/2000/01/rdf-schema#seeAlso> <http://www.iana.org/assignments/media-types/text/html> .
<http://rdfs.co/juso/Town> <http://www.w3.org/1999/02/22-rdf-syntax-ns#type> <http://www.w3.org/2002/07/owl#Class> .
<http://rdfs.co/juso/Parish> <http://www.w3.org/2004/02/skos/core#definition> "\n    A parish is an administrative division used by several countries. In parts\n    of the British Isles it is known as a civil parish to distinguish it from\n    the ecclesiastical parish.\n    "@en .
<http://rdfs.co/juso/Street> <http://www.w3.org/2000/01/rdf-schema#seeAlso> <https://en.wikipedia.org/wiki/Street> .
<http://rdfs.co/juso/0.1.2> <http://www.w3.org/ns/adms#status> <http://purl.org/adms/status/UnderDevelopment> .
<http://rdfs.co/juso/thoroughfare> <http://purl.org/dc/terms/modified> "2015-10-02+09:00"^^<http://www.w3.org/2001/XMLSchema#date> .
<http://rdfs.co/juso/Address> <http://www.w3.org/2004/02/skos/core#prefLabel> "주소"@ko .
<http://rdfs.co/juso/second_level_administrative_division> <http://purl.org/dc/terms/issued> "2015-10-02+09:00"^^<http://www.w3.org/2001/XMLSchema#date> .
<http://rdfs.co/juso/full_address> <http://purl.org/dc/terms/modified> "2015-10-02+09:00"^^<http://www.w3.org/2001/XMLSchema#date> .
<http://rdfs.co/juso/Geometry> <http://purl.org/dc/terms/issued> "2015-10-02+09:00"^^<http://www.w3.org/2001/XMLSchema#date> .
<http://rdfs.co/juso/PostalCode> <http://purl.org/dc/terms/issued> "2015-10-02+09:00"^^<http://www.w3.org/2001/XMLSchema#date> .
<http://rdfs.co/juso/SpatialThing> <http://www.w3.org/2004/02/skos/core#altLabel> "Spatial Object"@en .
<http://rdfs.co/juso/post_office_box> <http://www.w3.org/2004/02/skos/core#definition> "\n    This property describes the post office box number for PO box addresses.\n    A post-office box or post office box (commonly referred to as a PO box or a\n    postal box) is a uniquely addressable lockable box located on the premises\n    of a post office station.\n    "@en .
<http://rdfs.co/juso/AdministrativeDivision> <http://www.w3.org/2004/02/skos/core#altLabel> "Geopolitical Division"@en .
<http://rdfs.co/juso/City> <http://www.w3.org/2000/01/rdf-schema#subClassOf> <http://rdfs.co/juso/AdministrativeDivision> .
<http://rdfs.co/juso/thoroughfare_address> <http://www.w3.org/2000/01/rdf-schema#seeAlso> <https://en.wikipedia.org/wiki/House_numbering> .
<http://rdfs.co/juso/SecondLevelAdministrativeDivision> <http://www.w3.org/2004/02/skos/core#prefLabel> "Second-level Administrative Division"@en .
<http://rdfs.co/juso/AddressGroup> <http://www.w3.org/1999/02/22-rdf-syntax-ns#_8> <http://rdfs.co/juso/Thoroughfare> .
<http://rdfs.co/juso/Township> <http://www.w3.org/2003/06/sw-vocab-status/ns#term_status> "unstable"@en .
<http://rdfs.co/juso/fourth_level_administrative_division> <http://www.w3.org/2004/02/skos/core#definition> "\n    The fourth-level administrative division of the address, if any.\n    "@en .
<http://rdfs.co/juso/official_name> <http://www.w3.org/2003/06/sw-vocab-status/ns#term_status> "unstable"@en .
<http://rdfs.co/juso/CapitalDistrict> <http://purl.org/dc/terms/modified> "2015-10-02+09:00"^^<http://www.w3.org/2001/XMLSchema#date> .
<http://rdfs.co/juso/wgs84_long> <http://www.w3.org/2003/06/sw-vocab-status/ns#term_status> "unstable"@en .
<http://rdfs.co/juso/thoroughfare_address> <http://www.w3.org/2003/06/sw-vocab-status/ns#term_status> "unstable"@en .
<http://rdfs.co/juso/Town> <http://www.w3.org/2002/07/owl#sameAs> <http://linkedgeodata.org/ontology/Town> .
<http://rdfs.co/juso/locator> <http://www.w3.org/2004/02/skos/core#definition> "\n    The real world entity identified by the address. The locator could be the\n    property or complex, of the building or part of the building, of it could\n    be a room inside a building.\n    "@en .
<http://rdfs.co/juso/parent> <http://www.w3.org/2000/01/rdf-schema#subPropertyOf> <http://rdfs.co/juso/political_division> .
<http://rdfs.co/juso/0.1.2> <http://www.w3.org/2004/02/skos/core#historyNote> _:B7af76555X2D95fbX2D4024X2Da653X2D1ecbadf9e9c2 .
<http://rdfs.co/juso/within> <http://www.w3.org/2000/01/rdf-schema#domain> <http://rdfs.co/juso/SpatialThing> .
<http://rdfs.co/juso/official_name> <http://purl.org/dc/terms/issued> "2015-12-30+09:00"^^<http://www.w3.org/2001/XMLSchema#date> .
<http://rdfs.co/juso/Town> <http://www.w3.org/2004/02/skos/core#prefLabel> "읍"@ko .
<http://rdfs.co/juso/post_office_box> <http://purl.org/dc/terms/modified> "2015-10-02+09:00"^^<http://www.w3.org/2001/XMLSchema#date> .
<http://rdfs.co/juso/SecondLevelAdministrativeDivision> <http://www.w3.org/2000/01/rdf-schema#subClassOf> <http://rdfs.co/juso/AdministrativeDivision> .
<http://rdfs.co/juso/SecondLevelAdministrativeDivision> <http://www.w3.org/2004/02/skos/core#definition> "\n    A subdivision of a first-level administrative division.\n    "@en .
<http://rdfs.co/juso/Township> <http://www.w3.org/1999/02/22-rdf-syntax-ns#type> <http://www.w3.org/2002/07/owl#Class> .
<http://rdfs.co/juso/endonym> <http://www.w3.org/2000/01/rdf-schema#seeAlso> <https://en.wikipedia.org/wiki/Exonym_and_endonym> .
<http://rdfs.co/juso/AdministrativeDivision> <http://www.w3.org/2004/02/skos/core#prefLabel> "Administrative Division"@en .
<http://rdfs.co/juso/Village> <http://www.w3.org/2004/02/skos/core#prefLabel> "리"@ko .
<http://rdfs.co/juso/Country> <http://www.w3.org/2004/02/skos/core#prefLabel> "나라"@ko .
<http://rdfs.co/juso/0.1.2> <http://purl.org/vocab/vann/termGroup> <http://rdfs.co/juso/PoliticalDivisionGroup> .
_:B6fb959b7X2Db6fbX2D4cbeX2D9eabX2Df833eee3b669 <http://www.w3.org/1999/02/22-rdf-syntax-ns#first> <http://www.w3.org/1999/02/22-rdf-syntax-ns#value> .
<http://rdfs.co/juso/0.1.2> <http://purl.org/dc/terms/hasFormat> <http://rdfs.co/juso/0.1.2/rdf> .
<http://rdfs.co/juso/Address> <http://www.w3.org/2003/06/sw-vocab-status/ns#term_status> "testing"@en .
<http://rdfs.co/juso/Town> <http://www.w3.org/2003/06/sw-vocab-status/ns#term_status> "unstable"@en .
<http://rdfs.co/juso/endonym> <http://purl.org/dc/terms/modified> "2015-10-02+09:00"^^<http://www.w3.org/2001/XMLSchema#date> .
<http://rdfs.co/juso/within> <http://www.w3.org/2002/07/owl#sameAs> <http://geovocab.org/spatial#P> .
<http://rdfs.co/juso/FirstLevelAdministrativeDivision> <http://www.w3.org/2004/02/skos/core#altLabel> "First Administrative Level"@en .
<http://rdfs.co/juso/exonym> <http://www.w3.org/2000/01/rdf-schema#range> <http://www.w3.org/2001/XMLSchema#string> .
_:B6fb959b7X2Db6fbX2D4cbeX2D9eabX2Df833eee3b669 <http://www.w3.org/1999/02/22-rdf-syntax-ns#rest> <http://www.w3.org/1999/02/22-rdf-syntax-ns#nil> .
<http://rdfs.co/juso/name> <http://www.w3.org/2000/01/rdf-schema#subPropertyOf> <http://purl.org/dc/terms/title> .
<http://rdfs.co/juso/locator> <http://www.w3.org/2003/06/sw-vocab-status/ns#term_status> "unstable"@en .
<http://rdfs.co/juso/political_division> <http://purl.org/dc/terms/modified> "2015-10-02+09:00"^^<http://www.w3.org/2001/XMLSchema#date> .
<http://rdfs.co/juso/first_level_administrative_division> <http://purl.org/dc/terms/modified> "2015-10-02+09:00"^^<http://www.w3.org/2001/XMLSchema#date> .
<http://schema.org/geo> <http://www.w3.org/2000/01/rdf-schema#subPropertyOf> <http://rdfs.co/juso/geometry> .
_:B8944e783X2D91c4X2D4ed8X2Db4ecX2Df633899c71c7 <http://www.w3.org/2000/01/rdf-schema#label> "Turtle"@en .
<http://rdfs.co/juso/Address> <http://purl.org/dc/terms/issued> "2015-10-02+09:00"^^<http://www.w3.org/2001/XMLSchema#date> .
<http://rdfs.co/juso/historical_address> <http://www.w3.org/2003/06/sw-vocab-status/ns#term_status> "unstable"@en .
_:B72d2cd9fX2D75e4X2D414bX2D94ceX2Dec81117dce46 <http://www.w3.org/1999/02/22-rdf-syntax-ns#type> <http://purl.org/dc/terms/MediaType> .
<http://rdfs.co/juso/PoliticalDivision> <http://www.w3.org/2000/01/rdf-schema#isDefinedBy> <http://rdfs.co/juso/> .
<http://rdfs.co/juso/parent> <http://www.w3.org/2000/01/rdf-schema#isDefinedBy> <http://rdfs.co/juso/> .
<http://rdfs.co/juso/exonym> <http://www.w3.org/2004/02/skos/core#prefLabel> "exonym"@en .
<http://rdfs.co/juso/geometry> <http://purl.org/dc/terms/modified> "2015-10-02+09:00"^^<http://www.w3.org/2001/XMLSchema#date> .
<http://rdfs.co/juso/first_level_administrative_division> <http://www.w3.org/2004/02/skos/core#prefLabel> "first-level administrative division"@en .
<http://listinc.kr/id/listinc> <http://xmlns.com/foaf/0.1/mbox_sha1sum> "de068365487dd2da1f2e88f1eaad0217bff79b40" .
<http://rdfs.co/juso/County> <http://www.w3.org/1999/02/22-rdf-syntax-ns#type> <http://www.w3.org/2002/07/owl#Class> .
<http://rdfs.co/juso/AdministrativeDivision> <http://www.w3.org/2000/01/rdf-schema#seeAlso> <http://www.geonames.org/ontology#A.ADMD> .
<http://rdfs.co/juso/FirstLevelAdministrativeDivision> <http://www.w3.org/2000/01/rdf-schema#subClassOf> <http://rdfs.co/juso/AdministrativeDivision> .
<http://rdfs.co/juso/Municipality> <http://purl.org/dc/terms/modified> "2015-10-02+09:00"^^<http://www.w3.org/2001/XMLSchema#date> .
<http://rdfs.co/juso/Country> <http://www.w3.org/2002/07/owl#sameAs> <http://linkedgeodata.org/ontology/Country> .
<http://rdfs.co/juso/first_level_administrative_division> <http://www.w3.org/2004/02/skos/core#definition> "\n    The first-level administrative division (region) of the address, usually a\n    county, state or other such area that typically encompasses several\n    localities.\n    "@en .
<http://rdfs.co/juso/FederatedState> <http://www.w3.org/2004/02/skos/core#prefLabel> "Federated State"@en .
<http://rdfs.co/juso/Thoroughfare> <http://www.w3.org/2003/06/sw-vocab-status/ns#term_status> "unstable"@en .
<http://rdfs.co/juso/second_level_administrative_division> <http://www.w3.org/1999/02/22-rdf-syntax-ns#type> <http://www.w3.org/2002/07/owl#ObjectProperty> .
<http://rdfs.co/juso/alternate_name> <http://www.w3.org/2002/07/owl#propertyDisjointWith> <http://rdfs.co/juso/official_name> .
_:B8944e783X2D91c4X2D4ed8X2Db4ecX2Df633899c71c7 <http://www.w3.org/2002/07/owl#sameAs> <https://w3id.org/spar/mediatype/text/turtle> .
<http://rdfs.co/juso/official_name> <http://www.w3.org/2004/02/skos/core#prefLabel> "공식 이름"@ko .
<http://rdfs.co/juso/PoliticalDivisionGroup> <http://www.w3.org/1999/02/22-rdf-syntax-ns#_5> <http://rdfs.co/juso/SecondLevelAdministrativeDivision> .
<http://rdfs.co/juso/CoreGroup> <http://www.w3.org/1999/02/22-rdf-syntax-ns#_14> <http://rdfs.co/juso/address> .
<http://rdfs.co/juso/Country> <http://www.w3.org/2000/01/rdf-schema#seeAlso> <https://en.wikipedia.org/wiki/Country> .
<http://rdfs.co/juso/endonym> <http://www.w3.org/2004/02/skos/core#prefLabel> "endonym"@en .
<http://rdfs.co/juso/ConsolidatedCityCounty> <http://www.w3.org/1999/02/22-rdf-syntax-ns#type> <http://www.w3.org/2002/07/owl#Class> .
<http://rdfs.co/juso/Feature> <http://www.w3.org/2000/01/rdf-schema#subClassOf> <http://rdfs.co/juso/SpatialThing> .
<http://rdfs.co/juso/within> <http://purl.org/dc/terms/modified> "2015-10-02+09:00"^^<http://www.w3.org/2001/XMLSchema#date> .
<http://rdfs.co/juso/ConsolidatedCityCounty> <http://www.w3.org/2003/06/sw-vocab-status/ns#term_status> "unstable"@en .
<http://rdfs.co/juso/Hamlet> <http://purl.org/dc/terms/issued> "2015-10-02+09:00"^^<http://www.w3.org/2001/XMLSchema#date> .
<http://rdfs.co/juso/Address> <http://www.w3.org/2002/07/owl#sameAs> <http://ontology.eil.utoronto.ca/icontact.owl#Address> .
<http://rdfs.co/juso/name> <http://www.w3.org/2000/01/rdf-schema#isDefinedBy> <http://rdfs.co/juso/> .
<http://rdfs.co/juso/PostalCode> <http://www.w3.org/2004/02/skos/core#prefLabel> "Postal Code"@en .
<http://rdfs.co/juso/Thoroughfare> <http://www.w3.org/1999/02/22-rdf-syntax-ns#type> <http://www.w3.org/2002/07/owl#Class> .
<http://rdfs.co/juso/alternate_name> <http://www.w3.org/2000/01/rdf-schema#isDefinedBy> <http://rdfs.co/juso/> .
<http://rdfs.co/juso/Town> <http://www.w3.org/2004/02/skos/core#definition> "\n    A town is a human settlement larger than a village but smaller than a city.\n    The size definition for what constitutes a \"town\" varies considerably in\n    different parts of the world.\n    "@en .
<http://rdfs.co/juso/0.1.2> <http://www.w3.org/2000/01/rdf-schema#seeAlso> <https://github.com/listinc/juso-ontology> .
<http://rdfs.co/juso/Neighborhood> <http://www.w3.org/2000/01/rdf-schema#seeAlso> <https://en.wikipedia.org/wiki/Neighbourhood> .
<http://rdfs.co/juso/exonym> <http://www.w3.org/2000/01/rdf-schema#subPropertyOf> <http://rdfs.co/juso/name> .
<http://rdfs.co/juso/AdministrativeDivision> <http://purl.org/dc/terms/modified> "2015-10-02+09:00"^^<http://www.w3.org/2001/XMLSchema#date> .
<http://rdfs.co/juso/address> <http://www.w3.org/2004/02/skos/core#prefLabel> "address"@en .
<http://rdfs.co/juso/ThirdLevelAdministrativeDivision> <http://www.w3.org/2004/02/skos/core#altLabel> "Third-order Administrative Division"@en .
<http://rdfs.co/juso/County> <http://www.w3.org/2003/06/sw-vocab-status/ns#term_status> "unstable"@en .
<http://rdfs.co/juso/geometry> <http://www.w3.org/2000/01/rdf-schema#subPropertyOf> <http://geovocab.org/geometry#geometry> .
<http://rdfs.co/juso/AddressGroup> <http://www.w3.org/1999/02/22-rdf-syntax-ns#_1> <http://rdfs.co/juso/full_address> .
<http://rdfs.co/juso/Feature> <http://www.w3.org/2002/07/owl#sameAs> <http://geovocab.org/spatial#Feature> .
<http://rdfs.co/juso/Point> <http://www.w3.org/2004/02/skos/core#prefLabel> "점"@ko .
<http://rdfs.co/juso/PoliticalDivisionGroup> <http://www.w3.org/1999/02/22-rdf-syntax-ns#_3> <http://rdfs.co/juso/AdministrativeDivision> .
<http://rdfs.co/juso/PoliticalDivision> <http://www.w3.org/2004/02/skos/core#prefLabel> "Political Division"@en .
<http://rdfs.co/juso/PoliticalDivisionGroup> <http://www.w3.org/1999/02/22-rdf-syntax-ns#_13> <http://rdfs.co/juso/Borough> .
<http://rdfs.co/juso/FirstLevelAdministrativeDivision> <http://www.w3.org/2004/02/skos/core#prefLabel> "First-level Administrative Division"@en .
<http://rdfs.co/juso/Geometry> <http://www.w3.org/2004/02/skos/core#prefLabel> "Geometry"@en .
<http://rdfs.co/juso/Point> <http://www.w3.org/2004/02/skos/core#prefLabel> "Point"@en .
<http://rdfs.co/juso/PostalCode> <http://www.w3.org/2004/02/skos/core#prefLabel> "우편번호"@ko .
<http://rdfs.co/juso/FederatedState> <http://www.w3.org/2004/02/skos/core#definition> "\n    A federated state is a territorial and constitutional community forming\n    part of a federal union (federation) such as the United States and\n    Australia.\n    "@en .
<http://rdfs.co/juso/Feature> <http://www.w3.org/2000/01/rdf-schema#subClassOf> <http://www.opengis.net/ont/geosparql#Feature> .
<http://rdfs.co/juso/postal_code> <http://www.w3.org/2003/06/sw-vocab-status/ns#term_status> "unstable"@en .
<http://rdfs.co/juso/short_name> <http://www.w3.org/2000/01/rdf-schema#domain> <http://rdfs.co/juso/SpatialThing> .
<http://rdfs.co/juso/Street> <http://www.w3.org/2000/01/rdf-schema#subClassOf> <http://rdfs.co/juso/Thoroughfare> .
<http://rdfs.co/juso/name> <http://www.w3.org/2004/02/skos/core#prefLabel> "name"@en .
<http://rdfs.co/juso/FirstLevelAdministrativeDivision> <http://www.w3.org/2004/02/skos/core#altLabel> "First-order Administrative Division"@en .
<http://rdfs.co/juso/historical_address> <http://www.w3.org/2004/02/skos/core#prefLabel> "historical address"@en .
<http://rdfs.co/juso/official_name> <http://purl.org/dc/terms/modified> "2015-12-30+09:00"^^<http://www.w3.org/2001/XMLSchema#date> .
<http://rdfs.co/juso/alternate_name> <http://www.w3.org/2004/02/skos/core#prefLabel> "alternate name"@en .
<http://rdfs.co/juso/post_office_box> <http://purl.org/dc/terms/issued> "2015-10-02+09:00"^^<http://www.w3.org/2001/XMLSchema#date> .
<http://rdfs.co/juso/Province> <http://www.w3.org/2000/01/rdf-schema#subClassOf> <http://rdfs.co/juso/AdministrativeDivision> .
<http://rdfs.co/juso/endonym> <http://purl.org/dc/terms/issued> "2015-10-02+09:00"^^<http://www.w3.org/2001/XMLSchema#date> .
<http://ontology.eil.utoronto.ca/icontact.owl#hasStreetNumber> <http://www.w3.org/2000/01/rdf-schema#subPropertyOf> <http://rdfs.co/juso/thoroughfare_address> .
<http://rdfs.co/juso/political_division> <http://purl.org/dc/terms/issued> "2015-10-02+09:00"^^<http://www.w3.org/2001/XMLSchema#date> .
<http://rdfs.co/juso/first_level_administrative_division> <http://purl.org/dc/terms/issued> "2015-10-02+09:00"^^<http://www.w3.org/2001/XMLSchema#date> .
<http://rdfs.co/juso/Country> <http://www.w3.org/2000/01/rdf-schema#subClassOf> <http://rdfs.co/juso/PoliticalDivision> .
<http://rdfs.co/juso/Country> <http://www.w3.org/2000/01/rdf-schema#isDefinedBy> <http://rdfs.co/juso/> .
<http://rdfs.co/juso/Parish> <http://www.w3.org/2003/06/sw-vocab-status/ns#term_status> "unstable"@en .
<http://rdfs.co/juso/fourth_level_administrative_division> <http://www.w3.org/2000/01/rdf-schema#domain> <http://rdfs.co/juso/Address> .
<http://rdfs.co/juso/locator> <http://www.w3.org/2000/01/rdf-schema#range> <http://rdfs.co/juso/Feature> .
<http://rdfs.co/juso/fifth_level_administrative_division> <http://www.w3.org/2000/01/rdf-schema#domain> <http://rdfs.co/juso/Address> .
<http://schema.org/GeoShape> <http://www.w3.org/2000/01/rdf-schema#subClassOf> <http://rdfs.co/juso/Geometry> .
<http://rdfs.co/juso/Parish> <http://www.w3.org/1999/02/22-rdf-syntax-ns#type> <http://www.w3.org/2002/07/owl#Class> .
<http://rdfs.co/juso/geometry> <http://www.w3.org/1999/02/22-rdf-syntax-ns#type> <http://www.w3.org/2002/07/owl#ObjectProperty> .
<http://www.geonames.org/ontology#alternateName> <http://www.w3.org/2000/01/rdf-schema#subPropertyOf> <http://rdfs.co/juso/alternate_name> .
<http://rdfs.co/juso/AdministrativeDivision> <http://www.w3.org/2004/02/skos/core#altLabel> "Subnational Entity"@en .
<http://rdfs.co/juso/country> <http://www.w3.org/2000/01/rdf-schema#domain> <http://rdfs.co/juso/Address> .
<http://rdfs.co/juso/County> <http://www.w3.org/2000/01/rdf-schema#seeAlso> <https://en.wikipedia.org/wiki/County> .
<http://rdfs.co/juso/itrf2000_lat> <http://www.w3.org/2003/06/sw-vocab-status/ns#term_status> "unstable"@en .
<http://rdfs.co/juso/Geometry> <http://www.w3.org/2002/07/owl#sameAs> <http://www.opengis.net/ont/geosparql#Geometry> .
<http://rdfs.co/juso/CapitalDistrict> <http://purl.org/dc/terms/issued> "2015-10-02+09:00"^^<http://www.w3.org/2001/XMLSchema#date> .
<http://rdfs.co/juso/0.1.2> <http://purl.org/vocab/vann/termGroup> <http://rdfs.co/juso/CoreGroup> .
<http://rdfs.co/juso/exonym> <http://www.w3.org/2000/01/rdf-schema#subPropertyOf> <http://www.geonames.org/ontology#alternateName> .
<http://rdfs.co/juso/Address> <http://www.w3.org/2004/02/skos/core#altLabel> "Postal Address"@en .
<http://rdfs.co/juso/thoroughfare> <http://purl.org/dc/terms/issued> "2015-10-02+09:00"^^<http://www.w3.org/2001/XMLSchema#date> .
<http://rdfs.co/juso/second_level_administrative_division> <http://purl.org/dc/terms/modified> "2015-10-02+09:00"^^<http://www.w3.org/2001/XMLSchema#date> .
<http://rdfs.co/juso/0.1.2> <http://purl.org/dc/terms/hasFormat> <http://rdfs.co/juso/0.1.2/ttl> .
<http://rdfs.co/juso/full_address> <http://purl.org/dc/terms/issued> "2015-10-02+09:00"^^<http://www.w3.org/2001/XMLSchema#date> .
<http://rdfs.co/juso/Geometry> <http://purl.org/dc/terms/modified> "2015-10-02+09:00"^^<http://www.w3.org/2001/XMLSchema#date> .
<http://rdfs.co/juso/PostalCode> <http://purl.org/dc/terms/modified> "2015-10-02+09:00"^^<http://www.w3.org/2001/XMLSchema#date> .
<http://rdfs.co/juso/within> <http://www.w3.org/2003/06/sw-vocab-status/ns#term_status> "testing"@en .
<http://rdfs.co/juso/AddressGroup> <http://www.w3.org/1999/02/22-rdf-syntax-ns#_3> <http://rdfs.co/juso/first_level_administrative_division> .
<http://rdfs.co/juso/Thoroughfare> <http://purl.org/dc/terms/issued> "2015-10-02+09:00"^^<http://www.w3.org/2001/XMLSchema#date> .
<http://rdfs.co/juso/short_name> <http://purl.org/dc/terms/issued> "2015-12-30+09:00"^^<http://www.w3.org/2001/XMLSchema#date> .
<http://rdfs.co/juso/alternate_name> <http://www.w3.org/2000/01/rdf-schema#range> <http://www.w3.org/2001/XMLSchema#string> .
<http://rdfs.co/juso/parent> <http://www.w3.org/2000/01/rdf-schema#subPropertyOf> <http://www.geonames.org/ontology#parentFeature> .
<http://rdfs.co/juso/Hamlet> <http://www.w3.org/1999/02/22-rdf-syntax-ns#type> <http://www.w3.org/2002/07/owl#Class> .
<http://rdfs.co/juso/name> <http://www.w3.org/2000/01/rdf-schema#range> <http://www.w3.org/2001/XMLSchema#string> .
<http://rdfs.co/juso/Thoroughfare> <http://www.w3.org/2004/02/skos/core#definition> "\n    A passage or way through from one location to another, which is usually\n    used a component of an address. A thoroughfare is not necessarily a road,\n    it might be a waterway or some other feature.\n    "@en .
_:B85974e57X2D7cdfX2D4960X2Da14cX2D01aad0844ec3 <http://www.w3.org/1999/02/22-rdf-syntax-ns#first> <http://www.w3.org/1999/02/22-rdf-syntax-ns#value> .
<http://rdfs.co/juso/historical_address> <http://purl.org/dc/terms/issued> "2015-10-02+09:00"^^<http://www.w3.org/2001/XMLSchema#date> .
<http://rdfs.co/juso/political_division> <http://www.w3.org/1999/02/22-rdf-syntax-ns#type> <http://www.w3.org/2002/07/owl#TransitiveProperty> .
<http://ontology.eil.utoronto.ca/icontact.owl#hasState> <http://www.w3.org/2000/01/rdf-schema#subPropertyOf> <http://rdfs.co/juso/first_level_administrative_division> .
<http://rdfs.co/juso/historical_address> <http://www.w3.org/2000/01/rdf-schema#range> <http://rdfs.co/juso/Address> .
<http://rdfs.co/juso/Neighborhood> <http://purl.org/dc/terms/modified> "2015-10-02+09:00"^^<http://www.w3.org/2001/XMLSchema#date> .
<http://rdfs.co/juso/FourthLevelAdministrativeDivision> <http://www.w3.org/2000/01/rdf-schema#isDefinedBy> <http://rdfs.co/juso/> .
<http://rdfs.co/juso/Feature> <http://www.w3.org/2000/01/rdf-schema#isDefinedBy> <http://rdfs.co/juso/> .
<http://rdfs.co/juso/AddressGroup> <http://www.w3.org/1999/02/22-rdf-syntax-ns#_9> <http://rdfs.co/juso/Street> .
_:B85974e57X2D7cdfX2D4960X2Da14cX2D01aad0844ec3 <http://www.w3.org/1999/02/22-rdf-syntax-ns#rest> <http://www.w3.org/1999/02/22-rdf-syntax-ns#nil> .
<http://rdfs.co/juso/PoliticalDivision> <http://www.w3.org/2004/02/skos/core#definition> "\n    A political division is a geographic region accepted to be in the\n    jurisdiction of a particular governmental entity. The particular government\n    entity varies as each organizes its operations by further divisions\n    (subdivisions of the state) to further its tasks and satisfy its\n    responsibilities.\n    "@en .
<http://rdfs.co/juso/County> <http://purl.org/dc/terms/issued> "2015-10-02+09:00"^^<http://www.w3.org/2001/XMLSchema#date> .
<http://rdfs.co/juso/PoliticalDivisionGroup> <http://www.w3.org/1999/02/22-rdf-syntax-ns#_23> <http://rdfs.co/juso/Hamlet> .
<http://rdfs.co/juso/SpatialThing> <http://www.w3.org/2002/07/owl#sameAs> <http://www.opengis.net/ont/geosparql#SpatialObject> .
<http://rdfs.co/juso/City> <http://www.w3.org/2004/02/skos/core#prefLabel> "市"@ja .
<http://rdfs.co/juso/locator_address> <http://purl.org/dc/terms/modified> "2015-10-02+09:00"^^<http://www.w3.org/2001/XMLSchema#date> .
<http://rdfs.co/juso/PoliticalDivisionGroup> <http://www.w3.org/1999/02/22-rdf-syntax-ns#_10> <http://rdfs.co/juso/Province> .
<http://rdfs.co/juso/within> <http://www.w3.org/2000/01/rdf-schema#subPropertyOf> <http://www.w3.org/ns/locn#location> .
<http://rdfs.co/juso/County> <http://www.w3.org/2004/02/skos/core#altLabel> "Cnty."@en-us .
<http://rdfs.co/juso/exonym> <http://www.w3.org/2004/02/skos/core#definition> "\n    The exonym is an external name for a geographical place: a common name used\n    only outside the place in question, usually for historical reasons.\n    "@en .
<http://rdfs.co/juso/FifthLevelAdministrativeDivision> <http://purl.org/dc/terms/modified> "2015-10-02+09:00"^^<http://www.w3.org/2001/XMLSchema#date> .
<http://rdfs.co/juso/AddressGroup> <http://www.w3.org/1999/02/22-rdf-syntax-ns#_14> <http://rdfs.co/juso/po_box> .
<http://rdfs.co/juso/Address> <http://www.w3.org/1999/02/22-rdf-syntax-ns#type> <http://www.w3.org/2002/07/owl#Class> .
<http://rdfs.co/juso/locator> <http://www.w3.org/1999/02/22-rdf-syntax-ns#type> <http://www.w3.org/2002/07/owl#ObjectProperty> .
<http://rdfs.co/juso/District> <http://www.w3.org/2000/01/rdf-schema#subClassOf> <http://rdfs.co/juso/AdministrativeDivision> .
<http://rdfs.co/juso/within> <http://www.w3.org/2004/02/skos/core#prefLabel> "within"@en .
<http://rdfs.co/juso/Thoroughfare> <http://www.w3.org/2000/01/rdf-schema#subClassOf> <http://rdfs.co/juso/Feature> .
_:B8944e783X2D91c4X2D4ed8X2Db4ecX2Df633899c71c7 <http://www.w3.org/1999/02/22-rdf-syntax-ns#value> "text/turtle" .
<http://rdfs.co/juso/Village> <http://www.w3.org/2000/01/rdf-schema#subClassOf> <http://rdfs.co/juso/AdministrativeDivision> .
<http://listinc.kr/id/listinc> <http://xmlns.com/foaf/0.1/name> "주식회사 리스트"@ko .
<http://rdfs.co/juso/itrf2000_long> <http://www.w3.org/2003/06/sw-vocab-status/ns#term_status> "unstable"@en .
<http://rdfs.co/juso/FifthLevelAdministrativeDivision> <http://www.w3.org/2004/02/skos/core#altLabel> "Fifth Administrative Level"@en .
<http://rdfs.co/juso/locator> <http://www.w3.org/2004/02/skos/core#prefLabel> "locator"@en .
<http://rdfs.co/juso/ConsolidatedCityCounty> <http://purl.org/dc/terms/issued> "2015-10-02+09:00"^^<http://www.w3.org/2001/XMLSchema#date> .
<http://rdfs.co/juso/Hamlet> <http://www.w3.org/2003/06/sw-vocab-status/ns#term_status> "unstable"@en .
<http://rdfs.co/juso/ThirdLevelAdministrativeDivision> <http://www.w3.org/2000/01/rdf-schema#isDefinedBy> <http://rdfs.co/juso/> .
<http://rdfs.co/juso/short_name> <http://www.w3.org/2003/06/sw-vocab-status/ns#term_status> "unstable"@en .
<http://rdfs.co/juso/FederatedState> <http://www.w3.org/2000/01/rdf-schema#subClassOf> <http://rdfs.co/juso/AdministrativeDivision> .
<http://rdfs.co/juso/0.1.2> <http://purl.org/dc/terms/hasFormat> <http://rdfs.co/juso/0.1.2/html> .
<http://rdfs.co/juso/FourthLevelAdministrativeDivision> <http://www.w3.org/2004/02/skos/core#altLabel> "Fourth Administrative Level"@en .
<http://rdfs.co/juso/third_level_administrative_division> <http://www.w3.org/2000/01/rdf-schema#isDefinedBy> <http://rdfs.co/juso/> .
<http://rdfs.co/juso/endonym> <http://www.w3.org/2003/06/sw-vocab-status/ns#term_status> "unstable"@en .
<http://rdfs.co/juso/first_level_administrative_division> <http://www.w3.org/2003/06/sw-vocab-status/ns#term_status> "unstable"@en .
<http://rdfs.co/juso/SecondLevelAdministrativeDivision> <http://www.w3.org/2000/01/rdf-schema#isDefinedBy> <http://rdfs.co/juso/> .
<http://rdfs.co/juso/locator> <http://purl.org/dc/terms/modified> "2015-10-02+09:00"^^<http://www.w3.org/2001/XMLSchema#date> .
<http://rdfs.co/juso/political_division> <http://www.w3.org/2003/06/sw-vocab-status/ns#term_status> "unstable"@en .
<http://rdfs.co/juso/Neighborhood> <http://www.w3.org/2004/02/skos/core#prefLabel> "동"@ko .
<http://rdfs.co/juso/Parish> <http://purl.org/dc/terms/issued> "2015-10-02+09:00"^^<http://www.w3.org/2001/XMLSchema#date> .
<http://rdfs.co/juso/Township> <http://www.w3.org/2004/02/skos/core#definition> "\n    The word township is used to refer to different kinds of settlements in\n    different countries.\n    "@en .
<http://rdfs.co/juso/AddressGroup> <http://www.w3.org/1999/02/22-rdf-syntax-ns#_15> <http://rdfs.co/juso/PostalCode> .
<http://rdfs.co/juso/wgs84_long> <http://www.w3.org/2004/02/skos/core#prefLabel> "경도(WGS84)"@ko .
<http://rdfs.co/juso/within> <http://www.w3.org/2004/02/skos/core#definition> "\n    A spatial thing that contains the current one within the borders of its own\n    region.\n    "@en .
<http://rdfs.co/juso/Point> <http://www.w3.org/2002/07/owl#sameAs> <http://www.w3.org/2003/01/geo/wgs84_pos#Point> .
<http://rdfs.co/juso/third_level_administrative_division> <http://www.w3.org/2004/02/skos/core#prefLabel> "third-level administrative division"@en .
<http://rdfs.co/juso/Town> <http://purl.org/dc/terms/modified> "2015-10-02+09:00"^^<http://www.w3.org/2001/XMLSchema#date> .
<http://rdfs.co/juso/Municipality> <http://www.w3.org/2004/02/skos/core#definition> "\n    A municipality is usually an urban administrative division having corporate\n    status and usually powers of self-government or jurisdiction.\n    "@en .
<http://rdfs.co/juso/District> <http://www.w3.org/2004/02/skos/core#definition> "\n    A district is a type of administrative division that, in some countries, is\n    managed by local government. Across the world, areas known as \"districts\"\n    vary greatly in size, spanning entire regions or counties, several\n    municipalities, subdivisions of municipalities, school district, or\n    political district.\n    "@en .
<http://rdfs.co/juso/Hamlet> <http://www.w3.org/2004/02/skos/core#definition> "\n    A hamlet is a type of settlement. The definition of hamlet varies by\n    country. It usually refers to a small settlement, with a small population\n    that is usually under 100, in a rural area, or a component of a larger\n    settlement or municipality. Hamlets are typically unincorporated\n    communities.\n    "@en .
<http://rdfs.co/juso/postal_code> <http://purl.org/dc/terms/issued> "2015-10-02+09:00"^^<http://www.w3.org/2001/XMLSchema#date> .
<http://rdfs.co/juso/fifth_level_administrative_division> <http://www.w3.org/2004/02/skos/core#definition> "\n    The fifth-level administrative division of the address, if any.\n    "@en .
<http://rdfs.co/juso/CoreGroup> <http://www.w3.org/2000/01/rdf-schema#comment> "\n    These classes and properties form the core of Juso Ontology. They describe\n    fundamental characteristics of geography in relatively broad terms.\n    "@en .
<http://rdfs.co/juso/CapitalDistrict> <http://www.w3.org/2004/02/skos/core#altLabel> "Capital Territory"@en .
<http://rdfs.co/juso/AddressGroup> <http://www.w3.org/1999/02/22-rdf-syntax-ns#_16> <http://rdfs.co/juso/postal_code> .
<http://rdfs.co/juso/CapitalDistrict> <http://www.w3.org/1999/02/22-rdf-syntax-ns#type> <http://www.w3.org/2002/07/owl#Class> .
<http://rdfs.co/juso/AdministrativeDivision> <http://www.w3.org/2000/01/rdf-schema#seeAlso> <https://en.wikipedia.org/wiki/Administrative_division> .
<http://rdfs.co/juso/post_office_box> <http://www.w3.org/2003/06/sw-vocab-status/ns#term_status> "unstable"@en .
<http://rdfs.co/juso/AddressGroup> <http://www.w3.org/2000/01/rdf-schema#label> "Address Terms"@en .
_:B68a7b51bX2Dfa3dX2D4d94X2Dadc1X2D2be21cdb7d78 <http://purl.org/dc/terms/creator> <http://jayg.me/> .
<http://rdfs.co/juso/CapitalDistrict> <http://www.w3.org/2003/06/sw-vocab-status/ns#term_status> "unstable"@en .
<http://rdfs.co/juso/AdministrativeDivision> <http://www.w3.org/2004/02/skos/core#definition> "\n    An administrative division is a portion of a country or other region\n    delineated for the purpose of administration. Administrative divisions are\n    each granted a certain degree of autonomy and are usually required to\n    manage themselves through their own local governments.\n    "@en .
<http://rdfs.co/juso/thoroughfare_address> <http://purl.org/dc/terms/modified> "2015-10-02+09:00"^^<http://www.w3.org/2001/XMLSchema#date> .
<http://rdfs.co/juso/parent> <http://www.w3.org/2000/01/rdf-schema#domain> <http://rdfs.co/juso/Feature> .
<http://rdfs.co/juso/exonym> <http://www.w3.org/1999/02/22-rdf-syntax-ns#type> <http://www.w3.org/2002/07/owl#DatatypeProperty> .
_:Bdb835a76X2D643fX2D4ba0X2Db7efX2De49279b0f79d <http://purl.org/dc/terms/creator> <http://jayg.me/> .
<http://rdfs.co/juso/Hamlet> <http://www.w3.org/2000/01/rdf-schema#seeAlso> <https://en.wikipedia.org/wiki/Hamlet_(place)> .
<http://rdfs.co/juso/address> <http://www.w3.org/2004/02/skos/core#definition> "\n    This property associates anything with its address.\n    "@en .
<http://rdfs.co/juso/thoroughfare> <http://www.w3.org/2003/06/sw-vocab-status/ns#term_status> "unstable"@en .
<http://rdfs.co/juso/Township> <http://purl.org/dc/terms/modified> "2015-10-02+09:00"^^<http://www.w3.org/2001/XMLSchema#date> .
<http://rdfs.co/juso/FifthLevelAdministrativeDivision> <http://www.w3.org/2000/01/rdf-schema#seeAlso> <http://www.geonames.org/ontology#A.ADM5> .
<http://rdfs.co/juso/CoreGroup> <http://www.w3.org/1999/02/22-rdf-syntax-ns#_12> <http://rdfs.co/juso/exonym> .
<http://rdfs.co/juso/political_division> <http://www.w3.org/2004/02/skos/core#definition> "\n    A politial or administrative division that contain the current feature.\n    "@en .
<http://rdfs.co/juso/Village> <http://www.w3.org/2002/07/owl#sameAs> <http://dbpedia.org/ontology/Village> .
<http://rdfs.co/juso/address> <http://www.w3.org/2000/01/rdf-schema#subPropertyOf> <http://ontology.eil.utoronto.ca/icontact.owl#address> .
<http://rdfs.co/juso/PoliticalDivisionGroup> <http://www.w3.org/1999/02/22-rdf-syntax-ns#_21> <http://rdfs.co/juso/Neighborhood> .
<http://rdfs.co/juso/post_office_box> <http://www.w3.org/2002/07/owl#sameAs> <http://www.w3.org/ns/locn#poBox> .
<http://rdfs.co/juso/geometry> <http://www.w3.org/2000/01/rdf-schema#range> <http://rdfs.co/juso/Geometry> .
_:B72d2cd9fX2D75e4X2D414bX2D94ceX2Dec81117dce46 <http://purl.org/dc/dcam/memberOf> <http://purl.org/dc/terms/IMT> .
<http://rdfs.co/juso/second_level_administrative_division> <http://www.w3.org/2004/02/skos/core#prefLabel> "second-level administrative division"@en .
<http://rdfs.co/juso/City> <http://www.w3.org/2000/01/rdf-schema#isDefinedBy> <http://rdfs.co/juso/> .
<http://rdfs.co/juso/historical_address> <http://www.w3.org/2000/01/rdf-schema#domain> <http://rdfs.co/juso/SpatialThing> .
<http://rdfs.co/juso/itrf2000_lat> <http://www.w3.org/2004/02/skos/core#definition> "\n    The ITRF2000 latitude of a point (decimal degrees).\n    "@en .
_:B72d2cd9fX2D75e4X2D414bX2D94ceX2Dec81117dce46 <http://www.w3.org/1999/02/22-rdf-syntax-ns#value> "application/rdf+xml" .
<http://rdfs.co/juso/wgs84_long> <http://purl.org/dc/terms/modified> "2015-11-10+09:00"^^<http://www.w3.org/2001/XMLSchema#date> .
<http://rdfs.co/juso/political_division> <http://www.w3.org/2000/01/rdf-schema#range> <http://rdfs.co/juso/PoliticalDivision> .
<http://rdfs.co/juso/Address> <http://www.w3.org/2002/07/owl#sameAs> <http://www.w3.org/ns/locn#Address> .
<http://rdfs.co/juso/exonym> <http://purl.org/dc/terms/issued> "2015-10-02+09:00"^^<http://www.w3.org/2001/XMLSchema#date> .
<http://rdfs.co/juso/City> <http://purl.org/dc/terms/modified> "2015-10-02+09:00"^^<http://www.w3.org/2001/XMLSchema#date> .
<http://rdfs.co/juso/Village> <http://www.w3.org/2000/01/rdf-schema#seeAlso> <https://en.wikipedia.org/wiki/Village> .
<http://rdfs.co/juso/Street> <http://www.w3.org/2004/02/skos/core#prefLabel> "Street"@en .
<http://rdfs.co/juso/CapitalDistrict> <http://www.w3.org/2000/01/rdf-schema#subClassOf> <http://rdfs.co/juso/AdministrativeDivision> .
<http://rdfs.co/juso/Neighborhood> <http://www.w3.org/2004/02/skos/core#prefLabel> "Neighbourhood"@en-gb .
<http://rdfs.co/juso/wgs84_long> <http://www.w3.org/2000/01/rdf-schema#domain> <http://rdfs.co/juso/Point> .
<http://rdfs.co/juso/ThirdLevelAdministrativeDivision> <http://www.w3.org/2000/01/rdf-schema#seeAlso> <http://www.geonames.org/ontology#A.ADM3> .
<http://rdfs.co/juso/0.1.2> <http://purl.org/dc/terms/type> <http://purl.org/adms/assettype/Ontology> .
<http://rdfs.co/juso/Township> <http://www.w3.org/2000/01/rdf-schema#isDefinedBy> <http://rdfs.co/juso/> .
<http://rdfs.co/juso/Feature> <http://www.w3.org/2004/02/skos/core#altLabel> "Feature"@en .
<http://rdfs.co/juso/Province> <http://www.w3.org/2000/01/rdf-schema#subClassOf> <http://schema.org/State> .
<http://rdfs.co/juso/geometry> <http://www.w3.org/2000/01/rdf-schema#domain> <http://rdfs.co/juso/Feature> .
<http://rdfs.co/juso/ConsolidatedCityCounty> <http://www.w3.org/2000/01/rdf-schema#subClassOf> <http://rdfs.co/juso/City> .
<http://rdfs.co/juso/itrf2000_lat> <http://www.w3.org/1999/02/22-rdf-syntax-ns#type> <http://www.w3.org/2002/07/owl#DatatypeProperty> .
<http://rdfs.co/juso/thoroughfare_address> <http://www.w3.org/2000/01/rdf-schema#isDefinedBy> <http://rdfs.co/juso/> .
<http://rdfs.co/juso/0.1.2> <http://www.w3.org/2000/01/rdf-schema#comment> "\n    <div>\n      The master version of this vocabulary is maintained in <a\n      href=\"https://github.com/listinc/juso-ontology\">the GitHub repository</a>\n      so others can contribute edits and improvements.\n    </div>\n    "^^<http://www.w3.org/1999/02/22-rdf-syntax-ns#HTML> .
<http://rdfs.co/juso/wgs84_long> <http://www.w3.org/2000/01/rdf-schema#isDefinedBy> <http://rdfs.co/juso/> .
<http://rdfs.co/juso/itrf2000_lat> <http://purl.org/dc/terms/issued> "2015-11-10+09:00"^^<http://www.w3.org/2001/XMLSchema#date> .
<http://rdfs.co/juso/official_name> <http://www.w3.org/2000/01/rdf-schema#isDefinedBy> <http://rdfs.co/juso/> .
<http://rdfs.co/juso/ConsolidatedCityCounty> <http://www.w3.org/2000/01/rdf-schema#subClassOf> <http://rdfs.co/juso/County> .
<http://rdfs.co/juso/Point> <http://www.w3.org/2004/02/skos/core#definition> "\n    A point is a geographical point on the surface of the Earth, typically\n    described using a coordinate system relative to the Earth, such as WGS84.\n  "@en .
<http://rdfs.co/juso/0.1.2> <http://purl.org/dc/terms/creator> <http://jayg.me/> .
_:B5f94f7eeX2D87b3X2D4b12X2D952fX2D2915101e3e3b <http://purl.org/dc/dcam/memberOf> <http://purl.org/dc/terms/IMT> .
<http://rdfs.co/juso/name> <http://www.w3.org/2004/02/skos/core#prefLabel> "이름"@ko .
<http://rdfs.co/juso/short_name> <http://www.w3.org/2000/01/rdf-schema#seeAlso> <http://www.geonames.org/ontology#shortName> .
<http://rdfs.co/juso/parent> <http://www.w3.org/2004/02/skos/core#definition> "\n    A politial or administrative division that is a direct parent of the\n    current feature.\n    "@en .
<http://rdfs.co/juso/PoliticalDivisionGroup> <http://www.w3.org/1999/02/22-rdf-syntax-ns#_20> <http://rdfs.co/juso/Township> .
<http://rdfs.co/juso/FourthLevelAdministrativeDivision> <http://www.w3.org/2000/01/rdf-schema#seeAlso> <http://www.geonames.org/ontology#A.ADM4> .
<http://rdfs.co/juso/Province> <http://purl.org/dc/terms/issued> "2015-10-02+09:00"^^<http://www.w3.org/2001/XMLSchema#date> .
<http://rdfs.co/juso/Town> <http://www.w3.org/2000/01/rdf-schema#seeAlso> <https://en.wikipedia.org/wiki/Town> .
<http://rdfs.co/juso/SpatialThing> <http://www.w3.org/2002/07/owl#sameAs> <http://www.w3.org/2003/01/geo/wgs84_pos#SpatialThing> .
<http://rdfs.co/juso/Hamlet> <http://www.w3.org/2004/02/skos/core#prefLabel> "Hamlet"@en .
<http://rdfs.co/juso/FourthLevelAdministrativeDivision> <http://www.w3.org/2004/02/skos/core#prefLabel> "Fourth-level Administrative Division"@en .
<http://rdfs.co/juso/short_name> <http://www.w3.org/2000/01/rdf-schema#subPropertyOf> <http://rdfs.co/juso/alternate_name> .
<http://rdfs.co/juso/address> <http://www.w3.org/2000/01/rdf-schema#range> <http://rdfs.co/juso/Address> .
<http://rdfs.co/juso/Town> <http://www.w3.org/2000/01/rdf-schema#isDefinedBy> <http://rdfs.co/juso/> .
<http://rdfs.co/juso/Province> <http://www.w3.org/2004/02/skos/core#prefLabel> "도"@ko .
<http://www.geonames.org/ontology#name> <http://www.w3.org/2000/01/rdf-schema#subPropertyOf> <http://rdfs.co/juso/name> .
<http://rdfs.co/juso/ThirdLevelAdministrativeDivision> <http://www.w3.org/2004/02/skos/core#definition> "\n    A subdivision of a second-level administrative division.\n    "@en .
<http://rdfs.co/juso/wgs84_lat> <http://www.w3.org/2004/02/skos/core#prefLabel> "latitude (WGS84)"@en .
_:B8944e783X2D91c4X2D4ed8X2Db4ecX2Df633899c71c7 <http://purl.org/dc/dcam/memberOf> <http://purl.org/dc/terms/IMT> .
<http://rdfs.co/juso/postal_code> <http://www.w3.org/1999/02/22-rdf-syntax-ns#type> <http://www.w3.org/2002/07/owl#DatatypeProperty> .
<http://rdfs.co/juso/third_level_administrative_division> <http://www.w3.org/2000/01/rdf-schema#range> <http://rdfs.co/juso/ThirdLevelAdministrativeDivision> .
<http://rdfs.co/juso/0.1.2> <http://www.w3.org/2000/01/rdf-schema#comment> "\n    Most of the descriptions given here are from Wikipedia or from the related\n    ontologies and vocabularies.\n    "@en .
<http://rdfs.co/juso/SecondLevelAdministrativeDivision> <http://purl.org/dc/terms/modified> "2015-10-02+09:00"^^<http://www.w3.org/2001/XMLSchema#date> .
<http://rdfs.co/juso/Geometry> <http://www.w3.org/2000/01/rdf-schema#subClassOf> <http://rdfs.co/juso/SpatialThing> .
<http://rdfs.co/juso/0.1.2> <http://www.w3.org/2004/02/skos/core#changeNote> _:Bdb835a76X2D643fX2D4ba0X2Db7efX2De49279b0f79d .
<http://rdfs.co/juso/County> <http://www.w3.org/2002/07/owl#sameAs> <http://linkedgeodata.org/ontology/County> .
<http://rdfs.co/juso/locator> <http://www.w3.org/2000/01/rdf-schema#isDefinedBy> <http://rdfs.co/juso/> .
<http://rdfs.co/juso/address> <http://purl.org/dc/terms/issued> "2015-10-02+09:00"^^<http://www.w3.org/2001/XMLSchema#date> .
<http://rdfs.co/juso/third_level_administrative_division> <http://purl.org/dc/terms/modified> "2015-10-02+09:00"^^<http://www.w3.org/2001/XMLSchema#date> .
<http://ontology.eil.utoronto.ca/icontact.owl#hasPostalCode> <http://www.w3.org/2002/07/owl#propertyChainAxiom> _:B17925ab7X2D4341X2D48e5X2D86bfX2Dfe59340945bd .
<http://rdfs.co/juso/Geometry> <http://www.w3.org/2002/07/owl#sameAs> <http://geovocab.org/geometry#Geometry> .
<http://rdfs.co/juso/fifth_level_administrative_division> <http://www.w3.org/2003/06/sw-vocab-status/ns#term_status> "unstable"@en .
<http://rdfs.co/juso/fourth_level_administrative_division> <http://www.w3.org/2003/06/sw-vocab-status/ns#term_status> "unstable"@en .
<http://rdfs.co/juso/locator_address> <http://www.w3.org/2004/02/skos/core#prefLabel> "locator address"@en .
<http://rdfs.co/juso/District> <http://www.w3.org/2003/06/sw-vocab-status/ns#term_status> "unstable"@en .
<http://rdfs.co/juso/itrf2000_long> <http://www.w3.org/2004/02/skos/core#prefLabel> "경도(ITRF2000)"@ko .
<http://rdfs.co/juso/Neighborhood> <http://www.w3.org/2004/02/skos/core#definition> "\n    A neighborhood, or neighbourhood, is a geographically localised community\n    within a larger city, town, suburb or rural area.\n    "@en .
<http://listinc.kr/id/listinc> <http://xmlns.com/foaf/0.1/name> "LiST Inc."@en .
<http://rdfs.co/juso/ThirdLevelAdministrativeDivision> <http://purl.org/dc/terms/modified> "2015-10-02+09:00"^^<http://www.w3.org/2001/XMLSchema#date> .
<http://jayg.me/> <http://www.w3.org/2002/07/owl#sameAs> <http://listinc.kr/id/member/jgkim> .
<http://rdfs.co/juso/second_level_administrative_division> <http://www.w3.org/2004/02/skos/core#definition> "\n    The second-level administrative division (locality) of the address, usually\n    a city.\n    "@en .
<http://rdfs.co/juso/PoliticalDivisionGroup> <http://www.w3.org/1999/02/22-rdf-syntax-ns#_9> <http://rdfs.co/juso/FederatedState> .
<http://rdfs.co/juso/Street> <http://purl.org/dc/terms/issued> "2015-10-02+09:00"^^<http://www.w3.org/2001/XMLSchema#date> .
<http://rdfs.co/juso/wgs84_lat> <http://www.w3.org/2000/01/rdf-schema#range> <http://www.w3.org/2001/XMLSchema#string> .
<http://rdfs.co/juso/address> <http://www.w3.org/2000/01/rdf-schema#domain> <http://rdfs.co/juso/SpatialThing> .
<http://rdfs.co/juso/third_level_administrative_division> <http://www.w3.org/1999/02/22-rdf-syntax-ns#type> <http://www.w3.org/2002/07/owl#ObjectProperty> .
<http://rdfs.co/juso/FederatedState> <http://www.w3.org/2003/06/sw-vocab-status/ns#term_status> "unstable"@en .
<http://rdfs.co/juso/FifthLevelAdministrativeDivision> <http://www.w3.org/2000/01/rdf-schema#isDefinedBy> <http://rdfs.co/juso/> .
<http://rdfs.co/juso/Province> <http://www.w3.org/2004/02/skos/core#definition> "\n    A province is almost always an administrative division, within a country or\n    state.\n    "@en .
<http://rdfs.co/juso/Thoroughfare> <http://www.w3.org/2000/01/rdf-schema#seeAlso> <https://en.wikipedia.org/wiki/Thoroughfare> .
<http://rdfs.co/juso/postal_code> <http://www.w3.org/2000/01/rdf-schema#domain> <http://rdfs.co/juso/Address> .
<http://rdfs.co/juso/locator_address> <http://www.w3.org/2000/01/rdf-schema#isDefinedBy> <http://rdfs.co/juso/> .
<http://rdfs.co/juso/Hamlet> <http://www.w3.org/2000/01/rdf-schema#subClassOf> <http://rdfs.co/juso/AdministrativeDivision> .
<http://rdfs.co/juso/Village> <http://www.w3.org/2003/06/sw-vocab-status/ns#term_status> "unstable"@en .
<http://rdfs.co/juso/CoreGroup> <http://www.w3.org/1999/02/22-rdf-syntax-ns#_4> <http://rdfs.co/juso/Point> .
<http://listinc.kr/id/listinc> <http://xmlns.com/foaf/0.1/homepage> <http://li-st.com/> .
<http://rdfs.co/juso/PoliticalDivisionGroup> <http://www.w3.org/1999/02/22-rdf-syntax-ns#_24> <http://rdfs.co/juso/political_division> .
<http://rdfs.co/juso/Feature> <http://purl.org/dc/terms/modified> "2015-10-02+09:00"^^<http://www.w3.org/2001/XMLSchema#date> .
<http://rdfs.co/juso/FourthLevelAdministrativeDivision> <http://purl.org/dc/terms/modified> "2015-10-02+09:00"^^<http://www.w3.org/2001/XMLSchema#date> .
<http://rdfs.co/juso/country> <http://www.w3.org/2002/07/owl#sameAs> <http://ontology.eil.utoronto.ca/icontact.owl#hasCountry> .
<http://rdfs.co/juso/Neighborhood> <http://www.w3.org/2000/01/rdf-schema#isDefinedBy> <http://rdfs.co/juso/> .
<http://rdfs.co/juso/Village> <http://www.w3.org/1999/02/22-rdf-syntax-ns#type> <http://www.w3.org/2002/07/owl#Class> .
<http://rdfs.co/juso/Village> <http://www.w3.org/2002/07/owl#sameAs> <http://linkedgeodata.org/ontology/Village> .
<http://rdfs.co/juso/0.1.2> <http://purl.org/dc/terms/modified> "2015-12-30+09:00"^^<http://www.w3.org/2001/XMLSchema#date> .
<http://rdfs.co/juso/FederatedState> <http://www.w3.org/1999/02/22-rdf-syntax-ns#type> <http://www.w3.org/2002/07/owl#Class> .
<http://rdfs.co/juso/Geometry> <http://www.w3.org/2004/02/skos/core#prefLabel> "기하"@ko .
<http://rdfs.co/juso/thoroughfare_address> <http://www.w3.org/2004/02/skos/core#definition> "\n    This property is used to describe a unique number given to each building\n    (residential or not) or vacant lot with a mailbox in a street or other\n    thoroughfares.\n    "@en .
<http://rdfs.co/juso/SecondLevelAdministrativeDivision> <http://www.w3.org/2000/01/rdf-schema#seeAlso> <http://www.geonames.org/ontology#A.ADM2> .
<http://rdfs.co/juso/Feature> <http://www.w3.org/2000/01/rdf-schema#seeAlso> <https://en.wikipedia.org/wiki/Geographical_feature> .
<http://rdfs.co/juso/FirstLevelAdministrativeDivision> <http://purl.org/dc/terms/issued> "2015-10-02+09:00"^^<http://www.w3.org/2001/XMLSchema#date> .
<http://rdfs.co/juso/PoliticalDivisionGroup> <http://www.w3.org/1999/02/22-rdf-syntax-ns#_7> <http://rdfs.co/juso/FourthLevelAdministrativeDivision> .
<http://rdfs.co/juso/thoroughfare> <http://www.w3.org/2004/02/skos/core#prefLabel> "thoroughfare"@en .
<http://rdfs.co/juso/country> <http://www.w3.org/2003/06/sw-vocab-status/ns#term_status> "unstable"@en .
<http://rdfs.co/juso/0.1.2> <http://purl.org/vocab/vann/preferredNamespacePrefix> "juso" .
<http://rdfs.co/juso/endonym> <http://www.w3.org/2000/01/rdf-schema#subPropertyOf> <http://rdfs.co/juso/name> .
<http://rdfs.co/juso/SpatialThing> <http://purl.org/dc/terms/issued> "2015-10-02+09:00"^^<http://www.w3.org/2001/XMLSchema#date> .
<http://rdfs.co/juso/endonym> <http://www.w3.org/2000/01/rdf-schema#subPropertyOf> <http://www.geonames.org/ontology#officialName> .
<http://rdfs.co/juso/alternate_name> <http://purl.org/dc/terms/modified> "2015-12-30+09:00"^^<http://www.w3.org/2001/XMLSchema#date> .
<http://rdfs.co/juso/PoliticalDivisionGroup> <http://www.w3.org/1999/02/22-rdf-syntax-ns#_25> <http://rdfs.co/juso/parent> .
<http://rdfs.co/juso/District> <http://www.w3.org/1999/02/22-rdf-syntax-ns#type> <http://www.w3.org/2002/07/owl#Class> .
<http://rdfs.co/juso/Province> <http://www.w3.org/1999/02/22-rdf-syntax-ns#type> <http://www.w3.org/2002/07/owl#Class> .
<http://rdfs.co/juso/geometry> <http://www.w3.org/2004/02/skos/core#prefLabel> "geometry"@en .
<http://rdfs.co/juso/name> <http://www.w3.org/2003/06/sw-vocab-status/ns#term_status> "testing"@en .
<http://rdfs.co/juso/City> <http://www.w3.org/2004/02/skos/core#prefLabel> "City"@en .
<http://rdfs.co/juso/PostalCode> <http://www.w3.org/2000/01/rdf-schema#isDefinedBy> <http://rdfs.co/juso/> .
<http://rdfs.co/juso/endonym> <http://www.w3.org/2004/02/skos/core#definition> "\n    The endonym is a name given by members of a particular ethnolinguistic\n    group to its homeland or a specific place within it.\n    "@en .
<http://rdfs.co/juso/Geometry> <http://www.w3.org/2000/01/rdf-schema#isDefinedBy> <http://rdfs.co/juso/> .
<http://rdfs.co/juso/City> <http://www.w3.org/2002/07/owl#sameAs> <http://linkedgeodata.org/ontology/City> .
<http://rdfs.co/juso/first_level_administrative_division> <http://www.w3.org/2000/01/rdf-schema#range> <http://rdfs.co/juso/FirstLevelAdministrativeDivision> .
<http://rdfs.co/juso/second_level_administrative_division> <http://www.w3.org/2000/01/rdf-schema#isDefinedBy> <http://rdfs.co/juso/> .
<http://listinc.kr/id/listinc> <http://www.w3.org/1999/02/22-rdf-syntax-ns#type> <http://xmlns.com/foaf/0.1/Organization> .
<http://rdfs.co/juso/0.1.2> <http://purl.org/dc/terms/isVersionOf> <http://rdfs.co/juso/> .
<http://rdfs.co/juso/second_level_administrative_division> <http://www.w3.org/2000/01/rdf-schema#range> <http://rdfs.co/juso/SecondLevelAdministrativeDivision> .
_:Bde26aa6aX2D2065X2D4c51X2D8013X2D4cef3dacf87c <http://www.w3.org/1999/02/22-rdf-syntax-ns#first> <http://www.w3.org/1999/02/22-rdf-syntax-ns#value> .
<http://rdfs.co/juso/CoreGroup> <http://www.w3.org/1999/02/22-rdf-syntax-ns#_2> <http://rdfs.co/juso/Feature> .
<http://rdfs.co/juso/PoliticalDivisionGroup> <http://www.w3.org/1999/02/22-rdf-syntax-ns#_19> <http://rdfs.co/juso/Town> .
<http://rdfs.co/juso/parent> <http://www.w3.org/1999/02/22-rdf-syntax-ns#type> <http://www.w3.org/2002/07/owl#ObjectProperty> .
<http://jayg.me/> <http://www.w3.org/ns/org#memberOf> <http://listinc.kr/id/listinc> .
<http://rdfs.co/juso/fourth_level_administrative_division> <http://www.w3.org/2004/02/skos/core#prefLabel> "fourth-level administrative division"@en .
<http://rdfs.co/juso/0.1.2> <http://purl.org/dc/terms/rights> "Copyright © 2015 LiST Inc. Some Rights Reserved." .
<http://rdfs.co/juso/exonym> <http://www.w3.org/2003/06/sw-vocab-status/ns#term_status> "unstable"@en .
<http://rdfs.co/juso/ConsolidatedCityCounty> <http://www.w3.org/2000/01/rdf-schema#seeAlso> <https://en.wikipedia.org/wiki/Consolidated_city-county> .
<http://rdfs.co/juso/full_address> <http://www.w3.org/1999/02/22-rdf-syntax-ns#type> <http://www.w3.org/2002/07/owl#DatatypeProperty> .
<http://rdfs.co/juso/0.1.2> <http://www.w3.org/1999/02/22-rdf-syntax-ns#type> <http://purl.org/vocommons/voaf#Vocabulary> .
_:Bde26aa6aX2D2065X2D4c51X2D8013X2D4cef3dacf87c <http://www.w3.org/1999/02/22-rdf-syntax-ns#rest> <http://www.w3.org/1999/02/22-rdf-syntax-ns#nil> .
<http://rdfs.co/juso/Municipality> <http://www.w3.org/2004/02/skos/core#prefLabel> "Municipality"@en .
<http://rdfs.co/juso/0.1.2> <http://www.w3.org/2004/02/skos/core#historyNote> _:B68a7b51bX2Dfa3dX2D4d94X2Dadc1X2D2be21cdb7d78 .
<http://rdfs.co/juso/wgs84_lat> <http://www.w3.org/2004/02/skos/core#prefLabel> "위도(WGS84)"@ko .
<http://rdfs.co/juso/Point> <http://www.w3.org/2000/01/rdf-schema#isDefinedBy> <http://rdfs.co/juso/> .
<http://rdfs.co/juso/CoreGroup> <http://www.w3.org/1999/02/22-rdf-syntax-ns#_11> <http://rdfs.co/juso/endonym> .
<http://rdfs.co/juso/FederatedState> <http://www.w3.org/2004/02/skos/core#altLabel> "주"@ko .
<http://rdfs.co/juso/Country> <http://purl.org/dc/terms/modified> "2015-10-02+09:00"^^<http://www.w3.org/2001/XMLSchema#date> .
<http://rdfs.co/juso/wgs84_long> <http://www.w3.org/2004/02/skos/core#definition> "\n    The WGS84 longitude of a point (decimal degrees).\n    "@en .
<http://rdfs.co/juso/address> <http://www.w3.org/2003/06/sw-vocab-status/ns#term_status> "unstable"@en .
<http://rdfs.co/juso/post_office_box> <http://www.w3.org/1999/02/22-rdf-syntax-ns#type> <http://www.w3.org/2002/07/owl#DatatypeProperty> .
<http://rdfs.co/juso/PostalCode> <http://www.w3.org/2004/02/skos/core#altLabel> "Eircode"@en .
<http://rdfs.co/juso/Parish> <http://www.w3.org/2000/01/rdf-schema#subClassOf> <http://rdfs.co/juso/AdministrativeDivision> .
<http://rdfs.co/juso/wgs84_long> <http://www.w3.org/2000/01/rdf-schema#range> <http://www.w3.org/2001/XMLSchema#string> .
<http://rdfs.co/juso/thoroughfare_address> <http://www.w3.org/2000/01/rdf-schema#range> <http://www.w3.org/2001/XMLSchema#string> .
<http://rdfs.co/juso/endonym> <http://www.w3.org/1999/02/22-rdf-syntax-ns#type> <http://www.w3.org/2002/07/owl#DatatypeProperty> .
<http://rdfs.co/juso/official_name> <http://www.w3.org/2000/01/rdf-schema#range> <http://www.w3.org/2001/XMLSchema#string> .
_:B7af76555X2D95fbX2D4024X2Da653X2D1ecbadf9e9c2 <http://purl.org/dc/terms/date> "2015-11-10+09:00"^^<http://www.w3.org/2001/XMLSchema#date> .
<http://rdfs.co/juso/full_address> <http://www.w3.org/2004/02/skos/core#prefLabel> "full address"@en .
<http://rdfs.co/juso/Point> <http://purl.org/dc/terms/modified> "2015-11-10+09:00"^^<http://www.w3.org/2001/XMLSchema#date> .
<http://rdfs.co/juso/0.1.2/html> <http://purl.org/dc/terms/format> _:B5f94f7eeX2D87b3X2D4b12X2D952fX2D2915101e3e3b .
<http://rdfs.co/juso/Province> <http://www.w3.org/2003/06/sw-vocab-status/ns#term_status> "unstable"@en .
<http://rdfs.co/juso/FourthLevelAdministrativeDivision> <http://www.w3.org/2004/02/skos/core#definition> "\n    A subdivision of a third-level administrative division.\n    "@en .
<http://rdfs.co/juso/endonym> <http://www.w3.org/2000/01/rdf-schema#subPropertyOf> <http://www.w3.org/2004/02/skos/core#prefLabel> .
<http://rdfs.co/juso/itrf2000_long> <http://purl.org/dc/terms/issued> "2015-11-10+09:00"^^<http://www.w3.org/2001/XMLSchema#date> .
<http://rdfs.co/juso/post_office_box> <http://www.w3.org/2000/01/rdf-schema#domain> <http://rdfs.co/juso/Address> .
<http://rdfs.co/juso/Street> <http://www.w3.org/2003/06/sw-vocab-status/ns#term_status> "unstable"@en .
<http://rdfs.co/juso/fifth_level_administrative_division> <http://www.w3.org/2000/01/rdf-schema#range> <http://rdfs.co/juso/FifthLevelAdministrativeDivision> .
<http://rdfs.co/juso/PoliticalDivision> <http://www.w3.org/2000/01/rdf-schema#seeAlso> <https://en.wikipedia.org/wiki/Political_division> .
<http://rdfs.co/juso/FederatedState> <http://purl.org/dc/terms/issued> "2015-10-02+09:00"^^<http://www.w3.org/2001/XMLSchema#date> .
<http://rdfs.co/juso/country> <http://www.w3.org/2000/01/rdf-schema#range> <http://rdfs.co/juso/Country> .
_:B8944e783X2D91c4X2D4ed8X2Db4ecX2Df633899c71c7 <http://www.w3.org/1999/02/22-rdf-syntax-ns#type> <http://purl.org/dc/terms/MediaType> .
<http://rdfs.co/juso/itrf2000_long> <http://www.w3.org/1999/02/22-rdf-syntax-ns#type> <http://www.w3.org/2002/07/owl#DatatypeProperty> .
<http://rdfs.co/juso/0.1.2> <http://purl.org/vocab/vann/example> _:Be368c69eX2Dace7X2D4a9dX2D82a8X2Dae90ab3c5611 .
<http://rdfs.co/juso/short_name> <http://www.w3.org/1999/02/22-rdf-syntax-ns#type> <http://www.w3.org/2002/07/owl#DatatypeProperty> .
<http://rdfs.co/juso/PoliticalDivisionGroup> <http://www.w3.org/1999/02/22-rdf-syntax-ns#_14> <http://rdfs.co/juso/CapitalDistrict> .
<http://rdfs.co/juso/Village> <http://purl.org/dc/terms/issued> "2015-10-02+09:00"^^<http://www.w3.org/2001/XMLSchema#date> .
<http://rdfs.co/juso/AdministrativeDivision> <http://www.w3.org/2000/01/rdf-schema#isDefinedBy> <http://rdfs.co/juso/> .
<http://rdfs.co/juso/AdministrativeDivision> <http://www.w3.org/2000/01/rdf-schema#subClassOf> <http://rdfs.co/juso/PoliticalDivision> .
<http://rdfs.co/juso/Parish> <http://www.w3.org/2004/02/skos/core#altLabel> "Civil Parish"@en-gb .
<http://rdfs.co/juso/fifth_level_administrative_division> <http://purl.org/dc/terms/issued> "2015-10-02+09:00"^^<http://www.w3.org/2001/XMLSchema#date> .
_:B5f94f7eeX2D87b3X2D4b12X2D952fX2D2915101e3e3b <http://www.w3.org/1999/02/22-rdf-syntax-ns#type> <http://purl.org/dc/terms/MediaType> .
<http://rdfs.co/juso/SpatialThing> <http://www.w3.org/1999/02/22-rdf-syntax-ns#type> <http://www.w3.org/2002/07/owl#Class> .
<http://rdfs.co/juso/Village> <http://www.w3.org/2004/02/skos/core#definition> "\n    A village is a clustered human settlement or community, larger than a\n    hamlet but smaller than a town, with a population ranging from a few\n    hundred to a few thousand.\n    "@en .
<http://rdfs.co/juso/fourth_level_administrative_division> <http://purl.org/dc/terms/issued> "2015-10-02+09:00"^^<http://www.w3.org/2001/XMLSchema#date> .
<http://rdfs.co/juso/District> <http://purl.org/dc/terms/issued> "2015-10-02+09:00"^^<http://www.w3.org/2001/XMLSchema#date> .
<http://rdfs.co/juso/within> <http://www.w3.org/2000/01/rdf-schema#isDefinedBy> <http://rdfs.co/juso/> .
_:B68a7b51bX2Dfa3dX2D4d94X2Dadc1X2D2be21cdb7d78 <http://www.w3.org/1999/02/22-rdf-syntax-ns#value> "\n      Added juso:official_name, juso:alternate_name, juso:short_name\n      "@en .
<http://rdfs.co/juso/address> <http://www.w3.org/2000/01/rdf-schema#subPropertyOf> <http://www.w3.org/ns/locn#address> .
<http://rdfs.co/juso/FirstLevelAdministrativeDivision> <http://www.w3.org/1999/02/22-rdf-syntax-ns#type> <http://www.w3.org/2002/07/owl#Class> .
<http://rdfs.co/juso/name> <http://purl.org/dc/terms/modified> "2015-10-02+09:00"^^<http://www.w3.org/2001/XMLSchema#date> .
<http://rdfs.co/juso/County> <http://www.w3.org/2000/01/rdf-schema#subClassOf> <http://rdfs.co/juso/AdministrativeDivision> .
<http://rdfs.co/juso/first_level_administrative_division> <http://www.w3.org/2000/01/rdf-schema#domain> <http://rdfs.co/juso/Address> .
<http://rdfs.co/juso/wgs84_lat> <http://purl.org/dc/terms/modified> "2015-11-10+09:00"^^<http://www.w3.org/2001/XMLSchema#date> .
<http://rdfs.co/juso/FirstLevelAdministrativeDivision> <http://www.w3.org/2003/06/sw-vocab-status/ns#term_status> "unstable"@en .
<http://rdfs.co/juso/FourthLevelAdministrativeDivision> <http://www.w3.org/2004/02/skos/core#altLabel> "Fourth-order Administrative Division"@en .
_:B5f94f7eeX2D87b3X2D4b12X2D952fX2D2915101e3e3b <http://www.w3.org/2000/01/rdf-schema#label> "HTML"@en .
<http://rdfs.co/juso/PoliticalDivisionGroup> <http://www.w3.org/1999/02/22-rdf-syntax-ns#_6> <http://rdfs.co/juso/ThirdLevelAdministrativeDivision> .
<http://rdfs.co/juso/country> <http://purl.org/dc/terms/issued> "2015-10-02+09:00"^^<http://www.w3.org/2001/XMLSchema#date> .
_:Be368c69eX2Dace7X2D4a9dX2D82a8X2Dae90ab3c5611 <http://www.w3.org/2000/01/rdf-schema#label> "LiST Inc."@en .
<http://rdfs.co/juso/wgs84_lat> <http://www.w3.org/2000/01/rdf-schema#domain> <http://rdfs.co/juso/Point> .
<http://rdfs.co/juso/itrf2000_lat> <http://www.w3.org/2004/02/skos/core#prefLabel> "latitude (ITRF2000)"@en .
<http://rdfs.co/juso/postal_code> <http://www.w3.org/2004/02/skos/core#definition> "\n    This property associates any address with its postal code.\n    "@en .
<http://rdfs.co/juso/exonym> <http://www.w3.org/2000/01/rdf-schema#subPropertyOf> <http://www.w3.org/2004/02/skos/core#altLabel> .
<http://rdfs.co/juso/Municipality> <http://www.w3.org/2000/01/rdf-schema#isDefinedBy> <http://rdfs.co/juso/> .
<http://rdfs.co/juso/locator_address> <http://www.w3.org/2000/01/rdf-schema#range> <http://www.w3.org/2001/XMLSchema#string> .
<http://rdfs.co/juso/CoreGroup> <http://www.w3.org/1999/02/22-rdf-syntax-ns#_3> <http://rdfs.co/juso/Geometry> .
<http://rdfs.co/juso/geometry> <http://www.w3.org/2000/01/rdf-schema#isDefinedBy> <http://rdfs.co/juso/> .
<http://rdfs.co/juso/thoroughfare> <http://www.w3.org/2000/01/rdf-schema#domain> <http://rdfs.co/juso/Address> .
<http://rdfs.co/juso/AddressGroup> <http://www.w3.org/1999/02/22-rdf-syntax-ns#type> <http://www.w3.org/1999/02/22-rdf-syntax-ns#Bag> .
<http://rdfs.co/juso/full_address> <http://www.w3.org/2000/01/rdf-schema#domain> <http://rdfs.co/juso/Address> .
<http://rdfs.co/juso/Street> <http://www.w3.org/1999/02/22-rdf-syntax-ns#type> <http://www.w3.org/2002/07/owl#Class> .
<http://rdfs.co/juso/short_name> <http://www.w3.org/2004/02/skos/core#prefLabel> "짧은 이름"@ko .
<http://rdfs.co/juso/0.1.2> <http://purl.org/vocab/vann/termGroup> <http://rdfs.co/juso/AddressGroup> .
<http://rdfs.co/juso/FederatedState> <http://www.w3.org/2000/01/rdf-schema#subClassOf> <http://schema.org/State> .
<http://rdfs.co/juso/parent> <http://purl.org/dc/terms/modified> "2015-10-02+09:00"^^<http://www.w3.org/2001/XMLSchema#date> .
<http://rdfs.co/juso/wgs84_lat> <http://www.w3.org/2000/01/rdf-schema#isDefinedBy> <http://rdfs.co/juso/> .
<http://rdfs.co/juso/PoliticalDivision> <http://purl.org/dc/terms/modified> "2015-10-02+09:00"^^<http://www.w3.org/2001/XMLSchema#date> .
<http://www.w3.org/2006/vcard/ns#Address> <http://www.w3.org/2000/01/rdf-schema#subClassOf> <http://rdfs.co/juso/Address> .
