<http://ns.inria.fr/l4lod/v2#Reproduction>
        a       <http://www.w3.org/2002/07/owl#Class> ;
        <http://www.w3.org/2000/01/rdf-schema#comment>
                "This class is used to express the permission of making multiple copies of the licensed data."@en ;
        <http://www.w3.org/2000/01/rdf-schema#isDefinedBy>
                <http://ns.inria.fr/l4lod/v2#> ;
        <http://www.w3.org/2000/01/rdf-schema#label>
                "Reproduction"@en ;
        <http://www.w3.org/2000/01/rdf-schema#subClassOf>
                <limo:UseConditions> , <http://ns.inria.fr/l4lod/v2#Permission> ;
        <http://www.w3.org/2003/06/sw-vocab-status/ns#term_status>
                "stable" ;
        <http://www.w3.org/2004/02/skos/core#related>
                <cc:Reproduction> .

<http://ns.inria.fr/l4lod/v2>
        a       <http://www.w3.org/2002/07/owl#Ontology> ;
        <http://creativecommons.org/ns#license>
                <http://creativecommons.org/licenses/by/3.0/> ;
        <http://purl.org/dc/elements/1.1/description>
                "A vocabulary to describe the licensing terms associated to linked open data."@en ;
        <http://purl.org/dc/elements/1.1/issued>
                "2013-05-10"^^<http://www.w3.org/2001/XMLSchema#date> ;
        <http://purl.org/dc/elements/1.1/publisher>
                <http://dbpedia.org/resource/National_Institute_for_Research_in_Computer_Science_and_Control> ;
        <http://purl.org/dc/elements/1.1/title>
                "Licences for Linked Open Data (L4LOD) Ontology"@en ;
        <http://purl.org/vocab/vann/preferredNamespacePrefix>
                "" ;
        <http://purl.org/vocab/vann/preferredNamespaceUri>
                "http://ns.inria.fr/l4lod/v2#" ;
        <http://www.w3.org/2002/07/owl#versionInfo>
                0.2 ;
        <http://xmlns.com/foaf/0.1/page>
                <http://ns.inria.fr/l4lod/v1/l4lod_v2.html> .

<http://ns.inria.fr/l4lod/v2#Sharing>
        a       <http://www.w3.org/2002/07/owl#Class> ;
        <http://www.w3.org/2000/01/rdf-schema#comment>
                "This class is used to express the permission to copy, distribute and use the licensed data."@en ;
        <http://www.w3.org/2000/01/rdf-schema#isDefinedBy>
                <http://ns.inria.fr/l4lod/v2#> ;
        <http://www.w3.org/2000/01/rdf-schema#label>
                "Sharing"@en ;
        <http://www.w3.org/2000/01/rdf-schema#subClassOf>
                <limo:Rights> , <http://ns.inria.fr/l4lod/v2#Permission> ;
        <http://www.w3.org/2003/06/sw-vocab-status/ns#term_status>
                "stable" ;
        <http://www.w3.org/2004/02/skos/core#related>
                <cc:Sharing> .

<http://ns.inria.fr/l4lod/v2#CommercialExpl>
        a       <http://www.w3.org/2002/07/owl#Class> ;
        <http://www.w3.org/2000/01/rdf-schema#comment>
                "This class is used to express the permission to commercially exploit the licensed data."@en ;
        <http://www.w3.org/2000/01/rdf-schema#isDefinedBy>
                <http://ns.inria.fr/l4lod/v2#> ;
        <http://www.w3.org/2000/01/rdf-schema#label>
                "CommercialExpl"@en ;
        <http://www.w3.org/2000/01/rdf-schema#subClassOf>
                <limo:DistributionConditions> , <http://ns.inria.fr/l4lod/v2#Permission> ;
        <http://www.w3.org/2003/06/sw-vocab-status/ns#term_status>
                "stable" .

<http://ns.inria.fr/l4lod/v2#License>
        a       <http://www.w3.org/2002/07/owl#Class> ;
        <http://www.w3.org/2000/01/rdf-schema#comment>
                "A license is a set of prohibitions, permissions and obligations."@en ;
        <http://www.w3.org/2000/01/rdf-schema#isDefinedBy>
                <http://ns.inria.fr/l4lod/v2#> ;
        <http://www.w3.org/2000/01/rdf-schema#label>
                "License"@en ;
        <http://www.w3.org/2002/07/owl#equivalentClass>
                <limo:LicenseModel> , <cc:License> ;
        <http://www.w3.org/2003/06/sw-vocab-status/ns#term_status>
                "stable" ;
        <http://www.w3.org/2004/02/skos/core#exactMatch>
                <http://eurovoc.europa.eu/259007> ;
        <http://www.w3.org/2004/02/skos/core#related>
                <gr:License> , <omv:LicenseModel> , <voag:LicenseModel> , <premis:LicenseInformation> , <meb:License> .

<http://ns.inria.fr/l4lod/v2#ShareAlike>
        a       <http://www.w3.org/2002/07/owl#Class> ;
        <http://www.w3.org/2000/01/rdf-schema#comment>
                "This class is used to express the obligation of for the derivative works be licensed under the same terms of the licensed data."@en ;
        <http://www.w3.org/2000/01/rdf-schema#isDefinedBy>
                <http://ns.inria.fr/l4lod/v2#> ;
        <http://www.w3.org/2000/01/rdf-schema#label>
                "ShareAlike"@en ;
        <http://www.w3.org/2000/01/rdf-schema#subClassOf>
                <limo:DistributionConditions> , <http://ns.inria.fr/l4lod/v2#Obligation> ;
        <http://www.w3.org/2003/06/sw-vocab-status/ns#term_status>
                "stable" ;
        <http://www.w3.org/2004/02/skos/core#related>
                <cc:ShareAlike> .

<http://ns.inria.fr/l4lod/v2#Distribution>
        a       <http://www.w3.org/2002/07/owl#Class> ;
        <http://www.w3.org/2000/01/rdf-schema#comment>
                "This class is used to express the permission to distribute the licensed data."@en ;
        <http://www.w3.org/2000/01/rdf-schema#isDefinedBy>
                <http://ns.inria.fr/l4lod/v2#> ;
        <http://www.w3.org/2000/01/rdf-schema#label>
                "Distribution"@en ;
        <http://www.w3.org/2000/01/rdf-schema#subClassOf>
                <limo:DistributionConditions> , <http://ns.inria.fr/l4lod/v2#Permission> ;
        <http://www.w3.org/2003/06/sw-vocab-status/ns#term_status>
                "stable" ;
        <http://www.w3.org/2004/02/skos/core#related>
                <cc:Distribution> .

<http://ns.inria.fr/l4lod/v2#Derivative>
        a       <http://www.w3.org/2002/07/owl#Class> ;
        <http://www.w3.org/2000/01/rdf-schema#comment>
                "This class is used to express the permission to distribute derivative works from the licensed data."@en ;
        <http://www.w3.org/2000/01/rdf-schema#isDefinedBy>
                <http://ns.inria.fr/l4lod/v2#> ;
        <http://www.w3.org/2000/01/rdf-schema#label>
                "Derivative"@en ;
        <http://www.w3.org/2000/01/rdf-schema#subClassOf>
                <limo:DistributionConditions> , <http://ns.inria.fr/l4lod/v2#Permission> ;
        <http://www.w3.org/2003/06/sw-vocab-status/ns#term_status>
                "stable" ;
        <http://www.w3.org/2004/02/skos/core#related>
                <cc:DerivativeWorks> .

<http://ns.inria.fr/l4lod/v2#permits>
        a       <http://www.w3.org/2002/07/owl#ObjectProperty> ;
        <http://www.w3.org/2000/01/rdf-schema#comment>
                "The property defines the permissions associated to the license."@en ;
        <http://www.w3.org/2000/01/rdf-schema#domain>
                <http://ns.inria.fr/l4lod/v2#License> ;
        <http://www.w3.org/2000/01/rdf-schema#isDefinedBy>
                <http://ns.inria.fr/l4lod/v2#> ;
        <http://www.w3.org/2000/01/rdf-schema#label>
                "permits"@en ;
        <http://www.w3.org/2000/01/rdf-schema#range>
                <http://ns.inria.fr/l4lod/v2#Permission> ;
        <http://www.w3.org/2003/06/sw-vocab-status/ns#term_status>
                "stable" ;
        <http://www.w3.org/2004/02/skos/core#exactMatch>
                <o:permission> .

<http://ns.inria.fr/l4lod/v2#prohibits>
        a       <http://www.w3.org/2002/07/owl#ObjectProperty> ;
        <http://www.w3.org/2000/01/rdf-schema#comment>
                "The property defines the prohibitions associated to the license."@en ;
        <http://www.w3.org/2000/01/rdf-schema#domain>
                <http://ns.inria.fr/l4lod/v2#License> ;
        <http://www.w3.org/2000/01/rdf-schema#isDefinedBy>
                <http://ns.inria.fr/l4lod/v2#> ;
        <http://www.w3.org/2000/01/rdf-schema#label>
                "prohibits"@en ;
        <http://www.w3.org/2000/01/rdf-schema#range>
                <http://ns.inria.fr/l4lod/v2#Prohibition> ;
        <http://www.w3.org/2003/06/sw-vocab-status/ns#term_status>
                "stable" ;
        <http://www.w3.org/2004/02/skos/core#exactMatch>
                <o:prohibition> .

<http://ns.inria.fr/l4lod/v2#Publishing>
        a       <http://www.w3.org/2002/07/owl#Class> ;
        <http://www.w3.org/2000/01/rdf-schema#comment>
                "This class is used to express the permission to publish the licensed data."@en ;
        <http://www.w3.org/2000/01/rdf-schema#isDefinedBy>
                <http://ns.inria.fr/l4lod/v2#> ;
        <http://www.w3.org/2000/01/rdf-schema#label>
                "Publishing"@en ;
        <http://www.w3.org/2000/01/rdf-schema#subClassOf>
                <limo:UseConditions> , <http://ns.inria.fr/l4lod/v2#Permission> ;
        <http://www.w3.org/2003/06/sw-vocab-status/ns#term_status>
                "stable" .

<http://ns.inria.fr/l4lod/v2#NoCommercial>
        a       <http://www.w3.org/2002/07/owl#Class> ;
        <http://www.w3.org/2000/01/rdf-schema#comment>
                "The class is used to express the prohibition of commercial use of the licensed data."@en ;
        <http://www.w3.org/2000/01/rdf-schema#isDefinedBy>
                <http://ns.inria.fr/l4lod/v2#> ;
        <http://www.w3.org/2000/01/rdf-schema#label>
                "NoCommercial"@en ;
        <http://www.w3.org/2000/01/rdf-schema#subClassOf>
                <limo:UseConditions> , <http://ns.inria.fr/l4lod/v2#Prohibition> ;
        <http://www.w3.org/2003/06/sw-vocab-status/ns#term_status>
                "stable" ;
        <http://www.w3.org/2004/02/skos/core#related>
                <cc:CommercialUse> .

<http://ns.inria.fr/l4lod/v2#Obligation>
        a       <http://www.w3.org/2002/07/owl#Class> ;
        <http://www.w3.org/2000/01/rdf-schema#comment>
                "The class is used to express the obligations associated to the licensed data."@en ;
        <http://www.w3.org/2000/01/rdf-schema#isDefinedBy>
                <http://ns.inria.fr/l4lod/v2#> ;
        <http://www.w3.org/2000/01/rdf-schema#label>
                "Obligation"@en ;
        <http://www.w3.org/2000/01/rdf-schema#subClassOf>
                <limo:LegalTerms> ;
        <http://www.w3.org/2003/06/sw-vocab-status/ns#term_status>
                "stable" ;
        <http://www.w3.org/2004/02/skos/core#exactMatch>
                <cc:Requirement> , <o:Duty> .

<http://ns.inria.fr/l4lod/v2#Attribution>
        a       <http://www.w3.org/2002/07/owl#Class> ;
        <http://www.w3.org/2000/01/rdf-schema#comment>
                "This class is used to express the obligation of attribution to author of the licensed data."@en ;
        <http://www.w3.org/2000/01/rdf-schema#isDefinedBy>
                <http://ns.inria.fr/l4lod/v2#> ;
        <http://www.w3.org/2000/01/rdf-schema#label>
                "Attribution"@en ;
        <http://www.w3.org/2000/01/rdf-schema#subClassOf>
                <limo:DistributionConditions> , <http://ns.inria.fr/l4lod/v2#Obligation> ;
        <http://www.w3.org/2003/06/sw-vocab-status/ns#term_status>
                "stable" ;
        <http://www.w3.org/2004/02/skos/core#related>
                <cc:Attribution> .

<http://ns.inria.fr/l4lod/v2#Citation>
        a       <http://www.w3.org/2002/07/owl#Class> ;
        <http://www.w3.org/2000/01/rdf-schema#comment>
                "This class is used to express the obligation of citation of the licensed data."@en ;
        <http://www.w3.org/2000/01/rdf-schema#isDefinedBy>
                <http://ns.inria.fr/l4lod/v2#> ;
        <http://www.w3.org/2000/01/rdf-schema#label>
                "Citation"@en ;
        <http://www.w3.org/2000/01/rdf-schema#subClassOf>
                <http://ns.inria.fr/l4lod/v2#Obligation> , <limo:DistributionConditions> ;
        <http://www.w3.org/2003/06/sw-vocab-status/ns#term_status>
                "stable" .

<http://ns.inria.fr/l4lod/v2#licensor>
        a       <http://www.w3.org/2002/07/owl#ObjectProperty> ;
        <http://www.w3.org/2000/01/rdf-schema#comment>
                "This property associates the License to issuer of the license."@en ;
        <http://www.w3.org/2000/01/rdf-schema#domain>
                <http://ns.inria.fr/l4lod/v2#License> ;
        <http://www.w3.org/2000/01/rdf-schema#isDefinedBy>
                <http://ns.inria.fr/l4lod/v2#> ;
        <http://www.w3.org/2000/01/rdf-schema#label>
                "licensor"@en ;
        <http://www.w3.org/2000/01/rdf-schema#range>
                <http://www.w3.org/2000/01/rdf-schema#Literal> ;
        <http://www.w3.org/2003/06/sw-vocab-status/ns#term_status>
                "stable" ;
        <http://www.w3.org/2004/02/skos/core#related>
                <limo:creator> , <odrl:assigner> .

<http://ns.inria.fr/l4lod/v2#licensingTerms>
        a       <http://www.w3.org/2002/07/owl#ObjectProperty> ;
        <http://www.w3.org/2000/01/rdf-schema#comment>
                "This property associates the License to the URI of the human-readable text describing the license."@en ;
        <http://www.w3.org/2000/01/rdf-schema#domain>
                <http://ns.inria.fr/l4lod/v2#License> ;
        <http://www.w3.org/2000/01/rdf-schema#isDefinedBy>
                <http://ns.inria.fr/l4lod/v2#> ;
        <http://www.w3.org/2000/01/rdf-schema#label>
                "licensingTerms"@en ;
        <http://www.w3.org/2000/01/rdf-schema#range>
                <dcterms:LicenseDocument> ;
        <http://www.w3.org/2003/06/sw-vocab-status/ns#term_status>
                "stable" ;
        <http://www.w3.org/2004/02/skos/core#related>
                <waiver:declaration> , <cc:legalCode> , <nie:licenseType> , <premis:licenseTerms> .

<http://ns.inria.fr/l4lod/v2#Prohibition>
        a       <http://www.w3.org/2002/07/owl#Class> ;
        <http://www.w3.org/2000/01/rdf-schema#comment>
                "The class is used to express the prohibitions associated to the licensed data."@en ;
        <http://www.w3.org/2000/01/rdf-schema#isDefinedBy>
                <http://ns.inria.fr/l4lod/v2#> ;
        <http://www.w3.org/2000/01/rdf-schema#label>
                "Prohibition"@en ;
        <http://www.w3.org/2000/01/rdf-schema#subClassOf>
                <limo:LegalTerms> ;
        <http://www.w3.org/2003/06/sw-vocab-status/ns#term_status>
                "stable" ;
        <http://www.w3.org/2004/02/skos/core#exactMatch>
                <cc:Prohibition> , <o:Prohibition> .

<http://ns.inria.fr/l4lod/v2#NoDerivative>
        a       <http://www.w3.org/2002/07/owl#Class> ;
        <http://www.w3.org/2000/01/rdf-schema#comment>
                "The class is used to express the prohibition of producing derivative work of the licensed data."@en ;
        <http://www.w3.org/2000/01/rdf-schema#isDefinedBy>
                <http://ns.inria.fr/l4lod/v2#> ;
        <http://www.w3.org/2000/01/rdf-schema#label>
                "NoDerivative"@en ;
        <http://www.w3.org/2000/01/rdf-schema#subClassOf>
                <http://ns.inria.fr/l4lod/v2#Prohibition> , <limo:UseConditions> ;
        <http://www.w3.org/2003/06/sw-vocab-status/ns#term_status>
                "stable" .

<http://ns.inria.fr/l4lod/v2#Using>
        a       <http://www.w3.org/2002/07/owl#Class> ;
        <http://www.w3.org/2000/01/rdf-schema#comment>
                "This class is used to express the permission to use the licensed data."@en ;
        <http://www.w3.org/2000/01/rdf-schema#isDefinedBy>
                <http://ns.inria.fr/l4lod/v2#> ;
        <http://www.w3.org/2000/01/rdf-schema#label>
                "Using"@en ;
        <http://www.w3.org/2000/01/rdf-schema#subClassOf>
                <http://ns.inria.fr/l4lod/v2#Permission> , <limo:UseConditions> ;
        <http://www.w3.org/2003/06/sw-vocab-status/ns#term_status>
                "stable" .

<http://ns.inria.fr/l4lod/v2#Permission>
        a       <http://www.w3.org/2002/07/owl#Class> ;
        <http://www.w3.org/2000/01/rdf-schema#comment>
                "The class is used to express the permissions associated to the licensed data."@en ;
        <http://www.w3.org/2000/01/rdf-schema#isDefinedBy>
                <http://ns.inria.fr/l4lod/v2#> ;
        <http://www.w3.org/2000/01/rdf-schema#label>
                "Permission"@en ;
        <http://www.w3.org/2000/01/rdf-schema#subClassOf>
                <limo:LegalTerms> ;
        <http://www.w3.org/2003/06/sw-vocab-status/ns#term_status>
                "stable" ;
        <http://www.w3.org/2004/02/skos/core#exactMatch>
                <cc:Permission> , <o:Permission> .

<http://ns.inria.fr/l4lod/v2#obliges>
        a       <http://www.w3.org/2002/07/owl#ObjectProperty> ;
        <http://www.w3.org/2000/01/rdf-schema#comment>
                "The property defines the obligations associated to the license."@en ;
        <http://www.w3.org/2000/01/rdf-schema#domain>
                <http://ns.inria.fr/l4lod/v2#License> ;
        <http://www.w3.org/2000/01/rdf-schema#isDefinedBy>
                <http://ns.inria.fr/l4lod/v2#> ;
        <http://www.w3.org/2000/01/rdf-schema#label>
                "obliges"@en ;
        <http://www.w3.org/2000/01/rdf-schema#range>
                <http://ns.inria.fr/l4lod/v2#Obligation> ;
        <http://www.w3.org/2003/06/sw-vocab-status/ns#term_status>
                "stable" ;
        <http://www.w3.org/2004/02/skos/core#exactMatch>
                <o:duty> .

<http://dbpedia.org/resource/National_Institute_for_Research_in_Computer_Science_and_Control>
        a       <http://xmlns.com/foaf/0.1/Organization> .
