<http://lemon-model.net/lemon#semArg>
        a       <http://www.w3.org/1999/02/22-rdf-syntax-ns#Property> , <http://www.w3.org/2002/07/owl#ObjectProperty> ;
        <http://www.w3.org/2000/01/rdf-schema#comment>
                "Denotes a semantic argument slot of a semantic unit"@en ;
        <http://www.w3.org/2000/01/rdf-schema#domain>
                <http://lemon-model.net/lemon#LexicalSense> ;
        <http://www.w3.org/2000/01/rdf-schema#label>
                "Actant sémantique"@fr , "Semantische Argument"@de , "Semantic argument"@en , "Argumento semántico"@es , "Semantisch argument"@nl ;
        <http://www.w3.org/2000/01/rdf-schema#range>
                <http://lemon-model.net/lemon#Argument> .

<http://lemon-model.net/lemon#propertyRange>
        a       <http://www.w3.org/1999/02/22-rdf-syntax-ns#Property> , <http://www.w3.org/2002/07/owl#ObjectProperty> ;
        <http://www.w3.org/2000/01/rdf-schema#comment>
                "Indicates a restrictions on the range of the property. That is, this sense only applies if the property the sense refers to has a object in the class referred to by this property"@en ;
        <http://www.w3.org/2000/01/rdf-schema#domain>
                <http://lemon-model.net/lemon#LexicalSense> ;
        <http://www.w3.org/2000/01/rdf-schema#label>
                "Prädikatszielmenge"@de , "Image de la propiété"@fr , "Bereik van het predikaat"@nl , "Rango de la propiedad"@es , "Property range"@en ;
        <http://www.w3.org/2000/01/rdf-schema#subPropertyOf>
                <http://lemon-model.net/lemon#condition> .

<http://lemon-model.net/lemon#MorphPattern>
        a       <http://www.w3.org/2002/07/owl#Class> , <http://www.w3.org/2000/01/rdf-schema#Class> ;
        <http://www.w3.org/2000/01/rdf-schema#label>
                "Morphological pattern"@en , "Patron morphologique"@fr , "Morphologische Muster"@de , "Patrón morfológico"@es , "Morphologisch Patroon"@nl ;
        <http://www.w3.org/2000/01/rdf-schema#subClassOf>
                <http://lemon-model.net/lemon#HasLanguage> , <http://lemon-model.net/lemon#LemonElement> .

<http://lemon-model.net/lemon#formVariant>
        a       <http://www.w3.org/2002/07/owl#ObjectProperty> , <http://www.w3.org/1999/02/22-rdf-syntax-ns#Property> ;
        <http://www.w3.org/2000/01/rdf-schema#domain>
                <http://lemon-model.net/lemon#Form> ;
        <http://www.w3.org/2000/01/rdf-schema#label>
                "Form variant"@en , "Variante de la forma"@es , "Vorm variant"@nl , "Variante de la forme"@fr , "Form-Variante"@de ;
        <http://www.w3.org/2000/01/rdf-schema#range>
                <http://lemon-model.net/lemon#Form> .

<http://lemon-model.net/lemon#property>
        a       <http://www.w3.org/1999/02/22-rdf-syntax-ns#Property> , <http://www.w3.org/2002/07/owl#ObjectProperty> ;
        <http://www.w3.org/2000/01/rdf-schema#comment>
                "Denotes a lexical property of a lexical entry, form, component or MWE node. For the lexical entry this is assumed to be static properties e.g., part of speech and gender and for the others this is assumed to be specific properties e.g., case, number"@en ;
        <http://www.w3.org/2000/01/rdf-schema#domain>
                <http://lemon-model.net/lemon#LemonElement> ;
        <http://www.w3.org/2000/01/rdf-schema#label>
                "Lexical property"@en , "Propiedad léxica"@es , "Lexikalische Prädikat"@de , "Lexikaal predikaat"@nl , "Propiété lexicale"@fr ;
        <http://www.w3.org/2000/01/rdf-schema#range>
                <http://lemon-model.net/lemon#PropertyValue> .

<http://lemon-model.net/lemon#senseRelation>
        a       <http://www.w3.org/2002/07/owl#ObjectProperty> , <http://www.w3.org/1999/02/22-rdf-syntax-ns#Property> ;
        <http://www.w3.org/2000/01/rdf-schema#comment>
                "Denotes a relationship between senses"@en ;
        <http://www.w3.org/2000/01/rdf-schema#domain>
                <http://lemon-model.net/lemon#LexicalSense> ;
        <http://www.w3.org/2000/01/rdf-schema#label>
                "Relation de Signification"@fr , "Zin relatie"@nl , "Relación de Acepción"@es , "Sense relation"@en , "Sinn-Relation"@de ;
        <http://www.w3.org/2000/01/rdf-schema#range>
                <http://lemon-model.net/lemon#LexicalSense> .

<http://lemon-model.net/lemon#NodeConstituent>
        a       <http://www.w3.org/2002/07/owl#Class> , <http://www.w3.org/2000/01/rdf-schema#Class> ;
        <http://www.w3.org/2000/01/rdf-schema#comment>
                "The class of constituents, that is types applied to nodes in a phrase structure graph"@en ;
        <http://www.w3.org/2000/01/rdf-schema#label>
                "Constituent"@fr , "Constituent"@en , "Constituent"@nl , "Konstituent"@de , "Constituyente"@es ;
        <http://www.w3.org/2000/01/rdf-schema#subClassOf>
                <http://lemon-model.net/lemon#LemonElement> .

<http://lemon-model.net/lemon#condition>
        a       <http://www.w3.org/2002/07/owl#ObjectProperty> , <http://www.w3.org/1999/02/22-rdf-syntax-ns#Property> ;
        <http://www.w3.org/2000/01/rdf-schema#comment>
                "Indicates an evaluable test, the is necessary for this sense to apply"@en ;
        <http://www.w3.org/2000/01/rdf-schema#domain>
                <http://lemon-model.net/lemon#LexicalSense> ;
        <http://www.w3.org/2000/01/rdf-schema#label>
                "Condición"@es , "Condition"@fr , "Bedingung"@de , "Condition"@en , "Voorwaarde"@nl ;
        <http://www.w3.org/2000/01/rdf-schema#range>
                <http://lemon-model.net/lemon#LexicalCondition> .

<http://lemon-model.net/lemon#incompatible>
        a       <http://www.w3.org/2002/07/owl#SymmetricProperty> , <http://www.w3.org/1999/02/22-rdf-syntax-ns#Property> , <http://www.w3.org/2002/07/owl#ObjectProperty> ;
        <http://www.w3.org/2000/01/rdf-schema#comment>
                "Says that the two senses are disjoint. From a lexical point of view, this means substituting the lexical entries must change the meaning of the phrase. From an ontological point of view, this property is implied if both references are also disjoint, but does not imply disjointness, but non-equivalence of the references. For the mapping point of view  there is not instance when both mappings are valid."@en ;
        <http://www.w3.org/2000/01/rdf-schema#domain>
                <http://lemon-model.net/lemon#LexicalSense> ;
        <http://www.w3.org/2000/01/rdf-schema#label>
                "Inkompatibel"@de , "Onverenigbaar"@nl , "Incompatible"@fr , "Incompatible"@es , "Incompatible"@en ;
        <http://www.w3.org/2000/01/rdf-schema#range>
                <http://lemon-model.net/lemon#LexicalSense> ;
        <http://www.w3.org/2000/01/rdf-schema#subPropertyOf>
                <http://lemon-model.net/lemon#senseRelation> .

<http://lemon-model.net/lemon#phraseRoot>
        a       <http://www.w3.org/2002/07/owl#ObjectProperty> , <http://www.w3.org/1999/02/22-rdf-syntax-ns#Property> ;
        <http://www.w3.org/2000/01/rdf-schema#comment>
                "Indicates the head node of a phrase structure or dependency parse graph"@en ;
        <http://www.w3.org/2000/01/rdf-schema#domain>
                <http://lemon-model.net/lemon#LexicalEntry> ;
        <http://www.w3.org/2000/01/rdf-schema#label>
                "Phrasewurzel"@de , "Raíz del sintagma"@es , "Base de la syntagme"@fr , "Phrase root"@en , "Zinsdeel wortel"@nl ;
        <http://www.w3.org/2000/01/rdf-schema#range>
                <http://lemon-model.net/lemon#Node> .

<http://lemon-model.net/lemon#MorphTransform>
        a       <http://www.w3.org/2002/07/owl#Class> , <http://www.w3.org/2000/01/rdf-schema#Class> ;
        <http://www.w3.org/2000/01/rdf-schema#label>
                "Morphologische Transformation"@de , "Morphological Transform"@en , "Morphologisch transformatie"@nl , "Transformación morfológica"@es , "Transformation morphologique"@fr ;
        <http://www.w3.org/2000/01/rdf-schema#subClassOf>
                <http://lemon-model.net/lemon#LemonElement> .

<http://lemon-model.net/lemon#lexicalForm>
        a       <http://www.w3.org/2002/07/owl#InverseFunctionalProperty> , <http://www.w3.org/1999/02/22-rdf-syntax-ns#Property> , <http://www.w3.org/2002/07/owl#ObjectProperty> ;
        <http://www.w3.org/2000/01/rdf-schema#comment>
                "Denotes a written representation of a lexical entry"@en ;
        <http://www.w3.org/2000/01/rdf-schema#domain>
                <http://lemon-model.net/lemon#LexicalEntry> ;
        <http://www.w3.org/2000/01/rdf-schema#label>
                "Forma léxica"@es , "Lexikaal vorm"@nl , "Lexical form"@en , "Lexikalische Form"@de , "Forme lexicale"@fr ;
        <http://www.w3.org/2000/01/rdf-schema#range>
                <http://lemon-model.net/lemon#Form> .

<http://lemon-model.net/lemon#nextTransform>
        a       <http://www.w3.org/2002/07/owl#ObjectProperty> , <http://www.w3.org/1999/02/22-rdf-syntax-ns#Property> ;
        <http://www.w3.org/2000/01/rdf-schema#domain>
                <http://lemon-model.net/lemon#MorphTransform> ;
        <http://www.w3.org/2000/01/rdf-schema#label>
                "Transformación siguiente"@es , "Transformation suivante"@fr , "Folgende Transformation"@de , "Next transform"@en , "Volgende transformatie"@nl ;
        <http://www.w3.org/2000/01/rdf-schema#range>
                <http://lemon-model.net/lemon#MorphTransform> .

<http://lemon-model.net/lemon#hiddenRef>
        a       <http://www.w3.org/1999/02/22-rdf-syntax-ns#Property> , <http://www.w3.org/2002/07/owl#ObjectProperty> ;
        <http://www.w3.org/2000/01/rdf-schema#comment>
                "The sense of a non-admissible lexicalization for a ontology entity. This is used to denote incorrect or deprecated language that may be useful for information extraction but not generation"@en ;
        <http://www.w3.org/2000/01/rdf-schema#label>
                "Référence cachée de"@fr , "Verborgen referentie van"@nl , "Referencia oculta de"@es , "Hidden reference of"@en , "Verborgene Referenz von"@de ;
        <http://www.w3.org/2000/01/rdf-schema#range>
                <http://lemon-model.net/lemon#LexicalSense> ;
        <http://www.w3.org/2000/01/rdf-schema#subPropertyOf>
                <http://lemon-model.net/lemon#isReferenceOf> .

<http://lemon-model.net/lemon#element>
        a       <http://www.w3.org/1999/02/22-rdf-syntax-ns#Property> , <http://www.w3.org/2002/07/owl#FunctionalProperty> , <http://www.w3.org/2002/07/owl#ObjectProperty> ;
        <http://www.w3.org/2000/01/rdf-schema#comment>
                "Denotes the lexical entry represented by the component"@en ;
        <http://www.w3.org/2000/01/rdf-schema#domain>
                <http://lemon-model.net/lemon#Component> ;
        <http://www.w3.org/2000/01/rdf-schema#label>
                "Elément"@fr , "Elemento"@es , "Element"@de , "Element"@en , "Element"@nl ;
        <http://www.w3.org/2000/01/rdf-schema#range>
                <http://lemon-model.net/lemon#LexicalEntry> .

<http://lemon-model.net/lemon#pattern>
        a       <http://www.w3.org/2002/07/owl#ObjectProperty> , <http://www.w3.org/1999/02/22-rdf-syntax-ns#Property> ;
        <http://www.w3.org/2000/01/rdf-schema#domain>
                <http://lemon-model.net/lemon#HasPattern> ;
        <http://www.w3.org/2000/01/rdf-schema#label>
                "Pattern"@en , "Patron"@fr , "Patrón"@es , "Patroon"@nl , "Muster"@de ;
        <http://www.w3.org/2000/01/rdf-schema#range>
                <http://lemon-model.net/lemon#MorphPattern> .

<http://lemon-model.net/lemon#SynRoleMarker>
        a       <http://www.w3.org/2000/01/rdf-schema#Class> , <http://www.w3.org/2002/07/owl#Class> ;
        <http://www.w3.org/2000/01/rdf-schema#comment>
                "The indicator of a given syntactic argument, normally a preposition or other particle marker or a linguistic property such as case"@en ;
        <http://www.w3.org/2000/01/rdf-schema#label>
                "Syntactic role marker"@en , "Syntactische Rolle-Marker"@de , "Marcador de la función sintáctica"@es , "Marqueur du rôle syntaxique"@fr , "Syntactisch rol merker"@nl ;
        <http://www.w3.org/2000/01/rdf-schema#subClassOf>
                <http://lemon-model.net/lemon#LemonElement> ;
        <http://www.w3.org/2000/01/rdf-schema#subClassOf>
                [ a       <http://www.w3.org/2000/01/rdf-schema#Class> ;
                  <http://www.w3.org/2002/07/owl#unionOf>
                          ( <http://lemon-model.net/lemon#LexicalEntry> <http://lemon-model.net/lemon#PropertyValue> )
                ] ;
        <http://www.w3.org/2002/07/owl#disjointWith>
                <http://lemon-model.net/lemon#UsageExample> .

<http://lemon-model.net/lemon#objOfProp>
        a       <http://www.w3.org/1999/02/22-rdf-syntax-ns#Property> , <http://www.w3.org/2002/07/owl#ObjectProperty> ;
        <http://www.w3.org/2000/01/rdf-schema#comment>
                "Indicates the semantic argument which represents the objects (ranges) of the property referred to by this sense"@en ;
        <http://www.w3.org/2000/01/rdf-schema#domain>
                <http://lemon-model.net/lemon#LexicalSense> ;
        <http://www.w3.org/2000/01/rdf-schema#label>
                "Complemento de la propiedad"@es , "Complément de la propiété"@fr , "Object van predikaat"@nl , "Object of property"@en , "Objekt von Prädikat"@de ;
        <http://www.w3.org/2000/01/rdf-schema#range>
                <http://lemon-model.net/lemon#Argument> ;
        <http://www.w3.org/2000/01/rdf-schema#subPropertyOf>
                <http://lemon-model.net/lemon#semArg> .

<http://lemon-model.net/lemon#rule>
        a       <http://www.w3.org/2002/07/owl#DatatypeProperty> , <http://www.w3.org/1999/02/22-rdf-syntax-ns#Property> ;
        <http://www.w3.org/2000/01/rdf-schema#domain>
                <http://lemon-model.net/lemon#MorphTransform> ;
        <http://www.w3.org/2000/01/rdf-schema#label>
                "Regla"@es , "Regel"@nl , "Règle"@fr , "Rule"@en , "Regel"@de ;
        <http://www.w3.org/2000/01/rdf-schema#range>
                <http://www.w3.org/2001/XMLSchema#string> .

<http://lemon-model.net/lemon#SenseCondition>
        a       <http://www.w3.org/2000/01/rdf-schema#Class> , <http://www.w3.org/2002/07/owl#Class> ;
        <http://www.w3.org/2000/01/rdf-schema#comment>
                "Indicates a logical condition that is used indicate when a particular term has the given meaning"@en ;
        <http://www.w3.org/2000/01/rdf-schema#label>
                "Condición"@es , "Bedingung"@de , "Condition"@en , "Voorwaarde"@nl , "Condition"@fr ;
        <http://www.w3.org/2000/01/rdf-schema#subClassOf>
                <http://lemon-model.net/lemon#LemonElement> .

<http://lemon-model.net/lemon#Node>
        a       <http://www.w3.org/2002/07/owl#Class> , <http://www.w3.org/2000/01/rdf-schema#Class> ;
        <http://www.w3.org/2000/01/rdf-schema#comment>
                "A node in a phrase structure or dependency parse graph"@en ;
        <http://www.w3.org/2000/01/rdf-schema#label>
                "Node"@en , "Nœud"@fr , "Punt"@nl , "Knoten"@de , "Vértice"@es ;
        <http://www.w3.org/2000/01/rdf-schema#subClassOf>
                <http://lemon-model.net/lemon#LemonElement> ;
        <http://www.w3.org/2000/01/rdf-schema#subClassOf>
                [ a       <http://www.w3.org/2000/01/rdf-schema#Class> ;
                  <http://www.w3.org/2002/07/owl#unionOf>
                          ( [ a       <http://www.w3.org/2002/07/owl#Restriction> ;
                              <http://www.w3.org/2002/07/owl#minCardinality>
                                      "1"^^<http://www.w3.org/2001/XMLSchema#nonNegativeInteger> ;
                              <http://www.w3.org/2002/07/owl#onProperty>
                                      <http://lemon-model.net/lemon#edge>
                            ]
                            [ a       <http://www.w3.org/2002/07/owl#Restriction> ;
                              <http://www.w3.org/2002/07/owl#minCardinality>
                                      "1"^^<http://www.w3.org/2001/XMLSchema#nonNegativeInteger> ;
                              <http://www.w3.org/2002/07/owl#onProperty>
                                      <http://lemon-model.net/lemon#leaf>
                            ]
                          )
                ] ;
        <http://www.w3.org/2002/07/owl#disjointWith>
                <http://lemon-model.net/lemon#SenseDefinition> , <http://lemon-model.net/lemon#UsageExample> , <http://lemon-model.net/lemon#PropertyValue> , <http://lemon-model.net/lemon#SynRoleMarker> .

<http://lemon-model.net/lemon#LexicalCondition>
        a       <http://www.w3.org/2002/07/owl#Class> , <http://www.w3.org/2000/01/rdf-schema#Class> ;
        <http://www.w3.org/2000/01/rdf-schema#comment>
                "An evaluable condition on when a sense applies."@en ;
        <http://www.w3.org/2000/01/rdf-schema#label>
                "Lexikaal Voorwaarde"@nl , "Condition lexicale"@fr , "Condición léxica"@es , "Lexical Condition"@en , "Lexikonbedingung"@de ;
        <http://www.w3.org/2000/01/rdf-schema#subClassOf>
                <http://lemon-model.net/lemon#LemonElement> .

<http://lemon-model.net/lemon#leaf>
        a       <http://www.w3.org/2002/07/owl#ObjectProperty> , <http://www.w3.org/1999/02/22-rdf-syntax-ns#Property> ;
        <http://www.w3.org/2000/01/rdf-schema#comment>
                "Denotes the component referred to by the lex (pre-terminal) of the phrase structure"@en ;
        <http://www.w3.org/2000/01/rdf-schema#domain>
                <http://lemon-model.net/lemon#Node> ;
        <http://www.w3.org/2000/01/rdf-schema#label>
                "Feuille"@fr , "Blad"@nl , "Leaf"@en , "Hoja"@es , "Blatt"@de ;
        <http://www.w3.org/2000/01/rdf-schema#range>
                <http://lemon-model.net/lemon#PhraseElement> .

<http://lemon-model.net/lemon#extrinsicArg>
        a       <http://www.w3.org/1999/02/22-rdf-syntax-ns#Property> , <http://www.w3.org/2002/07/owl#ObjectProperty> ;
        <http://www.w3.org/2000/01/rdf-schema#comment>
                "A raisable semantic argument is not in fact the semantic argument of the current frame-sense but instead is \"raised\" into a frame-sense used for an argument. For example the phrase \"John seemed to be happy\", is interpreted as \"it seemed that X\" where X is \"John is happy\", hence the subject of \"seem\" is a raisable argument."@en ;
        <http://www.w3.org/2000/01/rdf-schema#label>
                "Actant extrinsèque"@fr , "Extrinsic argument"@en , "Äußerliche Argument"@de , "Extrinsiek argument"@nl , "Argumento extrínseco"@es ;
        <http://www.w3.org/2000/01/rdf-schema#subPropertyOf>
                <http://lemon-model.net/lemon#semArg> .

<http://lemon-model.net/lemon#lexicalVariant>
        a       <http://www.w3.org/2002/07/owl#ObjectProperty> , <http://www.w3.org/1999/02/22-rdf-syntax-ns#Property> ;
        <http://www.w3.org/2000/01/rdf-schema#comment>
                "Indicates a non-semantic relationship between two lexical entries. E.g., a term is derived from another term, such as \"lexical\" and \"lexicalize\""@en ;
        <http://www.w3.org/2000/01/rdf-schema#domain>
                <http://lemon-model.net/lemon#LexicalEntry> ;
        <http://www.w3.org/2000/01/rdf-schema#label>
                "Lexical variant"@en , "Variante léxica"@es , "Lexikaal variant"@nl , "Variante lexicale"@fr , "Lexikalische Variante"@de ;
        <http://www.w3.org/2000/01/rdf-schema#range>
                <http://lemon-model.net/lemon#LexicalEntry> .

<http://lemon-model.net/lemon#isA>
        a       <http://www.w3.org/2002/07/owl#ObjectProperty> , <http://www.w3.org/1999/02/22-rdf-syntax-ns#Property> ;
        <http://www.w3.org/2000/01/rdf-schema#comment>
                "Denotes that the single argument of a class predicate is represented in the lexicon by the given semantic argument. That is Class(?x) or ?x rdf:type Class"@en ;
        <http://www.w3.org/2000/01/rdf-schema#domain>
                <http://lemon-model.net/lemon#LexicalSense> ;
        <http://www.w3.org/2000/01/rdf-schema#label>
                "Instanz von"@de , "Instantie van"@nl , "Instancia de"@es , "Instance of"@en , "Instance de"@fr ;
        <http://www.w3.org/2000/01/rdf-schema#range>
                <http://lemon-model.net/lemon#Argument> ;
        <http://www.w3.org/2000/01/rdf-schema#subPropertyOf>
                <http://lemon-model.net/lemon#semArg> .

<http://lemon-model.net/lemon#equivalent>
        a       <http://www.w3.org/1999/02/22-rdf-syntax-ns#Property> , <http://www.w3.org/2002/07/owl#SymmetricProperty> , <http://www.w3.org/2002/07/owl#TransitiveProperty> , <http://www.w3.org/2002/07/owl#ObjectProperty> ;
        <http://www.w3.org/2000/01/rdf-schema#comment>
                "Indicates that two senses are equivalent. From a lexical point of view , this indicates that the lexical entries can be substituted for each other with no change in meaning. From an ontological point of view it means that the two references are not disjoint. From a mapping point of view it means if one mapping apply the other must necessarily apply"@en ;
        <http://www.w3.org/2000/01/rdf-schema#domain>
                <http://lemon-model.net/lemon#LexicalSense> ;
        <http://www.w3.org/2000/01/rdf-schema#label>
                "Equivalente"@es , "Equivalent"@nl , "Equivalent"@fr , "Equivalent"@en , "Äquivalent"@de ;
        <http://www.w3.org/2000/01/rdf-schema#range>
                <http://lemon-model.net/lemon#LexicalSense> ;
        <http://www.w3.org/2000/01/rdf-schema#subPropertyOf>
                <http://lemon-model.net/lemon#senseRelation> .

<http://lemon-model.net/lemon#edge>
        a       <http://www.w3.org/2002/07/owl#ObjectProperty> , <http://www.w3.org/1999/02/22-rdf-syntax-ns#Property> ;
        <http://www.w3.org/2000/01/rdf-schema#comment>
                "Denotes the relation between a node in a multi-word expression structure and an edge"@en ;
        <http://www.w3.org/2000/01/rdf-schema#domain>
                <http://lemon-model.net/lemon#Node> ;
        <http://www.w3.org/2000/01/rdf-schema#label>
                "Lien"@fr , "Arista"@es , "Lijn"@nl , "Kante"@de , "Edge"@en ;
        <http://www.w3.org/2000/01/rdf-schema#range>
                <http://lemon-model.net/lemon#Node> .

<http://lemon-model.net/lemon#LexicalTopic>
        a       <http://www.w3.org/2000/01/rdf-schema#Class> , <http://www.w3.org/2002/07/owl#Class> ;
        <http://www.w3.org/2000/01/rdf-schema#comment>
                "Indicates the topic of a lexicon or a lexical entry"@en ;
        <http://www.w3.org/2000/01/rdf-schema#label>
                "Tema léxica"@es , "Lexical Topic"@en , "Lexikonthema"@de , "Thème lexicale"@fr , "Lexikaal Thema"@nl ;
        <http://www.w3.org/2000/01/rdf-schema#subClassOf>
                <http://lemon-model.net/lemon#LemonElement> .

<http://lemon-model.net/lemon#context>
        a       <http://www.w3.org/1999/02/22-rdf-syntax-ns#Property> , <http://www.w3.org/2002/07/owl#ObjectProperty> ;
        <http://www.w3.org/2000/01/rdf-schema#comment>
                "Denotes the pragmatic or discursive context of a sense mapping or a constraint on the mapping by syntactic or semantic properites"@en ;
        <http://www.w3.org/2000/01/rdf-schema#domain>
                <http://lemon-model.net/lemon#LexicalSense> ;
        <http://www.w3.org/2000/01/rdf-schema#label>
                "Context"@en , "Kontext"@de , "Context"@nl , "Contexto"@es , "Contexte"@fr ;
        <http://www.w3.org/2000/01/rdf-schema#range>
                <http://lemon-model.net/lemon#LexicalContext> .

<http://lemon-model.net/lemon#isSenseOf>
        a       <http://www.w3.org/1999/02/22-rdf-syntax-ns#Property> , <http://www.w3.org/2002/07/owl#ObjectProperty> ;
        <http://www.w3.org/2000/01/rdf-schema#comment>
                "Indicate that a sense is realised by the given lexical entry"@en ;
        <http://www.w3.org/2000/01/rdf-schema#domain>
                <http://lemon-model.net/lemon#LexicalSense> ;
        <http://www.w3.org/2000/01/rdf-schema#label>
                "Acepción de"@es , "Zin van"@nl , "Sinn von"@de , "Signfication de"@fr , "Sense of"@en ;
        <http://www.w3.org/2000/01/rdf-schema#range>
                <http://lemon-model.net/lemon#LexicalEntry> ;
        <http://www.w3.org/2002/07/owl#inverseOf>
                <http://lemon-model.net/lemon#sense> .

<http://lemon-model.net/lemon#tree>
        a       <http://www.w3.org/1999/02/22-rdf-syntax-ns#Property> , <http://www.w3.org/2002/07/owl#ObjectProperty> ;
        <http://www.w3.org/2000/01/rdf-schema#label>
                "Árbol"@es , "Tree"@en , "Boom"@nl , "Arbre"@fr , "Baum"@de .

<http://lemon-model.net/lemon#LexicalEntry>
        a       <http://www.w3.org/2002/07/owl#Class> , <http://www.w3.org/2000/01/rdf-schema#Class> ;
        <http://www.w3.org/2000/01/rdf-schema#comment>
                "An entry in the lexicon. This may be any morpheme, word, compound, phrase or clause that is included in the lexicon"@en ;
        <http://www.w3.org/2000/01/rdf-schema#label>
                "Entrée lexicale"@fr , "Lexikaal item"@nl , "Lexikoneintrag"@de , "Entrada léxica"@es , "Lexical entry"@en ;
        <http://www.w3.org/2000/01/rdf-schema#subClassOf>
                <http://lemon-model.net/lemon#HasLanguage> , <http://lemon-model.net/lemon#LemonElement> , <http://lemon-model.net/lemon#HasPattern> ;
        <http://www.w3.org/2000/01/rdf-schema#subClassOf>
                [ a       <http://www.w3.org/2002/07/owl#Restriction> ;
                  <http://www.w3.org/2002/07/owl#maxCardinality>
                          "1"^^<http://www.w3.org/2001/XMLSchema#nonNegativeInteger> ;
                  <http://www.w3.org/2002/07/owl#onProperty>
                          <http://lemon-model.net/lemon#canonicalForm>
                ] ;
        <http://www.w3.org/2000/01/rdf-schema#subClassOf>
                [ a       <http://www.w3.org/2002/07/owl#Restriction> ;
                  <http://www.w3.org/2002/07/owl#minCardinality>
                          "1"^^<http://www.w3.org/2001/XMLSchema#nonNegativeInteger> ;
                  <http://www.w3.org/2002/07/owl#onProperty>
                          <http://lemon-model.net/lemon#lexicalForm>
                ] ;
        <http://www.w3.org/2002/07/owl#disjointWith>
                <http://lemon-model.net/lemon#PropertyValue> , <http://lemon-model.net/lemon#Lexicon> , <http://lemon-model.net/lemon#UsageExample> , <http://lemon-model.net/lemon#SenseDefinition> , <http://lemon-model.net/lemon#Node> , <http://lemon-model.net/lemon#LexicalSense> .

<http://lemon-model.net/lemon#entry>
        a       <http://www.w3.org/1999/02/22-rdf-syntax-ns#Property> , <http://www.w3.org/2002/07/owl#ObjectProperty> ;
        <http://www.w3.org/2000/01/rdf-schema#comment>
                "Indicates an entry in a lexicon"@en ;
        <http://www.w3.org/2000/01/rdf-schema#domain>
                <http://lemon-model.net/lemon#Lexicon> ;
        <http://www.w3.org/2000/01/rdf-schema#label>
                "Eintrag"@de , "Entrada"@es , "Entrée"@fr , "Item"@nl , "Entry"@en ;
        <http://www.w3.org/2000/01/rdf-schema#range>
                <http://lemon-model.net/lemon#LexicalEntry> .

<http://lemon-model.net/lemon#synArg>
        a       <http://www.w3.org/2002/07/owl#ObjectProperty> , <http://www.w3.org/1999/02/22-rdf-syntax-ns#Property> ;
        <http://www.w3.org/2000/01/rdf-schema#comment>
                "Indicates a slot in a syntactic frame"@en ;
        <http://www.w3.org/2000/01/rdf-schema#domain>
                <http://lemon-model.net/lemon#Frame> ;
        <http://www.w3.org/2000/01/rdf-schema#label>
                "Syntactic argument"@en , "Actant syntaxique"@fr , "Argumento sintáctico"@es , "Syntactische Argument"@de , "Syntactisch argument"@nl ;
        <http://www.w3.org/2000/01/rdf-schema#range>
                <http://lemon-model.net/lemon#Argument> .

<http://lemon-model.net/lemon#LexicalSense>
        a       <http://www.w3.org/2002/07/owl#Class> , <http://www.w3.org/2000/01/rdf-schema#Class> ;
        <http://www.w3.org/2000/01/rdf-schema#comment>
                "Represents the intersection in meaning between the lexical entry and the ontology entity. This is used as the ontology entity and lexical entry may not be in one-to-one correspondence as such the existence of a sense between them states meerly that there are some cases when this lexical entry refer to the ontology entity and vica versa. Mapping elements can be used to further specify this relation"@en ;
        <http://www.w3.org/2000/01/rdf-schema#label>
                "Signification lexicale"@fr , "Acepción léxica"@es , "Lexical sense"@en , "Lexikonsinn"@de , "Lexikaal zin"@nl ;
        <http://www.w3.org/2000/01/rdf-schema#subClassOf>
                <http://lemon-model.net/lemon#LemonElement> ;
        <http://www.w3.org/2000/01/rdf-schema#subClassOf>
                [ a       <http://www.w3.org/2000/01/rdf-schema#Class> ;
                  <http://www.w3.org/2002/07/owl#unionOf>
                          ( [ a       <http://www.w3.org/2002/07/owl#Restriction> ;
                              <http://www.w3.org/2002/07/owl#minCardinality>
                                      "1"^^<http://www.w3.org/2001/XMLSchema#nonNegativeInteger> ;
                              <http://www.w3.org/2002/07/owl#onProperty>
                                      <http://lemon-model.net/lemon#subsense>
                            ]
                            [ a       <http://www.w3.org/2002/07/owl#Restriction> ;
                              <http://www.w3.org/2002/07/owl#cardinality>
                                      "1"^^<http://www.w3.org/2001/XMLSchema#nonNegativeInteger> ;
                              <http://www.w3.org/2002/07/owl#onProperty>
                                      <http://lemon-model.net/lemon#reference>
                            ]
                          )
                ] ;
        <http://www.w3.org/2002/07/owl#disjointWith>
                <http://lemon-model.net/lemon#SenseDefinition> , <http://lemon-model.net/lemon#Node> , <http://lemon-model.net/lemon#UsageExample> , <http://lemon-model.net/lemon#Lexicon> , <http://lemon-model.net/lemon#SynRoleMarker> , <http://lemon-model.net/lemon#PropertyValue> .

<http://lemon-model.net/lemon#reference>
        a       <http://www.w3.org/1999/02/22-rdf-syntax-ns#Property> , <http://www.w3.org/2002/07/owl#FunctionalProperty> , <http://www.w3.org/2002/07/owl#ObjectProperty> ;
        <http://www.w3.org/2000/01/rdf-schema#comment>
                "A reference to an external resource"@en ;
        <http://www.w3.org/2000/01/rdf-schema#domain>
                <http://lemon-model.net/lemon#LexicalSense> ;
        <http://www.w3.org/2000/01/rdf-schema#label>
                "Referentie"@nl , "Référence"@fr , "Referencia"@es , "Reference"@en , "Referenz"@de .

<http://lemon-model.net/lemon#PhraseElement>
        a       <http://www.w3.org/2002/07/owl#Class> , <http://www.w3.org/2000/01/rdf-schema#Class> ;
        <http://www.w3.org/2000/01/rdf-schema#comment>
                "A terminal node in a phrase structure graph, i.e., a realisable, lexical element."@en ;
        <http://www.w3.org/2000/01/rdf-schema#label>
                "Phrase element"@en , "Zinselement"@nl , "Phrase-Element"@de , "Elément du syntagme"@fr , "Elemento del sintagma"@es ;
        <http://www.w3.org/2000/01/rdf-schema#subClassOf>
                <http://lemon-model.net/lemon#LemonElement> .

<http://lemon-model.net/lemon#Frame>
        a       <http://www.w3.org/2002/07/owl#Class> , <http://www.w3.org/2000/01/rdf-schema#Class> ;
        <http://www.w3.org/2000/01/rdf-schema#comment>
                "A stereotypical example of the usage of a given lexical entry. The most common example of projections are subcategorization frames which describe the slots taken by the arguments of a verb."@en ;
        <http://www.w3.org/2000/01/rdf-schema#label>
                "Frame"@en , "Rahmen"@de , "Marco"@es , "Cadre"@fr , "Raam"@nl ;
        <http://www.w3.org/2000/01/rdf-schema#subClassOf>
                <http://lemon-model.net/lemon#LemonElement> ;
        <http://www.w3.org/2002/07/owl#disjointWith>
                <http://lemon-model.net/lemon#UsageExample> , <http://lemon-model.net/lemon#LexicalEntry> , <http://lemon-model.net/lemon#SenseDefinition> , <http://lemon-model.net/lemon#Node> , <http://lemon-model.net/lemon#LexicalSense> , <http://lemon-model.net/lemon#SynRoleMarker> , <http://lemon-model.net/lemon#PropertyValue> , <http://lemon-model.net/lemon#Lexicon> .

<http://lemon-model.net/lemon#writtenRep>
        a       <http://www.w3.org/1999/02/22-rdf-syntax-ns#Property> , <http://www.w3.org/2002/07/owl#DatatypeProperty> ;
        <http://www.w3.org/2000/01/rdf-schema#comment>
                "Gives the written representation of a given form"@en ;
        <http://www.w3.org/2000/01/rdf-schema#domain>
                <http://lemon-model.net/lemon#Form> ;
        <http://www.w3.org/2000/01/rdf-schema#label>
                "Representación escrita"@es , "Représentation écrite"@fr , "Written representation"@en , "Schriftliche Darstellung"@de , "Schriftelijke voorstelling"@nl ;
        <http://www.w3.org/2000/01/rdf-schema#range>
                <http://www.w3.org/2001/XMLSchema#string> ;
        <http://www.w3.org/2000/01/rdf-schema#subPropertyOf>
                <http://lemon-model.net/lemon#representation> .

<http://lemon-model.net/lemon#generates>
        a       <http://www.w3.org/1999/02/22-rdf-syntax-ns#Property> , <http://www.w3.org/2002/07/owl#ObjectProperty> ;
        <http://www.w3.org/2000/01/rdf-schema#domain>
                <http://lemon-model.net/lemon#MorphTransform> ;
        <http://www.w3.org/2000/01/rdf-schema#label>
                "Genereert"@nl , "Generates"@en , "Genera"@es , "Erzeugt"@de , "Génère"@fr ;
        <http://www.w3.org/2000/01/rdf-schema#range>
                <http://lemon-model.net/lemon#Prototype> ;
        <http://www.w3.org/2000/01/rdf-schema#subClassOf>
                [ a       <http://www.w3.org/2002/07/owl#Restriction> ;
                  <http://www.w3.org/2002/07/owl#minCardinality>
                          "1"^^<http://www.w3.org/2001/XMLSchema#nonNegativeInteger> ;
                  <http://www.w3.org/2002/07/owl#onProperty>
                          <http://lemon-model.net/lemon#rule>
                ] .

<http://lemon-model.net/lemon#broader>
        a       <http://www.w3.org/2002/07/owl#ObjectProperty> , <http://www.w3.org/1999/02/22-rdf-syntax-ns#Property> ;
        <http://www.w3.org/2000/01/rdf-schema#comment>
                "Denotes that one sense is broader than another. From a lexical point of view  this means replacing one lexical entry with another generalizes the meaning of the phrase. From an ontological point of view this property makes not strong assertions. From a mapping point of view if the broader sense applies the narrower sense must also"@en ;
        <http://www.w3.org/2000/01/rdf-schema#domain>
                <http://lemon-model.net/lemon#LexicalSense> ;
        <http://www.w3.org/2000/01/rdf-schema#label>
                "Plus large"@fr , "Breder"@nl , "Más amplio"@es , "Breiter"@de , "Broader"@en ;
        <http://www.w3.org/2000/01/rdf-schema#range>
                <http://lemon-model.net/lemon#LexicalSense> ;
        <http://www.w3.org/2000/01/rdf-schema#subPropertyOf>
                <http://lemon-model.net/lemon#senseRelation> ;
        <http://www.w3.org/2002/07/owl#inverseOf>
                <http://lemon-model.net/lemon#narrower> .

<http://lemon-model.net/lemon#prefRef>
        a       <http://www.w3.org/2002/07/owl#ObjectProperty> , <http://www.w3.org/1999/02/22-rdf-syntax-ns#Property> ;
        <http://www.w3.org/2000/01/rdf-schema#comment>
                "The sense of the preferred lexicalization of a given ontology entity"@en ;
        <http://www.w3.org/2000/01/rdf-schema#label>
                "Preferred reference of"@en , "Referencia preferida de"@es , "Voorkeursreferentie van"@nl , "Référence préféré de"@fr , "Bevorzugte Referenz von"@de ;
        <http://www.w3.org/2000/01/rdf-schema#range>
                <http://lemon-model.net/lemon#LexicalSense> ;
        <http://www.w3.org/2000/01/rdf-schema#subPropertyOf>
                <http://lemon-model.net/lemon#isReferenceOf> .

<http://lemon-model.net/lemon#Phrase>
        a       <http://www.w3.org/2002/07/owl#Class> , <http://www.w3.org/2000/01/rdf-schema#Class> ;
        <http://www.w3.org/2000/01/rdf-schema#comment>
                "A phrase in lemon is defined in the looser sense of a sequence of words, it does not have to a fully grammatical phrase"@en ;
        <http://www.w3.org/2000/01/rdf-schema#label>
                "Syntagme"@fr , "Zinsdeel"@nl , "Sintagma"@es , "Phrase"@de , "Phrase"@en ;
        <http://www.w3.org/2000/01/rdf-schema#subClassOf>
                <http://lemon-model.net/lemon#LexicalEntry> ;
        <http://www.w3.org/2000/01/rdf-schema#subClassOf>
                [ a       <http://www.w3.org/2002/07/owl#Restriction> ;
                  <http://www.w3.org/2002/07/owl#minCardinality>
                          "1"^^<http://www.w3.org/2001/XMLSchema#nonNegativeInteger> ;
                  <http://www.w3.org/2002/07/owl#onProperty>
                          <http://lemon-model.net/lemon#decomposition>
                ] .

<http://lemon-model.net/lemon#topic>
        a       <http://www.w3.org/2002/07/owl#ObjectProperty> , <http://www.w3.org/1999/02/22-rdf-syntax-ns#Property> ;
        <http://www.w3.org/2000/01/rdf-schema#comment>
                "Indicates the topic of the overrall lexicon, this is property is sometimes called \"subject field\". Note that in addition to the topic of a lexicon each lexical entry may belong to a given domain, this can be modelled as equal or not equal to the topic of the associated lexicon"@en ;
        <http://www.w3.org/2000/01/rdf-schema#domain>
                [ a       <http://www.w3.org/2000/01/rdf-schema#Class> ;
                  <http://www.w3.org/2002/07/owl#unionOf>
                          ( <http://lemon-model.net/lemon#LexicalEntry> <http://lemon-model.net/lemon#Lexicon> )
                ] ;
        <http://www.w3.org/2000/01/rdf-schema#label>
                "Tema"@es , "Thema"@nl , "Thema"@de , "Thème"@fr , "Topic"@en ;
        <http://www.w3.org/2000/01/rdf-schema#range>
                <http://lemon-model.net/lemon#LexicalTopic> .

<http://lemon-model.net/lemon#altRef>
        a       <http://www.w3.org/2002/07/owl#ObjectProperty> , <http://www.w3.org/1999/02/22-rdf-syntax-ns#Property> ;
        <http://www.w3.org/2000/01/rdf-schema#comment>
                "The sense of a non-preferred but admissible lexicalization of a given ontology entity"@en ;
        <http://www.w3.org/2000/01/rdf-schema#label>
                "Alternative Referenz von"@de , "Référence alternative de"@fr , "Alternatieve referentie van"@nl , "Referencia alternativa de"@es , "Alternative reference of"@en ;
        <http://www.w3.org/2000/01/rdf-schema#range>
                <http://lemon-model.net/lemon#LexicalSense> ;
        <http://www.w3.org/2000/01/rdf-schema#subPropertyOf>
                <http://lemon-model.net/lemon#isReferenceOf> .

<http://lemon-model.net/lemon#Word>
        a       <http://www.w3.org/2000/01/rdf-schema#Class> , <http://www.w3.org/2002/07/owl#Class> ;
        <http://www.w3.org/2000/01/rdf-schema#comment>
                "A word is a single unit of writing or speech. In languages written in Latin, Cyrillic, Greek, Arabic scripts etc. these are assumed to be separated by white-space characters. For Chinese, Japanese, Korean this should correspond to some agreed segmentation scheme."@en ;
        <http://www.w3.org/2000/01/rdf-schema#label>
                "Woord"@nl , "Wort"@de , "Word"@en , "Mot"@fr , "Palabra"@es ;
        <http://www.w3.org/2000/01/rdf-schema#subClassOf>
                <http://lemon-model.net/lemon#LexicalEntry> .

<http://lemon-model.net/lemon#optional>
        a       <http://www.w3.org/1999/02/22-rdf-syntax-ns#Property> , <http://www.w3.org/2002/07/owl#DatatypeProperty> ;
        <http://www.w3.org/2000/01/rdf-schema#comment>
                "Denotes that the syntactic argument is optional (may be omitted)"@en ;
        <http://www.w3.org/2000/01/rdf-schema#domain>
                <http://lemon-model.net/lemon#Argument> ;
        <http://www.w3.org/2000/01/rdf-schema#label>
                "Optional"@en , "Optional"@de , "Optionele"@nl , "Optionnel"@fr , "Opcional"@es ;
        <http://www.w3.org/2000/01/rdf-schema#range>
                <http://www.w3.org/2001/XMLSchema#boolean> .

<http://lemon-model.net/lemon#SenseDefinition>
        a       <http://www.w3.org/2002/07/owl#Class> , <http://www.w3.org/2000/01/rdf-schema#Class> ;
        <http://www.w3.org/2000/01/rdf-schema#comment>
                "A definition of a sememe, that is the a text describing the exact meaning of the lexical entry when its sense is the given ontology reference"@en ;
        <http://www.w3.org/2000/01/rdf-schema#label>
                "Definitie"@nl , "Definition"@en , "Definition"@de , "Définition"@fr , "Definición"@es ;
        <http://www.w3.org/2000/01/rdf-schema#subClassOf>
                <http://lemon-model.net/lemon#LemonElement> ;
        <http://www.w3.org/2000/01/rdf-schema#subClassOf>
                [ a       <http://www.w3.org/2002/07/owl#Restriction> ;
                  <http://www.w3.org/2002/07/owl#minCardinality>
                          "1"^^<http://www.w3.org/2001/XMLSchema#nonNegativeInteger> ;
                  <http://www.w3.org/2002/07/owl#onProperty>
                          <http://lemon-model.net/lemon#value>
                ] ;
        <http://www.w3.org/2002/07/owl#disjointWith>
                <http://lemon-model.net/lemon#SynRoleMarker> , <http://lemon-model.net/lemon#UsageExample> .

<http://lemon-model.net/lemon#transform>
        a       <http://www.w3.org/2002/07/owl#ObjectProperty> , <http://www.w3.org/1999/02/22-rdf-syntax-ns#Property> ;
        <http://www.w3.org/2000/01/rdf-schema#domain>
                <http://lemon-model.net/lemon#MorphPattern> ;
        <http://www.w3.org/2000/01/rdf-schema#label>
                "Transformation"@de , "Transformation"@fr , "Transformatie"@nl , "Transformación"@es , "Transform"@en ;
        <http://www.w3.org/2000/01/rdf-schema#range>
                <http://lemon-model.net/lemon#MorphTransform> .

<http://lemon-model.net/lemon#propertyDomain>
        a       <http://www.w3.org/1999/02/22-rdf-syntax-ns#Property> , <http://www.w3.org/2002/07/owl#ObjectProperty> ;
        <http://www.w3.org/2000/01/rdf-schema#comment>
                "Indicates a restrictions on the domain of the property. That is, this sense only applies if the property the sense refers to has a subject in the class referred to by this property"@en ;
        <http://www.w3.org/2000/01/rdf-schema#domain>
                <http://lemon-model.net/lemon#LexicalSense> ;
        <http://www.w3.org/2000/01/rdf-schema#label>
                "Prädikatsbereich"@de , "Domein van het predikaat"@nl , "Dominio de la propiedad"@es , "Ensemble de la propiété"@fr , "Property domain"@en ;
        <http://www.w3.org/2000/01/rdf-schema#subPropertyOf>
                <http://lemon-model.net/lemon#condition> .

<http://lemon-model.net/lemon>
        a       <http://www.w3.org/2002/07/owl#Ontology> ;
        <http://www.w3.org/2000/01/rdf-schema#comment>
                "Lemon: The lexicon model for ontologies is designed to allow  for descriptions of lexical information regarding ontological elements and other RDF resources. Lemon covers mapping of lexical decomposition, phrase structure, syntax,  variation, morphology, and lexicon-ontology mapping."@en ;
        <http://www.w3.org/2000/01/rdf-schema#label>
                "lemon"@en ;
        <http://www.w3.org/2000/01/rdf-schema#seeAlso>
                <http://www.monnet-project.eu/lemon> .

<http://lemon-model.net/lemon#LemonElement>
        a       <http://www.w3.org/2000/01/rdf-schema#Class> , <http://www.w3.org/2002/07/owl#Class> .

<http://lemon-model.net/lemon#representation>
        a       <http://www.w3.org/1999/02/22-rdf-syntax-ns#Property> , <http://www.w3.org/2002/07/owl#DatatypeProperty> ;
        <http://www.w3.org/2000/01/rdf-schema#comment>
                "A realisation of a given form"@en ;
        <http://www.w3.org/2000/01/rdf-schema#domain>
                <http://lemon-model.net/lemon#Form> ;
        <http://www.w3.org/2000/01/rdf-schema#label>
                "Représentation"@fr , "Representación"@es , "Representation"@en , "Voorstelling"@nl , "Darstellung"@de ;
        <http://www.w3.org/2000/01/rdf-schema#range>
                <http://www.w3.org/2001/XMLSchema#string> .

<http://lemon-model.net/lemon#Argument>
        a       <http://www.w3.org/2000/01/rdf-schema#Class> , <http://www.w3.org/2002/07/owl#Class> ;
        <http://www.w3.org/2000/01/rdf-schema#comment>
                "A slot representing a gap that must be filled in realising a lexical entry in a given projection"@en ;
        <http://www.w3.org/2000/01/rdf-schema#label>
                "Actant"@fr , "Argumento"@es , "Argument"@de , "Argument"@en , "Argument"@nl ;
        <http://www.w3.org/2000/01/rdf-schema#subClassOf>
                <http://lemon-model.net/lemon#LemonElement> , <http://lemon-model.net/lemon#PhraseElement> ;
        <http://www.w3.org/2002/07/owl#disjointWith>
                <http://lemon-model.net/lemon#Lexicon> , <http://lemon-model.net/lemon#Form> , <http://lemon-model.net/lemon#PropertyValue> , <http://lemon-model.net/lemon#SynRoleMarker> , <http://lemon-model.net/lemon#LexicalSense> , <http://lemon-model.net/lemon#Node> , <http://lemon-model.net/lemon#SenseDefinition> , <http://lemon-model.net/lemon#LexicalEntry> , <http://lemon-model.net/lemon#Frame> , <http://lemon-model.net/lemon#UsageExample> , <http://lemon-model.net/lemon#Component> .

<http://lemon-model.net/lemon#decomposition>
        a       <http://www.w3.org/1999/02/22-rdf-syntax-ns#Property> , <http://www.w3.org/2002/07/owl#ObjectProperty> ;
        <http://www.w3.org/2000/01/rdf-schema#comment>
                "Denotes a component of a lexical entry"@en ;
        <http://www.w3.org/2000/01/rdf-schema#domain>
                <http://lemon-model.net/lemon#LexicalEntry> ;
        <http://www.w3.org/2000/01/rdf-schema#label>
                "Décomposition"@fr , "Dekompositum"@de , "Descomposición"@es , "Decomposition"@en , "Decompositie"@nl ;
        <http://www.w3.org/2000/01/rdf-schema#range>
                <http://lemon-model.net/lemon#ComponentList> .

<http://lemon-model.net/lemon#sense>
        a       <http://www.w3.org/2002/07/owl#ObjectProperty> , <http://www.w3.org/1999/02/22-rdf-syntax-ns#Property> ;
        <http://www.w3.org/2000/01/rdf-schema#comment>
                "Indicates the sense of a lexical entry"@en ;
        <http://www.w3.org/2000/01/rdf-schema#domain>
                <http://lemon-model.net/lemon#LexicalEntry> ;
        <http://www.w3.org/2000/01/rdf-schema#label>
                "Sense"@en , "Zin"@nl , "Acepción"@es , "Signification"@fr , "Sinn"@de ;
        <http://www.w3.org/2000/01/rdf-schema#range>
                <http://lemon-model.net/lemon#LexicalSense> .

<http://lemon-model.net/lemon#subjOfProp>
        a       <http://www.w3.org/1999/02/22-rdf-syntax-ns#Property> , <http://www.w3.org/2002/07/owl#ObjectProperty> ;
        <http://www.w3.org/2000/01/rdf-schema#comment>
                "Indicates the semantic argument which represents the subjects (domain) of the property referred to by this sense"@en ;
        <http://www.w3.org/2000/01/rdf-schema#domain>
                <http://lemon-model.net/lemon#LexicalSense> ;
        <http://www.w3.org/2000/01/rdf-schema#label>
                "Onderwerp van predikaat"@nl , "Sujeto de la propiedad"@es , "Subjekt von Prädikat"@de , "Subject of property"@en , "Sujet de la propiété"@fr ;
        <http://www.w3.org/2000/01/rdf-schema#range>
                <http://lemon-model.net/lemon#Argument> ;
        <http://www.w3.org/2000/01/rdf-schema#subPropertyOf>
                <http://lemon-model.net/lemon#semArg> .

<http://lemon-model.net/lemon#Component>
        a       <http://www.w3.org/2002/07/owl#Class> , <http://www.w3.org/2000/01/rdf-schema#Class> ;
        <http://www.w3.org/2000/01/rdf-schema#comment>
                "A constituent element of a lexical entry. This may be a word in a multi-word lexical element or a constituent of a compound word"@en ;
        <http://www.w3.org/2000/01/rdf-schema#label>
                "Component"@en , "Komponente"@de , "Componente"@es , "Bestanddeel"@nl , "Composant"@fr ;
        <http://www.w3.org/2000/01/rdf-schema#subClassOf>
                <http://lemon-model.net/lemon#PhraseElement> , <http://lemon-model.net/lemon#LemonElement> ;
        <http://www.w3.org/2000/01/rdf-schema#subClassOf>
                [ a       <http://www.w3.org/2002/07/owl#Restriction> ;
                  <http://www.w3.org/2002/07/owl#maxCardinality>
                          "1"^^<http://www.w3.org/2001/XMLSchema#nonNegativeInteger> ;
                  <http://www.w3.org/2002/07/owl#onProperty>
                          <http://lemon-model.net/lemon#element>
                ] ;
        <http://www.w3.org/2002/07/owl#disjointWith>
                <http://lemon-model.net/lemon#UsageExample> , <http://lemon-model.net/lemon#LexicalEntry> , <http://lemon-model.net/lemon#Frame> , <http://lemon-model.net/lemon#SenseDefinition> , <http://lemon-model.net/lemon#Node> , <http://lemon-model.net/lemon#LexicalSense> , <http://lemon-model.net/lemon#PropertyValue> , <http://lemon-model.net/lemon#SynRoleMarker> , <http://lemon-model.net/lemon#Form> , <http://lemon-model.net/lemon#Lexicon> .

<http://lemon-model.net/lemon#Lexicon>
        a       <http://www.w3.org/2000/01/rdf-schema#Class> , <http://www.w3.org/2002/07/owl#Class> ;
        <http://www.w3.org/2000/01/rdf-schema#comment>
                "The lexicon object. This object is specific to the given language and/or domain it describes"@en ;
        <http://www.w3.org/2000/01/rdf-schema#label>
                "Lexicon"@en , "Lexicón"@es , "Lexique"@fr , "Lexicon"@nl , "Lexikon"@de ;
        <http://www.w3.org/2000/01/rdf-schema#subClassOf>
                <http://lemon-model.net/lemon#LemonElement> , <http://lemon-model.net/lemon#HasLanguage> , <http://lemon-model.net/lemon#HasPattern> ;
        <http://www.w3.org/2000/01/rdf-schema#subClassOf>
                [ a       <http://www.w3.org/2002/07/owl#Restriction> ;
                  <http://www.w3.org/2002/07/owl#minCardinality>
                          "1"^^<http://www.w3.org/2001/XMLSchema#nonNegativeInteger> ;
                  <http://www.w3.org/2002/07/owl#onProperty>
                          <http://lemon-model.net/lemon#entry>
                ] ;
        <http://www.w3.org/2000/01/rdf-schema#subClassOf>
                [ a       <http://www.w3.org/2002/07/owl#Restriction> ;
                  <http://www.w3.org/2002/07/owl#cardinality>
                          "1"^^<http://www.w3.org/2001/XMLSchema#nonNegativeInteger> ;
                  <http://www.w3.org/2002/07/owl#onProperty>
                          <http://lemon-model.net/lemon#language>
                ] ;
        <http://www.w3.org/2002/07/owl#disjointWith>
                <http://lemon-model.net/lemon#SynRoleMarker> , <http://lemon-model.net/lemon#PropertyValue> , <http://lemon-model.net/lemon#Node> , <http://lemon-model.net/lemon#SenseDefinition> , <http://lemon-model.net/lemon#UsageExample> .

<http://lemon-model.net/lemon#narrower>
        a       <http://www.w3.org/1999/02/22-rdf-syntax-ns#Property> , <http://www.w3.org/2002/07/owl#ObjectProperty> ;
        <http://www.w3.org/2000/01/rdf-schema#comment>
                "Denotes that one sense is narrower than another. From a lexical point of view  this means replacing one lexical entry with another specializes the meaning of the phrase. From an ontological point of view this property makes not strong assertions. From a mapping point of view if the broader sense applies the narrower sense must also"@en ;
        <http://www.w3.org/2000/01/rdf-schema#domain>
                <http://lemon-model.net/lemon#LexicalSense> ;
        <http://www.w3.org/2000/01/rdf-schema#label>
                "Enger"@de , "Plus restreint"@fr , "Narrower"@en , "Más estrecho"@es , "Enger"@nl ;
        <http://www.w3.org/2000/01/rdf-schema#range>
                <http://lemon-model.net/lemon#LexicalSense> ;
        <http://www.w3.org/2000/01/rdf-schema#subPropertyOf>
                <http://lemon-model.net/lemon#senseRelation> .

<http://lemon-model.net/lemon#isReferenceOf>
        a       <http://www.w3.org/1999/02/22-rdf-syntax-ns#Property> , <http://www.w3.org/2002/07/owl#ObjectProperty> ;
        <http://www.w3.org/2000/01/rdf-schema#comment>
                "Indicate that a reference has a given sense"@en ;
        <http://www.w3.org/2000/01/rdf-schema#label>
                "Referenz von"@de , "Referentie van"@nl , "Référence de"@fr , "Referencia de"@es , "Reference of"@en ;
        <http://www.w3.org/2000/01/rdf-schema#range>
                <http://lemon-model.net/lemon#LexicalSense> ;
        <http://www.w3.org/2002/07/owl#inverseOf>
                <http://lemon-model.net/lemon#reference> .

<http://lemon-model.net/lemon#Form>
        a       <http://www.w3.org/2000/01/rdf-schema#Class> , <http://www.w3.org/2002/07/owl#Class> ;
        <http://www.w3.org/2000/01/rdf-schema#comment>
                "A given written or spoken realisation of a lexical entry"@en ;
        <http://www.w3.org/2000/01/rdf-schema#label>
                "Vorm"@nl , "Forma"@es , "Forme"@fr , "Form"@en , "Form"@de ;
        <http://www.w3.org/2000/01/rdf-schema#subClassOf>
                <http://lemon-model.net/lemon#LemonElement> ;
        <http://www.w3.org/2000/01/rdf-schema#subClassOf>
                [ a       <http://www.w3.org/2002/07/owl#Restriction> ;
                  <http://www.w3.org/2002/07/owl#minCardinality>
                          "1"^^<http://www.w3.org/2001/XMLSchema#nonNegativeInteger> ;
                  <http://www.w3.org/2002/07/owl#onProperty>
                          <http://lemon-model.net/lemon#representation>
                ] ;
        <http://www.w3.org/2002/07/owl#disjointWith>
                <http://lemon-model.net/lemon#SynRoleMarker> , <http://lemon-model.net/lemon#PropertyValue> , <http://lemon-model.net/lemon#Lexicon> , <http://lemon-model.net/lemon#Frame> , <http://lemon-model.net/lemon#LexicalEntry> , <http://lemon-model.net/lemon#UsageExample> , <http://lemon-model.net/lemon#Node> , <http://lemon-model.net/lemon#LexicalSense> , <http://lemon-model.net/lemon#SenseDefinition> .

<http://lemon-model.net/lemon#LexicalContext>
        a       <http://www.w3.org/2002/07/owl#Class> , <http://www.w3.org/2000/01/rdf-schema#Class> ;
        <http://www.w3.org/2000/01/rdf-schema#comment>
                "Indicates the pragmatic or discourse context in which a sense applies"@en ;
        <http://www.w3.org/2000/01/rdf-schema#label>
                "Lexikaal Context"@nl , "Contexte lexical"@fr , "Lexical Context"@en , "Contexto léxico"@es , "Lexikonkontext"@de ;
        <http://www.w3.org/2000/01/rdf-schema#subClassOf>
                <http://lemon-model.net/lemon#LemonElement> .

<http://lemon-model.net/lemon#separator>
        a       <http://www.w3.org/1999/02/22-rdf-syntax-ns#Property> , <http://www.w3.org/2002/07/owl#DatatypeProperty> ;
        <http://www.w3.org/2000/01/rdf-schema#comment>
                "Indicates the graphical element used to seperate the subnodes of this phrase structure. It is generally recommended that you use a string value with the language tag used to indicate script, (i.e., using ISO-15924 codes, such as \"Latn\"), as orthographic features may change with script."@en ;
        <http://www.w3.org/2000/01/rdf-schema#domain>
                <http://lemon-model.net/lemon#Node> ;
        <http://www.w3.org/2000/01/rdf-schema#label>
                "Separador"@es , "Separator"@en , "Separator"@de , "Séparateur"@fr , "Afscheider"@nl ;
        <http://www.w3.org/2000/01/rdf-schema#range>
                <http://www.w3.org/2001/XMLSchema#string> .

<http://lemon-model.net/lemon#UsageExample>
        a       <http://www.w3.org/2002/07/owl#Class> , <http://www.w3.org/2000/01/rdf-schema#Class> ;
        <http://www.w3.org/2000/01/rdf-schema#comment>
                "An example of the usage of a lexical entry when refering to the ontology entity given by the sememe's reference. This should in effect be an example of the form used in context. E.g., \"this is a *usage example*\""@en ;
        <http://www.w3.org/2000/01/rdf-schema#label>
                "Ejemplo de uso"@es , "Voorbeeld van het gebruik"@nl , "Exemple d'utilisation"@fr , "Usage Example"@en , "Anwendungsbeispiel"@de ;
        <http://www.w3.org/2000/01/rdf-schema#subClassOf>
                <http://lemon-model.net/lemon#LemonElement> ;
        <http://www.w3.org/2000/01/rdf-schema#subClassOf>
                [ a       <http://www.w3.org/2002/07/owl#Restriction> ;
                  <http://www.w3.org/2002/07/owl#minCardinality>
                          "1"^^<http://www.w3.org/2001/XMLSchema#nonNegativeInteger> ;
                  <http://www.w3.org/2002/07/owl#onProperty>
                          <http://lemon-model.net/lemon#value>
                ] .

<http://lemon-model.net/lemon#canonicalForm>
        a       <http://www.w3.org/2002/07/owl#ObjectProperty> , <http://www.w3.org/1999/02/22-rdf-syntax-ns#Property> , <http://www.w3.org/2002/07/owl#FunctionalProperty> ;
        <http://www.w3.org/2000/01/rdf-schema#comment>
                "The canonical (\"dictionary\") form of the lexical entry. This can be used to indicate the \"lemma\" form of a lexical entry"@en ;
        <http://www.w3.org/2000/01/rdf-schema#domain>
                <http://lemon-model.net/lemon#LexicalEntry> ;
        <http://www.w3.org/2000/01/rdf-schema#label>
                "Canonical form"@en , "Kanonische Form"@de , "Forme canonique"@fr , "Canonieke vorm"@nl , "Forma canónica"@es ;
        <http://www.w3.org/2000/01/rdf-schema#range>
                <http://lemon-model.net/lemon#Form> ;
        <http://www.w3.org/2000/01/rdf-schema#subPropertyOf>
                <http://lemon-model.net/lemon#lexicalForm> .

<http://lemon-model.net/lemon#value>
        a       <http://www.w3.org/2002/07/owl#DatatypeProperty> , <http://www.w3.org/1999/02/22-rdf-syntax-ns#Property> ;
        <http://www.w3.org/2000/01/rdf-schema#comment>
                "This indicates the value of a pseudo-data node. An example of this is definition where the value would generally be a string but it would not be possible to add further annotations, such as source or creation date."@en ;
        <http://www.w3.org/2000/01/rdf-schema#label>
                "Valeur"@fr , "Value"@en , "Wert"@de , "Valor"@es , "Waarde"@nl .

<http://lemon-model.net/lemon#SenseContext>
        a       <http://www.w3.org/2002/07/owl#Class> , <http://www.w3.org/2000/01/rdf-schema#Class> ;
        <http://www.w3.org/2000/01/rdf-schema#comment>
                "Indicates the context in which a term is to be used. The context refers not to the immediate syntactic context, but the document and register the document is used in"@en ;
        <http://www.w3.org/2000/01/rdf-schema#label>
                "Contexte"@fr , "Contexto"@es , "Kontext"@de , "Context"@nl , "Context"@en ;
        <http://www.w3.org/2000/01/rdf-schema#subClassOf>
                <http://lemon-model.net/lemon#LemonElement> .

<http://lemon-model.net/lemon#language>
        a       <http://www.w3.org/2002/07/owl#DatatypeProperty> , <http://www.w3.org/1999/02/22-rdf-syntax-ns#Property> ;
        <http://www.w3.org/2000/01/rdf-schema#comment>
                "The language of a given lexicon. This should be some ISO-639 string"@en ;
        <http://www.w3.org/2000/01/rdf-schema#domain>
                <http://lemon-model.net/lemon#HasLanguage> ;
        <http://www.w3.org/2000/01/rdf-schema#label>
                "Sprache"@de , "Language"@en , "Lengua"@es , "Taal"@nl , "Langue"@fr ;
        <http://www.w3.org/2000/01/rdf-schema#range>
                <http://www.w3.org/2001/XMLSchema#string> .

<http://lemon-model.net/lemon#synBehavior>
        a       <http://www.w3.org/2002/07/owl#ObjectProperty> , <http://www.w3.org/1999/02/22-rdf-syntax-ns#Property> ;
        <http://www.w3.org/2000/01/rdf-schema#comment>
                "Indicates a syntactic behavior of a lexical entry"@en ;
        <http://www.w3.org/2000/01/rdf-schema#domain>
                <http://lemon-model.net/lemon#LexicalEntry> ;
        <http://www.w3.org/2000/01/rdf-schema#label>
                "Syntactisch optreden"@nl , "Conduite syntaxique"@fr , "Syntactic behavior"@en , "Funcionamiento sintáctico"@es , "Syntactische Verhalten"@de ;
        <http://www.w3.org/2000/01/rdf-schema#range>
                <http://lemon-model.net/lemon#Frame> .

<http://lemon-model.net/lemon#constituent>
        a       <http://www.w3.org/2002/07/owl#ObjectProperty> , <http://www.w3.org/1999/02/22-rdf-syntax-ns#Property> ;
        <http://www.w3.org/2000/01/rdf-schema#domain>
                <http://lemon-model.net/lemon#Node> ;
        <http://www.w3.org/2000/01/rdf-schema#label>
                "Constitutif"@fr , "Constituent"@en , "Constituent"@nl , "Konstituent"@de , "Constituyente"@es ;
        <http://www.w3.org/2000/01/rdf-schema#range>
                <http://lemon-model.net/lemon#NodeConstituent> ;
        <http://www.w3.org/2000/01/rdf-schema#subPropertyOf>
                <http://www.w3.org/2002/07/owl#topObjectProperty> .

<http://lemon-model.net/lemon#example>
        a       <http://www.w3.org/1999/02/22-rdf-syntax-ns#Property> , <http://www.w3.org/2002/07/owl#ObjectProperty> ;
        <http://www.w3.org/2000/01/rdf-schema#domain>
                <http://lemon-model.net/lemon#LexicalSense> ;
        <http://www.w3.org/2000/01/rdf-schema#label>
                "Example"@en , "Beispiel"@de , "Exemple"@fr , "Ejemplo"@es , "Voorbeeld"@nl ;
        <http://www.w3.org/2000/01/rdf-schema#range>
                <http://lemon-model.net/lemon#UsageExample> .

<http://lemon-model.net/lemon#Part>
        a       <http://www.w3.org/2000/01/rdf-schema#Class> , <http://www.w3.org/2002/07/owl#Class> ;
        <http://www.w3.org/2000/01/rdf-schema#comment>
                "An affix is a morpheme that is attached to a word stem to form a new word.  Use this for lexical entries with only abstract forms"@en ;
        <http://www.w3.org/2000/01/rdf-schema#label>
                "Parte de la palabra"@es , "Wortteil"@de , "Deel van een woord"@nl , "Partie du mot"@fr , "Part of word"@en ;
        <http://www.w3.org/2000/01/rdf-schema#subClassOf>
                <http://lemon-model.net/lemon#LexicalEntry> .

<http://lemon-model.net/lemon#subsense>
        a       <http://www.w3.org/1999/02/22-rdf-syntax-ns#Property> , <http://www.w3.org/2002/07/owl#ObjectProperty> ;
        <http://www.w3.org/2000/01/rdf-schema#comment>
                "Indicates that the relation between a compound sense and its atomic subsenses"@en ;
        <http://www.w3.org/2000/01/rdf-schema#domain>
                <http://lemon-model.net/lemon#LexicalSense> ;
        <http://www.w3.org/2000/01/rdf-schema#label>
                "Parte del acepción"@es , "Deel van de zin"@nl , "Subsense"@en , "Teil des Sinnes"@de , "Signification composante"@fr ;
        <http://www.w3.org/2000/01/rdf-schema#range>
                <http://lemon-model.net/lemon#LexicalSense> .

<http://lemon-model.net/lemon#marker>
        a       <http://www.w3.org/1999/02/22-rdf-syntax-ns#Property> , <http://www.w3.org/2002/07/owl#ObjectProperty> ;
        <http://www.w3.org/2000/01/rdf-schema#comment>
                "Denotes the marker of a semantic argument. This should generally either be a semantic property i.e., case or another lexical entry e.g., a preposition or particle"@en ;
        <http://www.w3.org/2000/01/rdf-schema#domain>
                <http://lemon-model.net/lemon#Argument> ;
        <http://www.w3.org/2000/01/rdf-schema#label>
                "Merker"@nl , "Marqueur"@fr , "Marcador"@es , "Marker"@en , "Marker"@de ;
        <http://www.w3.org/2000/01/rdf-schema#range>
                <http://lemon-model.net/lemon#SynRoleMarker> .

<http://lemon-model.net/lemon#PropertyValue>
        a       <http://www.w3.org/2000/01/rdf-schema#Class> , <http://www.w3.org/2002/07/owl#Class> ;
        <http://www.w3.org/2000/01/rdf-schema#comment>
                "A value that can be used in the range of linguistic property"@en ;
        <http://www.w3.org/2000/01/rdf-schema#label>
                "Valor de la propiedad"@es , "Property Value"@en , "Prädikatswert"@de , "Waarde van het predikaat"@nl , "Valeur de la propriété"@fr ;
        <http://www.w3.org/2000/01/rdf-schema#subClassOf>
                <http://lemon-model.net/lemon#LemonElement> ;
        <http://www.w3.org/2002/07/owl#disjointWith>
                <http://lemon-model.net/lemon#UsageExample> , <http://lemon-model.net/lemon#SenseDefinition> .

<http://lemon-model.net/lemon#abstractForm>
        a       <http://www.w3.org/1999/02/22-rdf-syntax-ns#Property> , <http://www.w3.org/2002/07/owl#ObjectProperty> ;
        <http://www.w3.org/2000/01/rdf-schema#comment>
                "A representation of a lexical entry that should not be considered canonical. This is primarily from a linguistic view for non-realisable forms such as stems but may also include misspellings and other unusual forms"@en ;
        <http://www.w3.org/2000/01/rdf-schema#domain>
                <http://lemon-model.net/lemon#LexicalEntry> ;
        <http://www.w3.org/2000/01/rdf-schema#label>
                "Abstrakte Form"@de , "Forme abstraite"@fr , "Abstracte vorm"@nl , "Abstract form"@en , "Forma abstracta"@es ;
        <http://www.w3.org/2000/01/rdf-schema#range>
                <http://lemon-model.net/lemon#Form> ;
        <http://www.w3.org/2000/01/rdf-schema#subPropertyOf>
                <http://lemon-model.net/lemon#lexicalForm> .

<http://lemon-model.net/lemon#definition>
        a       <http://www.w3.org/1999/02/22-rdf-syntax-ns#Property> , <http://www.w3.org/2002/07/owl#ObjectProperty> ;
        <http://www.w3.org/2000/01/rdf-schema#comment>
                "Indicates a natural language definition. Note there is a pseudo-node to allow for further description of the definition (e.g., source, creation date etc.). The value property should be used to indicate the string value of the definition."@en ;
        <http://www.w3.org/2000/01/rdf-schema#domain>
                <http://lemon-model.net/lemon#LexicalSense> ;
        <http://www.w3.org/2000/01/rdf-schema#label>
                "Definición"@es , "Definitie"@nl , "Definition"@en , "Definition"@de , "Définition"@fr ;
        <http://www.w3.org/2000/01/rdf-schema#range>
                <http://lemon-model.net/lemon#SenseDefinition> .

<http://lemon-model.net/lemon#ComponentList>
        a       <http://www.w3.org/2002/07/owl#Class> , <http://www.w3.org/2000/01/rdf-schema#Class> ;
        <http://www.w3.org/2000/01/rdf-schema#comment>
                "A node within a list of components. This should generally be a blank node,see rdf:List"@en ;
        <http://www.w3.org/2000/01/rdf-schema#subClassOf>
                <http://www.w3.org/1999/02/22-rdf-syntax-ns#List> ;
        <http://www.w3.org/2000/01/rdf-schema#subClassOf>
                [ a       <http://www.w3.org/2002/07/owl#Restriction> ;
                  <http://www.w3.org/2002/07/owl#cardinality>
                          "1"^^<http://www.w3.org/2001/XMLSchema#nonNegativeInteger> ;
                  <http://www.w3.org/2002/07/owl#onProperty>
                          <http://www.w3.org/1999/02/22-rdf-syntax-ns#rest>
                ] ;
        <http://www.w3.org/2000/01/rdf-schema#subClassOf>
                [ a       <http://www.w3.org/2002/07/owl#Restriction> ;
                  <http://www.w3.org/2002/07/owl#allValuesFrom>
                          [ a       <http://www.w3.org/2000/01/rdf-schema#Class> ;
                            <http://www.w3.org/2002/07/owl#unionOf>
                                    ( <http://lemon-model.net/lemon#ComponentList>
                                      [ a       <http://www.w3.org/2000/01/rdf-schema#Class> ;
                                        <http://www.w3.org/2002/07/owl#oneOf>
                                                ( () )
                                      ]
                                    )
                          ] ;
                  <http://www.w3.org/2002/07/owl#onProperty>
                          <http://www.w3.org/1999/02/22-rdf-syntax-ns#rest>
                ] ;
        <http://www.w3.org/2000/01/rdf-schema#subClassOf>
                [ a       <http://www.w3.org/2002/07/owl#Restriction> ;
                  <http://www.w3.org/2002/07/owl#cardinality>
                          "1"^^<http://www.w3.org/2001/XMLSchema#nonNegativeInteger> ;
                  <http://www.w3.org/2002/07/owl#onProperty>
                          <http://www.w3.org/1999/02/22-rdf-syntax-ns#first>
                ] ;
        <http://www.w3.org/2000/01/rdf-schema#subClassOf>
                [ a       <http://www.w3.org/2002/07/owl#Restriction> ;
                  <http://www.w3.org/2002/07/owl#allValuesFrom>
                          <http://lemon-model.net/lemon#Component> ;
                  <http://www.w3.org/2002/07/owl#onProperty>
                          <http://www.w3.org/1999/02/22-rdf-syntax-ns#first>
                ] .

<http://lemon-model.net/lemon#Prototype>
        a       <http://www.w3.org/2000/01/rdf-schema#Class> , <http://www.w3.org/2002/07/owl#Class> ;
        <http://www.w3.org/2000/01/rdf-schema#label>
                "Prototype"@nl , "Prototyp"@nl , "Prototype"@fr , "Prototype"@en , "Prototipo"@es ;
        <http://www.w3.org/2000/01/rdf-schema#subClassOf>
                <http://lemon-model.net/lemon#LemonElement> .

<http://lemon-model.net/lemon#HasLanguage>
        a       <http://www.w3.org/2000/01/rdf-schema#Class> , <http://www.w3.org/2002/07/owl#Class> ;
        <http://www.w3.org/2000/01/rdf-schema#comment>
                "Structural element for all elements that can be tagged with a language"@en ;
        <http://www.w3.org/2000/01/rdf-schema#subClassOf>
                <http://lemon-model.net/lemon#LemonElement> .

<http://lemon-model.net/lemon#otherForm>
        a       <http://www.w3.org/1999/02/22-rdf-syntax-ns#Property> , <http://www.w3.org/2002/07/owl#ObjectProperty> ;
        <http://www.w3.org/2000/01/rdf-schema#comment>
                "A non-preferred (\"non-dictionary\") representation of a lexical entry. This should be variant that is either a morphological variant, an abbreviation, short form or acronym"@en ;
        <http://www.w3.org/2000/01/rdf-schema#domain>
                <http://lemon-model.net/lemon#LexicalEntry> ;
        <http://www.w3.org/2000/01/rdf-schema#label>
                "Andere vorm"@nl , "Andere Form"@de , "Other form"@en , "Otra forma"@es , "Autre forme"@fr ;
        <http://www.w3.org/2000/01/rdf-schema#range>
                <http://lemon-model.net/lemon#Form> ;
        <http://www.w3.org/2000/01/rdf-schema#subPropertyOf>
                <http://lemon-model.net/lemon#lexicalForm> .

<http://lemon-model.net/lemon#HasPattern>
        a       <http://www.w3.org/2002/07/owl#Class> , <http://www.w3.org/2000/01/rdf-schema#Class> ;
        <http://www.w3.org/2000/01/rdf-schema#subClassOf>
                <http://lemon-model.net/lemon#LemonElement> .
