<http://w3id.org/lindt/voc#divide>
        a       <http://w3id.org/lindt/voc#Function> ;
        <http://www.w3.org/2000/01/rdf-schema#comment>
                "A function to programmatically divide two literals."@en ;
        <http://www.w3.org/2000/01/rdf-schema#isDefinedBy>
                <http://w3id.org/lindt/voc#> ;
        <http://www.w3.org/2000/01/rdf-schema#label>
                "divide"@en ;
        <http://www.w3.org/2000/01/rdf-schema#seeAlso>
                <https://w3id.org/lindt/spec.html> ;
        <http://semweb.mmlab.be/ns/function#expects>
                ( [ <http://semweb.mmlab.be/ns/function#name>
                            "lexicalForm1" ;
                    <http://semweb.mmlab.be/ns/function#nullable>
                            false ;
                    <http://semweb.mmlab.be/ns/function#required>
                            true ;
                    <http://semweb.mmlab.be/ns/function#type>
                            <http://www.w3.org/2001/XMLSchema#string>
                  ]
                  [ <http://semweb.mmlab.be/ns/function#name>
                            "lexicalForm2" ;
                    <http://semweb.mmlab.be/ns/function#nullable>
                            false ;
                    <http://semweb.mmlab.be/ns/function#required>
                            true ;
                    <http://semweb.mmlab.be/ns/function#type>
                            <http://www.w3.org/2001/XMLSchema#string>
                  ]
                  [ <http://semweb.mmlab.be/ns/function#name>
                            "datatypeIri2" ;
                    <http://semweb.mmlab.be/ns/function#nullable>
                            false ;
                    <http://semweb.mmlab.be/ns/function#required>
                            false ;
                    <http://semweb.mmlab.be/ns/function#type>
                            <http://www.w3.org/2001/XMLSchema#string>
                  ]
                ) ;
        <http://semweb.mmlab.be/ns/function#name>
                "divide" ;
        <http://semweb.mmlab.be/ns/function#outputs>
                [ <http://semweb.mmlab.be/ns/function#type>
                          <http://www.w3.org/2001/XMLSchema#string> ] ;
        <http://www.w3.org/2003/06/sw-vocab-status/ns#term_status>
                "testing" .

<http://w3id.org/lindt/voc#hasComponentType>
        a       <http://www.w3.org/2002/07/owl#ObjectProperty> ;
        <http://www.w3.org/2000/01/rdf-schema#comment>
                "The datatype of the components of a list in this list datatype. For instance, the list datatype my:ListOfIntegers, having literals such as \"{35,42,12000,14,-3,33}\"^^my:ListOfIntegers, has component type xsd:integer."@en ;
        <http://www.w3.org/2000/01/rdf-schema#domain>
                <http://w3id.org/lindt/voc#ListDatatype> ;
        <http://www.w3.org/2000/01/rdf-schema#isDefinedBy>
                <http://w3id.org/lindt/voc#> ;
        <http://www.w3.org/2000/01/rdf-schema#label>
                "has component type"@en ;
        <http://www.w3.org/2000/01/rdf-schema#range>
                <http://www.w3.org/2000/01/rdf-schema#Datatype> ;
        <http://www.w3.org/2003/06/sw-vocab-status/ns#term_status>
                "testing" .

<http://w3id.org/lindt/voc#compare>
        a       <http://w3id.org/lindt/voc#Function> ;
        <http://www.w3.org/2000/01/rdf-schema#comment>
                "Answers if the value of literal with lexical form lexicalForm1 and this datatype is lower, equal, or greater than the value of literal with lexical form lexicalForm2 and datatype identified by IRI datatypeIri2."@en ;
        <http://www.w3.org/2000/01/rdf-schema#isDefinedBy>
                <http://w3id.org/lindt/voc#> ;
        <http://www.w3.org/2000/01/rdf-schema#label>
                "compare"@en ;
        <http://www.w3.org/2000/01/rdf-schema#seeAlso>
                <https://w3id.org/lindt/spec.html> ;
        <http://semweb.mmlab.be/ns/function#expects>
                ( [ a       <http://semweb.mmlab.be/ns/function#Parameter> ;
                    <http://semweb.mmlab.be/ns/function#name>
                            "lexicalForm1" ;
                    <http://semweb.mmlab.be/ns/function#nullable>
                            false ;
                    <http://semweb.mmlab.be/ns/function#required>
                            true ;
                    <http://semweb.mmlab.be/ns/function#type>
                            <http://www.w3.org/2001/XMLSchema#string>
                  ]
                  [ a       <http://semweb.mmlab.be/ns/function#Parameter> ;
                    <http://semweb.mmlab.be/ns/function#name>
                            "lexicalForm2" ;
                    <http://semweb.mmlab.be/ns/function#nullable>
                            false ;
                    <http://semweb.mmlab.be/ns/function#required>
                            true ;
                    <http://semweb.mmlab.be/ns/function#type>
                            <http://www.w3.org/2001/XMLSchema#string>
                  ]
                  [ a       <http://semweb.mmlab.be/ns/function#Parameter> ;
                    <http://semweb.mmlab.be/ns/function#name>
                            "datatypeIri2" ;
                    <http://semweb.mmlab.be/ns/function#nullable>
                            false ;
                    <http://semweb.mmlab.be/ns/function#required>
                            false ;
                    <http://semweb.mmlab.be/ns/function#type>
                            <http://www.w3.org/2001/XMLSchema#string>
                  ]
                ) ;
        <http://semweb.mmlab.be/ns/function#name>
                "compare" ;
        <http://semweb.mmlab.be/ns/function#outputs>
                [ a       <http://semweb.mmlab.be/ns/function#Output> ;
                  <http://semweb.mmlab.be/ns/function#type>
                          <http://www.w3.org/2001/XMLSchema#integer>
                ] ;
        <http://www.w3.org/2003/06/sw-vocab-status/ns#term_status>
                "testing" .

<http://w3id.org/lindt/voc#Ring>
        a       <http://www.w3.org/2002/07/owl#Class> ;
        <http://www.w3.org/2000/01/rdf-schema#comment>
                "The class of datatypes that are algebraic rings, which are also algebraic groups. The Javascript object representing this datatype should implement functions add, substract, and additiveIdentity as specified by class lindt:Group. Furthermore, it should also implement functions multiply(lexicalForm1:string, lexicalForm2:string):string and divide(lexicalForm1:string, lexicalForm2:string):string to multiply and divide two literals with this datatype. It should also implement function multiplicativeIdentity():string to retrieve the multiplicative identity element."@en ;
        <http://www.w3.org/2000/01/rdf-schema#isDefinedBy>
                <http://w3id.org/lindt/voc#> ;
        <http://www.w3.org/2000/01/rdf-schema#label>
                "Ring"@en ;
        <http://www.w3.org/2000/01/rdf-schema#subClassOf>
                <http://w3id.org/lindt/voc#Datatype> ;
        <http://www.w3.org/2000/01/rdf-schema#subClassOf>
                [ <http://www.w3.org/2002/07/owl#hasValue>
                          <http://w3id.org/lindt/voc#multiply> ;
                  <http://www.w3.org/2002/07/owl#onProperty>
                          <http://w3id.org/lindt/voc#implements>
                ] ;
        <http://www.w3.org/2000/01/rdf-schema#subClassOf>
                [ <http://www.w3.org/2002/07/owl#hasValue>
                          <http://w3id.org/lindt/voc#multiplicativeIdentity> ;
                  <http://www.w3.org/2002/07/owl#onProperty>
                          <http://w3id.org/lindt/voc#implements>
                ] ;
        <http://www.w3.org/2000/01/rdf-schema#subClassOf>
                [ <http://www.w3.org/2002/07/owl#hasValue>
                          <http://w3id.org/lindt/voc#divide> ;
                  <http://www.w3.org/2002/07/owl#onProperty>
                          <http://w3id.org/lindt/voc#implements>
                ] ;
        <http://www.w3.org/2003/06/sw-vocab-status/ns#term_status>
                "testing" .

<http://w3id.org/lindt/voc#>
        a       <http://purl.org/vocommons/voaf#Vocabulary> , <http://www.w3.org/2002/07/owl#Ontology> , <http://xmlns.com/foaf/0.1/Document> ;
        <http://www.w3.org/2000/01/rdf-schema#seeAlso>
                <https://w3id.org/lindt/spec.html> ;
        <http://creativecommons.org/ns#license>
                <https://www.apache.org/licenses/LICENSE-2.0> ;
        <http://purl.org/dc/terms/creator>
                <http://maxime-lefrancois.info/me#> , <http://zimmer.aprilfoolsreview.com/antoine#me> ;
        <http://purl.org/dc/terms/description>
                "The lindt (Linked Datatypes) vocabulary describes custom datatypes. \nThis vocabulary may be used by RDF processors and SPARQL engines to recognize custom datatypes on the fly.\n\n\nSee also:\n\n- [The Specification](spec.html)\n- [The Ontology](index.ttl)\n- [Some custom datatypes](custom_datatypes)\n\n"@en ;
        <http://purl.org/dc/terms/issued>
                "2016-04-22"^^<http://www.w3.org/2001/XMLSchema#date> ;
        <http://purl.org/dc/terms/modified>
                "2016-06-03T10:46:00+02:00"^^<http://www.w3.org/2001/XMLSchema#dateTime> , "2016-04-22"^^<http://www.w3.org/2001/XMLSchema#date> , "2016-04-22T10:42:42+02:00"^^<http://www.w3.org/2001/XMLSchema#dateTime> ;
        <http://purl.org/dc/terms/title>
                "The lindt Vocabulary "@en ;
        <http://purl.org/vocab/vann/preferredNamespacePrefix>
                "lindt" ;
        <http://purl.org/vocab/vann/preferredNamespaceUri>
                <http://w3id.org/lindt/voc#> ;
        <http://www.w3.org/2002/07/owl#imports>
                <http://semweb.mmlab.be/ns/function> .

<http://w3id.org/lindt/voc#Datatype>
        a       <http://www.w3.org/2002/07/owl#Class> ;
        <http://www.w3.org/2000/01/rdf-schema#comment>
                "The class of Linked Datatypes, that RDF processors and SPARQL engines should be able to recognize on the fly."@en ;
        <http://www.w3.org/2000/01/rdf-schema#isDefinedBy>
                <http://w3id.org/lindt/voc#> ;
        <http://www.w3.org/2000/01/rdf-schema#label>
                "Datatype"@en ;
        <http://www.w3.org/2000/01/rdf-schema#seeAlso>
                <https://w3id.org/lindt/spec.html> ;
        <http://www.w3.org/2000/01/rdf-schema#subClassOf>
                <http://www.w3.org/2000/01/rdf-schema#Datatype> ;
        <http://www.w3.org/2000/01/rdf-schema#subClassOf>
                [ <http://www.w3.org/2002/07/owl#hasValue>
                          <http://w3id.org/lindt/voc#recognisesDatatype> ;
                  <http://www.w3.org/2002/07/owl#onProperty>
                          <http://w3id.org/lindt/voc#implements>
                ] ;
        <http://www.w3.org/2000/01/rdf-schema#subClassOf>
                [ <http://www.w3.org/2002/07/owl#hasValue>
                          <http://w3id.org/lindt/voc#getNormalForm> ;
                  <http://www.w3.org/2002/07/owl#onProperty>
                          <http://w3id.org/lindt/voc#implements>
                ] ;
        <http://www.w3.org/2000/01/rdf-schema#subClassOf>
                [ <http://www.w3.org/2002/07/owl#hasValue>
                          <http://w3id.org/lindt/voc#isWellFormed> ;
                  <http://www.w3.org/2002/07/owl#onProperty>
                          <http://w3id.org/lindt/voc#implements>
                ] ;
        <http://www.w3.org/2000/01/rdf-schema#subClassOf>
                [ <http://www.w3.org/2002/07/owl#hasValue>
                          <http://w3id.org/lindt/voc#exportLiteral> ;
                  <http://www.w3.org/2002/07/owl#onProperty>
                          <http://w3id.org/lindt/voc#implements>
                ] ;
        <http://www.w3.org/2000/01/rdf-schema#subClassOf>
                [ <http://www.w3.org/2002/07/owl#hasValue>
                          <http://w3id.org/lindt/voc#getIri> ;
                  <http://www.w3.org/2002/07/owl#onProperty>
                          <http://w3id.org/lindt/voc#implements>
                ] ;
        <http://www.w3.org/2000/01/rdf-schema#subClassOf>
                [ <http://www.w3.org/2002/07/owl#hasValue>
                          <http://w3id.org/lindt/voc#importLiteral> ;
                  <http://www.w3.org/2002/07/owl#onProperty>
                          <http://w3id.org/lindt/voc#implements>
                ] ;
        <http://www.w3.org/2000/01/rdf-schema#subClassOf>
                [ <http://www.w3.org/2002/07/owl#hasValue>
                          <http://w3id.org/lindt/voc#getRecognisedDatatypes> ;
                  <http://www.w3.org/2002/07/owl#onProperty>
                          <http://w3id.org/lindt/voc#implements>
                ] ;
        <http://www.w3.org/2000/01/rdf-schema#subClassOf>
                [ <http://www.w3.org/2002/07/owl#hasValue>
                          <http://w3id.org/lindt/voc#isEqual> ;
                  <http://www.w3.org/2002/07/owl#onProperty>
                          <http://w3id.org/lindt/voc#implements>
                ] ;
        <http://www.w3.org/2003/06/sw-vocab-status/ns#term_status>
                "testing" .

<http://w3id.org/lindt/voc#literalsEndWith>
        a       <http://www.w3.org/2002/07/owl#FunctionalProperty> , <http://www.w3.org/2002/07/owl#DatatypeProperty> ;
        <http://www.w3.org/2000/01/rdf-schema#comment>
                "The string that must be present at the end of a literal of a compound datatype, when excluding the starting string. For instance \")\"."@en ;
        <http://www.w3.org/2000/01/rdf-schema#domain>
                <http://w3id.org/lindt/voc#CompoundDatatype> ;
        <http://www.w3.org/2000/01/rdf-schema#isDefinedBy>
                <http://w3id.org/lindt/voc#> ;
        <http://www.w3.org/2000/01/rdf-schema#label>
                "literals end with"@en ;
        <http://www.w3.org/2000/01/rdf-schema#range>
                <http://www.w3.org/2001/XMLSchema#string> ;
        <http://www.w3.org/2003/06/sw-vocab-status/ns#term_status>
                "testing" .

<http://w3id.org/lindt/voc#Group>
        a       <http://www.w3.org/2002/07/owl#Class> ;
        <http://www.w3.org/2000/01/rdf-schema#comment>
                "The class of datatypes that are algebraic groups. The Javascript object representing this datatype should implement functions add(lexicalForm1:string, lexicalForm2:string):string and substract(lexicalForm1:string, lexicalForm2:string):string to add and substract two literals with this datatype. It should also implement function additiveIdentity():string to retrieve the additive identity element."@en ;
        <http://www.w3.org/2000/01/rdf-schema#isDefinedBy>
                <http://w3id.org/lindt/voc#> ;
        <http://www.w3.org/2000/01/rdf-schema#label>
                "Group"@en ;
        <http://www.w3.org/2000/01/rdf-schema#subClassOf>
                <http://w3id.org/lindt/voc#Datatype> ;
        <http://www.w3.org/2000/01/rdf-schema#subClassOf>
                [ <http://www.w3.org/2002/07/owl#hasValue>
                          <http://w3id.org/lindt/voc#additiveIdentity> ;
                  <http://www.w3.org/2002/07/owl#onProperty>
                          <http://w3id.org/lindt/voc#implements>
                ] ;
        <http://www.w3.org/2000/01/rdf-schema#subClassOf>
                [ <http://www.w3.org/2002/07/owl#hasValue>
                          <http://w3id.org/lindt/voc#add> ;
                  <http://www.w3.org/2002/07/owl#onProperty>
                          <http://w3id.org/lindt/voc#implements>
                ] ;
        <http://www.w3.org/2000/01/rdf-schema#subClassOf>
                [ <http://www.w3.org/2002/07/owl#hasValue>
                          <http://w3id.org/lindt/voc#substract> ;
                  <http://www.w3.org/2002/07/owl#onProperty>
                          <http://w3id.org/lindt/voc#implements>
                ] ;
        <http://www.w3.org/2003/06/sw-vocab-status/ns#term_status>
                "testing" .

<http://w3id.org/lindt/voc#multiply>
        a       <http://w3id.org/lindt/voc#Function> ;
        <http://www.w3.org/2000/01/rdf-schema#comment>
                "A function to programmatically multiply two literals."@en ;
        <http://www.w3.org/2000/01/rdf-schema#isDefinedBy>
                <http://w3id.org/lindt/voc#> ;
        <http://www.w3.org/2000/01/rdf-schema#label>
                "multiply"@en ;
        <http://www.w3.org/2000/01/rdf-schema#seeAlso>
                <https://w3id.org/lindt/spec.html> ;
        <http://semweb.mmlab.be/ns/function#expects>
                ( [ <http://semweb.mmlab.be/ns/function#name>
                            "lexicalForm1" ;
                    <http://semweb.mmlab.be/ns/function#nullable>
                            false ;
                    <http://semweb.mmlab.be/ns/function#required>
                            true ;
                    <http://semweb.mmlab.be/ns/function#type>
                            <http://www.w3.org/2001/XMLSchema#string>
                  ]
                  [ <http://semweb.mmlab.be/ns/function#name>
                            "lexicalForm2" ;
                    <http://semweb.mmlab.be/ns/function#nullable>
                            false ;
                    <http://semweb.mmlab.be/ns/function#required>
                            true ;
                    <http://semweb.mmlab.be/ns/function#type>
                            <http://www.w3.org/2001/XMLSchema#string>
                  ]
                  [ <http://semweb.mmlab.be/ns/function#name>
                            "datatypeIri2" ;
                    <http://semweb.mmlab.be/ns/function#nullable>
                            false ;
                    <http://semweb.mmlab.be/ns/function#required>
                            false ;
                    <http://semweb.mmlab.be/ns/function#type>
                            <http://www.w3.org/2001/XMLSchema#string>
                  ]
                ) ;
        <http://semweb.mmlab.be/ns/function#name>
                "multiply" ;
        <http://semweb.mmlab.be/ns/function#outputs>
                [ <http://semweb.mmlab.be/ns/function#type>
                          <http://www.w3.org/2001/XMLSchema#string> ] ;
        <http://www.w3.org/2003/06/sw-vocab-status/ns#term_status>
                "testing" .

<http://w3id.org/lindt/voc#TotallyOrdered>
        a       <http://www.w3.org/2002/07/owl#Class> ;
        <http://www.w3.org/2000/01/rdf-schema#comment>
                "The class of datatypes that are totally ordered. The Javascript object representing this datatype should implement function compare(lexicalForm1:string, lexicalForm2:string):string, to compare two literals with this datatype."@en ;
        <http://www.w3.org/2000/01/rdf-schema#isDefinedBy>
                <http://w3id.org/lindt/voc#> ;
        <http://www.w3.org/2000/01/rdf-schema#label>
                "TotallyOrdered"@en ;
        <http://www.w3.org/2000/01/rdf-schema#subClassOf>
                <http://w3id.org/lindt/voc#Datatype> ;
        <http://www.w3.org/2000/01/rdf-schema#subClassOf>
                [ <http://www.w3.org/2002/07/owl#hasValue>
                          <http://w3id.org/lindt/voc#substract> ;
                  <http://www.w3.org/2002/07/owl#onProperty>
                          <http://w3id.org/lindt/voc#implements>
                ] ;
        <http://www.w3.org/2000/01/rdf-schema#subClassOf>
                [ <http://www.w3.org/2002/07/owl#hasValue>
                          <http://w3id.org/lindt/voc#additiveIdentity> ;
                  <http://www.w3.org/2002/07/owl#onProperty>
                          <http://w3id.org/lindt/voc#implements>
                ] ;
        <http://www.w3.org/2000/01/rdf-schema#subClassOf>
                [ <http://www.w3.org/2002/07/owl#hasValue>
                          <http://w3id.org/lindt/voc#compare> ;
                  <http://www.w3.org/2002/07/owl#onProperty>
                          <http://w3id.org/lindt/voc#implements>
                ] ;
        <http://www.w3.org/2003/06/sw-vocab-status/ns#term_status>
                "testing" .

<http://w3id.org/lindt/voc#implements>
        a       <http://www.w3.org/2002/07/owl#ObjectProperty> ;
        <http://www.w3.org/2000/01/rdf-schema#comment>
                "Links a datatype to the name of a function that the object representing this datatype should implement."@en ;
        <http://www.w3.org/2000/01/rdf-schema#domain>
                <http://w3id.org/lindt/voc#Datatype> ;
        <http://www.w3.org/2000/01/rdf-schema#isDefinedBy>
                <http://w3id.org/lindt/voc#> ;
        <http://www.w3.org/2000/01/rdf-schema#label>
                "implements"@en ;
        <http://www.w3.org/2000/01/rdf-schema#range>
                <http://w3id.org/lindt/voc#Function> ;
        <http://www.w3.org/2000/01/rdf-schema#seeAlso>
                <https://w3id.org/lindt/spec.html> ;
        <http://www.w3.org/2003/06/sw-vocab-status/ns#term_status>
                "testing" .

<http://w3id.org/lindt/voc#base>
        a       <http://www.w3.org/2002/07/owl#ObjectProperty> ;
        <http://www.w3.org/2000/01/rdf-schema#comment>
                "Links a datatype to one of its base datatype: \n(1) the lexical space of the subject datatype includes the lexical space of the object datatype; \n(2) the lexical-to-value mapping of the subject extends the lexical-to-value mapping of the object;\n(3) the ordering of lexical forms for the subject datatype extends the ordering of lexical forms of the object."@en ;
        <http://www.w3.org/2000/01/rdf-schema#domain>
                <http://w3id.org/lindt/voc#Datatype> ;
        <http://www.w3.org/2000/01/rdf-schema#isDefinedBy>
                <http://w3id.org/lindt/voc#> ;
        <http://www.w3.org/2000/01/rdf-schema#label>
                "base"@en ;
        <http://www.w3.org/2000/01/rdf-schema#range>
                <http://w3id.org/lindt/voc#Datatype> ;
        <http://www.w3.org/2000/01/rdf-schema#seeAlso>
                <https://w3id.org/lindt/spec.html> ;
        <http://www.w3.org/2003/06/sw-vocab-status/ns#term_status>
                "testing" .

<http://w3id.org/lindt/voc.ttl>
        a       <http://xmlns.com/foaf/0.1/Document> ;
        <http://purl.org/dc/terms/creator>
                <http://maxime-lefrancois.info/me#> , <http://zimmer.aprilfoolsreview.com/antoine#me> .

<http://w3id.org/lindt/voc#hasComponentTypes>
        a       <http://www.w3.org/1999/02/22-rdf-syntax-ns#Property> ;
        <http://www.w3.org/2000/01/rdf-schema#comment>
                "The datatypes of the components of a tuple in this tuple datatype. For instance, the tuple datatype my:sensorData, having literals such as \"(2013-10-09T11:14:22Z,129,metre)\"^^my:sensorData, has component types (xsd:dateTime, xsd:integer, xsd:string)."@en ;
        <http://www.w3.org/2000/01/rdf-schema#domain>
                <http://w3id.org/lindt/voc#TupleDatatype> ;
        <http://www.w3.org/2000/01/rdf-schema#isDefinedBy>
                <http://w3id.org/lindt/voc#> ;
        <http://www.w3.org/2000/01/rdf-schema#label>
                "has component types"@en ;
        <http://www.w3.org/2000/01/rdf-schema#range>
                <http://www.w3.org/1999/02/22-rdf-syntax-ns#List> ;
        <http://www.w3.org/2003/06/sw-vocab-status/ns#term_status>
                "testing" .

<http://w3id.org/lindt/voc#CompoundDatatype>
        a       <http://www.w3.org/2002/07/owl#Class> ;
        <http://www.w3.org/2000/01/rdf-schema#comment>
                "The class of datatypes that are composed of multiple values inside delimiting characters and separated by a certain string. For instance \"(0.234,846)\"^^my:pair."@en ;
        <http://www.w3.org/2000/01/rdf-schema#isDefinedBy>
                <http://w3id.org/lindt/voc#> ;
        <http://www.w3.org/2000/01/rdf-schema#label>
                "compound datatype"@en ;
        <http://www.w3.org/2000/01/rdf-schema#subClassOf>
                <http://w3id.org/lindt/voc#Datatype> ;
        <http://www.w3.org/2003/06/sw-vocab-status/ns#term_status>
                "testing" .

<http://w3id.org/lindt/voc#separator>
        a       <http://www.w3.org/2002/07/owl#FunctionalProperty> , <http://www.w3.org/2002/07/owl#DatatypeProperty> ;
        <http://www.w3.org/2000/01/rdf-schema#comment>
                "The string that must separate two values within a literal of a compound datatype. For instance \",\"."@en ;
        <http://www.w3.org/2000/01/rdf-schema#domain>
                <http://w3id.org/lindt/voc#CompoundDatatype> ;
        <http://www.w3.org/2000/01/rdf-schema#isDefinedBy>
                <http://w3id.org/lindt/voc#> ;
        <http://www.w3.org/2000/01/rdf-schema#label>
                "separator"@en ;
        <http://www.w3.org/2000/01/rdf-schema#range>
                <http://www.w3.org/2001/XMLSchema#string> ;
        <http://www.w3.org/2003/06/sw-vocab-status/ns#term_status>
                "testing" .

<http://w3id.org/lindt/voc#additiveIdentity>
        a       <http://w3id.org/lindt/voc#Function> ;
        <http://www.w3.org/2000/01/rdf-schema#comment>
                "A function to programmatically get the neutral literal for function lindt:add."@en ;
        <http://www.w3.org/2000/01/rdf-schema#isDefinedBy>
                <http://w3id.org/lindt/voc#> ;
        <http://www.w3.org/2000/01/rdf-schema#label>
                "additiveIdentity"@en ;
        <http://www.w3.org/2000/01/rdf-schema#seeAlso>
                <https://w3id.org/lindt/spec.html> ;
        <http://semweb.mmlab.be/ns/function#expects>
                () ;
        <http://semweb.mmlab.be/ns/function#name>
                "additiveIdentity" ;
        <http://semweb.mmlab.be/ns/function#outputs>
                [ <http://semweb.mmlab.be/ns/function#type>
                          <http://www.w3.org/2001/XMLSchema#string> ] ;
        <http://www.w3.org/2003/06/sw-vocab-status/ns#term_status>
                "testing" .

<http://w3id.org/lindt/voc#Function>
        a       <http://www.w3.org/2002/07/owl#Class> ;
        <http://www.w3.org/2000/01/rdf-schema#comment>
                "The class of functions that objects representing lindt datatype implement."@en ;
        <http://www.w3.org/2000/01/rdf-schema#isDefinedBy>
                <http://w3id.org/lindt/voc#> ;
        <http://www.w3.org/2000/01/rdf-schema#label>
                "Function"@en ;
        <http://www.w3.org/2000/01/rdf-schema#seeAlso>
                <https://w3id.org/lindt/spec.html> ;
        <http://www.w3.org/2000/01/rdf-schema#subClassOf>
                <http://semweb.mmlab.be/ns/function#Function> ;
        <http://www.w3.org/2003/06/sw-vocab-status/ns#term_status>
                "testing" .

<http://w3id.org/lindt/voc#isEqual>
        a       <http://w3id.org/lindt/voc#Function> ;
        <http://www.w3.org/2000/01/rdf-schema#comment>
                "Answers if literal with lexical form lexicalForm1 and this datatype has the same value as literal with lexical form lexicalForm2 and datatype identified by IRI datatypeIri2."@en ;
        <http://www.w3.org/2000/01/rdf-schema#isDefinedBy>
                <http://w3id.org/lindt/voc#> ;
        <http://www.w3.org/2000/01/rdf-schema#label>
                "isEqual"@en ;
        <http://www.w3.org/2000/01/rdf-schema#seeAlso>
                <https://w3id.org/lindt/spec.html> ;
        <http://semweb.mmlab.be/ns/function#expects>
                ( [ <http://semweb.mmlab.be/ns/function#name>
                            "lexicalForm1" ;
                    <http://semweb.mmlab.be/ns/function#nullable>
                            false ;
                    <http://semweb.mmlab.be/ns/function#required>
                            true ;
                    <http://semweb.mmlab.be/ns/function#type>
                            <http://www.w3.org/2001/XMLSchema#string>
                  ]
                  [ <http://semweb.mmlab.be/ns/function#name>
                            "lexicalForm2" ;
                    <http://semweb.mmlab.be/ns/function#nullable>
                            false ;
                    <http://semweb.mmlab.be/ns/function#required>
                            true ;
                    <http://semweb.mmlab.be/ns/function#type>
                            <http://www.w3.org/2001/XMLSchema#string>
                  ]
                  [ <http://semweb.mmlab.be/ns/function#name>
                            "datatypeIri2" ;
                    <http://semweb.mmlab.be/ns/function#nullable>
                            false ;
                    <http://semweb.mmlab.be/ns/function#required>
                            false ;
                    <http://semweb.mmlab.be/ns/function#type>
                            <http://www.w3.org/2001/XMLSchema#string>
                  ]
                ) ;
        <http://semweb.mmlab.be/ns/function#name>
                "isEqual" ;
        <http://semweb.mmlab.be/ns/function#outputs>
                [ <http://semweb.mmlab.be/ns/function#type>
                          <http://www.w3.org/2001/XMLSchema#boolean> ] ;
        <http://www.w3.org/2003/06/sw-vocab-status/ns#term_status>
                "testing" .

<http://w3id.org/lindt/voc#stringListDatatype>
        a       <http://w3id.org/lindt/voc#ListDatatype> ;
        <http://www.w3.org/2000/01/rdf-schema#comment>
                "a list of strings, starting with \"(\", separated by \",\", and ending with \")\""@en ;
        <http://www.w3.org/2000/01/rdf-schema#isDefinedBy>
                <http://w3id.org/lindt/voc#> ;
        <http://www.w3.org/2000/01/rdf-schema#label>
                "stringListDatatype"@en ;
        <http://w3id.org/lindt/voc#literalsEndsWith>
                ")" ;
        <http://w3id.org/lindt/voc#literalsStartWith>
                "(" ;
        <http://w3id.org/lindt/voc#separator>
                "," ;
        <http://www.w3.org/2003/06/sw-vocab-status/ns#term_status>
                "testing" .

<http://w3id.org/lindt/voc#TupleDatatype>
        a       <http://www.w3.org/2002/07/owl#Class> ;
        <http://www.w3.org/2000/01/rdf-schema#comment>
                "The class of datatypes where literals consist of a starting string, followed by a sequence of values from a predefined list of datatypes. For instance \"(2013-10-09T11:14:22Z,129,metre)\"^^my:sensorData."@en ;
        <http://www.w3.org/2000/01/rdf-schema#isDefinedBy>
                <http://w3id.org/lindt/voc#> ;
        <http://www.w3.org/2000/01/rdf-schema#label>
                "tuple datatype"@en ;
        <http://www.w3.org/2000/01/rdf-schema#subClassOf>
                <http://w3id.org/lindt/voc#CompoundDatatype> ;
        <http://www.w3.org/2003/06/sw-vocab-status/ns#term_status>
                "testing" .

<http://w3id.org/lindt/voc#importLiteral>
        a       <http://w3id.org/lindt/voc#Function> ;
        <http://www.w3.org/2000/01/rdf-schema#comment>
                "Answers the lexical form of a literal with this datatype, with a value equal to that of a literal with lexical form lexicalForm and datatype identified by datatypeIri."@en ;
        <http://www.w3.org/2000/01/rdf-schema#isDefinedBy>
                <http://w3id.org/lindt/voc#> ;
        <http://www.w3.org/2000/01/rdf-schema#label>
                "importLiteral"@en ;
        <http://www.w3.org/2000/01/rdf-schema#seeAlso>
                <https://w3id.org/lindt/spec.html> ;
        <http://semweb.mmlab.be/ns/function#expects>
                ( [ <http://semweb.mmlab.be/ns/function#name>
                            "lexicalForm" ;
                    <http://semweb.mmlab.be/ns/function#nullable>
                            false ;
                    <http://semweb.mmlab.be/ns/function#required>
                            true ;
                    <http://semweb.mmlab.be/ns/function#type>
                            <http://www.w3.org/2001/XMLSchema#string>
                  ]
                  [ <http://semweb.mmlab.be/ns/function#name>
                            "datatypeIri" ;
                    <http://semweb.mmlab.be/ns/function#nullable>
                            false ;
                    <http://semweb.mmlab.be/ns/function#required>
                            true ;
                    <http://semweb.mmlab.be/ns/function#type>
                            <http://www.w3.org/2001/XMLSchema#string>
                  ]
                ) ;
        <http://semweb.mmlab.be/ns/function#name>
                "importLiteral" ;
        <http://semweb.mmlab.be/ns/function#outputs>
                [ <http://semweb.mmlab.be/ns/function#type>
                          <http://www.w3.org/2001/XMLSchema#string> ] ;
        <http://www.w3.org/2003/06/sw-vocab-status/ns#term_status>
                "testing" .

<http://w3id.org/lindt/voc#add>
        a       <http://w3id.org/lindt/voc#Function> ;
        <http://www.w3.org/2000/01/rdf-schema#comment>
                "A function to programmatically add two literals."@en ;
        <http://www.w3.org/2000/01/rdf-schema#isDefinedBy>
                <http://w3id.org/lindt/voc#> ;
        <http://www.w3.org/2000/01/rdf-schema#label>
                "add"@en ;
        <http://www.w3.org/2000/01/rdf-schema#seeAlso>
                <https://w3id.org/lindt/spec.html> ;
        <http://semweb.mmlab.be/ns/function#expects>
                ( [ <http://semweb.mmlab.be/ns/function#name>
                            "lexicalForm1" ;
                    <http://semweb.mmlab.be/ns/function#nullable>
                            false ;
                    <http://semweb.mmlab.be/ns/function#required>
                            true ;
                    <http://semweb.mmlab.be/ns/function#type>
                            <http://www.w3.org/2001/XMLSchema#string>
                  ]
                  [ <http://semweb.mmlab.be/ns/function#name>
                            "lexicalForm2" ;
                    <http://semweb.mmlab.be/ns/function#nullable>
                            false ;
                    <http://semweb.mmlab.be/ns/function#required>
                            true ;
                    <http://semweb.mmlab.be/ns/function#type>
                            <http://www.w3.org/2001/XMLSchema#string>
                  ]
                  [ <http://semweb.mmlab.be/ns/function#name>
                            "datatypeIri2" ;
                    <http://semweb.mmlab.be/ns/function#nullable>
                            false ;
                    <http://semweb.mmlab.be/ns/function#required>
                            false ;
                    <http://semweb.mmlab.be/ns/function#type>
                            <http://www.w3.org/2001/XMLSchema#string>
                  ]
                ) ;
        <http://semweb.mmlab.be/ns/function#name>
                "add" ;
        <http://semweb.mmlab.be/ns/function#outputs>
                [ <http://semweb.mmlab.be/ns/function#type>
                          <http://www.w3.org/2001/XMLSchema#string> ] ;
        <http://www.w3.org/2003/06/sw-vocab-status/ns#term_status>
                "testing" .

<http://w3id.org/lindt/voc#getRecognisedDatatypes>
        a       <http://w3id.org/lindt/voc#Function> ;
        <http://www.w3.org/2000/01/rdf-schema#comment>
                "Answers an array of datatypes IRI this custom datatype recognises."@en ;
        <http://www.w3.org/2000/01/rdf-schema#isDefinedBy>
                <http://w3id.org/lindt/voc#> ;
        <http://www.w3.org/2000/01/rdf-schema#label>
                "getRecognisedDatatypes"@en ;
        <http://www.w3.org/2000/01/rdf-schema#seeAlso>
                <https://w3id.org/lindt/spec.html> ;
        <http://semweb.mmlab.be/ns/function#expects>
                () ;
        <http://semweb.mmlab.be/ns/function#name>
                "getRecognisedDatatypes" ;
        <http://semweb.mmlab.be/ns/function#outputs>
                [ <http://semweb.mmlab.be/ns/function#type>
                          <http://w3id.org/lindt/voc#stringListDatatype> ] ;
        <http://www.w3.org/2003/06/sw-vocab-status/ns#term_status>
                "testing" .

<http://w3id.org/lindt/voc#recognisesDatatype>
        a       <http://w3id.org/lindt/voc#Function> ;
        <http://www.w3.org/2000/01/rdf-schema#comment>
                "Answers if this custom datatype recognises the datatype with the given IRI."@en ;
        <http://www.w3.org/2000/01/rdf-schema#isDefinedBy>
                <http://w3id.org/lindt/voc#> ;
        <http://www.w3.org/2000/01/rdf-schema#label>
                "recognisesDatatype"@en ;
        <http://www.w3.org/2000/01/rdf-schema#seeAlso>
                <https://w3id.org/lindt/spec.html> ;
        <http://semweb.mmlab.be/ns/function#expects>
                ( [ <http://semweb.mmlab.be/ns/function#name>
                            "datatypeIri" ;
                    <http://semweb.mmlab.be/ns/function#nullable>
                            false ;
                    <http://semweb.mmlab.be/ns/function#required>
                            true ;
                    <http://semweb.mmlab.be/ns/function#type>
                            <http://www.w3.org/2001/XMLSchema#string>
                  ]
                ) ;
        <http://semweb.mmlab.be/ns/function#name>
                "recognisesDatatype" ;
        <http://semweb.mmlab.be/ns/function#outputs>
                [ <http://semweb.mmlab.be/ns/function#type>
                          <http://www.w3.org/2001/XMLSchema#boolean> ] ;
        <http://www.w3.org/2003/06/sw-vocab-status/ns#term_status>
                "testing" .

<http://w3id.org/lindt/voc#getIri>
        a       <http://w3id.org/lindt/voc#Function> ;
        <http://www.w3.org/2000/01/rdf-schema#comment>
                "Returns the IRI of this custom datatype."@en ;
        <http://www.w3.org/2000/01/rdf-schema#isDefinedBy>
                <http://w3id.org/lindt/voc#> ;
        <http://www.w3.org/2000/01/rdf-schema#label>
                "getIri"@en ;
        <http://www.w3.org/2000/01/rdf-schema#seeAlso>
                <https://w3id.org/lindt/spec.html> ;
        <http://semweb.mmlab.be/ns/function#expects>
                () ;
        <http://semweb.mmlab.be/ns/function#name>
                "getIri" ;
        <http://semweb.mmlab.be/ns/function#outputs>
                [ <http://semweb.mmlab.be/ns/function#type>
                          <http://www.w3.org/2001/XMLSchema#string> ] ;
        <http://www.w3.org/2003/06/sw-vocab-status/ns#term_status>
                "testing" .

<http://w3id.org/lindt/voc#substract>
        a       <http://w3id.org/lindt/voc#Function> ;
        <http://www.w3.org/2000/01/rdf-schema#comment>
                "A function to programmatically substract two literals."@en ;
        <http://www.w3.org/2000/01/rdf-schema#isDefinedBy>
                <http://w3id.org/lindt/voc#> ;
        <http://www.w3.org/2000/01/rdf-schema#label>
                "substract"@en ;
        <http://www.w3.org/2000/01/rdf-schema#seeAlso>
                <https://w3id.org/lindt/spec.html> ;
        <http://semweb.mmlab.be/ns/function#expects>
                ( [ <http://semweb.mmlab.be/ns/function#name>
                            "lexicalForm1" ;
                    <http://semweb.mmlab.be/ns/function#nullable>
                            false ;
                    <http://semweb.mmlab.be/ns/function#required>
                            true ;
                    <http://semweb.mmlab.be/ns/function#type>
                            <http://www.w3.org/2001/XMLSchema#string>
                  ]
                  [ <http://semweb.mmlab.be/ns/function#name>
                            "lexicalForm2" ;
                    <http://semweb.mmlab.be/ns/function#nullable>
                            false ;
                    <http://semweb.mmlab.be/ns/function#required>
                            true ;
                    <http://semweb.mmlab.be/ns/function#type>
                            <http://www.w3.org/2001/XMLSchema#string>
                  ]
                  [ <http://semweb.mmlab.be/ns/function#name>
                            "datatypeIri2" ;
                    <http://semweb.mmlab.be/ns/function#nullable>
                            false ;
                    <http://semweb.mmlab.be/ns/function#required>
                            false ;
                    <http://semweb.mmlab.be/ns/function#type>
                            <http://www.w3.org/2001/XMLSchema#string>
                  ]
                ) ;
        <http://semweb.mmlab.be/ns/function#name>
                "substract" ;
        <http://semweb.mmlab.be/ns/function#outputs>
                [ <http://semweb.mmlab.be/ns/function#type>
                          <http://www.w3.org/2001/XMLSchema#string> ] ;
        <http://www.w3.org/2003/06/sw-vocab-status/ns#term_status>
                "testing" .

<http://w3id.org/lindt/voc#isWellFormed>
        a       <http://w3id.org/lindt/voc#Function> ;
        <http://www.w3.org/2000/01/rdf-schema#comment>
                "Answers if this lexical form is well formed."@en ;
        <http://www.w3.org/2000/01/rdf-schema#isDefinedBy>
                <http://w3id.org/lindt/voc#> ;
        <http://www.w3.org/2000/01/rdf-schema#label>
                "isWellFormed"@en ;
        <http://www.w3.org/2000/01/rdf-schema#seeAlso>
                <https://w3id.org/lindt/spec.html> ;
        <http://semweb.mmlab.be/ns/function#expects>
                ( [ <http://semweb.mmlab.be/ns/function#name>
                            "lexicalForm" ;
                    <http://semweb.mmlab.be/ns/function#nullable>
                            false ;
                    <http://semweb.mmlab.be/ns/function#required>
                            true ;
                    <http://semweb.mmlab.be/ns/function#type>
                            <http://www.w3.org/2001/XMLSchema#string>
                  ]
                ) ;
        <http://semweb.mmlab.be/ns/function#name>
                "isWellFormed" ;
        <http://semweb.mmlab.be/ns/function#outputs>
                [ <http://semweb.mmlab.be/ns/function#type>
                          <http://www.w3.org/2001/XMLSchema#boolean> ] ;
        <http://www.w3.org/2003/06/sw-vocab-status/ns#term_status>
                "testing" .

<http://w3id.org/lindt/voc#literalsStartWith>
        a       <http://www.w3.org/2002/07/owl#FunctionalProperty> , <http://www.w3.org/2002/07/owl#DatatypeProperty> ;
        <http://www.w3.org/2000/01/rdf-schema#comment>
                "The string that must be present at the beginning of a literal of a compound datatype. For instance \"(\"."@en ;
        <http://www.w3.org/2000/01/rdf-schema#domain>
                <http://w3id.org/lindt/voc#CompoundDatype> ;
        <http://www.w3.org/2000/01/rdf-schema#isDefinedBy>
                <http://w3id.org/lindt/voc#> ;
        <http://www.w3.org/2000/01/rdf-schema#label>
                "literals start with"@en ;
        <http://www.w3.org/2000/01/rdf-schema#range>
                <http://www.w3.org/2001/XMLSchema#string> ;
        <http://www.w3.org/2003/06/sw-vocab-status/ns#term_status>
                "testing" .

<http://w3id.org/lindt/voc#exportLiteral>
        a       <http://w3id.org/lindt/voc#Function> ;
        <http://www.w3.org/2000/01/rdf-schema#comment>
                "Answers the lexical form of a literal with datatype identified by datatypeIri, with a value equal to that of a literal with lexical form lexicalForm and this datatype."@en ;
        <http://www.w3.org/2000/01/rdf-schema#isDefinedBy>
                <http://w3id.org/lindt/voc#> ;
        <http://www.w3.org/2000/01/rdf-schema#label>
                "exportLiteral"@en ;
        <http://www.w3.org/2000/01/rdf-schema#seeAlso>
                <https://w3id.org/lindt/spec.html> ;
        <http://semweb.mmlab.be/ns/function#expects>
                ( [ <http://semweb.mmlab.be/ns/function#name>
                            "lexicalForm" ;
                    <http://semweb.mmlab.be/ns/function#nullable>
                            false ;
                    <http://semweb.mmlab.be/ns/function#required>
                            true ;
                    <http://semweb.mmlab.be/ns/function#type>
                            <http://www.w3.org/2001/XMLSchema#string>
                  ]
                  [ <http://semweb.mmlab.be/ns/function#name>
                            "datatypeIri" ;
                    <http://semweb.mmlab.be/ns/function#nullable>
                            false ;
                    <http://semweb.mmlab.be/ns/function#required>
                            true ;
                    <http://semweb.mmlab.be/ns/function#type>
                            <http://www.w3.org/2001/XMLSchema#string>
                  ]
                ) ;
        <http://semweb.mmlab.be/ns/function#name>
                "exportLiteral" ;
        <http://semweb.mmlab.be/ns/function#outputs>
                [ <http://semweb.mmlab.be/ns/function#type>
                          <http://www.w3.org/2001/XMLSchema#string> ] ;
        <http://www.w3.org/2003/06/sw-vocab-status/ns#term_status>
                "testing" .

<http://w3id.org/lindt/voc#ListDatatype>
        a       <http://www.w3.org/2002/07/owl#Class> ;
        <http://www.w3.org/2000/01/rdf-schema#comment>
                "The class of datatypes where literals consist of a starting string, followed by a possibly empty list of values in a given datatype separated by a separating string, and finishing with an ending string. For instance \"{35,42,12000,14,-3,33}\"^^my:ListOfIntegers."@en ;
        <http://www.w3.org/2000/01/rdf-schema#isDefinedBy>
                <http://w3id.org/lindt/voc#> ;
        <http://www.w3.org/2000/01/rdf-schema#label>
                "list datatype"@en ;
        <http://www.w3.org/2000/01/rdf-schema#subClassOf>
                <http://w3id.org/lindt/voc#CompoundDatatype> ;
        <http://www.w3.org/2003/06/sw-vocab-status/ns#term_status>
                "testing" .

<http://w3id.org/lindt/voc#multiplicativeIdentity>
        a       <http://w3id.org/lindt/voc#Function> ;
        <http://www.w3.org/2000/01/rdf-schema#comment>
                "A function to programmatically get the neutral literal for function lindt:multiply."@en ;
        <http://www.w3.org/2000/01/rdf-schema#isDefinedBy>
                <http://w3id.org/lindt/voc#> ;
        <http://www.w3.org/2000/01/rdf-schema#label>
                "multiplicativeIdentity"@en ;
        <http://www.w3.org/2000/01/rdf-schema#seeAlso>
                <https://w3id.org/lindt/spec.html> ;
        <http://semweb.mmlab.be/ns/function#expects>
                () ;
        <http://semweb.mmlab.be/ns/function#name>
                "getNormalForm" ;
        <http://semweb.mmlab.be/ns/function#outputs>
                [ <http://semweb.mmlab.be/ns/function#type>
                          <http://www.w3.org/2001/XMLSchema#string> ] ;
        <http://www.w3.org/2003/06/sw-vocab-status/ns#term_status>
                "testing" .

<http://w3id.org/lindt/voc#getNormalForm>
        a       <http://w3id.org/lindt/voc#Function> ;
        <http://www.w3.org/2000/01/rdf-schema#comment>
                "Answers the normalized lexical form of the literal with lexical form lexicalForm and this datatype."@en ;
        <http://www.w3.org/2000/01/rdf-schema#isDefinedBy>
                <http://w3id.org/lindt/voc#> ;
        <http://www.w3.org/2000/01/rdf-schema#label>
                "getNormalForm"@en ;
        <http://www.w3.org/2000/01/rdf-schema#seeAlso>
                <https://w3id.org/lindt/spec.html> ;
        <http://semweb.mmlab.be/ns/function#expects>
                ( [ <http://semweb.mmlab.be/ns/function#name>
                            "lexicalForm" ;
                    <http://semweb.mmlab.be/ns/function#nullable>
                            false ;
                    <http://semweb.mmlab.be/ns/function#required>
                            true ;
                    <http://semweb.mmlab.be/ns/function#type>
                            <http://www.w3.org/2001/XMLSchema#string>
                  ]
                ) ;
        <http://semweb.mmlab.be/ns/function#name>
                "getNormalForm" ;
        <http://semweb.mmlab.be/ns/function#outputs>
                [ <http://semweb.mmlab.be/ns/function#type>
                          <http://www.w3.org/2001/XMLSchema#string> ] ;
        <http://www.w3.org/2003/06/sw-vocab-status/ns#term_status>
                "testing" .
