<http://purl.org/olia/olia.owl#IndicativeMood>
        a       <http://www.w3.org/2002/07/owl#Class> ;
        <http://www.w3.org/2000/01/rdf-schema#comment>
                "\n\t\tThe indicative is the unmarked mood. It is used when no special modal \n\t\tnuance in the clause or sentence is intended. It is the default mood \n\t\tof independent declarative and often also of interrogative sentences. \n\t\t(http://www.uni-erfurt.de/sprachwissenschaft/proxy.php?port=8080&file=lido/servlet/Lido_Servlet Indikativ 18.06.07)\n\t\t\n\t\tExpression of assertion. (Bybee 1985:22) \n\t\tPertaining to the mood or mode of a verb form or clause such that it \n\t\tpredicates a stated relation of objective fact (OED).\n\t\t(http://languagelink.let.uu.nl/tds/onto/LinguisticOntology.owl#indicativeModality)\n\t" ;
        <http://www.w3.org/2000/01/rdf-schema#subClassOf>
                <http://purl.org/olia/olia.owl#DeclarativeModality> , <http://purl.org/olia/olia-top.owl#MoodFeature> ;
        <http://www.w3.org/2002/07/owl#versionInfo>
                "\n\t\thttp://purl.org/linguistics/gold/Indicative, \n\t\thttp://languagelink.let.uu.nl/tds/onto/LinguisticOntology.owl#indicativeModality\n\t" , "TODO: check relationship with DeclarativeMood" .

<http://purl.org/olia/olia.owl#DegreeAdverb>
        a       <http://www.w3.org/2002/07/owl#Class> ;
        <http://www.w3.org/2000/01/rdf-schema#comment>
                "\n\t\t\tAny adverb which modifies an adjective, an adverb, a verbal particle, a preposition, \n\t\t\ta conjunction or a determiner is a degree adverb. \n\t\t\t(http://xlex.uni-muenster.de/Portal/MTPE/tagsetDescriptionEN.doc, p. 113, 8.1 Degree Adverbs 23.09.06)\n\t\t\t\n\t\t\tAlso known as specifier adverb (http://www.unlweb.net/unlarium/dictionary/export_tagset.php)\n\t\t" ;
        <http://www.w3.org/2000/01/rdf-schema#label>
                "specifier adverb" , "degree adverb" ;
        <http://www.w3.org/2000/01/rdf-schema#subClassOf>
                <http://purl.org/olia/olia.owl#Adverb> ;
        <http://www.w3.org/2002/07/owl#versionInfo>
                "EAGLES Adverb with Adverb-Type=\"Degree\"." .

<http://purl.org/olia/olia.owl#AffirmativeParticle>
        a       <http://www.w3.org/2002/07/owl#Class> ;
        <http://www.w3.org/2000/01/rdf-schema#comment>
                "\n                            Particle used to express affirmation.\n                                (http://www.isocat.org/datcat/DC-1918)\n                            " ;
        <http://www.w3.org/2000/01/rdf-schema#label>
                "particule affirmative" ;
        <http://www.w3.org/2000/01/rdf-schema#subClassOf>
                <http://purl.org/olia/olia.owl#Particle> ;
        <http://www.w3.org/2002/07/owl#versionInfo>
                "subClassOf particle (dcif:isA)" , "http://www.isocat.org/datcat/DC-1918" .

<http://purl.org/olia/olia.owl#AbessiveCase>
        a       <http://www.w3.org/2002/07/owl#Class> ;
        <http://www.w3.org/2000/01/rdf-schema#comment>
                "\n\t\t\tAbessiveCase expresses the lack or absence of the referent of the \n\t\t\tnoun it marks. It has the meaning of the English preposition 'without' \n\t\t\t(Pei and Gaynor 1954: 3,35; Gove, et al. 1966: 3).\n\t\t\t(http://purl.org/linguistics/gold/Abessive)\n\t\t" ;
        <http://www.w3.org/2000/01/rdf-schema#subClassOf>
                <http://purl.org/olia/olia-top.owl#CaseFeature> ;
        <http://www.w3.org/2002/07/owl#versionInfo>
                "http://purl.org/linguistics/gold/Abessive, http://www.isocat.org/datcat/DC-1223" .

<http://purl.org/olia/olia.owl#VerbalAdverb>
        a       <http://www.w3.org/2002/07/owl#Class> ;
        <http://www.w3.org/2000/01/rdf-schema#comment>
                "\n\t\t\tAdverb/Type=\"verbal\" applies to adverbs derived from from verbs (verbal adverbs) in the Serbian, Macedonian and Hungarian MTE v4 specs. Macedonian verbal adverbs (gerunds) like odejkji are thus not considered as verbal forms, but as Adverb/Type=\"verbal\". (MTE v4)\n\t\t\t(http://purl.org/olia/mte/multext-east.owl#VerbalAdverb)" ;
        <http://www.w3.org/2000/01/rdf-schema#subClassOf>
                <http://purl.org/olia/olia.owl#Adverb> ;
        <http://www.w3.org/2002/07/owl#versionInfo>
                "http://purl.org/olia/mte/multext-east.owl#VerbalAdverb" .

<http://purl.org/olia/olia.owl#AgentDeletionPassive>
        a       <http://www.w3.org/2002/07/owl#Class> ;
        <http://www.w3.org/2000/01/rdf-schema#comment>
                "\n\t\t\tThe object of the active retains its old case-marking in the passive, \n\t\t\tthe subject of the active cannot appear in the passive clause, and the \n\t\t\tpassive tends to be semantically active. (Givon 1988:419)\n\t\t\t(http://purl.org/linguistics/gold/AgentDeletionPassive)\n\t\t" ;
        <http://www.w3.org/2000/01/rdf-schema#subClassOf>
                <http://purl.org/olia/olia.owl#PassiveVoice> ;
        <http://www.w3.org/2002/07/owl#versionInfo>
                "http://purl.org/linguistics/gold/AgentDeletionPassive" .

<http://purl.org/olia/olia.owl#ForeignPhrase>
        a       <http://www.w3.org/2002/07/owl#Class> ;
        <http://www.w3.org/2000/01/rdf-schema#comment>
                "\n\t\tSingle foreign words are projected to a syntactic level assigned the node label FX, which is\n\t\tan universal label for any syntactic category (phrasal and sentential) in the respective\n\t\tforeign language.\n\t\t(Telljohann et al. 2009, p.44)\n\t\t" ;
        <http://www.w3.org/2000/01/rdf-schema#subClassOf>
                <http://purl.org/olia/olia.owl#Phrase> ;
        <http://www.w3.org/2002/07/owl#versionInfo>
                "TüBa-D/Z" .

<http://purl.org/olia/olia.owl#SupertranslativeCase>
        a       <http://www.w3.org/2002/07/owl#Class> ;
        <http://www.w3.org/2000/01/rdf-schema#comment>
                "\n\t\t\tSupertranslativeCase expresses the notion of something moving along a trajectory \n\t\t\tabove the referent of the noun it marks. It has the meaning 'along the region over'.\n\t\t\t(http://purl.org/linguistics/gold/Supertranslative)\n\t\t" ;
        <http://www.w3.org/2000/01/rdf-schema#subClassOf>
                <http://purl.org/olia/olia-top.owl#CaseFeature> ;
        <http://www.w3.org/2002/07/owl#versionInfo>
                "http://purl.org/linguistics/gold/Supertranslative" .

<http://purl.org/olia/olia.owl#Adjective>
        a       <http://www.w3.org/2002/07/owl#Class> ;
        <http://www.w3.org/2000/01/rdf-schema#comment>
                "\n\t\tAn Adjective is a noun-modifying expression that specifies the properties or attributes of the nominal referent.\n\t\t(http://www.sil.org/linguistics/GlossaryOfLinguisticTerms/WhatIsAnAdjective.htm  18.9.06)\n\t" ;
        <http://www.w3.org/2000/01/rdf-schema#label>
                "adjectif"@fr , "adjective"@en ;
        <http://www.w3.org/2000/01/rdf-schema#subClassOf>
                <http://purl.org/olia/olia-top.owl#MorphosyntacticCategory> ;
        <http://www.w3.org/2002/07/owl#versionInfo>
                "EAGLES top-level category Adjective (AJ)." , "the subclassification of Adjective currently conflates syntactic (PredicativeAdjective), morphological (ParticipleAdjective) and semantic (QualifierAdjective, RelativeAdjective) criteria. to be resolved" .

<http://purl.org/olia/olia.owl#PartitiveArticle>
        a       <http://www.w3.org/2002/07/owl#Class> ;
        <http://www.w3.org/2000/01/rdf-schema#comment>
                "\n\t\t\tA partitive article indicates an indefinite quantity of a mass noun; there is no partitive \n\t\t\tarticle in English, though the words some or any often have that function. An example is \n\t\t\tFrench du / de la / des, as in Voulez-vous du café? (\"Do you want some coffee?\" or \"Do you \n\t\t\twant coffee\").\n\t\t\t(http://en.wikipedia.org/wiki/Article_(grammar) 19.09.06)\n\t\t" ;
        <http://www.w3.org/2000/01/rdf-schema#subClassOf>
                <http://purl.org/olia/olia.owl#Article> ;
        <http://www.w3.org/2002/07/owl#versionInfo>
                "EAGLES Article with Article-Type=\"Partitive\". (optional for French)" , "TODO: Check relationship with PartitiveDeterminer" .

<http://purl.org/olia/olia.owl#SubordinatingConjunctionWithComparative>
        a       <http://www.w3.org/2002/07/owl#Class> ;
        <http://www.w3.org/2000/01/rdf-schema#comment>
                "\n\t\t\tFor example, in German the subordinating conjunction \"als\" is followed \n\t\t\tby various kinds of comparative clause (including clauses without finite \n\t\t\tverbs). \n\t\t\t(http://www.ilc.cnr.it/EAGLES96/annotate/node19.html#oav2u  17.11.06)\n\t\t" ;
        <http://www.w3.org/2000/01/rdf-schema#subClassOf>
                <http://purl.org/olia/olia.owl#SubordinatingConjunction> ;
        <http://www.w3.org/2002/07/owl#versionInfo>
                "EAGLES" .

<http://purl.org/olia/olia.owl#AffixedPersonalPronoun>
        a       <http://www.w3.org/2002/07/owl#Class> ;
        <http://www.w3.org/2000/01/rdf-schema#comment>
                "\n                            Personnal pronoun that is affixed.\n                                (MIRACL & LSCA; http://www.isocat.org/datcat/DC-2221)\n                            " ;
        <http://www.w3.org/2000/01/rdf-schema#label>
                "affixed personal pronoun" ;
        <http://www.w3.org/2000/01/rdf-schema#subClassOf>
                <http://purl.org/olia/olia.owl#PersonalPronoun> ;
        <http://www.w3.org/2002/07/owl#versionInfo>
                "subClassOf pronoun (dcif:isA)" , "\n\t\thttp://www.isocat.org/datcat/DC-2221, modelled as a subClassOf PersonalPronoun, clitic pronouns are weak personal pronouns\n\t  " .

<http://purl.org/olia/olia.owl#EvaluativeModality>
        a       <http://www.w3.org/2002/07/owl#Class> ;
        <http://www.w3.org/2000/01/rdf-schema#comment>
                "EvaluativeProperty: A term used in semantics for a type of modality\n                        where propositions express the speaker's attitude (e.g. surprise, regret)\n                        towards what is being said. [Crystal 2003: 168]" ;
        <http://www.w3.org/2000/01/rdf-schema#isDefinedBy>
                "http://www.isocat.org/datcat/DC-3184 (EvaluativeProperty)" ;
        <http://www.w3.org/2000/01/rdf-schema#label>
                "evaluative property" ;
        <http://www.w3.org/2000/01/rdf-schema#subClassOf>
                <http://purl.org/olia/olia-top.owl#ModalityFeature> .

<http://purl.org/olia/olia.owl#IndefiniteArticle>
        a       <http://www.w3.org/2002/07/owl#Class> ;
        <http://www.w3.org/2000/01/rdf-schema#comment>
                "\n\t\t\tAn indefinite article is used before singular nouns that refer to \n\t\t\tany member of a group.\n\t\t\t(http://en.wikipedia.org/wiki/Article_%28grammar%29 18.09.06)\n\t\t" ;
        <http://www.w3.org/2000/01/rdf-schema#subClassOf>
                <http://purl.org/olia/olia.owl#Article> ;
        <http://www.w3.org/2002/07/owl#versionInfo>
                "EAGLES Article with Article-Type=\"Indefinite\"." .

<http://purl.org/olia/olia.owl#Infinitive>
        a       <http://www.w3.org/2002/07/owl#Class> ;
        <http://www.w3.org/2000/01/rdf-schema#comment>
                "\n\t\tAn infinitive is the base form of a verb. \n\t\tIt is unmarked for inflectional categories such as the following: Aspect,  Modality, Number, Person and Tense.\n\t\t(http://www.sil.org/linguistics/GlossaryOfLinguisticTerms/WhatIsAnInfinitive.htm 19.09.06)\n\t" ;
        <http://www.w3.org/2000/01/rdf-schema#subClassOf>
                <http://purl.org/olia/olia.owl#NonFiniteVerb> ;
        <http://www.w3.org/2002/07/owl#versionInfo>
                "EAGLES NonFiniteVerbs with VerbForm=\"Infinitive\"" .

<http://purl.org/olia/olia.owl#RelativeParticle>
        a       <http://www.w3.org/2002/07/owl#Class> ;
        <http://www.w3.org/2000/01/rdf-schema#comment>
                "\n                            relative particle\n                                (MIRACL & LSCA; http://www.isocat.org/datcat/DC-2229)\n                            " ;
        <http://www.w3.org/2000/01/rdf-schema#label>
                "relative particle" ;
        <http://www.w3.org/2000/01/rdf-schema#subClassOf>
                <http://purl.org/olia/olia.owl#Particle> ;
        <http://www.w3.org/2002/07/owl#versionInfo>
                "http://www.isocat.org/datcat/DC-2229" , "subClassOf particle (dcif:isA)" .

<http://purl.org/olia/olia.owl#ComplementizerField>
        a       <http://www.w3.org/2002/07/owl#Class> ;
        <http://www.w3.org/2000/01/rdf-schema#comment>
                "\nThe C-Feld occurs in verb-final clauses in German (exception: the conjunction als in\nsubordinated sentences of comparison als w¨are es nie geschehen.). It is obligatorily\noccupied in finite verb-final clauses if there is no conjunction in the Linke Klammer. In\nnon-finite verb-final clauses the C-position may be empty. This field can be occupied by\nconjunctions of sentential objects (e.g. daß, ob) or sentence initial conjunctions like um,\nobwohl, wenn and also by complex interrogative or relative phrases, e.g. ..., ’um wieviel\nGeld’ geht es dabei? / ..., ’an der’ Max Daniel Professor f¨ur Klavier ist.\n(Telljohann et al. 2009, p.17)\n\t\t" ;
        <http://www.w3.org/2000/01/rdf-schema#subClassOf>
                <http://purl.org/olia/olia-top.owl#TopologicalField> .

<http://purl.org/olia/olia.owl#ModifierAdverb>
        a       <http://www.w3.org/2002/07/owl#Class> ;
        <http://www.w3.org/2000/01/rdf-schema#comment>
                "Adverb/Type=\"modifier\" is used in the English, Romanian and Hungarian MTE v4 specs.\n\t\t\tFor Romanian, Adverb/Type=\"modifier\" applies to adverbs which can have predicative role, that is they can govern a subordinate sentence (ex. Fireşte că o ştiu -- Certainly I know it). Here (for uniformity within a multilingual environment), they are squeezed into the modifier class. (MTE v4)\n\t\t\te.g., better (en) (http://purl.org/olia/mte/multext-east.owl#ModifierAdverb)\n\t\t" ;
        <http://www.w3.org/2000/01/rdf-schema#subClassOf>
                <http://purl.org/olia/olia.owl#Adverb> ;
        <http://www.w3.org/2002/07/owl#versionInfo>
                "http://purl.org/olia/mte/multext-east.owl#ModifierAdverb" .

<http://purl.org/olia/olia.owl#InvertedQuestionMark>
        a       <http://www.w3.org/2002/07/owl#Class> ;
        <http://www.w3.org/2000/01/rdf-schema#comment>
                "\n                            Punctuation used in certain languages at the beginning of an interrogative sentence.\n                                (http://www.isocat.org/datcat/DC-2088)\n                            " ;
        <http://www.w3.org/2000/01/rdf-schema#label>
                "inverted question mark" , "inverted interrogative point" ;
        <http://www.w3.org/2000/01/rdf-schema#subClassOf>
                <http://purl.org/olia/olia.owl#LeftParentheticalPunctuation> ;
        <http://www.w3.org/2002/07/owl#versionInfo>
                "http://www.isocat.org/datcat/DC-2088" .

<http://purl.org/olia/olia.owl#ApplicativeVoice>
        a       <http://www.w3.org/2002/07/owl#Class> ;
        <http://www.w3.org/2000/01/rdf-schema#comment>
                "voice which promotes an oblique argument of a verb to the core patient argument and indicates the oblique role within the meaning of the verb" ;
        <http://www.w3.org/2000/01/rdf-schema#isDefinedBy>
                "http://www.isocat.org/datcat/DC-3846" ;
        <http://www.w3.org/2000/01/rdf-schema#subClassOf>
                <http://purl.org/olia/olia-top.owl#VoiceFeature> .

<http://purl.org/olia/olia.owl#AspectMarkingAuxiliary>
        a       <http://www.w3.org/2002/07/owl#Class> ;
        <http://www.w3.org/2000/01/rdf-schema#comment>
                "An auxiliary that marks exclusively aspect, e.g., in Urdu:\n\t\t\n\t\tAuxiliaries:\n\t\tBased on the syntactic nature of Urdu, auxiliaries are divided into two categories. Aspectual\n\t\tauxiliaries always occur after main verb of the sentence. Tense auxiliaries are used to show the\n\t\ttime of the action. They occurred at the end of the verb phrase (Sajjad 2007).\n\t\t\n\t\tE.g., Urdu rahā, an auxiliary element is used to mark the durative aspect. (Hardie 2004, http://purl.org/olia/emille.owl#RahaAuxiliary)\n\t\t" ;
        <http://www.w3.org/2000/01/rdf-schema#subClassOf>
                <http://purl.org/olia/olia.owl#StrictAuxiliaryVerb> ;
        <http://www.w3.org/2002/07/owl#versionInfo>
                "adopted from Sajjad (2007) for Urdu, cf. http://purl.org/olia/urdu.owl#AspectualAuxiliary" .

<http://purl.org/olia/olia.owl#WHCleft>
        a       <http://www.w3.org/2002/07/owl#Class> ;
        <http://www.w3.org/2000/01/rdf-schema#comment>
                "Wh-clefts are constructions in which a wh-clause functions as the subject of a sentence. A simple\nexample is What matters is the price. Here, the wh-clause What matters is the subject, and is the price is\nthe predicate. The internal structure of the subject is:\n(NP (SBAR (WHNP what)\n(S (NP T)\n(VP matters))))\n(Santorini 1991)" ;
        <http://www.w3.org/2000/01/rdf-schema#subClassOf>
                <http://purl.org/olia/olia.owl#SubordinateClause> , <http://purl.org/olia/olia-top.owl#SyntacticConstruction> ;
        <http://www.w3.org/2002/07/owl#versionInfo>
                "PTB bracketing guidelines (Santorini 1991, Bies et al. 1995)" .

<http://purl.org/olia/olia.owl#Preposition>
        a       <http://www.w3.org/2002/07/owl#Class> ;
        <http://www.w3.org/2000/01/rdf-schema#comment>
                "\n      A preposition is an adposition that occurs before its complement.\n      (http://www.sil.org/linguistics/GlossaryOfLinguisticTerms/WhatIsAPreposition.htm 19.09.06)" ;
        <http://www.w3.org/2000/01/rdf-schema#label>
                "preposition"@en , "préposition"@fr ;
        <http://www.w3.org/2000/01/rdf-schema#subClassOf>
                <http://purl.org/olia/olia.owl#Adposition> ;
        <http://www.w3.org/2002/07/owl#versionInfo>
                "EAGLES adposition with Type=\"Preposition\"." .

<http://purl.org/olia/olia.owl#ElativeNoun>
        a       <http://www.w3.org/2002/07/owl#Class> ;
        <http://www.w3.org/2000/01/rdf-schema#comment>
                "noun to express both comparative and superlative" ;
        <http://www.w3.org/2000/01/rdf-schema#isDefinedBy>
                "http://www.isocat.org/datcat/DC-3860" ;
        <http://www.w3.org/2000/01/rdf-schema#subClassOf>
                <http://purl.org/olia/olia.owl#CommonNoun> , <http://purl.org/olia/olia.owl#ElativeDegree> ;
        <http://www.w3.org/2002/07/owl#versionInfo>
                "added in compliance with ISOcat" .

<http://purl.org/olia/olia.owl#ThemeRole>
        a       <http://www.w3.org/2002/07/owl#Class> ;
        <http://www.w3.org/2000/01/rdf-schema#comment>
                "\n\t\t\tTheme is a general term covering the notions of patient that means an entity \n\t\t\taffected by the action, of result that means an entity effected by the action, \n\t\t\ti.e. which emerges out of the action, or of theme that means an entity effected \n\t\t\tby the action, i.e. which emerges out of the action.\n\t\t\t(Dipper et al. 2007: §5.3.3)\n\t\t" ;
        <http://www.w3.org/2000/01/rdf-schema#subClassOf>
                <http://purl.org/olia/olia-top.owl#SemanticRole> ;
        <http://www.w3.org/2002/07/owl#versionInfo>
                "added in conformance with SFB632 Theme" , "TODO: check definition, AFAIK Theme also applies to the third (non-ACTOR, non-UNDERGOER) argument (Ch. Chiarcos)" .

<http://purl.org/olia/olia.owl#Quadrial>
        a       <http://www.w3.org/2002/07/owl#Class> ;
        <http://www.w3.org/2000/01/rdf-schema#comment>
                "\n                            Property related to four elements.\n                                (http://www.isocat.org/datcat/DC-2000)\n                            " ;
        <http://www.w3.org/2000/01/rdf-schema#label>
                "quadrial" ;
        <http://www.w3.org/2000/01/rdf-schema#subClassOf>
                <http://purl.org/olia/olia-top.owl#NumberFeature> ;
        <http://www.w3.org/2002/07/owl#versionInfo>
                "http://www.isocat.org/datcat/DC-2000" , "subClassOf grammaticalNumber (dcif:conceptualDomain)" .

<http://purl.org/olia/olia.owl#DirectionRole>
        a       <http://www.w3.org/2002/07/owl#Class> ;
        <http://www.w3.org/2000/01/rdf-schema#comment>
                "-DIR (direction)\nâ ´ marks adverbials that answer the questions â ¼from where?â ½ and â ¼to where?â ½ It implies motion, which can be metaphorical as in â ¼...rose 5 pts. to 57-1/2â ½ or â ¼increased 70% to 5.8 billion yenâ ½ (see section 23 [â ¼Financialspeakâ ½ Conventions]). -DIR is most often used with verbs of motion/transit and financial verbs: \n\n  (S (NP-SBJ I)\n     (VP flew\n         (PP-DIR from\n                 (NP Tokyo))\n         (PP-DIR to\n                 (NP New York))))\n(Bies et al. 1995)" ;
        <http://www.w3.org/2000/01/rdf-schema#subClassOf>
                <http://purl.org/olia/olia-top.owl#SemanticRole> ;
        <http://www.w3.org/2002/07/owl#versionInfo>
                "added in conformance with PTB bracketing guidelines, Bies et al. (1995)" .

<http://purl.org/olia/olia.owl#DitransitiveTheme>
        a       <http://www.w3.org/2002/07/owl#Class> ;
        <http://www.w3.org/2000/01/rdf-schema#comment>
                "\n\t\t\tDitransitive theme (T) (Siewierska 2004:57).\n\t\t\t(http://languagelink.let.uu.nl/tds/onto/LinguisticOntology.owl#T)\n\t\t" ;
        <http://www.w3.org/2000/01/rdf-schema#subClassOf>
                <http://purl.org/olia/olia.owl#DirectObject> ;
        <http://www.w3.org/2002/07/owl#versionInfo>
                "http://languagelink.let.uu.nl/tds/onto/LinguisticOntology.owl#T" .

<http://purl.org/olia/olia.owl#InstrumentRole>
        a       <http://www.w3.org/2002/07/owl#Class> ;
        <http://www.w3.org/2000/01/rdf-schema#comment>
                "SemanticRole added in conformance with TIGER" ;
        <http://www.w3.org/2000/01/rdf-schema#subClassOf>
                <http://purl.org/olia/olia-top.owl#SemanticRole> ;
        <http://www.w3.org/2002/07/owl#versionInfo>
                "\n\t\t\thttp://languagelink.let.uu.nl/tds/onto/LinguisticOntology.owl#instrumentRole, \n\t\t\tcf. TIGER edge label \"Instrumental\"\n\t\t" .

<http://purl.org/olia/olia.owl#LayoutElement>
        a       <http://www.w3.org/2002/07/owl#Class> ;
        <http://www.w3.org/2000/01/rdf-schema#subClassOf>
                <http://purl.org/olia/olia.owl#Residual> ;
        <http://www.w3.org/2002/07/owl#versionInfo>
                "Introduced to account for Bullet http://www.isocat.org/datcat/DC-1438" .

<http://purl.org/olia/olia.owl#Homonym>
        a       <http://www.w3.org/2002/07/owl#Class> ;
        <http://www.w3.org/2000/01/rdf-schema#comment>
                "Word that sounds the same and is written the same as another word but is different in meaning." ;
        <http://www.w3.org/2000/01/rdf-schema#isDefinedBy>
                "http://www.isocat.org/datcat/DC-1301" ;
        <http://www.w3.org/2000/01/rdf-schema#label>
                "homonym" ;
        <http://www.w3.org/2000/01/rdf-schema#subClassOf>
                <http://purl.org/olia/system.owl#Relation> , <http://purl.org/olia/olia-top.owl#LexicalRelation> .

<http://purl.org/olia/olia.owl#Nonspecific>
        a       <http://www.w3.org/2002/07/owl#Class> ;
        <http://www.w3.org/2000/01/rdf-schema#comment>
                "\"By ʻspecificʼ and ʻnon-specificʼ I intend the difference between the\n\t\t\ttwo readings of English indefinites like (3):\n\t\t\t\n\t\t\t(3) Iʼm looking for a deer.\n\t\t\t\n\t\t\tIn the specific reading there is a particular deer, say Bambi, that I am\n\t\t\tlooking for. In the non-specific reading I will be happy to find any deer.\n\t\t\tVon Heusinger (2002) likes the test in English of inserting ʻcertainʼ after the\n\t\t\tʻaʼ to fix the specific reading. In either reading of (3) a deer is being\n\t\t\tintroduced as a new discourse referent. This is opposed to ʻdefiniteʼ which\n\t\t\trequires a previous pragmatic instantiation as in ʻIʼm looking for the deer.ʼ\n\t\t\tIn English both the readings of (3) are indefinite. In Klallam, the specific\n\t\t\tdemonstratives are neither definite nor indefinite.\"\n\t\t\t(Montler, Timothy. 2007. Klallam demonstratives. Papers ICSNL XLVII. The 42nd International Conference on Salish and Neighbouring Language, pp. 409-425. University of British Columbia Working Papers in Linguistics, Volume 20; on specific vs. nonspecific determiners in Klallam, a Salish language, http://montler.net/papers/KlallamDemons.pdf)\n\n\t\t\tA nonspecific pronoun refers to an unidentified or general entity (e.g., \"I saw *someone*\", \"I saw *everyone*\"). A nonspecific pronoun is not, therefore, a personal pronoun, but an indefinite one. (Andrews 2003).\n\n\t\t\tAndrews, Richard J. (2003), Introduction to Classical Nahuatl. University of Oklahoma Press.\n\t\t\tHalliday, M.A.K. (1985), An introduction to Functional Grammar, London: Edward Arnold\n\t\t\t(http://purl.org/olia/mte/multext-east.owl#NonspecificPronoun)\n\t\t" ;
        <http://www.w3.org/2000/01/rdf-schema#subClassOf>
                <http://purl.org/olia/olia-top.owl#SpecificityFeature> ;
        <http://www.w3.org/2002/07/owl#versionInfo>
                "see olia:NonspecificArticle, http://purl.org/olia/mte/multext-east.owl#NonspecificPronoun" .

<http://purl.org/olia/olia.owl#Collective>
        a       <http://www.w3.org/2002/07/owl#Class> ;
        <http://www.w3.org/2000/01/rdf-schema#comment>
                "\n                            A collective number is a number referring to 'a set of things'. Languages that have this feature can use it to get a phrase like 'flock of sheeps' by using 'sheep' in collective number.\n                                (en2.wikipedia.org/wiki/Collective_number; http://www.isocat.org/datcat/DC-1254)\n                            " ;
        <http://www.w3.org/2000/01/rdf-schema#label>
                "collective" ;
        <http://www.w3.org/2000/01/rdf-schema#subClassOf>
                <http://purl.org/olia/olia.owl#Derivation> , <http://purl.org/olia/olia-top.owl#NumberFeature> ;
        <http://www.w3.org/2002/07/owl#versionInfo>
                "rename to CollectiveNumber" , "subClassOf grammaticalNumber (dcif:conceptualDomain)" , "http://www.isocat.org/datcat/DC-1254" , "Normally realized by derivation rather than inflection, unless other evidence is provided, OLiA follows *both* the modelling of EAGLES (Collective rdf:type Number) and the modelling of the MTE ontology (Collective rdf:type MorphologicalDerivation, cf. http://purl.org/olia/mte/multext-east.owl#Collective)" .

<http://purl.org/olia/olia.owl#ElativeCase>
        a       <http://www.w3.org/2002/07/owl#Class> ;
        <http://www.w3.org/2000/01/rdf-schema#comment>
                "\n\t\t\tElativeCase expresses that  the referent of the noun it marks is \n\t\t\tthe location out of which another referent is moving. It has the \n\t\t\tmeaning 'out of' (Lyons 1968: 299; Pei and Gaynor 1954: 64; Crystal \n\t\t\t1985: 106; Gove, et al. 1966: 730).\n\t\t\t(http://purl.org/linguistics/gold/Elative)\n\t\t" ;
        <http://www.w3.org/2000/01/rdf-schema#subClassOf>
                <http://purl.org/olia/olia-top.owl#CaseFeature> ;
        <http://www.w3.org/2002/07/owl#versionInfo>
                "http://purl.org/linguistics/gold/Elative, http://www.isocat.org/datcat/DC-1276, note that the latter conflates ElativeDegree and ElativeCase" .

<http://purl.org/olia/olia.owl#ZeroComplementizer>
        a       <http://www.w3.org/2002/07/owl#Class> ;
        <http://www.w3.org/2000/01/rdf-schema#comment>
                "0|Zero represents a zero complementizer (= subordinating conjunction); it may need to be deleted. The\nzero complementizer is generally the counterpart of the overt complementizer that. Example: Iâ ¹m sure 0\nheâ ¹ll be here any minute. ...\n\n0 stands in for overt subordinating conjunctions like that in tensed subordinate clauses, including\nrelative clauses. So the relative clause the man I saw should be bracketed as follows:\n(NP (NP the man) (SBAR 0 (S (NP I) (VP saw) (NP T)))))\n\n(Santorini 1991)" ;
        <http://www.w3.org/2000/01/rdf-schema#subClassOf>
                <http://purl.org/olia/olia-top.owl#NullElement> , <http://purl.org/olia/olia.owl#SubordinatingConjunction> ;
        <http://www.w3.org/2002/07/owl#versionInfo>
                "added in conformance with PTB bracketing guidelines (Santorini 1991)" .

<http://purl.org/olia/olia.owl#hasTense>
        a       <http://www.w3.org/2002/07/owl#ObjectProperty> ;
        <http://www.w3.org/2000/01/rdf-schema#domain>
                <http://purl.org/olia/olia.owl#Verb> ;
        <http://www.w3.org/2000/01/rdf-schema#range>
                <http://purl.org/olia/olia-top.owl#TenseFeature> ;
        <http://www.w3.org/2000/01/rdf-schema#subPropertyOf>
                <http://purl.org/olia/system.owl#hasFeature> .

<http://purl.org/olia/olia.owl#ElativeDegree>
        a       <http://www.w3.org/2002/07/owl#Class> ;
        <http://www.w3.org/2000/01/rdf-schema#comment>
                "e.g., прешпионска/шпионски, прешпионскава/шпионски, прешпионскана/шпионски, прешпионската/шпионски, прешпионски/шпионски, прешпионскиве/шпионски, прешпионскине/шпионски, прешпионскиов/шпионски, прешпионскион/шпионски (mk)" , "MULTEXT-East Degree=\"elative\" (Adjective: Resian, Serbian, Macedonian)<br/>\n\t\t\t\n\t\t\tIn Semitic languages, ElativeDegree refers to the “adjective of superiority.” In some languages such as Arabic, the concepts of comparative and superlative degree of an adjective are merged into a single form, the elative. How this form is understood or translated depends upon context and definiteness. In the absence of comparison, the elative conveys the notion of “greatest”, “supreme.” The elative of كبير (kabí:r, \"big\") is أكبر (’ákbar, “bigger/biggest”, “greater/greatest”). (http://en.wiktionary.org/wiki/elative)\n\t\t\t\n\t\t\tIn Slavic languages, as well, it is pretty standard. I do agree with the definition though, that \"the elative conveys the notion of “greatest”, “supreme.”\" So, Slovene \"lep\" is beautiful, \"prelep\" is very (or supremely) beautiful; I guess the \"pre-\" prefix could be roughly translated as \"over-\". Used in Resian, Serbian, Macedonian. In Slovenian, we banished it, as even \"ordinary\" degrees are borderline inflection / derivation, but, I think, elative is is definitely not inflection. (Tomaž Erjavec, email 2010/06/21)" , "e.g., predivan, prekasan, premanjeg/premali, premanjega/premali, premanjem/premali, premanjemu/premali, premanji/premali (sr)" ;
        <http://www.w3.org/2000/01/rdf-schema#subClassOf>
                <http://purl.org/olia/olia-top.owl#DegreeFeature> ;
        <http://www.w3.org/2002/07/owl#versionInfo>
                "http://purl.org/olia/mte/multext-east.owl#ElativeDegree, http://www.isocat.org/datcat/DC-1276, note that the latter conflates ElativeDegree and ElativeCase" .

<http://purl.org/olia/olia.owl#Qualifier>
        a       <http://www.w3.org/2002/07/owl#Class> ;
        <http://www.w3.org/2000/01/rdf-schema#comment>
                "\n                            Also called MODIFIER : A word or phrase that qualifies the sense of another word; for example, the noun alarm is a modifier of clock in \"alarm clock\" and the phrase every day is an adverbial modifier of walks in \"he walks every day\"\n                                (www.wordreference.com/English/definition.asp?en=modifier; http://www.isocat.org/datcat/DC-1373)\n                            " ;
        <http://www.w3.org/2000/01/rdf-schema#label>
                "Qualifier" ;
        <http://www.w3.org/2000/01/rdf-schema#subClassOf>
                <http://purl.org/olia/olia.owl#Modifier> ;
        <http://www.w3.org/2002/07/owl#versionInfo>
                "http://www.isocat.org/datcat/DC-1373" .

<http://purl.org/olia/olia.owl#ReflexiveDeterminer>
        a       <http://www.w3.org/2002/07/owl#Class> ;
        <http://www.w3.org/2000/01/rdf-schema#comment>
                "\n                            Determiner that refers to the same entity.\n                                (http://www.isocat.org/datcat/DC-1377)\n                            " ;
        <http://www.w3.org/2000/01/rdf-schema#label>
                "reflexive adjective" ;
        <http://www.w3.org/2000/01/rdf-schema#subClassOf>
                <http://purl.org/olia/olia.owl#Determiner> ;
        <http://www.w3.org/2002/07/owl#versionInfo>
                "TOCHECK: Are there non-possessive reflexive determiners ?" , "http://www.isocat.org/datcat/DC-1377" , "subClassOf determiner (dcif:isA)" .

<http://purl.org/olia/olia.owl#HonorificCommonNoun>
        a       <http://www.w3.org/2002/07/owl#Class> ;
        <http://www.w3.org/2000/01/rdf-schema#comment>
                "Dzongkha uses honorific forms: ན་བཟའ་/nam za/\n\t\t\t(cloths) is the honorific form of the noun གོ་\n\t\t\tལ་/gola/(cloths), གསངས་/sung/(tell) the honorific\n\t\t\tform of the verb སབ་/lab/(tell). We opted to mark\n\t\t\tthem by adding the tag NNH (honorific\n\t\t\tcommon noun) and VBH (honorific verb) to\n\t\t\tenable future research on this specific usage of\n\t\t\tDzongkha language. A number of tags were\n\t\t\tadded to the set, of which we describe four in\n\t\t\tmore detail: two of the additional tags are subclasses\n\t\t\tof verbs: VBH (honorific verb form),\n\t\t\tand VBN which describes past participle forms,\n\t\t\tlike, e.g. བངམ་/jun/(created), the past particle\n\t\t\tform of བང་/jung/(create).\n\t\t\t(Chungku et al. 2010)\n\t\t\t\n\t\t\tA noun, which indicates respect for the person being addressed, e.g., Miwang Gel-poi Yab “A king's father” [Though father=Apa, but colloquially we say YAB in Dzongkha]\n\t\t\t(http://panl10n.net/english/Outputs%20Phase%202/CCs/Bhutan/Papers/2007/0701/PartOfSpeech.pdf)" ;
        <http://www.w3.org/2000/01/rdf-schema#subClassOf>
                <http://purl.org/olia/olia.owl#CommonNoun> ;
        <http://www.w3.org/2002/07/owl#versionInfo>
                "adopted from Dzongkha tagset (Chungku et al. 2010)" .

<http://purl.org/olia/olia.owl#ConditionalIrrealisMood>
        a       <http://www.w3.org/2002/07/owl#Class> ;
        <http://www.w3.org/2000/01/rdf-schema#comment>
                "Conditional Mood (modality) with Irrealis meaning (ILPOSTS)" ;
        <http://www.w3.org/2000/01/rdf-schema#subClassOf>
                <http://purl.org/olia/olia.owl#ConditionalMood> , <http://purl.org/olia/olia.owl#ConditionalIrrealisModality> ;
        <http://www.w3.org/2002/07/owl#versionInfo>
                "ILPOSTS (Indian languages), http://purl.org/olia/ilposts.owl#NonReal is restricted to conditional participles, hence probably a subtype of ConditionalMood" .

<http://purl.org/olia/olia.owl#SubjunctiveParticle>
        a       <http://www.w3.org/2002/07/owl#Class> ;
        <http://www.w3.org/2000/01/rdf-schema#comment>
                "In the Romanian MULTEXT-East scheme, a verbal particle with Particle/Type=\"future\" modifies the verbs and marks the verb as being subjunctive, e.g., s-/să, să (Dan Tufis, email 2010/06/09, http://purl.org/olia/mte/multext-east.owl#SubjunctiveParticle)" ;
        <http://www.w3.org/2000/01/rdf-schema#subClassOf>
                <http://purl.org/olia/olia.owl#VerbalParticle> ;
        <http://www.w3.org/2002/07/owl#versionInfo>
                "http://purl.org/olia/mte/multext-east.owl#SubjunctiveParticle" .

<http://purl.org/olia/olia.owl#ThirdObviative>
        a       <http://www.w3.org/2002/07/owl#Class> ;
        <http://www.w3.org/2000/01/rdf-schema#comment>
                "\n\t\t\tObviative refers to one or more non-participants that are in some \n\t\t\tway further removed from the speaker  than other non-particpants.\n\t\t\t(http://purl.org/linguistics/gold/ThirdObviative)\n\t\t" ;
        <http://www.w3.org/2000/01/rdf-schema#subClassOf>
                <http://purl.org/olia/olia.owl#Third> ;
        <http://www.w3.org/2002/07/owl#versionInfo>
                "\n\t\t\thttp://purl.org/linguistics/gold/ThirdObviative,\n\t\t\tmodelled here as a subconcept of Third\n\t\t" .

<http://purl.org/olia/olia.owl#RelativeDeterminer>
        a       <http://www.w3.org/2002/07/owl#Class> ;
        <http://www.w3.org/2000/01/rdf-schema#comment>
                "\n\t\t\tThe relative determiner describes a attributive relative pronoun. In German  \n\t\t\t\"wessen\" in \"Ich weiss nicht, wessen Auto das ist.\" or  the English  \"whose\" \n\t\t\tin \"The man whose daughter became ill.\".\n\t\t\tThe relative determiner needs a noun to complete a NP (Nominal Phrase).\n\t\t\t(http://www.ilc.cnr.it/EAGLES96/pub/eagles/lexicons/elm_en.ps.gz, p.28, 07.05.07)\n\t\t" ;
        <http://www.w3.org/2000/01/rdf-schema#subClassOf>
                <http://purl.org/olia/olia.owl#WHDeterminer> ;
        <http://www.w3.org/2002/07/owl#versionInfo>
                "\n\t\t\tEAGLES Determiner with Wh-Type=\"Relative\".\n\t\t" .

<http://purl.org/olia/olia.owl#RarelyUsed>
        a       <http://www.w3.org/2002/07/owl#Class> ;
        <http://www.w3.org/2000/01/rdf-schema#comment>
                "\n                            Said of a term that is almost never used.\n                                (ISO12620; http://www.isocat.org/datcat/DC-1986)\n                            " ;
        <http://www.w3.org/2000/01/rdf-schema#label>
                "rarely used" ;
        <http://www.w3.org/2000/01/rdf-schema#subClassOf>
                <http://purl.org/olia/olia.owl#Possible> ;
        <http://www.w3.org/2002/07/owl#versionInfo>
                "subClassOf frequency (dcif:conceptualDomain)" , "http://www.isocat.org/datcat/DC-1986" .

<http://purl.org/olia/olia.owl#PurposeRole>
        a       <http://www.w3.org/2002/07/owl#Class> ;
        <http://www.w3.org/2000/01/rdf-schema#comment>
                "-PRP (purpose or reason)\nâ ´ marks purpose or reason clauses and PPs. \n(Bies et al. 1995)" ;
        <http://www.w3.org/2000/01/rdf-schema#subClassOf>
                <http://purl.org/olia/olia-top.owl#SemanticRole> ;
        <http://www.w3.org/2002/07/owl#versionInfo>
                "added in conformance with PTB bracketing guidelines (Bies et al. 1995)" .

<http://purl.org/olia/olia.owl#NonEmphatic>
        a       <http://www.w3.org/2002/07/owl#Class> ;
        <http://www.w3.org/2000/01/rdf-schema#comment>
                "In languages where emphasis can be grammatically marked, the unmarked form would be considered NonEmphatic, see #Emphatic" ;
        <http://www.w3.org/2000/01/rdf-schema#subClassOf>
                <http://purl.org/olia/olia-top.owl#EmphasisFeature> ;
        <http://www.w3.org/2002/07/owl#versionInfo>
                "added in accordance with ILPOSTS, cf. http://purl.org/olia/mte/multext-east.owl#EmphaticDeterminer, http://purl.org/olia/mte/multext-east.owl#EmphaticPronoun" .

<http://purl.org/olia/olia.owl#SpatiotemporalNoun>
        a       <http://www.w3.org/2002/07/owl#Class> ;
        <http://www.w3.org/2000/01/rdf-schema#comment>
                "\n\t\t\tNoun denoting spatial and temporal expressions\n\t\t\t\n\t\t\t\"A tag NST has been included to cover an important phenomenon of Indian languages. Certain expressions such as 'Upara' (above/up), 'nIce' (below) 'pahale' (before), 'Age' (front) etc are content words denoting time and space. These expressions, however, are used in various ways. For example,\n\t\t\t5.1.2.1 These words often occur as temporal or spatial arguments of a verb in a given sentence taking the appropriate vibhakti (case marker):\n\t\t\th3. vaha Upara so rahA thA .\n\t\t\t'he' 'upstairs' 'sleep' 'PROG' 'was'\n\t\t\t“He was sleepign upstairs”.\n\t\t\th4. vaha pahale se kamare meM bEThA thA .\n\t\t\t'he' 'beforehand' 'from' ' room' 'in' 'sitting' 'was'\n\t\t\t“He was sitting in the room from beforehand”\n\t\t\th5. tuma bAhara bETho\n\t\t\t'you' 'outside' 'sit'\n\t\t\t“You sit outside”.\n\t\t\tApart from functioning like an argument of a verb, these elements also modify another noun taking postposition 'kA'.\n\t\t\th6. usakA baDZA bhAI Upara ke hisse meM rahatA hE\n\t\t\t'his' 'elder' 'brother' 'upstairs' 'of' 'portion' 'in' 'live' 'PRES'\n\t\t\t“His elder brother lives in the upper portion of the house”.\n\t\t\t5.1.2.2 Apart from occuring as a nominal expression, they also occur as a part of a postposition along with 'ke'. For example,\n\t\t\th7. ghaDZe ke Upara thAlI rakhI hE.\n\t\t\t'pot' 'of' 'above' 'plate' 'kept' 'is'\n\t\t\tThe plate is kept on the pot”.\n\t\t\th8. tuma ghara ke bAhara bETho\n\t\t\t'you' 'home' 'of' 'outside' 'sit'\n\t\t\t“You sit outside the house”.\n\t\t\t'Upara' and 'bAhara' are parts of complex postpositions 'ke Upara' and 'ke bAhara' in (h6) and (h7) respectively which can be translated into English prepositions 'on' and 'outside'.\n\t\t\tFor tagging such words, one possible option is to tag them according to their syntactic function in the given context. For example in 5.2.2 (h7) above, the word 'Upara' is occurring as part of a postposition or a relation marker. It can, therefore, be marked as a postposition. Similarly, in 5.2.1. (h3) and (h6) above, it is a noun, therefore, mark it as a noun and so on. Alternatively, since these words are more like nouns, as is evident from 5.2.1 above they can be tagged as nouns in all there occurrences. The same would apply to 'bAhAra' (outside)\n\t\t\tin examples examples (h4), (h5) and (h8).\n\t\t\tHowever, if we follow any of the above approaches we miss out on the fact that this class of words is slightly different from other nouns. These are nouns which indicate 'location' or 'time'. At the same time, they also function as postpositions in certain contexts. Moreover, such words, if tagged according to their syntactic function, will hamper machine learning. Considering their special status, it was considered whether to introduce a new tag, NST, for such expressions. The following five possibilities were discussed :\n\t\t\ta) Tag both (h5) & (h8) as NN\n\t\t\tb) Tag both (h5) & (h8) as NST\n\t\t\tc) Tag (h5) as NN & (h8) as NST\n\t\t\td) Tag (h5) as NST & (h8) as PSP\n\t\t\te) Tag (h5) as NN & (h8) as PSP\n\t\t\tAfter considering all the above, the decision was taken in favour of (b). The decision was primarily based on the following observations:\n\t\t\t(i) 'bAhara' in both (h5) and (h8) denotes the same expression (place expression 'outside')\n\t\t\t(ii) In both (h5) and (h8), 'bAhara' can take a vibhakti like a noun ( bAhara ko bETho, ghara ke bAhara ko bETho)\n\t\t\t(iii) If a single tag is kept for both the usages, the decision making for annotators would also be easier.\n\t\t\tTherefore, a new tag NST is introduced for such expressions. The tag NST will be used for a finite set of such words in any language. For example, Hindi has\n\t\t\tAge (front), pIche (behind), Upara (above/upstairs), nIce (below/down), bAda (after), pahale (before), andara (inside), bAhara (outside) etc.\"\n\t\t(Akshar Bharati, Dipti Misra Sharma, Lakshmi Bai, Rajeev Sangal (2006), AnnCorra : Annotating Corpora. Guidelines For POS And Chunk Annotation For Indian Languages, Tech. Rep., L anguage Technologies Research Centre IIIT, Hyderabad, version of 15-12-2006, http://ltrc.iiit.ac.in/tr031/posguidelines.pdf)\n\t\t" , "\n\t\t\tNLOC Noun Location\n\t\t\tThis is an entirely new tag introduced to cover an important phenomenon\n\t\t\tof Indian Languages. Words like 'Age', 'upara', 'pahele', 'bAda', etc.\n\t\t\tare used in various ways in Hindi.\n\t\t\t1. They act as a postposition along with 'ke'\n\t\t\te.g. ghade ke upara thAlI rakhI HE.\n\t\t\t(\"pot\" \"on\" \"plate\" \"kept\" \"is\")\n\t\t\tHere 'ke upara' is a post position which is the direct equivalent of\n\t\t\tthe English preposition 'on'.\n\t\t\t2. They also act as adverbs.\n\t\t\te.g. tuma upara jAo.\n\t\t\t(\"You\" \"up\" \"go\")\n\t\t\tHere 'upara' is an adverbial of place.\n\t\t\t3. These words also take post positions themselves and so in some sense\n\t\t\tbehave like nouns.\n\t\t\te.g. vaHa upara se AyA.\n\t\t\t(\"He\" \"above\" \"from\" \"came\")\n\t\t\t4. As pointed out in 3. above, these words take postpositions and act\n\t\t\tas arguments of the verb in the sentence. And they also take a post\n\t\t\tposition to join with a another noun. So in that sense also they behave\n\t\t\tlike nouns.\n\t\t\te.g. upara kA HissA\n\t\t\t(\"above\" \"of\" \"portion\")\n\t\t\tTo tag such words one option is to tag them according to the category\n\t\t\tto which they belong in the given sentence. For example in 1. above,\n\t\t\tthe word is occurring as a postposition so can be marked as a\n\t\t\tpostposition. In example 2. above, it is an adverb so can be marked as\n\t\t\tan adverb and so on.\n\t\t\tBut we feel that these words are more like nouns as is evident from 3.\n\t\t\tand 4. above, and also if we consider for examples, 'aage', 'upara',\n\t\t\tetc. as places which are in front, up, etc then we can tag them as\n\t\t\tnouns.\n\t\t\tBut these are not pure nouns. They are nouns which indicate a location\n\t\t\tor time. These also function as adverbs or prepositions in a context.\n\t\t\tSo a new tag NLOC is introduced for such words. This tag will cater to\n\t\t\ta finite set of such words.\n\t\t\tset: (Age, piche, upara, nIce, bAda, pahele)\n\t\t\t(\"front\", \"behind\", \"above\", \"below\", \"before\")\n\t\t\tSuch words if tagged according to their syntactic function, it will\n\t\t\thamper machine learning. So a single tag, NLOC has been devised for\n\t\t\tsuch words which indicate location and time.\n\t\t\t\n\t\t\te.g., (upara, Age, pahele, bAda)\n\t\t\t(IIIT (2007), A Part of Speech Tagger for Indian Languages (POS tagger), Tagset developed at IIIT - Hyderabad after consultations with several institutions through two workshops. available under http://shiva.iiit.ac.in/SPSAL2007/iiit_tagset_guidelines.pdf)\n\t\t" ;
        <http://www.w3.org/2000/01/rdf-schema#label>
                "location noun" , "spatio-temporal noun" ;
        <http://www.w3.org/2000/01/rdf-schema#subClassOf>
                <http://purl.org/olia/olia.owl#CommonNoun> ;
        <http://www.w3.org/2002/07/owl#versionInfo>
                "adopted from Ancorra, http://purl.org/olia/ancorra.owl#SpatiotemporalNoun" .

<http://purl.org/olia/olia.owl#NonpromotionalInverseVoice>
        a       <http://www.w3.org/2002/07/owl#Class> ;
        <http://www.w3.org/2000/01/rdf-schema#comment>
                "\n\t\t\tInvolves demotion of the non-topical obviate-agent from subjecthood. (Givon 1994:24)\n\t\t\t(http://purl.org/linguistics/gold/NonpromotionalInverse)\n\t\t" ;
        <http://www.w3.org/2000/01/rdf-schema#subClassOf>
                <http://purl.org/olia/olia.owl#InverseVoice> ;
        <http://www.w3.org/2002/07/owl#versionInfo>
                "http://purl.org/linguistics/gold/NonpromotionalInverse" .

<http://purl.org/olia/olia.owl#PartitiveCase>
        a       <http://www.w3.org/2002/07/owl#Class> ;
        <http://www.w3.org/2000/01/rdf-schema#comment>
                "\n\t\t\tThe partitive case is a grammatical case which denotes \"partialness\", \n\t\t\t\"without result\", or \"without specific identity\".\n\t\t\t(http://languagelink.let.uu.nl/tds/onto/LinguisticOntology.owl#partitiveCase \n\t\t\twith reference to http://en.wikipedia.org/wiki/Partitive)\n\t\t\t\n\t\t\tPartitiveCase expresses the partial nature of the referent of the \n\t\t\tnoun it marks, as opposed to expressing the whole unit or class \n\t\t\tof which the referent is a part. This case may be found in items \n\t\t\tsuch as the following: existential clauses, nouns that are \n\t\t\taccompanied by numerals or units of measure, or predications of \n\t\t\tmaterial from which something is made. It often has a meaning \n\t\t\tsimilar to the English word 'some' (Pei and Gaynor 1954: 161; \n\t\t\tRichards, Platt, and Weber 1985: 208; Quirk, et al. 1985: 249; \n\t\t\tGove, et al. 1966: 1648; Sebeok 1946: 1214).\n\t\t\t(http://purl.org/linguistics/gold/Partitive)\n\t\t" ;
        <http://www.w3.org/2000/01/rdf-schema#subClassOf>
                <http://purl.org/olia/olia-top.owl#CaseFeature> ;
        <http://www.w3.org/2002/07/owl#versionInfo>
                "TDS ontology; http://purl.org/linguistics/gold/Partitive; http://www.isocat.org/datcat/DC-2003" .

<http://purl.org/olia/olia.owl#WordOrderInverse>
        a       <http://www.w3.org/2002/07/owl#Class> ;
        <http://www.w3.org/2000/01/rdf-schema#comment>
                "SINV|Inverted declarative sentence, i.e. one in which the subject follows the verb. See Section 5.19.\n(Santorini 1991)\n\nThe SINV label is used for subject-auxiliary inversion in the case of negative inversion, conditional inversion, locative inversion, and some topicalizations. ...\nSINV â ´ Inverted declarative sentence, i.e. one in which the subject follows the tensed verb or modal. \n(Bies et al. 1995)" ;
        <http://www.w3.org/2000/01/rdf-schema#subClassOf>
                <http://purl.org/olia/olia-top.owl#SyntacticConstruction> ;
        <http://www.w3.org/2002/07/owl#versionInfo>
                "PTB bracketing guidelines (Santorini 1991, Bies et al. 1995)" .

<http://purl.org/olia/olia.owl#AbbreviatedPronoun>
        a       <http://www.w3.org/2002/07/owl#Class> ;
        <http://www.w3.org/2000/01/rdf-schema#comment>
                "Abbreviation/Syntactic_Type=\"pronominal\" (Romanian), e.g., d-ta/dumneata, d-tale/dumitale, d-voastră/dumneavoastră, dv./dumneavoastră, dvs./dumneavoastră (http://purl.org/olia/mte/multext-east.owl#Pronominal)" ;
        <http://www.w3.org/2000/01/rdf-schema#subClassOf>
                <http://purl.org/olia/olia.owl#Pronoun> , <http://purl.org/olia/olia.owl#Abbreviation> ;
        <http://www.w3.org/2002/07/owl#versionInfo>
                "http://purl.org/olia/mte/multext-east.owl#Pronominal" .

<http://purl.org/olia/olia.owl#hasAspect>
        a       <http://www.w3.org/2002/07/owl#ObjectProperty> ;
        <http://www.w3.org/2000/01/rdf-schema#domain>
                <http://purl.org/olia/olia.owl#Verb> ;
        <http://www.w3.org/2000/01/rdf-schema#range>
                <http://purl.org/olia/olia-top.owl#AspectFeature> ;
        <http://www.w3.org/2000/01/rdf-schema#subPropertyOf>
                <http://purl.org/olia/system.owl#hasFeature> .

<http://purl.org/olia/olia.owl#FinalField>
        a       <http://www.w3.org/2002/07/owl#Class> ;
        <http://www.w3.org/2000/01/rdf-schema#comment>
                "\nIn a German clause, the finite verb can appear in three different positions: verb-second, \nverb-initial, and verb-final. Only in verb-final clauses the verb complex consisting of the\nfinite verb and non-finite verbal elements forms a unit. The discontinuous positioning\nof the verbal elements in verb-first and verb-second clauses is the traditional reason\nfor structuring German clauses into fields. The positions of the verbal elements form\nthe Satzklammer (sentence bracket) which divides the sentence into a Vorfeld (initial\nfield), a Mittelfeld (middle field), and a Nachfeld (final field). The Vorfeld and the\nMittelfeld are divided by the linke Satzklammer (left sentence bracket), which is the finite\nverb, the rechte Satzklammer (right sentence bracket) is the verb complex between the\nMittelfeld and the Nachfeld. \n(Telljohann et al. 2009, p.13)\n\t\t" ;
        <http://www.w3.org/2000/01/rdf-schema#subClassOf>
                <http://purl.org/olia/olia-top.owl#TopologicalField> .

<http://purl.org/olia/olia.owl#FamilyName>
        a       <http://www.w3.org/2002/07/owl#Class> ;
        <http://www.w3.org/2000/01/rdf-schema#comment>
                "\n\t\tIn most European cultures, family names have been introduced into name formulas to identify a person's family, so that individuals with the same given name can be distinguished. (CC)\n\t" ;
        <http://www.w3.org/2000/01/rdf-schema#subClassOf>
                <http://purl.org/olia/olia.owl#ProperNoun> ;
        <http://www.w3.org/2002/07/owl#versionInfo>
                "\n\t\tintroduced as generalization over http://purl.org/olia/ubyPos.owl#nounProperSecondName\n\t" .

<http://purl.org/olia/olia.owl#ReciprocalPronoun>
        a       <http://www.w3.org/2002/07/owl#Class> ;
        <http://www.w3.org/2000/01/rdf-schema#comment>
                "\n\t\t\tA reciprocal pronoun is a pronoun that expresses a mutual feeling or action among the referents of a plural subject.\n\t\t\t(http://www.sil.org/linguistics/GlossaryOfLinguisticTerms/WhatIsAReciprocalPronoun.htm 19.09.06)\n\t\t" ;
        <http://www.w3.org/2000/01/rdf-schema#subClassOf>
                <http://purl.org/olia/olia.owl#PersReflPronoun> ;
        <http://www.w3.org/2002/07/owl#versionInfo>
                "\n\t\t\tEAGLES PersReflPronoun with \"Special PronounType\"=\"Reciprocal\".\n\t\t" .

<http://purl.org/olia/olia.owl#SemanticInverseVoice>
        a       <http://www.w3.org/2002/07/owl#Class> ;
        <http://www.w3.org/2000/01/rdf-schema#comment>
                "\n\t\t\tIf the agent outranks the patient on the relevant generic topic hierarchy, \n\t\t\tthe direct-active clause is used.  If the relevant norm is reversed and the \n\t\t\tpatient outranks the agent on the relevant hierarchy, the inverse clause is \n\t\t\tused. (Givon 1994:23)\n\t\t\t(http://purl.org/linguistics/gold/SemanticInverse)\n\t\t" ;
        <http://www.w3.org/2000/01/rdf-schema#subClassOf>
                <http://purl.org/olia/olia.owl#InverseVoice> ;
        <http://www.w3.org/2002/07/owl#versionInfo>
                "http://purl.org/linguistics/gold/SemanticInverse" .

<http://purl.org/olia/olia.owl#SubjunctiveVerb>
        a       <http://www.w3.org/2002/07/owl#Class> ;
        <http://www.w3.org/2000/01/rdf-schema#comment>
                "\n\t\tA subjunctive verb is  typically used to expresses wishes, \n\t\tcommands (in subordinate clauses), emotion, possibility, \n\t\tjudgment, necessity, and statements that are contrary to \n\t\tfact at present.\n\t\t(http://en.wikipedia.org/wiki/Subjunctive_mood 19.09.06)\n\t" ;
        <http://www.w3.org/2000/01/rdf-schema#subClassOf>
                <http://purl.org/olia/olia.owl#FiniteVerb> ;
        <http://www.w3.org/2002/07/owl#versionInfo>
                "TODO: remodelling by properties" , "\n\t\t\tEAGLES finite verbs with VerbForm=\"Subjunctive\".\n\t\t" .

<http://purl.org/olia/olia.owl#VerbalParticle>
        a       <http://www.w3.org/2002/07/owl#Class> ;
        <http://www.w3.org/2000/01/rdf-schema#comment>
                "A verbal particle modifies the verb and carries information on the verb form (e.g., finiteness, tense and aspect). (Dimitrova et al. 2009, Dan Tufis, email 2010/06/09).\n\t\t\t\n\t\t\tIn the Bulgarian MTE specs, Particle/Type=verbal(v) is used to form different type of verbal syntactical relationships, e.g. to create future tense (ще говориш), or particles like се, да. (Dimitrova et al. 2009) \n\t\t\tThe Romanian MTE v4 specs provide a more fine-grained subclassification of (verbal) particles (MTE v4, http://purl.org/olia/mte/multext-east.owl#VerbalParticle)" ;
        <http://www.w3.org/2000/01/rdf-schema#subClassOf>
                <http://purl.org/olia/olia.owl#Particle> ;
        <http://www.w3.org/2002/07/owl#versionInfo>
                "http://purl.org/olia/mte/multext-east.owl#VerbalParticle" .

<http://purl.org/olia/olia.owl#ReflexivePronoun>
        a       <http://www.w3.org/2002/07/owl#Class> ;
        <http://www.w3.org/2000/01/rdf-schema#comment>
                "\n\t\t\tA reflexive pronoun is a pronoun that has coreference with the subject.\n\t\t\t(http://www.sil.org/linguistics/GlossaryOfLinguisticTerms/WhatIsAReflexivePronoun.htm 19.09.06)\n\t\t" ;
        <http://www.w3.org/2000/01/rdf-schema#subClassOf>
                <http://purl.org/olia/olia.owl#PersReflPronoun> ;
        <http://www.w3.org/2002/07/owl#versionInfo>
                "EAGLES PersReflPronoun with SpecialPronounType=\"Reflexive\"." .

<http://purl.org/olia/olia.owl#hasSentenceConjunct>
        a       <http://www.w3.org/2002/07/owl#Class> ;
        <http://www.w3.org/2000/01/rdf-schema#subClassOf>
                <http://purl.org/olia/olia.owl#hasConjunct> ;
        <http://www.w3.org/2000/01/rdf-schema#subClassOf>
                [ a       <http://www.w3.org/2002/07/owl#Restriction> ;
                  <http://www.w3.org/2002/07/owl#onProperty>
                          <http://purl.org/olia/olia.owl#hasChild> ;
                  <http://www.w3.org/2002/07/owl#someValuesFrom>
                          [ a       <http://www.w3.org/2002/07/owl#Class> ;
                            <http://www.w3.org/2002/07/owl#unionOf>
                                    ( <http://purl.org/olia/olia.owl#Sentence> <http://purl.org/olia/olia.owl#Clause> )
                          ]
                ] ;
        <http://www.w3.org/2002/07/owl#versionInfo>
                "http://purl.org/olia/mte/multext-east.owl#SentenceCoordinatingConjunction" .

<http://purl.org/olia/olia.owl#RelativeModality>
        a       <http://www.w3.org/2002/07/owl#Class> ;
        <http://www.w3.org/2000/01/rdf-schema#comment>
                "Mood to express reported speech (or indirect speech) as opposed to direct speech." ;
        <http://www.w3.org/2000/01/rdf-schema#isDefinedBy>
                "http://www.isocat.org/datcat/DC-3836" ;
        <http://www.w3.org/2000/01/rdf-schema#subClassOf>
                <http://purl.org/olia/olia-top.owl#ModalityFeature> ;
        <http://www.w3.org/2002/07/owl#versionInfo>
                "Clarify relationship with DirectSpeech" .

<http://purl.org/olia/olia.owl#ImpersonalVerb>
        a       <http://www.w3.org/2002/07/owl#Class> ;
        <http://www.w3.org/2000/01/rdf-schema#comment>
                "\n                            An impersonal verb is a verb that - occurs only in third person singular forms - has no specified agent , and - has a dummy subject or no subject.\n                                (www.sil.org/linguistics/GlossaryOfLinguisticTerms/WhatIsAnImpersonalVerb.htm; http://www.isocat.org/datcat/DC-1306)\n                            " , "\n                            (of a verb) having no logical subject. Usually in English the pronoun it is used in such cases as a grammatical subject, as for example in It is raining. (of a pronoun) not denoting a person\n                                (www.wordreference.com/English/definition.asp?en=impersonal; http://www.isocat.org/datcat/DC-1306)\n                            " ;
        <http://www.w3.org/2000/01/rdf-schema#label>
                "Impersonal" ;
        <http://www.w3.org/2000/01/rdf-schema#subClassOf>
                <http://purl.org/olia/olia.owl#MainVerb> ;
        <http://www.w3.org/2000/01/rdf-schema#subClassOf>
                [ a       <http://www.w3.org/2002/07/owl#Restriction> ;
                  <http://www.w3.org/2002/07/owl#onProperty>
                          <http://purl.org/olia/olia.owl#hasSemanticValency> ;
                  <http://www.w3.org/2002/07/owl#someValuesFrom>
                          <http://purl.org/olia/olia.owl#Atransitive>
                ] ;
        <http://www.w3.org/2002/07/owl#versionInfo>
                "http://www.isocat.org/datcat/DC-1306" .

<http://purl.org/olia/olia.owl#LexicalUnit>
        a       <http://www.w3.org/2002/07/owl#Class> ;
        <http://www.w3.org/2000/01/rdf-schema#comment>
                "A LexicalUnit is a grammatical expression that is known to the speakers of that language as a conventional expression of a particular concept. It consists of a single lexeme or a conventional combination of lexemes with certain unchangeable characteristics (CC).\n\t" ;
        <http://www.w3.org/2000/01/rdf-schema#subClassOf>
                <http://purl.org/olia/olia-top.owl#SemanticUnit> ;
        <http://www.w3.org/2002/07/owl#versionInfo>
                "introduced as a generalization over Lexeme and Phraseme (as opposed to phrase) with the extension to lexical-semantic resources like Uby" .

<http://purl.org/olia/olia.owl#hasCase>
        a       <http://www.w3.org/2002/07/owl#ObjectProperty> ;
        <http://www.w3.org/2000/01/rdf-schema#domain>
                [ a       <http://www.w3.org/2002/07/owl#Class> ;
                  <http://www.w3.org/2002/07/owl#unionOf>
                          ( <http://purl.org/olia/olia.owl#Noun> <http://purl.org/olia/olia.owl#PronounOrDeterminer> <http://purl.org/olia/olia.owl#Adjective> <http://purl.org/olia/olia.owl#Numeral> <http://purl.org/olia/olia.owl#Article> )
                ] ;
        <http://www.w3.org/2000/01/rdf-schema#range>
                <http://purl.org/olia/olia-top.owl#CaseFeature> ;
        <http://www.w3.org/2000/01/rdf-schema#subPropertyOf>
                <http://purl.org/olia/system.owl#hasFeature> .

<http://purl.org/olia/olia.owl#AdnominalConstituent>
        a       <http://www.w3.org/2002/07/owl#Class> ;
        <http://www.w3.org/2000/01/rdf-schema#comment>
                "\n\t\t\tEach element in a construction is called adnominal that modifies a \n\t\t\tnominal, such as, all types of attributives, such as adjectives, possessives,\n\t\t\tprepositional attributes and relative clauses, such as the beautiful \n\t\t\thouse; the neighbour’s house, the house at the sea, the house, that I want.\n\t\t\t(http://languagelink.let.uu.nl/tds/onto/LinguisticOntology.owl#nominalModifier)\n\t\t"@en , "\n\t\t\tAdnominal wird jedes Element in einer Konstruktion bezeichnet, das der \n\t\t\tModifizierung eines Nomens dient, d.h. alle Formen von Attributen wie \n\t\t\tAdjektive, Genitivattribute, PrÃ¤positionalattribute, RelativsÃ¤tze. Zum \n\t\t\tBeispiel, das schÃ¶ne Haus; das Haus des Nachbars; das Haus am See; das \n\t\t\tHaus, das ich mir schon immer gewÃ¼nscht habe. \n\t\t\t(http://www.uni-trier.de/uni/fb2/ldv/ldv_wiki/index.php/Adnominal)\n\t\t"@de ;
        <http://www.w3.org/2000/01/rdf-schema#label>
                "adnominal modifier" , "nominal modifier" , "adnominal constituent" ;
        <http://www.w3.org/2000/01/rdf-schema#subClassOf>
                <http://purl.org/olia/olia.owl#Modifier> ;
        <http://www.w3.org/2002/07/owl#versionInfo>
                "TODO: rename to AdnominalModifier" , "http://languagelink.let.uu.nl/tds/onto/LinguisticOntology.owl#nominalModifier" .

<http://purl.org/olia/olia.owl#WithFinite>
        a       <http://www.w3.org/2002/07/owl#Class> ;
        <http://www.w3.org/2000/01/rdf-schema#comment>
                "\n\t\t\tFor example, in German the subordinating conjunction \"weil\" introduces \n\t\t\ta clause with a finite verb. \n\t\t\t(http://www.ilc.cnr.it/EAGLES96/annotate/node19.html#oav2u  17.11.06)\n\t\t" ;
        <http://www.w3.org/2000/01/rdf-schema#subClassOf>
                <http://purl.org/olia/olia-top.owl#SubordTypeFeature> ;
        <http://www.w3.org/2002/07/owl#deprecated>
                true ;
        <http://www.w3.org/2002/07/owl#versionInfo>
                "EAGLES, reimplemented within SubordinatingConjunction taxonomy" .

<http://purl.org/olia/olia.owl#OpenCurlyBracket>
        a       <http://www.w3.org/2002/07/owl#Class> ;
        <http://www.w3.org/2000/01/rdf-schema#comment>
                "\n                            Punctuation that is graphically represented as {\n                                (http://www.isocat.org/datcat/DC-2084)\n                            " ;
        <http://www.w3.org/2000/01/rdf-schema#label>
                "open curly bracket" ;
        <http://www.w3.org/2000/01/rdf-schema#subClassOf>
                <http://purl.org/olia/olia.owl#LeftParentheticalPunctuation> ;
        <http://www.w3.org/2002/07/owl#versionInfo>
                "http://www.isocat.org/datcat/DC-2084" .

<http://purl.org/olia/olia.owl#hasReflexivity>
        a       <http://www.w3.org/2002/07/owl#ObjectProperty> ;
        <http://www.w3.org/2000/01/rdf-schema#domain>
                <http://purl.org/olia/olia.owl#Verb> ;
        <http://www.w3.org/2000/01/rdf-schema#range>
                <http://purl.org/olia/olia-top.owl#ReflexivityFeature> ;
        <http://www.w3.org/2000/01/rdf-schema#subPropertyOf>
                <http://purl.org/olia/system.owl#hasFeature> .

<http://purl.org/olia/olia.owl#Numeral>
        a       <http://www.w3.org/2002/07/owl#Class> ;
        <http://www.w3.org/2000/01/rdf-schema#comment>
                "\n\t\t\tA numeral is a word, functioning most typically as an adjective or pronoun, \n\t\t\tthat expresses a number, and relation to the number, such as one of the \n\t\t\tfollowing: Quantity, Sequence, Frequency, Fraction.\n\t\t\t(http://www.sil.org/linguistics/GlossaryOfLinguisticTerms/WhatIsANumeral.htm 19.09.06)\n\t\t" ;
        <http://www.w3.org/2000/01/rdf-schema#label>
                "numeral"@en , "numératif"@fr ;
        <http://www.w3.org/2000/01/rdf-schema#subClassOf>
                <http://purl.org/olia/olia.owl#Quantifier> ;
        <http://www.w3.org/2002/07/owl#versionInfo>
                "Subclassification combines syntactic (Ordinal/CardinalNumeral) and morphological (Fraction, ApproximateNumeral) criteria. To be resolved. In the MULTEXT-East ontology, the latter aspect is represented as http://purl.org/olia/mte/multext-east.owl#MorphologicalFormOfNumeral" , "\n\t\t\tEAGLES top-level category Numeral (NU).\n\t\t\tModelled as subclass of Quantifier (a concept that is absent in EAGLES) in accordance with GOLD.\n\t\t\tDCR subclassification (numberBoth, numeralRoman) ignored\n\t\t" .

<http://purl.org/olia/olia.owl#FrequentiveAspect>
        a       <http://www.w3.org/2002/07/owl#Class> ;
        <http://www.w3.org/2000/01/rdf-schema#comment>
                "\n\t\t\tEvents which are frequently repeated, differs from habitual in that it can \n\t\t\tonly be based upon the observation of several occurrences of the event concerned,\n\t\t\twhereas habitual can be based upon the observation of a single occurrence (Bhat 1999: 53).\n\t\t\t(http://purl.org/linguistics/gold/Frequentive)\n\t\t" ;
        <http://www.w3.org/2000/01/rdf-schema#subClassOf>
                <http://purl.org/olia/olia-top.owl#AspectFeature> ;
        <http://www.w3.org/2002/07/owl#versionInfo>
                "http://purl.org/linguistics/gold/Frequentive" .

<http://purl.org/olia/olia.owl#ConditionalMood>
        a       <http://www.w3.org/2002/07/owl#Class> ;
        <http://www.w3.org/2000/01/rdf-schema#comment>
                "\n      \tIn Inuktitut, conditionality is expressed by verbal inflection. Conditional mood signifies conditional relationships in a sentence. (Nowak 1996, p.39)\n      \t\n      \tA conditional relation is a logical relation in which the illocutionary act employing one of a pair of propositions is expressed or implied to be true or in force if the other proposition is true.\n        (www.sil.org/linguistics/GlossaryOfLinguisticTerms/WhatIsAConditionalRelation.htm; http://www.isocat.org/datcat/DC-1258)\n        \n         Elke Nowak (1996), Transforming the images: Ergativity and transitivity in Inuktitut (Eskimo). Walter de Gruyter, Berlin." ;
        <http://www.w3.org/2000/01/rdf-schema#label>
                "conditional" ;
        <http://www.w3.org/2000/01/rdf-schema#subClassOf>
                <http://purl.org/olia/olia-top.owl#MoodFeature> , <http://purl.org/olia/olia.owl#ConditionalModality> ;
        <http://www.w3.org/2002/07/owl#versionInfo>
                "subClassOf verbFormMood (dcif:conceptualDomain)" , "http://www.isocat.org/datcat/DC-1258" .

<http://purl.org/olia/olia.owl#WHDeterminer>
        a       <http://www.w3.org/2002/07/owl#Class> ;
        <http://www.w3.org/2000/01/rdf-schema#subClassOf>
                <http://purl.org/olia/olia.owl#Determiner> ;
        <http://www.w3.org/2000/01/rdf-schema#subClassOf>
                [ a       <http://www.w3.org/2002/07/owl#Class> ;
                  <http://www.w3.org/2002/07/owl#unionOf>
                          ( <http://purl.org/olia/olia.owl#InterrogativeDeterminer> <http://purl.org/olia/olia.owl#RelativeDeterminer> )
                ] ;
        <http://www.w3.org/2002/07/owl#deprecated>
                true ;
        <http://www.w3.org/2002/07/owl#versionInfo>
                "EAGLES Determiner with Det.-Type=\"Int./Rel.\"." , "TODO: This class is based on surface criteria of Indo-European languages.\n\t\t\t\tIn other (and even IE) languages, relative pronouns are partly also derived from\n\t\t\t\tnon-interrogatives, but rather from demonstratives, cf. English \"that\".\n\t\t\t\tShould be abandoned unless language-independent evidence for its existence \n\t\t\t\tis provided.\n\t\t\t\t\n\t\t\t\tDEPRECATED: to be replaced by InterrogativeDeterminer or RelativeDeterminer\n\t\t" .

<http://purl.org/olia/olia.owl#FirstExclusive>
        a       <http://www.w3.org/2002/07/owl#Class> ;
        <http://www.w3.org/2000/01/rdf-schema#comment>
                "\n\t\t\tRefers to the speaker and one or more nonparticipants, \n\t\t\tbut not hearer(s). Contrasts with  FirstPersonInclusive \n\t\t\t(Crystal 1997: 285).\n\t\t\t(http://purl.org/linguistics/gold/FirstExclusive)\n\t\t" ;
        <http://www.w3.org/2000/01/rdf-schema#subClassOf>
                <http://purl.org/olia/olia.owl#First> , <http://purl.org/olia/olia.owl#Exclusive> ;
        <http://www.w3.org/2002/07/owl#versionInfo>
                "\n\t\t\thttp://purl.org/linguistics/gold/FirstExclusive,\n\t\t\tmodelled as a subconcept of First here\n\t\t" .

<http://purl.org/olia/olia.owl#Homograph>
        a       <http://www.w3.org/2002/07/owl#Class> ;
        <http://www.w3.org/2000/01/rdf-schema#comment>
                "Word that is written like another, but that has a different pronunciation, meaning, and/or origin." ;
        <http://www.w3.org/2000/01/rdf-schema#isDefinedBy>
                "http://www.isocat.org/datcat/DC-1300" ;
        <http://www.w3.org/2000/01/rdf-schema#subClassOf>
                <http://purl.org/olia/olia-top.owl#LexicalRelation> , <http://purl.org/olia/system.owl#Relation> .

<http://purl.org/olia/olia.owl#Point>
        a       <http://www.w3.org/2002/07/owl#Class> ;
        <http://www.w3.org/2000/01/rdf-schema#comment>
                "\n                            Sign (.) used to expresses the end of a sentence or an abbreviation.\n                                (http://www.isocat.org/datcat/DC-1445)\n                            " ;
        <http://www.w3.org/2000/01/rdf-schema#label>
                "dot" , "point" ;
        <http://www.w3.org/2000/01/rdf-schema#subClassOf>
                <http://purl.org/olia/olia.owl#SentenceFinalPunctuation> ;
        <http://www.w3.org/2002/07/owl#versionInfo>
                "http://www.isocat.org/datcat/DC-1445" , "subClassOf partOfSpeech (dcif:conceptualDomain)" .

<http://purl.org/olia/olia.owl#LocationRole>
        a       <http://www.w3.org/2002/07/owl#Class> ;
        <http://www.w3.org/2000/01/rdf-schema#comment>
                "\n\t\t\tSemantic role for the final location of action or a time of the action. \n\t\t\t(http://www.isocat.org/datcat/DC-1326)\n\t\t\t\n\t\t\tAdverbials that indicate place/setting of the event. \n\t\t\t(PP-LOC on (NP the moon))\n\t\t\tMay also indicate metaphorical location:\n\t\t\t(PP-LOC amongst (NP yourselves))\n\t\t\t(Bies et al. 1995)\n\t\t" ;
        <http://www.w3.org/2000/01/rdf-schema#subClassOf>
                <http://purl.org/olia/olia-top.owl#SemanticRole> ;
        <http://www.w3.org/2002/07/owl#versionInfo>
                "http://languagelink.let.uu.nl/tds/onto/LinguisticOntology.owl#locationRole, cf. the TIGER edge label \"Locative\"" .

<http://purl.org/olia/olia.owl#Verbal>
        a       <http://www.w3.org/2002/07/owl#Class> ;
        <http://www.w3.org/2000/01/rdf-schema#comment>
                "In MULTEXT-East a characteristic of abbreviated verbs (http://purl.org/olia/mte/multext-east.owl#Verbal)\n\t\t" ;
        <http://www.w3.org/2000/01/rdf-schema#subClassOf>
                <http://purl.org/olia/olia-top.owl#SyntacticFunction> ;
        <http://www.w3.org/2002/07/owl#versionInfo>
                "http://purl.org/olia/mte/multext-east.owl#Verbal" .

<http://purl.org/olia/olia.owl#OnceNoun>
        a       <http://www.w3.org/2002/07/owl#Class> ;
        <http://www.w3.org/2000/01/rdf-schema#comment>
                "noun conveying the meaning that the action is performed once" ;
        <http://www.w3.org/2000/01/rdf-schema#isDefinedBy>
                "http://www.isocat.org/datcat/DC-3853" ;
        <http://www.w3.org/2000/01/rdf-schema#subClassOf>
                <http://purl.org/olia/olia.owl#CommonNoun> ;
        <http://www.w3.org/2002/07/owl#deprecated>
                true ;
        <http://www.w3.org/2002/07/owl#versionInfo>
                "onceNoun [DC-3853] ``noun conveying the meaning that the action is performed once''. Clearly, this noun carries a meaning that is closely related to aspect information (e.g., SemelfactiveAspect), but as aspect is a verb-centered concept, it would have been counter-intuitive to model this as Noun and hasAspect some SemelfactiveAspect. Hence, this concept is directly adopted in the OLiA Reference Model, but marked as deprecated until an ontologically satisfying modeling of aspect-related features of nouns has been achieved." .

<http://purl.org/olia/olia.owl#RelevanceAspect>
        a       <http://www.w3.org/2002/07/owl#Class> ;
        <http://www.w3.org/2000/01/rdf-schema#comment>
                "\n\t\t\trelevance aspect\n\t\t\t(http://languagelink.let.uu.nl/tds/onto/LinguisticOntology.owl#relevanceAspect)\n\t\t" ;
        <http://www.w3.org/2000/01/rdf-schema#subClassOf>
                <http://purl.org/olia/olia-top.owl#AspectFeature> ;
        <http://www.w3.org/2002/07/owl#versionInfo>
                "http://languagelink.let.uu.nl/tds/onto/LinguisticOntology.owl#relevanceAspect" .

<http://purl.org/olia/olia.owl#AdjutativeVoice>
        a       <http://www.w3.org/2002/07/owl#Class> ;
        <http://www.w3.org/2000/01/rdf-schema#comment>
                "voice for a construction where the subject of the verb is not an agent of the action denoted by the verb but is assisting an unstated agent in performing the action" ;
        <http://www.w3.org/2000/01/rdf-schema#isDefinedBy>
                "http://www.isocat.org/datcat/DC-3844" ;
        <http://www.w3.org/2000/01/rdf-schema#subClassOf>
                <http://purl.org/olia/olia-top.owl#VoiceFeature> .

<http://purl.org/olia/olia.owl#PossessiveAdjective>
        a       <http://www.w3.org/2002/07/owl#Class> ;
        <http://www.w3.org/2000/01/rdf-schema#comment>
                "A PossessiveAdjective is an denominal adjective, often derived from a ProperNoun, that serves to indicate possession in most Slavic languages. \n\t\tUnlike a genitival construction, a possessive adjective shows agreement with its head noun. (Chiarcos)" , "Adjective/Type=\"possessive\" are denominal, not pronominal expressions of possession (Ivan A Derzhanski, email 2010/06/09). Therefore not to be confused with Pronoun/Type=adjectival(a) (Bulgarian only), for words like умно /cleverly, wisely, sensibly/, which are derived from adjectives. (Dimitrova et al. 2009)\n\t\t\te.g., Slovene dušikovima/dušikov, Marsovi/Marsov,\n\t\t\tSlovak vojvodova/vojvodov, vojvodove/vojvodov, vojvodovej/vojvodov, vojvodovho/vojvodov, vojvodovi/vojvodov, vojvodovmu/vojvodov, vojvodovo/vojvodov, vojvodovom/vojvodov, vojvodovou/vojvodov,\n\t\t\tSerbian evroazijske/evroazijska, evroazijskih/evroazijski, Goldštajnov, govornikov, Jehovine/Jehovin, malabarskom/malabarski, O'Brajenov, O'Brajenovog/O'Brajenov, oficirov,\n\t\t\tCzech Riegrovými/Riegrův, Stradellovými/Stradellův, Tristanovou/Tristanův, Wagnerových/Wagnerův, Wagnerovým/Wagnerův, Weberovi/Weberův, Weberových/Weberův, Wertherovi/Wertherův, Winstonovi/Winstonův \n\t\t\t(http://purl.org/olia/mte/multext-east.owl#PossessiveAdjective)" ;
        <http://www.w3.org/2000/01/rdf-schema#subClassOf>
                <http://purl.org/olia/olia.owl#Adjective> ;
        <http://www.w3.org/2002/07/owl#versionInfo>
                "http://purl.org/olia/mte/multext-east.owl#PossessiveAdjective" .

<http://purl.org/olia/olia.owl#Perfect>
        a       <http://www.w3.org/2002/07/owl#Class> ;
        <http://www.w3.org/2000/01/rdf-schema#comment>
                "\n                            A verb tense that refers to completed action in the past. It corresponds to three English tenses.\n                                (www.southwestern.edu/~carlg/Latin_Web/glossary.html; http://www.isocat.org/datcat/DC-1351)\n                            " ;
        <http://www.w3.org/2000/01/rdf-schema#label>
                "Perfect" ;
        <http://www.w3.org/2000/01/rdf-schema#subClassOf>
                <http://purl.org/olia/olia.owl#AbsoluteTense> ;
        <http://www.w3.org/2002/07/owl#versionInfo>
                "http://www.isocat.org/datcat/DC-1351, modelled as an absolute tense here" .

<http://purl.org/olia/olia.owl#StrongPersonalPronoun>
        a       <http://www.w3.org/2002/07/owl#Class> ;
        <http://www.w3.org/2000/01/rdf-schema#comment>
                "\n                            Personal pronoun that can occupy the position after a preposition and/or reinforce a weak personal pronoun.\n                                (Eagles; http://www.isocat.org/datcat/DC-1390)\n                            " ;
        <http://www.w3.org/2000/01/rdf-schema#label>
                "strong personal pronoun" ;
        <http://www.w3.org/2000/01/rdf-schema#subClassOf>
                <http://purl.org/olia/olia.owl#PersonalPronoun> ;
        <http://www.w3.org/2002/07/owl#versionInfo>
                "subClassOf personalPronoun (dcif:isA)" , "http://www.isocat.org/datcat/DC-1390" .

<http://purl.org/olia/olia.owl#Morpheme>
        a       <http://www.w3.org/2002/07/owl#Class> ;
        <http://www.w3.org/2000/01/rdf-schema#comment>
                "\n                            A morpheme is the smallest meaningful unit in the grammar of a language.\n                                (www.sil.org/linguistics/GlossaryOfLinguisticTerms/WhatIsAMorpheme.htm; http://www.isocat.org/datcat/DC-1330)\n                            " ;
        <http://www.w3.org/2000/01/rdf-schema#label>
                "morpheme" ;
        <http://www.w3.org/2000/01/rdf-schema#subClassOf>
                <http://purl.org/olia/olia-top.owl#MorphologicalCategory> ;
        <http://www.w3.org/2002/07/owl#versionInfo>
                "http://www.isocat.org/datcat/DC-1330" .

<http://purl.org/olia/olia.owl#ConditionalPronoun>
        a       <http://www.w3.org/2002/07/owl#Class> ;
        <http://www.w3.org/2000/01/rdf-schema#comment>
                "\n                            conditional pronoun\n                                (MIRACL & LSCA; http://www.isocat.org/datcat/DC-2222)\n                            " ;
        <http://www.w3.org/2000/01/rdf-schema#label>
                "conditional pronoun" ;
        <http://www.w3.org/2000/01/rdf-schema#subClassOf>
                <http://purl.org/olia/olia.owl#Pronoun> ;
        <http://www.w3.org/2002/07/owl#versionInfo>
                "subClassOf pronoun (dcif:isA)" , "check for a definition" , "http://www.isocat.org/datcat/DC-2222" .

<http://purl.org/olia/olia.owl#Prefix>
        a       <http://www.w3.org/2002/07/owl#Class> ;
        <http://www.w3.org/2000/01/rdf-schema#comment>
                "\n                            Affix added before a word to change its meaning or part of speech.\n                                (Sue Ellen Wright + Gil Francopoulo; http://www.isocat.org/datcat/DC-1365)\n                            " ;
        <http://www.w3.org/2000/01/rdf-schema#label>
                "prefix" ;
        <http://www.w3.org/2000/01/rdf-schema#subClassOf>
                <http://purl.org/olia/olia.owl#Affix> ;
        <http://www.w3.org/2002/07/owl#versionInfo>
                "http://www.isocat.org/datcat/DC-1365" .

<http://purl.org/olia/olia.owl#ProperNoun>
        a       <http://www.w3.org/2002/07/owl#Class> ;
        <http://www.w3.org/2000/01/rdf-schema#comment>
                "\n\t\tProper nouns (also called proper names) are the names of unique entities. \n\t\t(http://en.wikipedia.org/wiki/Noun 19.09.06)\n\t" ;
        <http://www.w3.org/2000/01/rdf-schema#label>
                "nom propre"@fr , "proper noun"@en , "proper name"@en ;
        <http://www.w3.org/2000/01/rdf-schema#subClassOf>
                <http://purl.org/olia/olia.owl#Noun> ;
        <http://www.w3.org/2002/07/owl#versionInfo>
                "\n\t\tEAGLES Noun with Type=\"Proper\".\n\t" .

<http://purl.org/olia/olia.owl#OnomatopoeticWord>
        a       <http://www.w3.org/2002/07/owl#Class> ;
        <http://www.w3.org/2000/01/rdf-schema#comment>
                "no definition given" ;
        <http://www.w3.org/2000/01/rdf-schema#label>
                "onomatopoetic word"@en , "onomatopée"@fr ;
        <http://www.w3.org/2000/01/rdf-schema#subClassOf>
                <http://purl.org/olia/olia.owl#Residual> ;
        <http://www.w3.org/2002/07/owl#versionInfo>
                "Bambara Reference Corpus \"Onomatopée\", http://cormand.huma-num.fr" ;
        <http://www.w3.org/2004/02/skos/core#altLabel>
                "onomatopée"@fr .

<http://purl.org/olia/olia.owl#NominalNumber>
        a       <http://www.w3.org/2002/07/owl#Class> ;
        <http://www.w3.org/2000/01/rdf-schema#comment>
                "Nominal numbers are used to identify or refer the things. It does not show the quantity or rank.\n\t\t\t\n\t\t\tExample:\n\t\t\tངེ་གི་ འགལ་འཕིན་ ཨང་གངས་ འདི་ ༡༧༦༤༩༠༣༧ ཨིན།\n\t\t\tNGIGI DRUELTHRIN ANGDRANG 'DI 17649037 INN\n\t\t\tmy mobile number is 17649037 be\n\t\t\t“ My mobile number is 17649037.”\n\t\t\t(Jurmey Rabgay, email Sep 20, 2010, http://purl.org/olia/dzongkha.owl#NominalNumber)" ;
        <http://www.w3.org/2000/01/rdf-schema#subClassOf>
                <http://purl.org/olia/olia.owl#Numeral> ;
        <http://www.w3.org/2002/07/owl#versionInfo>
                "adopted from Dzongkha tagset (Chunkgu et al. 2010, http://purl.org/olia/dzongkha.owl#NominalNumber)" .

<http://purl.org/olia/olia.owl#IndefiniteCardinalQuantifier>
        a       <http://www.w3.org/2002/07/owl#Class> ;
        <http://www.w3.org/2000/01/rdf-schema#comment>
                "ndefiniteCardinalNumeral: A word used to express imprecise quantity." ;
        <http://www.w3.org/2000/01/rdf-schema#isDefinedBy>
                "http://www.isocat.org/datcat/DC-3023 (indefiniteCardinalNumeral)" ;
        <http://www.w3.org/2000/01/rdf-schema#label>
                "indefinite cardinal numeral" ;
        <http://www.w3.org/2000/01/rdf-schema#subClassOf>
                <http://purl.org/olia/olia.owl#IndefiniteQuantifier> .

<http://purl.org/olia/olia.owl#FuturePerfect>
        a       <http://www.w3.org/2002/07/owl#Class> ;
        <http://www.w3.org/2000/01/rdf-schema#comment>
                "\n\t\t\tRelativeFutureTense locates the situation in question after a contextually \n\t\t\tdetermined temporal reference point, regardless of the latter's relation to\n\t\t\tthe moment of utterance. Also called FuturePerfectTense (Comrie 1985:69-71).\n\t\t\t(http://purl.org/linguistics/gold/RelativeFuture)\n\n\t\t\tA verb tense that refers to an action or state of being completed in the future. \n\t\t\tTranslation into English requires the use of the auxiliary verbs will/shall have. \n\t\t\t(www.southwestern.edu/~carlg/Latin_Web/glossary.html; http://www.isocat.org/datcat/DC-1292)\n\n\t\t\tA tense of verbs describing an action that will have been performed by a certain time. \n\t\t\tIn English this is formed with will have or shall have plus the past participle.\n            (www.wordreference.com/English/definition.asp?en=future+perfect; http://www.isocat.org/datcat/DC-1292)\n            " ;
        <http://www.w3.org/2000/01/rdf-schema#subClassOf>
                <http://purl.org/olia/olia.owl#RelativeTense> ;
        <http://www.w3.org/2002/07/owl#versionInfo>
                "http://purl.org/linguistics/gold/RelativeFuture, http://www.isocat.org/datcat/DC-1292" .

<http://purl.org/olia/olia.owl#FirstInclusive>
        a       <http://www.w3.org/2002/07/owl#Class> ;
        <http://www.w3.org/2000/01/rdf-schema#comment>
                "\n\t\t\tRefers to the speaker, hearer(s) and possibly others. \n\t\t\tContrasts with FirstPersonExclusive (Crystal 1997: 285).\n\t\t\t(http://purl.org/linguistics/gold/FirstInclusive)\n\t\t" ;
        <http://www.w3.org/2000/01/rdf-schema#subClassOf>
                <http://purl.org/olia/olia.owl#First> , <http://purl.org/olia/olia.owl#Inclusive> ;
        <http://www.w3.org/2002/07/owl#versionInfo>
                "\n\t\t\thttp://purl.org/linguistics/gold/FirstInclusive, \n\t\t\tmodelled here as subconcept of First\n\t\t" .

<http://purl.org/olia/olia.owl#BenefactiveCase>
        a       <http://www.w3.org/2002/07/owl#Class> ;
        <http://www.w3.org/2000/01/rdf-schema#comment>
                "\n\t\t\tBenefactiveCase expresses that the referent of the noun it marks \n\t\t\treceives the benefit of the situation expressed by the clause \n\t\t\t(Crystal 1980: 43; Gove, et al. 1966: 203).\n\t\t\t(http://purl.org/linguistics/gold/Benefactive)\n\t\t" ;
        <http://www.w3.org/2000/01/rdf-schema#subClassOf>
                <http://purl.org/olia/olia-top.owl#CaseFeature> ;
        <http://www.w3.org/2002/07/owl#versionInfo>
                "http://purl.org/linguistics/gold/Benefactive; http://www.isocat.org/datcat/DC-1247" .

<http://purl.org/olia/olia.owl#InterrogativeCardinalQuantifier>
        a       <http://www.w3.org/2002/07/owl#Class> ;
        <http://www.w3.org/2000/01/rdf-schema#comment>
                "interrogativeCardinalNumeral: An interrogative/relative word used to ask about quantity." ;
        <http://www.w3.org/2000/01/rdf-schema#isDefinedBy>
                "http://www.isocat.org/datcat/DC-3018 (interrogativeCardinalNumeral)" ;
        <http://www.w3.org/2000/01/rdf-schema#label>
                "interrogative cardinal numeral" ;
        <http://www.w3.org/2000/01/rdf-schema#subClassOf>
                <http://purl.org/olia/olia.owl#InterrogativeQuantifier> .

<http://purl.org/olia/olia.owl#BenchLevelRegister>
        a       <http://www.w3.org/2002/07/owl#Class> ;
        <http://www.w3.org/2000/01/rdf-schema#comment>
                "\n                            Register of terms used in applications-oriented as opposed to theoretical or academic levels of language.\n                                (ISO12620; http://www.isocat.org/datcat/DC-1989)\n                            " ;
        <http://www.w3.org/2000/01/rdf-schema#label>
                "shop term" , "bench-level register" ;
        <http://www.w3.org/2000/01/rdf-schema#subClassOf>
                <http://purl.org/olia/olia-top.owl#RegisterFeature> ;
        <http://www.w3.org/2002/07/owl#versionInfo>
                "subClassOf register (dcif:conceptualDomain)" , "http://www.isocat.org/datcat/DC-1989" .

<http://purl.org/olia/olia.owl#hasChild>
        a       <http://www.w3.org/2002/07/owl#ObjectProperty> ;
        <http://www.w3.org/2000/01/rdf-schema#comment>
                "In hierarchical relations, the parent is modelled as source, the child as target." ;
        <http://www.w3.org/2000/01/rdf-schema#subPropertyOf>
                <http://purl.org/olia/system.owl#hasTarget> .

<http://purl.org/olia/olia.owl#AdmonitiveModality>
        a       <http://www.w3.org/2002/07/owl#Class> ;
        <http://www.w3.org/2000/01/rdf-schema#comment>
                "\n\t\t\tExpression of warning (Bybee 1985:22)\n\t\t\t(http://languagelink.let.uu.nl/tds/onto/LinguisticOntology.owl#admonitiveModality)\n\t\t" ;
        <http://www.w3.org/2000/01/rdf-schema#subClassOf>
                <http://purl.org/olia/olia-top.owl#ModalityFeature> ;
        <http://www.w3.org/2002/07/owl#versionInfo>
                "\n\t\t\thttp://languagelink.let.uu.nl/tds/onto/LinguisticOntology.owl#admonitiveModality\n\t\t" .

<http://purl.org/olia/olia.owl#EmphaticPronoun>
        a       <http://www.w3.org/2002/07/owl#Class> ;
        <http://www.w3.org/2000/01/rdf-schema#comment>
                "\n                            Pronoun marked to show its importance.\n                                (http://www.isocat.org/datcat/DC-1941)\n                            " ;
        <http://www.w3.org/2000/01/rdf-schema#label>
                "emphatic pronoun" ;
        <http://www.w3.org/2000/01/rdf-schema#subClassOf>
                <http://purl.org/olia/olia.owl#Pronoun> ;
        <http://www.w3.org/2002/07/owl#deprecated>
                true ;
        <http://www.w3.org/2002/07/owl#equivalentClass>
                [ a       <http://www.w3.org/2002/07/owl#Class> ;
                  <http://www.w3.org/2002/07/owl#intersectionOf>
                          ( <http://purl.org/olia/olia.owl#Pronoun>
                            [ a       <http://www.w3.org/2002/07/owl#Restriction> ;
                              <http://www.w3.org/2002/07/owl#onProperty>
                                      <http://purl.org/olia/olia.owl#hasEmphasis> ;
                              <http://www.w3.org/2002/07/owl#someValuesFrom>
                                      <http://purl.org/olia/olia.owl#Emphatic>
                            ]
                          )
                ] ;
        <http://www.w3.org/2002/07/owl#versionInfo>
                "subClassOf pronoun (dcif:isA)" , "http://www.isocat.org/datcat/DC-1941" , "DEPRECATED: shorthand for Pronoun and hasEmphasis some Emphatic" .

<http://purl.org/olia/olia.owl#LocativePronoun>
        a       <http://www.w3.org/2002/07/owl#Class> ;
        <http://www.w3.org/2000/01/rdf-schema#comment>
                "A Locative pronoun is a pronoun, which locates the object of a noun or place of anything.\n\t\t\t\n\t\t\t་ ན་ གས་ ང་ ་ ག།\n\t\t\tNâ[LP] PhÜntsho'ling-lu ShÔ\n\t\t\t'Come here at Phuntsholing'\n\t\t\t(http://panl10n.net/english/Outputs%20Phase%202/CCs/Bhutan/Papers/2007/0701/PartOfSpeech.pdf)" ;
        <http://www.w3.org/2000/01/rdf-schema#subClassOf>
                <http://purl.org/olia/olia.owl#Pronoun> ;
        <http://www.w3.org/2002/07/owl#versionInfo>
                "TODO: clarify relationship with pronominal adverb" , "adopted from Dzongkha tagset (Chungku et al. 2010)" .

<http://purl.org/olia/olia.owl#PossessedCase>
        a       <http://www.w3.org/2002/07/owl#Class> ;
        <http://www.w3.org/2000/01/rdf-schema#comment>
                "\n\t\t\tPossessedCase is used to mark the noun whose referent is possessed \n\t\t\tby the referent of another noun.\n\t\t\t(http://purl.org/linguistics/gold/Possessed)\n\t\t" ;
        <http://www.w3.org/2000/01/rdf-schema#subClassOf>
                <http://purl.org/olia/olia-top.owl#CaseFeature> ;
        <http://www.w3.org/2002/07/owl#versionInfo>
                "http://purl.org/linguistics/gold/Possessed" .

<http://purl.org/olia/olia.owl#IrrealisMood>
        a       <http://www.w3.org/2002/07/owl#Class> ;
        <http://www.w3.org/2000/01/rdf-schema#comment>
                "\n\t\t\tIrrealis modality indicates the situation to which it pertains is \n\t\t\tnon-actual or non-factual.\n\t\t\t(http://languagelink.let.uu.nl/tds/onto/LinguisticOntology.owl#irrealisModality)\n\t\t" ;
        <http://www.w3.org/2000/01/rdf-schema#subClassOf>
                <http://purl.org/olia/olia-top.owl#MoodFeature> , <http://purl.org/olia/olia.owl#IrrealisModality> ;
        <http://www.w3.org/2002/07/owl#versionInfo>
                "http://languagelink.let.uu.nl/tds/onto/LinguisticOntology.owl#irrealisModality" .

<http://purl.org/olia/olia.owl#CloseCurlyBracket>
        a       <http://www.w3.org/2002/07/owl#Class> ;
        <http://www.w3.org/2000/01/rdf-schema#comment>
                "\n                            Punctuation that is graphically represented by }\n                                (http://www.isocat.org/datcat/DC-2085)\n                            " ;
        <http://www.w3.org/2000/01/rdf-schema#label>
                "close curly bracket" ;
        <http://www.w3.org/2000/01/rdf-schema#subClassOf>
                <http://purl.org/olia/olia.owl#RightParentheticalPunctuation> ;
        <http://www.w3.org/2002/07/owl#versionInfo>
                "http://www.isocat.org/datcat/DC-2085" .

<http://purl.org/olia/olia.owl#PastParticiple>
        a       <http://www.w3.org/2002/07/owl#Class> ;
        <http://www.w3.org/2000/01/rdf-schema#subClassOf>
                <http://purl.org/olia/olia.owl#Participle> ;
        <http://www.w3.org/2002/07/owl#equivalentClass>
                [ a       <http://www.w3.org/2002/07/owl#Class> ;
                  <http://www.w3.org/2002/07/owl#intersectionOf>
                          ( <http://purl.org/olia/olia.owl#Participle>
                            [ a       <http://www.w3.org/2002/07/owl#Restriction> ;
                              <http://www.w3.org/2002/07/owl#onProperty>
                                      <http://purl.org/olia/olia.owl#hasTense> ;
                              <http://www.w3.org/2002/07/owl#someValuesFrom>
                                      <http://purl.org/olia/olia.owl#Past>
                            ]
                          )
                ] ;
        <http://www.w3.org/2002/07/owl#versionInfo>
                "introduced as a shorthand for Participle and hasTense some Past" .

<http://purl.org/olia/olia.owl#ContinuousAspect>
        a       <http://www.w3.org/2002/07/owl#Class> ;
        <http://www.w3.org/2000/01/rdf-schema#comment>
                "\n\t\t\tSimilar to progressive, however an aspect is continuous versus progressive \n\t\t\twhen it is anchored to non-punctual time reference (Salaberry 2002:264).\n\t\t\t(http://purl.org/linguistics/gold/Continuous)\n\t\t" ;
        <http://www.w3.org/2000/01/rdf-schema#subClassOf>
                <http://purl.org/olia/olia-top.owl#AspectFeature> ;
        <http://www.w3.org/2002/07/owl#versionInfo>
                "\n\t\t\thttp://purl.org/linguistics/gold/Continuous\n\t\t" .

<http://purl.org/olia/olia.owl#Definite>
        a       <http://www.w3.org/2002/07/owl#Class> ;
        <http://www.w3.org/2000/01/rdf-schema#comment>
                "\n\t\t\tValue referring to the capacity of identification of an entity. (http://www.isocat.org/datcat/DC-2004)\n\t\t\n\t\t\tAn entity is specified as definite when it refers to a particularized individual of the species denoted by the noun.\n\t\t\t(http://languagelink.let.uu.nl/tds/onto/LinguisticOntology.owl#definite)\n\t\t\n\t\t\tDefinite noun phrases are used to refer to entities which are specific \n\t\t\tand identifiable in a given context. \n\t\t\t(http://en.wikipedia.org/wiki/Definiteness  20.11.06)\n\t\t"@en ;
        <http://www.w3.org/2000/01/rdf-schema#subClassOf>
                <http://purl.org/olia/olia-top.owl#DefinitenessFeature> ;
        <http://www.w3.org/2002/07/owl#versionInfo>
                "\n\t\t\tEAGLES, http://languagelink.let.uu.nl/tds/onto/LinguisticOntology.owl#definite, http://www.isocat.org/datcat/DC-2004\n\t\t" .

<http://purl.org/olia/olia.owl#Personal>
        a       <http://www.w3.org/2002/07/owl#Class> ;
        <http://www.w3.org/2000/01/rdf-schema#comment>
                "\n                            Property that refers to the person.\n                                (http://www.isocat.org/datcat/DC-1946)\n                            " ;
        <http://www.w3.org/2000/01/rdf-schema#label>
                "personal" ;
        <http://www.w3.org/2000/01/rdf-schema#subClassOf>
                <http://purl.org/olia/olia-top.owl#ReferentTypeFeature> ;
        <http://www.w3.org/2002/07/owl#versionInfo>
                "subClassOf referentType (dcif:conceptualDomain)" , "http://www.isocat.org/datcat/DC-1946" .

<http://purl.org/olia/olia.owl#Augmentative>
        a       <http://www.w3.org/2002/07/owl#Class> ;
        <http://www.w3.org/2000/01/rdf-schema#comment>
                "A special form of a noun that signals that the\n                        object being referred to is large relative to the usual size of such an\n                        object [Crystal 1980: 34]." ;
        <http://www.w3.org/2000/01/rdf-schema#isDefinedBy>
                "http://www.isocat.org/datcat/DC-3094 (augmentativeSize)" ;
        <http://www.w3.org/2000/01/rdf-schema#subClassOf>
                <http://purl.org/olia/olia.owl#Derivation> ;
        <http://www.w3.org/2002/07/owl#versionInfo>
                "modelled as a derivational process analoguously to Diminuitive" .

<http://purl.org/olia/olia.owl#hasCoordType>
        a       <http://www.w3.org/2002/07/owl#ObjectProperty> ;
        <http://www.w3.org/2000/01/rdf-schema#domain>
                <http://purl.org/olia/olia.owl#CoordinatingConjunction> ;
        <http://www.w3.org/2000/01/rdf-schema#range>
                <http://purl.org/olia/olia-top.owl#CoordTypeFeature> ;
        <http://www.w3.org/2000/01/rdf-schema#subPropertyOf>
                <http://purl.org/olia/system.owl#hasFeature> .

<http://purl.org/olia/olia.owl#AdjectivalModifier>
        a       <http://www.w3.org/2002/07/owl#Class> ;
        <http://www.w3.org/2000/01/rdf-schema#comment>
                "\n\t\t\tA nominal is modified by an adjective.\n\t\t\t(http://languagelink.let.uu.nl/tds/onto/LinguisticOntology.owl#adjectivalModifier)\n\t\t" ;
        <http://www.w3.org/2000/01/rdf-schema#subClassOf>
                <http://purl.org/olia/olia.owl#AdnominalConstituent> ;
        <http://www.w3.org/2002/07/owl#versionInfo>
                "http://languagelink.let.uu.nl/tds/onto/LinguisticOntology.owl#adjectivalModifier" .

<http://purl.org/olia/olia.owl#NonInitial>
        a       <http://www.w3.org/2002/07/owl#Class> ;
        <http://www.w3.org/2000/01/rdf-schema#comment>
                "\n\t\t\tWhen two distinct words occur, as in German weder...noch..., then the second is given the Non-initial value. \n\t\t\t(http://www.ilc.cnr.it/EAGLES96/annotate/node18.html#oav1av  17.11.06)\n\t\t" ;
        <http://www.w3.org/2000/01/rdf-schema#subClassOf>
                <http://purl.org/olia/olia-top.owl#CoordTypeFeature> ;
        <http://www.w3.org/2002/07/owl#deprecated>
                true ;
        <http://www.w3.org/2002/07/owl#versionInfo>
                "EAGLES, reimplemented as subhierarchy of CoordinatingConjunction" .

<http://purl.org/olia/olia.owl#InallativeCase>
        a       <http://www.w3.org/2002/07/owl#Class> ;
        <http://www.w3.org/2000/01/rdf-schema#comment>
                "\n\t\t\tInallativeCase expresses that  something is moving toward the region \n\t\t\tthat is inside the referent of the noun it marks. It has the meaning \n\t\t\t'towards in(side)'.\n\t\t\t(http://purl.org/linguistics/gold/Inallative)\n\t\t" ;
        <http://www.w3.org/2000/01/rdf-schema#subClassOf>
                <http://purl.org/olia/olia-top.owl#CaseFeature> ;
        <http://www.w3.org/2002/07/owl#versionInfo>
                "http://purl.org/linguistics/gold/Inallative" .

<http://purl.org/olia/olia.owl#DifferentialPronoun>
        a       <http://www.w3.org/2002/07/owl#Class> ;
        <http://www.w3.org/2000/01/rdf-schema#comment>
                "A pronoun, which classifies or differentiates(pronoun) by a single basis, like everybody; each; individual etc. \n\t\t\t\n\t\t\tའ ག་པ ་ ་ ར་ ག་ར་ ན་ ང་ ང་ཁ་ ས་ད །\n\t\t\tDrupai Miser Gara Enrung Dzongkha ShegÔ\n\t\t\t'Every Bhutanese must know Dzongkha'\n\t\t\t(http://panl10n.net/english/Outputs%20Phase%202/CCs/Bhutan/Papers/2007/0701/PartOfSpeech.pdf)" ;
        <http://www.w3.org/2000/01/rdf-schema#subClassOf>
                <http://purl.org/olia/olia.owl#Pronoun> ;
        <http://www.w3.org/2002/07/owl#versionInfo>
                "adopted from Dzongkha tagset (Chungku et al. 2010)" , "TOCHECK: maybe this is a quantifier ?" .

<http://purl.org/olia/olia.owl#NecessitativePassive>
        a       <http://www.w3.org/2002/07/owl#Class> ;
        <http://www.w3.org/2000/01/rdf-schema#comment>
                "\n\t\t\tA passive in Irish in which the preposition \"with\" is used, and a semantic \n\t\t\tmeaning of necessity is added. (Noonan 1994:280)\n\t\t\t(http://purl.org/linguistics/gold/NecessitativePassive)\n\t\t" ;
        <http://www.w3.org/2000/01/rdf-schema#subClassOf>
                <http://purl.org/olia/olia.owl#PassiveVoice> ;
        <http://www.w3.org/2002/07/owl#versionInfo>
                "http://purl.org/linguistics/gold/NecessitativePassive" .

<http://purl.org/olia/olia.owl#TranslativeCase>
        a       <http://www.w3.org/2002/07/owl#Class> ;
        <http://www.w3.org/2000/01/rdf-schema#comment>
                "\n\t\t\tTranslativeCase expresses that the referent of the noun, or the quality \n\t\t\tof the adjective, that it marks is the result of a process of change \n\t\t\t(Lyons 1968: 299301, Gove, et al. 1966: 813,2429, Sebeok 1946: 17, \n\t\t\tHakulinen 1961: 70). X along, across Y.\n\t\t\t(http://purl.org/linguistics/gold/Translative)\n\t\t" ;
        <http://www.w3.org/2000/01/rdf-schema#subClassOf>
                <http://purl.org/olia/olia-top.owl#CaseFeature> ;
        <http://www.w3.org/2002/07/owl#versionInfo>
                "http://purl.org/linguistics/gold/Translative, http://www.isocat.org/datcat/DC-1406" .

<http://purl.org/olia/olia.owl#Coordination>
        a       <http://www.w3.org/2002/07/owl#Class> ;
        <http://www.w3.org/2000/01/rdf-schema#comment>
                "\n\t\t\tAs has already been shown in some of the preceding examples, the issue of coordination necessarily arises: how is\n\t\t\tcoordination to be represented in terms of constituency? Different approaches have been taken, and in the example\n\t\t\tanalyses given in this document, we have chosen to take a traditional approach, showing the coordinated constituents\n\t\t\tat the same level, with the conjunction between them (see also 47 and 48):\n\n\t\t\t(51)  \t[NP [NP John NP] and [NP Mary NP] NP]\n\t\t\t(52)  \tShe went [PP [PP to the library PP] or [PP to the cafeteria PP] PP]\n\t\t\t(53)  \tHe works [ADVP [ADVP very slowly ADVP] but [ADVP very meticulously ADVP] ADVP]\n\t\t\t\n\t\t\tHowever, in practice, in an automated parsing system, this is not an easy differentiation to make, and in some\n\t\t\texisting schemes, a slightly less satisfactory solution has been found, viz. analysing coordination in a similar\n\t\t\tfashion to subordination.\n\n\t\t\tMost constituents (both phrases and clauses) can be coordinated, but the extent to which this is possible will\n\t\t\tdiffer across languages. The conjuncts may be marked as such by separate descriptors: NPtex2html_wrap_inline4084\n\t\t\tetc. However, there are many occasions where the conjuncts are not of the same formal category, or where they do not\n\t\t\tcorrespond to an entire phrasal or clausal constituent. There is much to be said, in these cases, or perhaps for all\n\t\t\tcases of coordination, for the use of a generalised label applied to all coordinate constituents or conjuncts, e.g.\n\t\t\tthe label CO used in the TOSCA system. We do not offer a definitive solution for the annotation of coordination, and\n\t\t\tthe many variants of coordination will not be considered further in this report. See Sampson (1995: 310f) for a\n\t\t\tdetailed treatment. \n\t\t\t(http://www.ilc.cnr.it/EAGLES96/segsasg1/node37.html)\n\t\t" ;
        <http://www.w3.org/2000/01/rdf-schema#subClassOf>
                <http://purl.org/olia/olia.owl#Phrase> .

<http://purl.org/olia/olia.owl#SecondPolite>
        a       <http://www.w3.org/2002/07/owl#Class> ;
        <http://www.w3.org/2000/01/rdf-schema#comment>
                "\n\t\t\tIn several European languages exist special forms of pronouns for polite or respectful reference,\n\t\t\te.g. Dutch u and Spanish usted.\n\t\t\t(http://www.ilc.cnr.it/EAGLES96/annotate/node18.html#oav1p 19.09.06)\n\t\t" ;
        <http://www.w3.org/2000/01/rdf-schema#subClassOf>
                <http://purl.org/olia/olia.owl#Second> ;
        <http://www.w3.org/2002/07/owl#versionInfo>
                "\n\t\tEAGLES PersonalPronoun attribute Politeness=\"Polite\". \n\t\tThe EAGLES attribute politeness (polite/ familiar) is limited to second-person pronouns.\n\t\t\n\t\tIn French, for example, it is possible to treat Polite simply as pragmatic values encoded \n\t\tthrough other attributes - especially person and number.\n\t\tIn languages where there are special polite pronoun forms (e.g. Dutch u and Spanish usted), \n\t\tthe additional Politeness attribute is required.\n\t\t(http://www.ilc.cnr.it/EAGLES96/annotate/node18.html#oav1p 19.09.06)\n\t\t" .

<http://purl.org/olia/olia.owl#hasWordConjunct>
        a       <http://www.w3.org/2002/07/owl#Class> ;
        <http://www.w3.org/2000/01/rdf-schema#subClassOf>
                <http://purl.org/olia/olia.owl#hasConjunct> ;
        <http://www.w3.org/2000/01/rdf-schema#subClassOf>
                [ a       <http://www.w3.org/2002/07/owl#Restriction> ;
                  <http://www.w3.org/2002/07/owl#onProperty>
                          <http://purl.org/olia/olia.owl#hasChild> ;
                  <http://www.w3.org/2002/07/owl#someValuesFrom>
                          <http://purl.org/olia/olia.owl#Token>
                ] ;
        <http://www.w3.org/2002/07/owl#versionInfo>
                "http://purl.org/olia/mte/multext-east.owl#WordCoordinatingConjunction" .

<http://purl.org/olia/olia.owl#Clause>
        a       <http://www.w3.org/2002/07/owl#Class> ;
        <http://www.w3.org/2000/01/rdf-schema#comment>
                "\n\t\t\tClause is the class of constructions that form minimal sentential units. \n\t\t\tThey must include a predicate, all arguments of the predicate, and all \n\t\t\tmodifiers of the predicate and the arguments.\n\t\t\t(http://purl.org/linguistics/gold/Clause)\n\t\t" , "\n\t\t\tTraditionally sentences are deemed to be composed of major constituents \n\t\t\tknown as clauses, which may be main clauses (not included in a superordinate \n\t\t\tclause) or embedded clauses (included in a superordinate clause) such as \n\t\t\trelative clauses or adverbial clauses. A main clause, unless it is coordinated, \n\t\t\tis equivalent to a simple sentence, and does not need to be separately labelled. \n\t\t\tEmbedded and coordinated clauses, on the other hand, will need to be separately \n\t\t\tidentified. We recommend that such units be identified in the annotation, and \n\t\t\tlabelled either as sentences (S) or as clauses (CL), according to the preference \n\t\t\tspecified in the annotation scheme.\n\n\t\t\tThe reason for allowing choice here is that different theoretical preferences \n\t\t\thave to be accommodated. In some syntactic models, the `clause' category is not \n\t\t\tused (except informally), embedded clauses being marked by included [S] \n\t\t\tconstituents. In other models, clauses are identified as such, even where they \n\t\t\tare coextensive with an independent sentence.\n\n\t\t\tOne solution which commends itself (and is employed in the Lancaster Treebank and \n\t\t\tthe SUSANNE Corpus) is to retain [S ... S] as the delimiter of sentences, whether \n\t\t\tincluded or not, and also to use [S ... S] for the coordinated parts of a compound \n\t\t\tsentence; but to use `clause' labels for subordinate clauses. An example which \n\t\t\tillustrates this division is 12:\n\n\t\t\t(12)  \t[S [S The distinction at issue is relatively clear S] , but [S closer \n\t\t\t\t\texamination reveals [CL that all is not quite so straightforward \n\t\t\t\t\t[CL as it seems CL] CL] S] . S]\n\t\t\t\t\t\n\t\t\tEmbedded (subordinate) clauses are generally identified by some sign of their \n\t\t\tdependence on the superordinate clause or sentence, such as an introductory \n\t\t\tconjunction or a non-finite verb form. It is noticeable that the coordinated \n\t\t\tparts of the compound sentence do not have to be clause-like units with subjects \n\t\t\tand verbs, and to this extent [CL] would be a misleading label to apply to them. \n\t\t\tThis is true, in 13, of so far so good in:\n\n\t\t\t(13)  \t[S [S So far so good S] , but [S now consider gender in adjectives S] . S] \n\t\t\t(http://www.ilc.cnr.it/EAGLES96/segsasg1/node31.html)\n\t\t" ;
        <http://www.w3.org/2000/01/rdf-schema#subClassOf>
                <http://purl.org/olia/olia-top.owl#Constituent> ;
        <http://www.w3.org/2002/07/owl#versionInfo>
                "\n\t\t\tEAGLES, http://purl.org/linguistics/gold/Clause\n\t\t" .

<http://purl.org/olia/olia.owl#FiniteClause>
        a       <http://www.w3.org/2002/07/owl#Class> ;
        <http://www.w3.org/2000/01/rdf-schema#subClassOf>
                <http://purl.org/olia/olia.owl#Clause> .

<http://purl.org/olia/olia.owl#Collocation>
        a       <http://www.w3.org/2002/07/owl#Class> ;
        <http://www.w3.org/2000/01/rdf-schema#comment>
                "\n\t\t\tA collocation is any habitually linked group of words - a kind of lexical partnership, e.g. 'fish and chips', 'salt and pepper', 'don't mention it', 'it's nothing...', 'Oh well!', 'bangers and mash'... and so on. Many idioms or idiomatic phrases exhibit collocation, e.g. in a jiffy.\n\t\t\t(http://www.englishbiz.co.uk/grammar/main_files/definitionsa-m.htm)\n\t\t" ;
        <http://www.w3.org/2000/01/rdf-schema#label>
                "collocation" ;
        <http://www.w3.org/2000/01/rdf-schema#subClassOf>
                <http://purl.org/olia/olia-top.owl#SemanticUnit> ;
        <http://www.w3.org/2002/07/owl#versionInfo>
                "http://purl.org/olia/mte/multext-east.owl#Collocation" .

<http://purl.org/olia/system.owl#hasTarget>
        a       <http://www.w3.org/2002/07/owl#ObjectProperty> .

<http://purl.org/olia/olia.owl#DefiniteArticle>
        a       <http://www.w3.org/2002/07/owl#Class> ;
        <http://www.w3.org/2000/01/rdf-schema#comment>
                "\n\t\t\tA definite article is used before singular and plural nouns that refer to a \n\t\t\tparticular member of a group.\n\t\t\t(http://en.wikipedia.org/wiki/Article_%28grammar%29 18.09.06)\n\t\t" ;
        <http://www.w3.org/2000/01/rdf-schema#subClassOf>
                <http://purl.org/olia/olia.owl#Article> ;
        <http://www.w3.org/2002/07/owl#versionInfo>
                "EAGLES Article with Article-Type=\"Definite\"." .

<http://purl.org/olia/olia.owl#StrongInflection>
        a       <http://www.w3.org/2002/07/owl#Class> ;
        <http://www.w3.org/2000/01/rdf-schema#comment>
                "\n\t\t\tIn German (and other Germanic languages), when gender, number and case are not expressed \n\t\t\tby a determiner, the adjective takes the endings of the strong inflection.\n\t\t\t(http://www.canoo.net/services/OnlineGrammar/Wort/Adjektiv/Deklinationstyp/Stark.html  20.11.06)\n\t\t\t\n\t\t\tStrong inflection is a characteristic of lexemes, not individual tokens.\n\t\t" ;
        <http://www.w3.org/2000/01/rdf-schema#subClassOf>
                <http://purl.org/olia/olia-top.owl#InflectionTypeFeature> ;
        <http://www.w3.org/2002/07/owl#versionInfo>
                "EAGLES" .

<http://purl.org/olia/olia.owl#ExpletivePronoun>
        a       <http://www.w3.org/2002/07/owl#Class> ;
        <http://www.w3.org/2000/01/rdf-schema#comment>
                "\n\t\t\tAn expletive (also known as a dummy word) is a part of speech whose members have no meaning, \n\t\t\tbut complete a sentence to make it grammatical [Crystal 1997, 127]\n\t\t\t(http://purl.org/linguistics/gold/Expletive)\n\n\t\t\tIn European languages, expletives are pronouns. A verbal part of speech that \n\t\t\t\"has no meaning, but complete a sentence to make it grammatical\" is a copula (see AuxiliaryVerb).\n\t\t" ;
        <http://www.w3.org/2000/01/rdf-schema#subClassOf>
                <http://purl.org/olia/olia.owl#Expletive> , <http://purl.org/olia/olia.owl#ThirdPersonPronoun> ;
        <http://www.w3.org/2002/07/owl#versionInfo>
                "TODO: compare with GOLD, modeled as a PartOfSpeechProperty there" , "\n\t\t\tMissing in the EAGLES recommendations, added in accordance with the TIGER annotation scheme (for German).\n\t\t\tAs expletive pronouns often (e.g., in German or English) have the form of 3.sg personal pronouns, \n\t\t\texpletives are modelled here as subclass of ThirdPersonPronoun.\n\t\t" , "TODO: revise definition, the GOLD definition applies to copula, too." .

<http://purl.org/olia/olia.owl#Predicate>
        a       <http://www.w3.org/2002/07/owl#Class> ;
        <http://www.w3.org/2000/01/rdf-schema#comment>
                "\n\t\t\tThe predicate is the relation between the Clause and a portion of a  clause, excluding the subject, \n\t\t\tthat expresses something about the subject (Crystal 1980: 280; Hartmann and Stork 1972: 182; Pei and\n\t\t\tGaynor 1954: 173; Pike and Pike 1982: 40; Mish et al. 1990: 926; Crystal 1985: 241-242).\n\t\t\t(http://purl.org/linguistics/gold/predicate)\n\t\t" ;
        <http://www.w3.org/2000/01/rdf-schema#subClassOf>
                <http://purl.org/olia/olia-top.owl#SyntacticRole> ;
        <http://www.w3.org/2002/07/owl#versionInfo>
                "\n\t\t\t\tNote that most predicates are also (semantic) Heads of the respective clause \n\t\t\t\t(cf. van Valin and Lapolla 1997, who, however, use the term \"nucleus\").\n\t\t\t\tA syntax-centered approach on heads may, however, assign the label Head to an\n\t\t\t\tauxiliary. As \"head\" is ambiguous between a syntactic function (finite verb) and\n\t\t\t\ta semantic function (predicate), a direct association is avoided here.\n\t\t" , "adapted from http://purl.org/linguistics/gold/predicate" .

<http://purl.org/olia/olia.owl#DigitNumeral>
        a       <http://www.w3.org/2002/07/owl#Class> ;
        <http://www.w3.org/2000/01/rdf-schema#comment>
                "Numeral expressed by Arabic digits." ;
        <http://www.w3.org/2000/01/rdf-schema#isDefinedBy>
                "http://www.isocat.org/datcat/DC-1935" ;
        <http://www.w3.org/2000/01/rdf-schema#subClassOf>
                <http://purl.org/olia/olia.owl#Numeral> , <http://purl.org/olia/olia.owl#String> .

<http://purl.org/olia/olia.owl#DelativeCase>
        a       <http://www.w3.org/2002/07/owl#Class> ;
        <http://www.w3.org/2000/01/rdf-schema#comment>
                "\n\t\t\tDelativeCase expresses motion downward from the referent of the \n\t\t\tnoun it marks (Pei and Gaynor 1954: 53; Gove, et al. 1966: 595).\n\t\t\t(http://purl.org/linguistics/gold/Delative)\n\t\t" ;
        <http://www.w3.org/2000/01/rdf-schema#subClassOf>
                <http://purl.org/olia/olia-top.owl#CaseFeature> ;
        <http://www.w3.org/2002/07/owl#versionInfo>
                "http://purl.org/linguistics/gold/Delative, http://www.isocat.org/datcat/DC-1268" .

<http://purl.org/olia/olia.owl#SecondaryPunctuation>
        a       <http://www.w3.org/2002/07/owl#Class> ;
        <http://www.w3.org/2000/01/rdf-schema#comment>
                "\n                            Punctuation that is not very important with regards to sentence splitting in a text.\n                                (http://www.isocat.org/datcat/DC-2076)\n                            " ;
        <http://www.w3.org/2000/01/rdf-schema#label>
                "secondary punctuation" ;
        <http://www.w3.org/2000/01/rdf-schema#subClassOf>
                <http://purl.org/olia/olia.owl#Punctuation> ;
        <http://www.w3.org/2002/07/owl#versionInfo>
                "subClassOf punctuation (dcif:isA)" , "http://www.isocat.org/datcat/DC-2076" .

<http://purl.org/olia/olia.owl#AttributiveAdjective>
        a       <http://www.w3.org/2002/07/owl#Class> ;
        <http://www.w3.org/2000/01/rdf-schema#comment>
                "\n\t\t\tAn attributive adjective is an adjective that qualifies or \n\t\t\tmodifies a noun and that precedes the noun, e.g.\"a delicious \n\t\t\tapple\", \"a short letter\".\n\t\t\t(http://en.wikipedia.org/wiki/Adjective 18.09.06)\n\t\t" ;
        <http://www.w3.org/2000/01/rdf-schema#subClassOf>
                <http://purl.org/olia/olia.owl#Adjective> ;
        <http://www.w3.org/2002/07/owl#versionInfo>
                "\n\t\t\tEAGLES Adjective with Use=\"Attributive\".\n\t\t" .

<http://purl.org/olia/olia.owl#Elision>
        a       <http://www.w3.org/2002/07/owl#Class> ;
        <http://www.w3.org/2000/01/rdf-schema#comment>
                "\n\t\t\tThe omission of a syllable or vowel at the beginning or end of a word, esp. when a word ending with a vowel is next to one beginning with a vowel.\n\t\t\t(www.wordreference.com/English/definition.asp?en=elision; http://www.isocat.org/datcat/DC-1277)\n\t\t" ;
        <http://www.w3.org/2000/01/rdf-schema#label>
                "elision" ;
        <http://www.w3.org/2000/01/rdf-schema#subClassOf>
                <http://purl.org/olia/olia-top.owl#PhonologicalProcess> ;
        <http://www.w3.org/2002/07/owl#versionInfo>
                "http://www.isocat.org/datcat/DC-1277" .

<http://purl.org/olia/olia.owl#GenitiveCase>
        a       <http://www.w3.org/2002/07/owl#Class> ;
        <http://www.w3.org/2000/01/rdf-schema#comment>
                "\n\t\t\tGenitive case signals that the referent of the marked noun is the possessor \n\t\t\tof the referent of another noun, e.g. \"the man's foot\".  In some languages, \n\t\t\tgenitive case may express an associative relation between the marked noun \n\t\t\tand another noun. \n\t\t\t(http://www.sil.org/linguistics/glossaryoflinguisticterms/WhatIsGenitiveCase.htm 17.11.06)\n\t\t" ;
        <http://www.w3.org/2000/01/rdf-schema#subClassOf>
                <http://purl.org/olia/olia-top.owl#CaseFeature> ;
        <http://www.w3.org/2002/07/owl#versionInfo>
                "EAGLES-recommended case feature" .

<http://purl.org/olia/olia.owl#hasConjunct>
        a       <http://www.w3.org/2002/07/owl#Class> ;
        <http://www.w3.org/2000/01/rdf-schema#subClassOf>
                <http://purl.org/olia/olia-top.owl#SyntacticRelation> ;
        <http://www.w3.org/2000/01/rdf-schema#subClassOf>
                [ a       <http://www.w3.org/2002/07/owl#Restriction> ;
                  <http://www.w3.org/2002/07/owl#onProperty>
                          <http://purl.org/olia/olia.owl#hasParent> ;
                  <http://www.w3.org/2002/07/owl#someValuesFrom>
                          <http://purl.org/olia/olia.owl#CoordinatingConjunction>
                ] ;
        <http://www.w3.org/2002/07/owl#versionInfo>
                "http://purl.org/olia/mte/multext-east.owl#CoordinatingConjunction_ConjunctType" .

<http://purl.org/olia/olia.owl#hasOwnerGender>
        a       <http://www.w3.org/2002/07/owl#ObjectProperty> ;
        <http://www.w3.org/2000/01/rdf-schema#comment>
                "\n                            Indication concerning the gender of the person that ownes something.\n                                (http://www.isocat.org/datcat/DC-1416)\n                            " ;
        <http://www.w3.org/2000/01/rdf-schema#label>
                "owner gender" ;
        <http://www.w3.org/2000/01/rdf-schema#range>
                <http://purl.org/olia/olia-top.owl#GenderFeature> ;
        <http://www.w3.org/2000/01/rdf-schema#subPropertyOf>
                <http://purl.org/olia/system.owl#hasFeature> ;
        <http://www.w3.org/2002/07/owl#versionInfo>
                "http://www.isocat.org/datcat/DC-1416" .

<http://purl.org/olia/olia.owl#ParticipleAdjective>
        a       <http://www.w3.org/2002/07/owl#Class> ;
        <http://www.w3.org/2000/01/rdf-schema#comment>
                "\n                            Adjective based on a verb.\n                                (http://www.isocat.org/datcat/DC-1598)\n                            " ;
        <http://www.w3.org/2000/01/rdf-schema#label>
                "participle adjective" ;
        <http://www.w3.org/2000/01/rdf-schema#subClassOf>
                <http://purl.org/olia/olia.owl#Adjective> , <http://purl.org/olia/olia.owl#Participle> ;
        <http://www.w3.org/2002/07/owl#versionInfo>
                "http://www.isocat.org/datcat/DC-1598" , "subClassOf adjective (dcif:isA)" .

<http://purl.org/olia/olia.owl#SlangRegister>
        a       <http://www.w3.org/2002/07/owl#Class> ;
        <http://www.w3.org/2000/01/rdf-schema#comment>
                "\n                            An extremely informal register of a word, term, or text that is used in spoken and everyday language and less commonly in documents.\n                                (ISO12620; http://www.isocat.org/datcat/DC-1995)\n                            " ;
        <http://www.w3.org/2000/01/rdf-schema#label>
                "slang register" ;
        <http://www.w3.org/2000/01/rdf-schema#subClassOf>
                <http://purl.org/olia/olia-top.owl#RegisterFeature> ;
        <http://www.w3.org/2002/07/owl#versionInfo>
                "subClassOf register (dcif:conceptualDomain)" , "http://www.isocat.org/datcat/DC-1995" .

<http://purl.org/olia/olia.owl#InterminativeCase>
        a       <http://www.w3.org/2002/07/owl#Class> ;
        <http://www.w3.org/2000/01/rdf-schema#comment>
                "\n\t\t\t'into in(side of)'.\n\t\t\t(http://purl.org/linguistics/gold/Interminative)\n\t\t" ;
        <http://www.w3.org/2000/01/rdf-schema#subClassOf>
                <http://purl.org/olia/olia-top.owl#CaseFeature> ;
        <http://www.w3.org/2002/07/owl#versionInfo>
                "http://purl.org/linguistics/gold/Interminative" .

<http://purl.org/olia/olia.owl#WithInfinite>
        a       <http://www.w3.org/2002/07/owl#Class> ;
        <http://www.w3.org/2000/01/rdf-schema#comment>
                "\n\t\t\tFor example, in German the subordinating conjunction \"ohne\" (\"zu\"...) \n\t\t\tis followed by an infinitive. \n\t\t\t(http://www.ilc.cnr.it/EAGLES96/annotate/node19.html#oav2u  17.11.06)\n\t\t" ;
        <http://www.w3.org/2000/01/rdf-schema#subClassOf>
                <http://purl.org/olia/olia-top.owl#SubordTypeFeature> ;
        <http://www.w3.org/2002/07/owl#deprecated>
                true ;
        <http://www.w3.org/2002/07/owl#versionInfo>
                "EAGLES, reimplemented within SubordinatingConjunction taxonomy" .

<http://purl.org/olia/olia.owl#ConditionRole>
        a       <http://www.w3.org/2002/07/owl#Class> ;
        <http://www.w3.org/2000/01/rdf-schema#comment>
                "Adverbial that denotes a condition. (Petrova and Odebrecht 2011)" ;
        <http://www.w3.org/2000/01/rdf-schema#subClassOf>
                <http://purl.org/olia/olia-top.owl#SemanticRole> ;
        <http://www.w3.org/2002/07/owl#versionInfo>
                "http://purl.org/olia/tcodex.owl#ConditionalAdverb" .

<http://purl.org/olia/olia.owl#Clitic>
        a       <http://www.w3.org/2002/07/owl#Class> ;
        <http://www.w3.org/2000/01/rdf-schema#comment>
                "Categorization of the different types of clitics\n\t  (MultText-East; http://www.isocat.org/datcat/DC-1903)\n      " ;
        <http://www.w3.org/2000/01/rdf-schema#label>
                "cliticness" ;
        <http://www.w3.org/2000/01/rdf-schema#subClassOf>
                <http://purl.org/olia/olia.owl#Morpheme> ;
        <http://www.w3.org/2002/07/owl#deprecated>
                true ;
        <http://www.w3.org/2002/07/owl#equivalentClass>
                <http://purl.org/olia/olia.owl#CliticElement> ;
        <http://www.w3.org/2002/07/owl#versionInfo>
                "http://www.isocat.org/datcat/DC-1903 (cliticness), http://purl.org/olia/mte/multext-east.owl#Cliticness" , "Deprecated: Note that the original MULTEXT-East definition of cliticness conflates four different aspects under this label: (a) whether an element *is* a clitic, (b) whether an element *contains* a clitic, (c) whether an element *should contain* a clitic that is, however, represented as a separate token, and (d) whether an element is part of a collocation.\n\t  In the MULTEXT-East ontology (and here), this is made explicit by CliticElement, NoncliticElement, ElementWithClitic, ElementWithoutClitic and Collocation. Instead of the original \"Clitic\", CliticElement (state of being a clitic) and Cliticization (process of adding a clitic) are to be used" .

<http://purl.org/olia/olia.owl#InterrogativeQuantifier>
        a       <http://www.w3.org/2002/07/owl#Class> ;
        <http://www.w3.org/2000/01/rdf-schema#comment>
                "In the Czech and Slovak MTE v4 pecs, Numeral/Class=\"interrogative\" are items meaning `how many/much', etc. Strictly speaking, they are pronumerals (pro-quantifiers), but traditional descriptions don't recognise such a category, so they are described variously as pronouns or as numerals (because their syntactic distribution is that of numerals, or very close).\" (Ivan A Derzhanski, email 2010/06/11, http://purl.org/olia/mte/multext-east.owl#InterrogativeQuantifier)" ;
        <http://www.w3.org/2000/01/rdf-schema#subClassOf>
                <http://purl.org/olia/olia.owl#ProQuantifier> ;
        <http://www.w3.org/2002/07/owl#equivalentClass>
                [ a       <http://www.w3.org/2002/07/owl#Class> ;
                  <http://www.w3.org/2002/07/owl#intersectionOf>
                          ( <http://purl.org/olia/olia.owl#ProQuantifier> <http://purl.org/olia/olia.owl#QuestionWord> )
                ] ;
        <http://www.w3.org/2002/07/owl#versionInfo>
                "http://purl.org/olia/mte/multext-east.owl#InterrogativeQuantifier" .

<http://purl.org/olia/olia.owl#PluralQuantifier>
        a       <http://www.w3.org/2002/07/owl#Class> ;
        <http://www.w3.org/2000/01/rdf-schema#comment>
                "A PluralQuantifier is a Quantifier (or Numeral) that specifies a large multitude of entities. The agreement pattern of a plural quantifier is different from that or an singular quantifier, but as opposed to DualQuantifier and PaucalQuantifier, PluralQuantifier includes quantifiers that denote arbitrarily large sets of entities. (Chiarcos)\n\t\t\tThe corresponding category in Czech, Polish and Slovak MTE v4 specs is Numeral/Class=\"definite\", that refers to numerals larger than four. (MTE v4)\n\t\t" ;
        <http://www.w3.org/2000/01/rdf-schema#subClassOf>
                <http://purl.org/olia/olia-top.owl#NumeralAgreementClass> ;
        <http://www.w3.org/2002/07/owl#equivalentClass>
                [ a       <http://www.w3.org/2002/07/owl#Class> ;
                  <http://www.w3.org/2002/07/owl#intersectionOf>
                          ( <http://purl.org/olia/olia.owl#Quantifier>
                            [ a       <http://www.w3.org/2002/07/owl#Restriction> ;
                              <http://www.w3.org/2002/07/owl#onProperty>
                                      <http://purl.org/olia/olia.owl#hasNumeralAgreementClass> ;
                              <http://www.w3.org/2002/07/owl#someValuesFrom>
                                      <http://purl.org/olia/olia.owl#PluralQuantifier>
                            ]
                          )
                ] ;
        <http://www.w3.org/2002/07/owl#versionInfo>
                "http://purl.org/olia/mte/multext-east.owl#PluralQuantifier\t\t\t\n\t\t\tNumeral/Class=\"definite\", Numeral/Class=\"definite1\", Numeral/Class=\"definite234\" etc. refer to specific patterns of congruency with Slavic numerals that originate from the difference between Old Slavic singular (definite1), dual (definite2, definite234) and plural (definite)." .

<http://purl.org/olia/olia.owl#Postposition>
        a       <http://www.w3.org/2002/07/owl#Class> ;
        <http://www.w3.org/2000/01/rdf-schema#comment>
                "\n      A postposition is an adposition that occurs after its complement.\n      (http://www.sil.org/linguistics/GlossaryOfLinguisticTerms/WhatIsAPostposition.htm 19.09.06)" ;
        <http://www.w3.org/2000/01/rdf-schema#subClassOf>
                <http://purl.org/olia/olia.owl#Adposition> ;
        <http://www.w3.org/2002/07/owl#versionInfo>
                "EAGLES adposition with the optional attribute Type=\"Preposition\"." .

<http://purl.org/olia/olia.owl#SuperablativeCase>
        a       <http://www.w3.org/2002/07/owl#Class> ;
        <http://www.w3.org/2000/01/rdf-schema#comment>
                "\n\t\t\tSuperablative expresses that  the referent of the noun it marks is \n\t\t\tthe location from over which another referent is moving. It has the \n\t\t\tmeaning 'from over'.\n\t\t\t(http://purl.org/linguistics/gold/Superablative)\n\t\t" ;
        <http://www.w3.org/2000/01/rdf-schema#subClassOf>
                <http://purl.org/olia/olia-top.owl#CaseFeature> ;
        <http://www.w3.org/2002/07/owl#versionInfo>
                "http://purl.org/linguistics/gold/Superablative" .

<http://purl.org/olia/olia.owl#hasRegister>
        a       <http://www.w3.org/2002/07/owl#ObjectProperty> ;
        <http://www.w3.org/2000/01/rdf-schema#comment>
                "\n                            Classification indicating the relative level of language individually assigned to a lexeme or term or to a text type.\n                                (ISO12620; http://www.isocat.org/datcat/DC-1988)\n                            " ;
        <http://www.w3.org/2000/01/rdf-schema#range>
                <http://purl.org/olia/olia-top.owl#RegisterFeature> ;
        <http://www.w3.org/2000/01/rdf-schema#subPropertyOf>
                <http://purl.org/olia/system.owl#hasFeature> ;
        <http://www.w3.org/2002/07/owl#versionInfo>
                "http://www.isocat.org/datcat/DC-1988" .

<http://purl.org/olia/olia.owl#hasUsage>
        a       <http://www.w3.org/2002/07/owl#ObjectProperty> ;
        <http://www.w3.org/2000/01/rdf-schema#comment>
                "\n                            The relative commonness with which a term occurs.\n                                (ISO12620; http://www.isocat.org/datcat/DC-1965)\n                            " ;
        <http://www.w3.org/2000/01/rdf-schema#range>
                <http://purl.org/olia/olia-top.owl#UsageAndFrequencyFeature> ;
        <http://www.w3.org/2000/01/rdf-schema#subPropertyOf>
                <http://purl.org/olia/system.owl#hasFeature> ;
        <http://www.w3.org/2002/07/owl#versionInfo>
                "http://www.isocat.org/datcat/DC-1965" .

<http://purl.org/olia/olia.owl#Adverb>
        a       <http://www.w3.org/2002/07/owl#Class> ;
        <http://www.w3.org/2000/01/rdf-schema#comment>
                "\n\t\tAn adverb is a part of speech that serves to modify non-nominal parts of speech, \n\t\ti.e., verbs, adjectives (including numbers), clauses, sentences and other adverbs. \n\t\tModifiers of nouns are primarily determiners and adjectives. \n\t\t(http://en.wikipedia.org/wiki/Adverbs 18.09.06)\n\t" ;
        <http://www.w3.org/2000/01/rdf-schema#label>
                "adverb"@en , "adverbe"@fr ;
        <http://www.w3.org/2000/01/rdf-schema#subClassOf>
                <http://purl.org/olia/olia-top.owl#MorphosyntacticCategory> ;
        <http://www.w3.org/2002/07/owl#versionInfo>
                "DCR general adverb (http://www.isocat.org/datcat/DC-1435) ignored" , "EAGLES top-level category Adverb (AV).\n\t\tSkipped subconcepts ParticleAdverb and GeneralAdverb:\n\t\t\tParticleAdverb is better described by the join of particles or adverbs rather than positing an independent category;\n\t\t\tGeneralAdverb is merely the complement of DegreeAdverb.\n\t" , "TODO: currently, different criteria are employed to characterize Adverbs, including lexical criteria (e.g., AdjectivalAdverb) and semantic criteria (e.g., CausalAdverb). The subclassification according to semantic criteria is to be expressed with hasSemanticRole, the classes are thus deprecated." .

<http://purl.org/olia/olia.owl#VerbalHead>
        a       <http://www.w3.org/2002/07/owl#Class> ;
        <http://www.w3.org/2000/01/rdf-schema#comment>
                "\n\t\t\tA Verb (V) at the syntax layer is either a lexical (VLEX) or a copula verb (VCOP) at the POS layer. \n\t\t\tModal verbs and auxiliaries are not annotated in the constituent structure. The verb and its arguments \n\t\t\tare placed at the same CSn layer. Raising and control verbs are treated like ordinary verbs. \n\t\t\tThey subcategorize for a sentential complement.\n\t\t\t(Dipper et al 2007, §3.3.3)\n\t\t" ;
        <http://www.w3.org/2000/01/rdf-schema#subClassOf>
                <http://purl.org/olia/olia.owl#Head> ;
        <http://www.w3.org/2002/07/owl#equivalentClass>
                <http://purl.org/olia/olia.owl#VerbalHead> ;
        <http://www.w3.org/2002/07/owl#versionInfo>
                "added in conformance with the SFB632 Annotation Guidelines (Dipper et al. 2007)" .

<http://purl.org/olia/olia.owl#hasSyntacticFunction>
        a       <http://www.w3.org/2002/07/owl#ObjectProperty> ;
        <http://www.w3.org/2000/01/rdf-schema#comment>
                "\n\t\t\tRelation to be used when the syntactic function of a constituent is different from its morphosyntactic type, \n\t\t\tcf. FormFunctionDiscrepancy in the PTB bracketing guidelines, Bies et al. (1995, §2.2.1)\n\t\t" ;
        <http://www.w3.org/2000/01/rdf-schema#range>
                <http://purl.org/olia/olia-top.owl#SyntacticFunction> ;
        <http://www.w3.org/2000/01/rdf-schema#subPropertyOf>
                <http://purl.org/olia/system.owl#hasFeature> ;
        <http://www.w3.org/2002/07/owl#versionInfo>
                "TODO: apply this to primitive concepts, too" , "Bies et al. 1995" .

<http://purl.org/olia/olia.owl#ExistentialPronoun>
        a       <http://www.w3.org/2002/07/owl#Class> ;
        <http://www.w3.org/2000/01/rdf-schema#comment>
                "pronoun that indicates the existence of something or someone" ;
        <http://www.w3.org/2000/01/rdf-schema#isDefinedBy>
                "http://www.isocat.org/datcat/DC-3012" ;
        <http://www.w3.org/2002/07/owl#deprecated>
                true ;
        <http://www.w3.org/2002/07/owl#equivalentClass>
                [ a       <http://www.w3.org/2002/07/owl#Class> ;
                  <http://www.w3.org/2002/07/owl#intersectionOf>
                          ( <http://purl.org/olia/olia.owl#ExistentialParticle> <http://purl.org/olia/olia.owl#Pronoun> )
                ] ;
        <http://www.w3.org/2002/07/owl#versionInfo>
                "merely a shorthand for ExistentialParticle and Pronoun, hence deprecated" .

<http://purl.org/olia/olia.owl#DeclarativeModality>
        a       <http://www.w3.org/2002/07/owl#Class> ;
        <http://www.w3.org/2000/01/rdf-schema#comment>
                "\n\t\t\tPertaining to the mood or mode of a verb form or clause such that it \n\t\t\tpredicates a type of (formal) assertion (OED).\n\t\t\t(http://languagelink.let.uu.nl/tds/onto/LinguisticOntology.owl#declarativeModality)\n\t\t" ;
        <http://www.w3.org/2000/01/rdf-schema#subClassOf>
                <http://purl.org/olia/olia-top.owl#ModalityFeature> ;
        <http://www.w3.org/2002/07/owl#versionInfo>
                "generalization over DeclarativeMood" .

<http://purl.org/olia/olia.owl#LativeCase>
        a       <http://www.w3.org/2002/07/owl#Class> ;
        <http://www.w3.org/2000/01/rdf-schema#comment>
                "\n\t\t\tLativeCase expresses 'motion up to the location of,' or 'as far as' \n\t\t\tthe referent of the noun it marks (Pei and Gaynor 1954: 121; Gove, \n\t\t\tet al. 1966: 1277).\n\t\t\t(http://purl.org/linguistics/gold/Lative)\n\t\t" ;
        <http://www.w3.org/2000/01/rdf-schema#subClassOf>
                <http://purl.org/olia/olia-top.owl#CaseFeature> ;
        <http://www.w3.org/2002/07/owl#versionInfo>
                "http://purl.org/linguistics/gold/Lative; http://www.isocat.org/datcat/DC-1323" .

<http://purl.org/olia/olia.owl#DubitiveMood>
        a       <http://www.w3.org/2002/07/owl#Class> ;
        <http://www.w3.org/2000/01/rdf-schema#comment>
                "\n\t\t\tDubitiveMood indicates a speaker's doubt or uncertainty about a proposition (Palmer 2001).\n\t\t\t(http://purl.org/linguistics/gold/Dubitive)\n\t\t" ;
        <http://www.w3.org/2000/01/rdf-schema#subClassOf>
                <http://purl.org/olia/olia-top.owl#MoodFeature> , <http://purl.org/olia/olia.owl#DubitiveModality> ;
        <http://www.w3.org/2002/07/owl#versionInfo>
                "http://purl.org/linguistics/gold/Dubitive" .

<http://purl.org/olia/olia.owl#Izafat>
        a       <http://www.w3.org/2002/07/owl#Class> ;
        <http://www.w3.org/2000/01/rdf-schema#comment>
                "The izāfat (pronounced as a shorter form of –ē–) is an enclitic of Persian origin which \n\t\t\tis used in Farsi and neighboring languages.\n\t\t\tIn Urdu, it can be considered a preposition under certain circumstances: it links\n\t\t\ttwo nouns in a possessive relationship, although the phrase thus produced may often\n\t\t\thave a different meaning to a phrase produced with the native Urdu postposition kā.\n\t\t\tHowever, the izāfat may also join a noun to an adjective, in which case it is not so\n\t\t\tclearly accurate to describe it as a preposition parallel to the prepositions in European\n\t\t\tlanguages for which the EAGLES guidelines were compiled. A better way to treat\n\t\t\tizāfat is in the context of the Unique category of miscellaneous one-member wordclasses,\n\t\t\tdiscussed below.\n\t\t\t(Hardie 2003, http://purl.org/olia/emille.owl#Izafat)\n\t\t\t\n\t\t\tenclitic morpheme used to form noun phrases and that can denote possession, can form apposition or can join adjectives to nouns. (http://www.isocat.org/datcat/DC-2999)\n\t\t" ;
        <http://www.w3.org/2000/01/rdf-schema#isDefinedBy>
                "http://www.isocat.org/datcat/DC-2999" ;
        <http://www.w3.org/2000/01/rdf-schema#label>
                "izafat" , "ezafe" ;
        <http://www.w3.org/2000/01/rdf-schema#subClassOf>
                <http://purl.org/olia/olia.owl#Unique> ;
        <http://www.w3.org/2002/07/owl#versionInfo>
                "from the EMILLE tagset for Urdu, http://purl.org/olia/emille.owl#Izafat, cf. http://purl.org/olia/mte/multext-east.owl#GenitiveCase for the modelling of the Izafat in the Farsi MULTEXT-East." .

<http://purl.org/olia/olia.owl#Imperfect>
        a       <http://www.w3.org/2002/07/owl#Class> ;
        <http://www.w3.org/2000/01/rdf-schema#comment>
                "\n                            Verb tense that refers to action in the past that is incomplete or ongoing.\n                                (www.southwestern.edu/~carlg/Latin_Web/glossary.html; http://www.isocat.org/datcat/DC-1304)\n                            " ;
        <http://www.w3.org/2000/01/rdf-schema#label>
                "imperfect" ;
        <http://www.w3.org/2000/01/rdf-schema#subClassOf>
                <http://purl.org/olia/olia.owl#StillPresent> ;
        <http://www.w3.org/2002/07/owl#versionInfo>
                "http://www.isocat.org/datcat/DC-1304" , "subClassOf grammaticalTense (dcif:conceptualDomain)" .

<http://purl.org/olia/olia.owl#ReducedRelativeClause>
        a       <http://www.w3.org/2002/07/owl#Class> ;
        <http://www.w3.org/2000/01/rdf-schema#comment>
                "RRC (reduced relative clause)\nReduced relative clauses are adjoined to the NP they modify. \n(Bies et al. 1995)\n\nWe will use the term \\reduced relative clause\" to refer to participial or adjectival constituents of the\ntype illustrated in (@26).\n\n(26) He bought two watches designed by Paloma Picasso.\n\nReduced relative clauses should be bracketed as adjunction structures. The structure of ( 26) is thus as in\n(@27). Note that the reduced relative clause, which is headed by a participle, is bracketed as a VP.\n\n(27)\n(S (NP He)\n(VP bought\n(NP (NP two watches)\n(VP designed\n(PP by\n(PNP (PNP Paloma)\n(PNP Picasso))))))\n.)\n(Santorini 1991)" ;
        <http://www.w3.org/2000/01/rdf-schema#subClassOf>
                <http://purl.org/olia/olia.owl#SubordinateClause> ;
        <http://www.w3.org/2002/07/owl#versionInfo>
                "Santorini 1991" .

<http://purl.org/olia/olia.owl#PermissiveModality>
        a       <http://www.w3.org/2002/07/owl#Class> ;
        <http://www.w3.org/2000/01/rdf-schema#comment>
                "PermissiveModality indicates that an agent has\n                        permission to perform the action expressed by the predicate [Palmer 2001:\n                        10, 71]." ;
        <http://www.w3.org/2000/01/rdf-schema#isDefinedBy>
                "http://www.isocat.org/datcat/DC-3384" ;
        <http://www.w3.org/2000/01/rdf-schema#subClassOf>
                <http://purl.org/olia/olia-top.owl#ModalityFeature> .

<http://purl.org/olia/olia.owl#ShortDefiniteArticle>
        a       <http://www.w3.org/2002/07/owl#Class> ;
        <http://www.w3.org/2000/01/rdf-schema#comment>
                "\n                            For definiteness, when a specific form is not the syntactic subject of the clause.\n                                (http://www.isocat.org/datcat/DC-1927)\n                            " ;
        <http://www.w3.org/2000/01/rdf-schema#label>
                "short article" ;
        <http://www.w3.org/2000/01/rdf-schema#subClassOf>
                <http://purl.org/olia/olia.owl#DefiniteArticle> ;
        <http://www.w3.org/2002/07/owl#versionInfo>
                "DCR: subClassOf definiteness (dcif:conceptualDomain)" , "http://www.isocat.org/datcat/DC-1927 (short article)" .

<http://purl.org/olia/olia.owl#hasSubordType>
        a       <http://www.w3.org/2002/07/owl#ObjectProperty> ;
        <http://www.w3.org/2000/01/rdf-schema#domain>
                <http://purl.org/olia/olia.owl#SubordinatingConjunction> ;
        <http://www.w3.org/2000/01/rdf-schema#subPropertyOf>
                <http://purl.org/olia/system.owl#hasFeature> ;
        <http://www.w3.org/2002/07/owl#deprecated>
                true ;
        <http://www.w3.org/2002/07/owl#versionInfo>
                "remodelled within the hierarchy" .

<http://purl.org/olia/olia.owl#NonreducedInflection>
        a       <http://www.w3.org/2002/07/owl#Class> ;
        <http://www.w3.org/2000/01/rdf-schema#comment>
                "Nonreduced adjective inflection of Slavic languages, e.g., Czech nejubožejšími/ubohý, nejvyspělejších/vyspělý, nejvyšších/vysoký, nejvznešenějšímu/vznešený, nejvážnějšímu/vážný, nejvýznamnějších/významný, nejvýznamnějšími/významný, nejvýznamnějšímu/významný, největšími/velký (http://purl.org/olia/mte/multext-east.owl#CompoundAdjective)" ;
        <http://www.w3.org/2000/01/rdf-schema#subClassOf>
                <http://purl.org/olia/olia-top.owl#StrengthFeature> ;
        <http://www.w3.org/2002/07/owl#versionInfo>
                "http://purl.org/olia/mte/multext-east.owl#CompoundAdjective" .

<http://purl.org/olia/olia.owl#InvertedComma>
        a       <http://www.w3.org/2002/07/owl#Class> ;
        <http://www.w3.org/2000/01/rdf-schema#comment>
                "\n                            Inverted comma.\n                                (http://www.isocat.org/datcat/DC-1443)\n                            " ;
        <http://www.w3.org/2000/01/rdf-schema#label>
                "inverted comma" ;
        <http://www.w3.org/2000/01/rdf-schema#subClassOf>
                <http://purl.org/olia/olia.owl#LeftParentheticalPunctuation> ;
        <http://www.w3.org/2002/07/owl#versionInfo>
                "http://www.isocat.org/datcat/DC-1443, used as left-parenthetical punctuation in German single quotes" , "subClassOf partOfSpeech (dcif:conceptualDomain)" .

<http://purl.org/olia/olia.owl#TimeNoun>
        a       <http://www.w3.org/2002/07/owl#Class> ;
        <http://www.w3.org/2000/01/rdf-schema#comment>
                "noun expressing time" ;
        <http://www.w3.org/2000/01/rdf-schema#isDefinedBy>
                "http://www.isocat.org/datcat/DC-3855" ;
        <http://www.w3.org/2002/07/owl#deprecated>
                true ;
        <http://www.w3.org/2002/07/owl#equivalentClass>
                [ a       <http://www.w3.org/2002/07/owl#Class> ;
                  <http://www.w3.org/2002/07/owl#intersectionOf>
                          ( <http://purl.org/olia/olia.owl#Noun>
                            [ a       <http://www.w3.org/2002/07/owl#Restriction> ;
                              <http://www.w3.org/2002/07/owl#onProperty>
                                      <http://purl.org/olia/olia.owl#hasSemanticRole> ;
                              <http://www.w3.org/2002/07/owl#someValuesFrom>
                                      <http://purl.org/olia/olia.owl#TimeRole>
                            ]
                          )
                ] ;
        <http://www.w3.org/2002/07/owl#versionInfo>
                "deprecated, as merely a shorthand for Noun and hasSemanticRole some TimeRole" .

<http://purl.org/olia/olia.owl#Noun>
        a       <http://www.w3.org/2002/07/owl#Class> ;
        <http://www.w3.org/2000/01/rdf-schema#comment>
                "\n\tA noun, or noun substantive, is a part of speech (a word or phrase) which can co-occur with \n\t(in)definite articles and attributive adjectives, and function as the head of a noun phrase.\n\n\tThe word \"noun\" derives from the Latin 'nomen' meaning \"name\", and a traditional definition \n\tof nouns is that they are all and only those expressions that refer to a person, place, \n\tthing, event, substance, quality, idea or an appointment. They serve as the subject or object \n\tof a verb, and the object of a preposition.\n\t(http://en.wikipedia.org/wiki/Noun 19.09.06)\n\t" ;
        <http://www.w3.org/2000/01/rdf-schema#label>
                "nom"@fr , "noun"@en ;
        <http://www.w3.org/2000/01/rdf-schema#subClassOf>
                <http://purl.org/olia/olia-top.owl#MorphosyntacticCategory> ;
        <http://www.w3.org/2002/07/owl#versionInfo>
                "EAGLES top-level category \"Noun\"." .

<http://purl.org/olia/olia.owl#ProQuantifier>
        a       <http://www.w3.org/2002/07/owl#Class> ;
        <http://www.w3.org/2000/01/rdf-schema#comment>
                "A ProQuantifier is a quantifier derived from a pronominal element. ProQuantifiers thus partly characterized as pronouns (e.g., as pronominal adverbs) or quantifiers (e.g., \"indefinite numeral\" as in MTE v.4). (http://purl.org/olia/mte/multext-east.owl#ProQuantifier)" ;
        <http://www.w3.org/2000/01/rdf-schema#subClassOf>
                <http://purl.org/olia/olia.owl#Pronoun> , <http://purl.org/olia/olia.owl#Quantifier> ;
        <http://www.w3.org/2002/07/owl#versionInfo>
                "http://purl.org/olia/mte/multext-east.owl#ProQuantifier" .

<http://purl.org/olia/olia.owl#CoordinationParticle>
        a       <http://www.w3.org/2002/07/owl#Class> ;
        <http://www.w3.org/2000/01/rdf-schema#comment>
                "\n                            particle for coordination\n                                (MIRACL & LSCA; http://www.isocat.org/datcat/DC-2227)\n                            " ;
        <http://www.w3.org/2000/01/rdf-schema#label>
                "coordination particle" ;
        <http://www.w3.org/2000/01/rdf-schema#subClassOf>
                <http://purl.org/olia/olia.owl#CoordinatingConjunction> , <http://purl.org/olia/olia.owl#Particle> ;
        <http://www.w3.org/2002/07/owl#versionInfo>
                "http://www.isocat.org/datcat/DC-2227" , "subClassOf particle (dcif:isA)" .

<http://purl.org/olia/olia.owl#hasValency>
        a       <http://www.w3.org/2002/07/owl#ObjectProperty> ;
        <http://www.w3.org/2000/01/rdf-schema#range>
                <http://purl.org/olia/olia-top.owl#ValencyFeature> ;
        <http://www.w3.org/2000/01/rdf-schema#subPropertyOf>
                <http://purl.org/olia/system.owl#hasFeature> .

<http://purl.org/olia/olia.owl#InfrequentlyUsed>
        a       <http://www.w3.org/2002/07/owl#Class> ;
        <http://www.w3.org/2000/01/rdf-schema#comment>
                "\n                            Said of a term that does not appear frequently.\n                                (ISO12620; http://www.isocat.org/datcat/DC-1985)\n                            " ;
        <http://www.w3.org/2000/01/rdf-schema#label>
                "infrequently used" ;
        <http://www.w3.org/2000/01/rdf-schema#subClassOf>
                <http://purl.org/olia/olia.owl#Possible> ;
        <http://www.w3.org/2002/07/owl#versionInfo>
                "subClassOf frequency (dcif:conceptualDomain)" , "http://www.isocat.org/datcat/DC-1985" .

<http://purl.org/olia/olia.owl#SubjunctiveMood>
        a       <http://www.w3.org/2002/07/owl#Class> ;
        <http://www.w3.org/2000/01/rdf-schema#comment>
                "\n\t\t\tThe subjunctive is the mood that is minimally marked as opposed to \n\t\t\tthe indicative and that marks a clause as not directly representing \n\t\t\tan assertion of the speaker. \n\t\t\t(http://www.uni-erfurt.de/sprachwissenschaft/proxy.php?port=8080&file=lido/servlet/Lido_Servlet Subjunktiv 18.06.07)\n\t\t" ;
        <http://www.w3.org/2000/01/rdf-schema#subClassOf>
                <http://purl.org/olia/olia-top.owl#MoodFeature> , <http://purl.org/olia/olia.owl#SubjunctiveModality> ;
        <http://www.w3.org/2002/07/owl#versionInfo>
                "\n\t\t\thttp://purl.org/linguistics/gold/Subjunctive,\n\t\t\thttp://languagelink.let.uu.nl/tds/onto/LinguisticOntology.owl#subjunctiveModality\n\t\t" .

<http://purl.org/olia/olia.owl#PatientRole>
        a       <http://www.w3.org/2002/07/owl#Class> ;
        <http://www.w3.org/2000/01/rdf-schema#comment>
                "\n\t\t\tA patient instantiates the role of an entity which undergoes a change of \n\t\t\tstate (Cruse 2000:284)\n\t\t\thttp://languagelink.let.uu.nl/tds/onto/LinguisticOntology.owl#patientRole\n\t\t" ;
        <http://www.w3.org/2000/01/rdf-schema#subClassOf>
                <http://purl.org/olia/olia.owl#UndergoerMacroRole> ;
        <http://www.w3.org/2002/07/owl#versionInfo>
                "http://languagelink.let.uu.nl/tds/onto/LinguisticOntology.owl#patientRole" .

<http://purl.org/olia/olia.owl#CausalAdverb>
        a       <http://www.w3.org/2002/07/owl#Class> ;
        <http://www.w3.org/2000/01/rdf-schema#comment>
                "Adverb/Type=\"causal\" is used in the Hungarian MTE v4, but no examples are provided. (http://purl.org/olia/mte/multext-east.owl#CausalAdverb)" ;
        <http://www.w3.org/2000/01/rdf-schema#subClassOf>
                <http://purl.org/olia/olia.owl#Adverb> ;
        <http://www.w3.org/2002/07/owl#deprecated>
                true ;
        <http://www.w3.org/2002/07/owl#equivalentClass>
                [ a       <http://www.w3.org/2002/07/owl#Class> ;
                  <http://www.w3.org/2002/07/owl#intersectionOf>
                          ( <http://purl.org/olia/olia.owl#Adverb>
                            [ a       <http://www.w3.org/2002/07/owl#Restriction> ;
                              <http://www.w3.org/2002/07/owl#onProperty>
                                      <http://purl.org/olia/olia.owl#hasSemanticRole> ;
                              <http://www.w3.org/2002/07/owl#someValuesFrom>
                                      <http://purl.org/olia/olia.owl#CauseRole>
                            ]
                          )
                ] ;
        <http://www.w3.org/2002/07/owl#versionInfo>
                "DEPRECATED: equivalent to Adverb and hasSemanticRole some CauseRole" , "http://purl.org/olia/mte/multext-east.owl#CausalAdverb" .

<http://purl.org/olia/olia.owl#NominalQuantifier>
        a       <http://www.w3.org/2002/07/owl#Class> ;
        <http://www.w3.org/2000/01/rdf-schema#comment>
                "A noun which quantifies one or more things, regardless of subject and an object.\n\t\t\t\n\t\t\tང་གིས་ བམོ་ ལ་ དང་ ཕད་ཅི།\n\t\t\tNGAGI BUM 'NGA 'DA CHECI\n\t\t\tI girl five with met\n\t\t\t“I met with five girls.”\n\t\t\t(Jurmey Rabgay, email Sep 20, 2010)" ;
        <http://www.w3.org/2000/01/rdf-schema#label>
                "quantifier noun" ;
        <http://www.w3.org/2000/01/rdf-schema#subClassOf>
                <http://purl.org/olia/olia.owl#Quantifier> ;
        <http://www.w3.org/2002/07/owl#equivalentClass>
                [ a       <http://www.w3.org/2002/07/owl#Class> ;
                  <http://www.w3.org/2002/07/owl#intersectionOf>
                          ( <http://purl.org/olia/olia.owl#Quantifier> <http://purl.org/olia/olia.owl#Noun> )
                ] ;
        <http://www.w3.org/2002/07/owl#versionInfo>
                "shorthand for Quantifier and Noun, adopted from Dzongkha tagset (Chungku et al. 2010)" .

<http://purl.org/olia/olia.owl#AdjectivePhrase>
        a       <http://www.w3.org/2002/07/owl#Class> ;
        <http://www.w3.org/2000/01/rdf-schema#comment>
                "\n\t\t\tAdjectivePhrase is the class of phrases that have adjectives as heads.\n\t\t\t(http://purl.org/linguistics/gold/AdjectivePhrase)\n\t\t" , "\n\t\t\tAn adjective phrase may consist of an adjective, or a sequence of words in which an adjective is the head of the\n\t\t\tphrase, as shown in 47 to 50 below.\n\n\t\t\t(47)  \t[NP his [ADJP surprisingly thick and hairy ADJP] wrists NP]\n\t\t\t(48)  \t[NP some [ADJP [ADJP wholly unanticipated ADJP] but [ADJP remotely possible ADJP] ADJP] event NP]\n\t\t\t(49)  \t[S [NP His speeches NP] [VP are [ADVP always ADVP] [ADJP too long [PP for comfort PP] ADJP] VP] S]\n\t\t\t(50)  \t[AUX have AUX] [NP you NP] [VP found [NP something \n\t\t\t\t\t[ADJP suitable [PP for [NP your needs NP] PP] ADJP] NP] VP] ?\n\t\t\t(http://www.ilc.cnr.it/EAGLES96/segsasg1/node36.html)\n\t\t" ;
        <http://www.w3.org/2000/01/rdf-schema#subClassOf>
                <http://purl.org/olia/olia.owl#Phrase> ;
        <http://www.w3.org/2002/07/owl#versionInfo>
                "http://purl.org/linguistics/gold/AdjectivePhrase" .

<http://purl.org/olia/olia.owl#RelativeMood>
        a       <http://www.w3.org/2002/07/owl#Class> ;
        <http://www.w3.org/2000/01/rdf-schema#comment>
                "Mood to express reported speech (or indirect speech) as opposed to direct speech." ;
        <http://www.w3.org/2000/01/rdf-schema#isDefinedBy>
                "http://www.isocat.org/datcat/DC-3836" ;
        <http://www.w3.org/2000/01/rdf-schema#subClassOf>
                <http://purl.org/olia/olia-top.owl#MoodFeature> , <http://purl.org/olia/olia.owl#RelativeModality> ;
        <http://www.w3.org/2002/07/owl#versionInfo>
                "Clarify relationship with DirectSpeech" .

<http://purl.org/olia/olia-top.owl#SyntacticFunction>
        a       <http://www.w3.org/2002/07/owl#Class> ;
        <http://www.w3.org/2000/01/rdf-schema#subClassOf>
                [ a       <http://www.w3.org/2002/07/owl#Restriction> ;
                  <http://www.w3.org/2002/07/owl#hasSelf>
                          true ;
                  <http://www.w3.org/2002/07/owl#onProperty>
                          <http://purl.org/olia/olia.owl#hasSyntacticFunction>
                ] ;
        <http://www.w3.org/2000/01/rdf-schema#subClassOf>
                [ a       <http://www.w3.org/2002/07/owl#Restriction> ;
                  <http://www.w3.org/2002/07/owl#hasSelf>
                          true ;
                  <http://www.w3.org/2002/07/owl#onProperty>
                          <http://purl.org/olia/olia.owl#hasSyntacticFunction>
                ] .

<http://purl.org/olia/olia.owl#ExpansionVariation>
        a       <http://www.w3.org/2002/07/owl#Class> ;
        <http://www.w3.org/2000/01/rdf-schema#comment>
                "Description of the kind of variation between full and abbreviated forms." ;
        <http://www.w3.org/2000/01/rdf-schema#isDefinedBy>
                "http://www.isocat.org/datcat/DC-1850" ;
        <http://www.w3.org/2000/01/rdf-schema#subClassOf>
                <http://purl.org/olia/system.owl#Relation> , <http://purl.org/olia/olia-top.owl#LexicalRelation> .

<http://purl.org/olia/olia.owl#SubordinatingConjunctionWithInfinite>
        a       <http://www.w3.org/2002/07/owl#Class> ;
        <http://www.w3.org/2000/01/rdf-schema#comment>
                "\n\t\t\tFor example, in German the subordinating conjunction \"ohne\" (\"zu\"...) \n\t\t\tis followed by an infinitive. \n\t\t\t(http://www.ilc.cnr.it/EAGLES96/annotate/node19.html#oav2u  17.11.06)\n\t\t" ;
        <http://www.w3.org/2000/01/rdf-schema#subClassOf>
                <http://purl.org/olia/olia.owl#SubordinatingConjunction> ;
        <http://www.w3.org/2002/07/owl#versionInfo>
                "EAGLES" .

<http://purl.org/olia/olia.owl#hasProximity>
        a       <http://www.w3.org/2002/07/owl#ObjectProperty> ;
        <http://www.w3.org/2000/01/rdf-schema#range>
                <http://purl.org/olia/olia-top.owl#ProximityFeature> ;
        <http://www.w3.org/2000/01/rdf-schema#subPropertyOf>
                <http://purl.org/olia/system.owl#hasFeature> .

<http://purl.org/olia/olia.owl#PreHodiernalPast>
        a       <http://www.w3.org/2002/07/owl#Class> ;
        <http://www.w3.org/2000/01/rdf-schema#comment>
                "\n\t\t\tPreHodiernalPastTense locates the situation in question before that of a \n\t\t\tcontrasting HodiernalPastTense. According to Bybee, Perkins, Pagliuca 1994: \n\t\t\t98. this category must be defined relative to a HodiernalPastTense.\n\t\t\t(http://purl.org/linguistics/gold/PreHodiernalPast)\n\t\t" ;
        <http://www.w3.org/2000/01/rdf-schema#subClassOf>
                <http://purl.org/olia/olia.owl#AbsoluteTense> ;
        <http://www.w3.org/2002/07/owl#versionInfo>
                "http://purl.org/linguistics/gold/PreHodiernalPast, classified as absolute tense" .

<http://purl.org/olia/olia.owl#RelativeAdjective>
        a       <http://www.w3.org/2002/07/owl#Class> ;
        <http://www.w3.org/2000/01/rdf-schema#comment>
                "Relative adjectives express similarity or a comparison. (Schmidt 1999, p.218, http://purl.org/olia/emille.owl#RelativeAdjective)" ;
        <http://www.w3.org/2000/01/rdf-schema#subClassOf>
                <http://purl.org/olia/olia.owl#Adjective> ;
        <http://www.w3.org/2002/07/owl#versionInfo>
                "adopted from EMILLE for Urdu, http://purl.org/olia/emille.owl#RelativeAdjective" .

<http://purl.org/olia/olia.owl#Impossible>
        a       <http://www.w3.org/2002/07/owl#Class> ;
        <http://www.w3.org/2000/01/rdf-schema#comment>
                "to denote something that cannot be considered as being correct in a given language" ;
        <http://www.w3.org/2000/01/rdf-schema#isDefinedBy>
                "http://www.isocat.org/datcat/DC-1866" ;
        <http://www.w3.org/2000/01/rdf-schema#subClassOf>
                <http://purl.org/olia/olia-top.owl#UsageAndFrequencyFeature> .

<http://purl.org/olia/olia.owl#ImperativeVerb>
        a       <http://www.w3.org/2002/07/owl#Class> ;
        <http://www.w3.org/2000/01/rdf-schema#comment>
                "\n\t\t\tAn imperative verb is used to express commands, direct requests, and \n\t\t\tprohibitions. Often, direct use of the imperative mood may appear\n\t\t\tblunt or even rude, so it is often used with care. Example: \"Paul, \n\t\t\tread that book\".\n\t\t\t(http://en.wikipedia.org/wiki/Grammatical_mood#Imperative_mood 19.09.06)\n\t\t" ;
        <http://www.w3.org/2000/01/rdf-schema#subClassOf>
                <http://purl.org/olia/olia.owl#FiniteVerb> ;
        <http://www.w3.org/2002/07/owl#versionInfo>
                "EAGLES FiniteVerb with VerbForm=\"Imperative\"" .

<http://purl.org/olia/olia.owl#TransitiveObject>
        a       <http://www.w3.org/2002/07/owl#Class> ;
        <http://www.w3.org/2000/01/rdf-schema#comment>
                "\n\t\t\tSecond argument of a transitive verb, transitive object (P)\n\t\t\t(http://languagelink.let.uu.nl/tds/onto/LinguisticOntology.owl#P)\n\t\t" ;
        <http://www.w3.org/2000/01/rdf-schema#subClassOf>
                <http://purl.org/olia/olia.owl#DirectObject> ;
        <http://www.w3.org/2002/07/owl#versionInfo>
                "http://languagelink.let.uu.nl/tds/onto/LinguisticOntology.owl#P" .

<http://purl.org/olia/olia.owl#ProgressivePassive>
        a       <http://www.w3.org/2002/07/owl#Class> ;
        <http://www.w3.org/2000/01/rdf-schema#comment>
                "\n\t\t\tA passive in Irish  in which the preposition \"at\" is used, and a semantic \n\t\t\tmeaning of progressive tense is found (Noonan 1994:280)\n\t\t\t(http://purl.org/linguistics/gold/ProgressivePassive)\n\t\t" ;
        <http://www.w3.org/2000/01/rdf-schema#subClassOf>
                <http://purl.org/olia/olia.owl#PassiveVoice> ;
        <http://www.w3.org/2002/07/owl#versionInfo>
                "http://purl.org/linguistics/gold/ProgressivePassive" .

<http://purl.org/olia/olia.owl#AbsolutiveAntipassive>
        a       <http://www.w3.org/2002/07/owl#Class> ;
        <http://www.w3.org/2000/01/rdf-schema#comment>
                "\n\t\t\tAn Antipassive in which the P or logical object is suppressed \n\t\t\tor overtly absent. (Klaiman 1991:232)\n\t\t\t(http://purl.org/linguistics/gold/AbsolutiveAntipassive)\n\t\t" ;
        <http://www.w3.org/2000/01/rdf-schema#subClassOf>
                <http://purl.org/olia/olia.owl#Antipassive> ;
        <http://www.w3.org/2002/07/owl#versionInfo>
                "http://purl.org/linguistics/gold/AbsolutiveAntipassive" .

<http://purl.org/olia/olia.owl#OpenSquareBracket>
        a       <http://www.w3.org/2002/07/owl#Class> ;
        <http://www.w3.org/2000/01/rdf-schema#comment>
                "[\n*LSB*\nLeft square bracket\n(Santorini 1991)" ;
        <http://www.w3.org/2000/01/rdf-schema#subClassOf>
                <http://purl.org/olia/olia.owl#LeftParentheticalPunctuation> ;
        <http://www.w3.org/2002/07/owl#versionInfo>
                "PTB bracketing guidelines, Santorini 1991" .

<http://purl.org/olia/olia.owl#AuxiliaryVerb>
        a       <http://www.w3.org/2002/07/owl#Class> ;
        <http://www.w3.org/2000/01/rdf-schema#comment>
                "    \n\t\tAn auxiliary verb is a verb which accompanies the lexical verb of a verb phrase, \n\t\tand expresses grammatical distinctions not carried by the lexical verb, such as \n\t\tperson, number, tense aspect, and voice. \n\t\t(http://www.sil.org/linguistics/GlossaryOfLinguisticTerms/WhatIsAnAuxiliaryVerb.htm 19.09.06)\n\t\t\n\t\tBesides modal verbs (\"semiauxiliary\") and \"strict\" auxiliary verbs, also copulas \n\t\tare classified under auxiliary verbs here, as this is a praxis applied in practically every\n\t\tEAGLES-conformant morphosyntactic annotation scheme.\n\n\t\tPart of speech referring to the set of verbs, subordinate to the main lexical verb which help \n\t\tto make distinction in mood, aspect, voice etc.\n        (Crystal 2003; http://www.isocat.org/datcat/DC-1244)\n        " ;
        <http://www.w3.org/2000/01/rdf-schema#label>
                "auxiliary verb"@en , "auxiliaire"@fr ;
        <http://www.w3.org/2000/01/rdf-schema#subClassOf>
                <http://purl.org/olia/olia.owl#Verb> ;
        <http://www.w3.org/2002/07/owl#versionInfo>
                "EAGLES Verbs with Status=\"Auxiliary\", http://www.isocat.org/datcat/DC-1244" ;
        <http://www.w3.org/2004/02/skos/core#altLabel>
                "auxiliary"@en .

<http://purl.org/olia/olia.owl#SubessiveCase>
        a       <http://www.w3.org/2002/07/owl#Class> ;
        <http://www.w3.org/2000/01/rdf-schema#comment>
                "\n\t\t\tSubessiveCase expresses that  the referent of the noun it marks is \n\t\t\tthe location under which another referent exists. It has the meaning \n\t\t\tof 'under' or 'beneath'.\n\t\t\t(http://purl.org/linguistics/gold/Subessive)\n\t\t" ;
        <http://www.w3.org/2000/01/rdf-schema#subClassOf>
                <http://purl.org/olia/olia-top.owl#CaseFeature> ;
        <http://www.w3.org/2002/07/owl#versionInfo>
                "http://purl.org/linguistics/gold/Subessive" .

<http://purl.org/olia/olia.owl#TimitiveModality>
        a       <http://www.w3.org/2002/07/owl#Class> ;
        <http://www.w3.org/2000/01/rdf-schema#comment>
                "\n\t\t\tTimitiveMood expresses that the speaker fears something expressed in what is said \n\t\t\t(Palmer 2001: 13, 22).\n\t\t\t(http://purl.org/linguistics/gold/Timitive)\n\t\t" ;
        <http://www.w3.org/2000/01/rdf-schema#subClassOf>
                <http://purl.org/olia/olia-top.owl#ModalityFeature> ;
        <http://www.w3.org/2002/07/owl#versionInfo>
                "http://purl.org/linguistics/gold/Timitive" .

<http://purl.org/olia/olia.owl#AdessiveCase>
        a       <http://www.w3.org/2002/07/owl#Class> ;
        <http://www.w3.org/2000/01/rdf-schema#comment>
                "\n\t\t\tAdessiveCase expresses that  the referent of the noun it marks is \n\t\t\tthe location near/at which another referent exists. It has the \n\t\t\tmeaning of 'at' or 'near' (Crystal 1997: 8).\n\t\t\t(http://purl.org/linguistics/gold/Adessive)\n\t\t" ;
        <http://www.w3.org/2000/01/rdf-schema#subClassOf>
                <http://purl.org/olia/olia-top.owl#CaseFeature> ;
        <http://www.w3.org/2002/07/owl#versionInfo>
                "http://purl.org/linguistics/gold/Adessive, http://www.isocat.org/datcat/DC-1228" .

<http://purl.org/olia/olia.owl#ContallativeCase>
        a       <http://www.w3.org/2002/07/owl#Class> ;
        <http://www.w3.org/2000/01/rdf-schema#comment>
                "\n\t\t\tContallativeCase expresses that  something is moving toward the \n\t\t\tvicinity of the referent of the noun it marks. It has the meaning  \n\t\t\t'towards the vicinity of'.\n\t\t\t(http://purl.org/linguistics/gold/Contallative)\n\t\t" ;
        <http://www.w3.org/2000/01/rdf-schema#subClassOf>
                <http://purl.org/olia/olia-top.owl#CaseFeature> ;
        <http://www.w3.org/2002/07/owl#versionInfo>
                "http://purl.org/linguistics/gold/Contallative" .

<http://purl.org/olia/olia-top.owl#ReflexivityFeature>
        a       <http://www.w3.org/2002/07/owl#Class> ;
        <http://www.w3.org/2000/01/rdf-schema#subClassOf>
                <http://purl.org/olia/olia-top.owl#VoiceFeature> ;
        <http://www.w3.org/2000/01/rdf-schema#subClassOf>
                [ a       <http://www.w3.org/2002/07/owl#Restriction> ;
                  <http://www.w3.org/2002/07/owl#hasSelf>
                          true ;
                  <http://www.w3.org/2002/07/owl#onProperty>
                          <http://purl.org/olia/olia.owl#hasReflexivity>
                ] ;
        <http://www.w3.org/2000/01/rdf-schema#subClassOf>
                [ a       <http://www.w3.org/2002/07/owl#Restriction> ;
                  <http://www.w3.org/2002/07/owl#hasSelf>
                          true ;
                  <http://www.w3.org/2002/07/owl#onProperty>
                          <http://purl.org/olia/olia.owl#hasReflexivity>
                ] ;
        <http://www.w3.org/2002/07/owl#versionInfo>
                "TODO: integrate with VoiceFeature (as in the TDS Ontology) implementation" .

<http://purl.org/olia/olia.owl#MalefactiveCase>
        a       <http://www.w3.org/2002/07/owl#Class> ;
        <http://www.w3.org/2000/01/rdf-schema#comment>
                "\n\t\t\tOpposite of BenefactiveCase; used when the marked noun is negatively \n\t\t\taffected in the clause.\n\t\t\t(http://purl.org/linguistics/gold/Malefactive)\n\t\t" ;
        <http://www.w3.org/2000/01/rdf-schema#subClassOf>
                <http://purl.org/olia/olia-top.owl#CaseFeature> ;
        <http://www.w3.org/2002/07/owl#versionInfo>
                "http://purl.org/linguistics/gold/Malefactive" .

<http://purl.org/olia/olia.owl#ProgressiveAspect>
        a       <http://www.w3.org/2002/07/owl#Class> ;
        <http://www.w3.org/2000/01/rdf-schema#comment>
                "\n\t\t\tProgressiveAspect, also called the continuative or the durative, \n\t\t\tencodes a single event as an ongoing process. Thus, states cannot \n\t\t\tgenerally be encoded with the progressive (Comrie 1976: 32-35; \n\t\t\tBybee, Perkins and Pagliuca 1994: 127-139; Payne 1997: 240). An \n\t\t\texponent of phasal aspect which expresses a stative situation that \n\t\t\tholds during the time at which an event is occurring (e. g., He is \n\t\t\tfixing the fence) \n\t\t\t(Michaelis 1998:xv).\n\t\t\t(http://purl.org/linguistics/gold/Progressive)\n\t\t" ;
        <http://www.w3.org/2000/01/rdf-schema#subClassOf>
                <http://purl.org/olia/olia-top.owl#AspectFeature> ;
        <http://www.w3.org/2002/07/owl#versionInfo>
                "\n\t\t\thttp://purl.org/linguistics/gold/Progressive\n\t\t" .

<http://purl.org/olia/olia.owl#TimeRole>
        a       <http://www.w3.org/2002/07/owl#Class> ;
        <http://www.w3.org/2000/01/rdf-schema#comment>
                "\n\t\t\t\tSemantic role corresponding to the label \"TIME\" used by the Stanford Dependency Parser.\n\t\t\t\tTime covers a point or an interval of time at which the action takes place. (Dipper et al. 2007, §5.3.9)\n\t\t\t\t\n\t\t\t\t-TMP (temporal) — marks temporal or aspectual adverbials that answer the questions when, how often, or how \n\t\t\t\tlong. It has some uses that are not strictly adverbial, such as with dates that modify other NPs (see \n\t\t\t\tsection 11 [Modification of NP]). \n\t\t\t\t(Bies et al. 1995)\n\t\t" ;
        <http://www.w3.org/2000/01/rdf-schema#subClassOf>
                <http://purl.org/olia/olia-top.owl#SemanticRole> ;
        <http://www.w3.org/2002/07/owl#versionInfo>
                "added in conformance with Stanford Parser Dependency Label TIME and SFB632 annotation guidelines (Dipper et al. 2007)" .

<http://purl.org/olia/olia.owl#InterrogativeDeterminer>
        a       <http://www.w3.org/2002/07/owl#Class> ;
        <http://www.w3.org/2000/01/rdf-schema#comment>
                "\n\t\t\tA interrogative is a function word used to introduce an interrogative clause.\n\t\t\tE.g. \"which\", \"what\", \"whose\" (interrogative possessive determiner) are  \n\t\t\tinterrogative determiner in English. \n\t\t\t(http://en.wikipedia.org/wiki/Interrogative_word  02.05.07)\n\t\t" ;
        <http://www.w3.org/2000/01/rdf-schema#subClassOf>
                <http://purl.org/olia/olia.owl#WHDeterminer> ;
        <http://www.w3.org/2002/07/owl#equivalentClass>
                [ a       <http://www.w3.org/2002/07/owl#Class> ;
                  <http://www.w3.org/2002/07/owl#intersectionOf>
                          ( <http://purl.org/olia/olia.owl#WHDeterminer> <http://purl.org/olia/olia.owl#QuestionWord> )
                ] ;
        <http://www.w3.org/2002/07/owl#versionInfo>
                "EAGLES Determiner with WhType=\"Interrogative\"" .

<http://purl.org/olia/olia.owl#String>
        a       <http://www.w3.org/2002/07/owl#Class> ;
        <http://www.w3.org/2000/01/rdf-schema#comment>
                "Character string to be interpreted in context" ;
        <http://www.w3.org/2000/01/rdf-schema#isDefinedBy>
                "http://www.isocat.org/datcat/DC-2182" ;
        <http://www.w3.org/2000/01/rdf-schema#subClassOf>
                <http://purl.org/olia/olia-top.owl#OrthographicEntity> ;
        <http://www.w3.org/2002/07/owl#versionInfo>
                "Introduced as a generalization over numeralRoman which is orthographically defined but not a single character" .

<http://purl.org/olia/olia.owl#InterrogativePunctuation>
        a       <http://www.w3.org/2002/07/owl#Class> ;
        <http://www.w3.org/2000/01/rdf-schema#comment>
                "\n                            Punctuation used when the sentence is interrogative.\n                                (http://www.isocat.org/datcat/DC-2087)\n                            " ;
        <http://www.w3.org/2000/01/rdf-schema#label>
                "interrogative punctuation" ;
        <http://www.w3.org/2000/01/rdf-schema#subClassOf>
                <http://purl.org/olia/olia.owl#MainPunctuation> ;
        <http://www.w3.org/2002/07/owl#versionInfo>
                "http://www.isocat.org/datcat/DC-2087" .

<http://purl.org/olia/olia.owl#Space>
        a       <http://www.w3.org/2002/07/owl#Class> ;
        <http://www.w3.org/2000/01/rdf-schema#comment>
                "\n                            Empty area between words, lines or columns\n                                (http://www.isocat.org/datcat/DC-2189)\n                            " ;
        <http://www.w3.org/2000/01/rdf-schema#label>
                "space" ;
        <http://www.w3.org/2000/01/rdf-schema#subClassOf>
                <http://purl.org/olia/olia.owl#GraphicalSeparator> ;
        <http://www.w3.org/2002/07/owl#versionInfo>
                "http://www.isocat.org/datcat/DC-2189" .

<http://purl.org/olia/olia.owl#MultiplicativeCase>
        a       <http://www.w3.org/2002/07/owl#Class> ;
        <http://www.w3.org/2000/01/rdf-schema#comment>
                "A case used in the Hungarian MULTEXT-East scheme, e.g., tizennegyedszer/tizennegyed, tucatszor/tucat, tízezredszer/tízezred (hu)\n\t\t\t(http://purl.org/olia/mte/multext-east.owl#MultiplicativeCase)" , "\n\t\t\tThe multiplicative case is a grammatical case used for marking a number of something (\"three times\").\n\t\t\tThe case is found in the Hungarian language, for example nyolc (eight), nyolcszor (eight times).\n\t\t\tThe case appears also in Finnish as an adverbial (adverb-forming) case. Used with a cardinal number it denotes the number of actions; for example, viisi (five) -> viidesti (five times). Used with adjectives it refers to the mean of the action, corresponding the English suffix -ly: kaunis (beautiful) -> kauniisti (beautifully). It is also used with a small number of nouns: leikki (play) -> leikisti (just kidding, not really). In addition, it acts as an intensifier when used with a swearword: piru -> pirusti.\n\t\t\t(http://en.wikipedia.org/wiki/Multiplicative_case)\n\t\t" ;
        <http://www.w3.org/2000/01/rdf-schema#subClassOf>
                <http://purl.org/olia/olia-top.owl#CaseFeature> ;
        <http://www.w3.org/2002/07/owl#versionInfo>
                "http://purl.org/olia/mte/multext-east.owl#MultiplicativeCase" .

<http://purl.org/olia/olia.owl#WHTypeAdverbs>
        a       <http://www.w3.org/2002/07/owl#Class> ;
        <http://www.w3.org/2000/01/rdf-schema#comment>
                "\n\t\t\tAdverb that serves to express interrogativity, exclamation or that serves to link a subordinate clause to the matrix clause.\n\t\t\t(Ch. Chiarcos)\n\t\t" ;
        <http://www.w3.org/2000/01/rdf-schema#subClassOf>
                <http://purl.org/olia/olia.owl#Adverb> ;
        <http://www.w3.org/2002/07/owl#versionInfo>
                "TODO: rename to WHTypeAdverb" , "See remarks on WHPronoun, this is actually a language-specific trait and should probably be removed." , "EAGLES Adverb with Polarity=\"Wh-type\"." .

<http://purl.org/olia/olia.owl#Participle>
        a       <http://www.w3.org/2002/07/owl#Class> ;
        <http://www.w3.org/2000/01/rdf-schema#comment>
                "\n\tA participle is a lexical item, derived from a verb that has some of the characteristics and functions of both verbs and adjectives.\n\tIn English, participles may be used as adjectives, and in non-finite forms of verbs.\n\t(http://www.sil.org/linguistics/GlossaryOfLinguisticTerms/WhatIsAParticiple.htm 19.09.06)\n\t\n\tNon-finite form of a verb other than the infinitive that is used in many languages possibly in conjunction with an auxiliary and that functions attributively, predicatively or adverbially. (http://www.isocat.org/datcat/DC-1341)" ;
        <http://www.w3.org/2000/01/rdf-schema#isDefinedBy>
                "http://www.isocat.org/datcat/DC-1341" ;
        <http://www.w3.org/2000/01/rdf-schema#label>
                "participe"@fr , "participle"@en ;
        <http://www.w3.org/2000/01/rdf-schema#subClassOf>
                <http://purl.org/olia/olia.owl#NonFiniteVerb> ;
        <http://www.w3.org/2002/07/owl#versionInfo>
                "EAGLES NonFinite with VerbForm=\"Participle\"." .

<http://purl.org/olia/olia.owl#HabitualAspect>
        a       <http://www.w3.org/2002/07/owl#Class> ;
        <http://www.w3.org/2000/01/rdf-schema#comment>
                "\n\t\t\tHabitual tense pertains to verbs which refer to an action that occurs repeatedly.\n\t\t\t(http://languagelink.let.uu.nl/tds/onto/LinguisticOntology.owl#habitualTense)\n\t\t\n\t\t\tRefers to the internal temporal contour of a situation — a repeated \n\t\t\tsituation that occupies a large slice of time. Can be based on the \n\t\t\tobservation of a single occurrence.\n\t\t\t(Bhat 1999:177)\n\t\t\t(http://purl.org/linguistics/gold/Habitual)\n\t\t" ;
        <http://www.w3.org/2000/01/rdf-schema#subClassOf>
                <http://purl.org/olia/olia-top.owl#AspectFeature> ;
        <http://www.w3.org/2002/07/owl#versionInfo>
                "\n\t\t\thttp://purl.org/linguistics/gold/Habitual (as Aspect),\n\t\t\thttp://languagelink.let.uu.nl/tds/onto/LinguisticOntology.owl#habitualTense (as Tense),\n\t\t\tmodelled as an aspect here (temporally unmarked Habitual should be modelled as NotTemporallyAnchored)\n\t\t" .

<http://purl.org/olia/olia.owl#NearFuture>
        a       <http://www.w3.org/2002/07/owl#Class> ;
        <http://www.w3.org/2000/01/rdf-schema#comment>
                "\n\t\t\tadopted from GOLD, no definition given there\n\t\t\t(http://purl.org/linguistics/gold/NearFuture)\n\t\t" ;
        <http://www.w3.org/2000/01/rdf-schema#subClassOf>
                <http://purl.org/olia/olia.owl#Future> ;
        <http://www.w3.org/2002/07/owl#versionInfo>
                "http://purl.org/linguistics/gold/NearFuture, classified as Future here" .

<http://purl.org/olia/olia.owl#DeterminalPronoun>
        a       <http://www.w3.org/2002/07/owl#Class> ;
        <http://www.w3.org/2000/01/rdf-schema#comment>
                "The Estonian determinal pronouns _ise_, _end(a)_ `(one)self'.\" combine aspects of emphatic pronouns and reflexive pronouns.\n\t\t\tIt could also be described as an intensifier that is formally identical with the reflexive pronoun or as an emphatic reflexive pronoun.\n\t\t\t(Ivan A. Derzhanski, Heiki-Jaan Kaalep, http://purl.org/olia/mte/multext-east.owl#DeterminalPronoun;\n\t\t\tInsa Gülzow (2006), The acquisition of intensifiers: Emphatic reflexives in English and German child language, Mouton de Gruyter, Berlin, p. 258)\n\t\t" ;
        <http://www.w3.org/2000/01/rdf-schema#subClassOf>
                <http://purl.org/olia/olia.owl#PersReflPronoun> ;
        <http://www.w3.org/2002/07/owl#versionInfo>
                "Not to be confused with pronominal determiners" , "http://purl.org/olia/mte/multext-east.owl#DeterminalPronoun" .

<http://purl.org/olia/olia.owl#ObligativeModality>
        a       <http://www.w3.org/2002/07/owl#Class> ;
        <http://www.w3.org/2000/01/rdf-schema#comment>
                "ObligativeModality indicates that an agent is\n                        required to perform the action expressed by the predicate [Bybee, Perkins\n                        and Pagliuca 1994: 177; Palmer 2001: 71]." ;
        <http://www.w3.org/2000/01/rdf-schema#isDefinedBy>
                "http://www.isocat.org/datcat/DC-3356" ;
        <http://www.w3.org/2000/01/rdf-schema#subClassOf>
                <http://purl.org/olia/olia-top.owl#ModalityFeature> .

<http://purl.org/olia/olia.owl#PronominalAdverb>
        a       <http://www.w3.org/2002/07/owl#Class> ;
        <http://www.w3.org/2000/01/rdf-schema#comment>
                "\n\t\t\tPronominal adverbs substitute for a preposition (which is incorporated into them) and an NP, cf.\n\t\t\tEnglish therefore lit. \"for this (reason, ...)\", German deswegen lit. \"because of this (reason, ...)\".\n\t\t\t(http://www.ilc.cnr.it/EAGLES96/elm_de/node235.html 21.09.06, examples Ch. Chiarcos)\n\t\t" ;
        <http://www.w3.org/2000/01/rdf-schema#isDefinedBy>
                "http://www.isocat.org/datcat/DC-3011 (adverbialPronoun)" ;
        <http://www.w3.org/2000/01/rdf-schema#label>
                "pronominal adverb" , "adverbial pronoun" ;
        <http://www.w3.org/2000/01/rdf-schema#subClassOf>
                <http://purl.org/olia/olia.owl#Adverb> ;
        <http://www.w3.org/2002/07/owl#versionInfo>
                "\n\t\t\tEAGLES Adverb with Adverb-Type=\"Pronominal\".\n\n\t\t\tAgainst the EAGLES definition given below, pronominal adverbs can but don't have to be used for \n\t\t\tpronominal references, thus this special and diachronically important case is better described \n\t\t\tby the join of this with personal pronoun.\n\t\t" .

<http://purl.org/olia/olia-top.owl#NumeralAgreementClass>
        a       <http://www.w3.org/2002/07/owl#Class> ;
        <http://www.w3.org/2000/01/rdf-schema#subClassOf>
                [ a       <http://www.w3.org/2002/07/owl#Restriction> ;
                  <http://www.w3.org/2002/07/owl#hasSelf>
                          true ;
                  <http://www.w3.org/2002/07/owl#onProperty>
                          <http://purl.org/olia/olia.owl#hasNumeralAgreementClass>
                ] .

<http://purl.org/olia/olia.owl#Punctuation>
        a       <http://www.w3.org/2002/07/owl#Class> ;
        <http://www.w3.org/2000/01/rdf-schema#comment>
                "\n\t\tPunctuation marks (PU) are treated here as a part of morphosyntactic annotation, as it \n\t\tis very common for punctuation marks to be tagged and to be treated as equivalent to \n\t\twords for the purposes of automatic tag assignment.\n\t\t(http://www.ilc.cnr.it/EAGLES96/annotate/node16.html#mp 19.09.06)\n\t" ;
        <http://www.w3.org/2000/01/rdf-schema#subClassOf>
                <http://purl.org/olia/olia-top.owl#MorphosyntacticCategory> ;
        <http://www.w3.org/2002/07/owl#versionInfo>
                "EAGLES top-level category Punctuation (PU).\n\t\n\t\tFor subconcepts, Wilson and Leech (1996) propose two alternative classifications: \n\t\tHere, we implement the more interesting, i.e. position (the alternative is just enumeration of possible signs)\n\t" .

<http://purl.org/olia/olia.owl#TimitiveMood>
        a       <http://www.w3.org/2002/07/owl#Class> ;
        <http://www.w3.org/2000/01/rdf-schema#comment>
                "\n\t\t\tTimitiveMood expresses that the speaker fears something expressed in what is said \n\t\t\t(Palmer 2001: 13, 22).\n\t\t\t(http://purl.org/linguistics/gold/Timitive)\n\t\t" ;
        <http://www.w3.org/2000/01/rdf-schema#subClassOf>
                <http://purl.org/olia/olia.owl#TimitiveModality> , <http://purl.org/olia/olia-top.owl#MoodFeature> ;
        <http://www.w3.org/2002/07/owl#versionInfo>
                "http://purl.org/linguistics/gold/Timitive" .

<http://purl.org/olia/olia.owl#CloseFuture>
        a       <http://www.w3.org/2002/07/owl#Class> ;
        <http://www.w3.org/2000/01/rdf-schema#comment>
                "\n\t\t\tAdopted from GOLD. No definition given.\n\t\t" ;
        <http://www.w3.org/2000/01/rdf-schema#subClassOf>
                <http://purl.org/olia/olia.owl#AbsoluteTense> ;
        <http://www.w3.org/2002/07/owl#versionInfo>
                "http://purl.org/linguistics/gold/CloseFuture, classified as AbsoluteTense here" .

<http://purl.org/olia/olia.owl#Sequel>
        a       <http://www.w3.org/2002/07/owl#Class> ;
        <http://www.w3.org/2000/01/rdf-schema#comment>
                "Adopted from ILPOSTS for Indian languages. No definition or examples provided: Distance=Sequel (http://purl.org/olia/ilposts.owl#Sequel)" ;
        <http://www.w3.org/2000/01/rdf-schema#subClassOf>
                <http://purl.org/olia/olia-top.owl#ProximityFeature> ;
        <http://www.w3.org/2002/07/owl#versionInfo>
                "TODO: provide definition" , "added in accordance with ILPOSTS (for Indian languages), http://purl.org/olia/ilposts.owl#Sequel" .

<http://purl.org/olia/olia.owl#Reflexive>
        a       <http://www.w3.org/2002/07/owl#Class> ;
        <http://www.w3.org/2000/01/rdf-schema#comment>
                "\n\t\t\tA reflexive verb is a verb whose semantic agent and patient (typically \n\t\t\trepresented syntactically by the subject and the direct object) are the \n\t\t\tsame. In many languages, reflexive constructions are rendered by transitive \n\t\t\tverbs followed by a reflexive pronoun, as in English -self (e. g., She \n\t\t\tthrew herself to the floor.). (http://en.wikipedia.org/wiki/Reflexive_verbs  \n\t\t\t20.11.06)\n\t\t" ;
        <http://www.w3.org/2000/01/rdf-schema#subClassOf>
                <http://purl.org/olia/olia-top.owl#ReflexivityFeature> , <http://purl.org/olia/olia-top.owl#VoiceFeature> ;
        <http://www.w3.org/2002/07/owl#versionInfo>
                "TODO: integrate with Voice, rename to ReflexiveVoice" .

<http://purl.org/olia/olia.owl#InteressiveCase>
        a       <http://www.w3.org/2002/07/owl#Class> ;
        <http://www.w3.org/2000/01/rdf-schema#comment>
                "\n\t\t\tInteressiveCase expresses that  the referent of the noun it marks is \n\t\t\tthe location between which another referent exists. It has the meaning \n\t\t\tof 'between'.\n\t\t\t(http://purl.org/linguistics/gold/Interessive)\n\t\t" ;
        <http://www.w3.org/2000/01/rdf-schema#subClassOf>
                <http://purl.org/olia/olia-top.owl#CaseFeature> ;
        <http://www.w3.org/2002/07/owl#versionInfo>
                "http://purl.org/linguistics/gold/Interessive" .

<http://purl.org/olia/olia.owl#RemotePast>
        a       <http://www.w3.org/2002/07/owl#Class> ;
        <http://www.w3.org/2000/01/rdf-schema#comment>
                "\n\t\t\tRemotePastTense locates the situation in question prior to the present \n\t\t\tmoment, usually more than a few days ago (Dahl 1985:121; Comrie 1985:88). \n\t\t\tSubsumes notion of PreHesternalPast tense, which locates the situation in \n\t\t\tquestion before that of an opposing hesternal past tense. \n\t\t\t(Bybee, Perkins, Pagliuca 1994: 98).\n\t\t\t(http://purl.org/linguistics/gold/RemotePast)\n\t\t" ;
        <http://www.w3.org/2000/01/rdf-schema#subClassOf>
                <http://purl.org/olia/olia.owl#Past> ;
        <http://www.w3.org/2002/07/owl#versionInfo>
                "http://purl.org/linguistics/gold/RemotePast, classified as absolute-relative here" .

<http://purl.org/olia/olia.owl#ActiveVoice>
        a       <http://www.w3.org/2002/07/owl#Class> ;
        <http://www.w3.org/2000/01/rdf-schema#comment>
                "\n\t\t\tWhen the subject is the agent or actor of the verb, \n\t\t\tthe verb is in the active voice. \n\t\t\t(http://en.wikipedia.org/wiki/Grammatical_voice  17.11.06)\n\t\t\t\n\t\t\tAssociated with transitivity, when the action is performed by an agent \n\t\t\t(subject) on another participant (object), or with intransitivity \n\t\t\t(McIntosh 1984:108). Refers to the category of underived verb forms \n\t\t\tassociated with the basic diathesis: Diathesis=D0:(X=SUBabs/nom) (Y=DIROBacc)\n\t\t\t(Shibatani 1995:7)\n\t\t\t(http://purl.org/linguistics/gold/Active)\n\t\t" ;
        <http://www.w3.org/2000/01/rdf-schema#subClassOf>
                <http://purl.org/olia/olia-top.owl#VoiceFeature> ;
        <http://www.w3.org/2002/07/owl#versionInfo>
                "http://languagelink.let.uu.nl/tds/onto/LinguisticOntology.owl#activeVoice" .

<http://purl.org/olia/olia.owl#Exclusive>
        a       <http://www.w3.org/2002/07/owl#Class> ;
        <http://www.w3.org/2000/01/rdf-schema#comment>
                "a form denoting that the addressee (addressees) are not included into the set of their referents which contain also the speaker" ;
        <http://www.w3.org/2000/01/rdf-schema#isDefinedBy>
                "http://www.isocat.org/datcat/DC-3029" ;
        <http://www.w3.org/2000/01/rdf-schema#subClassOf>
                <http://purl.org/olia/olia-top.owl#ClusivityFeature> .

<http://purl.org/olia/olia.owl#AdverbialParticiple>
        a       <http://www.w3.org/2002/07/owl#Class> ;
        <http://www.w3.org/2000/01/rdf-schema#comment>
                "Adverb/Type=\"participle\" is used in the Slovene MTE v4 specs, e.g., 'leže' / lying. Slovenian adverbial participles are, however, not attested for Resian. (MTE v4)(http://purl.org/olia/mte/multext-east.owl#AdverbialParticiple)" ;
        <http://www.w3.org/2000/01/rdf-schema#subClassOf>
                <http://purl.org/olia/olia.owl#Participle> , <http://purl.org/olia/olia.owl#Adverb> ;
        <http://www.w3.org/2002/07/owl#versionInfo>
                "http://purl.org/olia/mte/multext-east.owl#AdverbialParticiple" .

<http://purl.org/olia/olia-top.owl#SpecificityFeature>
        a       <http://www.w3.org/2002/07/owl#Class> ;
        <http://www.w3.org/2000/01/rdf-schema#subClassOf>
                [ a       <http://www.w3.org/2002/07/owl#Restriction> ;
                  <http://www.w3.org/2002/07/owl#hasSelf>
                          true ;
                  <http://www.w3.org/2002/07/owl#onProperty>
                          <http://purl.org/olia/olia.owl#hasSpecificity>
                ] ;
        <http://www.w3.org/2000/01/rdf-schema#subClassOf>
                [ a       <http://www.w3.org/2002/07/owl#Restriction> ;
                  <http://www.w3.org/2002/07/owl#hasSelf>
                          true ;
                  <http://www.w3.org/2002/07/owl#onProperty>
                          <http://purl.org/olia/olia.owl#hasSpecificity>
                ] .

<http://purl.org/olia/olia-top.owl#SyntacticRelation>
        a       <http://www.w3.org/2002/07/owl#Class> ;
        <http://www.w3.org/2000/01/rdf-schema#subClassOf>
                <http://purl.org/olia/system.owl#Relation> ;
        <http://www.w3.org/2000/01/rdf-schema#subClassOf>
                [ a       <http://www.w3.org/2002/07/owl#Class> ;
                  <http://www.w3.org/2002/07/owl#intersectionOf>
                          ( [ a       <http://www.w3.org/2002/07/owl#Restriction> ;
                              <http://www.w3.org/2002/07/owl#cardinality>
                                      "1"^^<http://www.w3.org/2001/XMLSchema#int> ;
                              <http://www.w3.org/2002/07/owl#onProperty>
                                      <http://purl.org/olia/olia.owl#hasParent>
                            ]
                            [ a       <http://www.w3.org/2002/07/owl#Restriction> ;
                              <http://www.w3.org/2002/07/owl#cardinality>
                                      "1"^^<http://www.w3.org/2001/XMLSchema#int> ;
                              <http://www.w3.org/2002/07/owl#onProperty>
                                      <http://purl.org/olia/olia.owl#hasChild>
                            ]
                          )
                ] ;
        <http://www.w3.org/2002/07/owl#versionInfo>
                "TODO: check TDS and GOLD" .

<http://purl.org/olia/olia.owl#VerbalNoun>
        a       <http://www.w3.org/2002/07/owl#Class> ;
        <http://www.w3.org/2000/01/rdf-schema#comment>
                "A verbal noun is a noun formed directly as an inflexion of a verb or a verb stem, sharing at least in part its constructions. \n\t This term is applied especially to gerunds, and sometimes also to infinitives and supines.\n     (http://en.wikipedia.org/wiki/Verbal_noun 19.09.06)\n\t" ;
        <http://www.w3.org/2000/01/rdf-schema#subClassOf>
                <http://purl.org/olia/olia.owl#NonFiniteVerb> , <http://purl.org/olia/olia.owl#CommonNoun> ;
        <http://www.w3.org/2002/07/owl#versionInfo>
                "\n\tMissing in EAGLES, added as subclass of Verb and Noun in accordance with the SFB632 annotation guidelines:\n\n   VN verbal noun (§4.3.12.2):\n   Some of the Chadic\n   languages have morphologically opaque verbal noun stems in\n   the progresive aspect, i.e. it is not obvious from the morphology that\n   we deal with a deverbal noun, instead of a verb proper. In such cases,\n   use the tag VN.\n\t" .

<http://purl.org/olia/olia.owl#GoalRole>
        a       <http://www.w3.org/2002/07/owl#Class> ;
        <http://www.w3.org/2000/01/rdf-schema#comment>
                "\n\t\t\tA goal role instantiates the (intended) end location (directional path) of an event.\n\t\t\t(http://languagelink.let.uu.nl/tds/onto/LinguisticOntology.owl#goalRole)\n\t\t" ;
        <http://www.w3.org/2000/01/rdf-schema#subClassOf>
                <http://purl.org/olia/olia-top.owl#SemanticRole> ;
        <http://www.w3.org/2002/07/owl#versionInfo>
                "http://languagelink.let.uu.nl/tds/onto/LinguisticOntology.owl#goalRole" .

<http://purl.org/olia/hasSemanticRole>
        a       <http://www.w3.org/2002/07/owl#ObjectProperty> ;
        <http://www.w3.org/2000/01/rdf-schema#range>
                <http://purl.org/olia/olia-top.owl#SemanticRole> ;
        <http://www.w3.org/2000/01/rdf-schema#subPropertyOf>
                <http://purl.org/olia/system.owl#hasFeature> .

<http://purl.org/olia/olia.owl#Acronym>
        a       <http://www.w3.org/2002/07/owl#Class> ;
        <http://www.w3.org/2000/01/rdf-schema#comment>
                "\n      An acronym is an abbreviation, such as NATO, laser, and ABC, written as the initial \n      letter or letters of words, and pronounced on the basis of this abbreviated written \n      form. Acronyms are used most often to abbreviate names of organizations and long or \n      frequently referenced terms. \n      (http://en.wikipedia.org/wiki/Acronym 19.09.06)" ;
        <http://www.w3.org/2000/01/rdf-schema#subClassOf>
                <http://purl.org/olia/olia.owl#Residual> ;
        <http://www.w3.org/2002/07/owl#versionInfo>
                "EAGLES category Residual with Type=\"Acronym\"." .

<http://purl.org/olia/olia.owl#ItCleft>
        a       <http://www.w3.org/2002/07/owl#Class> ;
        <http://www.w3.org/2000/01/rdf-schema#comment>
                "-CLF (cleft)\n— marks it-clefts (“true” clefts) and may be added to the labels S, SINV, or SQ. See section 16 [Clefts]. \n\n  (SQ-CLF Was\n          (NP-SBJ it)\n          (NP-PRD (NP John's)\n                  car)\n          (SBAR (WHNP-6 0)\n                (S (NP-SBJ you)\n                   (VP borrowed\n                       (NP *T*-6))))\n          ?)\n(Bies et al. 1995)\n\nS-CLF\n(it-cleft or “true” cleft) \n\nDeclarative it-clefts are labeled S-CLF, expletive it is tagged as the surface subject (-SBJ), the SBAR is attached at VP-level, and a trace is coindexed to the wh-complementizer of the clefted portion. (See section 16 [Clefts] for more information.) \n(Bies et al. 1995)" ;
        <http://www.w3.org/2000/01/rdf-schema#subClassOf>
                <http://purl.org/olia/olia-top.owl#SyntacticConstruction> ;
        <http://www.w3.org/2002/07/owl#versionInfo>
                "PTB bracketing guidelines (Santorini 1991, Bies et al. 1995)" .

<http://purl.org/olia/olia.owl#PersonalPronoun>
        a       <http://www.w3.org/2002/07/owl#Class> ;
        <http://www.w3.org/2000/01/rdf-schema#comment>
                "\n\t\t\tA personal pronoun is a pronoun that expresses a distinction of person deixis. \t\t\n\t\t\t(http://www.sil.org/linguistics/GlossaryOfLinguisticTerms/WhatIsAPersonalPronoun.htm 19.09.06)\n\t\t\t\n\t\t\tNote that (despite the SIL definition), an olia:PersonalPronoun refers to irreflexive personal pronouns. Personal pronoun categories without reflexivity sensitivity should be mapped onto olia:PersReflPronoun. (CC)\n\t\t" ;
        <http://www.w3.org/2000/01/rdf-schema#isDefinedBy>
                "http://www.isocat.org/datcat/DC-3013 (irreflexive personal pronoun)" ;
        <http://www.w3.org/2000/01/rdf-schema#label>
                "irreflexive personal pronoun" , "personal pronoun" , "pronom personnel"@fr ;
        <http://www.w3.org/2000/01/rdf-schema#subClassOf>
                <http://purl.org/olia/olia.owl#PersReflPronoun> ;
        <http://www.w3.org/2002/07/owl#versionInfo>
                "EAGLES PersReflPronoun with \"Special PronounType\"=\"Personal\"." , "TODO: the SIL definition (also used in GOLD) is nonsatisfactory. \n\t\t\tGerman reflexive pronouns have person distinction, so this definition actually\n\t\t\tapplies to EAGLES PersReflPronoun rather than EAGLES PersonalPronoun.\n\t\t" .

<http://purl.org/olia/olia-top.owl#SemanticRole>
        a       <http://www.w3.org/2002/07/owl#Class> ;
        <http://www.w3.org/2000/01/rdf-schema#subClassOf>
                [ a       <http://www.w3.org/2002/07/owl#Restriction> ;
                  <http://www.w3.org/2002/07/owl#hasSelf>
                          true ;
                  <http://www.w3.org/2002/07/owl#onProperty>
                          <http://purl.org/olia/olia.owl#hasSemanticRole>
                ] ;
        <http://www.w3.org/2000/01/rdf-schema#subClassOf>
                [ a       <http://www.w3.org/2002/07/owl#Restriction> ;
                  <http://www.w3.org/2002/07/owl#hasSelf>
                          true ;
                  <http://www.w3.org/2002/07/owl#onProperty>
                          <http://purl.org/olia/olia.owl#hasSemanticRole>
                ] ;
        <http://www.w3.org/2002/07/owl#versionInfo>
                "TODO:\n\t\t\tCheck subcategorization in MacroRoles. Currently, this follows the TDS ontology,\n\t\t\tbut the strict assignment of semantic roles to macroroles contradicts\n\t\t\tthe selection algorithm as described by van Valin and Lapolla (1997):\n\t\t\tMacroRoles are not assigned a priori, but on on the basis of *relative \n\t\t\tagentivity* among the arguments.\n\t\t" , "One may consider modelling SemanticRoles and discourse relations within the same dimension. In particular, the semantics of adverbial modifiers (causal, temporal, 3al, etc.) closely resembles discourse relations." .

<http://purl.org/olia/olia.owl#WHAdjectivePhrase>
        a       <http://www.w3.org/2002/07/owl#Class> ;
        <http://www.w3.org/2000/01/rdf-schema#comment>
                "WHADJP â ´ Wh-adjective Phrase. Adjectival phrase containing a wh-adverb, as in how hot. \n(Bies et al. 1995)" ;
        <http://www.w3.org/2000/01/rdf-schema#subClassOf>
                <http://purl.org/olia/olia.owl#AdjectivePhrase> ;
        <http://www.w3.org/2002/07/owl#versionInfo>
                "added in conformance with PTB bracketing guidelines (Santorini 1991, Bies et al. 1995)" .

<http://purl.org/olia/olia.owl>
        a       <http://www.w3.org/2002/07/owl#Ontology> ;
        <http://www.w3.org/2000/01/rdf-schema#comment>
                "\n\tOLiA Reference Model for Morphology, Morphosyntax and Syntax\n\t(originally \n    based on the EAGLES recommendations, with modifications in accordance to \n    DCR (ISOcat, June 2013), TDS ontology, GOLD v.03, the SFB 632 annotation guidelines, \n    the MULTEXT-East ontology and various annotation schemes)\n\t" ;
        <http://www.w3.org/2002/07/owl#imports>
                <http://purl.org/olia/system.owl> , <http://purl.org/olia/olia-top.owl> ;
        <http://www.w3.org/2002/07/owl#versionInfo>
                "\n\tOct. 2005 created by Christian Chiarcos \n\t2006-2008 maintained by Christian Chiarcos and Angelika Adam \n\tsince 2008 maintained by Christian Chiarcos\n\t10/01/08 updated by Christian Chiarcos \n\t10/01/25 added SyntacticUnit categorization \n\t\t(from GOLD [http://www.linguistics-ontology.org/gold/2008] and EAGLES recommendations \n\t\t[http://www.ilc.cnr.it/EAGLES96/segsasg1/node29.html#SECTION00052000000000000000]) \n    \t10/01/28 removed all owl:disjointWith and owl:complementOf, these are language-specific\n\t\tand have to be represented in a separate language model.\n    \t10/02/17 extended SyntacticUnit categorization in accordance with the TDS ontologies \n\t\t(http://languagelink.let.uu.nl/tds/onto/LinguisticOntology.owl) Christian \n    \t10/02/18 adopted TIGER edge labels as syntactic role and semantic role\n    \t10/03/11 manual restructuring of OWL file begun\n\t10/03/23 morphosyntactic classes revised\n\t10/03/24 CaseFeature extended by TDS grammaticalCase, GOLD CaseValue and DCR case features\n\t\t\tDefinitenessFeature checked against TDS definitenessProperty and DCR (missing in GOLD)\n\t\t\tDegreeFeature checked against DCR (missing in GOLD and TDS)\n\t\t\tTenseFeature extended in accordance with TDS tenseProperty and GOLD TenseValue (DCR not yet)\n\t\t\tGenderFeature checked against TDS case and GOLD GenderValue (DCR not yet)\n\t\t\tSemanticRole extended in accordance with TDS semanticRoleProperty (missing in GOLD, \n\t\t\t\t\tmerged with grammatical case there)\n\t\t\tPersonFeature checked and extended against GOLD and TDS\n\t\t\tMoodFeature extended in accordance with TDS modalityProperty and GOLD MoodValue\n\t\t\tAspectFeature extended in accordance with TDS aspectProperty and GOLD AspectValue\n\t\t\t\tHabitual remodelled as Aspect\n\t10/03/25 SyntacticRole checked and extended against GOLD syntacticRole (properties) \n\t\t\t\tand DCR syntacticCategory, modifyingRelation\n\t\t\tVoiceFeature extended against GOLD VoiceValue and TDS grammaticalVoice\n\t\t\t\thierarchically structured\n\t\t\trestructuring concluded\n\t10/04/06 extended InflectionType, added Countability and Valency as features and properties (in accordance with\n\t\t\tSampson (1995), see susa.owl\n\t10/04/08 extensions with respect to constituent types, syntactic relations and semantic roles \n\t\t\tin accordance with Dipper et al. (2007), see sfb632.owl\n\t10/04/13 extension wrt. the morphosyntactic profile of the DCR (ISOcat, www.isocat.org)\n\t10/04/14 validation, PossessiveFeature removed\n\t10/04/15-18 additions in accordance to the PTB Bracketing Guidelines (Santorini 1991, Bies et al. 1995)\n\t10/11/26 introduced NounHeadedPhrase for improved compatibility with dependency parsing schemes (e.g., Connexor)\n\t10/11/29 added categories for topological fields in German (as used in TüBa-D/Z)\n\t10/12/02 added DeterminerPhrase, ForeignPhrase, subclasses of ExpletivePronoun (TüBa-D/Z)\n\t11/07/29 replaced url http://purl.org/olia with purl http://purl.olcl.org/olia\n\t11/07/31-11/08/04 linking with MULTEXT-East (http://nl.ijs.si/ME/owl/multext-east.owl = http://purl.org/olia/mte/multext-east.owl)\n\t\tClitic deprecated (replaced by CliticElement because of the ambiguity of the category in MULTEXT-East and ISOcat)\n\t\tadditions: hasProximity, Distal, Proximal, CliticElement, CliticDefiniteArticle, SpecificArticle, CliticSpecificArticle,\n\t\thasSpecificity, Specific, Nonspecific, Cliticization, ElementWithClitic, ElementWithoutClitic, ElementDemandingClitic, \n\t\tDistributiveCase, FactiveCase, DirectCase, FormalCase, MultiplicativeCase, TemporalisCase, ElativeDegree, CountNumber, \n\t\tAspectParticle, SubjunctiveParticle, VerbalParticle, LightVerb, VerbalAdverb, NegativeAdverb, ModifierAdverb, AdjectivalAdverb, \n\t\tNonspecificPronoun, DeterminalPronoun, AttributivePronoun, EmphaticDeterminer, NegativeDeterminer, UniquitiveDeterminer, PossessiveArticle,\n\t\thasConjunct, hasWordConjunct, hasSentenceConjunct, RepetitiveCoordinatingConjunction, SubordinatingConjunctionWithNegation,\n\t\tSubordinatingConjunctionWithoutNegation, RelationalAdjective, PossessiveAdjective, NonreducedInflection, ReducedInflection, CollectiveNumeral,\n\t\thasNumeralAgreement, DualQuantifier, PaucalQuantifier, SingularQuantifier, PluralQuantifier, Fraction, ApproximateNumeral, MultipleNumeral,\n\t\tProQuantifier, InterrogativeQuantifier, IndefiniteQuantifier, DemonstrativeQuantifier, RelativeQuantifier, QuotativeVerb, QuotativeMood,\n\t\tNonNegated, Diminuitive, Human, AbbreviatedPronoun, FixedExpression, Adjectival, Typo, Verbal, hasObjectNumber, hasNumeralForm, ExistentialParticle\n\t11/08/04 eliminated redundancy of olia-top:SyntacticRelation and olia:SyntacticRelation\n\t\tSubordType, CoordType deprecated, remodelled as subconcepts of Sub/CoordinatingConjunction\n\t11/08/05 validation\n\t11/08/11 VoiceParticle (from Portuguese EAGLES)\n\t11/08/12 linking with T-CODEX (Old High German)\n\t\t\t VocativeExpression, Fronting, ConditionRole, HangingTopic (for Old High German, T-CODEX)\n\t\t\t CausalAdverb deprecated (= Adverb and hasSemanticRole some CauseRole)\n\t\t\t DeclarativeSentence = Sentence and hasMood some DeclarativeMood\n\t\t\t PresentParticiple (= Sentence and hasTense some Present)\n\t\t\t PastParticiple (= Sentence and hasTense some Past)\n\t11/08/12-15 linking with ILPOSTS (for Indian languages)\n\t\t\tadded PurposiveCase, PurposiveAspect, DistributivePronoun, ConditionalParticiple, ConditionalRealisMood, ConditionalIrrealisMood, PresumptiveMood, Sequel, AbilitativeMood, SecondHonorific, SecondNonHonorific, hasEmphasis, Emphatic, NonEmphatic, SimpleAspect\n\t\t\tEmphaticDeterminer, EmphaticPronoun deprecated\n\t\t\tCausalMood (from Nowak 1996, for Inuktitut)\n\t\t\tMannerAdverb (= Adverb and hasSemanticRole some MannerRole) {introduced as deprecated}\n\t\t\tLocationAdverb (= Adverb and hasSemanticRole some LocationRole) {introduced as deprecated}\n\t\t\tHabitualMood (= HabitualAspect)\n\t11/08/15 olia_top:PhonologicalProcess introduced (reorganization of MorphologicalProcess)\n\t11/08/15 linking with Ancorra and IIIT tagset (for Indian languages)\n\t\t\tGerundVerbPhrase, SpatiotemporalNoun, InfinitiveVerbPhrase, EchoWord, Composition\n\t\t\tIntensifier\n\t11/08/15 linking with Urdu tagset (Sajjad 2007)\n\t\tTitleNoun, UnitNoun, AspectMarkingAuxiliary, TenseMarkingAuxiliary, Date added\n\t11/08/16 linking with EMILLE Urdu tagset (Hardie 2003)\n\t\tAdjectivalParticle, ModalityMarkingAdverb, OpenQuote, CloseQuote, ContrastiveParticle, EmphaticParticle, MultiplicativeMarker, ExclusiveEmphaticParticle, InclusiveEmphaticParticle, ReflexivePossessiveDeterminer, Izafat, RelativeAdjective added\n\t\tContrastiveEmphaticParticle (= ContrastiveParticle and EmphaticParticle)\n\t11/08/16 linking with Dzongkha tagset (Chungku et al. 2010)\n\t\tadded AspirationalVerb, AgentiveVerb, TenseMarkingParticle, NonAgentiveVerb, LocativePronoun, NominalNumber, CaseMarker, PeriodicAdjective, CharacteristicAdjective, DifferentialPronoun, NominalQuantifier\n\t\tHonorificVerb, HonorificCommonNoun added (=> Honorificity to be remodelled)\n\t13/03/03 linking with Uby Pos annotation model (http://www.ukp.tu-darmstadt.de/data/lexical-resources/uby/)\n\t\tadded GivenName, FamilyName, comments for PersonalPronoun, Separability\n\t13/03/03 partial \"hasFeature Self\"-modeling for ...Feature concepts: not inferable through Fact++ or Hermit, though, hence incomplete\n\t13/03/04 linking with Uby Pos annotation model (http://www.ukp.tu-darmstadt.de/data/lexical-resources/uby/)\n\t\tContraction, Phraseme, LexicalUnit (as generalization over Phraseme and Lexeme), Initialism\n\t13/03/04 olia-top:XYFeature olia:hasXY Self for most XYFeatures\n\t13/06/24 additions from ISOcat morphosyntactic profile: FusedPrepositionPronoun, ElativeNoun, InterrogativeMultiplicativeQuantifier, FocusMarker, AdjutativeVoice, AversiveCase\n\t13/06/25 additions from ISOcat morphosyntactic profile: VisualEvidentiality, OtherSourceEvidentiality, DeductiveEvidentiality, Exclusive, Inclusive, Homonym, Homophone, CircumstantialVoice\n\t13/06/27 ISOcat additions: MannerNoun (deprecated), QuestionWord (extended to be a generalization over InterrogativeXY, deprecated), GeneralizationWord, EpistemicPossibilityModality, DebitiveMood, InchoativeAspect, PresentativePronoun, IndefiniteCardinalQuantifier, NumeralBoth (deprecated), GraphicalSeparator, Impossible, Possible, EpistemicNecessityModality, TemporallyDefinedUsage, PrepositionalAdverb, DeclarativePunctuation, Multal, ObligativeModality, RomanNumeral, DigitNumeral, Script, ParticleAdverb (deprecrated), ApplicativeVoice, EvaluativeModality, PlaceNoun (deprecated), String [generalized as orthographical anchor point for RomanNumeral]\n\t13/06/28 ISOcat additions: Masdar, Ideophone, DeficientVerb (deprecated), IndefiniteMultiplicativeQuantifier, PermissiveModality, WeakObligativeModality, ExistentialPronoun (deprecated), InstrumentNoun, PhysicalAbilitiveModality, MedioPassiveVoice, InterrogativeCardinalQuantifier, CompletiveAspect, PseudopassiveVoice, LetterNumeral, ContextualVariation, Homograph, CollectivePronoun, PossessiveRelativePronoun, ExpansionVariation, CausativeVoice, Augmentative, FusedPronounAuxiliary, AntiCausativeVoice, StatusConstructus, PreferredEvaluative, PejorativeEvaluative, CommissiveForce, ActionalForce, VolitiveForce\n\t\thasEvaluativeFeature (for ISOcat PreferredEvaluative and PejorativeEvaluative), HortativeModality (from GOLD, missing in the corresponding ISOcat export)\n\t\tdisentangled Modality and Mood: for every Mood, created a corresponding Modality as superclass; XYMood is subconcept of Mood and XYModality concept, hasMood only for Mood, hasModality for Modality\t\n\t16/04/18 selected French labels for the Bambara Reference Corpus (BRC)\n\t\tadded OnomatopoeticWord, QualitativeVerb, PredicativeMarker\n\tOWL/DL validation\n\t16/08/29 added Frame, hasMovementFeature, Control and Raising for compliance with lexinfo\n\t17/06/26 fixed occasional type errors at owl:deprecated\n\t18/01/08 added Converb (for Eastern Armenian National Corpus)\n\t\nChristian Chiarcos chiarcos@informatik.uni-frankfurt.de\n\t" , "TODO: simplify {Interrogative,Indefinite,...}/{Cardinal,Multiplicative,...}Quantifier dichothomies\n\tIn subsequent versions, however, orthographical definitions should be handled with existing ontologies specializing on the description on language, e.g., lexvo\n\tcheck gerundive vs. gerund\n\tupdate GOLD linking\n\t" .

<http://purl.org/olia/olia.owl#PredicativeMarker>
        a       <http://www.w3.org/2002/07/owl#Class> ;
        <http://www.w3.org/2000/01/rdf-schema#comment>
                "no definition given" ;
        <http://www.w3.org/2000/01/rdf-schema#label>
                "marque predicative"@fr , "predicative marker"@en ;
        <http://www.w3.org/2000/01/rdf-schema#subClassOf>
                <http://purl.org/olia/olia.owl#VerbalParticle> ;
        <http://www.w3.org/2002/07/owl#versionInfo>
                "adopted from Bambara Reference Corpus, http://cormand.huma-num.fr/gloses.html" .

<http://purl.org/olia/olia.owl#HonorificVerb>
        a       <http://www.w3.org/2002/07/owl#Class> ;
        <http://www.w3.org/2000/01/rdf-schema#comment>
                "Dzongkha uses honorific forms: ན་བཟའ་/nam za/\n\t\t\t(cloths) is the honorific form of the noun གོ་\n\t\t\tལ་/gola/(cloths), གསངས་/sung/(tell) the honorific\n\t\t\tform of the verb སབ་/lab/(tell). We opted to mark\n\t\t\tthem by adding the tag NNH (honorific\n\t\t\tcommon noun) and VBH (honorific verb) to\n\t\t\tenable future research on this specific usage of\n\t\t\tDzongkha language. A number of tags were\n\t\t\tadded to the set, of which we describe four in\n\t\t\tmore detail: two of the additional tags are subclasses\n\t\t\tof verbs: VBH (honorific verb form),\n\t\t\tand VBN which describes past participle forms,\n\t\t\tlike, e.g. བངམ་/jun/(created), the past particle\n\t\t\tform of བང་/jung/(create)." ;
        <http://www.w3.org/2000/01/rdf-schema#subClassOf>
                <http://purl.org/olia/olia.owl#MainVerb> ;
        <http://www.w3.org/2002/07/owl#versionInfo>
                "adopted from Dzongkha tagset (Chungku et al. 2010, http://purl.org/olia/dzongkha.owl#HonorificVerb)" .

<http://purl.org/olia/olia.owl#NeutralRegister>
        a       <http://www.w3.org/2002/07/owl#Class> ;
        <http://www.w3.org/2000/01/rdf-schema#comment>
                "\n                            The register appropriate to general texts or discourse.\n                                (ISO12620; http://www.isocat.org/datcat/DC-1999)\n                            " ;
        <http://www.w3.org/2000/01/rdf-schema#label>
                "neutral register" , "standard register" ;
        <http://www.w3.org/2000/01/rdf-schema#subClassOf>
                <http://purl.org/olia/olia-top.owl#RegisterFeature> ;
        <http://www.w3.org/2002/07/owl#versionInfo>
                "subClassOf register (dcif:conceptualDomain)" , "http://www.isocat.org/datcat/DC-1999" .

<http://purl.org/olia/olia.owl#ExclamatoryPronoun>
        a       <http://www.w3.org/2002/07/owl#Class> ;
        <http://www.w3.org/2000/01/rdf-schema#comment>
                "\n\t\t\tAn exclamative pronoun is a word which marks an exclamation.\n\t\t\t(http://www.sil.org/linguistics/GlossaryOfLinguisticTerms/WhatIsAnExclamative.htm 19.09.06)\n\t\t" ;
        <http://www.w3.org/2000/01/rdf-schema#subClassOf>
                <http://purl.org/olia/olia.owl#WHPronoun> ;
        <http://www.w3.org/2002/07/owl#versionInfo>
                "EAGLES WHPronoun with Wh-Type=\"Exclamatory\"." .

<http://purl.org/olia/olia.owl#FactiveCase>
        a       <http://www.w3.org/2002/07/owl#Class> ;
        <http://www.w3.org/2000/01/rdf-schema#comment>
                "case category of the Hungarian MULTEXT-East scheme, e.g., amilyenné/amilyen, azzá/az, erőddé/erő, jelmezeivé/jelmez, jelükké/jel, kevéssé/kevés, Kissé/Kiss, legjelentéktelenebbekké/jelentéktelen (hu)\n\t\t\t(http://purl.org/olia/mte/multext-east.owl#FactiveCase)" ;
        <http://www.w3.org/2000/01/rdf-schema#subClassOf>
                <http://purl.org/olia/olia-top.owl#CaseFeature> ;
        <http://www.w3.org/2002/07/owl#versionInfo>
                "http://purl.org/olia/mte/multext-east.owl#FactiveCase" .

<http://purl.org/olia/olia.owl#EssiveCase>
        a       <http://www.w3.org/2002/07/owl#Class> ;
        <http://www.w3.org/2000/01/rdf-schema#comment>
                "\n\t\t\tEssiveCase expresses that  the referent of the noun it marks is the \n\t\t\tlocation at which another referent exists (Lyons 1968: 299,301; Gove, \n\t\t\tet al. 1966: 778; Crystal 1985: 112; Blake 1994: 154-5).\n\t\t\t(http://purl.org/linguistics/gold/Essive)\n\t\t" ;
        <http://www.w3.org/2000/01/rdf-schema#subClassOf>
                <http://purl.org/olia/olia-top.owl#CaseFeature> ;
        <http://www.w3.org/2002/07/owl#versionInfo>
                "http://purl.org/linguistics/gold/Essive, http://www.isocat.org/datcat/DC-1281" .

<http://purl.org/olia/olia.owl#SubordinatingConjunctionWithFiniteClause>
        a       <http://www.w3.org/2002/07/owl#Class> ;
        <http://www.w3.org/2000/01/rdf-schema#comment>
                "\n\t\t\tFor example, in German the subordinating conjunction \"weil\" introduces \n\t\t\ta clause with a finite verb. \n\t\t\t(http://www.ilc.cnr.it/EAGLES96/annotate/node19.html#oav2u  17.11.06)\n\t\t" ;
        <http://www.w3.org/2000/01/rdf-schema#subClassOf>
                <http://purl.org/olia/olia.owl#SubordinatingConjunction> ;
        <http://www.w3.org/2002/07/owl#versionInfo>
                "EAGLES" .

<http://purl.org/olia/olia.owl#ObliqueCase>
        a       <http://www.w3.org/2002/07/owl#Class> ;
        <http://www.w3.org/2000/01/rdf-schema#comment>
                "\n\t\tCase that is used when a noun is the object of a verb or a\n\t\tproposition, except for nominative and vocative case. \n\t\t(http://www.isocat.org/datcat/DC-1336)\n\t\t"@en ;
        <http://www.w3.org/2000/01/rdf-schema#label>
                "oblique case"@en ;
        <http://www.w3.org/2000/01/rdf-schema#subClassOf>
                <http://purl.org/olia/olia-top.owl#CaseFeature> ;
        <http://www.w3.org/2002/07/owl#versionInfo>
                "http://www.isocat.org/datcat/DC-1336; in EAGLES applied to non-subject pronouns in English and Dutch" .

<http://purl.org/olia/olia.owl#Infix>
        a       <http://www.w3.org/2002/07/owl#Class> ;
        <http://www.w3.org/2000/01/rdf-schema#comment>
                "\n                            Affix inserted in the middle of a word to change its meaning or part of speech value.\n                                (Sue Ellen Wright; http://www.isocat.org/datcat/DC-1313)\n                            " ;
        <http://www.w3.org/2000/01/rdf-schema#label>
                "infix" ;
        <http://www.w3.org/2000/01/rdf-schema#subClassOf>
                <http://purl.org/olia/olia.owl#Affix> ;
        <http://www.w3.org/2002/07/owl#versionInfo>
                "http://www.isocat.org/datcat/DC-1313" .

<http://purl.org/olia/olia.owl#Topicalization>
        a       <http://www.w3.org/2002/07/owl#Class> ;
        <http://www.w3.org/2000/01/rdf-schema#comment>
                "Topicalization structures are ones where a non-subject immediately precedes a subject, which\n\t\t\timmediately precedes the verb/auxiliary of the sentence. Two examples:\n\t\t\tPizza, John likes.\n\t\t\tTomorrow, I will go to the store.\n\t\t\tSuch examples should be bracketed as adjunction structures.\n\t\t\t(Santorini 1991)\n\t\t\t\n\t\t\t-TPC (“topicalized”)\n\t\t\t— marks elements that appear before the subject in a declarative sentence, but in two cases only: \n\t\t\t\n\t\t\t(i) if the fronted element is associated with a *T* in the position of the gap.\n\t\t\t\n\t\t\t(ii) if the fronted element is left-dislocated (i.e., it is associated with a resumptive pronoun in the position of the gap). (See the section on fronted elements in section 1 [Overview of Basic Clause Structure] for more details on the treatment of fronted elements and the section on *T* with fronted elements in section 4 [Null Elements] for more details on the distribution of *T*.) \n\t\t\t(Bies et al. 1995)\n\t\t\t\n\t\t\tFronted elements are placed inside the top clause level (e.g. S, SINV, SQ, SBAR). (Only certain fronted elements are tagged -TPC: (i) constituents associated with a *T* in the position of the gap and (ii) left-dislocated constituents (those associated with a resumptive pronoun in the position of the gap).) (See section 1 [Overview of Basic Clause Structure] for more details on the treatment of fronted elements.) \n\t\t\t(Bies et al. 1995)" ;
        <http://www.w3.org/2000/01/rdf-schema#subClassOf>
                <http://purl.org/olia/olia.owl#Fronting> ;
        <http://www.w3.org/2002/07/owl#versionInfo>
                "PTB bracketing guidelines, Bies et al. 1995" .

<http://purl.org/olia/olia.owl#Sentence>
        a       <http://www.w3.org/2002/07/owl#Class> ;
        <http://www.w3.org/2000/01/rdf-schema#comment>
                "\n\t\t\tThe maximal, syntactically independent, segments into which a text is subdivided, \n\t\t\tfor parsing purposes, are normally considered to be sentences. In a written text, \n\t\t\tthey are typically (though by no means invariably) delimited by an initial capital \n\t\t\tletter and a final full stop (`.') or other terminal punctuation. It is convenient \n\t\t\tto accept this primary orthographic definition of `sentence' for the purposes of \n\t\t\tsyntactic annotation. However, a sentence, so defined, may be either a full \n\t\t\tsentence (9) or a `grammatically incomplete' one (10).\n\n\t\t\t(9)  \t[S This is a sentence. S]\n\t\t\t(10)  \t[S Well done. S]\n\n\t\t\tThe same applies to sentences included within other sentences, as in (11)\n\n\t\t\t(11)  \t[S [S ``Well done'', S] she said. S] }\n\t\t\t\n\t\t\t``Well done'' in 11 is labelled as a sentence, since it clearly has an independent \n\t\t\tsyntactic status equivalent to those of 9, even though it is included in another \n\t\t\tsentence. This inclusion of one independent sentence within another is found both \n\t\t\twith reported speech and elsewhere. Phenomena such as those illustrated in 10 are \n\t\t\tby no means exceptional in text corpora.\n\n\t\t\tIn transcriptions of spoken discourse, there is no simple answer to the question \n\t\t\t``What is a sentence?''. Some transcriptions, based on standard orthography, yield \n\t\t\tde facto sentences in the form of units beginning with a capital letter and closing \n\t\t\twith a terminal punctuation mark. For these, there is no problem in recognising the \n\t\t\tprimary sentential segments and delimiting them by [S ... S], even though these \n\t\t\tsegments frequently lack the canonical structure of a complete written sentence. \n\t\t\tMoreover, even in other transcriptions, where the standard orthographic practices of \n\t\t\tsentence delimitation are avoided, it is possible to identify `primary segments' \n\t\t\tanalogous to the written sentence, viz. the primary units into which the transcribed \n\t\t\tdiscourse is divided for parsing purposes. For spoken as well as written language, \n\t\t\tthen, the [S] unit may be retained, although it may be interpreted differently, and \n\t\t\tsome other term, such as `primary segment', may be preferred to `sentence'.\n\n\t\t\tWe conclude by recommending, for the syntactic annotation of any text (including a \n\t\t\ttranscription of spoken language), an exhaustive division of the text into units \n\t\t\tlabelled [S ... S].\n\t\t\t(http://www.ilc.cnr.it/EAGLES96/segsasg1/node30.html#SECTION00052100000000000000)\n\t\t" ;
        <http://www.w3.org/2000/01/rdf-schema#subClassOf>
                <http://purl.org/olia/olia-top.owl#Constituent> ;
        <http://www.w3.org/2002/07/owl#versionInfo>
                "\n\t\t\tEAGLES category Sentence (S), \n\t\t\thttp://purl.org/linguistics/gold/OrthographicSentence\n\t\t" , "\n\t\tTODO: model Sentence as separate concept indepdendently from Constituent (cf. TüBa-DZ \"Root\").\n\t\tBut what would be an appropriate name for that ?\n\t\t" .

<http://purl.org/olia/olia.owl#Copula>
        a       <http://www.w3.org/2002/07/owl#Class> ;
        <http://www.w3.org/2000/01/rdf-schema#comment>
                "\n\t\t\tA copula is an intransitivity verb which links a subject to a noun phrase, \n\t\t\tan adjective or an other constituent which expresses the predicate.\n\t\t\t(http://www.sil.org/linguistics/GlossaryOfLinguisticTerms/WhatIsACopula.htm 19.09.06)\n\t\t" ;
        <http://www.w3.org/2000/01/rdf-schema#label>
                "copule"@fr , "copula"@en ;
        <http://www.w3.org/2000/01/rdf-schema#subClassOf>
                <http://purl.org/olia/olia.owl#AuxiliaryVerb> ;
        <http://www.w3.org/2002/07/owl#versionInfo>
                "\n\t\t\tAdopted from the SFB632 annotation guidelines.\n\t\t\tIn EAGLES, copulas are not distinguished from auxiliaries, hence represented as such here.\n\t\t" .

<http://purl.org/olia/olia.owl#Typo>
        a       <http://www.w3.org/2002/07/owl#Class> ;
        <http://www.w3.org/2000/01/rdf-schema#comment>
                "a mis-typed word" ;
        <http://www.w3.org/2000/01/rdf-schema#subClassOf>
                <http://purl.org/olia/olia.owl#Residual> ;
        <http://www.w3.org/2002/07/owl#versionInfo>
                "http://purl.org/olia/mte/multext-east.owl#Typo" .

<http://purl.org/olia/olia.owl#PossessiveParticle>
        a       <http://www.w3.org/2002/07/owl#Class> ;
        <http://www.w3.org/2000/01/rdf-schema#comment>
                "\n                            Particle expressing ownship.\n                                (http://www.isocat.org/datcat/DC-1895)\n                            " ;
        <http://www.w3.org/2000/01/rdf-schema#label>
                "possessive particle" ;
        <http://www.w3.org/2000/01/rdf-schema#subClassOf>
                <http://purl.org/olia/olia.owl#Particle> ;
        <http://www.w3.org/2002/07/owl#versionInfo>
                "subClassOf particle (dcif:isA)" , "http://www.isocat.org/datcat/DC-1895" .

<http://purl.org/olia/olia.owl#ActionalModality>
        a       <http://www.w3.org/2002/07/owl#Class> ;
        <http://www.w3.org/2000/01/rdf-schema#comment>
                "ActionalForce indicates that the speaker or\n                        hearer is to undertake some action. Actional force subsumes Imperative,\n                        Commissive and Hortatory force." ;
        <http://www.w3.org/2000/01/rdf-schema#isDefinedBy>
                "http://www.isocat.org/datcat/DC-3063" ;
        <http://www.w3.org/2000/01/rdf-schema#label>
                "actional force" ;
        <http://www.w3.org/2000/01/rdf-schema#subClassOf>
                <http://purl.org/olia/olia-top.owl#MoodFeature> .

<http://purl.org/olia/olia.owl#GivenName>
        a       <http://www.w3.org/2002/07/owl#Class> ;
        <http://www.w3.org/2000/01/rdf-schema#comment>
                "\n\t\tIn most European cultures, a given name designates an individual person throughout her/his life span. To distinguish people with the same name but from different families, additional elements have been introduced into name formulas that identify a person's family or ancestry. (CC)\n\t" ;
        <http://www.w3.org/2000/01/rdf-schema#subClassOf>
                <http://purl.org/olia/olia.owl#ProperNoun> ;
        <http://www.w3.org/2002/07/owl#versionInfo>
                "\n\t\tintroduced as generalization over http://purl.org/olia/ubyPos.owl#nounProperFirstName\n\t" .

<http://purl.org/olia/olia.owl#Verb>
        a       <http://www.w3.org/2002/07/owl#Class> ;
        <http://www.w3.org/2000/01/rdf-schema#comment>
                "\n\t\tA verb is a part of speech that usually denotes action (\"bring\", \"read\"), \n\t\toccurrence (\"decompose\", \"glitter\"), or a state of being (\"exist\", \"stand\"). \n\t\tDepending on the language, a verb may vary in form according to many factors, \n\t\tpossibly including its tense, aspect, mood and voice. It may also agree with \n\t\tthe person, gender, and/or number of some of its arguments (subject, object, etc.).\n\t\t(http://en.wikipedia.org/wiki/Verb 19.09.06)\n\t" ;
        <http://www.w3.org/2000/01/rdf-schema#label>
                "verbe"@fr , "verb"@en ;
        <http://www.w3.org/2000/01/rdf-schema#subClassOf>
                <http://purl.org/olia/olia-top.owl#MorphosyntacticCategory> ;
        <http://www.w3.org/2002/07/owl#versionInfo>
                "EAGLES top-level category \"Verb\" (V)" .

<http://purl.org/olia/olia.owl#RaisableSubject>
        a       <http://www.w3.org/2002/07/owl#Class> ;
        <http://www.w3.org/2002/07/owl#deprecated>
                true ;
        <http://www.w3.org/2002/07/owl#equivalentClass>
                [ a       <http://www.w3.org/2002/07/owl#Class> ;
                  <http://www.w3.org/2002/07/owl#intersectionOf>
                          ( <http://purl.org/olia/olia.owl#Raising> <http://purl.org/olia/olia.owl#SyntacticSubject> )
                ] ;
        <http://www.w3.org/2002/07/owl#versionInfo>
                "from http://lemon-model.net/lemon#RaisableSubject, deprecated because this is just a shorthand for Raising and SyntacticSubject" .

<http://purl.org/olia/olia.owl#Symbol>
        a       <http://www.w3.org/2002/07/owl#Class> ;
        <http://www.w3.org/2000/01/rdf-schema#comment>
                "\n      In morphosyntactic annotation schemes, a symbol is a single graphical sign \n      that occurs in a written text with a conventionalized meaning but that\n      does not represent a phoneme (like ordinary characters), an orthogaphic sign (punctuation),\n      or a number. (Christian Chiarcos)\n      \n      Symbols such as alphabetic characters can vary for singular and plural \n      (e.g. How many Ps are there in `psychopath'?), and are in this respect \n      like common nouns. In some languages (e.g. Portuguese) such symbols also have gender. \n      (http://www.ilc.cnr.it/EAGLES96/annotate/node17.html#recr)    \n      " ;
        <http://www.w3.org/2000/01/rdf-schema#subClassOf>
                <http://purl.org/olia/olia.owl#Residual> ;
        <http://www.w3.org/2002/07/owl#versionInfo>
                "EAGLES Category Residual with Type=\"Symbol\"." .

<http://purl.org/olia/olia.owl#hasSubjectNumber>
        a       <http://www.w3.org/2002/07/owl#ObjectProperty> ;
        <http://www.w3.org/2000/01/rdf-schema#comment>
                "\n\t\t\tNumber of the subject of a transitive verb. (By default, this is the meaning of hasNumber).\n\t\t" ;
        <http://www.w3.org/2000/01/rdf-schema#domain>
                [ a       <http://www.w3.org/2002/07/owl#Class> ;
                  <http://www.w3.org/2002/07/owl#intersectionOf>
                          ( <http://purl.org/olia/olia.owl#Verb>
                            [ a       <http://www.w3.org/2002/07/owl#Restriction> ;
                              <http://www.w3.org/2002/07/owl#onProperty>
                                      <http://purl.org/olia/olia.owl#hasSyntacticValency> ;
                              <http://www.w3.org/2002/07/owl#someValuesFrom>
                                      <http://purl.org/olia/olia.owl#Transitive>
                            ]
                          )
                ] ;
        <http://www.w3.org/2000/01/rdf-schema#label>
                "subject number" ;
        <http://www.w3.org/2000/01/rdf-schema#range>
                <http://purl.org/olia/olia-top.owl#NumberFeature> ;
        <http://www.w3.org/2000/01/rdf-schema#subPropertyOf>
                <http://purl.org/olia/olia.owl#hasNumber> ;
        <http://www.w3.org/2002/07/owl#versionInfo>
                "introduced for double agreement of transitive verbs, e.g., in Hungarian, see http://purl.org/olia/mte/multext-east.owl#FirstSgSecondSg" .

<http://purl.org/olia/olia.owl#MorphologicalParticle>
        a       <http://www.w3.org/2002/07/owl#Class> ;
        <http://www.w3.org/2000/01/rdf-schema#comment>
                "added in accordance with TIGER MorphologicalParticle" ;
        <http://www.w3.org/2000/01/rdf-schema#subClassOf>
                <http://purl.org/olia/olia.owl#Morpheme> , <http://purl.org/olia/olia.owl#Token> ;
        <http://www.w3.org/2002/07/owl#equivalentClass>
                [ a       <http://www.w3.org/2002/07/owl#Class> ;
                  <http://www.w3.org/2002/07/owl#intersectionOf>
                          ( <http://purl.org/olia/olia.owl#Morpheme> <http://purl.org/olia/olia.owl#Token> )
                ] ;
        <http://www.w3.org/2002/07/owl#versionInfo>
                "added in accordance with TIGER MorphologicalParticle" .

<http://purl.org/olia/olia.owl#SentenceMedialPunctuation>
        a       <http://www.w3.org/2002/07/owl#Class> ;
        <http://www.w3.org/2000/01/rdf-schema#comment>
                "\n\t\t\tSentenceMedialPunctuation are , ; : - . \n\t\t\t(http://www.ilc.cnr.it/EAGLES96/annotate/node17.html#recv 19.09.06)\n\t\t" ;
        <http://www.w3.org/2000/01/rdf-schema#subClassOf>
                <http://purl.org/olia/olia.owl#SecondaryPunctuation> ;
        <http://www.w3.org/2002/07/owl#versionInfo>
                "added in accordance with a suggestion by Wilson and Leech (1996)" .

<http://purl.org/olia/olia.owl#MannerRole>
        a       <http://www.w3.org/2002/07/owl#Class> ;
        <http://www.w3.org/2000/01/rdf-schema#comment>
                "\n\t\t\tManner applies to constituents that denote how something is carried out.\n\t\t\tAdverbs may also denote manner, however, they are not annotated at any of the\n\t\t\tsyntactic layers.\n\t\t\t(Dipper et al. 2007, §5.3.11)\n\t\t" ;
        <http://www.w3.org/2000/01/rdf-schema#subClassOf>
                <http://purl.org/olia/olia-top.owl#SemanticRole> ;
        <http://www.w3.org/2002/07/owl#versionInfo>
                "added in conformance with the SFB632 annotation scheme (Dipper et al. 2007)" .

<http://purl.org/olia/olia.owl#IronicRegister>
        a       <http://www.w3.org/2002/07/owl#Class> ;
        <http://www.w3.org/2000/01/rdf-schema#comment>
                "\n                            Register for irony.\n                                (12620; http://www.isocat.org/datcat/DC-1994)\n                            " ;
        <http://www.w3.org/2000/01/rdf-schema#label>
                "ironic register" ;
        <http://www.w3.org/2000/01/rdf-schema#subClassOf>
                <http://purl.org/olia/olia-top.owl#RegisterFeature> ;
        <http://www.w3.org/2002/07/owl#versionInfo>
                "subClassOf register (dcif:conceptualDomain)" , "http://www.isocat.org/datcat/DC-1994" .

<http://purl.org/olia/olia.owl#ParticleAdverb>
        a       <http://www.w3.org/2002/07/owl#Class> ;
        <http://www.w3.org/2000/01/rdf-schema#comment>
                "Word that is both an adverb and a particle." ;
        <http://www.w3.org/2000/01/rdf-schema#isDefinedBy>
                "http://www.isocat.org/datcat/DC-1917" ;
        <http://www.w3.org/2000/01/rdf-schema#subClassOf>
                <http://purl.org/olia/olia.owl#Adverb> , <http://purl.org/olia/olia.owl#Particle> ;
        <http://www.w3.org/2002/07/owl#deprecated>
                true ;
        <http://www.w3.org/2002/07/owl#equivalentClass>
                [ a       <http://www.w3.org/2002/07/owl#Class> ;
                  <http://www.w3.org/2002/07/owl#intersectionOf>
                          ( <http://purl.org/olia/olia.owl#Adverb> <http://purl.org/olia/olia.owl#Particle> )
                ] ;
        <http://www.w3.org/2002/07/owl#versionInfo>
                "merely a shorthand for the intersection of Adverb and Particle, hence deprecated" .

<http://purl.org/olia/olia.owl#EmphaticDeterminer>
        a       <http://www.w3.org/2002/07/owl#Class> ;
        <http://www.w3.org/2000/01/rdf-schema#comment>
                "Determiner/Type=\"emphatic\" (Romanian)<br/>\n\t\t\t\t\n\t\t\t\tIn Romanian, there are specific forms for the so-called emphatic determiner, which may accompany both a noun and a personal pronoun: fata însăşi (the girl herself), also ea însăşi (she herself). e.g., \n\t\t\tînsele/însumi, însemi/însumi, însene/însumi, însevă/însumi, înseşi/însumi, înseţi/însumi, însumi, însuşi/însumi, însuţi/însumi \n\t\t\t(http://purl.org/olia/mte/multext-east.owl#EmphaticDeterminer)" ;
        <http://www.w3.org/2000/01/rdf-schema#subClassOf>
                <http://purl.org/olia/olia.owl#Determiner> ;
        <http://www.w3.org/2002/07/owl#deprecated>
                true ;
        <http://www.w3.org/2002/07/owl#equivalentClass>
                [ a       <http://www.w3.org/2002/07/owl#Class> ;
                  <http://www.w3.org/2002/07/owl#intersectionOf>
                          ( <http://purl.org/olia/olia.owl#Determiner>
                            [ a       <http://www.w3.org/2002/07/owl#Restriction> ;
                              <http://www.w3.org/2002/07/owl#onProperty>
                                      <http://purl.org/olia/olia.owl#hasEmphasis> ;
                              <http://www.w3.org/2002/07/owl#someValuesFrom>
                                      <http://purl.org/olia/olia.owl#Emphatic>
                            ]
                          )
                ] ;
        <http://www.w3.org/2002/07/owl#versionInfo>
                "deprecated: merely shorthand for Determiner and hasEmphasis some Emphatic" , "http://purl.org/olia/mte/multext-east.owl#EmphaticDeterminer" .

<http://purl.org/olia/olia.owl#InterrogativeMultiplicativeQuantifier>
        a       <http://www.w3.org/2002/07/owl#Class> ;
        <http://www.w3.org/2000/01/rdf-schema#comment>
                "An interrogative/relative word used to ask about the number of times something happened." ;
        <http://www.w3.org/2000/01/rdf-schema#isDefinedBy>
                "http://www.isocat.org/datcat/DC-3021 (InterrogativeMultiplicativeNumeral)" ;
        <http://www.w3.org/2000/01/rdf-schema#subClassOf>
                <http://purl.org/olia/olia.owl#InterrogativeQuantifier> .

<http://purl.org/olia/olia.owl#WeakObligativeModality>
        a       <http://www.w3.org/2002/07/owl#Class> ;
        <http://www.w3.org/2000/01/rdf-schema#comment>
                "WeakObligativeModality indicates that an agent\n                        is under a moral obligation to perform the action expressed by the predicate\n                        [Bybee, Perkins and Pagliuca 1994: 186-187]." ;
        <http://www.w3.org/2000/01/rdf-schema#isDefinedBy>
                "http://www.isocat.org/datcat/DC-3557" ;
        <http://www.w3.org/2000/01/rdf-schema#subClassOf>
                <http://purl.org/olia/olia.owl#ObligativeModality> .

<http://purl.org/olia/olia.owl#CommonlyUsed>
        a       <http://www.w3.org/2002/07/owl#Class> ;
        <http://www.w3.org/2000/01/rdf-schema#comment>
                "\n                            Said of a term that appears frequently.\n                                (ISO12620; http://www.isocat.org/datcat/DC-1984)\n                            " ;
        <http://www.w3.org/2000/01/rdf-schema#label>
                "commonly used" ;
        <http://www.w3.org/2000/01/rdf-schema#subClassOf>
                <http://purl.org/olia/olia.owl#Possible> ;
        <http://www.w3.org/2002/07/owl#versionInfo>
                "subClassOf frequency (dcif:conceptualDomain)" , "http://www.isocat.org/datcat/DC-1984" .

<http://purl.org/olia/olia.owl#HodiernalFuture>
        a       <http://www.w3.org/2002/07/owl#Class> ;
        <http://www.w3.org/2000/01/rdf-schema#comment>
                "\n\t\t\tHodiernalFutureTense locates the situation in question after the moment \n\t\t\tof utterance within the span culturally defined as 'today' (Comrie 1985: \n\t\t\t86; Bybee, Perkins, and Pagliuca 1994: 247).\n\t\t\t(http://purl.org/linguistics/gold/HodiernalFuture)\n\t\t" ;
        <http://www.w3.org/2000/01/rdf-schema#subClassOf>
                <http://purl.org/olia/olia.owl#Future> ;
        <http://www.w3.org/2002/07/owl#versionInfo>
                "http://purl.org/linguistics/gold/HodiernalFuture, classified as Future here" .

<http://purl.org/olia/olia.owl#hasCountability>
        a       <http://www.w3.org/2002/07/owl#ObjectProperty> ;
        <http://www.w3.org/2000/01/rdf-schema#domain>
                <http://purl.org/olia/olia.owl#Noun> ;
        <http://www.w3.org/2000/01/rdf-schema#range>
                <http://purl.org/olia/olia-top.owl#CountabilityFeature> ;
        <http://www.w3.org/2000/01/rdf-schema#subPropertyOf>
                <http://purl.org/olia/system.owl#hasFeature> .

<http://purl.org/olia/olia.owl#AddresseeRole>
        a       <http://www.w3.org/2002/07/owl#Class> ;
        <http://www.w3.org/2000/01/rdf-schema#comment>
                "-VOC (vocative)\n— marks nouns of address, regardless of their position in the sentence. It is not coindexed to the subject and does not get -TPC when it is sentence-initial. \n\n  (SQ (NP-VOC Mike)\n      ,\n      would\n      (NP-SBJ you)\n      (INTJ please)\n      (VP close\n          (NP the door))\n      ?)\n(Bies et al. 1995)" ;
        <http://www.w3.org/2000/01/rdf-schema#subClassOf>
                <http://purl.org/olia/olia-top.owl#SemanticRole> ;
        <http://www.w3.org/2002/07/owl#versionInfo>
                "added in conformance with PTB vocative, Bies et al. 1995" .

<http://purl.org/olia/olia.owl#StrictAuxiliaryVerb>
        a       <http://www.w3.org/2002/07/owl#Class> ;
        <http://www.w3.org/2000/01/rdf-schema#comment>
                "\n\t\t\tNon-modal, non-copular auxiliary verb.\n\t\t" ;
        <http://www.w3.org/2000/01/rdf-schema#subClassOf>
                <http://purl.org/olia/olia.owl#AuxiliaryVerb> ;
        <http://www.w3.org/2002/07/owl#versionInfo>
                "\n\t\t\tDefinition in accordance with the SFB632 definition of \"auxiliary verb\" as non-copular and non-modal verb.\n\t\t\tIn EAGLES, auxiliary verb also seems to be non-modal:\n\t\t\t\tIn addition to main and auxiliary verbs, it may be useful (e.g. in English) to recognise an intermediate \n\t\t\t\tcategory of semi-auxiliary for such verbs as be going to, have got to, ought to.\n\t\t\t\t(http://www.ilc.cnr.it/EAGLES96/annotate/node18.html#oav1v 20.09.06)\n\t\t" .

<http://purl.org/olia/olia.owl#DirectObject>
        a       <http://www.w3.org/2002/07/owl#Class> ;
        <http://www.w3.org/2000/01/rdf-schema#comment>
                "\n\t\tA direct object is a grammatical relation that exhibits a combination of certain \n\t\tindependent syntactic properties, such as the following:  the usual grammatical \n\t\tcharacteristics of the patient of typically  transitive verbs; particular case \n\t\tmarking; a particular clause  position; the conditioning of an agreement  affix \n\t\ton the verb; the capability of becoming the clause subject in  passivization; the\n\t\tcapability of reflexivization. The identification of the direct object relation \n\t\tmay be further confirmed by finding significant overlap with similar direct object \n\t\trelations previously established in other languages. This may be done by analyzing \n\t\tcorrespondence between  translation equivalents (Crystal 1985: 94; Hartmann and \n\t\tStork 1972: 155; Mish et al. 1990: 358; Comrie 1989: 66; Andrews, Avery 1985: \n\t\t68,120,126; Comrie 1985a: 337).\n\t\t(http://purl.org/linguistics/gold/directObject)\n\t\t" ;
        <http://www.w3.org/2000/01/rdf-schema#subClassOf>
                <http://purl.org/olia/olia.owl#SyntacticObject> ;
        <http://www.w3.org/2002/07/owl#versionInfo>
                "\n\t\t\thttp://purl.org/linguistics/gold/directObject,\n\t\t\thttp://www.isocat.org/datcat/DC-1274\n\t\t" .

<http://purl.org/olia/olia.owl#Specific>
        a       <http://www.w3.org/2002/07/owl#Class> ;
        <http://www.w3.org/2000/01/rdf-schema#comment>
                "\"By ʻspecificʼ and ʻnon-specificʼ I intend the difference between the\n\t\t\ttwo readings of English indefinites like (3):\n\t\t\t\n\t\t\t(3) Iʼm looking for a deer.\n\t\t\t\n\t\t\tIn the specific reading there is a particular deer, say Bambi, that I am\n\t\t\tlooking for. In the non-specific reading I will be happy to find any deer.\n\t\t\tVon Heusinger (2002) likes the test in English of inserting ʻcertainʼ after the\n\t\t\tʻaʼ to fix the specific reading. In either reading of (3) a deer is being\n\t\t\tintroduced as a new discourse referent. This is opposed to ʻdefiniteʼ which\n\t\t\trequires a previous pragmatic instantiation as in ʻIʼm looking for the deer.ʼ\n\t\t\tIn English both the readings of (3) are indefinite. In Klallam, the specific\n\t\t\tdemonstratives are neither definite nor indefinite.\"\n\t\t\t(Montler, Timothy. 2007. Klallam demonstratives. Papers ICSNL XLVII. The 42nd International Conference on Salish and Neighbouring Language, pp. 409-425. University of British Columbia Working Papers in Linguistics, Volume 20; on specific vs. nonspecific determiners in Klallam, a Salish language, http://montler.net/papers/KlallamDemons.pdf)\n\t\t" ;
        <http://www.w3.org/2000/01/rdf-schema#subClassOf>
                <http://purl.org/olia/olia-top.owl#SpecificityFeature> ;
        <http://www.w3.org/2002/07/owl#versionInfo>
                "http://purl.org/olia/mte/multext-east.owl#CliticSpecificDeterminer" .

<http://purl.org/olia/olia.owl#Causative>
        a       <http://www.w3.org/2002/07/owl#Class> ;
        <http://www.w3.org/2000/01/rdf-schema#comment>
                "\n\t\t\tExpressing the causation of an action.\n\t\t\t(http://purl.org/linguistics/gold/Causative)\n\t\t" ;
        <http://www.w3.org/2000/01/rdf-schema#subClassOf>
                <http://purl.org/olia/olia.owl#ActiveVoice> ;
        <http://www.w3.org/2002/07/owl#versionInfo>
                "TODO: rename to CausativeVoice" , "http://purl.org/linguistics/gold/Causative, cf. Anticausative" .

<http://purl.org/olia/olia.owl#InstrumentalCase>
        a       <http://www.w3.org/2002/07/owl#Class> ;
        <http://www.w3.org/2000/01/rdf-schema#comment>
                "\n\t\t\tInstrumentalCase indicates that the referent of the noun it marks is the means of the accomplishment \n\t\t\tof the action expressed by the clause\n\t\t\t(http://purl.org/linguistics/gold/Instrumental)\n\t\t" ;
        <http://www.w3.org/2000/01/rdf-schema#subClassOf>
                <http://purl.org/olia/olia-top.owl#CaseFeature> ;
        <http://www.w3.org/2002/07/owl#versionInfo>
                "\n\t\t\tTDS Ontology, http://languagelink.let.uu.nl/tds/onto/LinguisticOntology.owl#instrumentalCase-grammatical;\n\t\t\tGOLD, http://purl.org/linguistics/gold/Instrumental;\n\t\t\thttp://www.isocat.org/datcat/DC-1316\n\t\t" .

<http://purl.org/olia/olia.owl#CorrelativeCoordinatingConjunction>
        a       <http://www.w3.org/2002/07/owl#Class> ;
        <http://www.w3.org/2000/01/rdf-schema#comment>
                "Conjunction/Coord_Type=\"correlat\" (Romanian).\t\t\t\n\t\t\tIn Romanian, there are three kinds of conjunctions depending on their usage: as such or together with other conjunctions or adverbs: (1) simple, between conjuncts: Ion ori Maria (John or Mary); (2) repetitive, before each conjunct: fie Ion fie Maria fie... (either John or Mary or...) (3) correlative, before a conjoined phrase, it requires specific coordinators between conjuncts: atât mama cât şi tata (both mother and father). (MTE v4, http://purl.org/olia/mte/multext-east.owl#CorrelativeCoordinatingConjunction)\n\t\t" , "\n\t\t\tWhen the same word is also placed before the first conjunct, as in French \n\t\t\t\"ou...ou...\", the former occurrence is given the Correlative value and the\n\t\t\tlatter the Simple value. \n\t\t\t(http://www.ilc.cnr.it/EAGLES96/annotate/node18.html#oav1av  17.11.06)\n\t\t" ;
        <http://www.w3.org/2000/01/rdf-schema#subClassOf>
                <http://purl.org/olia/olia.owl#CoordinatingConjunction> ;
        <http://www.w3.org/2002/07/owl#versionInfo>
                "EAGLES, http://purl.org/olia/mte/multext-east.owl#CorrelativeCoordinatingConjunction" .

<http://purl.org/olia/olia.owl#Present>
        a       <http://www.w3.org/2002/07/owl#Class> ;
        <http://www.w3.org/2000/01/rdf-schema#comment>
                "\n\t\t\tPresent tense refers to the moment of utterance.\n\t\t\t(http://languagelink.let.uu.nl/tds/onto/LinguisticOntology.owl#presentTense)\n\t\t\n\t\t\tPresent tense refers to the moment of utterance. \n\t\t\tIt often refers to events or states that do not merely coincide \n\t\t\twith the moment of utterance, such as those that are continuous, \n\t\t\thabitual, or lawlike. \n\t\t\t(http://www.sil.org/linguistics/glossaryoflinguisticterms/WhatIsPresentTense.htm  17.11.06)\n\t\t" ;
        <http://www.w3.org/2000/01/rdf-schema#subClassOf>
                <http://purl.org/olia/olia.owl#AbsoluteTense> ;
        <http://www.w3.org/2002/07/owl#versionInfo>
                "EAGLES, http://languagelink.let.uu.nl/tds/onto/LinguisticOntology.owl#presentTense" .

<http://purl.org/olia/olia.owl#ConditionalVerb>
        a       <http://www.w3.org/2002/07/owl#Class> ;
        <http://www.w3.org/2000/01/rdf-schema#comment>
                "\n\t\t\tA conditional verb is a verb form in many languages. It is used \n\t\t\tto express degrees of certainty or uncertainty and hypothesis \n\t\t\tabout past, present, or future. Such forms often occur in \n\t\t\tconditional sentences.\n\t\t\t(http://en.wikipedia.org/wiki/Conditional_mood 19.09.06)\n\t\t" ;
        <http://www.w3.org/2000/01/rdf-schema#subClassOf>
                <http://purl.org/olia/olia.owl#FiniteVerb> ;
        <http://www.w3.org/2002/07/owl#versionInfo>
                "TODO: reimplement with properties" , "\n\t\t\tEAGLES finite verb with VerbForm=\"Conditional\".\n\t\t" .

<http://purl.org/olia/olia.owl#NounPhrase>
        a       <http://www.w3.org/2002/07/owl#Class> ;
        <http://www.w3.org/2000/01/rdf-schema#comment>
                "\n\t\t\tAt phrase level, the noun phrase is probably the least problematic of the categories to be dealt \n\t\t\twith. In general, a noun phrase will a have noun or a pronoun as its head, and included within \n\t\t\tthe noun phrase are the determinative elements, any premodification, and any postmodification. \n\t\t\tThe examples below, 14 to 17 show noun phrases with the head noun/pronoun in bold:\n\n\t\t\t(14)  \t[NP He NP] was a tiny man\n\t\t\t(15)  \t[NP his white shirt cuffs NP]\n\t\t\t(16)  \t[NP his surprisingly thick and hairy wrists NP]\n\t\t\t(17)  \t[NP some wholly unanticipated but remotely possible event of absorbing interest NP]\n\n\t\t\tHowever, noun phrases may also occur with adjectival heads, as in 18 and 19:\n\n\t\t\t(18)  \t[NP The unemployed NP] have had enough\n\t\t\t(19)  \tWe've beaten [NP the best NP]\n\n\t\t\tor with a head which is a cardinal or ordinal number, as in 20 and 21:\n\n\t\t\t(20)  \t[NP The ninth NP] is my particular favourite\n\t\t\t(21)  \t[NP The other seven NP] continued with the trip\n\t\t\t\n\t\t\tIn `pro-drop' languages, such as Spanish and Italian, pronominal Subjects are usually not expressed. \n\t\t\tDepending on the chosen type of analysis, this may require another definition of noun phrase, in order \n\t\t\tto include `empty noun phrases', in which the pronoun is not actually present, but may be inferred \n\t\t\tfrom the verb ending.\n\n\t\t\tA classic constituency test for Noun Phrases is that only whole NPs can be moved within the same sentence. \n\t\t\tIn English, constituents can be preposed to achieve some effect, as in 23 (from Radford 1988: 70):\n\n\t\t\t(22)  \tI can't stand your elder sister\n\t\t\t(23)  \tYour elder sister I can't stand (though your brother's OK).\n\t\t\t\n\t\t\tExamples 24 and 25 show that it is not possible to move only part of the NP:\n\n\t\t\t(24)  \t*Your elder I can't stand sister\n\t\t\t(25)  \t*Elder sister, I can't stand your\n\n\t\t\tHowever, this test should be used with caution. It works well in English, but not always in other languages. \n\t\t\tFor example, in 26 Neue Bücher is moved to the beginning of the sentence while keine is left at the end:\n\n\t\t\t(26) \tNeue\tBücher\thabe\tich\tkeine\n\t\t\t\t\tnew\tbooks\thave\tI\tno\n\t\t\t\t\t`I have not got any new books'\n\t\t\t(http://www.ilc.cnr.it/EAGLES96/segsasg1/node32.html)\n\t\t" , "\n\t\t\tNounPhrase is the class of phrases that have nouns as heads. They can play the role of subject \n\t\t\tin a main clause.\n\t\t\t(http://purl.org/linguistics/gold/NounPhrase)\n\t\t" ;
        <http://www.w3.org/2000/01/rdf-schema#subClassOf>
                <http://purl.org/olia/olia.owl#NounHeadedPhrase> .

<http://purl.org/olia/olia.owl#WeakPersonalPronoun>
        a       <http://www.w3.org/2002/07/owl#Class> ;
        <http://www.w3.org/2000/01/rdf-schema#comment>
                "\n                            Personal pronoun that cannot occupy the position after a preposition and/or reinforce a strong personal pronoun.\n                                (http://www.isocat.org/datcat/DC-1414)\n                            " ;
        <http://www.w3.org/2000/01/rdf-schema#label>
                "weak personal pronoun" ;
        <http://www.w3.org/2000/01/rdf-schema#subClassOf>
                <http://purl.org/olia/olia.owl#PersonalPronoun> ;
        <http://www.w3.org/2002/07/owl#versionInfo>
                "http://www.isocat.org/datcat/DC-1414" , "subClassOf personalPronoun (dcif:isA)" .

<http://purl.org/olia/olia.owl#Raising>
        a       <http://www.w3.org/2002/07/owl#Class> ;
        <http://www.w3.org/2000/01/rdf-schema#comment>
                "Control indicates how a an argument from a main clause will be utilized in a subclause. Control includes both control structures and raising structures of verbs/clauses (see Control). As opposed to this, the OLiA Raising class pertains to raisable/raised arguments, cf. http://www.lexinfo.net/ontology/2.0/lexinfo#RaisableArgument"@en ;
        <http://www.w3.org/2000/01/rdf-schema#subClassOf>
                <http://purl.org/olia/olia-top.owl#MovementFeature> ;
        <http://www.w3.org/2002/07/owl#versionInfo>
                "http://www.lexinfo.net/ontology/2.0/lexinfo#RaisableArgument" .

<http://purl.org/olia/olia.owl#SubordinateClause>
        a       <http://www.w3.org/2002/07/owl#Class> ;
        <http://www.w3.org/2000/01/rdf-schema#comment>
                "\n\t\t\tSubordinateClause is the class of clauses that cannot stand on their \n\t\t\town as sentences. A matrix clause combined with a subordinate clause \n\t\t\tform a main clause. In the sentence 'John thinks that Mary is sick', \n\t\t\t'Mary is sick' is the subordinate clause.\n\t\t\t(http://purl.org/linguistics/gold/SubordinateClause)\n\n\t\t\tDependent clauses (which are also sometimes referred to as subordinate \n\t\t\tclauses) cannot stand alone as sentences. They usually begin with \n\t\t\tsubordinating conjunctions. A sentence with an independent clause and \n\t\t\tany number of dependent clauses is referred to as a complex sentence. \n\t\t\tOne with two or more independent clauses and any number of dependent \n\t\t\tclauses is referred to as a compound-complex sentence \n\t\t\t(http://en.wikipedia.org/wiki/Clause, cf. \n\t\t\thttp://languagelink.let.uu.nl/tds/onto/LinguisticOntology.owl#subordinateClause).\n\n\t\t\tA subordinate clause is an embedded construction which contains a finite verb form. \t\t\t\n\t\t\t(http://languagelink.let.uu.nl/tds/onto/LinguisticOntology.owl#finiteEmbeddedConstruction)\n\t\t" ;
        <http://www.w3.org/2000/01/rdf-schema#subClassOf>
                <http://purl.org/olia/olia.owl#FiniteClause> ;
        <http://www.w3.org/2002/07/owl#versionInfo>
                "\n\t\t\tSubclassification here follows the functional subclassification \n\t\t\tof subordinate clauses in the TDS ontologies. GOLD proposes an \n\t\t\talternative syntax-based subclassification (yet without documentation \n\t\t\tor explanation) in AdjunctSubordinate and ComplementSubordinate. \t\t\n\t\t\t(http://purl.org/linguistics/gold/ComplementSubordinate, \n\t\t\thttp://purl.org/linguistics/gold/AdjunctSubordinate)\n\t\t" .

<http://purl.org/olia/olia.owl#EssiveFormalCase>
        a       <http://www.w3.org/2002/07/owl#Class> ;
        <http://www.w3.org/2000/01/rdf-schema#comment>
                "\n\t\t\tThe Hungarian \"formativus, or essivus-formalis `-ként' ... usually expresses a position, task and manner of the person or the thing.\" (Nose 2003), e.g., Hungarian 'katonaként' -> [serves] as a soldier. (Csaba Oravecz, email 2010/06/15)<br/><br/>\n\t\t\t\n\t\t\t\"Haspelmath & Buchholz (1998:321) explained the function of the essive case as ``role phrases''. Role phrases represent the role of the function in which a participant appears. They regard the role phrases as adverbial.\"\n\t\t\t(Nose 2003, p. 117)<br/>\n\t\t\t\n\t\t\tIn the Hungarian language this case combines the Essive case and the Formal case, and it can express the position, task, state (e.g. \"as a tourist\"), or the manner (e.g. \"like a hunted animal\"). The status of the suffix -ként in the declension system is disputed for several reasons. First, in general, Hungarian case suffixes are absolute word-final, while -ként permits further suffixation by the locative suffix -i. Second, most Hungarian case endings participate in vowel harmony, while -ként does not. For these reasons, many modern analyses of the Hungarian case system, starting with László Antal's \"A magyar esetrendszer\" (1961) do not consider the essive/formal to be a case.\n\t\t\t(http://en.wikipedia.org/wiki/Essive-formal_case)<br/>\n\t\t\t\n\t\t\tcf. Masahiko Nose (2003), Adverbial Usage of the Hungarian Essive Case" ;
        <http://www.w3.org/2000/01/rdf-schema#subClassOf>
                <http://purl.org/olia/olia-top.owl#CaseFeature> ;
        <http://www.w3.org/2002/07/owl#versionInfo>
                "http://purl.org/olia/mte/multext-east.owl#EssiveFormalCase" .

<http://purl.org/olia/olia.owl#hasEmphasis>
        a       <http://www.w3.org/2002/07/owl#ObjectProperty> ;
        <http://www.w3.org/2000/01/rdf-schema#range>
                <http://purl.org/olia/olia-top.owl#EmphasisFeature> ;
        <http://www.w3.org/2000/01/rdf-schema#subPropertyOf>
                <http://purl.org/olia/system.owl#hasFeature> .

<http://purl.org/olia/olia.owl#Phraseme>
        a       <http://www.w3.org/2002/07/owl#Class> ;
        <http://www.w3.org/2000/01/rdf-schema#comment>
                "Conventional lexical unit consisting of a particular phrase (CC)" ;
        <http://www.w3.org/2000/01/rdf-schema#subClassOf>
                <http://purl.org/olia/olia.owl#FixedExpression> ;
        <http://www.w3.org/2002/07/owl#equivalentClass>
                [ a       <http://www.w3.org/2002/07/owl#Class> ;
                  <http://www.w3.org/2002/07/owl#intersectionOf>
                          ( <http://purl.org/olia/olia.owl#LexicalUnit> <http://purl.org/olia/olia.owl#Phrase> )
                ] ;
        <http://www.w3.org/2002/07/owl#versionInfo>
                "http://purl.org/olia/ubyPos.owl#phraseme, no definition there" .

<http://purl.org/olia/olia.owl#CollectiveNumeral>
        a       <http://www.w3.org/2002/07/owl#Class> ;
        <http://www.w3.org/2000/01/rdf-schema#comment>
                "e.g., czworga/czworo, czworgiem/czworo, czworgu/czworo, czworo/czworo, dwoje/dwoje, dwojga/dwoje, dwojgiem/dwoje, dwojgu/dwoje, jedenaścioro/jedenaścioro (pl, http://purl.org/olia/mte/multext-east.owl#CollectiveNumeral)" , "e.g., dvadesetora/dvadesetoro, dvoja/dvoje, dvoje, dvoji/dvoje, dvojih/dvoje, dvojim/dvoje, oboje, tridesetora/tridesetoro, troja/troje (sr, http://purl.org/olia/mte/multext-east.owl#CollectiveNumeral)" , "e.g., ambelor/ambii, ambilor/ambii, amânduror/amândoi, amândurora/amândoi, câteşipatru, tuspatru (ro, http://purl.org/olia/mte/multext-east.owl#CollectiveNumeral)" , "e.g., обата, обајцата, обете, шеесетминава/шеесетмина, шеесетминана/шеесетмина, шеесетмината/шеесетмина, шеснаесетминава/шеснаесетмина, шеснаесетминана/шеснаесетмина, шеснаесетмината/шеснаесетмина (mk, http://purl.org/olia/mte/multext-east.owl#CollectiveNumeral)" , "Numeral/Type=\"collect\" (Romanian)<br/>\t\t\t\n\t\t\tIn traditional Romanian grammars, expressions like amândoi \"both\", toţi trei \"all three\" are referred to as collective numerals. (MTE v4, http://purl.org/olia/mte/multext-east.owl#CollectiveNumeral)" ;
        <http://www.w3.org/2000/01/rdf-schema#subClassOf>
                <http://purl.org/olia/olia.owl#Numeral> ;
        <http://www.w3.org/2002/07/owl#versionInfo>
                "http://purl.org/olia/mte/multext-east.owl#CollectiveNumeral" .

<http://purl.org/olia/olia.owl#DeterminerPhrase>
        a       <http://www.w3.org/2002/07/owl#Class> ;
        <http://www.w3.org/2000/01/rdf-schema#comment>
                "\n\t\tCertain pronouns serving as determiners in noun phrases may be premodified, for instance, \n\t\tby degree adverbs such as in German \"so viele ¨Altere\", \"gar kein Schutz\", etc.\n\t\tIn the case of \"so viele Ältere\", the premodifying adverb so is attached to the indefinite\n\t\tpronoun viele. Together, they form a determiner phrase (DP), which is attached to the\n\t\thead noun Ältere on the same level: [so viele] Ältere\n\t\t(Telljohann et al. 2009, p.63)\n\t\t" ;
        <http://www.w3.org/2000/01/rdf-schema#subClassOf>
                <http://purl.org/olia/olia.owl#Phrase> ;
        <http://www.w3.org/2002/07/owl#versionInfo>
                "\n\t\tTüBa-D/Z, NOTE: not to be confused with \"determiner phrase\" in generative grammar, \n\t\twhich would be a NounPhrase in most annotation frameworks" .

<http://purl.org/olia/olia.owl#Intransitive>
        a       <http://www.w3.org/2002/07/owl#Class> ;
        <http://www.w3.org/2000/01/rdf-schema#comment>
                "\n\t\t\tA predicate/verb that takes one argument, e.g., English \"to go\", cf. van Valin and Lapolla (1997).\n\t\t" ;
        <http://www.w3.org/2000/01/rdf-schema#subClassOf>
                <http://purl.org/olia/olia-top.owl#ValencyFeature> ;
        <http://www.w3.org/2002/07/owl#versionInfo>
                "SUSANNE (Sampson 1995)" .

<http://purl.org/olia/olia.owl#Extraposition>
        a       <http://www.w3.org/2002/07/owl#Class> ;
        <http://www.w3.org/2000/01/rdf-schema#comment>
                "*EXP*\n— Expletive (extraposition) ...\nIn cases where a clausal subject has been extraposed and replaced by an expletive it, we use a type of pseudo-attach called *EXP*. (In the small ATIS sample included with this release, it is also used for existential there.) Use of *EXP*-attach is discussed in more detail in section 17 [It-Extraposition]. \n\n  (S (NP-SBJ (NP It)\n             (SBAR *EXP*-1))\n     (VP is\n         (ADJP-PRD clear)\n         (PP to\n             (NP me))\n         (SBAR-1 that\n                 (S (NP-SBJ this message)\n                    (VP is\n                        (ADJP-PRD unclear))))))\n\n(Bies et al. 1995)" ;
        <http://www.w3.org/2000/01/rdf-schema#subClassOf>
                <http://purl.org/olia/olia-top.owl#SyntacticConstruction> ;
        <http://www.w3.org/2002/07/owl#versionInfo>
                "PTB bracketing guidelines, Bies et al. 1995" .

<http://purl.org/olia/olia.owl#BrokenPlural>
        a       <http://www.w3.org/2002/07/owl#Class> ;
        <http://www.w3.org/2000/01/rdf-schema#comment>
                "\n                            Internal plural that do not have any inflection.\n                                (http://www.isocat.org/datcat/DC-2218)\n                            " ;
        <http://www.w3.org/2000/01/rdf-schema#label>
                "broken plural" ;
        <http://www.w3.org/2000/01/rdf-schema#subClassOf>
                <http://purl.org/olia/olia.owl#Plural> ;
        <http://www.w3.org/2002/07/owl#versionInfo>
                "http://www.isocat.org/datcat/DC-2218" , "subClassOf plural (dcif:isA)" .

<http://purl.org/olia/olia.owl#SyntacticArgument>
        a       <http://www.w3.org/2002/07/owl#Class> ;
        <http://www.w3.org/2000/01/rdf-schema#comment>
                "\n\t\t\tAn inherent (morpho)syntactic constituent subcategorized for by a predicate.<br/>\n\t\t\t'Arguments are those terms which are required by some predicate in \n\t\t\torder to form a complete nuclear predication. They are essential to \n\t\t\tthe integrity of the SoA designated by the predicate frame. If we \n\t\t\tleave them out, the property/relation designated by the predicate is \n\t\t\tnot fulfilled or satisfied.' (Dik, 1997:86f)<br/>\n\t\t\tAn argument can be a controller in an agreement relation.\n\t\t\t(http://languagelink.let.uu.nl/tds/onto/LinguisticOntology.owl#syntacticArgument)<br/>\n\t\t\t\n\t\t\tThe category ARG is assigned to those syntactic constituents that appear as obligatory complements \n\t\t\tto the main verb. This means that they cannot be left out without a change in grammaticality or a \n\t\t\tsignificant change in meaning.\n\t\t\t(Dipper et al. 2007, §4.3.3)\n\t\t" ;
        <http://www.w3.org/2000/01/rdf-schema#subClassOf>
                <http://purl.org/olia/olia-top.owl#SyntacticRole> ;
        <http://www.w3.org/2002/07/owl#versionInfo>
                "\n\t\t\tadded to account for TIGER edge labels with syntactic function\n\t\t" .

<http://purl.org/olia/olia.owl#FiniteVerb>
        a       <http://www.w3.org/2002/07/owl#Class> ;
        <http://www.w3.org/2000/01/rdf-schema#comment>
                "\n\t\tA finite verb is a verb form that occurs in an independent clause, and \n\t\tis fully inflected according to the inflectional categories marked on \n\t\tverbs in the language.  \n\t\t(http://www.sil.org/linguistics/GlossaryOfLinguisticTerms/WhatIsAFiniteVerb.htm 19.09.06)\n\t\t\n\t\tProperty applied to a verb form that can occur on its own in an independent sentence.\n        (Crystal 2003; http://www.isocat.org/datcat/DC-1287)\n\t\t" ;
        <http://www.w3.org/2000/01/rdf-schema#subClassOf>
                <http://purl.org/olia/olia.owl#Verb> ;
        <http://www.w3.org/2002/07/owl#versionInfo>
                "\n\t\t\tEAGLES Verb with Finiteness=\"Finite\".\n\t\t" .

<http://purl.org/olia/olia.owl#NegativeParticle>
        a       <http://www.w3.org/2002/07/owl#Class> ;
        <http://www.w3.org/2000/01/rdf-schema#comment>
                "\n                            Particle used to express negation.\n                                (Gil Francopoulo; http://www.isocat.org/datcat/DC-1894)\n                            " ;
        <http://www.w3.org/2000/01/rdf-schema#label>
                "negative particle" ;
        <http://www.w3.org/2000/01/rdf-schema#subClassOf>
                <http://purl.org/olia/olia.owl#Particle> ;
        <http://www.w3.org/2002/07/owl#versionInfo>
                "subClassOf particle (dcif:isA)" , "http://www.isocat.org/datcat/DC-1894" .

<http://purl.org/olia/olia.owl#Past>
        a       <http://www.w3.org/2002/07/owl#Class> ;
        <http://www.w3.org/2000/01/rdf-schema#comment>
                "\n\t\t\tThe past tense is a verb tense expressing action, activity, state \n\t\t\tor being in the past. (http://en.wikipedia.org/wiki/Past_tense  17.11.06)\n\t\t\t\n\t\t\tThe past tense refers to a tense category which places an event in the past.\n\t\t\t(http://languagelink.let.uu.nl/tds/onto/LinguisticOntology.owl#pastTense)\n\t\t" ;
        <http://www.w3.org/2000/01/rdf-schema#subClassOf>
                <http://purl.org/olia/olia.owl#AbsoluteTense> ;
        <http://www.w3.org/2002/07/owl#versionInfo>
                "EAGLES, http://languagelink.let.uu.nl/tds/onto/LinguisticOntology.owl#pastTense" .

<http://purl.org/olia/olia.owl#Stem>
        a       <http://www.w3.org/2002/07/owl#Class> ;
        <http://www.w3.org/2000/01/rdf-schema#comment>
                "\n                            Root of a word, together with any derivational affixes, to which inflectional affixes are added.\n                                (www.sil.org/linguistics/GlossaryOfLinguisticTerms/WhatIsAStem.htm; http://www.isocat.org/datcat/DC-1389)\n                            " ;
        <http://www.w3.org/2000/01/rdf-schema#label>
                "root" , "stem" , "base" ;
        <http://www.w3.org/2000/01/rdf-schema#subClassOf>
                <http://purl.org/olia/olia.owl#Morpheme> ;
        <http://www.w3.org/2002/07/owl#versionInfo>
                "http://www.isocat.org/datcat/DC-1389" .

<http://purl.org/olia/olia.owl#DemonstrativeAdverb>
        a       <http://www.w3.org/2002/07/owl#Class> ;
        <http://www.w3.org/2000/01/rdf-schema#comment>
                "\n\t\t\tPronominal adverb derived from a demonstrative stem (Ch. Chiarcos)\n\t\t" ;
        <http://www.w3.org/2000/01/rdf-schema#subClassOf>
                <http://purl.org/olia/olia.owl#PronominalAdverb> ;
        <http://www.w3.org/2002/07/owl#versionInfo>
                "http://purl.org/olia/urdu.owl#AdverbialDemonstrative, http://purl.org/olia/emille.owl#DistalDemonstrativeAdverb" .

<http://purl.org/olia/olia.owl#PossessivePronoun>
        a       <http://www.w3.org/2002/07/owl#Class> ;
        <http://www.w3.org/2000/01/rdf-schema#comment>
                "\n\t\t\tA possessive pronoun is a pronoun that expresses relationships like ownership, such as kinship, and other forms of association.\n\t\t\t(http://www.sil.org/linguistics/GlossaryOfLinguisticTerms/WhatIsAPossessivePronoun.htm 19.09.06)\n\t\t" ;
        <http://www.w3.org/2000/01/rdf-schema#subClassOf>
                <http://purl.org/olia/olia.owl#Pronoun> ;
        <http://www.w3.org/2002/07/owl#versionInfo>
                "EAGLES Pronoun with Pron.-Type=\"Possessive\"." , "TODO: Check regrouping possibilities, as it is covered by the GOLD definition of PersonalPronoun \n\t\t\t\t\t(i.e., person marking, although no person congruency).\n\t\t\n\t\t\t\t\tPossessivePronoun isn't disjoint with IndefinitePronoun (German: \"jemandes\" nach jemandes Pfeife tanzen), \n\t\t\t\t\tDemonstrativePronoun (German:\"dessen\" Zähne alle exakt gleich waren), WHPronoun (German: \n\t\t\t\t\t\"wessen\" Bedürfnissen soll sie genügen), ReflexivePronoun (Old English \"sin\" his/her/its).\n\t\t" .

<http://purl.org/olia/olia.owl#FusedPrepArt>
        a       <http://www.w3.org/2002/07/owl#Class> ;
        <http://www.w3.org/2000/01/rdf-schema#comment>
                "\n\t\t\tThe additional value Fused prep-art is for the benefit of those who do not find it \n\t\t\tpractical to split fused words such as French au (= à + le) into two text words. \n\t\t\tThis very common phenomenon of a fused preposition + article in West European \n\t\t\tlanguages should preferably, however, be handled by assigning two tags to the \n\t\t\tsame orthographic word (one for the preposition and one for the article).\n\t\t\t(http://www.ilc.cnr.it/EAGLES96/annotate/node18.html#oav1ap 19.09.06)\n\t\t" ;
        <http://www.w3.org/2000/01/rdf-schema#subClassOf>
                <http://purl.org/olia/olia.owl#Preposition> , <http://purl.org/olia/olia.owl#Article> ;
        <http://www.w3.org/2002/07/owl#versionInfo>
                "EAGLES Adposition with Type=\"FusedPrepArt\"" .

<http://purl.org/olia/olia.owl#QualifierAdjective>
        a       <http://www.w3.org/2002/07/owl#Class> ;
        <http://www.w3.org/2000/01/rdf-schema#comment>
                "\n                            Adjective used to qualify.\n                                (http://www.isocat.org/datcat/DC-1477)\n                            " ;
        <http://www.w3.org/2000/01/rdf-schema#label>
                "qualifier adjective" , "qualificative adjective" ;
        <http://www.w3.org/2000/01/rdf-schema#subClassOf>
                <http://purl.org/olia/olia.owl#Qualifier> , <http://purl.org/olia/olia.owl#Adjective> ;
        <http://www.w3.org/2002/07/owl#versionInfo>
                "subClassOf adjective (dcif:isA)" , "http://www.isocat.org/datcat/DC-1477, http://purl.org/olia/mte/multext-east.owl#QualificativeAdjective" .

<http://purl.org/olia/olia.owl#PoliteSecondPersonPronoun>
        a       <http://www.w3.org/2002/07/owl#Class> ;
        <http://www.w3.org/2000/01/rdf-schema#comment>
                "\n\t\t\tIn several European languages exist special forms of pronouns for polite or respectful reference,\n\t\t\te.g. Dutch u and Spanish usted.\n\t\t\t(http://www.ilc.cnr.it/EAGLES96/annotate/node18.html#oav1p 19.09.06)\n\t\t" ;
        <http://www.w3.org/2000/01/rdf-schema#subClassOf>
                <http://purl.org/olia/olia.owl#SecondPersonPronoun> ;
        <http://www.w3.org/2002/07/owl#versionInfo>
                "TODO:\n\t\t\tPoliteness as feature rather than a concept.\n\t\t" , "\n\t\t\tEAGLES PersonalPronoun with Politeness=\"Polite\". \n\t\t\tThe EAGLES attribute politeness (polite/ familiar) is limited to second-person pronouns.\n\t\t\t\n\t\t\tIn French, for example, it is possible to treat Polite simply as pragmatic values encoded \n\t\t\tthrough other attributes - especially person and number.\n\t\t\tIn languages where there are special polite pronoun forms (e.g. Dutch u and Spanish usted), \n\t\t\tthe additional Politeness attribute is required.\n\t\t\t(http://www.ilc.cnr.it/EAGLES96/annotate/node18.html#oav1p 19.09.06)\n\t\t" .

<http://purl.org/olia/olia.owl#CliticDefiniteArticle>
        a       <http://www.w3.org/2002/07/owl#Class> ;
        <http://www.w3.org/2000/01/rdf-schema#comment>
                "\n\t\t\tclitic definite determiner, e.g., in Macedonian, Bulgarian, and Romanian (http://purl.org/olia/mte/multext-east.owl#CliticDeterminerType)\n\t\t" ;
        <http://www.w3.org/2000/01/rdf-schema#label>
                "clitic definite determiner" , "clitic definite article" ;
        <http://www.w3.org/2000/01/rdf-schema#subClassOf>
                <http://purl.org/olia/olia.owl#CliticElement> , <http://purl.org/olia/olia.owl#DefiniteArticle> ;
        <http://www.w3.org/2002/07/owl#versionInfo>
                "cf. http://purl.org/olia/mte/multext-east.owl#CliticDistalDeterminer" .

<http://purl.org/olia/olia.owl#CessativeAspect>
        a       <http://www.w3.org/2002/07/owl#Class> ;
        <http://www.w3.org/2000/01/rdf-schema#comment>
                "\n                            Aspect that expresses the cessation of an event or state.\n                                (SIL; http://www.isocat.org/datcat/DC-2001)\n                            " ;
        <http://www.w3.org/2000/01/rdf-schema#label>
                "accomplished" , "cessative" ;
        <http://www.w3.org/2000/01/rdf-schema#subClassOf>
                <http://purl.org/olia/olia-top.owl#AspectFeature> ;
        <http://www.w3.org/2002/07/owl#versionInfo>
                "subClassOf aspect (dcif:conceptualDomain)" , "http://www.isocat.org/datcat/DC-2001" .

<http://purl.org/olia/olia.owl#RightParentheticalPunctuation>
        a       <http://www.w3.org/2002/07/owl#Class> ;
        <http://www.w3.org/2000/01/rdf-schema#comment>
                "\n\t\t\tEnd of a paired punctuation.\n            (http://www.isocat.org/datcat/DC-2079)\n\t\t\n\t\t\tRightParentheticalPunctuation is a punctuation mark which concludes a constituent \n\t\t\twhose the opening is marked by a LeftParentheticalPunctuation, e.g. ), ] and Spanish ?.\n\t\t\t(http://www.ilc.cnr.it/EAGLES96/annotate/node17.html#recv 19.09.06)\n\t\t" ;
        <http://www.w3.org/2000/01/rdf-schema#subClassOf>
                <http://purl.org/olia/olia.owl#ParentheticalPunctuation> ;
        <http://www.w3.org/2002/07/owl#versionInfo>
                "added in accordance with EAGLES suggestions (http://www.ilc.cnr.it/EAGLES96/annotate/node17.html#recv)" , "TODO: rename to ClosePunctuation to support scripts running from left to right" , "http://www.isocat.org/datcat/DC-2079" .

<http://purl.org/olia/olia.owl#TitleNoun>
        a       <http://www.w3.org/2002/07/owl#Class> ;
        <http://www.w3.org/2000/01/rdf-schema#comment>
                "A title designates the function or the social status of an individual. Often, it accompanies a proper noun, but it can also be used in place of a proper noun (if the bearer of the title is contextually unambiguous).\n\t\t\tE.g. \"The/Det German/Adj Chancellor/Title Angela/Name Merkel/Name said ...\" can be used besides \"the German Chancellor said ...\".\n\t\t\tAccordingly, some schemes (e.g., Chungku et al. 2010, for Dzongkha) group titles together with proper names (http://purl.org/olia/dzongkha.owl#ParticularPersonNoun).\n\t\t\t\n\t\t\tHowever, if multiple people hold the same title, they can be referred to as a group, e.g., \"Since WWII, the politics of the German chancellors always followed ...\", and in this usage, \n\t\t\ttitles are more comparable to common nouns.\n\t\t\tFunctionally, titles are thus an intermediate category between CommonNoun and ProperNoun (cf. also Mulkern 1996).\n\t\t\t\n\t\t\tTitles do, however, share important characteristics with common nouns. \n\t\t\tIn English, for example, titles generally require a definite determiner (unlike proper nouns), even if unambiguous (\"the pope\"). \n\t\t\tThey are thus classified here as a subtype of CommonNoun.\n\t\t\t\n\t\t\t(Ann E. Mulkern. The name of the game. In Jeanette Gundel and Thorstein Fretheim, editors. Reference and Referent Accessibility: Pragmatics\n\t\t\tand Beyond. John Benjamins, Amsterdam and Philadelphia, 1996, pages 235–250.)  \t\t\n\t\t" ;
        <http://www.w3.org/2000/01/rdf-schema#subClassOf>
                <http://purl.org/olia/olia.owl#CommonNoun> ;
        <http://www.w3.org/2002/07/owl#versionInfo>
                "added in accordance with Sajjad (2007, for Urdu, http://purl.org/olia/urdu.owl#Title)" .

<http://purl.org/olia/olia-top.owl#SubordTypeFeature>
        a       <http://www.w3.org/2002/07/owl#Class> ;
        <http://www.w3.org/2002/07/owl#deprecated>
                true ;
        <http://www.w3.org/2002/07/owl#versionInfo>
                "reimplemented as concepts" .

<http://purl.org/olia/olia.owl#Anticausative>
        a       <http://www.w3.org/2002/07/owl#Class> ;
        <http://www.w3.org/2000/01/rdf-schema#comment>
                "\n\t\t\tAn intransitive verb is derived from a basically transitive one \n\t\t\twith the direct object of the transitive verb corresponding to \n\t\t\tthe subject of the intransitive.\n\t\t\t(Siewierska 1988:267)\n\t\t\t(http://purl.org/linguistics/gold/Anticausative)\n\t\t" ;
        <http://www.w3.org/2000/01/rdf-schema#subClassOf>
                <http://purl.org/olia/olia.owl#ActiveVoice> ;
        <http://www.w3.org/2002/07/owl#versionInfo>
                "\n\t\t\thttp://purl.org/linguistics/gold/Anticausative\n\t\t\tThis is a semantic manipulation of the verb frame \n\t\t\t(and thus limited to a specific semantic class of verbs)\n\t\t\trather than a grammatical device for the manipulation\n\t\t\tof argument structure, therefore classified as Active here.\n\t\t" .

<http://purl.org/olia/olia-top.owl#DefinitenessFeature>
        a       <http://www.w3.org/2002/07/owl#Class> ;
        <http://www.w3.org/2000/01/rdf-schema#subClassOf>
                [ a       <http://www.w3.org/2002/07/owl#Restriction> ;
                  <http://www.w3.org/2002/07/owl#hasSelf>
                          true ;
                  <http://www.w3.org/2002/07/owl#onProperty>
                          <http://purl.org/olia/olia.owl#hasDefiniteness>
                ] ;
        <http://www.w3.org/2002/07/owl#versionInfo>
                "TODO:\n\t\t\tuse this property to define Definite/IndefiniteArticle\n\t\t" , "\n\t\t\tSkipped EAGLES \"Unmarked\" definiteness that was only introduced \"to handle the suffixed \n\t\t\tdefinite article in Danish: e.g. \"haven\" (`the garden'); \"havet\" (`the sea').\" \n\t\t\t(http://www.ilc.cnr.it/EAGLES96/annotate/node19.html#oav2  16.11.06)\n\t\t" .

<http://purl.org/olia/olia.owl#Conjugated>
        a       <http://www.w3.org/2002/07/owl#Class> ;
        <http://www.w3.org/2000/01/rdf-schema#comment>
                "\n                            Property of a verbal form when inflected\n                                (http://www.isocat.org/datcat/DC-2207)\n                            " ;
        <http://www.w3.org/2000/01/rdf-schema#label>
                "conjugated" ;
        <http://www.w3.org/2000/01/rdf-schema#subClassOf>
                <http://purl.org/olia/olia.owl#Inflected> ;
        <http://www.w3.org/2002/07/owl#versionInfo>
                "http://www.isocat.org/datcat/DC-2207" .

<http://purl.org/olia/olia.owl#CardinalNumber>
        a       <http://www.w3.org/2002/07/owl#Class> ;
        <http://www.w3.org/2000/01/rdf-schema#comment>
                "\n\t\t\tA cardinal numeral is a numeral of the class whose members are considered basic \n\t\t\tin form, used in counting, and used in expressing how many objects are referred to.\n\t\t\t(http://www.sil.org/linguistics/GlossaryOfLinguisticTerms/WhatIsACardinalNumeral.htm 19.09.06)\n\t\t" ;
        <http://www.w3.org/2000/01/rdf-schema#subClassOf>
                <http://purl.org/olia/olia.owl#Numeral> ;
        <http://www.w3.org/2002/07/owl#versionInfo>
                "EAGLES Numeral with Type=\"Cardinal\"." .

<http://purl.org/olia/olia.owl#Nominative>
        a       <http://www.w3.org/2002/07/owl#Class> ;
        <http://www.w3.org/2000/01/rdf-schema#comment>
                "\n\t\t\tIn nominative-accusative languages, nominative case marks clausal subjects and is applies to nouns in isolation.\n\t\t\t(http://www.sil.org/linguistics/glossaryoflinguisticterms/WhatIsNominativeCase.htm  17.11.06)\n\t\t" ;
        <http://www.w3.org/2000/01/rdf-schema#subClassOf>
                <http://purl.org/olia/olia-top.owl#CaseFeature> ;
        <http://www.w3.org/2002/07/owl#versionInfo>
                "EAGLES" .

<http://purl.org/olia/olia.owl#InterrogativeParticle>
        a       <http://www.w3.org/2002/07/owl#Class> ;
        <http://www.w3.org/2000/01/rdf-schema#comment>
                "\n                            Particle used to express a question.\n                                (http://www.isocat.org/datcat/DC-1921)\n                            " ;
        <http://www.w3.org/2000/01/rdf-schema#label>
                "interrogative particle" ;
        <http://www.w3.org/2000/01/rdf-schema#subClassOf>
                <http://purl.org/olia/olia.owl#Particle> ;
        <http://www.w3.org/2002/07/owl#equivalentClass>
                [ a       <http://www.w3.org/2002/07/owl#Class> ;
                  <http://www.w3.org/2002/07/owl#intersectionOf>
                          ( <http://purl.org/olia/olia.owl#Particle> <http://purl.org/olia/olia.owl#QuestionWord> )
                ] ;
        <http://www.w3.org/2002/07/owl#versionInfo>
                "http://www.isocat.org/datcat/DC-1921" , "subClassOf particle (dcif:isA)" , "TODO: check relationship with interrogative adverb" .

<http://purl.org/olia/olia.owl#SubablativeCase>
        a       <http://www.w3.org/2002/07/owl#Class> ;
        <http://www.w3.org/2000/01/rdf-schema#comment>
                "\n\t\t\tSubablativeCase expresses that  the referent of the noun it marks \n\t\t\tis the location from under which another referent is moving. It \n\t\t\thas the meaning 'from under'.\n\t\t\t(http://purl.org/linguistics/gold/Subablative)\n\t\t" ;
        <http://www.w3.org/2000/01/rdf-schema#subClassOf>
                <http://purl.org/olia/olia-top.owl#CaseFeature> ;
        <http://www.w3.org/2002/07/owl#versionInfo>
                "http://purl.org/linguistics/gold/Subablative" .

<http://purl.org/olia/olia.owl#PejorativeEvaluative>
        a       <http://www.w3.org/2002/07/owl#Class> ;
        <http://www.w3.org/2000/01/rdf-schema#comment>
                "An evaluative property of a noun that indicates\n                        the speaker regards the person or object being referred to with distaste,\n                        contempt, or displeasure [Valentine 2001: 190-193]." ;
        <http://www.w3.org/2000/01/rdf-schema#isDefinedBy>
                "http://www.isocat.org/datcat/DC-3380" ;
        <http://www.w3.org/2000/01/rdf-schema#subClassOf>
                <http://purl.org/olia/olia-top.owl#EvaluativeFeature> .

<http://purl.org/olia/olia.owl#SecondHonorific>
        a       <http://www.w3.org/2002/07/owl#Class> ;
        <http://www.w3.org/2000/01/rdf-schema#subClassOf>
                <http://purl.org/olia/olia.owl#Second> ;
        <http://www.w3.org/2002/07/owl#versionInfo>
                "TOCHECK: is SecondHonorific different from SecondPolite ?" , "Adopted from ILPOSTS for Indian languages, http://purl.org/olia/ilposts.owl#Honorific" .

<http://purl.org/olia/olia.owl#ExistentialParticle>
        a       <http://www.w3.org/2002/07/owl#Class> ;
        <http://www.w3.org/2000/01/rdf-schema#comment>
                "English existential there is specified as a subtype of pronoun in MTE v4, i.e., Pronoun/Type=\"ex-there\" (http://purl.org/olia/mte/multext-east.owl#ExistentialThere)" ;
        <http://www.w3.org/2000/01/rdf-schema#subClassOf>
                <http://purl.org/olia/olia.owl#Particle> ;
        <http://www.w3.org/2002/07/owl#versionInfo>
                "http://purl.org/olia/mte/multext-east.owl#ExistentialThere" .

<http://purl.org/olia/olia.owl#ObliqueRole>
        a       <http://www.w3.org/2002/07/owl#Class> ;
        <http://www.w3.org/2000/01/rdf-schema#comment>
                "\n\t\t\tA semantic role which is not straightforward.\n\t\t\t(http://languagelink.let.uu.nl/tds/onto/LinguisticOntology.owl#obliqueCase)\n\t\t" ;
        <http://www.w3.org/2000/01/rdf-schema#subClassOf>
                <http://purl.org/olia/olia-top.owl#SemanticRole> ;
        <http://www.w3.org/2002/07/owl#versionInfo>
                "http://languagelink.let.uu.nl/tds/onto/LinguisticOntology.owl#obliqueRole" .

<http://purl.org/olia/olia.owl#Particle>
        a       <http://www.w3.org/2002/07/owl#Class> ;
        <http://www.w3.org/2000/01/rdf-schema#comment>
                "synonym of Unique, to be avoided because of its divergent definitions (Chiarcos)" ;
        <http://www.w3.org/2000/01/rdf-schema#subClassOf>
                <http://purl.org/olia/olia.owl#Unique> ;
        <http://www.w3.org/2002/07/owl#versionInfo>
                "synonym of Unique, to be avoided because of its divergent definitions, applies to every category that *contains* the expression \"Particle\" in its name" .

<http://purl.org/olia/olia.owl#Circumposition>
        a       <http://www.w3.org/2002/07/owl#Class> ;
        <http://www.w3.org/2000/01/rdf-schema#comment>
                "\n      A circumposition is an adposition with a part before the noun phrase and a part after. \n      It is much less common than prepositions or postpositions.\n      (http://en.wikipedia.org/wiki/Circumposition 19.09.06)\n      " ;
        <http://www.w3.org/2000/01/rdf-schema#subClassOf>
                <http://purl.org/olia/olia.owl#Adposition> ;
        <http://www.w3.org/2002/07/owl#versionInfo>
                "EAGLES adposition with optional attribute Type=\"Circumposition\". \n      \n      The relationship between circumpositions and pre-/postpositions in EAGLES is not clear.\n      We do not prohibit Circumpositions from being Prepositions or Postpositions, though \n      the EAGLES feature assignment (with all optional values implemented) would possibly rule this out. (Chiarcos)" .

<http://purl.org/olia/olia.owl#Colon>
        a       <http://www.w3.org/2002/07/owl#Class> ;
        <http://www.w3.org/2000/01/rdf-schema#comment>
                "\n                            Sign with two vertical points that is used in writing and printing to introduce an explanation, example or quotation.\n                                (Gil Francopoulo; http://www.isocat.org/datcat/DC-1439)\n                            " ;
        <http://www.w3.org/2000/01/rdf-schema#label>
                "colon" ;
        <http://www.w3.org/2000/01/rdf-schema#subClassOf>
                <http://purl.org/olia/olia.owl#SentenceMedialPunctuation> ;
        <http://www.w3.org/2002/07/owl#versionInfo>
                "http://www.isocat.org/datcat/DC-1439" , "subClassOf partOfSpeech (dcif:conceptualDomain)" .

<http://purl.org/olia/olia.owl#NominalizedVerb>
        a       <http://www.w3.org/2002/07/owl#Class> ;
        <http://www.w3.org/2000/01/rdf-schema#comment>
                "\n\t\t\tA non-finite embedded construction which contains features \n\t\t\twith nominal properties \n\t\t\t(http://languagelink.let.uu.nl/tds/onto/LinguisticOntology.owl#withNominalProperites, \n\t\t\twith reference to Dik 1997)\n\t\t" ;
        <http://www.w3.org/2000/01/rdf-schema#subClassOf>
                <http://purl.org/olia/olia.owl#NonFiniteEmbeddedConstruction> ;
        <http://www.w3.org/2002/07/owl#versionInfo>
                "http://languagelink.let.uu.nl/tds/onto/LinguisticOntology.owl#withNominalProperites" .

<http://purl.org/olia/olia.owl#ModernUsage>
        a       <http://www.w3.org/2002/07/owl#Class> ;
        <http://www.w3.org/2000/01/rdf-schema#comment>
                "\n                            Currently in use.\n                                (http://www.isocat.org/datcat/DC-1962)\n                            " ;
        <http://www.w3.org/2000/01/rdf-schema#label>
                "modern" ;
        <http://www.w3.org/2000/01/rdf-schema#subClassOf>
                <http://purl.org/olia/olia.owl#TemporallyDefinedUsage> ;
        <http://www.w3.org/2002/07/owl#versionInfo>
                "subClassOf dating (dcif:conceptualDomain)" , "http://www.isocat.org/datcat/DC-1962 (modern)" .

<http://purl.org/olia/olia.owl#TechnicalRegister>
        a       <http://www.w3.org/2002/07/owl#Class> ;
        <http://www.w3.org/2000/01/rdf-schema#comment>
                "\n                            The register appropriate to scientific texts or special languages.\n                                (ISO12620; http://www.isocat.org/datcat/DC-1997)\n                            " ;
        <http://www.w3.org/2000/01/rdf-schema#label>
                "technical register" ;
        <http://www.w3.org/2000/01/rdf-schema#subClassOf>
                <http://purl.org/olia/olia-top.owl#RegisterFeature> ;
        <http://www.w3.org/2002/07/owl#versionInfo>
                "subClassOf register (dcif:conceptualDomain)" , "http://www.isocat.org/datcat/DC-1997" .

<http://purl.org/olia/olia.owl#WHPronoun>
        a       <http://www.w3.org/2002/07/owl#Class> ;
        <http://www.w3.org/2000/01/rdf-schema#subClassOf>
                <http://purl.org/olia/olia.owl#Pronoun> ;
        <http://www.w3.org/2000/01/rdf-schema#subClassOf>
                [ a       <http://www.w3.org/2002/07/owl#Class> ;
                  <http://www.w3.org/2002/07/owl#unionOf>
                          ( <http://purl.org/olia/olia.owl#RelativePronoun> <http://purl.org/olia/olia.owl#InterrogativePronoun> )
                ] ;
        <http://www.w3.org/2002/07/owl#deprecated>
                true ;
        <http://www.w3.org/2002/07/owl#versionInfo>
                "EAGLES Pronoun with Pron.-Type=\"Int./Rel.\"." , "TODO: Check cross-linguistic validity of this class.\n\t\t\t\tThis class is based on surface criteria of Indo-European languages.\n\t\t\t\tIn other (and even IE) languages, relative pronouns are partly also derived from\n\t\t\t\tnon-interrogatives, but rather from demonstratives, cf. English \"that\".\n\t\t\t\tShould be abandoned unless language-independent evidence for its existence \n\t\t\t\tis provided.\n\t\t\t\t\n\t\t\t\tDEPRECATED: to be replaced with InterrogativePronoun or RelativePronoun\n\t\t" .

<http://purl.org/olia/olia-top.owl#VoiceFeature>
        a       <http://www.w3.org/2002/07/owl#Class> ;
        <http://www.w3.org/2000/01/rdf-schema#subClassOf>
                [ a       <http://www.w3.org/2002/07/owl#Restriction> ;
                  <http://www.w3.org/2002/07/owl#hasSelf>
                          true ;
                  <http://www.w3.org/2002/07/owl#onProperty>
                          <http://purl.org/olia/olia.owl#hasVoice>
                ] ;
        <http://www.w3.org/2000/01/rdf-schema#subClassOf>
                [ a       <http://www.w3.org/2002/07/owl#Restriction> ;
                  <http://www.w3.org/2002/07/owl#hasSelf>
                          true ;
                  <http://www.w3.org/2002/07/owl#onProperty>
                          <http://purl.org/olia/olia.owl#hasVoice>
                ] ;
        <http://www.w3.org/2002/07/owl#versionInfo>
                "hierarchically restructured" .

<http://purl.org/olia/olia.owl#Control>
        a       <http://www.w3.org/2002/07/owl#Class> ;
        <http://www.w3.org/2000/01/rdf-schema#comment>
                "Control indicates how a an argument from a main clause will be utilized in a subclause. This class includes both control structures and raising structures (http://www.lexinfo.net/ontology/2.0/lexinfo#Control)"@en ;
        <http://www.w3.org/2000/01/rdf-schema#subClassOf>
                <http://purl.org/olia/olia-top.owl#MovementFeature> ;
        <http://www.w3.org/2002/07/owl#versionInfo>
                "From http://www.lexinfo.net/ontology/2.0/lexinfo#Control. But note that we regard Control as a feature of syntactic units (either verbs [=> control/raising] or arguments [=> raisable argument], not as a subclass of Frame, this reflects a different understanding of \"Frame\", in OLiA, Frames are semantic units, in lexinfo, they seem to be syntactic patterns, in other resources, e.g., VerbNet, both aspects are combined." .

<http://purl.org/olia/olia.owl#OrdinalAdjective>
        a       <http://www.w3.org/2002/07/owl#Class> ;
        <http://www.w3.org/2000/01/rdf-schema#comment>
                "\n                            Adjective expressing a numeric ranking.\n                                (http://www.isocat.org/datcat/DC-1338)\n\t\t\t\t\t\t\t\n\t\t\t\t\t\t\tCf. \"second\", \"next\", \"last\"\n                            " ;
        <http://www.w3.org/2000/01/rdf-schema#label>
                "ordinal adjective" ;
        <http://www.w3.org/2000/01/rdf-schema#subClassOf>
                <http://purl.org/olia/olia.owl#Adjective> ;
        <http://www.w3.org/2002/07/owl#deprecated>
                true ;
        <http://www.w3.org/2002/07/owl#equivalentClass>
                <http://purl.org/olia/olia.owl#RelationalAdjective> ;
        <http://www.w3.org/2002/07/owl#versionInfo>
                "subClassOf adjective (dcif:isA)" , "DEPRECATED: The DCR definition and this term are incorrect. \n\t\t\t\"Ordinal adjective\" entered ISOcat from MULTEXT-East, where it was originally applied to relational adjectives (Slovene, Resian, Ukrainian, Czech).\n\t\t\t\"Ordinal adjective\" is a mistranslation from Slovene _vrstni pridevniki_ that should be properly rendered in English as \"relational adjective\" (Derzhanski and Kotsyba 2009).\n\t\t\tHowever, the Macedonian MULTEXT v.4 guidelines use this category for ordinal numerals. Due to its inherent ambiguity, this category is to be avoided. \n\t\t" , "http://www.isocat.org/datcat/DC-1338" .

<http://purl.org/olia/olia.owl#SingularQuantifier>
        a       <http://www.w3.org/2002/07/owl#Class> ;
        <http://www.w3.org/2000/01/rdf-schema#comment>
                "A singular quantifier is a quantifier or a numeral that specifies a single referent from a set. (Chiarcos) \n\t\tIn Czech and Slovak MTE v4 specs, the corresponding category Numeral/Class=\"definite1\" is applied to the numeral \"one\". (MTE v4)" ;
        <http://www.w3.org/2000/01/rdf-schema#subClassOf>
                <http://purl.org/olia/olia-top.owl#NumeralAgreementClass> ;
        <http://www.w3.org/2002/07/owl#equivalentClass>
                [ a       <http://www.w3.org/2002/07/owl#Class> ;
                  <http://www.w3.org/2002/07/owl#intersectionOf>
                          ( <http://purl.org/olia/olia.owl#Quantifier>
                            [ a       <http://www.w3.org/2002/07/owl#Restriction> ;
                              <http://www.w3.org/2002/07/owl#onProperty>
                                      <http://purl.org/olia/olia.owl#hasNumeralAgreementClass> ;
                              <http://www.w3.org/2002/07/owl#someValuesFrom>
                                      <http://purl.org/olia/olia.owl#SingularQuantifier>
                            ]
                          )
                ] ;
        <http://www.w3.org/2002/07/owl#versionInfo>
                "http://purl.org/olia/mte/multext-east.owl#SingularQuantifier (MTE v4 Numeral/Class=\"definite1\", http://purl.org/olia/mte/multext-east.owl#SingularQuantifier)\t\t\t\n\t\t\tNumeral/Class=\"definite\", Numeral/Class=\"definite1\", Numeral/Class=\"definite234\" etc. refer to specific patterns of congruency with Slavic numerals that originate from the difference between Old Slavic singular (definite1), dual (definite2, definite234) and plural (definite)." .

<http://purl.org/olia/olia.owl#CoordinateClause>
        a       <http://www.w3.org/2002/07/owl#Class> ;
        <http://www.w3.org/2000/01/rdf-schema#comment>
                "\n\t\t\tA coordinate clause is a clause belonging to a series of two or more clauses which are not \n\t\t\tsyntactically dependent on one another, and are joined by means of a coordinate conjunction, \n\t\t\ta connective or parataxis.  \n\t\t\t(http://www.sil.org/linguistics/glossaryoflinguisticterms/WhatIsACoordinateClause.htm).\n\t\t" ;
        <http://www.w3.org/2000/01/rdf-schema#subClassOf>
                <http://purl.org/olia/olia.owl#FiniteClause> ;
        <http://www.w3.org/2002/07/owl#versionInfo>
                "\n\t\t\tadopted from http://languagelink.let.uu.nl/tds/onto/LinguisticOntology.owl#coordinateClause\n\t\t" .

<http://purl.org/olia/olia.owl#Adverbial>
        a       <http://www.w3.org/2002/07/owl#Class> ;
        <http://www.w3.org/2000/01/rdf-schema#comment>
                "-ADV (adverbial)\n— marks a constituent other than ADVP or PP when it is used adverbially (e.g., NPs or free (“headless”) relatives). However, constituents that themselves are modifying an ADVP generally do not get -ADV. \n(Bies et al. 1995)" ;
        <http://www.w3.org/2000/01/rdf-schema#subClassOf>
                <http://purl.org/olia/olia-top.owl#SyntacticFunction> ;
        <http://www.w3.org/2002/07/owl#versionInfo>
                "Bies et al. 1995" .

<http://purl.org/olia/olia.owl#SyntacticAdjunct>
        a       <http://www.w3.org/2002/07/owl#Class> ;
        <http://www.w3.org/2000/01/rdf-schema#comment>
                "\n\t\t\tPrototypically, an optional (morpho)syntactic constituent.\n\n\t\t\t'Satellites are not ... required by the predicate; they give \n\t\t\toptional further information pertaining to additional features of the \n\t\t\tSoA ..., the location of the SoA ..., the speaker's attitude towards \n\t\t\tor evaluation of the propositional content ..., or the character of \n\t\t\tthe speech act...' (Dik, 1997:87)\n\t\t\t(http://languagelink.let.uu.nl/tds/onto/LinguisticOntology.owl#syntacticAdjunct)\n\t\t\t\n\t\t\tThe category adjunct (ADJ) is assigned to those constituents that appear as optional additions, \n\t\t\tbe it to the main verb or to a given noun. This means that they can be left out freely without \n\t\t\ta change in grammaticality or a significant change in meaning.\n\t\t\tIn  \"John called Mary (from school) (with his cell phone)\"  the optional additions \"from school\" \n\t\t\tand \"with his cell phone\" are such optional additions that can be left out freely.\n\t\t\tAdjuncts are generally used to convey additional information about the time, place, manner, or \n\t\t\tcause of the event or situation described by the clause (see below). That is, they restrict the \n\t\t\tclass of events/  situations described by the clause to a subset. If required the category ADJ \n\t\t\tcan be split up into semantic sub-categories, that are annotated in layer semantic roles (time, \n\t\t\tlocation, etc.).\n\t\t\t(Dipper et al. 2007, §4.3.3)\n\t\t" ;
        <http://www.w3.org/2000/01/rdf-schema#subClassOf>
                <http://purl.org/olia/olia-top.owl#SyntacticRole> ;
        <http://www.w3.org/2002/07/owl#versionInfo>
                "http://languagelink.let.uu.nl/tds/onto/LinguisticOntology.owl#syntacticAdjunct" .

<http://purl.org/olia/olia.owl#PersReflPronoun>
        a       <http://www.w3.org/2002/07/owl#Class> ;
        <http://www.w3.org/2000/01/rdf-schema#comment>
                "\n\t\t\tIn Eagles personal and reflexive pronouns are brought together as a single value Pers./Refl. \t\t\n\t\t\t(http://www.ilc.cnr.it/EAGLES96/annotate/node17.html#recp 19.09.06)\n\t\t" ;
        <http://www.w3.org/2000/01/rdf-schema#subClassOf>
                <http://purl.org/olia/olia.owl#Pronoun> ;
        <http://www.w3.org/2002/07/owl#versionInfo>
                "EAGLES Pronoun with Pron.-Type=\"Pers/Ref\"." , "TODO: This class should be renamed to PersonalPronoun, as it corresponds \n\t\t\tto the definition of PersonalPronoun in GOLD.\n\t\t\tSubclasses then should be renamed to ReflexivePronoun and NonreflexivePersonalPronoun.\n\t\t\t" .

<http://purl.org/olia/olia.owl#Animate>
        a       <http://www.w3.org/2002/07/owl#Class> ;
        <http://www.w3.org/2000/01/rdf-schema#comment>
                "\n                            Perceived as alive.\n                                (ISO12620; http://www.isocat.org/datcat/DC-1911)\n                            " ;
        <http://www.w3.org/2000/01/rdf-schema#label>
                "animate" ;
        <http://www.w3.org/2000/01/rdf-schema#subClassOf>
                <http://purl.org/olia/olia-top.owl#AnimacyFeature> ;
        <http://www.w3.org/2002/07/owl#versionInfo>
                "http://www.isocat.org/datcat/DC-1911" , "subClassOf animacy (dcif:conceptualDomain)" .

<http://purl.org/olia/olia.owl#PresumptiveModality>
        a       <http://www.w3.org/2002/07/owl#Class> ;
        <http://www.w3.org/2000/01/rdf-schema#comment>
                "The presumptive mood is used in Romanian to express presupposition or hypothesis regarding the fact denoted by the verb, as well as other more or less similar attitudes: doubt, curiosity, concern, condition, indifference, inevitability. For example, acolo s-o fi dus \"he might have gone there\" shows the basic presupposition use, while the following excerpt from a poem by Eminescu shows the use both in a conditional clause de-o fi \"suppose it is\" and in a main clause showing an attitude of submission to fate le-om duce \"we would bear\".\n\t\t\t\n\t\t\tDe-o fi una, de-o fi alta... Ce e scris și pentru noi,\n\t\t\tBucuroși le-om duce toate, de e pace, de-i război.\n\t\t\t\n\t\t\tBe it one, be it the other... Whatever fate we have,\n\t\t\tWe will gladly go through all, be it peace or be it war \n\t\t\t(http://en.wikipedia.org/wiki/Irrealis_mood#Presumptive)\n\t\t" ;
        <http://www.w3.org/2000/01/rdf-schema#subClassOf>
                <http://purl.org/olia/olia.owl#IrrealisModality> ;
        <http://www.w3.org/2002/07/owl#versionInfo>
                "adopted from ILPOSTS (http://purl.org/olia/ilposts.owl#PresumptiveMood) for Indian languages" .

<http://purl.org/olia/olia.owl#Diacritic>
        a       <http://www.w3.org/2002/07/owl#Class> ;
        <http://www.w3.org/2000/01/rdf-schema#subClassOf>
                <http://purl.org/olia/olia-top.owl#OrthographicEntity> .

<http://purl.org/olia/olia.owl#ListMarker>
        a       <http://www.w3.org/2002/07/owl#Class> ;
        <http://www.w3.org/2000/01/rdf-schema#comment>
                "LST — List marker.\n(Bies et al. 1995)" ;
        <http://www.w3.org/2000/01/rdf-schema#subClassOf>
                <http://purl.org/olia/olia.owl#LayoutElement> ;
        <http://www.w3.org/2002/07/owl#versionInfo>
                "PTB bracketing guidelines, Bies et al. 1995)" .

<http://purl.org/olia/olia.owl#Residual>
        a       <http://www.w3.org/2002/07/owl#Class> ;
        <http://www.w3.org/2000/01/rdf-schema#comment>
                "\n      The residual value (R) is assigned to classes of text words which lie outside the \n      traditionally accepted range of grammatical classes, although they occur quite \n      commonly in many texts and very commonly in some. For example: foreign words, \n      or mathematical formulae. It can be argued that these are on the fringes of the \n      grammar or lexicon of the language in which the text is written. Nevertheless, \n      they need to be tagged. (http://www.ilc.cnr.it/EAGLES96/annotate/node16.html#mr 19.09.06)\n      \n      Although words in the Residual category are on the periphery of the lexicon, they may \n      take some of the grammatical characteristics, e.g., of nouns. Acronyms such as IBM are \n      similar to proper nouns; symbols such as alphabetic characters can vary for singular and \n      plural (e.g. How many Ps are there in `psychopath'?), and are in this respect like common \n      nouns. In some languages (e.g. Portuguese) such symbols also have gender. It is quite \n      reasonable that in some tagging schemes some of these classes of word will be classified \n      under other parts of speech. (The Unclassified category applies to word-like text segments \n      which do not easily fit into any of the foregoing values. For example: incomplete words \n      and pause fillers such as er and erm in transcriptions of speech, or written representations of singing such as dum-de-dum. (http://www.ilc.cnr.it/EAGLES96/annotate/node17.html#recr 19.09.06)" , "\n      From a linguistic point of view, Residuals are a heterogeneous class and so, Residual\n      may overlap with every linguistically motivate annotation concept.\n      Also between subconcepts, overlap may occur (e.g. \\LaTeX \n      which is a symbol which can be read as an Acronym or acronyms which are related \n      to Abbreviations, e.g. GNU \"Gnu is not Unix\")\n    " ;
        <http://www.w3.org/2000/01/rdf-schema#subClassOf>
                <http://purl.org/olia/olia-top.owl#MorphosyntacticCategory> ;
        <http://www.w3.org/2002/07/owl#versionInfo>
                "EAGLES top-level category Residual (R) with the exception of its subclass\n      \"Unclassified\". Unclassified is not represented in the OLiA ontology, as it does not\n      represent information, but the absence of information.\n    " .

<http://purl.org/olia/olia.owl#hasSubjectPerson>
        a       <http://www.w3.org/2002/07/owl#ObjectProperty> ;
        <http://www.w3.org/2000/01/rdf-schema#comment>
                "\n                            person for the subject of the verb \n\t\t\t\t\t\t\t(in languages with double congruency)\n                                (http://www.isocat.org/datcat/DC-2278)\n                            " ;
        <http://www.w3.org/2000/01/rdf-schema#domain>
                <http://purl.org/olia/olia.owl#Verb> ;
        <http://www.w3.org/2000/01/rdf-schema#label>
                "subject person" ;
        <http://www.w3.org/2000/01/rdf-schema#subPropertyOf>
                <http://purl.org/olia/olia.owl#hasPerson> ;
        <http://www.w3.org/2002/07/owl#versionInfo>
                "http://www.isocat.org/datcat/DC-2278 (subject person)" .

<http://purl.org/olia/olia.owl#OrdinalNumber>
        a       <http://www.w3.org/2002/07/owl#Class> ;
        <http://www.w3.org/2000/01/rdf-schema#comment>
                "\n\t\t\tAn ordinal number is a number belonging to a class whose members designate \n\t\t\tpositions in a sequence, e.g. in English \"First\", \"Second\", \"Third\". \n\t\t\t(http://www.sil.org/linguistics/GlossaryOfLinguisticTerms/WhatIsAOrdinalNumeral.htm 19.09.06)\n\t\t" ;
        <http://www.w3.org/2000/01/rdf-schema#subClassOf>
                <http://purl.org/olia/olia.owl#Numeral> ;
        <http://www.w3.org/2002/07/owl#versionInfo>
                "EAGLES Numeral with Type=\"Ordinal\"." .

<http://purl.org/olia/olia.owl#Fraction>
        a       <http://www.w3.org/2002/07/owl#Class> ;
        <http://www.w3.org/2000/01/rdf-schema#comment>
                "Numeral/Form=\"fractional\" (Romanian)<br/>\n\t\t\tIn traditional Romanian grammars, FractionalNumeral refers to expressions like treime-one third. (MTE v4, http://purl.org/olia/mte/multext-east.owl#FractalNumeral)" , "e.g., treisprezecimea/treisprezecime, treisprezecimi/treisprezecime, treisprezecimii/treisprezecime, treisprezecimile/treisprezecime, treisprezecimilor/treisprezecime, unsprezecimea/unsprezecime, unsprezecimi/unsprezecime, unsprezecimii/unsprezecime, unsprezecimile/unsprezecime (ro, http://purl.org/olia/mte/multext-east.owl#FractalNumeral)" , "e.g., يک‌چهارمِ/يک‌چهار يک‌پنجمِ/يک‌پنج (fa, http://purl.org/olia/mte/multext-east.owl#FractalNumeral)" ;
        <http://www.w3.org/2000/01/rdf-schema#label>
                "fraction" , "fractional numeral" ;
        <http://www.w3.org/2000/01/rdf-schema#subClassOf>
                <http://purl.org/olia/olia.owl#Numeral> ;
        <http://www.w3.org/2002/07/owl#versionInfo>
                "http://purl.org/olia/mte/multext-east.owl#FractalNumeral, http://purl.org/olia/urdu.owl#FractionalNumeral" .

<http://purl.org/olia/olia.owl#ExpletiveCorrelate>
        a       <http://www.w3.org/2002/07/owl#Class> ;
        <http://www.w3.org/2000/01/rdf-schema#comment>
                "\n\t\t\tThree different expletive usages [of the German expletive pronoun es]\n\t\t\tare traditionally distinguished: formal subject or object (expletive argument), \n\t\t\tcorrelate of an extraposed clausal argument (expletive correlate), and Vorfeld-es (structural expletive)\n\t\t\t(cf. (Eisenberg 1999 2001), (Pütz 1986)).\n\t\t\t(Telljohann et al. 2009, p.60)\n\t\t\t\n\t\t\tExtraposed clausal arguments:\n\t\t\t\"Aber [es] ist übertrieben zu sagen, damit bekäme die FU erst eine Identität.\"\n\t\t\t(Telljohann et al. 2009, p.62)\n\t\t" ;
        <http://www.w3.org/2000/01/rdf-schema#subClassOf>
                <http://purl.org/olia/olia.owl#ExpletivePronoun> ;
        <http://www.w3.org/2002/07/owl#versionInfo>
                "\n\t\t\tTüBa-D/Z\n\t\t" .

<http://purl.org/olia/olia.owl#NonFiniteVerb>
        a       <http://www.w3.org/2002/07/owl#Class> ;
        <http://www.w3.org/2000/01/rdf-schema#comment>
                "\n             Verb forms occurring on their own only in dependent clauses and lacking tense and mood contrasts.\n\t\t\t (adapted from Crystal 2003; http://www.isocat.org/datcat/DC-1332)\n\t\t\t \n\t\t\tA non-finite verb is a verb that is not fully inflected for categories that are marked inflectionally in a language, \n\t\t\tsuch as the following: Tense, Aspect, Modality, Number,  Person.  \n\t\t\t(http://www.sil.org/linguistics/GlossaryOfLinguisticTerms/WhatIsANonfiniteVerb.htm 19.09.06)\n\t\t" ;
        <http://www.w3.org/2000/01/rdf-schema#subClassOf>
                <http://purl.org/olia/olia.owl#Verb> ;
        <http://www.w3.org/2002/07/owl#versionInfo>
                "http://www.isocat.org/datcat/DC-1332" , "EAGLES Verb with Finiteness=\"Non-finite\"." .

<http://purl.org/olia/olia.owl#QuotativeMood>
        a       <http://www.w3.org/2002/07/owl#Class> ;
        <http://www.w3.org/2000/01/rdf-schema#comment>
                "A quotative is grammatical device to mark reported speech in some languages (http://en.wikipedia.org/wiki/Quotative), e.g., in Estonian.<br/>\n\t\t\t\n\t\t\t‘Reportedly, while he was going (in his boat), he turned over.’\n\t\t\tTa olevat        oma     paadiga   ümber läinud\n\t\t\tHe was_QUOTATIVE his_own boat_WITH over  gone.<br/>\n\t\t\t\n\t\t\t(Estonian translation of an example given under http://www.sil.org/linguistics/GlossaryOfLinguisticTerms/WhatIsAQuotativeEvidential.htm)\n\t\t\t(Heiki-Jaan.Kaalep, email 2010/06/22)" ;
        <http://www.w3.org/2000/01/rdf-schema#subClassOf>
                <http://purl.org/olia/olia-top.owl#MoodFeature> , <http://purl.org/olia/olia.owl#QuotativeModality> ;
        <http://www.w3.org/2002/07/owl#versionInfo>
                "http://purl.org/olia/mte/multext-east.owl#Quotative, MTE VForm=\"quotative\" (Estonian)" .

<http://purl.org/olia/olia.owl#SimpleAspect>
        a       <http://www.w3.org/2002/07/owl#Class> ;
        <http://www.w3.org/2000/01/rdf-schema#comment>
                "non-progressive, non-purposive aspect (for Indian languages defined by http://purl.org/olia/ilposts.owl#SimpleAspect)" ;
        <http://www.w3.org/2000/01/rdf-schema#subClassOf>
                <http://purl.org/olia/olia-top.owl#AspectFeature> ;
        <http://www.w3.org/2002/07/owl#versionInfo>
                "ILPOSTS, http://purl.org/olia/ilposts.owl#SimpleAspect" , "TODO: check whether this is properly defined" .

<http://purl.org/olia/olia.owl#CollectivePronoun>
        a       <http://www.w3.org/2002/07/owl#Class> ;
        <http://www.w3.org/2000/01/rdf-schema#comment>
                "A pronoun that refers to all elements of a set." ;
        <http://www.w3.org/2000/01/rdf-schema#isDefinedBy>
                "http://www.isocat.org/datcat/DC-3006" ;
        <http://www.w3.org/2000/01/rdf-schema#subClassOf>
                <http://purl.org/olia/olia.owl#Pronoun> .

<http://purl.org/olia/olia.owl#Head>
        a       <http://www.w3.org/2002/07/owl#Class> ;
        <http://www.w3.org/2000/01/rdf-schema#comment>
                "\n\t\tHeads are single words that function as the nucleus of a phrase. For instance, the head of the noun\nphrase John’s book is book. Book is also the head of the more complex noun phrase that interesting book\nthat you were telling me about the other day. The head of the verb phrase telling me about the other day is\ntelling. The head of a prepositional phrase is the preposition.\n(Santorini 1991)\n\t\t" , "TIGER edge label HD" ;
        <http://www.w3.org/2000/01/rdf-schema#subClassOf>
                <http://purl.org/olia/olia-top.owl#SyntacticRole> ;
        <http://www.w3.org/2002/07/owl#versionInfo>
                "TIGER edge label HD, definition according to Penn Treebank Bracketing Guidelines (Santorini 1991)" .

<http://purl.org/olia/olia.owl#OtherAnimacy>
        a       <http://www.w3.org/2002/07/owl#Class> ;
        <http://www.w3.org/2000/01/rdf-schema#comment>
                "\n                            Perceived as related to animacy, but without specific reference to the previous items.\n                                (ISO12620; http://www.isocat.org/datcat/DC-1953)\n                            " ;
        <http://www.w3.org/2000/01/rdf-schema#label>
                "other animacy" ;
        <http://www.w3.org/2000/01/rdf-schema#subClassOf>
                <http://purl.org/olia/olia-top.owl#AnimacyFeature> ;
        <http://www.w3.org/2002/07/owl#versionInfo>
                "http://www.isocat.org/datcat/DC-1953" , "subClassOf animacy (dcif:conceptualDomain)" .

<http://purl.org/olia/olia.owl#RemoteFuture>
        a       <http://www.w3.org/2002/07/owl#Class> ;
        <http://www.w3.org/2000/01/rdf-schema#comment>
                "\n\t\t\tRemoteFutureTense locates the situation in question at a time that \n\t\t\tis considered relatively distant. It is characteristically after \n\t\t\tthe span of time culturally defined as 'tomorrow' (Dahl 1985:121; \n\t\t\tComrie 1985:94).\n\t\t\t(http://purl.org/linguistics/gold/RemoteFuture)\n\t\t" ;
        <http://www.w3.org/2000/01/rdf-schema#subClassOf>
                <http://purl.org/olia/olia.owl#Future> ;
        <http://www.w3.org/2002/07/owl#versionInfo>
                "http://purl.org/linguistics/gold/RemoteFuture, classified as Future here" .

<http://purl.org/olia/olia.owl#ComitativeCase>
        a       <http://www.w3.org/2002/07/owl#Class> ;
        <http://www.w3.org/2000/01/rdf-schema#comment>
                "\n\t\t\tComitativeCase expresses accompaniment. It carries the meaning 'with' \n\t\t\tor 'accompanied by' (Anderson, Stephen 1985: 186; Pei and Gaynor 1954: \n\t\t\t42;Dixon, R. 1972: 12; Gove, et al. 1966: 455).\n\t\t\t(http://purl.org/linguistics/gold/Comitative)\n\t\t" ;
        <http://www.w3.org/2000/01/rdf-schema#subClassOf>
                <http://purl.org/olia/olia-top.owl#CaseFeature> ;
        <http://www.w3.org/2002/07/owl#versionInfo>
                "http://purl.org/linguistics/gold/Comitative; http://www.isocat.org/datcat/DC-1255" .

<http://purl.org/olia/olia.owl#Comma>
        a       <http://www.w3.org/2002/07/owl#Class> ;
        <http://www.w3.org/2000/01/rdf-schema#comment>
                "\n                            Mark (,) used in writing to show a short pause or to separate items in a list.\n                                (Longman DCE 2005; http://www.isocat.org/datcat/DC-1448)\n                            " ;
        <http://www.w3.org/2000/01/rdf-schema#label>
                "comma" ;
        <http://www.w3.org/2000/01/rdf-schema#subClassOf>
                <http://purl.org/olia/olia.owl#SentenceMedialPunctuation> ;
        <http://www.w3.org/2002/07/owl#versionInfo>
                "http://www.isocat.org/datcat/DC-1448" , "subClassOf partOfSpeech (dcif:conceptualDomain)" .

<http://purl.org/olia/olia.owl#LetterNumeral>
        a       <http://www.w3.org/2002/07/owl#Class> ;
        <http://www.w3.org/2000/01/rdf-schema#comment>
                "Numeral expressed with letters." ;
        <http://www.w3.org/2000/01/rdf-schema#isDefinedBy>
                "http://www.isocat.org/datcat/DC-1937" ;
        <http://www.w3.org/2000/01/rdf-schema#subClassOf>
                <http://purl.org/olia/olia.owl#Numeral> , <http://purl.org/olia/olia.owl#String> .

<http://purl.org/olia/olia.owl#InfinitiveParticle>
        a       <http://www.w3.org/2002/07/owl#Class> ;
        <http://www.w3.org/2000/01/rdf-schema#comment>
                "\n                            Particle used to express infinitive.\n                                (http://www.isocat.org/datcat/DC-1896)\n                            " ;
        <http://www.w3.org/2000/01/rdf-schema#label>
                "infinitive particle" ;
        <http://www.w3.org/2000/01/rdf-schema#subClassOf>
                <http://purl.org/olia/olia.owl#VerbalParticle> ;
        <http://www.w3.org/2002/07/owl#versionInfo>
                "http://www.isocat.org/datcat/DC-1896, taxonomic organization follows http://purl.org/olia/mte/multext-east.owl#InfinitiveParticle" , "subClassOf particle (dcif:isA)" .

<http://purl.org/olia/olia.owl#AbsoluteRelativeTense>
        a       <http://www.w3.org/2002/07/owl#Class> ;
        <http://www.w3.org/2000/01/rdf-schema#comment>
                "\n\t\t\tAbsolute-relative tense is a tense that \n\t\t\t\t(i) refers to a time in relation to a temporal reference point that, \n\t\t\t\t\tin turn, is referred to in relation to the moment of utterance \n\t\t\t\t(ii) in which the time and the reference point are not identical, and \n\t\t\t\t(iii) the reference point and the moment of utterance are not identical.\n\t\t\t\t(http://languagelink.let.uu.nl/tds/onto/LinguisticOntology.owl#absoluteRelativeTense with\n\t\t\t\treference to http://www.sil.org/linguistics/glossaryoflinguisticterms/whatisabsoluterelativetense.htm)\n\t\t" ;
        <http://www.w3.org/2000/01/rdf-schema#label>
                "absolute-relative tense" ;
        <http://www.w3.org/2000/01/rdf-schema#subClassOf>
                <http://purl.org/olia/olia-top.owl#TenseFeature> ;
        <http://www.w3.org/2002/07/owl#versionInfo>
                "http://languagelink.let.uu.nl/tds/onto/LinguisticOntology.owl#absoluteRelativeTense" .

<http://purl.org/olia/olia.owl#VoiceParticle>
        a       <http://www.w3.org/2002/07/owl#Class> ;
        <http://www.w3.org/2000/01/rdf-schema#comment>
                "E.g., the mediopassive (middle) voice marker se in the Portuguese EAGLES scheme. (Leech and Wilson 1996)" ;
        <http://www.w3.org/2000/01/rdf-schema#subClassOf>
                <http://purl.org/olia/olia.owl#VerbalParticle> ;
        <http://www.w3.org/2002/07/owl#versionInfo>
                "generalization over EAGLES: http://purl.org/olia/eagles.owl#MediopassiveVoiceParticle" .

<http://purl.org/olia/olia.owl#DemonstrativeModifier>
        a       <http://www.w3.org/2002/07/owl#Class> ;
        <http://www.w3.org/2000/01/rdf-schema#comment>
                "\n\t\t\tA nominal is modified by a demonstrative.\n\t\t\t(http://languagelink.let.uu.nl/tds/onto/LinguisticOntology.owl#demonstrativeModifier)\n\t\t" ;
        <http://www.w3.org/2000/01/rdf-schema#subClassOf>
                <http://purl.org/olia/olia.owl#AdnominalConstituent> ;
        <http://www.w3.org/2002/07/owl#versionInfo>
                "http://languagelink.let.uu.nl/tds/onto/LinguisticOntology.owl#demonstrativeModifier" .

<http://purl.org/olia/olia.owl#Superlative>
        a       <http://www.w3.org/2002/07/owl#Class> ;
        <http://www.w3.org/2000/01/rdf-schema#comment>
                "\n\t\t\tThe superlative of an adjective or adverb is a form of adjective or \n\t\t\tadverb which indicates that something has some feature to a greater \n\t\t\tdegree than anything it is being compared to in a given context. \n\t\t\t(http://en.wikipedia.org/wiki/Superlative  17.11.06)\n\t\t" ;
        <http://www.w3.org/2000/01/rdf-schema#subClassOf>
                <http://purl.org/olia/olia-top.owl#DegreeFeature> ;
        <http://www.w3.org/2002/07/owl#versionInfo>
                "EAGLES, http://www.isocat.org/datcat/DC-1422" .

<http://purl.org/olia/olia.owl#SuperterminativeCase>
        a       <http://www.w3.org/2002/07/owl#Class> ;
        <http://www.w3.org/2000/01/rdf-schema#comment>
                "\n\t\t\tSuperterminativeCase expresses the notion of something moving into \n\t\t\tthe region over the referent of the noun it marks, but not through \n\t\t\tthat region. It has the meaning 'into the region over'.\n\t\t\t(http://purl.org/linguistics/gold/Superterminative)\n\t\t" ;
        <http://www.w3.org/2000/01/rdf-schema#subClassOf>
                <http://purl.org/olia/olia-top.owl#CaseFeature> ;
        <http://www.w3.org/2002/07/owl#versionInfo>
                "http://purl.org/linguistics/gold/Superterminative" .

<http://purl.org/olia/olia.owl#InflectedWithOvertMarker>
        a       <http://www.w3.org/2002/07/owl#Class> ;
        <http://www.w3.org/2000/01/rdf-schema#comment>
                "\n\t\t\tAn inflected form with overt morphological marking (as opposed to the base form and lexemes that do not inflect at all).\n\t\t" ;
        <http://www.w3.org/2000/01/rdf-schema#subClassOf>
                <http://purl.org/olia/olia.owl#Inflected> ;
        <http://www.w3.org/2002/07/owl#versionInfo>
                "Chiarcos, motivated by BaseForm in SUSANNE (Sampson 1995) and related schemes; cf. http://purl.org/olia/emille.owl#MarkedForGender" .

<http://purl.org/olia/olia.owl#SimpleCoordinatingConjunction>
        a       <http://www.w3.org/2002/07/owl#Class> ;
        <http://www.w3.org/2000/01/rdf-schema#comment>
                "\n\t\t\tSimple applies to the regular type of coordinator occurring between \n\t\t\tconjuncts: German und, for example. (http://www.ilc.cnr.it/EAGLES96/annotate/node18.html#oav1av  17.11.06)\n\t\t" , "In the Romanian MTE v4 specs, Conjunction/Coord_Type=\"simple\" is defined in contrast to repetitive and correlative coordinating conjunctions.\n\t\t\tIn Romanian, there are three kinds of conjunctions depending on their usage: as such or together with other conjunctions or adverbs: (1) simple, between conjuncts: Ion ori Maria (John or Mary); (2) repetitive, before each conjunct: fie Ion fie Maria fie... (either John or Mary or...) (3) correlative, before a conjoined phrase, it requires specific coordinators between conjuncts: atât mama cât şi tata (both mother and father). (MTE v4), e.g., aşa_că, va_să_zică (ro)\n\t\t\t(http://purl.org/olia/mte/multext-east.owl#SimpleCoordinatingConjunction)" ;
        <http://www.w3.org/2000/01/rdf-schema#subClassOf>
                <http://purl.org/olia/olia.owl#CoordinatingConjunction> ;
        <http://www.w3.org/2002/07/owl#versionInfo>
                "EAGLES, http://purl.org/olia/mte/multext-east.owl#SimpleCoordinatingConjunction" .

<http://purl.org/olia/olia.owl#FusedPronounAuxiliary>
        a       <http://www.w3.org/2002/07/owl#Class> ;
        <http://www.w3.org/2000/01/rdf-schema#comment>
                "word resulting from the aggregation of a pronoun and an auxiliary" ;
        <http://www.w3.org/2000/01/rdf-schema#isDefinedBy>
                "http://www.isocat.org/datcat/DC-3008" ;
        <http://www.w3.org/2000/01/rdf-schema#subClassOf>
                <http://purl.org/olia/olia.owl#Pronoun> , <http://purl.org/olia/olia.owl#AuxiliaryVerb> .

<http://purl.org/olia/olia.owl#PurposiveAspect>
        a       <http://www.w3.org/2002/07/owl#Class> ;
        <http://www.w3.org/2000/01/rdf-schema#comment>
                "The purposive aspect appears to add the notion of intention or probability, both negative and positive.\n\t\t(Steckley, 2007, p. 14, about Huron)\n\t\t\n\t\t(John Steckley, 2007, Words of the Huron, Wilfrid Laurier Univ. Press)\n\t\t" ;
        <http://www.w3.org/2000/01/rdf-schema#subClassOf>
                <http://purl.org/olia/olia-top.owl#AspectFeature> ;
        <http://www.w3.org/2002/07/owl#versionInfo>
                "adapted from ILPOSTS (for Indian languages), http://purl.org/olia/ilposts.owl#PurposiveAspect" .

<http://purl.org/olia/olia.owl#AllusivePronoun>
        a       <http://www.w3.org/2002/07/owl#Class> ;
        <http://www.w3.org/2000/01/rdf-schema#comment>
                "\n                            pronoun that have reference to something characterized by allusions.\n                                (MIRACL & LSCA; http://www.isocat.org/datcat/DC-2223)\n\t\t\t\t\t\t\t\n\t\t\t\t\t\t\tan invariable pronoun expressing a specific intention by means of unclear term\n\t\t\t\t\t\t\t(Khemakhem Aida, 2010-05-10 via isocat-morpho@loria.fr)\n\t\t\t\t\t\t\t\n\t\t\t\t\t\t\texamples from Arabic (Monica Monachini 2010-05-06 via isocat-morpho@loria.fr):\n\t\t\t\t\t\t\t\"kam nahaituhu\" (how often I forbade him, Hans Wehr),\n\t\t\t\t\t\t\t\"baas Saar `amra `ashr isniin, gam (= kam) yriid paysikil\" (He just turned ten, and here [how] he wants a bicycle, Georgetown University Iraqi Arabic-English Dictionary),\n\t\t\t\t\t\t\t\"gam (= kam) yurguS imnil-faraH\" ([how] he jumped for joy, Georgetown University Iraqi Arabic-English Dictionary)\n                            " ;
        <http://www.w3.org/2000/01/rdf-schema#label>
                "allusive pronoun" ;
        <http://www.w3.org/2000/01/rdf-schema#subClassOf>
                <http://purl.org/olia/olia.owl#Pronoun> ;
        <http://www.w3.org/2002/07/owl#versionInfo>
                "http://www.isocat.org/datcat/DC-2223" , "subClassOf pronoun (dcif:isA)" .

<http://purl.org/olia/olia.owl#RelativePronoun>
        a       <http://www.w3.org/2002/07/owl#Class> ;
        <http://www.w3.org/2000/01/rdf-schema#comment>
                "\n\t\t\tA relative pronoun is a pronoun that marks a relative clause, \n\t\t\tfunctions grammatically within the relative clause, and is \n\t\t\tcoreferential to the word modified by the relative clause.\n\t\t\t(http://www.sil.org/linguistics/GlossaryOfLinguisticTerms/WhatIsARelativePronoun.htm 19.09.06)\n\t\t" ;
        <http://www.w3.org/2000/01/rdf-schema#subClassOf>
                <http://purl.org/olia/olia.owl#WHPronoun> ;
        <http://www.w3.org/2002/07/owl#versionInfo>
                "EAGLES WHPronoun with Wh-Type=\"Relative\"." .

<http://purl.org/olia/olia.owl#DativeCase>
        a       <http://www.w3.org/2002/07/owl#Class> ;
        <http://www.w3.org/2000/01/rdf-schema#comment>
                "\n\t\t\tDative case marks indirect objects (for languages in which they are held to exist), or \n\t\t\tnouns having the role of a recipient (as of things given), \n\t\t\ta beneficiary of an action, or a possessor of an item. \t\t\t\n\t\t\t(http://www.sil.org/linguistics/glossaryoflinguisticterms/WhatIsDativeCase.htm  17.11.06)\n\t\t" ;
        <http://www.w3.org/2000/01/rdf-schema#subClassOf>
                <http://purl.org/olia/olia-top.owl#CaseFeature> ;
        <http://www.w3.org/2002/07/owl#versionInfo>
                "EAGLES" .

<http://purl.org/olia/olia.owl#ComparativeParticle>
        a       <http://www.w3.org/2002/07/owl#Class> ;
        <http://www.w3.org/2000/01/rdf-schema#comment>
                "\n                            Particle used to compare.\n                                (http://www.isocat.org/datcat/DC-1922)\n                            " ;
        <http://www.w3.org/2000/01/rdf-schema#label>
                "comparative particle" ;
        <http://www.w3.org/2000/01/rdf-schema#subClassOf>
                <http://purl.org/olia/olia.owl#Particle> ;
        <http://www.w3.org/2002/07/owl#versionInfo>
                "http://www.isocat.org/datcat/DC-1922" , "subClassOf particle (dcif:isA)" .

<http://purl.org/olia/olia.owl#AttributivePronoun>
        a       <http://www.w3.org/2002/07/owl#Class> ;
        <http://www.w3.org/2000/01/rdf-schema#comment>
                "\n\t\t\tAn attributive pronoun is a pronoun that modifies an NP.\n\t\t" ;
        <http://www.w3.org/2000/01/rdf-schema#subClassOf>
                <http://purl.org/olia/olia.owl#Determiner> , <http://purl.org/olia/olia.owl#Pronoun> ;
        <http://www.w3.org/2002/07/owl#equivalentClass>
                [ a       <http://www.w3.org/2002/07/owl#Class> ;
                  <http://www.w3.org/2002/07/owl#intersectionOf>
                          ( <http://purl.org/olia/olia.owl#Determiner> <http://purl.org/olia/olia.owl#Pronoun> )
                ] ;
        <http://www.w3.org/2002/07/owl#versionInfo>
                "\n\t\t\tIn languages with grammaticalized determiners, attributive pronouns are determiners. \n\t\t\tIn languages without grammaticalized determiners, attributive pronouns are described as adjectives.\n\t\t\tIn order to provide a uniform modeling of attributive pronouns, they are defined here as being the intersection of Determiner and Pronoun.\n\t\t\tNote that this entails that the definition of \"Determiner\" is broadened to include determiner-like elements in languages without grammatical determiners.\n\t\t\t(Chiarcos)\n\t\t" .

<http://purl.org/olia/olia.owl#Simple>
        a       <http://www.w3.org/2002/07/owl#Class> ;
        <http://www.w3.org/2000/01/rdf-schema#comment>
                "\n\t\t\tSimple applies to the regular type of coordinator occurring between \n\t\t\tconjuncts: German und, for example. (http://www.ilc.cnr.it/EAGLES96/annotate/node18.html#oav1av  17.11.06)\n\t\t" ;
        <http://www.w3.org/2000/01/rdf-schema#subClassOf>
                <http://purl.org/olia/olia-top.owl#CoordTypeFeature> ;
        <http://www.w3.org/2002/07/owl#deprecated>
                true ;
        <http://www.w3.org/2002/07/owl#versionInfo>
                "EAGLES" .

<http://purl.org/olia/olia.owl#DualQuantifier>
        a       <http://www.w3.org/2002/07/owl#Class> ;
        <http://www.w3.org/2000/01/rdf-schema#comment>
                "Quantifiers that enforce dual agreement (i.e., as with the numeral \"2\").\n\t\t\tSome feminine and neuter body parts in Czech have preserved dual forms, and if the noun is dual, so are its attributes (adjectives, pronouns).  So the agreement of the numeral 2 differs formally from 3-4 (Ivan A. Derzhanski, email 2010/06/16, http://purl.org/olia/mte/multext-east.owl#DualQuantifier)\n\t\t\tNumeral/Class=\"definite\", Numeral/Class=\"definite1\", Numeral/Class=\"definite234\" etc. refer to specific patterns of congruency with Slavic numerals that originate from the difference between Old Slavic singular (definite1), dual (definite2, definite234) and plural (definite). (http://purl.org/olia/mte/multext-east.owl#DualQuantifier)\n\t\t" ;
        <http://www.w3.org/2000/01/rdf-schema#subClassOf>
                <http://purl.org/olia/olia-top.owl#NumeralAgreementClass> ;
        <http://www.w3.org/2002/07/owl#equivalentClass>
                [ a       <http://www.w3.org/2002/07/owl#Class> ;
                  <http://www.w3.org/2002/07/owl#intersectionOf>
                          ( <http://purl.org/olia/olia.owl#Quantifier>
                            [ a       <http://www.w3.org/2002/07/owl#Restriction> ;
                              <http://www.w3.org/2002/07/owl#onProperty>
                                      <http://purl.org/olia/olia.owl#hasNumeralAgreementClass> ;
                              <http://www.w3.org/2002/07/owl#someValuesFrom>
                                      <http://purl.org/olia/olia.owl#DualQuantifier>
                            ]
                          )
                ] ;
        <http://www.w3.org/2002/07/owl#versionInfo>
                "http://purl.org/olia/mte/multext-east.owl#DualQuantifier" .

<http://purl.org/olia/olia.owl#InverseVoice>
        a       <http://www.w3.org/2002/07/owl#Class> ;
        <http://www.w3.org/2000/01/rdf-schema#comment>
                "\n\t\t\tSignals when actions proceed from ontologically less salient to more \n\t\t\tsalient participants (Klaiman 1991:32)\n\t\t\t(http://purl.org/linguistics/gold/InverseVoice)\n\t\t" ;
        <http://www.w3.org/2000/01/rdf-schema#subClassOf>
                <http://purl.org/olia/olia.owl#PassiveVoice> ;
        <http://www.w3.org/2002/07/owl#versionInfo>
                "http://purl.org/linguistics/gold/InverseVoice" .

<http://purl.org/olia/olia.owl#RelativeTense>
        a       <http://www.w3.org/2002/07/owl#Class> ;
        <http://www.w3.org/2000/01/rdf-schema#comment>
                "\n\t\tRelative tense is a tense that refers to a time in relation to a contextually \n\t\tdetermined temporal reference point, regardless of the latter’s temporal \n\t\trelation to the moment of utterance. \n\t\t(http://languagelink.let.uu.nl/tds/onto/LinguisticOntology.owl#relativeTense \n\t\twith reference to http://www.sil.org/linguistics/glossaryoflinguisticterms/whatisrelativetense.htm)\n\t" ;
        <http://www.w3.org/2000/01/rdf-schema#label>
                "relative tense" ;
        <http://www.w3.org/2000/01/rdf-schema#subClassOf>
                <http://purl.org/olia/olia-top.owl#TenseFeature> ;
        <http://www.w3.org/2002/07/owl#versionInfo>
                "http://languagelink.let.uu.nl/tds/onto/LinguisticOntology.owl#relativeTense" .

<http://purl.org/olia/olia.owl#VocativeExpression>
        a       <http://www.w3.org/2002/07/owl#Class> ;
        <http://www.w3.org/2000/01/rdf-schema#comment>
                "An expression referring to a person to which the utterance is addressed, e.g. Old High German \"truhtin\",  \"meistar\" or \"fater\". The vocative expression typically occurs outside of the clause and not in an argument position selected by the predicate. (Petrova 2008, see http://purl.org/olia/tcodex.owl)" ;
        <http://www.w3.org/2000/01/rdf-schema#label>
                "vocative expression" ;
        <http://www.w3.org/2000/01/rdf-schema#subClassOf>
                <http://purl.org/olia/olia-top.owl#DiscourseEntity> ;
        <http://www.w3.org/2002/07/owl#versionInfo>
                "http://purl.org/olia/tcodex.owl#VocativeForm" .

<http://purl.org/olia/olia.owl#ParentheticalPunctuation>
        a       <http://www.w3.org/2002/07/owl#Class> ;
        <http://www.w3.org/2000/01/rdf-schema#comment>
                "Parenthetical elements are dominated by a node labeled PRN. Punctuation marks that set off a parenthetical (i.e., commas, dashes, parentheses (-LRB- and -RRB-)) are contained within the PRN node. Use of PRN is determined ultimately by individual annotator intuition, though the presence of dashes or parentheses strongly suggests a parenthetical. \n(Bies et al. 1995)" ;
        <http://www.w3.org/2000/01/rdf-schema#subClassOf>
                <http://purl.org/olia/olia.owl#SecondaryPunctuation> ;
        <http://www.w3.org/2002/07/owl#versionInfo>
                "added in conformance with Penn Treebank Bracketing Guidelines (Bies et al. 1995)" .

<http://purl.org/olia/olia.owl#IntensiveNoun>
        a       <http://www.w3.org/2002/07/owl#Class> ;
        <http://www.w3.org/2000/01/rdf-schema#comment>
                "noun that emphasizes another noun" ;
        <http://www.w3.org/2000/01/rdf-schema#isDefinedBy>
                "http://www.isocat.org/datcat/DC-3859" ;
        <http://www.w3.org/2000/01/rdf-schema#subClassOf>
                <http://purl.org/olia/olia.owl#CommonNoun> ;
        <http://www.w3.org/2002/07/owl#deprecated>
                true ;
        <http://www.w3.org/2002/07/owl#equivalentClass>
                [ a       <http://www.w3.org/2002/07/owl#Class> ;
                  <http://www.w3.org/2002/07/owl#intersectionOf>
                          ( <http://purl.org/olia/olia.owl#CommonNoun>
                            [ a       <http://www.w3.org/2002/07/owl#Restriction> ;
                              <http://www.w3.org/2002/07/owl#onProperty>
                                      <http://purl.org/olia/olia.owl#hasEmphasis> ;
                              <http://www.w3.org/2002/07/owl#someValuesFrom>
                                      <http://purl.org/olia/olia.owl#Emphatic>
                            ]
                          )
                ] ;
        <http://www.w3.org/2002/07/owl#versionInfo>
                "deprecated, as merely a shorthand for CommonNoun and hasEmphasis some Emphatic" .

<http://purl.org/olia/olia.owl#GeneralizationWord>
        a       <http://www.w3.org/2002/07/owl#Class> ;
        <http://www.w3.org/2000/01/rdf-schema#comment>
                "A word that does not carry its own meaning but generalizes the meaning of a neighboring word, adding the \"etc.\" sense." ;
        <http://www.w3.org/2000/01/rdf-schema#isDefinedBy>
                "http://www.isocat.org/datcat/DC-3033" ;
        <http://www.w3.org/2000/01/rdf-schema#subClassOf>
                <http://purl.org/olia/olia.owl#Residual> .

<http://purl.org/olia/olia.owl#MainPunctuation>
        a       <http://www.w3.org/2002/07/owl#Class> ;
        <http://www.w3.org/2000/01/rdf-schema#comment>
                "\n                            Punctuation that is more important than a secondary punctuation with regards to sentence splitting in a text.\n                                (http://www.isocat.org/datcat/DC-2075)\n                            " ;
        <http://www.w3.org/2000/01/rdf-schema#label>
                "main punctuation" ;
        <http://www.w3.org/2000/01/rdf-schema#subClassOf>
                <http://purl.org/olia/olia.owl#Punctuation> ;
        <http://www.w3.org/2002/07/owl#versionInfo>
                "http://www.isocat.org/datcat/DC-2075" , "subClassOf punctuation (dcif:isA)" .

<http://purl.org/olia/olia.owl#IndefiniteQuantifier>
        a       <http://www.w3.org/2002/07/owl#Class> ;
        <http://www.w3.org/2000/01/rdf-schema#comment>
                "In the Czech and Slovak MTE v4 specs, Numeral/Class=\"indefinite\" are items meaning `several/some',  etc. Strictly speaking, they are pronumerals (pro-quantifiers), but traditional descriptions don't recognise such a category, so they are described variously as pronouns or as numerals (because their syntactic distribution is that of numerals, or very close).\" (Ivan A Derzhanski, email 2010/06/11, http://purl.org/olia/mte/multext-east.owl#IndefiniteQuantifier)" ;
        <http://www.w3.org/2000/01/rdf-schema#subClassOf>
                <http://purl.org/olia/olia.owl#ProQuantifier> ;
        <http://www.w3.org/2002/07/owl#versionInfo>
                "http://purl.org/olia/mte/multext-east.owl#IndefiniteQuantifier" .

<http://purl.org/olia/olia.owl#ForceRole>
        a       <http://www.w3.org/2002/07/owl#Class> ;
        <http://www.w3.org/2000/01/rdf-schema#comment>
                "\n\t\tA force role is one in which the instantiator (the “force”) exerts \n        some degree of energy which initiates (or impacts on) the execution of \n        the event. In contrast to an agent, an instantitor of a force may be \n        an inanimate entity, such as a climactic condition.\n        The non-controlling entity instigating a Process (=Dynamism or Change) \n        (Dik, 1997:118)\n\t\t(http://languagelink.let.uu.nl/tds/onto/LinguisticOntology.owl#forceRole)\n\t\t" ;
        <http://www.w3.org/2000/01/rdf-schema#subClassOf>
                <http://purl.org/olia/olia.owl#ActorMacroRole> ;
        <http://www.w3.org/2002/07/owl#versionInfo>
                "http://languagelink.let.uu.nl/tds/onto/LinguisticOntology.owl#forceRole" .

<http://purl.org/olia/olia.owl#DistributivePronoun>
        a       <http://www.w3.org/2002/07/owl#Class> ;
        <http://www.w3.org/2000/01/rdf-schema#comment>
                "\n\t\t\tWhen the subject is conjoined, the reflexive cannot refer to only one of them. The proform has to be a distributive pronoun, i.e., the reduplicated form, when it has coreference to respective subjects, e.g.,\t\t\t\n\t\t\t*kumaarum_i/Kumar.and umaavum_j/Uma.and tan_i+j/self-poss puunekki/cat.to paalu/milk kuDuttaanaanga/give-pst-aggr.\n\t\t\t\"*Kumar_i and Uma gave milk to his_i/her_j cat.\"\n\t\t\t(Annamalai 2000, p. 189, on Tamil)\n\t\t\t\n\t\t\tUnlike reciprocals, the two parts of a distributive pronoun cannot be considered as two full, independent NPs. In \"awar/1 awar/2\", only \"awar/2\" is case marked; \"awar/1\" is its citation form. Also, the two parts cannot be separated by intervening material (cf. English \"one another\").\n\t\t\t(Jayaseelan 2000, p. 149, on Malayalam)\n\t\t\n\t\t(K.A. Jayaseelan, 2000, Lexical anaphors and pronouns in Malayalam, In: Barbara C. Lust, Kashi Wali, James W. Gair, K.V.Subharao (eds.), Lexical Anaphors and Pronouns in Selected South Asian Languages. A Principled Typology, Mouton de Gruyter, Berlin, p. 113-168)\n\t\t(E. Annamalai, 2000, Lexical anaphors and pronouns in Tamil, , In: Barbara C. Lust, Kashi Wali, James W. Gair, K.V.Subharao (eds.), Lexical Anaphors and Pronouns in Selected South Asian Languages. A Principled Typology, Mouton de Gruyter, Berlin, p. 169-216)\n\t\t" ;
        <http://www.w3.org/2000/01/rdf-schema#subClassOf>
                <http://purl.org/olia/olia.owl#Pronoun> ;
        <http://www.w3.org/2002/07/owl#versionInfo>
                "adopted from ILPOSTS (for Indian languages), http://purl.org/olia/ilposts.owl#Distributivity is a property of Pronominals" .

<http://purl.org/olia/olia.owl#RelationalAdjective>
        a       <http://www.w3.org/2002/07/owl#Class> ;
        <http://www.w3.org/2000/01/rdf-schema#comment>
                "The Slovene adjective expresses three main ideas: quality (qualitative adjectives, kakovostni pridevniki), relation (relational adjectives, vrstni pridevniki) and possession (possessive adjectives, svojilni pridevniki).\n\t\t\tRelational adjectives express type, class or numerical sequence of a noun. For instance: kemijska in fizikalna sprememba (chemical and physical change), fotografski aparat (photographic device (=camera)). (http://en.wikipedia.org/wiki/Slovene_grammar)" ;
        <http://www.w3.org/2000/01/rdf-schema#label>
                "relational adjective" ;
        <http://www.w3.org/2000/01/rdf-schema#subClassOf>
                <http://purl.org/olia/olia.owl#Adjective> ;
        <http://www.w3.org/2002/07/owl#versionInfo>
                "cf. OrdinalAdjective" .

<http://purl.org/olia/olia.owl#SimplePast>
        a       <http://www.w3.org/2002/07/owl#Class> ;
        <http://www.w3.org/2000/01/rdf-schema#comment>
                "\n\t\t\tPastTense locates the situation in question prior to the present moment, \n\t\t\twith no specification on the distance in time (Comrie 1985).\n\t\t\t(http://purl.org/linguistics/gold/Past)\n\t\t" ;
        <http://www.w3.org/2000/01/rdf-schema#subClassOf>
                <http://purl.org/olia/olia.owl#Past> ;
        <http://www.w3.org/2002/07/owl#versionInfo>
                "http://purl.org/linguistics/gold/Past" .

<http://purl.org/olia/olia.owl#MainClause>
        a       <http://www.w3.org/2002/07/owl#Class> ;
        <http://www.w3.org/2000/01/rdf-schema#comment>
                "\n\t\t\tMainClause is the class of clauses that can stand on their own as a full, independent sentence. \n\t\t\tIf a sentence contains any embedded clauses, the main clause is understood as the matrix plus \n\t\t\tthe embedded clauses. In the sentence 'John thinks that Mary is sick', 'John thinks that Mary \n\t\t\tis sick' is the main clause [Crystal 2001, 231].\n\t\t\t(http://purl.org/linguistics/gold/MainClause)\n\n\t\t\tThe independent clause can stand by itself as a grammatically viable simple sentence. Multiple \n\t\t\tindependent clauses can be joined (usually with a comma and a coordinating conjunction) to form \n\t\t\ta compound sentence (http://languagelink.let.uu.nl/tds/onto/LinguisticOntology.owl#mainClause \n\t\t\twith reference to http://en.wikipedia.org/wiki/Clause).\n\t\t" ;
        <http://www.w3.org/2000/01/rdf-schema#subClassOf>
                <http://purl.org/olia/olia.owl#FiniteClause> .

<http://purl.org/olia/olia.owl#AbsolutiveCase>
        a       <http://www.w3.org/2002/07/owl#Class> ;
        <http://www.w3.org/2000/01/rdf-schema#comment>
                "\n\t\t\tAbsolutive case marks the first argument of an intransitive verb and the \n\t\t\tsecond argument of a transitive verb in ergative-absolutive languages.\n\t\t\t(http://languagelink.let.uu.nl/tds/onto/LinguisticOntology.owl#absolutiveCase)\n\t\t" ;
        <http://www.w3.org/2000/01/rdf-schema#subClassOf>
                <http://purl.org/olia/olia-top.owl#CaseFeature> ;
        <http://www.w3.org/2002/07/owl#versionInfo>
                "TDS Ontology, http://www.isocat.org/datcat/DC-1225" .

<http://purl.org/olia/olia.owl#WHPrepositionalPhrase>
        a       <http://www.w3.org/2002/07/owl#Class> ;
        <http://www.w3.org/2000/01/rdf-schema#comment>
                "WHPP|Wh-prepositional phrase. Prepositional phrase containing a wh-determiner, as in by whatever\nmeans necessary.\n(Santorini 1991)\n\nWHPP â ´ Wh-prepositional Phrase. Prepositional phrase containing a wh-noun phrase (such as of which or by whose authority) that either introduces a PP gap or is contained by a WHNP. \n(Bies et al. 1995)" ;
        <http://www.w3.org/2000/01/rdf-schema#subClassOf>
                <http://purl.org/olia/olia.owl#PrepositionalPhrase> ;
        <http://www.w3.org/2002/07/owl#versionInfo>
                "added in conformance with PTB bracketing guidelines (Santorini 1991, Bies et al. 1995)" .

<http://purl.org/olia/olia.owl#hasMovementFeature>
        a       <http://www.w3.org/2002/07/owl#ObjectProperty> ;
        <http://www.w3.org/2000/01/rdf-schema#domain>
                <http://purl.org/olia/system.owl#UnitOfAnnotation> ;
        <http://www.w3.org/2000/01/rdf-schema#range>
                <http://purl.org/olia/olia-top.owl#MovementFeature> ;
        <http://www.w3.org/2000/01/rdf-schema#subPropertyOf>
                <http://purl.org/olia/system.owl#hasFeature> .

<http://purl.org/olia/olia.owl#BoundClitic>
        a       <http://www.w3.org/2002/07/owl#Class> ;
        <http://www.w3.org/2000/01/rdf-schema#comment>
                "Linked to a particular element.\n                                (http://www.isocat.org/datcat/DC-1933)\n                            " ;
        <http://www.w3.org/2000/01/rdf-schema#label>
                "bound" ;
        <http://www.w3.org/2000/01/rdf-schema#subClassOf>
                <http://purl.org/olia/olia.owl#CliticElement> ;
        <http://www.w3.org/2002/07/owl#versionInfo>
                "subClassOf cliticness (dcif:conceptualDomain)" , "http://www.isocat.org/datcat/DC-1933 (bound as value of cliticness http://www.isocat.org/datcat/DC-1933), originally from MULTEXT-East, see http://purl.org/olia/mte/multext-east.owl#BoundClitic, but note that as it is used in MULTEXT-East, BoundClitic is ambiguous between \"being\" a bound clitic and \"containing a bound clitic\". Here, only the first aspect is preserved, is is thus a subclass of CliticElement." .

<http://purl.org/olia/olia.owl#PossessionMarker>
        a       <http://www.w3.org/2002/07/owl#Class> ;
        <http://www.w3.org/2000/01/rdf-schema#comment>
                "In Urdu, wālā can be added to substantives to derive nouns implying possession or general relationships, e.g., go-wāl, or \n\t\t\tgo-wālā, s.m. cow-keeper, cow-herd (from go, 'cow'), or ghar-wālā, s.m. master or owner of the house (from ghar, \n\t\t\t'house') (Plats 1884, cf. http://purl.org/olia/urdu.owl#Wala)" ;
        <http://www.w3.org/2000/01/rdf-schema#subClassOf>
                <http://purl.org/olia/olia.owl#Unique> ;
        <http://www.w3.org/2002/07/owl#versionInfo>
                "introduced for Urdu wala, as used in the tagset by Sajjad (2007, http://purl.org/olia/urdu.owl#Wala)" .

<http://purl.org/olia/olia.owl#FacetiousRegister>
        a       <http://www.w3.org/2002/07/owl#Class> ;
        <http://www.w3.org/2000/01/rdf-schema#comment>
                "\n                            Register related to an expression that is intended to be clever and funny but that is really silly and annoying.\n                                (Longma DCE; http://www.isocat.org/datcat/DC-1991)\n                            " ;
        <http://www.w3.org/2000/01/rdf-schema#label>
                "facecious register" ;
        <http://www.w3.org/2000/01/rdf-schema#subClassOf>
                <http://purl.org/olia/olia-top.owl#RegisterFeature> ;
        <http://www.w3.org/2002/07/owl#versionInfo>
                "http://www.isocat.org/datcat/DC-1991" , "subClassOf register (dcif:conceptualDomain)" .

<http://purl.org/olia/olia.owl#MiddleVoice>
        a       <http://www.w3.org/2002/07/owl#Class> ;
        <http://www.w3.org/2000/01/rdf-schema#comment>
                "\n\t\t\tA verb that appears active but expresses a passive action may be called middle voice, e.g. \n\t\t\t'The chicken cooked in the oven'. In Greek the middle voice is often reflexive expressing a\n\t\t\tcausative reading or that the action is performed for one's own benefit.\n\t\t\t(http://languagelink.let.uu.nl/tds/onto/LinguisticOntology.owl#middleVoice)\n\t\t" ;
        <http://www.w3.org/2000/01/rdf-schema#subClassOf>
                <http://purl.org/olia/olia-top.owl#VoiceFeature> ;
        <http://www.w3.org/2002/07/owl#versionInfo>
                "http://languagelink.let.uu.nl/tds/onto/LinguisticOntology.owl#middleVoice" .

<http://purl.org/olia/olia.owl#Negation>
        a       <http://www.w3.org/2002/07/owl#Class> ;
        <http://www.w3.org/2000/01/rdf-schema#comment>
                "denotes the negation or the absence (http://www.isocat.org/datcat/DC-1839)\n\t\thttp://purl.org/olia/mte/multext-east.owl#Negated: Negative=\"yes\" encodes negative verbal word-forms in Slavic languages and Estonian. (MTE v4) \n    \tIn Slovak, for example, verbs form negative by prefix 'ne-', with the exception of the verb \"byť\" (E. \"to be\") which forms the negative in indicative by using separate particle \"nie\", e.g. \"nie je\" (is not). Here, Slovak \"je\" would be marked as negative, despite having positive form. In Resian, negative is always marked as 'n' except for two verbs: 'nïman' / not to have, 'nïsi' / not to be. (MTE v4)" ;
        <http://www.w3.org/2000/01/rdf-schema#isDefinedBy>
                "http://www.isocat.org/datcat/DC-1839" ;
        <http://www.w3.org/2000/01/rdf-schema#label>
                "negative" ;
        <http://www.w3.org/2000/01/rdf-schema#subClassOf>
                <http://purl.org/olia/olia-top.owl#PolarityFeature> .

<http://purl.org/olia/olia-top.owl#SemanticUnit>
        a       <http://www.w3.org/2002/07/owl#Class> .

<http://purl.org/olia/olia.owl#Possible>
        a       <http://www.w3.org/2002/07/owl#Class> ;
        <http://www.w3.org/2000/01/rdf-schema#comment>
                "Value that denotes a linguistic situation considered as being correct in the given language" ;
        <http://www.w3.org/2000/01/rdf-schema#isDefinedBy>
                "http://www.isocat.org/datcat/DC-1865" ;
        <http://www.w3.org/2000/01/rdf-schema#subClassOf>
                <http://purl.org/olia/olia-top.owl#UsageAndFrequencyFeature> .

<http://purl.org/olia/olia.owl#ThirdPersonPronoun>
        a       <http://www.w3.org/2002/07/owl#Class> ;
        <http://www.w3.org/2000/01/rdf-schema#comment>
                "\n\t\t\tThird person reference is a deictic reference to a referent(s) not identified as the speaker or addressee.\n\t\t\t(http://www.sil.org/linguistics/GlossaryOfLinguisticTerms/WhatIsThirdPersonDeixis.htm 19.09.06)\n\t\t" ;
        <http://www.w3.org/2000/01/rdf-schema#subClassOf>
                <http://purl.org/olia/olia.owl#PersReflPronoun> ;
        <http://www.w3.org/2002/07/owl#versionInfo>
                "\n\t\t\tEAGLES Pronoun with Person=\"Third\". As only personal and reflexive pronouns show person differentiation,\n\t\t\tThirdPersonPronoun is modelled as a subclass of PersReflConcept here.\n\t\t" .

<http://purl.org/olia/olia.owl#PostNominalModifier>
        a       <http://www.w3.org/2002/07/owl#Class> ;
        <http://www.w3.org/2000/01/rdf-schema#comment>
                "\n\t\t\tPostmodifying is a function of an adjective that can modify, describe, or qualify a preceding noun.\n\t\t\t(EAGLES)\n\t\t\tmodificationType: Refers to the prenominal or postnominal positions of determiners which distinguish different forms. (http://www.isocat.org/datcat/DC-1931)" ;
        <http://www.w3.org/2000/01/rdf-schema#subClassOf>
                <http://purl.org/olia/olia.owl#AdnominalConstituent> ;
        <http://www.w3.org/2002/07/owl#versionInfo>
                "EAGLES, NPFunction=\"postmodifying\", http://www.isocat.org/datcat/DC-1945 (without restriction on nominal heads ?)" .

<http://purl.org/olia/olia.owl#LocativeCase>
        a       <http://www.w3.org/2002/07/owl#Class> ;
        <http://www.w3.org/2000/01/rdf-schema#comment>
                "\n\t\tCase that indicates a final location of action or a time of the action. (http://www.isocat.org/datcat/DC-1326)\n\t\t"@en ;
        <http://www.w3.org/2000/01/rdf-schema#label>
                "locative case"@en ;
        <http://www.w3.org/2000/01/rdf-schema#subClassOf>
                <http://purl.org/olia/olia-top.owl#CaseFeature> ;
        <http://www.w3.org/2002/07/owl#versionInfo>
                "http://www.isocat.org/datcat/DC-1326" .

<http://purl.org/olia/olia.owl#SpecificArticle>
        a       <http://www.w3.org/2002/07/owl#Class> ;
        <http://www.w3.org/2000/01/rdf-schema#comment>
                "\n\t\t\t\"By ʻspecificʼ and ʻnon-specificʼ I intend the difference between the\n\t\t\ttwo readings of English indefinites like (3):\n\t\t\t\n\t\t\t(3) Iʼm looking for a deer.\n\t\t\t\n\t\t\tIn the specific reading there is a particular deer, say Bambi, that I am\n\t\t\tlooking for. In the non-specific reading I will be happy to find any deer.\n\t\t\tVon Heusinger (2002) likes the test in English of inserting ʻcertainʼ after the\n\t\t\tʻaʼ to fix the specific reading. In either reading of (3) a deer is being\n\t\t\tintroduced as a new discourse referent. This is opposed to ʻdefiniteʼ which\n\t\t\trequires a previous pragmatic instantiation as in ʻIʼm looking for the deer.ʼ\n\t\t\tIn English both the readings of (3) are indefinite. In Klallam, the specific\n\t\t\tdemonstratives are neither definite nor indefinite.\"\n\t\t\t(Montler, Timothy. 2007. Klallam demonstratives. Papers ICSNL XLVII. The 42nd International Conference on Salish and Neighbouring Language, pp. 409-425. University of British Columbia Working Papers in Linguistics, Volume 20; on specific vs. nonspecific determiners in Klallam, a Salish language, http://montler.net/papers/KlallamDemons.pdf)\n\t\t" ;
        <http://www.w3.org/2000/01/rdf-schema#label>
                "specific determiner"@en , "specific article"@en ;
        <http://www.w3.org/2000/01/rdf-schema#subClassOf>
                <http://purl.org/olia/olia.owl#Article> ;
        <http://www.w3.org/2002/07/owl#versionInfo>
                "introduced to account for the specific determiner in Farsi (http://purl.org/olia/mte/multext-east.owl#CliticSpecificDeterminer)" .

<http://purl.org/olia/olia.owl#hasOwnerNumber>
        a       <http://www.w3.org/2002/07/owl#ObjectProperty> ;
        <http://www.w3.org/2000/01/rdf-schema#comment>
                "\n\t\t\t\tThe EAGLES-recommended attribute Possessive accounts for the fact that a possessive \n\t\t\t\tpronoun or possessive determiner may have two different numbers. This attribute handles \n\t\t\t\tthe number which is inherent to the possessive form (e.g. Italian \"(la) mia\", \"(la) \n\t\t\t\tnostra\" as first-person singular and first-person plural) as contrasted with the number \n\t\t\t\tit has by virtue of agreeing with a particular noun (e.g. Italian \"(la) mia\", \"(le) mie)\".  \t\t\n\t\t\t\t(http://www.ilc.cnr.it/EAGLES96/annotate/node17.html#recc  20.11.06)\n\t\t\n                Indication concerning the number of the person that ownes something.\n                (http://www.isocat.org/datcat/DC-1417)\n\t\t\t\t\t\t\t\t\n\t\t\t\tInherent plural or singular of possessive pronouns and possessive determiners.\n\t\t" ;
        <http://www.w3.org/2000/01/rdf-schema#label>
                "owner number" ;
        <http://www.w3.org/2000/01/rdf-schema#subPropertyOf>
                <http://purl.org/olia/system.owl#hasFeature> ;
        <http://www.w3.org/2002/07/owl#versionInfo>
                "\n\t\tEAGLES feature for the inherent plural/singular of possessive pronouns and possessive determiners;\n\t\thttp://www.isocat.org/datcat/DC-1417, does not entail hasNumber (against hasOwnedNumber), \n\t\tbecause hasNumber applies to agreement information\n\t  " .

<http://purl.org/olia/olia.owl#RelativeClause>
        a       <http://www.w3.org/2002/07/owl#Class> ;
        <http://www.w3.org/2000/01/rdf-schema#comment>
                "\n\t\t\tA relative clause is a subordinate clause that modifies a noun. For example, the noun phrase \n\t\t\t[the man who wasn't there] contains the noun [man], which is modified by the relative clause \n\t\t\t[who wasn't there]\n\t\t\t(http://languagelink.let.uu.nl/tds/onto/LinguisticOntology.owl#relativeClause with reference \n\t\t\tto  http://en.wikipedia.org/wiki/Relative_clause and Dik 1997)\n\t\t\t\n\t\t\tThere are three di erent types of relative clauses in English (be careful not to confuse relative clauses\n\t\t\tand complement clauses):\n\t\t\t(i) wh-relative clauses (a guy who(m) I know),\n\t\t\t(ii) that-relative clauses (a guy that I know), and\n\t\t\t(iii) zero relative clauses (a guy I know).\n\t\t\t(Santorini 1991)\n\t\t" ;
        <http://www.w3.org/2000/01/rdf-schema#subClassOf>
                <http://purl.org/olia/olia.owl#SubordinateClause> ;
        <http://www.w3.org/2002/07/owl#versionInfo>
                "http://languagelink.let.uu.nl/tds/onto/LinguisticOntology.owl#relativeClause" .

<http://purl.org/olia/olia.owl#PresentParticiple>
        a       <http://www.w3.org/2002/07/owl#Class> ;
        <http://www.w3.org/2000/01/rdf-schema#subClassOf>
                <http://purl.org/olia/olia.owl#Participle> ;
        <http://www.w3.org/2002/07/owl#equivalentClass>
                [ a       <http://www.w3.org/2002/07/owl#Class> ;
                  <http://www.w3.org/2002/07/owl#intersectionOf>
                          ( <http://purl.org/olia/olia.owl#Participle>
                            [ a       <http://www.w3.org/2002/07/owl#Restriction> ;
                              <http://www.w3.org/2002/07/owl#onProperty>
                                      <http://purl.org/olia/olia.owl#hasTense> ;
                              <http://www.w3.org/2002/07/owl#someValuesFrom>
                                      <http://purl.org/olia/olia.owl#Present>
                            ]
                          )
                ] ;
        <http://www.w3.org/2002/07/owl#versionInfo>
                "introduced as a shorthand for Participle and hasTense some Present" .

<http://purl.org/olia/olia.owl#AnimateGender>
        a       <http://www.w3.org/2002/07/owl#Class> ;
        <http://www.w3.org/2000/01/rdf-schema#comment>
                "\n\t\t\tOne of the two grammatical genders, or classes of nouns, the other being inanimate. \n\t\t\tMembership in the animate grammatical class is largely based on meanings, in that living things, \n\t\t\tincluding humans, animals, spirits, trees, and most plants are included in the animate class of \n\t\t\tnouns (Valentine 2001:  114).\n\t\t\t(http://purl.org/linguistics/gold/Animate)\n\t\t" ;
        <http://www.w3.org/2000/01/rdf-schema#subClassOf>
                <http://purl.org/olia/olia-top.owl#GenderFeature> ;
        <http://www.w3.org/2002/07/owl#versionInfo>
                "http://purl.org/linguistics/gold/Animate" .

<http://purl.org/olia/olia.owl#DebitiveModality>
        a       <http://www.w3.org/2002/07/owl#Class> ;
        <http://www.w3.org/2000/01/rdf-schema#comment>
                "Mood to express necessity or requirement" ;
        <http://www.w3.org/2000/01/rdf-schema#isDefinedBy>
                "http://www.isocat.org/datcat/DC-3835" ;
        <http://www.w3.org/2000/01/rdf-schema#subClassOf>
                <http://purl.org/olia/olia-top.owl#ModalityFeature> .

<http://purl.org/olia/olia.owl#NonspecificPronoun>
        a       <http://www.w3.org/2002/07/owl#Class> ;
        <http://www.w3.org/2000/01/rdf-schema#comment>
                "In the Russian MTE v4 specs, Pronoun/Type=\"nonspecific\" marks the following Russian words: весь 'all', всякий 'any, every', сам 'oneself', самый 'the very', каждый 'every, each', иной 'other', любой 'any', другой 'other'. The name \"nonspecific\" follows Halliday (1985, Section 6.2.1.1). (MTE v4)\n\t\t\t\n\t\t\tA nonspecific pronoun refers to an unidentified or general entity (e.g., \"I saw *someone*\", \"I saw *everyone*\"). A nonspecific pronoun is not, therefore, a personal pronoun, but an indefinite one. (Andrews 2003).\n\t\t\t\n\t\t\tAndrews, Richard J. (2003), Introduction to Classical Nahuatl. University of Oklahoma Press.\n\t\t\tHalliday, M.A.K. (1985), An introduction to Functional Grammar, London: Edward Arnold\n\t\t\t(http://purl.org/olia/mte/multext-east.owl#NonspecificPronoun)\n\t\t" ;
        <http://www.w3.org/2000/01/rdf-schema#subClassOf>
                <http://purl.org/olia/olia.owl#IndefinitePronoun> ;
        <http://www.w3.org/2000/01/rdf-schema#subClassOf>
                [ a       <http://www.w3.org/2002/07/owl#Restriction> ;
                  <http://www.w3.org/2002/07/owl#onProperty>
                          <http://purl.org/olia/olia.owl#hasSpecificity> ;
                  <http://www.w3.org/2002/07/owl#someValuesFrom>
                          <http://purl.org/olia/olia.owl#Nonspecific>
                ] ;
        <http://www.w3.org/2002/07/owl#versionInfo>
                "http://purl.org/olia/mte/multext-east.owl#NonspecificPronoun" .

<http://purl.org/olia/olia.owl#PastParticipleAdjective>
        a       <http://www.w3.org/2002/07/owl#Class> ;
        <http://www.w3.org/2000/01/rdf-schema#comment>
                "\n                            Adjective based on a past participle.\n                                (http://www.isocat.org/datcat/DC-1596)\n                            " ;
        <http://www.w3.org/2000/01/rdf-schema#label>
                "past participle adjective" ;
        <http://www.w3.org/2000/01/rdf-schema#subClassOf>
                <http://purl.org/olia/olia.owl#ParticipleAdjective> , <http://purl.org/olia/olia.owl#PastParticiple> ;
        <http://www.w3.org/2002/07/owl#versionInfo>
                "http://www.isocat.org/datcat/DC-1596" , "subClassOf participleAdjective (dcif:isA)" .

<http://purl.org/olia/olia.owl#Singular>
        a       <http://www.w3.org/2002/07/owl#Class> ;
        <http://www.w3.org/2000/01/rdf-schema#comment>
                "\n\t\t\tSingular is a grammatical number denoting a unit quantity (as opposed \n\t\t\tto the plural and other forms). (http://en.wikipedia.org/wiki/Singular\n\t\t\t17.11.06)\n\t\t" ;
        <http://www.w3.org/2000/01/rdf-schema#subClassOf>
                <http://purl.org/olia/olia-top.owl#NumberFeature> ;
        <http://www.w3.org/2002/07/owl#versionInfo>
                "EAGLES" .

<http://purl.org/olia/olia.owl#Character>
        a       <http://www.w3.org/2002/07/owl#Class> ;
        <http://www.w3.org/2000/01/rdf-schema#subClassOf>
                <http://purl.org/olia/olia-top.owl#OrthographicEntity> .

<http://purl.org/olia/olia.owl#RaisingSubject>
        a       <http://www.w3.org/2002/07/owl#Class> ;
        <http://www.w3.org/2000/01/rdf-schema#comment>
                "Indicates the syntactic subject of the main clause is in fact the subject of the subclause. The main clause should then be interpreted as being impersonal. (http://www.lexinfo.net/ontology/2.0/lexinfo#RaisingSubject)"@en ;
        <http://www.w3.org/2000/01/rdf-schema#subClassOf>
                <http://purl.org/olia/olia.owl#Control> ;
        <http://www.w3.org/2002/07/owl#versionInfo>
                "http://www.lexinfo.net/ontology/2.0/lexinfo#RaisingSubject" .

<http://purl.org/olia/olia.owl#FutureInPast>
        a       <http://www.w3.org/2002/07/owl#Class> ;
        <http://www.w3.org/2000/01/rdf-schema#comment>
                "\n\t\t\tFutureInPastTense locates the situation in question in the future, \n\t\t\trelative to a contextually determined temporal reference point that \n\t\t\titself must be located in the past relative to the moment of utterance.\n\t\t\t(http://purl.org/linguistics/gold/FutureInPast)\n\t\t" ;
        <http://www.w3.org/2000/01/rdf-schema#subClassOf>
                <http://purl.org/olia/olia.owl#AbsoluteRelativeTense> ;
        <http://www.w3.org/2002/07/owl#versionInfo>
                "http://purl.org/linguistics/gold/FutureInPast, classified as absolute-relative tense here" .

<http://purl.org/olia/olia.owl#AbilitativeMood>
        a       <http://www.w3.org/2002/07/owl#Class> ;
        <http://www.w3.org/2000/01/rdf-schema#comment>
                "Abilitative is a mood that indicates ability, comparable to the use of \"can\" in English. (http://zbb.spinnwebe.com/viewtopic.php?f=7&t=34901)" ;
        <http://www.w3.org/2000/01/rdf-schema#subClassOf>
                <http://purl.org/olia/olia.owl#AbilitativeModality> , <http://purl.org/olia/olia-top.owl#MoodFeature> ;
        <http://www.w3.org/2002/07/owl#versionInfo>
                "Adopted from ILPOSTS (for Indian languages), http://purl.org/olia/ilposts.owl#AbilitativeMood" .

<http://purl.org/olia/olia.owl#SyntacticComplement>
        a       <http://www.w3.org/2002/07/owl#Class> ;
        <http://www.w3.org/2000/01/rdf-schema#comment>
                "\n\t\t\tA complement is a phrase that fits a particular slot in the syntax \n\t\t\trequirements of a parent phrase \n\t\t\t(http://en.wikipedia.org/wiki/Complement_%28linguistics%29).\n\t\t\tAn additional (morpho)syntactic constituent that may be subcategorized \n\t\t\tfor by the predicate.\n\t\t\t(http://languagelink.let.uu.nl/tds/onto/LinguisticOntology.owl#syntacticComplement)\n\t\t" , "\nThe complement is attached inside the VP, NP, ADJP, or PP. \n\nVerbs:\nThe term “complement” as it is used here refers to: \n1.\tinternal arguments such as NP objects, S and SBAR with no adverbial dash tags (including some if-clauses, as in I wonder if the Cubs are winning), and quoted constituents (including SINV and FRAG)\n2.\tthe passive logical-subject by-phrase \n3.\tVP \n4.\tconstituents tagged -BNF, -CLR, -DTV, -PRD, and -PUT\n\t\n\t  (S (NP-SBJ-1 the guide)\n\t     (VP was\n\t         (VP given\n\t             (NP *-1)\n\t             (PP-DTV to\n\t                     (NP Arthur))\n\t             (PP by\n\t                 (NP-LGS Ford)))))\n\t\n\t\n\nNouns: \nSince it is difficult to consistently annotate an argument/adjunct distinction, all PP modifiers of nouns are Chomsky-adjoined to the NP: \n\t\n\t  (NP (NP a teacher)\n\t      (PP of\n\t          (NP chemistry)))\n\nAdjectives: \nExcept in comparatives, any modifier following an adjective is bracketed as a complement. \n\t\n\t  (ADJP eager/likely/ready\n\t        (S to believe anything))\n\t\nPrepositions: \nThe NP or S complement of a preposition is placed inside the PP.\n\n(Bies et al. 1995)\n\t\t" ;
        <http://www.w3.org/2000/01/rdf-schema#subClassOf>
                <http://purl.org/olia/olia-top.owl#SyntacticRole> ;
        <http://www.w3.org/2002/07/owl#versionInfo>
                "according to the PennTreebank definition (Bies et al. 1995), arguments are complements" .

<http://purl.org/olia/olia-top.owl#EvaluativeFeature>
        a       <http://www.w3.org/2002/07/owl#Class> ;
        <http://www.w3.org/2000/01/rdf-schema#subClassOf>
                [ a       <http://www.w3.org/2002/07/owl#Restriction> ;
                  <http://www.w3.org/2002/07/owl#hasSelf>
                          true ;
                  <http://www.w3.org/2002/07/owl#onProperty>
                          <http://purl.org/olia/olia.owl#hasEvaluativeFeature>
                ] .

<http://purl.org/olia/olia-top.owl#ProximityFeature>
        a       <http://www.w3.org/2002/07/owl#Class> ;
        <http://www.w3.org/2000/01/rdf-schema#subClassOf>
                [ a       <http://www.w3.org/2002/07/owl#Restriction> ;
                  <http://www.w3.org/2002/07/owl#hasSelf>
                          true ;
                  <http://www.w3.org/2002/07/owl#onProperty>
                          <http://purl.org/olia/olia.owl#hasProximity>
                ] ;
        <http://www.w3.org/2000/01/rdf-schema#subClassOf>
                [ a       <http://www.w3.org/2002/07/owl#Restriction> ;
                  <http://www.w3.org/2002/07/owl#hasSelf>
                          true ;
                  <http://www.w3.org/2002/07/owl#onProperty>
                          <http://purl.org/olia/olia.owl#hasProximity>
                ] .

<http://purl.org/olia/olia.owl#PlainMiddle>
        a       <http://www.w3.org/2002/07/owl#Class> ;
        <http://www.w3.org/2000/01/rdf-schema#comment>
                "\n\t\t\tResults of action occur to subject. (Siewierska 1988:257)\n\t\t\t(http://purl.org/linguistics/gold/PlainMiddle)\n\t\t" ;
        <http://www.w3.org/2000/01/rdf-schema#subClassOf>
                <http://purl.org/olia/olia.owl#MiddleVoice> ;
        <http://www.w3.org/2002/07/owl#versionInfo>
                "http://purl.org/linguistics/gold/PlainMiddle" .

<http://purl.org/olia/olia.owl#VerbPhrase>
        a       <http://www.w3.org/2002/07/owl#Class> ;
        <http://www.w3.org/2000/01/rdf-schema#comment>
                "\n\t\t\tVerbPhrase is the class of phrases that have verbs as heads. They can play the role of predicate in a main clause.\n\t\t\t(http://purl.org/linguistics/gold/VerbPhrase)\n\t\t" , "\n\t\t\tThis category is slightly more difficult to define, since there is disagreement over the extent of the verb phrase.\n\t\t\tIn particular, should the verb phrase include only the words that are verbs, or should it also include the\n\t\t\tcomplements of the verb? In the examples given in this document, and in the sample texts in the appendices, we have\n\t\t\tchosen to include the complements, but it must be noted that this is an open issue, and we are in no way implying\n\t\t\tthat this analysis is preferable to the alternative. The choice to be made at this level, i.e. the inclusion or\n\t\t\texclusion of verbal complements in the Verb Phrase, is shown by the examples in 27 and 28, 27 showing the inclusion\n\t\t\tof the complement of the verb in the verb phrase and 28 excluding the complement:\n\n\t\t\t(27)  \tHe [VP took up [NP a clothes brush NP] VP]\n\t\t\t(28)  \tHe [VP took up VP] [NP a clothes brush NP]\n\n\t\t\tAn advantage in the type of analysis shown in 27 is that the relative levels of the constituents can be shown to a\n\t\t\tgreater extent -- i.e. complements of the verb are included in the verb phrase, while adjuncts and peripheral\n\t\t\tadverbials are left at sentence level.\n\n\t\t\tHowever, in a case where an adjunct occurs before the complement of the verb, the approaches used in 27 and 28 would\n\t\t\tcause problems, since either both the adjunct and the complement would be included as daughters of the verb phrase,\n\t\t\tor both would be daughters of the sentence, rather than keeping the complement as a daughter of the verb phrase and\n\t\t\tthe adjunct as a sister of the verb phrase. These problems may be solved by an additional notation, but at some\n\t\t\tlevel, arbitrariness is inevitable.\n\n\t\t\tRegardless of the choice made over the extent of the Verb Phrase, there arises a problem of discontinuous Verb\n\t\t\tPhrases. A complex verbal construction may be discontinuous, e.g. the auxiliary and the main verb are separated in\n\t\t\tinverted constructions in English, or the main verb is positioned at the end of the sentence in German and Dutch.\n\t\t\tSuch discontinuity can be avoided by having different labels and constituents for the auxiliary verb and the main\n\t\t\tverb, resulting in an analysis as shown in the Dutch example 29 below:\n\n\t\t\t(29)  \t[NP Ze NP] [AUX zullen AUX] [ADVP er ADVP] [VP [NP de VN-agenda \n\t\t\t\t\t[PP voor [NP het komende jaar NP] PP] NP] behandelen VP].\n\t\t\t\t\t\n\t\t\tand in the English interrogative inverted example 30, using the so-called `dummy auxiliary' do:\n\n\t\t\t(30)  \t[AUX Do AUX] [NP they NP] [VP confide [PP in you PP] VP]?\n\n\t\t\tAs with Noun Phrases, Verb Phrases can be identified by a constituency test. In strong constituency languages like\n\t\t\tEnglish, the whole VP can be moved, but not part of it: compare 31 and 32:\n\n\t\t\t(31)  \t  Give in to blackmail, I never will\n\t\t\t(32)  \t*Give in, I never will to blackmail\n\t\t\t\n\t\t\tHowever, there are languages in which constituent tests do not work. These will typically be languages with flexible\n\t\t\tword order, such as Finnish. 33 is an example of a discontinuous VP (Vilkuna 1989: 26):\n\n\t\t\t(33)  \tMaailmaa\tnähnyt\thän\ton.\n\t\t\t    \tworld-Part\tseen\the\tis\n\t\t\t\t\t`He IS a widely-travelled person.'\n\n\t\t\tFor Finnish, then, evidence for a VP is less convincing than it is for English, and a dependency approach seems the\n\t\t\tmore natural choice. (Covington (1990) provides a parsing strategy for variable word order languages and Covington\n\t\t\t(1991) for parsing discontinuous constituents, both using a dependency syntax approach.)\n\n\t\t\tIn Italian also, constituency tests cannot be applied. This can be shown through the distribution of VP-adverbs\n\t\t\t(e.g. completamente `completely', intenzionalmente `intentionally', attentamente `carefully') and S-adverbs (e.g.\n\t\t\tprobabilmente `probably', certamente `certainly'). In English, these different classes of adverbs have a different\n\t\t\tdistribution within the sentence. In contrast, in Italian, the distinct adverb classes cannot be distinguished on\n\t\t\tthe basis of their distribution in the sentence. S-adverbs and VP-adverbs can occur in the same positions within the\n\t\t\tsentence, as illustrated in examples 34 to 37:\n\n\t\t\t(34)  \tAttentamente/certamente, il bambino ascoltó la storia\n\t\t\t\t\t`Carefully/certainly, the child listened to the story'\n\t\t\t(35)  \tIl bambino attentamente/certamente ascoltó la storia\n\t\t\t\t\t`The child carefully/certainly listened to the story'\n\t\t\t(36)  \tIl bambino ascoltó attentamente/certamente la storia\n\t\t\t\t\t`The child listened carefully/certainly to the story'\n\t\t\t(37)  \tIl bambino ascoltó la storia attentamente/certamente\n\t\t\t\t\t`The child listened to the story carefully/certainly'\n\n\t\t\tThus, in Italian as well as other languages, neither the position nor the syntactic context can help to decide\n\t\t\twhether an adverb is an S-adverb or a VP-adverb; this can only be stated by considering its semantic content and the\n\t\t\tway it relates to the content of the predicate or the sentence. This situation has consequences for the success of\n\t\t\tstandard VP-tests. \n\t\t\t(http://www.ilc.cnr.it/EAGLES96/segsasg1/node33.html)\n\t\t" ;
        <http://www.w3.org/2000/01/rdf-schema#subClassOf>
                <http://purl.org/olia/olia.owl#Phrase> .

<http://purl.org/olia/olia.owl#Plural>
        a       <http://www.w3.org/2002/07/owl#Class> ;
        <http://www.w3.org/2000/01/rdf-schema#comment>
                "\n\t\tPlural is a grammatical number, typically referring to more than one of \n\t\tthe referent in the real world. In English, nouns, pronouns, and demonstratives \n\t\tinflect for plurality. In many other languages, for example German and the \n\t\tvarious Romance languages, articles and adjectives also inflect for plurality. \n\t\t(http://en.wikipedia.org/wiki/Plural  17.11.06)\n\t\t" ;
        <http://www.w3.org/2000/01/rdf-schema#subClassOf>
                <http://purl.org/olia/olia-top.owl#NumberFeature> ;
        <http://www.w3.org/2002/07/owl#versionInfo>
                "EAGLES" .

<http://purl.org/olia/olia.owl#ConditionalModality>
        a       <http://www.w3.org/2002/07/owl#Class> ;
        <http://www.w3.org/2000/01/rdf-schema#comment>
                "\n      \tIn Inuktitut, conditionality is expressed by verbal inflection. Conditional mood signifies conditional relationships in a sentence. (Nowak 1996, p.39)\n      \t\n      \tA conditional relation is a logical relation in which the illocutionary act employing one of a pair of propositions is expressed or implied to be true or in force if the other proposition is true.\n        (www.sil.org/linguistics/GlossaryOfLinguisticTerms/WhatIsAConditionalRelation.htm; http://www.isocat.org/datcat/DC-1258)\n        \n         Elke Nowak (1996), Transforming the images: Ergativity and transitivity in Inuktitut (Eskimo). Walter de Gruyter, Berlin." ;
        <http://www.w3.org/2000/01/rdf-schema#label>
                "conditional" ;
        <http://www.w3.org/2000/01/rdf-schema#subClassOf>
                <http://purl.org/olia/olia-top.owl#ModalityFeature> ;
        <http://www.w3.org/2002/07/owl#versionInfo>
                "subClassOf verbFormMood (dcif:conceptualDomain)" , "http://www.isocat.org/datcat/DC-1258" .

<http://purl.org/olia/olia.owl#OptativeModality>
        a       <http://www.w3.org/2002/07/owl#Class> ;
        <http://www.w3.org/2000/01/rdf-schema#comment>
                "\n\t\t\tOptative indicates that the speaker wishes or hopes that the expressed proposition \n\t\t\tbe the case (Bybee, Perkins, and Pagliuca 1994: 179; Palmer 2001: 204).\n\t\t\t(http://purl.org/linguistics/gold/Optative)\n\t\t" ;
        <http://www.w3.org/2000/01/rdf-schema#subClassOf>
                <http://purl.org/olia/olia-top.owl#ModalityFeature> ;
        <http://www.w3.org/2002/07/owl#versionInfo>
                "\n\t\t\thttp://purl.org/linguistics/gold/Optative,\n\t\t\thttp://languagelink.let.uu.nl/tds/onto/LinguisticOntology.owl#optativeModality\n\t\t" .

<http://purl.org/olia/olia.owl#ConditionalIrrealisModality>
        a       <http://www.w3.org/2002/07/owl#Class> ;
        <http://www.w3.org/2000/01/rdf-schema#comment>
                "Conditional Mood (modality) with Irrealis meaning (ILPOSTS)" ;
        <http://www.w3.org/2000/01/rdf-schema#subClassOf>
                <http://purl.org/olia/olia.owl#ConditionalModality> ;
        <http://www.w3.org/2002/07/owl#versionInfo>
                "ILPOSTS (Indian languages), http://purl.org/olia/ilposts.owl#NonReal is restricted to conditional participles, hence probably a subtype of ConditionalMood" .

<http://purl.org/olia/olia-top.owl#MoodFeature>
        a       <http://www.w3.org/2002/07/owl#Class> ;
        <http://www.w3.org/2000/01/rdf-schema#subClassOf>
                [ a       <http://www.w3.org/2002/07/owl#Restriction> ;
                  <http://www.w3.org/2002/07/owl#hasSelf>
                          true ;
                  <http://www.w3.org/2002/07/owl#onProperty>
                          <http://purl.org/olia/olia.owl#hasMood>
                ] ;
        <http://www.w3.org/2000/01/rdf-schema#subClassOf>
                [ a       <http://www.w3.org/2002/07/owl#Restriction> ;
                  <http://www.w3.org/2002/07/owl#hasSelf>
                          true ;
                  <http://www.w3.org/2002/07/owl#onProperty>
                          <http://purl.org/olia/olia.owl#hasMood>
                ] ;
        <http://www.w3.org/2002/07/owl#versionInfo>
                "Mood feature pertains to grammaticalized moods (as expressed in verbal inflection), Modality refers to the underlying concept that can also be manifested by other grammatical or orthographic markers. Every Mood concept however, entails the corresponding Modality, hence modelled as subsmption between these." .

<http://purl.org/olia/olia.owl#CommonNoun>
        a       <http://www.w3.org/2002/07/owl#Class> ;
        <http://www.w3.org/2000/01/rdf-schema#comment>
                "\n\t\tA common noun is a noun that signifies a non-specific member of a group.\n\t\t(http://www.sil.org/linguistics/GlossaryOfLinguisticTerms/WhatIsACommonNoun.htm 19.09.06)\n\t" ;
        <http://www.w3.org/2000/01/rdf-schema#subClassOf>
                <http://purl.org/olia/olia.owl#Noun> ;
        <http://www.w3.org/2002/07/owl#versionInfo>
                "\n\t\tEAGLES Noun with Type=\"Common\".\n\t" .

<http://purl.org/olia/olia.owl#PromotionalInverseVoice>
        a       <http://www.w3.org/2002/07/owl#Class> ;
        <http://www.w3.org/2000/01/rdf-schema#comment>
                "\n\t\t\tInvolves promotion of the topical proximate-patient to subjecthood. (Givon 1994:24)\n\t\t\t(http://purl.org/linguistics/gold/PromotionalInverse)\n\t\t" ;
        <http://www.w3.org/2000/01/rdf-schema#subClassOf>
                <http://purl.org/olia/olia.owl#InverseVoice> ;
        <http://www.w3.org/2002/07/owl#versionInfo>
                "\n\t\t\thttp://purl.org/linguistics/gold/PromotionalInverse\n\t\t" .

<http://purl.org/olia/olia.owl#ExclamatoryAdverb>
        a       <http://www.w3.org/2002/07/owl#Class> ;
        <http://www.w3.org/2000/01/rdf-schema#comment>
                "\n\t\t\tAn ExclamatoryAdverb seves to express exclamation, cf. how in \"How well everyone played!\"\n\t\t\t\n\t\t\tExclamative sentences or exclamatives \n\t\t\tAn exclamatory sentence or exclamation is generally a more emphatic form of statement,\n\t\t\tin particular, they are used are used to express strong feelings (Latin exclamare : \"to call out, to cry out\").\n\t\t\t(http://english.unitecnology.ac.nz/resources/resources/exp_lang/sentence.html 07.05.07, \n\t\t\t http://en.wikipedia.org/wiki/Sentence_(linguistics)  07.05.07)\n\t\t" ;
        <http://www.w3.org/2000/01/rdf-schema#subClassOf>
                <http://purl.org/olia/olia.owl#WHTypeAdverbs> ;
        <http://www.w3.org/2002/07/owl#versionInfo>
                "\n\t\t\tEAGLES WHAdverb with Wh-Type=\"Exclamatory\".\n\t\t" .

<http://purl.org/olia/olia.owl#GenitiveAttribute>
        a       <http://www.w3.org/2002/07/owl#Class> ;
        <http://www.w3.org/2000/01/rdf-schema#comment>
                "added in conformance to the TIGER scheme" ;
        <http://www.w3.org/2000/01/rdf-schema#subClassOf>
                <http://purl.org/olia/olia.owl#AdnominalConstituent> ;
        <http://www.w3.org/2002/07/owl#versionInfo>
                "added in conformance to the TIGER scheme" , "TODO: check definition" .

<http://purl.org/olia/olia.owl#Ditransitive>
        a       <http://www.w3.org/2002/07/owl#Class> ;
        <http://www.w3.org/2000/01/rdf-schema#comment>
                "\n\t\t\tA predicate/verb that takes two arguments, e.g., English \"to give\", cf. van Valin and Lapolla (1997).\n\t\t" ;
        <http://www.w3.org/2000/01/rdf-schema#subClassOf>
                <http://purl.org/olia/olia-top.owl#ValencyFeature> ;
        <http://www.w3.org/2002/07/owl#versionInfo>
                "SUSANNE (Sampson 1995)" .

<http://purl.org/olia/olia.owl#RecentPast>
        a       <http://www.w3.org/2002/07/owl#Class> ;
        <http://www.w3.org/2000/01/rdf-schema#comment>
                "\n\t\t\tRecentPastTense locates the situation in question prior to the present moment, \n\t\t\tbut by culturally and situationally defined criteria, usually within the span \n\t\t\tranging from yesterday to a week or a few months previous (Comrie 1985:87; \n\t\t\tDahl 1985:121-122).\n\t\t\t(http://purl.org/linguistics/gold/RecentPast)\n\t\t" ;
        <http://www.w3.org/2000/01/rdf-schema#subClassOf>
                <http://purl.org/olia/olia.owl#Past> ;
        <http://www.w3.org/2002/07/owl#versionInfo>
                "http://purl.org/linguistics/gold/RecentPast" .

<http://purl.org/olia/olia.owl#CausativeCase>
        a       <http://www.w3.org/2002/07/owl#Class> ;
        <http://www.w3.org/2000/01/rdf-schema#comment>
                "\n\t\tCase which expresses that the referent of the noun it marks is the\n\t\tcause of the situation expressed by the clause. \n\t\t(http://www.isocat.org/datcat/DC-1253)\n\t\t"@en ;
        <http://www.w3.org/2000/01/rdf-schema#label>
                "causative case"@en ;
        <http://www.w3.org/2000/01/rdf-schema#subClassOf>
                <http://purl.org/olia/olia-top.owl#CaseFeature> ;
        <http://www.w3.org/2002/07/owl#versionInfo>
                "http://www.isocat.org/datcat/DC-1253" .

<http://purl.org/olia/olia.owl#CircumstantialVoice>
        a       <http://www.w3.org/2002/07/owl#Class> ;
        <http://www.w3.org/2000/01/rdf-schema#comment>
                "voice that promotes an oblique argument of a verb to the role of subject" ;
        <http://www.w3.org/2000/01/rdf-schema#isDefinedBy>
                "http://www.isocat.org/datcat/DC-3848" ;
        <http://www.w3.org/2000/01/rdf-schema#subClassOf>
                <http://purl.org/olia/olia-top.owl#VoiceFeature> .

<http://purl.org/olia/olia.owl#UnaccomplishedAspect>
        a       <http://www.w3.org/2002/07/owl#Class> ;
        <http://www.w3.org/2000/01/rdf-schema#comment>
                "\n                            aspect that expresses an event or state that is not finished.\n                                (http://www.isocat.org/datcat/DC-2217)\n                            " ;
        <http://www.w3.org/2000/01/rdf-schema#label>
                "unaccomplished" ;
        <http://www.w3.org/2000/01/rdf-schema#subClassOf>
                <http://purl.org/olia/olia-top.owl#AspectFeature> ;
        <http://www.w3.org/2002/07/owl#versionInfo>
                "http://www.isocat.org/datcat/DC-2217" , "subClassOf aspect (dcif:conceptualDomain)" .

<http://purl.org/olia/olia.owl#Reduplication>
        a       <http://www.w3.org/2002/07/owl#Class> ;
        <http://www.w3.org/2000/01/rdf-schema#comment>
                "\n                            process to modify the sense of a word by some operations to repeat the sound of a word.\n                                (http://www.isocat.org/datcat/DC-2346)\n                            " ;
        <http://www.w3.org/2000/01/rdf-schema#label>
                "reduplication" ;
        <http://www.w3.org/2000/01/rdf-schema#subClassOf>
                <http://purl.org/olia/olia-top.owl#MorphologicalProcess> ;
        <http://www.w3.org/2002/07/owl#versionInfo>
                "http://www.isocat.org/datcat/DC-2346 (reduplication)" .

<http://purl.org/olia/olia.owl#TabooRegister>
        a       <http://www.w3.org/2002/07/owl#Class> ;
        <http://www.w3.org/2000/01/rdf-schema#comment>
                "\n                            Register that expresses a situation that people avoid because it is extremely offensive or embarrassing.\n                                (ISO12620; http://www.isocat.org/datcat/DC-1996)\n                            " ;
        <http://www.w3.org/2000/01/rdf-schema#label>
                "taboo register" ;
        <http://www.w3.org/2000/01/rdf-schema#subClassOf>
                <http://purl.org/olia/olia-top.owl#RegisterFeature> ;
        <http://www.w3.org/2002/07/owl#versionInfo>
                "http://www.isocat.org/datcat/DC-1996" , "subClassOf register (dcif:conceptualDomain)" .

<http://purl.org/olia/olia.owl#ConterminativeCase>
        a       <http://www.w3.org/2002/07/owl#Class> ;
        <http://www.w3.org/2000/01/rdf-schema#comment>
                "\n\t\t\tConterminativeCase expresses the notion of something moving into \n\t\t\tthe vicinity of the referent of the noun it marks, but not through \n\t\t\tthat region. It has the meaning 'moving into the vicinity of'.\n\t\t\t(http://purl.org/linguistics/gold/Conterminative)\n\t\t" ;
        <http://www.w3.org/2000/01/rdf-schema#subClassOf>
                <http://purl.org/olia/olia-top.owl#CaseFeature> ;
        <http://www.w3.org/2002/07/owl#versionInfo>
                "http://purl.org/linguistics/gold/Conterminative" .

<http://purl.org/olia/olia.owl#VolitiveModality>
        a       <http://www.w3.org/2002/07/owl#Class> ;
        <http://www.w3.org/2000/01/rdf-schema#comment>
                "VolitiveForce indicates that the speaker is\n                        willing to perform some action [Palmer 2001: 76]." ;
        <http://www.w3.org/2000/01/rdf-schema#isDefinedBy>
                "http://www.isocat.org/datcat/DC-3555" ;
        <http://www.w3.org/2000/01/rdf-schema#label>
                "volitive force" ;
        <http://www.w3.org/2000/01/rdf-schema#subClassOf>
                <http://purl.org/olia/olia-top.owl#ModalityFeature> .

<http://purl.org/olia/olia.owl#Fronting>
        a       <http://www.w3.org/2002/07/owl#Class> ;
        <http://www.w3.org/2000/01/rdf-schema#comment>
                "Expression occurs at the left periphery of the sentence. This includes various noncanonical and canonical word order possibilities. (Note that it is not restricted here to noncanonical word order; for noncanonical fronting see subconcepts, e.g., Topicalization.) (Chiarcos)" ;
        <http://www.w3.org/2000/01/rdf-schema#subClassOf>
                <http://purl.org/olia/olia-top.owl#SyntacticConstruction> ;
        <http://www.w3.org/2002/07/owl#versionInfo>
                "T-CODEX (Petrova 2008, http://purl.org/olia/tcodex.owl#InitionalPosition)" .

<http://purl.org/olia/olia.owl#ImperfectiveAspect>
        a       <http://www.w3.org/2002/07/owl#Class> ;
        <http://www.w3.org/2000/01/rdf-schema#comment>
                "\n\t\t\tThe Imperfective aspect is an aspect that expresses an event or state, \n\t\t\twith respect to its internal structure, instead of expressing it as a \n\t\t\tsimple whole. \n\t\t\t(http://www.sil.org/linguistics/glossaryoflinguisticterms/WhatIsImperfectiveAspect.htm  17.11.06)\n\t\t\t\n\t\t\tThe imperfective aspects ... do not view the situation as bounded, \n\t\t\tbut rather as ongoing in either a durative, continuative or habitual \n\t\t\tsense (Bybee 1985:21)\n\t\t\t(http://languagelink.let.uu.nl/tds/onto/LinguisticOntology.owl#imperfectiveAspect)\n\t\t\t\n\t\t\tA viewpoint aspect which encodes the speaker’s lack of attention to the endpoints \n\t\t\tof the situation referred to. Imperfective aspect is the prototypical mode of \n\t\t\tpresentation for states (Michaelis 1998:xiv).\n\t\t\t(http://purl.org/linguistics/gold/Imperfective)\n\t\t" ;
        <http://www.w3.org/2000/01/rdf-schema#subClassOf>
                <http://purl.org/olia/olia-top.owl#AspectFeature> ;
        <http://www.w3.org/2002/07/owl#versionInfo>
                "\n\t\t\tEAGLES,\n\t\t\thttp://languagelink.let.uu.nl/tds/onto/LinguisticOntology.owl#imperfectiveAspect,\n\t\t\thttp://purl.org/linguistics/gold/Imperfective\n\t\t" .

<http://purl.org/olia/olia.owl#PreNominalModifier>
        a       <http://www.w3.org/2002/07/owl#Class> ;
        <http://www.w3.org/2000/01/rdf-schema#comment>
                "\n\t\t\tPremodifying is a function of an adjective that can modify a following noun.\n\t\t\t(EAGLES)\n\t\t\tmodificationType: Refers to the prenominal or postnominal positions of determiners which distinguish different forms. (http://www.isocat.org/datcat/DC-1931)" ;
        <http://www.w3.org/2000/01/rdf-schema#subClassOf>
                <http://purl.org/olia/olia.owl#AdnominalConstituent> ;
        <http://www.w3.org/2002/07/owl#versionInfo>
                "EAGLES, NPFunction=\"premodifying\", cf. http://www.isocat.org/datcat/DC-1943 (preModifier, but without reference to nominal heads)" .

<http://purl.org/olia/olia.owl#SuperlativeParticle>
        a       <http://www.w3.org/2002/07/owl#Class> ;
        <http://www.w3.org/2000/01/rdf-schema#comment>
                "\n                            Particle expressing superlative degree. Superlative is the comparison between more than two entities and contrasts with comparative where only two entities are involved and positive where no comparison is implied.\n                                (Crystal 2003; http://www.isocat.org/datcat/DC-1923)\n                            " ;
        <http://www.w3.org/2000/01/rdf-schema#label>
                "superlative particle" ;
        <http://www.w3.org/2000/01/rdf-schema#subClassOf>
                <http://purl.org/olia/olia.owl#Particle> ;
        <http://www.w3.org/2002/07/owl#versionInfo>
                "http://www.isocat.org/datcat/DC-1923" , "subClassOf particle (dcif:isA)" .

<http://purl.org/olia/olia.owl#Countable>
        a       <http://www.w3.org/2002/07/owl#Class> ;
        <http://www.w3.org/2000/01/rdf-schema#comment>
                "\n\t\t\tA countable noun (also count noun) is a noun which can be modified by a numeral \n\t\t\tand occur in both singular and plural form, as well as co-occurring with \n\t\t\tquantificational determiners like every, each, several, most, etc..\n\t\t\t(http://en.wikipedia.org/wiki/Countable_noun 19.09.06)\n\t\t" ;
        <http://www.w3.org/2000/01/rdf-schema#subClassOf>
                <http://purl.org/olia/olia-top.owl#CountabilityFeature> ;
        <http://www.w3.org/2002/07/owl#versionInfo>
                "EAGLES, remodelling of MassNoun vs. CommonNoun" .

<http://purl.org/olia/olia.owl#Atransitive>
        a       <http://www.w3.org/2002/07/owl#Class> ;
        <http://www.w3.org/2000/01/rdf-schema#comment>
                "\n\t\t\tA predicate/verb that takes no argument.\n\t\t\tEnglish \"to rain\" is semantically atransitive, hence, an expletive is to be used in \"it's raining\",\n\t\t\tcf. van Valin and Lapolla (1997).\n\t\t" ;
        <http://www.w3.org/2000/01/rdf-schema#subClassOf>
                <http://purl.org/olia/olia-top.owl#ValencyFeature> ;
        <http://www.w3.org/2002/07/owl#versionInfo>
                "Chiarcos" .

<http://purl.org/olia/olia.owl#FusedPrepositionPronoun>
        a       <http://www.w3.org/2002/07/owl#Class> ;
        <http://www.w3.org/2000/01/rdf-schema#comment>
                "word resulting from the aggregation of a preposition and a pronoun" ;
        <http://www.w3.org/2000/01/rdf-schema#isDefinedBy>
                "http://www.isocat.org/datcat/DC-3009" ;
        <http://www.w3.org/2000/01/rdf-schema#subClassOf>
                <http://purl.org/olia/olia.owl#Pronoun> , <http://purl.org/olia/olia.owl#Preposition> .

<http://purl.org/olia/olia.owl#Adjectival>
        a       <http://www.w3.org/2002/07/owl#Class> ;
        <http://www.w3.org/2000/01/rdf-schema#comment>
                "In MULTEXT-East a characteristic of attributive pronouns and abbreviated adjectives, e.g., in Ukrainian e.g., абичий/= бозна-чий/= будь-чий/= дечий/= хтозна-чий/= чий-будь/= чий-небудь/= чийсь/=, абичийого/абичий аби до чийого/абичий бозна-чийого/бозна-чий будь-чийого/будь-чий дечийого/дечий хтозна-чийого/хтозна-чий чийого-будь/чий-будь чийого-небудь/чий-небудь чийогось/чийсь, абичийого/абичий бозна-чийого/бозна-чий будь-чийого/будь-чий дечийого/дечий хтозна-чийого/хтозна-чий чийого-будь/чий-будь чийого-небудь/чий-небудь чийогось/чийсь, абичийому/абичий абичиєму/абичий абичиїм/абичий аби на чийому/абичий аби на чиєму/абичий аби на чиїм/абичий бозна на чийому/бозна-чий бозна на чиєму/бозна-чий бозна на чиїм/бозна-чий будь-чийому/будь-чий будь-чиєму/будь-чий будь-чиїм/будь-чий будь на чийому/будь-чий будь на чиєму/будь-чий будь на чиїм/будь-чий дечийому/дечий дечиєму/дечий дечиїм/дечий де на чийому/дечий де на чиєму/дечий, абичийому/абичий абичиєму/абичий бозна-чийому/бозна-чий бозна-чиєму/бозна-чий будь-чийому/будь-чий будь-чиєму/будь-чий дечийому/дечий дечиєму/дечий хтозна-чийому/хтозна-чий хтозна-чиєму/хтозна-чий чийому-будь/чий-будь чиєму-будь/чий-будь чийому-небудь/чий-небудь чиєму-небудь/чий-небудь чийомусь/чийсь чиємусь/чийсь, абичийому/абичий абичиєму/абичий бозна-чийому/бозна-чий будь-чийому/будь-чий будь-чиєму/будь-чий дечийому/дечий хтозна-чийому/хтозна-чий чийому-будь/чий-будь чийому-небудь/чий-небудь чийомусь/чийсь, абичию/абичий бозна-чию/бозна-чий будь-чию/будь-чий дечию/дечий хтозна-чию/хтозна-чий чию-будь/чий-будь чию-небудь/чий-небудь чиюсь/чийсь, абичия/абичий бозна-чия/бозна-чий будь-чия/будь-чий дечия/дечий хтозна-чия/хтозна-чий чия-будь/чий-будь чия-небудь/чий-небудь чиясь/чийсь, абичиє/абичий бозна-чиє/бозна-чий будь-чиє/будь-чий дечиє/дечий хтозна-чиє/хтозна-чий чиє-будь/чий-будь чиє-небудь/чий-небудь чиєсь/чийсь\n\t\t\t(http://purl.org/olia/mte/multext-east.owl#Adjectival)\n\t\t" ;
        <http://www.w3.org/2000/01/rdf-schema#subClassOf>
                <http://purl.org/olia/olia-top.owl#SyntacticFunction> ;
        <http://www.w3.org/2002/07/owl#versionInfo>
                "http://purl.org/olia/mte/multext-east.owl#Adjectival" .

<http://purl.org/olia/olia.owl#EmphaticParticle>
        a       <http://www.w3.org/2002/07/owl#Class> ;
        <http://www.w3.org/2000/01/rdf-schema#comment>
                "Emphatic particle, e.g., (one of the uses of) Urdu tô: \n\t\t\n\t\tvo urdû parhê gâ\n\t\t\"He will study Urdu.\" (simple statement)\n\t\t\n\t\tvo urdû parhê gâ tô lêkin imtihân nahîm dê gâ\n\t\t\"He will STUDY Urdu, OF COURSE, but he won't take the examination.\"\n\t\t(Schmidt 1999, p. 232, see http://purl.org/olia/emille.owl#ContrastiveEmphaticParticle)\t\t\n\t\t" ;
        <http://www.w3.org/2000/01/rdf-schema#subClassOf>
                <http://purl.org/olia/olia.owl#Particle> , <http://purl.org/olia/olia.owl#Intensifier> ;
        <http://www.w3.org/2002/07/owl#equivalentClass>
                [ a       <http://www.w3.org/2002/07/owl#Class> ;
                  <http://www.w3.org/2002/07/owl#intersectionOf>
                          ( <http://purl.org/olia/olia.owl#Particle>
                            [ a       <http://www.w3.org/2002/07/owl#Restriction> ;
                              <http://www.w3.org/2002/07/owl#onProperty>
                                      <http://purl.org/olia/olia.owl#hasEmphasis> ;
                              <http://www.w3.org/2002/07/owl#someValuesFrom>
                                      <http://purl.org/olia/olia.owl#Emphatic>
                            ]
                          )
                ] ;
        <http://www.w3.org/2002/07/owl#versionInfo>
                "adopted from EMILLE, http://purl.org/olia/emille.owl#ContrastiveEmphaticParticle, http://purl.org/olia/emille.owl#ExclusiveEmphaticParticle, etc. \n\t\t\tFrom a logical point of view, emphasis is closely related to intensification, hence, subconcept of Intensifier" .

<http://purl.org/olia/olia.owl#PronounOrDeterminer>
        a       <http://www.w3.org/2002/07/owl#Class> ;
        <http://www.w3.org/2000/01/rdf-schema#comment>
                "\n\t\tThe parts of speech Pronoun, Determiner and Article heavily overlap in their formal and functional \n\t\tcharacteristics, and different analyses for different languages entail separating them out in \n\t\tdifferent ways.\n\t\tIn Eagles, Pronouns and Determiners are placed in one `super-category'. For some descriptions it may \n\t\tbe thought best to treat them as totally different parts of speech.\n\t\t(http://www.ilc.cnr.it/EAGLES96/annotate/node17.html#recp 19.09.06)\n\t" ;
        <http://www.w3.org/2000/01/rdf-schema#label>
                "pronom / determinatif"@fr , "pronoun or determiner"@en ;
        <http://www.w3.org/2000/01/rdf-schema#subClassOf>
                <http://purl.org/olia/olia-top.owl#MorphosyntacticCategory> ;
        <http://www.w3.org/2002/07/owl#versionInfo>
                "\n\t\tEAGLES top-level category PronounOrDeterminer (PD).\n\t\t\n\t\tThe existence of this class is, however, controversial. In EAGLES, it \n\t\thas been introduced for reasons of lexical ambiguity in European languages \n\t\tthus it could be described by the joint of Pronoun and Determiner rather \n\t\tthan as an independent class.\n\t\tIndeed, at least one fundamental difference is blurred here: \n\t\tDeterminers are purely modifiers whereas pronouns contribute independent \n\t\tmeaning. This could be adopted here as a criterion for higher-level organization \n\t\tof the OLiA Reference Model.\n\t\t\n\t\tThe original EAGLES definition is not very specific about the difference between \n\t\tPronouns and Determiners. Here, we assume two definitions:\n\t\t\n\t\t* semantic definition of pronouns: Pronouns are bound variables. They are referential.\n\t\t* syntactic definition of determiners: Determiners turn nominal expressions (of type <e,t>) into \n\t\t  noun phrases (of type <e>).\n\n\t\tNote that these definitions are not exclusive (which is why annotation schemes differ in this aspect). \n\t\tAttributive possessive pronouns ('my book', 'their article') are semantically pronouns (they have an \n\t\tindependent reference), but syntactically determiners.\n\t\tFor the sub-classes, no exclusivity is required as Olia allows a hybrid (\"both\") category by multiple \n\t\tinheritance.\n\t" .

<http://purl.org/olia/olia.owl#DiminutiveNoun>
        a       <http://www.w3.org/2002/07/owl#Class> ;
        <http://www.w3.org/2000/01/rdf-schema#comment>
                "\n                            diminutive noun\n                                (MIRACL LSCA; http://www.isocat.org/datcat/DC-2225)\n                            " ;
        <http://www.w3.org/2000/01/rdf-schema#label>
                "diminutive noun" ;
        <http://www.w3.org/2000/01/rdf-schema#subClassOf>
                <http://purl.org/olia/olia.owl#Noun> ;
        <http://www.w3.org/2002/07/owl#versionInfo>
                "http://www.isocat.org/datcat/DC-2225" , "\n\t\tsubClassOf noun (dcif:isA); \n\t\tcan be proper name (German Julchen from Julia, Russian Olichka from Olga) \n\t\tor common noun (German Blümchen from Blume \"flower\", Russian yozhik from yozh \"hedgehock\")\n\t  " .

<http://purl.org/olia/olia.owl#QuestionMark>
        a       <http://www.w3.org/2002/07/owl#Class> ;
        <http://www.w3.org/2000/01/rdf-schema#comment>
                "\n                            Sign used to express a question.\n                                (http://www.isocat.org/datcat/DC-1444)\n                            " ;
        <http://www.w3.org/2000/01/rdf-schema#label>
                "interrogative point" , "question mark" ;
        <http://www.w3.org/2000/01/rdf-schema#subClassOf>
                <http://purl.org/olia/olia.owl#SentenceFinalPunctuation> ;
        <http://www.w3.org/2002/07/owl#versionInfo>
                "http://www.isocat.org/datcat/DC-1444" , "subClassOf partOfSpeech (dcif:conceptualDomain)" .

<http://purl.org/olia/olia.owl#ImperativeModality>
        a       <http://www.w3.org/2002/07/owl#Class> ;
        <http://www.w3.org/2000/01/rdf-schema#comment>
                "\n\t\t\tPertaining to the mood or mode of a verb form or clause such that it \n\t\t\tpredicates a command, request, or exhortation (OED).\n\t\t\t(http://languagelink.let.uu.nl/tds/onto/LinguisticOntology.owl#imperativeModality)\n\t\t" ;
        <http://www.w3.org/2000/01/rdf-schema#subClassOf>
                <http://purl.org/olia/olia.owl#ActionalModality> ;
        <http://www.w3.org/2002/07/owl#versionInfo>
                "http://languagelink.let.uu.nl/tds/onto/LinguisticOntology.owl#imperativeModality" .

<http://purl.org/olia/olia.owl#FormalCase>
        a       <http://www.w3.org/2002/07/owl#Class> ;
        <http://www.w3.org/2000/01/rdf-schema#comment>
                "In Hungarian, `essive-formal' is in some descriptions simply called `formal', with the affix _-képp(en)_ and meaning (`in\n\t\t\tthe form of ...', they probably meant when they came up with the term).\n\t\t\tIn the Hungarian MULTEXT-East scheme, essive-formal and formal are distinguished.\n\t\t\t(Ivan A. Derzhanski, email 2010/06/15, http://purl.org/olia/mte/multext-east.owl#FormalCase)<br/>\n\t\t" ;
        <http://www.w3.org/2000/01/rdf-schema#subClassOf>
                <http://purl.org/olia/olia-top.owl#CaseFeature> ;
        <http://www.w3.org/2002/07/owl#versionInfo>
                "http://purl.org/olia/mte/multext-east.owl#FormalCase" .

<http://purl.org/olia/olia.owl#Emphatic>
        a       <http://www.w3.org/2002/07/owl#Class> ;
        <http://www.w3.org/2000/01/rdf-schema#comment>
                " Pronoun marked to show its importance. (http://www.isocat.org/datcat/DC-1941)\n\t\t\tIn Romanian, the so-called emphatic determiner may accompany both a noun and a personal pronoun: fata *însăşi* (the girl *herself*), also ea *însăşi* (she *herself*). (http://purl.org/olia/mte/multext-east.owl#EmphaticDeterminer)\n\t\t\tEmphasis can not only be expressed on nouns and pronouns, but also at verbs, adverbs, adpositions, etc., cf. http://purl.org/olia/ilposts.owl#Emphasis" ;
        <http://www.w3.org/2000/01/rdf-schema#subClassOf>
                <http://purl.org/olia/olia-top.owl#EmphasisFeature> ;
        <http://www.w3.org/2002/07/owl#versionInfo>
                "added in accordance with ILPOSTS, cf. http://purl.org/olia/mte/multext-east.owl#EmphaticDeterminer, http://purl.org/olia/mte/multext-east.owl#EmphaticPronoun, http://www.isocat.org/datcat/DC-1941 (emphatic pronoun)" .

<http://purl.org/olia/olia.owl#DubitiveModality>
        a       <http://www.w3.org/2002/07/owl#Class> ;
        <http://www.w3.org/2000/01/rdf-schema#comment>
                "\n\t\t\tDubitiveMood indicates a speaker's doubt or uncertainty about a proposition (Palmer 2001).\n\t\t\t(http://purl.org/linguistics/gold/Dubitive)\n\t\t" ;
        <http://www.w3.org/2000/01/rdf-schema#subClassOf>
                <http://purl.org/olia/olia-top.owl#ModalityFeature> ;
        <http://www.w3.org/2002/07/owl#versionInfo>
                "http://purl.org/linguistics/gold/Dubitive" .

<http://purl.org/olia/olia.owl#Distal>
        a       <http://www.w3.org/2002/07/owl#Class> ;
        <http://www.w3.org/2000/01/rdf-schema#comment>
                "The referent denoted by a distal demonstrative pronoun (e.g., English that) is usually spatially more \n\t\t\tremote or discoursally less salient as compared to a referent denoted by a proximal demonstrative pronoun (e.g., English this)\n\t\t\t(Chiarcos)\n\t\t" ;
        <http://www.w3.org/2000/01/rdf-schema#subClassOf>
                <http://purl.org/olia/olia-top.owl#ProximityFeature> ;
        <http://www.w3.org/2002/07/owl#versionInfo>
                "added in accordance with http://purl.org/olia/mte/multext-east.owl#CliticDistalDeterminer" .

<http://purl.org/olia/olia.owl#zuInclusion>
        a       <http://www.w3.org/2002/07/owl#Class> ;
        <http://www.w3.org/2000/01/rdf-schema#comment>
                "\n                            Inclusion of zu.\n                                (DFKI; http://www.isocat.org/datcat/DC-1954)\n                            " ;
        <http://www.w3.org/2000/01/rdf-schema#label>
                "zu inclusion" ;
        <http://www.w3.org/2000/01/rdf-schema#subClassOf>
                <http://purl.org/olia/olia.owl#Infix> ;
        <http://www.w3.org/2002/07/owl#versionInfo>
                "http://www.isocat.org/datcat/DC-1954" .

<http://purl.org/olia/olia.owl#DeclarativeSentence>
        a       <http://www.w3.org/2002/07/owl#Class> ;
        <http://www.w3.org/2000/01/rdf-schema#comment>
                "S|Simple declarative clause, i.e. one that is not introduced by a (possibly empty) subordinating\nconjunction or wh-word and that does not exhibit subject-verb inversion.\n(Santorini 1991)\n\nSimple declarative sentences: \n(S (NP-SBJ Casey) (VP threw (NP the ball))) ...\n\nS â ´ Simple declarative clause, i.e. one that is not introduced by a (possibly empty) subordinating conjunction or wh-word and that does not exhibit subject-verb inversion. \n(Bies et al. 1995)" ;
        <http://www.w3.org/2000/01/rdf-schema#subClassOf>
                <http://purl.org/olia/olia-top.owl#SentenceTypeFeature> , <http://purl.org/olia/olia.owl#DeclarativeModality> ;
        <http://www.w3.org/2002/07/owl#equivalentClass>
                [ a       <http://www.w3.org/2002/07/owl#Class> ;
                  <http://www.w3.org/2002/07/owl#intersectionOf>
                          ( <http://purl.org/olia/olia.owl#Sentence>
                            [ a       <http://www.w3.org/2002/07/owl#Restriction> ;
                              <http://www.w3.org/2002/07/owl#onProperty>
                                      <http://purl.org/olia/olia.owl#hasModality> ;
                              <http://www.w3.org/2002/07/owl#someValuesFrom>
                                      <http://purl.org/olia/olia.owl#DeclarativeModality>
                            ]
                          )
                ] ;
        <http://www.w3.org/2002/07/owl#versionInfo>
                "Santorini 1991, Bies et al. 1995" .

<http://purl.org/olia/olia.owl#InceptiveAspect>
        a       <http://www.w3.org/2002/07/owl#Class> ;
        <http://www.w3.org/2000/01/rdf-schema#comment>
                "\n\t\t\tInceptiveAspect, also called the ingressive, encodes the beginning \n\t\t\tportion of some event (Bybee 1985: 147, 149; Payne 1997: 240; Bhat 1999:176).\n\t\t\t(http://purl.org/linguistics/gold/Inceptive)\n\t\t" ;
        <http://www.w3.org/2000/01/rdf-schema#subClassOf>
                <http://purl.org/olia/olia-top.owl#AspectFeature> ;
        <http://www.w3.org/2002/07/owl#versionInfo>
                "http://purl.org/linguistics/gold/Inceptive" .

<http://purl.org/olia/olia.owl#hasSemanticValency>
        a       <http://www.w3.org/2002/07/owl#ObjectProperty> ;
        <http://www.w3.org/2000/01/rdf-schema#comment>
                "\n\t\tSemantic valency pertains to the number of semantic arguments a predicate takes.\n\t\tThis is not necessarily the same as syntactic valency: In English, expletive \"it\" is\n\t\tused as a syntactic argument if no semantic argument is available, cf. van Valin and \n\t\tLapolla (1997).\n\t" ;
        <http://www.w3.org/2000/01/rdf-schema#range>
                <http://purl.org/olia/olia-top.owl#ValencyFeature> ;
        <http://www.w3.org/2000/01/rdf-schema#subPropertyOf>
                <http://purl.org/olia/system.owl#hasFeature> ;
        <http://www.w3.org/2002/07/owl#versionInfo>
                "Ch. Chiarcos" .

<http://purl.org/olia/olia.owl#SubordinatingConjunction>
        a       <http://www.w3.org/2002/07/owl#Class> ;
        <http://www.w3.org/2000/01/rdf-schema#comment>
                "\n\t\t\tSubordinating conjunctions, also called subordinators, are conjunctions \n\t\t\tthat introduce a dependent clause.\n\t\t\t(http://en.wikipedia.org/wiki/Grammatical_conjunction 19.09.06)\n\t\t" ;
        <http://www.w3.org/2000/01/rdf-schema#subClassOf>
                <http://purl.org/olia/olia.owl#Conjunction> ;
        <http://www.w3.org/2002/07/owl#versionInfo>
                "Following EAGLES and MULTEXT-East, the subclassification of SubordinatingConjunction reflects constraints on MorphosyntacticFeatures of verbal and nominal arguments of subordinating conjunctions, in these cases verbal inflection (finiteness, negation) and Degree" , "EAGLES Conjunction with Type=\"Subordinating\".\n\t\t\t\t\tThe language- (German-) specific EAGLES feature \"subord-type\" was originally modelled as MorphosyntacticFeature, when integrating the MULTEXT-East ontology, it was remodelled within the taxonomy\n\t\t" .

<http://purl.org/olia/olia.owl#NucleonicMiddle>
        a       <http://www.w3.org/2002/07/owl#Class> ;
        <http://www.w3.org/2000/01/rdf-schema#comment>
                "\n\t\t\tObject of action belongs to. Moves into, or moves from sphere of subject.\n\t\t\t(Siewierska 1988:257)\n\t\t\t(http://purl.org/linguistics/gold/NucleonicMiddle)\n\t\t" ;
        <http://www.w3.org/2000/01/rdf-schema#subClassOf>
                <http://purl.org/olia/olia.owl#MiddleVoice> ;
        <http://www.w3.org/2002/07/owl#versionInfo>
                "\n\t\t\thttp://purl.org/linguistics/gold/NucleonicMiddle\n\t\t" .

<http://purl.org/olia/olia.owl#ReflexiveMiddle>
        a       <http://www.w3.org/2002/07/owl#Class> ;
        <http://www.w3.org/2000/01/rdf-schema#comment>
                "\n\t\t\tReflexive middle makes use of \n\t\t\tgrammatical devices that normally indicate reflexivity.\n\t\t\t(Ch. Chiarcos)\n\t\t" ;
        <http://www.w3.org/2000/01/rdf-schema#subClassOf>
                <http://purl.org/olia/olia.owl#MiddleVoice> ;
        <http://www.w3.org/2002/07/owl#versionInfo>
                "TODO: Check Siewierska (1988:257)" , "\n\t\t\thttp://purl.org/linguistics/gold/ReflexiveMiddle,\n\t\t\tbut the definition given there (\"Subjects perform action to self\")\n\t\t\tmay be oversimplistic as it entails that ReflectiveMiddle\n\t\t\tis the *same* as Reflexive.\n\t\t\tIn my current understanding, reflexive middle is a middle construction \n\t\t\tthat makes use of grammatical devices that normally indicate reflexivity,\n\t\t\tcf. the definition of ReflexivePassive.\n\t\t\tThe definition given below is a generalization that covers the original\n\t\t\tdefinition as well.\n\t\t" .

<http://purl.org/olia/olia.owl#Phrase>
        a       <http://www.w3.org/2002/07/owl#Class> ;
        <http://www.w3.org/2000/01/rdf-schema#comment>
                "\n\t\t\tPhrase is the class of syntactic constructions that consist of one or more \n\t\t\tsyntactic words, but lack the subject-predicate organization of a clause. \n\t\t\tPhrases get their grammatical characteristics according to what word occupies \n\t\t\tthe head position; thus, all phrases have heads [Crystal 1980, 232-233; Pei \n\t\t\tand Gaynor 1954, 169; Pike and Pike 1982, 453].\n\t\t\t(http://purl.org/linguistics/gold/Phrase)\n\t\t" ;
        <http://www.w3.org/2000/01/rdf-schema#subClassOf>
                <http://purl.org/olia/olia-top.owl#Constituent> ;
        <http://www.w3.org/2002/07/owl#versionInfo>
                "http://purl.org/linguistics/gold/Phrase" .

<http://purl.org/olia/olia.owl#EpistemicPossibilityModality>
        a       <http://www.w3.org/2002/07/owl#Class> ;
        <http://www.w3.org/2000/01/rdf-schema#comment>
                "EpistemicPossibilityModality indicates that the\n                        designated state of affairs is not known not to be true." ;
        <http://www.w3.org/2000/01/rdf-schema#isDefinedBy>
                "http://www.isocat.org/datcat/DC-3181" ;
        <http://www.w3.org/2000/01/rdf-schema#subClassOf>
                <http://purl.org/olia/olia-top.owl#ModalityFeature> .

<http://purl.org/olia/olia.owl#InitialField>
        a       <http://www.w3.org/2002/07/owl#Class> ;
        <http://www.w3.org/2000/01/rdf-schema#comment>
                "\nIn a German clause, the finite verb can appear in three different positions: verb-second, \nverb-initial, and verb-final. Only in verb-final clauses the verb complex consisting of the\nfinite verb and non-finite verbal elements forms a unit. The discontinuous positioning\nof the verbal elements in verb-first and verb-second clauses is the traditional reason\nfor structuring German clauses into fields. The positions of the verbal elements form\nthe Satzklammer (sentence bracket) which divides the sentence into a Vorfeld (initial\nfield), a Mittelfeld (middle field), and a Nachfeld (final field). The Vorfeld and the\nMittelfeld are divided by the linke Satzklammer (left sentence bracket), which is the finite\nverb, the rechte Satzklammer (right sentence bracket) is the verb complex between the\nMittelfeld and the Nachfeld. \n(Telljohann et al. 2009, p.13)\n\t\t" ;
        <http://www.w3.org/2000/01/rdf-schema#subClassOf>
                <http://purl.org/olia/olia-top.owl#TopologicalField> , <http://purl.org/olia/olia.owl#Fronting> ;
        <http://www.w3.org/2002/07/owl#versionInfo>
                "In the canonical sentence, the initial field is the first position in the sentence, hence grouped under Fronting." .

<http://purl.org/olia/olia.owl#Foreign>
        a       <http://www.w3.org/2002/07/owl#Class> ;
        <http://www.w3.org/2000/01/rdf-schema#comment>
                "\n      A foreign word is a text word which lies outside the traditionally accepted range of \n      grammatical classes, it occurs quite commonly in many texts and very commonly in some. \n      (http://www.ilc.cnr.it/EAGLES96/annotate/node16.html#mr 19.09.06)" ;
        <http://www.w3.org/2000/01/rdf-schema#label>
                "foreign word"@en , "mot etranger"@fr ;
        <http://www.w3.org/2000/01/rdf-schema#subClassOf>
                <http://purl.org/olia/olia.owl#Residual> ;
        <http://www.w3.org/2002/07/owl#versionInfo>
                "EAGLES Category Residuals with Type=\"ForeignWord\"." .

<http://purl.org/olia/olia.owl#Initialism>
        a       <http://www.w3.org/2002/07/owl#Class> ;
        <http://www.w3.org/2000/01/rdf-schema#isDefinedBy>
                "http://www.isocat.org/datcat/DC-333" ;
        <http://www.w3.org/2000/01/rdf-schema#subClassOf>
                <http://purl.org/olia/olia.owl#Abbreviation> ;
        <http://www.w3.org/2002/07/owl#versionInfo>
                "adopted from ubyPos.owl" .

<http://purl.org/olia/olia.owl#Quote>
        a       <http://www.w3.org/2002/07/owl#Class> ;
        <http://www.w3.org/2000/01/rdf-schema#comment>
                "\n                            Punctuation usually used to surround a quotation.\n                                (http://www.isocat.org/datcat/DC-2081)\n                            " ;
        <http://www.w3.org/2000/01/rdf-schema#label>
                "quote" ;
        <http://www.w3.org/2000/01/rdf-schema#subClassOf>
                <http://purl.org/olia/olia.owl#SecondaryPunctuation> ;
        <http://www.w3.org/2002/07/owl#versionInfo>
                "http://www.isocat.org/datcat/DC-2081" .

<http://purl.org/olia/olia.owl#HabitualMood>
        a       <http://www.w3.org/2002/07/owl#Class> ;
        <http://www.w3.org/2000/01/rdf-schema#comment>
                "\"Habitual\" is normally considered to be an aspect. Occasionally, it is, however, also described as a mood, e.g., by Bittner (2008, p. 354) for Kalaalisut (Greenlandic).\n\t\t\n\t\tMaria Bittner (2008), Aspectual universals of temporal anaphora, In: Susan Deborah Rothstein (ed.), Theoretical and crosslinguistic approaches to the semantics of aspect, John Benjamins, Amsterdam, p. 349-386.\n\t\t" ;
        <http://www.w3.org/2000/01/rdf-schema#subClassOf>
                <http://purl.org/olia/olia-top.owl#MoodFeature> ;
        <http://www.w3.org/2002/07/owl#equivalentClass>
                <http://purl.org/olia/olia.owl#HabitualAspect> ;
        <http://www.w3.org/2002/07/owl#versionInfo>
                "adopted from ILPOSTS, http://purl.org/olia/ilposts.owl#HabitualMood, I assume that HabitualMood is equivalent with HabitualAspect, \n\t\thence no corresponding HabitualModality has been introduced" .

<http://purl.org/olia/olia.owl#hasObjectPerson>
        a       <http://www.w3.org/2002/07/owl#ObjectProperty> ;
        <http://www.w3.org/2000/01/rdf-schema#comment>
                "\n                            person for the object of the verb\n                                (http://www.isocat.org/datcat/DC-2279)\n                            " ;
        <http://www.w3.org/2000/01/rdf-schema#domain>
                <http://purl.org/olia/olia.owl#Verb> ;
        <http://www.w3.org/2000/01/rdf-schema#label>
                "object person" ;
        <http://www.w3.org/2000/01/rdf-schema#range>
                <http://purl.org/olia/olia-top.owl#PersonFeature> ;
        <http://www.w3.org/2000/01/rdf-schema#subPropertyOf>
                <http://purl.org/olia/system.owl#hasFeature> ;
        <http://www.w3.org/2002/07/owl#versionInfo>
                "http://www.isocat.org/datcat/DC-2279" .

<http://purl.org/olia/olia.owl#PostHodiernalFuture>
        a       <http://www.w3.org/2002/07/owl#Class> ;
        <http://www.w3.org/2000/01/rdf-schema#comment>
                "\n\t\t\tPostHodiernalFutureTense locates the situation in question after \n\t\t\tthe span that is culturally defined as 'today' (Bybee, Perkins, \n\t\t\tand Pagliuca 1994: 247).\n\t\t\t(http://purl.org/linguistics/gold/PostHodiernalFuture)\n\t\t" ;
        <http://www.w3.org/2000/01/rdf-schema#subClassOf>
                <http://purl.org/olia/olia.owl#Future> ;
        <http://www.w3.org/2002/07/owl#versionInfo>
                "http://purl.org/linguistics/gold/PostHodiernalFuture, classified as Future here" .

<http://purl.org/olia/olia.owl#PaucalQuantifier>
        a       <http://www.w3.org/2002/07/owl#Class> ;
        <http://www.w3.org/2000/01/rdf-schema#comment>
                "Quantifiers that enforce paucal agreement. In many Slavic languages, numerals between 2 and 4 (and some quantifiers) involve a specific agreement patterns that is different from that of smaller and greater numbers. In Russian, for example, genitive singular is requires. These numerals and quantifiers with the same characteristics are referred to here as \"paucal quantifiers\".\n\t\t\t(cf. David Pesetsky, http://www.uni-leipzig.de/~jtrommer/Harvard/pesetsky.pdf)" ;
        <http://www.w3.org/2000/01/rdf-schema#subClassOf>
                <http://purl.org/olia/olia-top.owl#NumeralAgreementClass> ;
        <http://www.w3.org/2002/07/owl#equivalentClass>
                [ a       <http://www.w3.org/2002/07/owl#Class> ;
                  <http://www.w3.org/2002/07/owl#intersectionOf>
                          ( <http://purl.org/olia/olia.owl#Quantifier>
                            [ a       <http://www.w3.org/2002/07/owl#Restriction> ;
                              <http://www.w3.org/2002/07/owl#onProperty>
                                      <http://purl.org/olia/olia.owl#hasNumeralAgreementClass> ;
                              <http://www.w3.org/2002/07/owl#someValuesFrom>
                                      <http://purl.org/olia/olia.owl#PaucalQuantifier>
                            ]
                          )
                ] ;
        <http://www.w3.org/2002/07/owl#versionInfo>
                "http://purl.org/olia/mte/multext-east.owl#PaucalQuantifier" .

<http://purl.org/olia/olia.owl#PreverbalParticle>
        a       <http://www.w3.org/2002/07/owl#Class> ;
        <http://www.w3.org/2000/01/rdf-schema#subClassOf>
                <http://purl.org/olia/olia.owl#Particle> ;
        <http://www.w3.org/2002/07/owl#versionInfo>
                "http://www.isocat.org/datcat/DC-1455 (preverbalParticleLmf)" .

<http://purl.org/olia/olia.owl#LeftDislocationField>
        a       <http://www.w3.org/2002/07/owl#Class> ;
        <http://www.w3.org/2000/01/rdf-schema#comment>
                "\nThe German Linksversetzungsfeld is a field for the left-dislocated phrase of resumptive constructions. A Linksversetzung is a pendent constituent. \nIt can be regarded as a syntactic anticipation of a part of a sentence\n(Telljohann et al. 2009, p.16)\n\t\t" ;
        <http://www.w3.org/2000/01/rdf-schema#subClassOf>
                <http://purl.org/olia/olia-top.owl#TopologicalField> , <http://purl.org/olia/olia.owl#Extraposition> , <http://purl.org/olia/olia.owl#Fronting> .

<http://purl.org/olia/olia.owl#LocativePassive>
        a       <http://www.w3.org/2002/07/owl#Class> ;
        <http://www.w3.org/2000/01/rdf-schema#comment>
                "\n\t\t\tAn oblique locative nominal assumes the subject relation.\n\t\t\t(Klaiman 1991:17)\n\t\t\t(http://purl.org/linguistics/gold/LocativePassive)\n\t\t" ;
        <http://www.w3.org/2000/01/rdf-schema#subClassOf>
                <http://purl.org/olia/olia.owl#PassiveVoice> ;
        <http://www.w3.org/2002/07/owl#versionInfo>
                "http://purl.org/linguistics/gold/LocativePassive" .

<http://purl.org/olia/olia.owl#Accusative>
        a       <http://www.w3.org/2002/07/owl#Class> ;
        <http://www.w3.org/2000/01/rdf-schema#comment>
                "\n\t\t\tIn nominative-accusative languages, accusative case marks certain syntactic functions, usually direct objects. \t\t\n\t\t\t(http://www.sil.org/linguistics/glossaryoflinguisticterms/WhatIsAccusativeCase.htm 17.11.06)\n\t\t" ;
        <http://www.w3.org/2000/01/rdf-schema#subClassOf>
                <http://purl.org/olia/olia-top.owl#CaseFeature> ;
        <http://www.w3.org/2002/07/owl#versionInfo>
                "EAGLES" .

<http://purl.org/olia/olia.owl#Affix>
        a       <http://www.w3.org/2002/07/owl#Class> ;
        <http://www.w3.org/2000/01/rdf-schema#comment>
                "\n                            Letter or group of letters which are added to a word to make a new word.\n                                (Sue Ellen Wright; http://www.isocat.org/datcat/DC-1234)\n                            " ;
        <http://www.w3.org/2000/01/rdf-schema#label>
                "affix" ;
        <http://www.w3.org/2000/01/rdf-schema#subClassOf>
                <http://purl.org/olia/olia.owl#Morpheme> ;
        <http://www.w3.org/2002/07/owl#versionInfo>
                "http://www.isocat.org/datcat/DC-1234" .

<http://purl.org/olia/olia.owl#PluperfectTense>
        a       <http://www.w3.org/2002/07/owl#Class> ;
        <http://www.w3.org/2000/01/rdf-schema#comment>
                "\n\t\t\tPastInPast tense locates the situation in question prior to a reference time in the past. \n\t\t\tAlso known as PluperfectTense.\n\t\t\t(http://purl.org/linguistics/gold/PastInPast)\n\t\t" ;
        <http://www.w3.org/2000/01/rdf-schema#subClassOf>
                <http://purl.org/olia/olia.owl#AbsoluteRelativeTense> ;
        <http://www.w3.org/2002/07/owl#versionInfo>
                "http://purl.org/linguistics/gold/PastInPast, classified as absolute-relative tense here." .

<http://purl.org/olia/olia.owl#BenefactorRole>
        a       <http://www.w3.org/2002/07/owl#Class> ;
        <http://www.w3.org/2000/01/rdf-schema#comment>
                "\n\t\t\tA beneficiary (benefactor) instantiates the role of an entity (usually animate) who \n\t\t\tstands to benefit in some way from the event. Prototypically “benefit” \n\t\t\there means “to do or be good to, to be of advantage or profit to; to \n\t\t\timprove, help forward” in some way.\n\t\t\t(http://languagelink.let.uu.nl/tds/onto/LinguisticOntology.owl#beneficiaryRole)\n\t\t" ;
        <http://www.w3.org/2000/01/rdf-schema#subClassOf>
                <http://purl.org/olia/olia.owl#UndergoerMacroRole> ;
        <http://www.w3.org/2002/07/owl#versionInfo>
                "http://languagelink.let.uu.nl/tds/onto/LinguisticOntology.owl#beneficiaryRole" .

<http://purl.org/olia/olia.owl#ReducedInflection>
        a       <http://www.w3.org/2002/07/owl#Class> ;
        <http://www.w3.org/2000/01/rdf-schema#comment>
                "Reduced adjective inflection of Slavic languages, e.g., Czech e.g., brillská/brillský, neznámo/neznámý, samo/sám, samy/sám (http://purl.org/olia/mte/multext-east.owl#NominalAdjective)" ;
        <http://www.w3.org/2000/01/rdf-schema#subClassOf>
                <http://purl.org/olia/olia-top.owl#StrengthFeature> ;
        <http://www.w3.org/2002/07/owl#versionInfo>
                "http://purl.org/olia/mte/multext-east.owl#NominalAdjective" .

<http://purl.org/olia/olia.owl#Quantifier>
        a       <http://www.w3.org/2002/07/owl#Class> ;
        <http://www.w3.org/2000/01/rdf-schema#comment>
                "\n\t\tA quantifier is a determiner that expresses a referent's definite or indefinite number or amount. \n\t\tA quantifier functions as a modifier of a noun, or pronoun. \n\t\t(http://www.sil.org/linguistics/GlossaryOfLinguisticTerms/WhatIsAQuantifier.htm 19.09.06)\n\t" ;
        <http://www.w3.org/2000/01/rdf-schema#subClassOf>
                <http://purl.org/olia/olia-top.owl#MorphosyntacticCategory> ;
        <http://www.w3.org/2002/07/owl#versionInfo>
                "\n\t\tA category \"Quantifier\" is missing in EAGLES, but seems to be conflated with IndefiniteDeterminer.\n\t\tAdded as top-level concept in accordance with the SFB632 annotation guidelines.\n\t\tAgainst the original (and meanwhile corrected) modelling in GOLD, Quantifier is not a subconcept of Determiner.\n\t" .

<http://purl.org/olia/olia.owl#First>
        a       <http://www.w3.org/2002/07/owl#Class> ;
        <http://www.w3.org/2000/01/rdf-schema#comment>
                "First person deixis is deictic reference that refers to the speaker, or both the speaker and referents grouped with the speaker (http://www.isocat.org/datcat/DC-1288)\n\t  \n\t  cf. gold:First: Refers to the speaker and one or more nonparticipants, but not hearer(s). Contrasts with  FirstPersonInclusive (Crystal 1997: 285).\n\t\t\t(http://purl.org/linguistics/gold/First)\n\t\t" ;
        <http://www.w3.org/2000/01/rdf-schema#isDefinedBy>
                "http://www.isocat.org/datcat/DC-1288" ;
        <http://www.w3.org/2000/01/rdf-schema#label>
                "first person" ;
        <http://www.w3.org/2000/01/rdf-schema#subClassOf>
                <http://purl.org/olia/olia-top.owl#PersonFeature> ;
        <http://www.w3.org/2002/07/owl#versionInfo>
                "EAGLES, http://purl.org/linguistics/gold/First" .

<http://purl.org/olia/olia.owl#SubterminativeCase>
        a       <http://www.w3.org/2002/07/owl#Class> ;
        <http://www.w3.org/2000/01/rdf-schema#comment>
                "\n\t\t\tSubterminativeCase expresses the notion of something moving into \n\t\t\tthe region under the referent of the noun it marks, but not through \n\t\t\tthat region. It has the meaning 'into the region under'.\n\t\t\t(http://purl.org/linguistics/gold/Subterminative)\n\t\t" ;
        <http://www.w3.org/2000/01/rdf-schema#subClassOf>
                <http://purl.org/olia/olia-top.owl#CaseFeature> ;
        <http://www.w3.org/2002/07/owl#versionInfo>
                "http://purl.org/linguistics/gold/Subterminative" .

<http://purl.org/olia/olia.owl#StructuralExpletive>
        a       <http://www.w3.org/2002/07/owl#Class> ;
        <http://www.w3.org/2000/01/rdf-schema#comment>
                "\n\t\t\tThree different expletive usages [of the German expletive pronoun es]\n\t\t\tare traditionally distinguished: formal subject or object (expletive argument), \n\t\t\tcorrelate of an extraposed clausal argument (expletive correlate), and Vorfeld-es (structural expletive)\n\t\t\t(cf. (Eisenberg 1999 2001), (Pütz 1986)).\n\t\t\t(Telljohann et al. 2009, p.60)\n\t\t\t\n\t\t\tIn German, a purely structural dummy element ... occurs in Vorfeld position only\n\t\t\tand is not correlated with any argument of the clause. It does not agree with the verb\n\t\t\twhich becomes evident if there is a plural subject in the Mittelfeld: \n\t\t\t\n\t\t\t\"es zahlen ihn die Völker, deren Menschenrechte angeblich verteidigt werden.\"\n\t\t\t\n\t\t\tIt is ungrammatical in the Mittelfeld, e.g. *\". . . dass es ihn die Völker zahlen\".\n\t\t" ;
        <http://www.w3.org/2000/01/rdf-schema#subClassOf>
                <http://purl.org/olia/olia.owl#ExpletivePronoun> ;
        <http://www.w3.org/2002/07/owl#versionInfo>
                "\n\t\t\tTüBa-D/Z\n\t\t" .

<http://purl.org/olia/olia.owl#Date>
        a       <http://www.w3.org/2002/07/owl#Class> ;
        <http://www.w3.org/2000/01/rdf-schema#comment>
                "Date is a stretch of text that specifies a specific point in time and that is not further linguistically analysed. (Chiarcos)" ;
        <http://www.w3.org/2000/01/rdf-schema#subClassOf>
                <http://purl.org/olia/olia.owl#Residual> ;
        <http://www.w3.org/2002/07/owl#versionInfo>
                "adopted from Sajjad (2007, for Urdu, cf. http://purl.org/olia/urdu.owl#Date)" .

<http://purl.org/olia/olia.owl#hasDegree>
        a       <http://www.w3.org/2002/07/owl#ObjectProperty> ;
        <http://www.w3.org/2000/01/rdf-schema#domain>
                [ a       <http://www.w3.org/2002/07/owl#Class> ;
                  <http://www.w3.org/2002/07/owl#unionOf>
                          ( <http://purl.org/olia/olia.owl#Adjective> <http://purl.org/olia/olia.owl#Adverb> )
                ] ;
        <http://www.w3.org/2000/01/rdf-schema#range>
                <http://purl.org/olia/olia-top.owl#DegreeFeature> ;
        <http://www.w3.org/2000/01/rdf-schema#subPropertyOf>
                <http://purl.org/olia/system.owl#hasFeature> .

<http://purl.org/olia/olia.owl#Converb>
        a       <http://www.w3.org/2002/07/owl#Class> ;
        <http://www.w3.org/2000/01/rdf-schema#comment>
                "A converb is \"[...] a nonfinite verb form whose main function is to mark adverbial subordination. Another way of putting it is that converbs are verbal adverbs, just like participles are verbal adjectives.\" \nHaspelmath, M., & König, E. (1995). Converbs in cross-linguistic perspective, p. 3" ;
        <http://www.w3.org/2000/01/rdf-schema#subClassOf>
                <http://purl.org/olia/olia.owl#NonFiniteVerb> ;
        <http://www.w3.org/2002/07/owl#versionInfo>
                "Introduced to account for Converbs in Armenian and other languages, a generalization over деепричастие" , "TODO: clarify terminological relation between Converb, Supine and AdverbialParticiple" .

<http://purl.org/olia/olia.owl#OpenBracket>
        a       <http://www.w3.org/2002/07/owl#Class> ;
        <http://www.w3.org/2000/01/rdf-schema#comment>
                "\n                            Punctuation that is represented graphically as [\n                                (http://www.isocat.org/datcat/DC-2082)\n                            " ;
        <http://www.w3.org/2000/01/rdf-schema#label>
                "open bracket" ;
        <http://www.w3.org/2000/01/rdf-schema#subClassOf>
                <http://purl.org/olia/olia.owl#LeftParentheticalPunctuation> ;
        <http://www.w3.org/2002/07/owl#versionInfo>
                "http://www.isocat.org/datcat/DC-2082" .

<http://purl.org/olia/olia.owl#Adjunction>
        a       <http://www.w3.org/2002/07/owl#Class> ;
        <http://www.w3.org/2000/01/rdf-schema#comment>
                "The term \\adjunction structure\" refers to structures which would be represented by tree diagrams of\nthe general form in (@9). The de ning characteristic of adjunction structures is that a node X dominates\nanother instance of X.\n(Santorini 1991)\n\t\t" ;
        <http://www.w3.org/2000/01/rdf-schema#subClassOf>
                <http://purl.org/olia/olia-top.owl#SyntacticConstruction> ;
        <http://www.w3.org/2002/07/owl#versionInfo>
                "PTB Bracketing Guidelines, Santorini (1991)" .

<http://purl.org/olia/olia.owl#ConditionalRealisModality>
        a       <http://www.w3.org/2002/07/owl#Class> ;
        <http://www.w3.org/2000/01/rdf-schema#comment>
                "Conditional Mood (modality) with Realis meaning (ILPOSTS)" ;
        <http://www.w3.org/2000/01/rdf-schema#subClassOf>
                <http://purl.org/olia/olia.owl#ConditionalModality> ;
        <http://www.w3.org/2002/07/owl#versionInfo>
                "ILPOSTS (Indian languages), http://purl.org/olia/ilposts.owl#Real is restricted to conditional participles, hence probably a subtype of ConditionalMood" .

<http://purl.org/olia/olia.owl#Inclusive>
        a       <http://www.w3.org/2002/07/owl#Class> ;
        <http://www.w3.org/2000/01/rdf-schema#comment>
                "the form denoting that the addressee (addressees) are included into the set of their referents which contain also the speaker" ;
        <http://www.w3.org/2000/01/rdf-schema#isDefinedBy>
                "http://www.isocat.org/datcat/DC-3030" ;
        <http://www.w3.org/2000/01/rdf-schema#subClassOf>
                <http://purl.org/olia/olia-top.owl#ClusivityFeature> .

<http://purl.org/olia/olia.owl#Trial>
        a       <http://www.w3.org/2002/07/owl#Class> ;
        <http://www.w3.org/2000/01/rdf-schema#comment>
                "\n                            Grammatical number referring to 'three things', as opposed to 'singular' and 'plural'.\n                                (en2.wikipedia.org/wiki/Trial_number; http://www.isocat.org/datcat/DC-1407)\n                            " ;
        <http://www.w3.org/2000/01/rdf-schema#label>
                "trial" ;
        <http://www.w3.org/2000/01/rdf-schema#subClassOf>
                <http://purl.org/olia/olia-top.owl#NumberFeature> ;
        <http://www.w3.org/2002/07/owl#versionInfo>
                "http://www.isocat.org/datcat/DC-1407" , "subClassOf grammaticalNumber (dcif:conceptualDomain)" .

<http://purl.org/olia/olia.owl#InitialCoordinatingConjunction>
        a       <http://www.w3.org/2002/07/owl#Class> ;
        <http://www.w3.org/2000/01/rdf-schema#comment>
                "\n\t\t\tWhen two distinct words occur, as in German \"weder...noch...\", then \n\t\t\tthe first is given the Initial value. \n\t\t\t(http://www.ilc.cnr.it/EAGLES96/annotate/node18.html#oav1av  17.11.06)\n\t\t" ;
        <http://www.w3.org/2000/01/rdf-schema#subClassOf>
                <http://purl.org/olia/olia.owl#CoordinatingConjunction> ;
        <http://www.w3.org/2002/07/owl#versionInfo>
                "EAGLES" .

<http://purl.org/olia/olia.owl#FiniteVerbPhrase>
        a       <http://www.w3.org/2002/07/owl#Class> ;
        <http://www.w3.org/2000/01/rdf-schema#subClassOf>
                <http://purl.org/olia/olia.owl#VerbPhrase> ;
        <http://www.w3.org/2002/07/owl#versionInfo>
                "TüBa-D/Z" .

<http://purl.org/olia/olia.owl#WithComparative>
        a       <http://www.w3.org/2002/07/owl#Class> ;
        <http://www.w3.org/2000/01/rdf-schema#comment>
                "\n\t\t\tFor example, in German the subordinating conjunction \"als\" is followed \n\t\t\tby various kinds of comparative clause (including clauses without finite \n\t\t\tverbs). \n\t\t\t(http://www.ilc.cnr.it/EAGLES96/annotate/node19.html#oav2u  17.11.06)\n\t\t" ;
        <http://www.w3.org/2000/01/rdf-schema#subClassOf>
                <http://purl.org/olia/olia-top.owl#SubordTypeFeature> ;
        <http://www.w3.org/2002/07/owl#deprecated>
                true ;
        <http://www.w3.org/2002/07/owl#versionInfo>
                "EAGLES, reimplemented within SubordinatingConjunction taxonomy" .

<http://purl.org/olia/olia.owl#PseudopassiveVoice>
        a       <http://www.w3.org/2002/07/owl#Class> ;
        <http://www.w3.org/2000/01/rdf-schema#comment>
                "voice in a specify passive construction (different from the regular passive) where the patient is the syntactic subject and agent is the syntactic object" ;
        <http://www.w3.org/2000/01/rdf-schema#isDefinedBy>
                "http://www.isocat.org/datcat/DC-3851" ;
        <http://www.w3.org/2000/01/rdf-schema#subClassOf>
                <http://purl.org/olia/olia.owl#PassiveVoice> .

<http://purl.org/olia/olia.owl#Suffix>
        a       <http://www.w3.org/2002/07/owl#Class> ;
        <http://www.w3.org/2000/01/rdf-schema#comment>
                "\n                            Affix added at the end of the word to change its meaning or part of speech.\n                                (Sue Ellen Wright + Gil Francopoulo; http://www.isocat.org/datcat/DC-1395)\n                            " ;
        <http://www.w3.org/2000/01/rdf-schema#label>
                "suffix" ;
        <http://www.w3.org/2000/01/rdf-schema#subClassOf>
                <http://purl.org/olia/olia.owl#Affix> ;
        <http://www.w3.org/2002/07/owl#versionInfo>
                "http://www.isocat.org/datcat/DC-1395" .

<http://purl.org/olia/olia-top.owl#CaseFeature>
        a       <http://www.w3.org/2002/07/owl#Class> ;
        <http://www.w3.org/2000/01/rdf-schema#subClassOf>
                [ a       <http://www.w3.org/2002/07/owl#Restriction> ;
                  <http://www.w3.org/2002/07/owl#hasSelf>
                          true ;
                  <http://www.w3.org/2002/07/owl#onProperty>
                          <http://purl.org/olia/olia.owl#hasCase>
                ] ;
        <http://www.w3.org/2002/07/owl#versionInfo>
                "TODO: \n\t\t\trename all subconcepts to ...Case\n\t\t" , "Note that also Indian case markers were included here (ILPOSTS). These are described differently, either as postpositions or as grammatical cases." , "\n\t\t\tSkipped EAGLES case feature values Uninflected (uninformative), and\n\t\t\tNonGenitive (= complement of Genitive).\n\t\t\tAs for TDS case feature values, only \"grammaticalCase\" has been adopted.\n\t\t\tAs for GOLD case feature values, everything has been adopted, although it seems\n\t\t\tthat some of these cases are actually semantic (theta) roles, i.e., \"case\" in the\n\t\t\tsense of Fillmore (1966), e.g., BenefactiveCase.\n\t\t" .

<http://purl.org/olia/olia.owl#CommonGender>
        a       <http://www.w3.org/2002/07/owl#Class> ;
        <http://www.w3.org/2000/01/rdf-schema#comment>
                "\n\t\t\tCommon is an optional attribute for nouns in EAGLES. \n\t\t\tThe Common gender contrasts with Neuter in a two-gender system e.g. Danish, Dutch. \n\t\t\tThis value is also used for articles, pronouns and determiners especially for Danish. \t\n\t\t\t(http://www.ilc.cnr.it/EAGLES96/annotate/node19.html#oav2at  17.11.06)\n\t\t" ;
        <http://www.w3.org/2000/01/rdf-schema#subClassOf>
                <http://purl.org/olia/olia-top.owl#GenderFeature> ;
        <http://www.w3.org/2002/07/owl#versionInfo>
                "EAGLES" .

<http://purl.org/olia/olia.owl#Classifier>
        a       <http://www.w3.org/2002/07/owl#Class> ;
        <http://www.w3.org/2000/01/rdf-schema#comment>
                "\n\t\t\tA classifier is a word or affix that expresses the classification of a noun.\n\t\t\t(http://www.sil.org/linguistics/GlossaryOfLinguisticTerms/WhatIsAClassifier.htm 19.09.06)\n\n\t\t\tClassifiers are a very typical feature of sign languages.\n\t\t\tIn some Asian languages, classifiers are used as particles to combine a noun with a numeral,\n\t\t\te.g. chin. _san ge ren_ 'three pieces of people', 'three people' (Bußmann 2002, under Klassifikator)\n\t\t\t\n\t\t\tBharati et al. (2006, for Indian languages) group Classifiers together with Quantifiers and Numerals, but they do not provide a detailed characterization of this class.\n\n\t\t\tAkshar Bharati, Dipti Misra Sharma, Lakshmi Bai, Rajeev Sangal (2006), AnnCorra : Annotating Corpora. Guidelines For POS And Chunk Annotation For Indian Languages, Tech. Rep., L anguage Technologies Research Centre IIIT, Hyderabad, version of 15-12-2006, http://ltrc.iiit.ac.in/tr031/posguidelines.pdf\n\t\t" ;
        <http://www.w3.org/2000/01/rdf-schema#subClassOf>
                <http://purl.org/olia/olia.owl#Unique> ;
        <http://www.w3.org/2002/07/owl#versionInfo>
                "Added for compatibility with the SFB632 annotation guidelines." .

<http://purl.org/olia/olia.owl#FutureInFuture>
        a       <http://www.w3.org/2002/07/owl#Class> ;
        <http://www.w3.org/2000/01/rdf-schema#comment>
                "\n\t\t\tFutureInFutureTense locates the situation in question in the future, \n\t\t\trelative to a temporal reference point that itself is located in the \n\t\t\tfuture relative to the moment of utterance.\n\t\t\t(http://purl.org/linguistics/gold/FutureInFuture)\n\t\t" ;
        <http://www.w3.org/2000/01/rdf-schema#subClassOf>
                <http://purl.org/olia/olia.owl#AbsoluteRelativeTense> ;
        <http://www.w3.org/2002/07/owl#versionInfo>
                "http://purl.org/linguistics/gold/FutureInFuture, classified as absolute-relative tense here." .

<http://purl.org/olia/olia.owl#QuotativeVerb>
        a       <http://www.w3.org/2002/07/owl#Class> ;
        <http://www.w3.org/2000/01/rdf-schema#comment>
                "A quotative is grammatical device to mark reported speech in some languages (http://en.wikipedia.org/wiki/Quotative), e.g., in Estonian.<br/>\n\t\t\n\t\t‘Reportedly, while he was going (in his boat), he turned over.’\n\t\tTa olevat        oma     paadiga   ümber läinud\n\t\tHe was_QUOTATIVE his_own boat_WITH over  gone.<br/>\n\t\t\n\t\t(Estonian translation of an example given under http://www.sil.org/linguistics/GlossaryOfLinguisticTerms/WhatIsAQuotativeEvidential.htm)\n\t\t(Heiki-Jaan Kaalep, email 2010/06/22)" ;
        <http://www.w3.org/2000/01/rdf-schema#subClassOf>
                <http://purl.org/olia/olia-top.owl#MoodFeature> ;
        <http://www.w3.org/2002/07/owl#versionInfo>
                "http://purl.org/olia/mte/multext-east.owl#Quotative, MTE VForm=\"quotative\" (Estonian)" .

<http://purl.org/olia/olia.owl#hasObjectNumber>
        a       <http://www.w3.org/2002/07/owl#ObjectProperty> ;
        <http://www.w3.org/2000/01/rdf-schema#comment>
                "\n\t\t\tNumber of the object of a transitive verb. (Note that this does not entail of hasNumber).\n\t\t" ;
        <http://www.w3.org/2000/01/rdf-schema#domain>
                [ a       <http://www.w3.org/2002/07/owl#Class> ;
                  <http://www.w3.org/2002/07/owl#intersectionOf>
                          ( <http://purl.org/olia/olia.owl#Verb>
                            [ a       <http://www.w3.org/2002/07/owl#Restriction> ;
                              <http://www.w3.org/2002/07/owl#onProperty>
                                      <http://purl.org/olia/olia.owl#hasSyntacticValency> ;
                              <http://www.w3.org/2002/07/owl#someValuesFrom>
                                      <http://purl.org/olia/olia.owl#Transitive>
                            ]
                          )
                ] ;
        <http://www.w3.org/2000/01/rdf-schema#range>
                <http://purl.org/olia/olia-top.owl#NumberFeature> ;
        <http://www.w3.org/2000/01/rdf-schema#subPropertyOf>
                <http://purl.org/olia/system.owl#hasFeature> ;
        <http://www.w3.org/2002/07/owl#versionInfo>
                "introduced for double agreement of transitive verbs, e.g., in Hungarian, see http://purl.org/olia/mte/multext-east.owl#FirstSgSecondSg" .

<http://purl.org/olia/olia.owl#RaisableArgument>
        a       <http://www.w3.org/2002/07/owl#Class> ;
        <http://www.w3.org/2002/07/owl#deprecated>
                true ;
        <http://www.w3.org/2002/07/owl#equivalentClass>
                [ a       <http://www.w3.org/2002/07/owl#Class> ;
                  <http://www.w3.org/2002/07/owl#intersectionOf>
                          ( <http://purl.org/olia/olia.owl#Raising> <http://purl.org/olia/olia.owl#SyntacticArgument> )
                ] ;
        <http://www.w3.org/2002/07/owl#versionInfo>
                "from http://lemon-model.net/lemon#RaisableArgument, deprecated because this is just a shorthand for Raising and SyntacticArgument" .

<http://purl.org/olia/olia.owl#InchoativeAspect>
        a       <http://www.w3.org/2002/07/owl#Class> ;
        <http://www.w3.org/2000/01/rdf-schema#comment>
                "Aspect that expresses the beginning of an event or state." ;
        <http://www.w3.org/2000/01/rdf-schema#isDefinedBy>
                "http://www.isocat.org/datcat/DC-2002" ;
        <http://www.w3.org/2000/01/rdf-schema#label>
                "inchoative" ;
        <http://www.w3.org/2000/01/rdf-schema#subClassOf>
                <http://purl.org/olia/olia-top.owl#AspectFeature> .

<http://purl.org/olia/olia.owl#AdverbPhrase>
        a       <http://www.w3.org/2002/07/owl#Class> ;
        <http://www.w3.org/2000/01/rdf-schema#comment>
                "\n\t\t\tAn adverb phrase may consist of an adverb, or a sequence of words in which an adverb is the head of the phrase.\n\t\t\tAdverb phrases may function as adverbials, as in 41:\n\n\t\t\t(41)  \t[NP Her beautiful white hat NP] [VP was [ADVP very nearly ADVP] ruined VP]\n\t\t\t\n\t\t\tor as modifiers of adjectives, as in 42:\n\t\t\t\n\t\t\t(42)  \t[NP Il NP] [VP parle [ADVP infiniment plus couramment ADVP] VP]\n\n\t\t\tor noun phrases, as in 43:\n\n\t\t\t(43)  \t[NP They NP] [VP let [NP me NP] [VP speak VP] [ADVP now and then ADVP] VP]\n\t\t\t\n\t\t\tor as the complement of a preposition, as in 44:\n\t\t\t\n\t\t\t(44)  \t[ADVP Strangely enough ADVP] , [NP we NP] [VP received [NP a reply NP] [NP the next day NP] VP]\n\n\t\t\tOther examples:\n\n\t\t\t(45)  \t[NP The book NP] [VP is [ADVP right here ADVP] VP]\n\t\t\t(46)  \t[ADVP Como [NP resultado [PP de [NP esa trama NP] PP] NP] ADVP] \n\t\t\t\t\t[VP no se lleva [PP a cabo PP] [NP ninguna acción NP] VP] \n\t\t\t\t\t\n\t\t\t(http://www.ilc.cnr.it/EAGLES96/segsasg1/node35.html)\n\t\t" ;
        <http://www.w3.org/2000/01/rdf-schema#subClassOf>
                <http://purl.org/olia/olia.owl#Phrase> .

<http://purl.org/olia/olia.owl#HesternalPast>
        a       <http://www.w3.org/2002/07/owl#Class> ;
        <http://www.w3.org/2000/01/rdf-schema#comment>
                "\n\t\t\tHesternalPastTense locates the situation in question somewhere in \n\t\t\tthe span beginning with the period defined culturally as 'yesterday' \n\t\t\tand extends back through some period that is considered nonremote \n\t\t\t(Comrie 1985:87-88; Dahl 1985:126).\n\t\t\t(http://purl.org/linguistics/gold/HesternalPast)\n\t\t" ;
        <http://www.w3.org/2000/01/rdf-schema#subClassOf>
                <http://purl.org/olia/olia.owl#Past> ;
        <http://www.w3.org/2002/07/owl#versionInfo>
                "http://purl.org/linguistics/gold/HesternalPast, classified as Past here" .

<http://purl.org/olia/olia.owl#IndefiniteDeterminer>
        a       <http://www.w3.org/2002/07/owl#Class> ;
        <http://www.w3.org/2000/01/rdf-schema#comment>
                "\n\t\t\tAn indefinite determiner is a determiner that expresses a referent's  \n\t\t\tindefinite number or amount, i.e. \"some\", \"any\", \"many\". \n\t\t\t(http://www.sil.org/linguistics/GlossaryOfLinguisticTerms/WhatIsAQuantifier.htm 22.09.06)\n\t\t\t\n\t\t\tNote that here, a separate top-level class Quantifier has been introduced that\n\t\t\tcovers expressions of number and amount as *semantic* concepts. Plural indefinite\n\t\t\tdeterminers are thus to be modeled as IndefiniteDeteriner and Quantifier.\n\t\t" ;
        <http://www.w3.org/2000/01/rdf-schema#subClassOf>
                <http://purl.org/olia/olia.owl#Determiner> ;
        <http://www.w3.org/2002/07/owl#versionInfo>
                "EAGLES Determiner with DetType=\"Indefinite\"" .

<http://purl.org/olia/olia.owl#FullDefiniteArticle>
        a       <http://www.w3.org/2002/07/owl#Class> ;
        <http://www.w3.org/2000/01/rdf-schema#comment>
                "\n                            For definiteness, when a specific form is the syntactic subject of the clause.\n                                (DFKI; http://www.isocat.org/datcat/DC-1928)\n                            " ;
        <http://www.w3.org/2000/01/rdf-schema#label>
                "full article" ;
        <http://www.w3.org/2000/01/rdf-schema#subClassOf>
                <http://purl.org/olia/olia.owl#DefiniteArticle> ;
        <http://www.w3.org/2002/07/owl#versionInfo>
                "DCR: \"full article\" in dcif:conceptualDomain definiteness, remodelled as a property of DefiniteArticles here" , "http://www.isocat.org/datcat/DC-1928" .

<http://purl.org/olia/olia.owl#NegativeAdverb>
        a       <http://www.w3.org/2002/07/owl#Class> ;
        <http://www.w3.org/2000/01/rdf-schema#comment>
                "Adverb/Type=\"negative\" are used in the Serbian and Romanian MTE v4 specs, e.g., for Romanian nicăieri - nowhere, niciodată - never. (MTE v4)\n\t\t(http://purl.org/olia/mte/multext-east.owl#NegativeAdverb)" ;
        <http://www.w3.org/2000/01/rdf-schema#subClassOf>
                <http://purl.org/olia/olia.owl#Adverb> ;
        <http://www.w3.org/2002/07/owl#versionInfo>
                "to be modelled as SemanticRole (cf. CausalAdverb) ?" , "http://purl.org/olia/mte/multext-east.owl#NegativeAdverb" .

<http://purl.org/olia/olia.owl#Composition>
        a       <http://www.w3.org/2002/07/owl#Class> ;
        <http://www.w3.org/2000/01/rdf-schema#comment>
                "In linguistics, a compound is a lexeme (less precisely, a word) that consists of more than one stem. Compounding or composition is the word formation that creates compound lexemes (the other word-formation process being derivation). Compounding or Word-compounding refers to the faculty and device of language to form new words by combining or putting together old words. In other words, compound, compounding or word-compounding occurs when a person attaches two or more words together to make them one word. The meanings of the words interrelate in such a way that a new meaning comes out which is very different from the meanings of the words in isolation.\n\t\t(http://en.wikipedia.org/wiki/Compound_%28linguistics%29)" ;
        <http://www.w3.org/2000/01/rdf-schema#subClassOf>
                <http://purl.org/olia/olia-top.owl#MorphologicalProcess> ;
        <http://www.w3.org/2002/07/owl#versionInfo>
                "adopted from Ancorra, http://purl.org/olia/ancorra.owl#Compound" .

<http://purl.org/olia/olia.owl#Paucal>
        a       <http://www.w3.org/2002/07/owl#Class> ;
        <http://www.w3.org/2000/01/rdf-schema#comment>
                "\n                            Number that specifies 'a few' things.\n                                (en2.wikipedia.org/wiki/Paucal_number; http://www.isocat.org/datcat/DC-1350)\n                            " ;
        <http://www.w3.org/2000/01/rdf-schema#label>
                "paucal" ;
        <http://www.w3.org/2000/01/rdf-schema#subClassOf>
                <http://purl.org/olia/olia-top.owl#NumberFeature> ;
        <http://www.w3.org/2002/07/owl#versionInfo>
                "TODO: rename to PaucalNumber, because of the existence of PaucalQuantifier in MULTEXT-East" , "subClassOf grammaticalNumber (dcif:conceptualDomain)" , "http://www.isocat.org/datcat/DC-1350" .

<http://purl.org/olia/olia.owl#PathRole>
        a       <http://www.w3.org/2002/07/owl#Class> ;
        <http://www.w3.org/2000/01/rdf-schema#comment>
                "added in accordance with TIGER way (directional modifier)" ;
        <http://www.w3.org/2000/01/rdf-schema#subClassOf>
                <http://purl.org/olia/olia.owl#DirectionRole> ;
        <http://www.w3.org/2002/07/owl#versionInfo>
                "added in accordance with TIGER way (directional modifier)" .

<http://purl.org/olia/olia.owl#Nominal>
        a       <http://www.w3.org/2002/07/owl#Class> ;
        <http://www.w3.org/2000/01/rdf-schema#comment>
                "-NOM (nominal)\n— marks free (“headless”) relatives and gerunds when they act nominally. (See section 9 [WH-Phrases] for more information about free relatives, and section 13 [Gerunds and Participles] for more information about gerunds.) \n(Bies et al. 1995)" ;
        <http://www.w3.org/2000/01/rdf-schema#subClassOf>
                <http://purl.org/olia/olia-top.owl#SyntacticFunction> ;
        <http://www.w3.org/2002/07/owl#versionInfo>
                "Bies et al. 1995" .

<http://purl.org/olia/olia.owl#EquativeCase>
        a       <http://www.w3.org/2002/07/owl#Class> ;
        <http://www.w3.org/2000/01/rdf-schema#comment>
                "\n\t\tCase that expresses likeness or identity to the \n\t\treferent of the noun it marks. It can have meaning, \n\t\tsuch as: 'as', 'like', or 'in the capacity of'. \n\t\t(http://www.isocat.org/datcat/DC-1279)\n\t\t"@en ;
        <http://www.w3.org/2000/01/rdf-schema#subClassOf>
                <http://purl.org/olia/olia-top.owl#CaseFeature> ;
        <http://www.w3.org/2002/07/owl#versionInfo>
                "http://www.isocat.org/datcat/DC-1279" .

<http://purl.org/olia/olia-top.owl#OrthographicEntity>
        a       <http://www.w3.org/2002/07/owl#Class> .

<http://purl.org/olia/olia.owl#Pronoun>
        a       <http://www.w3.org/2002/07/owl#Class> ;
        <http://www.w3.org/2000/01/rdf-schema#comment>
                "\n\t\tA pronoun is a pro-form which functions like a noun and substitutes for a \n\t\tnoun or a noun-phrase. A language may have several classes of pronouns.\n\t\t(http://www.sil.org/linguistics/GlossaryOfLinguisticTerms/WhatIsAPronoun.htm 19.09.06)\n\t\t\n\t\tA pronominal is a phrase that functions as a pronoun\n        (www.sil.org/linguistics/GlossaryOfLinguisticTerms/WhatIsAPronominal.htm; http://www.isocat.org/datcat/DC-1369)\n\t" ;
        <http://www.w3.org/2000/01/rdf-schema#subClassOf>
                <http://purl.org/olia/olia.owl#PronounOrDeterminer> ;
        <http://www.w3.org/2002/07/owl#versionInfo>
                "\n\t\tEAGLES PronounOrDeterminer with Category=\"Pronoun\".\n\t" .

<http://purl.org/olia/olia.owl#PartitiveDeterminer>
        a       <http://www.w3.org/2002/07/owl#Class> ;
        <http://www.w3.org/2000/01/rdf-schema#comment>
                "\n\t\t\tA partitive determiner indicates an indefinite quantity of a mass noun; \n\t\t\tthere is no partitive article in English, though the words some or any \n\t\t\toften have that function.\n\t\t\t(Wilson and Leech 1996)\n\t\t" ;
        <http://www.w3.org/2000/01/rdf-schema#subClassOf>
                <http://purl.org/olia/olia.owl#Determiner> ;
        <http://www.w3.org/2002/07/owl#versionInfo>
                "EAGLES Determiner with DetType=\"Partitive\"." , "TODO: Check the relationship between PartitiveDeterminer and PartitiveCase:\n\t\t\n\t\t\tThe partitive case is a grammatical case which denotes \"partialness\", \n\t\t\t\"without result\", or \"without specific identity\" \n\t\t\t(http://languagelink.let.uu.nl/tds/onto/LinguisticOntology.owl#partitiveCase, \n\t\t\twith reference to http://en.wikipedia.org/wiki/Partitive).\n\t\t\t\n\t\t\tPartitiveCase expresses the partial nature of the referent of the noun \n\t\t\tit marks, as opposed to expressing the whole unit or class of which the \n\t\t\treferent is a part. This case may be found in items such as the \n\t\t\tfollowing: existential clauses, nouns that are accompanied by numerals \n\t\t\tor units of measure, or predications of material from which something \n\t\t\tis made. It often has a meaning similar to the English word 'some'.\n\t\t\t(GOLD, \"Partitive\"; see there for references)\n\t\t" .

<http://purl.org/olia/olia-top.owl#SyntacticRole>
        a       <http://www.w3.org/2002/07/owl#Class> ;
        <http://www.w3.org/2000/01/rdf-schema#subClassOf>
                [ a       <http://www.w3.org/2002/07/owl#Restriction> ;
                  <http://www.w3.org/2002/07/owl#hasSelf>
                          true ;
                  <http://www.w3.org/2002/07/owl#onProperty>
                          <http://purl.org/olia/olia.owl#hasSyntacticRole>
                ] ;
        <http://www.w3.org/2002/07/owl#versionInfo>
                "\n\t\t\t2010/04/08 merged with EAGLES NPFunction\n\t\t\t\"NPFunction is an additional optional attribute for adjectives. \n\t\t\tIt subsumes the values HeadFunction, Postmodifying and Premodifying.\" \n\t\t\t(http://www.ilc.cnr.it/EAGLES96/annotate/node18.html#oav1a  20.11.06)\n\t\t" .

<http://purl.org/olia/olia-top.owl#DiscourseEntity>
        a       <http://www.w3.org/2002/07/owl#Class> .

<http://purl.org/olia/olia.owl#AspectParticle>
        a       <http://www.w3.org/2002/07/owl#Class> ;
        <http://www.w3.org/2000/01/rdf-schema#comment>
                "In the Romanian MULTEXT-East scheme, a verbal particle with Particle/Type=\"aspect\" modifies the verbs and carries information on the verb form, i.e., on its aspect  (Dan Tufis, email 2010/06/09, http://purl.org/olia/mte/multext-east.owl#AspectParticle)" ;
        <http://www.w3.org/2000/01/rdf-schema#subClassOf>
                <http://purl.org/olia/olia.owl#VerbalParticle> ;
        <http://www.w3.org/2002/07/owl#versionInfo>
                "http://purl.org/olia/mte/multext-east.owl#AspectParticle" .

<http://purl.org/olia/olia.owl#LocationalCase>
        a       <http://www.w3.org/2002/07/owl#Class> ;
        <http://www.w3.org/2000/01/rdf-schema#comment>
                "\n\t\t\tCategory of case that denotes that the referent of the noun it \n\t\t\tmarks is a location.\n\t\t\t(http://purl.org/linguistics/gold/Locational)\n\t\t" ;
        <http://www.w3.org/2000/01/rdf-schema#subClassOf>
                <http://purl.org/olia/olia-top.owl#CaseFeature> ;
        <http://www.w3.org/2002/07/owl#versionInfo>
                "http://purl.org/linguistics/gold/Locational" .

<http://purl.org/olia/olia.owl#FixedExpression>
        a       <http://www.w3.org/2002/07/owl#Class> ;
        <http://www.w3.org/2000/01/rdf-schema#comment>
                "\n\t\t\tSome forms can only be used in a fixed context, e.g., polsku in po polsku. They are classified as special kinds of adjectives in the IPIC. In the MTE version this information is preserved in the status of a \"burkinostka\". This term is devised by Magdalena Derwojedowa and refers to dependent words like Burkina which only make sense and can be morphosyntactically identified in a fixed combination (Burkina Faso)." ;
        <http://www.w3.org/2000/01/rdf-schema#subClassOf>
                <http://purl.org/olia/olia.owl#Collocation> ;
        <http://www.w3.org/2002/07/owl#versionInfo>
                "Corresponds to MTE Burkinostka (Adverb/Clitic=\"burkinostka\"; Polish)\n\t\t\t\"Burkinostka was a local joke :). IsPartOfFixedExpression, to be more precise. Or somehow shorter.\"\n\t\t\t(Natalia Kotsyba, email 2010/06/21, http://purl.org/olia/mte/multext-east.owl#PartOfFixedExpression)" , "http://purl.org/olia/mte/multext-east.owl#PartOfFixedExpression" .

<http://purl.org/olia/olia.owl#SubstantiveAdjective>
        a       <http://www.w3.org/2002/07/owl#Class> ;
        <http://www.w3.org/2000/01/rdf-schema#comment>
                "\n                            An adjective that modifies an implied, but not expressed, noun. When translating such an adjective into English, you must supply the missing noun.\n                                (www.southwestern.edu/~carlg/Latin_Web/glossary.html; http://www.isocat.org/datcat/DC-1394)\n\t\t\t\t\t\t\t\t\n\t\t\t\t\t\t\t(Chiarcos: this seems to pertain to nominalization)\n        " ;
        <http://www.w3.org/2000/01/rdf-schema#label>
                "Substantive adjective" ;
        <http://www.w3.org/2000/01/rdf-schema#subClassOf>
                <http://purl.org/olia/olia.owl#Adjective> ;
        <http://www.w3.org/2002/07/owl#versionInfo>
                "http://www.isocat.org/datcat/DC-1394" .

<http://purl.org/olia/olia-top.owl#StrengthFeature>
        a       <http://www.w3.org/2002/07/owl#Class> ;
        <http://www.w3.org/2000/01/rdf-schema#subClassOf>
                [ a       <http://www.w3.org/2002/07/owl#Restriction> ;
                  <http://www.w3.org/2002/07/owl#hasSelf>
                          true ;
                  <http://www.w3.org/2002/07/owl#onProperty>
                          <http://purl.org/olia/olia.owl#hasStrength>
                ] ;
        <http://www.w3.org/2000/01/rdf-schema#subClassOf>
                [ a       <http://www.w3.org/2002/07/owl#Restriction> ;
                  <http://www.w3.org/2002/07/owl#hasSelf>
                          true ;
                  <http://www.w3.org/2002/07/owl#onProperty>
                          <http://purl.org/olia/olia.owl#hasStrength>
                ] ;
        <http://www.w3.org/2002/07/owl#versionInfo>
                "TODO: rename to ReductionFeature" , "TODO: link with concept hierarchy" , "merged with http://purl.org/olia/mte/multext-east.owl#AdjectiveFormation, http://purl.org/olia/mte/multext-east.owl#ReductionFeature: reduced vs. full inflection" .

<http://purl.org/olia/olia.owl#MannerAdverb>
        a       <http://www.w3.org/2002/07/owl#Class> ;
        <http://www.w3.org/2000/01/rdf-schema#subClassOf>
                <http://purl.org/olia/olia.owl#Adverb> ;
        <http://www.w3.org/2002/07/owl#deprecated>
                true ;
        <http://www.w3.org/2002/07/owl#equivalentClass>
                [ a       <http://www.w3.org/2002/07/owl#Class> ;
                  <http://www.w3.org/2002/07/owl#intersectionOf>
                          ( <http://purl.org/olia/olia.owl#Adverb>
                            [ a       <http://www.w3.org/2002/07/owl#Restriction> ;
                              <http://www.w3.org/2002/07/owl#onProperty>
                                      <http://purl.org/olia/olia.owl#hasSemanticRole> ;
                              <http://www.w3.org/2002/07/owl#someValuesFrom>
                                      <http://purl.org/olia/olia.owl#MannerRole>
                            ]
                          )
                ] ;
        <http://www.w3.org/2002/07/owl#versionInfo>
                "DEPRECATED: equivalent to Adverb and hasSemanticRole some MannerRole\n\t\t\n\t\tfrom ILPOSTS, http://purl.org/olia/ilposts.owl#MannerAdverb" .

<http://purl.org/olia/olia.owl#DistinctiveParticle>
        a       <http://www.w3.org/2002/07/owl#Class> ;
        <http://www.w3.org/2000/01/rdf-schema#comment>
                "\n                            distinctive particle\n                                (MIRACL & LSCA; http://www.isocat.org/datcat/DC-2228)\n                            " ;
        <http://www.w3.org/2000/01/rdf-schema#label>
                "distinctive particle" ;
        <http://www.w3.org/2000/01/rdf-schema#subClassOf>
                <http://purl.org/olia/olia.owl#Particle> ;
        <http://www.w3.org/2002/07/owl#versionInfo>
                "subClassOf particle (dcif:isA)" , "http://www.isocat.org/datcat/DC-2228" .

<http://purl.org/olia/olia.owl#Lexeme>
        a       <http://www.w3.org/2002/07/owl#Class> ;
        <http://www.w3.org/2000/01/rdf-schema#comment>
                "\n                            Minimal unit of language which : has a semantic interpretation and embodies a distinct cultural concept.\n                                (www.sil.org/linguistics/GlossaryOfLinguisticTerms/WhatIsALexeme.htm; http://www.isocat.org/datcat/DC-1325)\n                            " ;
        <http://www.w3.org/2000/01/rdf-schema#label>
                "lexeme" ;
        <http://www.w3.org/2000/01/rdf-schema#subClassOf>
                <http://purl.org/olia/olia.owl#LexicalUnit> ;
        <http://www.w3.org/2002/07/owl#versionInfo>
                "http://www.isocat.org/datcat/DC-1325" .

<http://purl.org/olia/olia.owl#InclusiveEmphaticParticle>
        a       <http://www.w3.org/2002/07/owl#Class> ;
        <http://www.w3.org/2000/01/rdf-schema#comment>
                "In Urdu, bhî is an emphatic particle meaning 'even'. In opposition to contrastive tô and exclusive hî, bhî is inclusive:\n\t\t\t\n\t\t\tmaim *bhî* faisalâ karûm gâ\n\t\t\t\"I'll *also* make a decision\"\n\t\t\t\n\t\t\tmaim *hî* faisalâ karûm gâ\n\t\t\t\"*I'm the one who* will make the decision.\"\n\t\t\t\n\t\t\t(Schmidt 1999, p.237, http://purl.org/olia/emille.owl#InclusiveEmphaticParticle)" ;
        <http://www.w3.org/2000/01/rdf-schema#subClassOf>
                <http://purl.org/olia/olia.owl#EmphaticParticle> , <http://purl.org/olia/olia.owl#Inclusive> ;
        <http://www.w3.org/2002/07/owl#versionInfo>
                "adopted from EMILLE for Urdu, http://purl.org/olia/emille.owl#InclusiveEmphaticParticle" .

<http://purl.org/olia/olia.owl#hasModality>
        a       <http://www.w3.org/2002/07/owl#ObjectProperty> ;
        <http://www.w3.org/2000/01/rdf-schema#range>
                <http://purl.org/olia/olia-top.owl#ModalityFeature> ;
        <http://www.w3.org/2000/01/rdf-schema#subPropertyOf>
                <http://purl.org/olia/system.owl#hasFeature> .

<http://purl.org/olia/olia.owl#YesNoQuestion>
        a       <http://www.w3.org/2002/07/owl#Class> ;
        <http://www.w3.org/2000/01/rdf-schema#comment>
                "There are two types of direct questions: yes-no questions and wh-questions. Yes-no questions should be\nbracketed as SQ. The auxiliary verb or form of do that precedes the subject in a yes-no question is a child\nof SQ. Note that yes-no questions need not contain a VP node\n(Santorini 1991)" ;
        <http://www.w3.org/2000/01/rdf-schema#subClassOf>
                <http://purl.org/olia/olia.owl#DirectQuestion> ;
        <http://www.w3.org/2002/07/owl#versionInfo>
                "Santorini 1991, Bies et al. 1995" .

<http://purl.org/olia/olia.owl#Uninflected>
        a       <http://www.w3.org/2002/07/owl#Class> ;
        <http://www.w3.org/2000/01/rdf-schema#comment>
                "\n\t\t\tIn many inflecting languages, there occur lexemes whose form does not change throughout the paradigm, e.g.,\n\t\t\tRussian papa \"dad\". For such forms, the category uninflected may be assigned.\n\t\t\tHowever, Uninflected is not to be confused with BaseForm that applies to forms in a paradigm where overt\n\t\t\tmarking exists.\n\t\t\t\n\t\t\tUninflected is a characteristic of lexemes, not individual tokens.\n\t\t" ;
        <http://www.w3.org/2000/01/rdf-schema#subClassOf>
                <http://purl.org/olia/olia-top.owl#InflectionTypeFeature> ;
        <http://www.w3.org/2002/07/owl#versionInfo>
                "Chiarcos, cf. BaseForm in Susanne (Sampson 1995) and related schemes, and http://purl.org/olia/emille.owl#UnmarkedForGender" , "For the EMILLE tagset (for Urdu, Hardi 2003), we need the possibility to specify that a lexeme is (un)inflected ([un]marked) *for a specific feature* (e.g., Gender, http://purl.org/olia/emille.owl#GenderMarking).\n\t\t\tAt the moment, this cannot be expressed." .

<http://purl.org/olia/olia.owl#ConditionalParticiple>
        a       <http://www.w3.org/2002/07/owl#Class> ;
        <http://www.w3.org/2000/01/rdf-schema#comment>
                "e.g. Bengali বুঝলে (bujhle) from বোঝা (bojha) \"to understand\" (http://en.wiktionary.org/wiki/%E0%A6%AC%E0%A7%8B%E0%A6%9D%E0%A6%BE)" , "[In Bengali, t]he Conditional Participle is widely used to convey \"if a certain action [pertaining to the parent verb] is done,...\". The logic is: \"in the\n\t\t\tcase or condition of a certain action being done\". Being impersonal, without regard for the doer of the action that caused the condition, it\n\t\t\tis not declined to suit number or gender. If this doer is not defined in the Bengali condition clause but needs to be stated in a\n\t\t\tnatural-sounding English translation, this is identified and drawn from the second clause. For example:-\n\t\t\tStudent: Teaching Truth in Bengali\n\t\t\t\n\t\t\tIf you pay attention,* you will learn.\n\t\t\tmanoyog kar-*le* tumi shikh-be.\n\t\t\t* [or, If attention is paid]\n\t\t\t\n\t\t\t(http://www.jaspell.co.uk/bengalicourse2007/wb149study49.pdf)\n\t\t" ;
        <http://www.w3.org/2000/01/rdf-schema#subClassOf>
                <http://purl.org/olia/olia.owl#Participle> ;
        <http://www.w3.org/2002/07/owl#versionInfo>
                "TODO: check whether this could be modelled as Participle and hasMood some ConditionalMood" , "adopted from ILPOSTS for Indian languages" .

<http://purl.org/olia/olia.owl#Question>
        a       <http://www.w3.org/2002/07/owl#Class> ;
        <http://www.w3.org/2000/01/rdf-schema#comment>
                "There are two types of questions: direct questions (which are main clauses ending with a question\nmark) and indirect questions (which are subordinate clauses embedded under a verb). In this section, we\ndiscuss only direct questions; indirect questions are bracketed as SBARâ ¹s (see Section 5.17).\n(Santorini 1991)" ;
        <http://www.w3.org/2000/01/rdf-schema#subClassOf>
                <http://purl.org/olia/olia-top.owl#SentenceTypeFeature> , <http://purl.org/olia/olia.owl#InterrogativeModality> ;
        <http://www.w3.org/2002/07/owl#versionInfo>
                "Santorini 1991, Bies et al. 1995" .

<http://purl.org/olia/olia.owl#RepetitiveCoordinatingConjunction>
        a       <http://www.w3.org/2002/07/owl#Class> ;
        <http://www.w3.org/2000/01/rdf-schema#comment>
                "Conjunction/Coord_Type=\"repetit\" (Romanian).\t\t\t\n\t\t\tIn Romanian, there are three kinds of conjunctions depending on their usage: as such or together with other conjunctions or adverbs: (1) simple, between conjuncts: Ion ori Maria (John or Mary); (2) repetitive, before each conjunct: fie Ion fie Maria fie... (either John or Mary or...) (3) correlative, before a conjoined phrase, it requires specific coordinators between conjuncts: atât mama cât şi tata (both mother and father). (MTE v4, http://purl.org/olia/mte/multext-east.owl#RepetitiveCoordinatingConjunction)" ;
        <http://www.w3.org/2000/01/rdf-schema#subClassOf>
                <http://purl.org/olia/olia.owl#CoordinatingConjunction> ;
        <http://www.w3.org/2002/07/owl#versionInfo>
                "http://purl.org/olia/mte/multext-east.owl#RepetitiveCoordinatingConjunction" .

<http://purl.org/olia/olia.owl#GerundVerbPhrase>
        a       <http://www.w3.org/2002/07/owl#Class> ;
        <http://www.w3.org/2000/01/rdf-schema#comment>
                "\n\t\tVGNN Gerunds\n\t\tA verb chunk having a gerund will be annotated as VGNN. For example,\n\t\th18a. sharAba ((pInA_VM))_VGNN sehata ke liye hAnikAraka hE.\n\t\t'liquor' 'drinking' 'heath' 'for' 'harmful' 'is'\n\t\t“Drinking (liquor) is bad for health”\n\t\th19a. mujhe rAta meM ((khAnA_VM))_VGNN acchA lagatA hai\n\t\t'to me' 'night' 'in' 'eating' 'good' 'appeals'\n\t\t“I like eating at night”\n\t\th20a. ((sunane_VM meM_PSP))_VGNN saba kuccha acchA lagatA hE\n\t\t'listening' 'in' 'all' 'things' 'good' 'appeal' 'is'\n\t\t\n\t\t(Akshar Bharati, Dipti Misra Sharma, Lakshmi Bai, Rajeev Sangal (2006), AnnCorra : Annotating Corpora. Guidelines For POS And Chunk Annotation For Indian Languages, Tech. Rep., L anguage Technologies Research Centre IIIT, Hyderabad, version of 15-12-2006, http://ltrc.iiit.ac.in/tr031/posguidelines.pdf)\n\t\t" ;
        <http://www.w3.org/2000/01/rdf-schema#subClassOf>
                <http://purl.org/olia/olia.owl#NonfiniteVerbPhrase> ;
        <http://www.w3.org/2002/07/owl#versionInfo>
                "Ancorra, http://purl.org/olia/ancorra.owl#GerundChunk" .

<http://purl.org/olia/olia.owl#ComplementClause>
        a       <http://www.w3.org/2002/07/owl#Class> ;
        <http://www.w3.org/2000/01/rdf-schema#comment>
                "In noun phrases like the fact that she is late, the subordinate clause that she is late is a complement of\nthe noun fact and should not be confused with a relative clause. (Note that the embedded clause she is\nlate is not missing a constituent; by contrast, in a relative clause construction like the TV that she bought\nthe other day, the clause that she bought\nthe other day is incomplete.) The entire noun phrase should be\nbracketed as a sister of the head noun.\n\n(NP the fact \n(SBAR that\n(S (NP she)\n(VP is\n(ADJP late)))))\n\n(Santorini 1991)" ;
        <http://www.w3.org/2000/01/rdf-schema#subClassOf>
                <http://purl.org/olia/olia.owl#SubordinateClause> ;
        <http://www.w3.org/2002/07/owl#versionInfo>
                "Santorini 1991" .

<http://purl.org/olia/olia.owl#SubstitutivePronoun>
        a       <http://www.w3.org/2002/07/owl#Class> ;
        <http://www.w3.org/2000/01/rdf-schema#comment>
                "non-attributive pronoun" ;
        <http://www.w3.org/2000/01/rdf-schema#subClassOf>
                <http://purl.org/olia/olia.owl#Pronoun> ;
        <http://www.w3.org/2000/01/rdf-schema#subClassOf>
                [ a       <http://www.w3.org/2002/07/owl#Class> ;
                  <http://www.w3.org/2002/07/owl#complementOf>
                          <http://purl.org/olia/olia.owl#Adjective>
                ] ;
        <http://www.w3.org/2002/07/owl#equivalentClass>
                [ a       <http://www.w3.org/2002/07/owl#Class> ;
                  <http://www.w3.org/2002/07/owl#intersectionOf>
                          ( <http://purl.org/olia/olia.owl#Pronoun>
                            [ a       <http://www.w3.org/2002/07/owl#Class> ;
                              <http://www.w3.org/2002/07/owl#complementOf>
                                      <http://purl.org/olia/olia.owl#AttributivePronoun>
                            ]
                          )
                ] ;
        <http://www.w3.org/2002/07/owl#versionInfo>
                "introduced to account for non-attributive pronouns, see olia:AttributivePronoun" .

<http://purl.org/olia/olia.owl#NonSeparable>
        a       <http://www.w3.org/2002/07/owl#Class> ;
        <http://www.w3.org/2000/01/rdf-schema#comment>
                "\n\t\t\tNon-separable verbs are not composed of a verb stem and a separable \n\t\t\taffix. (cf. SeparabilityFeature: Separable)\n\t\t" ;
        <http://www.w3.org/2000/01/rdf-schema#subClassOf>
                <http://purl.org/olia/olia-top.owl#SeparabilityFeature> ;
        <http://www.w3.org/2002/07/owl#versionInfo>
                "EAGLES; note that UbyPos extends separability to particles" .

<http://purl.org/olia/olia.owl#CountNumber>
        a       <http://www.w3.org/2002/07/owl#Class> ;
        <http://www.w3.org/2000/01/rdf-schema#comment>
                "MULTEXT-East feature Number=\"count\" (Nouns in Serbian, Macedonian, Bulgarian), e.g., Bulgarian яка/як, язовира/язовир, яда/яд, юргана/юрган, юбилея/юбилей, ъгъла/ъгъл (http://purl.org/olia/mte/multext-east.owl#CountNumber)" ;
        <http://www.w3.org/2000/01/rdf-schema#subClassOf>
                <http://purl.org/olia/olia-top.owl#NumberFeature> ;
        <http://www.w3.org/2002/07/owl#versionInfo>
                "http://purl.org/olia/mte/multext-east.owl#CountNumber" .

<http://purl.org/olia/olia.owl#Utterance>
        a       <http://www.w3.org/2002/07/owl#Class> ;
        <http://www.w3.org/2000/01/rdf-schema#comment>
                "\n                            Complete unit of talk, bounded by the speaker's silence.\n                                (www.sil.org/linguistics/GlossaryOfLinguisticTerms/WhatIsAnUtterance.htm; http://www.isocat.org/datcat/DC-1409)\n                            " ;
        <http://www.w3.org/2000/01/rdf-schema#label>
                "utterance" ;
        <http://www.w3.org/2000/01/rdf-schema#subClassOf>
                <http://purl.org/olia/olia-top.owl#DiscourseEntity> ;
        <http://www.w3.org/2002/07/owl#versionInfo>
                "http://www.isocat.org/datcat/DC-1409" .

<http://purl.org/olia/olia.owl#MultiplicativeMarker>
        a       <http://www.w3.org/2002/07/owl#Class> ;
        <http://www.w3.org/2000/01/rdf-schema#comment>
                "In Urdu, multiplicative numerals are formed by adding the suffix gunâ (Schmidt 1999, p. 260,http://purl.org/olia/emille.owl#MultiplicativeMarker)" ;
        <http://www.w3.org/2000/01/rdf-schema#subClassOf>
                <http://purl.org/olia/olia.owl#Unique> ;
        <http://www.w3.org/2002/07/owl#versionInfo>
                "introduced for Urdu gunâ (http://purl.org/olia/emille.owl#MultiplicativeMarker)" .

<http://purl.org/olia/olia.owl#ing>
        a       <http://www.w3.org/2002/07/owl#Class> ;
        <http://www.w3.org/2000/01/rdf-schema#comment>
                "English verb forms ending in '-ing' that represent either Gerunds or Participles." ;
        <http://www.w3.org/2000/01/rdf-schema#subClassOf>
                <http://purl.org/olia/olia.owl#Gerund> , <http://purl.org/olia/olia.owl#Participle> ;
        <http://www.w3.org/2002/07/owl#versionInfo>
                "\n\t\tIntroduced in accordance with EAGLES, where 'Ing' is suggested as a cover term for the Gerund-Participle-Merger in English.\n\t\tThis is, however, a language-specific phenomenon and should instead be represented by multiple inheritance from \n\t\tOLiA Reference Model concepts.\n\t" .

<http://purl.org/olia/olia.owl#OpenParenthesis>
        a       <http://www.w3.org/2002/07/owl#Class> ;
        <http://www.w3.org/2000/01/rdf-schema#comment>
                "\n                            Beginning of a pair of parenthesis.\n                                (http://www.isocat.org/datcat/DC-1442)\n                            " ;
        <http://www.w3.org/2000/01/rdf-schema#label>
                "open parenthesis" ;
        <http://www.w3.org/2000/01/rdf-schema#subClassOf>
                <http://purl.org/olia/olia.owl#LeftParentheticalPunctuation> ;
        <http://www.w3.org/2002/07/owl#versionInfo>
                "subClassOf partOfSpeech (dcif:conceptualDomain)" , "http://www.isocat.org/datcat/DC-1442" .

<http://purl.org/olia/olia.owl#ConditionalRealisMood>
        a       <http://www.w3.org/2002/07/owl#Class> ;
        <http://www.w3.org/2000/01/rdf-schema#comment>
                "Conditional Mood (modality) with Realis meaning (ILPOSTS)" ;
        <http://www.w3.org/2000/01/rdf-schema#subClassOf>
                <http://purl.org/olia/olia.owl#ConditionalMood> , <http://purl.org/olia/olia.owl#ConditionalRealisModality> ;
        <http://www.w3.org/2002/07/owl#versionInfo>
                "ILPOSTS (Indian languages), http://purl.org/olia/ilposts.owl#Real is restricted to conditional participles, hence probably a subtype of ConditionalMood" .

<http://purl.org/olia/olia.owl#OldUsage>
        a       <http://www.w3.org/2002/07/owl#Class> ;
        <http://www.w3.org/2000/01/rdf-schema#comment>
                "\n                            Used in the past.\n                                (http://www.isocat.org/datcat/DC-1961)\n                            " ;
        <http://www.w3.org/2000/01/rdf-schema#label>
                "old" ;
        <http://www.w3.org/2000/01/rdf-schema#subClassOf>
                <http://purl.org/olia/olia.owl#TemporallyDefinedUsage> ;
        <http://www.w3.org/2002/07/owl#versionInfo>
                "http://www.isocat.org/datcat/DC-1961" , "subClassOf dating (dcif:conceptualDomain)" .

<http://purl.org/olia/olia.owl#ConditionalParticle>
        a       <http://www.w3.org/2002/07/owl#Class> ;
        <http://www.w3.org/2000/01/rdf-schema#comment>
                "\n                            conditional particule\n                                (MIRACL & LSCA; http://www.isocat.org/datcat/DC-2230)\n                            " ;
        <http://www.w3.org/2000/01/rdf-schema#label>
                "conditional particule" ;
        <http://www.w3.org/2000/01/rdf-schema#subClassOf>
                <http://purl.org/olia/olia.owl#Particle> ;
        <http://www.w3.org/2002/07/owl#versionInfo>
                "http://www.isocat.org/datcat/DC-2230" , "DCR subClassOf particle (dcif:isA)" .

<http://purl.org/olia/olia-top.owl#ClusivityFeature>
        a       <http://www.w3.org/2002/07/owl#Class> ;
        <http://www.w3.org/2000/01/rdf-schema#subClassOf>
                [ a       <http://www.w3.org/2002/07/owl#Restriction> ;
                  <http://www.w3.org/2002/07/owl#hasSelf>
                          true ;
                  <http://www.w3.org/2002/07/owl#onProperty>
                          <http://purl.org/olia/olia.owl#hasClusivity>
                ] ;
        <http://www.w3.org/2000/01/rdf-schema#subClassOf>
                [ a       <http://www.w3.org/2002/07/owl#Restriction> ;
                  <http://www.w3.org/2002/07/owl#hasSelf>
                          true ;
                  <http://www.w3.org/2002/07/owl#onProperty>
                          <http://purl.org/olia/olia.owl#hasClusivity>
                ] .

<http://purl.org/olia/olia.owl#Indefinite>
        a       <http://www.w3.org/2002/07/owl#Class> ;
        <http://www.w3.org/2000/01/rdf-schema#comment>
                "\n\t\t\tAn entity is specified as indefinite when it refers to a non-particularized individual of the species denoted by the noun. \n\t\t\t(http://languagelink.let.uu.nl/tds/onto/LinguisticOntology.owl#indefinite)\n\t\t\t\n\t\t\tIndefinite noun phrases are used to refer to entities which are not specific and identifiable in a given context.\n\t\t\t(http://en.wikipedia.org/wiki/Definiteness  20.11.06)\n\t\t" ;
        <http://www.w3.org/2000/01/rdf-schema#subClassOf>
                <http://purl.org/olia/olia-top.owl#DefinitenessFeature> ;
        <http://www.w3.org/2002/07/owl#versionInfo>
                "EAGLES, http://languagelink.let.uu.nl/tds/onto/LinguisticOntology.owl#indefinite" .

<http://purl.org/olia/olia-top.owl#TopologicalField>
        a       <http://www.w3.org/2002/07/owl#Class> ;
        <http://www.w3.org/2000/01/rdf-schema#comment>
                "\n\t\tTopological fields are a descriptive formalism to describe regularities of the makro-structure of sentences, \n\t\tfor example, in the traditional description of word order inseveral Germanic languages (e.g., German, Dutch, Danish). \n\t\tMore recently, similar conceptions of topological fields have been further developed in the context of constructivistic\n\t\tgrammar formalisms, e.g., Role and Reference Grammar (van Valin and LaPolla 1997).\n\t\t" ;
        <http://www.w3.org/2002/07/owl#versionInfo>
                "Telljohann et al. (2009, p.13)" .

<http://purl.org/olia/olia.owl#Possessive>
        a       <http://www.w3.org/2002/07/owl#Class> ;
        <http://www.w3.org/2000/01/rdf-schema#comment>
                "\n                            Relative to the possession or association.\n                                (www.wordreference.com/English/definition.asp?en=possessive; http://www.isocat.org/datcat/DC-1355)\n                            " ;
        <http://www.w3.org/2000/01/rdf-schema#label>
                "possessive" ;
        <http://www.w3.org/2000/01/rdf-schema#subClassOf>
                <http://purl.org/olia/olia-top.owl#ReferentTypeFeature> ;
        <http://www.w3.org/2002/07/owl#versionInfo>
                "subClassOf referentType (dcif:conceptualDomain)" , "http://www.isocat.org/datcat/DC-1355" .

<http://purl.org/olia/olia.owl#hasPolarity>
        a       <http://www.w3.org/2002/07/owl#ObjectProperty> ;
        <http://www.w3.org/2000/01/rdf-schema#range>
                <http://purl.org/olia/olia-top.owl#PolarityFeature> ;
        <http://www.w3.org/2000/01/rdf-schema#subPropertyOf>
                <http://purl.org/olia/system.owl#hasFeature> .

<http://purl.org/olia/olia.owl#Macron>
        a       <http://www.w3.org/2002/07/owl#Class> ;
        <http://www.w3.org/2000/01/rdf-schema#comment>
                "\n                            Mark placed over a long vowel to mark quantity.\n                                (www.southwestern.edu/~carlg/Latin_Web/glossary.html; http://www.isocat.org/datcat/DC-1327)\n                            " ;
        <http://www.w3.org/2000/01/rdf-schema#label>
                "macron" ;
        <http://www.w3.org/2000/01/rdf-schema#subClassOf>
                <http://purl.org/olia/olia.owl#Diacritic> ;
        <http://www.w3.org/2002/07/owl#versionInfo>
                "http://www.isocat.org/datcat/DC-1327" .

<http://purl.org/olia/olia.owl#Third>
        a       <http://www.w3.org/2002/07/owl#Class> ;
        <http://www.w3.org/2000/01/rdf-schema#comment>
                "\n\t\t\tThird person is deictic reference to a referent(s) not identified \n\t\t\tas the speaker or addressee. For example in English \"he\", \"she\", \n\t\t\t\"they\"  or the third person singular verb suffix -s, e.g. in  \"He \n\t\t\tsometimes flies.\" \t\t\n\t\t\t(http://www.sil.org/linguistics/GlossaryOfLinguisticTerms/WhatIsThirdPersonDeixis.htm  20.11.06)\n\t\t" ;
        <http://www.w3.org/2000/01/rdf-schema#subClassOf>
                <http://purl.org/olia/olia-top.owl#PersonFeature> ;
        <http://www.w3.org/2002/07/owl#versionInfo>
                "EAGLES, http://purl.org/linguistics/gold/Third" .

<http://purl.org/olia/olia.owl#VerbalComplex>
        a       <http://www.w3.org/2002/07/owl#Class> ;
        <http://www.w3.org/2000/01/rdf-schema#comment>
                "\nIn a German clause, the finite verb can appear in three different positions: verb-second, \nverb-initial, and verb-final. Only in verb-final clauses the verb complex consisting of the\nfinite verb and non-finite verbal elements forms a unit. The discontinuous positioning\nof the verbal elements in verb-first and verb-second clauses is the traditional reason\nfor structuring German clauses into fields. The positions of the verbal elements form\nthe Satzklammer (sentence bracket) which divides the sentence into a Vorfeld (initial\nfield), a Mittelfeld (middle field), and a Nachfeld (final field). The Vorfeld and the\nMittelfeld are divided by the linke Satzklammer (left sentence bracket), which is the finite\nverb, the rechte Satzklammer (right sentence bracket) is the verb complex between the\nMittelfeld and the Nachfeld. \n(Telljohann et al. 2009, p.13)\n\nThe Verbkomplex is a sequence of verb forms. In verb-second and verb-first\nclauses it consists of one or more non-finite elements or - depending on the verb - of\na separable prefix. In verb-final clauses it also contains the finite verb. The rule for\nthe linear order in general is: right determines left. If there is a finite verb in the verb\ncomplex, it is usually the right-most element.\n(Telljohann et al. 2009, p.15)\n\t\t" ;
        <http://www.w3.org/2000/01/rdf-schema#subClassOf>
                <http://purl.org/olia/olia-top.owl#TopologicalField> .

<http://purl.org/olia/olia.owl#Abbreviation>
        a       <http://www.w3.org/2002/07/owl#Class> ;
        <http://www.w3.org/2000/01/rdf-schema#comment>
                "\n     Abbreviation (from Latin brevis \"short\") is strictly speaking a shorter form of a word, but more \n     particularly, an abbreviation is a letter or group of letters, taken from a word or words, \n     and employed to represent them for the sake of brevity. For example, the word \"abbreviation\" \n     can be abbreviated as \"abbr.\" or \"abbrev.\"\n     (http://en.wikipedia.org/wiki/Abbreviation 19.09.06)" ;
        <http://www.w3.org/2000/01/rdf-schema#label>
                "abbreviation"@en , "abreviation"@fr ;
        <http://www.w3.org/2000/01/rdf-schema#subClassOf>
                <http://purl.org/olia/olia.owl#Residual> ;
        <http://www.w3.org/2002/07/owl#versionInfo>
                "EAGLES Category Abbreviations with Type=\"Abbreviation\"." .

<http://purl.org/olia/olia.owl#hasSyntacticRole>
        a       <http://www.w3.org/2002/07/owl#ObjectProperty> ;
        <http://www.w3.org/2000/01/rdf-schema#domain>
                <http://purl.org/olia/system.owl#UnitOfAnnotation> ;
        <http://www.w3.org/2000/01/rdf-schema#range>
                <http://purl.org/olia/olia-top.owl#SyntacticRole> ;
        <http://www.w3.org/2000/01/rdf-schema#subPropertyOf>
                <http://purl.org/olia/system.owl#hasFeature> .

<http://purl.org/olia/olia.owl#UndergoerMacroRole>
        a       <http://www.w3.org/2002/07/owl#Class> ;
        <http://www.w3.org/2000/01/rdf-schema#comment>
                "\n\t\t\tThe least agentive argument of the current clause (van Valin and Lapolla 1997), \n\t\t\tthe designated object (from a semantic perspective).\n\t\t" ;
        <http://www.w3.org/2000/01/rdf-schema#subClassOf>
                <http://purl.org/olia/olia-top.owl#SemanticRole> ;
        <http://www.w3.org/2002/07/owl#versionInfo>
                "http://languagelink.let.uu.nl/tds/onto/LinguisticOntology.owl#undergoerRole" .

<http://purl.org/olia/olia.owl#ContrastiveEmphaticParticle>
        a       <http://www.w3.org/2002/07/owl#Class> ;
        <http://www.w3.org/2000/01/rdf-schema#subClassOf>
                <http://purl.org/olia/olia.owl#EmphaticParticle> ;
        <http://www.w3.org/2002/07/owl#equivalentClass>
                [ a       <http://www.w3.org/2002/07/owl#Class> ;
                  <http://www.w3.org/2002/07/owl#intersectionOf>
                          ( <http://purl.org/olia/olia.owl#ContrastiveParticle> <http://purl.org/olia/olia.owl#EmphaticParticle> )
                ] ;
        <http://www.w3.org/2002/07/owl#versionInfo>
                "adopted from EMILLE, http://purl.org/olia/emille.owl#ContrastiveEmphaticParticle, shorthand for ContrastiveParticle and EmphaticParticle" .

<http://purl.org/olia/olia-top.owl#NullElement>
        a       <http://www.w3.org/2002/07/owl#Class> .

<http://purl.org/olia/olia.owl#ImmediateFuture>
        a       <http://www.w3.org/2002/07/owl#Class> ;
        <http://www.w3.org/2000/01/rdf-schema#comment>
                "\n\t\t\tImmediateFutureTense, also called 'close future', locates the situation \n\t\t\tin question shortly after the moment of utterance (Dahl 1985:121; Comrie\n\t\t\t1985:94; Bybee, Perkins, and Pagliuca 1994: 244-245).\n\t\t\t(http://purl.org/linguistics/gold/ImmediateFuture)\n\t\t" ;
        <http://www.w3.org/2000/01/rdf-schema#subClassOf>
                <http://purl.org/olia/olia.owl#Future> ;
        <http://www.w3.org/2002/07/owl#versionInfo>
                "http://purl.org/linguistics/gold/ImmediateFuture" .

<http://purl.org/olia/olia.owl#Weak>
        a       <http://www.w3.org/2002/07/owl#Class> ;
        <http://www.w3.org/2000/01/rdf-schema#comment>
                "\n\t\t\tWeak pronouns are helping pronouns many languages have for easily \n\t\t\texplaining the possessive status of something, to which something \n\t\t\tbelongs. Many languages have different ways to express this. For \n\t\t\texample, English has distinctive words for all of these: \"my\", \"mine\". \n\t\t\tGermanic languages and Romance languages have the same, but inflect \n\t\t\tthem for gender: (Spanish example) \"mío\", \"mía\", \"míos\" and \"mías\" \n\t\t\t(\"mine\", in the masculine singular, feminine singular, masculine plural,\n\t\t\tand feminine plural form, respectively). \n\t\t\t(http://en.wikipedia.org/wiki/Weak_pronoun  20.11.06)\n\t\t" ;
        <http://www.w3.org/2000/01/rdf-schema#subClassOf>
                <http://purl.org/olia/olia-top.owl#StrengthFeature> ;
        <http://www.w3.org/2002/07/owl#versionInfo>
                "EAGLES" .

<http://purl.org/olia/olia.owl#QuestionPredicate>
        a       <http://www.w3.org/2002/07/owl#Class> ;
        <http://www.w3.org/2000/01/rdf-schema#comment>
                "SQ â ´ Inverted yes/no question, or main clause of a wh-question, following the wh-phrase in SBARQ. \n(Bies et al. 1995)\n\nSQ|That part of an SBARQ that excludes the wh-word or wh-phrase. See Section 5.32.\n(Santorini 1991)\n\nThe SBARQ label marks wh-questions (i.e., those that contain a gap and therefore require a trace). A further level of structure, SQ, contains the inverted auxiliary (if there is one) and the rest of the sentence. The inverted auxiliary in wh-questions is not labeled. ...\n\nSQ\n(See also section 1.2.7.) \nâ ¢\tinside SBARQ:\n\nAs described above, inside wh-questions, SQ holds the subject, inverted auxiliary (if any), main verb phrase, and some adjuncts.\nâ ¢\tyes/no questions: \n\nSQ is used for yes/no questions (i.e., those with inversion but no wh-movement). ...\n\nâ ¢\tsubject-less yes/no questions: \n\nIn questions where the auxiliary and subject do not appear, the auxiliary is unlabeled and a null subject (NP-SBJ *) is used. ...\n\nNote that questions with overt subjects and auxiliaries that show declarative word order are simply labeled S.\n\nâ ¢\tTag questions: \n\nTag questions are treated as an adjunction of SQ to S. The resulting structure is labeled SQ, since the whole thing is interrogative in nature. The lower SQ is annotated to show predicate deletion; that is, an appropriate null *?* is inserted. \n(Bies et al. 1995)" ;
        <http://www.w3.org/2000/01/rdf-schema#subClassOf>
                <http://purl.org/olia/olia.owl#Question> ;
        <http://www.w3.org/2002/07/owl#versionInfo>
                "Santorini 1991, Bies et al. 1995" .

<http://purl.org/olia/olia.owl#hasReferentType>
        a       <http://www.w3.org/2002/07/owl#ObjectProperty> ;
        <http://www.w3.org/2000/01/rdf-schema#range>
                <http://purl.org/olia/olia-top.owl#ReferentTypeFeature> ;
        <http://www.w3.org/2000/01/rdf-schema#subPropertyOf>
                <http://purl.org/olia/system.owl#hasFeature> ;
        <http://www.w3.org/2002/07/owl#versionInfo>
                "http://www.isocat.org/datcat/DC-1376 (referentType)" .

<http://purl.org/olia/olia.owl#hasEvidentiality>
        a       <http://www.w3.org/2002/07/owl#ObjectProperty> ;
        <http://www.w3.org/2000/01/rdf-schema#range>
                <http://purl.org/olia/olia-top.owl#EvidentialityFeature> ;
        <http://www.w3.org/2000/01/rdf-schema#subPropertyOf>
                <http://purl.org/olia/system.owl#hasFeature> .

<http://purl.org/olia/olia.owl#AspirationalVerb>
        a       <http://www.w3.org/2002/07/owl#Class> ;
        <http://www.w3.org/2000/01/rdf-schema#comment>
                "It is a verb, which indicates a strong desire to achieve something, without the doer.\n\t\t\t\n\t\t\tདག་པ ་ ང་ ་ ་བར་ ག།\n\t\t\tdag-pai zhing-lu kewa shÔ\n\t\t\t'May i be born in pure land'\n\t\t\t(http://panl10n.net/english/Outputs%20Phase%202/CCs/Bhutan/Papers/2007/0701/PartOfSpeech.pdf)" ;
        <http://www.w3.org/2000/01/rdf-schema#subClassOf>
                <http://purl.org/olia/olia.owl#MainVerb> ;
        <http://www.w3.org/2002/07/owl#versionInfo>
                "adopted from Dzongkha tagset (Chungku et al. 2010, http://purl.org/olia/dzongkha.owl#AspirationalVerb)" .

<http://purl.org/olia/olia.owl#DirectVoice>
        a       <http://www.w3.org/2002/07/owl#Class> ;
        <http://www.w3.org/2000/01/rdf-schema#comment>
                "\n\t\t\tSignals that the action proceeds in an ontologically salient way, \n\t\t\ti.e. that salience is assigned to nominals based on their referent's \n\t\t\trelative real-world capacities to control situations. (Klaiman 1991:32)\n\t\t\t(http://purl.org/linguistics/gold/DirectVoice)\n\t\t" ;
        <http://www.w3.org/2000/01/rdf-schema#subClassOf>
                <http://purl.org/olia/olia.owl#ActiveVoice> ;
        <http://www.w3.org/2002/07/owl#versionInfo>
                "http://purl.org/linguistics/gold/DirectVoice" .

<http://purl.org/olia/olia.owl#HaveAuxiliary>
        a       <http://www.w3.org/2002/07/owl#Class> ;
        <http://www.w3.org/2000/01/rdf-schema#comment>
                "\n                            The verb have as an auxiliary.\n                                (www.sil.org/linguistics/GlossaryOfLinguisticTerms/WhatIsAnAuxiliaryVerb.htm; http://www.isocat.org/datcat/DC-1299)\n                            " ;
        <http://www.w3.org/2000/01/rdf-schema#label>
                "have" ;
        <http://www.w3.org/2000/01/rdf-schema#subClassOf>
                <http://purl.org/olia/olia.owl#StrictAuxiliaryVerb> ;
        <http://www.w3.org/2002/07/owl#versionInfo>
                "subClassOf partOfSpeech (dcif:conceptualDomain)" , "http://www.isocat.org/datcat/DC-1299" .

<http://purl.org/olia/olia-top.owl#Constituent>
        a       <http://www.w3.org/2002/07/owl#Class> ;
        <http://www.w3.org/2000/01/rdf-schema#comment>
                "\n\t\t\tConstituents correspond to a GOLD SyntacticConstruction:\n\t\t\tSyntacticConstruction is the class of grammar units that \n\t\t\thave syntactic structure, i.e., consisting of more than \n\t\t\tone syntactic word or construction in a syntactic \n\t\t\tconfiguration. [Crystal 1980, 85-86]. \n\t\t\t(http://www.linguistics-ontology.org/gold/2008)\n\n\t\t\tCorresponds to units of annotation in the EAGLES recommendations for syntactic annotation\n\t\t\t(http://www.ilc.cnr.it/EAGLES96/segsasg1/node29.html#SECTION00052000000000000000)\n\t\t" ;
        <http://www.w3.org/2002/07/owl#versionInfo>
                "http://www.linguistics-ontology.org/gold/2008/SyntacticConstruction" .

<http://purl.org/olia/olia.owl#CloseAngleBracket>
        a       <http://www.w3.org/2002/07/owl#Class> ;
        <http://www.w3.org/2000/01/rdf-schema#comment>
                ">\n*RAB*\nRight angle bracket\n(Santorini 1991)" ;
        <http://www.w3.org/2000/01/rdf-schema#subClassOf>
                <http://purl.org/olia/olia.owl#RightParentheticalPunctuation> ;
        <http://www.w3.org/2002/07/owl#versionInfo>
                "PTB bracketing guidelines, Santorini 1991" .

<http://purl.org/olia/olia.owl#Modifier>
        a       <http://www.w3.org/2002/07/owl#Class> ;
        <http://www.w3.org/2000/01/rdf-schema#comment>
                "added in conformance with TIGER" ;
        <http://www.w3.org/2000/01/rdf-schema#subClassOf>
                <http://purl.org/olia/olia-top.owl#SyntacticRole> ;
        <http://www.w3.org/2002/07/owl#equivalentClass>
                <http://purl.org/olia/olia.owl#Modifier> , <http://purl.org/olia/olia.owl#SyntacticAdjunct> ;
        <http://www.w3.org/2002/07/owl#versionInfo>
                "added in conformance with TIGER, equivalent to SyntacticAdjunct, cf. definition by Dipper et al. (2007) there" .

<http://purl.org/olia/olia-top.owl#ValencyFeature>
        a       <http://www.w3.org/2002/07/owl#Class> ;
        <http://www.w3.org/2000/01/rdf-schema#comment>
                "ValencyFeature cannot be reflexive, because hasSyntacticValency is distinguished from hasSemanticValency" ;
        <http://www.w3.org/2000/01/rdf-schema#subClassOf>
                [ a       <http://www.w3.org/2002/07/owl#Restriction> ;
                  <http://www.w3.org/2002/07/owl#hasSelf>
                          true ;
                  <http://www.w3.org/2002/07/owl#onProperty>
                          <http://purl.org/olia/olia.owl#hasValency>
                ] .

<http://purl.org/olia/olia.owl#ArbitraryControl>
        a       <http://www.w3.org/2002/07/owl#Class> ;
        <http://www.w3.org/2000/01/rdf-schema#comment>
                "Indicates either the subject or object of the main clause may be the omitted argument of the subclause (http://www.lexinfo.net/ontology/2.0/lexinfo#ArbitraryControl)"@en ;
        <http://www.w3.org/2000/01/rdf-schema#subClassOf>
                <http://purl.org/olia/olia.owl#Control> ;
        <http://www.w3.org/2002/07/owl#versionInfo>
                "http://www.lexinfo.net/ontology/2.0/lexinfo#ArbitraryControl" .

<http://purl.org/olia/olia.owl#NonNegated>
        a       <http://www.w3.org/2002/07/owl#Class> ;
        <http://www.w3.org/2000/01/rdf-schema#comment>
                "Non-negated verbs carry no morphological marks of negation. In Resian, negative is always marked as 'no' except for two verbs: 'nïman' / not to have, 'nïsi' / not to be. In Slovak, verbs form negative by prefix 'ne-', with the exception of the verb \"byť\" (E. \"to be\") which forms the negative in indicative by using separate particle \"nie\", e.g. \"nie je\" (is not). Here, \"je\" would be marked as negative, despite having positive form. (MTE v4, http://purl.org/olia/mte/multext-east.owl#NonNegated)" ;
        <http://www.w3.org/2000/01/rdf-schema#subClassOf>
                <http://purl.org/olia/olia-top.owl#PolarityFeature> ;
        <http://www.w3.org/2002/07/owl#versionInfo>
                "http://purl.org/olia/mte/multext-east.owl#NonNegated" .

<http://purl.org/olia/olia.owl#hasGender>
        a       <http://www.w3.org/2002/07/owl#ObjectProperty> ;
        <http://www.w3.org/2000/01/rdf-schema#domain>
                [ a       <http://www.w3.org/2002/07/owl#Class> ;
                  <http://www.w3.org/2002/07/owl#unionOf>
                          ( <http://purl.org/olia/olia.owl#Noun> <http://purl.org/olia/olia.owl#Verb> <http://purl.org/olia/olia.owl#Adjective> <http://purl.org/olia/olia.owl#PronounOrDeterminer> <http://purl.org/olia/olia.owl#Article> <http://purl.org/olia/olia.owl#Numeral> <http://purl.org/olia/olia.owl#Residual> )
                ] ;
        <http://www.w3.org/2000/01/rdf-schema#range>
                <http://purl.org/olia/olia-top.owl#GenderFeature> ;
        <http://www.w3.org/2000/01/rdf-schema#subPropertyOf>
                <http://purl.org/olia/system.owl#hasFeature> .

<http://purl.org/olia/olia.owl#ProlativeCase>
        a       <http://www.w3.org/2002/07/owl#Class> ;
        <http://www.w3.org/2000/01/rdf-schema#comment>
                "\n\t\t\tCase for a noun or a pronoun that expresses motion within \n\t\t\ta place or a period of time needed for an event.\n\t\t\t(http://www.isocat.org/datcat/DC-1368)\n\t\t" ;
        <http://www.w3.org/2000/01/rdf-schema#subClassOf>
                <http://purl.org/olia/olia-top.owl#CaseFeature> ;
        <http://www.w3.org/2002/07/owl#versionInfo>
                "http://www.isocat.org/datcat/DC-1368" .

<http://purl.org/olia/olia.owl#DirectWHQuestion>
        a       <http://www.w3.org/2002/07/owl#Class> ;
        <http://www.w3.org/2000/01/rdf-schema#comment>
                "SBARQ|Direct question introduced by a wh-word or wh-phrase. See Section 5.32. Indirect questions\nand relative clauses should be bracketed as SBAR, not SBARQ.\n(Santorini 1991)\n\nWh-questions should be bracketed as SBARQ. The wh-constituent (whether it is a subject or not) is a\nchild of SBARQ; the rest of the question is an SQ. If the wh-constituent is a subject or an object, the\nposition where it is interpreted should be represented by the empty element T.\n(Santorini 1991)\n\nThe SBARQ label marks wh-questions (i.e., those that contain a gap and therefore require a trace). A further level of structure, SQ, contains the inverted auxiliary (if there is one) and the rest of the sentence. The inverted auxiliary in wh-questions is not labeled. ...\nSBARQ â ´ Direct question introduced by a wh-word or wh-phrase. See section 1 [Overview of Basic Clause Structure]. Indirect questions and relative clauses should be bracketed as SBAR, not SBARQ. \n(Bies et al. 1995)" ;
        <http://www.w3.org/2000/01/rdf-schema#subClassOf>
                <http://purl.org/olia/olia.owl#DirectQuestion> ;
        <http://www.w3.org/2002/07/owl#versionInfo>
                "Santorini 1991, Bies et al. 1995" .

<http://purl.org/olia/olia.owl#Letter>
        a       <http://www.w3.org/2002/07/owl#Class> ;
        <http://www.w3.org/2000/01/rdf-schema#comment>
                "\n                            Letter.\n                                (http://www.isocat.org/datcat/DC-1889)\n                            " ;
        <http://www.w3.org/2000/01/rdf-schema#label>
                "letter" ;
        <http://www.w3.org/2000/01/rdf-schema#subClassOf>
                <http://purl.org/olia/olia.owl#Character> ;
        <http://www.w3.org/2002/07/owl#versionInfo>
                "http://www.isocat.org/datcat/DC-1889" .

<http://purl.org/olia/olia.owl#FutureParticle>
        a       <http://www.w3.org/2002/07/owl#Class> ;
        <http://www.w3.org/2000/01/rdf-schema#comment>
                "\n                            Particle used in order to express future.\n                                (http://www.isocat.org/datcat/DC-1919)\n                            " ;
        <http://www.w3.org/2000/01/rdf-schema#label>
                "future particle" ;
        <http://www.w3.org/2000/01/rdf-schema#subClassOf>
                <http://purl.org/olia/olia.owl#TenseMarkingParticle> ;
        <http://www.w3.org/2002/07/owl#versionInfo>
                "http://www.isocat.org/datcat/DC-1919, taxonomic organization (under VerbalParticle) follows  http://purl.org/olia/mte/multext-east.owl#FutureParticle, regrouped under TenseMarkingParticle" , "subClassOf particle (dcif:isA)" .

<http://purl.org/olia/olia.owl#SubjunctiveModality>
        a       <http://www.w3.org/2002/07/owl#Class> ;
        <http://www.w3.org/2000/01/rdf-schema#comment>
                "\n\t\t\tThe subjunctive is the mood that is minimally marked as opposed to \n\t\t\tthe indicative and that marks a clause as not directly representing \n\t\t\tan assertion of the speaker. \n\t\t\t(http://www.uni-erfurt.de/sprachwissenschaft/proxy.php?port=8080&file=lido/servlet/Lido_Servlet Subjunktiv 18.06.07)\n\t\t" ;
        <http://www.w3.org/2000/01/rdf-schema#subClassOf>
                <http://purl.org/olia/olia-top.owl#ModalityFeature> ;
        <http://www.w3.org/2002/07/owl#versionInfo>
                "\n\t\t\thttp://purl.org/linguistics/gold/Subjunctive,\n\t\t\thttp://languagelink.let.uu.nl/tds/onto/LinguisticOntology.owl#subjunctiveModality\n\t\t" .

<http://purl.org/olia/olia.owl#Separable>
        a       <http://www.w3.org/2002/07/owl#Class> ;
        <http://www.w3.org/2000/01/rdf-schema#comment>
                "\n\t\t\tA separable verb is a verb that is composed of a verb stem and a separable \n\t\t\taffix. In some verb forms, the verb appears in one word, whilst in others \n\t\t\tthe verb stem and the affix are separated. German and Dutch are notable for \n\t\t\thaving many separable verbs. For example, the Dutch verb \"aankomen\" is a \n\t\t\tseparable verb. (http://en.wikipedia.org/wiki/Separable_verb  20.11.06)\n\t\t" ;
        <http://www.w3.org/2000/01/rdf-schema#subClassOf>
                <http://purl.org/olia/olia-top.owl#SeparabilityFeature> ;
        <http://www.w3.org/2002/07/owl#versionInfo>
                "EAGLES; note that UbyPos extends separability to particles" .

<http://purl.org/olia/olia.owl#Conjunct>
        a       <http://www.w3.org/2002/07/owl#Class> ;
        <http://www.w3.org/2000/01/rdf-schema#comment>
                "TIGER edge label CJ" ;
        <http://www.w3.org/2000/01/rdf-schema#subClassOf>
                <http://purl.org/olia/olia-top.owl#SyntacticRole> ;
        <http://www.w3.org/2002/07/owl#versionInfo>
                "TIGER edge label CJ" .

<http://purl.org/olia/olia.owl#TemporalisCase>
        a       <http://www.w3.org/2002/07/owl#Class> ;
        <http://www.w3.org/2000/01/rdf-schema#comment>
                "The so-called Temporalis Case is formed in Hungarian with -kor. Expresses a point of time or a period. (http://member.melbpc.org.au/~tmajlath/form-suffix.html)" ;
        <http://www.w3.org/2000/01/rdf-schema#subClassOf>
                <http://purl.org/olia/olia-top.owl#CaseFeature> ;
        <http://www.w3.org/2002/07/owl#versionInfo>
                "http://purl.org/olia/mte/multext-east.owl#TemporalisCase" .

<http://purl.org/olia/olia-top.owl#PhonologicalProcess>
        a       <http://www.w3.org/2002/07/owl#Class> .

<http://purl.org/olia/olia.owl#RhetoricalModifier>
        a       <http://www.w3.org/2002/07/owl#Class> ;
        <http://www.w3.org/2000/01/rdf-schema#comment>
                "added in conformance with TIGER" ;
        <http://www.w3.org/2000/01/rdf-schema#subClassOf>
                <http://purl.org/olia/olia.owl#Modifier> ;
        <http://www.w3.org/2002/07/owl#versionInfo>
                "added in conformance with TIGER" , "TODO: check definition" .

<http://purl.org/olia/olia.owl#UnitNoun>
        a       <http://www.w3.org/2002/07/owl#Class> ;
        <http://www.w3.org/2000/01/rdf-schema#comment>
                "Measuring units are frequently used with numerals. However, they have a different syntactic structure than\n\t\t\tnumerals (Sajjad 2007). \n\t\t\t\n\t\t\tIn European languages, Units are generally expressed as nouns, e.g., English \"ten/Numeral kilogram/Unit\".\n\t\t\t\"Kilogram\" can also be used as a common noun: \"The kilogram is losing weight\" (http://www.bbc.co.uk/news/science-environment-12276822)\n\t\t\t\n\t\t\tHassan Sajjad (2007), Urdu Part of Speech Tagset, version 1.0.0.0, 07-12-2007, Center for research in Urdu Language Processing. National University of Computer and Emerging Sciences, Lahore, Pakistan, http://www.crulp.org/Downloads/langproc/UrduPOStagger/UrduPOStagset.pdf\n\t\t" ;
        <http://www.w3.org/2000/01/rdf-schema#subClassOf>
                <http://purl.org/olia/olia.owl#CommonNoun> ;
        <http://www.w3.org/2002/07/owl#versionInfo>
                "adopted from Sajjad (2007), http://purl.org/olia/urdu.owl#MeasuringUnit, TOCHECK: are units in Urdu Nouns ?" .

<http://purl.org/olia/olia.owl#MeasureArgument>
        a       <http://www.w3.org/2002/07/owl#Class> ;
        <http://www.w3.org/2000/01/rdf-schema#comment>
                "added in conformance with TIGER" ;
        <http://www.w3.org/2000/01/rdf-schema#subClassOf>
                <http://purl.org/olia/olia.owl#AdnominalConstituent> ;
        <http://www.w3.org/2002/07/owl#versionInfo>
                "TODO: check definition" , "added in conformance with TIGER" .

<http://purl.org/olia/olia.owl#PositionerRole>
        a       <http://www.w3.org/2002/07/owl#Class> ;
        <http://www.w3.org/2000/01/rdf-schema#comment>
                "\n\t\t\tThe entity controlling a Position (Dik, 1997:118)\n\t\t\t(http://languagelink.let.uu.nl/tds/onto/LinguisticOntology.owl#positionerRole)\n\t\t" ;
        <http://www.w3.org/2000/01/rdf-schema#subClassOf>
                <http://purl.org/olia/olia.owl#ActorMacroRole> ;
        <http://www.w3.org/2002/07/owl#versionInfo>
                "\n\t\t\thttp://languagelink.let.uu.nl/tds/onto/LinguisticOntology.owl#positionerRole\n\t\t" .

<http://purl.org/olia/olia.owl#ReciprocalMiddle>
        a       <http://www.w3.org/2002/07/owl#Class> ;
        <http://www.w3.org/2000/01/rdf-schema#comment>
                "\n\t\t\tReferents of plural subject do action to one another. (Siewierska 1988:257)\n\t\t\t(http://purl.org/linguistics/gold/ReciprocalMiddle)\n\t\t" ;
        <http://www.w3.org/2000/01/rdf-schema#subClassOf>
                <http://purl.org/olia/olia.owl#MiddleVoice> ;
        <http://www.w3.org/2002/07/owl#versionInfo>
                "\n\t\t\thttp://purl.org/linguistics/gold/ReciprocalMiddle\n\t\t" .

<http://purl.org/olia/olia.owl#NamedEntity>
        a       <http://www.w3.org/2002/07/owl#Class> ;
        <http://www.w3.org/2000/01/rdf-schema#comment>
                "\n                            segment of text for which one or many rigid designators stands for the referent\n                                (Gil Francopoulo; http://www.isocat.org/datcat/DC-2275)\n                            " ;
        <http://www.w3.org/2000/01/rdf-schema#label>
                "named entity" ;
        <http://www.w3.org/2000/01/rdf-schema#subClassOf>
                <http://purl.org/olia/olia-top.owl#DiscourseEntity> ;
        <http://www.w3.org/2002/07/owl#versionInfo>
                "http://www.isocat.org/datcat/DC-2275" .

<http://purl.org/olia/olia.owl#AdjectivalParticle>
        a       <http://www.w3.org/2002/07/owl#Class> ;
        <http://www.w3.org/2000/01/rdf-schema#comment>
                "Particle that serves to form adjective phrases, e.g., Urdu sā (http://purl.org/olia/emille.owl#AdjectivalParticle)" ;
        <http://www.w3.org/2000/01/rdf-schema#subClassOf>
                <http://purl.org/olia/olia.owl#Particle> ;
        <http://www.w3.org/2002/07/owl#versionInfo>
                "adopted from the EMILLE Urdu tagset (Hardie 2003, http://purl.org/olia/emille.owl#AdjectivalParticle)" .

<http://purl.org/olia/olia.owl#ExtentRole>
        a       <http://www.w3.org/2002/07/owl#Class> ;
        <http://www.w3.org/2000/01/rdf-schema#comment>
                "-EXT (extent)\nâ ´ marks adverbial phrases that describe the spatial extent of an activity. -EXT was incorporated primarily for cases of movement in financial space, but is also used in analogous situations elsewhere. \n\n  (S (NP-SBJ the Dow Jones Industrial Average)\n     (VP plunged\n         (NP-EXT 190.58 points)))\n\n\n  (S (NP-SBJ She)\n     (VP walked\n         (NP-EXT 5 miles)))\n\nObligatory complements do not receive -EXT: \n\n  (S (NP-SBJ The sumo wrestler)\n     (VP gained\n         (NP 80 pounds)))\n\nWords such as fully and completely are absolutes and do not receive -EXT.\n(Bies et al. 1995)" ;
        <http://www.w3.org/2000/01/rdf-schema#subClassOf>
                <http://purl.org/olia/olia-top.owl#SemanticRole> ;
        <http://www.w3.org/2002/07/owl#versionInfo>
                "added in conformance with PTB bracketing guidelines, Bies et al. (1995)" .

<http://purl.org/olia/olia.owl#PastPerfectTense>
        a       <http://www.w3.org/2002/07/owl#Class> ;
        <http://www.w3.org/2000/01/rdf-schema#comment>
                "\n                            denoting a tense of verbs used in relating past events where the action had already occurred at the time of the action of a main verb that is itself in a past tense. In English this is a compound tense formed with had plus the past participle\n                                (www.wordreference.com/English/definition.asp?en=past+perfect; http://www.isocat.org/datcat/DC-1348)\n                            " , "\n                            Past perfect tense is an absolute-relative tense that refers to a time in the past relative to a reference point, which itself is in the past relative to the moment of utterance\n                                (www.sil.org/linguistics/GlossaryOfLinguisticTerms/WhatIsPastPerfectTense.htm; http://www.isocat.org/datcat/DC-1348)\n                            " ;
        <http://www.w3.org/2000/01/rdf-schema#label>
                "Past perfect" ;
        <http://www.w3.org/2000/01/rdf-schema#subClassOf>
                <http://purl.org/olia/olia.owl#AbsoluteRelativeTense> ;
        <http://www.w3.org/2002/07/owl#versionInfo>
                "http://www.isocat.org/datcat/DC-1348" .

<http://purl.org/olia/olia.owl#PhysicalAbilitiveModality>
        a       <http://www.w3.org/2002/07/owl#Class> ;
        <http://www.w3.org/2000/01/rdf-schema#comment>
                "PhysicalAbilitiveModality indicates that an\n                        agent has the physical capacity to perform some action. [Bybee, Perkins and\n                        Pagliuca 1994: 192; Palmer 2001: 77]" ;
        <http://www.w3.org/2000/01/rdf-schema#isDefinedBy>
                "http://www.isocat.org/datcat/DC-3394" ;
        <http://www.w3.org/2000/01/rdf-schema#subClassOf>
                <http://purl.org/olia/olia.owl#AbilitativeModality> .

<http://purl.org/olia/olia.owl#InterlativeCase>
        a       <http://www.w3.org/2002/07/owl#Class> ;
        <http://www.w3.org/2000/01/rdf-schema#comment>
                "\n\t\t\tInterlativeCase expresses that  the referent of the noun it marks \n\t\t\tis the location between which another referent is moving. It has \n\t\t\tthe meaning 'to the middle of'.\n\t\t\t(http://purl.org/linguistics/gold/Interlative)\n\t\t" ;
        <http://www.w3.org/2000/01/rdf-schema#subClassOf>
                <http://purl.org/olia/olia-top.owl#CaseFeature> ;
        <http://www.w3.org/2002/07/owl#versionInfo>
                "http://purl.org/linguistics/gold/Interlative" .

<http://purl.org/olia/olia.owl#PrepositionalCase>
        a       <http://www.w3.org/2002/07/owl#Class> ;
        <http://www.w3.org/2000/01/rdf-schema#comment>
                "\n\t\t\tIn many grammars, the term \"prepositional case\" is to refer to case marking that only occurs in \n\t\t\tcombination with prepositions. Normally, this is an oblique case, e.g., the Russian 6th case,\n\t\t\talso referred to as \"locative\". (Ch. Chiarcos)\n\t\t" ;
        <http://www.w3.org/2000/01/rdf-schema#subClassOf>
                <http://purl.org/olia/olia-top.owl#CaseFeature> ;
        <http://www.w3.org/2002/07/owl#versionInfo>
                "\n\t\t\tPrepositional case is an in EAGLES optional value of CaseFeature for Spanish pronouns and determiners.\n\t\t\t(http://www.ilc.cnr.it/EAGLES96/annotate/node19.html#oav2v  15.11.06)\n\t\t" .

<http://purl.org/olia/system.owl#UnitOfAnnotation>
        a       <http://www.w3.org/2002/07/owl#Class> .

<http://purl.org/olia/olia.owl#EchoWord>
        a       <http://www.w3.org/2002/07/owl#Class> ;
        <http://www.w3.org/2000/01/rdf-schema#comment>
                "The word is a copy of a previous word. In Hindi, this would add the meaning of distribution (\"one rupee each\"), separation (\"sit separately\"), variety, diversity or just emphasis. (http://www.isocat.org/datcat/DC-4209, reduplicative)\n\t  \n\t\t\tEcho word is a linguistic term that refers to a particular kind of reduplication which is a widespread areal feature in the languages of South Asia. Echo words are characterized by reduplication of a complete word or phrase, with the initial segment or syllable of the reduplicant being overwritten by a fixed segment or syllable. In most languages in which this phenomenon is present, echo words serve to express a meaning of \"... and such; and things like that.\" In some cases the echo word may express a depreciative meaning as well.\n\t\t\t\n\t\t\tEcho words in Hindi are typically created with a fixed initial v:\n\t\t\taam \t\"mango\"\n\t\t\taam vaam \t\"mangoes and the like\"\n\t\t\ttras \t\"grief\"\n\t\t\ttras vras \t\"grief and the like\"\n\t\t\t(http://en.wikipedia.org/wiki/Echo_word)\n\t\t\t" ;
        <http://www.w3.org/2000/01/rdf-schema#isDefinedBy>
                "http://www.isocat.org/datcat/DC-4209" ;
        <http://www.w3.org/2000/01/rdf-schema#label>
                "reduplicative" , "echo word" ;
        <http://www.w3.org/2000/01/rdf-schema#subClassOf>
                <http://purl.org/olia/olia.owl#Reduplication> , <http://purl.org/olia/olia-top.owl#Word> ;
        <http://www.w3.org/2002/07/owl#versionInfo>
                "adopted from Ancorra for Indian languages, http://purl.org/olia/ancorra.owl#EchoWord" .

<http://purl.org/olia/olia.owl#FocusMarker>
        a       <http://www.w3.org/2002/07/owl#Class> ;
        <http://www.w3.org/2000/01/rdf-schema#comment>
                "a morpheme indicating that the element it marks is the focus of the utterance." ;
        <http://www.w3.org/2000/01/rdf-schema#isDefinedBy>
                "http://www.isocat.org/datcat/DC-4196" ;
        <http://www.w3.org/2000/01/rdf-schema#subClassOf>
                <http://purl.org/olia/olia.owl#Morpheme> ;
        <http://www.w3.org/2002/07/owl#versionInfo>
                "In compliance with ISOcat, this is defined here as a morpheme. However, focus markers can be independent words, as well." .

<http://purl.org/olia/olia.owl#Correlative>
        a       <http://www.w3.org/2002/07/owl#Class> ;
        <http://www.w3.org/2000/01/rdf-schema#comment>
                "\n\t\tWhen the same word is also placed before the first conjunct, as in French \n\t\t\"ou...ou...\", the former occurrence is given the Correlative value and the\n\t\tlatter the Simple value. \n\t\t(http://www.ilc.cnr.it/EAGLES96/annotate/node18.html#oav1av  17.11.06)\n\t\t" ;
        <http://www.w3.org/2000/01/rdf-schema#subClassOf>
                <http://purl.org/olia/olia-top.owl#CoordTypeFeature> ;
        <http://www.w3.org/2002/07/owl#deprecated>
                true ;
        <http://www.w3.org/2002/07/owl#versionInfo>
                "from EAGLES, reimplemented as subhierarchy of CoordinatingConjunction" .

<http://purl.org/olia/olia.owl#CauseRole>
        a       <http://www.w3.org/2002/07/owl#Class> ;
        <http://www.w3.org/2000/01/rdf-schema#comment>
                "Cause indicates the reason why something happens and is often expressed by a\n\t\t\tPP (because of, with, through etc.). Sometimes this role is close to the role of\n\t\t\tInstrument. The criterion for the choice of tag CAUSE is if the expression can\n\t\t\tbe paraphrased through a clausal subordinate clause.\n\t\t\t(Dipper et al. 2007, 5.3.10)" ;
        <http://www.w3.org/2000/01/rdf-schema#subClassOf>
                <http://purl.org/olia/olia-top.owl#SemanticRole> ;
        <http://www.w3.org/2002/07/owl#versionInfo>
                "added in conformance with the SFB632 Annotation Guidelines (Dipper et al. 2007)" .

<http://purl.org/olia/olia.owl#Uncountable>
        a       <http://www.w3.org/2002/07/owl#Class> ;
        <http://www.w3.org/2000/01/rdf-schema#comment>
                "\n\t\t\tA mass noun (also uncountable noun or non-count noun) can't be modified by a numeral, \n\t\t\toccur in singular/plural or co-occur with the relevant kind of determiner.\n\t\t\t(http://en.wikipedia.org/wiki/Mass_noun 19.09.06)\n\t\t" ;
        <http://www.w3.org/2000/01/rdf-schema#subClassOf>
                <http://purl.org/olia/olia-top.owl#CountabilityFeature> ;
        <http://www.w3.org/2002/07/owl#versionInfo>
                "EAGLES, remodelling of MassNoun vs. CommonNoun" .

<http://purl.org/olia/olia.owl#IntransitiveSubject>
        a       <http://www.w3.org/2002/07/owl#Class> ;
        <http://www.w3.org/2000/01/rdf-schema#comment>
                "\n\t\t\tIntransitive argument (S), single argument of an intransitive verb or \n\t\t\tonly argument in a one-place predicate (frame). \n\t\t\t(http://languagelink.let.uu.nl/tds/onto/LinguisticOntology.owl#S)\n\t\t" ;
        <http://www.w3.org/2000/01/rdf-schema#subClassOf>
                <http://purl.org/olia/olia.owl#SyntacticSubject> ;
        <http://www.w3.org/2002/07/owl#versionInfo>
                "http://languagelink.let.uu.nl/tds/onto/LinguisticOntology.owl#S" .

<http://purl.org/olia/olia.owl#CaseMarker>
        a       <http://www.w3.org/2002/07/owl#Class> ;
        <http://www.w3.org/2000/01/rdf-schema#subClassOf>
                <http://purl.org/olia/olia.owl#Unique> ;
        <http://www.w3.org/2000/01/rdf-schema#subClassOf>
                [ a       <http://www.w3.org/2002/07/owl#Class> ;
                  <http://www.w3.org/2002/07/owl#unionOf>
                          ( <http://purl.org/olia/olia.owl#MorphologicalParticle> <http://purl.org/olia/olia.owl#Adposition> )
                ] ;
        <http://www.w3.org/2002/07/owl#versionInfo>
                "adopted from Dzongkha tagset (Chungku et al. 2010). If its tradition of grammar description is influenced by the Indian, these case markers are variously described as case morphemes or as postpositions. Therefore introduced as a shorthand for Adposition or MorphologicalParticle" .

<http://purl.org/olia/olia.owl#ZeroPronoun>
        a       <http://www.w3.org/2002/07/owl#Class> ;
        <http://www.w3.org/2000/01/rdf-schema#comment>
                "*|An asterisk represents a zero pronoun; it may need to be deleted. ...\n* is used to represent the empty subject of gerunds, imperatives and to-infinitive clauses. \n(Santorini 1991)\n\n(NP *) â ´ arbitrary PRO, controlled PRO, and trace of A-movement \n(Bies et al. 1995)" ;
        <http://www.w3.org/2000/01/rdf-schema#subClassOf>
                <http://purl.org/olia/olia-top.owl#NullElement> , <http://purl.org/olia/olia.owl#PersonalPronoun> ;
        <http://www.w3.org/2002/07/owl#versionInfo>
                "PTB bracketing guidelines, Santorini 1991, Bies et al. 1995; \n\t\t\toften considered as extremely weak form of personal pronouns (Ariel 1990; Givón 1995)\n\t\t" .

<http://purl.org/olia/olia.owl#MassNoun>
        a       <http://www.w3.org/2002/07/owl#Class> ;
        <http://www.w3.org/2000/01/rdf-schema#comment>
                "\n\t\tA mass noun (also uncountable noun or non-count noun) can't be modified by a numeral, \n\t\toccur in singular/plural or co-occur with the relevant kind of determiner.\n\t\t(http://en.wikipedia.org/wiki/Mass_noun 19.09.06)\n\t" ;
        <http://www.w3.org/2000/01/rdf-schema#subClassOf>
                [ a       <http://www.w3.org/2002/07/owl#Class> ;
                  <http://www.w3.org/2002/07/owl#intersectionOf>
                          ( [ a       <http://www.w3.org/2002/07/owl#Restriction> ;
                              <http://www.w3.org/2002/07/owl#onProperty>
                                      <http://purl.org/olia/olia.owl#hasCountability> ;
                              <http://www.w3.org/2002/07/owl#someValuesFrom>
                                      <http://purl.org/olia/olia.owl#Uncountable>
                            ]
                            <http://purl.org/olia/olia.owl#Noun>
                          )
                ] ;
        <http://www.w3.org/2002/07/owl#versionInfo>
                "\n\t\tEAGLES Noun with Countability=\"Mass\".\n\t" .

<http://purl.org/olia/olia-top.owl#TenseFeature>
        a       <http://www.w3.org/2002/07/owl#Class> ;
        <http://www.w3.org/2000/01/rdf-schema#subClassOf>
                [ a       <http://www.w3.org/2002/07/owl#Restriction> ;
                  <http://www.w3.org/2002/07/owl#hasSelf>
                          true ;
                  <http://www.w3.org/2002/07/owl#onProperty>
                          <http://purl.org/olia/olia.owl#hasTense>
                ] ;
        <http://www.w3.org/2002/07/owl#versionInfo>
                "\n\t\t\tSubclassification in absolute, relaive and absolute-relative adopted from TDS.\n\t\t\tHabitual is modelled here as Aspect, in accordance with GOLD, replaced here by\n\t\t\tNotTemporallyAnchored.\n\t\t\tSkipped TDS non-presentTense (= complement of Present), \n\t\t\thttp://purl.org/linguistics/gold/NonFuture,\n\t\t\thttp://purl.org/linguistics/gold/NonPast,\n\t\t\tredefined Future and Past as superconcepts to cover different future and past tenses\n\t\t" .

<http://purl.org/olia/olia.owl#TargetRole>
        a       <http://www.w3.org/2002/07/owl#Class> ;
        <http://www.w3.org/2000/01/rdf-schema#comment>
                "\n\t\tThe target role instantiates the destination of an event or entity.\n\t\t" ;
        <http://www.w3.org/2000/01/rdf-schema#subClassOf>
                <http://purl.org/olia/olia.owl#DirectionRole> ;
        <http://www.w3.org/2002/07/owl#versionInfo>
                "added as counterpart of SourceRole, see there" .

<http://purl.org/olia/olia.owl#TemporallyDefinedUsage>
        a       <http://www.w3.org/2002/07/owl#Class> ;
        <http://www.w3.org/2000/01/rdf-schema#comment>
                "Indication specifying whether the usage is old or modern." ;
        <http://www.w3.org/2000/01/rdf-schema#isDefinedBy>
                "http://www.isocat.org/datcat/DC-1959" ;
        <http://www.w3.org/2000/01/rdf-schema#label>
                "dating" ;
        <http://www.w3.org/2000/01/rdf-schema#subClassOf>
                <http://purl.org/olia/olia.owl#Possible> .

<http://purl.org/olia/olia.owl#DebitiveMood>
        a       <http://www.w3.org/2002/07/owl#Class> ;
        <http://www.w3.org/2000/01/rdf-schema#comment>
                "Mood to express necessity or requirement" ;
        <http://www.w3.org/2000/01/rdf-schema#isDefinedBy>
                "http://www.isocat.org/datcat/DC-3835" ;
        <http://www.w3.org/2000/01/rdf-schema#subClassOf>
                <http://purl.org/olia/olia-top.owl#MoodFeature> , <http://purl.org/olia/olia.owl#DebitiveModality> .

<http://purl.org/olia/olia.owl#CliticSpecificArticle>
        a       <http://www.w3.org/2002/07/owl#Class> ;
        <http://www.w3.org/2000/01/rdf-schema#comment>
                "\n\t\t\tPersian does have an article, but it marks specificity rather than definiteness. The Persian article is similar to the Balkan one (a clitic of pronominal origin that's written together with the word), except that it isn't exactly definite (you can even see it described as an indefinite article).\n\t\t\t(Ivan A. Derzhanski, p.c. 2010/06/18)\n\t\t" ;
        <http://www.w3.org/2000/01/rdf-schema#label>
                "clitic specific determiner" , "clitic specific article" ;
        <http://www.w3.org/2000/01/rdf-schema#subClassOf>
                <http://purl.org/olia/olia.owl#CliticElement> , <http://purl.org/olia/olia.owl#SpecificArticle> ;
        <http://www.w3.org/2002/07/owl#versionInfo>
                "http://purl.org/olia/mte/multext-east.owl#CliticSpecificDeterminer" .

<http://purl.org/olia/olia.owl#Supine>
        a       <http://www.w3.org/2002/07/owl#Class> ;
        <http://www.w3.org/2000/01/rdf-schema#comment>
                "\n\t\tSupine is a nonfinite form of motion verbs with functions similar to that of an infinitive (Angelika Adams)" ;
        <http://www.w3.org/2000/01/rdf-schema#subClassOf>
                <http://purl.org/olia/olia.owl#Converb> ;
        <http://www.w3.org/2002/07/owl#versionInfo>
                "EAGLES NonFiniteVerb with VerbForm=\"Supine\"." .

<http://purl.org/olia/olia.owl#IterativeAspect>
        a       <http://www.w3.org/2002/07/owl#Class> ;
        <http://www.w3.org/2000/01/rdf-schema#comment>
                "\n\t\t\tIterativeAspect, also called repetitives, encodes a number of events \n\t\t\tof the same type that are repeated on a particular occasion. The time\n\t\t\tinterval which is relevant to the iterative is relatively shorter than \n\t\t\tin the case of the habitual (Bybee 1985: 150; Bybee, Perkins and Pagliuca \n\t\t\t1994: 127). Portrays events repeated on the same occasion (like the \n\t\t\titerative knocking on the door) (Bhat 1999: 53)\n\t\t\t(http://purl.org/linguistics/gold/Iterative)\n\t\t" ;
        <http://www.w3.org/2000/01/rdf-schema#subClassOf>
                <http://purl.org/olia/olia-top.owl#AspectFeature> ;
        <http://www.w3.org/2002/07/owl#versionInfo>
                "\n\t\t\thttp://purl.org/linguistics/gold/Iterative\n\t\t" .

<http://purl.org/olia/olia.owl#DeficientVerb>
        a       <http://www.w3.org/2002/07/owl#Class> ;
        <http://www.w3.org/2000/01/rdf-schema#comment>
                "verb lacking certain morphosyntactic properties" ;
        <http://www.w3.org/2000/01/rdf-schema#isDefinedBy>
                "http://www.isocat.org/datcat/DC-3007" ;
        <http://www.w3.org/2000/01/rdf-schema#subClassOf>
                <http://purl.org/olia/olia.owl#Verb> ;
        <http://www.w3.org/2002/07/owl#deprecated>
                true ;
        <http://www.w3.org/2002/07/owl#versionInfo>
                "This is an ill-defined concept originating from ISOcat. It is however, not possible to circumscribe it in OLiA as it lacks an established concept of deficiency. Despite the unsatisfactory definition, this was thus adopted in OLiA for compatibility with ISOcat, but marked as deprecated." .

<http://purl.org/olia/olia.owl#AditiveCase>
        a       <http://www.w3.org/2002/07/owl#Class> ;
        <http://www.w3.org/2000/01/rdf-schema#comment>
                "Case expressing \"to\" in Basque studies. (http://www.isocat.org/datcat/DC-1229)"@en ;
        <http://www.w3.org/2000/01/rdf-schema#label>
                "aditive case"@en ;
        <http://www.w3.org/2000/01/rdf-schema#subClassOf>
                <http://purl.org/olia/olia-top.owl#CaseFeature> ;
        <http://www.w3.org/2002/07/owl#versionInfo>
                "http://www.isocat.org/datcat/DC-1229" , "TODO: rename to AdditiveCase" .

<http://purl.org/olia/olia.owl#TenseMarkingParticle>
        a       <http://www.w3.org/2002/07/owl#Class> ;
        <http://www.w3.org/2000/01/rdf-schema#comment>
                "Dzongkha has also a tense marker, which is not complicated like in other languages. It has got only six tense markers and can be used in a very simple and effective way. They are: ('Ni'+'Wong') for future, ('D'o'+'D'ä') for present and ('Ci'+'Yi') for past tense.\n\t\t\t\n\t\t\tང་ ནངས་པ་ འ ་ །\n\t\t\tNga naba jo-ni[past tense]\n\t\t\tI tomorrow go-will-[past]\n\t\t\t'I am going tomorrow'\n\t\t\t(http://panl10n.net/english/Outputs%20Phase%202/CCs/Bhutan/Papers/2007/0701/PartOfSpeech.pdf)" ;
        <http://www.w3.org/2000/01/rdf-schema#subClassOf>
                <http://purl.org/olia/olia.owl#VerbalParticle> ;
        <http://www.w3.org/2002/07/owl#versionInfo>
                "adopted from Dzongkha tagset (Chungku et al. 2010, http://purl.org/olia/dzongkha.owl#TenseMarker)" .

<http://purl.org/olia/olia.owl#SubordinatingConjunctionWithoutNegation>
        a       <http://www.w3.org/2002/07/owl#Class> ;
        <http://www.w3.org/2000/01/rdf-schema#comment>
                "Conjunction/Sub_Type=\"negative\" (Romanian, Serbian, Russian)\n\t\t\tIn Romanian, each conjunction requires another mood, so that the diversity may be controlled by subcategorisation rules. The attribute Sub_Type distinguishes among the positive and negative conjunctions, providing means to control verbal double negation, (as in case of the negative pronouns, determiners and adverbs): nici NU am venit, nimeni NU vorbeşte, nici_un tren N-a trecut, nicăieri N-am văzut (MTE v4, http://purl.org/olia/mte/multext-east.owl#PositiveSubordinatingConjunction)" ;
        <http://www.w3.org/2000/01/rdf-schema#subClassOf>
                <http://purl.org/olia/olia.owl#SubordinatingConjunction> ;
        <http://www.w3.org/2002/07/owl#versionInfo>
                "http://purl.org/olia/mte/multext-east.owl#PositiveSubordinatingConjunction" .

<http://purl.org/olia/olia.owl#AllativeCase>
        a       <http://www.w3.org/2002/07/owl#Class> ;
        <http://www.w3.org/2000/01/rdf-schema#comment>
                "\n\t\t\tAllativeCase expresses motion to or toward the referent of the noun \n\t\t\tit marks (Pei and Gaynor 1954: 6,9,216; Lyons 1968: 299; Crystal 1985: \n\t\t\t1213; Gove, et al. 1966: 55,2359).\n\t\t\t(http://purl.org/linguistics/gold/Allative)\n\t\t" ;
        <http://www.w3.org/2000/01/rdf-schema#subClassOf>
                <http://purl.org/olia/olia-top.owl#CaseFeature> ;
        <http://www.w3.org/2002/07/owl#versionInfo>
                "http://purl.org/linguistics/gold/Allative; http://www.isocat.org/datcat/DC-1236" .

<http://purl.org/olia/olia.owl#GeographicalVariant>
        a       <http://www.w3.org/2002/07/owl#Class> ;
        <http://www.w3.org/2000/01/rdf-schema#comment>
                "\n                            Description of a specific form used in a certain region as opposed to another form used in another region\n                                (http://www.isocat.org/datcat/DC-1851)\n                            " ;
        <http://www.w3.org/2000/01/rdf-schema#label>
                "geographical variant" ;
        <http://www.w3.org/2000/01/rdf-schema#subClassOf>
                <http://purl.org/olia/olia.owl#Possible> ;
        <http://www.w3.org/2002/07/owl#versionInfo>
                "http://www.isocat.org/datcat/DC-1851" .

<http://purl.org/olia/olia.owl#MannerNoun>
        a       <http://www.w3.org/2002/07/owl#Class> ;
        <http://www.w3.org/2000/01/rdf-schema#comment>
                "noun expressing a manner" ;
        <http://www.w3.org/2000/01/rdf-schema#isDefinedBy>
                "http://www.isocat.org/datcat/DC-3854" ;
        <http://www.w3.org/2000/01/rdf-schema#label>
                "manner noun" ;
        <http://www.w3.org/2002/07/owl#deprecated>
                true ;
        <http://www.w3.org/2002/07/owl#equivalentClass>
                [ a       <http://www.w3.org/2002/07/owl#Class> ;
                  <http://www.w3.org/2002/07/owl#intersectionOf>
                          ( <http://purl.org/olia/olia.owl#CommonNoun>
                            [ a       <http://www.w3.org/2002/07/owl#Restriction> ;
                              <http://www.w3.org/2002/07/owl#onProperty>
                                      <http://purl.org/olia/olia.owl#hasSemanticRole> ;
                              <http://www.w3.org/2002/07/owl#someValuesFrom>
                                      <http://purl.org/olia/olia.owl#MannerRole>
                            ]
                          )
                ] ;
        <http://www.w3.org/2002/07/owl#versionInfo>
                "deprecated, as merely a shorthand for CommonNoun and hasSemanticRole some MannerRole" .

<http://purl.org/olia/olia.owl#InstrumentNoun>
        a       <http://www.w3.org/2002/07/owl#Class> ;
        <http://www.w3.org/2000/01/rdf-schema#comment>
                "noun expressing an instrument of the action" ;
        <http://www.w3.org/2000/01/rdf-schema#isDefinedBy>
                "http://www.isocat.org/datcat/DC-3856" ;
        <http://www.w3.org/2002/07/owl#deprecated>
                true ;
        <http://www.w3.org/2002/07/owl#equivalentClass>
                [ a       <http://www.w3.org/2002/07/owl#Class> ;
                  <http://www.w3.org/2002/07/owl#intersectionOf>
                          ( <http://purl.org/olia/olia.owl#Noun>
                            [ a       <http://www.w3.org/2002/07/owl#Restriction> ;
                              <http://www.w3.org/2002/07/owl#onProperty>
                                      <http://purl.org/olia/olia.owl#hasSemanticRole> ;
                              <http://www.w3.org/2002/07/owl#someValuesFrom>
                                      <http://purl.org/olia/olia.owl#InstrumentRole>
                            ]
                          )
                ] ;
        <http://www.w3.org/2002/07/owl#versionInfo>
                "deprecated, as merely a shorthand for Noun and hasSemanticRole some InstrumentRole" .

<http://purl.org/olia/olia.owl#CountableNoun>
        a       <http://www.w3.org/2002/07/owl#Class> ;
        <http://www.w3.org/2000/01/rdf-schema#comment>
                "\n\t\tA countable noun (also count noun) is a noun which can be modified by a numeral \n\t\tand occur in both singular and plural form, as well as co-occurring with \n\t\tquantificational determiners like every, each, several, most, etc..\n\t\t(http://en.wikipedia.org/wiki/Countable_noun 19.09.06)\n\t" ;
        <http://www.w3.org/2000/01/rdf-schema#subClassOf>
                [ a       <http://www.w3.org/2002/07/owl#Class> ;
                  <http://www.w3.org/2002/07/owl#intersectionOf>
                          ( <http://purl.org/olia/olia.owl#Noun>
                            [ a       <http://www.w3.org/2002/07/owl#Restriction> ;
                              <http://www.w3.org/2002/07/owl#onProperty>
                                      <http://purl.org/olia/olia.owl#hasCountability> ;
                              <http://www.w3.org/2002/07/owl#someValuesFrom>
                                      <http://purl.org/olia/olia.owl#Countable>
                            ]
                          )
                ] ;
        <http://www.w3.org/2002/07/owl#versionInfo>
                "\n\t\tEAGLES Noun with Countability=\"Countable\".\n\t" .

<http://purl.org/olia/olia.owl#ImpersonalPassive>
        a       <http://www.w3.org/2002/07/owl#Class> ;
        <http://www.w3.org/2000/01/rdf-schema#comment>
                "\n\t\t\tA Passive that alters the mapping of a nominal to the Subject \n\t\t\trelation in a basic intransitive structure (Klaiman 1991:23)\n\t\t\t(http://purl.org/linguistics/gold/ImpersonalPassive)\n\t\t" ;
        <http://www.w3.org/2000/01/rdf-schema#subClassOf>
                <http://purl.org/olia/olia.owl#PassiveVoice> ;
        <http://www.w3.org/2002/07/owl#versionInfo>
                "http://purl.org/linguistics/gold/ImpersonalPassive" .

<http://purl.org/olia/olia.owl#DiscourseMarker>
        a       <http://www.w3.org/2002/07/owl#Class> ;
        <http://www.w3.org/2000/01/rdf-schema#comment>
                "\n\t\tGenerally, discourse markers are expressions or phrases of greeting, apologizing, thanking,\n\t\tshort emotional utterances, and interjections. Their node label is DM. ... Typical discourse markers are:\n\t\tja, nein, hallo, oh, aha, pst, nunja, gewiß, toll, nun ja, etc.\n\t\t(Telljohann et al. 2009, p. 136)\n\t\t" ;
        <http://www.w3.org/2000/01/rdf-schema#subClassOf>
                <http://purl.org/olia/olia.owl#Unique> ;
        <http://www.w3.org/2002/07/owl#versionInfo>
                "Introduced in accordance with the TIGER and TüBa-D/Z annotation schemes (syntactic edge label)" .

<http://purl.org/olia/olia.owl#ImperativeMood>
        a       <http://www.w3.org/2002/07/owl#Class> ;
        <http://www.w3.org/2000/01/rdf-schema#comment>
                "\n\t\t\tPertaining to the mood or mode of a verb form or clause such that it \n\t\t\tpredicates a command, request, or exhortation (OED).\n\t\t\t(http://languagelink.let.uu.nl/tds/onto/LinguisticOntology.owl#imperativeModality)\n\t\t" ;
        <http://www.w3.org/2000/01/rdf-schema#subClassOf>
                <http://purl.org/olia/olia-top.owl#MoodFeature> , <http://purl.org/olia/olia.owl#ImperativeModality> .

<http://purl.org/olia/olia.owl#Article>
        a       <http://www.w3.org/2002/07/owl#Class> ;
        <http://www.w3.org/2000/01/rdf-schema#comment>
                "\n\t\t\tAn article is a member of a small class of determiners that identify \n\t\t\ta noun's definite or indefinite reference, and the new or given status.\n\t\t\t(http://www.sil.org/linguistics/GlossaryOfLinguisticTerms/WhatIsAnArticle.htm  02.05.07)\n\t\t" ;
        <http://www.w3.org/2000/01/rdf-schema#subClassOf>
                <http://purl.org/olia/olia.owl#Determiner> ;
        <http://www.w3.org/2002/07/owl#versionInfo>
                "\n\t\t\tEAGLE top-level category \"Article\" (AT):\n\t\t\t\n\t\t\tIn Eagles articles are subsumed under determiners and kept\n\t\t\tas a separate class. It is a sub-class of determiners which is disjoint with the other determiner classes.\n\t\t\t(http://www.ilc.cnr.it/EAGLES96/annotate/node17.html#recn 18.09.06)\n\t\t\t\n\t\t\tModelled here as sub-class of Determiner because of its syntactic\n\t\t\tfunction.\n\t\t" .

<http://purl.org/olia/olia.owl#AgentRole>
        a       <http://www.w3.org/2002/07/owl#Class> ;
        <http://www.w3.org/2000/01/rdf-schema#comment>
                "\n\t\t\tAn agentive role is one in which the actor exerts some degree \n\t\t\tof will(-power) in the execution of the event.\n\t\t\t(http://languagelink.let.uu.nl/tds/onto/LinguisticOntology.owl#agentRole)\n\t\t" ;
        <http://www.w3.org/2000/01/rdf-schema#subClassOf>
                <http://purl.org/olia/olia.owl#ActorMacroRole> ;
        <http://www.w3.org/2002/07/owl#versionInfo>
                "http://languagelink.let.uu.nl/tds/onto/LinguisticOntology.owl#agentRole" .

<http://purl.org/olia/olia.owl#Headline>
        a       <http://www.w3.org/2002/07/owl#Class> ;
        <http://www.w3.org/2000/01/rdf-schema#comment>
                "-HLN (headline)\n— marks headlines and datelines. Note that headlines and datelines always constitute a unit of text that is structurally independent from the following sentence. \n(Bies et al. 1995)" ;
        <http://www.w3.org/2000/01/rdf-schema#subClassOf>
                <http://purl.org/olia/olia-top.owl#DiscourseEntity> ;
        <http://www.w3.org/2002/07/owl#versionInfo>
                "PTB bracketing guidelines, Bies et al. 1995" .

<http://purl.org/olia/olia.owl#ReferentialVoice>
        a       <http://www.w3.org/2002/07/owl#Class> ;
        <http://www.w3.org/2000/01/rdf-schema#comment>
                "\n\t\t\tentails assignment of the absolutive to certain kinds of arguments other \n\t\t\tthan the logical subjects (A) and objects (P), including the dative, \n\t\t\tbenefactive, malefactive, and possessor.  (Klaiman 1991:239)\n\t\t\t(http://purl.org/linguistics/gold/ReferentialVoice)\n\t\t" ;
        <http://www.w3.org/2000/01/rdf-schema#subClassOf>
                <http://purl.org/olia/olia.owl#Antipassive> ;
        <http://www.w3.org/2002/07/owl#versionInfo>
                "\n\t\t\thttp://purl.org/linguistics/gold/ReferentialVoice,\n\t\t\tclassified as Antipassive here in analogy with ObliquePassive\n\t\t" .

<http://purl.org/olia/olia.owl#ApproximateNumeral>
        a       <http://www.w3.org/2002/07/owl#Class> ;
        <http://www.w3.org/2000/01/rdf-schema#comment>
                "Bulgarian has Numeral/Form=approx(a), used for approximate numerals (десетина /about a ten/, стотина /about a hundred/) (Dimitrova et al. 2009, http://purl.org/olia/mte/multext-east.owl#ApproximateNumeral)" ;
        <http://www.w3.org/2000/01/rdf-schema#subClassOf>
                <http://purl.org/olia/olia.owl#Numeral> ;
        <http://www.w3.org/2002/07/owl#versionInfo>
                "http://purl.org/olia/mte/multext-east.owl#ApproximateNumeral" .

<http://purl.org/olia/olia.owl#QualitativeVerb>
        a       <http://www.w3.org/2002/07/owl#Class> ;
        <http://www.w3.org/2000/01/rdf-schema#comment>
                "no definition given" ;
        <http://www.w3.org/2000/01/rdf-schema#label>
                "qualitative verb"@en , "verbe qualitatif"@fr ;
        <http://www.w3.org/2000/01/rdf-schema#subClassOf>
                <http://purl.org/olia/olia.owl#MainVerb> ;
        <http://www.w3.org/2002/07/owl#versionInfo>
                "adopted from the Bambara Reference Corpus (BRC, http://cormand.huma-num.fr/gloses.html)" .

<http://purl.org/olia/olia.owl#ReflexiveVoice>
        a       <http://www.w3.org/2002/07/owl#Class> ;
        <http://www.w3.org/2000/01/rdf-schema#comment>
                "\n\t\t\tThe reflexive voice is a grammatical voice in which the subject is both the agent and the patient or recipient.\n\t\t\t(http://languagelink.let.uu.nl/tds/onto/LinguisticOntology.owl#reflexiveVoice)\n\t\t" ;
        <http://www.w3.org/2000/01/rdf-schema#subClassOf>
                <http://purl.org/olia/olia-top.owl#VoiceFeature> ;
        <http://www.w3.org/2002/07/owl#versionInfo>
                "\n\t\t\thttp://languagelink.let.uu.nl/tds/onto/LinguisticOntology.owl#reflexiveVoice\n\t\t" .

<http://purl.org/olia/olia.owl#CloseBracket>
        a       <http://www.w3.org/2002/07/owl#Class> ;
        <http://www.w3.org/2000/01/rdf-schema#comment>
                "\n                            Punctuation that is graphically represented by ]\n                                (http://www.isocat.org/datcat/DC-2083)\n                            " ;
        <http://www.w3.org/2000/01/rdf-schema#label>
                "close bracket" ;
        <http://www.w3.org/2000/01/rdf-schema#subClassOf>
                <http://purl.org/olia/olia.owl#RightParentheticalPunctuation> ;
        <http://www.w3.org/2002/07/owl#versionInfo>
                "http://www.isocat.org/datcat/DC-2083" .

<http://purl.org/olia/olia.owl#SuballativeCase>
        a       <http://www.w3.org/2002/07/owl#Class> ;
        <http://www.w3.org/2000/01/rdf-schema#comment>
                "\n\t\t\tSuballativeCase expresses that  something is moving toward the \n\t\t\tregion that is under the referent of the noun it marks. It has \n\t\t\tthe meaning 'towards the region that is under'.\n\t\t\t(http://purl.org/linguistics/gold/Suballative)\n\t\t" ;
        <http://www.w3.org/2000/01/rdf-schema#subClassOf>
                <http://purl.org/olia/olia-top.owl#CaseFeature> ;
        <http://www.w3.org/2002/07/owl#versionInfo>
                "http://purl.org/linguistics/gold/Suballative" .

<http://purl.org/olia/olia.owl#PerfectiveAspect>
        a       <http://www.w3.org/2002/07/owl#Class> ;
        <http://www.w3.org/2000/01/rdf-schema#comment>
                "\n\t\t\tThe perfective aspects (inceptive, punctual and completive) view \n\t\t\tthe situation as a bounded entity, and often put an emphasis on \n\t\t\tits beginning or end. (Bybee 1985:21)\n\t\t\t(http://languagelink.let.uu.nl/tds/onto/LinguisticOntology.owl#perfectiveAspect)\n\t\t\n\t\t\tThe Perfective aspect is an aspect that expresses a temporal view \n\t\t\tof an event or state as a simple whole, apart from the consideration \n\t\t\tof the internal structure of the time in which it occurs. \n\t\t\t(http://www.sil.org/linguistics/glossaryoflinguisticterms/WhatIsPerfectiveAspect.htm  17.11.06)\n\t\t\t\n\t\t\tA viewpoint aspect which encodes the speaker’s willingness to attend to the endpoints \n\t\t\tof the situation referred to. Perfective aspect is the canonical mode of presentation \n\t\t\tfor events (Michaelis 1998: xv).\n\t\t\t(http://purl.org/linguistics/gold/Perfective)\n\t\t" ;
        <http://www.w3.org/2000/01/rdf-schema#subClassOf>
                <http://purl.org/olia/olia-top.owl#AspectFeature> ;
        <http://www.w3.org/2002/07/owl#versionInfo>
                "\n\t\t\tEAGLES,\n\t\t\thttp://purl.org/linguistics/gold/Perfective\n\t\t" .

<http://purl.org/olia/olia.owl#SuperessiveCase>
        a       <http://www.w3.org/2002/07/owl#Class> ;
        <http://www.w3.org/2000/01/rdf-schema#comment>
                "\n\t\t\tSuperessiveCase expresses that  the referent of the noun it \n\t\t\tmarks is the location on which another referent exists. It has \n\t\t\tthe meaning of 'on' or 'upon'. (Pei and Gaynor 1954: 207, Gove, \n\t\t\tet al. 1966: 2293).\n\t\t\t(http://purl.org/linguistics/gold/Superessive)\n\t\t" ;
        <http://www.w3.org/2000/01/rdf-schema#subClassOf>
                <http://purl.org/olia/olia-top.owl#CaseFeature> ;
        <http://www.w3.org/2002/07/owl#versionInfo>
                "http://purl.org/linguistics/gold/Superessive, http://www.isocat.org/datcat/DC-1396" .

<http://purl.org/olia/olia.owl#VulgarRegister>
        a       <http://www.w3.org/2002/07/owl#Class> ;
        <http://www.w3.org/2000/01/rdf-schema#comment>
                "\n                            Register of a term or text type that can be characterized as profane or socially unacceptable.\n                                (ISO12620; http://www.isocat.org/datcat/DC-1998)\n                            " ;
        <http://www.w3.org/2000/01/rdf-schema#label>
                "vulgar register" ;
        <http://www.w3.org/2000/01/rdf-schema#subClassOf>
                <http://purl.org/olia/olia-top.owl#RegisterFeature> ;
        <http://www.w3.org/2002/07/owl#versionInfo>
                "http://www.isocat.org/datcat/DC-1998" , "subClassOf register (dcif:conceptualDomain)" .

<http://purl.org/olia/olia.owl#InterallativeCase>
        a       <http://www.w3.org/2002/07/owl#Class> ;
        <http://www.w3.org/2000/01/rdf-schema#comment>
                "\n\t\t\tInterallativeCase expresses that  something is moving toward the \n\t\t\tregion that is in the middle of the referent of the noun it marks. \n\t\t\tIt has the meaning  'towards the middle of'.\n\t\t\t(http://purl.org/linguistics/gold/Interallative)\n\t\t" ;
        <http://www.w3.org/2000/01/rdf-schema#subClassOf>
                <http://purl.org/olia/olia-top.owl#CaseFeature> ;
        <http://www.w3.org/2002/07/owl#versionInfo>
                "http://purl.org/linguistics/gold/Interallative" .

<http://purl.org/olia/olia.owl#RelationNoun>
        a       <http://www.w3.org/2002/07/owl#Class> ;
        <http://www.w3.org/2000/01/rdf-schema#comment>
                "\n                            relation noun\n                                (MIRACL & LSCA; http://www.isocat.org/datcat/DC-2226)\n                            " ;
        <http://www.w3.org/2000/01/rdf-schema#label>
                "relation noun" ;
        <http://www.w3.org/2000/01/rdf-schema#subClassOf>
                <http://purl.org/olia/olia.owl#CommonNoun> ;
        <http://www.w3.org/2002/07/owl#versionInfo>
                "subClassOf partOfSpeech (dcif:conceptualDomain)" , "http://www.isocat.org/datcat/DC-2226" .

<http://purl.org/olia/olia.owl#Strong>
        a       <http://www.w3.org/2002/07/owl#Class> ;
        <http://www.w3.org/2000/01/rdf-schema#comment>
                "\n\t\t\tStrong pronouns are different from the weak pronouns (cf.  StrengthFeature:Weak)\n\t\t" ;
        <http://www.w3.org/2000/01/rdf-schema#subClassOf>
                <http://purl.org/olia/olia-top.owl#StrengthFeature> ;
        <http://www.w3.org/2002/07/owl#versionInfo>
                "EAGLES" , "TODO: rename to StrongPronoun" .

<http://purl.org/olia/olia.owl#Determiner>
        a       <http://www.w3.org/2002/07/owl#Class> ;
        <http://www.w3.org/2000/01/rdf-schema#comment>
                "\n\t\t\tA determiner is a noun modifier that expresses the reference of a noun or noun phrase \n\t\t\tin the context, including quantity, rather than attributes expressed by adjectives. \n\t\t\tThis part of speech is defined in some languages, such as in English, as it is distinct \n\t\t\tfrom adjectives grammatically, though most English dictionaries still identify the \n\t\t\tdeterminers as adjectives. \n\t\t\t(http://en.wikipedia.org/wiki/Determiner 19.09.06)\n\t\t" ;
        <http://www.w3.org/2000/01/rdf-schema#label>
                "determiner"@en , "determinatif"@fr ;
        <http://www.w3.org/2000/01/rdf-schema#subClassOf>
                <http://purl.org/olia/olia.owl#PronounOrDeterminer> ;
        <http://www.w3.org/2002/07/owl#versionInfo>
                "EAGLES PronounOrDeterminer with category=\"Determiner\"" , "introduced AttributivePronoun as subclass of Determiner (Article is no AttributivePronoun)" , "\n\t\t\tNote that \"Determiner\" in OLiA also covers determiner-like elements in languages without grammaticalized determiner category.\n\t\t\tThis is because AttributePronoun is defined as being in the intersection of Determiner and Pronoun. \n\t\t\tIn languages without grammaticalized determiners, attributive pronouns are, howevetr, not characterized as determiners, but rather as adjectives.\n\t\t\tIn order to provide a uniform modeling of attributive pronouns, they are defined here as being the intersection of Determiner and Pronoun.\n\t\t\t(Chiarcos)\n\t\t" .

<http://purl.org/olia/olia.owl#MultipleNumeral>
        a       <http://www.w3.org/2002/07/owl#Class> ;
        <http://www.w3.org/2000/01/rdf-schema#comment>
                "A Multiple Numeral serves to define a complex whole, with respect to the number of its parts, e.g., English \"twofold\", \"twice\" or \"manyfold\". Used in morphosyntactic descriptions of, e.g., Romanian, Slovak and Czech.\n\t\t\t(Joseph Ghostwick [1878], English language -- Grammar, Historical, London, Longmans, Green, and Co.; http://purl.org/olia/mte/multext-east.owl#MultipleNumeral)" ;
        <http://www.w3.org/2000/01/rdf-schema#label>
                "multiplicative numeral" , "multiple numeral" ;
        <http://www.w3.org/2000/01/rdf-schema#subClassOf>
                <http://purl.org/olia/olia.owl#Quantifier> ;
        <http://www.w3.org/2002/07/owl#versionInfo>
                "TODO: rename to MultiplicativeNumeral" , "http://purl.org/olia/mte/multext-east.owl#MultipleNumeral, http://purl.org/olia/urdu.owl#MultiplicativeNumeral; As \"manyfold\" fits Ghostwick's definition, MultipleNumeral is modelled as a subclass of Quantifier rather than Numeral. In MULTEXT-East, \"Numeral\" was extended to coover non-numerical quantifiers, hence the name." .

<http://purl.org/olia/olia.owl#Antipassive>
        a       <http://www.w3.org/2002/07/owl#Class> ;
        <http://www.w3.org/2000/01/rdf-schema#comment>
                "\n\t\t\tDerives an intransitive verb from a transitive stem whereby the original agent (only) \n\t\t\tis cross-referrenced by the absolutive markers on the verb and the original patient, \n\t\t\tif it appears, is in an oblique phrase. (England 1983:110)\n\t\t\t(http://purl.org/linguistics/gold/Antipassive)\n\t\t" ;
        <http://www.w3.org/2000/01/rdf-schema#subClassOf>
                <http://purl.org/olia/olia-top.owl#VoiceFeature> ;
        <http://www.w3.org/2002/07/owl#versionInfo>
                "http://purl.org/linguistics/gold/Antipassive" .

<http://purl.org/olia/olia.owl#AbilitativeModality>
        a       <http://www.w3.org/2002/07/owl#Class> ;
        <http://www.w3.org/2000/01/rdf-schema#comment>
                "modality expressed by AbilitativeMood: Abilitative is a mood that indicates ability, comparable to the use of \"can\" in English. (http://zbb.spinnwebe.com/viewtopic.php?f=7&t=34901)" ;
        <http://www.w3.org/2000/01/rdf-schema#subClassOf>
                <http://purl.org/olia/olia-top.owl#ModalityFeature> ;
        <http://www.w3.org/2002/07/owl#versionInfo>
                "Adopted from ILPOSTS (for Indian languages), http://purl.org/olia/ilposts.owl#AbilitativeMood" .

<http://purl.org/olia/olia.owl#DeponentMiddle>
        a       <http://www.w3.org/2002/07/owl#Class> ;
        <http://www.w3.org/2000/01/rdf-schema#comment>
                "\n\t\t\tAction denotes physical/mental disposition of subject. (Siewierska 1988:257)\n\t\t\t(http://purl.org/linguistics/gold/DeponentMiddle)\n\t\t" ;
        <http://www.w3.org/2000/01/rdf-schema#subClassOf>
                <http://purl.org/olia/olia.owl#MiddleVoice> ;
        <http://www.w3.org/2002/07/owl#versionInfo>
                "http://purl.org/linguistics/gold/DeponentMiddle" .

<http://purl.org/olia/olia.owl#DeclarativePunctuation>
        a       <http://www.w3.org/2002/07/owl#Class> ;
        <http://www.w3.org/2000/01/rdf-schema#comment>
                "Punctuation used at the end a declarative sentence." ;
        <http://www.w3.org/2000/01/rdf-schema#isDefinedBy>
                "http://www.isocat.org/datcat/DC-2086" ;
        <http://www.w3.org/2000/01/rdf-schema#subClassOf>
                <http://purl.org/olia/olia.owl#SentenceFinalPunctuation> , <http://purl.org/olia/olia.owl#DeclarativeModality> .

<http://purl.org/olia/olia.owl#DemonstrativeDeterminer>
        a       <http://www.w3.org/2002/07/owl#Class> ;
        <http://www.w3.org/2000/01/rdf-schema#comment>
                "\n\t\t\tDemonstratives are deictic expressions (they depend on an external frame of reference) \n\t\t\twhich indicate  entities a speaker refers to, and distinguishes those entities from \n\t\t\tothers. Demonstratives are usually employed for spatial deixis (using the context of \n\t\t\tthe physical surroundings), but in many languages they double as discourse deictics, \n\t\t\treferring not to concrete objects but to words, phrases and propositions mentioned in \n\t\t\tspeech.\n            (http://en.wikipedia.org/wiki/Demonstrative 19.09.06)\n\t\t" ;
        <http://www.w3.org/2000/01/rdf-schema#subClassOf>
                <http://purl.org/olia/olia.owl#AttributivePronoun> ;
        <http://www.w3.org/2002/07/owl#versionInfo>
                "\n\t\t\tEAGLES Determiner with DetType=\"Demonstrative\".\n\t\t" .

<http://purl.org/olia/olia.owl#IndicativeVerb>
        a       <http://www.w3.org/2002/07/owl#Class> ;
        <http://www.w3.org/2000/01/rdf-schema#comment>
                "\n\t\t\tIndicative mood is used in factual statements. All intentions in \n\t\t\tspeaking that a particular language does not put into another mood \n\t\t\tuse the indicative. It is the most commonly used mood and is found \n\t\t\tin all languages. \n\t\t\t(http://en.wikipedia.org/wiki/Grammatical_mood#Indicative_mood 19.09.06)\n\t\t" ;
        <http://www.w3.org/2000/01/rdf-schema#subClassOf>
                <http://purl.org/olia/olia.owl#FiniteVerb> ;
        <http://www.w3.org/2002/07/owl#versionInfo>
                "EAGLES FiniteVerb with VerbForm=\"Indicative\"" .

<http://purl.org/olia/olia.owl#InanimateGender>
        a       <http://www.w3.org/2002/07/owl#Class> ;
        <http://www.w3.org/2000/01/rdf-schema#comment>
                "\n\t\t\tOne of the two grammatical genders, or noun classes, of Nishnaabemwin, \n\t\t\tthe other being animate. Membership in the inanimate grammatical class \n\t\t\tis largely based on meaning, in that non-living things, such as objects \n\t\t\tof manufacture and natural 'non-living' things are included in it \n\t\t\t(Valentine 2001:  114).\n\t\t\t(http://purl.org/linguistics/gold/Inanimate)\n\t\t" ;
        <http://www.w3.org/2000/01/rdf-schema#subClassOf>
                <http://purl.org/olia/olia-top.owl#GenderFeature> ;
        <http://www.w3.org/2002/07/owl#versionInfo>
                "http://purl.org/linguistics/gold/Inanimate" .

<http://purl.org/olia/olia.owl#PresentParticipleAdjective>
        a       <http://www.w3.org/2002/07/owl#Class> ;
        <http://www.w3.org/2000/01/rdf-schema#comment>
                "\n                            Adjective based on a present participle.\n                                (http://www.isocat.org/datcat/DC-1597)\n                            " ;
        <http://www.w3.org/2000/01/rdf-schema#label>
                "present participle adjective" ;
        <http://www.w3.org/2000/01/rdf-schema#subClassOf>
                <http://purl.org/olia/olia.owl#PresentParticiple> , <http://purl.org/olia/olia.owl#ParticipleAdjective> ;
        <http://www.w3.org/2002/07/owl#versionInfo>
                "subClassOf participleAdjective (dcif:isA)" , "http://www.isocat.org/datcat/DC-1597" .

<http://purl.org/olia/olia.owl#ProcessedRole>
        a       <http://www.w3.org/2002/07/owl#Class> ;
        <http://www.w3.org/2000/01/rdf-schema#comment>
                "\n\t\t\tThe entity that undergoes a Process (Dik, 1997:118).\n\t\t\t(http://languagelink.let.uu.nl/tds/onto/LinguisticOntology.owl#processedRole)\n\t\t" ;
        <http://www.w3.org/2000/01/rdf-schema#subClassOf>
                <http://purl.org/olia/olia.owl#UndergoerMacroRole> ;
        <http://www.w3.org/2002/07/owl#versionInfo>
                "http://languagelink.let.uu.nl/tds/onto/LinguisticOntology.owl#processedRole" .

<http://purl.org/olia/olia.owl#MainVerb>
        a       <http://www.w3.org/2002/07/owl#Class> ;
        <http://www.w3.org/2000/01/rdf-schema#comment>
                "\n                            Main verb in contrast to a modal or an auxiliary.\n                                (http://www.isocat.org/datcat/DC-1400)\n\t\t\t\t\t\t\t\t\n\t\t\t\t\t\t\t\tverb which has its own semantics (http://www.isocat.org/datcat/DC-3004, plainVerb)\n                            " ;
        <http://www.w3.org/2000/01/rdf-schema#isDefinedBy>
                "http://www.isocat.org/datcat/DC-3004 (plainVerb)" ;
        <http://www.w3.org/2000/01/rdf-schema#label>
                "main verb" , "plain verb" ;
        <http://www.w3.org/2000/01/rdf-schema#subClassOf>
                <http://purl.org/olia/olia.owl#Verb> ;
        <http://www.w3.org/2002/07/owl#versionInfo>
                "http://www.isocat.org/datcat/DC-1400 (main verb)" , "subClassOf verb (dcif:isA)" , "to be renamed to LexicalVerb (\"main verb\" can also mean \"head of a finite clause\")" .

<http://purl.org/olia/olia-top.owl>
        a       <http://www.w3.org/2002/07/owl#Ontology> .

<http://purl.org/olia/olia.owl#SubtranslativeCase>
        a       <http://www.w3.org/2002/07/owl#Class> ;
        <http://www.w3.org/2000/01/rdf-schema#comment>
                "\n\t\t\tSubtranslativeCase expresses the notion of something moving along a \n\t\t\ttrajectory underneath the referent of the noun it marks. It has the \n\t\t\tmeaning 'along the region underneath'. Unfortunate name clash with \n\t\t\t'Superlative' as a feature of adjectives.\n\t\t\t(http://purl.org/linguistics/gold/Subtranslative)\n\t\t" ;
        <http://www.w3.org/2000/01/rdf-schema#subClassOf>
                <http://purl.org/olia/olia-top.owl#CaseFeature> ;
        <http://www.w3.org/2002/07/owl#versionInfo>
                "http://purl.org/linguistics/gold/Subtranslative" .

<http://purl.org/olia/olia.owl#Proximal>
        a       <http://www.w3.org/2002/07/owl#Class> ;
        <http://www.w3.org/2000/01/rdf-schema#comment>
                "The referent denoted by a distal demonstrative pronoun (e.g., English that) is usually spatially more \n\t\t\tremote or discoursally less salient as compared to a referent denoted by a proximal demonstrative pronoun (e.g., English this)\n\t\t\t(Chiarcos)\n\t\t" ;
        <http://www.w3.org/2000/01/rdf-schema#subClassOf>
                <http://purl.org/olia/olia-top.owl#ProximityFeature> ;
        <http://www.w3.org/2002/07/owl#versionInfo>
                "added in accordance with http://purl.org/olia/mte/multext-east.owl#CliticProximalDeterminer" .

<http://purl.org/olia/olia.owl#Neuter>
        a       <http://www.w3.org/2002/07/owl#Class> ;
        <http://www.w3.org/2000/01/rdf-schema#comment>
                "\n\t\t\tNeuter gender is a grammatical gender that includes those nouns, \n\t\t\tarticles, pronouns, etc. having referents which do not have \n\t\t\tdistinctions of sex, and often includes some which do have a \n\t\t\tnatural sex distinction. \n\t\t\t(http://www.sil.org/linguistics/glossaryoflinguisticterms/WhatIsNeuterGender.htm  17.11.06)\n\t\t" ;
        <http://www.w3.org/2000/01/rdf-schema#subClassOf>
                <http://purl.org/olia/olia-top.owl#GenderFeature> ;
        <http://www.w3.org/2002/07/owl#versionInfo>
                "\n\t\t\tEAGLES, \n\t\t\thttp://languagelink.let.uu.nl/tds/onto/LinguisticOntology.owl#neuterGender\n\t\t" .

<http://purl.org/olia/olia.owl#IntranslativeCase>
        a       <http://www.w3.org/2002/07/owl#Class> ;
        <http://www.w3.org/2000/01/rdf-schema#comment>
                "\n\t\t\tIntranslativeCase expresses the notion of something moving through \n\t\t\tthe referent of the noun it marks. It has the meaning 'along through'.\n\t\t\t(http://purl.org/linguistics/gold/Intranslative)\n\t\t" ;
        <http://www.w3.org/2000/01/rdf-schema#subClassOf>
                <http://purl.org/olia/olia-top.owl#CaseFeature> ;
        <http://www.w3.org/2002/07/owl#versionInfo>
                "http://purl.org/linguistics/gold/Intranslative" .

<http://purl.org/olia/olia.owl#InfinitiveVerbPhrase>
        a       <http://www.w3.org/2002/07/owl#Class> ;
        <http://www.w3.org/2000/01/rdf-schema#comment>
                "\n\t\t\tVGINF Infinitival Verb Chunk\n\t\t\tThis tag is to mark the infinitival verb form. In Hindi, both, gerunds and infinitive forms of the verb end with a -nA suffix. Since both behave functionally in a similar manner, the distinction is not very clear. However, languages such as Bangla etc have two different forms for the two types. Examples from Bangla are given below.\n\t\t\tb8. Borabela ((snAna karA))_VGNN SorIrera pokze BAlo\n\t\t\t'Morning' 'bath' 'do-verbal noun' 'health-gen' 'for' 'good'\n\t\t\t‘Taking bath in the early morning is good for health”\n\t\t\tb9. bindu Borabela ((snAna karawe))_VGINF BAlobAse\n\t\t\t'Bindu' 'morning' 'bath' 'take-inf' 'love-3pr'\n\t\t\t“Bindu likes to take bath in the early morning”\n\t\t\tIn Bangla, the gerund form takes the suffix –A / -Ano, while the infinitive marker is –we. The syntactic distribution of these two forms of verbs is different. For example, the gerund form is allowed in the context of the word darakAra “necessary” while the infinitive form is not, as exemplified below:\n\t\t\tb10 Borabela ((snAna karA))_VGNN darakAra\n\t\t\t'Morning' 'bath' 'do-verbal noun' 'necessary'\n\t\t\t“It is necessary to take bath in the early morning”\n\t\t\tb11. *Borabela ((snAna karawe))_VGINF darakAra\n\t\t\tBased on the above evidence from Bangla, the tag VGINF has been included to mark a verb chunk.\n\t\t\t\n\t\t\t(Akshar Bharati, Dipti Misra Sharma, Lakshmi Bai, Rajeev Sangal (2006), AnnCorra : Annotating Corpora. Guidelines For POS And Chunk Annotation For Indian Languages, Tech. Rep., L anguage Technologies Research Centre IIIT, Hyderabad, version of 15-12-2006, http://ltrc.iiit.ac.in/tr031/posguidelines.pdf)\n\t\t" ;
        <http://www.w3.org/2000/01/rdf-schema#subClassOf>
                <http://purl.org/olia/olia.owl#NonfiniteVerbPhrase> ;
        <http://www.w3.org/2002/07/owl#versionInfo>
                "Ancorra, http://purl.org/olia/ancorra.owl#InfiniteVerbChunk" .

<http://purl.org/olia/olia.owl#Derivation>
        a       <http://www.w3.org/2002/07/owl#Class> ;
        <http://www.w3.org/2000/01/rdf-schema#comment>
                "\n                            Change in the form of a linguistic unit, usually modification in the base/root or affixation to create a new word.\n                                (Sue Ellen Wright + Gil Francopoulo; http://www.isocat.org/datcat/DC-1271)\n                            " ;
        <http://www.w3.org/2000/01/rdf-schema#label>
                "derivation" ;
        <http://www.w3.org/2000/01/rdf-schema#subClassOf>
                <http://purl.org/olia/olia-top.owl#MorphologicalProcess> ;
        <http://www.w3.org/2002/07/owl#versionInfo>
                "http://www.isocat.org/datcat/DC-1271" .

<http://purl.org/olia/olia.owl#MediopassiveVoice>
        a       <http://www.w3.org/2002/07/owl#Class> ;
        <http://www.w3.org/2000/01/rdf-schema#comment>
                "voice which subsumes both the middle voice and the passive voice" ;
        <http://www.w3.org/2000/01/rdf-schema#isDefinedBy>
                "http://www.isocat.org/datcat/DC-3850" ;
        <http://www.w3.org/2000/01/rdf-schema#subClassOf>
                <http://purl.org/olia/olia-top.owl#VoiceFeature> ;
        <http://www.w3.org/2002/07/owl#equivalentClass>
                [ a       <http://www.w3.org/2002/07/owl#Class> ;
                  <http://www.w3.org/2002/07/owl#unionOf>
                          ( <http://purl.org/olia/olia.owl#MiddleVoice> <http://purl.org/olia/olia.owl#PassiveVoice> )
                ] .

<http://purl.org/olia/olia.owl#ObliquePassive>
        a       <http://www.w3.org/2002/07/owl#Class> ;
        <http://www.w3.org/2000/01/rdf-schema#comment>
                "\n\t\t\tA Passive in which a basic Oblique nominal assumes the Subject relation \n\t\t\tin a corresponding nonbasic configuration.  Can include locative passives, \n\t\t\tbenefactive passives and instrumental passives. (Klaiman 1991:23)\n\t\t\t(http://purl.org/linguistics/gold/ObliquePassive)\n\t\t" ;
        <http://www.w3.org/2000/01/rdf-schema#subClassOf>
                <http://purl.org/olia/olia.owl#PassiveVoice> ;
        <http://www.w3.org/2002/07/owl#versionInfo>
                "http://purl.org/linguistics/gold/ObliquePassive" .

<http://purl.org/olia/olia.owl#Human>
        a       <http://www.w3.org/2002/07/owl#Class> ;
        <http://www.w3.org/2000/01/rdf-schema#comment>
                "For Slavic languages, animacy, and in particular, Humanness, defines so-called \"sub-genders\" that manifest themselves in the accusative ending of masculine and neuter singular nouns. Humans are by definition animate. \n\t\t\t(http://purl.org/olia/mte/multext-east.owl#Human)" ;
        <http://www.w3.org/2000/01/rdf-schema#subClassOf>
                <http://purl.org/olia/olia.owl#Animate> ;
        <http://www.w3.org/2002/07/owl#versionInfo>
                "http://purl.org/olia/mte/multext-east.owl#Human" .

<http://purl.org/olia/olia.owl#ModalParticle>
        a       <http://www.w3.org/2002/07/owl#Class> ;
        <http://www.w3.org/2000/01/rdf-schema#comment>
                "\n                            Particle which functions as a modal.\n                                (http://www.isocat.org/datcat/DC-1920)\n                            " ;
        <http://www.w3.org/2000/01/rdf-schema#label>
                "modal particle" ;
        <http://www.w3.org/2000/01/rdf-schema#subClassOf>
                <http://purl.org/olia/olia.owl#Particle> ;
        <http://www.w3.org/2002/07/owl#versionInfo>
                "subClassOf particle (dcif:isA)" , "TOCHECK: is this definition correct ? Could it be that ModalParticle actually means \"VerbalParticle marking mood\" ? (Cf. ModalityMarkingAdverb)" , "http://www.isocat.org/datcat/DC-1920" .

<http://purl.org/olia/olia.owl#PastInFuture>
        a       <http://www.w3.org/2002/07/owl#Class> ;
        <http://www.w3.org/2000/01/rdf-schema#comment>
                "\n\t\t\tLocates the situation in question in the future, prior to a reference \n\t\t\ttime in the future.\n\t\t" ;
        <http://www.w3.org/2000/01/rdf-schema#subClassOf>
                <http://purl.org/olia/olia.owl#AbsoluteRelativeTense> ;
        <http://www.w3.org/2002/07/owl#versionInfo>
                "http://purl.org/linguistics/gold/PastInFuture" .

<http://purl.org/olia/olia.owl#ObjectiveCase>
        a       <http://www.w3.org/2002/07/owl#Class> ;
        <http://www.w3.org/2000/01/rdf-schema#comment>
                "Case used to express the direct object, indirect object, object of a preposition, object complement and subject of an infinitive." ;
        <http://www.w3.org/2000/01/rdf-schema#isDefinedBy>
                "http://www.isocat.org/datcat/DC-2798" ;
        <http://www.w3.org/2000/01/rdf-schema#subClassOf>
                <http://purl.org/olia/olia-top.owl#CaseFeature> .

<http://purl.org/olia/olia.owl#PragmaticInverseVoice>
        a       <http://www.w3.org/2002/07/owl#Class> ;
        <http://www.w3.org/2000/01/rdf-schema#comment>
                "\n\t\t\tIf the agent is more topical than the patient, the direct-active clause \n\t\t\tis used.  If norm is reversed and the patient is more topical, the inverse \n\t\t\tclause is used. (Givon 1994:23)\n\t\t\t(http://purl.org/linguistics/gold/PragmaticInverse)\n\t\t" ;
        <http://www.w3.org/2000/01/rdf-schema#subClassOf>
                <http://purl.org/olia/olia.owl#InverseVoice> ;
        <http://www.w3.org/2002/07/owl#versionInfo>
                "http://purl.org/linguistics/gold/PragmaticInverse" .

<http://purl.org/olia/olia.owl#SociativeCase>
        a       <http://www.w3.org/2002/07/owl#Class> ;
        <http://www.w3.org/2000/01/rdf-schema#comment>
                "\n\t\tCase related to the person in whose company the action is carried out,\n\t\tor to any belongings of people which take part in the action. \n\t\t(http://www.isocat.org/datcat/DC-1388)\n\t  "@en ;
        <http://www.w3.org/2000/01/rdf-schema#label>
                "sociative case"@en ;
        <http://www.w3.org/2000/01/rdf-schema#subClassOf>
                <http://purl.org/olia/olia-top.owl#CaseFeature> ;
        <http://www.w3.org/2002/07/owl#versionInfo>
                "adopted from http://www.isocat.org/datcat/DC-1388" , "TODO: check whether this is really different from comitative" .

<http://purl.org/olia/olia.owl#Expletive>
        a       <http://www.w3.org/2002/07/owl#Class> ;
        <http://www.w3.org/2000/01/rdf-schema#comment>
                "\n                            Word which serves no grammatical function, but which fills up a sentence or gives emphasis.\n                                (www.southwestern.edu/~carlg/Latin_Web/glossary.html; http://www.isocat.org/datcat/DC-1283)\n                            " ;
        <http://www.w3.org/2000/01/rdf-schema#label>
                "expletive" ;
        <http://www.w3.org/2000/01/rdf-schema#subClassOf>
                <http://purl.org/olia/olia.owl#Unique> ;
        <http://www.w3.org/2002/07/owl#versionInfo>
                "http://www.isocat.org/datcat/DC-1283" , "modelled as a Unique concept here, although normally not considered a Particle" .

<http://purl.org/olia/olia.owl#SuperlativeCase>
        a       <http://www.w3.org/2002/07/owl#Class> ;
        <http://www.w3.org/2000/01/rdf-schema#comment>
                "\n\t\t\tSuperlativeCase expresses that  the referent of the noun it marks is the location onto \n\t\t\twhich another referent is moving. It has the meaning of 'onto'. Unfortunate name clash \n\t\t\twith 'Superlative' as a property of adjectives.\n\t\t\t(http://purl.org/linguistics/gold/Superlative)\n\t\t" ;
        <http://www.w3.org/2000/01/rdf-schema#subClassOf>
                <http://purl.org/olia/olia-top.owl#CaseFeature> ;
        <http://www.w3.org/2002/07/owl#versionInfo>
                "http://purl.org/linguistics/gold/Superlative" .

<http://purl.org/olia/olia.owl#ImmediatePast>
        a       <http://www.w3.org/2002/07/owl#Class> ;
        <http://www.w3.org/2000/01/rdf-schema#comment>
                "\n\t\t\tImmediatePastTense locates the situation in question at a time considered \n\t\t\tvery recent in relation to the moment of utterance (Comrie 1985: 87).\n\t\t\t(http://purl.org/linguistics/gold/ImmediatePast)\n\t\t" ;
        <http://www.w3.org/2000/01/rdf-schema#subClassOf>
                <http://purl.org/olia/olia.owl#Past> ;
        <http://www.w3.org/2002/07/owl#versionInfo>
                "http://purl.org/linguistics/gold/ImmediatePast, classified as Past here" .

<http://purl.org/olia/olia.owl#Cliticization>
        a       <http://www.w3.org/2002/07/owl#Class> ;
        <http://www.w3.org/2000/01/rdf-schema#comment>
                "\n\t\t\tIn morphosyntax, cliticization is a process by which a complex word is formed by attaching a clitic to a fully inflected word.\n\t\t\tExsmple: In Je t'aime, t' is the clitic attached to aime. \n\t\t\t(http://www.glottopedia.de/index.php/Cliticization)\n\t\t\n\t\t\tNote that cliticization can also be understood as the process of an independent word developing into a clitic. This is not the meaning intended here, as the OLiA ontologies are currently not applied to the description of diachronic processes. (Chiarcos)\n\t\t" ;
        <http://www.w3.org/2000/01/rdf-schema#label>
                "cliticization" ;
        <http://www.w3.org/2000/01/rdf-schema#subClassOf>
                <http://purl.org/olia/olia-top.owl#MorphologicalProcess> ;
        <http://www.w3.org/2002/07/owl#versionInfo>
                "http://www.glottopedia.de/index.php/Cliticization; http://www.isocat.org/datcat/DC-1903 (cliticness), http://purl.org/olia/mte/multext-east.owl#Cliticness. Note that Cliticization covers only one aspect of the original MULTEXT-East (and ISOcat) definitions of cliticness, i.e., that an element is a clitic" .

<http://purl.org/olia/olia.owl#PhasalAspect>
        a       <http://www.w3.org/2002/07/owl#Class> ;
        <http://www.w3.org/2000/01/rdf-schema#comment>
                "\n\t\t\tA set of aspectual distinctions involving relations between a background \n\t\t\tsituation (the reference situation) and a situation located relative to \n\t\t\tthe reference situation (the denoted situation). In English, phasal \n\t\t\tdistinctions are expressed by auxiliary-headed constructions, like the \n\t\t\tinceptive, progressive, and perfect constructions, whose head verbs express \n\t\t\tthe aspectual class of the denoted situation. The aspectual class of the \n\t\t\tdenoted situation differs from that of the reference situation \n\t\t\t(Michaelis 1998:xv). \n\t\t\tAn event may have a beginning and an end, a middle portion (continuing or \n\t\t\tchanging), and also an ensuing result or an altered state. These are \n\t\t\tconsidered to be the various “phases‽ of an event. A speaker may talk about \n\t\t\tan event from the point of view of any of these individual phases, and his \n\t\t\tlanguage may have inflectional (or other type of) markers for representing \n\t\t\tthese distinctions. Since such markers indicate distinctions in the temporal \n\t\t\tstructure of an event, we may regard them as belonging to the category of \n\t\t\taspect. It has been suggested (Dik 1989: 186) that these may be grouped \n\t\t\tunder a subcategory (or “level\") of aspect called “phasal aspect\". \n\t\t\t(Bhat 1999:49)\t\t\n\t\t\t(http://purl.org/linguistics/gold/Phasal)\n\t\t" ;
        <http://www.w3.org/2000/01/rdf-schema#subClassOf>
                <http://purl.org/olia/olia-top.owl#AspectFeature> ;
        <http://www.w3.org/2002/07/owl#versionInfo>
                "\n\t\t\thttp://languagelink.let.uu.nl/tds/onto/LinguisticOntology.owl#phaseAspect,\n\t\t\thttp://purl.org/linguistics/gold/Phasal\n\t\t" .

<http://purl.org/olia/olia.owl#hasSyntacticValency>
        a       <http://www.w3.org/2002/07/owl#ObjectProperty> ;
        <http://www.w3.org/2000/01/rdf-schema#comment>
                "\n\t\tIn annotation schemes for morphosyntax, \"valency\" normally means syntactic valency, i.e., the number of syntactic arguments \n\t\ta verb/clause takes.\n\t" ;
        <http://www.w3.org/2000/01/rdf-schema#range>
                <http://purl.org/olia/olia-top.owl#ValencyFeature> ;
        <http://www.w3.org/2000/01/rdf-schema#subPropertyOf>
                <http://purl.org/olia/system.owl#hasFeature> ;
        <http://www.w3.org/2002/07/owl#versionInfo>
                "SUSANNE (Sampson 1995)" .

<http://purl.org/olia/olia.owl#Adposition>
        a       <http://www.w3.org/2002/07/owl#Class> ;
        <http://www.w3.org/2000/01/rdf-schema#comment>
                "\n      An adposition is a cover term for prepositions, postpositions and \n      circumpositions. It expresses a grammatical and semantic relation \n      to another unit within a clause.\n      (http://www.sil.org/linguistics/GlossaryOfLinguisticTerms/WhatIsAnAdposition.htm, http://en.wikipedia.org/wiki/Adposition 19.09.06)\n      \n      The majority of cases of adpositions we have to consider in European languages are prepositions.\n      (http://www.ilc.cnr.it/EAGLES96/annotate/node17.html#SECTION00062200000000000000 19.09.06)" ;
        <http://www.w3.org/2000/01/rdf-schema#subClassOf>
                <http://purl.org/olia/olia-top.owl#MorphosyntacticCategory> ;
        <http://www.w3.org/2002/07/owl#versionInfo>
                "EAGLES top-level category Adposition (AP)." .

<http://purl.org/olia/olia.owl#LeftSentenceBracket>
        a       <http://www.w3.org/2002/07/owl#Class> ;
        <http://www.w3.org/2000/01/rdf-schema#comment>
                "\nIn a German clause, the finite verb can appear in three different positions: verb-second, \nverb-initial, and verb-final. Only in verb-final clauses the verb complex consisting of the\nfinite verb and non-finite verbal elements forms a unit. The discontinuous positioning\nof the verbal elements in verb-first and verb-second clauses is the traditional reason\nfor structuring German clauses into fields. The positions of the verbal elements form\nthe Satzklammer (sentence bracket) which divides the sentence into a Vorfeld (initial\nfield), a Mittelfeld (middle field), and a Nachfeld (final field). The Vorfeld and the\nMittelfeld are divided by the linke Satzklammer (left sentence bracket), which is the finite\nverb, the rechte Satzklammer (right sentence bracket) is the verb complex between the\nMittelfeld and the Nachfeld. \n(Telljohann et al. 2009, p.13)\n\t\t" ;
        <http://www.w3.org/2000/01/rdf-schema#subClassOf>
                <http://purl.org/olia/olia-top.owl#TopologicalField> .

<http://purl.org/olia/olia.owl#FormalRegister>
        a       <http://www.w3.org/2002/07/owl#Class> ;
        <http://www.w3.org/2000/01/rdf-schema#comment>
                "\n                            Formal register.\n                                (12620; http://www.isocat.org/datcat/DC-1992)\n                            " ;
        <http://www.w3.org/2000/01/rdf-schema#label>
                "formal register" ;
        <http://www.w3.org/2000/01/rdf-schema#subClassOf>
                <http://purl.org/olia/olia-top.owl#RegisterFeature> ;
        <http://www.w3.org/2002/07/owl#versionInfo>
                "http://www.isocat.org/datcat/DC-1992" , "subClassOf register (dcif:conceptualDomain)" .

<http://purl.org/olia/olia.owl#MixedInflection>
        a       <http://www.w3.org/2002/07/owl#Class> ;
        <http://www.w3.org/2000/01/rdf-schema#comment>
                "\n\t\t\tGerman mixed inflection takes its name from \n\t\t\tthe fact that it has endings from both the strong inflection and \n\t\t\tthe weak inflection. The mixed inflection is used after the indefinite \n\t\t\tarticle \"ein\" and after \"irgendein\" e.g. \"(irgend) ein kleines Kind\", \n\t\t\tafter \"kein\" or after possessive pronouns e.g. \"ihr kleines Kind\". \n\t\t\t(http://www.canoo.net/services/OnlineGrammar/Wort/Adjektiv/Deklinationstyp/Gemischt.html?MenuId=Word3132  20.11.06)\n\t\t\t\n\t\t\tMixed inflection is a characteristic of lexemes, not individual tokens.\n\t\t" ;
        <http://www.w3.org/2000/01/rdf-schema#subClassOf>
                <http://purl.org/olia/olia-top.owl#InflectionTypeFeature> ;
        <http://www.w3.org/2002/07/owl#versionInfo>
                "EAGLES" .

<http://purl.org/olia/olia-top.owl#EvidentialityFeature>
        a       <http://www.w3.org/2002/07/owl#Class> ;
        <http://www.w3.org/2000/01/rdf-schema#subClassOf>
                [ a       <http://www.w3.org/2002/07/owl#Restriction> ;
                  <http://www.w3.org/2002/07/owl#hasSelf>
                          true ;
                  <http://www.w3.org/2002/07/owl#onProperty>
                          <http://purl.org/olia/olia.owl#hasGender>
                ] .

<http://purl.org/olia/olia.owl#MiddleField>
        a       <http://www.w3.org/2002/07/owl#Class> ;
        <http://www.w3.org/2000/01/rdf-schema#comment>
                "\nIn a German clause, the finite verb can appear in three different positions: verb-second, \nverb-initial, and verb-final. Only in verb-final clauses the verb complex consisting of the\nfinite verb and non-finite verbal elements forms a unit. The discontinuous positioning\nof the verbal elements in verb-first and verb-second clauses is the traditional reason\nfor structuring German clauses into fields. The positions of the verbal elements form\nthe Satzklammer (sentence bracket) which divides the sentence into a Vorfeld (initial\nfield), a Mittelfeld (middle field), and a Nachfeld (final field). The Vorfeld and the\nMittelfeld are divided by the linke Satzklammer (left sentence bracket), which is the finite\nverb, the rechte Satzklammer (right sentence bracket) is the verb complex between the\nMittelfeld and the Nachfeld. \n(Telljohann et al. 2009, p.13)\n\t\t" ;
        <http://www.w3.org/2000/01/rdf-schema#subClassOf>
                <http://purl.org/olia/olia-top.owl#TopologicalField> .

<http://purl.org/olia/olia.owl#PerlativeCase>
        a       <http://www.w3.org/2002/07/owl#Class> ;
        <http://www.w3.org/2000/01/rdf-schema#comment>
                "\n\t\t\tPerlativeCase expresses that something moved 'through','across', \n\t\t\tor 'along' the referent of the noun that is marked (Blake 1998: \n\t\t\t38, 203).\n\t\t\t(http://purl.org/linguistics/gold/Perlative)\n\t\t" ;
        <http://www.w3.org/2000/01/rdf-schema#subClassOf>
                <http://purl.org/olia/olia-top.owl#CaseFeature> ;
        <http://www.w3.org/2002/07/owl#versionInfo>
                "http://purl.org/linguistics/gold/Perlative" .

<http://purl.org/olia/olia.owl#NonspecificArticle>
        a       <http://www.w3.org/2002/07/owl#Class> ;
        <http://www.w3.org/2000/01/rdf-schema#comment>
                "\n\t\t\t\"By ʻspecificʼ and ʻnon-specificʼ I intend the difference between the\n\t\t\ttwo readings of English indefinites like (3):\n\t\t\t\n\t\t\t(3) Iʼm looking for a deer.\n\t\t\t\n\t\t\tIn the specific reading there is a particular deer, say Bambi, that I am\n\t\t\tlooking for. In the non-specific reading I will be happy to find any deer.\n\t\t\tVon Heusinger (2002) likes the test in English of inserting ʻcertainʼ after the\n\t\t\tʻaʼ to fix the specific reading. In either reading of (3) a deer is being\n\t\t\tintroduced as a new discourse referent. This is opposed to ʻdefiniteʼ which\n\t\t\trequires a previous pragmatic instantiation as in ʻIʼm looking for the deer.ʼ\n\t\t\tIn English both the readings of (3) are indefinite. In Klallam, the specific\n\t\t\tdemonstratives are neither definite nor indefinite.\"\n\t\t\t(Montler, Timothy. 2007. Klallam demonstratives. Papers ICSNL XLVII. The 42nd International Conference on Salish and Neighbouring Language, pp. 409-425. University of British Columbia Working Papers in Linguistics, Volume 20; on specific vs. nonspecific determiners in Klallam, a Salish language, http://montler.net/papers/KlallamDemons.pdf)\n\t\t" ;
        <http://www.w3.org/2000/01/rdf-schema#label>
                "nonspecific article"@en , "nonspecific determiner"@en ;
        <http://www.w3.org/2000/01/rdf-schema#subClassOf>
                <http://purl.org/olia/olia.owl#Article> ;
        <http://www.w3.org/2002/07/owl#versionInfo>
                "introduced in analogy with SpecificArticle" .

<http://purl.org/olia/olia.owl#GraphicalSeparator>
        a       <http://www.w3.org/2002/07/owl#Class> ;
        <http://www.w3.org/2000/01/rdf-schema#comment>
                "Character string that appears between two written forms" ;
        <http://www.w3.org/2000/01/rdf-schema#isDefinedBy>
                "http://www.isocat.org/datcat/DC-1863" ;
        <http://www.w3.org/2000/01/rdf-schema#subClassOf>
                <http://purl.org/olia/olia.owl#Character> .

<http://purl.org/olia/olia.owl#Token>
        a       <http://www.w3.org/2002/07/owl#Class> ;
        <http://www.w3.org/2000/01/rdf-schema#comment>
                "\n                            Character string surrounded by separators.\n                                (Gil Francopoulo; http://www.isocat.org/datcat/DC-1403)\n                            " ;
        <http://www.w3.org/2000/01/rdf-schema#label>
                "token" ;
        <http://www.w3.org/2000/01/rdf-schema#subClassOf>
                <http://purl.org/olia/olia-top.owl#OrthographicEntity> ;
        <http://www.w3.org/2002/07/owl#versionInfo>
                "http://www.isocat.org/datcat/DC-1403" .

<http://purl.org/olia/olia.owl#Root>
        a       <http://www.w3.org/2002/07/owl#Class> ;
        <http://www.w3.org/2000/01/rdf-schema#comment>
                "\n                            base of a word\n                                (MIRACL & LSCA; http://www.isocat.org/datcat/DC-2231)\n                            " ;
        <http://www.w3.org/2000/01/rdf-schema#label>
                "root" ;
        <http://www.w3.org/2000/01/rdf-schema#subClassOf>
                <http://purl.org/olia/olia.owl#Morpheme> ;
        <http://www.w3.org/2002/07/owl#versionInfo>
                "http://www.isocat.org/datcat/DC-2231" .

<http://purl.org/olia/olia.owl#CloseParenthesis>
        a       <http://www.w3.org/2002/07/owl#Class> ;
        <http://www.w3.org/2000/01/rdf-schema#comment>
                "\n                            End of a parenthesis pair.\n                                (http://www.isocat.org/datcat/DC-1440)\n                            " ;
        <http://www.w3.org/2000/01/rdf-schema#label>
                "close parenthesis" ;
        <http://www.w3.org/2000/01/rdf-schema#subClassOf>
                <http://purl.org/olia/olia.owl#RightParentheticalPunctuation> ;
        <http://www.w3.org/2002/07/owl#versionInfo>
                "subClassOf partOfSpeech (dcif:conceptualDomain)" , "http://www.isocat.org/datcat/DC-1440" .

<http://purl.org/olia/olia.owl#PlaceNoun>
        a       <http://www.w3.org/2002/07/owl#Class> ;
        <http://www.w3.org/2000/01/rdf-schema#comment>
                "noun expressing a location, equivalent to ProperNoun and hasSemanticRole some LocationRole" ;
        <http://www.w3.org/2000/01/rdf-schema#isDefinedBy>
                "http://www.isocat.org/datcat/DC-3857" ;
        <http://www.w3.org/2000/01/rdf-schema#subClassOf>
                <http://purl.org/olia/olia.owl#ProperNoun> ;
        <http://www.w3.org/2002/07/owl#deprecated>
                true ;
        <http://www.w3.org/2002/07/owl#equivalentClass>
                [ a       <http://www.w3.org/2002/07/owl#Class> ;
                  <http://www.w3.org/2002/07/owl#intersectionOf>
                          ( <http://purl.org/olia/olia.owl#ProperNoun>
                            [ a       <http://www.w3.org/2002/07/owl#Restriction> ;
                              <http://www.w3.org/2002/07/owl#onProperty>
                                      <http://purl.org/olia/olia.owl#hasSemanticRole> ;
                              <http://www.w3.org/2002/07/owl#someValuesFrom>
                                      <http://purl.org/olia/olia.owl#LocationRole>
                            ]
                          )
                ] .

<http://purl.org/olia/olia.owl#CharacteristicAdjective>
        a       <http://www.w3.org/2002/07/owl#Class> ;
        <http://www.w3.org/2000/01/rdf-schema#comment>
                "It is an adjective, which expresses the character and feature of subject or an object, while modifying a noun.\n\t\t\t\n\t\t\tང་འ ་ ང ་ འ ག།\n\t\t\tShing-di rim du\n\t\t\t'The tree is tall'\n\t\t\t(http://panl10n.net/english/Outputs%20Phase%202/CCs/Bhutan/Papers/2007/0701/PartOfSpeech.pdf)" ;
        <http://www.w3.org/2000/01/rdf-schema#subClassOf>
                <http://purl.org/olia/olia.owl#Adjective> ;
        <http://www.w3.org/2002/07/owl#versionInfo>
                "adopted from Dzongkha tagset (Chungku et al. 2010, http://purl.org/olia/dzongkha.owl#CharacteristicAdjective)" .

<http://purl.org/olia/olia.owl#Transitive>
        a       <http://www.w3.org/2002/07/owl#Class> ;
        <http://www.w3.org/2000/01/rdf-schema#comment>
                "\n\t\t\tA predicate/verb that takes two arguments, e.g., English \"to kiss\", cf. van Valin and Lapolla (1997).\n\t\t" ;
        <http://www.w3.org/2000/01/rdf-schema#subClassOf>
                <http://purl.org/olia/olia-top.owl#ValencyFeature> ;
        <http://www.w3.org/2002/07/owl#versionInfo>
                "SUSANNE (Sampson 1995)" .

<http://purl.org/olia/olia.owl#DemonstrativeQuantifier>
        a       <http://www.w3.org/2002/07/owl#Class> ;
        <http://www.w3.org/2000/01/rdf-schema#comment>
                "In the Czech and Slovak MTE v4 specs, Numeral/Class=\"demonstrative\" are items meaning `this many/much', etc. Strictly speaking, they are pronumerals (pro-quantifiers), but traditional descriptions don't recognise such a category, so they are described variously as pronouns (because they contain a demonstrative element) or as numerals (because their syntactic distribution is that of numerals, or very close).\" (Ivan A Derzhanski, email 2010/06/11, http://purl.org/olia/mte/multext-east.owl#DemonstrativeQuantifier)" ;
        <http://www.w3.org/2000/01/rdf-schema#subClassOf>
                <http://purl.org/olia/olia.owl#ProQuantifier> ;
        <http://www.w3.org/2002/07/owl#versionInfo>
                "http://purl.org/olia/mte/multext-east.owl#DemonstrativeQuantifier" .

<http://purl.org/olia/olia.owl#IndefiniteMultiplicativeQuantifier>
        a       <http://www.w3.org/2002/07/owl#Class> ;
        <http://www.w3.org/2000/01/rdf-schema#comment>
                "A word indicating imprecise number of times something happened." ;
        <http://www.w3.org/2000/01/rdf-schema#isDefinedBy>
                "http://www.isocat.org/datcat/DC-3024 (IndefiniteMultiplicativeNumeral)" ;
        <http://www.w3.org/2000/01/rdf-schema#subClassOf>
                <http://purl.org/olia/olia.owl#IndefiniteQuantifier> .

<http://purl.org/olia/olia.owl#EmbeddedParticiple>
        a       <http://www.w3.org/2002/07/owl#Class> ;
        <http://www.w3.org/2000/01/rdf-schema#comment>
                "A participle is the head of the embedded construction. (http://languagelink.let.uu.nl/tds/onto/LinguisticOntology.owl#withParticipleAsHead)\n\t\t\tParticipial constructions are used as adjunct clauses in Old High German. As they lack a finite verb form they are kept separately from finite subordinate clauses. (http://purl.org/olia/tcodex.owl#ParticipialConstruction)" ;
        <http://www.w3.org/2000/01/rdf-schema#label>
                "participle construction" ;
        <http://www.w3.org/2000/01/rdf-schema#subClassOf>
                <http://purl.org/olia/olia.owl#NonFiniteEmbeddedConstruction> ;
        <http://www.w3.org/2002/07/owl#versionInfo>
                "http://languagelink.let.uu.nl/tds/onto/LinguisticOntology.owl#withParticipleAsHead, http://purl.org/olia/tcodex.owl#ParticipialConstruction" .

<http://purl.org/olia/olia.owl#hasMood>
        a       <http://www.w3.org/2002/07/owl#ObjectProperty> ;
        <http://www.w3.org/2000/01/rdf-schema#range>
                <http://purl.org/olia/olia-top.owl#MoodFeature> ;
        <http://www.w3.org/2000/01/rdf-schema#subPropertyOf>
                <http://purl.org/olia/olia.owl#hasModality> .

<http://purl.org/olia/olia.owl#NegativePronoun>
        a       <http://www.w3.org/2002/07/owl#Class> ;
        <http://www.w3.org/2000/01/rdf-schema#comment>
                "\n                            Pronoun used in a context of a negation or for expressing a negation.\n                                (http://www.isocat.org/datcat/DC-1925)\n                            " ;
        <http://www.w3.org/2000/01/rdf-schema#label>
                "negative pronoun" ;
        <http://www.w3.org/2000/01/rdf-schema#subClassOf>
                <http://purl.org/olia/olia.owl#IndefinitePronoun> ;
        <http://www.w3.org/2002/07/owl#versionInfo>
                "subClassOf pronoun (dcif:isA), reclassification as IndefinitePronoun follows EAGLES and STTS praxis" , "http://www.isocat.org/datcat/DC-1925" .

<http://purl.org/olia/olia.owl#CausalModality>
        a       <http://www.w3.org/2002/07/owl#Class> ;
        <http://www.w3.org/2000/01/rdf-schema#comment>
                "In Inuktitut, causality is expressed by verbal inflection. Causal mood signifies causal relationships in a sentence. (Nowak 1996, p.39)\n\t\t\n\t\tElke Nowak (1996), Transforming the images: Ergativity and transitivity in Inuktitut (Eskimo). Walter de Gruyter, Berlin.\n\t\t" ;
        <http://www.w3.org/2000/01/rdf-schema#subClassOf>
                <http://purl.org/olia/olia-top.owl#ModalityFeature> ;
        <http://www.w3.org/2002/07/owl#versionInfo>
                "Nowak (1996)" .

<http://purl.org/olia/olia.owl#TerminativeCase>
        a       <http://www.w3.org/2002/07/owl#Class> ;
        <http://www.w3.org/2000/01/rdf-schema#comment>
                "\n\t\t\tCase that indicates to what or where something ends.\n\t\t\t(http://www.isocat.org/datcat/DC-1401)\n\t\t\t\n\t\t\tTerminativeCase expresses the notion of something into but not further \n\t\t\tthan (ie, not through) the referent of the noun it marks. It has the \n\t\t\tmeaning 'into but not through'.\n\t\t\t(http://purl.org/linguistics/gold/TerminativeCase)\n\t\t" ;
        <http://www.w3.org/2000/01/rdf-schema#subClassOf>
                <http://purl.org/olia/olia-top.owl#CaseFeature> ;
        <http://www.w3.org/2002/07/owl#versionInfo>
                "http://purl.org/linguistics/gold/TerminativeCase, http://www.isocat.org/datcat/DC-1401" .

<http://purl.org/olia/olia.owl#ExclamativePoint>
        a       <http://www.w3.org/2002/07/owl#Class> ;
        <http://www.w3.org/2000/01/rdf-schema#comment>
                "\n                            Special sign (!) usually used in writing to mark exclamation.\n                                (http://www.isocat.org/datcat/DC-1441)\n                            " ;
        <http://www.w3.org/2000/01/rdf-schema#label>
                "exclamative point" ;
        <http://www.w3.org/2000/01/rdf-schema#subClassOf>
                <http://purl.org/olia/olia.owl#MainPunctuation> ;
        <http://www.w3.org/2002/07/owl#versionInfo>
                "subClassOf partOfSpeech (dcif:conceptualDomain)" , "http://www.isocat.org/datcat/DC-1441" , "MainPunctuation, not SentenceFinalPunctuation because of the Spanish inverted exclamation point (Chiarcos)" .

<http://purl.org/olia/olia.owl#PrepositionalPhrase>
        a       <http://www.w3.org/2002/07/owl#Class> ;
        <http://www.w3.org/2000/01/rdf-schema#comment>
                "\n\t\t\tA sequence of a preposition and its complement is a prepositional phrase. The complement of a preposition is usually\n\t\t\ta noun phrase (see examples 38 to 40), but may also be a clause or an adverb phrase. According to the categories\n\t\t\trecommended here, a prepositional phrase may be analysed further into preposition and noun phrase. The examples\n\t\t\tbelow demonstrate how this further analysis can be a recursive procedure.\n\n\t\t\t(38)  \t[PP en [NP sustitucion [PP de [NP los canales correspondientes [PP de [NP 50 baudios NP] PP] NP] PP] NP] PP].\n\t\t\t(39)  \t[NP Fairbanks NP] [VP hummed [NP a few bars NP] VP] [PP in [NP a voice [VP made resonant \n\t\t\t\t\t[PP by [NP the very weakness [PP of [NP his chest NP] PP] NP] PP] VP] NP] PP].\n\t\t\t(40)  \t[PP En [NP el caso [PP de [NP un sistema mixto [PP en [NP el \n\t\t\t\t\t[CL que [VP se utilicen [NP canales [PP con [NP tres velocidades \n\t\t\t\t\t[PP de [NP modulacion NP] PP] diferentes NP] PP] NP] VP] CL] NP] PP] NP] PP] NP] PP]\n\n\t\t\tIn a language such as Spanish, where a large proportion of the modification of nouns takes the form of a following\n\t\t\tpreposition de and another noun, this recursion is extremely prevalent, as in 40. In cases where the prepositional\n\t\t\tphrase is complemented by a one word noun phrase, it may be advantageous to leave the analysis at this point, rather\n\t\t\tthan continuing to analyse further by enclosing the complement (see also one-word constituents).\n\n\t\t\t(http://www.ilc.cnr.it/EAGLES96/segsasg1/node34.html#SECTION00052500000000000000)\n\t\t" ;
        <http://www.w3.org/2000/01/rdf-schema#subClassOf>
                <http://purl.org/olia/olia.owl#NounHeadedPhrase> ;
        <http://www.w3.org/2002/07/owl#versionInfo>
                "EAGLES" .

<http://purl.org/olia/olia.owl#DialectRegister>
        a       <http://www.w3.org/2002/07/owl#Class> ;
        <http://www.w3.org/2000/01/rdf-schema#comment>
                "\n                            Register that is specific to a dialect.\n                                (http://www.isocat.org/datcat/DC-1990)\n                            " ;
        <http://www.w3.org/2000/01/rdf-schema#label>
                "dialect register" ;
        <http://www.w3.org/2000/01/rdf-schema#subClassOf>
                <http://purl.org/olia/olia-top.owl#RegisterFeature> ;
        <http://www.w3.org/2002/07/owl#versionInfo>
                "subClassOf register (dcif:conceptualDomain)" , "http://www.isocat.org/datcat/DC-1990" .

<http://purl.org/olia/olia.owl#RomanNumeral>
        a       <http://www.w3.org/2002/07/owl#Class> ;
        <http://www.w3.org/2000/01/rdf-schema#comment>
                "Numeral expressed with roman digits." ;
        <http://www.w3.org/2000/01/rdf-schema#isDefinedBy>
                "http://www.isocat.org/datcat/DC-1936" ;
        <http://www.w3.org/2000/01/rdf-schema#subClassOf>
                <http://purl.org/olia/olia.owl#Numeral> , <http://purl.org/olia/olia.owl#String> .

<http://purl.org/olia/olia-top.owl#SentenceTypeFeature>
        a       <http://www.w3.org/2002/07/owl#Class> .

<http://purl.org/olia/olia.owl#Unique>
        a       <http://www.w3.org/2002/07/owl#Class> ;
        <http://www.w3.org/2000/01/rdf-schema#comment>
                "\n\t\tUnique approximates the linguistic concept \"Particle\".\n\t\tIt covers categories with unique or very small membership, \n\t\tsuch as negative particle, which are `unassigned' to any of the standard part-of-speech categories. \n\t\t(http://www.ilc.cnr.it/EAGLES96/annotate/node16.html#mp 19.09.06) \n\t" ;
        <http://www.w3.org/2000/01/rdf-schema#subClassOf>
                <http://purl.org/olia/olia-top.owl#MorphosyntacticCategory> ;
        <http://www.w3.org/2002/07/owl#versionInfo>
                "EAGLES top-level category Unique (U).\n\t\n\t\t\"The unique value (U) is applied to categories with a unique or\n\t\tvery small membership, such as negative particle, which are\n\t\t‘unassigned’ to any of the standard part-of-speech categories. The\n\t\tvalue unique cannot always be strictly applied, since (for example)\n\t\tGreek has three negative particles ... \n\t\tNo subcategories are recommended, although it is expected that\n\t\ttagsets for individual languages will need to identify such one-member\n\t\tword-classes as Negative particle, Existential particle, Infinitive\n\t\tmarker, etc\" (http://www.ilc.cnr.it/EAGLES96/annotate/node16.html)\n\t\n\t\tAccording to the EAGLES definition and examples, this seems to be closely related to \"particle\".\n\t\tParticles are uninflected function words, in a broader sense, everything which is not inflected is a \n\t\tparticle, i.e. including interjections, in GOLD, uninflected items such as adpositions, \n\t\tconjunctions and interjections are excluded: \"A particle is a partOfSpeech whose members \n\t\tdo not belong to one of the main classes of words, is invariable, and typically has grammatical \n\t\tor pragmatic meaning.\"\n\t\t\n\t\tThe EAGLES definition emphasizes the invariability of particles.\n\t" , "TODO: rename to Particle" .

<http://purl.org/olia/olia.owl#ConjunctionPhrase>
        a       <http://www.w3.org/2002/07/owl#Class> ;
        <http://www.w3.org/2000/01/rdf-schema#comment>
                "Multi-word conjunction\n\t\n\tBesides the usual and, or, but, etc., certain prepositions and subordinating conjunctions can be used as coordinating conjunctions. Multi-word coordinating conjunctions are labeled CONJP (see section 7 [Coordination]). ...\nCONJP — Conjunction Phrase. Used to mark certain “multi-word” conjunctions, such as as well as, instead of. \n(Bies et al. 1995)" ;
        <http://www.w3.org/2000/01/rdf-schema#subClassOf>
                <http://purl.org/olia/olia.owl#Phrase> , <http://purl.org/olia/olia.owl#Conjunction> ;
        <http://www.w3.org/2002/07/owl#versionInfo>
                "Penn bracketing guidelines, Bies et al. 1995" .

<http://purl.org/olia/olia.owl#SourceRole>
        a       <http://www.w3.org/2002/07/owl#Class> ;
        <http://www.w3.org/2000/01/rdf-schema#comment>
                "\n\t\tA source role instantiates the origin of an event or entity.\n\t\t(http://languagelink.let.uu.nl/tds/onto/LinguisticOntology.owl#sourceRole)\n\t\t" ;
        <http://www.w3.org/2000/01/rdf-schema#subClassOf>
                <http://purl.org/olia/olia.owl#DirectionRole> ;
        <http://www.w3.org/2002/07/owl#versionInfo>
                "http://languagelink.let.uu.nl/tds/onto/LinguisticOntology.owl#sourceRole" .

<http://purl.org/olia/olia.owl#RecipientRole>
        a       <http://www.w3.org/2002/07/owl#Class> ;
        <http://www.w3.org/2000/01/rdf-schema#comment>
                "\n\t\t\tA recipient instantiates the role of an entity (usually animate) who \n\t\t\trecieves an entity in some way from the event.\n\t\t\t<p>\n\t\t\tPrototypically “recieve” here means “to take in one’s hand, or into \n\t\t\tone’s possession (something held out or offered by another); to take \n\t\t\tdelivery of (a thing) from another” in some way. (OED)\n\t\t\t</p>\n\t\t\t(http://languagelink.let.uu.nl/tds/onto/LinguisticOntology.owl#recipientRole)\n\t\t" ;
        <http://www.w3.org/2000/01/rdf-schema#subClassOf>
                <http://purl.org/olia/olia.owl#UndergoerMacroRole> ;
        <http://www.w3.org/2002/07/owl#versionInfo>
                "http://languagelink.let.uu.nl/tds/onto/LinguisticOntology.owl#recipientRole" .

<http://purl.org/olia/olia.owl#CompletiveAspect>
        a       <http://www.w3.org/2002/07/owl#Class> ;
        <http://www.w3.org/2000/01/rdf-schema#comment>
                "To do something thoroughly and to completion." ;
        <http://www.w3.org/2000/01/rdf-schema#isDefinedBy>
                "http://www.isocat.org/datcat/DC-5474" ;
        <http://www.w3.org/2000/01/rdf-schema#label>
                "completive" ;
        <http://www.w3.org/2000/01/rdf-schema#subClassOf>
                <http://purl.org/olia/olia-top.owl#AspectFeature> .

<http://purl.org/olia/olia.owl#IntertranslativeCase>
        a       <http://www.w3.org/2002/07/owl#Class> ;
        <http://www.w3.org/2000/01/rdf-schema#comment>
                "\n\t\t\tIntertranslativeCase expresses the notion of something moving along \n\t\t\ta trajectory between the referent of the noun it marks. It has the \n\t\t\tmeaning 'along the in between.\n\t\t\t(http://purl.org/linguistics/gold/Intertranslative)\n\t\t" ;
        <http://www.w3.org/2000/01/rdf-schema#subClassOf>
                <http://purl.org/olia/olia-top.owl#CaseFeature> ;
        <http://www.w3.org/2002/07/owl#versionInfo>
                "http://purl.org/linguistics/gold/Intertranslative" .

<http://purl.org/olia/olia-top.owl#EmphasisFeature>
        a       <http://www.w3.org/2002/07/owl#Class> ;
        <http://www.w3.org/2000/01/rdf-schema#subClassOf>
                [ a       <http://www.w3.org/2002/07/owl#Restriction> ;
                  <http://www.w3.org/2002/07/owl#hasSelf>
                          true ;
                  <http://www.w3.org/2002/07/owl#onProperty>
                          <http://purl.org/olia/olia.owl#hasEmphasis>
                ] ;
        <http://www.w3.org/2002/07/owl#versionInfo>
                "in EAGLES and MULTEXT-East restricted to pronouns, in ILPOSTS applicable to many different WordClasses, hence modelled as an independent feature, cf. http://purl.org/olia/ilposts.owl#Emphasis" .

<http://purl.org/olia/olia.owl#ComitativeRole>
        a       <http://www.w3.org/2002/07/owl#Class> ;
        <http://www.w3.org/2000/01/rdf-schema#comment>
                "\n\t\t\tComitative carries the meaning 'with' \n\t\t\tor 'accompanied by' (Anderson, Stephen 1985: 186; Pei and Gaynor 1954: \n\t\t\t42;Dixon, R. 1972: 12; Gove, et al. 1966: 455).\n\t\t\t(http://purl.org/linguistics/gold/Comitative)\n\t\t\t\n\t\t\tComitative applies to an animate entity that accompanies a participant of the\n\t\t\taction. (Dipper et al. 2007,  §5.3.12)\n\t\t" ;
        <http://www.w3.org/2000/01/rdf-schema#subClassOf>
                <http://purl.org/olia/olia-top.owl#SemanticRole> ;
        <http://www.w3.org/2002/07/owl#versionInfo>
                "TODO: Check whether to be merged with ComitativeCase" , "\n\t\t\tadded in conformance with TIGER edge labels, this is explicitly not defined as a grammatical case\n\t\t" .

<http://purl.org/olia/olia.owl#SimpleFuture>
        a       <http://www.w3.org/2002/07/owl#Class> ;
        <http://www.w3.org/2000/01/rdf-schema#comment>
                "\n\t\t\tFutureTense locates the situation in question after the present moment, \n\t\t\twith no specification on the distance in time.\n\t\t\t(adapted from the definition of http://purl.org/linguistics/gold/Past)\n\t\t" ;
        <http://www.w3.org/2000/01/rdf-schema#subClassOf>
                <http://purl.org/olia/olia.owl#Future> ;
        <http://www.w3.org/2002/07/owl#versionInfo>
                "http://purl.org/linguistics/gold/Future, cf. http://purl.org/linguistics/gold/Past" .

<http://purl.org/olia/olia.owl#PeriodicAdjective>
        a       <http://www.w3.org/2002/07/owl#Class> ;
        <http://www.w3.org/2000/01/rdf-schema#comment>
                "It is an adjective, which expresses the time or period of the circumstances, while modifying a noun.\n\t\t\t\n\t\t\tན་ ང་ ང་ ་ ལ་ ་ འ ་ །\n\t\t\tNahing Nga chigyel-lu joyi\n\t\t\t'I went abroad last year'\n\t\t\t(http://panl10n.net/english/Outputs%20Phase%202/CCs/Bhutan/Papers/2007/0701/PartOfSpeech.pdf)" ;
        <http://www.w3.org/2000/01/rdf-schema#subClassOf>
                <http://purl.org/olia/olia.owl#Adjective> ;
        <http://www.w3.org/2002/07/owl#versionInfo>
                "http://purl.org/olia/dzongkha.owl#PeriodicAdjective" .

<http://purl.org/olia/olia.owl#Apposition>
        a       <http://www.w3.org/2002/07/owl#Class> ;
        <http://www.w3.org/2000/01/rdf-schema#comment>
                "Apposition is a relation between two phrases: (1) the nucleus phrase and (2) an appositive phrase,\ngenerally set o by punctuation, which modi es the nucleus phrase. An example of apposition is given in\n(@11).\n\n(11) Ryukichi Imai, Japan’s ambassador to Mexico, agrees that Mexico may be too eager.\n\nHere, Ryukichi Imai is the nucleus phrase, and the phrase enclosed in commas, Japan’s ambassador to\nMexico, is the appositive.\nInstances of apposition should be represented as adjunction structures (see Section 3.1). \n(Santorini 1991)" ;
        <http://www.w3.org/2000/01/rdf-schema#subClassOf>
                <http://purl.org/olia/olia.owl#Adjunction> ;
        <http://www.w3.org/2002/07/owl#versionInfo>
                "added in accordance with TIGER, definition according to PTB Bracketing Guidelines (Santorini 1991)" .

<http://purl.org/olia/olia.owl#PossessiveArticle>
        a       <http://www.w3.org/2002/07/owl#Class> ;
        <http://www.w3.org/2000/01/rdf-schema#comment>
                "In Romanian,  the possessive article (also called genitival article) is an element in the structure of the possessive pronoun, of the ordinal numeral (e.g. al meu (mine) and al treilea (the third)), and of the indefinite genitive forms of the nouns (e.g. capitol al cărţii (chapter of the book)), e.g., -al/al, a/al, ai/al, al, ale/al, alor/al (http://purl.org/olia/mte/multext-east.owl#PossessiveArticle)" ;
        <http://www.w3.org/2000/01/rdf-schema#subClassOf>
                <http://purl.org/olia/olia.owl#Article> ;
        <http://www.w3.org/2002/07/owl#versionInfo>
                "http://purl.org/olia/mte/multext-east.owl#PossessiveArticle" , "not to be confused with PoessiveDeterminer" .

<http://purl.org/olia/olia.owl#hasInflectionType>
        a       <http://www.w3.org/2002/07/owl#ObjectProperty> ;
        <http://www.w3.org/2000/01/rdf-schema#range>
                <http://purl.org/olia/olia-top.owl#InflectionTypeFeature> ;
        <http://www.w3.org/2000/01/rdf-schema#subPropertyOf>
                <http://purl.org/olia/system.owl#hasFeature> .

<http://purl.org/olia/olia.owl#LocationAdverb>
        a       <http://www.w3.org/2002/07/owl#Class> ;
        <http://www.w3.org/2000/01/rdf-schema#subClassOf>
                <http://purl.org/olia/olia.owl#Adverb> ;
        <http://www.w3.org/2002/07/owl#deprecated>
                true ;
        <http://www.w3.org/2002/07/owl#equivalentClass>
                [ a       <http://www.w3.org/2002/07/owl#Class> ;
                  <http://www.w3.org/2002/07/owl#intersectionOf>
                          ( <http://purl.org/olia/olia.owl#Adverb>
                            [ a       <http://www.w3.org/2002/07/owl#Restriction> ;
                              <http://www.w3.org/2002/07/owl#onProperty>
                                      <http://purl.org/olia/olia.owl#hasSemanticRole> ;
                              <http://www.w3.org/2002/07/owl#someValuesFrom>
                                      <http://purl.org/olia/olia.owl#LocationRole>
                            ]
                          )
                ] ;
        <http://www.w3.org/2002/07/owl#versionInfo>
                "ILPOSTS, http://purl.org/olia/ilposts.owl#LocationAdverb\n\t\t\t\t\tDEPRECATED: equivalent to Adverb and hasSemanticRole some LocationRole\n\t\t" .

<http://purl.org/olia/olia.owl#ObjectControl>
        a       <http://www.w3.org/2002/07/owl#Class> ;
        <http://www.w3.org/2000/01/rdf-schema#comment>
                "Indicates the object of the main clause is also the (omitted) object of the subclause (http://www.lexinfo.net/ontology/2.0/lexinfo#ObjectControl)"@en ;
        <http://www.w3.org/2000/01/rdf-schema#subClassOf>
                <http://purl.org/olia/olia.owl#Control> ;
        <http://www.w3.org/2002/07/owl#versionInfo>
                "http://www.lexinfo.net/ontology/2.0/lexinfo#ObjectControl" .

<http://purl.org/olia/olia.owl#QuestionWord>
        a       <http://www.w3.org/2002/07/owl#Class> ;
        <http://www.w3.org/2000/01/rdf-schema#comment>
                "A proform that is used in questions to stand for the item questioned." ;
        <http://www.w3.org/2000/01/rdf-schema#isDefinedBy>
                "http://www.isocat.org/datcat/DC-4205" ;
        <http://www.w3.org/2000/01/rdf-schema#label>
                "question word" ;
        <http://www.w3.org/2000/01/rdf-schema#subClassOf>
                <http://purl.org/olia/olia.owl#Lexeme> ;
        <http://www.w3.org/2002/07/owl#deprecated>
                true ;
        <http://www.w3.org/2002/07/owl#equivalentClass>
                [ a       <http://www.w3.org/2002/07/owl#Class> ;
                  <http://www.w3.org/2002/07/owl#intersectionOf>
                          ( <http://purl.org/olia/olia.owl#Lexeme>
                            [ a       <http://www.w3.org/2002/07/owl#Restriction> ;
                              <http://www.w3.org/2002/07/owl#onProperty>
                                      <http://purl.org/olia/olia.owl#hasModality> ;
                              <http://www.w3.org/2002/07/owl#someValuesFrom>
                                      <http://purl.org/olia/olia.owl#InterrogativeModality>
                            ]
                          )
                ] ;
        <http://www.w3.org/2002/07/owl#versionInfo>
                "deprecated, as merely a shorthand for Lexeme and hasModality some InterrogativeModality" .

<http://purl.org/olia/olia.owl#CliticElement>
        a       <http://www.w3.org/2002/07/owl#Class> ;
        <http://www.w3.org/2000/01/rdf-schema#comment>
                "Note that Clitic covers only one aspect of the original MULTEXT-East (and ISOcat) definitions of cliticness, i.e., that an element is a clitic" ;
        <http://www.w3.org/2000/01/rdf-schema#label>
                "cliticness" ;
        <http://www.w3.org/2000/01/rdf-schema#subClassOf>
                <http://purl.org/olia/olia.owl#Morpheme> ;
        <http://www.w3.org/2002/07/owl#versionInfo>
                "http://www.isocat.org/datcat/DC-1903 (cliticness), http://purl.org/olia/mte/multext-east.owl#Cliticness" .

<http://purl.org/olia/olia.owl#ContlativeCase>
        a       <http://www.w3.org/2002/07/owl#Class> ;
        <http://www.w3.org/2000/01/rdf-schema#comment>
                "\n\t\t\tContlativeCase expresses that  the referent of the noun it marks \n\t\t\tis the location in the vicinity of which another referent is moving. \n\t\t\tIt has the meaning 'in the vicinity of'.\n\t\t\t(http://purl.org/linguistics/gold/Contlative)\n\t\t" ;
        <http://www.w3.org/2000/01/rdf-schema#subClassOf>
                <http://purl.org/olia/olia-top.owl#CaseFeature> ;
        <http://www.w3.org/2002/07/owl#versionInfo>
                "http://purl.org/linguistics/gold/Contlative" .

<http://purl.org/olia/olia-top.owl#CoordTypeFeature>
        a       <http://www.w3.org/2002/07/owl#Class> ;
        <http://www.w3.org/2000/01/rdf-schema#subClassOf>
                [ a       <http://www.w3.org/2002/07/owl#Restriction> ;
                  <http://www.w3.org/2002/07/owl#hasSelf>
                          true ;
                  <http://www.w3.org/2002/07/owl#onProperty>
                          <http://purl.org/olia/olia.owl#hasCoordType>
                ] ;
        <http://www.w3.org/2002/07/owl#deprecated>
                true ;
        <http://www.w3.org/2002/07/owl#versionInfo>
                "DEPRECATED: reimplemented as class hierarchy" .

<http://purl.org/olia/olia.owl#SimplePreposition>
        a       <http://www.w3.org/2002/07/owl#Class> ;
        <http://www.w3.org/2000/01/rdf-schema#comment>
                "\n                            Preposition that is a pure simple word in contrast with the notion of fused preposition.\n                                (http://www.isocat.org/datcat/DC-1900)\n                            " ;
        <http://www.w3.org/2000/01/rdf-schema#label>
                "simple preposition" ;
        <http://www.w3.org/2000/01/rdf-schema#subClassOf>
                <http://purl.org/olia/olia.owl#Preposition> ;
        <http://www.w3.org/2002/07/owl#versionInfo>
                "subClassOf preposition (dcif:isA)" , "http://www.isocat.org/datcat/DC-1900" .

<http://purl.org/olia/olia.owl#CloseSquareBracket>
        a       <http://www.w3.org/2002/07/owl#Class> ;
        <http://www.w3.org/2000/01/rdf-schema#comment>
                "]\n*RSB*\nRight square bracket\n(Santorini 1991)" ;
        <http://www.w3.org/2000/01/rdf-schema#subClassOf>
                <http://purl.org/olia/olia.owl#RightParentheticalPunctuation> ;
        <http://www.w3.org/2002/07/owl#versionInfo>
                "PTB bracketing guidelines, Santorini 1991" .

<http://purl.org/olia/olia.owl#Text>
        a       <http://www.w3.org/2002/07/owl#Class> ;
        <http://www.w3.org/2000/01/rdf-schema#comment>
                "\n                            Series of sentences expressed in a natural language.\n                                (Gil Francopoulo; http://www.isocat.org/datcat/DC-1847)\n                            " ;
        <http://www.w3.org/2000/01/rdf-schema#label>
                "text" ;
        <http://www.w3.org/2000/01/rdf-schema#subClassOf>
                <http://purl.org/olia/olia-top.owl#OrthographicEntity> ;
        <http://www.w3.org/2002/07/owl#versionInfo>
                "http://www.isocat.org/datcat/DC-1847" .

<http://purl.org/olia/olia.owl#PresentativePronoun>
        a       <http://www.w3.org/2002/07/owl#Class> ;
        <http://www.w3.org/2000/01/rdf-schema#comment>
                "pronoun that identify the current locative or temporal situation" ;
        <http://www.w3.org/2000/01/rdf-schema#isDefinedBy>
                "http://www.isocat.org/datcat/DC-3015" ;
        <http://www.w3.org/2000/01/rdf-schema#subClassOf>
                <http://purl.org/olia/olia.owl#Pronoun> ;
        <http://www.w3.org/2002/07/owl#versionInfo>
                "Should be redefined in terms of deixis" .

<http://purl.org/olia/olia.owl#hasSeparability>
        a       <http://www.w3.org/2002/07/owl#ObjectProperty> ;
        <http://www.w3.org/2000/01/rdf-schema#range>
                <http://purl.org/olia/olia-top.owl#SeparabilityFeature> ;
        <http://www.w3.org/2000/01/rdf-schema#subPropertyOf>
                <http://purl.org/olia/system.owl#hasFeature> .

<http://purl.org/olia/olia.owl#NumeralBoth>
        a       <http://www.w3.org/2002/07/owl#Class> ;
        <http://www.w3.org/2000/01/rdf-schema#comment>
                "Numeric value for two." ;
        <http://www.w3.org/2000/01/rdf-schema#isDefinedBy>
                "http://www.isocat.org/datcat/DC-1938" ;
        <http://www.w3.org/2000/01/rdf-schema#subClassOf>
                <http://purl.org/olia/olia.owl#Numeral> ;
        <http://www.w3.org/2002/07/owl#deprecated>
                true ;
        <http://www.w3.org/2002/07/owl#versionInfo>
                "The ISOcat definition entails that this just represents the value of \"2\". I guess, this is not true, but that this Numeral is actually a DualQuantifier (and should be renamed as such), otherwise, it should be eliminated" .

<http://purl.org/olia/olia.owl#hasOwnerPerson>
        a       <http://www.w3.org/2002/07/owl#ObjectProperty> ;
        <http://www.w3.org/2000/01/rdf-schema#comment>
                "\n                            Indication concerning the person that ownes something.\n                                (http://www.isocat.org/datcat/DC-1929)\n                            " ;
        <http://www.w3.org/2000/01/rdf-schema#label>
                "owner person" ;
        <http://www.w3.org/2000/01/rdf-schema#range>
                <http://purl.org/olia/olia-top.owl#PersonFeature> ;
        <http://www.w3.org/2000/01/rdf-schema#subPropertyOf>
                <http://purl.org/olia/system.owl#hasFeature> ;
        <http://www.w3.org/2002/07/owl#versionInfo>
                "does not entail hasPerson: hasPerson pertains to agreement" , "http://www.isocat.org/datcat/DC-1929" .

<http://purl.org/olia/olia.owl#ContrastiveParticle>
        a       <http://www.w3.org/2002/07/owl#Class> ;
        <http://www.w3.org/2000/01/rdf-schema#comment>
                "Contrastive particle, e.g., (one of the uses of) Urdu tô: \n\t\t\t\n\t\t\tvo urdû parhê gâ\n\t\t\t\"He will study Urdu.\" (simple statement)\n\n\t\t\tvo tô urdû parhê gâ\n\t\t\t\"HE will study Urdu.\" (Contrast: the other students may not.)\n\n\t\t\t(Schmidt 1999, p. 232, see http://purl.org/olia/emille.owl#ContrastiveEmphaticParticle)\n\t\t" ;
        <http://www.w3.org/2000/01/rdf-schema#subClassOf>
                <http://purl.org/olia/olia.owl#Particle> ;
        <http://www.w3.org/2002/07/owl#versionInfo>
                "adopted from EMILLE, http://purl.org/olia/emille.owl#ContrastiveEmphaticParticle, note: there may be contrastive particles that are not emphatic" .

<http://purl.org/olia/olia.owl#Comparative>
        a       <http://www.w3.org/2002/07/owl#Class> ;
        <http://www.w3.org/2000/01/rdf-schema#comment>
                "\n\t\t\tThe comparative is the form of an adjective or adverb which denotes \n\t\t\tthe degree or grade by which a person, thing, or other entity has a \n\t\t\tproperty or quality greater or less in extent than that of another. \n\t\t\tIn English the structure of a comparative consists normally of the \n\t\t\tpositive form of the adjective or adverb, plus the suffix -er, or \n\t\t\t(especially in the case of longer words) the modifier \"more\" (or \n\t\t\t\"less\") before the adjective or adverb. The form is usually completed \n\t\t\tby \"than\" and the noun which is being compared, e.g. \"he is taller \n\t\t\tthan his father is\", or \"the village is less picturesque than the \n\t\t\ttown near by is\". (http://en.wikipedia.org/wiki/Comparative  17.11.06)\n\t\t" ;
        <http://www.w3.org/2000/01/rdf-schema#subClassOf>
                <http://purl.org/olia/olia-top.owl#DegreeFeature> ;
        <http://www.w3.org/2002/07/owl#versionInfo>
                "EAGLES, http://www.isocat.org/datcat/DC-1421" .

<http://purl.org/olia/olia.owl#Formula>
        a       <http://www.w3.org/2002/07/owl#Class> ;
        <http://www.w3.org/2000/01/rdf-schema#comment>
                "\n      A formula (mathematical formulae) is a text word which lies outside the traditionally \n      accepted range of grammatical classes, it occurs quite commonly in many texts and very \n      commonly in some. (http://www.ilc.cnr.it/EAGLES96/annotate/node16.html#mr 19.09.06)" ;
        <http://www.w3.org/2000/01/rdf-schema#subClassOf>
                <http://purl.org/olia/olia.owl#Residual> ;
        <http://www.w3.org/2002/07/owl#versionInfo>
                "EAGLES category Residual with the attribute Type=\"Formula\"." .

<http://purl.org/olia/olia.owl#CausativeVoice>
        a       <http://www.w3.org/2002/07/owl#Class> ;
        <http://www.w3.org/2000/01/rdf-schema#comment>
                "voice where the subject causes someone or something else to do or be something" ;
        <http://www.w3.org/2000/01/rdf-schema#isDefinedBy>
                "http://www.isocat.org/datcat/DC-3847" ;
        <http://www.w3.org/2000/01/rdf-schema#subClassOf>
                <http://purl.org/olia/olia-top.owl#VoiceFeature> .

<http://purl.org/olia/olia.owl#HangingTopic>
        a       <http://www.w3.org/2002/07/owl#Class> ;
        <http://www.w3.org/2000/01/rdf-schema#comment>
                "HangingTopic constructions are closely related to LeftDislocation. \n\t\t\tUnlike LeftDislocation, the dislocated element and its resuming pronoun do not \n\t\t\tnecessarily agree in case, number and gender. (Petrova and Odebrecht 2011, http://purl.org/olia/tcodex.owl#HangingTopic)" ;
        <http://www.w3.org/2000/01/rdf-schema#label>
                "hanging topic" ;
        <http://www.w3.org/2000/01/rdf-schema#subClassOf>
                <http://purl.org/olia/olia.owl#Fronting> ;
        <http://www.w3.org/2002/07/owl#versionInfo>
                "http://purl.org/olia/tcodex.owl#HangingTopic" .

<http://purl.org/olia/olia.owl#AdjectivalAdverb>
        a       <http://www.w3.org/2002/07/owl#Class> ;
        <http://www.w3.org/2000/01/rdf-schema#comment>
                "An adjectival adverb is an adverb that is formally identical to an adjective.<br/>\t\t\n\t\t\tMULTEXT-East Adverb/Type=\"adjectival\" (Serbian, Macedonian, Bulgarian)<br/>\n\t\t\tBulgarian AdjectivalAdverbs have the same form as adjectives in Gender = neuter, Person = 3, Number = singular. (MTE v4, http://purl.org/olia/mte/multext-east.owl#AdjectivalAdverb)" ;
        <http://www.w3.org/2000/01/rdf-schema#subClassOf>
                <http://purl.org/olia/olia.owl#Adverb> ;
        <http://www.w3.org/2002/07/owl#versionInfo>
                "http://purl.org/olia/mte/multext-east.owl#AdjectivalAdverb" .

<http://purl.org/olia/olia.owl#EmbeddedInfinitive>
        a       <http://www.w3.org/2002/07/owl#Class> ;
        <http://www.w3.org/2000/01/rdf-schema#comment>
                "\n\t\t\tAn infinitive is the head of the embedded construction. (http://languagelink.let.uu.nl/tds/onto/LinguisticOntology.owl#withInfinitiveAsHead)\n\t\t\t\n\t\t\tInfinitival relatives. See section 14 [Infinitives] for more information. \n\t\n\t  (NP (NP a movie)\n\t      (SBAR (WHNP-1 0)\n\t            (S (NP-SBJ *)\n\t               (VP to\n\t                   (VP see\n\t                       (NP *T*-1))))))\n\t(Bies et al. 1995)\n\t\t" ;
        <http://www.w3.org/2000/01/rdf-schema#label>
                "infinitival clause" ;
        <http://www.w3.org/2000/01/rdf-schema#subClassOf>
                <http://purl.org/olia/olia.owl#NonFiniteEmbeddedConstruction> ;
        <http://www.w3.org/2002/07/owl#versionInfo>
                "http://languagelink.let.uu.nl/tds/onto/LinguisticOntology.owl#withInfinitiveAsHead, http://purl.org/olia/tcodex.owl#InfinitivalClause" .

<http://purl.org/olia/olia.owl#ExperiencerRole>
        a       <http://www.w3.org/2002/07/owl#Class> ;
        <http://www.w3.org/2000/01/rdf-schema#comment>
                "\n\t\t\tAn experiencer instantiates the role of an entity (usually animate) who \n\t\t\ttakes the event in through sensory means in some way.\n\t\t\t(http://languagelink.let.uu.nl/tds/onto/LinguisticOntology.owl#experiencerRole)\n\t\t" ;
        <http://www.w3.org/2000/01/rdf-schema#subClassOf>
                <http://purl.org/olia/olia.owl#UndergoerMacroRole> ;
        <http://www.w3.org/2002/07/owl#versionInfo>
                "\n\t\t\thttp://languagelink.let.uu.nl/tds/onto/LinguisticOntology.owl#experiencerRole, \n\t\t\toriginally a subconcept of UndergoerMacroRole\n\t\t" .

<http://purl.org/olia/olia.owl#Apocope>
        a       <http://www.w3.org/2002/07/owl#Class> ;
        <http://www.w3.org/2000/01/rdf-schema#comment>
                "\n\t\t\tdeletion of the final element in a word\n\t\t\t(http://www.isocat.org/datcat/DC-2254)\n\t\t" ;
        <http://www.w3.org/2000/01/rdf-schema#label>
                "apocopate" , "apocope" ;
        <http://www.w3.org/2000/01/rdf-schema#subClassOf>
                <http://purl.org/olia/olia-top.owl#PhonologicalProcess> ;
        <http://www.w3.org/2002/07/owl#versionInfo>
                "http://www.isocat.org/datcat/DC-2254" .

<http://purl.org/olia/olia-top.owl#RegisterFeature>
        a       <http://www.w3.org/2002/07/owl#Class> .

<http://purl.org/olia/olia.owl#NumeralModifier>
        a       <http://www.w3.org/2002/07/owl#Class> ;
        <http://www.w3.org/2000/01/rdf-schema#comment>
                "\n\t\t\tA nominal is modified by a numeral.\n\t\t\t(http://languagelink.let.uu.nl/tds/onto/LinguisticOntology.owl#numeralModifier)\n\t\t" ;
        <http://www.w3.org/2000/01/rdf-schema#subClassOf>
                <http://purl.org/olia/olia.owl#AdnominalConstituent> ;
        <http://www.w3.org/2002/07/owl#versionInfo>
                "http://languagelink.let.uu.nl/tds/onto/LinguisticOntology.owl#numeralModifier" .

<http://purl.org/olia/olia.owl#VegetableGender>
        a       <http://www.w3.org/2002/07/owl#Class> ;
        <http://www.w3.org/2000/01/rdf-schema#comment>
                "Vegetable gender refers to inanimates and exists\n                        in some four-way gender systems, e.g., masculine, feminine, neuter, and\n                        vegetable as in Bininj Gun-wok [Evans 2003: 202]." ;
        <http://www.w3.org/2000/01/rdf-schema#isDefinedBy>
                "http://www.isocat.org/datcat/DC-3541" ;
        <http://www.w3.org/2000/01/rdf-schema#subClassOf>
                <http://purl.org/olia/olia.owl#InanimateGender> .

<http://purl.org/olia/olia.owl#PreferredEvaluative>
        a       <http://www.w3.org/2002/07/owl#Class> ;
        <http://www.w3.org/2000/01/rdf-schema#comment>
                "An evaluative property of a noun that indicates\n                        the speaker regards the person or object being referred to with favor or\n                        admiration." ;
        <http://www.w3.org/2000/01/rdf-schema#isDefinedBy>
                "http://www.isocat.org/datcat/DC-3416" ;
        <http://www.w3.org/2000/01/rdf-schema#subClassOf>
                <http://purl.org/olia/olia-top.owl#EvaluativeFeature> .

<http://purl.org/olia/olia.owl#NonAgentiveVerb>
        a       <http://www.w3.org/2002/07/owl#Class> ;
        <http://www.w3.org/2000/01/rdf-schema#comment>
                "\n\t\tA non-agentive verb is a type of verb, which indicates an action without the doer.\n\t\t\n\t\tExample:\n\t\tང་མ་ འ ར་ ས།\n\t\t'lungma phur-dä\n\t\t'A wind is blowing'\n\t\t(http://panl10n.net/english/Outputs%20Phase%202/CCs/Bhutan/Papers/2007/0701/PartOfSpeech.pdf)\n\t\t" ;
        <http://www.w3.org/2000/01/rdf-schema#subClassOf>
                <http://purl.org/olia/olia.owl#MainVerb> ;
        <http://www.w3.org/2002/07/owl#versionInfo>
                "adopted from Dzongkha tagset (Chungku et al. 2010, http://purl.org/olia/dzongkha.owl#NonAgentiveVerb" .

<http://purl.org/olia/olia.owl#Gerund>
        a       <http://www.w3.org/2002/07/owl#Class> ;
        <http://www.w3.org/2000/01/rdf-schema#comment>
                "\n    \tproperty for a non-finite form of a verb other than the infinitive.\n    \t(http://www.isocat.org/datcat/DC-2243)\n    \t\n\t A gerund is a kind of verbal noun that exists in some languages. In today's English, \n\t gerunds are nouns built from a verb with an '-ing' suffix. They can be used as the \n\t subject of a sentence, an object, or an object of preposition. They can also be used \n\t to complement a subject. Often, gerunds exist side-by-side with nouns that come from \n\t the same root but the gerund and the common noun have different shades of meaning.\n\t(http://en.wikipedia.org/wiki/Gerund, http://en.wikibooks.org/wiki/English:Gerund 19.09.06)\n\n\tThe term _gerund_ is ambiguous: with respect  to Latin, in whose grammatical tradition it originates, it refers to a  deverbal noun, and is needed in this function for Polish as well; in  descriptions of some other languages, however, it has been used for an  adverbial participle.  \n\tThe two meanings have nothing in common, except  that the English _ing_-form can translate both. (Ivan A Derzhanski, email 2010/06/09)\n\tHere, it is assumed that Gerund refers only to deverbal nouns, cf. NominalNonfiniteVerb in the IIIT tagset (http://purl.org/olia/iiit.owl#NominalNonFiniteVerb)\n    " ;
        <http://www.w3.org/2000/01/rdf-schema#subClassOf>
                <http://purl.org/olia/olia.owl#NonFiniteVerb> ;
        <http://www.w3.org/2002/07/owl#versionInfo>
                "EAGLES NonFiniteVerb with VerbForm=\"Gerund\"; http://www.isocat.org/datcat/DC-2243 (gerundive)" , "cf. ILPOSTS NominalParticiple, for Indian languages, there in contrast with AdjectivalParticiple, AdverbialParticiple and ConditionalParticiple, but no definition provided.\n\t\t\t(http://purl.org/olia/ilposts.owl#NominalParticiple)" .

<http://purl.org/olia/olia.owl#BeAuxiliary>
        a       <http://www.w3.org/2002/07/owl#Class> ;
        <http://www.w3.org/2000/01/rdf-schema#comment>
                "\n                            Verb used to link the subject of a sentence and its noun or adjective complement or complementing phrase in certain languages. This verb could be used also to form the passive voice.\n                                (www.wordreference.com/English/definition.asp?en=be -> 4); http://www.isocat.org/datcat/DC-1246)\n                            " ;
        <http://www.w3.org/2000/01/rdf-schema#label>
                "be" ;
        <http://www.w3.org/2000/01/rdf-schema#subClassOf>
                <http://purl.org/olia/olia.owl#StrictAuxiliaryVerb> ;
        <http://www.w3.org/2002/07/owl#versionInfo>
                "http://www.isocat.org/datcat/DC-1246" , "subClassOf partOfSpeech (dcif:conceptualDomain)" .

<http://purl.org/olia/olia.owl#hasStrength>
        a       <http://www.w3.org/2002/07/owl#ObjectProperty> ;
        <http://www.w3.org/2000/01/rdf-schema#domain>
                <http://purl.org/olia/olia.owl#PronounOrDeterminer> ;
        <http://www.w3.org/2000/01/rdf-schema#range>
                <http://purl.org/olia/olia-top.owl#StrengthFeature> ;
        <http://www.w3.org/2000/01/rdf-schema#subPropertyOf>
                <http://purl.org/olia/system.owl#hasFeature> .

<http://purl.org/olia/olia.owl#PredicativeAdjective>
        a       <http://www.w3.org/2002/07/owl#Class> ;
        <http://www.w3.org/2000/01/rdf-schema#comment>
                "\n\t\t\tA predicative adjective is one which functions as part of the predicate \n\t\t\tof a sentence. This means that it is linked to the noun by a verb, often \n\t\t\ta copula (such as to be).\n\t\t\t(http://en.wikipedia.org/wiki/Adjective 18.09.06)\n\t\t" ;
        <http://www.w3.org/2000/01/rdf-schema#subClassOf>
                <http://purl.org/olia/olia.owl#Adjective> ;
        <http://www.w3.org/2002/07/owl#versionInfo>
                "\n\t\t\tEAGLES Adjective with Use=\"Predicative\".\n\t\t" .

<http://purl.org/olia/olia.owl#InterterminativeCase>
        a       <http://www.w3.org/2002/07/owl#Class> ;
        <http://www.w3.org/2000/01/rdf-schema#comment>
                "\n\t\t\tInterterminativeCase expresses the notion of something moving into \n\t\t\tthe middle of the referent of the noun it marks, but not through it. \n\t\t\tIt has the meaning 'into the middle of'.\n\t\t\t(http://purl.org/linguistics/gold/Interminative)\n\t\t" ;
        <http://www.w3.org/2000/01/rdf-schema#subClassOf>
                <http://purl.org/olia/olia-top.owl#CaseFeature> ;
        <http://www.w3.org/2002/07/owl#versionInfo>
                "http://purl.org/linguistics/gold/Interminative" .

<http://purl.org/olia/olia.owl#SublativeCase>
        a       <http://www.w3.org/2002/07/owl#Class> ;
        <http://www.w3.org/2000/01/rdf-schema#comment>
                "\n\t\t\tSublativeCase expresses that  the referent of the noun it marks is \n\t\t\tthe location under which another referent is moving toward. It has \n\t\t\tthe meaning 'towards the underneath of'.\n\t\t\t(http://purl.org/linguistics/gold/Sublative)\n\t\t" ;
        <http://www.w3.org/2000/01/rdf-schema#subClassOf>
                <http://purl.org/olia/olia-top.owl#CaseFeature> ;
        <http://www.w3.org/2002/07/owl#versionInfo>
                "http://purl.org/linguistics/gold/Sublative; http://www.isocat.org/datcat/DC-1392" .

<http://purl.org/olia/olia.owl#CausalMood>
        a       <http://www.w3.org/2002/07/owl#Class> ;
        <http://www.w3.org/2000/01/rdf-schema#comment>
                "In Inuktitut, causality is expressed by verbal inflection. Causal mood signifies causal relationships in a sentence. (Nowak 1996, p.39)\n\t\t\n\t\tElke Nowak (1996), Transforming the images: Ergativity and transitivity in Inuktitut (Eskimo). Walter de Gruyter, Berlin.\n\t\t" ;
        <http://www.w3.org/2000/01/rdf-schema#subClassOf>
                <http://purl.org/olia/olia.owl#CausalModality> , <http://purl.org/olia/olia-top.owl#MoodFeature> ;
        <http://www.w3.org/2002/07/owl#versionInfo>
                "Nowak (1996)" .

<http://purl.org/olia/olia.owl#InHouseRegister>
        a       <http://www.w3.org/2002/07/owl#Class> ;
        <http://www.w3.org/2000/01/rdf-schema#comment>
                "\n                            Register of terms that are company-specific and not readily recognized outside this environment.\n                                (ISO12620; http://www.isocat.org/datcat/DC-1993)\n                            " ;
        <http://www.w3.org/2000/01/rdf-schema#label>
                "in house register" ;
        <http://www.w3.org/2000/01/rdf-schema#subClassOf>
                <http://purl.org/olia/olia-top.owl#RegisterFeature> ;
        <http://www.w3.org/2002/07/owl#versionInfo>
                "subClassOf register (dcif:conceptualDomain)" , "http://www.isocat.org/datcat/DC-1993" .

<http://purl.org/olia/olia.owl#Inanimate>
        a       <http://www.w3.org/2002/07/owl#Class> ;
        <http://www.w3.org/2000/01/rdf-schema#comment>
                "\n                            Perceived as not living.\n                                (ISO12620; http://www.isocat.org/datcat/DC-1952)\n                            " ;
        <http://www.w3.org/2000/01/rdf-schema#label>
                "inanimate" ;
        <http://www.w3.org/2000/01/rdf-schema#subClassOf>
                <http://purl.org/olia/olia-top.owl#AnimacyFeature> ;
        <http://www.w3.org/2002/07/owl#versionInfo>
                "http://www.isocat.org/datcat/DC-1952" , "subClassOf animacy (dcif:conceptualDomain)" .

<http://purl.org/olia/olia.owl#CompoundPreposition>
        a       <http://www.w3.org/2002/07/owl#Class> ;
        <http://www.w3.org/2000/01/rdf-schema#comment>
                "\n                            Preposition that is a aggregation of words\n                                (http://www.isocat.org/datcat/DC-1934)\n                            " ;
        <http://www.w3.org/2000/01/rdf-schema#label>
                "compound preposition" ;
        <http://www.w3.org/2000/01/rdf-schema#subClassOf>
                <http://purl.org/olia/olia.owl#Preposition> ;
        <http://www.w3.org/2002/07/owl#versionInfo>
                "subClassOf preposition (dcif:isA)" , "http://www.isocat.org/datcat/DC-1934" .

<http://purl.org/olia/olia.owl#Transgressive>
        a       <http://www.w3.org/2002/07/owl#Class> ;
        <http://www.w3.org/2000/01/rdf-schema#comment>
                "\n                            present (action in the same time as of the predicate): The dog going through the house barks. past (action premature to the one of predicate): He has started to read the book after he had sat down.\n                                (ark.wz.cz/cidarke/mverb.html; http://www.isocat.org/datcat/DC-1404)\n                            " ;
        <http://www.w3.org/2000/01/rdf-schema#label>
                "Transgressive" ;
        <http://www.w3.org/2000/01/rdf-schema#subClassOf>
                <http://purl.org/olia/olia.owl#Present> ;
        <http://www.w3.org/2002/07/owl#versionInfo>
                "http://www.isocat.org/datcat/DC-1404" .

<http://purl.org/olia/olia.owl#HeadOfNP>
        a       <http://www.w3.org/2002/07/owl#Class> ;
        <http://www.w3.org/2000/01/rdf-schema#comment>
                "\n\t\t\tThe HeadFunction is a function of an adjective or participle that can serve as the focus of the phrase.\n\t\t" ;
        <http://www.w3.org/2000/01/rdf-schema#subClassOf>
                <http://purl.org/olia/olia.owl#Head> ;
        <http://www.w3.org/2002/07/owl#versionInfo>
                "EAGLES NPFunction=\"head\"" .

<http://purl.org/olia/olia.owl#VerbalPredicate>
        a       <http://www.w3.org/2002/07/owl#Class> ;
        <http://www.w3.org/2000/01/rdf-schema#comment>
                "\n\t\t\tThe predicate of the clause is represented by a verbal lexeme. (Ch. Chiarcos)\n\t\t" ;
        <http://www.w3.org/2000/01/rdf-schema#subClassOf>
                <http://purl.org/olia/olia.owl#Predicate> ;
        <http://www.w3.org/2002/07/owl#versionInfo>
                "introduced for non-nominal predicates, normally referred to as ``predicate'' (Ch. Chiarcos)" .

<http://purl.org/olia/olia.owl#hasEvaluativeFeature>
        a       <http://www.w3.org/2002/07/owl#ObjectProperty> ;
        <http://www.w3.org/2000/01/rdf-schema#range>
                <http://purl.org/olia/olia-top.owl#EvaluativeFeature> ;
        <http://www.w3.org/2000/01/rdf-schema#subPropertyOf>
                <http://purl.org/olia/system.owl#hasFeature> .

<http://purl.org/olia/olia.owl#ActorMacroRole>
        a       <http://www.w3.org/2002/07/owl#Class> ;
        <http://www.w3.org/2000/01/rdf-schema#comment>
                "\n\t\t\tThe most agentive semantic role of the current clause (van Valin and \n\t\t\tLapolla 1997), designated subject (from a semantic point of view)\n\t\t" ;
        <http://www.w3.org/2000/01/rdf-schema#subClassOf>
                <http://purl.org/olia/olia-top.owl#SemanticRole> ;
        <http://www.w3.org/2002/07/owl#versionInfo>
                "\n\t\t\thttp://languagelink.let.uu.nl/tds/onto/LinguisticOntology.owl#actorRole\n\t\t" .

<http://purl.org/olia/olia.owl#ReflexivePossessiveDeterminer>
        a       <http://www.w3.org/2002/07/owl#Class> ;
        <http://www.w3.org/2000/01/rdf-schema#comment>
                "Attributive possessive pronoun form of the reflexive pronoun, e.g., Russian свой:\n\t\t\n\t\tОбама на свой день рождения угощал гостей стейками и хот-догами.\n\t\tObama on his day of.birth entertained guests with.steaks and hot.dogs\n\t\t\"On his birthday, Obama entertained his guests with steaks and hot dogs.\" (http://ua.rian.ru/world_news/20110805/78815136.html)\n\t\t\n\t\tThe antecedent of a possessive reflexive is not determined by its gender, but by its syntactic prominence.\n\t\t" ;
        <http://www.w3.org/2002/07/owl#equivalentClass>
                [ a       <http://www.w3.org/2002/07/owl#Class> ;
                  <http://www.w3.org/2002/07/owl#intersectionOf>
                          ( <http://purl.org/olia/olia.owl#ReflexiveDeterminer> <http://purl.org/olia/olia.owl#PossessiveDeterminer> )
                ] ;
        <http://www.w3.org/2002/07/owl#versionInfo>
                "shorthand for ReflexiveDeterminer and PossessiveDeterminer, relevant for MULTEXT-East (Slavic) and EMILLE (Urdu), http://purl.org/olia/emille.owl#ReflexivePossessiveAdjective" .

<http://purl.org/olia/olia.owl#StatusConstructus>
        a       <http://www.w3.org/2002/07/owl#Class> ;
        <http://www.w3.org/2000/01/rdf-schema#comment>
                "morphological form of the nominal head of noun+noun-phrases which in spite of a missing determiner (article) is invariably understood as semantically determined. (http://www.isocat.org/datcat/DC-2997)\n\t  \n\t  The construct state or status constructus is a noun form occurring in Afro-Asiatic languages. It is particularly common in Semitic languages (such as Arabic, Hebrew, and Syriac), in the Berber languages, and in the extinct Egyptian language. ... \n\t  In Semitic languages, nouns are placed in the construct state when they are semantically definite and modified by another noun in a genitive construction. Note that this differs from the genitive case of European languages in that it is the head (modified) noun rather than the dependent (modifying) noun which is marked. However, in Semitic languages with grammatical case (e.g. Classical Arabic), the modifying noun in a genitive construction is placed in the genitive case, in addition to marking the head noun with the construct state. ...\n\t  The construct state is one of the three grammatical states of nouns in Arabic, the other two being the indefinite state and the definite state. ... (http://en.wikipedia.org/wiki/Construct_state)" ;
        <http://www.w3.org/2000/01/rdf-schema#isDefinedBy>
                "http://www.isocat.org/datcat/DC-2997" ;
        <http://www.w3.org/2000/01/rdf-schema#subClassOf>
                <http://purl.org/olia/olia-top.owl#DefinitenessFeature> ;
        <http://www.w3.org/2002/07/owl#versionInfo>
                "According to the Arabic usage of this category, modeled here as a DefinitenessFeature, though not directly a subconcept of definite, because it has other functions in other languages." .

<http://purl.org/olia/olia.owl#hasSemanticRole>
        a       <http://www.w3.org/2002/07/owl#ObjectProperty> ;
        <http://www.w3.org/2000/01/rdf-schema#range>
                <http://purl.org/olia/olia-top.owl#SemanticRole> ;
        <http://www.w3.org/2000/01/rdf-schema#subPropertyOf>
                <http://purl.org/olia/system.owl#hasFeature> .

<http://purl.org/olia/olia.owl#ElementDemandingClitic>
        a       <http://www.w3.org/2002/07/owl#Class> ;
        <http://www.w3.org/2000/01/rdf-schema#comment>
                "Expression representing a lexeme with cliticization whose clitics are, however, represented as a separate token" ;
        <http://www.w3.org/2000/01/rdf-schema#subClassOf>
                <http://purl.org/olia/olia.owl#ElementWithoutClitic> ;
        <http://www.w3.org/2002/07/owl#versionInfo>
                "http://purl.org/olia/mte/multext-east.owl#DemandingClitic" .

<http://purl.org/olia/olia.owl#Intensifier>
        a       <http://www.w3.org/2002/07/owl#Class> ;
        <http://www.w3.org/2000/01/rdf-schema#comment>
                "For Hindi, words like 'bahuta', 'kama', etc. when intensifying adjectives or adverbs will be annotated as INTF. Example,\n\t\t\th37. hEdarAbAda meM aMgUra bahuta_INTF acche milate hEM\n\t\t\t'HyderabAd' 'in' 'grapes' 'very' 'good' 'available' 'are'\n\t\t\t“Very good grapes are available in Hyderabad” (Bharati et al. 2006)\n\t\t\t\n\t\t\tAkshar Bharati, Dipti Misra Sharma, Lakshmi Bai, Rajeev Sangal (2006), AnnCorra : Annotating Corpora. Guidelines For POS And Chunk Annotation For Indian Languages, Tech. Rep., L anguage Technologies Research Centre IIIT, Hyderabad, version of 15-12-2006, http://ltrc.iiit.ac.in/tr031/posguidelines.pdf\n\t\t" ;
        <http://www.w3.org/2000/01/rdf-schema#subClassOf>
                <http://purl.org/olia/olia.owl#Unique> ;
        <http://www.w3.org/2002/07/owl#versionInfo>
                "adopted from Ancorra, http://purl.org/olia/ancorra.owl#Intensifier" .

<http://purl.org/olia/olia.owl#Positive>
        a       <http://www.w3.org/2002/07/owl#Class> ;
        <http://www.w3.org/2000/01/rdf-schema#comment>
                "\n\t\t\tValue used in a comparison relationship when no comparison is involved.\n\t\t\t(http://www.isocat.org/datcat/DC-1420)\n\t\t\n\t\t\tThe Positive is the form of an adjective or \n\t\t\tadverb on which comparative and superlative are formed.\n\t\t\t(http://en.wikipedia.org/wiki/Positive  17.11.06)\n\t\t" ;
        <http://www.w3.org/2000/01/rdf-schema#subClassOf>
                <http://purl.org/olia/olia-top.owl#DegreeFeature> ;
        <http://www.w3.org/2002/07/owl#versionInfo>
                "EAGLES, http://www.isocat.org/datcat/DC-1420" .

<http://purl.org/olia/olia.owl#ReflexivePassive>
        a       <http://www.w3.org/2002/07/owl#Class> ;
        <http://www.w3.org/2000/01/rdf-schema#comment>
                "\n\t\t\tA Passive construction which contains reflexive markings. (Siewierska 1988:257)\n\t\t\t(http://purl.org/linguistics/gold/ReflexivePassive)\n\t\t" ;
        <http://www.w3.org/2000/01/rdf-schema#subClassOf>
                <http://purl.org/olia/olia.owl#PassiveVoice> ;
        <http://www.w3.org/2002/07/owl#versionInfo>
                "http://purl.org/linguistics/gold/ReflexivePassive" .

<http://purl.org/olia/olia.owl#AdverbialModifier>
        a       <http://www.w3.org/2002/07/owl#Class> ;
        <http://www.w3.org/2000/01/rdf-schema#comment>
                "\n\t\t\tAn adverbial modifier modifies a verb.\n\t\t\t(http://languagelink.let.uu.nl/tds/onto/LinguisticOntology.owl#adverbialModifier)\n\t\t" ;
        <http://www.w3.org/2000/01/rdf-schema#subClassOf>
                <http://purl.org/olia/olia.owl#Modifier> ;
        <http://www.w3.org/2002/07/owl#versionInfo>
                "http://languagelink.let.uu.nl/tds/onto/LinguisticOntology.owl#adverbialModifier" .

<http://purl.org/olia/olia.owl#DemonstrativePronoun>
        a       <http://www.w3.org/2002/07/owl#Class> ;
        <http://www.w3.org/2000/01/rdf-schema#comment>
                "\n\t\t\tDemonstrative pronouns are deictic words (they depend on an external frame of reference). \n\t\t\tThey indicate which entities a speaker refers to, and distinguishes those entities from others. \n\t\t\t(http://en.wikipedia.org/wiki/Demonstrative_pronoun 19.09.06)\n\t\t" ;
        <http://www.w3.org/2000/01/rdf-schema#subClassOf>
                <http://purl.org/olia/olia.owl#Pronoun> ;
        <http://www.w3.org/2002/07/owl#versionInfo>
                "EAGLES Pronoun with Pron.-Type=\"Demonstrative\"." , "TODO: \n\t\t\tThis definition is nonsatisfactory, cf. Ehlich (1982) for intra-textual (\"anadeictic\") uses of demonstratives.\n\t\t" .

<http://purl.org/olia/olia.owl#ErgativeCase>
        a       <http://www.w3.org/2002/07/owl#Class> ;
        <http://www.w3.org/2000/01/rdf-schema#comment>
                "\n\t\t\tIn ergative-absolutive languages, the ergative case identifies the subject of a transitive verb. \n\t\t\tIn such languages, the ergative case is typically marked (most salient), while the absolutive \n\t\t\tcase is unmarked. (http://languagelink.let.uu.nl/tds/onto/LinguisticOntology.owl#ergativeCase \n\t\t\twith reference to http://en.wikipedia.org/wiki/Ergative_case).\n\t\t" ;
        <http://www.w3.org/2000/01/rdf-schema#subClassOf>
                <http://purl.org/olia/olia-top.owl#CaseFeature> ;
        <http://www.w3.org/2002/07/owl#versionInfo>
                "TDS Ontology" .

<http://purl.org/olia/olia.owl#VoiceNoun>
        a       <http://www.w3.org/2002/07/owl#Class> ;
        <http://www.w3.org/2000/01/rdf-schema#comment>
                "\n                            noun of a voice\n                                (http://www.isocat.org/datcat/DC-2253)\n                            " ;
        <http://www.w3.org/2000/01/rdf-schema#label>
                "voice noun" ;
        <http://www.w3.org/2000/01/rdf-schema#subClassOf>
                <http://purl.org/olia/olia.owl#Noun> ;
        <http://www.w3.org/2002/07/owl#versionInfo>
                "http://www.isocat.org/datcat/DC-2253" , "subClassOf partOfSpeech (dcif:conceptualDomain)" .

<http://purl.org/olia/olia.owl#DirectCase>
        a       <http://www.w3.org/2002/07/owl#Class> ;
        <http://www.w3.org/2000/01/rdf-schema#comment>
                "\n\t\t\tIn the Romanian case system the value 'direct' conflates 'nominative' and 'accusative', \n\t\t\te.g., -acea/acel, -aceasta/acesta, -această/acest\n\t\t\t(http://purl.org/olia/mte/multext-east.owl#DirectCase)\n\t\t" ;
        <http://www.w3.org/2000/01/rdf-schema#subClassOf>
                <http://purl.org/olia/olia-top.owl#CaseFeature> ;
        <http://www.w3.org/2002/07/owl#versionInfo>
                "http://purl.org/olia/mte/multext-east.owl#DirectCase" .

<http://purl.org/olia/olia.owl#IndefinitePronoun>
        a       <http://www.w3.org/2002/07/owl#Class> ;
        <http://www.w3.org/2000/01/rdf-schema#comment>
                "\n\t\tAn indefinite pronoun is a pronoun that belongs to a class whose members \n\t\tindicate indefinite reference. Examples in English are \"anybody\",  \"one\",\n\t\t\"somebody\".\n\t\t(http://www.sil.org/linguistics/GlossaryOfLinguisticTerms/WhatIsAnIndefinitePronoun.htm 19.09.06)\n\t" ;
        <http://www.w3.org/2000/01/rdf-schema#subClassOf>
                <http://purl.org/olia/olia.owl#Pronoun> ;
        <http://www.w3.org/2002/07/owl#versionInfo>
                "\n\t\t\tEAGLES Pronoun with Pron.-Type=\"Indefinite\".\n\t\t" .

<http://purl.org/olia/olia.owl#AdverbialSubordinateClause>
        a       <http://www.w3.org/2002/07/owl#Class> ;
        <http://www.w3.org/2000/01/rdf-schema#comment>
                "\n\t\t\tSubordinate clauses with adverbial function are annotated as ADV, e.g. \"Tom sleeps when the sun rises.\"\n\t\t\t(Dipper et al. 2007, §4.3.6)\n\t\t" ;
        <http://www.w3.org/2000/01/rdf-schema#subClassOf>
                <http://purl.org/olia/olia.owl#SubordinateClause> ;
        <http://www.w3.org/2002/07/owl#versionInfo>
                "added in conformance with the SFB632 Annotation Guidelines (Dipper et al. 2007)" .

<http://purl.org/olia/olia.owl#ImpersonalPronoun>
        a       <http://www.w3.org/2002/07/owl#Class> ;
        <http://www.w3.org/2000/01/rdf-schema#comment>
                "\n                            Pronoun lacking person referent.\n                                (Gil Francopoulo; http://www.isocat.org/datcat/DC-1426)\n\t\t\t\t\t\t\t\t\n\t\t\t\t\t\t\tMore precisely, a form of pronoun that denotes the absence of a concrete or specific referent, e.g., German \"man\".\n\t\t\t\t\t\t\tAs opposed to IndefinitePronoun, this referent is not just discourse-new, but generic or hypothetical.\n                            " ;
        <http://www.w3.org/2000/01/rdf-schema#label>
                "impersonal pronoun" ;
        <http://www.w3.org/2000/01/rdf-schema#subClassOf>
                <http://purl.org/olia/olia.owl#IndefinitePronoun> ;
        <http://www.w3.org/2002/07/owl#versionInfo>
                "subClassOf pronoun (dcif:isA)" , "http://www.isocat.org/datcat/DC-1426" .

<http://purl.org/olia/olia.owl#IrrealisModality>
        a       <http://www.w3.org/2002/07/owl#Class> ;
        <http://www.w3.org/2000/01/rdf-schema#comment>
                "\n\t\t\tIrrealis modality indicates the situation to which it pertains is \n\t\t\tnon-actual or non-factual.\n\t\t\t(http://languagelink.let.uu.nl/tds/onto/LinguisticOntology.owl#irrealisModality)\n\t\t" ;
        <http://www.w3.org/2000/01/rdf-schema#subClassOf>
                <http://purl.org/olia/olia-top.owl#ModalityFeature> ;
        <http://www.w3.org/2002/07/owl#versionInfo>
                "http://languagelink.let.uu.nl/tds/onto/LinguisticOntology.owl#irrealisModality" .

<http://purl.org/olia/olia.owl#PurposiveCase>
        a       <http://www.w3.org/2002/07/owl#Class> ;
        <http://www.w3.org/2000/01/rdf-schema#comment>
                "Purposive marks the goal of an activity, e.g., 'going out FOR (i.e. to catch) KANGAROOS'; 'call them FOR (i.e. to eat) FOOD'. \n\t\tThe common purposive suffix -gu is a recurrent suffix on verbs ... The purposive case suffix is often used on a nominalised clause (and this may possibly be the origin of the verbal purposive).\n\t\t(Dixon 2002, p.134, on purposive case in [several] Australian languages)\n\t\t\n\t\tR.M.W. Dixon (2002), Australian Languages. CUP, Cambridge" ;
        <http://www.w3.org/2000/01/rdf-schema#subClassOf>
                <http://purl.org/olia/olia-top.owl#CaseFeature> ;
        <http://www.w3.org/2002/07/owl#versionInfo>
                "added in accordance with the ILPOSTS tagset for a case marker (postposition) in Indian languages, cf. http://purl.org/olia/ilposts.owl#PurposiveCase" .

<http://purl.org/olia/olia.owl#Conjunction>
        a       <http://www.w3.org/2002/07/owl#Class> ;
        <http://www.w3.org/2000/01/rdf-schema#comment>
                "\n\t\tA conjunction is a word that syntactically links words or larger constituents, \n\t\tand expresses a semantic relationship between them.\n\t\t(http://www.sil.org/linguistics/GlossaryOfLinguisticTerms/WhatIsAConjunction.htm 19.09.06)\n\t" ;
        <http://www.w3.org/2000/01/rdf-schema#label>
                "conjunction"@en , "conjonction"@fr ;
        <http://www.w3.org/2000/01/rdf-schema#subClassOf>
                <http://purl.org/olia/olia-top.owl#MorphosyntacticCategory> ;
        <http://www.w3.org/2002/07/owl#versionInfo>
                "EAGLES top-level concept Conjunction (C)." .

<http://purl.org/olia/olia.owl#IllativeCase>
        a       <http://www.w3.org/2002/07/owl#Class> ;
        <http://www.w3.org/2000/01/rdf-schema#comment>
                "\n\t\t\tIllativeCase expresses that  the referent of the noun it marks is \n\t\t\tthe location into which another referent is moving. It has the \n\t\t\tmeaning 'into' (Lyons 1968: 299; Gove, et al. 1966: 1126; Crystal \n\t\t\t1985: 152).\n\t\t\t(http://purl.org/linguistics/gold/Illative)\n\t\t" ;
        <http://www.w3.org/2000/01/rdf-schema#subClassOf>
                <http://purl.org/olia/olia-top.owl#CaseFeature> ;
        <http://www.w3.org/2002/07/owl#versionInfo>
                "http://purl.org/linguistics/gold/Illative; http://www.isocat.org/datcat/DC-1303" .

<http://purl.org/olia/olia.owl#RelativeQuantifier>
        a       <http://www.w3.org/2002/07/owl#Class> ;
        <http://www.w3.org/2000/01/rdf-schema#comment>
                "In the Czech MTE v4 specs, Numeral/Class=\"relative\" are items meaning `how many/much', `as many/much' etc. Strictly speaking, they are pronumerals (pro-quantifiers), but traditional descriptions don't recognise such a category, so they are described variously as pronouns or as numerals (because their syntactic distribution is that of numerals, or very close).\" (Ivan A Derzhanski, email 2010/06/11, http://purl.org/olia/mte/multext-east.owl#RelativeQuantifier)" ;
        <http://www.w3.org/2000/01/rdf-schema#subClassOf>
                <http://purl.org/olia/olia.owl#ProQuantifier> ;
        <http://www.w3.org/2002/07/owl#versionInfo>
                "http://purl.org/olia/mte/multext-east.owl#RelativeQuantifier" .

<http://purl.org/olia/olia.owl#Ideophone>
        a       <http://www.w3.org/2002/07/owl#Class> ;
        <http://www.w3.org/2000/01/rdf-schema#comment>
                "Ideophones are marked words that depict sensory imagery." ;
        <http://www.w3.org/2000/01/rdf-schema#isDefinedBy>
                "http://www.isocat.org/datcat/DC-4192" ;
        <http://www.w3.org/2000/01/rdf-schema#subClassOf>
                <http://purl.org/olia/olia-top.owl#SemanticUnit> .

<http://purl.org/olia/olia.owl#SeparablePrefix>
        a       <http://www.w3.org/2002/07/owl#Class> ;
        <http://www.w3.org/2000/01/rdf-schema#comment>
                "separable verb prefix, e.g., \"Auch die Vertreter der AfB [stimmten] den 86 Millionen [zu].\"" ;
        <http://www.w3.org/2000/01/rdf-schema#subClassOf>
                <http://purl.org/olia/olia.owl#Prefix> ;
        <http://www.w3.org/2002/07/owl#versionInfo>
                "TüBa-D/Z" .

<http://purl.org/olia/olia.owl#NotTemporallyAnchored>
        a       <http://www.w3.org/2002/07/owl#Class> ;
        <http://www.w3.org/2000/01/rdf-schema#comment>
                "\n\t\t\tTo be used for actions that are not bound to a particular reference point.\n\t\t" ;
        <http://www.w3.org/2000/01/rdf-schema#subClassOf>
                <http://purl.org/olia/olia-top.owl#TenseFeature> ;
        <http://www.w3.org/2002/07/owl#versionInfo>
                "\n\t\t\tA replacement for TDS Habitual that is modelled here as an Aspect:\n\t\t\t\n\t\t\tHabitual tense pertains to verbs which refer to an action that occurs repeatedly.\n\t\t\t(http://languagelink.let.uu.nl/tds/onto/LinguisticOntology.owl#habitualTense)\t\t\t\t\t\n\t\t" .

<http://purl.org/olia/olia.owl#Nominalization>
        a       <http://www.w3.org/2002/07/owl#Class> ;
        <http://www.w3.org/2000/01/rdf-schema#subClassOf>
                <http://purl.org/olia/olia.owl#Derivation> ;
        <http://www.w3.org/2002/07/owl#versionInfo>
                "TODO: compare against Lehmann, Handbuch Relativsätze" , "Nominalization is the process of forming a noun from (mostly) a verbal form, often marked morphologically or via zero derivation. (Hasmik Sargsian and Christian Chiarcos)" .

<http://purl.org/olia/olia.owl#Masdar>
        a       <http://www.w3.org/2002/07/owl#Class> ;
        <http://www.w3.org/2000/01/rdf-schema#comment>
                "property that expresses a verbal idea under an abstract form. (http://www.isocat.org/datcat/DC-2224)\n\t  \n\t  the verbal noun present in Arabic and various Caucasian languages, such as Georgian and North-Caucasian languages. This grammatical term is an Arabic word, used later as a specialized, technical term to name the verbal noun in Arabic and Caucasian grammar. (http://en.wikipedia.org/wiki/Masdar)\n\t  " ;
        <http://www.w3.org/2000/01/rdf-schema#isDefinedBy>
                "http://www.isocat.org/datcat/DC-2224" ;
        <http://www.w3.org/2000/01/rdf-schema#label>
                "masdar" ;
        <http://www.w3.org/2000/01/rdf-schema#subClassOf>
                <http://purl.org/olia/olia.owl#VerbalNoun> .

<http://purl.org/olia/olia.owl#RelativePast>
        a       <http://www.w3.org/2002/07/owl#Class> ;
        <http://www.w3.org/2000/01/rdf-schema#comment>
                "\n\t\t\tRelativePastTense locates the situation in question before that of \n\t\t\ta contextually determined temporal reference point (Comrie 1985: \n\t\t\t104). Also called PastPerfectTense.\n\t\t\t(http://purl.org/linguistics/gold/RelativePast)\n\t\t" ;
        <http://www.w3.org/2000/01/rdf-schema#subClassOf>
                <http://purl.org/olia/olia.owl#RelativeTense> ;
        <http://www.w3.org/2002/07/owl#versionInfo>
                "http://purl.org/linguistics/gold/RelativePast" .

<http://purl.org/olia/olia.owl#ContextualVariation>
        a       <http://www.w3.org/2002/07/owl#Class> ;
        <http://www.w3.org/2000/01/rdf-schema#comment>
                "Variation on a particular usage or immediate proximity of words." ;
        <http://www.w3.org/2000/01/rdf-schema#isDefinedBy>
                "http://www.isocat.org/datcat/DC-1977" ;
        <http://www.w3.org/2000/01/rdf-schema#subClassOf>
                <http://purl.org/olia/olia.owl#Possible> .

<http://purl.org/olia/olia.owl#SyntacticObject>
        a       <http://www.w3.org/2002/07/owl#Class> ;
        <http://www.w3.org/2000/01/rdf-schema#comment>
                "\n\t\t\tIn linguistics, the object of a transitive verb is one of its core \n\t\t\targuments, which generally represents the target of the verb's action or \n\t\t\tthe undergoer of its effects. In more general terms, an object is a \n\t\t\tpatient.\n\n\t\t\tVerbs with no object (as in the sentence \"I run\") are called \n\t\t\tintransitive verbs. Those which do take objects are called transitive \n\t\t\tverbs. Transitive verbs which take only one object are known as \n\t\t\tmonotransitive. Ditransitive verbs have two objects, a patient and a \n\t\t\trecipient. (http://en.wikipedia.org/wiki/Object_%28grammar%29).\n\t\t\t(http://languagelink.let.uu.nl/tds/onto/LinguisticOntology.owl#syntacticObject)\n\t\t\t\n\t\t\tAn object, traditionally defined, is either a direct object or an indirect object. \n\t\t\tAn object, in some usages, is any  grammatical relation other than subject \n\t\t\t(Crystal 1985: 211; Hartmann and Stork 1972: 155-156; Mish et al. 1990: 814, Comrie 1989: 66).\n\t\t\t(http://purl.org/linguistics/gold/object)\n\t\t" ;
        <http://www.w3.org/2000/01/rdf-schema#subClassOf>
                <http://purl.org/olia/olia.owl#SyntacticArgument> ;
        <http://www.w3.org/2002/07/owl#versionInfo>
                "http://languagelink.let.uu.nl/tds/onto/LinguisticOntology.owl#syntacticObject" .

<http://purl.org/olia/olia-top.owl#NarrativeType>
        a       <http://www.w3.org/2002/07/owl#Class> .

<http://purl.org/olia/olia.owl#NonReflexive>
        a       <http://www.w3.org/2002/07/owl#Class> ;
        <http://www.w3.org/2000/01/rdf-schema#comment>
                "\n\t\t\tA non-reflexive verb is a verb whose semantic agent and patient \n\t\t\t(typically represented syntactically by the subject and the direct \n\t\t\tobject) are not the same. \n\t\t\t(http://en.wikipedia.org/wiki/Reflexive_verbs  20.11.06)\n\t\t" ;
        <http://www.w3.org/2000/01/rdf-schema#subClassOf>
                <http://purl.org/olia/olia-top.owl#ReflexivityFeature> ;
        <http://www.w3.org/2002/07/owl#versionInfo>
                "TODO: remove" .

<http://purl.org/olia/olia.owl#PrepositionalObject>
        a       <http://www.w3.org/2002/07/owl#Class> ;
        <http://www.w3.org/2000/01/rdf-schema#comment>
                "Prepositional object" ;
        <http://www.w3.org/2000/01/rdf-schema#subClassOf>
                <http://purl.org/olia/olia.owl#SyntacticObject> ;
        <http://www.w3.org/2002/07/owl#versionInfo>
                "added in conformance with SFB632 annotation guidelines (Dipper et al. 2007, §4.3.4)" .

<http://purl.org/olia/olia.owl#Slash>
        a       <http://www.w3.org/2002/07/owl#Class> ;
        <http://www.w3.org/2000/01/rdf-schema#comment>
                "\n                            The punctuation sign /\n                                (http://www.isocat.org/datcat/DC-1437)\n                            " ;
        <http://www.w3.org/2000/01/rdf-schema#label>
                "slash" ;
        <http://www.w3.org/2000/01/rdf-schema#subClassOf>
                <http://purl.org/olia/olia.owl#SecondaryPunctuation> ;
        <http://www.w3.org/2002/07/owl#versionInfo>
                "http://www.isocat.org/datcat/DC-1437" , "subClassOf partOfSpeech (dcif:conceptualDomain)" , "Parenthetical in Russian (instead of \"(\", \")\"), sentence medial in English" .

<http://purl.org/olia/olia.owl#ConditionalClause>
        a       <http://www.w3.org/2002/07/owl#Class> ;
        <http://www.w3.org/2000/01/rdf-schema#comment>
                "\n\t\t\tConditional clauses refer to a hypothetical situation, in English they are introduced by \n\t\t\t'if' or 'unless'.\n\t\t\t(http://languagelink.let.uu.nl/tds/onto/LinguisticOntology.owl#conditionalClause)\n\t\t" ;
        <http://www.w3.org/2000/01/rdf-schema#subClassOf>
                <http://purl.org/olia/olia.owl#SubordinateClause> ;
        <http://www.w3.org/2002/07/owl#versionInfo>
                "http://languagelink.let.uu.nl/tds/onto/LinguisticOntology.owl#conditionalClause" .

<http://purl.org/olia/olia.owl#ProprietiveCase>
        a       <http://www.w3.org/2002/07/owl#Class> ;
        <http://www.w3.org/2000/01/rdf-schema#comment>
                "\n\t\t\tProprietive case marks a possessional relation, i.e. 'having' something.\n\t\t\t(http://languagelink.let.uu.nl/tds/onto/LinguisticOntology.owl#proprietiveCase-grammatical)\n\t\t" ;
        <http://www.w3.org/2000/01/rdf-schema#subClassOf>
                <http://purl.org/olia/olia-top.owl#CaseFeature> ;
        <http://www.w3.org/2002/07/owl#versionInfo>
                "TDS Ontology, http://languagelink.let.uu.nl/tds/onto/LinguisticOntology.owl#proprietiveCase-grammatical" .

<http://purl.org/olia/olia.owl#Image>
        a       <http://www.w3.org/2002/07/owl#Class> ;
        <http://www.w3.org/2000/01/rdf-schema#comment>
                "\n                            graphical representation\n                                (http://www.isocat.org/datcat/DC-2249)\n                            " ;
        <http://www.w3.org/2000/01/rdf-schema#label>
                "image" ;
        <http://www.w3.org/2000/01/rdf-schema#subClassOf>
                <http://purl.org/olia/olia.owl#LayoutElement> ;
        <http://www.w3.org/2002/07/owl#versionInfo>
                "http://www.isocat.org/datcat/DC-2249" .

<http://purl.org/olia/olia.owl#SubjectControl>
        a       <http://www.w3.org/2002/07/owl#Class> ;
        <http://www.w3.org/2000/01/rdf-schema#comment>
                "Indicates the subject of the main clause is the (omitted) subject of the subclause (http://www.lexinfo.net/ontology/2.0/lexinfo#SubjectControl)"@en ;
        <http://www.w3.org/2000/01/rdf-schema#subClassOf>
                <http://purl.org/olia/olia.owl#Control> ;
        <http://www.w3.org/2002/07/owl#versionInfo>
                "http://www.lexinfo.net/ontology/2.0/lexinfo#SubjectControl" .

<http://purl.org/olia/olia.owl#OptativeMood>
        a       <http://www.w3.org/2002/07/owl#Class> ;
        <http://www.w3.org/2000/01/rdf-schema#comment>
                "\n\t\t\tOptative indicates that the speaker wishes or hopes that the expressed proposition \n\t\t\tbe the case (Bybee, Perkins, and Pagliuca 1994: 179; Palmer 2001: 204).\n\t\t\t(http://purl.org/linguistics/gold/Optative)\n\t\t" ;
        <http://www.w3.org/2000/01/rdf-schema#subClassOf>
                <http://purl.org/olia/olia.owl#OptativeModality> , <http://purl.org/olia/olia-top.owl#MoodFeature> ;
        <http://www.w3.org/2002/07/owl#versionInfo>
                "\n\t\t\thttp://purl.org/linguistics/gold/Optative,\n\t\t\thttp://languagelink.let.uu.nl/tds/onto/LinguisticOntology.owl#optativeModality\n\t\t" .

<http://purl.org/olia/olia.owl#SuperallativeCase>
        a       <http://www.w3.org/2002/07/owl#Class> ;
        <http://www.w3.org/2000/01/rdf-schema#comment>
                "\n\t\t\tSuperallativeCase expresses that  something is moving toward the region \n\t\t\tthat is above the referent of the noun it marks. It has the meaning \n\t\t\t'towards the region that is over'.\n\t\t\t(http://purl.org/linguistics/gold/Superallative)\n\t\t" ;
        <http://www.w3.org/2000/01/rdf-schema#subClassOf>
                <http://purl.org/olia/olia-top.owl#CaseFeature> ;
        <http://www.w3.org/2002/07/owl#versionInfo>
                "http://purl.org/linguistics/gold/Superallative" .

<http://purl.org/olia/olia.owl#CommissiveModality>
        a       <http://www.w3.org/2002/07/owl#Class> ;
        <http://www.w3.org/2000/01/rdf-schema#comment>
                "CommissiveForce indicates that the speaker\n                        promises or threatens to perform some action [Palmer 2001: 10,\n                        72]." ;
        <http://www.w3.org/2000/01/rdf-schema#isDefinedBy>
                "http://www.isocat.org/datcat/DC-3120" ;
        <http://www.w3.org/2000/01/rdf-schema#label>
                "commissive force" ;
        <http://www.w3.org/2000/01/rdf-schema#subClassOf>
                <http://purl.org/olia/olia.owl#ActionalModality> .

<http://purl.org/olia/olia.owl#InterrogativeAdverb>
        a       <http://www.w3.org/2002/07/owl#Class> ;
        <http://www.w3.org/2000/01/rdf-schema#comment>
                "\n\t\t\tInterrogative adverbs are used to introduce questions, e.g. \"When are you coming?\" (Angelika Adam)\n\t\t" ;
        <http://www.w3.org/2000/01/rdf-schema#subClassOf>
                <http://purl.org/olia/olia.owl#WHTypeAdverbs> ;
        <http://www.w3.org/2002/07/owl#equivalentClass>
                [ a       <http://www.w3.org/2002/07/owl#Class> ;
                  <http://www.w3.org/2002/07/owl#intersectionOf>
                          ( <http://purl.org/olia/olia.owl#WHTypeAdverbs> <http://purl.org/olia/olia.owl#QuestionWord> )
                ] ;
        <http://www.w3.org/2002/07/owl#versionInfo>
                "EAGLES Adverb with Wh-Type=\"Interrogative\"." .

<http://purl.org/olia/olia.owl#UniquitiveDeterminer>
        a       <http://www.w3.org/2002/07/owl#Class> ;
        <http://www.w3.org/2000/01/rdf-schema#comment>
                "Determiner/Type=\"exceptional\" is applied to the Persian uniquitive determiner تنها  i.e., \"the only\" (MTE v4; Hamidreza Kobdani, email 2010/06/15, http://purl.org/olia/mte/multext-east.owl#UniquitiveDeterminer)" ;
        <http://www.w3.org/2000/01/rdf-schema#subClassOf>
                <http://purl.org/olia/olia.owl#Determiner> ;
        <http://www.w3.org/2002/07/owl#versionInfo>
                "http://purl.org/olia/mte/multext-east.owl#UniquitiveDeterminer" .

<http://purl.org/olia/olia.owl#PossessorRole>
        a       <http://www.w3.org/2002/07/owl#Class> ;
        <http://www.w3.org/2000/01/rdf-schema#comment>
                "Semantic role as used by the Stanford Dependency Parser" ;
        <http://www.w3.org/2000/01/rdf-schema#subClassOf>
                <http://purl.org/olia/olia-top.owl#SemanticRole> ;
        <http://www.w3.org/2002/07/owl#versionInfo>
                "added in conformance with Stanford Parser Dependency Labels" .

<http://purl.org/olia/olia.owl#Contraction>
        a       <http://www.w3.org/2002/07/owl#Class> ;
        <http://www.w3.org/2000/01/rdf-schema#comment>
                "no definition given" ;
        <http://www.w3.org/2000/01/rdf-schema#subClassOf>
                <http://purl.org/olia/olia.owl#Residual> ;
        <http://www.w3.org/2002/07/owl#versionInfo>
                "Uby POS, undocumented, http://purl.org/olia/ubyPos.owl" .

<http://purl.org/olia/olia.owl#NominalPredicate>
        a       <http://www.w3.org/2002/07/owl#Class> ;
        <http://www.w3.org/2000/01/rdf-schema#comment>
                "\n\t\t\tA nominal predicate (noun or adjective), either with or without copula. \n\t\t\tThe term nominal predicate may be used for the complements of further \n\t\t\tcopulative verbs (cf. small clauses), e.g. \"consider\", \"call\", etc.\n\t\t\t(Dipper et al. 2007, §4.3.5)\n\t\t" ;
        <http://www.w3.org/2000/01/rdf-schema#subClassOf>
                <http://purl.org/olia/olia.owl#Predicate> ;
        <http://www.w3.org/2002/07/owl#versionInfo>
                "added in conformance with SFB632 annotation guidelines (Dipper et al., 2007)" .

<http://purl.org/olia/olia.owl#hasPerson>
        a       <http://www.w3.org/2002/07/owl#ObjectProperty> ;
        <http://www.w3.org/2000/01/rdf-schema#domain>
                [ a       <http://www.w3.org/2002/07/owl#Class> ;
                  <http://www.w3.org/2002/07/owl#unionOf>
                          ( <http://purl.org/olia/olia.owl#Verb> <http://purl.org/olia/olia.owl#PronounOrDeterminer> )
                ] ;
        <http://www.w3.org/2000/01/rdf-schema#range>
                <http://purl.org/olia/olia-top.owl#PersonFeature> ;
        <http://www.w3.org/2000/01/rdf-schema#subPropertyOf>
                <http://purl.org/olia/system.owl#hasFeature> .

<http://purl.org/olia/olia.owl#OpenQuote>
        a       <http://www.w3.org/2002/07/owl#Class> ;
        <http://www.w3.org/2000/01/rdf-schema#comment>
                "quotation mark, opening" ;
        <http://www.w3.org/2000/01/rdf-schema#subClassOf>
                <http://purl.org/olia/olia.owl#Quote> ;
        <http://www.w3.org/2002/07/owl#versionInfo>
                "adopted from EMILLE, http://purl.org/olia/emille.owl#OpenQuotationMark" .

<http://purl.org/olia/olia.owl#SentenceFinalPunctuation>
        a       <http://www.w3.org/2002/07/owl#Class> ;
        <http://www.w3.org/2000/01/rdf-schema#comment>
                "\n\t\t\tSentenceFinalPunctuation are . ? !. \n\t\t\t(http://www.ilc.cnr.it/EAGLES96/annotate/node17.html#recv 19.09.06)\n\t\t" ;
        <http://www.w3.org/2000/01/rdf-schema#subClassOf>
                <http://purl.org/olia/olia.owl#MainPunctuation> ;
        <http://www.w3.org/2002/07/owl#versionInfo>
                "added in accordance with http://www.ilc.cnr.it/EAGLES96/annotate/node17.html#recv" .

<http://purl.org/olia/olia.owl#Fragment>
        a       <http://www.w3.org/2002/07/owl#Class> ;
        <http://www.w3.org/2000/01/rdf-schema#comment>
                "FRAG marks those portions of text that appear to be clauses, but lack too many essential elements for the exact structure to be easily determined (e.g., answers to questions). Predicate argument structure therefore cannot be extracted from FRAGs.\n(Bies et al. 1995)\n\nSentence fragments that end with sentence- nal punctuation like Not even an earthquake. should not\nbe bracketed as S, but only with the highest appropriate label|in this case, NP. Do not attach such\nfragments to the preceding or following full sentence.\n(Santorini 1991)" ;
        <http://www.w3.org/2000/01/rdf-schema#subClassOf>
                <http://purl.org/olia/olia-top.owl#Constituent> ;
        <http://www.w3.org/2002/07/owl#versionInfo>
                "PTB bracketing guidelines, Santorini 1991, Bies et al. 1995" .

<http://purl.org/olia/olia.owl#Future>
        a       <http://www.w3.org/2002/07/owl#Class> ;
        <http://www.w3.org/2000/01/rdf-schema#comment>
                "\n\t\t\tThe future tense refers to events that have yet to happen. \n\t\t\t(http://en.wikipedia.org/wiki/Future  17.11.06)\n\t\t\t\n\t\t\tThe future tense refers to a tense category which places an event in the future.\n\t\t\t(http://languagelink.let.uu.nl/tds/onto/LinguisticOntology.owl#futureTense)\n\t\t\t\n\t\t\tFutureTense locates the situation in question later than the present moment (time of speaking.)\n\t\t\t(http://purl.org/linguistics/gold/Future)\n\t\t" ;
        <http://www.w3.org/2000/01/rdf-schema#subClassOf>
                <http://purl.org/olia/olia.owl#AbsoluteTense> ;
        <http://www.w3.org/2002/07/owl#versionInfo>
                "\n\t\t\tEAGLES, \n\t\t\thttp://languagelink.let.uu.nl/tds/onto/LinguisticOntology.owl#futureTense,\n\t\t\thttp://purl.org/linguistics/gold/Future\n\t\t" .

<http://purl.org/olia/olia.owl#VocativeCase>
        a       <http://www.w3.org/2002/07/owl#Class> ;
        <http://www.w3.org/2000/01/rdf-schema#comment>
                "\n\t\t\tVocative case marks a noun whose referent is being addressed.\n\t\t\t(http://www.sil.org/linguistics/glossaryoflinguisticterms/WhatIsVocativeCase.htm 17.11.06)\n\t\t" ;
        <http://www.w3.org/2000/01/rdf-schema#subClassOf>
                <http://purl.org/olia/olia-top.owl#CaseFeature> ;
        <http://www.w3.org/2002/07/owl#versionInfo>
                "EAGLES-recommended case feature" .

<http://purl.org/olia/olia.owl#WHNounPhrase>
        a       <http://www.w3.org/2002/07/owl#Class> ;
        <http://www.w3.org/2000/01/rdf-schema#comment>
                "WHNP|Wh-noun phrase. Noun phrase containing (among other things) a wh-determiner, as in which\nbook or whose daughter, or consisting of a wh-pronoun like who.\n(Santorini 1991)\n\nWHNP\nâ ´ Wh-noun Phrase. Introduces a clause with an NP gap. May be null (containing the 0 complementizer) or lexical, containing some wh-word, e.g. who, which book, whose daughter, none of which, or how many leopards. \n(Bies et al. 1995)" ;
        <http://www.w3.org/2000/01/rdf-schema#subClassOf>
                <http://purl.org/olia/olia.owl#NounPhrase> ;
        <http://www.w3.org/2002/07/owl#versionInfo>
                "added in conformance with PTB bracketing guidelines (Santorini 1991, Bies et al. 1995)" .

<http://purl.org/olia/olia.owl#AversiveCase>
        a       <http://www.w3.org/2002/07/owl#Class> ;
        <http://www.w3.org/2000/01/rdf-schema#comment>
                "AversiveCase expresses fear or is literally\n                        translated as 'turning from' in some languages [Blake 2001:\n                        156]." ;
        <http://www.w3.org/2000/01/rdf-schema#isDefinedBy>
                "http://www.isocat.org/datcat/DC-3096" ;
        <http://www.w3.org/2000/01/rdf-schema#subClassOf>
                <http://purl.org/olia/olia-top.owl#CaseFeature> .

<http://purl.org/olia/olia.owl#PossessiveRelativePronoun>
        a       <http://www.w3.org/2002/07/owl#Class> ;
        <http://www.w3.org/2000/01/rdf-schema#comment>
                "A relative pronoun whose antecedent is the possessor of the subject or object in the relative clause." ;
        <http://www.w3.org/2000/01/rdf-schema#isDefinedBy>
                "http://www.isocat.org/datcat/DC-3005" ;
        <http://www.w3.org/2002/07/owl#equivalentClass>
                [ a       <http://www.w3.org/2002/07/owl#Class> ;
                  <http://www.w3.org/2002/07/owl#intersectionOf>
                          ( <http://purl.org/olia/olia.owl#PossessivePronoun> <http://purl.org/olia/olia.owl#RelativePronoun> )
                ] ;
        <http://www.w3.org/2002/07/owl#versionInfo>
                "here \"Pronoun\" seems to refer to attributive pronoun, as the corresponding possessiverelativeDeterminer is not found in ISOcat\n\t\t(substitutive possessive relative pronouns [without accompanying noun] do exist, but are comparably marked, cf. \"I remember whose lines these are.\" vs. \"I remember certain lines and whose they are.\" In this example, the latter is actually an elliptical construction with an elided head noun)" .

<http://purl.org/olia/olia-top.owl#AspectFeature>
        a       <http://www.w3.org/2002/07/owl#Class> ;
        <http://www.w3.org/2000/01/rdf-schema#subClassOf>
                [ a       <http://www.w3.org/2002/07/owl#Restriction> ;
                  <http://www.w3.org/2002/07/owl#hasSelf>
                          true ;
                  <http://www.w3.org/2002/07/owl#onProperty>
                          <http://purl.org/olia/olia.owl#hasAspect>
                ] ;
        <http://www.w3.org/2000/01/rdf-schema#subClassOf>
                [ a       <http://www.w3.org/2002/07/owl#Restriction> ;
                  <http://www.w3.org/2002/07/owl#hasSelf>
                          true ;
                  <http://www.w3.org/2002/07/owl#onProperty>
                          <http://purl.org/olia/olia.owl#hasAspect>
                ] .

<http://purl.org/olia/olia.owl#hasOwnedNumber>
        a       <http://www.w3.org/2002/07/owl#ObjectProperty> ;
        <http://www.w3.org/2000/01/rdf-schema#comment>
                "\n                            Indication concerning the number of the possessed thing.\n                                (http://www.isocat.org/datcat/DC-1930)\n                            " ;
        <http://www.w3.org/2000/01/rdf-schema#label>
                "owned number" ;
        <http://www.w3.org/2000/01/rdf-schema#range>
                <http://purl.org/olia/olia-top.owl#NumberFeature> ;
        <http://www.w3.org/2000/01/rdf-schema#subPropertyOf>
                <http://purl.org/olia/olia.owl#hasNumber> ;
        <http://www.w3.org/2002/07/owl#versionInfo>
                "http://www.isocat.org/datcat/DC-1930" .

<http://purl.org/olia/olia.owl#InessiveCase>
        a       <http://www.w3.org/2002/07/owl#Class> ;
        <http://www.w3.org/2000/01/rdf-schema#comment>
                "\n\t\t\tInessiveCase expresses that  the referent of the noun it marks is\n\t\t\tthe location within which another referent exists. It has the \n\t\t\tmeaning of 'within' or 'inside' (Lyons 1968: 299; Gove, et al. \n\t\t\t1966: 1156; Crystal 1985: 156). X in Y.\n\t\t\t(http://purl.org/linguistics/gold/Inessive)\n\t\t" ;
        <http://www.w3.org/2000/01/rdf-schema#subClassOf>
                <http://purl.org/olia/olia-top.owl#CaseFeature> ;
        <http://www.w3.org/2002/07/owl#versionInfo>
                "http://purl.org/linguistics/gold/Inessive, http://www.isocat.org/datcat/DC-1311" .

<http://purl.org/olia/olia.owl#Multal>
        a       <http://www.w3.org/2002/07/owl#Class> ;
        <http://www.w3.org/2000/01/rdf-schema#comment>
                "Multal is a number property that refers to a\n                        large number of individuals." ;
        <http://www.w3.org/2000/01/rdf-schema#isDefinedBy>
                "http://www.isocat.org/datcat/DC-3327" ;
        <http://www.w3.org/2000/01/rdf-schema#label>
                "multal number" ;
        <http://www.w3.org/2000/01/rdf-schema#subClassOf>
                <http://purl.org/olia/olia-top.owl#NumberFeature> .

<http://purl.org/olia/olia.owl#CosubordinateClause>
        a       <http://www.w3.org/2002/07/owl#Class> ;
        <http://www.w3.org/2000/01/rdf-schema#subClassOf>
                <http://purl.org/olia/olia.owl#CoordinateClause> ;
        <http://www.w3.org/2002/07/owl#versionInfo>
                "\n\t\t\thttp://languagelink.let.uu.nl/tds/onto/LinguisticOntology.owl#non-embeddedSubordinateClause\n\t\t\tTermed \"cosubordination\" here in accordance with van Valin and LaPolla (1997)\n\t\t" .

<http://purl.org/olia/olia.owl#NonInitialCoordinatingConjunction>
        a       <http://www.w3.org/2002/07/owl#Class> ;
        <http://www.w3.org/2000/01/rdf-schema#comment>
                "\n\t\t\tWhen two distinct words occur, as in German weder...noch..., then the second is given the Non-initial value. \n\t\t\t(http://www.ilc.cnr.it/EAGLES96/annotate/node18.html#oav1av  17.11.06)\n\t\t" ;
        <http://www.w3.org/2000/01/rdf-schema#subClassOf>
                <http://purl.org/olia/olia.owl#CoordinatingConjunction> ;
        <http://www.w3.org/2002/07/owl#versionInfo>
                "EAGLES" .

<http://purl.org/olia/olia.owl#ElementWithClitic>
        a       <http://www.w3.org/2002/07/owl#Class> ;
        <http://www.w3.org/2000/01/rdf-schema#comment>
                "Expression representing a lexeme together with its clitics (Chiarcos)" ;
        <http://www.w3.org/2000/01/rdf-schema#subClassOf>
                <http://purl.org/olia/olia.owl#Cliticization> ;
        <http://www.w3.org/2002/07/owl#versionInfo>
                "http://purl.org/olia/mte/multext-east.owl#ElementWithClitic\"" .

<http://purl.org/olia/olia.owl#InablativeCase>
        a       <http://www.w3.org/2002/07/owl#Class> ;
        <http://www.w3.org/2000/01/rdf-schema#comment>
                "\n\t\t\tInablativeCase expresses that  the referent of the noun it marks is \n\t\t\tthe location from within which another referent is moving. It has \n\t\t\tthe meaning 'from within'.\n\t\t\t(http://purl.org/linguistics/gold/Inablative)\n\t\t" ;
        <http://www.w3.org/2000/01/rdf-schema#subClassOf>
                <http://purl.org/olia/olia-top.owl#CaseFeature> ;
        <http://www.w3.org/2002/07/owl#versionInfo>
                "http://purl.org/linguistics/gold/Inablative" .

<http://purl.org/olia/olia.owl#IncorporatingAntipassive>
        a       <http://www.w3.org/2002/07/owl#Class> ;
        <http://www.w3.org/2000/01/rdf-schema#comment>
                "\n\t\t\tBlocks the P or logical object (basic absolutive) nominal from being assigned Focus salience. \n\t\t\tThis correlates with the P's morphosyntactic downgrading, whereby it becomes insusceptible to \n\t\t\tany informational salience assignment. (Klaiman 1991:236)\n\t\t\t(http://purl.org/linguistics/gold/IncorporatingAntipassive)\n\t\t" ;
        <http://www.w3.org/2000/01/rdf-schema#subClassOf>
                <http://purl.org/olia/olia.owl#Antipassive> ;
        <http://www.w3.org/2002/07/owl#versionInfo>
                "http://purl.org/linguistics/gold/IncorporatingAntipassive" .

<http://purl.org/olia/olia.owl#ModalityMarkingAdverb>
        a       <http://www.w3.org/2002/07/owl#Class> ;
        <http://www.w3.org/2000/01/rdf-schema#comment>
                "A modality-marking adverb is a verbal particle that serves to indicate mood, aspect and/or tense (cf. Schmidt 1999).\n\t\t\tNote that this is not to be confused with the conventional meaning of \"modal adverb\" in the sense of \"manner adverb\" (cf. http://en.wiktionary.org/wiki/Category:English_modal_adverbs), \n\t\t\thence the uncommon name.\n\t\t\n\t\tRuth Laila Schmidt (1999) Urdu, an essential grammar, Routledge, London.\n\t\t" ;
        <http://www.w3.org/2000/01/rdf-schema#subClassOf>
                <http://purl.org/olia/olia.owl#VerbalParticle> , <http://purl.org/olia/olia.owl#Adverb> ;
        <http://www.w3.org/2002/07/owl#versionInfo>
                "despite the deviating terminology, this seems to be a subconcept of VerbalParticle, and maybe, it corresponds to ModalParticle (but only if the DCR definition is incorrect)" , "introduced for http://purl.org/olia/emille.owl#NegativeModalAdverb in the EMILLE tagset (Hardie 2003) for Urdu" .

<http://purl.org/olia/olia.owl#WeakInflection>
        a       <http://www.w3.org/2002/07/owl#Class> ;
        <http://www.w3.org/2000/01/rdf-schema#comment>
                "\n\t\t\tGerman adjectives take the endings of the weak inflection \n\t\t\twhen a determiner expresses number, gender and case.\n\t\t\tThe weak adjective inflection has only two endings: –e and –en. \n\t\t\t(http://www.canoo.net/services/OnlineGrammar/Wort/Adjektiv/Deklinationstyp/Schwach.html  20.11.06)\n\t\t\tIn other Germanic languages, similar systems exist.\n\t\t\t\n\t\t\tWeak inflection is a characteristic of lexemes, not individual tokens.\n\t\t" ;
        <http://www.w3.org/2000/01/rdf-schema#subClassOf>
                <http://purl.org/olia/olia-top.owl#InflectionTypeFeature> ;
        <http://www.w3.org/2002/07/owl#versionInfo>
                "EAGLES" .

<http://purl.org/olia/olia.owl#Feminine>
        a       <http://www.w3.org/2002/07/owl#Class> ;
        <http://www.w3.org/2000/01/rdf-schema#comment>
                "\n\t\t\tFeminine gender is a grammatical gender that marks nouns, articles, \n\t\t\tpronouns, etc. that have human or animal female referents, and often \n\t\t\tmarks nouns that have referents that do not carry distinctions of sex. \n\t\t\t(http://www.ilc.cnr.it/EAGLES96/annotate/node19.html#oav2at  17.11.06)\n\t\t" ;
        <http://www.w3.org/2000/01/rdf-schema#subClassOf>
                <http://purl.org/olia/olia-top.owl#GenderFeature> ;
        <http://www.w3.org/2002/07/owl#versionInfo>
                "EAGLES, http://languagelink.let.uu.nl/tds/onto/LinguisticOntology.owl#feminineGender" .

<http://purl.org/olia/olia.owl#SecondPersonPronoun>
        a       <http://www.w3.org/2002/07/owl#Class> ;
        <http://www.w3.org/2000/01/rdf-schema#comment>
                "\n\t\t\tSecond person deixis means deictic reference to a person or persons identified as addressee.\n\t\t\t(http://www.sil.org/linguistics/GlossaryOfLinguisticTerms/WhatIsSecondPersonDeixis.htm 19.09.06)\n\t\t" ;
        <http://www.w3.org/2000/01/rdf-schema#subClassOf>
                <http://purl.org/olia/olia.owl#PersReflPronoun> ;
        <http://www.w3.org/2002/07/owl#versionInfo>
                "\n\t\t\tEAGLES Pronoun with Person=\"Second\".\n\t\t\tAccording to Mish et al. (1990:878), this pertains to PersonalPronoun only (and ReflexivePronoun as German \"dich\"),\n\t\t\tso SecondPersonPronoun is modelled as a PersReflPronoun here.\n\t\t" , "TODO: Person as property" .

<http://purl.org/olia/olia-top.owl#PolarityFeature>
        a       <http://www.w3.org/2002/07/owl#Class> ;
        <http://www.w3.org/2000/01/rdf-schema#subClassOf>
                [ a       <http://www.w3.org/2002/07/owl#Restriction> ;
                  <http://www.w3.org/2002/07/owl#hasSelf>
                          true ;
                  <http://www.w3.org/2002/07/owl#onProperty>
                          <http://purl.org/olia/olia.owl#hasPolarity>
                ] ;
        <http://www.w3.org/2000/01/rdf-schema#subClassOf>
                [ a       <http://www.w3.org/2002/07/owl#Restriction> ;
                  <http://www.w3.org/2002/07/owl#hasSelf>
                          true ;
                  <http://www.w3.org/2002/07/owl#onProperty>
                          <http://purl.org/olia/olia.owl#hasPolarity>
                ] .

<http://purl.org/olia/olia.owl#hasClusivity>
        a       <http://www.w3.org/2002/07/owl#ObjectProperty> ;
        <http://www.w3.org/2000/01/rdf-schema#range>
                <http://purl.org/olia/olia-top.owl#ClusivityFeature> ;
        <http://www.w3.org/2000/01/rdf-schema#subPropertyOf>
                <http://purl.org/olia/system.owl#hasFeature> .

<http://purl.org/olia/olia.owl#PointOfViewAspect>
        a       <http://www.w3.org/2002/07/owl#Class> ;
        <http://www.w3.org/2000/01/rdf-schema#comment>
                "\n\t\t\tpoint of view aspect\n\t\t\t(http://languagelink.let.uu.nl/tds/onto/LinguisticOntology.owl#viewPointAspect)\n\t\t" ;
        <http://www.w3.org/2000/01/rdf-schema#subClassOf>
                <http://purl.org/olia/olia-top.owl#AspectFeature> ;
        <http://www.w3.org/2002/07/owl#versionInfo>
                "http://languagelink.let.uu.nl/tds/onto/LinguisticOntology.owl#viewPointAspect" .

<http://purl.org/olia/olia.owl#ThirdProximative>
        a       <http://www.w3.org/2002/07/owl#Class> ;
        <http://www.w3.org/2000/01/rdf-schema#comment>
                "\n\t\t\tProximative refers to one or more non-participants that are in some way \n\t\t\tdistinct/closer to the speaker  than other non-particpants.\n\t\t\t(http://purl.org/linguistics/gold/ThirdProximative)\n\t\t" ;
        <http://www.w3.org/2000/01/rdf-schema#subClassOf>
                <http://purl.org/olia/olia.owl#Third> ;
        <http://www.w3.org/2002/07/owl#versionInfo>
                "http://purl.org/linguistics/gold/ThirdProximative, modelled here under Third" .

<http://purl.org/olia/olia.owl#CoordinatingConjunction>
        a       <http://www.w3.org/2002/07/owl#Class> ;
        <http://www.w3.org/2000/01/rdf-schema#comment>
                "\n\t\t\tCoordinating conjunctions, also called coordinators, are conjunctions that \n\t\t\tjoin two items of equal syntactic importance.\n\t\t\t(http://en.wikipedia.org/wiki/Grammatical_conjunction 19.09.06)\n\t\t" ;
        <http://www.w3.org/2000/01/rdf-schema#subClassOf>
                <http://purl.org/olia/olia.owl#Conjunction> ;
        <http://www.w3.org/2002/07/owl#versionInfo>
                "EAGLES Conjunction with Type=\"Coordinating\".\n\t\t\tEAGLES' optional CoordType attribute subclassifies coordinating conjunctions, with respect to positional characteristics (repetition/pairing of expressions forming complex conjunctions). (http://www.ilc.cnr.it/EAGLES96/annotate/node18.html#oav1av  17.11.06)\n\t\t\t\t\tCoordType was originally implemented as MorphosyntacticFeature, the new modelling follows the MULTEXT-East ontology (http://purl.org/olia/mte/multext-east.owl#CoordinatingConjunction_PositionalType)\n\t\t" .

<http://purl.org/olia/olia.owl#OtherSourceEvidentiality>
        a       <http://www.w3.org/2002/07/owl#Class> ;
        <http://www.w3.org/2000/01/rdf-schema#comment>
                "An indication that the source of information is\n                        someone other than the speaker. [Aikhenvald 2006: 106]" ;
        <http://www.w3.org/2000/01/rdf-schema#isDefinedBy>
                "http://www.isocat.org/datcat/DC-3367" ;
        <http://www.w3.org/2000/01/rdf-schema#subClassOf>
                <http://purl.org/olia/olia-top.owl#EvidentialityFeature> .

<http://purl.org/olia/olia.owl#SemiColon>
        a       <http://www.w3.org/2002/07/owl#Class> ;
        <http://www.w3.org/2000/01/rdf-schema#comment>
                "\n                            Sign (;) usually used to separate phrases.\n                                (http://www.isocat.org/datcat/DC-1446)\n                            " ;
        <http://www.w3.org/2000/01/rdf-schema#label>
                "semi-colon" ;
        <http://www.w3.org/2000/01/rdf-schema#subClassOf>
                <http://purl.org/olia/olia.owl#SentenceMedialPunctuation> ;
        <http://www.w3.org/2002/07/owl#versionInfo>
                "http://www.isocat.org/datcat/DC-1446" , "subClassOf partOfSpeech (dcif:conceptualDomain)" .

<http://purl.org/olia/olia.owl#Initial>
        a       <http://www.w3.org/2002/07/owl#Class> ;
        <http://www.w3.org/2000/01/rdf-schema#comment>
                "\n\t\t\tWhen two distinct words occur, as in German \"weder...noch...\", then \n\t\t\tthe first is given the Initial value. \n\t\t\t(http://www.ilc.cnr.it/EAGLES96/annotate/node18.html#oav1av  17.11.06)\n\t\t" ;
        <http://www.w3.org/2000/01/rdf-schema#subClassOf>
                <http://purl.org/olia/olia-top.owl#CoordTypeFeature> ;
        <http://www.w3.org/2002/07/owl#deprecated>
                true ;
        <http://www.w3.org/2002/07/owl#versionInfo>
                "EAGLES, reimplemented as subhierarchy of CoordinatingConjunction" .

<http://purl.org/olia/olia.owl#PassiveVoice>
        a       <http://www.w3.org/2002/07/owl#Class> ;
        <http://www.w3.org/2000/01/rdf-schema#comment>
                "\n\t\t\tWhen the subject is the patient, target or undergoer of the action, \n\t\t\tit is said to be in the passive voice. \n\t\t\t(http://en.wikipedia.org/wiki/Grammatical_voice  17.11.06)\n\t\t\t\n\t\t\tWhen the subject is the agent or actor of the verb, the verb is said \n\t\t\tto be in the active voice. When the subject is the patient, target or\n\t\t\tundergoer of the action, it is said to be in the passive voice.\n\t\t\t(http://languagelink.let.uu.nl/tds/onto/LinguisticOntology.owl#passiveVoice)\n\t\t\t\n\t\t\tPassive is often not clearly distinguished from Inverse: According to Givón (1988),\n\t\t\tInverse is characterized by obligatory realization of the suppressed agent,\n\t\t\twhereas the realization of the agent in a passive construction is optional \n\t\t\t(or impossible).\n\t\t\tThis restrictive definition of passive does, however, conflict with the \n\t\t\tuse of the term \"passive\" for European languages. Then, English and German \n\t\t\t\"Passive\" would be Inverses. Therefore, Inverse is a subconcept of Passive here.\n\t\t\tGivón's original Passive is NonInversePassive.\n\t\t" ;
        <http://www.w3.org/2000/01/rdf-schema#isDefinedBy>
                "http://www.isocat.org/datcat/DC-3839" ;
        <http://www.w3.org/2000/01/rdf-schema#subClassOf>
                <http://purl.org/olia/olia-top.owl#VoiceFeature> ;
        <http://www.w3.org/2002/07/owl#versionInfo>
                "http://languagelink.let.uu.nl/tds/onto/LinguisticOntology.owl#passiveVoice" .

<http://purl.org/olia/olia.owl#DirectSpeech>
        a       <http://www.w3.org/2002/07/owl#Class> ;
        <http://www.w3.org/2000/01/rdf-schema#comment>
                "added in accordance with TIGER" ;
        <http://www.w3.org/2000/01/rdf-schema#subClassOf>
                <http://purl.org/olia/olia-top.owl#NarrativeType> ;
        <http://www.w3.org/2002/07/owl#versionInfo>
                "added in accordance with TIGER" .

<http://purl.org/olia/olia.owl#DynamicAspect>
        a       <http://www.w3.org/2002/07/owl#Class> ;
        <http://www.w3.org/2000/01/rdf-schema#comment>
                "\n\t\t\tdynamic aspect\n\t\t\t(http://languagelink.let.uu.nl/tds/onto/LinguisticOntology.owl#dynamicityAspect)\n\t\t" ;
        <http://www.w3.org/2000/01/rdf-schema#subClassOf>
                <http://purl.org/olia/olia-top.owl#AspectFeature> ;
        <http://www.w3.org/2002/07/owl#versionInfo>
                "http://languagelink.let.uu.nl/tds/onto/LinguisticOntology.owl#dynamicityAspect" .

<http://purl.org/olia/olia.owl#AbsoluteTense>
        a       <http://www.w3.org/2002/07/owl#Class> ;
        <http://www.w3.org/2000/01/rdf-schema#comment>
                "\n\t\t\tAbsolute tense refers to a time in relation to the moment of utterance. \n\t\t\t(http://languagelink.let.uu.nl/tds/onto/LinguisticOntology.owl#absoluteTense with \n\t\t\treference to http://www.sil.org/linguistics/glossaryoflinguisticterms/whatisabsolutetense.htm\")\n\t\t" ;
        <http://www.w3.org/2000/01/rdf-schema#label>
                "absolute tense" ;
        <http://www.w3.org/2000/01/rdf-schema#subClassOf>
                <http://purl.org/olia/olia-top.owl#TenseFeature> ;
        <http://www.w3.org/2002/07/owl#versionInfo>
                "http://languagelink.let.uu.nl/tds/onto/LinguisticOntology.owl#absoluteTense" .

<http://purl.org/olia/olia-top.owl#PersonFeature>
        a       <http://www.w3.org/2002/07/owl#Class> ;
        <http://www.w3.org/2000/01/rdf-schema#subClassOf>
                [ a       <http://www.w3.org/2002/07/owl#Restriction> ;
                  <http://www.w3.org/2002/07/owl#hasSelf>
                          true ;
                  <http://www.w3.org/2002/07/owl#onProperty>
                          <http://purl.org/olia/olia.owl#hasPerson>
                ] .

<http://purl.org/olia/olia.owl#hasReduplicationType>
        a       <http://www.w3.org/2002/07/owl#ObjectProperty> ;
        <http://www.w3.org/2000/01/rdf-schema#range>
                <http://purl.org/olia/olia-top.owl#ReduplicationTypeFeature> ;
        <http://www.w3.org/2000/01/rdf-schema#subPropertyOf>
                <http://purl.org/olia/system.owl#hasFeature> ;
        <http://www.w3.org/2002/07/owl#versionInfo>
                "cf. http://www.isocat.org/datcat/DC-2240" .

<http://purl.org/olia/olia.owl#MalefactorRole>
        a       <http://www.w3.org/2002/07/owl#Class> ;
        <http://www.w3.org/2000/01/rdf-schema#comment>
                "\n\t\t\tA maleficiary (malefactor) instantiates the role of an entity (usually animate) who \n\t\t\tstands to undergoe a misfortune, or be at a disadvantage in some way from \n\t\t\tthe event.\n\t\t\t(http://languagelink.let.uu.nl/tds/onto/LinguisticOntology.owl#maleficiaryRole)\n\t\t" ;
        <http://www.w3.org/2000/01/rdf-schema#subClassOf>
                <http://purl.org/olia/olia.owl#UndergoerMacroRole> ;
        <http://www.w3.org/2002/07/owl#versionInfo>
                "http://languagelink.let.uu.nl/tds/onto/LinguisticOntology.owl#maleficiaryRole" .

<http://purl.org/olia/olia.owl#hasDefiniteness>
        a       <http://www.w3.org/2002/07/owl#ObjectProperty> ;
        <http://www.w3.org/2000/01/rdf-schema#range>
                <http://purl.org/olia/olia-top.owl#DefinitenessFeature> ;
        <http://www.w3.org/2000/01/rdf-schema#subPropertyOf>
                <http://purl.org/olia/system.owl#hasFeature> .

<http://purl.org/olia/olia-top.owl#NumberFeature>
        a       <http://www.w3.org/2002/07/owl#Class> ;
        <http://www.w3.org/2000/01/rdf-schema#subClassOf>
                [ a       <http://www.w3.org/2002/07/owl#Restriction> ;
                  <http://www.w3.org/2002/07/owl#hasSelf>
                          true ;
                  <http://www.w3.org/2002/07/owl#onProperty>
                          <http://purl.org/olia/olia.owl#hasNumber>
                ] ;
        <http://www.w3.org/2000/01/rdf-schema#subClassOf>
                [ a       <http://www.w3.org/2002/07/owl#Restriction> ;
                  <http://www.w3.org/2002/07/owl#hasSelf>
                          true ;
                  <http://www.w3.org/2002/07/owl#onProperty>
                          <http://purl.org/olia/olia.owl#hasNumber>
                ] ;
        <http://www.w3.org/2002/07/owl#versionInfo>
                "TODO: extend with TDS numberProperty and GOLD NumberValue" .

<http://purl.org/olia/olia.owl#Masculine>
        a       <http://www.w3.org/2002/07/owl#Class> ;
        <http://www.w3.org/2000/01/rdf-schema#comment>
                "\n\t\t\tMasculine gender is a grammatical gender that marks nouns, articles, \n\t\t\tpronouns, etc.  having human or animal male referents, and often marks \n\t\t\tnouns having referents that do not have distinctions of sex. \t\t\n\t\t\t(http://www.sil.org/linguistics/glossaryoflinguisticterms/WhatIsMasculineGender.htm  17.11.06)\n\t\t" ;
        <http://www.w3.org/2000/01/rdf-schema#subClassOf>
                <http://purl.org/olia/olia-top.owl#GenderFeature> ;
        <http://www.w3.org/2002/07/owl#versionInfo>
                "EAGLES, http://languagelink.let.uu.nl/tds/onto/LinguisticOntology.owl#masculineGender" .

<http://purl.org/olia/olia.owl#TenseMarkingAuxiliary>
        a       <http://www.w3.org/2002/07/owl#Class> ;
        <http://www.w3.org/2000/01/rdf-schema#comment>
                "An auxiliary that marks exclusively tense, e.g., in Urdu:\n\t\t\t\n\t\t\tAuxiliaries:\n\t\t\tBased on the syntactic nature of Urdu, auxiliaries are divided into two categories. Aspectual\n\t\t\tauxiliaries always occur after main verb of the sentence. Tense auxiliaries are used to show the\n\t\t\ttime of the action. They occurred at the end of the verb phrase. (Sajjad 2007).\n\t\t\t\n\t\t\tIn Urdu, the auxiliary gā indicates future tense when it follows a verb in the subjunctive\n\t\t\tform. (http://purl.org/olia/emille.owl#GaAuxiliary)\n\t\t" ;
        <http://www.w3.org/2000/01/rdf-schema#subClassOf>
                <http://purl.org/olia/olia.owl#StrictAuxiliaryVerb> ;
        <http://www.w3.org/2002/07/owl#versionInfo>
                "adopted from Sajjad (2007) for Urdu, cf. http://purl.org/olia/urdu.owl#TenseAuxiliary" .

<http://purl.org/olia/olia.owl#PossessiveDeterminer>
        a       <http://www.w3.org/2002/07/owl#Class> ;
        <http://www.w3.org/2000/01/rdf-schema#comment>
                "\n\t\t\tA possessive determiner is a part of speech that modifies a noun \n\t\t\tby attributing ownership to someone or something.\n\t\t\t(http://en.wikipedia.org/wiki/Possessive_adjective 19.09.06)\n\t\t" ;
        <http://www.w3.org/2000/01/rdf-schema#subClassOf>
                <http://purl.org/olia/olia.owl#AttributivePronoun> , <http://purl.org/olia/olia.owl#PossessivePronoun> ;
        <http://www.w3.org/2002/07/owl#versionInfo>
                "EAGLES Determiner with DetType=\"Possessive\"." .

<http://purl.org/olia/olia.owl#FamiliarSecondPersonPronoun>
        a       <http://www.w3.org/2002/07/owl#Class> ;
        <http://www.w3.org/2000/01/rdf-schema#comment>
                "\n\t\t\tIn several European languages exist special forms of pronouns for polite or respectful reference,\n\t\t\te.g. Dutch u and Spanish usted. The concept FamiliarSecondPersonPronoun applies to the corresponding unmarked forms for \n\t\t\tinformal conversiation in such languages.\n\t\t\t(http://www.ilc.cnr.it/EAGLES96/annotate/node18.html#oav1p 19.09.06)\n\t\t" ;
        <http://www.w3.org/2000/01/rdf-schema#subClassOf>
                <http://purl.org/olia/olia.owl#SecondPersonPronoun> ;
        <http://www.w3.org/2002/07/owl#versionInfo>
                "EAGLES PersonalPronoun with Politeness=\"Familiar\". \n\t\t\tThe EAGLES attribute politeness (polite/ familiar) is limited to second-person pronouns.\n\t\t" .

<http://purl.org/olia/olia.owl#LeftParentheticalPunctuation>
        a       <http://www.w3.org/2002/07/owl#Class> ;
        <http://www.w3.org/2000/01/rdf-schema#comment>
                "\n\t\t\tBeginning of a paired punctuation.\n            (http://www.isocat.org/datcat/DC-2078)\n        " ;
        <http://www.w3.org/2000/01/rdf-schema#subClassOf>
                <http://purl.org/olia/olia.owl#ParentheticalPunctuation> ;
        <http://www.w3.org/2002/07/owl#versionInfo>
                "TODO: rename to OpeningPerentheticalPunctuation to support scripts running from left to right." , "TODO: rename to OpenPunctuation" , "added in accordance with a suggestion by Wilson and Leech (1996); http://www.isocat.org/datcat/DC-2078 (open punctuation)" .

<http://purl.org/olia/olia.owl#TransitiveSubject>
        a       <http://www.w3.org/2002/07/owl#Class> ;
        <http://www.w3.org/2000/01/rdf-schema#comment>
                "\n\t\t\tFirst argument of a transitive or ditransitive verb.\n\t\t\t(http://languagelink.let.uu.nl/tds/onto/LinguisticOntology.owl#A)\n\t\t" ;
        <http://www.w3.org/2000/01/rdf-schema#subClassOf>
                <http://purl.org/olia/olia.owl#SyntacticSubject> ;
        <http://www.w3.org/2002/07/owl#versionInfo>
                "http://languagelink.let.uu.nl/tds/onto/LinguisticOntology.owl#A" .

<http://purl.org/olia/olia.owl#ExpletiveArgument>
        a       <http://www.w3.org/2002/07/owl#Class> ;
        <http://www.w3.org/2000/01/rdf-schema#comment>
                "\n\t\t\tThree different expletive usages [of the German expletive pronoun es]\n\t\t\tare traditionally distinguished: formal subject or object (expletive argument), \n\t\t\tcorrelate of an extraposed clausal argument (expletive correlate), and Vorfeld-es (structural expletive)\n\t\t\t(cf. (Eisenberg 1999 2001), (Pütz 1986)). ...\n\t\t\t\n\t\t\tThe formal subject obligatorily occurs with weather verbs, e.g. \"Es regnet\" and unpersonal\n\t\t\tor agentless constructions such as \"Es gibt so eine Buchung\" or \"Es geht um populäre Unterhaltung.\" \n\t\t\tSome verbs optionally permit an expletive subject but also occur with referential subjects such as \n\t\t\t\"Max/Es kopft an der Tür.\" A formal object is found in constructions like\n\t\t\t\"jmd. legt es an auf etw.\" or \"jmd. verdirbt es mit jmdm.\" In all examples mentioned, es\n\t\t\tfunctions as a grammatical argument without semantic contribution, i.e. it does not refer\n\t\t\tto a person, object, or event.\n\t\t\t(Telljohann et al. 2009, p.60f)\n\t\t" ;
        <http://www.w3.org/2000/01/rdf-schema#subClassOf>
                <http://purl.org/olia/olia.owl#ExpletivePronoun> ;
        <http://www.w3.org/2002/07/owl#versionInfo>
                "\n\t\t\tTüBa-D/Z\n\t\t" .

<http://purl.org/olia/olia.owl#RelativePresent>
        a       <http://www.w3.org/2002/07/owl#Class> ;
        <http://www.w3.org/2000/01/rdf-schema#comment>
                "\n\t\t\tRelativePresentTense locates the situation in question simultaneously \n\t\t\twith some contextually determined temporal reference point.\n\t\t\t(http://purl.org/linguistics/gold/RelativePresent)\n\t\t" ;
        <http://www.w3.org/2000/01/rdf-schema#subClassOf>
                <http://purl.org/olia/olia.owl#RelativeTense> ;
        <http://www.w3.org/2002/07/owl#versionInfo>
                "http://purl.org/linguistics/gold/RelativePresent" .

<http://purl.org/olia/olia.owl#Honorific>
        a       <http://www.w3.org/2002/07/owl#Class> ;
        <http://www.w3.org/2000/01/rdf-schema#comment>
                "\n                            special form of language used when talking about those in positions of social situation\n                                (http://www.isocat.org/datcat/DC-2347)\n                            " ;
        <http://www.w3.org/2000/01/rdf-schema#label>
                "honorific" ;
        <http://www.w3.org/2000/01/rdf-schema#subClassOf>
                <http://purl.org/olia/olia.owl#Possible> ;
        <http://www.w3.org/2002/07/owl#versionInfo>
                "http://www.isocat.org/datcat/DC-2347" .

<http://purl.org/olia/olia.owl#InterrogativePronoun>
        a       <http://www.w3.org/2002/07/owl#Class> ;
        <http://www.w3.org/2000/01/rdf-schema#comment>
                "\n\t\t\tA interrogative pronoun is a pro-form that is used in questions in place of the item questioned for.\n\t\t\t(http://www.sil.org/linguistics/GlossaryOfLinguisticTerms/WhatIsAnInterrogativeProForm.htm 19.09.06)\n\t\t" ;
        <http://www.w3.org/2000/01/rdf-schema#subClassOf>
                <http://purl.org/olia/olia.owl#WHPronoun> ;
        <http://www.w3.org/2002/07/owl#equivalentClass>
                [ a       <http://www.w3.org/2002/07/owl#Class> ;
                  <http://www.w3.org/2002/07/owl#intersectionOf>
                          ( <http://purl.org/olia/olia.owl#WHPronoun> <http://purl.org/olia/olia.owl#QuestionWord> )
                ] ;
        <http://www.w3.org/2002/07/owl#versionInfo>
                "EAGLES WHPronoun with Wh-Type=\"Interrogative\"." .

<http://purl.org/olia/olia.owl#EpistemicNecessityModality>
        a       <http://www.w3.org/2002/07/owl#Class> ;
        <http://www.w3.org/2000/01/rdf-schema#comment>
                "EpistemicNecessityModality indicates that the\n                        expressed proposition is known to be true. Also known as CategoricalModality\n                        [Palmer 2001: 37, 68-69]." ;
        <http://www.w3.org/2000/01/rdf-schema#isDefinedBy>
                "http://www.isocat.org/datcat/DC-3180" ;
        <http://www.w3.org/2000/01/rdf-schema#label>
                "categorical modality" , "epistemic necessitiy modality" ;
        <http://www.w3.org/2000/01/rdf-schema#subClassOf>
                <http://purl.org/olia/olia-top.owl#ModalityFeature> .

<http://purl.org/olia/olia.owl#SyntacticSubject>
        a       <http://www.w3.org/2002/07/owl#Class> ;
        <http://www.w3.org/2000/01/rdf-schema#comment>
                "\t\n        The subject of a sentence is one of the two main parts of a sentence, \n        the other being the predicate. Providing an adequate definition of the \n        notion of a subject is notoriously difficult, and depends on a range \n        of grammatical properties that may vary from language to language. For \n        this reason, many current grammatical theories avoid using the term, \n        except for purely descriptive purposes, or define it in terms of \n        occupying a particular position in the clause. The term subject refers \n        to the grammatical function an expression may have in relation to \n        other expressions in a sentence, and it should be distinguished from \n        parts of speech, which classify expressions independently of their \n        relations to other constituents of a sentence.\n\n        The subject of a verb is the argument which generally refers to the \n        origin of the action or the undergoer of the state shown by the verb. \n        However, this definition depends on the particular language under \n        consideration. In languages where a passive voice exists, the subject \n        of a passive verb may be the target or result of the action. This is a \n        semantic definition. (http://en.wikipedia.org/wiki/Subject_(grammar)).\n\n\t\t(http://languagelink.let.uu.nl/tds/onto/LinguisticOntology.owl#syntacticSubject)\n\t\t" ;
        <http://www.w3.org/2000/01/rdf-schema#subClassOf>
                <http://purl.org/olia/olia.owl#SyntacticArgument> ;
        <http://www.w3.org/2002/07/owl#versionInfo>
                "http://languagelink.let.uu.nl/tds/onto/LinguisticOntology.owl#syntacticSubject" .

<http://purl.org/olia/olia.owl#MentalAbilitiveModality>
        a       <http://www.w3.org/2002/07/owl#Class> ;
        <http://www.w3.org/2000/01/rdf-schema#comment>
                "MentalAbilitiveModality indicates that an agent\n                        has the capacity to perform some mental action [Bybee, Perkins and Pagliuca\n                        1994: 192; Palmer 2001: 77]." ;
        <http://www.w3.org/2000/01/rdf-schema#isDefinedBy>
                "http://www.isocat.org/datcat/DC-3313" ;
        <http://www.w3.org/2000/01/rdf-schema#subClassOf>
                <http://purl.org/olia/olia.owl#AbilitativeModality> .

<http://purl.org/olia/olia.owl#Second>
        a       <http://www.w3.org/2002/07/owl#Class> ;
        <http://www.w3.org/2000/01/rdf-schema#comment>
                "\n\t\t\tRefers to the person(s) the speaker is addressing (Crystal 1997: 285).\n\t\t\t(http://purl.org/linguistics/gold/Second)\n\t\t" ;
        <http://www.w3.org/2000/01/rdf-schema#subClassOf>
                <http://purl.org/olia/olia-top.owl#PersonFeature> ;
        <http://www.w3.org/2002/07/owl#versionInfo>
                "EAGLES, http://purl.org/linguistics/gold/Second" .

<http://purl.org/olia/olia.owl#PrepositionalAdverb>
        a       <http://www.w3.org/2002/07/owl#Class> ;
        <http://www.w3.org/2000/01/rdf-schema#comment>
                "adverb which is very similar in its form to a preposition" ;
        <http://www.w3.org/2000/01/rdf-schema#isDefinedBy>
                "http://www.isocat.org/datcat/DC-3000" ;
        <http://www.w3.org/2000/01/rdf-schema#subClassOf>
                <http://purl.org/olia/olia.owl#Preposition> , <http://purl.org/olia/olia.owl#Adverb> .

<http://purl.org/olia/olia.owl#NonabsolutiveAntipassive>
        a       <http://www.w3.org/2002/07/owl#Class> ;
        <http://www.w3.org/2000/01/rdf-schema#comment>
                "\n\t\t\tAn Antipassive in which the P or logical object is overtly downgraded.  (Klaiman 1991:232)\n\t\t\t(http://purl.org/linguistics/gold/NonabsolutiveAntipassive)\n\t\t" ;
        <http://www.w3.org/2000/01/rdf-schema#subClassOf>
                <http://purl.org/olia/olia.owl#Antipassive> ;
        <http://www.w3.org/2002/07/owl#versionInfo>
                "http://purl.org/linguistics/gold/NonabsolutiveAntipassive" .

<http://purl.org/olia/olia.owl#Hyphen>
        a       <http://www.w3.org/2002/07/owl#Class> ;
        <http://www.w3.org/2000/01/rdf-schema#comment>
                "\n                            Punctuation that is graphically presented as \"-\".\n                                (http://www.isocat.org/datcat/DC-2077)\n                            " ;
        <http://www.w3.org/2000/01/rdf-schema#label>
                "hyphen" ;
        <http://www.w3.org/2000/01/rdf-schema#subClassOf>
                <http://purl.org/olia/olia.owl#SentenceMedialPunctuation> ;
        <http://www.w3.org/2002/07/owl#versionInfo>
                "http://www.isocat.org/datcat/DC-2077" .

<http://purl.org/olia/olia.owl#TerminativeAspect>
        a       <http://www.w3.org/2002/07/owl#Class> ;
        <http://www.w3.org/2000/01/rdf-schema#comment>
                "\n\t\t\tDenotes the termination of an event (Bhat 1999: 92).\n\t\t\t(http://purl.org/linguistics/gold/Terminative)\n\t\t" ;
        <http://www.w3.org/2000/01/rdf-schema#subClassOf>
                <http://purl.org/olia/olia-top.owl#AspectFeature> ;
        <http://www.w3.org/2002/07/owl#versionInfo>
                "http://purl.org/linguistics/gold/Terminative" .

<http://purl.org/olia/olia.owl#ExclamatoryDeterminer>
        a       <http://www.w3.org/2002/07/owl#Class> ;
        <http://www.w3.org/2000/01/rdf-schema#comment>
                "\n\t\t\tA exclamatory determiner is used in combination with a Nominal Phrase in order to create \n\t\t\tan exclamation (a more emphatic form of statement), e.g. \"What a lovely colour!\", \"What a wonderful day this is!\"\n\t\t\t(http://www.ilc.cnr.it/EAGLES96/pub/eagles/lexicons/elm_en.ps.gz, p.27, 07.05.07;\n\t\t\t http://en.wikipedia.org/wiki/Sentence_(linguistics), 07.05.07)\n\t\t" ;
        <http://www.w3.org/2000/01/rdf-schema#subClassOf>
                <http://purl.org/olia/olia.owl#WHDeterminer> ;
        <http://www.w3.org/2002/07/owl#versionInfo>
                "\n\t\t\tEAGLES Determiner with optional attribute WhType=\"Exclamatory\"\n\t\t" .

<http://purl.org/olia/olia.owl#QuantificationalAspect>
        a       <http://www.w3.org/2002/07/owl#Class> ;
        <http://www.w3.org/2000/01/rdf-schema#comment>
                "\n\t\t\tA speaker may report an event as occurring once only (semelfactive) or \n\t\t\tseveral times (iterative); he may view it as a specific event or as part \n\t\t\tof a general habit of carrying out similar events; he may also differentiate \n\t\t\tbetween different degrees of frequency with which the event occurs. The \n\t\t\tmarkers that a given language provides for one or more of these meaning \n\t\t\tdistinctions can be grouped under a subcategory called “quantificational \n\t\t\taspect\", as all of them refer to the quantitative aspect of the event \n\t\t\tconcerned (Bhat 1999:53).\n\t\t\t(http://purl.org/linguistics/gold/Quantificational)\n\t\t" ;
        <http://www.w3.org/2000/01/rdf-schema#subClassOf>
                <http://purl.org/olia/olia-top.owl#AspectFeature> ;
        <http://www.w3.org/2002/07/owl#versionInfo>
                "\n\t\t\thttp://purl.org/linguistics/gold/Quantificational,\n\t\t\thttp://languagelink.let.uu.nl/tds/onto/LinguisticOntology.owl#quantitativeAspect\n\t\t" .

<http://purl.org/olia/olia.owl#PresumptiveMood>
        a       <http://www.w3.org/2002/07/owl#Class> ;
        <http://www.w3.org/2000/01/rdf-schema#comment>
                "The presumptive mood is used in Romanian to express presupposition or hypothesis regarding the fact denoted by the verb, as well as other more or less similar attitudes: doubt, curiosity, concern, condition, indifference, inevitability. For example, acolo s-o fi dus \"he might have gone there\" shows the basic presupposition use, while the following excerpt from a poem by Eminescu shows the use both in a conditional clause de-o fi \"suppose it is\" and in a main clause showing an attitude of submission to fate le-om duce \"we would bear\".\n\t\t\t\n\t\t\tDe-o fi una, de-o fi alta... Ce e scris și pentru noi,\n\t\t\tBucuroși le-om duce toate, de e pace, de-i război.\n\t\t\t\n\t\t\tBe it one, be it the other... Whatever fate we have,\n\t\t\tWe will gladly go through all, be it peace or be it war \n\t\t\t(http://en.wikipedia.org/wiki/Irrealis_mood#Presumptive)\n\t\t" ;
        <http://www.w3.org/2000/01/rdf-schema#subClassOf>
                <http://purl.org/olia/olia.owl#PresumptiveModality> , <http://purl.org/olia/olia-top.owl#MoodFeature> ;
        <http://www.w3.org/2002/07/owl#versionInfo>
                "adopted from ILPOSTS (http://purl.org/olia/ilposts.owl#PresumptiveMood) for Indian languages" .

<http://purl.org/olia/olia.owl#HortativeModality>
        a       <http://www.w3.org/2002/07/owl#Class> ;
        <http://www.w3.org/2000/01/rdf-schema#comment>
                "A term sometimes used in the grammatical analysis of verbs, to refer to a type of modal meaning in which an exhortation is made. An example of a hortative usage ('a hortative') is the 'let us' construction in English ('let us pray'). [Crystal 2008: 232] (http://linguistics-ontology.org/gold/2010/HortatoryForce)" ;
        <http://www.w3.org/2000/01/rdf-schema#isDefinedBy>
                "http://linguistics-ontology.org/gold/2010/HortatoryForce" ;
        <http://www.w3.org/2000/01/rdf-schema#label>
                "hortative force" ;
        <http://www.w3.org/2000/01/rdf-schema#subClassOf>
                <http://purl.org/olia/olia.owl#ActionalModality> .

<http://purl.org/olia/olia.owl#LightVerb>
        a       <http://www.w3.org/2002/07/owl#Class> ;
        <http://www.w3.org/2000/01/rdf-schema#comment>
                "In linguistics, a light verb is a verb participating in complex predication that has little semantic content of its own, but provides through inflection some details on the event semantics, such as aspect, mood, or tense. The semantics of the compound, as well as its argument structure, are determined by the head or primary component of the compound, which may be a verb or noun (V+V or V+N compounds). Other names for \"light verb\" include: vector verb or explicator verb, emphasising its role within the compound; or thin verb or semantically weak verb, emphasising (as with \"light\") its lack of semantics. A \"semantically weak\" verb is not to be confused with a \"weak verb\" as in the Germanic weak inflection. Light verbs are similar to auxiliary verbs in some ways.\n\t\t\t\n\t\t\tMost English light verbs occur in V+N forms sometimes called \"stretched verbs\": for example, take in take a nap, where the primary sense is provided by \"nap\", and \"take\" is the light verb. The light verbs most common in these constructions are also common in phrasal verbs. A verb which is \"light\" in one context may be \"heavy\" in another: as with \"take\" in I will take a book to read.\n\t\t\t\n\t\t\tExamples in other languages include the Yiddish geb in geb a helf (literally give a help, \"help\"); the French faire in faire semblant (lit. make seeming, \"pretend\"); the Hindi nikal paRA (lit. leave fall, \"start to leave\"); and the bǎ construction in Chinese.[1] Some verbs are found in many such expressions; to reuse an earlier example, take is found in take a nap, take a shower, take a sip, take a bow, take turns, and so on. Light verbs are extremely common in Indo-Iranian languages, Japanese, and other languages in which verb compounding is a primary mechanism for marking aspectual distinctions.\n\t\t\t(http://en.wikipedia.org/wiki/Light_verb)" ;
        <http://www.w3.org/2000/01/rdf-schema#subClassOf>
                <http://purl.org/olia/olia.owl#Verb> ;
        <http://www.w3.org/2002/07/owl#versionInfo>
                "http://purl.org/olia/mte/multext-east.owl#LightVerb, for Farsi" .

<http://purl.org/olia/olia.owl#Frame>
        a       <http://www.w3.org/2002/07/owl#Class> ;
        <http://www.w3.org/2000/01/rdf-schema#comment>
                "According to \"Frame Semantics, deriving from the work of Charles J. Fillmore and colleagues (Fillmore 1976, 1977, 1982, 1985, Fillmore and Baker 2001, 2010) ... [,] the meanings of most words can best be understood on the basis of a semantic frame: a description of a type of event, relation, or entity and the participants in it. For example, the concept of cooking typically involves a person doing the cooking (Cook), the food that is to be cooked (Food), something to hold the food while cooking (Container) and a source of heat (Heating_instrument).\" (https://framenet.icsi.berkeley.edu/fndrupal/about)" ;
        <http://www.w3.org/2000/01/rdf-schema#subClassOf>
                <http://purl.org/olia/olia.owl#LexicalUnit> ;
        <http://www.w3.org/2002/07/owl#versionInfo>
                "Introduced to account for semantic frames in lexinfo, note that full-fledged semantic role annotation is subject to specialized resources (FrameNet, Verbnet, etc.) and beyond the scope of OLiA. For compliance with lexinfo, however, these have been added to OLiA." .

<http://purl.org/olia/olia.owl#DurativeAspect>
        a       <http://www.w3.org/2002/07/owl#Class> ;
        <http://www.w3.org/2000/01/rdf-schema#comment>
                "\n\t\t\tEvents which involve some duration (Bhat 1999:58).\n\t\t\t(http://purl.org/linguistics/gold/Durative)\n\t\t" ;
        <http://www.w3.org/2000/01/rdf-schema#subClassOf>
                <http://purl.org/olia/olia-top.owl#AspectFeature> ;
        <http://www.w3.org/2002/07/owl#versionInfo>
                "http://purl.org/linguistics/gold/Durative" .

<http://purl.org/olia/olia.owl#AblativeCase>
        a       <http://www.w3.org/2002/07/owl#Class> ;
        <http://www.w3.org/2000/01/rdf-schema#comment>
                "\n\t\t\tCase used to indicate locative or instrumental function.\n\t\t\t(http://www.isocat.org/datcat/DC-1224)\n\t\t\n\t\t\tAblativeCase expresses that  the referent of the noun it marks is \n\t\t\tthe location from which another referent is moving. It has the \n\t\t\tmeaning 'from'.\n\t\t\t(http://purl.org/linguistics/gold/Ablative)\n\t\t" ;
        <http://www.w3.org/2000/01/rdf-schema#subClassOf>
                <http://purl.org/olia/olia-top.owl#CaseFeature> ;
        <http://www.w3.org/2002/07/owl#versionInfo>
                "http://purl.org/linguistics/gold/Ablative, http://www.isocat.org/datcat/DC-1224" .

<http://purl.org/olia/olia.owl#IndirectObject>
        a       <http://www.w3.org/2002/07/owl#Class> ;
        <http://www.w3.org/2000/01/rdf-schema#comment>
                "\n\t\t\t An indirect object is a grammatical relation that is one means of    \n\t\t\t expressing the semantic role of goal and other similar roles. It is \n\t\t\t proposed for languages in    which the role is distinct from the \n\t\t\t direct object and the oblique object on the basis of multiple    \n\t\t\t independent syntactic or morphological criteria, such as the following: \n\t\t\t\t(i) Having a particular case marking, commonly dative \n\t\t\t\t(ii) Governing an agreement affix on the verb, such as person or number \n\t\t\t\t(iii) Being distinct from oblique relations in that it may be relativized \n\t\t\t A noun, pronoun, or    noun phrase indicating the recipient or beneficiary of the action of a verb and its direct object   \n\t\t\t (http://www.isocat.org/datcat/DC-1310)\n\t\t\t \n\t\t\t Third argument of a ditransitive verb. Ditransitive recipient (Siewierska 2004:57).\n\t\t\t (http://languagelink.let.uu.nl/tds/onto/LinguisticOntology.owl#R)\n\t\t" ;
        <http://www.w3.org/2000/01/rdf-schema#subClassOf>
                <http://purl.org/olia/olia.owl#SyntacticObject> ;
        <http://www.w3.org/2002/07/owl#versionInfo>
                "\n\t\t\thttp://languagelink.let.uu.nl/tds/onto/LinguisticOntology.owl#R,\n\t\t\thttp://www.isocat.org/datcat/DC-1310\n\t\t" .

<http://purl.org/olia/olia.owl#DistributiveCase>
        a       <http://www.w3.org/2002/07/owl#Class> ;
        <http://www.w3.org/2000/01/rdf-schema#comment>
                "\n\t\t\tThe distributive case is used on nouns for the meanings of per or each, e.g., Hungarian egyenként/egy, hetenként/hét, ilyenként/ily, kéthetenként/kéthét, rekordonként/rekord, tömbönként/tömb, vércsoportonként/vércsoport\n\t\t\t\n\t\t\tIn Hungarian it is -nként and expresses the manner when something happens to each member of a set one by one (e.g., fejenként \"per head\", esetenként \"in some case\"), or the frequency in time (hetenként \"once a week\", tízpercenként \"every ten minutes\").\n\t\t\tIn the Finnish language, this adverb type is rare, even rarer in the singular. Its ending is -ttain/-ttäin. The basic meaning is \"separately for each\". For example, maa (\"country\") becomes maittain for an expression like Laki ratifioidaan maittain (\"The law is ratified separately in each country\"). It can be used to distribute the action to frequent points in time, e.g., päivä (day) has the plural distributive päivittäin (each day). It can mean also \"in (or with) regard to the (cultural) perspective\" when combined with a word referring to an inhabitant (-lais-). Frequently Finns (suomalaiset) say that suomalaisittain tuntuu oudolta, että, or \"in the Finnish perspective, it feels strange that\".\n\t\t\t(http://purl.org/olia/mte/multext-east.owl#DistributiveCase, http://en.wikipedia.org/wiki/Distributive_case)\n\t\t" ;
        <http://www.w3.org/2000/01/rdf-schema#subClassOf>
                <http://purl.org/olia/olia-top.owl#CaseFeature> ;
        <http://www.w3.org/2002/07/owl#versionInfo>
                "http://purl.org/olia/mte/multext-east.owl#DistributiveCase" .

<http://purl.org/olia/olia.owl#Diminuitive>
        a       <http://www.w3.org/2002/07/owl#Class> ;
        <http://www.w3.org/2000/01/rdf-schema#comment>
                "A diminutive is a formation of a word used to convey a slight degree of the root meaning, smallness of the object or quality named, encapsulation, intimacy, or endearment. It is the opposite of an augmentative. (http://en.wikipedia.org/wiki/Diminutive)" ;
        <http://www.w3.org/2000/01/rdf-schema#subClassOf>
                <http://purl.org/olia/olia.owl#Derivation> ;
        <http://www.w3.org/2002/07/owl#versionInfo>
                "http://purl.org/olia/mte/multext-east.owl#Diminuitive, in MTE v.4 originally modelled as an aspect of Degree, but this is a misplacement. \n\t\t\tThere are languages where Degree and Diminuitivity are independent. In Latvian, for example, the diminutive suffix may be attached to an adjective, \n\t\t\tnot only in the positive but in the comparative and superlative degrees (Ruke-Dravina 1953).\n\t\t\t\n\t\t\tVelta Ruke-Dravina (1953), Adjectival Diminuitives in Latvian. The Slavonic and East European Review  31(77): 452-465\n\t\t" .

<http://purl.org/olia/olia.owl#RelativeAdverb>
        a       <http://www.w3.org/2002/07/owl#Class> ;
        <http://www.w3.org/2000/01/rdf-schema#comment>
                "\n\t\t\tThe value relative is used for adverbs in clear relative cases as in: \"The place 'where' I met you.\", \n\t\t\t\"The reason 'why' I did it.\"\n\t\t\t(http://www.ilc.cnr.it/EAGLES96/pub/eagles/lexicons/elm_en.ps.gz, p.33, 07.05.07)\n\t\t" ;
        <http://www.w3.org/2000/01/rdf-schema#subClassOf>
                <http://purl.org/olia/olia.owl#WHTypeAdverbs> ;
        <http://www.w3.org/2002/07/owl#versionInfo>
                "EAGLES Adverb with Wh-Type=\"Relative\"." .

<http://purl.org/olia/olia.owl#Script>
        a       <http://www.w3.org/2002/07/owl#Class> ;
        <http://www.w3.org/2000/01/rdf-schema#comment>
                "Set of graphic characters used for the written form of one or more languages." ;
        <http://www.w3.org/2000/01/rdf-schema#isDefinedBy>
                "http://www.isocat.org/datcat/DC-1855" ;
        <http://www.w3.org/2000/01/rdf-schema#subClassOf>
                <http://purl.org/olia/olia-top.owl#OrthographicEntity> .

<http://purl.org/olia/olia.owl#ContablativeCase>
        a       <http://www.w3.org/2002/07/owl#Class> ;
        <http://www.w3.org/2000/01/rdf-schema#comment>
                "\n\t\t\tContablativeCase expresses that  the referent of the noun it marks \n\t\t\tis the location from near which another referent is moving. It has \n\t\t\tthe meaning 'from near'.\n\t\t\t(http://purl.org/linguistics/gold/Contablative)\n\t\t" ;
        <http://www.w3.org/2000/01/rdf-schema#subClassOf>
                <http://purl.org/olia/olia-top.owl#CaseFeature> ;
        <http://www.w3.org/2002/07/owl#versionInfo>
                "http://purl.org/linguistics/gold/Contablative" .

<http://purl.org/olia/olia-top.owl#AnimacyFeature>
        a       <http://www.w3.org/2002/07/owl#Class> .

<http://purl.org/olia/olia.owl#SemelfactiveAspect>
        a       <http://www.w3.org/2002/07/owl#Class> ;
        <http://www.w3.org/2000/01/rdf-schema#comment>
                "\n\t\t\tMomentaneous, without an inherent end-point, as sneeze (Michaelis 1998:xvi).\n\t\t\t(http://purl.org/linguistics/gold/Semelfactive)\n\t\t" ;
        <http://www.w3.org/2000/01/rdf-schema#subClassOf>
                <http://purl.org/olia/olia-top.owl#AspectFeature> ;
        <http://www.w3.org/2002/07/owl#versionInfo>
                "http://purl.org/linguistics/gold/Semelfactive" .

<http://purl.org/olia/olia.owl#hasNumeralAgreementClass>
        a       <http://www.w3.org/2002/07/owl#ObjectProperty> ;
        <http://www.w3.org/2000/01/rdf-schema#domain>
                <http://purl.org/olia/olia.owl#Quantifier> ;
        <http://www.w3.org/2000/01/rdf-schema#range>
                <http://purl.org/olia/olia-top.owl#NumeralAgreementClass> ;
        <http://www.w3.org/2000/01/rdf-schema#subPropertyOf>
                <http://purl.org/olia/system.owl#hasFeature> .

<http://purl.org/olia/olia.owl#Inflected>
        a       <http://www.w3.org/2002/07/owl#Class> ;
        <http://www.w3.org/2000/01/rdf-schema#comment>
                "\n\t\t\tsee subclasses\n\t\t" ;
        <http://www.w3.org/2000/01/rdf-schema#subClassOf>
                <http://purl.org/olia/olia-top.owl#InflectionTypeFeature> ;
        <http://www.w3.org/2002/07/owl#versionInfo>
                "Chiarcos" .

<http://purl.org/olia/olia.owl#TitleInRunningText>
        a       <http://www.w3.org/2002/07/owl#Class> ;
        <http://www.w3.org/2000/01/rdf-schema#comment>
                "-TTL (title)\n— is attached to the top node of a title when this title appears inside running text.\n-TTL implies -NOM. The internal structure of the title is bracketed as usual. (See section 12 [Titles] for more information about the bracketing of titles.) \n(Bies et al. 1995)" ;
        <http://www.w3.org/2000/01/rdf-schema#subClassOf>
                <http://purl.org/olia/olia-top.owl#DiscourseEntity> ;
        <http://www.w3.org/2002/07/owl#versionInfo>
                "PTB bracketing guidelines, Bies et al. 1995" .

<http://purl.org/olia/olia.owl#WHAdverbPhrase>
        a       <http://www.w3.org/2002/07/owl#Class> ;
        <http://www.w3.org/2000/01/rdf-schema#comment>
                "WHADVP|Wh-adverb phrase. Phrasal category headed by a wh-adverb such as how or why.\n(Santorini 1991)\nWHADVP â ´ Wh-adverb Phrase. Introduces a clause with an ADVP gap. May be null (containing the 0 complementizer) or lexical, containing a wh-adverb such as how or why. \n(Bies et al. 1995)" ;
        <http://www.w3.org/2000/01/rdf-schema#subClassOf>
                <http://purl.org/olia/olia.owl#AdverbPhrase> ;
        <http://www.w3.org/2002/07/owl#versionInfo>
                "added in conformance with PTB bracketing guidelines (Santorini 1991, Bies et al. 1995)" .

<http://purl.org/olia/olia.owl#Gapping>
        a       <http://www.w3.org/2002/07/owl#Class> ;
        <http://www.w3.org/2000/01/rdf-schema#comment>
                "\n\t\tThe term \"gapping\" refers to a form of coordination in which the coordinated phrases after the rst\n\t\tare incomplete. For instance, the gapped equivalent of the full coordination structure in (@18a) is given in\n\t\t( 18b).\n\t\t\t( 18)\n\t\t\t\ta. Mary likes Bach and Susan likes Beethoven.\n\t\t\t\tb. Mary likes Bach and Susan, Beethoven.\n\t\tGapped sequences like Susan, Beethoven should be labelled X. On the other hand, while coordination\n\t\tconstructions containing gapped sequences involve coordination of unlike categories, it is clear that the\n\t\tentire coordination structure is a clause; hence, it should be labelled S.\n\t\t(Santorini 1991)\n\t" ;
        <http://www.w3.org/2000/01/rdf-schema#subClassOf>
                <http://purl.org/olia/olia-top.owl#NullElement> ;
        <http://www.w3.org/2002/07/owl#versionInfo>
                "PTB bracketing guidelines (Santorini 1991)" .

<http://purl.org/olia/olia.owl#InterablativeCase>
        a       <http://www.w3.org/2002/07/owl#Class> ;
        <http://www.w3.org/2000/01/rdf-schema#comment>
                "\n\t\t\tInterablativeCase expresses that  the referent of the noun it marks \n\t\t\tis the location from between which another referent is moving. It \n\t\t\thas the meaning 'from inbetween'.\n\t\t\t(http://purl.org/linguistics/gold/Interablative)\n\t\t" ;
        <http://www.w3.org/2000/01/rdf-schema#subClassOf>
                <http://purl.org/olia/olia-top.owl#CaseFeature> ;
        <http://www.w3.org/2002/07/owl#versionInfo>
                "http://purl.org/linguistics/gold/Interablative" .

<http://purl.org/olia/olia.owl#FusedPreposition>
        a       <http://www.w3.org/2002/07/owl#Class> ;
        <http://www.w3.org/2000/01/rdf-schema#comment>
                "\n                            Preposition that is the result of a morphological merge from at least two words.\n                                (http://www.isocat.org/datcat/DC-1901)\n                            " ;
        <http://www.w3.org/2000/01/rdf-schema#label>
                "fused preposition" ;
        <http://www.w3.org/2000/01/rdf-schema#subClassOf>
                <http://purl.org/olia/olia.owl#Preposition> ;
        <http://www.w3.org/2002/07/owl#versionInfo>
                "http://www.isocat.org/datcat/DC-1901" , "subClassOf preposition (dcif:isA)" .

<http://purl.org/olia/olia.owl#OpenAngleBracket>
        a       <http://www.w3.org/2002/07/owl#Class> ;
        <http://www.w3.org/2000/01/rdf-schema#comment>
                "<\n*LAB*\nLeft angle bracket\n(Santorini 1991)" ;
        <http://www.w3.org/2000/01/rdf-schema#subClassOf>
                <http://purl.org/olia/olia.owl#LeftParentheticalPunctuation> ;
        <http://www.w3.org/2002/07/owl#versionInfo>
                "PTB bracketing guidelines, Santorini 1991" .

<http://purl.org/olia/olia.owl#AntiCausativeVoice>
        a       <http://www.w3.org/2002/07/owl#Class> ;
        <http://www.w3.org/2000/01/rdf-schema#comment>
                "An intransitive verb is derived from a basically\n                        transitive one with the direct object of the transitive verb corresponding\n                        to the subject of the intransitive [Siewierska 1988: 267]." ;
        <http://www.w3.org/2000/01/rdf-schema#isDefinedBy>
                "http://www.isocat.org/datcat/DC-3080" ;
        <http://www.w3.org/2000/01/rdf-schema#subClassOf>
                <http://purl.org/olia/olia-top.owl#VoiceFeature> .

<http://purl.org/olia/olia.owl#hasParent>
        a       <http://www.w3.org/2002/07/owl#ObjectProperty> ;
        <http://www.w3.org/2000/01/rdf-schema#comment>
                "In hierarchical relations, the parent is modelled as source, the child as target." ;
        <http://www.w3.org/2000/01/rdf-schema#subPropertyOf>
                <http://purl.org/olia/system.owl#hasSource> .

<http://purl.org/olia/olia.owl#InterrogativeModality>
        a       <http://www.w3.org/2002/07/owl#Class> ;
        <http://www.w3.org/2000/01/rdf-schema#comment>
                "\n\t\t\tThe interrogative modality serves to indicate interrogative quality.\n\t\t\t(http://languagelink.let.uu.nl/tds/onto/LinguisticOntology.owl#interrogativeModality)\n\t\t" ;
        <http://www.w3.org/2000/01/rdf-schema#subClassOf>
                <http://purl.org/olia/olia-top.owl#ModalityFeature> ;
        <http://www.w3.org/2002/07/owl#versionInfo>
                "\n\t\t\thttp://languagelink.let.uu.nl/tds/onto/LinguisticOntology.owl#interrogativeModality\n\t\t" .

<http://purl.org/olia/olia-top.owl#InflectionTypeFeature>
        a       <http://www.w3.org/2002/07/owl#Class> ;
        <http://www.w3.org/2000/01/rdf-schema#comment>
                "\n\t\t\tIn this category, different inflection-relevant features are assembled. \n\t\t\tTypically, inflection phenomena are language-specific and pertain to different grammatial categories;\n\t\t\ttherefore, this collection is neither to be supposed exhaustive nor are the features necessarily disjoint\n\t\t\t(e.g., InflectedWithOvertMarker overlaps with StrongInflection or WeakInflection)\n\t\t" ;
        <http://www.w3.org/2000/01/rdf-schema#subClassOf>
                [ a       <http://www.w3.org/2002/07/owl#Restriction> ;
                  <http://www.w3.org/2002/07/owl#hasSelf>
                          true ;
                  <http://www.w3.org/2002/07/owl#onProperty>
                          <http://purl.org/olia/olia.owl#hasInflectionType>
                ] ;
        <http://www.w3.org/2000/01/rdf-schema#subClassOf>
                [ a       <http://www.w3.org/2002/07/owl#Restriction> ;
                  <http://www.w3.org/2002/07/owl#hasSelf>
                          true ;
                  <http://www.w3.org/2002/07/owl#onProperty>
                          <http://purl.org/olia/olia.owl#hasInflectionType>
                ] .

<http://purl.org/olia/olia.owl#NegativeDeterminer>
        a       <http://www.w3.org/2002/07/owl#Class> ;
        <http://www.w3.org/2000/01/rdf-schema#comment>
                "Determiner/Type=\"negative\" (Romanian)<br/>\t\t\t\n\t\t\tIn Romanian the negative determiner is expressed by the unit nici + indefinite article (e.g. nici un, nici o). (MTE v4)\n\t\t\te.g., nici-o/nici_un, nici_o/nici_un, nici_un, nici_unei/nici_un, nici_unii/nici_un, nici_unor/nici_un, nici_unui/nici_un \n\t\t\t(http://purl.org/olia/mte/multext-east.owl#NegativeDeterminer)" ;
        <http://www.w3.org/2000/01/rdf-schema#subClassOf>
                <http://purl.org/olia/olia.owl#IndefiniteDeterminer> ;
        <http://www.w3.org/2002/07/owl#versionInfo>
                "http://purl.org/olia/mte/multext-east.owl#NegativeDeterminer" .

<http://purl.org/olia/olia.owl#SecondFamiliar>
        a       <http://www.w3.org/2002/07/owl#Class> ;
        <http://www.w3.org/2000/01/rdf-schema#comment>
                "\n\t\t\tIn several European languages exist special forms of pronouns for polite or respectful reference,\n\t\t\te.g. Dutch u and Spanish usted. The feature SecondFamiliar applies to the corresponding unmarked \n\t\t\tforms for informal conversiation in such languages.\n\t\t\t(http://www.ilc.cnr.it/EAGLES96/annotate/node18.html#oav1p 19.09.06)\n\t\t" ;
        <http://www.w3.org/2000/01/rdf-schema#subClassOf>
                <http://purl.org/olia/olia.owl#Second> ;
        <http://www.w3.org/2002/07/owl#versionInfo>
                "EAGLES PersonalPronoun attribute Politeness=\"Familiar\". \n\t\t\tThe EAGLES attribute politeness (polite/ familiar) is limited to second-person pronouns.\n\t\t" .

<http://purl.org/olia/olia.owl#hasNumber>
        a       <http://www.w3.org/2002/07/owl#ObjectProperty> ;
        <http://www.w3.org/2000/01/rdf-schema#domain>
                [ a       <http://www.w3.org/2002/07/owl#Class> ;
                  <http://www.w3.org/2002/07/owl#unionOf>
                          ( <http://purl.org/olia/olia.owl#Noun> <http://purl.org/olia/olia.owl#Adjective> <http://purl.org/olia/olia.owl#Verb> <http://purl.org/olia/olia.owl#PronounOrDeterminer> <http://purl.org/olia/olia.owl#Article> <http://purl.org/olia/olia.owl#Numeral> <http://purl.org/olia/olia.owl#Residual> )
                ] ;
        <http://www.w3.org/2000/01/rdf-schema#range>
                <http://purl.org/olia/olia-top.owl#NumberFeature> ;
        <http://www.w3.org/2000/01/rdf-schema#subPropertyOf>
                <http://purl.org/olia/system.owl#hasFeature> .

<http://purl.org/olia/olia.owl#SubordinatorField>
        a       <http://www.w3.org/2002/07/owl#Class> ;
        <http://www.w3.org/2000/01/rdf-schema#comment>
                "\nIn the German clause, the PARORD-field is the field for non-coordinating particles which\noptionally occur as the left-most element of a verb-second clause \n(Telljohann et al. 2009, p.17)\n\t\t" ;
        <http://www.w3.org/2000/01/rdf-schema#subClassOf>
                <http://purl.org/olia/olia-top.owl#TopologicalField> .

<http://purl.org/olia/olia.owl#BaseForm>
        a       <http://www.w3.org/2002/07/owl#Class> ;
        <http://www.w3.org/2000/01/rdf-schema#comment>
                "\n\t\t\tStrong inflection is a characteristic of lexemes, not individual tokens.\n\t\t\tIn traditional English tagsets, e.g., SUSANNE  or the PennTreeBank tagset, surface ambiguities are normally not resolved.\n\t\t\tUninflected forms and forms that have the same form (e.g., \"be\" as an imperative) are tagged as BaseForm. (Ch. Chiarcos)\n\t\t\t\n\t\t\tSince it is impractical (...) to resolve automatically the \n\t\t\tambiguity of these six morphological functions, it is a common practice to assign a single value to the base form, \n\t\t\tor else to assign two values, one for the finite and one for the non-finite functions. Because of this, the tables \n\t\t\tbelow show two tagsets: one tagset representing the 6 attribute-values above, and a reduced tagset (`RTags'), which\n\t\t\tresembles most tagsets so far used for the English language in reducing the six values to two.\n\t\t\thttp://www.ilc.cnr.it/EAGLES96/morphsyn/node150.html#SECTION00054000000000000000\n\t\t\t\n\t\t\tBaseForm is not a characteristic of lexemes, but specific to certain forms in a complex paradigm.\n\t\t" ;
        <http://www.w3.org/2000/01/rdf-schema#subClassOf>
                <http://purl.org/olia/olia-top.owl#InflectionTypeFeature> ;
        <http://www.w3.org/2002/07/owl#versionInfo>
                "SUSANNE (Sampson 1995)" .

<http://purl.org/olia/olia.owl#Aorist>
        a       <http://www.w3.org/2002/07/owl#Class> ;
        <http://www.w3.org/2000/01/rdf-schema#comment>
                "\n                            Simple past tense that is predominantly used for narration. Both the perfective and the imperfective forms can be used in the aorist without any restrictions.\n                                (www.helsinki.fi/~bontchev/grammar/index.html; http://www.isocat.org/datcat/DC-1240)\n                            " ;
        <http://www.w3.org/2000/01/rdf-schema#label>
                "aorist" ;
        <http://www.w3.org/2000/01/rdf-schema#subClassOf>
                <http://purl.org/olia/olia.owl#Past> ;
        <http://www.w3.org/2002/07/owl#versionInfo>
                "http://www.isocat.org/datcat/DC-1240" .

<http://purl.org/olia/olia.owl#FocusAntipassive>
        a       <http://www.w3.org/2002/07/owl#Class> ;
        <http://www.w3.org/2000/01/rdf-schema#comment>
                "\n\t\t\tBlocks the P or logical object (basic absolutive) nominal from being \n\t\t\tassigned Focus salience.  Topic salience is available for assignment \n\t\t\tto various arguments, including the P, but Focus salience is always \n\t\t\tassigned to A, and is therefore inaccessible to P or any other nominal.\n\t\t\t(Klaiman 1991:236)\n\t\t\t(http://purl.org/linguistics/gold/FocusAntipassive)\n\t\t" ;
        <http://www.w3.org/2000/01/rdf-schema#subClassOf>
                <http://purl.org/olia/olia.owl#Antipassive> ;
        <http://www.w3.org/2002/07/owl#versionInfo>
                "http://purl.org/linguistics/gold/FocusAntipassive" .

<http://purl.org/olia/olia.owl#ModalVerb>
        a       <http://www.w3.org/2002/07/owl#Class> ;
        <http://www.w3.org/2000/01/rdf-schema#comment>
                "\n\t\t\tVerb form that is usually used with another verb to express ideas such as possibilities, permission, or intention.\n            (Gil Francopoulo; http://www.isocat.org/datcat/DC-1329)\n\t\t\n\t\t\tA modal verb (also modal, modal auxiliary verb, modal auxiliary) is a type of auxiliary \n\t\t\tverb that is used to indicate modality. The use of auxiliary verbs to express modality \n\t\t\tis characteristic of Germanic languages.\n\t\t\t(http://en.wikipedia.org/wiki/Modal_verb 19.09.06)\n\t\t\t\n\t\t\tIn addition to main and auxiliary verbs, it may be useful (e.g. in English) to recognise an intermediate \n\t\t\tcategory of semi-auxiliary for such verbs as be going to, have got to, ought to.\n\t\t\t(http://www.ilc.cnr.it/EAGLES96/annotate/node18.html#oav1v 20.09.06)\n\t\t\t\n\t\t\tThe auxiliaries in English subdivide into the primary verbs `be', `have', and `do', which can also function \n\t\t\tas main verbs, and the modal auxiliaries such as `can', `will', and `would', which are uninflected, and always \n\t\t\tfunction as auxiliaries.\n\t\t\t(http://www.ilc.cnr.it/EAGLES96/morphsyn/node158.html#SECTION00054800000000000000)\n\t\t" ;
        <http://www.w3.org/2000/01/rdf-schema#subClassOf>
                <http://purl.org/olia/olia.owl#AuxiliaryVerb> ;
        <http://www.w3.org/2002/07/owl#versionInfo>
                "TODO: rename to semiauxiliary, this seems to be a more language-independent term" , "\n\t\t\tAdded for compatibility with the SFB632 annotation guidelines.\n\t\t\tMay correspond to the (optional, French-only) EAGLES feature value \"semiauxiliary\".\n\t\t\t\n\t\t\thttp://www.isocat.org/datcat/DC-1329\n\t   " .

<http://purl.org/olia/olia-top.owl#ReduplicationTypeFeature>
        a       <http://www.w3.org/2002/07/owl#Class> ;
        <http://www.w3.org/2000/01/rdf-schema#subClassOf>
                [ a       <http://www.w3.org/2002/07/owl#Restriction> ;
                  <http://www.w3.org/2002/07/owl#hasSelf>
                          true ;
                  <http://www.w3.org/2002/07/owl#onProperty>
                          <http://purl.org/olia/olia.owl#hasReduplicationType>
                ] .

<http://purl.org/olia/olia.owl#QuotativeModality>
        a       <http://www.w3.org/2002/07/owl#Class> ;
        <http://www.w3.org/2000/01/rdf-schema#comment>
                "A quotative is grammatical device to mark reported speech in some languages (http://en.wikipedia.org/wiki/Quotative), e.g., in Estonian.<br/>\n\t\t\t\n\t\t\t‘Reportedly, while he was going (in his boat), he turned over.’\n\t\t\tTa olevat        oma     paadiga   ümber läinud\n\t\t\tHe was_QUOTATIVE his_own boat_WITH over  gone.<br/>\n\t\t\t\n\t\t\t(Estonian translation of an example given under http://www.sil.org/linguistics/GlossaryOfLinguisticTerms/WhatIsAQuotativeEvidential.htm)\n\t\t\t(Heiki-Jaan.Kaalep, email 2010/06/22)" ;
        <http://www.w3.org/2000/01/rdf-schema#subClassOf>
                <http://purl.org/olia/olia-top.owl#ModalityFeature> ;
        <http://www.w3.org/2002/07/owl#versionInfo>
                "http://purl.org/olia/mte/multext-east.owl#Quotative, MTE VForm=\"quotative\" (Estonian)" .

<http://purl.org/olia/olia.owl#ElementWithoutClitic>
        a       <http://www.w3.org/2002/07/owl#Class> ;
        <http://www.w3.org/2000/01/rdf-schema#comment>
                "Expression representing a lexeme without any clitics (i.e. because of the absence of cliticization or because the clitic is represented separately) (Chiarcos)" ;
        <http://www.w3.org/2000/01/rdf-schema#subClassOf>
                <http://purl.org/olia/olia.owl#Cliticization> ;
        <http://www.w3.org/2002/07/owl#versionInfo>
                "http://purl.org/olia/mte/multext-east.owl#ElementWithoutClitic\"" .

<http://purl.org/olia/olia.owl#NounHeadedPhrase>
        a       <http://www.w3.org/2002/07/owl#Class> ;
        <http://www.w3.org/2000/01/rdf-schema#comment>
                "\n\t\t\tA NounHeadedPhrase takes a nominal as its (semantic) head. \n\t\t\tIntroduced as a generalization over NounPhrase and PrepositionalPhrase for reasons of consistency with dependency parsers like \n\t\t\tConnexor where this differentiation is not made.\n\t\t" ;
        <http://www.w3.org/2000/01/rdf-schema#subClassOf>
                <http://purl.org/olia/olia.owl#Phrase> .

<http://purl.org/olia/olia.owl#FacultativePrepositionalObject>
        a       <http://www.w3.org/2002/07/owl#Class> ;
        <http://www.w3.org/2000/01/rdf-schema#comment>
                "facultative (i.e. optional) prepositional object, e.g., passivized subject (von-phrase)" ;
        <http://www.w3.org/2000/01/rdf-schema#subClassOf>
                <http://purl.org/olia/olia.owl#PrepositionalObject> ;
        <http://www.w3.org/2002/07/owl#versionInfo>
                "TüBa-D/Z edge label FOPP" .

<http://purl.org/olia/olia.owl#Bullet>
        a       <http://www.w3.org/2002/07/owl#Class> ;
        <http://www.w3.org/2000/01/rdf-schema#comment>
                "\n                            Sign used to mark an item in a list.\n                                (http://www.isocat.org/datcat/DC-1438)\n                            " ;
        <http://www.w3.org/2000/01/rdf-schema#label>
                "bullet" ;
        <http://www.w3.org/2000/01/rdf-schema#subClassOf>
                <http://purl.org/olia/olia.owl#LayoutElement> ;
        <http://www.w3.org/2002/07/owl#versionInfo>
                "http://www.isocat.org/datcat/DC-1438" , "subClassOf partOfSpeech (dcif:conceptualDomain)" .

<http://purl.org/olia/olia.owl#DeductiveEvidentiality>
        a       <http://www.w3.org/2002/07/owl#Class> ;
        <http://www.w3.org/2000/01/rdf-schema#comment>
                "DeductiveEvidentiality encodes the fact that the\n                        speaker came to believe the content of the expression through a sound\n                        inference procedure. [Palmer 2001: 6-8]." ;
        <http://www.w3.org/2000/01/rdf-schema#isDefinedBy>
                "http://www.isocat.org/datcat/DC-3150" ;
        <http://www.w3.org/2000/01/rdf-schema#subClassOf>
                <http://purl.org/olia/olia-top.owl#EvidentialityFeature> .

<http://purl.org/olia/olia.owl#StillPresent>
        a       <http://www.w3.org/2002/07/owl#Class> ;
        <http://www.w3.org/2000/01/rdf-schema#comment>
                "\n\t\t\tStillPresentTense is similar to PresentTense but carries the presupposition \n\t\t\tthat an event or state held before the moment of utterance. In positive \n\t\t\tdeclarative clauses, still present tense asserts that the event or state \n\t\t\tholds at the moment of utterance (Comrie 1985: 54; named changed from \n\t\t\t'StillTense').\n\t\t\t(http://purl.org/linguistics/gold/StillPresent)\n\t\t" ;
        <http://www.w3.org/2000/01/rdf-schema#subClassOf>
                <http://purl.org/olia/olia.owl#Past> ;
        <http://www.w3.org/2002/07/owl#versionInfo>
                "http://purl.org/linguistics/gold/StillPresent" .

<http://purl.org/olia/olia-top.owl#CountabilityFeature>
        a       <http://www.w3.org/2002/07/owl#Class> ;
        <http://www.w3.org/2000/01/rdf-schema#subClassOf>
                [ a       <http://www.w3.org/2002/07/owl#Restriction> ;
                  <http://www.w3.org/2002/07/owl#hasSelf>
                          true ;
                  <http://www.w3.org/2002/07/owl#onProperty>
                          <http://purl.org/olia/olia.owl#hasCountability>
                ] .

<http://purl.org/olia/olia-top.owl#ModalityFeature>
        a       <http://www.w3.org/2002/07/owl#Class> ;
        <http://www.w3.org/2000/01/rdf-schema#subClassOf>
                [ a       <http://www.w3.org/2002/07/owl#Restriction> ;
                  <http://www.w3.org/2002/07/owl#hasSelf>
                          true ;
                  <http://www.w3.org/2002/07/owl#onProperty>
                          <http://purl.org/olia/olia.owl#hasModality>
                ] ;
        <http://www.w3.org/2000/01/rdf-schema#subClassOf>
                [ a       <http://www.w3.org/2002/07/owl#Restriction> ;
                  <http://www.w3.org/2002/07/owl#hasSelf>
                          true ;
                  <http://www.w3.org/2002/07/owl#onProperty>
                          <http://purl.org/olia/olia.owl#hasModality>
                ] ;
        <http://www.w3.org/2002/07/owl#versionInfo>
                "note that Modality overlaps with SentenceType (cf. InterrogativeModality besides Question, DeclarativeModality vs. DeclarativeSentence, etc.). The main difference between both is the restriction of SentenceType to full sentences as a basis of analysis. Any updates should maintain this relationship." , "Mood feature pertains to grammaticalized moods (as expressed in verbal inflection), Modality refers to the underlying concept that can also be manifested by other grammatical or orthographic markers" .

<http://purl.org/olia/olia.owl#NonFiniteEmbeddedConstruction>
        a       <http://www.w3.org/2002/07/owl#Class> ;
        <http://www.w3.org/2000/01/rdf-schema#comment>
                "\n\t\t\tAn embedded construction which contains a non-finite verb form\n\t\t\t(http://languagelink.let.uu.nl/tds/onto/LinguisticOntology.owl#non-finiteEmbeddedConstruction \n\t\t\twith reference to Dik 1997)\n\t\t" ;
        <http://www.w3.org/2000/01/rdf-schema#subClassOf>
                <http://purl.org/olia/olia.owl#Clause> .

<http://purl.org/olia/olia.owl#Ellipsis>
        a       <http://www.w3.org/2002/07/owl#Class> ;
        <http://www.w3.org/2000/01/rdf-schema#comment>
                "*?* â ´ placeholder for ellipsed material ...\n\n*?* is now available in the following great-tasting flavors: (VP *?*), (ADJP-PRD *?*), (PP-PRD *), (NP *?*), (S *?*), (SBAR *?*). These act as placeholders for a missing predicate or piece thereof, especially in comparative constructions and other environments where predicate deletion occurs. Although the missing material represented by *?* is often identical to another constituent in the same sentence, the two are never coindexed. Postmodifiers of the verb (including traces) may be attached under (VP *?*), but not to any other null element, including the other *?* null elements and (VP *T*).\n\nNote that policy for *?* was never finalized, so its use varies to some extent. In general, *?* is used by the annotators as a last resort (short of the FRAG analysis) for the annotation of clauses with â ¼missingâ ½ material. Nonetheless, there are certain constructions that are particularly likely to contain *?*:\n(Bies et al. 1995)" ;
        <http://www.w3.org/2000/01/rdf-schema#subClassOf>
                <http://purl.org/olia/olia-top.owl#NullElement> ;
        <http://www.w3.org/2002/07/owl#versionInfo>
                "added in conformance with PTB bracketing guidelines (Santorini 1991, Bies et al. 1995)" .

<http://purl.org/olia/olia.owl#HodiernalPast>
        a       <http://www.w3.org/2002/07/owl#Class> ;
        <http://www.w3.org/2000/01/rdf-schema#comment>
                "\n\t\t\tHodiernalPastTense locates the situation in question before the moment of \n\t\t\tutterance within the span culturally defined as 'today' (Comrie 1985:87; \n\t\t\tDahl 1985:125-126). Contrasts with PreHodiernalPastTense.\n\t\t\t(http://purl.org/linguistics/gold/HodiernalPast)\n\t\t" ;
        <http://www.w3.org/2000/01/rdf-schema#subClassOf>
                <http://purl.org/olia/olia.owl#Past> ;
        <http://www.w3.org/2002/07/owl#versionInfo>
                "http://purl.org/linguistics/gold/HodiernalPast, classified as Past here" .

<http://purl.org/olia/olia.owl#FirstPersonPronoun>
        a       <http://www.w3.org/2002/07/owl#Class> ;
        <http://www.w3.org/2000/01/rdf-schema#comment>
                "\n\t\t\tA FirstPersonPronoun refers to the speaker, or to  both the speaker and referents grouped with the speaker.  \n\t\t\t(http://www.sil.org/linguistics/GlossaryOfLinguisticTerms/WhatIsFirstPersonDeixis.htm 19.09.06)\n\t\t" ;
        <http://www.w3.org/2000/01/rdf-schema#subClassOf>
                <http://purl.org/olia/olia.owl#PersReflPronoun> ;
        <http://www.w3.org/2002/07/owl#versionInfo>
                "\n\t\t\tEAGLES Pronoun with Person=\"First\". As only personal and reflexive pronouns show person differentiation,\n\t\t\tFirstPersonPronoun is modelled as a subclass of PersReflConcept here.\n\t\t" .

<http://purl.org/olia/olia.owl#AgentiveVerb>
        a       <http://www.w3.org/2002/07/owl#Class> ;
        <http://www.w3.org/2000/01/rdf-schema#comment>
                "\n\t\tAn agentive verb marks the semantic role of agent or the doer of an action.\n\t\t\n\t\tExample:\n\t\t་ ་ ས་ ་ ་ བསད་ ག།\n\t\tDorji-gi jele sänu\n\t\t'Dorji killed the cat'\n\t\t(http://panl10n.net/english/Outputs%20Phase%202/CCs/Bhutan/Papers/2007/0701/PartOfSpeech.pdf)\n\t\t" ;
        <http://www.w3.org/2000/01/rdf-schema#subClassOf>
                <http://purl.org/olia/olia.owl#MainVerb> ;
        <http://www.w3.org/2002/07/owl#versionInfo>
                "adopted from Dzongkha tagset (Chungku et al. 2010)" .

<http://purl.org/olia/olia.owl#ExclusiveEmphaticParticle>
        a       <http://www.w3.org/2002/07/owl#Class> ;
        <http://www.w3.org/2000/01/rdf-schema#comment>
                "In Urdu, the exclusive emphatic particle hî emphasizes the preceding word and excludes something else (which may not be expressed). (Schmidt 1999, p.233, http://purl.org/olia/emille.owl#ExclusiveEmphaticParticle)\n\t\t\n\t\tCompare with the inclusive emphatic particle bhî:\n\t\t\n\t\tmaim *bhî* faisalâ karûm gâ\n\t\t\"I'll *also* make a decision\"\n\t\t\n\t\tmaim *hî* faisalâ karûm gâ\n\t\t\"*I'm the one who* will make the decision.\"\n\t\t(Schmidt 1999, p.237, http://purl.org/olia/emille.owl#InclusiveEmphaticParticle)\n\t\t" ;
        <http://www.w3.org/2000/01/rdf-schema#subClassOf>
                <http://purl.org/olia/olia.owl#EmphaticParticle> , <http://purl.org/olia/olia.owl#Exclusive> ;
        <http://www.w3.org/2002/07/owl#versionInfo>
                "adopted from EMILLE for Urdu, http://purl.org/olia/emille.owl#ExclusiveEmphaticParticle" .

<http://purl.org/olia/olia.owl#SubordinatingConjunctionWithNegation>
        a       <http://www.w3.org/2002/07/owl#Class> ;
        <http://www.w3.org/2000/01/rdf-schema#comment>
                "Conjunction/Sub_Type=\"negative\" (Romanian, Serbian, Russian)\n\t\tIn Romanian, each conjunction requires another mood, so that the diversity may be controlled by subcategorisation rules. The attribute Sub_Type distinguishes among the positive and negative conjunctions, providing means to control verbal double negation, (as in case of the negative pronouns, determiners and adverbs): nici NU am venit, nimeni NU vorbeşte, nici_un tren N-a trecut, nicăieri N-am văzut (MTE v4, http://purl.org/olia/mte/multext-east.owl#NegativeSubordinatingConjunction)" ;
        <http://www.w3.org/2000/01/rdf-schema#subClassOf>
                <http://purl.org/olia/olia.owl#SubordinatingConjunction> ;
        <http://www.w3.org/2002/07/owl#versionInfo>
                "http://purl.org/olia/mte/multext-east.owl#NegativeSubordinatingConjunction" .

<http://purl.org/olia/olia.owl#DeclarativeMood>
        a       <http://www.w3.org/2002/07/owl#Class> ;
        <http://www.w3.org/2000/01/rdf-schema#comment>
                "\n\t\t\tPertaining to the mood or mode of a verb form or clause such that it \n\t\t\tpredicates a type of (formal) assertion (OED).\n\t\t\t(http://languagelink.let.uu.nl/tds/onto/LinguisticOntology.owl#declarativeModality)\n\t\t\t\n\t\t\tUnlike DeclarativeModality, a DeclarativeMood is morphologically marked.\n\t\t" ;
        <http://www.w3.org/2000/01/rdf-schema#subClassOf>
                <http://purl.org/olia/olia-top.owl#MoodFeature> , <http://purl.org/olia/olia.owl#DeclarativeModality> ;
        <http://www.w3.org/2002/07/owl#versionInfo>
                "http://languagelink.let.uu.nl/tds/onto/LinguisticOntology.owl#declarativeModality" .

<http://purl.org/olia/olia.owl#hasVoice>
        a       <http://www.w3.org/2002/07/owl#ObjectProperty> ;
        <http://www.w3.org/2000/01/rdf-schema#range>
                <http://purl.org/olia/olia-top.owl#VoiceFeature> ;
        <http://www.w3.org/2000/01/rdf-schema#subPropertyOf>
                <http://purl.org/olia/system.owl#hasFeature> .

<http://purl.org/olia/olia-top.owl#ReferentTypeFeature>
        a       <http://www.w3.org/2002/07/owl#Class> .

<http://purl.org/olia/olia.owl#CloseQuote>
        a       <http://www.w3.org/2002/07/owl#Class> ;
        <http://www.w3.org/2000/01/rdf-schema#comment>
                "quotation mark, closing" ;
        <http://www.w3.org/2000/01/rdf-schema#subClassOf>
                <http://purl.org/olia/olia.owl#Quote> ;
        <http://www.w3.org/2002/07/owl#versionInfo>
                "adopted from EMILLE, http://purl.org/olia/emille.owl#CloseQuotationMark" .

<http://purl.org/olia/olia.owl#hasSpecificity>
        a       <http://www.w3.org/2002/07/owl#ObjectProperty> ;
        <http://www.w3.org/2000/01/rdf-schema#range>
                <http://purl.org/olia/olia-top.owl#SpecificityFeature> ;
        <http://www.w3.org/2000/01/rdf-schema#subPropertyOf>
                <http://purl.org/olia/system.owl#hasFeature> .

<http://purl.org/olia/olia.owl#Interjection>
        a       <http://www.w3.org/2002/07/owl#Class> ;
        <http://www.w3.org/2000/01/rdf-schema#comment>
                "\n\t\tAn interjection is a form, typically brief, such as one syllable or word, \n\t\twhich is used most often as an exclamation or part of an exclamation. It \n\t\ttypically expresses an emotional reaction, often with respect to an \n\t\taccompanying sentence and may include a combination of sounds not otherwise \n\t\tfound in the language, e.g. in English:  psst; ugh; well, well\n\t\t(http://www.sil.org/linguistics/GlossaryOfLinguisticTerms/WhatIsAnInterjection.htm 19.09.06)\n\t" ;
        <http://www.w3.org/2000/01/rdf-schema#subClassOf>
                <http://purl.org/olia/olia-top.owl#MorphosyntacticCategory> ;
        <http://www.w3.org/2002/07/owl#versionInfo>
                "EAGLES top-level category Interjection (I)." .

<http://purl.org/olia/olia.owl#NonInversePassive>
        a       <http://www.w3.org/2002/07/owl#Class> ;
        <http://www.w3.org/2000/01/rdf-schema#comment>
                "\n\t\t\tAn agent-demoting voice construction where the realization of the demoted agent\n\t\t\tis not obligatory (against Inverse). In terminological systems that distinguish\n\t\t\t\"InverseVoice\" from \"Passive\" (e.g., Givon, 1988), this is the \"Passive\" concept. \n\t\t\t(Ch. Chiarcos)\n\t\t\t\n\t\t\tAssociated with actions performed on the subject by an unspecified agent.\n\t\t\t(McIntosh 1984:108) Refers to the category of verb forms, typically identifies \n\t\t\twith a specific morphological marking, that encode the derived diatheses in \n\t\t\twhich the agent role is not linked with a subject noun phrase (Shibatani 1995:7)\n\t\t\t(http://purl.org/linguistics/gold/Passive)\n\t\t" ;
        <http://www.w3.org/2000/01/rdf-schema#subClassOf>
                <http://purl.org/olia/olia.owl#PassiveVoice> ;
        <http://www.w3.org/2002/07/owl#disjointWith>
                <http://purl.org/olia/olia.owl#InverseVoice> ;
        <http://www.w3.org/2002/07/owl#versionInfo>
                "\n\t\t\thttp://purl.org/linguistics/gold/Passive\n\t\t\t\n\t\t\tUnlike the GOLD definition, Passive is often not clearly distinguished from Inverse: According to Givón (1988),\n\t\t\tInverse is characterized by obligatory realization of the suppressed agent,\n\t\t\twhereas the realization of the agent in a passive construction is optional \n\t\t\t(or impossible).\n\t\t\tThis restrictive definition of passive does, however, conflict with the \n\t\t\tuse of the term \"passive\" for European languages. Then, English and German \n\t\t\t\"Passive\" would be Inverses. Therefore, Inverse is a subconcept of Passive here.\n\t\t\tGivón's original Passive is NonInversePassive.\n\t\t" .

<http://purl.org/olia/olia.owl#Homophone>
        a       <http://www.w3.org/2002/07/owl#Class> ;
        <http://www.w3.org/2000/01/rdf-schema#comment>
                "Word that sounds like another word, but is different in writiing or meaning." ;
        <http://www.w3.org/2000/01/rdf-schema#isDefinedBy>
                "http://www.isocat.org/datcat/DC-1302" ;
        <http://www.w3.org/2000/01/rdf-schema#label>
                "homophone" ;
        <http://www.w3.org/2000/01/rdf-schema#subClassOf>
                <http://purl.org/olia/system.owl#Relation> , <http://purl.org/olia/olia-top.owl#LexicalRelation> .

<http://purl.org/olia/olia.owl#SuspensionPoints>
        a       <http://www.w3.org/2002/07/owl#Class> ;
        <http://www.w3.org/2000/01/rdf-schema#comment>
                "\n                            Sequence of three dots having the same meaning as \"et cetera\" (full form) or \"etc\" (abbreviated form).\n                                (http://www.isocat.org/datcat/DC-1447)\n                            " ;
        <http://www.w3.org/2000/01/rdf-schema#label>
                "suspension points" ;
        <http://www.w3.org/2000/01/rdf-schema#subClassOf>
                <http://purl.org/olia/olia.owl#SentenceMedialPunctuation> ;
        <http://www.w3.org/2002/07/owl#versionInfo>
                "http://www.isocat.org/datcat/DC-1447" , "subClassOf partOfSpeech (dcif:conceptualDomain)" .

<http://purl.org/olia/olia-top.owl#DependencyRelation>
        a       <http://www.w3.org/2002/07/owl#Class> ;
        <http://www.w3.org/2000/01/rdf-schema#subClassOf>
                <http://purl.org/olia/olia-top.owl#SyntacticRelation> .

<http://purl.org/olia/olia-top.owl#MorphologicalCategory>
        a       <http://www.w3.org/2002/07/owl#Class> .

<http://purl.org/olia/olia.owl#CoordinatorField>
        a       <http://www.w3.org/2002/07/owl#Class> ;
        <http://www.w3.org/2000/01/rdf-schema#comment>
                "\nThe KOORD-field is the field for coordinating particles in the German clause. In contrast to the PARORD-field, it can optionally occur as the left-most element of all clause types.\n(Telljohann et al. 2009, p.17)\n\t\t" ;
        <http://www.w3.org/2000/01/rdf-schema#subClassOf>
                <http://purl.org/olia/olia-top.owl#TopologicalField> .

<http://purl.org/olia/olia.owl#DirectQuestion>
        a       <http://www.w3.org/2002/07/owl#Class> ;
        <http://www.w3.org/2000/01/rdf-schema#comment>
                "There are two types of direct questions: yes-no questions and wh-questions. Yes-no questions should be\nbracketed as SQ. The auxiliary verb or form of do that precedes the subject in a yes-no question is a child\nof SQ. Note that yes-no questions need not contain a VP node\n(Santorini 1991)" ;
        <http://www.w3.org/2000/01/rdf-schema#subClassOf>
                <http://purl.org/olia/olia.owl#Question> ;
        <http://www.w3.org/2002/07/owl#versionInfo>
                "Santorini 1991, Bies et al. 1995" .

<http://purl.org/olia/olia.owl#Dual>
        a       <http://www.w3.org/2002/07/owl#Class> ;
        <http://www.w3.org/2000/01/rdf-schema#comment>
                "\n                            Form used in some languages to designate two persons or things.\n                                (ISO12620; http://www.isocat.org/datcat/DC-1879)\n                            " ;
        <http://www.w3.org/2000/01/rdf-schema#label>
                "dual" ;
        <http://www.w3.org/2000/01/rdf-schema#subClassOf>
                <http://purl.org/olia/olia-top.owl#NumberFeature> ;
        <http://www.w3.org/2002/07/owl#versionInfo>
                "http://www.isocat.org/datcat/DC-1879" , "subClassOf grammaticalNumber (dcif:conceptualDomain)" .

<http://purl.org/olia/olia-top.owl#DominanceRelation>
        a       <http://www.w3.org/2002/07/owl#Class> ;
        <http://www.w3.org/2000/01/rdf-schema#subClassOf>
                <http://purl.org/olia/olia-top.owl#SyntacticRelation> .

<http://purl.org/olia/olia.owl#OmittedUnit>
        a       <http://www.w3.org/2002/07/owl#Class> ;
        <http://www.w3.org/2000/01/rdf-schema#comment>
                "*U*\nâ ´ unit ...\nThis element marks the interpreted position of a unit symbol, such as $, # (British pounds), FFr (French francs), C$, US$, HK$, A$, M$, S$, and NZ$. It may also appear after % or even cents, when convenient. See section 11 [Modification of NP] for more details on the use of *U*. ...\nIn general, *U* is placed where the word corresponding to the symbol would appear in the string if the text were read aloud. One notable exception is in certain hyphenated compound adjectives, such as a $5-a-share increase (spoken: â ¼A five dollar a share increaseâ ½). Here, the bracketing will usually not reflect the spoken order, with *U* placed as the last element in the ADJP: \n\n  (NP a (ADJP $ 5-a-share *U*)\n      increase)\n\nSometimes, this type may lack the *U* entirely. \n(Bies et al. 1995)" ;
        <http://www.w3.org/2000/01/rdf-schema#subClassOf>
                <http://purl.org/olia/olia-top.owl#NullElement> ;
        <http://www.w3.org/2002/07/owl#versionInfo>
                "added in conformance with PTB bracketing guidelines (Santorini 1991, Bies et al. 1995)" .

<http://purl.org/olia/olia.owl#SecondNonHonorific>
        a       <http://www.w3.org/2002/07/owl#Class> ;
        <http://www.w3.org/2000/01/rdf-schema#subClassOf>
                <http://purl.org/olia/olia.owl#Second> ;
        <http://www.w3.org/2002/07/owl#versionInfo>
                "TOCHECK: is SecondNonHonorific different from SecondFamiliar ?" , "Adopted from ILPOSTS for Indian languages, http://purl.org/olia/ilposts.owl#NonHonorific" .

<http://purl.org/olia/olia-top.owl#SyntacticConstruction>
        a       <http://www.w3.org/2002/07/owl#Class> .

<http://purl.org/olia/olia.owl#Trace>
        a       <http://www.w3.org/2002/07/owl#Class> ;
        <http://www.w3.org/2000/01/rdf-schema#comment>
                "T|Trace. Marks the position where a fronted wh-constituent is interpreted. ...\n\nT marks the spot where an argument NP that has been moved by wh-movement or relative clause\nformation is interpreted. For instance, the relative clause the man that I saw should be bracketed as\nfollows, by analogy to the corresponding simple declarative I saw the man.\n\n(NP (NP the man) (SBAR that (S (NP I) (VP saw) (NP T)))))\n\nT is also used to represent the empty subjects of as-clauses.\n(Santorini 1991)\n\n*T*\nâ ´ trace of Aâ ²-movement \n(Bies et al. 1995)" ;
        <http://www.w3.org/2000/01/rdf-schema#subClassOf>
                <http://purl.org/olia/olia-top.owl#NullElement> ;
        <http://www.w3.org/2002/07/owl#versionInfo>
                "PTB bracketing guidelines, Bies et al. (1995)" .

<http://purl.org/olia/olia-top.owl#SeparabilityFeature>
        a       <http://www.w3.org/2002/07/owl#Class> ;
        <http://www.w3.org/2000/01/rdf-schema#subClassOf>
                [ a       <http://www.w3.org/2002/07/owl#Restriction> ;
                  <http://www.w3.org/2002/07/owl#hasSelf>
                          true ;
                  <http://www.w3.org/2002/07/owl#onProperty>
                          <http://purl.org/olia/olia.owl#hasSeparability>
                ] ;
        <http://www.w3.org/2000/01/rdf-schema#subClassOf>
                [ a       <http://www.w3.org/2002/07/owl#Restriction> ;
                  <http://www.w3.org/2002/07/owl#hasSelf>
                          true ;
                  <http://www.w3.org/2002/07/owl#onProperty>
                          <http://purl.org/olia/olia.owl#hasSeparability>
                ] .

<http://purl.org/olia/olia.owl#NonfiniteVerbPhrase>
        a       <http://www.w3.org/2002/07/owl#Class> ;
        <http://www.w3.org/2000/01/rdf-schema#subClassOf>
                <http://purl.org/olia/olia.owl#VerbPhrase> ;
        <http://www.w3.org/2002/07/owl#versionInfo>
                "TüBa-D/Z" .

<http://purl.org/olia/olia.owl#PersonalPassive>
        a       <http://www.w3.org/2002/07/owl#Class> ;
        <http://www.w3.org/2000/01/rdf-schema#comment>
                "\n\t\t\tA Passive in which the argument mapped to Object in a basic \n\t\t\tstructural configuration assumes the Subject relation in a \n\t\t\tcorresponding nonbasic configuration. (Klaiman 1991:23)\n\t\t\t(http://purl.org/linguistics/gold/PersonalPassive)\n\t\t" ;
        <http://www.w3.org/2000/01/rdf-schema#subClassOf>
                <http://purl.org/olia/olia.owl#PassiveVoice> ;
        <http://www.w3.org/2002/07/owl#versionInfo>
                "http://purl.org/linguistics/gold/PersonalPassive" .

<http://purl.org/olia/olia-top.owl#MovementFeature>
        a       <http://www.w3.org/2002/07/owl#Class> ;
        <http://www.w3.org/2000/01/rdf-schema#subClassOf>
                [ a       <http://www.w3.org/2002/07/owl#Restriction> ;
                  <http://www.w3.org/2002/07/owl#hasSelf>
                          true ;
                  <http://www.w3.org/2002/07/owl#onProperty>
                          <http://purl.org/olia/olia.owl#hasMovementFeature>
                ] ;
        <http://www.w3.org/2002/07/owl#versionInfo>
                "\n\t\t\t2016/08/29 introduced to account for raising and control features in lexinfo\n\t\t" .

<http://purl.org/olia/system.owl#hasFeature>
        a       <http://www.w3.org/2002/07/owl#ObjectProperty> .

<http://purl.org/olia/olia-top.owl#MorphosyntacticCategory>
        a       <http://www.w3.org/2002/07/owl#Class> .

<http://purl.org/olia/olia-top.owl#GenderFeature>
        a       <http://www.w3.org/2002/07/owl#Class> ;
        <http://www.w3.org/2000/01/rdf-schema#subClassOf>
                [ a       <http://www.w3.org/2002/07/owl#Restriction> ;
                  <http://www.w3.org/2002/07/owl#hasSelf>
                          true ;
                  <http://www.w3.org/2002/07/owl#onProperty>
                          <http://purl.org/olia/olia.owl#hasGender>
                ] .

<http://purl.org/olia/olia.owl#VisualEvidentiality>
        a       <http://www.w3.org/2002/07/owl#Class> ;
        <http://www.w3.org/2000/01/rdf-schema#comment>
                "VisualEvidentiality encodes the fact that the\n                        speaker came to believe the content of the expression through direct visual\n                        experience; they saw it [Palmer 2001: 57]." ;
        <http://www.w3.org/2000/01/rdf-schema#isDefinedBy>
                "http://www.isocat.org/datcat/DC-3549" ;
        <http://www.w3.org/2000/01/rdf-schema#subClassOf>
                <http://purl.org/olia/olia-top.owl#EvidentialityFeature> .

<http://purl.org/olia/olia-top.owl#DegreeFeature>
        a       <http://www.w3.org/2002/07/owl#Class> ;
        <http://www.w3.org/2000/01/rdf-schema#subClassOf>
                [ a       <http://www.w3.org/2002/07/owl#Restriction> ;
                  <http://www.w3.org/2002/07/owl#hasSelf>
                          true ;
                  <http://www.w3.org/2002/07/owl#onProperty>
                          <http://purl.org/olia/olia.owl#hasDegree>
                ] .

<http://purl.org/olia/system.owl>
        a       <http://www.w3.org/2002/07/owl#Ontology> .

<http://purl.org/olia/olia-top.owl#UsageAndFrequencyFeature>
        a       <http://www.w3.org/2002/07/owl#Class> .

<http://purl.org/olia/system.owl#hasSource>
        a       <http://www.w3.org/2002/07/owl#ObjectProperty> .

<http://purl.org/olia/system.owl#Relation>
        a       <http://www.w3.org/2002/07/owl#Class> .

<http://purl.org/olia/olia-top.owl#MorphologicalProcess>
        a       <http://www.w3.org/2002/07/owl#Class> .

<http://purl.org/olia/olia-top.owl#LexicalRelation>
        a       <http://www.w3.org/2002/07/owl#Class> .
