<http://def.seegrid.csiro.au/ontology/om/om-lite> <http://purl.org/dc/elements/1.1/title> "OWL for Observations" .
_:B1dde258848a73b3d73221fbc5cb2b4d8 <http://www.w3.org/1999/02/22-rdf-syntax-ns#type> <http://www.w3.org/2002/07/owl#Class> .
<http://def.seegrid.csiro.au/ontology/om/om-lite#result> <http://www.w3.org/2000/01/rdf-schema#isDefinedBy> <http://def.seegrid.csiro.au/ontology/om/om-lite> .
<http://def.seegrid.csiro.au/ontology/om/om-lite#count> <http://www.w3.org/1999/02/22-rdf-syntax-ns#type> <http://www.w3.org/2002/07/owl#DatatypeProperty> .
<http://def.seegrid.csiro.au/ontology/om/om-lite#stimulusTime> <http://www.w3.org/2000/01/rdf-schema#range> <http://def.seegrid.csiro.au/ontology/om/om-lite#TemporalObject> .
<http://def.seegrid.csiro.au/ontology/om/om-lite> <http://www.w3.org/2004/02/skos/core#changeNote> "2016-01-20 In order to satisfy OWLAPI requirements, changed oml:result to an ObjectProperty; changed the constraints on CountObservation and TruthObservation to refer to newly created CountObject and TruthObject to encapsulate the values as objects. " .
_:Bb8769301438bcead254f75e9f6f527ff <http://www.w3.org/2002/07/owl#cardinality> "1"^^<http://www.w3.org/2001/XMLSchema#nonNegativeInteger> .
_:B50eaf67a7bf22d8e8921561ecf98739d <http://www.w3.org/1999/02/22-rdf-syntax-ns#type> <http://www.w3.org/2002/07/owl#Restriction> .
_:B78d4842cX2Dc91fX2D4492X2D9f07X2D2fae7b8a3cca <http://www.w3.org/1999/02/22-rdf-syntax-ns#first> <http://def.seegrid.csiro.au/ontology/om/om-lite#ObservationCollection> .
<http://def.seegrid.csiro.au/ontology/om/om-lite#GeometryObject> <http://www.w3.org/2000/01/rdf-schema#label> "Geometry object" .
<http://def.seegrid.csiro.au/ontology/om/om-lite#phenomenonTime> <http://www.w3.org/2000/01/rdf-schema#domain> _:B1c17d32cd4610480f3ed1e8b276cb470 .
<http://def.seegrid.csiro.au/ontology/om/om-lite#Observation> <http://www.w3.org/2004/02/skos/core#prefLabel> "Observation"@en .
<http://def.seegrid.csiro.au/ontology/om/om-lite#TemporalObject> <http://purl.org/dc/terms/description> "Temporal object has properties relating to time only. " .
<http://def.seegrid.csiro.au/ontology/om/om-lite#result> <http://www.w3.org/1999/02/22-rdf-syntax-ns#type> <http://www.w3.org/2002/07/owl#ObjectProperty> .
_:Bf223756303d98c258aa73b4c1c1650ad <http://www.w3.org/2002/07/owl#unionOf> _:B6c38d313X2D552dX2D4271X2D9666X2Dd9debc6d6d28 .
<http://def.seegrid.csiro.au/ontology/om/om-lite#memberOf> <http://www.w3.org/2002/07/owl#inverseOf> <http://def.seegrid.csiro.au/ontology/om/om-lite#member> .
_:Baecbfb97X2Dd8b8X2D4c33X2D973bX2D2f53751c121b <http://www.w3.org/1999/02/22-rdf-syntax-ns#rest> <http://www.w3.org/1999/02/22-rdf-syntax-ns#nil> .
<http://def.seegrid.csiro.au/ontology/om/om-lite#procedure> <http://www.w3.org/2000/01/rdf-schema#label> "observation procedure"@en .
_:Bbdb601234954ca5ad43d51824dc68a82 <http://www.w3.org/2002/07/owl#allValuesFrom> <http://def.seegrid.csiro.au/ontology/om/om-lite#TemporalObject> .
<http://def.seegrid.csiro.au/ontology/om/om-lite#context> <http://purl.org/dc/terms/description> "link to related observation" .
_:B9983583fX2D80a6X2D482cX2Da8ceX2Dd9078ec63814 <http://www.w3.org/1999/02/22-rdf-syntax-ns#first> <http://def.seegrid.csiro.au/ontology/om/om-lite#ObservationCollection> .
_:B16d39e172dfa5589e895c76d6dbe71ec <http://www.w3.org/2002/07/owl#onProperty> <http://def.seegrid.csiro.au/ontology/om/om-lite#resultTime> .
_:Bb051caff24401dc682173242bb0fb13d <http://www.w3.org/1999/02/22-rdf-syntax-ns#type> <http://www.w3.org/2002/07/owl#Restriction> .
_:B50eaf67a7bf22d8e8921561ecf98739d <http://www.w3.org/2002/07/owl#minCardinality> "1"^^<http://www.w3.org/2001/XMLSchema#nonNegativeInteger> .
_:B3497aa63X2D3ab7X2D4000X2D8dcfX2D488a9324d29a <http://www.w3.org/1999/02/22-rdf-syntax-ns#first> <http://def.seegrid.csiro.au/ontology/om/om-lite#Observation> .
<http://def.seegrid.csiro.au/ontology/om/om-lite#TemporalObservation> <http://www.w3.org/2000/01/rdf-schema#subClassOf> <http://def.seegrid.csiro.au/ontology/om/om-lite#Observation> .
<http://def.seegrid.csiro.au/ontology/om/om-lite#MeasureObject> <http://www.w3.org/1999/02/22-rdf-syntax-ns#type> <http://www.w3.org/2002/07/owl#Class> .
<http://def.seegrid.csiro.au/ontology/om/om-lite> <http://purl.org/dc/terms/creator> <http://orcid.org/0000-0002-3884-3420> .
_:B888d011eX2Db4d6X2D4cdbX2D8fc1X2D1a97526f65eb <http://www.w3.org/1999/02/22-rdf-syntax-ns#rest> <http://www.w3.org/1999/02/22-rdf-syntax-ns#nil> .
<http://def.seegrid.csiro.au/ontology/om/om-lite#member> <http://www.w3.org/2000/01/rdf-schema#label> "has member" .
_:Bbdb601234954ca5ad43d51824dc68a82 <http://www.w3.org/1999/02/22-rdf-syntax-ns#type> <http://www.w3.org/2002/07/owl#Restriction> .
<http://def.seegrid.csiro.au/ontology/om/om-lite#role> <http://www.w3.org/2000/01/rdf-schema#comment> "role of related observation with respect to the observation of interest" .
_:B140e8a686820c18417c3e58bedc8a59c <http://www.w3.org/2002/07/owl#unionOf> _:B8c1681b3X2Daff1X2D4e96X2Db7e9X2Dcfa925323a50 .
_:B8a6f28921cceab0d9746aba4ee3cdcb7 <http://www.w3.org/2002/07/owl#onProperty> <http://def.seegrid.csiro.au/ontology/om/om-lite#featureOfInterest> .
_:Bd8d83bd31e604d7e3f203192c3bf5f94 <http://www.w3.org/1999/02/22-rdf-syntax-ns#type> <http://www.w3.org/2002/07/owl#Restriction> .
<http://def.seegrid.csiro.au/ontology/om/om-lite#memberOf> <http://www.w3.org/2000/01/rdf-schema#label> "is member of" .
_:B1c17d32cd4610480f3ed1e8b276cb470 <http://www.w3.org/1999/02/22-rdf-syntax-ns#type> <http://www.w3.org/2002/07/owl#Class> .
<http://def.seegrid.csiro.au/ontology/om/om-lite#truth> <http://www.w3.org/2000/01/rdf-schema#range> <http://www.w3.org/2001/XMLSchema#boolean> .
<http://def.seegrid.csiro.au/ontology/om/om-lite#TemporalObject> <http://www.w3.org/2000/01/rdf-schema#isDefinedBy> <http://def.seegrid.csiro.au/ontology/om/om-lite> .
<http://def.seegrid.csiro.au/ontology/om/om-lite> <http://purl.org/dc/terms/modified> "2016-10-27"^^<http://www.w3.org/2001/XMLSchema#date> .
<http://def.seegrid.csiro.au/ontology/om/om-lite#observedProperty> <http://www.w3.org/2000/01/rdf-schema#isDefinedBy> <http://def.seegrid.csiro.au/ontology/om/om-lite> .
_:B139b0cc72866386a3920a0445613f33f <http://www.w3.org/2002/07/owl#unionOf> _:B3471dad1X2D53d2X2D4655X2Da217X2Df14bf473f50b .
_:B6085a7cf84f730f2eb96448f8674cc83 <http://www.w3.org/2002/07/owl#cardinality> "1"^^<http://www.w3.org/2001/XMLSchema#nonNegativeInteger> .
<http://def.seegrid.csiro.au/ontology/om/om-lite#member> <http://www.w3.org/2000/01/rdf-schema#comment> "links from a collection to a member collection or observation" .
<http://def.seegrid.csiro.au/ontology/om/om-lite#observedProperty> <http://www.w3.org/1999/02/22-rdf-syntax-ns#type> <http://www.w3.org/2002/07/owl#ObjectProperty> .
<http://def.seegrid.csiro.au/ontology/om/om-lite#samplingStrategy> <http://www.w3.org/2000/01/rdf-schema#comment> "Links to a feature intended to sample the real-world object, as described in Clause 9 of ISO 19156:2011. \r\n\r\nN.B. this formulation varies from the UML model in ISO 19156, in which a sampling-feature is substitutable for the feature-of-interest. In this more explicit formulation, the (mandatory) feature-of-interest always refers to the ultimate feature of interest, whose type can carry the observed property, and the (optional) sampling strategy allows the sampling feature to be made explicit as an additional relationship. This overcomes some semantic sleight-of-hand in ISO 19156, in which the constraint the the observed property was commensurate with the feature-of-interest was allowed to be 'transitive' via the sampledFeature property." .
<http://def.seegrid.csiro.au/ontology/om/om-lite#procedure> <http://www.w3.org/2000/01/rdf-schema#comment> "re-usable procedure used in making observation. Typically a sensor or sensor-system, algorithm, computational procedure." .
<http://def.seegrid.csiro.au/ontology/om/om-lite#truth> <http://www.w3.org/1999/02/22-rdf-syntax-ns#type> <http://www.w3.org/2002/07/owl#DatatypeProperty> .
_:B20c87f74f75ee72db9eccc08f342473e <http://www.w3.org/2002/07/owl#onProperty> <http://def.seegrid.csiro.au/ontology/om/om-lite#result> .
<http://def.seegrid.csiro.au/ontology/om/om-lite#Measurement> <http://www.w3.org/2000/01/rdf-schema#comment> "Observation whose result is a scaled number" .
<http://def.seegrid.csiro.au/ontology/om/om-lite#result> <http://www.w3.org/2000/01/rdf-schema#label> "observation result"@en .
<http://def.seegrid.csiro.au/ontology/om/om-lite> <http://www.w3.org/2000/01/rdf-schema#seeAlso> <http://www.semantic-web-journal.net/content/ontology-observations-and-sampling-features-alignments-existing-models-0> .
<http://def.seegrid.csiro.au/ontology/om/om-lite> <http://purl.org/dc/terms/license> <http://creativecommons.org/licenses/by/3.0/au/> .
_:B812aa08271c375826eee91c12beb1d04 <http://www.w3.org/1999/02/22-rdf-syntax-ns#type> <http://www.w3.org/2002/07/owl#Restriction> .
_:B888d011eX2Db4d6X2D4cdbX2D8fc1X2D1a97526f65eb <http://www.w3.org/1999/02/22-rdf-syntax-ns#first> <http://def.seegrid.csiro.au/ontology/om/om-lite#ObservationCollection> .
_:B3497aa63X2D3ab7X2D4000X2D8dcfX2D488a9324d29a <http://www.w3.org/1999/02/22-rdf-syntax-ns#rest> _:B2882679eX2D556cX2D4616X2D9107X2D1a35bb0db0ba .
<http://def.seegrid.csiro.au/ontology/om/om-lite#TruthObject> <http://www.w3.org/2000/01/rdf-schema#comment> "Object to wrap a truth value" .
<http://def.seegrid.csiro.au/ontology/om/om-lite#CountObservation> <http://www.w3.org/1999/02/22-rdf-syntax-ns#type> <http://www.w3.org/2002/07/owl#Class> .
<http://def.seegrid.csiro.au/ontology/om/om-lite#count> <http://www.w3.org/2000/01/rdf-schema#isDefinedBy> <http://def.seegrid.csiro.au/ontology/om/om-lite> .
<http://def.seegrid.csiro.au/ontology/om/om-lite#TruthObservation> <http://www.w3.org/1999/02/22-rdf-syntax-ns#type> <http://www.w3.org/2002/07/owl#Class> .
<http://def.seegrid.csiro.au/ontology/om/om-lite#stimulusTime> <http://www.w3.org/2000/01/rdf-schema#label> "Stimulus time" .
<http://def.seegrid.csiro.au/ontology/om/om-lite#phenomenonTime> <http://www.w3.org/2004/02/skos/core#definition> "The attribute phenomenonTime:TM_Object shall describe the time that the result (7.2.2.9) applies to the property of the feature-of-interest (7.2.2.7). This is often the time of interaction by a sampling procedure (9.1.3) or observation procedure (7.2.2.10) with a real-world feature.\r\n\r\nNOTE The phenomenonTime is the temporal parameter normally used in geospatial analysis of the result.\r\n\r\nIf the observedProperty of an observation is ‘occurrence time’ then the result should be the same as the phenomenonTime." .
_:Bcaa52b8ca80d3545838555278ed1f713 <http://www.w3.org/1999/02/22-rdf-syntax-ns#type> <http://www.w3.org/2002/07/owl#Restriction> .
<http://def.seegrid.csiro.au/ontology/om/om-lite#uom> <http://www.w3.org/1999/02/22-rdf-syntax-ns#type> <http://www.w3.org/2002/07/owl#ObjectProperty> .
<http://def.seegrid.csiro.au/ontology/om/om-lite#TemporalObservation> <http://www.w3.org/2000/01/rdf-schema#comment> "Observation whose result is a temporal object, such as a time instant or period" .
<http://def.seegrid.csiro.au/ontology/om/om-lite#featureOfInterest> <http://www.w3.org/2000/01/rdf-schema#label> "feature of interest"@en .
<http://def.seegrid.csiro.au/ontology/om/om-lite#uom> <http://www.w3.org/2000/01/rdf-schema#isDefinedBy> <http://def.seegrid.csiro.au/ontology/om/om-lite> .
<http://def.seegrid.csiro.au/ontology/om/om-lite#TemporalObservation> <http://www.w3.org/2000/01/rdf-schema#isDefinedBy> <http://def.seegrid.csiro.au/ontology/om/om-lite> .
<http://def.seegrid.csiro.au/ontology/om/om-lite#ObservationCollection> <http://www.w3.org/2000/01/rdf-schema#isDefinedBy> <http://def.seegrid.csiro.au/ontology/om/om-lite> .
<http://def.seegrid.csiro.au/ontology/om/om-lite> <http://www.w3.org/2004/02/skos/core#changeNote> "2015-11-17 Added oml:member property, with fixed domain (ObservationCollection) and range (Observation), in place of rdfs:member, which is not liked by OWL-API. " .
_:B78d4842cX2Dc91fX2D4492X2D9f07X2D2fae7b8a3cca <http://www.w3.org/1999/02/22-rdf-syntax-ns#rest> <http://www.w3.org/1999/02/22-rdf-syntax-ns#nil> .
<http://def.seegrid.csiro.au/ontology/om/om-lite#resultTime> <http://www.w3.org/2000/01/rdf-schema#domain> _:B257584f566e1431eeab7d36f63c2e67f .
<http://def.seegrid.csiro.au/ontology/om/om-lite#uom> <http://www.w3.org/2000/01/rdf-schema#domain> _:B5231bb242b1062681893c57a25b8b174 .
_:B3471dad1X2D53d2X2D4655X2Da217X2Df14bf473f50b <http://www.w3.org/1999/02/22-rdf-syntax-ns#rest> _:B9983583fX2D80a6X2D482cX2Da8ceX2Dd9078ec63814 .
<http://def.seegrid.csiro.au/ontology/om/om-lite> <http://www.w3.org/2000/01/rdf-schema#comment> "An OWL representation of the Observation Schema described in clauses 7-8 of ISO 19156:2011 Geographic Information - Observations and Measurements. \r\nIn contrast to previous versions developed through SSN and in conjunction with ISO 19150-2, this ontology has minimal dependencies on existing ontologies, particularly those that trigger extended chains of imports. Stub classes are provided for time, geometry and measure (scaled number), which can be substituted at run-time by a suitable concrete representation of the concept. \r\nObservation Collection has been (re-)introduced, to support the common case where a collection is homogeneous in one or more properties (feature-of-interest, phenomenon-time, observed-property, units-of-measure, procedure). The value of the common property may be recorded against the collection instead of repetitively against every member.   \r\n\r\nIn this revision, the observation result is an Object Property, in order to conform to strict OWL2 semantics. The type constraints on Observation specializations TruthObservation and CountObservation have been changed, so that the range of oml:result is an Object containing the xsd type, rather than the data-type itself. " .
_:B58f8565765b4edcde463571c9484a8f1 <http://www.w3.org/1999/02/22-rdf-syntax-ns#type> <http://www.w3.org/2002/07/owl#Restriction> .
_:B9983583fX2D80a6X2D482cX2Da8ceX2Dd9078ec63814 <http://www.w3.org/1999/02/22-rdf-syntax-ns#rest> <http://www.w3.org/1999/02/22-rdf-syntax-ns#nil> .
<http://def.seegrid.csiro.au/ontology/om/om-lite#stimulusTime> <http://www.w3.org/2000/01/rdf-schema#comment> "the time when the sensor stimulus occurred. Usually the beginning of the observation activity (the result time is the end). " .
_:Baecbfb97X2Dd8b8X2D4c33X2D973bX2D2f53751c121b <http://www.w3.org/1999/02/22-rdf-syntax-ns#first> <http://def.seegrid.csiro.au/ontology/om/om-lite#ObservationCollection> .
<http://def.seegrid.csiro.au/ontology/om/om-lite#phenomenonTime> <http://www.w3.org/2000/01/rdf-schema#range> <http://def.seegrid.csiro.au/ontology/om/om-lite#TemporalObject> .
<http://def.seegrid.csiro.au/ontology/om/om-lite> <http://www.w3.org/2004/02/skos/core#changeNote> "2015-03-06\tAdded samplingStrategy property, in order to separate sampling from the feature of interest" .
_:B812aa08271c375826eee91c12beb1d04 <http://www.w3.org/2002/07/owl#onProperty> <http://def.seegrid.csiro.au/ontology/om/om-lite#observedProperty> .
<http://def.seegrid.csiro.au/ontology/om/om-lite#Observation> <http://www.w3.org/2004/02/skos/core#altLabel> "Generic observation" .
<http://def.seegrid.csiro.au/ontology/om/om-lite#TruthObject> <http://www.w3.org/1999/02/22-rdf-syntax-ns#type> <http://www.w3.org/2002/07/owl#Class> .
<http://def.seegrid.csiro.au/ontology/om/om-lite#truth> <http://www.w3.org/2000/01/rdf-schema#isDefinedBy> <http://def.seegrid.csiro.au/ontology/om/om-lite> .
<http://def.seegrid.csiro.au/ontology/om/om-lite#count> <http://www.w3.org/2000/01/rdf-schema#range> <http://www.w3.org/2001/XMLSchema#integer> .
<http://def.seegrid.csiro.au/ontology/om/om-lite#featureOfInterest> <http://www.w3.org/2004/02/skos/core#definition> "Links the Observation to the Feature that is the ultimate subject of the observation and carries the observed property. This feature is the real-world object whose properties are under observation. An observation instance serves as a propertyValueProvider for its feature-of-interest." .
_:B67ceae38X2Dea94X2D42ccX2D8f0dX2Dad5ab43c4b15 <http://www.w3.org/1999/02/22-rdf-syntax-ns#first> <http://def.seegrid.csiro.au/ontology/om/om-lite#Observation> .
_:B86fa036dX2Dc15aX2D45deX2Dae14X2D9ee642eecc9d <http://www.w3.org/1999/02/22-rdf-syntax-ns#first> <http://def.seegrid.csiro.au/ontology/om/om-lite#Observation> .
<http://def.seegrid.csiro.au/ontology/om/om-lite#CountObservation> <http://www.w3.org/2000/01/rdf-schema#subClassOf> _:B20c87f74f75ee72db9eccc08f342473e .
_:B6c38d313X2D552dX2D4271X2D9666X2Dd9debc6d6d28 <http://www.w3.org/1999/02/22-rdf-syntax-ns#rest> _:B8b9125beX2Dba46X2D4196X2Dab0cX2D22764eba82d3 .
<http://def.seegrid.csiro.au/ontology/om/om-lite#TruthObservation> <http://www.w3.org/2000/01/rdf-schema#label> "Truth Observation"@en .
<http://def.seegrid.csiro.au/ontology/om/om-lite#Observation> <http://www.w3.org/2000/01/rdf-schema#subClassOf> _:Bb8769301438bcead254f75e9f6f527ff .
_:Bf223756303d98c258aa73b4c1c1650ad <http://www.w3.org/1999/02/22-rdf-syntax-ns#type> <http://www.w3.org/2002/07/owl#Class> .
<http://def.seegrid.csiro.au/ontology/om/om-lite#phenomenonTime> <http://www.w3.org/2000/01/rdf-schema#label> "phenomenon time"@en .
_:Ba4ce6720X2D5c83X2D4adcX2D8300X2De9be357e3e8b <http://www.w3.org/1999/02/22-rdf-syntax-ns#rest> _:B0f39e608X2D6e7aX2D41a3X2Db722X2D9505b7d87375 .
<http://def.seegrid.csiro.au/ontology/om/om-lite#resultTime> <http://www.w3.org/1999/02/22-rdf-syntax-ns#type> <http://www.w3.org/2002/07/owl#DatatypeProperty> .
<http://def.seegrid.csiro.au/ontology/om/om-lite> <http://purl.org/dc/terms/created> "2014-10-07"^^<http://www.w3.org/2001/XMLSchema#date> .
<http://def.seegrid.csiro.au/ontology/om/om-lite#TemporalObservation> <http://www.w3.org/1999/02/22-rdf-syntax-ns#type> <http://www.w3.org/2002/07/owl#Class> .
<http://def.seegrid.csiro.au/ontology/om/om-lite#GeometryObject> <http://www.w3.org/2000/01/rdf-schema#subClassOf> <http://www.w3.org/2002/07/owl#Thing> .
<http://def.seegrid.csiro.au/ontology/om/om-lite#ObservationCollection> <http://www.w3.org/1999/02/22-rdf-syntax-ns#type> <http://www.w3.org/2002/07/owl#Class> .
_:B3471dad1X2D53d2X2D4655X2Da217X2Df14bf473f50b <http://www.w3.org/1999/02/22-rdf-syntax-ns#first> <http://def.seegrid.csiro.au/ontology/om/om-lite#Observation> .
<http://def.seegrid.csiro.au/ontology/om/om-lite#ObservationContext> <http://purl.org/dc/terms/description> "Context linking two or more observations" .
<http://def.seegrid.csiro.au/ontology/om/om-lite#TruthObservation> <http://www.w3.org/2000/01/rdf-schema#isDefinedBy> <http://def.seegrid.csiro.au/ontology/om/om-lite> .
<http://def.seegrid.csiro.au/ontology/om/om-lite#GeometryObservation> <http://www.w3.org/2000/01/rdf-schema#subClassOf> _:B535c16bb4a3db7a00d957fb3a8ebe55e .
<http://def.seegrid.csiro.au/ontology/om/om-lite> <http://purl.org/dc/elements/1.1/creator> "Simon Jonathan David COX\nCSIRO" .
<http://def.seegrid.csiro.au/ontology/om/om-lite> <http://purl.org/dc/elements/1.1/rights> "Copyright © 2014, 2015, 2016 CSIRO" .
<http://def.seegrid.csiro.au/ontology/om/om-lite#Observation> <http://www.w3.org/2000/01/rdf-schema#comment> "An observation is an act associated with a discrete time instant or period through which a number, term or other symbol is assigned to a phenomenon [2]. It involves application of a specified procedure, such as a sensor, instrument, algorithm or process chain. The procedure may be applied in-situ, remotely, or ex-situ with respect to the sampling location. The procedure may take inputs from the environment (as stimuli) or from the results of prior observations or processes. The result of an observation is an estimate of the value of a property of some feature. \r\n\r\nUse of a common model allows observation data using different procedures to be combined unambiguously.\r\n\r\nThe observation itself is also a feature, since it has properties and identity.\r\n\r\nObservation details are important for data discovery and for data quality estimation.\r\n\r\nThe observation could be considered to carry metadata about an instance of a property (of the feature of interest). This property-value metadata complements the dataset and feature metadata that have been conventionally considered (e.g. ISO 19115).\r\n\r\nThe values for the properties 'procedure', 'featureOfInterest', 'observedProperty', 'phenomenonTime', 'resultTime' may be inherited from a container resource." .
_:B774ffb5a0482acf60193dde3f13477dd <http://www.w3.org/2002/07/owl#cardinality> "1"^^<http://www.w3.org/2001/XMLSchema#nonNegativeInteger> .
<http://def.seegrid.csiro.au/ontology/om/om-lite#samplingStrategy> <http://www.w3.org/2000/01/rdf-schema#comment> "description of the sampling strategy used in an observation (usually a sampling-feature). " .
<http://def.seegrid.csiro.au/ontology/om/om-lite#SimpleMeasure> <http://www.w3.org/2000/01/rdf-schema#subClassOf> _:Bb051caff24401dc682173242bb0fb13d .
<http://def.seegrid.csiro.au/ontology/om/om-lite#Observation> <http://www.w3.org/2000/01/rdf-schema#subClassOf> _:B6085a7cf84f730f2eb96448f8674cc83 .
_:B5231bb242b1062681893c57a25b8b174 <http://www.w3.org/2002/07/owl#unionOf> _:Ba4ce6720X2D5c83X2D4adcX2D8300X2De9be357e3e8b .
<http://def.seegrid.csiro.au/ontology/om/om-lite#Observation> <http://www.w3.org/2000/01/rdf-schema#subClassOf> _:B8a6f28921cceab0d9746aba4ee3cdcb7 .
<http://def.seegrid.csiro.au/ontology/om/om-lite#member> <http://www.w3.org/1999/02/22-rdf-syntax-ns#type> <http://www.w3.org/2002/07/owl#ObjectProperty> .
_:B34f7c049bcbe3e1f79174c183e61696b <http://www.w3.org/1999/02/22-rdf-syntax-ns#type> <http://www.w3.org/2002/07/owl#Class> .
<http://def.seegrid.csiro.au/ontology/om/om-lite#CountObservation> <http://www.w3.org/2000/01/rdf-schema#isDefinedBy> <http://def.seegrid.csiro.au/ontology/om/om-lite> .
<http://def.seegrid.csiro.au/ontology/om/om-lite#member> <http://www.w3.org/2000/01/rdf-schema#isDefinedBy> <http://def.seegrid.csiro.au/ontology/om/om-lite> .
_:B50eaf67a7bf22d8e8921561ecf98739d <http://www.w3.org/2002/07/owl#onProperty> <http://def.seegrid.csiro.au/ontology/om/om-lite#member> .
_:B44f4de9d822ec3fde44a89c25a4c4a8f <http://www.w3.org/2002/07/owl#allValuesFrom> <http://def.seegrid.csiro.au/ontology/om/om-lite#MeasureObject> .
<http://def.seegrid.csiro.au/ontology/om/om-lite#truth> <http://www.w3.org/2000/01/rdf-schema#label> "Truth value" .
<http://def.seegrid.csiro.au/ontology/om/om-lite#SimpleMeasure> <http://www.w3.org/2000/01/rdf-schema#label> "Simple measure (quantity)" .
<http://def.seegrid.csiro.au/ontology/om/om-lite#observedProperty> <http://www.w3.org/2000/01/rdf-schema#label> "observed property"@en .
_:Be80c213bX2DbcecX2D4951X2D9e68X2D67704070d8c9 <http://www.w3.org/1999/02/22-rdf-syntax-ns#first> <http://def.seegrid.csiro.au/ontology/om/om-lite#Observation> .
_:Bca63bb81X2D5f78X2D4ea1X2D8db8X2D15169052a651 <http://www.w3.org/1999/02/22-rdf-syntax-ns#rest> <http://www.w3.org/1999/02/22-rdf-syntax-ns#nil> .
<http://def.seegrid.csiro.au/ontology/om/om-lite#TruthObject> <http://www.w3.org/2000/01/rdf-schema#isDefinedBy> <http://def.seegrid.csiro.au/ontology/om/om-lite> .
<http://def.seegrid.csiro.au/ontology/om/om-lite#Measurement> <http://www.w3.org/2000/01/rdf-schema#label> "Measurement"@en .
<http://def.seegrid.csiro.au/ontology/om/om-lite#role> <http://www.w3.org/2000/01/rdf-schema#domain> <http://def.seegrid.csiro.au/ontology/om/om-lite#ObservationContext> .
<http://def.seegrid.csiro.au/ontology/om/om-lite#resultTime> <http://www.w3.org/2000/01/rdf-schema#comment> "time at which the result became available, after all processing steps were completed" .
<http://def.seegrid.csiro.au/ontology/om/om-lite#procedure> <http://www.w3.org/1999/02/22-rdf-syntax-ns#type> <http://www.w3.org/2002/07/owl#ObjectProperty> .
<http://def.seegrid.csiro.au/ontology/om/om-lite#samplingStrategy> <http://www.w3.org/2000/01/rdf-schema#isDefinedBy> <http://def.seegrid.csiro.au/ontology/om/om-lite> .
<http://def.seegrid.csiro.au/ontology/om/om-lite#amount> <http://www.w3.org/2000/01/rdf-schema#label> "numeric amount value" .
<http://def.seegrid.csiro.au/ontology/om/om-lite#context> <http://www.w3.org/2000/01/rdf-schema#domain> _:B1dde258848a73b3d73221fbc5cb2b4d8 .
_:B8a6f28921cceab0d9746aba4ee3cdcb7 <http://www.w3.org/2002/07/owl#cardinality> "1"^^<http://www.w3.org/2001/XMLSchema#nonNegativeInteger> .
_:B257584f566e1431eeab7d36f63c2e67f <http://www.w3.org/2002/07/owl#unionOf> _:B0b84d8caX2Da2f9X2D4bb7X2D9039X2Dba58989551fb .
<http://def.seegrid.csiro.au/ontology/om/om-lite#result> <http://www.w3.org/2004/02/skos/core#definition> "The association Range shall link the OM_Observation to the value generated by the procedure. The value has the role result with respect to the observation. The type of the result is shown as “Any”, since it may represent the value of any feature property.\r\n\r\nNOTE 1 OGC SWE Common [20] provides a model suitable for describing many kinds of observation results.\r\n\r\nThe type of the observation result shall be consistent with the observed property, and the scale or scope for the value shall be consistent with the quantity or category type. If the observed property (7.2.2.8) is a spatial operation or function, the type of the result may be a coverage.\r\n\r\nNOTE 2 In some contexts, particularly in earth and environmental sciences, the term “observation” is used to refer to the result itself." .
<http://def.seegrid.csiro.au/ontology/om/om-lite#procedure> <http://www.w3.org/2000/01/rdf-schema#isDefinedBy> <http://def.seegrid.csiro.au/ontology/om/om-lite> .
_:Ba451582dX2D7bccX2D46f6X2D8deeX2D94293f70b8d1 <http://www.w3.org/1999/02/22-rdf-syntax-ns#rest> <http://www.w3.org/1999/02/22-rdf-syntax-ns#nil> .
_:B67ceae38X2Dea94X2D42ccX2D8f0dX2Dad5ab43c4b15 <http://www.w3.org/1999/02/22-rdf-syntax-ns#rest> _:B78d4842cX2Dc91fX2D4492X2D9f07X2D2fae7b8a3cca .
<http://def.seegrid.csiro.au/ontology/om/om-lite#samplingStrategy> <http://www.w3.org/1999/02/22-rdf-syntax-ns#type> <http://www.w3.org/2002/07/owl#ObjectProperty> .
<http://def.seegrid.csiro.au/ontology/om/om-lite#ObservationCollection> <http://www.w3.org/2000/01/rdf-schema#label> "Collection of observations"@en .
<http://def.seegrid.csiro.au/ontology/om/om-lite#MeasureObject> <http://www.w3.org/2000/01/rdf-schema#isDefinedBy> <http://def.seegrid.csiro.au/ontology/om/om-lite> .
<http://def.seegrid.csiro.au/ontology/om/om-lite> <http://purl.org/vocab/vann/preferredNamespaceUri> <http://def.seegrid.csiro.au/ontology/om/om-lite#> .
_:B20c87f74f75ee72db9eccc08f342473e <http://www.w3.org/1999/02/22-rdf-syntax-ns#type> <http://www.w3.org/2002/07/owl#Restriction> .
_:B16d39e172dfa5589e895c76d6dbe71ec <http://www.w3.org/2002/07/owl#cardinality> "1"^^<http://www.w3.org/2001/XMLSchema#nonNegativeInteger> .
_:Baf0b21a2701364adf4ee5cf1b319c1d0 <http://www.w3.org/1999/02/22-rdf-syntax-ns#type> <http://www.w3.org/2002/07/owl#Restriction> .
<http://def.seegrid.csiro.au/ontology/om/om-lite#Observation> <http://www.w3.org/2000/01/rdf-schema#subClassOf> _:Bd8d83bd31e604d7e3f203192c3bf5f94 .
<http://def.seegrid.csiro.au/ontology/om/om-lite#Observation> <http://www.w3.org/2002/07/owl#disjointWith> <http://def.seegrid.csiro.au/ontology/om/om-lite#Process> .
<http://def.seegrid.csiro.au/ontology/om/om-lite#resultTime> <http://www.w3.org/2000/01/rdf-schema#isDefinedBy> <http://def.seegrid.csiro.au/ontology/om/om-lite> .
<http://def.seegrid.csiro.au/ontology/om/om-lite#TruthObservation> <http://purl.org/dc/terms/description> "Observation whose result is either true or false" .
_:Bf661192888012e89bb717bb6c3a0e1f9 <http://www.w3.org/2002/07/owl#onProperty> <http://def.seegrid.csiro.au/ontology/om/om-lite#procedure> .
<http://def.seegrid.csiro.au/ontology/om/om-lite#TruthObservation> <http://www.w3.org/2000/01/rdf-schema#subClassOf> <http://def.seegrid.csiro.au/ontology/om/om-lite#Observation> .
<http://def.seegrid.csiro.au/ontology/om/om-lite#result> <http://www.w3.org/2000/01/rdf-schema#comment> "estimate of the value of the observed property" .
_:Bca63bb81X2D5f78X2D4ea1X2D8db8X2D15169052a651 <http://www.w3.org/1999/02/22-rdf-syntax-ns#first> <http://def.seegrid.csiro.au/ontology/om/om-lite#ObservationCollection> .
<http://def.seegrid.csiro.au/ontology/om/om-lite#CountObservation> <http://www.w3.org/2000/01/rdf-schema#subClassOf> <http://def.seegrid.csiro.au/ontology/om/om-lite#Observation> .
<http://def.seegrid.csiro.au/ontology/om/om-lite#Process> <http://www.w3.org/2000/01/rdf-schema#comment> "Agent, device, sensor, software, protocol, computational method, algorithm or plan responsible for generating an observation result. Input may be a sensor stimulus, or the output from a previous process. An oml:Process is re-usable, and might be involved in many observations.\r\n\r\nThis terminology is consistent with SensorML, which defines Process as the super-class of all sensors and sensor systems. But this usage is different to the use of the term \"Process\" in BCO and OBOE, where it denotes an observation occurrence. " .
_:B257584f566e1431eeab7d36f63c2e67f <http://www.w3.org/1999/02/22-rdf-syntax-ns#type> <http://www.w3.org/2002/07/owl#Class> .
_:Bf661192888012e89bb717bb6c3a0e1f9 <http://www.w3.org/1999/02/22-rdf-syntax-ns#type> <http://www.w3.org/2002/07/owl#Restriction> .
_:Ba451582dX2D7bccX2D46f6X2D8deeX2D94293f70b8d1 <http://www.w3.org/1999/02/22-rdf-syntax-ns#first> <http://def.seegrid.csiro.au/ontology/om/om-lite#ObservationCollection> .
_:Bbdb601234954ca5ad43d51824dc68a82 <http://www.w3.org/2002/07/owl#onProperty> <http://def.seegrid.csiro.au/ontology/om/om-lite#result> .
<http://def.seegrid.csiro.au/ontology/om/om-lite#Measurement> <http://www.w3.org/2000/01/rdf-schema#label> "Mesure"@fr .
<http://def.seegrid.csiro.au/ontology/om/om-lite> <http://www.w3.org/2002/07/owl#priorVersion> <http://def.seegrid.csiro.au/isotc211/iso19156/2011/observation> .
<http://def.seegrid.csiro.au/ontology/om/om-lite#CountObservation> <http://www.w3.org/2000/01/rdf-schema#comment> "Observation whose result is an integer" .
<http://def.seegrid.csiro.au/ontology/om/om-lite#phenomenonTime> <http://www.w3.org/2000/01/rdf-schema#comment> "time at which the estimate of the property that is the result of the observation is associated with the feature of interest" .
<http://def.seegrid.csiro.au/ontology/om/om-lite#TemporalObject> <http://www.w3.org/1999/02/22-rdf-syntax-ns#type> <http://www.w3.org/2002/07/owl#Class> .
_:Ba4ce6720X2D5c83X2D4adcX2D8300X2De9be357e3e8b <http://www.w3.org/1999/02/22-rdf-syntax-ns#first> <http://def.seegrid.csiro.au/ontology/om/om-lite#SimpleMeasure> .
<http://def.seegrid.csiro.au/ontology/om/om-lite#SimpleMeasure> <http://purl.org/dc/terms/description> "Simple implementation of a scaled number as an (amount, unit) pair" .
<http://def.seegrid.csiro.au/ontology/om/om-lite#ObservationContext> <http://www.w3.org/2000/01/rdf-schema#label> "Observation context"@en .
<http://def.seegrid.csiro.au/ontology/om/om-lite#TruthObject> <http://www.w3.org/2000/01/rdf-schema#subClassOf> _:B58f8565765b4edcde463571c9484a8f1 .
_:B696c433aX2Df705X2D4445X2D9dfbX2Df95c3cc181be <http://www.w3.org/1999/02/22-rdf-syntax-ns#rest> _:Baecbfb97X2Dd8b8X2D4c33X2D973bX2D2f53751c121b .
_:B140e8a686820c18417c3e58bedc8a59c <http://www.w3.org/1999/02/22-rdf-syntax-ns#type> <http://www.w3.org/2002/07/owl#Class> .
<http://def.seegrid.csiro.au/ontology/om/om-lite> <http://purl.org/dc/elements/1.1/source> "ISO 19156:2011" .
<http://def.seegrid.csiro.au/ontology/om/om-lite#observedProperty> <http://www.w3.org/2000/01/rdf-schema#comment> "property whose value is the result of the observation\r\n\r\nLink from the Observation to the PropertyType for which the Observation:result provides an estimate of its value. \r\n\r\nThe observed property shall be a phenomenon associated with the feature-of-interest." .
<http://def.seegrid.csiro.au/ontology/om/om-lite#samplingStrategy> <http://www.w3.org/2004/02/skos/core#definition> "Links to a feature intended to sample the real-world object, as described in Clause 9 of ISO 19156:2011. " .
_:B8c1681b3X2Daff1X2D4e96X2Db7e9X2Dcfa925323a50 <http://www.w3.org/1999/02/22-rdf-syntax-ns#first> <http://def.seegrid.csiro.au/ontology/om/om-lite#Observation> .
<http://def.seegrid.csiro.au/ontology/om/om-lite#samplingStrategy> <http://www.w3.org/2000/01/rdf-schema#label> "sampling strategy"@en .
<http://def.seegrid.csiro.au/ontology/om/om-lite#TruthObservation> <http://www.w3.org/2000/01/rdf-schema#subClassOf> _:Bad1fd98827a6852fa0c82d5a66ad41c0 .
<http://def.seegrid.csiro.au/ontology/om/om-lite#resultTime> <http://www.w3.org/2000/01/rdf-schema#range> <http://www.w3.org/2001/XMLSchema#dateTime> .
<http://def.seegrid.csiro.au/ontology/om/om-lite#GeometryObservation> <http://www.w3.org/2000/01/rdf-schema#comment> "Observation whose result is a geometry object, such as a point, curve, surface or solid" .
<http://def.seegrid.csiro.au/ontology/om/om-lite#resultTime> <http://www.w3.org/2000/01/rdf-schema#label> "result time"@en .
<http://def.seegrid.csiro.au/ontology/om/om-lite#ObservationContext> <http://www.w3.org/2000/01/rdf-schema#comment> "Some observations depend on other observations to provide context which is important, sometimes essential, in understanding the result. These dependencies are stronger than mere spatio-temporal coincidences, requiring explicit representation. If present, the association class class ObservationContext (Figure 2) shall link a OM_Observation to another OM_Observation, with the role name relatedObservation for the target. It shall support one attribute.\r\n\r\nEXAMPLES\tSome examples include the conditions associated with experimental replicates (e.g., experimental plots and treatments used), biotic factors (e.g., ecological community), interactions among features (e.g., predator-prey), or other temporary relationships occurring at the time of observation that are are not inherent to the observed features themselves (i.e., they change over time), or the related observation may provide input to a process that generates a new result.\r\nThis association complements the Intention association which describes relationships between a sampling feature and domain features." .
<http://def.seegrid.csiro.au/ontology/om/om-lite#samplingStrategy> <http://www.w3.org/2000/01/rdf-schema#domain> _:B34f7c049bcbe3e1f79174c183e61696b .
<http://def.seegrid.csiro.au/ontology/om/om-lite#context> <http://www.w3.org/2000/01/rdf-schema#range> <http://def.seegrid.csiro.au/ontology/om/om-lite#ObservationContext> .
<http://def.seegrid.csiro.au/ontology/om/om-lite#resultTime> <http://www.w3.org/2004/02/skos/core#definition> "The attribute resultTime:TM_Instant shall describe the time when the result became available, typically when the procedure (7.2.2.10) associated with the observation was completed. For some observations, this is identical to the phenomenonTime. However, there are important cases where they differ.\r\n\r\nEXAMPLE 1 Where a measurement is made on a specimen in a laboratory, the phenomenonTime is the time the specimen was retrieved from its host, while the resultTime is the time the laboratory procedure was applied.\r\n\r\nEXAMPLE 2 The resultTime also supports disambiguation of repeat measurements made of the same property of a feature using the same procedure.\r\n\r\nEXAMPLE 3 Where sensor observation results are post-processed, the resultTime is the post-processing time, while the phenomenonTime is the time of initial interaction with the world.\r\n\r\nEXAMPLE 4 Simulations can estimate the values for phenomena in the future or past. The phenomenonTime is the time that the result applies to, while the resultTime is the time that the simulation was executed." .
<http://def.seegrid.csiro.au/ontology/om/om-lite> <http://www.w3.org/2004/02/skos/core#changeNote> "2016-10-27 Add stimulus-time property" .
<http://def.seegrid.csiro.au/ontology/om/om-lite#GeometryObject> <http://www.w3.org/2000/01/rdf-schema#isDefinedBy> <http://def.seegrid.csiro.au/ontology/om/om-lite> .
_:Bb051caff24401dc682173242bb0fb13d <http://www.w3.org/2002/07/owl#cardinality> "1"^^<http://www.w3.org/2001/XMLSchema#nonNegativeInteger> .
_:B1c17d32cd4610480f3ed1e8b276cb470 <http://www.w3.org/2002/07/owl#unionOf> _:B696c433aX2Df705X2D4445X2D9dfbX2Df95c3cc181be .
<http://def.seegrid.csiro.au/ontology/om/om-lite#Observation> <http://www.w3.org/2004/02/skos/core#changeNote> "A new property oml:samplingStrategy is scoped to this class. In this  formulation, the (mandatory) feature-of-interest always refers to the ultimate feature of interest, whose type can carry the observed property, and the (optional) sampling strategy allows the sampling feature to be made explicit as an additional relationship. This overcomes some semantic sleight-of-hand in ISO 19156, in which the constraint the the observed property was commensurate with the feature-of-interest was allowed to be 'transitive' via the sampledFeature property." .
<http://def.seegrid.csiro.au/ontology/om/om-lite#TemporalObservation> <http://www.w3.org/2000/01/rdf-schema#label> "Temporal Observation"@en .
_:B34f7c049bcbe3e1f79174c183e61696b <http://www.w3.org/2002/07/owl#unionOf> _:Be80c213bX2DbcecX2D4951X2D9e68X2D67704070d8c9 .
<http://def.seegrid.csiro.au/ontology/om/om-lite#SimpleMeasure> <http://www.w3.org/2002/07/owl#equivalentClass> _:B774ffb5a0482acf60193dde3f13477dd .
_:B5b89d6d6X2D84b7X2D4bc4X2D9b42X2D8727feea10f6 <http://www.w3.org/1999/02/22-rdf-syntax-ns#first> <http://def.seegrid.csiro.au/ontology/om/om-lite#ObservationCollection> .
<http://def.seegrid.csiro.au/ontology/om/om-lite#Observation> <http://www.w3.org/2000/01/rdf-schema#subClassOf> _:B812aa08271c375826eee91c12beb1d04 .
<http://def.seegrid.csiro.au/ontology/om/om-lite#ObservationCollection> <http://www.w3.org/2000/01/rdf-schema#comment> "A collection of observations  or collections. \r\n\r\nThe collection may be homogeneous in any of the feature-of-interest, observed-property, procedure, phenomenon-time or result-time. If only one value for any of these properties is provided on the collection, then it may be inferred to be a common (default) value for all the member observations or collections, unless locally overridden." .
<http://def.seegrid.csiro.au/ontology/om/om-lite#GeometryObservation> <http://www.w3.org/2000/01/rdf-schema#isDefinedBy> <http://def.seegrid.csiro.au/ontology/om/om-lite> .
_:B139b0cc72866386a3920a0445613f33f <http://www.w3.org/1999/02/22-rdf-syntax-ns#type> <http://www.w3.org/2002/07/owl#Class> .
<http://def.seegrid.csiro.au/ontology/om/om-lite#ObservationContext> <http://www.w3.org/2000/01/rdf-schema#subClassOf> _:Baf0b21a2701364adf4ee5cf1b319c1d0 .
<http://def.seegrid.csiro.au/ontology/om/om-lite#procedure> <http://www.w3.org/2000/01/rdf-schema#domain> _:B139b0cc72866386a3920a0445613f33f .
<http://def.seegrid.csiro.au/ontology/om/om-lite#relatedObservation> <http://www.w3.org/2000/01/rdf-schema#range> <http://def.seegrid.csiro.au/ontology/om/om-lite#Observation> .
_:B8b9125beX2Dba46X2D4196X2Dab0cX2D22764eba82d3 <http://www.w3.org/1999/02/22-rdf-syntax-ns#rest> <http://www.w3.org/1999/02/22-rdf-syntax-ns#nil> .
<http://def.seegrid.csiro.au/ontology/om/om-lite#TemporalObservation> <http://purl.org/dc/terms/description> "Observation whose result is a temporal object, such as a time instant or period" .
<http://def.seegrid.csiro.au/ontology/om/om-lite> <http://www.w3.org/2000/01/rdf-schema#label> "OWL for Observations" .
_:Bb8769301438bcead254f75e9f6f527ff <http://www.w3.org/1999/02/22-rdf-syntax-ns#type> <http://www.w3.org/2002/07/owl#Restriction> .
_:B0f39e608X2D6e7aX2D41a3X2Db722X2D9505b7d87375 <http://www.w3.org/1999/02/22-rdf-syntax-ns#rest> <http://www.w3.org/1999/02/22-rdf-syntax-ns#nil> .
<http://def.seegrid.csiro.au/ontology/om/om-lite#observedProperty> <http://www.w3.org/2000/01/rdf-schema#domain> _:B2ac96b2632b3d2951fe666fa7cbb8421 .
<http://def.seegrid.csiro.au/ontology/om/om-lite#SimpleMeasure> <http://www.w3.org/2000/01/rdf-schema#isDefinedBy> <http://def.seegrid.csiro.au/ontology/om/om-lite> .
_:B2882679eX2D556cX2D4616X2D9107X2D1a35bb0db0ba <http://www.w3.org/1999/02/22-rdf-syntax-ns#first> <http://def.seegrid.csiro.au/ontology/om/om-lite#ObservationCollection> .
_:Bad1fd98827a6852fa0c82d5a66ad41c0 <http://www.w3.org/2002/07/owl#allValuesFrom> <http://def.seegrid.csiro.au/ontology/om/om-lite#TruthObject> .
_:B6085a7cf84f730f2eb96448f8674cc83 <http://www.w3.org/1999/02/22-rdf-syntax-ns#type> <http://www.w3.org/2002/07/owl#Restriction> .
<http://def.seegrid.csiro.au/ontology/om/om-lite#uom> <http://www.w3.org/2000/01/rdf-schema#comment> "Unit of measure or scale" .
_:B6085a7cf84f730f2eb96448f8674cc83 <http://www.w3.org/2002/07/owl#onProperty> <http://def.seegrid.csiro.au/ontology/om/om-lite#phenomenonTime> .
<http://def.seegrid.csiro.au/ontology/om/om-lite#ObservationContext> <http://www.w3.org/1999/02/22-rdf-syntax-ns#type> <http://www.w3.org/2002/07/owl#Class> .
<http://def.seegrid.csiro.au/ontology/om/om-lite#Observation> <http://www.w3.org/1999/02/22-rdf-syntax-ns#type> <http://www.w3.org/2002/07/owl#Class> .
_:Bd8d83bd31e604d7e3f203192c3bf5f94 <http://www.w3.org/2002/07/owl#cardinality> "1"^^<http://www.w3.org/2001/XMLSchema#nonNegativeInteger> .
<http://def.seegrid.csiro.au/ontology/om/om-lite#Process> <http://www.w3.org/2004/02/skos/core#historyNote> "Original description from ISO 19156 says: \r\n\r\nThe class OM_Process (Figure 2) is an instance of the «metaclass» GF_FeatureType (ISO 19109:2005), which therefore represents a feature type. OM_Process is abstract, and has no attributes, operations or associations. It serves as the base class for observation processes. The purpose of an observation process is to generate an observation result. An instance of OM_Process is often an instrument or sensor, but may be a human observer, a simulator, or a process or algorithm applied to more primitive results used as inputs. \r\n\r\nNOTE\tISO 19115-2:2008 provides MI_Instrument, LE_Processing and LE_Algorithm, which could all be modelled as specializations of OM_Process. OGC SensorML [10] provides a model which is suitable for many observation procedures." .
<http://def.seegrid.csiro.au/ontology/om/om-lite#CountObject> <http://www.w3.org/2000/01/rdf-schema#label> "Count object" .
<http://def.seegrid.csiro.au/ontology/om/om-lite#TemporalObservation> <http://www.w3.org/2000/01/rdf-schema#subClassOf> _:Bbdb601234954ca5ad43d51824dc68a82 .
<http://def.seegrid.csiro.au/ontology/om/om-lite#phenomenonTime> <http://www.w3.org/1999/02/22-rdf-syntax-ns#type> <http://www.w3.org/2002/07/owl#ObjectProperty> .
<http://def.seegrid.csiro.au/ontology/om/om-lite> <http://purl.org/dc/elements/1.1/description> "An OWL representation of the Observation Schema described in clauses 7-8 of ISO 19156:2011 Geographic Information - Observations and Measurements / OGC Abstract Specification - Topic 20." .
<http://def.seegrid.csiro.au/ontology/om/om-lite#phenomenonTime> <http://www.w3.org/2000/01/rdf-schema#isDefinedBy> <http://def.seegrid.csiro.au/ontology/om/om-lite> .
<http://def.seegrid.csiro.au/ontology/om/om-lite#procedure> <http://www.w3.org/2000/01/rdf-schema#range> <http://def.seegrid.csiro.au/ontology/om/om-lite#Process> .
<http://def.seegrid.csiro.au/ontology/om/om-lite#GeometryObject> <http://purl.org/dc/terms/description> "Geometry object has properties relating to geometry, incuding positional and topological attributes, reference system, accuracy and precision. Might be geolocated. " .
<http://def.seegrid.csiro.au/ontology/om/om-lite#context> <http://www.w3.org/1999/02/22-rdf-syntax-ns#type> <http://www.w3.org/2002/07/owl#ObjectProperty> .
_:B2882679eX2D556cX2D4616X2D9107X2D1a35bb0db0ba <http://www.w3.org/1999/02/22-rdf-syntax-ns#rest> <http://www.w3.org/1999/02/22-rdf-syntax-ns#nil> .
<http://def.seegrid.csiro.au/ontology/om/om-lite#stimulusTime> <http://www.w3.org/2000/01/rdf-schema#domain> _:Bf223756303d98c258aa73b4c1c1650ad .
<http://def.seegrid.csiro.au/ontology/om/om-lite#TemporalObject> <http://www.w3.org/2000/01/rdf-schema#label> "Temporal object" .
<http://def.seegrid.csiro.au/ontology/om/om-lite#TruthObject> <http://www.w3.org/2000/01/rdf-schema#label> "Truth object" .
<http://def.seegrid.csiro.au/ontology/om/om-lite#context> <http://www.w3.org/2000/01/rdf-schema#comment> "link to related observation\r\n\r\nThe first half of the property named 'relatedObservation' in the UML model. (The rule for implementing association classes needs clarification.)" .
<http://def.seegrid.csiro.au/ontology/om/om-lite#GeometryObject> <http://www.w3.org/2000/01/rdf-schema#comment> "This stub is included in the om: ontology to support references to geometry as the result of a GeometryObservation.  An existing OWL class that represents the notion of a geometry may be asserted to be a sub-class of this stub, without requiring use of a specific representation of Geometry in the context of observations instance." .
_:Bcaa52b8ca80d3545838555278ed1f713 <http://www.w3.org/2002/07/owl#cardinality> "1"^^<http://www.w3.org/2001/XMLSchema#nonNegativeInteger> .
_:B0b84d8caX2Da2f9X2D4bb7X2D9039X2Dba58989551fb <http://www.w3.org/1999/02/22-rdf-syntax-ns#rest> _:B5b89d6d6X2D84b7X2D4bc4X2D9b42X2D8727feea10f6 .
_:Be80c213bX2DbcecX2D4951X2D9e68X2D67704070d8c9 <http://www.w3.org/1999/02/22-rdf-syntax-ns#rest> _:Bca63bb81X2D5f78X2D4ea1X2D8db8X2D15169052a651 .
_:B8c1681b3X2Daff1X2D4e96X2Db7e9X2Dcfa925323a50 <http://www.w3.org/1999/02/22-rdf-syntax-ns#rest> _:Ba451582dX2D7bccX2D46f6X2D8deeX2D94293f70b8d1 .
<http://def.seegrid.csiro.au/ontology/om/om-lite#context> <http://www.w3.org/2000/01/rdf-schema#isDefinedBy> <http://def.seegrid.csiro.au/ontology/om/om-lite> .
<http://def.seegrid.csiro.au/ontology/om/om-lite#result> <http://www.w3.org/2000/01/rdf-schema#domain> <http://def.seegrid.csiro.au/ontology/om/om-lite#Observation> .
_:B535c16bb4a3db7a00d957fb3a8ebe55e <http://www.w3.org/2002/07/owl#allValuesFrom> <http://def.seegrid.csiro.au/ontology/om/om-lite#GeometryObject> .
<http://def.seegrid.csiro.au/ontology/om/om-lite#observedProperty> <http://www.w3.org/1999/02/22-rdf-syntax-ns#type> <http://www.w3.org/2002/07/owl#FunctionalProperty> .
<http://def.seegrid.csiro.au/ontology/om/om-lite#featureOfInterest> <http://www.w3.org/1999/02/22-rdf-syntax-ns#type> <http://www.w3.org/2002/07/owl#ObjectProperty> .
<http://def.seegrid.csiro.au/ontology/om/om-lite#relatedObservation> <http://www.w3.org/2000/01/rdf-schema#isDefinedBy> <http://def.seegrid.csiro.au/ontology/om/om-lite> .
<http://def.seegrid.csiro.au/ontology/om/om-lite#GeometryObservation> <http://www.w3.org/2000/01/rdf-schema#subClassOf> <http://def.seegrid.csiro.au/ontology/om/om-lite#Observation> .
<http://def.seegrid.csiro.au/ontology/om/om-lite#CountObject> <http://www.w3.org/2000/01/rdf-schema#isDefinedBy> <http://def.seegrid.csiro.au/ontology/om/om-lite> .
_:B2ac96b2632b3d2951fe666fa7cbb8421 <http://www.w3.org/2002/07/owl#unionOf> _:B86fa036dX2Dc15aX2D45deX2Dae14X2D9ee642eecc9d .
_:B6c38d313X2D552dX2D4271X2D9666X2Dd9debc6d6d28 <http://www.w3.org/1999/02/22-rdf-syntax-ns#first> <http://def.seegrid.csiro.au/ontology/om/om-lite#Observation> .
<http://def.seegrid.csiro.au/ontology/om/om-lite#memberOf> <http://www.w3.org/2000/01/rdf-schema#isDefinedBy> <http://def.seegrid.csiro.au/ontology/om/om-lite> .
<http://def.seegrid.csiro.au/ontology/om/om-lite#stimulusTime> <http://www.w3.org/2000/01/rdf-schema#isDefinedBy> <http://def.seegrid.csiro.au/ontology/om/om-lite> .
<http://def.seegrid.csiro.au/ontology/om/om-lite#ObservationCollection> <http://purl.org/dc/terms/description> "A collection of observations  or collections. \r\n\r\nThe collection may be homogeneous any of the feature-of-interest, observed-property, procedure, phenomenon-time or result-time. If only one value for any of these properties is provided on the collection, then it may be inferred to be a common (default) value for all the member observations or collections, unless locally overridden." .
_:B812aa08271c375826eee91c12beb1d04 <http://www.w3.org/2002/07/owl#cardinality> "1"^^<http://www.w3.org/2001/XMLSchema#nonNegativeInteger> .
_:B58f8565765b4edcde463571c9484a8f1 <http://www.w3.org/2002/07/owl#onProperty> <http://def.seegrid.csiro.au/ontology/om/om-lite#truth> .
<http://def.seegrid.csiro.au/ontology/om/om-lite#Measurement> <http://www.w3.org/1999/02/22-rdf-syntax-ns#type> <http://www.w3.org/2002/07/owl#Class> .
<http://def.seegrid.csiro.au/ontology/om/om-lite#featureOfInterest> <http://www.w3.org/2000/01/rdf-schema#isDefinedBy> <http://def.seegrid.csiro.au/ontology/om/om-lite> .
<http://def.seegrid.csiro.au/ontology/om/om-lite#relatedObservation> <http://www.w3.org/1999/02/22-rdf-syntax-ns#type> <http://www.w3.org/2002/07/owl#ObjectProperty> .
<http://def.seegrid.csiro.au/ontology/om/om-lite#stimulusTime> <http://www.w3.org/1999/02/22-rdf-syntax-ns#type> <http://www.w3.org/2002/07/owl#ObjectProperty> .
<http://def.seegrid.csiro.au/ontology/om/om-lite#Process> <http://www.w3.org/1999/02/22-rdf-syntax-ns#type> <http://www.w3.org/2002/07/owl#Class> .
_:B1dde258848a73b3d73221fbc5cb2b4d8 <http://www.w3.org/2002/07/owl#unionOf> _:B3497aa63X2D3ab7X2D4000X2D8dcfX2D488a9324d29a .
<http://def.seegrid.csiro.au/ontology/om/om-lite#memberOf> <http://www.w3.org/1999/02/22-rdf-syntax-ns#type> <http://www.w3.org/2002/07/owl#ObjectProperty> .
_:B535c16bb4a3db7a00d957fb3a8ebe55e <http://www.w3.org/2002/07/owl#onProperty> <http://def.seegrid.csiro.au/ontology/om/om-lite#result> .
<http://def.seegrid.csiro.au/ontology/om/om-lite#MeasureObject> <http://purl.org/dc/terms/description> "Scaled number" .
_:Bad1fd98827a6852fa0c82d5a66ad41c0 <http://www.w3.org/1999/02/22-rdf-syntax-ns#type> <http://www.w3.org/2002/07/owl#Restriction> .
<http://def.seegrid.csiro.au/ontology/om/om-lite#result> <http://www.w3.org/1999/02/22-rdf-syntax-ns#type> <http://www.w3.org/2002/07/owl#FunctionalProperty> .
<http://def.seegrid.csiro.au/ontology/om/om-lite#Observation> <http://www.w3.org/2000/01/rdf-schema#subClassOf> _:Bf661192888012e89bb717bb6c3a0e1f9 .
_:B7d8b0bfb132111b24c7007ce268c601d <http://www.w3.org/1999/02/22-rdf-syntax-ns#type> <http://www.w3.org/2002/07/owl#Class> .
_:B20c87f74f75ee72db9eccc08f342473e <http://www.w3.org/2002/07/owl#allValuesFrom> <http://def.seegrid.csiro.au/ontology/om/om-lite#CountObject> .
<http://def.seegrid.csiro.au/ontology/om/om-lite#relatedObservation> <http://www.w3.org/2000/01/rdf-schema#label> "related observation"@en .
<http://def.seegrid.csiro.au/ontology/om/om-lite> <http://www.w3.org/2004/02/skos/core#changeNote> "2015-08-18 Added ObservationCollection class; added to domain of key Observation properties (except oml:result) to support inheritance of common properties from a container. " .
<http://def.seegrid.csiro.au/ontology/om/om-lite#Observation> <http://www.w3.org/2000/01/rdf-schema#subClassOf> _:B16d39e172dfa5589e895c76d6dbe71ec .
<http://def.seegrid.csiro.au/ontology/om/om-lite#Process> <http://purl.org/dc/terms/description> "Agent, device, sensor, software, protocol, computational method, algorithm or plan responsible for generating an observation result. Input may be a sensor stimulus, or the output from a previous process. An oml:Process might be involved in many observations. " .
_:B5231bb242b1062681893c57a25b8b174 <http://www.w3.org/1999/02/22-rdf-syntax-ns#type> <http://www.w3.org/2002/07/owl#Class> .
<http://def.seegrid.csiro.au/ontology/om/om-lite#Measurement> <http://purl.org/dc/terms/description> "Observation whose result is a scaled number" .
<http://def.seegrid.csiro.au/ontology/om/om-lite#Process> <http://www.w3.org/2002/07/owl#disjointWith> <http://def.seegrid.csiro.au/ontology/om/om-lite#Observation> .
_:B44f4de9d822ec3fde44a89c25a4c4a8f <http://www.w3.org/1999/02/22-rdf-syntax-ns#type> <http://www.w3.org/2002/07/owl#Restriction> .
<http://def.seegrid.csiro.au/ontology/om/om-lite#featureOfInterest> <http://www.w3.org/2000/01/rdf-schema#domain> _:B140e8a686820c18417c3e58bedc8a59c .
_:B5b89d6d6X2D84b7X2D4bc4X2D9b42X2D8727feea10f6 <http://www.w3.org/1999/02/22-rdf-syntax-ns#rest> <http://www.w3.org/1999/02/22-rdf-syntax-ns#nil> .
_:B58f8565765b4edcde463571c9484a8f1 <http://www.w3.org/2002/07/owl#cardinality> "1"^^<http://www.w3.org/2001/XMLSchema#nonNegativeInteger> .
_:Baf0b21a2701364adf4ee5cf1b319c1d0 <http://www.w3.org/2002/07/owl#onProperty> <http://def.seegrid.csiro.au/ontology/om/om-lite#relatedObservation> .
<http://def.seegrid.csiro.au/ontology/om/om-lite#count> <http://www.w3.org/2000/01/rdf-schema#label> "Count value" .
_:B0f39e608X2D6e7aX2D41a3X2Db722X2D9505b7d87375 <http://www.w3.org/1999/02/22-rdf-syntax-ns#first> <http://def.seegrid.csiro.au/ontology/om/om-lite#ObservationCollection> .
<http://def.seegrid.csiro.au/ontology/om/om-lite#member> <http://www.w3.org/2000/01/rdf-schema#domain> <http://def.seegrid.csiro.au/ontology/om/om-lite#ObservationCollection> .
_:B8b9125beX2Dba46X2D4196X2Dab0cX2D22764eba82d3 <http://www.w3.org/1999/02/22-rdf-syntax-ns#first> <http://def.seegrid.csiro.au/ontology/om/om-lite#ObservationCollection> .
<http://def.seegrid.csiro.au/ontology/om/om-lite#TruthObservation> <http://www.w3.org/2000/01/rdf-schema#comment> "Observation whose result is either true or false" .
<http://def.seegrid.csiro.au/ontology/om/om-lite#Measurement> <http://www.w3.org/2000/01/rdf-schema#isDefinedBy> <http://def.seegrid.csiro.au/ontology/om/om-lite> .
_:B774ffb5a0482acf60193dde3f13477dd <http://www.w3.org/2002/07/owl#onProperty> <http://def.seegrid.csiro.au/ontology/om/om-lite#amount> .
_:B696c433aX2Df705X2D4445X2D9dfbX2Df95c3cc181be <http://www.w3.org/1999/02/22-rdf-syntax-ns#first> <http://def.seegrid.csiro.au/ontology/om/om-lite#Observation> .
<http://def.seegrid.csiro.au/ontology/om/om-lite> <http://www.w3.org/2002/07/owl#imports> <http://purl.org/dc/elements/1.1/> .
_:B7d8b0bfb132111b24c7007ce268c601d <http://www.w3.org/2002/07/owl#unionOf> _:B67ceae38X2Dea94X2D42ccX2D8f0dX2Dad5ab43c4b15 .
<http://def.seegrid.csiro.au/ontology/om/om-lite#Process> <http://www.w3.org/2000/01/rdf-schema#isDefinedBy> <http://def.seegrid.csiro.au/ontology/om/om-lite> .
<http://def.seegrid.csiro.au/ontology/om/om-lite#CountObject> <http://www.w3.org/1999/02/22-rdf-syntax-ns#type> <http://www.w3.org/2002/07/owl#Class> .
_:B44f4de9d822ec3fde44a89c25a4c4a8f <http://www.w3.org/2002/07/owl#onProperty> <http://def.seegrid.csiro.au/ontology/om/om-lite#result> .
_:Bd8d83bd31e604d7e3f203192c3bf5f94 <http://www.w3.org/2002/07/owl#onProperty> <http://def.seegrid.csiro.au/ontology/om/om-lite#stimulusTime> .
_:Bcaa52b8ca80d3545838555278ed1f713 <http://www.w3.org/2002/07/owl#onProperty> <http://def.seegrid.csiro.au/ontology/om/om-lite#count> .
_:B774ffb5a0482acf60193dde3f13477dd <http://www.w3.org/1999/02/22-rdf-syntax-ns#type> <http://www.w3.org/2002/07/owl#Restriction> .
_:B535c16bb4a3db7a00d957fb3a8ebe55e <http://www.w3.org/1999/02/22-rdf-syntax-ns#type> <http://www.w3.org/2002/07/owl#Restriction> .
_:Bad1fd98827a6852fa0c82d5a66ad41c0 <http://www.w3.org/2002/07/owl#onProperty> <http://def.seegrid.csiro.au/ontology/om/om-lite#result> .
<http://def.seegrid.csiro.au/ontology/om/om-lite#Process> <http://www.w3.org/2004/02/skos/core#historyNote> "Original description from OGC SensorML says:\r\n\r\nIn SensorML, all components are modeled as processes. This includes components normally viewed as hardware, including transducers, actuators, and processors (which are viewed as process components) and sensors and platforms (which are modeled as systems). All components are modeled as processes that take input, and which through the application of an algorithm defined by a method and parameter values, generate output. All such components can therefore participate in process chains. Process chains are themselves processes with inputs, outputs, and parameters.\r\n\r\nHence, SensorML can be viewed as a specialized process description language with an emphasis on application to sensor data. Process descriptions in SensorML are agnostic of the development environment in which they might be executed, or the protocol by which data is transported between process execution modules. SensorML does not try to replace other existing technologies (such as BPEL or MATLAB Simulink). It is also conceived that SensorML-defined processes could be imported and executed within other execution environments, such as BPEL or MATLAB Simulink, as well as within SenosrML-enabled process execution software." .
_:Bb051caff24401dc682173242bb0fb13d <http://www.w3.org/2002/07/owl#onProperty> <http://def.seegrid.csiro.au/ontology/om/om-lite#uom> .
<http://def.seegrid.csiro.au/ontology/om/om-lite#SimpleMeasure> <http://www.w3.org/2000/01/rdf-schema#comment> "Simple implementation of a scaled number as an (amount, unit) pair" .
<http://def.seegrid.csiro.au/ontology/om/om-lite#CountObservation> <http://purl.org/dc/terms/description> "Observation whose result is an integer" .
_:B8a6f28921cceab0d9746aba4ee3cdcb7 <http://www.w3.org/1999/02/22-rdf-syntax-ns#type> <http://www.w3.org/2002/07/owl#Restriction> .
<http://def.seegrid.csiro.au/ontology/om/om-lite#CountObservation> <http://www.w3.org/2000/01/rdf-schema#label> "Count Observation"@en .
<http://def.seegrid.csiro.au/ontology/om/om-lite#MeasureObject> <http://www.w3.org/2000/01/rdf-schema#comment> "Scaled number\r\n\r\nThis is an abstract class, which should be substituted by a suitable concrete representation of a measure or quantity at run-tme. \r\n\r\noml:SimpleMeasure \r\nqudt:QuantityValue <http://qudt.org/schema/qudt#QuantityValue> \r\nDUL:Region <http://www.loa-cnr.it/ontologies/DUL.owl#Region> \r\n\r\nare candidates. " .
<http://def.seegrid.csiro.au/ontology/om/om-lite#amount> <http://www.w3.org/2000/01/rdf-schema#domain> <http://def.seegrid.csiro.au/ontology/om/om-lite#SimpleMeasure> .
<http://def.seegrid.csiro.au/ontology/om/om-lite#Measurement> <http://www.w3.org/2000/01/rdf-schema#subClassOf> _:B44f4de9d822ec3fde44a89c25a4c4a8f .
<http://def.seegrid.csiro.au/ontology/om/om-lite#procedure> <http://www.w3.org/2004/02/skos/core#definition> "The association ProcessUsed shall link the OM_Observation to the OM_Process (7.2.3) used to generate the result. The process has the role procedure with respect to the observation. A process might be responsible for more than one generatedObservation.\r\n\r\nThe OM_Process shall be suitable for the observed property. As a corollary, details of the observed property are constrained by the procedure used.\r\n\r\nEXAMPLE Observed radiance wavelength is determined by the response characteristics of the sensor.\r\n\r\nA description of the observation procedure provides or implies an indication of the reliability or quality of the observation result." .
<http://def.seegrid.csiro.au/ontology/om/om-lite#ObservationCollection> <http://www.w3.org/2000/01/rdf-schema#subClassOf> _:B50eaf67a7bf22d8e8921561ecf98739d .
<http://def.seegrid.csiro.au/ontology/om/om-lite#Process> <http://www.w3.org/2000/01/rdf-schema#label> "Observation process"@en .
<http://def.seegrid.csiro.au/ontology/om/om-lite#resultTime> <http://www.w3.org/1999/02/22-rdf-syntax-ns#type> <http://www.w3.org/2002/07/owl#FunctionalProperty> .
<http://def.seegrid.csiro.au/ontology/om/om-lite#GeometryObservation> <http://purl.org/dc/terms/description> "Observation whose result is a geometry object, such as a point, curve, surface or solid" .
<http://def.seegrid.csiro.au/ontology/om/om-lite#context> <http://www.w3.org/2000/01/rdf-schema#label> "observation context"@en .
<http://def.seegrid.csiro.au/ontology/om/om-lite#amount> <http://www.w3.org/2000/01/rdf-schema#range> <http://www.w3.org/2001/XMLSchema#double> .
_:B86fa036dX2Dc15aX2D45deX2Dae14X2D9ee642eecc9d <http://www.w3.org/1999/02/22-rdf-syntax-ns#rest> _:B888d011eX2Db4d6X2D4cdbX2D8fc1X2D1a97526f65eb .
<http://def.seegrid.csiro.au/ontology/om/om-lite#SimpleMeasure> <http://www.w3.org/2000/01/rdf-schema#subClassOf> <http://def.seegrid.csiro.au/ontology/om/om-lite#MeasureObject> .
_:B2ac96b2632b3d2951fe666fa7cbb8421 <http://www.w3.org/1999/02/22-rdf-syntax-ns#type> <http://www.w3.org/2002/07/owl#Class> .
<http://def.seegrid.csiro.au/ontology/om/om-lite#amount> <http://www.w3.org/2000/01/rdf-schema#isDefinedBy> <http://def.seegrid.csiro.au/ontology/om/om-lite> .
<http://def.seegrid.csiro.au/ontology/om/om-lite#Observation> <http://www.w3.org/2004/02/skos/core#prefLabel> "Observation"@fr .
<http://def.seegrid.csiro.au/ontology/om/om-lite#Measurement> <http://www.w3.org/2000/01/rdf-schema#subClassOf> <http://def.seegrid.csiro.au/ontology/om/om-lite#Observation> .
_:Bf661192888012e89bb717bb6c3a0e1f9 <http://www.w3.org/2002/07/owl#cardinality> "1"^^<http://www.w3.org/2001/XMLSchema#nonNegativeInteger> .
<http://def.seegrid.csiro.au/ontology/om/om-lite#member> <http://www.w3.org/2000/01/rdf-schema#range> _:B7d8b0bfb132111b24c7007ce268c601d .
<http://def.seegrid.csiro.au/ontology/om/om-lite#TemporalObject> <http://www.w3.org/2000/01/rdf-schema#comment> "Temporal geometry or topology, collection or complex. \r\n\r\nTemporal object has properties relating to time only." .
<http://def.seegrid.csiro.au/ontology/om/om-lite#GeometryObservation> <http://www.w3.org/1999/02/22-rdf-syntax-ns#type> <http://www.w3.org/2002/07/owl#Class> .
<http://def.seegrid.csiro.au/ontology/om/om-lite#CountObject> <http://www.w3.org/2000/01/rdf-schema#comment> "Object to wrap a count value" .
<http://def.seegrid.csiro.au/ontology/om/om-lite#GeometryObservation> <http://www.w3.org/2000/01/rdf-schema#label> "Geometry Observation"@en .
<http://def.seegrid.csiro.au/ontology/om/om-lite#role> <http://www.w3.org/2000/01/rdf-schema#label> "role"@en .
<http://def.seegrid.csiro.au/ontology/om/om-lite#GeometryObject> <http://www.w3.org/1999/02/22-rdf-syntax-ns#type> <http://www.w3.org/2002/07/owl#Class> .
_:B0b84d8caX2Da2f9X2D4bb7X2D9039X2Dba58989551fb <http://www.w3.org/1999/02/22-rdf-syntax-ns#first> <http://def.seegrid.csiro.au/ontology/om/om-lite#Observation> .
<http://def.seegrid.csiro.au/ontology/om/om-lite#MeasureObject> <http://www.w3.org/2000/01/rdf-schema#label> "Measure" .
_:B16d39e172dfa5589e895c76d6dbe71ec <http://www.w3.org/1999/02/22-rdf-syntax-ns#type> <http://www.w3.org/2002/07/owl#Restriction> .
_:Baf0b21a2701364adf4ee5cf1b319c1d0 <http://www.w3.org/2002/07/owl#cardinality> "1"^^<http://www.w3.org/2001/XMLSchema#nonNegativeInteger> .
<http://def.seegrid.csiro.au/ontology/om/om-lite#featureOfInterest> <http://www.w3.org/2000/01/rdf-schema#comment> "feature of interest of an observation\r\n\r\nLinks the Observation to the Feature that is the ultimate subject of the observation and carries the observed property. This feature is the real-world object whose properties are under observation. An observation instance serves as a propertyValueProvider for its feature-of-interest." .
<http://def.seegrid.csiro.au/ontology/om/om-lite#role> <http://www.w3.org/2000/01/rdf-schema#isDefinedBy> <http://def.seegrid.csiro.au/ontology/om/om-lite> .
<http://def.seegrid.csiro.au/ontology/om/om-lite> <http://www.w3.org/1999/02/22-rdf-syntax-ns#type> <http://www.w3.org/2002/07/owl#Ontology> .
<http://def.seegrid.csiro.au/ontology/om/om-lite#observedProperty> <http://www.w3.org/2004/02/skos/core#definition> "property whose value is the result of the observation\r\n\r\nLink from the Observation to the PropertyType for which the Observation:result provides an estimate of its value. \r\n\r\nThe observed property shall be a phenomenon associated with the feature-of-interest.\r\n\r\nThe target of this shall describe a property that is either assignable or observable such as “temperature”, “height”, “colour”, “material”. A property type may be an operation or function such as a spatiotemporal coverage. Property-type definitions may be organized into a hierarchy or ontology and managed in a register and catalogued to support discovery functions. The observed property supports semantic or thematic classification of observations, which is useful for discovery and data fusion.\r\n\r\nNOTE In general, the value of a specific observedProperty can be associated with different feature types in different observations, thus allowing the results of observations made in different projects or campaigns, and even from different disciplines, to be combined when required. A property-type register used in observations is most useful if each property type is not tied to a single feature type, or if equivalence relationships between similar property types from different feature types are provided." .
_:Bb8769301438bcead254f75e9f6f527ff <http://www.w3.org/2002/07/owl#onProperty> <http://def.seegrid.csiro.au/ontology/om/om-lite#result> .
<http://def.seegrid.csiro.au/ontology/om/om-lite#role> <http://www.w3.org/1999/02/22-rdf-syntax-ns#type> <http://www.w3.org/2002/07/owl#ObjectProperty> .
<http://def.seegrid.csiro.au/ontology/om/om-lite> <http://purl.org/vocab/vann/preferredNamespacePrefix> "oml:" .
<http://def.seegrid.csiro.au/ontology/om/om-lite#relatedObservation> <http://www.w3.org/2000/01/rdf-schema#comment> "related observation" .
<http://def.seegrid.csiro.au/ontology/om/om-lite#Observation> <http://www.w3.org/2000/01/rdf-schema#label> "Observation"@en .
<http://def.seegrid.csiro.au/ontology/om/om-lite#stimulusTime> <http://www.w3.org/2004/02/skos/core#definition> "the time when the sensor stimulus occurred. Usually the beginning of the observation activity, with the result time being the end. May be the same as the phenomenon-time (e.g. most monitoring applications). May define the time of observations used to condition simulations and forecasting. \r\n\r\nThe relative positions of stimulus-time, phenomenon-time, result-time define whether the observation is monitoring, forecasting, or retrospective, as follows:\r\n* st = pt <= rt    is monitoring\r\n* st < rt < pt   is forecast\r\n* pt < st <=rt   is retrospective (e.g. geology, archeology) " .
<http://def.seegrid.csiro.au/ontology/om/om-lite#Observation> <http://purl.org/dc/terms/description> "An observation is an act associated with a discrete time instant or period through which a number, term or other symbol is assigned to a phenomenon [2]. It involves application of a specified procedure, such as a sensor, instrument, algorithm or process chain. The procedure may be applied in-situ, remotely, or ex-situ with respect to the sampling location. The result of an observation is an estimate of the value of a property of some feature. Use of a common model allows observation data using different procedures to be combined unambiguously.\r\n\r\nThe observation itself is also a feature, since it has properties and identity.\r\n\r\nObservation details are important for data discovery and for data quality estimation.\r\n\r\nThe observation could be considered to carry metadata about an instance of a property (of the feature of interest). This property-value metadata complements the dataset and feature metadata that have been conventionally considered (e.g. ISO 19115). " .
<http://def.seegrid.csiro.au/ontology/om/om-lite#stimulusTime> <http://www.w3.org/2004/02/skos/core#historyNote> "This property was introduced after discussions in the jint W3C/OGC Spatial Data on the Web Working Group in October 2016" .
<http://def.seegrid.csiro.au/ontology/om/om-lite#ObservationContext> <http://www.w3.org/2000/01/rdf-schema#isDefinedBy> <http://def.seegrid.csiro.au/ontology/om/om-lite> .
<http://def.seegrid.csiro.au/ontology/om/om-lite#Observation> <http://www.w3.org/2000/01/rdf-schema#isDefinedBy> <http://def.seegrid.csiro.au/ontology/om/om-lite> .
<http://def.seegrid.csiro.au/ontology/om/om-lite#amount> <http://www.w3.org/1999/02/22-rdf-syntax-ns#type> <http://www.w3.org/2002/07/owl#DatatypeProperty> .
<http://def.seegrid.csiro.au/ontology/om/om-lite#SimpleMeasure> <http://www.w3.org/1999/02/22-rdf-syntax-ns#type> <http://www.w3.org/2002/07/owl#Class> .
<http://def.seegrid.csiro.au/ontology/om/om-lite#CountObject> <http://www.w3.org/2000/01/rdf-schema#subClassOf> _:Bcaa52b8ca80d3545838555278ed1f713 .
