<http://www.w3.org/ns/lemon/ontolex#ConceptSet>
        a       <http://www.w3.org/2002/07/owl#Class> ;
        <http://www.w3.org/2000/01/rdf-schema#comment>
                "A concept set represents a collection of lexical concepts."@en , "'Набор понятий' представляет собой совокупность лексических понятий."@ru ;
        <http://www.w3.org/2000/01/rdf-schema#isDefinedBy>
                <http://www.w3.org/ns/lemon/ontolex> ;
        <http://www.w3.org/2000/01/rdf-schema#label>
                "banca concetti"@it , "banque de conepts"@fr , "Konzeptsatz"@de , "conjunto de conceptos"@es , "concept set"@en , "набор понятий"@ru , "verzameling van begrippen"@nl ;
        <http://www.w3.org/2000/01/rdf-schema#subClassOf>
                <http://www.w3.org/2004/02/skos/core#ConceptScheme> ;
        <http://www.w3.org/2002/07/owl#equivalentClass>
                [ a       <http://www.w3.org/2002/07/owl#Restriction> ;
                  <http://www.w3.org/2002/07/owl#minQualifiedCardinality>
                          "1"^^<http://www.w3.org/2001/XMLSchema#nonNegativeInteger> ;
                  <http://www.w3.org/2002/07/owl#onClass>
                          <http://www.w3.org/ns/lemon/ontolex#LexicalConcept> ;
                  <http://www.w3.org/2002/07/owl#onProperty>
                          <http://www.w3.org/2004/02/skos/core#inScheme>
                ] .

<http://www.w3.org/ns/lemon/ontolex#isReferenceOf>
        a       <http://www.w3.org/2002/07/owl#ObjectProperty> , <http://www.w3.org/2002/07/owl#InverseFunctionalProperty> ;
        <http://www.w3.org/2000/01/rdf-schema#comment>
                "Свойство объекта 'является референцией' представляет собой свойство, обратное к свойству 'референция'."@ru , "The object property isReferenceOf is the inverse property of reference."@en ;
        <http://www.w3.org/2000/01/rdf-schema#domain>
                <http://www.w3.org/2000/01/rdf-schema#Resource> ;
        <http://www.w3.org/2000/01/rdf-schema#isDefinedBy>
                <http://www.w3.org/ns/lemon/ontolex> ;
        <http://www.w3.org/2000/01/rdf-schema#label>
                "is referentie van"@nl , "é referência de"@pt , "es referencia de"@es , "è riferimento di"@it , "is verwysing van"@af , "este referință a(l)"@ro , "est référence de"@fr , "является референцией"@ru , "är referens för"@sv , "is reference of"@en , "ist Referenz von"@de ;
        <http://www.w3.org/2000/01/rdf-schema#range>
                [ a       <http://www.w3.org/2002/07/owl#Class> ;
                  <http://www.w3.org/2002/07/owl#unionOf>
                          ( <http://www.w3.org/ns/lemon/ontolex#LexicalSense> <http://www.w3.org/ns/lemon/synsem#OntoMap> )
                ] ;
        <http://www.w3.org/2002/07/owl#inverseOf>
                <http://www.w3.org/ns/lemon/ontolex#reference> .

<http://www.w3.org/ns/lemon/ontolex#lexicalForm>
        a       <http://www.w3.org/2002/07/owl#ObjectProperty> ;
        <http://www.w3.org/2000/01/rdf-schema#comment>
                "The 'lexical form' property relates a lexical entry to one grammatical form variant of the lexical entry."@en , "Свойство 'лексическая форма' соотносит словарную единицу с одним вариантом грамматической формы словарной единицы."@ru ;
        <http://www.w3.org/2000/01/rdf-schema#domain>
                <http://www.w3.org/ns/lemon/ontolex#LexicalEntry> ;
        <http://www.w3.org/2000/01/rdf-schema#isDefinedBy>
                <http://www.w3.org/ns/lemon/ontolex> ;
        <http://www.w3.org/2000/01/rdf-schema#label>
                "formă lexicală"@ro , "lexikalische Form"@de , "lexical form"@en , "forma lessicale"@it , "лексическая форма"@ru , "forma léxica"@es , "leksikale vorm"@af , "lexikaal vorm"@nl , "forme lexicale"@fr , "lexikonform"@sv ;
        <http://www.w3.org/2000/01/rdf-schema#range>
                <http://www.w3.org/ns/lemon/ontolex#Form> .

<http://www.w3.org/ns/lemon/ontolex#morphologicalPattern>
        a       <http://www.w3.org/2002/07/owl#ObjectProperty> ;
        <http://www.w3.org/2000/01/rdf-schema#comment>
                "Свойство 'морфологическая модель' обозначает морфологический класс слова."@ru , "The 'morphological pattern' property indicates the morphological class of a word."@en ;
        <http://www.w3.org/2000/01/rdf-schema#domain>
                <http://www.w3.org/ns/lemon/ontolex#LexicalEntry> ;
        <http://www.w3.org/2000/01/rdf-schema#isDefinedBy>
                <http://www.w3.org/ns/lemon/ontolex> ;
        <http://www.w3.org/2000/01/rdf-schema#label>
                "morphologisches Muster"@de , "morfologiskt mönster"@sv , "morfologiese patroon"@af , "model morfologic"@ro , "morfologische patroon"@nl , "patrón morfológico"@es , "motivo morfologico"@it , "морфологическая модель"@ru , "patron morphologique"@fr , "morphological pattern"@en .

<http://www.w3.org/ns/lemon/ontolex#lexicalizedSense>
        a       <http://www.w3.org/2002/07/owl#ObjectProperty> ;
        <http://www.w3.org/2000/01/rdf-schema#comment>
                "The 'lexicalized sense' property relates a lexical concept to a corresponding lexical sense that lexicalizes the concept."@en , "Свойство 'лексикализованный смысл' связывает лексическое понятие с соответствующим лексическим смыслом, который лексикализует понятие."@ru ;
        <http://www.w3.org/2000/01/rdf-schema#domain>
                <http://www.w3.org/ns/lemon/ontolex#LexicalConcept> ;
        <http://www.w3.org/2000/01/rdf-schema#isDefinedBy>
                <http://www.w3.org/ns/lemon/ontolex> ;
        <http://www.w3.org/2000/01/rdf-schema#label>
                "sens lexicalizat"@ro , "lexikaal zin"@nl , "lexicalized sense"@en , "lexikaliserad betydelse"@sv , "senso lessicalizzato"@it , "acepción lexicalizada"@es , "geleksikaliseerde Sin"@af , "signification lexicalisé"@fr , "lexikalisierter Sinn"@de , "лексикализованный смысл"@ru ;
        <http://www.w3.org/2000/01/rdf-schema#range>
                <http://www.w3.org/ns/lemon/ontolex#LexicalSense> .

<http://www.w3.org/ns/lemon/ontolex#canonicalForm>
        a       <http://www.w3.org/2002/07/owl#ObjectProperty> , <http://www.w3.org/2002/07/owl#FunctionalProperty> ;
        <http://www.w3.org/2000/01/rdf-schema#comment>
                "Свойство 'каноническая форма' связывает словарную единицу с ее канонической или словарной формой. Она обычно обозначает \"лемму\" словарной единицы."@ru , "The 'canonical form' property relates a lexical entry to its canoncical or dictionary form. This usually indicates the \"lemma\" form of a lexical entry. "@en ;
        <http://www.w3.org/2000/01/rdf-schema#domain>
                <http://www.w3.org/ns/lemon/ontolex#LexicalEntry> ;
        <http://www.w3.org/2000/01/rdf-schema#isDefinedBy>
                <http://www.w3.org/ns/lemon/ontolex> ;
        <http://www.w3.org/2000/01/rdf-schema#label>
                "kanoniese vorm"@af , "forme canonique"@fr , "forma canonica"@it , "каноническая форма"@ru , "forma canonica"@pt , "kanonische Form"@de , "canonical form"@en , "canonieke vorm"@nl , "forma canónica"@es , "kanonisk form "@sv , "formă canonică"@ro ;
        <http://www.w3.org/2000/01/rdf-schema#range>
                <http://www.w3.org/ns/lemon/ontolex#Form> ;
        <http://www.w3.org/2000/01/rdf-schema#subPropertyOf>
                <http://www.w3.org/ns/lemon/ontolex#lexicalForm> .

<http://www.w3.org/ns/lemon/ontolex#isDenotedBy>
        a       <http://www.w3.org/2002/07/owl#ObjectProperty> ;
        <http://www.w3.org/2000/01/rdf-schema#comment>
                "The object property isDenotedBy is the inverse of the object property denotes."@en , "Свойство объекта 'обозначается' является обратным к свойству объекта 'обозначает'."@ru ;
        <http://www.w3.org/2000/01/rdf-schema#domain>
                <http://www.w3.org/2000/01/rdf-schema#Resource> ;
        <http://www.w3.org/2000/01/rdf-schema#isDefinedBy>
                <http://www.w3.org/ns/lemon/ontolex> ;
        <http://www.w3.org/2000/01/rdf-schema#label>
                "betecknas av"@sv , "é denotado por"@pt , "est dénoté par"@fr , "word aangedui deur"@af , "wordt aangeduidet door"@nl , "es denotado por"@es , "wird bezeichnet von"@de , "обозначается"@ru , "è denotato da"@it , "este denotat cu"@ro , "is denoted by"@en ;
        <http://www.w3.org/2000/01/rdf-schema#range>
                <http://www.w3.org/ns/lemon/ontolex#LexicalEntry> ;
        <http://www.w3.org/2002/07/owl#inverseOf>
                <http://www.w3.org/ns/lemon/ontolex#denotes> .

<http://www.w3.org/ns/lemon/ontolex#isLexicalizedSenseOf>
        a       <http://www.w3.org/2002/07/owl#ObjectProperty> ;
        <http://www.w3.org/2000/01/rdf-schema#comment>
                "The object property isLexicalizedSenseOf is the inverse property of lexicalized sense."@en , "Свойство объекта 'является лексикализованным смыслом' представляет собой свойство, обратное к свойству 'лексикализованный смысл'."@ru ;
        <http://www.w3.org/2000/01/rdf-schema#domain>
                <http://www.w3.org/ns/lemon/ontolex#LexicalSense> ;
        <http://www.w3.org/2000/01/rdf-schema#isDefinedBy>
                <http://www.w3.org/ns/lemon/ontolex> ;
        <http://www.w3.org/2000/01/rdf-schema#label>
                "is lexikaal zin van"@nl , "is geleksikaliseerde sin van"@af , "is lexicalized sense of"@en , "является лексикализованным смыслом"@ru , "ist lexikalisierter Sinn von"@de , "è il senso lessicalizzato di"@it , "är lexikaliserad betydelse för"@sv , "este sens lexicalizat de"@ro , "es l'acepción lexicalizado de"@es , "est le sens lexicalisé de"@fr ;
        <http://www.w3.org/2000/01/rdf-schema#range>
                <http://www.w3.org/ns/lemon/ontolex#LexicalConcept> ;
        <http://www.w3.org/2002/07/owl#inverseOf>
                <http://www.w3.org/ns/lemon/ontolex#lexicalizedSense> .

<http://www.w3.org/ns/lemon/ontolex#Affix>
        a       <http://www.w3.org/2002/07/owl#Class> ;
        <http://www.w3.org/2000/01/rdf-schema#comment>
                "'Аффикс' - это словарная единица, которая представляет морфему (суффикс, префикс, инфикс, циркумфикс), добавляемую к основе слова для образования нового слова."@ru , "An affix is a lexical entry that represents a morpheme (suffix, prefix, infix, circumfix) that is attached to a word stem to form a new word."@en ;
        <http://www.w3.org/2000/01/rdf-schema#isDefinedBy>
                <http://www.w3.org/ns/lemon/ontolex> ;
        <http://www.w3.org/2000/01/rdf-schema#label>
                "affisso"@it , "affiks"@af , "affix"@en , "аффикс"@ru , "affixe"@fr , "affix"@sv , "aplică"@ro , "afijo"@es , "Affix"@de , "affix"@nl ;
        <http://www.w3.org/2000/01/rdf-schema#subClassOf>
                <http://www.w3.org/ns/lemon/ontolex#LexicalEntry> .

<http://www.w3.org/ns/lemon/ontolex#sense>
        a       <http://www.w3.org/2002/07/owl#InverseFunctionalProperty> , <http://www.w3.org/2002/07/owl#ObjectProperty> ;
        <http://www.w3.org/2000/01/rdf-schema#comment>
                "Свойство 'смысл' связывает словарную единицу с одним из ее лексических смыслов."@ru , "The 'sense' property relates a lexical entry to one of its lexical senses. "@en ;
        <http://www.w3.org/2000/01/rdf-schema#domain>
                <http://www.w3.org/ns/lemon/ontolex#LexicalEntry> ;
        <http://www.w3.org/2000/01/rdf-schema#isDefinedBy>
                <http://www.w3.org/ns/lemon/ontolex> ;
        <http://www.w3.org/2000/01/rdf-schema#label>
                "sense"@en , "zin"@nl , "Sinn"@de , "signification"@fr , "sinne"@af , "betydelse"@sv , "senso"@it , "смысл"@ru , "sens"@ro , "sentido"@pt , "acepción"@es ;
        <http://www.w3.org/2000/01/rdf-schema#range>
                <http://www.w3.org/ns/lemon/ontolex#LexicalSense> ;
        <http://www.w3.org/2002/07/owl#inverseOf>
                <http://www.w3.org/ns/lemon/ontolex#isSenseOf> .

<http://www.w3.org/ns/lemon/ontolex>
        a       <http://www.w3.org/2002/07/owl#Ontology> ;
        <http://creativecommons.org/ns#license>
                <https://creativecommons.org/publicdomain/zero/1.0/> ;
        <http://purl.org/dc/elements/1.1/contributor>
                <http://www.ilc.cnr.it/en/content/anas-fahad-khan> , <http://www.oeg-upm.net/index.php/teachers/53-lupe> , <http://www.dfki.de/~declerck/> , <https://sites.google.com/site/francescafrontini/> , <http://www.istc.cnr.it/people/aldo-gangemi> , <http://art.uniroma2.it/fiorelli/> , <http://mayor2.dia.fi.upm.es/oeg-upm/index.php/en/teachers/52-emontiel> , <http://art.uniroma2.it/stellato/> , <http://www.paulbuitelaar.net/> , <http://jogracia.url.ph/web/> ;
        <http://purl.org/dc/elements/1.1/creator>
                <http://www.cimiano.de/> , <http://john.mccr.ae/> ;
        <http://purl.org/dc/elements/1.1/description>
                "A model for the representation of lexical information relative to ontologies. Core module."@en ;
        <http://purl.org/dc/elements/1.1/issued>
                "2016-01-10"^^<http://www.w3.org/2001/XMLSchema#date> ;
        <http://purl.org/dc/elements/1.1/modified>
                "2016-01-10"^^<http://www.w3.org/2001/XMLSchema#date> ;
        <http://purl.org/dc/elements/1.1/publisher>
                <http://www.w3.org/community/ontolex> ;
        <http://purl.org/dc/elements/1.1/rights>
                "CC-Zero" ;
        <http://purl.org/dc/elements/1.1/title>
                "Lexicon Model for Ontologies - Core"@en ;
        <http://purl.org/vocab/vann/preferredNamespacePrefix>
                "ontolex" ;
        <http://purl.org/vocab/vann/preferredNamespaceUri>
                "http://www.w3.org/ns/lemon/ontolex#" ;
        <http://www.w3.org/2002/07/owl#versionInfo>
                1.0 .

<http://www.w3.org/ns/lemon/ontolex#concept>
        a       <http://www.w3.org/2002/07/owl#ObjectProperty> ;
        <http://www.w3.org/2000/01/rdf-schema#comment>
                "Свойство 'понятие' связывает сущность в онтологии с лексическим понятием, которое представляет соответствующее значение."@ru , "The 'concept' property relates an ontological entity to a lexical concept that represents the corresponding meaning."@en ;
        <http://www.w3.org/2000/01/rdf-schema#isDefinedBy>
                <http://www.w3.org/ns/lemon/ontolex> ;
        <http://www.w3.org/2000/01/rdf-schema#label>
                "begrip"@nl , "понятие"@ru , "conceito"@pt , "concetto"@it , "concept"@en , "concept"@fr , "begrepp"@sv , "Konzept"@de , "concepto"@es , "concept"@ro , "konsep"@af ;
        <http://www.w3.org/2000/01/rdf-schema#range>
                <http://www.w3.org/ns/lemon/ontolex#LexicalConcept> ;
        <http://www.w3.org/2002/07/owl#inverseOf>
                <http://www.w3.org/ns/lemon/ontolex#isConceptOf> .

<http://www.w3.org/ns/lemon/ontolex#Word>
        a       <http://www.w3.org/2002/07/owl#Class> ;
        <http://www.w3.org/2000/01/rdf-schema#comment>
                "'Слово' - это словарная единица, представяющая собой единичную реализацию лексемы."@ru , "A word is a lexical entry that consists of a single token."@en ;
        <http://www.w3.org/2000/01/rdf-schema#isDefinedBy>
                <http://www.w3.org/ns/lemon/ontolex> ;
        <http://www.w3.org/2000/01/rdf-schema#label>
                "parola"@it , "woord"@nl , "woord"@af , "cuvânt"@ro , "word"@en , "слово"@ru , "Wort"@de , "ord"@sv , "palabra"@es , "mot"@fr ;
        <http://www.w3.org/2000/01/rdf-schema#subClassOf>
                <http://www.w3.org/ns/lemon/ontolex#LexicalEntry> .

<http://www.w3.org/ns/lemon/ontolex#reference>
        a       <http://www.w3.org/2002/07/owl#FunctionalProperty> , <http://www.w3.org/2002/07/owl#ObjectProperty> ;
        <http://www.w3.org/2000/01/rdf-schema#comment>
                "The 'reference' property relates a lexical sense to an ontological predicate that represents the denotation of the corresponding lexical entry. "@en , "Свойство 'референция' соотносит лексический смысл с предикатом в онтологии, который уточняет значение денотата (соответствующей словарной единицы)."@ru ;
        <http://www.w3.org/2000/01/rdf-schema#domain>
                [ a       <http://www.w3.org/2002/07/owl#Class> ;
                  <http://www.w3.org/2002/07/owl#unionOf>
                          ( <http://www.w3.org/ns/lemon/ontolex#LexicalSense> <http://www.w3.org/ns/lemon/synsem#OntoMap> )
                ] ;
        <http://www.w3.org/2000/01/rdf-schema#isDefinedBy>
                <http://www.w3.org/ns/lemon/ontolex> ;
        <http://www.w3.org/2000/01/rdf-schema#label>
                "référence"@fr , "Referenz"@de , "verwysing"@af , "referens"@sv , "referință"@ro , "referntie"@nl , "референция"@ru , "referencia"@es , "riferimento"@it , "referência"@pt , "reference"@en ;
        <http://www.w3.org/2000/01/rdf-schema#range>
                <http://www.w3.org/2000/01/rdf-schema#Resource> .

<http://www.w3.org/ns/lemon/ontolex#representation>
        a       <http://www.w3.org/2002/07/owl#DatatypeProperty> ;
        <http://www.w3.org/2000/01/rdf-schema#comment>
                "The 'representation' property indicates a string by which the form is represented according to some orthography. "@en , "Свойство 'представление' обозначает некую последовательность, с помощью которой форма может быть представлена средствами орфографии."@ru ;
        <http://www.w3.org/2000/01/rdf-schema#domain>
                <http://www.w3.org/ns/lemon/ontolex#Form> ;
        <http://www.w3.org/2000/01/rdf-schema#isDefinedBy>
                <http://www.w3.org/ns/lemon/ontolex> ;
        <http://www.w3.org/2000/01/rdf-schema#label>
                "representation"@sv , "voorstelling"@nl , "reprezentare"@ro , "représentation"@fr , "Darstellung"@de , "representação"@pt , "представление"@ru , "rappresentazione"@it , "voorstelling"@af , "representation"@en , "representación"@es ;
        <http://www.w3.org/2000/01/rdf-schema#range>
                <http://www.w3.org/1999/02/22-rdf-syntax-ns#langString> .

<http://www.w3.org/ns/lemon/ontolex#phoneticRep>
        a       <http://www.w3.org/2002/07/owl#DatatypeProperty> ;
        <http://www.w3.org/2000/01/rdf-schema#comment>
                "The 'phonetic representation' property indicates one phonetic representation of the pronunciation of the form using a scheme such as the International Phonetic Alphabet (IPA). "@en , "Свойство 'фонетическое представление' обозначает фонетическое представление произношения формы с использованием какой-либо схемы, например, Международного фонетического алфавита (IPA, МФА)."@ru ;
        <http://www.w3.org/2000/01/rdf-schema#domain>
                <http://www.w3.org/ns/lemon/ontolex#Form> ;
        <http://www.w3.org/2000/01/rdf-schema#isDefinedBy>
                <http://www.w3.org/ns/lemon/ontolex> ;
        <http://www.w3.org/2000/01/rdf-schema#label>
                "fonetische voorstelling"@nl , "fonetiese voorstelling"@af , "phonetic representation"@en , "фонетическое представление"@ru , "representación fonética"@es , "fonetisk representation "@sv , "rappresentazione fonetica"@it , "phonetische Darstellung"@de , "représentation phonétique"@fr , "reprezentare fonetică"@ro ;
        <http://www.w3.org/2000/01/rdf-schema#range>
                <http://www.w3.org/1999/02/22-rdf-syntax-ns#langString> ;
        <http://www.w3.org/2000/01/rdf-schema#subPropertyOf>
                <http://www.w3.org/ns/lemon/ontolex#representation> .

<http://www.w3.org/ns/lemon/ontolex#Form>
        a       <http://www.w3.org/2002/07/owl#Class> ;
        <http://www.w3.org/2000/01/rdf-schema#comment>
                "A form represents one grammatical realization of a lexical entry."@en , "'Форма' представляет одну грамматическую реализацию словарной единицы."@ru ;
        <http://www.w3.org/2000/01/rdf-schema#isDefinedBy>
                <http://www.w3.org/ns/lemon/ontolex> ;
        <http://www.w3.org/2000/01/rdf-schema#label>
                "Forma"@pt , "formă"@ro , "форма"@ru , "form"@en , "Form"@de , "forma"@es , "forme"@fr , "vorm"@af , "form"@sv , "forma"@it , "vorm"@nl ;
        <http://www.w3.org/2000/01/rdf-schema#subClassOf>
                <http://www.w3.org/2002/07/owl#Thing> ;
        <http://www.w3.org/2000/01/rdf-schema#subClassOf>
                [ a       <http://www.w3.org/2002/07/owl#Restriction> ;
                  <http://www.w3.org/2002/07/owl#minQualifiedCardinality>
                          "1"^^<http://www.w3.org/2001/XMLSchema#nonNegativeInteger> ;
                  <http://www.w3.org/2002/07/owl#onDataRange>
                          <http://www.w3.org/1999/02/22-rdf-syntax-ns#langString> ;
                  <http://www.w3.org/2002/07/owl#onProperty>
                          <http://www.w3.org/ns/lemon/ontolex#writtenRep>
                ] .

<http://www.w3.org/ns/lemon/ontolex#denotes>
        a       <http://www.w3.org/2002/07/owl#ObjectProperty> ;
        <http://www.w3.org/2000/01/rdf-schema#comment>
                "Свойство 'обозначает' связывает словарную единицу с предикатом в онтологии, который представляет ее значение и обладает денотативной или теоретико-модельной семантикой."@ru , "The 'denotes' property relates a lexical entry to a predicate in a given ontology that represents its meaning and has some denotational or model-theoretic semantics. "@en ;
        <http://www.w3.org/2000/01/rdf-schema#domain>
                <http://www.w3.org/ns/lemon/ontolex#LexicalEntry> ;
        <http://www.w3.org/2000/01/rdf-schema#isDefinedBy>
                <http://www.w3.org/ns/lemon/ontolex> ;
        <http://www.w3.org/2000/01/rdf-schema#label>
                "обозначает"@ru , "betecknar"@sv , "denota"@es , "denotă"@ro , "bezeichnet"@de , "dénote"@fr , "denota"@it , "dui aan"@af , "duidet aan"@nl , "denotes"@en , "denota"@pt ;
        <http://www.w3.org/2000/01/rdf-schema#range>
                <http://www.w3.org/2000/01/rdf-schema#Resource> ;
        <http://www.w3.org/2000/01/rdf-schema#subPropertyOf>
                <http://www.ontologydesignpatterns.org/cp/owl/semiotics.owl#denotes> ;
        <http://www.w3.org/2002/07/owl#propertyChainAxiom>
                ( <http://www.w3.org/ns/lemon/ontolex#sense> <http://www.w3.org/ns/lemon/ontolex#reference> ) .

<http://xmlns.com/foaf/0.1/Organization>
        a       <http://www.w3.org/2002/07/owl#Class> .

<http://www.w3.org/ns/lemon/ontolex#isSenseOf>
        a       <http://www.w3.org/2002/07/owl#FunctionalProperty> , <http://www.w3.org/2002/07/owl#ObjectProperty> ;
        <http://www.w3.org/2000/01/rdf-schema#comment>
                "Свойство 'является смыслом' представляет собой свойство, обратное к свойству 'смысл'."@ru , "The property isSenseOf is the inverse property of sense."@en ;
        <http://www.w3.org/2000/01/rdf-schema#domain>
                <http://www.w3.org/ns/lemon/ontolex#LexicalSense> ;
        <http://www.w3.org/2000/01/rdf-schema#isDefinedBy>
                <http://www.w3.org/ns/lemon/ontolex> ;
        <http://www.w3.org/2000/01/rdf-schema#label>
                "est signification de"@fr , "es acepción de"@es , "is sense of"@en , "är betydelse för"@sv , "este sens a(l)"@ro , "è il senso di"@it , "является смыслом"@ru , "is sin van"@af , "é sentido de"@pt , "is zin van"@nl , "ist Sinn von"@de ;
        <http://www.w3.org/2000/01/rdf-schema#range>
                <http://www.w3.org/ns/lemon/ontolex#LexicalEntry> .

<http://www.w3.org/ns/lemon/ontolex#otherForm>
        a       <http://www.w3.org/2002/07/owl#ObjectProperty> ;
        <http://www.w3.org/2000/01/rdf-schema#comment>
                "Свойство 'другая форма' связывает словарную единицу с малоупотребительной формой (\"не леммой\"), которая является реализацией данной словарной единицы"@ru , "The  'other form' property relates a lexical entry to a non-preferred (\"non-lemma\") form that realizes the given lexical entry."@en ;
        <http://www.w3.org/2000/01/rdf-schema#domain>
                <http://www.w3.org/ns/lemon/ontolex#LexicalEntry> ;
        <http://www.w3.org/2000/01/rdf-schema#isDefinedBy>
                <http://www.w3.org/ns/lemon/ontolex> ;
        <http://www.w3.org/2000/01/rdf-schema#label>
                "otra forma"@es , "ander form"@af , "altra forma"@it , "andere Form"@de , "outra forma"@pt , "autre forme"@fr , "altă formă"@ro , "other form"@en , "другая форма"@ru , "annan form"@sv , "andere vorm"@nl ;
        <http://www.w3.org/2000/01/rdf-schema#range>
                <http://www.w3.org/ns/lemon/ontolex#Form> ;
        <http://www.w3.org/2000/01/rdf-schema#subPropertyOf>
                <http://www.w3.org/ns/lemon/ontolex#lexicalForm> .

<http://www.w3.org/ns/lemon/ontolex#isEvokedBy>
        a       <http://www.w3.org/2002/07/owl#ObjectProperty> ;
        <http://www.w3.org/2000/01/rdf-schema#comment>
                "Отношение обратное к 'порождает'."@ru , "The inverse relation to evokes."@en ;
        <http://www.w3.org/2000/01/rdf-schema#domain>
                <http://www.w3.org/ns/lemon/ontolex#LexicalConcept> ;
        <http://www.w3.org/2000/01/rdf-schema#isDefinedBy>
                <http://www.w3.org/ns/lemon/ontolex> ;
        <http://www.w3.org/2000/01/rdf-schema#label>
                "este evocat de"@ro , "wird hervorgerufen von"@de , "è evocato da"@it , "framkallas av "@sv , "es evocado por"@es , "word opgeroep deur"@af , "wordt uitgelokt door"@nl , "порождается"@ru , "is evoked by"@en , "est évoqué par"@fr ;
        <http://www.w3.org/2000/01/rdf-schema#range>
                <http://www.w3.org/ns/lemon/ontolex#LexicalEntry> ;
        <http://www.w3.org/2002/07/owl#inverseOf>
                <http://www.w3.org/ns/lemon/ontolex#evokes> .

<http://www.w3.org/ns/lemon/ontolex#LexicalConcept>
        a       <http://www.w3.org/2002/07/owl#Class> ;
        <http://www.w3.org/2000/01/rdf-schema#comment>
                "A lexical concept represents a mental abstraction, concept or unit of thought that embodies the meaning of one or more lexical entries."@en , "'Лексическое понятие' представляет элемент абстрактного мышления, понятие или единицу мысли, которая может быть лексикализована определенным набором смыслов."@ru ;
        <http://www.w3.org/2000/01/rdf-schema#isDefinedBy>
                <http://www.w3.org/ns/lemon/ontolex> ;
        <http://www.w3.org/2000/01/rdf-schema#label>
                "concept lexical"@ro , "lexikalisches Konzept"@de , "lexikaliskt begrepp"@sv , "lexikaal concept"@nl , "lexical concept"@en , "лексическое понятие"@ru , "leksikale konsep"@af , "concetto lessicale"@it , "conceito léxico"@pt , "concept lexical"@fr , "concepto lexicalizado"@es ;
        <http://www.w3.org/2000/01/rdf-schema#subClassOf>
                <http://www.ontologydesignpatterns.org/cp/owl/semiotics.owl#Meaning> , <http://www.w3.org/2004/02/skos/core#Concept> .

<http://www.w3.org/ns/lemon/ontolex#LexicalSense>
        a       <http://www.w3.org/2002/07/owl#Class> ;
        <http://www.w3.org/2000/01/rdf-schema#comment>
                "A lexical sense represents the lexical meaning of a lexical entry when interpreted as referring to the corresponding ontology element. A lexical sense thus represents a reification of a pair of a uniquely determined lexical entry and a uniquely determined ontology entity it refers to. A link between a lexical entry and an ontology entity via a Lexical Sense object implies that the lexical entry can be used to refer to the ontology entity in question."@en , "'Лексический смысл' обозначает лексическое значение словарной единицы, когда оно понимается как относящееся к соответствующему элементу онтологии. 'Лексический смысл' представляет собой овеществление пары, состоящей из однозначно определяемой словарной единицы и однозначно определяемой сущности отнологии, к которой относится данный лексический смысл. Связь между словарной единицей и сущностью в онтологии посредством объекта 'Лексический Смысл' подразумевает, что словарная статья может быть использована для отсылки к соответствующей сущности в онтологии."@ru ;
        <http://www.w3.org/2000/01/rdf-schema#isDefinedBy>
                <http://www.w3.org/ns/lemon/ontolex> ;
        <http://www.w3.org/2000/01/rdf-schema#label>
                "signification lexicale"@fr , "acepción léxica"@es , "sens lexical"@ro , "лексический смысл"@ru , "lexikonbetydelse"@sv , "lexical sense"@en , "leksikale sin"@af , "senso lessicale"@it , "lexikalischer Sinn"@de , "lexikaal zin"@nl ;
        <http://www.w3.org/2000/01/rdf-schema#subClassOf>
                <http://www.ontologydesignpatterns.org/cp/owl/semiotics.owl#Meaning> ;
        <http://www.w3.org/2000/01/rdf-schema#subClassOf>
                [ a       <http://www.w3.org/2002/07/owl#Restriction> ;
                  <http://www.w3.org/2002/07/owl#cardinality>
                          "1"^^<http://www.w3.org/2001/XMLSchema#nonNegativeInteger> ;
                  <http://www.w3.org/2002/07/owl#onProperty>
                          <http://www.w3.org/ns/lemon/ontolex#reference>
                ] ;
        <http://www.w3.org/2000/01/rdf-schema#subClassOf>
                [ a       <http://www.w3.org/2002/07/owl#Restriction> ;
                  <http://www.w3.org/2002/07/owl#onClass>
                          <http://www.w3.org/ns/lemon/ontolex#LexicalEntry> ;
                  <http://www.w3.org/2002/07/owl#onProperty>
                          <http://www.w3.org/ns/lemon/ontolex#isSenseOf> ;
                  <http://www.w3.org/2002/07/owl#qualifiedCardinality>
                          "1"^^<http://www.w3.org/2001/XMLSchema#nonNegativeInteger>
                ] .

<http://www.w3.org/ns/lemon/ontolex#writtenRep>
        a       <http://www.w3.org/2002/07/owl#DatatypeProperty> ;
        <http://www.w3.org/2000/01/rdf-schema#comment>
                "Свойство 'письменное представление' обозначает письменное представление формы."@ru , "The 'written representation' property indicates the written representation of a form."@en ;
        <http://www.w3.org/2000/01/rdf-schema#domain>
                <http://www.w3.org/ns/lemon/ontolex#Form> ;
        <http://www.w3.org/2000/01/rdf-schema#isDefinedBy>
                <http://www.w3.org/ns/lemon/ontolex> ;
        <http://www.w3.org/2000/01/rdf-schema#label>
                "representação escrita"@pt , "written representation"@en , "reprezentare scrisă"@ro , "représentation écrite"@fr , "schriftliche Darstellung"@de , "rappresentazione scritta"@it , "skriven form "@sv , "representación escrita"@es , "письменное представление"@ru , "schriftlijke voorstelling"@nl , "geskrewe voorstelling"@af ;
        <http://www.w3.org/2000/01/rdf-schema#range>
                <http://www.w3.org/1999/02/22-rdf-syntax-ns#langString> ;
        <http://www.w3.org/2000/01/rdf-schema#subPropertyOf>
                <http://www.w3.org/ns/lemon/ontolex#representation> .

<http://www.w3.org/ns/lemon/ontolex#evokes>
        a       <http://www.w3.org/2002/07/owl#ObjectProperty> ;
        <http://www.w3.org/2000/01/rdf-schema#comment>
                "Свойство 'порождает' связывает словарную единицу с одним из лексических понятий, которую она порождает, то есть мыслительное понятие, которое возникает в сознании говорящих, когда они слышат данную словарную единицу."@ru , "The 'evokes' property relates a lexical entry to one of the lexical concepts it evokes, i.e. the mental concept that speakers of a language might associate when hearing the lexical entry."@en ;
        <http://www.w3.org/2000/01/rdf-schema#domain>
                <http://www.w3.org/ns/lemon/ontolex#LexicalEntry> ;
        <http://www.w3.org/2000/01/rdf-schema#isDefinedBy>
                <http://www.w3.org/ns/lemon/ontolex> ;
        <http://www.w3.org/2000/01/rdf-schema#label>
                "evocă"@ro , "évoque"@fr , "evoca"@es , "roep op"@af , "ruft hervor"@de , "lokt uit"@nl , "framkallar"@sv , "evoca"@it , "порождает"@ru , "evokes"@en , "evoca"@pt ;
        <http://www.w3.org/2000/01/rdf-schema#range>
                <http://www.w3.org/ns/lemon/ontolex#LexicalConcept> ;
        <http://www.w3.org/2002/07/owl#propertyChainAxiom>
                ( <http://www.w3.org/ns/lemon/ontolex#sense> <http://www.w3.org/ns/lemon/ontolex#isLexicalizedSenseOf> ) .

<http://www.w3.org/2002/07/owl#topDataProperty>
        a       <http://www.w3.org/2002/07/owl#DatatypeProperty> .

<http://www.ontologydesignpatterns.org/cp/owl/semiotics.owl#Expression>
        a       <http://www.w3.org/2002/07/owl#Class> ;
        <http://www.w3.org/2000/01/rdf-schema#label>
                "expression"@en .

<http://www.w3.org/ns/lemon/synsem#OntoMap>
        a       <http://www.w3.org/2002/07/owl#Class> .

<http://www.w3.org/ns/lemon/ontolex#LexicalEntry>
        a       <http://www.w3.org/2002/07/owl#Class> ;
        <http://www.w3.org/2000/01/rdf-schema#comment>
                "'Словарная единица' представляет собой единицу анализа словаря, которая состоит из совокупности грамматически связанных форм и совокупности основных значений, ассоциирующихся со всеми этими формами. 'Словарная единица' - это слово, словосочетание или аффикс одной части речи, морфологической модели, этимологии и набора значений."@ru , "A lexical entry represents a unit of analysis of the lexicon that consists of a set of forms that are grammatically related and a set of base meanings that are associated with all of these forms. Thus, a lexical entry is a word, multiword expression or affix with a single part-of-speech, morphological pattern, etymology and set of senses."@en ;
        <http://www.w3.org/2000/01/rdf-schema#isDefinedBy>
                <http://www.w3.org/ns/lemon/ontolex> ;
        <http://www.w3.org/2000/01/rdf-schema#label>
                "leksikale inskrywing"@af , "словарная единица"@ru , "Lexikoneintrag"@de , "înregistrare lexicală"@ro , "lexikaal item"@nl , "entrée lexicale"@fr , "entrata lessicale"@it , "lexikoningång"@sv , "entrada léxica"@es , "lexical entry"@en ;
        <http://www.w3.org/2000/01/rdf-schema#subClassOf>
                <http://www.ontologydesignpatterns.org/cp/owl/semiotics.owl#Expression> , <http://www.w3.org/2002/07/owl#Thing> ;
        <http://www.w3.org/2000/01/rdf-schema#subClassOf>
                [ a       <http://www.w3.org/2002/07/owl#Restriction> ;
                  <http://www.w3.org/2002/07/owl#minQualifiedCardinality>
                          "1"^^<http://www.w3.org/2001/XMLSchema#nonNegativeInteger> ;
                  <http://www.w3.org/2002/07/owl#onClass>
                          <http://www.w3.org/ns/lemon/ontolex#Form> ;
                  <http://www.w3.org/2002/07/owl#onProperty>
                          <http://www.w3.org/ns/lemon/ontolex#lexicalForm>
                ] ;
        <http://www.w3.org/2000/01/rdf-schema#subClassOf>
                [ a       <http://www.w3.org/2002/07/owl#Restriction> ;
                  <http://www.w3.org/2002/07/owl#maxQualifiedCardinality>
                          "1"^^<http://www.w3.org/2001/XMLSchema#nonNegativeInteger> ;
                  <http://www.w3.org/2002/07/owl#onClass>
                          <http://www.w3.org/ns/lemon/ontolex#Form> ;
                  <http://www.w3.org/2002/07/owl#onProperty>
                          <http://www.w3.org/ns/lemon/ontolex#canonicalForm>
                ] .

<http://www.w3.org/ns/lemon/ontolex#usage>
        a       <http://www.w3.org/2002/07/owl#ObjectProperty> ;
        <http://www.w3.org/2000/01/rdf-schema#comment>
                "Свойство 'употребление' обозначает условия использования или прагматическое значение при употреблении словарной единицы для соотнесения с определенным значением в онтологии."@ru , "The 'usage' property indicates usage conditions or pragmatic implications when using the lexical entry to refer to the given ontological meaning."@en ;
        <http://www.w3.org/2000/01/rdf-schema#domain>
                <http://www.w3.org/ns/lemon/ontolex#LexicalSense> ;
        <http://www.w3.org/2000/01/rdf-schema#isDefinedBy>
                <http://www.w3.org/ns/lemon/ontolex> ;
        <http://www.w3.org/2000/01/rdf-schema#label>
                "Gebrauch"@de , "gebruik"@nl , "uso"@es , "употребление"@ru , "uso"@it , "usage"@fr , "usage"@en ;
        <http://www.w3.org/2000/01/rdf-schema#range>
                <http://www.w3.org/2000/01/rdf-schema#Resource> .

<http://purl.org/vocommons/voaf#Vocabulary>
        a       <http://www.w3.org/2002/07/owl#Class> .

<http://www.w3.org/2000/01/rdf-schema#isDefinedBy>
        a       <http://www.w3.org/2002/07/owl#AnnotationProperty> .

<http://www.ontologydesignpatterns.org/cp/owl/semiotics.owl#Meaning>
        a       <http://www.w3.org/2002/07/owl#Class> ;
        <http://www.w3.org/2000/01/rdf-schema#label>
                "meaning"@en .

<http://www.w3.org/ns/lemon/ontolex#isConceptOf>
        a       <http://www.w3.org/2002/07/owl#ObjectProperty> ;
        <http://www.w3.org/2000/01/rdf-schema#comment>
                "Это свойство формализует значение 'Лексического Понятия', связывая его с отдельным значением в онтологии."@ru , "This property formalizes the meaning of a Lexical Concept by linking it to a particular ontological meaning."@en ;
        <http://www.w3.org/2000/01/rdf-schema#domain>
                <http://www.w3.org/ns/lemon/ontolex#LexicalConcept> ;
        <http://www.w3.org/2000/01/rdf-schema#isDefinedBy>
                <http://www.w3.org/ns/lemon/ontolex> ;
        <http://www.w3.org/2000/01/rdf-schema#label>
                "est un concept pour "@fr , "is concept of"@en , "är begrepp för"@sv , "is konsep van"@af , "является понятием"@ru , "ist Konzept von"@de , "is concept van"@nl , "este concept a(l)"@ro , "es concepto de"@es , "é conceito de"@pt , "è concetto di "@it .

<http://www.w3.org/ns/lemon/ontolex#MultiWordExpression>
        a       <http://www.w3.org/2002/07/owl#Class> ;
        <http://www.w3.org/2000/01/rdf-schema#comment>
                "'Словосочетание' - это словарная единица, состоящая из двух или более слов."@ru , "A multiword expression is a lexical entry that consists of two or more words."@en ;
        <http://www.w3.org/2000/01/rdf-schema#isDefinedBy>
                <http://www.w3.org/ns/lemon/ontolex> ;
        <http://www.w3.org/2000/01/rdf-schema#label>
                "Mehrwortausdruck"@de , "flerordsuttryck"@sv , "mutliwoorduitdrukking"@nl , "multi-word expression"@en , "espressione di gruppi di parole"@it , "multiwoorduitdrukking"@af , "expresie din mai multe cuvinte"@ro , "словосочетание"@ru , "expresión multipalabra"@es , "expression à mots multiples"@fr ;
        <http://www.w3.org/2000/01/rdf-schema#subClassOf>
                <http://www.w3.org/ns/lemon/ontolex#LexicalEntry> .

<http://www.ontologydesignpatterns.org/cp/owl/semiotics.owl#denotes>
        a       <http://www.w3.org/2002/07/owl#ObjectProperty> .

<http://www.w3.org/2004/02/skos/core#inScheme>
        a       <http://www.w3.org/2002/07/owl#ObjectProperty> ;
        <http://www.w3.org/2000/01/rdf-schema#label>
                "in scheme"@en .

<http://www.w3.org/2004/02/skos/core#ConceptScheme>
        a       <http://www.w3.org/2002/07/owl#Class> ;
        <http://www.w3.org/2000/01/rdf-schema#label>
                "concept scheme"@en .

<http://www.w3.org/2002/07/owl#topObjectProperty>
        a       <http://www.w3.org/2002/07/owl#ObjectProperty> .

<http://www.w3.org/2004/02/skos/core#Concept>
        a       <http://www.w3.org/2002/07/owl#Class> ;
        <http://www.w3.org/2000/01/rdf-schema#label>
                "concept"@en .

<http://xmlns.com/foaf/0.1/Person>
        a       <http://www.w3.org/2002/07/owl#Class> .

<http://www.w3.org/1999/02/22-rdf-syntax-ns#langString>
        a       <http://www.w3.org/2000/01/rdf-schema#Datatype> .
