<http://www.gsi.dit.upm.es/ontologies/onyx/ns#hasDimension>
        a       <http://www.w3.org/2002/07/owl#ObjectProperty> ;
        <http://www.w3.org/2000/01/rdf-schema#comment>
                " Used to define the Dimensions of an Emotion Model" ;
        <http://www.w3.org/2000/01/rdf-schema#domain>
                <http://www.gsi.dit.upm.es/ontologies/onyx/ns#EmotionModel> ;
        <http://www.w3.org/2000/01/rdf-schema#isDefinedBy>
                "http://www.gsi.dit.upm.es/ontologies/onyx/ns" ;
        <http://www.w3.org/2000/01/rdf-schema#label>
                "hasDimension" ;
        <http://www.w3.org/2000/01/rdf-schema#range>
                <http://www.gsi.dit.upm.es/ontologies/onyx/ns#Dimension> .

<http://www.gsi.dit.upm.es/ontologies/onyx/ns#ActionTendency>
        a       <http://www.w3.org/2002/07/owl#DatatypeProperty> ;
        <http://www.w3.org/2000/01/rdf-schema#comment>
                "Action Tendency of the emotion: a desire to behave in select communicative or important actions that are connected to a particular feeling." ;
        <http://www.w3.org/2000/01/rdf-schema#isDefinedBy>
                "http://www.gsi.dit.upm.es/ontologies/onyx/ns" ;
        <http://www.w3.org/2000/01/rdf-schema#label>
                "ActionTendency" .

<http://www.gsi.dit.upm.es/ontologies/onyx/ns#Dimension>
        a       <http://www.w3.org/2002/07/owl#DatatypeProperty> ;
        <http://www.w3.org/2000/01/rdf-schema#comment>
                "Parent for Dimension properties." ;
        <http://www.w3.org/2000/01/rdf-schema#isDefinedBy>
                "http://www.gsi.dit.upm.es/ontologies/onyx/ns" ;
        <http://www.w3.org/2000/01/rdf-schema#label>
                "Dimension" .

<http://www.gsi.dit.upm.es/ontologies/onyx/ns#source>
        a       <http://www.w3.org/2002/07/owl#ObjectProperty> ;
        <http://www.w3.org/2000/01/rdf-schema#comment>
                "Source from which the emotion was extracted (URL, Site, Entity...)" ;
        <http://www.w3.org/2000/01/rdf-schema#domain>
                <http://www.gsi.dit.upm.es/ontologies/onyx/ns#EmotionAnalysis> ;
        <http://www.w3.org/2000/01/rdf-schema#isDefinedBy>
                "http://www.gsi.dit.upm.es/ontologies/onyx/ns" ;
        <http://www.w3.org/2000/01/rdf-schema#label>
                "source" .

<http://www.gsi.dit.upm.es/ontologies/onyx/ns#emotionText>
        a       <http://www.w3.org/2002/07/owl#DatatypeProperty> ;
        <http://www.w3.org/2000/01/rdf-schema#comment>
                "The exact text extract that expresses the emotion. This can be used when entity/text pointed by extractedFrom contains many emotions. \n\nFor example extractedFrom can point to a comment that contains many emotions about a movie, each emotion should have a separate onyx:Emotion and optionally an emotionText  property to indicate the specific text fragment of the comment."@en ;
        <http://www.w3.org/2000/01/rdf-schema#domain>
                <http://www.gsi.dit.upm.es/ontologies/onyx/ns#EmotionSet> ;
        <http://www.w3.org/2000/01/rdf-schema#isDefinedBy>
                "http://www.gsi.dit.upm.es/ontologies/onyx/ns" ;
        <http://www.w3.org/2000/01/rdf-schema#label>
                "emotionText"@en .

<http://www.gsi.dit.upm.es/ontologies/onyx/ns#hasAppraisal>
        a       <http://www.w3.org/2002/07/owl#ObjectProperty> ;
        <http://www.w3.org/2000/01/rdf-schema#comment>
                " Used to list the appraisals that a model defines" ;
        <http://www.w3.org/2000/01/rdf-schema#domain>
                <http://www.gsi.dit.upm.es/ontologies/onyx/ns#EmotionModel> ;
        <http://www.w3.org/2000/01/rdf-schema#isDefinedBy>
                "http://www.gsi.dit.upm.es/ontologies/onyx/ns" ;
        <http://www.w3.org/2000/01/rdf-schema#label>
                "hasAppraisal" ;
        <http://www.w3.org/2000/01/rdf-schema#range>
                <http://www.gsi.dit.upm.es/ontologies/onyx/ns#Appraisal> .

<http://www.gsi.dit.upm.es/ontologies/onyx/ns#Media>
        a       <http://www.w3.org/2002/07/owl#Class> ;
        <http://www.w3.org/2000/01/rdf-schema#comment>
                "Extends the NIF context to represent contexts with Multimedia. It is the equivalent of nif:String" ;
        <http://www.w3.org/2000/01/rdf-schema#isDefinedBy>
                "http://www.gsi.dit.upm.es/ontologies/onyx/ns" ;
        <http://www.w3.org/2000/01/rdf-schema#label>
                "MediaContext" ;
        <http://www.w3.org/2000/01/rdf-schema#subClassOf>
                <http://persistence.uni-leipzig.org/nlp2rdf/ontologies/nif-core#Context> .

<http://www.gsi.dit.upm.es/ontologies/onyx/ns#modelName>
        a       <http://www.w3.org/2002/07/owl#DatatypeProperty> ;
        <http://www.w3.org/2000/01/rdf-schema#comment>
                "Human readable name of the model" ;
        <http://www.w3.org/2000/01/rdf-schema#domain>
                <http://www.gsi.dit.upm.es/ontologies/onyx/ns#EmotionCategory> ;
        <http://www.w3.org/2000/01/rdf-schema#isDefinedBy>
                "http://www.gsi.dit.upm.es/ontologies/onyx/ns" ;
        <http://www.w3.org/2000/01/rdf-schema#label>
                "modelName" ;
        <http://www.w3.org/2000/01/rdf-schema#range>
                <http://www.w3.org/2001/XMLSchema#string> .

<http://www.gsi.dit.upm.es/ontologies/onyx/ns>
        a       <http://www.w3.org/2002/07/owl#Ontology> ;
        <http://www.w3.org/2000/01/rdf-schema#comment>
                "Onyx is an ontology designed to use for publishing the results of the emotion mining process in a form of structured data on the Web. The goal is to unify the access the numerical approximation of the emotion concept and allow extensive reasoning and search over multiple resources from different content providers."@en ;
        <http://www.w3.org/2000/01/rdf-schema#label>
                "Onyx Emotion Ontology"@en ;
        <http://www.w3.org/2000/01/rdf-schema#seeAlso>
                "http://www.gsi.dit.upm.es/ontologies/onyx" ;
        <http://purl.org/dc/terms/description>
                "Onyx is an ontology designed to use for publishing the results of the emotion mining process in a form of structured data on the Web. The goal is to unify the access the numerical approximation of the emotion concept and allow extensive reasoning and search over multiple resources from different content providers."@en ;
        <http://purl.org/vocab/vann/preferredNamespacePrefix>
                "onyx" ;
        <http://purl.org/vocab/vann/preferredNamespaceUri>
                "http://www.gsi.dit.upm.es/ontologies/onyx/ns#" ;
        <http://www.w3.org/2002/07/owl#imports>
                <http://www.w3.org/ns/prov-o#> ;
        <http://www.w3.org/2002/07/owl#priorVersion>
                "https://www.gsi.dit.upm.es/ontologies/onyx/1.4" ;
        <http://www.w3.org/2002/07/owl#versionInfo>
                "1.6" .

<http://www.gsi.dit.upm.es/ontologies/onyx/ns#aggregatesEmotionSet>
        a       <http://www.w3.org/2002/07/owl#ObjectProperty> ;
        <http://www.w3.org/2000/01/rdf-schema#comment>
                "Indicates that the emotions associated to this entity are a calculation (eg. average) of the emotions in other EmotionSets."@en ;
        <http://www.w3.org/2000/01/rdf-schema#domain>
                <http://www.gsi.dit.upm.es/ontologies/onyx/ns#AggregatedEmotionSet> ;
        <http://www.w3.org/2000/01/rdf-schema#isDefinedBy>
                "http://www.gsi.dit.upm.es/ontologies/onyx/ns" ;
        <http://www.w3.org/2000/01/rdf-schema#label>
                "aggregatesEmotionSet"@en ;
        <http://www.w3.org/2000/01/rdf-schema#range>
                <http://www.gsi.dit.upm.es/ontologies/onyx/ns#EmotionSet> .

<http://www.gsi.dit.upm.es/ontologies/onyx/ns#hasEmotionIntensity>
        a       <http://www.w3.org/2002/07/owl#DatatypeProperty> ;
        <http://www.w3.org/2000/01/rdf-schema#comment>
                "Value that quantifies the intensity of the emotion."@en ;
        <http://www.w3.org/2000/01/rdf-schema#domain>
                <http://www.gsi.dit.upm.es/ontologies/onyx/ns#Emotion> ;
        <http://www.w3.org/2000/01/rdf-schema#isDefinedBy>
                "http://www.gsi.dit.upm.es/ontologies/onyx/ns" ;
        <http://www.w3.org/2000/01/rdf-schema#label>
                "hasEmotionIntensity" ;
        <http://www.w3.org/2000/01/rdf-schema#range>
                <http://www.w3.org/2001/XMLSchema#float> .

<http://www.gsi.dit.upm.es/ontologies/onyx/ns#hasEmotionSet>
        a       <http://www.w3.org/2002/07/owl#ObjectProperty> ;
        <http://www.w3.org/2000/01/rdf-schema#comment>
                "Indicates that a certain text has a subjective set of emotions expressed in it."@en ;
        <http://www.w3.org/2000/01/rdf-schema#domain>
                <http://www.w3.org/2002/07/owl#Thing> ;
        <http://www.w3.org/2000/01/rdf-schema#isDefinedBy>
                "http://www.gsi.dit.upm.es/ontologies/onyx/ns" ;
        <http://www.w3.org/2000/01/rdf-schema#label>
                "hasEmotionSet"@en ;
        <http://www.w3.org/2000/01/rdf-schema#range>
                <http://www.gsi.dit.upm.es/ontologies/onyx/ns#EmotionSet> .

<http://www.gsi.dit.upm.es/ontologies/onyx/ns#domain>
        a       <http://www.w3.org/2002/07/owl#ObjectProperty> ;
        <http://www.w3.org/2000/01/rdf-schema#domain>
                <http://www.gsi.dit.upm.es/ontologies/onyx/ns#EmotionSet> ;
        <http://www.w3.org/2000/01/rdf-schema#isDefinedBy>
                "http://www.gsi.dit.upm.es/ontologies/onyx/ns" ;
        <http://www.w3.org/2000/01/rdf-schema#label>
                "domain" .

<http://www.gsi.dit.upm.es/ontologies/onyx/ns#hasEmotion>
        a       <http://www.w3.org/2002/07/owl#ObjectProperty> ;
        <http://www.w3.org/2000/01/rdf-schema#comment>
                "Used to express the individual emotions within an EmotionSet."@en ;
        <http://www.w3.org/2000/01/rdf-schema#domain>
                <http://www.gsi.dit.upm.es/ontologies/onyx/ns#EmotionSet> ;
        <http://www.w3.org/2000/01/rdf-schema#isDefinedBy>
                "http://www.gsi.dit.upm.es/ontologies/onyx/ns" ;
        <http://www.w3.org/2000/01/rdf-schema#label>
                "hasEmotion"@en ;
        <http://www.w3.org/2000/01/rdf-schema#range>
                <http://www.gsi.dit.upm.es/ontologies/onyx/ns#Emotion> .

<http://www.gsi.dit.upm.es/ontologies/onyx/ns#AggregatedEmotion>
        a       <http://www.w3.org/2002/07/owl#Class> ;
        <http://www.w3.org/2000/01/rdf-schema#comment>
                "The same as Emotion, used to aggregate several emotions"@en ;
        <http://www.w3.org/2000/01/rdf-schema#isDefinedBy>
                "http://www.gsi.dit.upm.es/ontologies/onyx/ns" ;
        <http://www.w3.org/2000/01/rdf-schema#label>
                "AggregatedEmotion" ;
        <http://www.w3.org/2000/01/rdf-schema#subClassOf>
                <http://www.gsi.dit.upm.es/ontologies/onyx/ns#Emotion> .

<http://www.gsi.dit.upm.es/ontologies/onyx/ns#hasActionTendency>
        a       <http://www.w3.org/2002/07/owl#ObjectProperty> ;
        <http://www.w3.org/2000/01/rdf-schema#comment>
                "Action tendency of the Emotion." ;
        <http://www.w3.org/2000/01/rdf-schema#domain>
                [ a       <http://www.w3.org/2002/07/owl#Class> ;
                  <http://www.w3.org/2002/07/owl#unionOf>
                          ( <http://www.gsi.dit.upm.es/ontologies/onyx/ns#EmotionModel> )
                ] ;
        <http://www.w3.org/2000/01/rdf-schema#isDefinedBy>
                "http://www.gsi.dit.upm.es/ontologies/onyx/ns" ;
        <http://www.w3.org/2000/01/rdf-schema#label>
                "hasActionTendency" ;
        <http://www.w3.org/2000/01/rdf-schema#range>
                <http://www.gsi.dit.upm.es/ontologies/onyx/ns#ActionTendency> .

<http://www.gsi.dit.upm.es/ontologies/onyx/ns#extractedFrom>
        a       <http://www.w3.org/2002/07/owl#ObjectProperty> ;
        <http://www.w3.org/2000/01/rdf-schema#comment>
                "Indicates the text from which the emotion has been extracted."@en ;
        <http://www.w3.org/2000/01/rdf-schema#domain>
                <http://www.gsi.dit.upm.es/ontologies/onyx/ns#EmotionSet> ;
        <http://www.w3.org/2000/01/rdf-schema#isDefinedBy>
                "http://www.gsi.dit.upm.es/ontologies/onyx/ns" ;
        <http://www.w3.org/2000/01/rdf-schema#label>
                "extractedFrom"@en ;
        <http://www.w3.org/2000/01/rdf-schema#range>
                <http://www.w3.org/2002/07/owl#Thing> ;
        <http://www.w3.org/2002/07/owl#inverseOf>
                <http://www.gsi.dit.upm.es/ontologies/onyx/ns#hasEmotionSet> .

<http://www.gsi.dit.upm.es/ontologies/onyx/ns#hasEmotionCategory>
        a       <http://www.w3.org/2002/07/owl#ObjectProperty> ;
        <http://www.w3.org/2000/01/rdf-schema#comment>
                "Value that represents the type of emotion."@en ;
        <http://www.w3.org/2000/01/rdf-schema#domain>
                [ a       <http://www.w3.org/2002/07/owl#Class> ;
                  <http://www.w3.org/2002/07/owl#unionOf>
                          ( <http://www.gsi.dit.upm.es/ontologies/onyx/ns#Emotion> <http://www.gsi.dit.upm.es/ontologies/onyx/ns#EmotionModel> )
                ] ;
        <http://www.w3.org/2000/01/rdf-schema#isDefinedBy>
                "http://www.gsi.dit.upm.es/ontologies/onyx/ns" ;
        <http://www.w3.org/2000/01/rdf-schema#label>
                "hasEmotionCategory" ;
        <http://www.w3.org/2000/01/rdf-schema#range>
                <http://www.gsi.dit.upm.es/ontologies/onyx/ns#EmotionCategory> .

<http://www.gsi.dit.upm.es/ontologies/onyx/ns#AggregatedEmotionSet>
        a       <http://www.w3.org/2002/07/owl#Class> ;
        <http://www.w3.org/2000/01/rdf-schema#comment>
                "The same as the EmotionSet class but indicates that the properties of this class aggregate all the emotions detected in the \"extractedFrom\" source. If the aggregatesEmotionSet property is used this class could be created to aggregate only certain emotions."@en ;
        <http://www.w3.org/2000/01/rdf-schema#isDefinedBy>
                "http://www.gsi.dit.upm.es/ontologies/onyx/ns" ;
        <http://www.w3.org/2000/01/rdf-schema#label>
                "AggregatedEmotionSet"@en ;
        <http://www.w3.org/2000/01/rdf-schema#subClassOf>
                <http://www.gsi.dit.upm.es/ontologies/onyx/ns#EmotionSet> .

<http://www.gsi.dit.upm.es/ontologies/onyx/ns#aggregatesEmotion>
        a       <http://www.w3.org/2002/07/owl#ObjectProperty> ;
        <http://www.w3.org/2000/01/rdf-schema#comment>
                "Indicates that the AggregatedEmotion has been derived from other Emotions."@en ;
        <http://www.w3.org/2000/01/rdf-schema#domain>
                <http://www.gsi.dit.upm.es/ontologies/onyx/ns#AggregatedEmotion> ;
        <http://www.w3.org/2000/01/rdf-schema#isDefinedBy>
                "http://www.gsi.dit.upm.es/ontologies/onyx/ns" ;
        <http://www.w3.org/2000/01/rdf-schema#label>
                "aggregatesEmotion"@en ;
        <http://www.w3.org/2000/01/rdf-schema#range>
                <http://www.gsi.dit.upm.es/ontologies/onyx/ns#Emotion> .

<http://www.gsi.dit.upm.es/ontologies/onyx/ns#Emotion>
        a       <http://www.w3.org/2002/07/owl#Class> ;
        <http://www.w3.org/2000/01/rdf-schema#comment>
                "Class that represents emotions in a generic way"@en ;
        <http://www.w3.org/2000/01/rdf-schema#isDefinedBy>
                "http://www.gsi.dit.upm.es/ontologies/onyx/ns" ;
        <http://www.w3.org/2000/01/rdf-schema#label>
                "Emotion" .

<http://www.gsi.dit.upm.es/ontologies/onyx/ns#sourceText>
        a       <http://www.w3.org/2002/07/owl#DatatypeProperty> ;
        <http://www.w3.org/2000/01/rdf-schema#comment>
                "Optional value that contains the text from which the emotionText was taken." ;
        <http://www.w3.org/2000/01/rdf-schema#isDefinedBy>
                "http://www.gsi.dit.upm.es/ontologies/onyx/ns" ;
        <http://www.w3.org/2000/01/rdf-schema#label>
                "sourceText" .

<http://www.gsi.dit.upm.es/ontologies/onyx/ns#EmotionAnalysis>
        a       <http://www.w3.org/2002/07/owl#Class> ;
        <http://www.w3.org/2000/01/rdf-schema#comment>
                "The action of analysing the sentiment in an entity. It produces an onyx:emotion"@en ;
        <http://www.w3.org/2000/01/rdf-schema#isDefinedBy>
                "http://www.gsi.dit.upm.es/ontologies/onyx/ns" ;
        <http://www.w3.org/2000/01/rdf-schema#label>
                "EmotionAnalysis" ;
        <http://www.w3.org/2000/01/rdf-schema#subClassOf>
                <http://www.w3.org/ns/prov#Activity> .

<http://www.gsi.dit.upm.es/ontologies/onyx/ns#algorithmConfidence>
        a       <http://www.w3.org/2002/07/owl#DatatypeProperty> ;
        <http://www.w3.org/2000/01/rdf-schema#comment>
                "A numerical value that represents the accuracy of result as estimated by the algorithm itself (how much the emotion matches a gives object/product)."@en ;
        <http://www.w3.org/2000/01/rdf-schema#domain>
                <http://www.gsi.dit.upm.es/ontologies/onyx/ns#Emotion> ;
        <http://www.w3.org/2000/01/rdf-schema#isDefinedBy>
                "http://www.gsi.dit.upm.es/ontologies/onyx/ns" ;
        <http://www.w3.org/2000/01/rdf-schema#label>
                "algorithmConfidence"@en ;
        <http://www.w3.org/2000/01/rdf-schema#range>
                <http://www.w3.org/2001/XMLSchema#float> .

<http://www.gsi.dit.upm.es/ontologies/onyx/ns#usesEmotionModel>
        a       <http://www.w3.org/2002/07/owl#ObjectProperty> ;
        <http://www.w3.org/2000/01/rdf-schema#comment>
                "Specifies the Emotion Model used. Mainly used to describe Emotion Analysis activities."@en ;
        <http://www.w3.org/2000/01/rdf-schema#isDefinedBy>
                "http://www.gsi.dit.upm.es/ontologies/onyx/ns" ;
        <http://www.w3.org/2000/01/rdf-schema#label>
                "usesEmotionModel" ;
        <http://www.w3.org/2000/01/rdf-schema#range>
                <http://www.gsi.dit.upm.es/ontologies/onyx/ns#EmotionModel> .

<http://www.gsi.dit.upm.es/ontologies/onyx/ns#Appraisal>
        a       <http://www.w3.org/2002/07/owl#DatatypeProperty> ;
        <http://www.w3.org/2000/01/rdf-schema#comment>
                "Parent for Appraisal properties." ;
        <http://www.w3.org/2000/01/rdf-schema#isDefinedBy>
                "http://www.gsi.dit.upm.es/ontologies/onyx/ns" ;
        <http://www.w3.org/2000/01/rdf-schema#label>
                "Appraisal" .

<http://www.gsi.dit.upm.es/ontologies/onyx/ns#EmotionCategory>
        a       <http://www.w3.org/2002/07/owl#Class> ;
        <http://www.w3.org/2000/01/rdf-schema#comment>
                "Class that represents an emotion category (anger, happiness, etc.)" ;
        <http://www.w3.org/2000/01/rdf-schema#isDefinedBy>
                "http://www.gsi.dit.upm.es/ontologies/onyx/ns" ;
        <http://www.w3.org/2000/01/rdf-schema#label>
                "EmotionCategory" .

<http://www.gsi.dit.upm.es/ontologies/onyx/ns#EmotionModel>
        a       <http://www.w3.org/2002/07/owl#Class> ;
        <http://www.w3.org/2000/01/rdf-schema#comment>
                "Represents an Emotion Representation Model, grouping its categories, dimensions, properties..." ;
        <http://www.w3.org/2000/01/rdf-schema#isDefinedBy>
                "http://www.gsi.dit.upm.es/ontologies/onyx/ns" ;
        <http://www.w3.org/2000/01/rdf-schema#label>
                "EmotionModel" .

<http://www.gsi.dit.upm.es/ontologies/onyx/ns#EmotionSet>
        a       <http://www.w3.org/2002/07/owl#Class> ;
        <http://www.w3.org/2000/01/rdf-schema#comment>
                "Describes the concept of emotion expressed in a certain text."@en ;
        <http://www.w3.org/2000/01/rdf-schema#isDefinedBy>
                "http://www.gsi.dit.upm.es/ontologies/onyx/ns" ;
        <http://www.w3.org/2000/01/rdf-schema#label>
                "EmotionSet"@en ;
        <http://www.w3.org/2000/01/rdf-schema#subClassOf>
                <http://www.w3.org/ns/prov#Entity> ;
        <http://www.w3.org/2002/07/owl#disjointWith>
                <http://www.w3.org/ns/prov#Collection> , <http://www.w3.org/ns/prov#Bundle> , <http://www.w3.org/ns/prov#Plan> .

<http://www.gsi.dit.upm.es/ontologies/onyx/ns#algorithm>
        a       <http://www.w3.org/2002/07/owl#ObjectProperty> ;
        <http://www.w3.org/2000/01/rdf-schema#comment>
                "The algorithm used in the Sentiment Analysis."@en ;
        <http://www.w3.org/2000/01/rdf-schema#domain>
                <http://www.gsi.dit.upm.es/ontologies/onyx/ns#EmotionAnalysis> ;
        <http://www.w3.org/2000/01/rdf-schema#isDefinedBy>
                "http://www.gsi.dit.upm.es/ontologies/onyx/ns" ;
        <http://www.w3.org/2000/01/rdf-schema#label>
                "algorithm" .
