<http://www.openlinksw.com/data/turtle/logging.ttl>
        a                            <http://schema.org/TechArticle> , <http://xmlns.com/foaf/0.1/Document> ;
        <http://www.w3.org/2000/01/rdf-schema#comment>
                "This is a turtle document that uses Linked Data oriented content to describe an OpenLink ontology for Logging and Errors."@en ;
        <http://www.w3.org/2000/01/rdf-schema#label>
                "OpenLink Logging Ontology Description Document (Turtle)" ;
        <http://creativecommons.org/ns#license>
                <http://creativecommons.org/licenses/by-sa/3.0/> ;
        <http://purl.org/dc/terms/created>
                "2014-05-18T13:00:00-05:00"^^<http://www.w3.org/2001/XMLSchema#dateTime> ;
        <http://purl.org/dc/terms/modified>
                "2015-03-20T13:38:00-05:00"^^<http://www.w3.org/2001/XMLSchema#dateTime> ;
        <http://purl.org/dc/terms/subject>
                <http://www.openlinksw.com/ontology/logging#> ;
        <http://schema.org/about>    <http://www.openlinksw.com/ontology/logging#> ;
        <http://schema.org/creator>  <http://www.openlinksw.com/#this> ;
        <http://www.w3.org/1999/xhtml/vocab#canonical>
                <http://www.openlinksw.com/ontology/logging> ;
        <http://www.w3.org/1999/xhtml/vocab#describes>
                <http://www.openlinksw.com/ontology/logging#> ;
        <http://xmlns.com/foaf/0.1/primaryTopic>
                <http://www.openlinksw.com/ontology/logging#> .

<http://www.openlinksw.com/ontology/logging>
        a                            <http://schema.org/TechArticle> , <http://xmlns.com/foaf/0.1/Document> ;
        <http://www.w3.org/2000/01/rdf-schema#comment>
                "This is a document that uses Linked Data oriented content to describe OpenLink Logging Ontology."@en ;
        <http://www.w3.org/2000/01/rdf-schema#label>
                "OpenLink Logging Ontology Description Document" ;
        <http://creativecommons.org/ns#license>
                <http://creativecommons.org/licenses/by-sa/3.0/> ;
        <http://purl.org/dc/terms/created>
                "2014-05-18T13:00:00-05:00"^^<http://www.w3.org/2001/XMLSchema#dateTime> ;
        <http://purl.org/dc/terms/modified>
                "2015-03-20T13:38:00-05:00"^^<http://www.w3.org/2001/XMLSchema#dateTime> ;
        <http://purl.org/dc/terms/subject>
                <http://www.openlinksw.com/ontology/logging#> ;
        <http://schema.org/creator>  <http://www.openlinksw.com/#this> ;
        <http://xmlns.com/foaf/0.1/primaryTopic>
                <http://www.openlinksw.com/ontology/logging#> ;
        <http://xmlns.com/foaf/0.1/topic>
                <http://www.openlinksw.com/ontology/logging#GraphStorageAction> , <http://www.openlinksw.com/ontology/logging#matchesLogEntryType> , <http://www.openlinksw.com/ontology/logging#hasTriggeringApplication> , <http://www.openlinksw.com/ontology/logging#LogFileAction> , <http://www.openlinksw.com/ontology/logging#hasTimestamp> , <http://www.openlinksw.com/ontology/logging#LogPattern> , <http://www.openlinksw.com/ontology/logging#hasRequestedUrl> , <http://www.openlinksw.com/ontology/logging#HttpContextError> , <http://www.openlinksw.com/ontology/logging#VirtuosoDebugAction> , <http://www.openlinksw.com/ontology/logging#ReplacementErrorAction> , <http://www.openlinksw.com/ontology/logging#DebugMessage> , <http://www.openlinksw.com/ontology/logging#Error> , <http://www.openlinksw.com/ontology/logging#hasPriorityLevel> , <http://www.openlinksw.com/ontology/logging#LogEntry> , <http://www.openlinksw.com/ontology/logging#hasErrorCode> , <http://www.openlinksw.com/ontology/logging#hasLogMessagePattern> , <http://www.openlinksw.com/ontology/logging#LogAction> , <http://www.openlinksw.com/ontology/logging#InfoMessage> , <http://www.openlinksw.com/ontology/logging#hasReplacementErrorMessage> , <http://www.openlinksw.com/ontology/logging#hasContext> , <http://www.openlinksw.com/ontology/logging#hasStorageGraph> , <http://www.openlinksw.com/ontology/logging#VirtuosoLogSystemAction> , <http://www.openlinksw.com/ontology/logging#hasLogMessage> , <http://www.openlinksw.com/ontology/logging#hasLogAction> , <http://www.openlinksw.com/ontology/logging#hasReplacementErrorMessageParamsPattern> , <http://www.openlinksw.com/ontology/logging#hasOwningApplication> , <http://www.openlinksw.com/ontology/logging#hasErrorCodePattern> , <http://www.openlinksw.com/ontology/logging#LogHandler> , <http://www.openlinksw.com/ontology/logging#hasEntrySeparator> , <http://www.openlinksw.com/ontology/logging#hasResourceNamespace> , <http://www.openlinksw.com/ontology/logging#EmailLogAction> , <http://www.openlinksw.com/ontology/logging#hasEmailRecipient> , <http://www.openlinksw.com/ontology/logging#hasLogPattern> , <http://www.openlinksw.com/ontology/logging#hasEmailSender> , <http://www.openlinksw.com/ontology/logging#hasAffectedUser> , <http://www.openlinksw.com/ontology/logging#hasReplacementErrorCode> .

<http://www.openlinksw.com/ontology/logging#hasEntrySeparator>
        a       <http://www.w3.org/1999/02/22-rdf-syntax-ns#Property> , <http://www.w3.org/2002/07/owl#DatatypeProperty> ;
        <http://www.w3.org/2000/01/rdf-schema#comment>
                "An optional string which will be written between each log file entry."@en ;
        <http://www.w3.org/2000/01/rdf-schema#domain>
                <http://www.openlinksw.com/ontology/logging#LogFileAction> ;
        <http://www.w3.org/2000/01/rdf-schema#isDefinedBy>
                <http://www.openlinksw.com/ontology/logging#> ;
        <http://www.w3.org/2000/01/rdf-schema#label>
                "hasEntrySeparator" ;
        <http://www.w3.org/2000/01/rdf-schema#range>
                <http://www.w3.org/2001/XMLSchema#string> ;
        <http://www.w3.org/2004/02/skos/core#altLabel>
                "Log Entry Separator" .

<http://www.openlinksw.com/ontology/logging#hasResourceNamespace>
        a       <http://www.w3.org/1999/02/22-rdf-syntax-ns#Property> , <http://www.w3.org/2002/07/owl#DatatypeProperty> ;
        <http://www.w3.org/2000/01/rdf-schema#comment>
                "When logging errors into a named graph new error resource URIs will be generated using this namespace."@en ;
        <http://www.w3.org/2000/01/rdf-schema#domain>
                <http://www.openlinksw.com/ontology/logging#GraphStorageAction> ;
        <http://www.w3.org/2000/01/rdf-schema#isDefinedBy>
                <http://www.openlinksw.com/ontology/logging#> ;
        <http://www.w3.org/2000/01/rdf-schema#label>
                "hasResourceNamespace" ;
        <http://www.w3.org/2000/01/rdf-schema#range>
                <http://www.w3.org/2001/XMLSchema#string> ;
        <http://www.w3.org/2004/02/skos/core#altLabel>
                "Resource Namespace" .

<http://www.openlinksw.com/ontology/logging#DebugMessage>
        a       <http://www.w3.org/2002/07/owl#Class> ;
        <http://www.w3.org/2000/01/rdf-schema#comment>
                "A debug message created by an application."@en ;
        <http://www.w3.org/2000/01/rdf-schema#isDefinedBy>
                <http://www.openlinksw.com/ontology/logging#> ;
        <http://www.w3.org/2000/01/rdf-schema#label>
                "DebugMessage" ;
        <http://www.w3.org/2000/01/rdf-schema#subClassOf>
                <http://www.openlinksw.com/ontology/logging#LogEntry> ;
        <http://www.w3.org/2004/02/skos/core#altLabel>
                "Debug Message" .

<http://www.openlinksw.com/ontology/logging#>
        a                            <http://www.w3.org/2002/07/owl#Ontology> ;
        <http://www.w3.org/2000/01/rdf-schema#comment>
                "Ontology that defines entity and relation types used to describe log messages, errors and log/error handlers."@en ;
        <http://www.w3.org/2000/01/rdf-schema#label>
                "OpenLink Logging Ontology" ;
        <http://open.vocab.org/terms/defines>
                <http://www.openlinksw.com/ontology/logging#hasTimestamp> , <http://www.openlinksw.com/ontology/logging#GraphStorageAction> , <http://www.openlinksw.com/ontology/logging#matchesLogEntryType> , <http://www.openlinksw.com/ontology/logging#hasTriggeringApplication> , <http://www.openlinksw.com/ontology/logging#LogFileAction> , <http://www.openlinksw.com/ontology/logging#LogAction> , <http://www.openlinksw.com/ontology/logging#InfoMessage> , <http://www.openlinksw.com/ontology/logging#hasErrorCode> , <http://www.openlinksw.com/ontology/logging#hasLogMessagePattern> , <http://www.openlinksw.com/ontology/logging#hasReplacementErrorMessage> , <http://www.openlinksw.com/ontology/logging#VirtuosoDebugAction> , <http://www.openlinksw.com/ontology/logging#ReplacementErrorAction> , <http://www.openlinksw.com/ontology/logging#hasRequestedUrl> , <http://www.openlinksw.com/ontology/logging#LogPattern> , <http://www.openlinksw.com/ontology/logging#HttpContextError> , <http://www.openlinksw.com/ontology/logging#LogEntry> , <http://www.openlinksw.com/ontology/logging#DebugMessage> , <http://www.openlinksw.com/ontology/logging#Error> , <http://www.openlinksw.com/ontology/logging#hasPriorityLevel> , <http://www.openlinksw.com/ontology/logging#hasLogMessage> , <http://www.openlinksw.com/ontology/logging#hasReplacementErrorMessageParamsPattern> , <http://www.openlinksw.com/ontology/logging#hasLogAction> , <http://www.openlinksw.com/ontology/logging#VirtuosoLogSystemAction> , <http://www.openlinksw.com/ontology/logging#hasContext> , <http://www.openlinksw.com/ontology/logging#hasStorageGraph> , <http://www.openlinksw.com/ontology/logging#hasLogPattern> , <http://www.openlinksw.com/ontology/logging#hasEmailSender> , <http://www.openlinksw.com/ontology/logging#hasEmailRecipient> , <http://www.openlinksw.com/ontology/logging#EmailLogAction> , <http://www.openlinksw.com/ontology/logging#hasEntrySeparator> , <http://www.openlinksw.com/ontology/logging#hasResourceNamespace> , <http://www.openlinksw.com/ontology/logging#hasReplacementErrorCode> , <http://www.openlinksw.com/ontology/logging#hasAffectedUser> , <http://www.openlinksw.com/ontology/logging#hasErrorCodePattern> , <http://www.openlinksw.com/ontology/logging#hasOwningApplication> , <http://www.openlinksw.com/ontology/logging#LogHandler> ;
        <http://purl.org/dc/terms/created>
                "2014-05-18T13:00:00-05:00"^^<http://www.w3.org/2001/XMLSchema#dateTime> ;
        <http://purl.org/dc/terms/modified>
                "2015-03-20T13:38:00-05:00"^^<http://www.w3.org/2001/XMLSchema#dateTime> ;
        <http://schema.org/about>    <http://www.openlinksw.com/ontology/logging#hasPriorityLevel> , <http://www.openlinksw.com/ontology/logging#DebugMessage> , <http://www.openlinksw.com/ontology/logging#Error> , <http://www.openlinksw.com/ontology/logging#LogEntry> , <http://www.openlinksw.com/ontology/logging#HttpContextError> , <http://www.openlinksw.com/ontology/logging#LogPattern> , <http://www.openlinksw.com/ontology/logging#hasRequestedUrl> , <http://www.openlinksw.com/ontology/logging#ReplacementErrorAction> , <http://www.openlinksw.com/ontology/logging#VirtuosoDebugAction> , <http://www.openlinksw.com/ontology/logging#hasReplacementErrorMessage> , <http://www.openlinksw.com/ontology/logging#hasLogMessagePattern> , <http://www.openlinksw.com/ontology/logging#hasErrorCode> , <http://www.openlinksw.com/ontology/logging#InfoMessage> , <http://www.openlinksw.com/ontology/logging#LogAction> , <http://www.openlinksw.com/ontology/logging#LogFileAction> , <http://www.openlinksw.com/ontology/logging#hasTriggeringApplication> , <http://www.openlinksw.com/ontology/logging#matchesLogEntryType> , <http://www.openlinksw.com/ontology/logging#GraphStorageAction> , <http://www.openlinksw.com/ontology/logging#hasTimestamp> , <http://www.openlinksw.com/ontology/logging#LogHandler> , <http://www.openlinksw.com/ontology/logging#hasOwningApplication> , <http://www.openlinksw.com/ontology/logging#hasErrorCodePattern> , <http://www.openlinksw.com/ontology/logging#hasAffectedUser> , <http://www.openlinksw.com/ontology/logging#hasReplacementErrorCode> , <http://www.openlinksw.com/ontology/logging#hasEntrySeparator> , <http://www.openlinksw.com/ontology/logging#hasResourceNamespace> , <http://www.openlinksw.com/ontology/logging#EmailLogAction> , <http://www.openlinksw.com/ontology/logging#hasEmailRecipient> , <http://www.openlinksw.com/ontology/logging#hasLogPattern> , <http://www.openlinksw.com/ontology/logging#hasEmailSender> , <http://www.openlinksw.com/ontology/logging#hasStorageGraph> , <http://www.openlinksw.com/ontology/logging#hasContext> , <http://www.openlinksw.com/ontology/logging#VirtuosoLogSystemAction> , <http://www.openlinksw.com/ontology/logging#hasLogAction> , <http://www.openlinksw.com/ontology/logging#hasReplacementErrorMessageParamsPattern> , <http://www.openlinksw.com/ontology/logging#hasLogMessage> ;
        <http://schema.org/creator>  <http://www.openlinksw.com/#this> ;
        <http://www.w3.org/2002/07/owl#imports>
                <http://www.w3.org/1999/02/22-rdf-syntax-ns#> , <http://purl.org/dc/terms/> , <http://xmlns.com/foaf/0.1/> , <http://www.w3.org/2002/07/owl#> ;
        <http://www.w3.org/2002/07/owl#versionInfo>
                "1.1.0" ;
        <http://www.w3.org/2007/05/powder-s#describedby>
                <http://www.openlinksw.com/ontology/logging> .

<http://www.openlinksw.com/DAV/data/turtle/logging.ttl>
        a                            <http://www.w3.org/ns/ldp#Resource> , <http://www.w3.org/2000/01/rdf-schema#Resource> , <http://schema.org/TechArticle> , <http://xmlns.com/foaf/0.1/Document> ;
        <http://www.w3.org/2000/01/rdf-schema#comment>
                "This is a turtle document that uses Linked Data oriented content to describe an OpenLink ontology for Logging and Errors."@en ;
        <http://www.w3.org/2000/01/rdf-schema#label>
                "OpenLink Logging Ontology Description Document (Turtle)" ;
        <http://creativecommons.org/ns#license>
                <http://creativecommons.org/licenses/by-sa/3.0/> ;
        <http://purl.org/dc/terms/created>
                "2014-05-18T13:00:00-05:00"^^<http://www.w3.org/2001/XMLSchema#dateTime> ;
        <http://purl.org/dc/terms/modified>
                "2015-03-20T13:38:00-05:00"^^<http://www.w3.org/2001/XMLSchema#dateTime> ;
        <http://purl.org/dc/terms/subject>
                <http://www.openlinksw.com/ontology/logging#> ;
        <http://schema.org/about>    <http://www.openlinksw.com/ontology/logging#> ;
        <http://schema.org/creator>  <http://www.openlinksw.com/#this> ;
        <http://www.w3.org/1999/xhtml/vocab#canonical>
                <http://www.openlinksw.com/ontology/logging> ;
        <http://www.w3.org/1999/xhtml/vocab#describes>
                <http://www.openlinksw.com/ontology/logging#> ;
        <http://xmlns.com/foaf/0.1/primaryTopic>
                <http://www.openlinksw.com/ontology/logging#> .

<http://www.openlinksw.com/ontology/logging#VirtuosoLogSystemAction>
        a       <http://www.w3.org/2002/07/owl#Class> ;
        <http://www.w3.org/2000/01/rdf-schema#comment>
                "A Virtuoso Log System action does use the internal Virtuoso logging to create\r\n    a log message."@en ;
        <http://www.w3.org/2000/01/rdf-schema#isDefinedBy>
                <http://www.openlinksw.com/ontology/logging#> ;
        <http://www.w3.org/2000/01/rdf-schema#label>
                "VirtuosoLogSystemAction" ;
        <http://www.w3.org/2000/01/rdf-schema#subClassOf>
                <http://www.openlinksw.com/ontology/logging#LogAction> ;
        <http://www.w3.org/2004/02/skos/core#altLabel>
                "Virtuoso Log System Action" .

<http://www.openlinksw.com/ontology/logging#VirtuosoDebugAction>
        a       <http://www.w3.org/2002/07/owl#Class> ;
        <http://www.w3.org/2000/01/rdf-schema#comment>
                "A Virtuoso Debug action does use dbg_printf to create\r\n    a debugging message."@en ;
        <http://www.w3.org/2000/01/rdf-schema#isDefinedBy>
                <http://www.openlinksw.com/ontology/logging#> ;
        <http://www.w3.org/2000/01/rdf-schema#label>
                "VirtuosoDebugAction" ;
        <http://www.w3.org/2000/01/rdf-schema#subClassOf>
                <http://www.openlinksw.com/ontology/logging#LogAction> ;
        <http://www.w3.org/2004/02/skos/core#altLabel>
                "Virtuoso Debug Action" .

<http://www.openlinksw.com/ontology/logging#hasErrorCodePattern>
        a       <http://www.w3.org/1999/02/22-rdf-syntax-ns#Property> , <http://www.w3.org/2002/07/owl#DatatypeProperty> ;
        <http://www.w3.org/2000/01/rdf-schema#comment>
                "A regular expression to match error codes that should be handled by the owning ErrorHandler."@en ;
        <http://www.w3.org/2000/01/rdf-schema#domain>
                <http://www.openlinksw.com/ontology/logging#LogPattern> ;
        <http://www.w3.org/2000/01/rdf-schema#isDefinedBy>
                <http://www.openlinksw.com/ontology/logging#> ;
        <http://www.w3.org/2000/01/rdf-schema#label>
                "hasErrorCodePattern" ;
        <http://www.w3.org/2000/01/rdf-schema#range>
                <http://www.w3.org/2001/XMLSchema#string> ;
        <http://www.w3.org/2004/02/skos/core#altLabel>
                "Error Code Pattern" .

<http://www.openlinksw.com/ontology/logging#hasLogFilePath>
        a       <http://www.w3.org/1999/02/22-rdf-syntax-ns#Property> , <http://www.w3.org/2002/07/owl#DatatypeProperty> ;
        <http://www.w3.org/2000/01/rdf-schema#comment>
                "The path of the file (typically relative to the Virtuoso instance directory) into which the errors\r\n    should be logged."@en ;
        <http://www.w3.org/2000/01/rdf-schema#domain>
                <http://www.openlinksw.com/ontology/logging#LogFileAction> ;
        <http://www.w3.org/2000/01/rdf-schema#isDefinedBy>
                <http://www.openlinksw.com/ontology/logging#> ;
        <http://www.w3.org/2000/01/rdf-schema#label>
                "hasLogFilePath" ;
        <http://www.w3.org/2000/01/rdf-schema#range>
                <http://www.w3.org/2001/XMLSchema#string> ;
        <http://www.w3.org/2004/02/skos/core#altLabel>
                "Log File Path" .

<http://www.openlinksw.com/ontology/logging#ReplacementErrorAction>
        a       <http://www.w3.org/2002/07/owl#Class> ;
        <http://www.w3.org/2000/01/rdf-schema#comment>
                "A Replacement Error Action will trigger a replacement error for the trapped error.\r\n    This is useful for user-facing UIs which do not want to expose internal details but simply\r\n    show a generic error message telling the user that the problem will be taken care of."@en ;
        <http://www.w3.org/2000/01/rdf-schema#isDefinedBy>
                <http://www.openlinksw.com/ontology/logging#> ;
        <http://www.w3.org/2000/01/rdf-schema#label>
                "ReplacementErrorAction" ;
        <http://www.w3.org/2000/01/rdf-schema#subClassOf>
                <http://www.openlinksw.com/ontology/logging#LogAction> ;
        <http://www.w3.org/2004/02/skos/core#altLabel>
                "Replacement Error Action" .

<http://www.openlinksw.com/ontology/logging#GraphStorageAction>
        a       <http://www.w3.org/2002/07/owl#Class> ;
        <http://www.w3.org/2000/01/rdf-schema#comment>
                "A Graph Storage Log Action will store the entry in a named graph for logging\r\n    purposes."@en ;
        <http://www.w3.org/2000/01/rdf-schema#isDefinedBy>
                <http://www.openlinksw.com/ontology/logging#> ;
        <http://www.w3.org/2000/01/rdf-schema#label>
                "GraphStorageAction" ;
        <http://www.w3.org/2000/01/rdf-schema#subClassOf>
                <http://www.openlinksw.com/ontology/logging#LogAction> ;
        <http://www.w3.org/2004/02/skos/core#altLabel>
                "Graph Storage Action" .

<http://www.openlinksw.com/ontology/logging#hasRequestedUrl>
        a       <http://www.w3.org/2002/07/owl#ObjectProperty> , <http://www.w3.org/1999/02/22-rdf-syntax-ns#Property> ;
        <http://www.w3.org/2000/01/rdf-schema#comment>
                "The requested URL of the HTTP context in which the error was thrown."@en ;
        <http://www.w3.org/2000/01/rdf-schema#domain>
                <http://www.openlinksw.com/ontology/logging#HttpContextError> ;
        <http://www.w3.org/2000/01/rdf-schema#isDefinedBy>
                <http://www.openlinksw.com/ontology/logging#> ;
        <http://www.w3.org/2000/01/rdf-schema#label>
                "hasRequestedUrl" ;
        <http://www.w3.org/2000/01/rdf-schema#range>
                <http://www.w3.org/2000/01/rdf-schema#Resource> ;
        <http://www.w3.org/2004/02/skos/core#altLabel>
                "Requested URL" .

<http://www.openlinksw.com/ontology/logging#hasLogMessage>
        a       <http://www.w3.org/1999/02/22-rdf-syntax-ns#Property> , <http://www.w3.org/2002/07/owl#DatatypeProperty> ;
        <http://www.w3.org/2000/01/rdf-schema#comment>
                "The Log Message. Typically a human-readable description of the log entry."@en ;
        <http://www.w3.org/2000/01/rdf-schema#domain>
                <http://www.openlinksw.com/ontology/logging#LogEntry> ;
        <http://www.w3.org/2000/01/rdf-schema#isDefinedBy>
                <http://www.openlinksw.com/ontology/logging#> ;
        <http://www.w3.org/2000/01/rdf-schema#label>
                "hasLogMessage" ;
        <http://www.w3.org/2000/01/rdf-schema#range>
                <http://www.w3.org/2001/XMLSchema#string> ;
        <http://www.w3.org/2004/02/skos/core#altLabel>
                "Log Message" .

<http://www.openlinksw.com/ontology/logging#hasReplacementErrorMessage>
        a       <http://www.w3.org/2002/07/owl#DatatypeProperty> , <http://www.w3.org/1999/02/22-rdf-syntax-ns#Property> ;
        <http://www.w3.org/2000/01/rdf-schema#comment>
                "The error message the replacement error should contain. The replacement error\r\n    message can contain parameter markers @1, @2 ... (not necessarily contiguous) to be replaced by subexpression matches\r\n    returned by a regex identified by the hasReplacementErrorMessageParamsPattern property."@en ;
        <http://www.w3.org/2000/01/rdf-schema#domain>
                <http://www.openlinksw.com/ontology/logging#ReplacementErrorAction> ;
        <http://www.w3.org/2000/01/rdf-schema#isDefinedBy>
                <http://www.openlinksw.com/ontology/logging#> ;
        <http://www.w3.org/2000/01/rdf-schema#label>
                "hasReplacementErrorMessage" ;
        <http://www.w3.org/2000/01/rdf-schema#range>
                <http://www.w3.org/2001/XMLSchema#string> ;
        <http://www.w3.org/2004/02/skos/core#altLabel>
                "Replacement Error Message" .

<http://www.openlinksw.com/ontology/logging#hasErrorCode>
        a       <http://www.w3.org/2002/07/owl#DatatypeProperty> , <http://www.w3.org/1999/02/22-rdf-syntax-ns#Property> ;
        <http://www.w3.org/2000/01/rdf-schema#comment>
                "The Error Code. Typically a short internal machine-readable identifier for the error type."@en ;
        <http://www.w3.org/2000/01/rdf-schema#domain>
                <http://www.openlinksw.com/ontology/logging#Error> ;
        <http://www.w3.org/2000/01/rdf-schema#isDefinedBy>
                <http://www.openlinksw.com/ontology/logging#> ;
        <http://www.w3.org/2000/01/rdf-schema#label>
                "hasErrorCode" ;
        <http://www.w3.org/2000/01/rdf-schema#range>
                <http://www.w3.org/2001/XMLSchema#string> ;
        <http://www.w3.org/2004/02/skos/core#altLabel>
                "Error Code" .

<http://www.openlinksw.com/ontology/logging#hasReplacementErrorMessageParamsPattern>
        a       <http://www.w3.org/1999/02/22-rdf-syntax-ns#Property> , <http://www.w3.org/2002/07/owl#DatatypeProperty> ;
        <http://www.w3.org/2000/01/rdf-schema#comment>
                "A regular expression returning portions of the original error message as\r\n    subexpression matches to be inserted into the replacement error message in place of\r\n    parameter markers"@en ;
        <http://www.w3.org/2000/01/rdf-schema#domain>
                <http://www.openlinksw.com/ontology/logging#ReplacementErrorAction> ;
        <http://www.w3.org/2000/01/rdf-schema#isDefinedBy>
                <http://www.openlinksw.com/ontology/logging#> ;
        <http://www.w3.org/2000/01/rdf-schema#label>
                "hasReplacementErrorMessageParamsPattern" ;
        <http://www.w3.org/2000/01/rdf-schema#range>
                <http://www.w3.org/2001/XMLSchema#string> ;
        <http://www.w3.org/2004/02/skos/core#altLabel>
                "Replacement Error Message Params Pattern" .

<http://www.openlinksw.com/ontology/logging#LogFileAction>
        a       <http://www.w3.org/2002/07/owl#Class> ;
        <http://www.w3.org/2000/01/rdf-schema#comment>
                "A log file action does write into a given log file."@en ;
        <http://www.w3.org/2000/01/rdf-schema#isDefinedBy>
                <http://www.openlinksw.com/ontology/logging#> ;
        <http://www.w3.org/2000/01/rdf-schema#label>
                "LogFileAction" ;
        <http://www.w3.org/2000/01/rdf-schema#subClassOf>
                <http://www.openlinksw.com/ontology/logging#LogAction> ;
        <http://www.w3.org/2004/02/skos/core#altLabel>
                "Log File Action" .

<http://www.openlinksw.com/ontology/logging#hasLogAction>
        a       <http://www.w3.org/1999/02/22-rdf-syntax-ns#Property> , <http://www.w3.org/2002/07/owl#ObjectProperty> ;
        <http://www.w3.org/2000/01/rdf-schema#comment>
                "A log handler can have a set of log actions which describe what the handler should do with\r\n    trapped errors and messages."@en ;
        <http://www.w3.org/2000/01/rdf-schema#domain>
                <http://www.openlinksw.com/ontology/logging#LogHandler> ;
        <http://www.w3.org/2000/01/rdf-schema#isDefinedBy>
                <http://www.openlinksw.com/ontology/logging#> ;
        <http://www.w3.org/2000/01/rdf-schema#label>
                "hasLogAction" ;
        <http://www.w3.org/2000/01/rdf-schema#range>
                <http://www.openlinksw.com/ontology/logging#LogAction> ;
        <http://www.w3.org/2004/02/skos/core#altLabel>
                "Has Log Action" .

<http://www.openlinksw.com/ontology/logging#hasContext>
        a       <http://www.w3.org/1999/02/22-rdf-syntax-ns#Property> , <http://www.w3.org/2002/07/owl#DatatypeProperty> ;
        <http://www.w3.org/2000/01/rdf-schema#comment>
                "Additional information relating to the circumstances that triggered the log message."@en ;
        <http://www.w3.org/2000/01/rdf-schema#domain>
                <http://www.openlinksw.com/ontology/logging#LogEntry> ;
        <http://www.w3.org/2000/01/rdf-schema#isDefinedBy>
                <http://www.openlinksw.com/ontology/logging#> ;
        <http://www.w3.org/2000/01/rdf-schema#label>
                "hasContext" ;
        <http://www.w3.org/2000/01/rdf-schema#range>
                <http://www.w3.org/2000/01/rdf-schema#Resource> ;
        <http://www.w3.org/2004/02/skos/core#altLabel>
                "Contextual Information" .

<http://www.openlinksw.com/ontology/logging#HttpContextError>
        a       <http://www.w3.org/2002/07/owl#Class> ;
        <http://www.w3.org/2000/01/rdf-schema#comment>
                "An error which has been thrown in an http context."@en ;
        <http://www.w3.org/2000/01/rdf-schema#isDefinedBy>
                <http://www.openlinksw.com/ontology/logging#> ;
        <http://www.w3.org/2000/01/rdf-schema#label>
                "HttpContextError" ;
        <http://www.w3.org/2000/01/rdf-schema#subClassOf>
                <http://www.openlinksw.com/ontology/logging#Error> ;
        <http://www.w3.org/2004/02/skos/core#altLabel>
                "HTTP Context Error" .

<http://www.openlinksw.com/ontology/logging#LogPattern>
        a       <http://www.w3.org/2002/07/owl#Class> ;
        <http://www.w3.org/2000/01/rdf-schema#comment>
                "A Log Pattern describes a set of log entries via conditions on an error's\r\n    state and/or the log message. It can be used to trap signals/messages for Log Handlers."@en ;
        <http://www.w3.org/2000/01/rdf-schema#isDefinedBy>
                <http://www.openlinksw.com/ontology/logging#> ;
        <http://www.w3.org/2000/01/rdf-schema#label>
                "LogPattern" ;
        <http://www.w3.org/2004/02/skos/core#altLabel>
                "Log Pattern" .

<http://www.openlinksw.com/ontology/logging#matchesLogEntryType>
        a       <http://www.w3.org/2002/07/owl#DatatypeProperty> , <http://www.w3.org/1999/02/22-rdf-syntax-ns#Property> ;
        <http://www.w3.org/2000/01/rdf-schema#comment>
                "Defines which types of log entries a pattern should match. Omitting means to match any type.\r\n    The range of this property is rdfs:Class but in practice only sub-classes of LogEntry should be used."@en ;
        <http://www.w3.org/2000/01/rdf-schema#domain>
                <http://www.openlinksw.com/ontology/logging#LogPattern> ;
        <http://www.w3.org/2000/01/rdf-schema#isDefinedBy>
                <http://www.openlinksw.com/ontology/logging#> ;
        <http://www.w3.org/2000/01/rdf-schema#label>
                "matchesLogEntryType" ;
        <http://www.w3.org/2000/01/rdf-schema#range>
                <http://www.w3.org/2000/01/rdf-schema#Class> ;
        <http://www.w3.org/2004/02/skos/core#altLabel>
                "Matches Log Entry Type" .

<http://www.openlinksw.com/ontology/logging#LogHandler>
        a       <http://www.w3.org/2002/07/owl#Class> ;
        <http://www.w3.org/2000/01/rdf-schema#comment>
                "A Log Handler describes a way how a log message or error should be handled. Entries\r\n    are trapped via a LogPattern and then handled according to a set of LogActions. A LogHandler without\r\n    a LogPattern will match all incoming messages and errors."@en ;
        <http://www.w3.org/2000/01/rdf-schema#isDefinedBy>
                <http://www.openlinksw.com/ontology/logging#> ;
        <http://www.w3.org/2000/01/rdf-schema#label>
                "LogHandler" ;
        <http://www.w3.org/2004/02/skos/core#altLabel>
                "Log Handler" .

<http://www.openlinksw.com/ontology/logging#EmailLogAction>
        a       <http://www.w3.org/2002/07/owl#Class> ;
        <http://www.w3.org/2000/01/rdf-schema#comment>
                "An Log Error Action will send details of the error to a set of specified\r\n    email addresses."@en ;
        <http://www.w3.org/2000/01/rdf-schema#isDefinedBy>
                <http://www.openlinksw.com/ontology/logging#> ;
        <http://www.w3.org/2000/01/rdf-schema#label>
                "EmailLogAction" ;
        <http://www.w3.org/2000/01/rdf-schema#subClassOf>
                <http://www.openlinksw.com/ontology/logging#LogAction> ;
        <http://www.w3.org/2004/02/skos/core#altLabel>
                "Email Log Action" .

<http://www.openlinksw.com/ontology/logging#hasOwningApplication>
        a       <http://www.w3.org/1999/02/22-rdf-syntax-ns#Property> , <http://www.w3.org/2002/07/owl#ObjectProperty> ;
        <http://www.w3.org/2000/01/rdf-schema#comment>
                "The application that a log handler belongs to. Only log entries from this application should\r\n    be handled via the actions defined in the handler."@en ;
        <http://www.w3.org/2000/01/rdf-schema#domain>
                <http://www.openlinksw.com/ontology/logging#LogHandler> ;
        <http://www.w3.org/2000/01/rdf-schema#isDefinedBy>
                <http://www.openlinksw.com/ontology/logging#> ;
        <http://www.w3.org/2000/01/rdf-schema#label>
                "hasOwningApplication" ;
        <http://www.w3.org/2000/01/rdf-schema#range>
                <http://www.w3.org/2000/01/rdf-schema#Resource> ;
        <http://www.w3.org/2004/02/skos/core#altLabel>
                "Owning Application" .

<http://www.openlinksw.com/ontology/logging#LogEntry>
        a       <http://www.w3.org/2002/07/owl#Class> ;
        <http://www.w3.org/2000/01/rdf-schema#comment>
                "The base class for all log entry types: info, debug, and error."@en ;
        <http://www.w3.org/2000/01/rdf-schema#isDefinedBy>
                <http://www.openlinksw.com/ontology/logging#> ;
        <http://www.w3.org/2000/01/rdf-schema#label>
                "LogEntry" ;
        <http://www.w3.org/2004/02/skos/core#altLabel>
                "Log Entry" .

<http://www.openlinksw.com/ontology/logging#hasEmailRecipient>
        a       <http://www.w3.org/1999/02/22-rdf-syntax-ns#Property> , <http://www.w3.org/2002/07/owl#ObjectProperty> ;
        <http://www.w3.org/2000/01/rdf-schema#comment>
                "An email address the email error action should send the error to. This is a mailto: URI."@en ;
        <http://www.w3.org/2000/01/rdf-schema#domain>
                <http://www.openlinksw.com/ontology/logging#EmailLogAction> ;
        <http://www.w3.org/2000/01/rdf-schema#isDefinedBy>
                <http://www.openlinksw.com/ontology/logging#> ;
        <http://www.w3.org/2000/01/rdf-schema#label>
                "hasEmailRecipient" ;
        <http://www.w3.org/2000/01/rdf-schema#range>
                <http://www.w3.org/2000/01/rdf-schema#Resource> ;
        <http://www.w3.org/2004/02/skos/core#altLabel>
                "Email Recipient" .

<http://www.openlinksw.com/ontology/logging#hasTimestamp>
        a       <http://www.w3.org/2002/07/owl#DatatypeProperty> , <http://www.w3.org/1999/02/22-rdf-syntax-ns#Property> ;
        <http://www.w3.org/2000/01/rdf-schema#comment>
                "The time an error was raised."@en ;
        <http://www.w3.org/2000/01/rdf-schema#domain>
                <http://www.openlinksw.com/ontology/logging#LogEntry> ;
        <http://www.w3.org/2000/01/rdf-schema#isDefinedBy>
                <http://www.openlinksw.com/ontology/logging#> ;
        <http://www.w3.org/2000/01/rdf-schema#label>
                "hasTimestamp" ;
        <http://www.w3.org/2000/01/rdf-schema#range>
                <http://www.w3.org/2001/XMLSchema#dateTime> ;
        <http://www.w3.org/2000/01/rdf-schema#subPropertyOf>
                <http://purl.org/dc/terms/date> ;
        <http://www.w3.org/2004/02/skos/core#altLabel>
                "Time stamp" .

<http://www.openlinksw.com/ontology/logging#hasReplacementErrorCode>
        a       <http://www.w3.org/1999/02/22-rdf-syntax-ns#Property> , <http://www.w3.org/2002/07/owl#DatatypeProperty> ;
        <http://www.w3.org/2000/01/rdf-schema#comment>
                "The error code the replacement error should contain."@en ;
        <http://www.w3.org/2000/01/rdf-schema#domain>
                <http://www.openlinksw.com/ontology/logging#ReplacementErrorAction> ;
        <http://www.w3.org/2000/01/rdf-schema#isDefinedBy>
                <http://www.openlinksw.com/ontology/logging#> ;
        <http://www.w3.org/2000/01/rdf-schema#label>
                "hasReplacementErrorCode" ;
        <http://www.w3.org/2000/01/rdf-schema#range>
                <http://www.w3.org/2001/XMLSchema#string> ;
        <http://www.w3.org/2004/02/skos/core#altLabel>
                "Replacement Error Code" .

<http://www.openlinksw.com/ontology/logging#InfoMessage>
        a       <http://www.w3.org/2002/07/owl#Class> ;
        <http://www.w3.org/2000/01/rdf-schema#comment>
                "An info message created by an application."@en ;
        <http://www.w3.org/2000/01/rdf-schema#isDefinedBy>
                <http://www.openlinksw.com/ontology/logging#> ;
        <http://www.w3.org/2000/01/rdf-schema#label>
                "InfoMessage" ;
        <http://www.w3.org/2000/01/rdf-schema#subClassOf>
                <http://www.openlinksw.com/ontology/logging#LogEntry> ;
        <http://www.w3.org/2004/02/skos/core#altLabel>
                "Info Message" .

<http://www.openlinksw.com/ontology/logging#hasPriorityLevel>
        a       <http://www.w3.org/2002/07/owl#DatatypeProperty> , <http://www.w3.org/1999/02/22-rdf-syntax-ns#Property> ;
        <http://www.w3.org/2000/01/rdf-schema#comment>
                "Log handlers are executed in order of their priority. A handler with a higher priority is evaluated\r\n    first. By default a handler has a priority level of 0. The priority level is mostly useful for handlers that have a\r\n    ReplacementErrorAction because only one replacement signal can be produced."@en ;
        <http://www.w3.org/2000/01/rdf-schema#domain>
                <http://www.openlinksw.com/ontology/logging#LogHandler> ;
        <http://www.w3.org/2000/01/rdf-schema#isDefinedBy>
                <http://www.openlinksw.com/ontology/logging#> ;
        <http://www.w3.org/2000/01/rdf-schema#label>
                "hasPriorityLevel" ;
        <http://www.w3.org/2000/01/rdf-schema#range>
                <http://www.w3.org/2001/XMLSchema#integer> ;
        <http://www.w3.org/2004/02/skos/core#altLabel>
                "Priority Level" .

<http://www.openlinksw.com/ontology/logging#hasAffectedUser>
        a       <http://www.w3.org/1999/02/22-rdf-syntax-ns#Property> , <http://www.w3.org/2002/07/owl#ObjectProperty> ;
        <http://www.w3.org/2000/01/rdf-schema#comment>
                "The optional user who was affected by the error. This is typically connected to the\r\n    authentication system of the application."@en ;
        <http://www.w3.org/2000/01/rdf-schema#domain>
                <http://www.openlinksw.com/ontology/logging#LogEntry> ;
        <http://www.w3.org/2000/01/rdf-schema#isDefinedBy>
                <http://www.openlinksw.com/ontology/logging#> ;
        <http://www.w3.org/2000/01/rdf-schema#label>
                "hasAffectedUser" ;
        <http://www.w3.org/2000/01/rdf-schema#range>
                <http://xmlns.com/foaf/0.1/Agent> ;
        <http://www.w3.org/2004/02/skos/core#altLabel>
                "Affected User" .

<http://www.openlinksw.com/ontology/logging#hasTriggeringApplication>
        a       <http://www.w3.org/2002/07/owl#ObjectProperty> , <http://www.w3.org/1999/02/22-rdf-syntax-ns#Property> ;
        <http://www.w3.org/2000/01/rdf-schema#comment>
                "The application that triggered the error. This is matched to the owning application\r\n    of an Error Handler."@en ;
        <http://www.w3.org/2000/01/rdf-schema#domain>
                <http://www.openlinksw.com/ontology/logging#LogEntry> ;
        <http://www.w3.org/2000/01/rdf-schema#isDefinedBy>
                <http://www.openlinksw.com/ontology/logging#> ;
        <http://www.w3.org/2000/01/rdf-schema#label>
                "hasTriggeringApplication" ;
        <http://www.w3.org/2000/01/rdf-schema#range>
                <http://www.w3.org/2000/01/rdf-schema#Resource> ;
        <http://www.w3.org/2004/02/skos/core#altLabel>
                "Triggering Application" .

<http://www.openlinksw.com/ontology/logging#hasEmailSender>
        a       <http://www.w3.org/1999/02/22-rdf-syntax-ns#Property> , <http://www.w3.org/2002/07/owl#ObjectProperty> ;
        <http://www.w3.org/2000/01/rdf-schema#comment>
                "An optional email address the error notification emails should be sent from. This is a mailto: URI."@en ;
        <http://www.w3.org/2000/01/rdf-schema#domain>
                <http://www.openlinksw.com/ontology/logging#EmailLogAction> ;
        <http://www.w3.org/2000/01/rdf-schema#isDefinedBy>
                <http://www.openlinksw.com/ontology/logging#> ;
        <http://www.w3.org/2000/01/rdf-schema#label>
                "hasEmailSender" ;
        <http://www.w3.org/2000/01/rdf-schema#range>
                <http://www.w3.org/2000/01/rdf-schema#Resource> ;
        <http://www.w3.org/2004/02/skos/core#altLabel>
                "Email Sender" .

<http://www.openlinksw.com/ontology/logging#hasLogPattern>
        a       <http://www.w3.org/1999/02/22-rdf-syntax-ns#Property> , <http://www.w3.org/2002/07/owl#ObjectProperty> ;
        <http://www.w3.org/2000/01/rdf-schema#comment>
                "An error handler can have a set of error patterns which are used to trap the errors the handler\r\n    should handle."@en ;
        <http://www.w3.org/2000/01/rdf-schema#domain>
                <http://www.openlinksw.com/ontology/logging#LogHandler> ;
        <http://www.w3.org/2000/01/rdf-schema#isDefinedBy>
                <http://www.openlinksw.com/ontology/logging#> ;
        <http://www.w3.org/2000/01/rdf-schema#label>
                "hasLogPattern" ;
        <http://www.w3.org/2000/01/rdf-schema#range>
                <http://www.openlinksw.com/ontology/logging#LogPattern> ;
        <http://www.w3.org/2004/02/skos/core#altLabel>
                "Has Log Pattern" .

<http://www.openlinksw.com/ontology/logging#hasLogMessagePattern>
        a       <http://www.w3.org/2002/07/owl#DatatypeProperty> , <http://www.w3.org/1999/02/22-rdf-syntax-ns#Property> ;
        <http://www.w3.org/2000/01/rdf-schema#comment>
                "A regular expression to match log messages that should be handled by the owning ErrorHandler."@en ;
        <http://www.w3.org/2000/01/rdf-schema#domain>
                <http://www.openlinksw.com/ontology/logging#LogPattern> ;
        <http://www.w3.org/2000/01/rdf-schema#isDefinedBy>
                <http://www.openlinksw.com/ontology/logging#> ;
        <http://www.w3.org/2000/01/rdf-schema#label>
                "hasLogMessagePattern" ;
        <http://www.w3.org/2000/01/rdf-schema#range>
                <http://www.w3.org/2001/XMLSchema#string> ;
        <http://www.w3.org/2004/02/skos/core#altLabel>
                "Log Message Pattern" .

<http://www.openlinksw.com/ontology/logging#Error>
        a       <http://www.w3.org/2002/07/owl#Class> ;
        <http://www.w3.org/2000/01/rdf-schema#comment>
                "An error produced by an application and typically thrown in a signal."@en ;
        <http://www.w3.org/2000/01/rdf-schema#isDefinedBy>
                <http://www.openlinksw.com/ontology/logging#> ;
        <http://www.w3.org/2000/01/rdf-schema#label>
                "Error" ;
        <http://www.w3.org/2000/01/rdf-schema#subClassOf>
                <http://www.openlinksw.com/ontology/logging#LogEntry> ;
        <http://www.w3.org/2004/02/skos/core#altLabel>
                "Error" .

<http://www.openlinksw.com/ontology/logging#hasStorageGraph>
        a       <http://www.w3.org/1999/02/22-rdf-syntax-ns#Property> , <http://www.w3.org/2002/07/owl#ObjectProperty> ;
        <http://www.w3.org/2000/01/rdf-schema#comment>
                "The named graph into which the errors should be logged."@en ;
        <http://www.w3.org/2000/01/rdf-schema#domain>
                <http://www.openlinksw.com/ontology/logging#GraphStorageAction> ;
        <http://www.w3.org/2000/01/rdf-schema#isDefinedBy>
                <http://www.openlinksw.com/ontology/logging#> ;
        <http://www.w3.org/2000/01/rdf-schema#label>
                "hasStorageGraph" ;
        <http://www.w3.org/2000/01/rdf-schema#range>
                <http://www.w3.org/2000/01/rdf-schema#Resource> ;
        <http://www.w3.org/2004/02/skos/core#altLabel>
                "Storage Graph" .

<http://www.openlinksw.com/ontology/logging#LogAction>
        a       <http://www.w3.org/2002/07/owl#Class> ;
        <http://www.w3.org/2000/01/rdf-schema#comment>
                "A Log Action defines how a log entry is handled after being trapped.\r\n    Log Action is an abstract class which means that it has no instances.\r\n    Instances are only created from its sub-classes."@en ;
        <http://www.w3.org/2000/01/rdf-schema#isDefinedBy>
                <http://www.openlinksw.com/ontology/logging#> ;
        <http://www.w3.org/2000/01/rdf-schema#label>
                "LogAction" ;
        <http://www.w3.org/2004/02/skos/core#altLabel>
                "Log Action" .
