<http://merlin.phys.uni.lodz.pl/onto/physo/observationMadeIn>
        a       <http://www.w3.org/2002/07/owl#ObjectProperty> ;
        <http://www.w3.org/2000/01/rdf-schema#comment>
                "Observation is made in some experiment"@en ;
        <http://www.w3.org/2000/01/rdf-schema#domain>
                <http://merlin.phys.uni.lodz.pl/onto/physo/Observation> ;
        <http://www.w3.org/2000/01/rdf-schema#label>
                "observation made in"@en ;
        <http://www.w3.org/2000/01/rdf-schema#range>
                <http://merlin.phys.uni.lodz.pl/onto/physo/Experiment> .

<http://merlin.phys.uni.lodz.pl/onto/physo/>
        a       <http://www.w3.org/2002/07/owl#Ontology> ;
        <http://purl.org/dc/elements/1.1/creator>
                "Marcin Skulimowski" ;
        <http://purl.org/dc/elements/1.1/date>
                "2012-01-17"^^<http://www.w3.org/2001/XMLSchema#dateTime> ;
        <http://purl.org/dc/elements/1.1/description>
                "PHYSO, the Physical Sciences Ontology, is an ontology for describing general concepts and relations of physical sciences."@en ;
        <http://purl.org/dc/elements/1.1/rights>
                "http://creativecommons.org/licenses/by/3.0/" ;
        <http://purl.org/dc/elements/1.1/title>
                "PHYSO: Physical Sciences Ontology"@en ;
        <http://www.w3.org/2002/07/owl#versionInfo>
                "Version 1.1" .

<http://purl.org/dc/elements/1.1/description>
        a       <http://www.w3.org/2002/07/owl#AnnotationProperty> .

<http://merlin.phys.uni.lodz.pl/onto/physo/formulaFor>
        a       <http://www.w3.org/2002/07/owl#ObjectProperty> ;
        <http://www.w3.org/2000/01/rdf-schema#label>
                "formula for"@en .

<http://merlin.phys.uni.lodz.pl/onto/physo/Effect>
        a       <http://www.w3.org/2002/07/owl#Class> ;
        <http://www.w3.org/2000/01/rdf-schema#comment>
                "A phenomenon that follows and is caused by some previous phenomenon."@en ;
        <http://www.w3.org/2000/01/rdf-schema#label>
                "effect"@en .

<http://merlin.phys.uni.lodz.pl/onto/physo/Experiment>
        a       <http://www.w3.org/2002/07/owl#Class> ;
        <http://www.w3.org/2000/01/rdf-schema#comment>
                "Experiment is the step in the scientific method that arbitrates between competing models or hypotheses."@en ;
        <http://www.w3.org/2000/01/rdf-schema#label>
                "experiment"@en .

<http://merlin.phys.uni.lodz.pl/onto/physo/forTheCaseOf>
        a       <http://www.w3.org/2002/07/owl#ObjectProperty> ;
        <http://www.w3.org/2000/01/rdf-schema#label>
                "for the case of"@en .

<http://merlin.phys.uni.lodz.pl/onto/physo/collectedThrough>
        a       <http://www.w3.org/2002/07/owl#ObjectProperty> ;
        <http://www.w3.org/2000/01/rdf-schema#domain>
                <http://merlin.phys.uni.lodz.pl/onto/physo/EmpiricalData> ;
        <http://www.w3.org/2000/01/rdf-schema#label>
                "collected through"@en ;
        <http://www.w3.org/2000/01/rdf-schema#range>
                <http://merlin.phys.uni.lodz.pl/onto/physo/Experiment> ;
        <http://www.w3.org/2000/01/rdf-schema#subPropertyOf>
                <http://www.w3.org/2002/07/owl#topObjectProperty> .

<http://merlin.phys.uni.lodz.pl/onto/physo/expressedAs>
        a       <http://www.w3.org/2002/07/owl#ObjectProperty> ;
        <http://www.w3.org/2000/01/rdf-schema#domain>
                <http://merlin.phys.uni.lodz.pl/onto/physo/SciTheoryElement> ;
        <http://www.w3.org/2000/01/rdf-schema#label>
                "expressed as"@en ;
        <http://www.w3.org/2000/01/rdf-schema#range>
                [ a       <http://www.w3.org/2002/07/owl#Class> ;
                  <http://www.w3.org/2002/07/owl#unionOf>
                          ( <http://merlin.phys.uni.lodz.pl/onto/physo/MathEquation> <http://merlin.phys.uni.lodz.pl/onto/physo/MathExpression> )
                ] .

<http://www.w3.org/2002/07/owl#topObjectProperty>
        a       <http://www.w3.org/2002/07/owl#ObjectProperty> .

<http://merlin.phys.uni.lodz.pl/onto/physo/Criterion>
        a       <http://www.w3.org/2002/07/owl#Class> ;
        <http://www.w3.org/2000/01/rdf-schema#comment>
                "A defining characteristic of something."@en ;
        <http://www.w3.org/2000/01/rdf-schema#label>
                "criterion"@en ;
        <http://www.w3.org/2000/01/rdf-schema#subClassOf>
                <http://merlin.phys.uni.lodz.pl/onto/physo/SciTheoryElement> .

<http://merlin.phys.uni.lodz.pl/onto/physo/Concept>
        a       <http://www.w3.org/2002/07/owl#Class> ;
        <http://www.w3.org/2000/01/rdf-schema#comment>
                "A general idea or notion that corresponds to some class of entities and that consists of the characteristic or essential features of the class."@en ;
        <http://www.w3.org/2000/01/rdf-schema#label>
                "concept"@en ;
        <http://www.w3.org/2000/01/rdf-schema#subClassOf>
                <http://merlin.phys.uni.lodz.pl/onto/physo/SciTheoryElement> .

<http://merlin.phys.uni.lodz.pl/onto/physo/conformsTo>
        a       <http://www.w3.org/2002/07/owl#ObjectProperty> ;
        <http://www.w3.org/2000/01/rdf-schema#domain>
                <http://merlin.phys.uni.lodz.pl/onto/physo/ScientificTheory> ;
        <http://www.w3.org/2000/01/rdf-schema#label>
                "conforms to"@en ;
        <http://www.w3.org/2000/01/rdf-schema#range>
                <http://merlin.phys.uni.lodz.pl/onto/physo/EmpiricalData> .

<http://merlin.phys.uni.lodz.pl/onto/physo/Principle>
        a       <http://www.w3.org/2002/07/owl#Class> ;
        <http://www.w3.org/2000/01/rdf-schema#comment>
                "A principle is a law or rule that has to be followed."@en ;
        <http://www.w3.org/2000/01/rdf-schema#label>
                "principle"@en ;
        <http://www.w3.org/2000/01/rdf-schema#subClassOf>
                <http://merlin.phys.uni.lodz.pl/onto/physo/Assumption> .

<http://merlin.phys.uni.lodz.pl/onto/physo/hasMathFramework>
        a       <http://www.w3.org/2002/07/owl#ObjectProperty> ;
        <http://www.w3.org/2000/01/rdf-schema#domain>
                <http://merlin.phys.uni.lodz.pl/onto/physo/ScientificTheory> ;
        <http://www.w3.org/2000/01/rdf-schema#label>
                "has mathematical framework"@en ;
        <http://www.w3.org/2000/01/rdf-schema#range>
                <http://merlin.phys.uni.lodz.pl/onto/physo/MathFramework> .

<http://purl.org/swan/2.0/discourse-relationships/consistentWith>
        a       <http://www.w3.org/2002/07/owl#ObjectProperty> ;
        <http://www.w3.org/2000/01/rdf-schema#comment>
                "Two elements (statements) of the theory are consistent if they do not contradict each other."@en ;
        <http://www.w3.org/2000/01/rdf-schema#label>
                "consistent with"@en .

<http://merlin.phys.uni.lodz.pl/onto/physo/Construction>
        a       <http://www.w3.org/2002/07/owl#Class> ;
        <http://www.w3.org/2000/01/rdf-schema#comment>
                "The way in which something (e.g. some element of the theory) is built (obtained, created) or put together."@en ;
        <http://www.w3.org/2000/01/rdf-schema#label>
                "construction"@en .

<http://merlin.phys.uni.lodz.pl/onto/physo/obtainedFrom>
        a       <http://www.w3.org/2002/07/owl#ObjectProperty> ;
        <http://www.w3.org/2000/01/rdf-schema#label>
                "obtained from"@en .

<http://merlin.phys.uni.lodz.pl/onto/physo/featureOf>
        a       <http://www.w3.org/2002/07/owl#ObjectProperty> ;
        <http://www.w3.org/2000/01/rdf-schema#domain>
                <http://merlin.phys.uni.lodz.pl/onto/physo/Feature> ;
        <http://www.w3.org/2000/01/rdf-schema#label>
                "feature of"@en .

<http://merlin.phys.uni.lodz.pl/onto/physo/interpretedAs>
        a       <http://www.w3.org/2002/07/owl#ObjectProperty> ;
        <http://www.w3.org/2000/01/rdf-schema#label>
                "interpreted as"@en .

<http://merlin.phys.uni.lodz.pl/onto/physo/hasAssumption>
        a       <http://www.w3.org/2002/07/owl#ObjectProperty> ;
        <http://www.w3.org/2000/01/rdf-schema#domain>
                <http://merlin.phys.uni.lodz.pl/onto/physo/ScientificTheory> ;
        <http://www.w3.org/2000/01/rdf-schema#label>
                "has assumption"@en ;
        <http://www.w3.org/2000/01/rdf-schema#range>
                <http://merlin.phys.uni.lodz.pl/onto/physo/Assumption> .

<http://merlin.phys.uni.lodz.pl/onto/physo/modificationOf>
        a       <http://www.w3.org/2002/07/owl#ObjectProperty> ;
        <http://www.w3.org/2000/01/rdf-schema#label>
                "modification of"@en .

<http://merlin.phys.uni.lodz.pl/onto/physo/explains>
        a       <http://www.w3.org/2002/07/owl#ObjectProperty> ;
        <http://www.w3.org/2000/01/rdf-schema#comment>
                "A scientific theory is constructed to conform to available empirical data about such observations, and is put forth as a principle or body of principles for explaining a class of phenomena."@en ;
        <http://www.w3.org/2000/01/rdf-schema#domain>
                <http://merlin.phys.uni.lodz.pl/onto/physo/ScientificTheory> ;
        <http://www.w3.org/2000/01/rdf-schema#label>
                "explains"@en ;
        <http://www.w3.org/2000/01/rdf-schema#range>
                <http://merlin.phys.uni.lodz.pl/onto/physo/EmpiricalData> .

<http://merlin.phys.uni.lodz.pl/onto/physo/interpretationOf>
        a       <http://www.w3.org/2002/07/owl#ObjectProperty> ;
        <http://www.w3.org/2000/01/rdf-schema#label>
                "interpretation of"@en .

<http://merlin.phys.uni.lodz.pl/onto/physo/problemDescription>
        a       <http://www.w3.org/2002/07/owl#ObjectProperty> ;
        <http://www.w3.org/2000/01/rdf-schema#label>
                "problem description"@en .

<http://merlin.phys.uni.lodz.pl/onto/physo/applicationOf>
        a       <http://www.w3.org/2002/07/owl#ObjectProperty> ;
        <http://www.w3.org/2000/01/rdf-schema#comment>
                "It expresses the fact that one entity is an application of another entity. "@en ;
        <http://www.w3.org/2000/01/rdf-schema#domain>
                <http://merlin.phys.uni.lodz.pl/onto/physo/Application> ;
        <http://www.w3.org/2000/01/rdf-schema#label>
                "application of"@en .

<http://merlin.phys.uni.lodz.pl/onto/physo/consistsOf>
        a       <http://www.w3.org/2002/07/owl#ObjectProperty> ;
        <http://www.w3.org/2000/01/rdf-schema#comment>
                "A scientific theory consists of some elements."@en ;
        <http://www.w3.org/2000/01/rdf-schema#domain>
                <http://merlin.phys.uni.lodz.pl/onto/physo/ScientificTheory> ;
        <http://www.w3.org/2000/01/rdf-schema#label>
                "consists of"@en ;
        <http://www.w3.org/2000/01/rdf-schema#range>
                <http://merlin.phys.uni.lodz.pl/onto/physo/SciTheoryElement> .

<http://merlin.phys.uni.lodz.pl/onto/physo/ScientificLaw>
        a       <http://www.w3.org/2002/07/owl#Class> ;
        <http://www.w3.org/2000/01/rdf-schema#comment>
                "A scientific law or scientific principle is a concise verbal or mathematical statement of a relation that expresses a fundamental principle of science."@en ;
        <http://www.w3.org/2000/01/rdf-schema#label>
                "scientific law"@en ;
        <http://www.w3.org/2000/01/rdf-schema#subClassOf>
                <http://merlin.phys.uni.lodz.pl/onto/physo/SciTheoryElement> .

<http://merlin.phys.uni.lodz.pl/onto/physo/Property>
        a       <http://www.w3.org/2002/07/owl#Class> ;
        <http://www.w3.org/2000/01/rdf-schema#comment>
                "A quality, attribute, or distinctive feature of something."@en ;
        <http://www.w3.org/2000/01/rdf-schema#label>
                "property"@en .

<http://merlin.phys.uni.lodz.pl/onto/physo/Feature>
        a       <http://www.w3.org/2002/07/owl#Class> ;
        <http://www.w3.org/2000/01/rdf-schema#comment>
                "A prominent attribute or aspect of something."@en ;
        <http://www.w3.org/2000/01/rdf-schema#label>
                "feature"@en ;
        <http://www.w3.org/2000/01/rdf-schema#subClassOf>
                <http://merlin.phys.uni.lodz.pl/onto/physo/Property> .

<http://merlin.phys.uni.lodz.pl/onto/physo/constructedFrom>
        a       <http://www.w3.org/2002/07/owl#ObjectProperty> ;
        <http://www.w3.org/2000/01/rdf-schema#label>
                "constructed from"@en ;
        <http://www.w3.org/2000/01/rdf-schema#subPropertyOf>
                <http://merlin.phys.uni.lodz.pl/onto/physo/obtainedFrom> .

<http://merlin.phys.uni.lodz.pl/onto/physo/Model>
        a       <http://www.w3.org/2002/07/owl#Class> ;
        <http://www.w3.org/2000/01/rdf-schema#comment>
                "A model represents empirical objects, phenomena, and physical processes in a logical and objective way. It is simplified reflections of reality, but despite their inherent falsity, they are nevertheless extremely useful reflections of reality."@en ;
        <http://www.w3.org/2000/01/rdf-schema#label>
                "model"@en ;
        <http://www.w3.org/2000/01/rdf-schema#subClassOf>
                <http://merlin.phys.uni.lodz.pl/onto/physo/SciTheoryElement> .

<http://merlin.phys.uni.lodz.pl/onto/physo/Condition>
        a       <http://www.w3.org/2002/07/owl#Class> ;
        <http://www.w3.org/2000/01/rdf-schema#comment>
                "Any kind of an assumption on which rests the validity or effect of something else."@en ;
        <http://www.w3.org/2000/01/rdf-schema#label>
                "condition"@en .

<http://merlin.phys.uni.lodz.pl/onto/physo/MathExpression>
        a       <http://www.w3.org/2002/07/owl#Class> ;
        <http://www.w3.org/2000/01/rdf-schema#comment>
                "A mathematical expression is a finite combination of symbols that are well-formed according to the rules applicable in the context at hand. Symbols can designate values (constants), variables, operations, relations, or can constitute punctuation or other syntactic entities. Expression cannot contain an equals sign."@en ;
        <http://www.w3.org/2000/01/rdf-schema#label>
                "mathematical expression"@en .

<http://merlin.phys.uni.lodz.pl/onto/physo/analogyTo>
        a       <http://www.w3.org/2002/07/owl#ObjectProperty> ;
        <http://www.w3.org/2000/01/rdf-schema#comment>
                "It expresses analogy between two resources."@en ;
        <http://www.w3.org/2000/01/rdf-schema#domain>
                <http://merlin.phys.uni.lodz.pl/onto/physo/SciTheoryElement> ;
        <http://www.w3.org/2000/01/rdf-schema#label>
                "analogy to"@en .

<http://merlin.phys.uni.lodz.pl/onto/physo/consequenceOf>
        a       <http://www.w3.org/2002/07/owl#ObjectProperty> ;
        <http://www.w3.org/2000/01/rdf-schema#label>
                "consequence of"@en .

<http://purl.org/dc/elements/1.1/title>
        a       <http://www.w3.org/2002/07/owl#AnnotationProperty> .

<http://merlin.phys.uni.lodz.pl/onto/physo/EmpiricalData>
        a       <http://www.w3.org/2002/07/owl#Class> ;
        <http://www.w3.org/2000/01/rdf-schema#comment>
                "Empirical data is data produced by an experiment or observation."@en ;
        <http://www.w3.org/2000/01/rdf-schema#label>
                "empirical data"@en .

<http://merlin.phys.uni.lodz.pl/onto/physo/specialCaseOf>
        a       <http://www.w3.org/2002/07/owl#ObjectProperty> ;
        <http://www.w3.org/2000/01/rdf-schema#label>
                "special case of"@en .

<http://merlin.phys.uni.lodz.pl/onto/physo/MathEquation>
        a       <http://www.w3.org/2002/07/owl#Class> ;
        <http://www.w3.org/2000/01/rdf-schema#comment>
                "An equation is a mathematical statement that asserts the equality of two mathematical expressions."@en ;
        <http://www.w3.org/2000/01/rdf-schema#label>
                "mathematical equation"@en ;
        <http://www.w3.org/2000/01/rdf-schema#subClassOf>
                <http://purl.org/spar/doco/MathematicalFormula> .

<http://merlin.phys.uni.lodz.pl/onto/physo/conditionFor>
        a       <http://www.w3.org/2002/07/owl#ObjectProperty> ;
        <http://www.w3.org/2000/01/rdf-schema#label>
                "condition for"@en .

<http://merlin.phys.uni.lodz.pl/onto/physo/hasFormulation>
        a       <http://www.w3.org/2002/07/owl#ObjectProperty> ;
        <http://www.w3.org/2000/01/rdf-schema#domain>
                <http://merlin.phys.uni.lodz.pl/onto/physo/ScientificTheory> ;
        <http://www.w3.org/2000/01/rdf-schema#label>
                "has formulation"@en ;
        <http://www.w3.org/2000/01/rdf-schema#range>
                <http://merlin.phys.uni.lodz.pl/onto/physo/TheoryFormulation> .

<http://purl.org/swan/2.0/discourse-relationships/inconsistentWith>
        a       <http://www.w3.org/2002/07/owl#ObjectProperty> ;
        <http://www.w3.org/2000/01/rdf-schema#label>
                "inconsistent with"@en .

<http://merlin.phys.uni.lodz.pl/onto/physo/solutionBasedOn>
        a       <http://www.w3.org/2002/07/owl#ObjectProperty> ;
        <http://www.w3.org/2000/01/rdf-schema#label>
                "solution based on"@en .

<http://www.w3.org/2002/07/owl#versionInfo>
        a       <http://www.w3.org/2002/07/owl#AnnotationProperty> .

<http://merlin.phys.uni.lodz.pl/onto/physo/Application>
        a       <http://www.w3.org/2002/07/owl#Class> ;
        <http://www.w3.org/2000/01/rdf-schema#comment>
                "The way of applying to a particular purpose or use"@en ;
        <http://www.w3.org/2000/01/rdf-schema#label>
                "application"@en .

<http://merlin.phys.uni.lodz.pl/onto/physo/problemWith>
        a       <http://www.w3.org/2002/07/owl#ObjectProperty> ;
        <http://www.w3.org/2000/01/rdf-schema#label>
                "problem with"@en .

<http://merlin.phys.uni.lodz.pl/onto/physo/TheoryFormulation>
        a       <http://www.w3.org/2002/07/owl#Class> ;
        <http://www.w3.org/2000/01/rdf-schema#label>
                "theory formulation"@en .

<http://merlin.phys.uni.lodz.pl/onto/physo/Theorem>
        a       <http://www.w3.org/2002/07/owl#Class> ;
        <http://www.w3.org/2000/01/rdf-schema#comment>
                "A theorem is a statement that has been proven on the basis of previously established statements, such as other theorems, and previously accepted statements, such as axioms."@en ;
        <http://www.w3.org/2000/01/rdf-schema#label>
                "theorem"@en ;
        <http://www.w3.org/2000/01/rdf-schema#subClassOf>
                <http://merlin.phys.uni.lodz.pl/onto/physo/SciTheoryElement> .

<http://merlin.phys.uni.lodz.pl/onto/physo/criterionFor>
        a       <http://www.w3.org/2002/07/owl#ObjectProperty> ;
        <http://www.w3.org/2000/01/rdf-schema#label>
                "criterion for"@en .

<http://merlin.phys.uni.lodz.pl/onto/physo/MathFramework>
        a       <http://www.w3.org/2002/07/owl#Class> ;
        <http://www.w3.org/2000/01/rdf-schema#label>
                "mathematical framework "@en .

<http://merlin.phys.uni.lodz.pl/onto/physo/Interpretation>
        a       <http://www.w3.org/2002/07/owl#Class> ;
        <http://www.w3.org/2000/01/rdf-schema#label>
                "interpretation"@en .

<http://purl.org/dc/elements/1.1/creator>
        a       <http://www.w3.org/2002/07/owl#AnnotationProperty> .

<http://merlin.phys.uni.lodz.pl/onto/physo/Assumption>
        a       <http://www.w3.org/2002/07/owl#Class> ;
        <http://www.w3.org/2000/01/rdf-schema#comment>
                "An assumption is not tesable or questionable statement (proposition, elelement) of the theory."@en ;
        <http://www.w3.org/2000/01/rdf-schema#label>
                "assumption"@en ;
        <http://www.w3.org/2000/01/rdf-schema#subClassOf>
                <http://merlin.phys.uni.lodz.pl/onto/physo/SciTheoryElement> .

<http://merlin.phys.uni.lodz.pl/onto/physo/applicationTo>
        a       <http://www.w3.org/2002/07/owl#ObjectProperty> ;
        <http://www.w3.org/2000/01/rdf-schema#comment>
                "It expresses the fact that one entity is applied to another entity. "@en ;
        <http://www.w3.org/2000/01/rdf-schema#domain>
                <http://merlin.phys.uni.lodz.pl/onto/physo/Application> ;
        <http://www.w3.org/2000/01/rdf-schema#label>
                "application to"@en .

<http://merlin.phys.uni.lodz.pl/onto/physo/Problem>
        a       <http://www.w3.org/2002/07/owl#Class> ;
        <http://www.w3.org/2000/01/rdf-schema#comment>
                "A contradictory situation that arises in the form of opposing views to the explanation of any given phenomenon, object, or process and that requires an adequate theory for its solution."@en ;
        <http://www.w3.org/2000/01/rdf-schema#label>
                "problem"@en .

<http://merlin.phys.uni.lodz.pl/onto/physo/hasProperty>
        a       <http://www.w3.org/2002/07/owl#ObjectProperty> ;
        <http://www.w3.org/2000/01/rdf-schema#domain>
                <http://merlin.phys.uni.lodz.pl/onto/physo/Concept> ;
        <http://www.w3.org/2000/01/rdf-schema#label>
                "has property"@en .

<http://merlin.phys.uni.lodz.pl/onto/physo/constructionOf>
        a       <http://www.w3.org/2002/07/owl#ObjectProperty> ;
        <http://www.w3.org/2000/01/rdf-schema#label>
                "construction of"@en .

<http://merlin.phys.uni.lodz.pl/onto/physo/ModelMathematical>
        a       <http://www.w3.org/2002/07/owl#Class> ;
        <http://www.w3.org/2000/01/rdf-schema#comment>
                "A mathematical model is a description of a system using mathematical language. "@en ;
        <http://www.w3.org/2000/01/rdf-schema#label>
                "mathematical model"@en ;
        <http://www.w3.org/2000/01/rdf-schema#subClassOf>
                <http://merlin.phys.uni.lodz.pl/onto/physo/Model> .

<http://merlin.phys.uni.lodz.pl/onto/physo/ExperimentalProblem>
        a       <http://www.w3.org/2002/07/owl#Class> ;
        <http://www.w3.org/2000/01/rdf-schema#label>
                "experimental problem"@en ;
        <http://www.w3.org/2000/01/rdf-schema#subClassOf>
                <http://merlin.phys.uni.lodz.pl/onto/physo/Problem> .

<http://merlin.phys.uni.lodz.pl/onto/physo/exampleOf>
        a       <http://www.w3.org/2002/07/owl#ObjectProperty> ;
        <http://www.w3.org/2000/01/rdf-schema#label>
                "example of"@en .

<http://merlin.phys.uni.lodz.pl/onto/physo/Solution>
        a       <http://www.w3.org/2002/07/owl#Class> ;
        <http://www.w3.org/2000/01/rdf-schema#comment>
                "A method for solving a problem."@en ;
        <http://www.w3.org/2000/01/rdf-schema#label>
                "solution"@en .

<http://purl.org/spar/doco/MathematicalFormula>
        a       <http://www.w3.org/2002/07/owl#Class> ;
        <http://www.w3.org/2000/01/rdf-schema#comment>
                "An equation expressing a definite fixed relationship between certain quantities. The quantities are usually expressed by letters, and their relationship is indicated by algebraic symbols."@en ;
        <http://www.w3.org/2000/01/rdf-schema#label>
                "mathematical formula"@en .

<http://merlin.phys.uni.lodz.pl/onto/physo/TheoreticalProblem>
        a       <http://www.w3.org/2002/07/owl#Class> ;
        <http://www.w3.org/2000/01/rdf-schema#label>
                "theoretical problem"@en ;
        <http://www.w3.org/2000/01/rdf-schema#subClassOf>
                <http://merlin.phys.uni.lodz.pl/onto/physo/Problem> .

<http://merlin.phys.uni.lodz.pl/onto/physo/methodForObtaining>
        a       <http://www.w3.org/2002/07/owl#ObjectProperty> ;
        <http://www.w3.org/2000/01/rdf-schema#label>
                "method for obtaining"@en .

<http://merlin.phys.uni.lodz.pl/onto/physo/SciTheoryElement>
        a       <http://www.w3.org/2002/07/owl#Class> ;
        <http://www.w3.org/2000/01/rdf-schema#label>
                "scientific theory element"@en .

<http://merlin.phys.uni.lodz.pl/onto/physo/appliedTo>
        a       <http://www.w3.org/2002/07/owl#ObjectProperty> ;
        <http://www.w3.org/2000/01/rdf-schema#label>
                "applied to"@en .

<http://merlin.phys.uni.lodz.pl/onto/physo/Process>
        a       <http://www.w3.org/2002/07/owl#Class> ;
        <http://www.w3.org/2000/01/rdf-schema#comment>
                "A method or event that results in a transformation in a physical object or substance."@en ;
        <http://www.w3.org/2000/01/rdf-schema#label>
                "process"@en .

<http://merlin.phys.uni.lodz.pl/onto/physo/Observation>
        a       <http://www.w3.org/2002/07/owl#Class> ;
        <http://www.w3.org/2000/01/rdf-schema#comment>
                "Observation is either an activity of a living being (such as a human), consisting of receiving knowledge of the outside world through the senses, or the recording of data using scientific instruments."@en ;
        <http://www.w3.org/2000/01/rdf-schema#label>
                "observation"@en .

<http://merlin.phys.uni.lodz.pl/onto/physo/Formalism>
        a       <http://www.w3.org/2002/07/owl#Class> ;
        <http://www.w3.org/2000/01/rdf-schema#label>
                "formalism"@en .

<http://merlin.phys.uni.lodz.pl/onto/physo/expTechForObtaining>
        a       <http://www.w3.org/2002/07/owl#ObjectProperty> ;
        <http://www.w3.org/2000/01/rdf-schema#label>
                "experimental technique for obtaining"@en .

<http://merlin.phys.uni.lodz.pl/onto/physo/Method>
        a       <http://www.w3.org/2002/07/owl#Class> ;
        <http://www.w3.org/2000/01/rdf-schema#label>
                "method"@en .

<http://purl.org/dc/elements/1.1/date>
        a       <http://www.w3.org/2002/07/owl#AnnotationProperty> .

<http://merlin.phys.uni.lodz.pl/onto/physo/propertyOf>
        a       <http://www.w3.org/2002/07/owl#ObjectProperty> ;
        <http://www.w3.org/2000/01/rdf-schema#label>
                "property of"@en .

<http://merlin.phys.uni.lodz.pl/onto/physo/mathExpressionFor>
        a       <http://www.w3.org/2002/07/owl#ObjectProperty> ;
        <http://www.w3.org/2000/01/rdf-schema#label>
                "mathematical expression for"@en .

<http://merlin.phys.uni.lodz.pl/onto/physo/methodForAvoiding>
        a       <http://www.w3.org/2002/07/owl#ObjectProperty> ;
        <http://www.w3.org/2000/01/rdf-schema#label>
                "method for avoiding"@en .

<http://merlin.phys.uni.lodz.pl/onto/physo/hasRelationshipWith>
        a       <http://www.w3.org/2002/07/owl#ObjectProperty> ;
        <http://www.w3.org/2000/01/rdf-schema#label>
                "has relationship with"@en .

<http://merlin.phys.uni.lodz.pl/onto/physo/solutionTo>
        a       <http://www.w3.org/2002/07/owl#ObjectProperty> ;
        <http://www.w3.org/2000/01/rdf-schema#label>
                "solution to"@en .

<http://merlin.phys.uni.lodz.pl/onto/physo/generalizes>
        a       <http://www.w3.org/2002/07/owl#ObjectProperty> ;
        <http://www.w3.org/2000/01/rdf-schema#comment>
                "One element of a theory is a generalization of another element"@en ;
        <http://www.w3.org/2000/01/rdf-schema#label>
                "generalizes"@en .

<http://merlin.phys.uni.lodz.pl/onto/physo/elementOf>
        a       <http://www.w3.org/2002/07/owl#ObjectProperty> ;
        <http://www.w3.org/2000/01/rdf-schema#label>
                "element of"@en .

<http://merlin.phys.uni.lodz.pl/onto/physo/ScientificTheory>
        a       <http://www.w3.org/2002/07/owl#Class> ;
        <http://www.w3.org/2000/01/rdf-schema#comment>
                "A scientific theory comprises a collection of concepts, including abstractions of observable phenomena expressed as quantifiable properties, together with rules (called scientific laws) that express relationships between observations of such concepts. A scientific theory is constructed to conform to available empirical data about such observations, and is put forth as a principle or body of principles for explaining a class of phenomena."@en ;
        <http://www.w3.org/2000/01/rdf-schema#label>
                "scientific theory"@en .

<http://www.w3.org/2000/01/rdf-schema#comment>
        a       <http://www.w3.org/2002/07/owl#AnnotationProperty> .

<http://purl.org/dc/elements/1.1/rights>
        a       <http://www.w3.org/2002/07/owl#AnnotationProperty> .

<http://merlin.phys.uni.lodz.pl/onto/physo/ExperimentalTechnique>
        a       <http://www.w3.org/2002/07/owl#Class> ;
        <http://www.w3.org/2000/01/rdf-schema#label>
                "experimental technique"@en .

<http://www.w3.org/2000/01/rdf-schema#label>
        a       <http://www.w3.org/2002/07/owl#AnnotationProperty> .

<http://www.w3.org/2002/07/owl#Thing>
        a       <http://www.w3.org/2002/07/owl#Class> .
