<http://purl.org/ontology/po/>
        a       <http://www.bbc.co.uk/ontologies/provenance/Ontology> , <http://www.w3.org/2002/07/owl#Ontology> ;
        <http://www.w3.org/2000/01/rdf-schema#comment>
                "\n\t\tA vocabulary for programme data.\n\t\tIt defines concepts such as brands, series, episodes, broadcasts, etc.\n\t" ;
        <http://www.w3.org/2000/01/rdf-schema#isDefinedBy>
                <http://purl.org/ontology/po/> ;
        <http://www.w3.org/2000/01/rdf-schema#label>
                "Programmes ontology" ;
        <http://purl.org/dc/elements/1.1/contributor>
                <http://www.aelius.com/njh#me> , <http://metade.org/foaf.rdf#me> , <http://smethur.st/#me> ;
        <http://purl.org/dc/elements/1.1/creator>
                <http://moustaki.org/foaf.rdf#moustaki> ;
        <http://purl.org/dc/elements/1.1/date>
                "2009/02/20 16:00:00" ;
        <http://purl.org/dc/terms/license>
                <http://creativecommons.org/licenses/by/4.0#id> ;
        <http://www.bbc.co.uk/ontologies/provenance/canonicalLocation>
                "https://repo.dev.bbc.co.uk/services/linked-data/ontologies/domain/programmes" ;
        <http://www.bbc.co.uk/ontologies/provenance/changeReason>
                "Adding contributor"@en-gb ;
        <http://www.bbc.co.uk/ontologies/provenance/public>
                true ;
        <http://www.bbc.co.uk/ontologies/provenance/slug>
                "po" ;
        <http://www.bbc.co.uk/ontologies/provenance/version>
                "1.1" ;
        <http://www.w3.org/2002/07/owl#imports>
                <http://purl.org/NET/c4dm/event.owl> , <http://purl.org/dc/terms/> , <http://purl.org/NET/c4dm/timeline.owl> , <http://purl.org/dc/elements/1.1/> , <http://www.bbc.co.uk/ontologies/provenance> ;
        <http://www.w3.org/2002/07/owl#priorVersion>
                <http://purl.org/ontology/po/1.0> ;
        <http://www.w3.org/2002/07/owl#versionIRI>
                <http://purl.org/ontology/po/1.1> ;
        <http://www.w3.org/2002/07/owl#versionInfo>
                "1.1" .

<http://purl.org/ontology/po/masterbrand>
        a       <http://www.w3.org/2002/07/owl#ObjectProperty> ;
        <http://www.w3.org/2000/01/rdf-schema#comment>
                "Associates a programme with its masterbrand (its commissioner)" ;
        <http://www.w3.org/2000/01/rdf-schema#domain>
                <http://purl.org/ontology/po/Programme> ;
        <http://www.w3.org/2000/01/rdf-schema#isDefinedBy>
                <http://purl.org/ontology/po/> ;
        <http://www.w3.org/2000/01/rdf-schema#label>
                "masterbrand" ;
        <http://www.w3.org/2000/01/rdf-schema#range>
                <http://purl.org/ontology/po/Service> ;
        <http://www.w3.org/2003/06/sw-vocab-status/ns#term_status>
                "stable" .

<http://purl.org/ontology/po/Genre>
        a       <http://www.w3.org/2002/07/owl#Class> ;
        <http://www.w3.org/2000/01/rdf-schema#comment>
                "\n        An anchor point for a programmes' genre taxonomy, e.g. 'Drama'/'Biographical'.\n\t" ;
        <http://www.w3.org/2000/01/rdf-schema#isDefinedBy>
                <http://purl.org/ontology/po/> ;
        <http://www.w3.org/2000/01/rdf-schema#label>
                "Genre" ;
        <http://www.w3.org/2000/01/rdf-schema#subClassOf>
                <http://purl.org/ontology/po/Category> ;
        <http://www.w3.org/2003/06/sw-vocab-status/ns#term_status>
                "testing" .

<http://purl.org/ontology/po/anchor>
        a       <http://www.w3.org/2002/07/owl#ObjectProperty> ;
        <http://www.w3.org/2000/01/rdf-schema#comment>
                "A television reporter who coordinates a programme" ;
        <http://www.w3.org/2000/01/rdf-schema#domain>
                <http://purl.org/ontology/po/Programme> ;
        <http://www.w3.org/2000/01/rdf-schema#isDefinedBy>
                <http://purl.org/ontology/po/> ;
        <http://www.w3.org/2000/01/rdf-schema#label>
                "anchor" ;
        <http://www.w3.org/2000/01/rdf-schema#range>
                <http://xmlns.com/foaf/0.1/Agent> ;
        <http://www.w3.org/2000/01/rdf-schema#subPropertyOf>
                <http://purl.org/ontology/po/credit> ;
        <http://www.w3.org/2003/06/sw-vocab-status/ns#term_status>
                "testing" .

<http://purl.org/ontology/po/producer>
        a       <http://www.w3.org/2002/07/owl#ObjectProperty> ;
        <http://www.w3.org/2000/01/rdf-schema#comment>
                "Relates a programme to its producer - the manager of an event, show, or other work, usually the individual in charge of finance, personnel, and other non-artistic aspects in the development of commercials, plays, movies, and other works" ;
        <http://www.w3.org/2000/01/rdf-schema#domain>
                <http://purl.org/ontology/po/Programme> ;
        <http://www.w3.org/2000/01/rdf-schema#isDefinedBy>
                <http://purl.org/ontology/po/> ;
        <http://www.w3.org/2000/01/rdf-schema#label>
                "producer" ;
        <http://www.w3.org/2000/01/rdf-schema#range>
                <http://xmlns.com/foaf/0.1/Agent> ;
        <http://www.w3.org/2000/01/rdf-schema#subPropertyOf>
                <http://purl.org/ontology/po/credit> ;
        <http://www.w3.org/2003/06/sw-vocab-status/ns#term_status>
                "testing" .

<http://purl.org/ontology/po/ShortenedVersion>
        a       <http://www.w3.org/2002/07/owl#Class> ;
        <http://www.w3.org/2000/01/rdf-schema#comment>
                "\n\t\tA shortened version.\n\t" ;
        <http://www.w3.org/2000/01/rdf-schema#isDefinedBy>
                <http://purl.org/ontology/po/> ;
        <http://www.w3.org/2000/01/rdf-schema#label>
                "ShortenedVersion" ;
        <http://www.w3.org/2000/01/rdf-schema#subClassOf>
                <http://purl.org/ontology/po/Version> ;
        <http://www.w3.org/2002/07/owl#disjointWith>
                <http://purl.org/ontology/po/OriginalVersion> ;
        <http://www.w3.org/2003/06/sw-vocab-status/ns#term_status>
                "testing" .

<http://purl.org/ontology/po/episode>
        a       <http://www.w3.org/2002/07/owl#ObjectProperty> ;
        <http://www.w3.org/2000/01/rdf-schema#comment>
                "\n\t\tAssociates a brand or a series to an episode constituting it.\n\t" ;
        <http://www.w3.org/2000/01/rdf-schema#isDefinedBy>
                <http://purl.org/ontology/po/> ;
        <http://www.w3.org/2000/01/rdf-schema#label>
                "episode" ;
        <http://www.w3.org/2000/01/rdf-schema#range>
                <http://purl.org/ontology/po/Episode> ;
        <http://www.w3.org/2000/01/rdf-schema#subPropertyOf>
                <http://purl.org/dc/terms/hasPart> ;
        <http://www.w3.org/2003/06/sw-vocab-status/ns#term_status>
                "testing" .

<http://purl.org/ontology/po/Subtitle>
        a       <http://www.w3.org/2002/07/owl#Class> ;
        <http://www.w3.org/2000/01/rdf-schema#comment>
                "\n        Classification of an episode version's region corresponding to a subtitle being shown.\n    " ;
        <http://www.w3.org/2000/01/rdf-schema#isDefinedBy>
                <http://purl.org/ontology/po/> ;
        <http://www.w3.org/2000/01/rdf-schema#label>
                "Subtitle" ;
        <http://www.w3.org/2000/01/rdf-schema#subClassOf>
                <http://purl.org/NET/c4dm/event.owl#Event> ;
        <http://www.w3.org/2003/06/sw-vocab-status/ns#term_status>
                "testing" .

<http://purl.org/ontology/po/text>
        a       <http://www.w3.org/2002/07/owl#DatatypeProperty> ;
        <http://www.w3.org/2000/01/rdf-schema#comment>
                "Associates a subtitle event to the corresponding text" ;
        <http://www.w3.org/2000/01/rdf-schema#domain>
                <http://purl.org/ontology/po/Subtitle> ;
        <http://www.w3.org/2000/01/rdf-schema#isDefinedBy>
                <http://purl.org/ontology/po/> ;
        <http://www.w3.org/2000/01/rdf-schema#label>
                "text" ;
        <http://www.w3.org/2000/01/rdf-schema#range>
                <http://www.w3.org/2001/XMLSchema#string> ;
        <http://www.w3.org/2003/06/sw-vocab-status/ns#term_status>
                "testing" .

<http://purl.org/ontology/po/subject>
        a       <http://www.w3.org/2002/07/owl#ObjectProperty> ;
        <http://www.w3.org/2000/01/rdf-schema#comment>
                "\n        Relates a programme to a subject (e.g. `Easter')\n    " ;
        <http://www.w3.org/2000/01/rdf-schema#domain>
                <http://purl.org/ontology/po/Programme> ;
        <http://www.w3.org/2000/01/rdf-schema#isDefinedBy>
                <http://purl.org/ontology/po/> ;
        <http://www.w3.org/2000/01/rdf-schema#label>
                "subject" ;
        <http://www.w3.org/2000/01/rdf-schema#range>
                <http://purl.org/ontology/po/Subject> ;
        <http://www.w3.org/2000/01/rdf-schema#subPropertyOf>
                <http://purl.org/ontology/po/category> ;
        <http://www.w3.org/2003/06/sw-vocab-status/ns#term_status>
                "testing" .

<http://purl.org/ontology/po/OriginalVersion>
        a       <http://www.w3.org/2002/07/owl#Class> ;
        <http://www.w3.org/2000/01/rdf-schema#comment>
                "\n\t\tAn `original' version, the legacy version of\n\t\ta particular episode.\n\t" ;
        <http://www.w3.org/2000/01/rdf-schema#isDefinedBy>
                <http://purl.org/ontology/po/> ;
        <http://www.w3.org/2000/01/rdf-schema#label>
                "OriginalVersion" ;
        <http://www.w3.org/2000/01/rdf-schema#subClassOf>
                <http://purl.org/ontology/po/Version> ;
        <http://www.w3.org/2002/07/owl#disjointWith>
                <http://purl.org/ontology/po/ShortenedVersion> ;
        <http://www.w3.org/2003/06/sw-vocab-status/ns#term_status>
                "testing" .

<http://purl.org/ontology/po/Radio>
        a       <http://www.w3.org/2002/07/owl#Class> ;
        <http://www.w3.org/2000/01/rdf-schema#comment>
                "\n\t\tServices that use a radio medium.\n\t" ;
        <http://www.w3.org/2000/01/rdf-schema#isDefinedBy>
                <http://purl.org/ontology/po/> ;
        <http://www.w3.org/2000/01/rdf-schema#label>
                "Radio" ;
        <http://www.w3.org/2000/01/rdf-schema#subClassOf>
                <http://purl.org/ontology/po/Service> ;
        <http://www.w3.org/2002/07/owl#disjointWith>
                <http://purl.org/ontology/po/Web> , <http://purl.org/ontology/po/TV> ;
        <http://www.w3.org/2003/06/sw-vocab-status/ns#term_status>
                "testing" .

<http://purl.org/ontology/po/service>
        a       <http://www.w3.org/2002/07/owl#FunctionalProperty> , <http://www.w3.org/2002/07/owl#ObjectProperty> ;
        <http://www.w3.org/2000/01/rdf-schema#comment>
                "\n\t\tAssociate a brand, series or episode to the master brand service.\n\t" ;
        <http://www.w3.org/2000/01/rdf-schema#domain>
                <http://purl.org/ontology/po/Programme> ;
        <http://www.w3.org/2000/01/rdf-schema#isDefinedBy>
                <http://purl.org/ontology/po/> ;
        <http://www.w3.org/2000/01/rdf-schema#label>
                "service" ;
        <http://www.w3.org/2000/01/rdf-schema#range>
                <http://purl.org/ontology/po/Service> ;
        <http://www.w3.org/2003/06/sw-vocab-status/ns#term_status>
                "testing" .

<http://purl.org/ontology/po/broadcast_of>
        a       <http://www.w3.org/2002/07/owl#ObjectProperty> ;
        <http://www.w3.org/2000/01/rdf-schema#comment>
                "\n\t\tRelates a particular broadcast to the version being broadcasted.\n\t\tSub-property of the event:factor one.\n\t" ;
        <http://www.w3.org/2000/01/rdf-schema#domain>
                <http://purl.org/ontology/po/Broadcast> ;
        <http://www.w3.org/2000/01/rdf-schema#isDefinedBy>
                <http://purl.org/ontology/po/> ;
        <http://www.w3.org/2000/01/rdf-schema#label>
                "broadcast of" ;
        <http://www.w3.org/2000/01/rdf-schema#range>
                <http://purl.org/ontology/po/Version> ;
        <http://www.w3.org/2000/01/rdf-schema#subPropertyOf>
                <http://purl.org/NET/c4dm/event.owl#factor> ;
        <http://www.w3.org/2003/06/sw-vocab-status/ns#term_status>
                "testing" .

<http://purl.org/ontology/po/Clip>
        a       <http://www.w3.org/2002/07/owl#Class> ;
        <http://www.w3.org/2000/01/rdf-schema#comment>
                "\n        A particular clip, e.g. `Clip of Top Gear, first series'\n    " ;
        <http://www.w3.org/2000/01/rdf-schema#isDefinedBy>
                <http://purl.org/ontology/po/> ;
        <http://www.w3.org/2000/01/rdf-schema#label>
                "Clip" ;
        <http://www.w3.org/2000/01/rdf-schema#subClassOf>
                <http://purl.org/ontology/po/ProgrammeItem> , <http://purl.org/ontology/po/Programme> ;
        <http://www.w3.org/2002/07/owl#disjointWith>
                <http://purl.org/ontology/po/Brand> , <http://purl.org/ontology/po/Series> ;
        <http://www.w3.org/2003/06/sw-vocab-status/ns#term_status>
                "testing" .

<http://purl.org/ontology/po/ProgrammeItem>
        a       <http://www.w3.org/2002/07/owl#Class> ;
        <http://www.w3.org/2000/01/rdf-schema#comment>
                "\n        A programme that can have versions, and as such can be broadcast or made available on-demand, e.g. a clip or an episode.\n    " ;
        <http://www.w3.org/2000/01/rdf-schema#isDefinedBy>
                <http://purl.org/ontology/po/> ;
        <http://www.w3.org/2000/01/rdf-schema#label>
                "ProgrammeItem" ;
        <http://www.w3.org/2000/01/rdf-schema#subClassOf>
                <http://purl.org/ontology/po/Programme> ;
        <http://www.w3.org/2002/07/owl#disjointWith>
                <http://purl.org/ontology/po/Series> , <http://purl.org/ontology/po/Brand> ;
        <http://www.w3.org/2003/06/sw-vocab-status/ns#term_status>
                "testing" .

<http://purl.org/ontology/po/clip>
        a       <http://www.w3.org/2002/07/owl#ObjectProperty> ;
        <http://www.w3.org/2000/01/rdf-schema#comment>
                "\n        Associates a brand, a series or an episode to a clip.\n    " ;
        <http://www.w3.org/2000/01/rdf-schema#isDefinedBy>
                <http://purl.org/ontology/po/> ;
        <http://www.w3.org/2000/01/rdf-schema#label>
                "clip" ;
        <http://www.w3.org/2000/01/rdf-schema#range>
                <http://purl.org/ontology/po/Clip> ;
        <http://www.w3.org/2000/01/rdf-schema#subPropertyOf>
                <http://purl.org/dc/terms/hasPart> ;
        <http://www.w3.org/2003/06/sw-vocab-status/ns#term_status>
                "testing" .

<http://purl.org/ontology/po/SignedVersion>
        a       <http://www.w3.org/2002/07/owl#Class> ;
        <http://www.w3.org/2000/01/rdf-schema#comment>
                "\n\t\tA version holding sign language.\n\t" ;
        <http://www.w3.org/2000/01/rdf-schema#isDefinedBy>
                <http://purl.org/ontology/po/> ;
        <http://www.w3.org/2000/01/rdf-schema#label>
                "SignLanguage" ;
        <http://www.w3.org/2000/01/rdf-schema#subClassOf>
                <http://purl.org/ontology/po/Version> ;
        <http://www.w3.org/2003/06/sw-vocab-status/ns#term_status>
                "testing" .

<http://purl.org/ontology/po/broadcast_on>
        a       <http://www.w3.org/2002/07/owl#ObjectProperty> ;
        <http://www.w3.org/2000/01/rdf-schema#comment>
                "\n\t\tRelates a particular broadcast to the service or outlet on which it was.\n\t\tSub-property of the event:factor one.\n\t" ;
        <http://www.w3.org/2000/01/rdf-schema#domain>
                <http://purl.org/ontology/po/Broadcast> ;
        <http://www.w3.org/2000/01/rdf-schema#isDefinedBy>
                <http://purl.org/ontology/po/> ;
        <http://www.w3.org/2000/01/rdf-schema#label>
                "broadcast on" ;
        <http://www.w3.org/2000/01/rdf-schema#range>
                <http://purl.org/ontology/po/Service> ;
        <http://www.w3.org/2000/01/rdf-schema#subPropertyOf>
                <http://purl.org/NET/c4dm/event.owl#factor> ;
        <http://www.w3.org/2002/07/owl#equivalentProperty>
                <http://purl.org/ontology/po/broadcasted_on> ;
        <http://www.w3.org/2003/06/sw-vocab-status/ns#term_status>
                "testing" .

<http://purl.org/ontology/po/location>
        a       <http://www.w3.org/2002/07/owl#ObjectProperty> ;
        <http://www.w3.org/2000/01/rdf-schema#comment>
                "\n\t\tAssociates a service to a geographic location,\n\t\taiming at capturing what this service aims at covering.\n\t" ;
        <http://www.w3.org/2000/01/rdf-schema#domain>
                <http://purl.org/ontology/po/Service> ;
        <http://www.w3.org/2000/01/rdf-schema#isDefinedBy>
                <http://purl.org/ontology/po/> ;
        <http://www.w3.org/2000/01/rdf-schema#label>
                "location" ;
        <http://www.w3.org/2000/01/rdf-schema#range>
                <http://www.w3.org/2003/01/geo/wgs84_pos#SpatialThing> ;
        <http://www.w3.org/2000/01/rdf-schema#subPropertyOf>
                <http://xmlns.com/foaf/0.1/based_near> ;
        <http://www.w3.org/2003/06/sw-vocab-status/ns#term_status>
                "testing" .

<http://purl.org/ontology/po/Format>
        a       <http://www.w3.org/2002/07/owl#Class> ;
        <http://www.w3.org/2000/01/rdf-schema#comment>
                "\n        Anchor point for format taxonomies, similar to po:Genre for genre taxonomies.\n        Instances of this concept include documentaries, talk shows, animation, etc.\n    " ;
        <http://www.w3.org/2000/01/rdf-schema#isDefinedBy>
                <http://purl.org/ontology/po/> ;
        <http://www.w3.org/2000/01/rdf-schema#label>
                "Format" ;
        <http://www.w3.org/2000/01/rdf-schema#subClassOf>
                <http://purl.org/ontology/po/Category> ;
        <http://www.w3.org/2003/06/sw-vocab-status/ns#term_status>
                "testing" .

<http://purl.org/ontology/po/short_synopsis>
        a       <http://www.w3.org/2002/07/owl#DatatypeProperty> ;
        <http://www.w3.org/2000/01/rdf-schema#comment>
                "\n\t\tA short synopsis of a series, brand or episode.\n\t\tSub-property of po:synopsis.\n\t" ;
        <http://www.w3.org/2000/01/rdf-schema#isDefinedBy>
                <http://purl.org/ontology/po/> ;
        <http://www.w3.org/2000/01/rdf-schema#label>
                "short synopsis" ;
        <http://www.w3.org/2000/01/rdf-schema#subPropertyOf>
                <http://purl.org/ontology/po/synopsis> ;
        <http://www.w3.org/2003/06/sw-vocab-status/ns#term_status>
                "testing" .

<http://purl.org/ontology/po/parent_service>
        a       <http://www.w3.org/2002/07/owl#TransitiveProperty> , <http://www.w3.org/2002/07/owl#ObjectProperty> ;
        <http://www.w3.org/2000/01/rdf-schema#comment>
                "\n\t\tRelates a service to another service encapsulating it (eg. `BBC One' and `BBC One South')\n\t" ;
        <http://www.w3.org/2000/01/rdf-schema#domain>
                <http://purl.org/ontology/po/Service> ;
        <http://www.w3.org/2000/01/rdf-schema#isDefinedBy>
                <http://purl.org/ontology/po/> ;
        <http://www.w3.org/2000/01/rdf-schema#label>
                "parent service" ;
        <http://www.w3.org/2000/01/rdf-schema#range>
                <http://purl.org/ontology/po/Service> ;
        <http://www.w3.org/2000/01/rdf-schema#subPropertyOf>
                <http://purl.org/dc/terms/isPartOf> ;
        <http://www.w3.org/2003/06/sw-vocab-status/ns#term_status>
                "testing" .

<http://purl.org/ontology/po/RegionalRadio>
        a       <http://www.w3.org/2002/07/owl#Class> ;
        <http://www.w3.org/2000/01/rdf-schema#comment>
                "\n\t\tRadio services aiming at a regional coverage.\n\t" ;
        <http://www.w3.org/2000/01/rdf-schema#isDefinedBy>
                <http://purl.org/ontology/po/> ;
        <http://www.w3.org/2000/01/rdf-schema#label>
                "RegionalRadio" ;
        <http://www.w3.org/2000/01/rdf-schema#subClassOf>
                <http://purl.org/ontology/po/Radio> ;
        <http://www.w3.org/2002/07/owl#disjointWith>
                <http://purl.org/ontology/po/NationalRadio> ;
        <http://www.w3.org/2003/06/sw-vocab-status/ns#term_status>
                "testing" .

<http://purl.org/ontology/po/executive_producer>
        a       <http://www.w3.org/2002/07/owl#ObjectProperty> ;
        <http://www.w3.org/2000/01/rdf-schema#comment>
                "Relates a programme to its executive producer - a producer who is not involved in any technical aspects of the making process, but who is still responsible for the overall production. Typically an executive producer handles business and legal issues" ;
        <http://www.w3.org/2000/01/rdf-schema#domain>
                <http://purl.org/ontology/po/Programme> ;
        <http://www.w3.org/2000/01/rdf-schema#isDefinedBy>
                <http://purl.org/ontology/po/> ;
        <http://www.w3.org/2000/01/rdf-schema#label>
                "executive producer" ;
        <http://www.w3.org/2000/01/rdf-schema#range>
                <http://xmlns.com/foaf/0.1/Agent> ;
        <http://www.w3.org/2000/01/rdf-schema#subPropertyOf>
                <http://purl.org/ontology/po/credit> ;
        <http://www.w3.org/2003/06/sw-vocab-status/ns#term_status>
                "testing" .

<http://purl.org/ontology/po/Season>
        a       <http://www.w3.org/2002/07/owl#Class> ;
        <http://www.w3.org/2000/01/rdf-schema#comment>
                "\n\t\tA season is a group of broadcasts.\n\t" ;
        <http://www.w3.org/2000/01/rdf-schema#isDefinedBy>
                <http://purl.org/ontology/po/> ;
        <http://www.w3.org/2000/01/rdf-schema#label>
                "Season" ;
        <http://www.w3.org/2003/06/sw-vocab-status/ns#term_status>
                "testing" .

<http://purl.org/ontology/po/Series>
        a       <http://www.w3.org/2002/07/owl#Class> ;
        <http://www.w3.org/2000/01/rdf-schema#comment>
                "\n\t\tA series, e.g. `Top Gear, first season'\n\t" ;
        <http://www.w3.org/2000/01/rdf-schema#isDefinedBy>
                <http://purl.org/ontology/po/> ;
        <http://www.w3.org/2000/01/rdf-schema#label>
                "Series" ;
        <http://www.w3.org/2000/01/rdf-schema#subClassOf>
                <http://purl.org/ontology/po/Programme> ;
        <http://www.w3.org/2003/06/sw-vocab-status/ns#term_status>
                "stable" .

<http://purl.org/ontology/po/director>
        a       <http://www.w3.org/2002/07/owl#ObjectProperty> ;
        <http://www.w3.org/2000/01/rdf-schema#comment>
                "Relates a programme to its supervisor. Generally refers to the person responsible for all audience-visible components of a program, film, or show, whereas the producer is responsible for the financial and other behind-the-scenes aspects. A director's duties might also include casting, script editing, shot selection, shot composition, and editing" ;
        <http://www.w3.org/2000/01/rdf-schema#domain>
                <http://purl.org/ontology/po/Programme> ;
        <http://www.w3.org/2000/01/rdf-schema#isDefinedBy>
                <http://purl.org/ontology/po/> ;
        <http://www.w3.org/2000/01/rdf-schema#label>
                "director" ;
        <http://www.w3.org/2000/01/rdf-schema#range>
                <http://xmlns.com/foaf/0.1/Agent> ;
        <http://www.w3.org/2000/01/rdf-schema#subPropertyOf>
                <http://purl.org/ontology/po/credit> ;
        <http://www.w3.org/2003/06/sw-vocab-status/ns#term_status>
                "testing" .

<http://purl.org/ontology/po/LocalRadio>
        a       <http://www.w3.org/2002/07/owl#Class> ;
        <http://www.w3.org/2000/01/rdf-schema#comment>
                "\n\t\tRadio services aiming at a local coverage.\n\t" ;
        <http://www.w3.org/2000/01/rdf-schema#isDefinedBy>
                <http://purl.org/ontology/po/> ;
        <http://www.w3.org/2000/01/rdf-schema#label>
                "LocalRadio" ;
        <http://www.w3.org/2000/01/rdf-schema#subClassOf>
                <http://purl.org/ontology/po/Radio> ;
        <http://www.w3.org/2002/07/owl#disjointWith>
                <http://purl.org/ontology/po/NationalRadio> , <http://purl.org/ontology/po/RegionalRadio> ;
        <http://www.w3.org/2003/06/sw-vocab-status/ns#term_status>
                "testing" .

<http://purl.org/ontology/po/Person>
        a       <http://www.w3.org/2002/07/owl#Class> ;
        <http://www.w3.org/2000/01/rdf-schema#comment>
                "A person" ;
        <http://www.w3.org/2000/01/rdf-schema#isDefinedBy>
                <http://purl.org/ontology/po/> ;
        <http://www.w3.org/2000/01/rdf-schema#label>
                "Person" ;
        <http://www.w3.org/2000/01/rdf-schema#subClassOf>
                <http://purl.org/ontology/po/Category> ;
        <http://www.w3.org/2002/07/owl#equivalentClass>
                <http://xmlns.com/foaf/0.1/Person> ;
        <http://www.w3.org/2003/06/sw-vocab-status/ns#term_status>
                "testing" .

<http://purl.org/ontology/po/Episode>
        a       <http://www.w3.org/2002/07/owl#Class> ;
        <http://www.w3.org/2000/01/rdf-schema#comment>
                "\n\t\tA particular episode, e.g. `Top Gear, first episode of the first series' or the film 'A Walk in the Sun' (http://www.bbc.co.uk/programmes/b00gfzdt)\n\t" ;
        <http://www.w3.org/2000/01/rdf-schema#isDefinedBy>
                <http://purl.org/ontology/po/> ;
        <http://www.w3.org/2000/01/rdf-schema#label>
                "Episode" ;
        <http://www.w3.org/2000/01/rdf-schema#subClassOf>
                <http://purl.org/ontology/po/ProgrammeItem> , <http://purl.org/ontology/po/Programme> ;
        <http://www.w3.org/2002/07/owl#disjointWith>
                <http://purl.org/ontology/po/Brand> , <http://purl.org/ontology/po/Series> ;
        <http://www.w3.org/2003/06/sw-vocab-status/ns#term_status>
                "stable" .

<http://purl.org/ontology/po/Brand>
        a       <http://www.w3.org/2002/07/owl#Class> ;
        <http://www.w3.org/2000/01/rdf-schema#comment>
                "\n\t\tA brand, e.g. `Top Gear'\n\t" ;
        <http://www.w3.org/2000/01/rdf-schema#isDefinedBy>
                <http://purl.org/ontology/po/> ;
        <http://www.w3.org/2000/01/rdf-schema#label>
                "Brand" ;
        <http://www.w3.org/2000/01/rdf-schema#subClassOf>
                <http://purl.org/ontology/po/Programme> ;
        <http://www.w3.org/2002/07/owl#disjointWith>
                <http://purl.org/ontology/po/Clip> , <http://purl.org/ontology/po/Series> , <http://purl.org/ontology/po/Episode> ;
        <http://www.w3.org/2003/06/sw-vocab-status/ns#term_status>
                "stable" .

<http://purl.org/ontology/po/broadcaster>
        a       <http://www.w3.org/2002/07/owl#ObjectProperty> ;
        <http://www.w3.org/2000/01/rdf-schema#comment>
                "\n\t\tAssociates a service to a broadcaster\n\t" ;
        <http://www.w3.org/2000/01/rdf-schema#domain>
                <http://purl.org/ontology/po/Service> ;
        <http://www.w3.org/2000/01/rdf-schema#isDefinedBy>
                <http://purl.org/ontology/po/> ;
        <http://www.w3.org/2000/01/rdf-schema#label>
                "broadcaster" ;
        <http://www.w3.org/2000/01/rdf-schema#range>
                <http://purl.org/ontology/po/Broadcaster> ;
        <http://www.w3.org/2003/06/sw-vocab-status/ns#term_status>
                "testing" .

<http://purl.org/ontology/po/Broadcaster>
        a       <http://www.w3.org/2002/07/owl#Class> ;
        <http://www.w3.org/2000/01/rdf-schema#comment>
                "\n\t\tAn organization responsible of some broadcasting services.\n        It can hold a set of services and outlets.\n\t" ;
        <http://www.w3.org/2000/01/rdf-schema#isDefinedBy>
                <http://purl.org/ontology/po/> ;
        <http://www.w3.org/2000/01/rdf-schema#label>
                "Broadcaster" ;
        <http://www.w3.org/2000/01/rdf-schema#subClassOf>
                <http://xmlns.com/foaf/0.1/Organization> ;
        <http://www.w3.org/2003/06/sw-vocab-status/ns#term_status>
                "stable" .

<http://purl.org/ontology/po/author>
        a       <http://www.w3.org/2002/07/owl#ObjectProperty> ;
        <http://www.w3.org/2000/01/rdf-schema#comment>
                "Relates a programme to its author - the person who created the content" ;
        <http://www.w3.org/2000/01/rdf-schema#domain>
                <http://purl.org/ontology/po/Programme> ;
        <http://www.w3.org/2000/01/rdf-schema#isDefinedBy>
                <http://purl.org/ontology/po/> ;
        <http://www.w3.org/2000/01/rdf-schema#label>
                "author" ;
        <http://www.w3.org/2000/01/rdf-schema#range>
                <http://xmlns.com/foaf/0.1/Agent> ;
        <http://www.w3.org/2000/01/rdf-schema#subPropertyOf>
                <http://purl.org/ontology/po/credit> ;
        <http://www.w3.org/2003/06/sw-vocab-status/ns#term_status>
                "testing" .

<http://purl.org/ontology/po/DVB>
        a       <http://www.w3.org/2002/07/owl#Class> ;
        <http://www.w3.org/2000/01/rdf-schema#comment>
                "\n\t\tDigital Video Broadcasting\n\t" ;
        <http://www.w3.org/2000/01/rdf-schema#isDefinedBy>
                <http://purl.org/ontology/po/> ;
        <http://www.w3.org/2000/01/rdf-schema#label>
                "DVB" ;
        <http://www.w3.org/2000/01/rdf-schema#subClassOf>
                <http://purl.org/ontology/po/Channel> ;
        <http://www.w3.org/2003/06/sw-vocab-status/ns#term_status>
                "testing" .

<http://purl.org/ontology/po/Segment>
        a       <http://www.w3.org/2002/07/owl#Class> ;
        <http://www.w3.org/2000/01/rdf-schema#comment>
                "\n\t\tClassification of an episode version's region, e.g. 'this track was played at that time'.\n\t" ;
        <http://www.w3.org/2000/01/rdf-schema#isDefinedBy>
                <http://purl.org/ontology/po/> ;
        <http://www.w3.org/2000/01/rdf-schema#label>
                "Segment" ;
        <http://www.w3.org/2000/01/rdf-schema#subClassOf>
                <http://purl.org/NET/c4dm/event.owl#Event> ;
        <http://www.w3.org/2003/06/sw-vocab-status/ns#term_status>
                "testing" .

<http://purl.org/ontology/po/synopsis>
        a       <http://www.w3.org/2002/07/owl#DatatypeProperty> ;
        <http://www.w3.org/2000/01/rdf-schema#comment>
                "\n\t\tThe synopsis of a series, brand or episode.\n\t" ;
        <http://www.w3.org/2000/01/rdf-schema#domain>
                <http://purl.org/ontology/po/Programme> ;
        <http://www.w3.org/2000/01/rdf-schema#isDefinedBy>
                <http://purl.org/ontology/po/> ;
        <http://www.w3.org/2000/01/rdf-schema#label>
                "synopsis" ;
        <http://www.w3.org/2000/01/rdf-schema#range>
                <http://www.w3.org/2001/XMLSchema#string> ;
        <http://www.w3.org/2003/06/sw-vocab-status/ns#term_status>
                "testing" .

<http://purl.org/ontology/po/long_synopsis>
        a       <http://www.w3.org/2002/07/owl#DatatypeProperty> ;
        <http://www.w3.org/2000/01/rdf-schema#comment>
                "\n\t\tA long synopsis of a series, brand or episode.\n\t\tSub-property of po:synopsis.\n\t" ;
        <http://www.w3.org/2000/01/rdf-schema#isDefinedBy>
                <http://purl.org/ontology/po/> ;
        <http://www.w3.org/2000/01/rdf-schema#label>
                "long synopsis" ;
        <http://www.w3.org/2000/01/rdf-schema#subPropertyOf>
                <http://purl.org/ontology/po/synopsis> ;
        <http://www.w3.org/2003/06/sw-vocab-status/ns#term_status>
                "testing" .

<http://purl.org/ontology/po/Subject>
        a       <http://www.w3.org/2002/07/owl#Class> ;
        <http://www.w3.org/2000/01/rdf-schema#comment>
                "\n        Anchor point for subject taxonomies.\n    " ;
        <http://www.w3.org/2000/01/rdf-schema#isDefinedBy>
                <http://purl.org/ontology/po/> ;
        <http://www.w3.org/2000/01/rdf-schema#label>
                "Subject" ;
        <http://www.w3.org/2000/01/rdf-schema#subClassOf>
                <http://purl.org/ontology/po/Category> ;
        <http://www.w3.org/2003/06/sw-vocab-status/ns#term_status>
                "testing" .

<http://purl.org/ontology/po/medium_synopsis>
        a       <http://www.w3.org/2002/07/owl#DatatypeProperty> ;
        <http://www.w3.org/2000/01/rdf-schema#comment>
                "\n\t\tA medium synopsis of a series, brand or episode.\n\t\tSub-property of po:synopsis.\n\t" ;
        <http://www.w3.org/2000/01/rdf-schema#isDefinedBy>
                <http://purl.org/ontology/po/> ;
        <http://www.w3.org/2000/01/rdf-schema#label>
                "medium synopsis" ;
        <http://www.w3.org/2000/01/rdf-schema#subPropertyOf>
                <http://purl.org/ontology/po/synopsis> ;
        <http://www.w3.org/2003/06/sw-vocab-status/ns#term_status>
                "testing" .

<http://purl.org/ontology/po/NationalRadio>
        a       <http://www.w3.org/2002/07/owl#Class> ;
        <http://www.w3.org/2000/01/rdf-schema#comment>
                "\n\t\tRadio services aiming at a national coverage.\n\t" ;
        <http://www.w3.org/2000/01/rdf-schema#isDefinedBy>
                <http://purl.org/ontology/po/> ;
        <http://www.w3.org/2000/01/rdf-schema#label>
                "NationalRadio" ;
        <http://www.w3.org/2000/01/rdf-schema#subClassOf>
                <http://purl.org/ontology/po/Radio> ;
        <http://www.w3.org/2003/06/sw-vocab-status/ns#term_status>
                "testing" .

<http://purl.org/ontology/po/Outlet>
        a       <http://www.w3.org/2002/07/owl#Class> ;
        <http://www.w3.org/2000/01/rdf-schema#comment>
                "\n        Outlet of a particular service, e.g. Radio 4 LW and FM for Radio 4.\n        Outlets are services which do not have variations.\n        The criterion for an outlet is its timeline.\n        For example, Radio 4 LW broadcasts on Analogue Long Wave, but also on Digital Satellite.\n        It corresponds to just one outlet, as they are simulcasts.\n        The two physical channels for broadcasts correspond to po:Channel.\n    " ;
        <http://www.w3.org/2000/01/rdf-schema#isDefinedBy>
                <http://purl.org/ontology/po/> ;
        <http://www.w3.org/2000/01/rdf-schema#label>
                "Outlet" ;
        <http://www.w3.org/2000/01/rdf-schema#subClassOf>
                <http://purl.org/ontology/po/Service> ;
        <http://www.w3.org/2003/06/sw-vocab-status/ns#term_status>
                "testing" .

<http://purl.org/ontology/po/FirstBroadcast>
        a       <http://www.w3.org/2002/07/owl#Class> ;
        <http://www.w3.org/2000/01/rdf-schema#comment>
                "\n\t\tSpecifies a broadcast as being the\n\t\tfirst one of a particular version.\n\t " ;
        <http://www.w3.org/2000/01/rdf-schema#isDefinedBy>
                <http://purl.org/ontology/po/> ;
        <http://www.w3.org/2000/01/rdf-schema#label>
                "FirstBroadcast" ;
        <http://www.w3.org/2000/01/rdf-schema#subClassOf>
                <http://purl.org/ontology/po/Broadcast> ;
        <http://www.w3.org/2002/07/owl#disjointWith>
                <http://purl.org/ontology/po/RepeatBroadcast> ;
        <http://www.w3.org/2003/06/sw-vocab-status/ns#term_status>
                "testing" .

<http://purl.org/ontology/po/subtitle_language>
        a       <http://www.w3.org/2002/07/owl#DatatypeProperty> ;
        <http://www.w3.org/2000/01/rdf-schema#comment>
                "Language of the subtitles embedded in a particular version" ;
        <http://www.w3.org/2000/01/rdf-schema#domain>
                <http://purl.org/ontology/po/Version> ;
        <http://www.w3.org/2000/01/rdf-schema#isDefinedBy>
                <http://purl.org/ontology/po/> ;
        <http://www.w3.org/2000/01/rdf-schema#label>
                "subtitle language" ;
        <http://www.w3.org/2000/01/rdf-schema#range>
                <http://www.w3.org/2001/XMLSchema#string> ;
        <http://www.w3.org/2003/06/sw-vocab-status/ns#term_status>
                "testing" .

<http://purl.org/ontology/po/news_reader>
        a       <http://www.w3.org/2002/07/owl#ObjectProperty> ;
        <http://www.w3.org/2000/01/rdf-schema#comment>
                "Relates a programme to its news reader" ;
        <http://www.w3.org/2000/01/rdf-schema#domain>
                <http://purl.org/ontology/po/Programme> ;
        <http://www.w3.org/2000/01/rdf-schema#isDefinedBy>
                <http://purl.org/ontology/po/> ;
        <http://www.w3.org/2000/01/rdf-schema#label>
                "news reader" ;
        <http://www.w3.org/2000/01/rdf-schema#range>
                <http://xmlns.com/foaf/0.1/Agent> ;
        <http://www.w3.org/2000/01/rdf-schema#subPropertyOf>
                <http://purl.org/ontology/po/credit> ;
        <http://www.w3.org/2003/06/sw-vocab-status/ns#term_status>
                "testing" .

<http://purl.org/ontology/po/AudioDescribedVersion>
        a       <http://www.w3.org/2002/07/owl#Class> ;
        <http://www.w3.org/2000/01/rdf-schema#comment>
                "\n\t\tA version holding an audio description.\n\t" ;
        <http://www.w3.org/2000/01/rdf-schema#isDefinedBy>
                <http://purl.org/ontology/po/> ;
        <http://www.w3.org/2000/01/rdf-schema#label>
                "AudioDescribedVersion" ;
        <http://www.w3.org/2000/01/rdf-schema#subClassOf>
                <http://purl.org/ontology/po/Version> ;
        <http://www.w3.org/2003/06/sw-vocab-status/ns#term_status>
                "testing" .

<http://purl.org/ontology/po/RepeatBroadcast>
        a       <http://www.w3.org/2002/07/owl#Class> ;
        <http://www.w3.org/2000/01/rdf-schema#comment>
                "\n\t\tSpecifies a broadcast as being a\n\t\trepeat.\n\t" ;
        <http://www.w3.org/2000/01/rdf-schema#isDefinedBy>
                <http://purl.org/ontology/po/> ;
        <http://www.w3.org/2000/01/rdf-schema#label>
                "Repeat" ;
        <http://www.w3.org/2000/01/rdf-schema#subClassOf>
                <http://purl.org/ontology/po/Broadcast> ;
        <http://www.w3.org/2002/07/owl#disjointWith>
                <http://purl.org/ontology/po/FirstBroadcast> ;
        <http://www.w3.org/2003/06/sw-vocab-status/ns#term_status>
                "testing" .

<http://purl.org/ontology/po/place>
        a       <http://www.w3.org/2002/07/owl#ObjectProperty> ;
        <http://www.w3.org/2000/01/rdf-schema#comment>
                "\n        Relates a programme to a place (e.g. `London')\n    " ;
        <http://www.w3.org/2000/01/rdf-schema#domain>
                <http://purl.org/ontology/po/Programme> ;
        <http://www.w3.org/2000/01/rdf-schema#isDefinedBy>
                <http://purl.org/ontology/po/> ;
        <http://www.w3.org/2000/01/rdf-schema#label>
                "place" ;
        <http://www.w3.org/2000/01/rdf-schema#range>
                <http://purl.org/ontology/po/Place> ;
        <http://www.w3.org/2000/01/rdf-schema#subPropertyOf>
                <http://purl.org/ontology/po/category> ;
        <http://www.w3.org/2003/06/sw-vocab-status/ns#term_status>
                "testing" .

<http://purl.org/ontology/po/frequency>
        a       <http://www.w3.org/2002/07/owl#DatatypeProperty> ;
        <http://www.w3.org/2000/01/rdf-schema#comment>
                "Associates a channel to its frequency" ;
        <http://www.w3.org/2000/01/rdf-schema#domain>
                <http://purl.org/ontology/po/Channel> ;
        <http://www.w3.org/2000/01/rdf-schema#isDefinedBy>
                <http://purl.org/ontology/po/> ;
        <http://www.w3.org/2000/01/rdf-schema#label>
                "frequency" ;
        <http://www.w3.org/2000/01/rdf-schema#range>
                <http://www.w3.org/2001/XMLSchema#float> ;
        <http://www.w3.org/2003/06/sw-vocab-status/ns#term_status>
                "testing" .

<http://purl.org/ontology/po/commentator>
        a       <http://www.w3.org/2002/07/owl#ObjectProperty> ;
        <http://www.w3.org/2000/01/rdf-schema#comment>
                "Relates a programme to one of its commentators" ;
        <http://www.w3.org/2000/01/rdf-schema#domain>
                <http://purl.org/ontology/po/Programme> ;
        <http://www.w3.org/2000/01/rdf-schema#isDefinedBy>
                <http://purl.org/ontology/po/> ;
        <http://www.w3.org/2000/01/rdf-schema#label>
                "commentator" ;
        <http://www.w3.org/2000/01/rdf-schema#range>
                <http://xmlns.com/foaf/0.1/Agent> ;
        <http://www.w3.org/2000/01/rdf-schema#subPropertyOf>
                <http://purl.org/ontology/po/credit> ;
        <http://www.w3.org/2003/06/sw-vocab-status/ns#term_status>
                "testing" .

<http://purl.org/ontology/po/TV>
        a       <http://www.w3.org/2002/07/owl#Class> ;
        <http://www.w3.org/2000/01/rdf-schema#comment>
                "\n\t\tServices that use a television medium.\n\t" ;
        <http://www.w3.org/2000/01/rdf-schema#isDefinedBy>
                <http://purl.org/ontology/po/> ;
        <http://www.w3.org/2000/01/rdf-schema#label>
                "TV" ;
        <http://www.w3.org/2000/01/rdf-schema#subClassOf>
                <http://purl.org/ontology/po/Service> ;
        <http://www.w3.org/2002/07/owl#disjointWith>
                <http://purl.org/ontology/po/Web> ;
        <http://www.w3.org/2003/06/sw-vocab-status/ns#term_status>
                "testing" .

<http://purl.org/ontology/po/performer>
        a       <http://www.w3.org/2002/07/owl#ObjectProperty> ;
        <http://www.w3.org/2000/01/rdf-schema#comment>
                "Relates a programme to an entertainer who performs a dramatic or musical work for audience" ;
        <http://www.w3.org/2000/01/rdf-schema#domain>
                <http://purl.org/ontology/po/Programme> ;
        <http://www.w3.org/2000/01/rdf-schema#isDefinedBy>
                <http://purl.org/ontology/po/> ;
        <http://www.w3.org/2000/01/rdf-schema#label>
                "performer" ;
        <http://www.w3.org/2000/01/rdf-schema#range>
                <http://xmlns.com/foaf/0.1/Agent> ;
        <http://www.w3.org/2000/01/rdf-schema#subPropertyOf>
                <http://purl.org/ontology/po/credit> ;
        <http://www.w3.org/2003/06/sw-vocab-status/ns#term_status>
                "testing" .

<http://purl.org/ontology/po/FM>
        a       <http://www.w3.org/2002/07/owl#Class> ;
        <http://www.w3.org/2000/01/rdf-schema#comment>
                "\n\t\tThe FM broadcast band\n\t" ;
        <http://www.w3.org/2000/01/rdf-schema#isDefinedBy>
                <http://purl.org/ontology/po/> ;
        <http://www.w3.org/2000/01/rdf-schema#label>
                "FM" ;
        <http://www.w3.org/2000/01/rdf-schema#subClassOf>
                <http://purl.org/ontology/po/Channel> ;
        <http://www.w3.org/2003/06/sw-vocab-status/ns#term_status>
                "testing" .

<http://purl.org/ontology/po/series>
        a       <http://www.w3.org/2002/07/owl#TransitiveProperty> , <http://www.w3.org/2002/07/owl#ObjectProperty> ;
        <http://www.w3.org/2000/01/rdf-schema#comment>
                "\n\t\tAssociates a brand or a series to a series constituting it.\n\t" ;
        <http://www.w3.org/2000/01/rdf-schema#isDefinedBy>
                <http://purl.org/ontology/po/> ;
        <http://www.w3.org/2000/01/rdf-schema#label>
                "series" ;
        <http://www.w3.org/2000/01/rdf-schema#range>
                <http://purl.org/ontology/po/Series> ;
        <http://www.w3.org/2000/01/rdf-schema#subPropertyOf>
                <http://purl.org/dc/terms/hasPart> ;
        <http://www.w3.org/2003/06/sw-vocab-status/ns#term_status>
                "testing" .

<http://purl.org/ontology/po/Broadcast>
        a       <http://www.w3.org/2002/07/owl#Class> ;
        <http://www.w3.org/2000/01/rdf-schema#comment>
                "\n\t\tA broadcast event.\n\t\tSubsumes the event concept defined in\n\t\tthe Event ontology.\n\t\tA broadcast is associated with a service, and with a\n\t\tparticular version of an episode.\n\t" ;
        <http://www.w3.org/2000/01/rdf-schema#isDefinedBy>
                <http://purl.org/ontology/po/> ;
        <http://www.w3.org/2000/01/rdf-schema#label>
                "Broadcast" ;
        <http://www.w3.org/2000/01/rdf-schema#subClassOf>
                <http://purl.org/NET/c4dm/event.owl#Event> ;
        <http://www.w3.org/2003/06/sw-vocab-status/ns#term_status>
                "stable" .

<http://purl.org/ontology/po/Place>
        a       <http://www.w3.org/2002/07/owl#Class> ;
        <http://www.w3.org/2000/01/rdf-schema#comment>
                "A physical place" ;
        <http://www.w3.org/2000/01/rdf-schema#isDefinedBy>
                <http://purl.org/ontology/po/> ;
        <http://www.w3.org/2000/01/rdf-schema#label>
                "Place" ;
        <http://www.w3.org/2000/01/rdf-schema#subClassOf>
                <http://purl.org/ontology/po/Category> ;
        <http://www.w3.org/2002/07/owl#equivalentClass>
                <http://www.w3.org/2003/01/geo/wgs84_pos#Feature> ;
        <http://www.w3.org/2003/06/sw-vocab-status/ns#term_status>
                "testing" .

<http://purl.org/ontology/po/MusicSegment>
        a       <http://www.w3.org/2002/07/owl#Class> ;
        <http://www.w3.org/2000/01/rdf-schema#comment>
                "\n\t\tClassification of an episode version's region corresponding to a musical track being played.\n\t" ;
        <http://www.w3.org/2000/01/rdf-schema#label>
                "MusicSegment" ;
        <http://www.w3.org/2000/01/rdf-schema#subClassOf>
                <http://purl.org/ontology/po/Segment> ;
        <http://www.w3.org/2003/06/sw-vocab-status/ns#term_status>
                "testing" .

<http://purl.org/ontology/po/category>
        a       <http://www.w3.org/2002/07/owl#ObjectProperty> ;
        <http://www.w3.org/2000/01/rdf-schema#comment>
                "\n        Relates a programme to a particular category, e.g. genre, format, place...\n    " ;
        <http://www.w3.org/2000/01/rdf-schema#domain>
                <http://purl.org/ontology/po/Programme> ;
        <http://www.w3.org/2000/01/rdf-schema#isDefinedBy>
                <http://purl.org/ontology/po/> ;
        <http://www.w3.org/2000/01/rdf-schema#label>
                "category" ;
        <http://www.w3.org/2000/01/rdf-schema#range>
                <http://purl.org/ontology/po/Genre> ;
        <http://www.w3.org/2003/06/sw-vocab-status/ns#term_status>
                "testing" .

<http://purl.org/ontology/po/time>
        a       <http://www.w3.org/2002/07/owl#ObjectProperty> ;
        <http://www.w3.org/2000/01/rdf-schema#comment>
                "Associates an episode's version or a version's segment with a temporal interval. This interval can be associated with a timeline, serving as an anchor for further temporal annotations, e.g. subtitles or played track" ;
        <http://www.w3.org/2000/01/rdf-schema#isDefinedBy>
                <http://purl.org/ontology/po/> ;
        <http://www.w3.org/2000/01/rdf-schema#label>
                "time" ;
        <http://www.w3.org/2000/01/rdf-schema#range>
                <http://purl.org/NET/c4dm/timeline.owl#Interval> ;
        <http://www.w3.org/2003/06/sw-vocab-status/ns#term_status>
                "stable" .

<http://purl.org/ontology/po/actor>
        a       <http://www.w3.org/2002/07/owl#ObjectProperty> ;
        <http://www.w3.org/2000/01/rdf-schema#comment>
                "Relates a programmes to one of its actors - a person who plays the role of a character" ;
        <http://www.w3.org/2000/01/rdf-schema#domain>
                <http://purl.org/ontology/po/Programme> ;
        <http://www.w3.org/2000/01/rdf-schema#isDefinedBy>
                <http://purl.org/ontology/po/> ;
        <http://www.w3.org/2000/01/rdf-schema#label>
                "actor" ;
        <http://www.w3.org/2000/01/rdf-schema#range>
                <http://xmlns.com/foaf/0.1/Agent> ;
        <http://www.w3.org/2000/01/rdf-schema#subPropertyOf>
                <http://purl.org/ontology/po/credit> ;
        <http://www.w3.org/2003/06/sw-vocab-status/ns#term_status>
                "testing" .

<http://purl.org/ontology/po/channel>
        a       <http://www.w3.org/2002/07/owl#ObjectProperty> ;
        <http://www.w3.org/2000/01/rdf-schema#comment>
                "\n        Associates a service to a channel, e.g. Radio 4 LW to Radio 4 LW on Analogue Long Wave.\n    " ;
        <http://www.w3.org/2000/01/rdf-schema#domain>
                <http://purl.org/ontology/po/Service> ;
        <http://www.w3.org/2000/01/rdf-schema#isDefinedBy>
                <http://purl.org/ontology/po/> ;
        <http://www.w3.org/2000/01/rdf-schema#label>
                "channel" ;
        <http://www.w3.org/2000/01/rdf-schema#range>
                <http://purl.org/ontology/po/Channel> ;
        <http://www.w3.org/2003/06/sw-vocab-status/ns#term_status>
                "testing" .

<http://purl.org/ontology/po/SpeechSegment>
        a       <http://www.w3.org/2002/07/owl#Class> ;
        <http://www.w3.org/2000/01/rdf-schema#comment>
                "\n        Classification of an episode version's region holding speech content.\n    " ;
        <http://www.w3.org/2000/01/rdf-schema#subClassOf>
                <http://purl.org/ontology/po/Segment> ;
        <http://www.w3.org/2003/06/sw-vocab-status/ns#term_status>
                "testing" .

<http://purl.org/ontology/po/parent_series>
        a       <http://www.w3.org/2002/07/owl#ObjectProperty> , <http://www.w3.org/2002/07/owl#TransitiveProperty> ;
        <http://www.w3.org/2000/01/rdf-schema#comment>
                "\n\t\tRelates a series to a series constituting it (eg. `Waking the dead').\n\t" ;
        <http://www.w3.org/2000/01/rdf-schema#domain>
                <http://purl.org/ontology/po/Series> ;
        <http://www.w3.org/2000/01/rdf-schema#isDefinedBy>
                <http://purl.org/ontology/po/> ;
        <http://www.w3.org/2000/01/rdf-schema#label>
                "parent series" ;
        <http://www.w3.org/2000/01/rdf-schema#range>
                <http://purl.org/ontology/po/Series> ;
        <http://www.w3.org/2000/01/rdf-schema#subPropertyOf>
                <http://purl.org/dc/terms/isPartOf> ;
        <http://www.w3.org/2003/06/sw-vocab-status/ns#term_status>
                "testing" .

<http://purl.org/ontology/po/microsite>
        a       <http://www.w3.org/2002/07/owl#ObjectProperty> ;
        <http://www.w3.org/2000/01/rdf-schema#comment>
                "Associates a programme to its microsite. For example http://www.bbc.co.uk/programmes/b00fm04s and http://www.bbc.co.uk/eastenders/" ;
        <http://www.w3.org/2000/01/rdf-schema#domain>
                <http://purl.org/ontology/po/Programme> ;
        <http://www.w3.org/2000/01/rdf-schema#isDefinedBy>
                <http://purl.org/ontology/po/> ;
        <http://www.w3.org/2000/01/rdf-schema#label>
                "microsite" ;
        <http://www.w3.org/2000/01/rdf-schema#range>
                <http://xmlns.com/foaf/0.1/Document> ;
        <http://www.w3.org/2000/01/rdf-schema#subPropertyOf>
                <http://xmlns.com/foaf/0.1/page> ;
        <http://www.w3.org/2003/06/sw-vocab-status/ns#term_status>
                "testing" .

<http://purl.org/ontology/po/season_broadcast>
        a       <http://www.w3.org/2002/07/owl#ObjectProperty> ;
        <http://www.w3.org/2000/01/rdf-schema#comment>
                "Associates a season to its constituent broadcasts" ;
        <http://www.w3.org/2000/01/rdf-schema#domain>
                <http://purl.org/ontology/po/Season> ;
        <http://www.w3.org/2000/01/rdf-schema#isDefinedBy>
                <http://purl.org/ontology/po/> ;
        <http://www.w3.org/2000/01/rdf-schema#label>
                "broadcast" ;
        <http://www.w3.org/2000/01/rdf-schema#range>
                <http://purl.org/ontology/po/Broadcast> ;
        <http://www.w3.org/2003/06/sw-vocab-status/ns#term_status>
                "testing" .

<http://purl.org/ontology/po/outlet>
        a       <http://www.w3.org/2002/07/owl#ObjectProperty> ;
        <http://www.w3.org/2000/01/rdf-schema#comment>
                "\n\t\tAssociates a service to an outlet, e.g. Radio 4 to Radio 4 LW.\n\t" ;
        <http://www.w3.org/2000/01/rdf-schema#domain>
                <http://purl.org/ontology/po/Service> ;
        <http://www.w3.org/2000/01/rdf-schema#isDefinedBy>
                <http://purl.org/ontology/po/> ;
        <http://www.w3.org/2000/01/rdf-schema#label>
                "outlet" ;
        <http://www.w3.org/2000/01/rdf-schema#range>
                <http://purl.org/ontology/po/Outlet> ;
        <http://www.w3.org/2003/06/sw-vocab-status/ns#term_status>
                "testing" .

<http://purl.org/ontology/po/credit>
        a       <http://www.w3.org/2002/07/owl#ObjectProperty> ;
        <http://www.w3.org/2000/01/rdf-schema#comment>
                "Relates a programmes to a person who is credited in it" ;
        <http://www.w3.org/2000/01/rdf-schema#domain>
                <http://purl.org/ontology/po/Programme> ;
        <http://www.w3.org/2000/01/rdf-schema#isDefinedBy>
                <http://purl.org/ontology/po/> ;
        <http://www.w3.org/2000/01/rdf-schema#label>
                "credit" ;
        <http://www.w3.org/2000/01/rdf-schema#range>
                <http://xmlns.com/foaf/0.1/Agent> ;
        <http://www.w3.org/2000/01/rdf-schema#subPropertyOf>
                <http://purl.org/dc/elements/1.1/contributor> ;
        <http://www.w3.org/2003/06/sw-vocab-status/ns#term_status>
                "testing" .

<http://purl.org/ontology/po/Category>
        a       <http://www.w3.org/2002/07/owl#Class> ;
        <http://www.w3.org/2000/01/rdf-schema#comment>
                "\n        A category provides a way of classifying a set of programmes. Such classifications\n        can be performed according to multiple dimensions and taxonomies, e.g. genre, format, places, people, subjects...\n    " ;
        <http://www.w3.org/2000/01/rdf-schema#isDefinedBy>
                <http://purl.org/ontology/po/> ;
        <http://www.w3.org/2000/01/rdf-schema#label>
                "Category" ;
        <http://www.w3.org/2003/06/sw-vocab-status/ns#term_status>
                "testing" .

<http://purl.org/ontology/po/broadcasted_on>
        a       <http://www.w3.org/2002/07/owl#ObjectProperty> ;
        <http://www.w3.org/2000/01/rdf-schema#comment>
                "Deprecated property, left here for historical reasons" .

<http://purl.org/ontology/po/Web>
        a       <http://www.w3.org/2002/07/owl#Class> ;
        <http://www.w3.org/2000/01/rdf-schema#comment>
                "\n\t\tServices that use a Web medium.\n\t" ;
        <http://www.w3.org/2000/01/rdf-schema#isDefinedBy>
                <http://purl.org/ontology/po/> ;
        <http://www.w3.org/2000/01/rdf-schema#label>
                "Web" ;
        <http://www.w3.org/2000/01/rdf-schema#subClassOf>
                <http://purl.org/ontology/po/Service> ;
        <http://www.w3.org/2003/06/sw-vocab-status/ns#term_status>
                "testing" .

<http://purl.org/ontology/po/Service>
        a       <http://www.w3.org/2002/07/owl#Class> ;
        <http://www.w3.org/2000/01/rdf-schema#comment>
                "\n        A broadcasting service.\n\t\tInstances of this concept include BBC Radio Wales, BBC Radio 4, BBC News, etc.\n        A service is a collection of outlets which contain common material, but with some variations, e.g. by\n        region.\n        Hence, a service may have multiple outlets (po:Outlet), e.g. BBC Radio 4 has BBC Radio 4 LW and BBC Radio 4 FM.\n        A hierarchy of services types is defined within this ontology, e.g. radio and TV.\n        A service that is a master brand only (a service that only commissions programmes, e.g. BBC Switch) should\n        be an instance of the top-level po:Service.\n\t" ;
        <http://www.w3.org/2000/01/rdf-schema#isDefinedBy>
                <http://purl.org/ontology/po/> ;
        <http://www.w3.org/2000/01/rdf-schema#label>
                "Service" ;
        <http://www.w3.org/2003/06/sw-vocab-status/ns#term_status>
                "stable" .

<http://purl.org/ontology/po/person>
        a       <http://www.w3.org/2002/07/owl#ObjectProperty> ;
        <http://www.w3.org/2000/01/rdf-schema#comment>
                "\n        Relates a programme to a person\n    " ;
        <http://www.w3.org/2000/01/rdf-schema#domain>
                <http://purl.org/ontology/po/Programme> ;
        <http://www.w3.org/2000/01/rdf-schema#isDefinedBy>
                <http://purl.org/ontology/po/> ;
        <http://www.w3.org/2000/01/rdf-schema#label>
                "person" ;
        <http://www.w3.org/2000/01/rdf-schema#range>
                <http://purl.org/ontology/po/Person> ;
        <http://www.w3.org/2000/01/rdf-schema#subPropertyOf>
                <http://purl.org/ontology/po/category> ;
        <http://www.w3.org/2003/06/sw-vocab-status/ns#term_status>
                "testing" .

<http://purl.org/ontology/po/duration>
        a       <http://www.w3.org/2002/07/owl#DatatypeProperty> ;
        <http://www.w3.org/2000/01/rdf-schema#comment>
                "The duration of a version, in seconds." ;
        <http://www.w3.org/2000/01/rdf-schema#isDefinedBy>
                <http://purl.org/ontology/po/> ;
        <http://www.w3.org/2000/01/rdf-schema#label>
                "duration" ;
        <http://www.w3.org/2000/01/rdf-schema#range>
                <http://www.w3.org/2001/XMLSchema#int> ;
        <http://www.w3.org/2003/06/sw-vocab-status/ns#term_status>
                "testing" .

<http://purl.org/ontology/po/schedule_date>
        a       <http://www.w3.org/2002/07/owl#DatatypeProperty> ;
        <http://www.w3.org/2000/01/rdf-schema#comment>
                "\n\t\tThe schedule date of a broadcast event.\n\t" ;
        <http://www.w3.org/2000/01/rdf-schema#domain>
                <http://purl.org/ontology/po/Broadcast> ;
        <http://www.w3.org/2000/01/rdf-schema#isDefinedBy>
                <http://purl.org/ontology/po/> ;
        <http://www.w3.org/2000/01/rdf-schema#label>
                "schedule date" ;
        <http://www.w3.org/2000/01/rdf-schema#range>
                <http://www.w3.org/2001/XMLSchema#date> ;
        <http://www.w3.org/2003/06/sw-vocab-status/ns#term_status>
                "testing" .

<http://purl.org/ontology/po/track>
        a       <http://www.w3.org/2002/07/owl#ObjectProperty> ;
        <http://www.w3.org/2000/01/rdf-schema#comment>
                "Associates a music segment with a track, as defined in MO" ;
        <http://www.w3.org/2000/01/rdf-schema#domain>
                <http://purl.org/ontology/po/MusicSegment> ;
        <http://www.w3.org/2000/01/rdf-schema#isDefinedBy>
                <http://purl.org/ontology/po/> ;
        <http://www.w3.org/2000/01/rdf-schema#label>
                "track" ;
        <http://www.w3.org/2000/01/rdf-schema#range>
                <http://purl.org/ontology/mo/Track> ;
        <http://www.w3.org/2000/01/rdf-schema#subPropertyOf>
                <http://purl.org/NET/c4dm/event.owl#factor> ;
        <http://www.w3.org/2003/06/sw-vocab-status/ns#term_status>
                "testing" .

<http://purl.org/ontology/po/version>
        a       <http://www.w3.org/2002/07/owl#InverseFunctionalProperty> , <http://www.w3.org/2002/07/owl#ObjectProperty> ;
        <http://www.w3.org/2000/01/rdf-schema#comment>
                "\n\t\tAssociate an episode to a version of it.\n\t\tDifferent versions of a same episode can exist (shortened version, version\n\t\tdesigned for the hearing impaired, etc.).\n\t" ;
        <http://www.w3.org/2000/01/rdf-schema#domain>
                <http://purl.org/ontology/po/ProgrammeItem> ;
        <http://www.w3.org/2000/01/rdf-schema#isDefinedBy>
                <http://purl.org/ontology/po/> ;
        <http://www.w3.org/2000/01/rdf-schema#label>
                "version" ;
        <http://www.w3.org/2000/01/rdf-schema#range>
                <http://purl.org/ontology/po/Version> ;
        <http://www.w3.org/2003/06/sw-vocab-status/ns#term_status>
                "testing" .

<http://purl.org/ontology/po/genre>
        a       <http://www.w3.org/2002/07/owl#ObjectProperty> ;
        <http://www.w3.org/2000/01/rdf-schema#comment>
                "\n\t\tRelates a programme to a particular genre.\n\t" ;
        <http://www.w3.org/2000/01/rdf-schema#domain>
                <http://purl.org/ontology/po/Programme> ;
        <http://www.w3.org/2000/01/rdf-schema#isDefinedBy>
                <http://purl.org/ontology/po/> ;
        <http://www.w3.org/2000/01/rdf-schema#label>
                "genre" ;
        <http://www.w3.org/2000/01/rdf-schema#range>
                <http://purl.org/ontology/po/Genre> ;
        <http://www.w3.org/2000/01/rdf-schema#subPropertyOf>
                <http://purl.org/ontology/po/category> ;
        <http://www.w3.org/2003/06/sw-vocab-status/ns#term_status>
                "testing" .

<http://purl.org/ontology/po/format>
        a       <http://www.w3.org/2002/07/owl#ObjectProperty> ;
        <http://www.w3.org/2000/01/rdf-schema#comment>
                "\n\t\tRelates a programme to a particular format (eg. `Animation', `Documentary', etc.).\n\t" ;
        <http://www.w3.org/2000/01/rdf-schema#domain>
                <http://purl.org/ontology/po/Programme> ;
        <http://www.w3.org/2000/01/rdf-schema#isDefinedBy>
                <http://purl.org/ontology/po/> ;
        <http://www.w3.org/2000/01/rdf-schema#label>
                "format" ;
        <http://www.w3.org/2000/01/rdf-schema#range>
                <http://purl.org/ontology/po/Format> ;
        <http://www.w3.org/2000/01/rdf-schema#subPropertyOf>
                <http://purl.org/ontology/po/category> ;
        <http://www.w3.org/2003/06/sw-vocab-status/ns#term_status>
                "testing" .

<http://purl.org/ontology/po/aspect_ratio>
        a       <http://www.w3.org/2002/07/owl#DatatypeProperty> ;
        <http://www.w3.org/2000/01/rdf-schema#comment>
                "\n\t\tThe aspect ration of a particular version.\n\t" ;
        <http://www.w3.org/2000/01/rdf-schema#domain>
                <http://purl.org/ontology/po/Version> ;
        <http://www.w3.org/2000/01/rdf-schema#isDefinedBy>
                <http://purl.org/ontology/po/> ;
        <http://www.w3.org/2000/01/rdf-schema#label>
                "aspect ratio" ;
        <http://www.w3.org/2000/01/rdf-schema#range>
                <http://www.w3.org/2001/XMLSchema#string> ;
        <http://www.w3.org/2003/06/sw-vocab-status/ns#term_status>
                "testing" .

<http://purl.org/ontology/po/IPStream>
        a       <http://www.w3.org/2002/07/owl#Class> ;
        <http://www.w3.org/2000/01/rdf-schema#comment>
                "\n\t\tIP stream\n\t" ;
        <http://www.w3.org/2000/01/rdf-schema#isDefinedBy>
                <http://purl.org/ontology/po/> ;
        <http://www.w3.org/2000/01/rdf-schema#label>
                "IP stream" ;
        <http://www.w3.org/2000/01/rdf-schema#subClassOf>
                <http://purl.org/ontology/po/Channel> ;
        <http://www.w3.org/2003/06/sw-vocab-status/ns#term_status>
                "testing" .

<http://purl.org/ontology/po/position>
        a       <http://www.w3.org/2002/07/owl#DatatypeProperty> ;
        <http://www.w3.org/2000/01/rdf-schema#comment>
                "The position of a particular series or episode within its containing programme. This property can also be used to give the position of an interval within the containing timeline." ;
        <http://www.w3.org/2000/01/rdf-schema#isDefinedBy>
                <http://purl.org/ontology/po/> ;
        <http://www.w3.org/2000/01/rdf-schema#label>
                "position" ;
        <http://www.w3.org/2000/01/rdf-schema#range>
                <http://www.w3.org/2001/XMLSchema#int> ;
        <http://www.w3.org/2003/06/sw-vocab-status/ns#term_status>
                "testing" .

<http://purl.org/ontology/po/sound_format>
        a       <http://www.w3.org/2002/07/owl#DatatypeProperty> ;
        <http://www.w3.org/2000/01/rdf-schema#comment>
                "\n\t\tThe sound format of a particular version.\n\t" ;
        <http://www.w3.org/2000/01/rdf-schema#domain>
                <http://purl.org/ontology/po/Version> ;
        <http://www.w3.org/2000/01/rdf-schema#isDefinedBy>
                <http://purl.org/ontology/po/> ;
        <http://www.w3.org/2000/01/rdf-schema#label>
                "sound format" ;
        <http://www.w3.org/2000/01/rdf-schema#range>
                <http://www.w3.org/2001/XMLSchema#string> ;
        <http://www.w3.org/2003/06/sw-vocab-status/ns#term_status>
                "testing" .

<http://purl.org/ontology/po/Version>
        a       <http://www.w3.org/2002/07/owl#Class> ;
        <http://www.w3.org/2000/01/rdf-schema#comment>
                "\n\t\tA particular version of an episode.\n\t\tSuch versions include shortened ones, audio described ones\n\t\tor ones that holds sign language.\n\t\tThe version is associated to a timeline.\n\t" ;
        <http://www.w3.org/2000/01/rdf-schema#isDefinedBy>
                <http://purl.org/ontology/po/> ;
        <http://www.w3.org/2000/01/rdf-schema#label>
                "Version" ;
        <http://www.w3.org/2003/06/sw-vocab-status/ns#term_status>
                "stable" .

<http://purl.org/ontology/po/LW>
        a       <http://www.w3.org/2002/07/owl#Class> ;
        <http://www.w3.org/2000/01/rdf-schema#comment>
                "\n\t\tThe AM broadcast band\n\t" ;
        <http://www.w3.org/2000/01/rdf-schema#isDefinedBy>
                <http://purl.org/ontology/po/> ;
        <http://www.w3.org/2000/01/rdf-schema#label>
                "AM" ;
        <http://www.w3.org/2000/01/rdf-schema#subClassOf>
                <http://purl.org/ontology/po/Channel> ;
        <http://www.w3.org/2003/06/sw-vocab-status/ns#term_status>
                "testing" .

<http://purl.org/ontology/po/DAB>
        a       <http://www.w3.org/2002/07/owl#Class> ;
        <http://www.w3.org/2000/01/rdf-schema#comment>
                "\n\t\tDigital Audio Broadcasting\n\t" ;
        <http://www.w3.org/2000/01/rdf-schema#isDefinedBy>
                <http://purl.org/ontology/po/> ;
        <http://www.w3.org/2000/01/rdf-schema#label>
                "DAB" ;
        <http://www.w3.org/2000/01/rdf-schema#subClassOf>
                <http://purl.org/ontology/po/Channel> ;
        <http://www.w3.org/2003/06/sw-vocab-status/ns#term_status>
                "testing" .

<http://purl.org/ontology/po/participant>
        a       <http://www.w3.org/2002/07/owl#ObjectProperty> ;
        <http://www.w3.org/2000/01/rdf-schema#comment>
                "Relates a programme to one of its participants" ;
        <http://www.w3.org/2000/01/rdf-schema#domain>
                <http://purl.org/ontology/po/Programme> ;
        <http://www.w3.org/2000/01/rdf-schema#isDefinedBy>
                <http://purl.org/ontology/po/> ;
        <http://www.w3.org/2000/01/rdf-schema#label>
                "participant" ;
        <http://www.w3.org/2000/01/rdf-schema#range>
                <http://xmlns.com/foaf/0.1/Agent> ;
        <http://www.w3.org/2000/01/rdf-schema#subPropertyOf>
                <http://purl.org/ontology/po/credit> ;
        <http://www.w3.org/2003/06/sw-vocab-status/ns#term_status>
                "testing" .

<http://purl.org/ontology/po/Programme>
        a       <http://www.w3.org/2002/07/owl#Class> ;
        <http://www.w3.org/2000/01/rdf-schema#comment>
                "\n\t\tA programme, can either be a brand, a series or an episode\n\t" ;
        <http://www.w3.org/2000/01/rdf-schema#isDefinedBy>
                <http://purl.org/ontology/po/> ;
        <http://www.w3.org/2000/01/rdf-schema#label>
                "Programme" ;
        <http://www.w3.org/2003/06/sw-vocab-status/ns#term_status>
                "stable" .

<http://purl.org/ontology/po/Channel>
        a       <http://www.w3.org/2002/07/owl#Class> ;
        <http://www.w3.org/2000/01/rdf-schema#comment>
                "\n        A physical channel on which a broadcast occurs.\n        A single outlet or service can be associated with multiple channels.\n        For example, Radio 4 LW broadcasts on Analogue Long Wave and on Digital\n        Satellite.\n    " ;
        <http://www.w3.org/2000/01/rdf-schema#isDefinedBy>
                <http://purl.org/ontology/po/> ;
        <http://www.w3.org/2000/01/rdf-schema#label>
                "Channel" ;
        <http://www.w3.org/2003/06/sw-vocab-status/ns#term_status>
                "testing" .
