<http://www.loc.gov/premis/rdf/v3/Copyright>
        a       <http://www.w3.org/2002/07/owl#Class> ;
        <http://www.w3.org/2000/01/rdf-schema#comment>
                "Copyright law."@en ;
        <http://www.w3.org/2000/01/rdf-schema#isDefinedBy>
                <http://www.loc.gov/premis/rdf/v3/> ;
        <http://www.w3.org/2000/01/rdf-schema#label>
                "Copyright"@en ;
        <http://www.w3.org/2000/01/rdf-schema#seeAlso>
                <http://id.loc.gov/vocabulary/preservation/copyrightStatus> ;
        <http://www.w3.org/2000/01/rdf-schema#subClassOf>
                <http://www.loc.gov/premis/rdf/v3/RightsBasis> ;
        <http://www.w3.org/2002/07/owl#disjointWith>
                <http://www.loc.gov/premis/rdf/v3/InstitutionalPolicy> , <http://www.loc.gov/premis/rdf/v3/Statute> , <http://www.loc.gov/premis/rdf/v3/License> .

<http://www.loc.gov/premis/rdf/v3/Statute>
        a       <http://www.w3.org/2002/07/owl#Class> ;
        <http://www.w3.org/2000/01/rdf-schema#comment>
                "A law that grants or revokes rights, such as laws governing privacy or orphan\n      works."@en ;
        <http://www.w3.org/2000/01/rdf-schema#isDefinedBy>
                <http://www.loc.gov/premis/rdf/v3/> ;
        <http://www.w3.org/2000/01/rdf-schema#label>
                "Statute"@en ;
        <http://www.w3.org/2000/01/rdf-schema#subClassOf>
                <http://www.loc.gov/premis/rdf/v3/RightsBasis> ;
        <http://www.w3.org/2002/07/owl#disjointWith>
                <http://www.loc.gov/premis/rdf/v3/License> , <http://www.loc.gov/premis/rdf/v3/Copyright> , <http://www.loc.gov/premis/rdf/v3/InstitutionalPolicy> .

<http://www.loc.gov/premis/rdf/v3/OutcomeStatus>
        a       <http://www.w3.org/2002/07/owl#Class> ;
        <http://www.w3.org/2000/01/rdf-schema#comment>
                "Overall result of the Event in terms of success, partial success, or failure."@en ;
        <http://www.w3.org/2000/01/rdf-schema#isDefinedBy>
                <http://www.loc.gov/premis/rdf/v3/> ;
        <http://www.w3.org/2000/01/rdf-schema#label>
                "Outcome status"@en ;
        <http://www.w3.org/2000/01/rdf-schema#seeAlso>
                <http://id.loc.gov/vocabulary/preservation/eventOutcome> .

<http://www.loc.gov/premis/rdf/v3/key>
        a       <http://www.w3.org/2002/07/owl#DatatypeProperty> ;
        <http://www.w3.org/2000/01/rdf-schema#domain>
                [ a       <http://www.w3.org/2002/07/owl#Class> ;
                  <http://www.w3.org/2002/07/owl#unionOf>
                          ( <http://www.loc.gov/premis/rdf/v3/Inhibitor> <http://www.loc.gov/premis/rdf/v3/Signature> )
                ] ;
        <http://www.w3.org/2000/01/rdf-schema#isDefinedBy>
                <http://www.loc.gov/premis/rdf/v3/> ;
        <http://www.w3.org/2000/01/rdf-schema#label>
                "has key"@en ;
        <http://www.w3.org/2000/01/rdf-schema#range>
                <http://www.w3.org/2000/01/rdf-schema#Literal> .

<http://www.loc.gov/premis/rdf/v3/Inhibitor>
        a       <http://www.w3.org/2002/07/owl#Class> ;
        <http://www.w3.org/2000/01/rdf-schema#comment>
                "Feature of a Digital Object intended to inhibit access, copying, dissemination, or\n      migration. Common Inhibitors are encryption and password protection."@en ;
        <http://www.w3.org/2000/01/rdf-schema#isDefinedBy>
                <http://www.loc.gov/premis/rdf/v3/> ;
        <http://www.w3.org/2000/01/rdf-schema#label>
                "Inhibitor"@en ;
        <http://www.w3.org/2000/01/rdf-schema#seeAlso>
                <http://id.loc.gov/vocabulary/preservation/inhibitorType> .

<http://www.loc.gov/premis/rdf/v3/StorageLocation>
        a       <http://www.w3.org/2002/07/owl#Class> ;
        <http://www.w3.org/2000/01/rdf-schema#comment>
                "Information needed to retrieve a physical item from its physical storage location or a file\n      from the storage system, or to access a bitstream within a file."@en ;
        <http://www.w3.org/2000/01/rdf-schema#isDefinedBy>
                <http://www.loc.gov/premis/rdf/v3/> ;
        <http://www.w3.org/2000/01/rdf-schema#label>
                "Storage location"@en ;
        <http://www.w3.org/2000/01/rdf-schema#seeAlso>
                <http://id.loc.gov/vocabulary/preservation/contentLocationType> .

<http://www.loc.gov/premis/rdf/v3/size>
        a       <http://www.w3.org/2002/07/owl#DatatypeProperty> ;
        <http://www.w3.org/2000/01/rdf-schema#domain>
                [ a       <http://www.w3.org/2002/07/owl#Class> ;
                  <http://www.w3.org/2002/07/owl#unionOf>
                          ( <http://www.loc.gov/premis/rdf/v3/Bitstream> <http://www.loc.gov/premis/rdf/v3/File> )
                ] ;
        <http://www.w3.org/2000/01/rdf-schema#isDefinedBy>
                <http://www.loc.gov/premis/rdf/v3/> ;
        <http://www.w3.org/2000/01/rdf-schema#label>
                "has size"@en ;
        <http://www.w3.org/2000/01/rdf-schema#range>
                <http://www.w3.org/2001/XMLSchema#nonNegativeInteger> ;
        <http://www.w3.org/2004/02/skos/core#narrowMatch>
                <http://www.ebu.ch/metadata/ontologies/ebucore/ebucore#fileSize> .

<http://www.loc.gov/premis/rdf/v3/EnvironmentCharacteristic>
        a       <http://www.w3.org/2002/07/owl#Class> ;
        <http://www.w3.org/2000/01/rdf-schema#comment>
                "An assessment of the extent to which the described environment supports its\n      purpose."@en ;
        <http://www.w3.org/2000/01/rdf-schema#isDefinedBy>
                <http://www.loc.gov/premis/rdf/v3/> ;
        <http://www.w3.org/2000/01/rdf-schema#label>
                "Environment characteristic"@en ;
        <http://www.w3.org/2000/01/rdf-schema#seeAlso>
                <http://id.loc.gov/vocabulary/preservation/environmentCharacteristic> .

<http://www.loc.gov/premis/rdf/v3/signature>
        a       <http://www.w3.org/2002/07/owl#ObjectProperty> ;
        <http://www.w3.org/2000/01/rdf-schema#domain>
                [ a       <http://www.w3.org/2002/07/owl#Class> ;
                  <http://www.w3.org/2002/07/owl#unionOf>
                          ( <http://www.loc.gov/premis/rdf/v3/Bitstream> <http://www.loc.gov/premis/rdf/v3/File> )
                ] ;
        <http://www.w3.org/2000/01/rdf-schema#isDefinedBy>
                <http://www.loc.gov/premis/rdf/v3/> ;
        <http://www.w3.org/2000/01/rdf-schema#label>
                "has signature"@en ;
        <http://www.w3.org/2000/01/rdf-schema#range>
                <http://www.loc.gov/premis/rdf/v3/Signature> .

<http://www.loc.gov/premis/rdf/v3/File>
        a       <http://www.w3.org/2002/07/owl#Class> ;
        <http://www.w3.org/2000/01/rdf-schema#comment>
                "Named and ordered sequence of bytes that is known to an operating system."@en ;
        <http://www.w3.org/2000/01/rdf-schema#isDefinedBy>
                <http://www.loc.gov/premis/rdf/v3/> ;
        <http://www.w3.org/2000/01/rdf-schema#label>
                "File"@en ;
        <http://www.w3.org/2000/01/rdf-schema#subClassOf>
                <http://www.loc.gov/premis/rdf/v3/Object> ;
        <http://www.w3.org/2002/07/owl#disjointWith>
                <http://www.loc.gov/premis/rdf/v3/Bitstream> , <http://www.loc.gov/premis/rdf/v3/IntellectualEntity> , <http://www.loc.gov/premis/rdf/v3/Representation> .

<http://www.loc.gov/premis/rdf/v3/dependency>
        a       <http://www.w3.org/2002/07/owl#ObjectProperty> ;
        <http://www.w3.org/2000/01/rdf-schema#domain>
                <http://www.loc.gov/premis/rdf/v3/Object> ;
        <http://www.w3.org/2000/01/rdf-schema#isDefinedBy>
                <http://www.loc.gov/premis/rdf/v3/> ;
        <http://www.w3.org/2000/01/rdf-schema#label>
                "has dependency"@en ;
        <http://www.w3.org/2000/01/rdf-schema#range>
                <http://www.loc.gov/premis/rdf/v3/Dependency> .

<http://www.loc.gov/premis/rdf/v3/Action>
        a       <http://www.w3.org/2002/07/owl#Class> ;
        <http://www.w3.org/2000/01/rdf-schema#comment>
                "Operation type to perform on an Object. Effectively performing this action may produce an Event."@en ;
        <http://www.w3.org/2000/01/rdf-schema#isDefinedBy>
                <http://www.loc.gov/premis/rdf/v3/> ;
        <http://www.w3.org/2000/01/rdf-schema#label>
                "Action"@en ;
        <http://www.w3.org/2000/01/rdf-schema#seeAlso>
                <http://id.loc.gov/vocabulary/preservation/actionsGranted> .

<http://www.loc.gov/premis/rdf/v3/inhibits>
        a       <http://www.w3.org/2002/07/owl#ObjectProperty> ;
        <http://www.w3.org/2000/01/rdf-schema#domain>
                <http://www.loc.gov/premis/rdf/v3/Inhibitor> ;
        <http://www.w3.org/2000/01/rdf-schema#isDefinedBy>
                <http://www.loc.gov/premis/rdf/v3/> ;
        <http://www.w3.org/2000/01/rdf-schema#label>
                "inhibits"@en ;
        <http://www.w3.org/2000/01/rdf-schema#range>
                <http://www.loc.gov/premis/rdf/v3/Action> .

<http://www.loc.gov/premis/rdf/v3/outcomeNote>
        a       <http://www.w3.org/2002/07/owl#DatatypeProperty> ;
        <http://www.w3.org/2000/01/rdf-schema#domain>
                <http://www.loc.gov/premis/rdf/v3/Event> ;
        <http://www.w3.org/2000/01/rdf-schema#isDefinedBy>
                <http://www.loc.gov/premis/rdf/v3/> ;
        <http://www.w3.org/2000/01/rdf-schema#label>
                "has outcome note"@en ;
        <http://www.w3.org/2000/01/rdf-schema#range>
                <http://www.w3.org/2000/01/rdf-schema#Literal> ;
        <http://www.w3.org/2000/01/rdf-schema#subPropertyOf>
                <http://www.loc.gov/premis/rdf/v3/note> .

<http://www.loc.gov/premis/rdf/v3/note>
        a       <http://www.w3.org/2002/07/owl#DatatypeProperty> ;
        <http://www.w3.org/2000/01/rdf-schema#isDefinedBy>
                <http://www.loc.gov/premis/rdf/v3/> ;
        <http://www.w3.org/2000/01/rdf-schema#label>
                "has note"@en ;
        <http://www.w3.org/2000/01/rdf-schema#range>
                <http://www.w3.org/2000/01/rdf-schema#Literal> ;
        <http://www.w3.org/2000/01/rdf-schema#subPropertyOf>
                <http://purl.org/dc/terms/description> .

<http://www.loc.gov/premis/rdf/v3/Object>
        a       <http://www.w3.org/2002/07/owl#Class> ;
        <http://www.w3.org/2000/01/rdf-schema#comment>
                "Discrete unit of information subject to digital preservation. Subclasses of Object are\n      Intellectual Entity, Representation, File and Bitstream."@en ;
        <http://www.w3.org/2000/01/rdf-schema#isDefinedBy>
                <http://www.loc.gov/premis/rdf/v3/> ;
        <http://www.w3.org/2000/01/rdf-schema#label>
                "Object"@en ;
        <http://www.w3.org/2000/01/rdf-schema#subClassOf>
                <http://www.w3.org/ns/prov#Entity> .

<http://www.loc.gov/premis/rdf/v3/PreservationPolicy>
        a       <http://www.w3.org/2002/07/owl#Class> ;
        <http://www.w3.org/2000/01/rdf-schema#comment>
                "Information indicating the decision or policy on the set of preservation functions to be\n      applied to an object and the context in which the decision or policy was made. Note that in addition to\n      subclasses declared at presLevType, SignificantProperties is also a subclass of PreservationPolicy.\n      Implementers may also wish to create locally-defined subclasses."@en ;
        <http://www.w3.org/2000/01/rdf-schema#isDefinedBy>
                <http://www.loc.gov/premis/rdf/v3/> ;
        <http://www.w3.org/2000/01/rdf-schema#label>
                "Preservation policy"@en ;
        <http://www.w3.org/2000/01/rdf-schema#seeAlso>
                <http://id.loc.gov/vocabulary/preservation/preservationLevelRole> ;
        <http://www.w3.org/2000/01/rdf-schema#subClassOf>
                <http://purl.org/dc/terms/Policy> .

<http://www.loc.gov/premis/rdf/v3/Organization>
        a       <http://www.w3.org/2002/07/owl#Class> ;
        <http://www.w3.org/2000/01/rdf-schema#isDefinedBy>
                <http://www.loc.gov/premis/rdf/v3/> ;
        <http://www.w3.org/2000/01/rdf-schema#label>
                "Organization"@en ;
        <http://www.w3.org/2000/01/rdf-schema#subClassOf>
                <http://xmlns.com/foaf/0.1/Organization> , <http://www.loc.gov/premis/rdf/v3/Agent> , <http://www.w3.org/ns/prov#Organization> ;
        <http://www.w3.org/2002/07/owl#disjointWith>
                <http://www.loc.gov/premis/rdf/v3/HardwareAgent> , <http://www.loc.gov/premis/rdf/v3/Person> , <http://www.loc.gov/premis/rdf/v3/SoftwareAgent> .

<http://www.loc.gov/premis/rdf/v3/storedAt>
        a       <http://www.w3.org/2002/07/owl#ObjectProperty> ;
        <http://www.w3.org/2000/01/rdf-schema#domain>
                [ a       <http://www.w3.org/2002/07/owl#Class> ;
                  <http://www.w3.org/2002/07/owl#unionOf>
                          ( <http://www.loc.gov/premis/rdf/v3/Bitstream> <http://www.loc.gov/premis/rdf/v3/File> <http://www.loc.gov/premis/rdf/v3/Representation> )
                ] ;
        <http://www.w3.org/2000/01/rdf-schema#isDefinedBy>
                <http://www.loc.gov/premis/rdf/v3/> ;
        <http://www.w3.org/2000/01/rdf-schema#label>
                "stored at"@en ;
        <http://www.w3.org/2000/01/rdf-schema#range>
                <http://www.loc.gov/premis/rdf/v3/StorageLocation> .

<http://www.loc.gov/premis/rdf/v3/IntellectualEntity>
        a       <http://www.w3.org/2002/07/owl#Class> ;
        <http://www.w3.org/2000/01/rdf-schema#comment>
                " set of content that is considered a single intellectual unit for purposes of management and\n      description: for example, a particular book, map, photograph, database, or piece of hardware or\n      software. An Intellectual Entity can include other Intellectual Entities; for example, a web site can\n      include a web page; a web page can include an image. An Intellectual Entity may have one or more digital\n      representations. An Intellectual Entity may also describe an environment, defined as technology\n      supporting a digital object in some way (e.g. by rendering or executing it). Environments can consist of\n      software, hardware, or a combination of both."@en ;
        <http://www.w3.org/2000/01/rdf-schema#isDefinedBy>
                <http://www.loc.gov/premis/rdf/v3/> ;
        <http://www.w3.org/2000/01/rdf-schema#label>
                "Intellectual entity"@en ;
        <http://www.w3.org/2000/01/rdf-schema#seeAlso>
                <http://id.loc.gov/vocabulary/preservation/environmentFunctionType> ;
        <http://www.w3.org/2000/01/rdf-schema#subClassOf>
                <http://www.loc.gov/premis/rdf/v3/Object> ;
        <http://www.w3.org/2002/07/owl#disjointWith>
                <http://www.loc.gov/premis/rdf/v3/Representation> , <http://www.loc.gov/premis/rdf/v3/File> , <http://www.loc.gov/premis/rdf/v3/Bitstream> .

<http://www.loc.gov/premis/rdf/v3/policy>
        a       <http://www.w3.org/2002/07/owl#ObjectProperty> ;
        <http://www.w3.org/2000/01/rdf-schema#domain>
                <http://www.loc.gov/premis/rdf/v3/Object> ;
        <http://www.w3.org/2000/01/rdf-schema#isDefinedBy>
                <http://www.loc.gov/premis/rdf/v3/> ;
        <http://www.w3.org/2000/01/rdf-schema#label>
                "has policy"@en ;
        <http://www.w3.org/2000/01/rdf-schema#range>
                <http://www.loc.gov/premis/rdf/v3/PreservationPolicy> ;
        <http://www.w3.org/2000/01/rdf-schema#seeAlso>
                <http://id.loc.gov/vocabulary/preservation/preservationLevelRole> .

<http://www.loc.gov/premis/rdf/v3/InstitutionalPolicy>
        a       <http://www.w3.org/2002/07/owl#Class> ;
        <http://www.w3.org/2000/01/rdf-schema#comment>
                "A policy decision made by an organization."@en ;
        <http://www.w3.org/2000/01/rdf-schema#isDefinedBy>
                <http://www.loc.gov/premis/rdf/v3/> ;
        <http://www.w3.org/2000/01/rdf-schema#label>
                "Institutional policy"@en ;
        <http://www.w3.org/2000/01/rdf-schema#subClassOf>
                <http://www.loc.gov/premis/rdf/v3/RightsBasis> ;
        <http://www.w3.org/2002/07/owl#disjointWith>
                <http://www.loc.gov/premis/rdf/v3/Copyright> , <http://www.loc.gov/premis/rdf/v3/License> , <http://www.loc.gov/premis/rdf/v3/Statute> .

<http://www.loc.gov/premis/rdf/v3/License>
        a       <http://www.w3.org/2002/07/owl#Class> ;
        <http://www.w3.org/2000/01/rdf-schema#comment>
                "A license agreement or other legal document that grants rights."@en ;
        <http://www.w3.org/2000/01/rdf-schema#isDefinedBy>
                <http://www.loc.gov/premis/rdf/v3/> ;
        <http://www.w3.org/2000/01/rdf-schema#label>
                "License"@en ;
        <http://www.w3.org/2000/01/rdf-schema#subClassOf>
                <http://www.loc.gov/premis/rdf/v3/RightsBasis> ;
        <http://www.w3.org/2002/07/owl#disjointWith>
                <http://www.loc.gov/premis/rdf/v3/Statute> , <http://www.loc.gov/premis/rdf/v3/InstitutionalPolicy> , <http://www.loc.gov/premis/rdf/v3/Copyright> .

<http://www.loc.gov/premis/rdf/v3/>
        a       <http://www.w3.org/2002/07/owl#Ontology> ;
        <http://www.w3.org/2000/01/rdf-schema#comment>
                "Ontology for PREMIS 3, the international standard\n      for metadata to support the preservation of digital objects and ensure their\n      long-term usability."@en ;
        <http://www.w3.org/2000/01/rdf-schema#label>
                "PREMIS 3 Ontology"@en ;
        <http://www.w3.org/2000/01/rdf-schema#seeAlso>
                <http://www.loc.gov/standards/premis/> , <https://github.com/PREMIS-OWL-Revision-Team/revise-premis-owl/> ;
        <http://purl.org/dc/terms/modified>
                "2018-10-12"^^<http://www.w3.org/2001/XMLSchema#date> ;
        <http://www.w3.org/2002/07/owl#imports>
                <http://www.w3.org/ns/prov-o-20130430> ;
        <http://www.w3.org/2002/07/owl#versionIRI>
                <http://www.loc.gov/premis/rdf/v3/2018/10/12/> ;
        <http://www.w3.org/2002/07/owl#versionInfo>
                "2018/10/12" .

<http://www.loc.gov/premis/rdf/v3/encoding>
        a       <http://www.w3.org/2002/07/owl#ObjectProperty> ;
        <http://www.w3.org/2000/01/rdf-schema#domain>
                <http://www.loc.gov/premis/rdf/v3/Signature> ;
        <http://www.w3.org/2000/01/rdf-schema#isDefinedBy>
                <http://www.loc.gov/premis/rdf/v3/> ;
        <http://www.w3.org/2000/01/rdf-schema#label>
                "has encoding"@en ;
        <http://www.w3.org/2000/01/rdf-schema#range>
                <http://www.loc.gov/premis/rdf/v3/SignatureEncoding> .

<http://www.loc.gov/premis/rdf/v3/Person>
        a       <http://www.w3.org/2002/07/owl#Class> ;
        <http://www.w3.org/2000/01/rdf-schema#isDefinedBy>
                <http://www.loc.gov/premis/rdf/v3/> ;
        <http://www.w3.org/2000/01/rdf-schema#label>
                "Person"@en ;
        <http://www.w3.org/2000/01/rdf-schema#subClassOf>
                <http://www.loc.gov/premis/rdf/v3/Agent> , <http://www.w3.org/ns/prov#Person> , <http://xmlns.com/foaf/0.1/Person> ;
        <http://www.w3.org/2002/07/owl#disjointWith>
                <http://www.loc.gov/premis/rdf/v3/SoftwareAgent> , <http://www.loc.gov/premis/rdf/v3/HardwareAgent> , <http://www.loc.gov/premis/rdf/v3/Organization> .

<http://www.loc.gov/premis/rdf/v3/rightsStatus>
        a       <http://www.w3.org/2002/07/owl#ObjectProperty> ;
        <http://www.w3.org/2000/01/rdf-schema#domain>
                <http://www.loc.gov/premis/rdf/v3/Object> ;
        <http://www.w3.org/2000/01/rdf-schema#isDefinedBy>
                <http://www.loc.gov/premis/rdf/v3/> ;
        <http://www.w3.org/2000/01/rdf-schema#label>
                "has rights status"@en ;
        <http://www.w3.org/2000/01/rdf-schema#range>
                <http://www.loc.gov/premis/rdf/v3/RightsStatus> ;
        <http://www.w3.org/2000/01/rdf-schema#subPropertyOf>
                <http://purl.org/dc/elements/1.1/rights> .

<http://www.loc.gov/premis/rdf/v3/jurisdiction>
        a       <http://www.w3.org/2002/07/owl#ObjectProperty> ;
        <http://www.w3.org/2000/01/rdf-schema#domain>
                <http://www.loc.gov/premis/rdf/v3/RightsBasis> ;
        <http://www.w3.org/2000/01/rdf-schema#isDefinedBy>
                <http://www.loc.gov/premis/rdf/v3/> ;
        <http://www.w3.org/2000/01/rdf-schema#label>
                "has jurisdiction"@en ;
        <http://www.w3.org/2000/01/rdf-schema#range>
                <http://www.w3.org/2000/01/rdf-schema#Resource> .

<http://www.loc.gov/premis/rdf/v3/HardwareAgent>
        a       <http://www.w3.org/2002/07/owl#Class> ;
        <http://www.w3.org/2000/01/rdf-schema#isDefinedBy>
                <http://www.loc.gov/premis/rdf/v3/> ;
        <http://www.w3.org/2000/01/rdf-schema#label>
                "Hardware agent"@en ;
        <http://www.w3.org/2000/01/rdf-schema#subClassOf>
                <http://www.loc.gov/premis/rdf/v3/Agent> ;
        <http://www.w3.org/2002/07/owl#disjointWith>
                <http://www.loc.gov/premis/rdf/v3/SoftwareAgent> , <http://www.loc.gov/premis/rdf/v3/Person> , <http://www.loc.gov/premis/rdf/v3/Organization> ;
        <http://www.w3.org/2002/07/owl#sameAs>
                <http://id.loc.gov/vocabulary/preservation/agentType/har> .

<http://www.loc.gov/premis/rdf/v3/medium>
        a       <http://www.w3.org/2002/07/owl#ObjectProperty> ;
        <http://www.w3.org/2000/01/rdf-schema#domain>
                <http://www.loc.gov/premis/rdf/v3/StorageLocation> ;
        <http://www.w3.org/2000/01/rdf-schema#isDefinedBy>
                <http://www.loc.gov/premis/rdf/v3/> ;
        <http://www.w3.org/2000/01/rdf-schema#label>
                "has medium"@en ;
        <http://www.w3.org/2000/01/rdf-schema#range>
                <http://www.loc.gov/premis/rdf/v3/StorageMedium> .

<http://www.loc.gov/premis/rdf/v3/Bitstream>
        a       <http://www.w3.org/2002/07/owl#Class> ;
        <http://www.w3.org/2000/01/rdf-schema#comment>
                "Contiguous or non-contiguous data within a file that has meaningful properties for\n      preservation purposes."@en ;
        <http://www.w3.org/2000/01/rdf-schema#isDefinedBy>
                <http://www.loc.gov/premis/rdf/v3/> ;
        <http://www.w3.org/2000/01/rdf-schema#label>
                "Bitstream"@en ;
        <http://www.w3.org/2000/01/rdf-schema#subClassOf>
                <http://www.loc.gov/premis/rdf/v3/Object> ;
        <http://www.w3.org/2002/07/owl#disjointWith>
                <http://www.loc.gov/premis/rdf/v3/IntellectualEntity> , <http://www.loc.gov/premis/rdf/v3/Representation> , <http://www.loc.gov/premis/rdf/v3/File> .

<http://www.loc.gov/premis/rdf/v3/identifier>
        a       <http://www.w3.org/2002/07/owl#ObjectProperty> ;
        <http://www.w3.org/2000/01/rdf-schema#isDefinedBy>
                <http://www.loc.gov/premis/rdf/v3/> ;
        <http://www.w3.org/2000/01/rdf-schema#label>
                "has identifier"@en ;
        <http://www.w3.org/2000/01/rdf-schema#range>
                <http://www.loc.gov/premis/rdf/v3/Identifier> .

<http://www.loc.gov/premis/rdf/v3/rationale>
        a       <http://www.w3.org/2002/07/owl#DatatypeProperty> ;
        <http://www.w3.org/2000/01/rdf-schema#isDefinedBy>
                <http://www.loc.gov/premis/rdf/v3/> ;
        <http://www.w3.org/2000/01/rdf-schema#label>
                "has rationale"@en ;
        <http://www.w3.org/2000/01/rdf-schema#range>
                <http://www.w3.org/2000/01/rdf-schema#Literal> ;
        <http://www.w3.org/2000/01/rdf-schema#subPropertyOf>
                <http://www.loc.gov/premis/rdf/v3/note> .

<http://www.loc.gov/premis/rdf/v3/RightsStatus>
        a       <http://www.w3.org/2002/07/owl#Class> ;
        <http://www.w3.org/2000/01/rdf-schema#comment>
                "Information about how a RightsBasis applies to a particular object."@en ;
        <http://www.w3.org/2000/01/rdf-schema#isDefinedBy>
                <http://www.loc.gov/premis/rdf/v3/> ;
        <http://www.w3.org/2000/01/rdf-schema#label>
                "Rights status"@en .

<http://www.loc.gov/premis/rdf/v3/prohibits>
        a       <http://www.w3.org/2002/07/owl#ObjectProperty> ;
        <http://www.w3.org/2000/01/rdf-schema#domain>
                <http://www.loc.gov/premis/rdf/v3/RightsBasis> ;
        <http://www.w3.org/2000/01/rdf-schema#isDefinedBy>
                <http://www.loc.gov/premis/rdf/v3/> ;
        <http://www.w3.org/2000/01/rdf-schema#label>
                "prohibits"@en ;
        <http://www.w3.org/2000/01/rdf-schema#range>
                <http://www.loc.gov/premis/rdf/v3/Rule> .

<http://www.loc.gov/premis/rdf/v3/Representation>
        a       <http://www.w3.org/2002/07/owl#Class> ;
        <http://www.w3.org/2000/01/rdf-schema#comment>
                "Digital or physical Object instantiating or embodying an Intellectual Entity. A digital\n      representation is the set of stored digital files and structural metadata needed to provide a complete\n      and reasonable rendition of the Intellectual Entity. A physical representation is an item such as a\n      manuscript, video cassette, or printed document."@en ;
        <http://www.w3.org/2000/01/rdf-schema#isDefinedBy>
                <http://www.loc.gov/premis/rdf/v3/> ;
        <http://www.w3.org/2000/01/rdf-schema#label>
                "Representation"@en ;
        <http://www.w3.org/2000/01/rdf-schema#subClassOf>
                <http://www.loc.gov/premis/rdf/v3/Object> ;
        <http://www.w3.org/2002/07/owl#disjointWith>
                <http://www.loc.gov/premis/rdf/v3/Bitstream> , <http://www.loc.gov/premis/rdf/v3/File> , <http://www.loc.gov/premis/rdf/v3/IntellectualEntity> .

<http://www.loc.gov/premis/rdf/v3/Rule>
        a       <http://www.w3.org/2002/07/owl#Class> ;
        <http://www.w3.org/2000/01/rdf-schema#comment>
                "Statement about the Actions an Agent is permitted to undertake or prohibited from\n      undertaking with respect to an Object."@en ;
        <http://www.w3.org/2000/01/rdf-schema#isDefinedBy>
                <http://www.loc.gov/premis/rdf/v3/> ;
        <http://www.w3.org/2000/01/rdf-schema#label>
                "Rule"@en .

<http://www.loc.gov/premis/rdf/v3/terms>
        a       <http://www.w3.org/2002/07/owl#DatatypeProperty> ;
        <http://www.w3.org/2000/01/rdf-schema#domain>
                <http://www.loc.gov/premis/rdf/v3/RightsBasis> ;
        <http://www.w3.org/2000/01/rdf-schema#isDefinedBy>
                <http://www.loc.gov/premis/rdf/v3/> ;
        <http://www.w3.org/2000/01/rdf-schema#label>
                "has terms"@en ;
        <http://www.w3.org/2000/01/rdf-schema#range>
                <http://www.w3.org/2000/01/rdf-schema#Literal> ;
        <http://www.w3.org/2000/01/rdf-schema#subPropertyOf>
                <http://www.loc.gov/premis/rdf/v3/note> .

<http://www.loc.gov/premis/rdf/v3/Identifier>
        a       <http://www.w3.org/2002/07/owl#Class> ;
        <http://www.w3.org/2000/01/rdf-schema#comment>
                "An unambiguous reference to the PREMIS entity within the preservation\n      repository."@en ;
        <http://www.w3.org/2000/01/rdf-schema#isDefinedBy>
                <http://www.loc.gov/premis/rdf/v3/> ;
        <http://www.w3.org/2000/01/rdf-schema#label>
                "Identifier"@en .

<http://www.loc.gov/premis/rdf/v3/act>
        a       <http://www.w3.org/2002/07/owl#ObjectProperty> ;
        <http://www.w3.org/2000/01/rdf-schema#domain>
                <http://www.loc.gov/premis/rdf/v3/Rule> ;
        <http://www.w3.org/2000/01/rdf-schema#isDefinedBy>
                <http://www.loc.gov/premis/rdf/v3/> ;
        <http://www.w3.org/2000/01/rdf-schema#label>
                "act"@en ;
        <http://www.w3.org/2000/01/rdf-schema#range>
                <http://www.loc.gov/premis/rdf/v3/Action> .

<http://www.loc.gov/premis/rdf/v3/relationship>
        a       <http://www.w3.org/2002/07/owl#ObjectProperty> ;
        <http://www.w3.org/2000/01/rdf-schema#domain>
                [ a       <http://www.w3.org/2002/07/owl#Class> ;
                  <http://www.w3.org/2002/07/owl#unionOf>
                          ( <http://www.loc.gov/premis/rdf/v3/Agent> <http://www.loc.gov/premis/rdf/v3/Object> )
                ] ;
        <http://www.w3.org/2000/01/rdf-schema#isDefinedBy>
                <http://www.loc.gov/premis/rdf/v3/> ;
        <http://www.w3.org/2000/01/rdf-schema#label>
                "has relationship"@en ;
        <http://www.w3.org/2000/01/rdf-schema#range>
                <http://www.loc.gov/premis/rdf/v3/Object> ;
        <http://www.w3.org/2000/01/rdf-schema#seeAlso>
                <http://id.loc.gov/vocabulary/preservation/relationshipSubType> .

<http://www.loc.gov/premis/rdf/v3/allows>
        a       <http://www.w3.org/2002/07/owl#ObjectProperty> ;
        <http://www.w3.org/2000/01/rdf-schema#domain>
                <http://www.loc.gov/premis/rdf/v3/RightsBasis> ;
        <http://www.w3.org/2000/01/rdf-schema#isDefinedBy>
                <http://www.loc.gov/premis/rdf/v3/> ;
        <http://www.w3.org/2000/01/rdf-schema#label>
                "allows"@en ;
        <http://www.w3.org/2000/01/rdf-schema#range>
                <http://www.loc.gov/premis/rdf/v3/Rule> .

<http://www.loc.gov/premis/rdf/v3/RightsBasis>
        a       <http://www.w3.org/2002/07/owl#Class> ;
        <http://www.w3.org/2000/01/rdf-schema#comment>
                "Designation of the basis for the right or permission governing the Object."@en ;
        <http://www.w3.org/2000/01/rdf-schema#isDefinedBy>
                <http://www.loc.gov/premis/rdf/v3/> ;
        <http://www.w3.org/2000/01/rdf-schema#label>
                "Rights basis"@en ;
        <http://www.w3.org/2000/01/rdf-schema#seeAlso>
                <http://id.loc.gov/vocabulary/preservation/rightsBasis> .

<http://www.loc.gov/premis/rdf/v3/SignatureEncoding>
        a       <http://www.w3.org/2002/07/owl#Class> ;
        <http://www.w3.org/2000/01/rdf-schema#comment>
                "Encoding used for the signature value and key information."@en ;
        <http://www.w3.org/2000/01/rdf-schema#isDefinedBy>
                <http://www.loc.gov/premis/rdf/v3/> ;
        <http://www.w3.org/2000/01/rdf-schema#label>
                "Signature encoding"@en ;
        <http://www.w3.org/2000/01/rdf-schema#seeAlso>
                <http://id.loc.gov/vocabulary/preservation/signatureEncoding> .

<http://www.loc.gov/premis/rdf/v3/version>
        a       <http://www.w3.org/2002/07/owl#DatatypeProperty> ;
        <http://www.w3.org/2000/01/rdf-schema#domain>
                [ a       <http://www.w3.org/2002/07/owl#Class> ;
                  <http://www.w3.org/2002/07/owl#unionOf>
                          ( <http://purl.org/dc/terms/FileFormat> <http://www.loc.gov/premis/rdf/v3/HardwareAgent> <http://www.loc.gov/premis/rdf/v3/IntellectualEntity> <http://www.loc.gov/premis/rdf/v3/SoftwareAgent> )
                ] ;
        <http://www.w3.org/2000/01/rdf-schema#isDefinedBy>
                <http://www.loc.gov/premis/rdf/v3/> ;
        <http://www.w3.org/2000/01/rdf-schema#label>
                "has version"@en ;
        <http://www.w3.org/2000/01/rdf-schema#range>
                <http://www.w3.org/2000/01/rdf-schema#Literal> .

<http://www.loc.gov/premis/rdf/v3/validationRules>
        a       <http://www.w3.org/2002/07/owl#DatatypeProperty> ;
        <http://www.w3.org/2000/01/rdf-schema#domain>
                <http://www.loc.gov/premis/rdf/v3/Signature> ;
        <http://www.w3.org/2000/01/rdf-schema#isDefinedBy>
                <http://www.loc.gov/premis/rdf/v3/> ;
        <http://www.w3.org/2000/01/rdf-schema#label>
                "has validation rules"@en ;
        <http://www.w3.org/2000/01/rdf-schema#range>
                <http://www.w3.org/2000/01/rdf-schema#Literal> ;
        <http://www.w3.org/2000/01/rdf-schema#subPropertyOf>
                <http://www.loc.gov/premis/rdf/v3/note> .

<http://www.loc.gov/premis/rdf/v3/Fixity>
        a       <http://www.w3.org/2002/07/owl#Class> ;
        <http://www.w3.org/2000/01/rdf-schema#comment>
                "Information used to verify whether an object has been altered in an undocumented or\n      unauthorized way."@en ;
        <http://www.w3.org/2000/01/rdf-schema#isDefinedBy>
                <http://www.loc.gov/premis/rdf/v3/> ;
        <http://www.w3.org/2000/01/rdf-schema#label>
                "Fixity"@en ;
        <http://www.w3.org/2000/01/rdf-schema#seeAlso>
                <http://id.loc.gov/vocabulary/preservation/cryptographicHashFunctions> .

<http://www.loc.gov/premis/rdf/v3/compositionLevel>
        a       <http://www.w3.org/2002/07/owl#DatatypeProperty> ;
        <http://www.w3.org/2000/01/rdf-schema#domain>
                <http://www.loc.gov/premis/rdf/v3/File> ;
        <http://www.w3.org/2000/01/rdf-schema#isDefinedBy>
                <http://www.loc.gov/premis/rdf/v3/> ;
        <http://www.w3.org/2000/01/rdf-schema#label>
                "has composition level"@en ;
        <http://www.w3.org/2000/01/rdf-schema#range>
                <http://www.w3.org/2001/XMLSchema#nonNegativeInteger> .

<http://www.loc.gov/premis/rdf/v3/StorageMedium>
        a       <http://www.w3.org/2002/07/owl#Class> ;
        <http://www.w3.org/2000/01/rdf-schema#comment>
                "The physical medium on which the Object is stored (e.g., magnetic tape, hard disk, CD-ROM,\n      DVD)."@en ;
        <http://www.w3.org/2000/01/rdf-schema#isDefinedBy>
                <http://www.loc.gov/premis/rdf/v3/> ;
        <http://www.w3.org/2000/01/rdf-schema#label>
                "Storage medium"@en ;
        <http://www.w3.org/2000/01/rdf-schema#seeAlso>
                <http://id.loc.gov/vocabulary/preservation/storageMedium> .

<http://www.loc.gov/premis/rdf/v3/originalName>
        a       <http://www.w3.org/2002/07/owl#DatatypeProperty> ;
        <http://www.w3.org/2000/01/rdf-schema#domain>
                [ a       <http://www.w3.org/2002/07/owl#Class> ;
                  <http://www.w3.org/2002/07/owl#unionOf>
                          ( <http://www.loc.gov/premis/rdf/v3/File> <http://www.loc.gov/premis/rdf/v3/IntellectualEntity> <http://www.loc.gov/premis/rdf/v3/Representation> )
                ] ;
        <http://www.w3.org/2000/01/rdf-schema#isDefinedBy>
                <http://www.loc.gov/premis/rdf/v3/> ;
        <http://www.w3.org/2000/01/rdf-schema#label>
                "has original name"@en ;
        <http://www.w3.org/2000/01/rdf-schema#range>
                <http://www.w3.org/2000/01/rdf-schema#Literal> .

<http://www.loc.gov/premis/rdf/v3/Event>
        a       <http://www.w3.org/2002/07/owl#Class> ;
        <http://www.w3.org/2000/01/rdf-schema#comment>
                "Action performed within or outside the repository that affects its capability to preserve Objects over the long term."@en ;
        <http://www.w3.org/2000/01/rdf-schema#isDefinedBy>
                <http://www.loc.gov/premis/rdf/v3/> ;
        <http://www.w3.org/2000/01/rdf-schema#label>
                "Event"@en ;
        <http://www.w3.org/2000/01/rdf-schema#seeAlso>
                <http://id.loc.gov/vocabulary/preservation/eventType> ;
        <http://www.w3.org/2000/01/rdf-schema#subClassOf>
                <http://www.w3.org/ns/prov#Activity> .

<http://www.loc.gov/premis/rdf/v3/governs>
        a       <http://www.w3.org/2002/07/owl#ObjectProperty> ;
        <http://www.w3.org/2000/01/rdf-schema#domain>
                <http://www.loc.gov/premis/rdf/v3/RightsBasis> ;
        <http://www.w3.org/2000/01/rdf-schema#isDefinedBy>
                <http://www.loc.gov/premis/rdf/v3/> ;
        <http://www.w3.org/2000/01/rdf-schema#label>
                "governs"@en ;
        <http://www.w3.org/2000/01/rdf-schema#range>
                <http://www.loc.gov/premis/rdf/v3/Object> .

<http://www.loc.gov/premis/rdf/v3/documentation>
        a       <http://www.w3.org/2002/07/owl#ObjectProperty> ;
        <http://www.w3.org/2000/01/rdf-schema#isDefinedBy>
                <http://www.loc.gov/premis/rdf/v3/> ;
        <http://www.w3.org/2000/01/rdf-schema#label>
                "has documentation"@en ;
        <http://www.w3.org/2000/01/rdf-schema#range>
                <http://www.w3.org/2000/01/rdf-schema#Resource> .

<http://www.loc.gov/premis/rdf/v3/endDate>
        a       <http://www.w3.org/2002/07/owl#DatatypeProperty> ;
        <http://www.w3.org/2000/01/rdf-schema#domain>
                [ a       <http://www.w3.org/2002/07/owl#Class> ;
                  <http://www.w3.org/2002/07/owl#unionOf>
                          ( <http://www.loc.gov/premis/rdf/v3/RightsStatus> <http://www.loc.gov/premis/rdf/v3/Rule> )
                ] ;
        <http://www.w3.org/2000/01/rdf-schema#isDefinedBy>
                <http://www.loc.gov/premis/rdf/v3/> ;
        <http://www.w3.org/2000/01/rdf-schema#label>
                "end date"@en ;
        <http://www.w3.org/2000/01/rdf-schema#subPropertyOf>
                <http://purl.org/dc/terms/date> .

<http://www.loc.gov/premis/rdf/v3/characteristic>
        a       <http://www.w3.org/2002/07/owl#ObjectProperty> ;
        <http://www.w3.org/2000/01/rdf-schema#domain>
                <http://www.loc.gov/premis/rdf/v3/Dependency> ;
        <http://www.w3.org/2000/01/rdf-schema#isDefinedBy>
                <http://www.loc.gov/premis/rdf/v3/> ;
        <http://www.w3.org/2000/01/rdf-schema#label>
                "has characteristic"@en ;
        <http://www.w3.org/2000/01/rdf-schema#range>
                <http://www.loc.gov/premis/rdf/v3/EnvironmentCharacteristic> .

<http://www.loc.gov/premis/rdf/v3/SignificantProperties>
        a       <http://www.w3.org/2002/07/owl#Class> ;
        <http://www.w3.org/2000/01/rdf-schema#comment>
                "Characteristics of a particular object subjectively determined to be important to maintain\n      through preservation actions."@en ;
        <http://www.w3.org/2000/01/rdf-schema#isDefinedBy>
                <http://www.loc.gov/premis/rdf/v3/> ;
        <http://www.w3.org/2000/01/rdf-schema#label>
                "Significant properties"@en ;
        <http://www.w3.org/2000/01/rdf-schema#subClassOf>
                <http://www.loc.gov/premis/rdf/v3/PreservationPolicy> .

<http://www.loc.gov/premis/rdf/v3/SoftwareAgent>
        a       <http://www.w3.org/2002/07/owl#Class> ;
        <http://www.w3.org/2000/01/rdf-schema#isDefinedBy>
                <http://www.loc.gov/premis/rdf/v3/> ;
        <http://www.w3.org/2000/01/rdf-schema#label>
                "Software agent"@en ;
        <http://www.w3.org/2000/01/rdf-schema#subClassOf>
                <http://www.w3.org/ns/prov#SoftwareAgent> , <http://www.loc.gov/premis/rdf/v3/Agent> ;
        <http://www.w3.org/2002/07/owl#disjointWith>
                <http://www.loc.gov/premis/rdf/v3/Organization> , <http://www.loc.gov/premis/rdf/v3/HardwareAgent> , <http://www.loc.gov/premis/rdf/v3/Person> .

<http://www.loc.gov/premis/rdf/v3/fixity>
        a       <http://www.w3.org/2002/07/owl#ObjectProperty> ;
        <http://www.w3.org/2000/01/rdf-schema#domain>
                [ a       <http://www.w3.org/2002/07/owl#Class> ;
                  <http://www.w3.org/2002/07/owl#unionOf>
                          ( <http://www.loc.gov/premis/rdf/v3/Bitstream> <http://www.loc.gov/premis/rdf/v3/File> )
                ] ;
        <http://www.w3.org/2000/01/rdf-schema#isDefinedBy>
                <http://www.loc.gov/premis/rdf/v3/> ;
        <http://www.w3.org/2000/01/rdf-schema#label>
                "has fixity"@en ;
        <http://www.w3.org/2000/01/rdf-schema#range>
                <http://www.loc.gov/premis/rdf/v3/Fixity> .

<http://www.loc.gov/premis/rdf/v3/basis>
        a       <http://www.w3.org/2002/07/owl#ObjectProperty> ;
        <http://www.w3.org/2000/01/rdf-schema#comment>
                "Links from a RightsStatus to the RightsBasis instance that supports or documents\n      it."@en ;
        <http://www.w3.org/2000/01/rdf-schema#domain>
                <http://www.loc.gov/premis/rdf/v3/RightsStatus> ;
        <http://www.w3.org/2000/01/rdf-schema#isDefinedBy>
                <http://www.loc.gov/premis/rdf/v3/> ;
        <http://www.w3.org/2000/01/rdf-schema#label>
                "has basis"@en ;
        <http://www.w3.org/2000/01/rdf-schema#range>
                <http://www.loc.gov/premis/rdf/v3/RightsBasis> .

<http://www.loc.gov/premis/rdf/v3/citation>
        a       <http://www.w3.org/2002/07/owl#DatatypeProperty> ;
        <http://www.w3.org/2000/01/rdf-schema#domain>
                <http://www.loc.gov/premis/rdf/v3/RightsBasis> ;
        <http://www.w3.org/2000/01/rdf-schema#isDefinedBy>
                <http://www.loc.gov/premis/rdf/v3/> ;
        <http://www.w3.org/2000/01/rdf-schema#label>
                "has citation"@en ;
        <http://www.w3.org/2000/01/rdf-schema#range>
                <http://www.w3.org/2000/01/rdf-schema#Literal> .

<http://www.loc.gov/premis/rdf/v3/purpose>
        a       <http://www.w3.org/2002/07/owl#ObjectProperty> ;
        <http://www.w3.org/2000/01/rdf-schema#domain>
                <http://www.loc.gov/premis/rdf/v3/Dependency> ;
        <http://www.w3.org/2000/01/rdf-schema#isDefinedBy>
                <http://www.loc.gov/premis/rdf/v3/> ;
        <http://www.w3.org/2000/01/rdf-schema#label>
                "has purpose"@en ;
        <http://www.w3.org/2000/01/rdf-schema#range>
                <http://www.loc.gov/premis/rdf/v3/Action> .

<http://www.loc.gov/premis/rdf/v3/restriction>
        a       <http://www.w3.org/2002/07/owl#DatatypeProperty> ;
        <http://www.w3.org/2000/01/rdf-schema#domain>
                <http://www.loc.gov/premis/rdf/v3/Rule> ;
        <http://www.w3.org/2000/01/rdf-schema#isDefinedBy>
                <http://www.loc.gov/premis/rdf/v3/> ;
        <http://www.w3.org/2000/01/rdf-schema#label>
                "has restriction"@en ;
        <http://www.w3.org/2000/01/rdf-schema#range>
                <http://www.w3.org/2000/01/rdf-schema#Literal> .

<http://www.loc.gov/premis/rdf/v3/outcome>
        a       <http://www.w3.org/2002/07/owl#ObjectProperty> ;
        <http://www.w3.org/2000/01/rdf-schema#domain>
                <http://www.loc.gov/premis/rdf/v3/Event> ;
        <http://www.w3.org/2000/01/rdf-schema#isDefinedBy>
                <http://www.loc.gov/premis/rdf/v3/> ;
        <http://www.w3.org/2000/01/rdf-schema#label>
                "has outcome"@en ;
        <http://www.w3.org/2000/01/rdf-schema#range>
                <http://www.loc.gov/premis/rdf/v3/OutcomeStatus> .

<http://www.loc.gov/premis/rdf/v3/inhibitedBy>
        a       <http://www.w3.org/2002/07/owl#ObjectProperty> ;
        <http://www.w3.org/2000/01/rdf-schema#domain>
                [ a       <http://www.w3.org/2002/07/owl#Class> ;
                  <http://www.w3.org/2002/07/owl#unionOf>
                          ( <http://www.loc.gov/premis/rdf/v3/Bitstream> <http://www.loc.gov/premis/rdf/v3/File> )
                ] ;
        <http://www.w3.org/2000/01/rdf-schema#isDefinedBy>
                <http://www.loc.gov/premis/rdf/v3/> ;
        <http://www.w3.org/2000/01/rdf-schema#label>
                "inhibited by"@en ;
        <http://www.w3.org/2000/01/rdf-schema#range>
                <http://www.loc.gov/premis/rdf/v3/Inhibitor> .

<http://purl.org/dc/terms/FileFormat>
        a       <http://www.w3.org/2002/07/owl#Class> .

<http://www.loc.gov/premis/rdf/v3/startDate>
        a       <http://www.w3.org/2002/07/owl#DatatypeProperty> ;
        <http://www.w3.org/2000/01/rdf-schema#domain>
                [ a       <http://www.w3.org/2002/07/owl#Class> ;
                  <http://www.w3.org/2002/07/owl#unionOf>
                          ( <http://www.loc.gov/premis/rdf/v3/RightsStatus> <http://www.loc.gov/premis/rdf/v3/Rule> )
                ] ;
        <http://www.w3.org/2000/01/rdf-schema#isDefinedBy>
                <http://www.loc.gov/premis/rdf/v3/> ;
        <http://www.w3.org/2000/01/rdf-schema#label>
                "start date"@en ;
        <http://www.w3.org/2000/01/rdf-schema#subPropertyOf>
                <http://purl.org/dc/terms/date> .

<http://www.loc.gov/premis/rdf/v3/Agent>
        a       <http://www.w3.org/2002/07/owl#Class> ;
        <http://www.w3.org/2000/01/rdf-schema#comment>
                "Actor (human, machine, or software) associated with one or more Event and/or Rights\n      statement associated with a digital object."@en ;
        <http://www.w3.org/2000/01/rdf-schema#isDefinedBy>
                <http://www.loc.gov/premis/rdf/v3/> ;
        <http://www.w3.org/2000/01/rdf-schema#label>
                "Agent"@en ;
        <http://www.w3.org/2000/01/rdf-schema#subClassOf>
                <http://www.w3.org/ns/prov#Agent> , <http://xmlns.com/foaf/0.1/Agent> .

<http://www.loc.gov/premis/rdf/v3/determinationDate>
        a       <http://www.w3.org/2002/07/owl#DatatypeProperty> ;
        <http://www.w3.org/2000/01/rdf-schema#domain>
                <http://www.loc.gov/premis/rdf/v3/RightsStatus> ;
        <http://www.w3.org/2000/01/rdf-schema#isDefinedBy>
                <http://www.loc.gov/premis/rdf/v3/> ;
        <http://www.w3.org/2000/01/rdf-schema#label>
                "has determination date"@en ;
        <http://www.w3.org/2000/01/rdf-schema#range>
                <http://www.w3.org/2001/XMLSchema#date> ;
        <http://www.w3.org/2000/01/rdf-schema#subPropertyOf>
                <http://purl.org/dc/terms/date> .

<http://www.loc.gov/premis/rdf/v3/Signature>
        a       <http://www.w3.org/2002/07/owl#Class> ;
        <http://www.w3.org/2000/01/rdf-schema#comment>
                "Mathematical technique used to validate the authenticity and integrity of a message,\n      software or digital document."@en ;
        <http://www.w3.org/2000/01/rdf-schema#isDefinedBy>
                <http://www.loc.gov/premis/rdf/v3/> ;
        <http://www.w3.org/2000/01/rdf-schema#label>
                "Signature"@en ;
        <http://www.w3.org/2000/01/rdf-schema#seeAlso>
                <http://id.loc.gov/vocabulary/preservation/signatureMethod> .

<http://www.loc.gov/premis/rdf/v3/Dependency>
        a       <http://www.w3.org/2002/07/owl#Class> ;
        <http://www.w3.org/2000/01/rdf-schema#comment>
                "Relationship where one Object requires another Object to support its function, delivery, or\n      the coherence of its content."@en ;
        <http://www.w3.org/2000/01/rdf-schema#isDefinedBy>
                <http://www.loc.gov/premis/rdf/v3/> ;
        <http://www.w3.org/2000/01/rdf-schema#label>
                "Dependency"@en .
