<http://purl.org/wf4ever/wf4ever#File>
        a       <http://www.w3.org/2002/07/owl#Class> ;
        <http://www.w3.org/2000/01/rdf-schema#subClassOf>
                <http://purl.org/wf4ever/wfdesc#Artifact> .

<http://purl.org/wf4ever/wf4ever>
        a       <http://www.w3.org/2002/07/owl#Ontology> ;
        <http://www.w3.org/2000/01/rdf-schema#comment>
                "The wf4ever ontology. This is based on the wf4ever ontologies ro, wf and wfprov - but adds custom classes like wf4ever:Image and wf4ever:WebServiceProcess"@en ;
        <http://www.w3.org/2002/07/owl#imports>
                <http://purl.org/wf4ever/wfprov> , <http://purl.org/wf4ever/wfdesc> , <http://purl.org/wf4ever/ro> ;
        <http://www.w3.org/2002/07/owl#versionIRI>
                <https://raw.github.com/wf4ever/ro/0.1.1/wf4ever.owl> ;
        <http://www.w3.org/2002/07/owl#versionInfo>
                "0.1.1" .

<http://purl.org/wf4ever/wf4ever#WebServiceProcess>
        a       <http://www.w3.org/2002/07/owl#Class> ;
        <http://www.w3.org/2000/01/rdf-schema#comment>
                "WebServiceProcess is a wfdesc:Process description, the enactment of which gives rise to a web service call." ;
        <http://www.w3.org/2000/01/rdf-schema#subClassOf>
                <http://purl.org/wf4ever/wfdesc#Process> .

<http://purl.org/wf4ever/wf4ever#Dataset>
        a       <http://www.w3.org/2002/07/owl#Class> ;
        <http://www.w3.org/2000/01/rdf-schema#subClassOf>
                <http://purl.org/wf4ever/wfdesc#Artifact> .

<http://purl.org/wf4ever/wf4ever#WorkflowResearchObject>
        a       <http://www.w3.org/2002/07/owl#Class> ;
        <http://www.w3.org/2000/01/rdf-schema#comment>
                "A workflow research object is a research object that contains at least one workflow description." ;
        <http://www.w3.org/2002/07/owl#equivalentClass>
                [ a       <http://www.w3.org/2002/07/owl#Class> ;
                  <http://www.w3.org/2002/07/owl#intersectionOf>
                          ( <http://purl.org/wf4ever/ro#ResearchObject>
                            [ a       <http://www.w3.org/2002/07/owl#Restriction> ;
                              <http://www.w3.org/2002/07/owl#onProperty>
                                      <http://www.openarchives.org/ore/terms/aggregates> ;
                              <http://www.w3.org/2002/07/owl#someValuesFrom>
                                      <http://purl.org/wf4ever/wfdesc#Workflow>
                            ]
                          )
                ] .

<http://purl.org/wf4ever/wf4ever#Image>
        a       <http://www.w3.org/2002/07/owl#Class> ;
        <http://www.w3.org/2000/01/rdf-schema#subClassOf>
                <http://purl.org/wf4ever/wfdesc#Artifact> .

<http://purl.org/wf4ever/wf4ever#Document>
        a       <http://www.w3.org/2002/07/owl#Class> ;
        <http://www.w3.org/2000/01/rdf-schema#subClassOf>
                <http://purl.org/wf4ever/wfdesc#Artifact> .
