<https://w3id.org/won/core#targetSocket>
        a       <http://www.w3.org/2002/07/owl#ObjectProperty> ;
        <http://www.w3.org/2000/01/rdf-schema#comment>
                "Indicates that a remote atom or remote connection supports the specified socket (=behavior) or specifies the remote socket to connect with."@en ;
        <http://www.w3.org/2000/01/rdf-schema#domain>
                <https://w3id.org/won/core#Connection> ;
        <http://www.w3.org/2000/01/rdf-schema#isDefinedBy>
                <https://w3id.org/won/core> ;
        <http://www.w3.org/2000/01/rdf-schema#label>
                "targetSocket" ;
        <http://www.w3.org/2000/01/rdf-schema#range>
                <https://w3id.org/won/core#Socket> .

<https://w3id.org/won/core>
        a       <http://www.w3.org/2002/07/owl#Ontology> ;
        <http://www.w3.org/2000/01/rdf-schema#comment>
                "Ontology for the Web of Needs data model."@en ;
        <http://purl.org/dc/elements/1.1/abstract>
                "The Web of Needs is a decentralized linked data application infrastructure for mediating cooperation in the broadest sense. \n\nBased on append-only message logs, users (or other agents) publish and manage objects (*Atoms*). The main goal of publishing Atoms is to express interest in cooperation, for example by specifying something that is needed or being offered. However, Atoms can contain arbitrary data and thus be used to build general linked data knowledge graphs.\n\nAtoms can establish *Connections*  with other Atoms, if both Atoms' owners agree to it.\n\nMatching services can make suggestions which atoms to connect to. An Atom specifies 'Sockets' indicating the kinds of Connections it is prepared to establish."@en ;
        <http://purl.org/dc/elements/1.1/creator>
                "Fabian Salcher" , "Florian Kleedorfer" ;
        <http://purl.org/dc/elements/1.1/title>
                "Web of Needs Core Ontology" ;
        <http://purl.org/dc/terms/created>
                "2013-12-13"^^<http://www.w3.org/2001/XMLSchema#date> ;
        <http://purl.org/dc/terms/license>
                <https://creativecommons.org/licenses/by/4.0/> ;
        <http://purl.org/vocab/vann/preferredNamespacePrefix>
                "won" ;
        <http://www.w3.org/2002/07/owl#versionIRI>
                <https://w3id.org/won/core/1.0> .

<https://w3id.org/won/core#ConnectionState>
        a       <http://www.w3.org/2002/07/owl#Class> ;
        <http://www.w3.org/2000/01/rdf-schema#comment>
                "A Connection's state."@en ;
        <http://www.w3.org/2000/01/rdf-schema#isDefinedBy>
                <https://w3id.org/won/core> ;
        <http://www.w3.org/2000/01/rdf-schema#label>
                "ConnectionState" .

<https://w3id.org/won/core#Node>
        a       <http://www.w3.org/2002/07/owl#Class> ;
        <http://www.w3.org/2000/01/rdf-schema#comment>
                "A server storing Atoms and the data associated with them."@en ;
        <http://www.w3.org/2000/01/rdf-schema#label>
                "Node" .

<https://w3id.org/won/core#Connected>
        a       <http://www.w3.org/2002/07/owl#NamedIndividual> , <https://w3id.org/won/core#ConnectionState> ;
        <http://www.w3.org/2000/01/rdf-schema#comment>
                "The connected state. Messages are forwarded to/from the owner."@en ;
        <http://www.w3.org/2000/01/rdf-schema#isDefinedBy>
                <https://w3id.org/won/core> ;
        <http://www.w3.org/2000/01/rdf-schema#label>
                "Connected" .

<https://w3id.org/won/core#RequestSent>
        a       <https://w3id.org/won/core#ConnectionState> , <http://www.w3.org/2002/07/owl#NamedIndividual> ;
        <http://www.w3.org/2000/01/rdf-schema#comment>
                "Half-open state. The Connection has been requested by the local end but not yet been accepted by the remote counterpart."@en ;
        <http://www.w3.org/2000/01/rdf-schema#isDefinedBy>
                <https://w3id.org/won/core> ;
        <http://www.w3.org/2000/01/rdf-schema#label>
                "RequestSent" .

<https://w3id.org/won/core#SocketDefinition>
        a       <http://www.w3.org/2002/07/owl#Class> ;
        <http://www.w3.org/2000/01/rdf-schema#comment>
                "A Socket's definition."@en ;
        <http://www.w3.org/2000/01/rdf-schema#label>
                "SocketDefinition" .

<https://w3id.org/won/core#atomUriPrefix>
        a       <http://www.w3.org/2002/07/owl#DatatypeProperty> ;
        <http://www.w3.org/2000/01/rdf-schema#comment>
                "Specifies the prefix an atom must have on the node this specification applies to. This specification allows clients to generate new valid new Atom URIs."@en ;
        <http://www.w3.org/2000/01/rdf-schema#domain>
                <https://w3id.org/won/core#UriPrefixSpecification> ;
        <http://www.w3.org/2000/01/rdf-schema#label>
                "atomUriPrefix" ;
        <http://www.w3.org/2000/01/rdf-schema#range>
                <http://www.w3.org/2001/XMLSchema#string> .

<https://w3id.org/won/core#connectionState>
        a       <http://www.w3.org/2002/07/owl#ObjectProperty> , <http://www.w3.org/2002/07/owl#FunctionalProperty> ;
        <http://www.w3.org/2000/01/rdf-schema#comment>
                "Indicates the state in which the Connection object is."@en ;
        <http://www.w3.org/2000/01/rdf-schema#domain>
                <https://w3id.org/won/core#Connection> ;
        <http://www.w3.org/2000/01/rdf-schema#isDefinedBy>
                <https://w3id.org/won/core> ;
        <http://www.w3.org/2000/01/rdf-schema#label>
                "connectionState" ;
        <http://www.w3.org/2000/01/rdf-schema#range>
                <https://w3id.org/won/core#ConnectionState> .

<https://w3id.org/won/core#MessageContainer>
        a       <http://www.w3.org/2002/07/owl#Class> ;
        <http://www.w3.org/2000/01/rdf-schema#comment>
                "Container for Messages. The container supports LDP paging as described here: https://github.com/researchstudio-sat/webofneeds/blob/master/webofneeds/won-node-webapp/doc/linked-data-paging.md."@en ;
        <http://www.w3.org/2000/01/rdf-schema#isDefinedBy>
                <https://w3id.org/won/core> ;
        <http://www.w3.org/2000/01/rdf-schema#label>
                "MessageContainer" ;
        <http://www.w3.org/2000/01/rdf-schema#subClassOf>
                <http://www.w3.org/ns/ldp#CompositeContainer> .

<http://purl.org/dc/elements/1.1/description>
        a       <http://www.w3.org/2002/07/owl#AnnotationProperty> .

<https://w3id.org/won/core#socketCapacity>
        a       <http://www.w3.org/2002/07/owl#DatatypeProperty> ;
        <http://www.w3.org/2000/01/rdf-schema#comment>
                "Defines the maximum number of established connections supported by the socket."@en ;
        <http://www.w3.org/2000/01/rdf-schema#domain>
                <https://w3id.org/won/core#SocketDefinition> ;
        <http://www.w3.org/2000/01/rdf-schema#label>
                "socketCapacity" ;
        <http://www.w3.org/2000/01/rdf-schema#range>
                <http://www.w3.org/2001/XMLSchema#integer> .

<https://w3id.org/won/core#suggestedCount>
        a       <http://www.w3.org/2002/07/owl#DatatypeProperty> ;
        <http://www.w3.org/2000/01/rdf-schema#comment>
                "The number of connections in the container that are in state SUGGESTED."@en ;
        <http://www.w3.org/2000/01/rdf-schema#domain>
                <https://w3id.org/won/core#ConnectionContainer> ;
        <http://www.w3.org/2000/01/rdf-schema#label>
                "suggestedCount" ;
        <http://www.w3.org/2000/01/rdf-schema#range>
                <http://www.w3.org/2001/XMLSchema#integer> .

[ a       <http://www.w3.org/2002/07/owl#AllDifferent> ;
  <http://www.w3.org/2002/07/owl#distinctMembers>
          ()
] .

<https://w3id.org/won/core#derivesInverseAtomProperty>
        a       <http://www.w3.org/2002/07/owl#ObjectProperty> ;
        <http://www.w3.org/2000/01/rdf-schema#comment>
                "Defines a property to be 'derived' when the connection is established. The property will be used to derive a triple '[targetAtom] [property] [sourceAtom]'."@en ;
        <http://www.w3.org/2000/01/rdf-schema#domain>
                <https://w3id.org/won/core#SocketDefinition> ;
        <http://www.w3.org/2000/01/rdf-schema#label>
                "derivesInverseAtomProperty" ;
        <http://www.w3.org/2000/01/rdf-schema#range>
                <http://www.w3.org/1999/02/22-rdf-syntax-ns#Property> .

<https://w3id.org/won/core#atomList>
        a       <http://www.w3.org/2002/07/owl#ObjectProperty> ;
        <http://www.w3.org/2000/01/rdf-schema#comment>
                "The Node's atoms, in a LDP-pageable container." ;
        <http://www.w3.org/2000/01/rdf-schema#domain>
                <https://w3id.org/won/core#Node> ;
        <http://www.w3.org/2000/01/rdf-schema#label>
                "atomList" ;
        <http://www.w3.org/2000/01/rdf-schema#range>
                <https://w3id.org/won/core#AtomContainer> .

<https://w3id.org/won/core#defaultSocket>
        a       <http://www.w3.org/2002/07/owl#ObjectProperty> ;
        <http://www.w3.org/2000/01/rdf-schema#comment>
                "Indicates the socket to connect to by default."@en ;
        <http://www.w3.org/2000/01/rdf-schema#domain>
                <https://w3id.org/won/core#Atom> ;
        <http://www.w3.org/2000/01/rdf-schema#isDefinedBy>
                <https://w3id.org/won/core> ;
        <http://www.w3.org/2000/01/rdf-schema#label>
                "defaultSocket" ;
        <http://www.w3.org/2000/01/rdf-schema#range>
                <https://w3id.org/won/core#Socket> .

<https://w3id.org/won/core#atomActivatedTopic>
        a       <http://www.w3.org/2002/07/owl#DatatypeProperty> ;
        <http://www.w3.org/2000/01/rdf-schema#comment>
                "The activeMQ topic to subscribe to to be informed when an atom is activated."@en ;
        <http://www.w3.org/2000/01/rdf-schema#domain>
                <https://w3id.org/won/core#WonOverActiveMq> ;
        <http://www.w3.org/2000/01/rdf-schema#label>
                "atomActivatedTopic" ;
        <http://www.w3.org/2000/01/rdf-schema#range>
                <http://www.w3.org/2001/XMLSchema#string> .

<https://w3id.org/won/core#atomState>
        a       <http://www.w3.org/2002/07/owl#FunctionalProperty> , <http://www.w3.org/2002/07/owl#ObjectProperty> ;
        <http://www.w3.org/2000/01/rdf-schema#comment>
                "Defines the Atom object's state."@en ;
        <http://www.w3.org/2000/01/rdf-schema#domain>
                <https://w3id.org/won/core#Atom> ;
        <http://www.w3.org/2000/01/rdf-schema#isDefinedBy>
                <https://w3id.org/won/core> ;
        <http://www.w3.org/2000/01/rdf-schema#label>
                "atomState" ;
        <http://www.w3.org/2000/01/rdf-schema#range>
                <https://w3id.org/won/core#AtomState> .

<https://w3id.org/won/core#atomDeletedTopic>
        a       <http://www.w3.org/2002/07/owl#DatatypeProperty> ;
        <http://www.w3.org/2000/01/rdf-schema#comment>
                "The activeMQ topic to subscribe to to be informed when an atom is deleted."@en ;
        <http://www.w3.org/2000/01/rdf-schema#domain>
                <https://w3id.org/won/core#WonOverActiveMq> ;
        <http://www.w3.org/2000/01/rdf-schema#label>
                "atomDeletedTopic" ;
        <http://www.w3.org/2000/01/rdf-schema#range>
                <http://www.w3.org/2001/XMLSchema#string> .

<https://w3id.org/won/core#targetConnection>
        a       <http://www.w3.org/2002/07/owl#InverseFunctionalProperty> , <http://www.w3.org/2002/07/owl#ObjectProperty> , <http://www.w3.org/2002/07/owl#SymmetricProperty> , <http://www.w3.org/2002/07/owl#FunctionalProperty> ;
        <http://www.w3.org/2000/01/rdf-schema#comment>
                "Links a Connection object to its remote counterpart."@en ;
        <http://www.w3.org/2000/01/rdf-schema#domain>
                <https://w3id.org/won/core#Connection> ;
        <http://www.w3.org/2000/01/rdf-schema#isDefinedBy>
                <https://w3id.org/won/core> ;
        <http://www.w3.org/2000/01/rdf-schema#label>
                "targetConnection" ;
        <http://www.w3.org/2000/01/rdf-schema#range>
                <https://w3id.org/won/core#Connection> .

<https://w3id.org/won/core#Closed>
        a       <http://www.w3.org/2002/07/owl#NamedIndividual> , <https://w3id.org/won/core#ConnectionState> ;
        <http://www.w3.org/2000/01/rdf-schema#comment>
                "The closed state. No Messages are forwarded in this state. Re-opening a connection is possbile."@en ;
        <http://www.w3.org/2000/01/rdf-schema#isDefinedBy>
                <https://w3id.org/won/core> ;
        <http://www.w3.org/2000/01/rdf-schema#label>
                "Closed" .

<https://w3id.org/won/core#AtomState>
        a       <http://www.w3.org/2002/07/owl#Class> ;
        <http://www.w3.org/2000/01/rdf-schema#comment>
                "The Atom's state."@en ;
        <http://www.w3.org/2000/01/rdf-schema#isDefinedBy>
                <https://w3id.org/won/core> ;
        <http://www.w3.org/2000/01/rdf-schema#label>
                "AtomState" .

<https://w3id.org/won/core#matcherQueue>
        a       <http://www.w3.org/2002/07/owl#DatatypeProperty> ;
        <http://www.w3.org/2000/01/rdf-schema#comment>
                "The activeMQ queue to be used by matchers to send messages to the node."@en ;
        <http://www.w3.org/2000/01/rdf-schema#domain>
                <https://w3id.org/won/core#WonOverActiveMq> ;
        <http://www.w3.org/2000/01/rdf-schema#label>
                "matcherQueue" ;
        <http://www.w3.org/2000/01/rdf-schema#range>
                <http://www.w3.org/2001/XMLSchema#string> .

<https://w3id.org/won/core#connectedCount>
        a       <http://www.w3.org/2002/07/owl#DatatypeProperty> ;
        <http://www.w3.org/2000/01/rdf-schema#comment>
                "The number of connections in the container that are in state CONNECTED."@en ;
        <http://www.w3.org/2000/01/rdf-schema#domain>
                <https://w3id.org/won/core#ConnectionContainer> ;
        <http://www.w3.org/2000/01/rdf-schema#label>
                "connectedCount" ;
        <http://www.w3.org/2000/01/rdf-schema#range>
                <http://www.w3.org/2001/XMLSchema#integer> .

<https://w3id.org/won/core#ConnectionContainer>
        a       <http://www.w3.org/2002/07/owl#Class> ;
        <http://www.w3.org/2000/01/rdf-schema#comment>
                "Container for Connections. The container supports LDP paging as described here: https://github.com/researchstudio-sat/webofneeds/blob/master/webofneeds/won-node-webapp/doc/linked-data-paging.md"@en ;
        <http://www.w3.org/2000/01/rdf-schema#isDefinedBy>
                <https://w3id.org/won/core> ;
        <http://www.w3.org/2000/01/rdf-schema#label>
                "ConnectionContainer" ;
        <http://www.w3.org/2000/01/rdf-schema#subClassOf>
                <http://www.w3.org/ns/ldp#CompositeContainer> ;
        <http://www.w3.org/2002/07/owl#disjointWith>
                <https://w3id.org/won/core#MessageContainer> .

<https://w3id.org/won/core#wonNode>
        a       <http://www.w3.org/2002/07/owl#ObjectProperty> ;
        <http://www.w3.org/2000/01/rdf-schema#comment>
                "Links an Atom or Connection to their WoN node."@en ;
        <http://www.w3.org/2000/01/rdf-schema#domain>
                [ a       <http://www.w3.org/2002/07/owl#Class> ;
                  <http://www.w3.org/2002/07/owl#unionOf>
                          ( <https://w3id.org/won/core#Atom> <https://w3id.org/won/core#Connection> )
                ] ;
        <http://www.w3.org/2000/01/rdf-schema#label>
                "wonNode" ;
        <http://www.w3.org/2000/01/rdf-schema#range>
                <https://w3id.org/won/core#Node> .

<https://w3id.org/won/core#closedCount>
        a       <http://www.w3.org/2002/07/owl#DatatypeProperty> ;
        <http://www.w3.org/2000/01/rdf-schema#comment>
                "The number of connections in the container that are in state CLOSED."@en ;
        <http://www.w3.org/2000/01/rdf-schema#domain>
                <https://w3id.org/won/core#ConnectionContainer> ;
        <http://www.w3.org/2000/01/rdf-schema#label>
                "closedCount" ;
        <http://www.w3.org/2000/01/rdf-schema#range>
                <http://www.w3.org/2001/XMLSchema#integer> .

<https://w3id.org/won/core#supportsWonProtocolImpl>
        a       <http://www.w3.org/2002/07/owl#ObjectProperty> ;
        <http://www.w3.org/2000/01/rdf-schema#comment>
                "Connects an WoN Node object with a description of a WON protocol it supports."@en ;
        <http://www.w3.org/2000/01/rdf-schema#domain>
                <https://w3id.org/won/core#Node> ;
        <http://www.w3.org/2000/01/rdf-schema#isDefinedBy>
                <https://w3id.org/won/core> ;
        <http://www.w3.org/2000/01/rdf-schema#label>
                "supportsWonProtocolImpl" ;
        <http://www.w3.org/2000/01/rdf-schema#range>
                <https://w3id.org/won/core#WonProtocol> .

<https://w3id.org/won/core#socketDefinition>
        a       <http://www.w3.org/2002/07/owl#ObjectProperty> ;
        <http://www.w3.org/2000/01/rdf-schema#comment>
                "Links the socket to its definition. A socket must have exactly one definition."@en ;
        <http://www.w3.org/2000/01/rdf-schema#domain>
                <https://w3id.org/won/core#Socket> ;
        <http://www.w3.org/2000/01/rdf-schema#label>
                "socketDefinition" ;
        <http://www.w3.org/2000/01/rdf-schema#range>
                <https://w3id.org/won/core#SocketDefinition> .

<https://w3id.org/won/core#nodeQueue>
        a       <http://www.w3.org/2002/07/owl#DatatypeProperty> ;
        <http://www.w3.org/2000/01/rdf-schema#comment>
                "The activeMQ queue to be used by other nodes to send messages to the node."@en ;
        <http://www.w3.org/2000/01/rdf-schema#domain>
                <https://w3id.org/won/core#WonOverActiveMq> ;
        <http://www.w3.org/2000/01/rdf-schema#label>
                "nodeQueue" ;
        <http://www.w3.org/2000/01/rdf-schema#range>
                <http://www.w3.org/2001/XMLSchema#string> .

<https://w3id.org/won/core#Suggested>
        a       <https://w3id.org/won/core#ConnectionState> , <http://www.w3.org/2002/07/owl#NamedIndividual> ;
        <http://www.w3.org/2000/01/rdf-schema#comment>
                "Suggested state. The Connection has been created through a Hint Event but not yet been opened by either of the sides."@en ;
        <http://www.w3.org/2000/01/rdf-schema#isDefinedBy>
                <https://w3id.org/won/core> ;
        <http://www.w3.org/2000/01/rdf-schema#label>
                "Suggested" .

<https://w3id.org/won/core#atomDeactivatedTopic>
        a       <http://www.w3.org/2002/07/owl#DatatypeProperty> ;
        <http://www.w3.org/2000/01/rdf-schema#comment>
                "The activeMQ topic to subscribe to to be informed when an atom is deactivated."@en ;
        <http://www.w3.org/2000/01/rdf-schema#domain>
                <https://w3id.org/won/core#WonOverActiveMq> ;
        <http://www.w3.org/2000/01/rdf-schema#label>
                "atomDeactivatedTopic" ;
        <http://www.w3.org/2000/01/rdf-schema#range>
                <http://www.w3.org/2001/XMLSchema#string> .

<https://w3id.org/won/core#Active>
        a       <http://www.w3.org/2002/07/owl#NamedIndividual> , <https://w3id.org/won/core#AtomState> ;
        <http://www.w3.org/2000/01/rdf-schema#comment>
                "The active state. "@en ;
        <http://www.w3.org/2000/01/rdf-schema#isDefinedBy>
                <https://w3id.org/won/core> ;
        <http://www.w3.org/2000/01/rdf-schema#label>
                "Active" .

<https://w3id.org/won/core#socket>
        a       <http://www.w3.org/2002/07/owl#ObjectProperty> ;
        <http://www.w3.org/2000/01/rdf-schema#comment>
                "Indicates that an atom or connection supports the specified socket (=behavior)."@en ;
        <http://www.w3.org/2000/01/rdf-schema#domain>
                [ a       <http://www.w3.org/2002/07/owl#Class> ;
                  <http://www.w3.org/2002/07/owl#unionOf>
                          ( <https://w3id.org/won/core#Atom> <https://w3id.org/won/core#Connection> )
                ] ;
        <http://www.w3.org/2000/01/rdf-schema#isDefinedBy>
                <https://w3id.org/won/core> ;
        <http://www.w3.org/2000/01/rdf-schema#label>
                "socket" ;
        <http://www.w3.org/2000/01/rdf-schema#range>
                <https://w3id.org/won/core#Socket> .

<https://w3id.org/won/core#targetAtom>
        a       <http://www.w3.org/2002/07/owl#ObjectProperty> ;
        <http://www.w3.org/2000/01/rdf-schema#comment>
                "links a Connection to its remote Atom. The remote Atom is the one holding the  targetConnection."@en ;
        <http://www.w3.org/2000/01/rdf-schema#domain>
                <https://w3id.org/won/core#Connection> ;
        <http://www.w3.org/2000/01/rdf-schema#isDefinedBy>
                "https://w3id.org/won/core"@en ;
        <http://www.w3.org/2000/01/rdf-schema#label>
                "targetAtom" ;
        <http://www.w3.org/2000/01/rdf-schema#range>
                <https://w3id.org/won/core#Atom> .

<https://w3id.org/won/core#autoOpen>
        a       <http://www.w3.org/2002/07/owl#DatatypeProperty> ;
        <http://www.w3.org/2000/01/rdf-schema#comment>
                "Indicates that any incoming CONNECT/OPEN message will be answered with OPEN unless the facet configuration forbids it."@en ;
        <http://www.w3.org/2000/01/rdf-schema#domain>
                <https://w3id.org/won/core#SocketDefinition> ;
        <http://www.w3.org/2000/01/rdf-schema#label>
                "autoOpen" ;
        <http://www.w3.org/2000/01/rdf-schema#range>
                <http://www.w3.org/2001/XMLSchema#boolean> .

<https://w3id.org/won/core#messageContainer>
        a       <http://www.w3.org/2002/07/owl#ObjectProperty> , <http://www.w3.org/2002/07/owl#FunctionalProperty> ;
        <http://www.w3.org/2000/01/rdf-schema#comment>
                "Links the Connection object to a container containing connection events (messages)."@en ;
        <http://www.w3.org/2000/01/rdf-schema#domain>
                [ a       <http://www.w3.org/2002/07/owl#Class> ;
                  <http://www.w3.org/2002/07/owl#unionOf>
                          ( <https://w3id.org/won/core#Atom> <https://w3id.org/won/core#Connection> )
                ] ;
        <http://www.w3.org/2000/01/rdf-schema#isDefinedBy>
                <https://w3id.org/won/core> ;
        <http://www.w3.org/2000/01/rdf-schema#label>
                "messageContainer" ;
        <http://www.w3.org/2000/01/rdf-schema#range>
                <https://w3id.org/won/core#MessageContainer> .

<https://w3id.org/won/core#eventUriPrefix>
        a       <http://www.w3.org/2002/07/owl#DatatypeProperty> ;
        <http://www.w3.org/2000/01/rdf-schema#comment>
                "Specifies the prefix an event must have on the node this specification applies to. This specification allows clients to generate new valid new event (message) URIs."@en ;
        <http://www.w3.org/2000/01/rdf-schema#domain>
                <https://w3id.org/won/core#UriPrefixSpecification> ;
        <http://www.w3.org/2000/01/rdf-schema#label>
                "eventUriPrefix" ;
        <http://www.w3.org/2000/01/rdf-schema#range>
                <http://www.w3.org/2001/XMLSchema#string> .

<https://w3id.org/won/core#requestSentCount>
        a       <http://www.w3.org/2002/07/owl#DatatypeProperty> ;
        <http://www.w3.org/2000/01/rdf-schema#comment>
                "The number of connections in the container that are in state REQUEST_RECEIVED."@en ;
        <http://www.w3.org/2000/01/rdf-schema#domain>
                <https://w3id.org/won/core#ConnectionContainer> ;
        <http://www.w3.org/2000/01/rdf-schema#label>
                "requestSentCount" ;
        <http://www.w3.org/2000/01/rdf-schema#range>
                <http://www.w3.org/2001/XMLSchema#integer> .

<https://w3id.org/won/core#RequestReceived>
        a       <http://www.w3.org/2002/07/owl#NamedIndividual> , <https://w3id.org/won/core#ConnectionState> ;
        <http://www.w3.org/2000/01/rdf-schema#comment>
                "Half-open state. The connection has been opened by the remote counterpart but not yet been accepted by the local end."@en ;
        <http://www.w3.org/2000/01/rdf-schema#isDefinedBy>
                <https://w3id.org/won/core> ;
        <http://www.w3.org/2000/01/rdf-schema#label>
                "RequestReceived" .

<https://w3id.org/won/core#Connection>
        a       <http://www.w3.org/2002/07/owl#Class> ;
        <http://www.w3.org/2000/01/rdf-schema#comment>
                "Represents a Connection to between two Atoms. Whenever two Atoms are connected, each Atom creates a dedicated Connection object which encapsulate all information about the connection."@en ;
        <http://www.w3.org/2000/01/rdf-schema#isDefinedBy>
                <https://w3id.org/won/core> ;
        <http://www.w3.org/2000/01/rdf-schema#label>
                "Connection" .

<http://purl.org/dc/elements/1.1/title>
        a       <http://www.w3.org/2002/07/owl#AnnotationProperty> .

<https://w3id.org/won/core#sourceAtom>
        a       <http://www.w3.org/2002/07/owl#ObjectProperty> ;
        <http://www.w3.org/2000/01/rdf-schema#comment>
                "Links a Connection to the Atom it belongs to (the source of this Connection)"@en ;
        <http://www.w3.org/2000/01/rdf-schema#domain>
                <https://w3id.org/won/core#Connection> ;
        <http://www.w3.org/2000/01/rdf-schema#label>
                "sourceAtom" ;
        <http://www.w3.org/2000/01/rdf-schema#range>
                <https://w3id.org/won/core#Atom> .

<https://w3id.org/won/core#Socket>
        a       <http://www.w3.org/2002/07/owl#Class> ;
        <http://www.w3.org/2000/01/rdf-schema#comment>
                "An Atom defines how Connections can be established using any number of Socket individuals. Each connection between two Atoms must specify the Socket it is attached to on each side."@en ;
        <http://www.w3.org/2000/01/rdf-schema#isDefinedBy>
                <https://w3id.org/won/core> ;
        <http://www.w3.org/2000/01/rdf-schema#label>
                "Socket" .

<http://purl.org/dc/elements/1.1/abstract>
        a       <http://www.w3.org/2002/07/owl#AnnotationProperty> .

<https://w3id.org/won/core#AtomContainer>
        a       <http://www.w3.org/2002/07/owl#Class> ;
        <http://www.w3.org/2000/01/rdf-schema#comment>
                "An LDP container with all the Atoms stored on the Node.\n\nThe container supports LDP paging as described here: https://github.com/researchstudio-sat/webofneeds/blob/master/webofneeds/won-node-webapp/doc/linked-data-paging.md" ;
        <http://www.w3.org/2000/01/rdf-schema#label>
                "AtomContainer" ;
        <http://www.w3.org/2000/01/rdf-schema#subClassOf>
                <http://www.w3.org/ns/ldp#CompositeContainer> .

<https://w3id.org/won/core#derivesAtomProperty>
        a       <http://www.w3.org/2002/07/owl#ObjectProperty> ;
        <http://www.w3.org/2000/01/rdf-schema#comment>
                "Defines a property to be 'derived' when the connection is established. The property will be used to derive a triple '[sourceAtom] [property] [targetAtom]'."@en ;
        <http://www.w3.org/2000/01/rdf-schema#domain>
                <https://w3id.org/won/core#SocketDefinition> ;
        <http://www.w3.org/2000/01/rdf-schema#label>
                "derivesAtomProperty" ;
        <http://www.w3.org/2000/01/rdf-schema#range>
                <http://www.w3.org/1999/02/22-rdf-syntax-ns#Property> .

<https://w3id.org/won/core#atomCreatedTopic>
        a       <http://www.w3.org/2002/07/owl#DatatypeProperty> ;
        <http://www.w3.org/2000/01/rdf-schema#comment>
                "The activeMQ topic to subscribe to to be informed when an atom is created."@en ;
        <http://www.w3.org/2000/01/rdf-schema#domain>
                <https://w3id.org/won/core#WonOverActiveMq> ;
        <http://www.w3.org/2000/01/rdf-schema#label>
                "atomCreatedTopic" ;
        <http://www.w3.org/2000/01/rdf-schema#range>
                <http://www.w3.org/2001/XMLSchema#string> .

<https://w3id.org/won/core#atomModifiedTopic>
        a       <http://www.w3.org/2002/07/owl#DatatypeProperty> ;
        <http://www.w3.org/2000/01/rdf-schema#comment>
                "The activeMQ topic to subscribe to to be informed when an atom is modified."@en ;
        <http://www.w3.org/2000/01/rdf-schema#domain>
                <https://w3id.org/won/core#WonOverActiveMq> ;
        <http://www.w3.org/2000/01/rdf-schema#label>
                "atomModifiedTopic" ;
        <http://www.w3.org/2000/01/rdf-schema#range>
                <http://www.w3.org/2001/XMLSchema#string> .

<https://w3id.org/won/core#connectionUriPrefix>
        a       <http://www.w3.org/2002/07/owl#DatatypeProperty> ;
        <http://www.w3.org/2000/01/rdf-schema#comment>
                "Specifies the prefix a connection must have on the node this specification applies to."@en ;
        <http://www.w3.org/2000/01/rdf-schema#domain>
                <https://w3id.org/won/core#UriPrefixSpecification> ;
        <http://www.w3.org/2000/01/rdf-schema#label>
                "connectionUriPrefix" ;
        <http://www.w3.org/2000/01/rdf-schema#range>
                <http://www.w3.org/2001/XMLSchema#string> .

<https://w3id.org/won/core#UriPrefixSpecification>
        a       <http://www.w3.org/2002/07/owl#Class> ;
        <http://www.w3.org/2000/01/rdf-schema#comment>
                "Specification of URI prefixes for atoms, events, and connections for a WoN node."@en ;
        <http://www.w3.org/2000/01/rdf-schema#label>
                "UriPrefixSpecification" .

<http://purl.org/dc/elements/1.1/creator>
        a       <http://www.w3.org/2002/07/owl#AnnotationProperty> .

<https://w3id.org/won/core#uriPrefixSpecification>
        a       <http://www.w3.org/2002/07/owl#ObjectProperty> ;
        <http://www.w3.org/2000/01/rdf-schema#comment>
                "Specification of URI prefixes used by this WoN node."@en ;
        <http://www.w3.org/2000/01/rdf-schema#domain>
                <https://w3id.org/won/core#Node> ;
        <http://www.w3.org/2000/01/rdf-schema#label>
                "uriPrefixSpecification" ;
        <http://www.w3.org/2000/01/rdf-schema#range>
                <https://w3id.org/won/core#UriPrefixSpecification> .

<https://w3id.org/won/core#WonProtocol>
        a       <http://www.w3.org/2002/07/owl#Class> ;
        <http://www.w3.org/2000/01/rdf-schema#comment>
                "Superclass for Web of Needs protocol implementations."@en ;
        <http://www.w3.org/2000/01/rdf-schema#isDefinedBy>
                <https://w3id.org/won/core> ;
        <http://www.w3.org/2000/01/rdf-schema#label>
                "WonProtocol" .

<https://w3id.org/won/core#brokerUri>
        a       <http://www.w3.org/2002/07/owl#DatatypeProperty> ;
        <http://www.w3.org/2000/01/rdf-schema#comment>
                "The URI of the activeMQ broker"@en ;
        <http://www.w3.org/2000/01/rdf-schema#domain>
                <https://w3id.org/won/core#WonOverActiveMq> ;
        <http://www.w3.org/2000/01/rdf-schema#label>
                "brokerUri" ;
        <http://www.w3.org/2000/01/rdf-schema#range>
                <http://www.w3.org/2001/XMLSchema#anyURI> .

<https://w3id.org/won/core#contentGraph>
        a       <http://www.w3.org/2002/07/owl#ObjectProperty> ;
        <http://www.w3.org/2000/01/rdf-schema#comment>
                "Links an Atom to an RDF graph holding some of its RDF content."@en ;
        <http://www.w3.org/2000/01/rdf-schema#domain>
                <https://w3id.org/won/core#Atom> ;
        <http://www.w3.org/2000/01/rdf-schema#label>
                "contentGraph" ;
        <http://www.w3.org/2000/01/rdf-schema#range>
                <http://www.w3.org/2002/07/owl#Thing> .

<http://www.linkedmodel.org/schema/vaem#rationale>
        a       <http://www.w3.org/2002/07/owl#AnnotationProperty> .

<https://w3id.org/won/core#WonOverActiveMq>
        a       <http://www.w3.org/2002/07/owl#Class> ;
        <http://www.w3.org/2000/01/rdf-schema#comment>
                "The Web of Needs protocol implementation that uses ActiveMQ."@en ;
        <http://www.w3.org/2000/01/rdf-schema#isDefinedBy>
                <https://w3id.org/won/core> ;
        <http://www.w3.org/2000/01/rdf-schema#label>
                "WonOverActiveMq" ;
        <http://www.w3.org/2000/01/rdf-schema#subClassOf>
                <https://w3id.org/won/core#WonProtocol> .

<https://w3id.org/won/core#requestReceivedCount>
        a       <http://www.w3.org/2002/07/owl#DatatypeProperty> ;
        <http://www.w3.org/2000/01/rdf-schema#comment>
                "The number of connections in the container that are in state REQUEST_RECEIVED."@en ;
        <http://www.w3.org/2000/01/rdf-schema#domain>
                <https://w3id.org/won/core#ConnectionContainer> ;
        <http://www.w3.org/2000/01/rdf-schema#label>
                "requestReceivedCount" ;
        <http://www.w3.org/2000/01/rdf-schema#range>
                <http://www.w3.org/2001/XMLSchema#integer> .

<https://w3id.org/won/core#Inactive>
        a       <https://w3id.org/won/core#AtomState> , <http://www.w3.org/2002/07/owl#NamedIndividual> ;
        <http://www.w3.org/2000/01/rdf-schema#comment>
                "The incative state. Atoms do not communicate in this state. Intended to stop receiving messages for something not currently of interest."@en ;
        <http://www.w3.org/2000/01/rdf-schema#isDefinedBy>
                <https://w3id.org/won/core> ;
        <http://www.w3.org/2000/01/rdf-schema#label>
                "Inactive" .

<https://w3id.org/won/core#compatibleSocketDefinition>
        a       <http://www.w3.org/2002/07/owl#ObjectProperty> ;
        <http://www.w3.org/2000/01/rdf-schema#comment>
                "Identifies another SocketDefinition that is compatible with this one. Connections with other kinds of sockets will not be allowed unless they are explicitly annotated."@en ;
        <http://www.w3.org/2000/01/rdf-schema#domain>
                <https://w3id.org/won/core#SocketDefinition> ;
        <http://www.w3.org/2000/01/rdf-schema#label>
                "compatibleSocketDefinition" ;
        <http://www.w3.org/2000/01/rdf-schema#range>
                <https://w3id.org/won/core#SocketDefinition> .

<https://w3id.org/won/core#ownerQueue>
        a       <http://www.w3.org/2002/07/owl#DatatypeProperty> ;
        <http://www.w3.org/2000/01/rdf-schema#comment>
                "The activeMQ queue to be used by owners to send messages to the node."@en ;
        <http://www.w3.org/2000/01/rdf-schema#domain>
                <https://w3id.org/won/core#WonOverActiveMq> ;
        <http://www.w3.org/2000/01/rdf-schema#label>
                "ownerQueue" ;
        <http://www.w3.org/2000/01/rdf-schema#range>
                <http://www.w3.org/2001/XMLSchema#string> .

<http://purl.org/dc/terms/license>
        a       <http://www.w3.org/2002/07/owl#AnnotationProperty> .

<http://purl.org/dc/elements/1.1/date>
        a       <http://www.w3.org/2002/07/owl#AnnotationProperty> .

<http://www.w3.org/2001/XMLSchema#duration>
        a       <http://www.w3.org/2000/01/rdf-schema#Datatype> .

<https://w3id.org/won/core#Atom>
        a       <http://www.w3.org/2002/07/owl#Class> ;
        <http://www.w3.org/2000/01/rdf-schema#comment>
                "An atom is an online entity controlled by a person or organization. Its purpose is to be connected to other such atoms via Connections, so it can be said that it represents the need to interact with others.\nIt specifies a content - what the atom is about, which may be something that is offered for sale, sought for rental etc."@en ;
        <http://www.w3.org/2000/01/rdf-schema#isDefinedBy>
                <https://w3id.org/won/core> ;
        <http://www.w3.org/2000/01/rdf-schema#label>
                "Atom" .

<https://w3id.org/won/core#connections>
        a       <http://www.w3.org/2002/07/owl#ObjectProperty> ;
        <http://www.w3.org/2000/01/rdf-schema#comment>
                "Links the Atom object to its connections."@en ;
        <http://www.w3.org/2000/01/rdf-schema#domain>
                <https://w3id.org/won/core#Atom> ;
        <http://www.w3.org/2000/01/rdf-schema#isDefinedBy>
                <https://w3id.org/won/core> ;
        <http://www.w3.org/2000/01/rdf-schema#label>
                "connections" ;
        <http://www.w3.org/2000/01/rdf-schema#range>
                <https://w3id.org/won/core#ConnectionContainer> .

<http://www.w3.org/ns/ldp#CompositeContainer>
        a       <http://www.w3.org/2002/07/owl#Class> ;
        <http://www.w3.org/2000/01/rdf-schema#isDefinedBy>
                <https://w3id.org/won/core> .

<http://www.w3.org/1999/02/22-rdf-syntax-ns#Property>
        a       <http://www.w3.org/2002/07/owl#Class> .

<http://purl.org/dc/terms/created>
        a       <http://www.w3.org/2002/07/owl#AnnotationProperty> .

<http://purl.org/vocab/vann/preferredNamespacePrefix>
        a       <http://www.w3.org/2002/07/owl#AnnotationProperty> .
